<?xml version="1.0"?>
<rdf:RDF xmlns="http://w3id.org/meta-share/meta-share"
     xml:base="http://w3id.org/meta-share/meta-share"
     xmlns:cc="http://creativecommons.org/ns#"
     xmlns:swrc="http://swrc.ontoware.org/ontology#"
     xmlns:owl="http://www.w3.org/2002/07/owl#"
     xmlns:ms="http://w3id.org/meta-share/meta-share/"
     xmlns:msxml="http://www.ilsp.gr/META-XMLSchema#"
     xmlns:datacite="http://purl.org/spar/datacite/"
     xmlns:xsd="http://www.w3.org/2001/XMLSchema#"
     xmlns:skos="http://www.w3.org/2004/02/skos/core#"
     xmlns:rdfs="http://www.w3.org/2000/01/rdf-schema#"
     xmlns:dct="http://purl.org/dc/terms/"
     xmlns:rdf="http://www.w3.org/1999/02/22-rdf-syntax-ns#"
     xmlns:xml="http://www.w3.org/XML/1998/namespace"
     xmlns:omtd="http://w3id.org/meta-share/omtd-share/"
     xmlns:odrl="http://www.w3.org/ns/odrl/2/"
     xmlns:dcat="http://www.w3.org/ns/dcat#"
     xmlns:vann="http://purl.org/vocab/vann/"
     xmlns:foaf="http://xmlns.com/foaf/0.1/"
     xmlns:dc="http://purl.org/dc/elements/1.1/">
    <owl:Ontology rdf:about="http://w3id.org/meta-share/meta-share">
        <owl:versionIRI rdf:resource="http://w3id.org/meta-share/meta-share/2.0.0"/>
        <owl:priorVersion rdf:resource="http://purl.org/ms-lod/MetaShareRights.ttl#"/>
        <dct:creator>Philipp Cimiano</dct:creator>
        <dct:creator>Dimitris Galanis</dct:creator>
        <vann:preferredNamespacePrefix>ms</vann:preferredNamespacePrefix>
        <dct:creator>John P. McCrae</dct:creator>
        <dct:creator>Jorge Gracia</dct:creator>
        <dct:creator rdf:resource="http://john.mccr.ae/"/>
        <dct:creator>Marta Villegas</dct:creator>
        <vann:preferredNamespaceUri rdf:resource="http://w3id.org/meta-share/meta-share/"/>
        <dct:creator>Victor Rodriguez Doncel</dct:creator>
        <dc:title xml:lang="en">META-SHARE ontology</dc:title>
        <dct:license rdf:resource="http://purl.org/NET/rdflicense/cc-by4.0"/>
        <owl:versionInfo xml:lang="en">v2.0.0 pre-release</owl:versionInfo>
        <owl:priorVersion rdf:resource="http://lodserver.iula.upf.edu/Metashare/ontology/"/>
        <dct:creator>Katerina Gkirtzou</dct:creator>
        <dct:modified>2020-03-20</dct:modified>
        <dct:creator>Penny Labropoulou</dct:creator>
        <dc:description xml:lang="en">Meta-Share ontology v2. The ontology caters for the description of Language resources  (corpora, lexical/conceptual resources, models, grammars, etc. and language processing tools and services) for Language Technology needs. 
It is also related to the OMTD-SHARE ontology (http://w3id.org/meta-share/omtd-share/) which caters for specific features (LT operation/area, data format, method, annotation type).</dc:description>
    </owl:Ontology>
    


    <!-- 
    ///////////////////////////////////////////////////////////////////////////////////////
    //
    // Annotation properties
    //
    ///////////////////////////////////////////////////////////////////////////////////////
     -->

    


    <!-- http://purl.org/dc/elements/1.1/description -->

    <owl:AnnotationProperty rdf:about="http://purl.org/dc/elements/1.1/description"/>
    


    <!-- http://purl.org/dc/elements/1.1/source -->

    <owl:AnnotationProperty rdf:about="http://purl.org/dc/elements/1.1/source"/>
    


    <!-- http://purl.org/dc/elements/1.1/title -->

    <owl:AnnotationProperty rdf:about="http://purl.org/dc/elements/1.1/title"/>
    


    <!-- http://purl.org/dc/terms/contributor -->

    <owl:AnnotationProperty rdf:about="http://purl.org/dc/terms/contributor"/>
    


    <!-- http://purl.org/dc/terms/creator -->

    <owl:AnnotationProperty rdf:about="http://purl.org/dc/terms/creator"/>
    


    <!-- http://purl.org/dc/terms/license -->

    <owl:AnnotationProperty rdf:about="http://purl.org/dc/terms/license"/>
    


    <!-- http://purl.org/dc/terms/modified -->

    <owl:AnnotationProperty rdf:about="http://purl.org/dc/terms/modified"/>
    


    <!-- http://purl.org/dc/terms/replaces -->

    <owl:AnnotationProperty rdf:about="http://purl.org/dc/terms/replaces"/>
    


    <!-- http://purl.org/dc/terms/source -->

    <owl:AnnotationProperty rdf:about="http://purl.org/dc/terms/source"/>
    


    <!-- http://purl.org/vocab/vann/preferredNamespacePrefix -->

    <owl:AnnotationProperty rdf:about="http://purl.org/vocab/vann/preferredNamespacePrefix"/>
    


    <!-- http://purl.org/vocab/vann/preferredNamespaceUri -->

    <owl:AnnotationProperty rdf:about="http://purl.org/vocab/vann/preferredNamespaceUri"/>
    


    <!-- http://www.w3.org/2000/01/rdf-schema#altLabel -->

    <owl:AnnotationProperty rdf:about="http://www.w3.org/2000/01/rdf-schema#altLabel"/>
    


    <!-- http://www.w3.org/2002/07/owl#equivalentProperty -->

    <owl:AnnotationProperty rdf:about="http://www.w3.org/2002/07/owl#equivalentProperty"/>
    


    <!-- http://www.w3.org/2004/02/skos/core#altLabel -->

    <owl:AnnotationProperty rdf:about="http://www.w3.org/2004/02/skos/core#altLabel"/>
    


    <!-- http://www.w3.org/2004/02/skos/core#broaderTransitive -->

    <owl:AnnotationProperty rdf:about="http://www.w3.org/2004/02/skos/core#broaderTransitive"/>
    


    <!-- http://www.w3.org/2004/02/skos/core#closeMatch -->

    <owl:AnnotationProperty rdf:about="http://www.w3.org/2004/02/skos/core#closeMatch"/>
    


    <!-- http://www.w3.org/2004/02/skos/core#comment -->

    <owl:AnnotationProperty rdf:about="http://www.w3.org/2004/02/skos/core#comment"/>
    


    <!-- http://www.w3.org/2004/02/skos/core#example -->

    <owl:AnnotationProperty rdf:about="http://www.w3.org/2004/02/skos/core#example"/>
    


    <!-- http://www.w3.org/2004/02/skos/core#note -->

    <owl:AnnotationProperty rdf:about="http://www.w3.org/2004/02/skos/core#note"/>
    


    <!-- http://www.w3.org/ns/odrl/2/action -->

    <owl:AnnotationProperty rdf:about="http://www.w3.org/ns/odrl/2/action"/>
    


    <!-- http://www.w3.org/ns/odrl/2/constraint -->

    <owl:AnnotationProperty rdf:about="http://www.w3.org/ns/odrl/2/constraint"/>
    


    <!-- http://www.w3.org/ns/odrl/2/duty -->

    <owl:AnnotationProperty rdf:about="http://www.w3.org/ns/odrl/2/duty"/>
    


    <!-- http://www.w3.org/ns/odrl/2/operator -->

    <owl:AnnotationProperty rdf:about="http://www.w3.org/ns/odrl/2/operator"/>
    


    <!-- http://www.w3.org/ns/odrl/2/permission -->

    <owl:AnnotationProperty rdf:about="http://www.w3.org/ns/odrl/2/permission"/>
    


    <!-- http://www.w3.org/ns/odrl/2/prohibition -->

    <owl:AnnotationProperty rdf:about="http://www.w3.org/ns/odrl/2/prohibition"/>
    


    <!-- http://www.w3.org/ns/odrl/2/purpose -->

    <owl:AnnotationProperty rdf:about="http://www.w3.org/ns/odrl/2/purpose"/>
    


    <!-- http://www.w3.org/ns/odrl/2/recipient -->

    <owl:AnnotationProperty rdf:about="http://www.w3.org/ns/odrl/2/recipient"/>
    


    <!-- 
    ///////////////////////////////////////////////////////////////////////////////////////
    //
    // Datatypes
    //
    ///////////////////////////////////////////////////////////////////////////////////////
     -->

    


    <!-- http://www.w3.org/1999/02/22-rdf-syntax-ns#langString -->

    <rdfs:Datatype rdf:about="http://www.w3.org/1999/02/22-rdf-syntax-ns#langString"/>
    


    <!-- http://www.w3.org/2001/XMLSchema#date -->

    <rdfs:Datatype rdf:about="http://www.w3.org/2001/XMLSchema#date"/>
    


    <!-- 
    ///////////////////////////////////////////////////////////////////////////////////////
    //
    // Object Properties
    //
    ///////////////////////////////////////////////////////////////////////////////////////
     -->

    


    <!-- http://purl.org/dc/terms/license -->

    <owl:ObjectProperty rdf:about="http://purl.org/dc/terms/license"/>
    


    <!-- http://purl.org/dc/terms/publisher -->

    <owl:ObjectProperty rdf:about="http://purl.org/dc/terms/publisher">
        <owl:equivalentProperty rdf:resource="http://w3id.org/meta-share/meta-share/resourceProvider"/>
    </owl:ObjectProperty>
    


    <!-- http://purl.org/spar/datacite/hasIdentifier -->

    <owl:ObjectProperty rdf:about="http://purl.org/spar/datacite/hasIdentifier">
        <rdfs:domain rdf:resource="http://www.w3.org/2002/07/owl#Thing"/>
        <rdfs:range rdf:resource="http://purl.org/spar/datacite/Identifier"/>
        <rdfs:comment xml:lang="en">Associates an entity to an identifier, i.e. a string used to uniquely identify it</rdfs:comment>
        <rdfs:label xml:lang="en">has identifier</rdfs:label>
    </owl:ObjectProperty>
    


    <!-- http://purl.org/spar/datacite/usesIdentifierScheme -->

    <owl:ObjectProperty rdf:about="http://purl.org/spar/datacite/usesIdentifierScheme">
        <rdfs:domain rdf:resource="http://purl.org/spar/datacite/Identifier"/>
        <rdfs:range rdf:resource="http://purl.org/spar/datacite/IdentifierScheme"/>
        <rdfs:comment xml:lang="en">Indicates the scheme used for a specific identifier</rdfs:comment>
        <rdfs:label xml:lang="en">uses identifier scheme</rdfs:label>
    </owl:ObjectProperty>
    


    <!-- http://w3id.org/meta-share/meta-share/LTArea -->

    <owl:ObjectProperty rdf:about="http://w3id.org/meta-share/meta-share/LTArea">
        <rdfs:domain>
            <owl:Class>
                <owl:unionOf rdf:parseType="Collection">
                    <rdf:Description rdf:about="http://w3id.org/meta-share/meta-share/Division"/>
                    <rdf:Description rdf:about="http://w3id.org/meta-share/meta-share/Document"/>
                    <rdf:Description rdf:about="http://w3id.org/meta-share/meta-share/Group"/>
                    <rdf:Description rdf:about="http://w3id.org/meta-share/meta-share/Organization"/>
                    <rdf:Description rdf:about="http://w3id.org/meta-share/meta-share/Person"/>
                    <rdf:Description rdf:about="http://w3id.org/meta-share/meta-share/Project"/>
                </owl:unionOf>
            </owl:Class>
        </rdfs:domain>
        <rdfs:range rdf:resource="http://w3id.org/meta-share/omtd-share/Operation"/>
        <rdfs:altLabel xml:lang="en">Language Technology area</rdfs:altLabel>
        <rdfs:comment xml:lang="en">Introduces a Language Technology-related area that a person or organization is involved or active in</rdfs:comment>
        <rdfs:label xml:lang="en">LT area</rdfs:label>
    </owl:ObjectProperty>
    


    <!-- http://w3id.org/meta-share/meta-share/LΤRelatedTo -->

    <owl:ObjectProperty rdf:about="http://w3id.org/meta-share/meta-share/LΤRelatedTo">
        <rdfs:subPropertyOf rdf:resource="http://w3id.org/meta-share/meta-share/isRelatedTo"/>
        <owl:inverseOf rdf:resource="http://w3id.org/meta-share/meta-share/isRelatedToLT"/>
        <rdfs:domain rdf:resource="http://w3id.org/meta-share/meta-share/ToolService"/>
        <rdfs:range rdf:resource="http://w3id.org/meta-share/meta-share/DataLanguageResource"/>
        <rdfs:comment xml:lang="en">Links a tool/service (the one being described) to a language resource that bears some relation to it</rdfs:comment>
        <rdfs:label xml:lang="en">LT tool/service related to</rdfs:label>
    </owl:ObjectProperty>
    


    <!-- http://w3id.org/meta-share/meta-share/MDRecordRelatedTo -->

    <owl:ObjectProperty rdf:about="http://w3id.org/meta-share/meta-share/MDRecordRelatedTo">
        <rdfs:subPropertyOf rdf:resource="http://w3id.org/meta-share/meta-share/isRelatedTo"/>
        <owl:inverseOf rdf:resource="http://w3id.org/meta-share/meta-share/isRelatedToMDRecord"/>
        <rdfs:domain rdf:resource="http://w3id.org/meta-share/meta-share/MetadataRecord"/>
        <rdfs:range>
            <owl:Class>
                <owl:unionOf rdf:parseType="Collection">
                    <rdf:Description rdf:about="http://w3id.org/meta-share/meta-share/LanguageResource"/>
                    <rdf:Description rdf:about="http://w3id.org/meta-share/meta-share/MetadataRecord"/>
                </owl:unionOf>
            </owl:Class>
        </rdfs:range>
        <rdfs:comment xml:lang="en">Links an external metadata record that has some relation with the metadata record of the resource being described or the resource itself</rdfs:comment>
        <rdfs:label xml:lang="en">metadata record related to</rdfs:label>
    </owl:ObjectProperty>
    


    <!-- http://w3id.org/meta-share/meta-share/accessRights -->

    <owl:ObjectProperty rdf:about="http://w3id.org/meta-share/meta-share/accessRights">
        <rdfs:domain rdf:resource="http://w3id.org/meta-share/meta-share/Distribution"/>
        <rdfs:range rdf:resource="http://w3id.org/meta-share/meta-share/AccessRightsStatement"/>
        <rdfs:comment xml:lang="en">Specifies the rights for accessing the distributable form(s) of a language resource (preferrably in accordance to a formalised vocabulary)</rdfs:comment>
        <rdfs:label xml:lang="en">access rights</rdfs:label>
    </owl:ObjectProperty>
    


    <!-- http://w3id.org/meta-share/meta-share/accesses -->

    <owl:ObjectProperty rdf:about="http://w3id.org/meta-share/meta-share/accesses">
        <rdfs:subPropertyOf rdf:resource="http://w3id.org/meta-share/meta-share/LΤRelatedTo"/>
        <owl:inverseOf rdf:resource="http://w3id.org/meta-share/meta-share/isAccessedBy"/>
        <rdfs:domain rdf:resource="http://w3id.org/meta-share/meta-share/ToolService"/>
        <rdfs:range>
            <owl:Class>
                <owl:unionOf rdf:parseType="Collection">
                    <rdf:Description rdf:about="http://w3id.org/meta-share/meta-share/DataLanguageResource"/>
                    <rdf:Description rdf:about="http://w3id.org/meta-share/meta-share/MediaPart"/>
                </owl:unionOf>
            </owl:Class>
        </rdfs:range>
        <rdfs:comment xml:lang="en">Links a tool/service B that is (or can be) used for accessing LR A (e.g.,  a corpus workbench, s/w for lexicon access) to the LR A</rdfs:comment>
        <rdfs:label xml:lang="en">accesses</rdfs:label>
    </owl:ObjectProperty>
    


    <!-- http://w3id.org/meta-share/meta-share/actorRelatedTo -->

    <owl:ObjectProperty rdf:about="http://w3id.org/meta-share/meta-share/actorRelatedTo">
        <rdfs:subPropertyOf rdf:resource="http://w3id.org/meta-share/meta-share/isRelatedTo"/>
        <owl:inverseOf rdf:resource="http://w3id.org/meta-share/meta-share/isRelatedToActor"/>
        <rdfs:domain rdf:resource="http://w3id.org/meta-share/meta-share/Actor"/>
        <rdfs:range rdf:resource="http://w3id.org/meta-share/meta-share/LanguageResource"/>
        <rdfs:comment xml:lang="en">Links actors to a language resource  with which they have some relation</rdfs:comment>
        <rdfs:label xml:lang="en">actor related to</rdfs:label>
    </owl:ObjectProperty>
    


    <!-- http://w3id.org/meta-share/meta-share/actualUse -->

    <owl:ObjectProperty rdf:about="http://w3id.org/meta-share/meta-share/actualUse">
        <rdfs:domain rdf:resource="http://w3id.org/meta-share/meta-share/LanguageResource"/>
        <rdfs:range rdf:resource="http://w3id.org/meta-share/meta-share/ActualUse"/>
        <rdfs:comment xml:lang="en">Provides information on how the resource has been used (e.g.,  in a project, for a publication, for testing a tool/service, etc.)</rdfs:comment>
        <rdfs:label xml:lang="en">actual use</rdfs:label>
    </owl:ObjectProperty>
    


    <!-- http://w3id.org/meta-share/meta-share/addressSet -->

    <owl:ObjectProperty rdf:about="http://w3id.org/meta-share/meta-share/addressSet">
        <rdfs:domain>
            <owl:Class>
                <owl:unionOf rdf:parseType="Collection">
                    <rdf:Description rdf:about="http://w3id.org/meta-share/meta-share/Affiliation"/>
                    <rdf:Description rdf:about="http://w3id.org/meta-share/meta-share/Division"/>
                    <rdf:Description rdf:about="http://w3id.org/meta-share/meta-share/Group"/>
                    <rdf:Description rdf:about="http://w3id.org/meta-share/meta-share/Organization"/>
                    <rdf:Description rdf:about="http://w3id.org/meta-share/meta-share/Person"/>
                </owl:unionOf>
            </owl:Class>
        </rdfs:domain>
        <rdfs:range rdf:resource="http://w3id.org/meta-share/meta-share/AddressSet"/>
        <rdfs:comment xml:lang="en">Links to a set of elements that describe the full address of a person or organization (i.e. including street address, zip code, etc.)</rdfs:comment>
        <rdfs:label xml:lang="en">address</rdfs:label>
    </owl:ObjectProperty>
    


    <!-- http://w3id.org/meta-share/meta-share/affiliatedOrganization -->

    <owl:ObjectProperty rdf:about="http://w3id.org/meta-share/meta-share/affiliatedOrganization">
        <rdfs:domain rdf:resource="http://w3id.org/meta-share/meta-share/Affiliation"/>
        <rdfs:range rdf:resource="http://w3id.org/meta-share/meta-share/Organization"/>
        <rdfs:comment xml:lang="en">Specifies the organization that a person is affiliated with or works for</rdfs:comment>
        <rdfs:label xml:lang="en">affiliated organization</rdfs:label>
    </owl:ObjectProperty>
    


    <!-- http://w3id.org/meta-share/meta-share/affiliation -->

    <owl:ObjectProperty rdf:about="http://w3id.org/meta-share/meta-share/affiliation">
        <rdfs:domain rdf:resource="http://w3id.org/meta-share/meta-share/Person"/>
        <rdfs:range rdf:resource="http://w3id.org/meta-share/meta-share/Affiliation"/>
        <rdfs:comment xml:lang="en">Introduces information on an organization to whom the person is affiliated and the data relevant to this relation (i.e. position, email , etc.)</rdfs:comment>
        <rdfs:label xml:lang="en">affiliation</rdfs:label>
    </owl:ObjectProperty>
    


    <!-- http://w3id.org/meta-share/meta-share/ageGroup -->

    <owl:ObjectProperty rdf:about="http://w3id.org/meta-share/meta-share/ageGroup">
        <rdfs:domain rdf:resource="http://w3id.org/meta-share/meta-share/Participant"/>
        <rdfs:range rdf:resource="http://w3id.org/meta-share/meta-share/AgeGroup"/>
        <rdfs:comment xml:lang="en">The age group to which the participant belongs</rdfs:comment>
        <rdfs:label xml:lang="en">age group</rdfs:label>
    </owl:ObjectProperty>
    


    <!-- http://w3id.org/meta-share/meta-share/ageGroupOfParticipants -->

    <owl:ObjectProperty rdf:about="http://w3id.org/meta-share/meta-share/ageGroupOfParticipants">
        <rdfs:domain>
            <owl:Class>
                <owl:unionOf rdf:parseType="Collection">
                    <rdf:Description rdf:about="http://w3id.org/meta-share/meta-share/CorpusAudioPart"/>
                    <rdf:Description rdf:about="http://w3id.org/meta-share/meta-share/CorpusImagePart"/>
                    <rdf:Description rdf:about="http://w3id.org/meta-share/meta-share/CorpusTextNumericalPart"/>
                    <rdf:Description rdf:about="http://w3id.org/meta-share/meta-share/CorpusVideoPart"/>
                </owl:unionOf>
            </owl:Class>
        </rdfs:domain>
        <rdfs:range rdf:resource="http://w3id.org/meta-share/meta-share/AgeGroup"/>
        <rdfs:comment xml:lang="en">The age range of the group of participants</rdfs:comment>
        <rdfs:label xml:lang="en">age group of participants</rdfs:label>
    </owl:ObjectProperty>
    


    <!-- http://w3id.org/meta-share/meta-share/annotatedElement -->

    <owl:ObjectProperty rdf:about="http://w3id.org/meta-share/meta-share/annotatedElement">
        <rdfs:domain rdf:resource="http://w3id.org/meta-share/meta-share/Annotation"/>
        <rdfs:range rdf:resource="http://w3id.org/meta-share/meta-share/AnnotatedElement"/>
        <rdfs:comment xml:lang="en">Specifies the elements annotated at each annotation level</rdfs:comment>
        <rdfs:label xml:lang="en">annotated element</rdfs:label>
    </owl:ObjectProperty>
    


    <!-- http://w3id.org/meta-share/meta-share/annotation -->

    <owl:ObjectProperty rdf:about="http://w3id.org/meta-share/meta-share/annotation">
        <rdfs:domain rdf:resource="http://w3id.org/meta-share/meta-share/CorpusMediaPart"/>
        <rdfs:range rdf:resource="http://w3id.org/meta-share/meta-share/Annotation"/>
        <rdfs:comment xml:lang="en">Links a corpus to its annotated part(s)</rdfs:comment>
        <rdfs:label xml:lang="en">annotation</rdfs:label>
    </owl:ObjectProperty>
    


    <!-- http://w3id.org/meta-share/meta-share/annotationMode -->

    <owl:ObjectProperty rdf:about="http://w3id.org/meta-share/meta-share/annotationMode">
        <rdfs:subPropertyOf rdf:resource="http://w3id.org/meta-share/meta-share/processMode"/>
        <rdfs:domain rdf:resource="http://w3id.org/meta-share/meta-share/Annotation"/>
        <rdfs:range rdf:resource="http://w3id.org/meta-share/meta-share/ProcessMode"/>
        <rdfs:comment xml:lang="en">Indicates whether the resource is annotated manually or by automatic processes</rdfs:comment>
        <rdfs:label xml:lang="en">annotation mode</rdfs:label>
    </owl:ObjectProperty>
    


    <!-- http://w3id.org/meta-share/meta-share/annotationReport -->

    <owl:ObjectProperty rdf:about="http://w3id.org/meta-share/meta-share/annotationReport">
        <rdfs:subPropertyOf rdf:resource="http://w3id.org/meta-share/meta-share/isDocumentedBy"/>
        <owl:inverseOf rdf:resource="http://w3id.org/meta-share/meta-share/documentsAnnotation"/>
        <rdfs:domain rdf:resource="http://w3id.org/meta-share/meta-share/Annotation"/>
        <rdfs:range rdf:resource="http://w3id.org/meta-share/meta-share/Document"/>
        <rdfs:comment xml:lang="en">Links to a report describing the annotation process, tool, method , etc. of the language resource</rdfs:comment>
        <rdfs:label xml:lang="en">annotation report</rdfs:label>
    </owl:ObjectProperty>
    


    <!-- http://w3id.org/meta-share/meta-share/annotationResource -->

    <owl:ObjectProperty rdf:about="http://w3id.org/meta-share/meta-share/annotationResource">
        <rdfs:subPropertyOf rdf:resource="http://w3id.org/meta-share/meta-share/dependsOn"/>
        <owl:inverseOf rdf:resource="http://w3id.org/meta-share/meta-share/isAnnotationResourceOf"/>
        <rdfs:domain>
            <owl:Class>
                <owl:unionOf rdf:parseType="Collection">
                    <rdf:Description rdf:about="http://w3id.org/meta-share/meta-share/MLModel"/>
                    <rdf:Description rdf:about="http://w3id.org/meta-share/meta-share/ProcessingResource"/>
                    <rdf:Description rdf:about="http://w3id.org/meta-share/meta-share/ToolService"/>
                </owl:unionOf>
            </owl:Class>
        </rdfs:domain>
        <rdfs:range rdf:resource="http://w3id.org/meta-share/meta-share/LexicalConceptualResource"/>
        <rdfs:comment xml:lang="en">Specifies the annotation resource used for annotating a corpus or that has been used for the input resource of a tool/service or that should be used (dependency) for the annotation</rdfs:comment>
        <rdfs:label xml:lang="en">annotation resource</rdfs:label>
    </owl:ObjectProperty>
    


    <!-- http://w3id.org/meta-share/meta-share/annotationSchema -->

    <owl:ObjectProperty rdf:about="http://w3id.org/meta-share/meta-share/annotationSchema">
        <rdfs:subPropertyOf rdf:resource="http://w3id.org/meta-share/meta-share/dependsOn"/>
        <owl:inverseOf rdf:resource="http://w3id.org/meta-share/meta-share/isAnnotationSchemaOf"/>
        <rdfs:domain>
            <owl:Class>
                <owl:unionOf rdf:parseType="Collection">
                    <rdf:Description rdf:about="http://w3id.org/meta-share/meta-share/MLModel"/>
                    <rdf:Description rdf:about="http://w3id.org/meta-share/meta-share/ProcessingResource"/>
                    <rdf:Description rdf:about="http://w3id.org/meta-share/meta-share/ToolService"/>
                </owl:unionOf>
            </owl:Class>
        </rdfs:domain>
        <rdfs:range rdf:resource="http://w3id.org/meta-share/meta-share/LexicalConceptualResource"/>
        <rdfs:comment xml:lang="en">The annotation schema used for annotating a resource or for the input resource (if annotated) of a tool/service or that should be used (dependency) for the annotation</rdfs:comment>
        <rdfs:label xml:lang="en">annotation schema</rdfs:label>
    </owl:ObjectProperty>
    


    <!-- http://w3id.org/meta-share/meta-share/annotationType -->

    <owl:ObjectProperty rdf:about="http://w3id.org/meta-share/meta-share/annotationType">
        <rdfs:domain rdf:resource="http://w3id.org/meta-share/meta-share/Annotation"/>
        <rdfs:range rdf:resource="http://w3id.org/meta-share/omtd-share/AnnotationType"/>
        <rdfs:comment xml:lang="en">Specifies the annotation type of the annotated version(s) of a resource or the annotation type a tool/ service requires or produces as an output</rdfs:comment>
        <rdfs:label xml:lang="en">annotation type</rdfs:label>
    </owl:ObjectProperty>
    


    <!-- http://w3id.org/meta-share/meta-share/annotator -->

    <owl:ObjectProperty rdf:about="http://w3id.org/meta-share/meta-share/annotator">
        <rdfs:subPropertyOf rdf:resource="http://w3id.org/meta-share/meta-share/isRelatedToActor"/>
        <owl:inverseOf rdf:resource="http://w3id.org/meta-share/meta-share/isAnnotatorOf"/>
        <rdfs:domain rdf:resource="http://w3id.org/meta-share/meta-share/Annotation"/>
        <rdfs:range rdf:resource="http://w3id.org/meta-share/meta-share/Actor"/>
        <rdfs:comment xml:lang="en">Identifies the person or organisation responsible for the annotation of a resource</rdfs:comment>
        <rdfs:label xml:lang="en">annotator</rdfs:label>
    </owl:ObjectProperty>
    


    <!-- http://w3id.org/meta-share/meta-share/audience -->

    <owl:ObjectProperty rdf:about="http://w3id.org/meta-share/meta-share/audience">
        <rdfs:domain>
            <owl:Class>
                <owl:unionOf rdf:parseType="Collection">
                    <rdf:Description rdf:about="http://w3id.org/meta-share/meta-share/CorpusAudioPart"/>
                    <rdf:Description rdf:about="http://w3id.org/meta-share/meta-share/CorpusVideoPart"/>
                </owl:unionOf>
            </owl:Class>
        </rdfs:domain>
        <rdfs:range rdf:resource="http://w3id.org/meta-share/meta-share/Audience"/>
        <rdfs:comment xml:lang="en">Indicates the intended audience size of a multimedia resource</rdfs:comment>
        <rdfs:label xml:lang="en">audience</rdfs:label>
    </owl:ObjectProperty>
    


    <!-- http://w3id.org/meta-share/meta-share/audioFormat -->

    <owl:ObjectProperty rdf:about="http://w3id.org/meta-share/meta-share/audioFormat">
        <rdfs:domain>
            <owl:Class>
                <owl:unionOf rdf:parseType="Collection">
                    <rdf:Description rdf:about="http://w3id.org/meta-share/meta-share/CorpusAudioPart"/>
                    <rdf:Description rdf:about="http://w3id.org/meta-share/meta-share/LexicalConceptualResourceAudioPart"/>
                </owl:unionOf>
            </owl:Class>
        </rdfs:domain>
        <rdfs:range rdf:resource="http://w3id.org/meta-share/meta-share/AudioFormat"/>
        <rdfs:comment xml:lang="en">Specifies the features of the format of the audio part of a language resource</rdfs:comment>
        <rdfs:label xml:lang="en">audio format</rdfs:label>
    </owl:ObjectProperty>
    


    <!-- http://w3id.org/meta-share/meta-share/audioQualityMeasureIncluded -->

    <owl:ObjectProperty rdf:about="http://w3id.org/meta-share/meta-share/audioQualityMeasureIncluded">
        <rdfs:domain rdf:resource="http://w3id.org/meta-share/meta-share/AudioFormat"/>
        <rdfs:range rdf:resource="http://w3id.org/meta-share/meta-share/AudioQualityMeasureIncluded"/>
        <rdfs:comment xml:lang="en">Specifies the audio quality measures</rdfs:comment>
        <rdfs:label xml:lang="en">audio quality measure included</rdfs:label>
    </owl:ObjectProperty>
    


    <!-- http://w3id.org/meta-share/meta-share/author -->

    <owl:ObjectProperty rdf:about="http://w3id.org/meta-share/meta-share/author">
        <rdfs:domain rdf:resource="http://w3id.org/meta-share/meta-share/Document"/>
        <rdfs:range rdf:resource="http://w3id.org/meta-share/meta-share/Person"/>
        <rdfs:comment xml:lang="en">Introduces the details for a person that has created the document being described</rdfs:comment>
        <rdfs:label xml:lang="en">author</rdfs:label>
    </owl:ObjectProperty>
    


    <!-- http://w3id.org/meta-share/meta-share/availability -->

    <owl:ObjectProperty rdf:about="http://w3id.org/meta-share/meta-share/availability">
        <rdfs:domain rdf:resource="http://w3id.org/meta-share/meta-share/Distribution"/>
        <rdfs:range rdf:resource="http://w3id.org/meta-share/meta-share/Availability"/>
        <rdfs:comment xml:lang="en">Specifies the availability status of the resource</rdfs:comment>
        <rdfs:label xml:lang="en">availability</rdfs:label>
    </owl:ObjectProperty>
    


    <!-- http://w3id.org/meta-share/meta-share/baseItem -->

    <owl:ObjectProperty rdf:about="http://w3id.org/meta-share/meta-share/baseItem">
        <rdfs:domain rdf:resource="http://w3id.org/meta-share/meta-share/NGramModel"/>
        <rdfs:range rdf:resource="http://w3id.org/meta-share/meta-share/BaseItem"/>
        <rdfs:comment xml:lang="en">Type of item that is represented in the n-gram resource</rdfs:comment>
        <rdfs:label xml:lang="en">base item</rdfs:label>
    </owl:ObjectProperty>
    


    <!-- http://w3id.org/meta-share/meta-share/bodyPart -->

    <owl:ObjectProperty rdf:about="http://w3id.org/meta-share/meta-share/bodyPart">
        <rdfs:domain>
            <owl:Class>
                <owl:unionOf rdf:parseType="Collection">
                    <rdf:Description rdf:about="http://w3id.org/meta-share/meta-share/DynamicElement"/>
                    <rdf:Description rdf:about="http://w3id.org/meta-share/meta-share/StaticElement"/>
                </owl:unionOf>
            </owl:Class>
        </rdfs:domain>
        <rdfs:range rdf:resource="http://w3id.org/meta-share/meta-share/BodyPart"/>
        <rdfs:comment xml:lang="en">Specifies the body parts visible in the video or image part of the resource</rdfs:comment>
        <rdfs:label xml:lang="en">body part</rdfs:label>
    </owl:ObjectProperty>
    


    <!-- http://w3id.org/meta-share/meta-share/byteOrder -->

    <owl:ObjectProperty rdf:about="http://w3id.org/meta-share/meta-share/byteOrder">
        <rdfs:domain rdf:resource="http://w3id.org/meta-share/meta-share/AudioFormat"/>
        <rdfs:range rdf:resource="http://w3id.org/meta-share/meta-share/ByteOrder"/>
        <rdfs:comment xml:lang="en">Specifies the byte order of 2 or more bytes sample</rdfs:comment>
        <rdfs:label xml:lang="en">byte order</rdfs:label>
    </owl:ObjectProperty>
    


    <!-- http://w3id.org/meta-share/meta-share/capturingDeviceType -->

    <owl:ObjectProperty rdf:about="http://w3id.org/meta-share/meta-share/capturingDeviceType">
        <rdfs:domain>
            <owl:Class>
                <owl:unionOf rdf:parseType="Collection">
                    <rdf:Description rdf:about="http://w3id.org/meta-share/meta-share/CorpusAudioPart"/>
                    <rdf:Description rdf:about="http://w3id.org/meta-share/meta-share/CorpusImagePart"/>
                    <rdf:Description rdf:about="http://w3id.org/meta-share/meta-share/CorpusTextNumericalPart"/>
                    <rdf:Description rdf:about="http://w3id.org/meta-share/meta-share/CorpusVideoPart"/>
                </owl:unionOf>
            </owl:Class>
        </rdfs:domain>
        <rdfs:range rdf:resource="http://w3id.org/meta-share/meta-share/CapturingDeviceType"/>
        <rdfs:comment xml:lang="en">Provides information on the type of the transducers through which the data is captured</rdfs:comment>
        <rdfs:label xml:lang="en">capturing device type</rdfs:label>
    </owl:ObjectProperty>
    


    <!-- http://w3id.org/meta-share/meta-share/capturingEnvironment -->

    <owl:ObjectProperty rdf:about="http://w3id.org/meta-share/meta-share/capturingEnvironment">
        <rdfs:domain>
            <owl:Class>
                <owl:unionOf rdf:parseType="Collection">
                    <rdf:Description rdf:about="http://w3id.org/meta-share/meta-share/CorpusAudioPart"/>
                    <rdf:Description rdf:about="http://w3id.org/meta-share/meta-share/CorpusImagePart"/>
                    <rdf:Description rdf:about="http://w3id.org/meta-share/meta-share/CorpusTextNumericalPart"/>
                    <rdf:Description rdf:about="http://w3id.org/meta-share/meta-share/CorpusVideoPart"/>
                </owl:unionOf>
            </owl:Class>
        </rdfs:domain>
        <rdfs:range rdf:resource="http://w3id.org/meta-share/meta-share/CapturingEnvironment"/>
        <rdfs:comment xml:lang="en">Specifies the type of the capturing environment</rdfs:comment>
        <rdfs:label xml:lang="en">capturing environment</rdfs:label>
    </owl:ObjectProperty>
    


    <!-- http://w3id.org/meta-share/meta-share/characterEncoding -->

    <owl:ObjectProperty rdf:about="http://w3id.org/meta-share/meta-share/characterEncoding">
        <rdfs:domain rdf:resource="http://w3id.org/meta-share/meta-share/DistributionTextFeature"/>
        <rdfs:range rdf:resource="http://w3id.org/meta-share/meta-share/CharacterEncoding"/>
        <rdfs:comment xml:lang="en">Specifies the character encoding used for a language resource data distribution</rdfs:comment>
        <rdfs:label xml:lang="en">character encoding</rdfs:label>
    </owl:ObjectProperty>
    


    <!-- http://w3id.org/meta-share/meta-share/cites -->

    <owl:ObjectProperty rdf:about="http://w3id.org/meta-share/meta-share/cites">
        <rdfs:subPropertyOf rdf:resource="http://w3id.org/meta-share/meta-share/documentRelatedTo"/>
        <owl:inverseOf rdf:resource="http://w3id.org/meta-share/meta-share/isCitedBy"/>
        <rdfs:domain rdf:resource="http://w3id.org/meta-share/meta-share/Document"/>
        <rdfs:range rdf:resource="http://w3id.org/meta-share/meta-share/LanguageResource"/>
        <rdfs:comment xml:lang="en">Links to the language resource(s) that a publication includes in its citations</rdfs:comment>
        <rdfs:label xml:lang="en">cites</rdfs:label>
    </owl:ObjectProperty>
    


    <!-- http://w3id.org/meta-share/meta-share/colourSpace -->

    <owl:ObjectProperty rdf:about="http://w3id.org/meta-share/meta-share/colourSpace">
        <rdfs:domain>
            <owl:Class>
                <owl:unionOf rdf:parseType="Collection">
                    <rdf:Description rdf:about="http://w3id.org/meta-share/meta-share/ImageFormat"/>
                    <rdf:Description rdf:about="http://w3id.org/meta-share/meta-share/VideoFormat"/>
                </owl:unionOf>
            </owl:Class>
        </rdfs:domain>
        <rdfs:range rdf:resource="http://w3id.org/meta-share/meta-share/ColourSpace"/>
        <rdfs:comment xml:lang="en">Defines the colour space for the video</rdfs:comment>
        <rdfs:label xml:lang="en">colour space</rdfs:label>
    </owl:ObjectProperty>
    


    <!-- http://w3id.org/meta-share/meta-share/compatibleLexiconType -->

    <owl:ObjectProperty rdf:about="http://w3id.org/meta-share/meta-share/compatibleLexiconType">
        <rdfs:domain rdf:resource="http://w3id.org/meta-share/meta-share/LanguageDescription"/>
        <rdfs:range rdf:resource="http://w3id.org/meta-share/meta-share/CompatibleLexiconType"/>
        <rdfs:comment xml:lang="en">Specifies the type of (external) lexicon that can be used with the grammar</rdfs:comment>
        <rdfs:label xml:lang="en">compatible lexicon type</rdfs:label>
    </owl:ObjectProperty>
    


    <!-- http://w3id.org/meta-share/meta-share/compliesWith -->

    <owl:ObjectProperty rdf:about="http://w3id.org/meta-share/meta-share/compliesWith">
        <rdfs:domain>
            <owl:Class>
                <owl:unionOf rdf:parseType="Collection">
                    <rdf:Description rdf:about="http://w3id.org/meta-share/meta-share/LanguageResource"/>
                    <rdf:Description rdf:about="http://w3id.org/meta-share/meta-share/MetadataRecord"/>
                </owl:unionOf>
            </owl:Class>
        </rdfs:domain>
        <rdfs:range rdf:resource="http://w3id.org/meta-share/meta-share/StandardBestPractice"/>
        <rdfs:comment xml:lang="en">Specifies the vocabulary/standard/best practice to which a resource is compliant with</rdfs:comment>
        <rdfs:label xml:lang="en">complies with</rdfs:label>
    </owl:ObjectProperty>
    


    <!-- http://w3id.org/meta-share/meta-share/compressionName -->

    <owl:ObjectProperty rdf:about="http://w3id.org/meta-share/meta-share/compressionName">
        <rdfs:domain>
            <owl:Class>
                <owl:unionOf rdf:parseType="Collection">
                    <rdf:Description rdf:about="http://w3id.org/meta-share/meta-share/AudioFormat"/>
                    <rdf:Description rdf:about="http://w3id.org/meta-share/meta-share/ImageFormat"/>
                    <rdf:Description rdf:about="http://w3id.org/meta-share/meta-share/VideoFormat"/>
                </owl:unionOf>
            </owl:Class>
        </rdfs:domain>
        <rdfs:range rdf:resource="http://w3id.org/meta-share/meta-share/CompressionName"/>
        <rdfs:comment xml:lang="en">The name of the compression applied</rdfs:comment>
        <rdfs:label xml:lang="en">compression name</rdfs:label>
    </owl:ObjectProperty>
    


    <!-- http://w3id.org/meta-share/meta-share/conditionOfUse -->

    <owl:ObjectProperty rdf:about="http://w3id.org/meta-share/meta-share/conditionOfUse">
        <rdfs:domain rdf:resource="http://w3id.org/meta-share/meta-share/LicenceTerms"/>
        <rdfs:range rdf:resource="http://w3id.org/meta-share/meta-share/ConditionOfUse"/>
        <rdfs:comment xml:lang="en">Links a licence with a specific condition/term of use imposed for accessing a language resource. It is an optional element and only to be taken as providing brief human readable information on the fact that the language resource is provided under a specific set of conditions. These correspond to the most frequently used conditions imposed by the licensor (via the specified licence). The proper exposition of all conditions and possible exceptions is to be found inside the licence text. Depositors should, hence, carefully choose the values of this field to match the licence chosen and users should carefully read that licence before using the language resource.</rdfs:comment>
        <rdfs:label xml:lang="en">condition of use</rdfs:label>
    </owl:ObjectProperty>
    


    <!-- http://w3id.org/meta-share/meta-share/conformsTo -->

    <owl:ObjectProperty rdf:about="http://w3id.org/meta-share/meta-share/conformsTo">
        <rdfs:domain rdf:resource="http://w3id.org/meta-share/meta-share/Classification"/>
        <rdfs:range rdf:resource="http://w3id.org/meta-share/meta-share/ClassificationScheme"/>
        <rdfs:comment xml:lang="en">Specifies the vocabulary/scheme to which a value (e.g.,  as of text genre, domain, etc.) conforms to</rdfs:comment>
        <rdfs:label xml:lang="en">conforms to</rdfs:label>
    </owl:ObjectProperty>
    


    <!-- http://w3id.org/meta-share/meta-share/contact -->

    <owl:ObjectProperty rdf:about="http://w3id.org/meta-share/meta-share/contact">
        <rdfs:subPropertyOf rdf:resource="http://w3id.org/meta-share/meta-share/isRelatedToActor"/>
        <owl:inverseOf rdf:resource="http://w3id.org/meta-share/meta-share/isContactFor"/>
        <rdfs:domain rdf:resource="http://w3id.org/meta-share/meta-share/LanguageResource"/>
        <rdfs:range rdf:resource="http://w3id.org/meta-share/meta-share/Actor"/>
        <rdfs:comment xml:lang="en">Specifies the data of the person/organization/group that can be contacted for information about a language resource</rdfs:comment>
        <rdfs:label xml:lang="en">contact</rdfs:label>
    </owl:ObjectProperty>
    


    <!-- http://w3id.org/meta-share/meta-share/contributor -->

    <owl:ObjectProperty rdf:about="http://w3id.org/meta-share/meta-share/contributor">
        <rdfs:domain rdf:resource="http://w3id.org/meta-share/meta-share/Document"/>
        <rdfs:range rdf:resource="http://w3id.org/meta-share/meta-share/Person"/>
        <rdfs:comment xml:lang="en">Introduces the details for a person that has contributed in some way to the production of a document or resource</rdfs:comment>
        <rdfs:label xml:lang="en">contributor</rdfs:label>
    </owl:ObjectProperty>
    


    <!-- http://w3id.org/meta-share/meta-share/conversationalType -->

    <owl:ObjectProperty rdf:about="http://w3id.org/meta-share/meta-share/conversationalType">
        <rdfs:domain>
            <owl:Class>
                <owl:unionOf rdf:parseType="Collection">
                    <rdf:Description rdf:about="http://w3id.org/meta-share/meta-share/CorpusAudioPart"/>
                    <rdf:Description rdf:about="http://w3id.org/meta-share/meta-share/CorpusVideoPart"/>
                </owl:unionOf>
            </owl:Class>
        </rdfs:domain>
        <rdfs:range rdf:resource="http://w3id.org/meta-share/meta-share/ConversationalType"/>
        <rdfs:comment xml:lang="en">Specifies the conversational type of a multimedia resource</rdfs:comment>
        <rdfs:label xml:lang="en">conversational type</rdfs:label>
    </owl:ObjectProperty>
    


    <!-- http://w3id.org/meta-share/meta-share/coordinator -->

    <owl:ObjectProperty rdf:about="http://w3id.org/meta-share/meta-share/coordinator">
        <rdfs:domain rdf:resource="http://w3id.org/meta-share/meta-share/Project"/>
        <rdfs:range rdf:resource="http://w3id.org/meta-share/meta-share/Organization"/>
        <rdfs:altLabel xml:lang="en">co-ordinator</rdfs:altLabel>
        <rdfs:comment xml:lang="en">Introduces the details for an organization that coordinates the project being described</rdfs:comment>
        <rdfs:label xml:lang="en">coordinator</rdfs:label>
    </owl:ObjectProperty>
    


    <!-- http://w3id.org/meta-share/meta-share/corpusSubclass -->

    <owl:ObjectProperty rdf:about="http://w3id.org/meta-share/meta-share/corpusSubclass">
        <rdfs:domain rdf:resource="http://w3id.org/meta-share/meta-share/Corpus"/>
        <rdfs:range rdf:resource="http://w3id.org/meta-share/meta-share/CorpusSubclass"/>
        <rdfs:comment xml:lang="en">Introduces a classification of corpora into types (used for descriptive reasons)</rdfs:comment>
        <rdfs:label xml:lang="en">corpus subclass</rdfs:label>
    </owl:ObjectProperty>
    


    <!-- http://w3id.org/meta-share/meta-share/cost -->

    <owl:ObjectProperty rdf:about="http://w3id.org/meta-share/meta-share/cost">
        <rdfs:domain rdf:resource="http://w3id.org/meta-share/meta-share/Project"/>
        <rdfs:range rdf:resource="http://w3id.org/meta-share/meta-share/Cost"/>
        <rdfs:comment xml:lang="en">Introduces the cost for accessing a resource, formally described as a set of amount and currency unit</rdfs:comment>
        <rdfs:label xml:lang="en">cost</rdfs:label>
    </owl:ObjectProperty>
    


    <!-- http://w3id.org/meta-share/meta-share/country -->

    <owl:ObjectProperty rdf:about="http://w3id.org/meta-share/meta-share/country">
        <rdfs:domain rdf:resource="http://w3id.org/meta-share/meta-share/AddressSet"/>
        <rdfs:range rdf:resource="http://w3id.org/meta-share/meta-share/Country"/>
        <rdfs:comment xml:lang="en">Introduces the name of the country mentioned in the postal address of a person or organization as defined in the list of values of ISO 3166</rdfs:comment>
        <rdfs:label xml:lang="en">country</rdfs:label>
    </owl:ObjectProperty>
    


    <!-- http://w3id.org/meta-share/meta-share/countryOfRegistration -->

    <owl:ObjectProperty rdf:about="http://w3id.org/meta-share/meta-share/countryOfRegistration">
        <rdfs:domain>
            <owl:Class>
                <owl:unionOf rdf:parseType="Collection">
                    <rdf:Description rdf:about="http://w3id.org/meta-share/meta-share/Division"/>
                    <rdf:Description rdf:about="http://w3id.org/meta-share/meta-share/Organization"/>
                </owl:unionOf>
            </owl:Class>
        </rdfs:domain>
        <rdfs:range rdf:resource="http://w3id.org/meta-share/meta-share/Country"/>
        <rdfs:comment xml:lang="en">Introduces the country in which a company has been first registered as a legal entity</rdfs:comment>
        <rdfs:label xml:lang="en">country of registration</rdfs:label>
    </owl:ObjectProperty>
    


    <!-- http://w3id.org/meta-share/meta-share/creationMode -->

    <owl:ObjectProperty rdf:about="http://w3id.org/meta-share/meta-share/creationMode">
        <rdfs:subPropertyOf rdf:resource="http://w3id.org/meta-share/meta-share/processMode"/>
        <rdfs:domain>
            <owl:Class>
                <owl:unionOf rdf:parseType="Collection">
                    <rdf:Description rdf:about="http://w3id.org/meta-share/meta-share/LexicalConceptualResource"/>
                    <rdf:Description rdf:about="http://w3id.org/meta-share/meta-share/MediaPart"/>
                </owl:unionOf>
            </owl:Class>
        </rdfs:domain>
        <rdfs:range rdf:resource="http://w3id.org/meta-share/meta-share/ProcessMode"/>
        <rdfs:comment xml:lang="en">Specifies whether the resource was created automatically or in a manual or interactive mode</rdfs:comment>
        <rdfs:label xml:lang="en">creation mode</rdfs:label>
    </owl:ObjectProperty>
    


    <!-- http://w3id.org/meta-share/meta-share/currency -->

    <owl:ObjectProperty rdf:about="http://w3id.org/meta-share/meta-share/currency">
        <rdfs:domain rdf:resource="http://w3id.org/meta-share/meta-share/Cost"/>
        <rdfs:range rdf:resource="http://w3id.org/meta-share/meta-share/Currency"/>
        <rdfs:comment xml:lang="en">Specifies the currency used for describing the cost of a resource</rdfs:comment>
        <rdfs:label xml:lang="en">currency</rdfs:label>
    </owl:ObjectProperty>
    


    <!-- http://w3id.org/meta-share/meta-share/dataFormat -->

    <owl:ObjectProperty rdf:about="http://w3id.org/meta-share/meta-share/dataFormat">
        <rdfs:domain>
            <owl:Class>
                <owl:unionOf rdf:parseType="Collection">
                    <rdf:Description rdf:about="http://w3id.org/meta-share/meta-share/AudioFormat"/>
                    <rdf:Description rdf:about="http://w3id.org/meta-share/meta-share/DistributionTextFeature"/>
                    <rdf:Description rdf:about="http://w3id.org/meta-share/meta-share/DistributionTextNumericalFeature"/>
                    <rdf:Description rdf:about="http://w3id.org/meta-share/meta-share/ImageFormat"/>
                    <rdf:Description rdf:about="http://w3id.org/meta-share/meta-share/Parameter"/>
                    <rdf:Description rdf:about="http://w3id.org/meta-share/meta-share/VideoFormat"/>
                </owl:unionOf>
            </owl:Class>
        </rdfs:domain>
        <rdfs:range rdf:resource="http://w3id.org/meta-share/omtd-share/DataFormat"/>
        <rdfs:comment xml:lang="en">Indicates the format(s) of a data resource</rdfs:comment>
        <rdfs:label xml:lang="en">data format</rdfs:label>
    </owl:ObjectProperty>
    


    <!-- http://w3id.org/meta-share/meta-share/dependentLR -->

    <owl:ObjectProperty rdf:about="http://w3id.org/meta-share/meta-share/dependentLR">
        <rdfs:subPropertyOf rdf:resource="http://w3id.org/meta-share/meta-share/isRelatedToLR"/>
        <owl:inverseOf rdf:resource="http://w3id.org/meta-share/meta-share/dependsOn"/>
        <rdfs:domain rdf:resource="http://w3id.org/meta-share/meta-share/LanguageResource"/>
        <rdfs:range rdf:resource="http://w3id.org/meta-share/meta-share/LanguageResource"/>
        <rdfs:comment xml:lang="en">Links to LR B that requires LR A (the one being described) for its operation or that has been processed with LR A</rdfs:comment>
        <rdfs:label xml:lang="en">dependent language resource</rdfs:label>
    </owl:ObjectProperty>
    


    <!-- http://w3id.org/meta-share/meta-share/dependsOn -->

    <owl:ObjectProperty rdf:about="http://w3id.org/meta-share/meta-share/dependsOn">
        <rdfs:subPropertyOf rdf:resource="http://w3id.org/meta-share/meta-share/isRelatedToLR"/>
        <rdf:type rdf:resource="http://www.w3.org/2002/07/owl#SymmetricProperty"/>
        <rdfs:domain rdf:resource="http://w3id.org/meta-share/meta-share/LanguageResource"/>
        <rdfs:range rdf:resource="http://w3id.org/meta-share/meta-share/LanguageResource"/>
        <rdfs:comment xml:lang="en">Links to LR B that is required for the operation of LR A (the one being described) or that has been used in its processing</rdfs:comment>
        <rdfs:label xml:lang="en">depends on</rdfs:label>
    </owl:ObjectProperty>
    


    <!-- http://w3id.org/meta-share/meta-share/describedEntity -->

    <owl:ObjectProperty rdf:about="http://w3id.org/meta-share/meta-share/describedEntity">
        <rdfs:domain rdf:resource="http://w3id.org/meta-share/meta-share/MetadataRecord"/>
        <rdfs:range rdf:resource="http://w3id.org/meta-share/meta-share/DescribedEntity"/>
        <rdfs:comment xml:lang="en">Links to the entity that is being described by a metadata record</rdfs:comment>
        <rdfs:label xml:lang="en">type of described entity</rdfs:label>
        <skos:note xml:lang="en">foaf:primaryTopic in DCAT</skos:note>
    </owl:ObjectProperty>
    


    <!-- http://w3id.org/meta-share/meta-share/describes -->

    <owl:ObjectProperty rdf:about="http://w3id.org/meta-share/meta-share/describes">
        <rdfs:subPropertyOf rdf:resource="http://w3id.org/meta-share/meta-share/documents"/>
        <owl:inverseOf rdf:resource="http://w3id.org/meta-share/meta-share/isDescribedBy"/>
        <rdfs:domain rdf:resource="http://w3id.org/meta-share/meta-share/Document"/>
        <rdfs:range rdf:resource="http://w3id.org/meta-share/meta-share/LanguageResource"/>
        <rdfs:comment xml:lang="en">Links to the language resource(s) that are described (contents, operation, etc.) in a document</rdfs:comment>
        <rdfs:label xml:lang="en">describes</rdfs:label>
    </owl:ObjectProperty>
    


    <!-- http://w3id.org/meta-share/meta-share/displays -->

    <owl:ObjectProperty rdf:about="http://w3id.org/meta-share/meta-share/displays">
        <rdfs:subPropertyOf rdf:resource="http://w3id.org/meta-share/meta-share/LΤRelatedTo"/>
        <owl:inverseOf rdf:resource="http://w3id.org/meta-share/meta-share/isDisplayedBy"/>
        <rdfs:domain rdf:resource="http://w3id.org/meta-share/meta-share/ToolService"/>
        <rdfs:range>
            <owl:Class>
                <owl:unionOf rdf:parseType="Collection">
                    <rdf:Description rdf:about="http://w3id.org/meta-share/meta-share/DataLanguageResource"/>
                    <rdf:Description rdf:about="http://w3id.org/meta-share/meta-share/MediaPart"/>
                </owl:unionOf>
            </owl:Class>
        </rdfs:range>
        <rdfs:altLabel xml:lang="en">visualises</rdfs:altLabel>
        <rdfs:altLabel xml:lang="en">visualizes</rdfs:altLabel>
        <rdfs:comment xml:lang="en">Links a tool/service B that is (or can be) used to display LR A (e.g.,  a tool for visualizing relations in a lexicon, or annotations in a corpus) to the LR A</rdfs:comment>
        <rdfs:label xml:lang="en">displays</rdfs:label>
    </owl:ObjectProperty>
    


    <!-- http://w3id.org/meta-share/meta-share/distribution -->

    <owl:ObjectProperty rdf:about="http://w3id.org/meta-share/meta-share/distribution">
        <rdfs:domain rdf:resource="http://w3id.org/meta-share/meta-share/LanguageResource"/>
        <rdfs:range rdf:resource="http://w3id.org/meta-share/meta-share/Distribution"/>
        <rdfs:comment xml:lang="en">Links a language resource to the various forms with which it is distributed</rdfs:comment>
        <rdfs:label xml:lang="en">distribution</rdfs:label>
        <skos:closeMatch rdf:resource="dcat:distribution"/>
    </owl:ObjectProperty>
    


    <!-- http://w3id.org/meta-share/meta-share/distributionAudioFeature -->

    <owl:ObjectProperty rdf:about="http://w3id.org/meta-share/meta-share/distributionAudioFeature">
        <rdfs:domain rdf:resource="http://w3id.org/meta-share/meta-share/DatasetDistribution"/>
        <rdfs:range rdf:resource="http://w3id.org/meta-share/meta-share/DistributionAudioFeature"/>
        <rdfs:comment xml:lang="en">Links to a feature that can be used for describing distinct distributable forms of audio resources/parts</rdfs:comment>
        <rdfs:label xml:lang="en">distribution audio feature</rdfs:label>
    </owl:ObjectProperty>
    


    <!-- http://w3id.org/meta-share/meta-share/distributionForm -->

    <owl:ObjectProperty rdf:about="http://w3id.org/meta-share/meta-share/distributionForm">
        <rdfs:domain rdf:resource="http://w3id.org/meta-share/meta-share/Distribution"/>
        <rdfs:range rdf:resource="http://w3id.org/meta-share/meta-share/DistributionForm"/>
        <rdfs:comment xml:lang="en">Specifies the form (medium/channel) with which a resource is distributed (delivered or provided access to)</rdfs:comment>
        <rdfs:label xml:lang="en">distribution form</rdfs:label>
    </owl:ObjectProperty>
    


    <!-- http://w3id.org/meta-share/meta-share/distributionImageFeature -->

    <owl:ObjectProperty rdf:about="http://w3id.org/meta-share/meta-share/distributionImageFeature">
        <rdfs:domain rdf:resource="http://w3id.org/meta-share/meta-share/DatasetDistribution"/>
        <rdfs:range rdf:resource="http://w3id.org/meta-share/meta-share/DistributionImageFeature"/>
        <rdfs:comment xml:lang="en">Links to a feature that can be used for describing distinct distributable forms of image resources/parts</rdfs:comment>
        <rdfs:label xml:lang="en">distribution image feature</rdfs:label>
    </owl:ObjectProperty>
    


    <!-- http://w3id.org/meta-share/meta-share/distributionRightsHolder -->

    <owl:ObjectProperty rdf:about="http://w3id.org/meta-share/meta-share/distributionRightsHolder">
        <rdfs:subPropertyOf rdf:resource="http://w3id.org/meta-share/meta-share/isRelatedToActor"/>
        <owl:inverseOf rdf:resource="http://w3id.org/meta-share/meta-share/isDistributionRightsHolderOf"/>
        <rdfs:domain rdf:resource="http://w3id.org/meta-share/meta-share/Distribution"/>
        <rdfs:range rdf:resource="http://w3id.org/meta-share/meta-share/Actor"/>
        <rdfs:comment xml:lang="en">Identifies a person or an organization that holds the distribution rights. The range and scope of distribution rights is defined in the distribution agreement. The distributor in most cases only has a limited licence to distribute the work and collect royalties on behalf of the licensor or the IPR holder and cannot give to any recipient of the work permissions that exceed the scope of the distribution agreement (e.g.,  to allow uses of the work that are not defined in the distribution agreement)</rdfs:comment>
        <rdfs:label xml:lang="en">distribution rights holder</rdfs:label>
    </owl:ObjectProperty>
    


    <!-- http://w3id.org/meta-share/meta-share/distributionTextFeature -->

    <owl:ObjectProperty rdf:about="http://w3id.org/meta-share/meta-share/distributionTextFeature">
        <rdfs:domain rdf:resource="http://w3id.org/meta-share/meta-share/DatasetDistribution"/>
        <rdfs:range rdf:resource="http://w3id.org/meta-share/meta-share/DistributionTextFeature"/>
        <rdfs:comment xml:lang="en">Links to a feature that can be used for describing distinct distributable forms of text resources/parts</rdfs:comment>
        <rdfs:label xml:lang="en">distribution text feature</rdfs:label>
    </owl:ObjectProperty>
    


    <!-- http://w3id.org/meta-share/meta-share/distributionTextNumericalFeature -->

    <owl:ObjectProperty rdf:about="http://w3id.org/meta-share/meta-share/distributionTextNumericalFeature">
        <rdfs:domain rdf:resource="http://w3id.org/meta-share/meta-share/DatasetDistribution"/>
        <rdfs:range rdf:resource="http://w3id.org/meta-share/meta-share/DistributionTextNumericalFeature"/>
        <rdfs:comment xml:lang="en">Links to a feature that can be used for describing distinct distributable forms of numerical text resources/parts</rdfs:comment>
        <rdfs:label xml:lang="en">distribution text numerical feature</rdfs:label>
    </owl:ObjectProperty>
    


    <!-- http://w3id.org/meta-share/meta-share/distributionVideoFeature -->

    <owl:ObjectProperty rdf:about="http://w3id.org/meta-share/meta-share/distributionVideoFeature">
        <rdfs:domain rdf:resource="http://w3id.org/meta-share/meta-share/DatasetDistribution"/>
        <rdfs:range rdf:resource="http://w3id.org/meta-share/meta-share/DistributionVideoFeature"/>
        <rdfs:comment xml:lang="en">Links to a feature that can be used for describing distinct distributable forms of video resources/parts</rdfs:comment>
        <rdfs:label xml:lang="en">distribution video feature</rdfs:label>
    </owl:ObjectProperty>
    


    <!-- http://w3id.org/meta-share/meta-share/divisionCategory -->

    <owl:ObjectProperty rdf:about="http://w3id.org/meta-share/meta-share/divisionCategory">
        <rdfs:domain rdf:resource="http://w3id.org/meta-share/meta-share/Division"/>
        <rdfs:range rdf:resource="http://w3id.org/meta-share/meta-share/DivisionCategory"/>
        <rdfs:comment xml:lang="en">Classifies the division of an organization according to a controlled vocabulary</rdfs:comment>
        <rdfs:label xml:lang="en">division category</rdfs:label>
    </owl:ObjectProperty>
    


    <!-- http://w3id.org/meta-share/meta-share/documentRelatedTo -->

    <owl:ObjectProperty rdf:about="http://w3id.org/meta-share/meta-share/documentRelatedTo">
        <rdfs:subPropertyOf rdf:resource="http://w3id.org/meta-share/meta-share/isRelatedTo"/>
        <owl:inverseOf rdf:resource="http://w3id.org/meta-share/meta-share/isRelatedToDocument"/>
        <rdfs:domain rdf:resource="http://w3id.org/meta-share/meta-share/Document"/>
        <rdfs:range>
            <owl:Class>
                <owl:unionOf rdf:parseType="Collection">
                    <rdf:Description rdf:about="http://w3id.org/meta-share/meta-share/LanguageResource"/>
                    <rdf:Description rdf:about="http://w3id.org/meta-share/meta-share/Project"/>
                </owl:unionOf>
            </owl:Class>
        </rdfs:range>
        <rdfs:comment xml:lang="en">Links to the entity (language resource, project, part of a language resource) that is somehow related to the document that is described</rdfs:comment>
        <rdfs:label xml:lang="en">document related to</rdfs:label>
    </owl:ObjectProperty>
    


    <!-- http://w3id.org/meta-share/meta-share/documentType -->

    <owl:ObjectProperty rdf:about="http://w3id.org/meta-share/meta-share/documentType">
        <rdfs:domain rdf:resource="http://w3id.org/meta-share/meta-share/Document"/>
        <rdfs:range rdf:resource="http://w3id.org/meta-share/meta-share/DocumentType"/>
        <rdfs:comment xml:lang="en">Specifies the type of the document (e.g.,  article, book, etc.) provided with or related to the language resource</rdfs:comment>
        <rdfs:label xml:lang="en">document type</rdfs:label>
    </owl:ObjectProperty>
    


    <!-- http://w3id.org/meta-share/meta-share/documentationType -->

    <owl:ObjectProperty rdf:about="http://w3id.org/meta-share/meta-share/documentationType">
        <rdfs:domain rdf:resource="http://w3id.org/meta-share/meta-share/Document"/>
        <rdfs:range rdf:resource="http://w3id.org/meta-share/meta-share/DocumentationType"/>
        <rdfs:comment xml:lang="en">Classifies the documentation vis-a-vis its relation with the language resource (e.g.,  general publication, user manual, url for online help, etc.)</rdfs:comment>
        <rdfs:label xml:lang="en">documentation type</rdfs:label>
    </owl:ObjectProperty>
    


    <!-- http://w3id.org/meta-share/meta-share/documents -->

    <owl:ObjectProperty rdf:about="http://w3id.org/meta-share/meta-share/documents">
        <rdfs:subPropertyOf rdf:resource="http://w3id.org/meta-share/meta-share/documentRelatedTo"/>
        <owl:inverseOf rdf:resource="http://w3id.org/meta-share/meta-share/isDocumentedBy"/>
        <rdfs:domain rdf:resource="http://w3id.org/meta-share/meta-share/Document"/>
        <rdfs:range rdf:resource="http://w3id.org/meta-share/meta-share/LanguageResource"/>
        <rdfs:comment xml:lang="en">Links a document to a language resource (e.g.,  research paper describing its contents or its use in a project, user manual, etc.)</rdfs:comment>
        <rdfs:label xml:lang="en">documents</rdfs:label>
    </owl:ObjectProperty>
    


    <!-- http://w3id.org/meta-share/meta-share/documentsAnnotation -->

    <owl:ObjectProperty rdf:about="http://w3id.org/meta-share/meta-share/documentsAnnotation">
        <rdfs:subPropertyOf rdf:resource="http://w3id.org/meta-share/meta-share/documents"/>
        <rdfs:domain rdf:resource="http://w3id.org/meta-share/meta-share/Document"/>
        <rdfs:range rdf:resource="http://w3id.org/meta-share/meta-share/Annotation"/>
        <rdfs:comment xml:lang="en">Links a report to the annotation process, tool, method , etc. of a language resource that it describes</rdfs:comment>
        <rdfs:label xml:lang="en">documents annotation</rdfs:label>
    </owl:ObjectProperty>
    


    <!-- http://w3id.org/meta-share/meta-share/documentsEvaluation -->

    <owl:ObjectProperty rdf:about="http://w3id.org/meta-share/meta-share/documentsEvaluation">
        <rdfs:subPropertyOf rdf:resource="http://w3id.org/meta-share/meta-share/documents"/>
        <owl:inverseOf rdf:resource="http://w3id.org/meta-share/meta-share/evaluationReport"/>
        <rdfs:domain rdf:resource="http://w3id.org/meta-share/meta-share/Document"/>
        <rdfs:range rdf:resource="http://w3id.org/meta-share/meta-share/Evaluation"/>
        <rdfs:comment xml:lang="en">Links a report to the evaluation process, tool, method , etc. of the tool or service it purports to describe</rdfs:comment>
        <rdfs:label xml:lang="en">documents evaluation</rdfs:label>
    </owl:ObjectProperty>
    


    <!-- http://w3id.org/meta-share/meta-share/documentsGuidelines -->

    <owl:ObjectProperty rdf:about="http://w3id.org/meta-share/meta-share/documentsGuidelines">
        <rdfs:subPropertyOf rdf:resource="http://w3id.org/meta-share/meta-share/documents"/>
        <owl:inverseOf rdf:resource="http://w3id.org/meta-share/meta-share/guidelines"/>
        <rdfs:domain rdf:resource="http://w3id.org/meta-share/meta-share/Document"/>
        <rdfs:range>
            <owl:Class>
                <owl:unionOf rdf:parseType="Collection">
                    <rdf:Description rdf:about="http://w3id.org/meta-share/meta-share/Annotation"/>
                    <rdf:Description rdf:about="http://w3id.org/meta-share/meta-share/LanguageResource"/>
                </owl:unionOf>
            </owl:Class>
        </rdfs:range>
        <rdfs:comment xml:lang="en">Links the guidelines used for the creation or annotation of a language resource to this language resource</rdfs:comment>
        <rdfs:label xml:lang="en">documents guidelines</rdfs:label>
    </owl:ObjectProperty>
    


    <!-- http://w3id.org/meta-share/meta-share/documentsUsage -->

    <owl:ObjectProperty rdf:about="http://w3id.org/meta-share/meta-share/documentsUsage">
        <rdfs:subPropertyOf rdf:resource="http://w3id.org/meta-share/meta-share/documents"/>
        <owl:inverseOf rdf:resource="http://w3id.org/meta-share/meta-share/usageReport"/>
        <rdfs:domain rdf:resource="http://w3id.org/meta-share/meta-share/Document"/>
        <rdfs:range rdf:resource="http://w3id.org/meta-share/meta-share/ActualUse"/>
        <rdfs:comment xml:lang="en">Links a document (e.g.,  research article, report) describing the use of a language resource (e.g.,  in a project, application, experiment or use case) to the data of this use</rdfs:comment>
        <rdfs:label xml:lang="en">documents usage</rdfs:label>
    </owl:ObjectProperty>
    


    <!-- http://w3id.org/meta-share/meta-share/documentsValidation -->

    <owl:ObjectProperty rdf:about="http://w3id.org/meta-share/meta-share/documentsValidation">
        <rdfs:subPropertyOf rdf:resource="http://w3id.org/meta-share/meta-share/documents"/>
        <owl:inverseOf rdf:resource="http://w3id.org/meta-share/meta-share/validationReport"/>
        <rdfs:domain rdf:resource="http://w3id.org/meta-share/meta-share/Document"/>
        <rdfs:range rdf:resource="http://w3id.org/meta-share/meta-share/Validation"/>
        <rdfs:comment xml:lang="en">Links a document with detailed information on the validation process and results to the data of this validation</rdfs:comment>
        <rdfs:label xml:lang="en">documents validation</rdfs:label>
    </owl:ObjectProperty>
    


    <!-- http://w3id.org/meta-share/meta-share/domain -->

    <owl:ObjectProperty rdf:about="http://w3id.org/meta-share/meta-share/domain">
        <rdfs:domain>
            <owl:Class>
                <owl:unionOf rdf:parseType="Collection">
                    <rdf:Description rdf:about="http://w3id.org/meta-share/meta-share/Actor"/>
                    <rdf:Description rdf:about="http://w3id.org/meta-share/meta-share/Division"/>
                    <rdf:Description rdf:about="http://w3id.org/meta-share/meta-share/Document"/>
                    <rdf:Description rdf:about="http://w3id.org/meta-share/meta-share/LanguageResource"/>
                    <rdf:Description rdf:about="http://w3id.org/meta-share/meta-share/ProcessingResource"/>
                    <rdf:Description rdf:about="http://w3id.org/meta-share/meta-share/Project"/>
                </owl:unionOf>
            </owl:Class>
        </rdfs:domain>
        <rdfs:range rdf:resource="http://w3id.org/meta-share/meta-share/Domain"/>
        <rdfs:comment xml:lang="en">Identifies the domain according to which a resource is classified</rdfs:comment>
        <rdfs:label xml:lang="en">domain</rdfs:label>
    </owl:ObjectProperty>
    


    <!-- http://w3id.org/meta-share/meta-share/durationOfAudio -->

    <owl:ObjectProperty rdf:about="http://w3id.org/meta-share/meta-share/durationOfAudio">
        <rdfs:domain rdf:resource="http://w3id.org/meta-share/meta-share/DatasetDistribution"/>
        <rdfs:range rdf:resource="http://w3id.org/meta-share/meta-share/Duration"/>
        <rdfs:comment xml:lang="en">Specifies the duration of the audio recording including silences, music, pauses, etc.</rdfs:comment>
        <rdfs:label xml:lang="en">duration of audio</rdfs:label>
    </owl:ObjectProperty>
    


    <!-- http://w3id.org/meta-share/meta-share/durationOfEffectiveSpeech -->

    <owl:ObjectProperty rdf:about="http://w3id.org/meta-share/meta-share/durationOfEffectiveSpeech">
        <rdfs:domain rdf:resource="http://w3id.org/meta-share/meta-share/DatasetDistribution"/>
        <rdfs:range rdf:resource="http://w3id.org/meta-share/meta-share/Duration"/>
        <rdfs:comment xml:lang="en">Specifies the duration of effective speech of the audio (part of a) resource</rdfs:comment>
        <rdfs:label xml:lang="en">duration of effective speech</rdfs:label>
    </owl:ObjectProperty>
    


    <!-- http://w3id.org/meta-share/meta-share/durationUnit -->

    <owl:ObjectProperty rdf:about="http://w3id.org/meta-share/meta-share/durationUnit">
        <rdfs:domain rdf:resource="http://w3id.org/meta-share/meta-share/Duration"/>
        <rdfs:range rdf:resource="http://w3id.org/meta-share/meta-share/DurationUnit"/>
        <rdfs:comment xml:lang="en">Specifies the unit used for measuring the duration of a resource</rdfs:comment>
        <rdfs:label xml:lang="en">duration unit</rdfs:label>
    </owl:ObjectProperty>
    


    <!-- http://w3id.org/meta-share/meta-share/dynamicElement -->

    <owl:ObjectProperty rdf:about="http://w3id.org/meta-share/meta-share/dynamicElement">
        <rdfs:domain>
            <owl:Class>
                <owl:unionOf rdf:parseType="Collection">
                    <rdf:Description rdf:about="http://w3id.org/meta-share/meta-share/CorpusVideoPart"/>
                    <rdf:Description rdf:about="http://w3id.org/meta-share/meta-share/LanguageDescriptionVideoPart"/>
                    <rdf:Description rdf:about="http://w3id.org/meta-share/meta-share/LexicalConceptualResourceVideoPart"/>
                </owl:unionOf>
            </owl:Class>
        </rdfs:domain>
        <rdfs:range rdf:resource="http://w3id.org/meta-share/meta-share/DynamicElement"/>
        <rdfs:comment xml:lang="en">Groups information on the dynamic elements that are represented in the video part of the resource</rdfs:comment>
        <rdfs:label xml:lang="en">dynamic element</rdfs:label>
        <skos:note xml:lang="en">it was like this in MS-OWL v1, although it&apos;s not multiple; helps to organise the elements though</skos:note>
    </owl:ObjectProperty>
    


    <!-- http://w3id.org/meta-share/meta-share/ecMaxContribution -->

    <owl:ObjectProperty rdf:about="http://w3id.org/meta-share/meta-share/ecMaxContribution">
        <rdfs:domain rdf:resource="http://w3id.org/meta-share/meta-share/Project"/>
        <rdfs:range rdf:resource="http://w3id.org/meta-share/meta-share/Cost"/>
        <rdfs:comment xml:lang="en">Introduces the maximum amount of money contributed from EC funds</rdfs:comment>
        <rdfs:label xml:lang="en">EC max contribution</rdfs:label>
    </owl:ObjectProperty>
    


    <!-- http://w3id.org/meta-share/meta-share/editor -->

    <owl:ObjectProperty rdf:about="http://w3id.org/meta-share/meta-share/editor">
        <rdfs:domain rdf:resource="http://w3id.org/meta-share/meta-share/Document"/>
        <rdfs:range rdf:resource="http://w3id.org/meta-share/meta-share/Person"/>
        <rdfs:comment xml:lang="en">Introduces the details for a person that has edited the document being described</rdfs:comment>
        <rdfs:label xml:lang="en">editor</rdfs:label>
    </owl:ObjectProperty>
    


    <!-- http://w3id.org/meta-share/meta-share/edits -->

    <owl:ObjectProperty rdf:about="http://w3id.org/meta-share/meta-share/edits">
        <rdfs:subPropertyOf rdf:resource="http://w3id.org/meta-share/meta-share/LΤRelatedTo"/>
        <owl:inverseOf rdf:resource="http://w3id.org/meta-share/meta-share/isEditedBy"/>
        <rdfs:domain rdf:resource="http://w3id.org/meta-share/meta-share/ToolService"/>
        <rdfs:range>
            <owl:Class>
                <owl:unionOf rdf:parseType="Collection">
                    <rdf:Description rdf:about="http://w3id.org/meta-share/meta-share/DataLanguageResource"/>
                    <rdf:Description rdf:about="http://w3id.org/meta-share/meta-share/MediaPart"/>
                </owl:unionOf>
            </owl:Class>
        </rdfs:range>
        <rdfs:comment xml:lang="en">Links a tool/service B that is (or can be) used for editing LR A (the one being described) to LR A</rdfs:comment>
        <rdfs:label xml:lang="en">edits</rdfs:label>
    </owl:ObjectProperty>
    


    <!-- http://w3id.org/meta-share/meta-share/encodingLevel -->

    <owl:ObjectProperty rdf:about="http://w3id.org/meta-share/meta-share/encodingLevel">
        <rdfs:domain>
            <owl:Class>
                <owl:unionOf rdf:parseType="Collection">
                    <rdf:Description rdf:about="http://w3id.org/meta-share/meta-share/LanguageDescription"/>
                    <rdf:Description rdf:about="http://w3id.org/meta-share/meta-share/LexicalConceptualResource"/>
                </owl:unionOf>
            </owl:Class>
        </rdfs:domain>
        <rdfs:range rdf:resource="http://w3id.org/meta-share/meta-share/EncodingLevel"/>
        <rdfs:comment xml:lang="en">Classifies the contents of a lexical/conceptual resource or language description as regards the linguistic level of analysis it caters for</rdfs:comment>
        <rdfs:label>encoding level</rdfs:label>
    </owl:ObjectProperty>
    


    <!-- http://w3id.org/meta-share/meta-share/evaluation -->

    <owl:ObjectProperty rdf:about="http://w3id.org/meta-share/meta-share/evaluation">
        <rdfs:domain rdf:resource="http://w3id.org/meta-share/meta-share/ToolService"/>
        <rdfs:range rdf:resource="http://w3id.org/meta-share/meta-share/Evaluation"/>
        <rdfs:comment xml:lang="en">Provides information on the evaluation process and results for a tool/service</rdfs:comment>
        <rdfs:label xml:lang="en">evaluation</rdfs:label>
    </owl:ObjectProperty>
    


    <!-- http://w3id.org/meta-share/meta-share/evaluationCriterion -->

    <owl:ObjectProperty rdf:about="http://w3id.org/meta-share/meta-share/evaluationCriterion">
        <rdfs:domain rdf:resource="http://w3id.org/meta-share/meta-share/Evaluation"/>
        <rdfs:range rdf:resource="http://w3id.org/meta-share/meta-share/EvaluationCriterion"/>
        <rdfs:comment xml:lang="en">Defines the criterion(s) of the evaluation of a tool</rdfs:comment>
        <rdfs:label xml:lang="en">evaluation criterion</rdfs:label>
    </owl:ObjectProperty>
    


    <!-- http://w3id.org/meta-share/meta-share/evaluationLevel -->

    <owl:ObjectProperty rdf:about="http://w3id.org/meta-share/meta-share/evaluationLevel">
        <rdfs:domain rdf:resource="http://w3id.org/meta-share/meta-share/Evaluation"/>
        <rdfs:range rdf:resource="http://w3id.org/meta-share/meta-share/EvaluationLevel"/>
        <rdfs:comment xml:lang="en">Indicates the evaluation level</rdfs:comment>
        <rdfs:label xml:lang="en">evaluation level</rdfs:label>
    </owl:ObjectProperty>
    


    <!-- http://w3id.org/meta-share/meta-share/evaluationMeasure -->

    <owl:ObjectProperty rdf:about="http://w3id.org/meta-share/meta-share/evaluationMeasure">
        <rdfs:domain rdf:resource="http://w3id.org/meta-share/meta-share/Evaluation"/>
        <rdfs:range rdf:resource="http://w3id.org/meta-share/meta-share/EvaluationMeasure"/>
        <rdfs:comment xml:lang="en">Defines whether the evaluation measure is human or automatic</rdfs:comment>
        <rdfs:label xml:lang="en">evaluation measure</rdfs:label>
    </owl:ObjectProperty>
    


    <!-- http://w3id.org/meta-share/meta-share/evaluationReport -->

    <owl:ObjectProperty rdf:about="http://w3id.org/meta-share/meta-share/evaluationReport">
        <rdfs:subPropertyOf rdf:resource="http://w3id.org/meta-share/meta-share/isDocumentedBy"/>
        <rdfs:domain rdf:resource="http://w3id.org/meta-share/meta-share/Evaluation"/>
        <rdfs:range rdf:resource="http://w3id.org/meta-share/meta-share/Document"/>
        <rdfs:comment xml:lang="en">Links to a report describing the evaluation process, tool, method , etc. of the tool or service</rdfs:comment>
        <rdfs:label xml:lang="en">evaluation report</rdfs:label>
    </owl:ObjectProperty>
    


    <!-- http://w3id.org/meta-share/meta-share/evaluationType -->

    <owl:ObjectProperty rdf:about="http://w3id.org/meta-share/meta-share/evaluationType">
        <rdfs:domain rdf:resource="http://w3id.org/meta-share/meta-share/Evaluation"/>
        <rdfs:range rdf:resource="http://w3id.org/meta-share/meta-share/EvaluationType"/>
        <rdfs:comment xml:lang="en">Indicates the evaluation type</rdfs:comment>
        <rdfs:label xml:lang="en">evaluation type</rdfs:label>
    </owl:ObjectProperty>
    


    <!-- http://w3id.org/meta-share/meta-share/evaluator -->

    <owl:ObjectProperty rdf:about="http://w3id.org/meta-share/meta-share/evaluator">
        <rdfs:subPropertyOf rdf:resource="http://w3id.org/meta-share/meta-share/isRelatedToActor"/>
        <owl:inverseOf rdf:resource="http://w3id.org/meta-share/meta-share/isEvaluatorOf"/>
        <rdfs:domain rdf:resource="http://w3id.org/meta-share/meta-share/Evaluation"/>
        <rdfs:range rdf:resource="http://w3id.org/meta-share/meta-share/Actor"/>
        <rdfs:comment xml:lang="en">Describes the person or organization that evaluated the tool or service</rdfs:comment>
        <rdfs:label xml:lang="en">evaluator</rdfs:label>
    </owl:ObjectProperty>
    


    <!-- http://w3id.org/meta-share/meta-share/externalReference -->

    <owl:ObjectProperty rdf:about="http://w3id.org/meta-share/meta-share/externalReference">
        <rdfs:domain rdf:resource="http://w3id.org/meta-share/meta-share/LexicalConceptualResource"/>
        <rdfs:range rdf:resource="http://w3id.org/meta-share/meta-share/LexicalConceptualResource"/>
        <rdfs:comment xml:lang="en">Provides reference to another resource to which the lexicalConceptualResource is linked (e.g.,  link to a wordnet or ontology)</rdfs:comment>
        <rdfs:label xml:lang="en">external reference</rdfs:label>
    </owl:ObjectProperty>
    


    <!-- http://w3id.org/meta-share/meta-share/extratextualInformation -->

    <owl:ObjectProperty rdf:about="http://w3id.org/meta-share/meta-share/extratextualInformation">
        <rdfs:domain rdf:resource="http://w3id.org/meta-share/meta-share/LexicalConceptualResource"/>
        <rdfs:range rdf:resource="http://w3id.org/meta-share/meta-share/ExtratextualInformation"/>
        <rdfs:comment xml:lang="en">Indicates the extratextual information contained in a lexical/conceptual resource; it can be used as an alternative to the representation of the audio, image, video , etc. part(s) of the resource when these are not considered important enough to fully describe</rdfs:comment>
        <rdfs:label xml:lang="en">extratextual information</rdfs:label>
    </owl:ObjectProperty>
    


    <!-- http://w3id.org/meta-share/meta-share/extratextualInformationUnit -->

    <owl:ObjectProperty rdf:about="http://w3id.org/meta-share/meta-share/extratextualInformationUnit">
        <rdfs:domain rdf:resource="http://w3id.org/meta-share/meta-share/LexicalConceptualResource"/>
        <rdfs:range rdf:resource="http://w3id.org/meta-share/meta-share/ExtratextualInformationUnit"/>
        <rdfs:comment xml:lang="en">Indicates the unit on which the extratextual information is attached to in the lexical conceptual resource</rdfs:comment>
        <rdfs:label xml:lang="en">extratextual information unit</rdfs:label>
    </owl:ObjectProperty>
    


    <!-- http://w3id.org/meta-share/meta-share/framework -->

    <owl:ObjectProperty rdf:about="http://w3id.org/meta-share/meta-share/framework">
        <rdfs:domain rdf:resource="http://w3id.org/meta-share/meta-share/ToolService"/>
        <rdfs:range rdf:resource="http://w3id.org/meta-share/meta-share/Framework"/>
        <rdfs:comment xml:lang="en">Specifies the implementation framework used for developing and running a tool/service</rdfs:comment>
        <rdfs:label xml:lang="en">framework</rdfs:label>
    </owl:ObjectProperty>
    


    <!-- http://w3id.org/meta-share/meta-share/function -->

    <owl:ObjectProperty rdf:about="http://w3id.org/meta-share/meta-share/function">
        <rdfs:domain rdf:resource="http://w3id.org/meta-share/meta-share/ToolService"/>
        <rdfs:range rdf:resource="http://w3id.org/meta-share/omtd-share/Operation"/>
        <rdfs:altLabel>operation</rdfs:altLabel>
        <rdfs:altLabel>task</rdfs:altLabel>
        <rdfs:comment xml:lang="en">Specifies the operation/function/task that a software object performs</rdfs:comment>
        <rdfs:label xml:lang="en">function</rdfs:label>
    </owl:ObjectProperty>
    


    <!-- http://w3id.org/meta-share/meta-share/funder -->

    <owl:ObjectProperty rdf:about="http://w3id.org/meta-share/meta-share/funder">
        <rdfs:subPropertyOf rdf:resource="http://w3id.org/meta-share/meta-share/isRelatedToActor"/>
        <owl:inverseOf rdf:resource="http://w3id.org/meta-share/meta-share/isFunderOf"/>
        <rdfs:domain rdf:resource="http://w3id.org/meta-share/meta-share/Project"/>
        <rdfs:range rdf:resource="http://w3id.org/meta-share/meta-share/Actor"/>
        <rdfs:comment xml:lang="en">Identifies the person/organization/group that has financed the project</rdfs:comment>
        <rdfs:label xml:lang="en">funder</rdfs:label>
    </owl:ObjectProperty>
    


    <!-- http://w3id.org/meta-share/meta-share/fundingCountry -->

    <owl:ObjectProperty rdf:about="http://w3id.org/meta-share/meta-share/fundingCountry">
        <rdfs:domain rdf:resource="http://w3id.org/meta-share/meta-share/Project"/>
        <rdfs:range rdf:resource="http://w3id.org/meta-share/meta-share/Country"/>
        <rdfs:comment xml:lang="en">Specifies the name of the funding country, in case of national funding as mentioned in ISO3166</rdfs:comment>
        <rdfs:label xml:lang="en">funding country</rdfs:label>
    </owl:ObjectProperty>
    


    <!-- http://w3id.org/meta-share/meta-share/fundingProject -->

    <owl:ObjectProperty rdf:about="http://w3id.org/meta-share/meta-share/fundingProject">
        <rdfs:subPropertyOf rdf:resource="http://w3id.org/meta-share/meta-share/isRelatedToProject"/>
        <owl:inverseOf rdf:resource="http://w3id.org/meta-share/meta-share/isFundingProjectOf"/>
        <rdfs:domain rdf:resource="http://w3id.org/meta-share/meta-share/LanguageResource"/>
        <rdfs:range rdf:resource="http://w3id.org/meta-share/meta-share/Project"/>
        <rdfs:comment xml:lang="en">Links a language resource to the project that has funded its creation, enrichment, extension , etc.</rdfs:comment>
        <rdfs:label xml:lang="en">funding project</rdfs:label>
    </owl:ObjectProperty>
    


    <!-- http://w3id.org/meta-share/meta-share/fundingType -->

    <owl:ObjectProperty rdf:about="http://w3id.org/meta-share/meta-share/fundingType">
        <rdfs:domain rdf:resource="http://w3id.org/meta-share/meta-share/Project"/>
        <rdfs:range rdf:resource="http://w3id.org/meta-share/meta-share/FundingType"/>
        <rdfs:comment xml:lang="en">Specifies the type of funding of a project with regard to the source of the funding</rdfs:comment>
        <rdfs:label xml:lang="en">funding type</rdfs:label>
    </owl:ObjectProperty>
    


    <!-- http://w3id.org/meta-share/meta-share/genre -->

    <owl:ObjectProperty rdf:about="http://w3id.org/meta-share/meta-share/genre">
        <rdfs:domain rdf:resource="http://w3id.org/meta-share/meta-share/CorpusMediaPart"/>
        <rdfs:range rdf:resource="http://w3id.org/meta-share/meta-share/Genre"/>
        <rdfs:comment xml:lang="en">Links a language resource (part) to the genre it belongs to</rdfs:comment>
        <rdfs:label xml:lang="en">genre</rdfs:label>
    </owl:ObjectProperty>
    


    <!-- http://w3id.org/meta-share/meta-share/grammaticalPhenomenaCoverage -->

    <owl:ObjectProperty rdf:about="http://w3id.org/meta-share/meta-share/grammaticalPhenomenaCoverage">
        <rdfs:domain rdf:resource="http://w3id.org/meta-share/meta-share/LanguageDescription"/>
        <rdfs:range rdf:resource="http://w3id.org/meta-share/meta-share/GrammaticalPhenomenaCoverage"/>
        <rdfs:comment xml:lang="en">Gives an indication of the grammatical phenomena covered by the grammar</rdfs:comment>
        <rdfs:label xml:lang="en">grammatical phenomena coverage</rdfs:label>
    </owl:ObjectProperty>
    


    <!-- http://w3id.org/meta-share/meta-share/guidelines -->

    <owl:ObjectProperty rdf:about="http://w3id.org/meta-share/meta-share/guidelines">
        <rdfs:subPropertyOf rdf:resource="http://w3id.org/meta-share/meta-share/isDocumentedBy"/>
        <rdfs:domain>
            <owl:Class>
                <owl:unionOf rdf:parseType="Collection">
                    <rdf:Description rdf:about="http://w3id.org/meta-share/meta-share/Annotation"/>
                    <rdf:Description rdf:about="http://w3id.org/meta-share/meta-share/LanguageResource"/>
                </owl:unionOf>
            </owl:Class>
        </rdfs:domain>
        <rdfs:range rdf:resource="http://w3id.org/meta-share/meta-share/Document"/>
    </owl:ObjectProperty>
    


    <!-- http://w3id.org/meta-share/meta-share/hasAlignedVersion -->

    <owl:ObjectProperty rdf:about="http://w3id.org/meta-share/meta-share/hasAlignedVersion">
        <rdfs:subPropertyOf rdf:resource="http://w3id.org/meta-share/meta-share/hasVersion"/>
        <owl:inverseOf rdf:resource="http://w3id.org/meta-share/meta-share/isAlignedVersionOf"/>
        <rdfs:domain rdf:resource="http://w3id.org/meta-share/meta-share/Corpus"/>
        <rdfs:range rdf:resource="http://w3id.org/meta-share/meta-share/Corpus"/>
        <rdfs:comment xml:lang="en">Links to a corpus B which contains an aligned version of corpus A (the one being described)</rdfs:comment>
        <rdfs:label xml:lang="en">has aligned version</rdfs:label>
    </owl:ObjectProperty>
    


    <!-- http://w3id.org/meta-share/meta-share/hasAnalysed -->

    <owl:ObjectProperty rdf:about="http://w3id.org/meta-share/meta-share/hasAnalysed">
        <rdfs:subPropertyOf rdf:resource="http://w3id.org/meta-share/meta-share/LΤRelatedTo"/>
        <owl:inverseOf rdf:resource="http://w3id.org/meta-share/meta-share/isAnalysedBy"/>
        <rdfs:domain rdf:resource="http://w3id.org/meta-share/meta-share/ToolService"/>
        <rdfs:range>
            <owl:Class>
                <owl:unionOf rdf:parseType="Collection">
                    <rdf:Description rdf:about="http://w3id.org/meta-share/meta-share/DataLanguageResource"/>
                    <rdf:Description rdf:about="http://w3id.org/meta-share/meta-share/MediaPart"/>
                </owl:unionOf>
            </owl:Class>
        </rdfs:range>
        <rdfs:comment xml:lang="en">Links a tool/service B that is (or can be or has been) used for analysing LR A (e.g.,  a statistical tool) to LR A</rdfs:comment>
        <rdfs:label xml:lang="en">has analysed</rdfs:label>
    </owl:ObjectProperty>
    


    <!-- http://w3id.org/meta-share/meta-share/hasAnnotated -->

    <owl:ObjectProperty rdf:about="http://w3id.org/meta-share/meta-share/hasAnnotated">
        <rdfs:subPropertyOf rdf:resource="http://w3id.org/meta-share/meta-share/LΤRelatedTo"/>
        <owl:inverseOf rdf:resource="http://w3id.org/meta-share/meta-share/isAnnotatedBy"/>
        <rdfs:domain rdf:resource="http://w3id.org/meta-share/meta-share/ToolService"/>
        <rdfs:range rdf:resource="http://w3id.org/meta-share/meta-share/Annotation"/>
        <rdfs:comment xml:lang="en">Links a tool/service B that has been used for annotating LR A (e.g.,  a tagger, NER , etc.) to LR A</rdfs:comment>
        <rdfs:label xml:lang="en">has annotated</rdfs:label>
    </owl:ObjectProperty>
    


    <!-- http://w3id.org/meta-share/meta-share/hasAnnotatedVersion -->

    <owl:ObjectProperty rdf:about="http://w3id.org/meta-share/meta-share/hasAnnotatedVersion">
        <rdfs:subPropertyOf rdf:resource="http://w3id.org/meta-share/meta-share/hasVersion"/>
        <owl:inverseOf rdf:resource="http://w3id.org/meta-share/meta-share/isAnnotatedVersionOf"/>
        <rdfs:domain rdf:resource="http://w3id.org/meta-share/meta-share/Corpus"/>
        <rdfs:range rdf:resource="http://w3id.org/meta-share/meta-share/Corpus"/>
        <rdfs:comment xml:lang="en">Links to a corpus B which contains the annotations of corpus A (the one being described)</rdfs:comment>
        <rdfs:label xml:lang="en">has annotated version</rdfs:label>
    </owl:ObjectProperty>
    


    <!-- http://w3id.org/meta-share/meta-share/hasArchived -->

    <owl:ObjectProperty rdf:about="http://w3id.org/meta-share/meta-share/hasArchived">
        <rdfs:subPropertyOf rdf:resource="http://w3id.org/meta-share/meta-share/LΤRelatedTo"/>
        <owl:inverseOf rdf:resource="http://w3id.org/meta-share/meta-share/isArchivedBy"/>
        <rdfs:domain rdf:resource="http://w3id.org/meta-share/meta-share/ToolService"/>
        <rdfs:range rdf:resource="http://w3id.org/meta-share/meta-share/DataLanguageResource"/>
        <rdfs:comment xml:lang="en">Links a tool/service B that is (or can be or has been) used for archiving LR A to LR A</rdfs:comment>
        <rdfs:label xml:lang="en">has archived</rdfs:label>
    </owl:ObjectProperty>
    


    <!-- http://w3id.org/meta-share/meta-share/hasConvertedVersion -->

    <owl:ObjectProperty rdf:about="http://w3id.org/meta-share/meta-share/hasConvertedVersion">
        <rdfs:subPropertyOf rdf:resource="http://w3id.org/meta-share/meta-share/hasVersion"/>
        <owl:inverseOf rdf:resource="http://w3id.org/meta-share/meta-share/isConvertedVersionOf"/>
        <rdfs:domain rdf:resource="http://w3id.org/meta-share/meta-share/DataLanguageResource"/>
        <rdfs:range rdf:resource="http://w3id.org/meta-share/meta-share/DataLanguageResource"/>
        <rdfs:comment xml:lang="en">Links to LR B that has been used for creating LR A (the one being described) through a conversion procedure, e.g.,  a PDF to text conversion</rdfs:comment>
        <rdfs:label xml:lang="en">has converted version</rdfs:label>
    </owl:ObjectProperty>
    


    <!-- http://w3id.org/meta-share/meta-share/hasCreated -->

    <owl:ObjectProperty rdf:about="http://w3id.org/meta-share/meta-share/hasCreated">
        <rdfs:subPropertyOf rdf:resource="http://w3id.org/meta-share/meta-share/LΤRelatedTo"/>
        <owl:inverseOf rdf:resource="http://w3id.org/meta-share/meta-share/isCreatedBy"/>
        <rdfs:domain rdf:resource="http://w3id.org/meta-share/meta-share/ToolService"/>
        <rdfs:range>
            <owl:Class>
                <owl:unionOf rdf:parseType="Collection">
                    <rdf:Description rdf:about="http://w3id.org/meta-share/meta-share/DataLanguageResource"/>
                    <rdf:Description rdf:about="http://w3id.org/meta-share/meta-share/MediaPart"/>
                </owl:unionOf>
            </owl:Class>
        </rdfs:range>
        <rdfs:comment xml:lang="en">Links a tool/service B that is (or can be or has been) used for creating LR A to LR A</rdfs:comment>
        <rdfs:label xml:lang="en">has created</rdfs:label>
    </owl:ObjectProperty>
    


    <!-- http://w3id.org/meta-share/meta-share/hasDivision -->

    <owl:ObjectProperty rdf:about="http://w3id.org/meta-share/meta-share/hasDivision">
        <owl:inverseOf rdf:resource="http://w3id.org/meta-share/meta-share/isDivisionOf"/>
        <rdfs:domain rdf:resource="http://w3id.org/meta-share/meta-share/Organization"/>
        <rdfs:range rdf:resource="http://w3id.org/meta-share/meta-share/Division"/>
        <rdfs:comment xml:lang="en">Links an organization to the division(s) it consists of</rdfs:comment>
        <rdfs:label xml:lang="en">has division</rdfs:label>
    </owl:ObjectProperty>
    


    <!-- http://w3id.org/meta-share/meta-share/hasElicited -->

    <owl:ObjectProperty rdf:about="http://w3id.org/meta-share/meta-share/hasElicited">
        <rdfs:subPropertyOf rdf:resource="http://w3id.org/meta-share/meta-share/LΤRelatedTo"/>
        <owl:inverseOf rdf:resource="http://w3id.org/meta-share/meta-share/isElicitedBy"/>
        <rdfs:domain rdf:resource="http://w3id.org/meta-share/meta-share/ToolService"/>
        <rdfs:range>
            <owl:Class>
                <owl:unionOf rdf:parseType="Collection">
                    <rdf:Description rdf:about="http://w3id.org/meta-share/meta-share/DataLanguageResource"/>
                    <rdf:Description rdf:about="http://w3id.org/meta-share/meta-share/MediaPart"/>
                </owl:unionOf>
            </owl:Class>
        </rdfs:range>
        <rdfs:comment xml:lang="en">Links a tool/service B that is (or can be or has been) used for eliciting LR A to LR A</rdfs:comment>
        <rdfs:label xml:lang="en">has elicited</rdfs:label>
    </owl:ObjectProperty>
    


    <!-- http://w3id.org/meta-share/meta-share/hasEvaluated -->

    <owl:ObjectProperty rdf:about="http://w3id.org/meta-share/meta-share/hasEvaluated">
        <rdfs:subPropertyOf rdf:resource="http://w3id.org/meta-share/meta-share/LΤRelatedTo"/>
        <owl:inverseOf rdf:resource="http://w3id.org/meta-share/meta-share/isEvaluatedBy"/>
        <rdfs:domain rdf:resource="http://w3id.org/meta-share/meta-share/ToolService"/>
        <rdfs:range rdf:resource="http://w3id.org/meta-share/meta-share/Evaluation"/>
        <rdfs:comment xml:lang="en">Links a tool/service that has been used for evaluating an LR A to the data of this evaluation</rdfs:comment>
        <rdfs:label xml:lang="en">has evaluated</rdfs:label>
    </owl:ObjectProperty>
    


    <!-- http://w3id.org/meta-share/meta-share/hasMetadata -->

    <owl:ObjectProperty rdf:about="http://w3id.org/meta-share/meta-share/hasMetadata">
        <rdfs:subPropertyOf rdf:resource="http://w3id.org/meta-share/meta-share/isRelatedToMDRecord"/>
        <owl:inverseOf rdf:resource="http://w3id.org/meta-share/meta-share/isMetadataOf"/>
        <rdfs:domain rdf:resource="http://w3id.org/meta-share/meta-share/LanguageResource"/>
        <rdfs:range rdf:resource="http://w3id.org/meta-share/meta-share/MetadataRecord"/>
        <rdfs:comment xml:lang="en">Links to an external metadata record that describes the same language resource in another catalogue, repository, etc.</rdfs:comment>
        <rdfs:label xml:lang="en">has metadata</rdfs:label>
    </owl:ObjectProperty>
    


    <!-- http://w3id.org/meta-share/meta-share/hasOriginalSource -->

    <owl:ObjectProperty rdf:about="http://w3id.org/meta-share/meta-share/hasOriginalSource">
        <rdfs:subPropertyOf rdf:resource="http://w3id.org/meta-share/meta-share/isRelatedToLR"/>
        <owl:inverseOf rdf:resource="http://w3id.org/meta-share/meta-share/hasOutcome"/>
        <rdfs:domain>
            <owl:Class>
                <owl:unionOf rdf:parseType="Collection">
                    <rdf:Description rdf:about="http://w3id.org/meta-share/meta-share/LanguageResource"/>
                    <rdf:Description rdf:about="http://w3id.org/meta-share/meta-share/MediaPart"/>
                </owl:unionOf>
            </owl:Class>
        </rdfs:domain>
        <rdfs:range rdf:resource="http://w3id.org/meta-share/meta-share/LanguageResource"/>
        <rdfs:comment xml:lang="en">Links a language resource to the original source that has been used for its creation, where it&apos;s derived or elicited from</rdfs:comment>
        <rdfs:label xml:lang="en">has original source</rdfs:label>
    </owl:ObjectProperty>
    


    <!-- http://w3id.org/meta-share/meta-share/hasOutcome -->

    <owl:ObjectProperty rdf:about="http://w3id.org/meta-share/meta-share/hasOutcome">
        <rdfs:subPropertyOf rdf:resource="http://w3id.org/meta-share/meta-share/isRelatedToLR"/>
        <rdfs:domain rdf:resource="http://w3id.org/meta-share/meta-share/ActualUse"/>
        <rdfs:range rdf:resource="http://w3id.org/meta-share/meta-share/LanguageResource"/>
        <rdfs:altLabel xml:lang="en">is source of</rdfs:altLabel>
        <rdfs:comment xml:lang="en">Links to LR B which is created / extracted from LR A (the one being described), i.e. LR A has been used as the basis/initial/source material for LR B</rdfs:comment>
        <rdfs:label xml:lang="en">has outcome</rdfs:label>
    </owl:ObjectProperty>
    


    <!-- http://w3id.org/meta-share/meta-share/hasPart -->

    <owl:ObjectProperty rdf:about="http://w3id.org/meta-share/meta-share/hasPart">
        <rdfs:subPropertyOf rdf:resource="http://w3id.org/meta-share/meta-share/isRelatedToLR"/>
        <owl:inverseOf rdf:resource="http://w3id.org/meta-share/meta-share/isPartOf"/>
        <rdfs:domain rdf:resource="http://w3id.org/meta-share/meta-share/LanguageResource"/>
        <rdfs:range rdf:resource="http://w3id.org/meta-share/meta-share/LanguageResource"/>
        <rdfs:comment xml:lang="en">Links to LR B which is contained in LR A (the one being described), e.g.,  a monolingual corpus part of a bilingual corpus</rdfs:comment>
        <rdfs:label xml:lang="en">has part</rdfs:label>
    </owl:ObjectProperty>
    


    <!-- http://w3id.org/meta-share/meta-share/hasRecorded -->

    <owl:ObjectProperty rdf:about="http://w3id.org/meta-share/meta-share/hasRecorded">
        <rdfs:subPropertyOf rdf:resource="http://w3id.org/meta-share/meta-share/LΤRelatedTo"/>
        <owl:inverseOf rdf:resource="http://w3id.org/meta-share/meta-share/isRecordedBy"/>
        <rdfs:domain rdf:resource="http://w3id.org/meta-share/meta-share/ToolService"/>
        <rdfs:range>
            <owl:Class>
                <owl:unionOf rdf:parseType="Collection">
                    <rdf:Description rdf:about="http://w3id.org/meta-share/meta-share/CorpusAudioPart"/>
                    <rdf:Description rdf:about="http://w3id.org/meta-share/meta-share/CorpusTextNumericalPart"/>
                    <rdf:Description rdf:about="http://w3id.org/meta-share/meta-share/CorpusVideoPart"/>
                </owl:unionOf>
            </owl:Class>
        </rdfs:range>
        <rdfs:comment xml:lang="en">Links a tool/service to the data of the language resource (e.g.,  audio or video part of a corpus) it has recorded</rdfs:comment>
        <rdfs:label xml:lang="en">has recorded</rdfs:label>
    </owl:ObjectProperty>
    


    <!-- http://w3id.org/meta-share/meta-share/hasSubset -->

    <owl:ObjectProperty rdf:about="http://w3id.org/meta-share/meta-share/hasSubset">
        <rdfs:domain rdf:resource="http://w3id.org/meta-share/meta-share/MediaPart"/>
        <rdfs:range rdf:resource="http://w3id.org/meta-share/meta-share/Subset"/>
        <rdfs:comment xml:lang="en">Links to a subset of the resource that is described in order to add specific information on the subset (e.g. size per language for multilingual corpora, size per domain for lexica with multiple domains, etc.)</rdfs:comment>
        <rdfs:label xml:lang="en">has subset</rdfs:label>
        <skos:note xml:lang="en">introduced to cater for all sizePer properties; decided not to use the isPartOf because I wanted to keep this for &quot;whole&quot; language resources</skos:note>
    </owl:ObjectProperty>
    


    <!-- http://w3id.org/meta-share/meta-share/hasValidated -->

    <owl:ObjectProperty rdf:about="http://w3id.org/meta-share/meta-share/hasValidated">
        <rdfs:subPropertyOf rdf:resource="http://w3id.org/meta-share/meta-share/LΤRelatedTo"/>
        <owl:inverseOf rdf:resource="http://w3id.org/meta-share/meta-share/isValidatedBy"/>
        <rdfs:domain rdf:resource="http://w3id.org/meta-share/meta-share/ToolService"/>
        <rdfs:range rdf:resource="http://w3id.org/meta-share/meta-share/Validation"/>
        <rdfs:comment xml:lang="en">Links a tool/service B that is (or can be) used for validating LR A to the data of this validation</rdfs:comment>
        <rdfs:label xml:lang="en">has validated</rdfs:label>
    </owl:ObjectProperty>
    


    <!-- http://w3id.org/meta-share/meta-share/hasVersion -->

    <owl:ObjectProperty rdf:about="http://w3id.org/meta-share/meta-share/hasVersion">
        <rdfs:subPropertyOf rdf:resource="http://w3id.org/meta-share/meta-share/isRelatedToLR"/>
        <owl:inverseOf rdf:resource="http://w3id.org/meta-share/meta-share/isVersionOf"/>
        <rdfs:domain rdf:resource="http://w3id.org/meta-share/meta-share/LanguageResource"/>
        <rdfs:range rdf:resource="http://w3id.org/meta-share/meta-share/LanguageResource"/>
        <rdfs:comment xml:lang="en">Links to LR B that is a version of LR A (the one being described)</rdfs:comment>
        <rdfs:label xml:lang="en">has version</rdfs:label>
    </owl:ObjectProperty>
    


    <!-- http://w3id.org/meta-share/meta-share/hearingImpairmentOfParticipants -->

    <owl:ObjectProperty rdf:about="http://w3id.org/meta-share/meta-share/hearingImpairmentOfParticipants">
        <rdfs:domain>
            <owl:Class>
                <owl:unionOf rdf:parseType="Collection">
                    <rdf:Description rdf:about="http://w3id.org/meta-share/meta-share/CorpusAudioPart"/>
                    <rdf:Description rdf:about="http://w3id.org/meta-share/meta-share/CorpusImagePart"/>
                    <rdf:Description rdf:about="http://w3id.org/meta-share/meta-share/CorpusTextNumericalPart"/>
                    <rdf:Description rdf:about="http://w3id.org/meta-share/meta-share/CorpusVideoPart"/>
                </owl:unionOf>
            </owl:Class>
        </rdfs:domain>
        <rdfs:range rdf:resource="http://w3id.org/meta-share/meta-share/HearingImpairmentOfParticipants"/>
        <rdfs:comment xml:lang="en">Specifies whether the group of participants contains persons with hearing impairments</rdfs:comment>
        <rdfs:label xml:lang="en">hearing impairment of participants</rdfs:label>
    </owl:ObjectProperty>
    


    <!-- http://w3id.org/meta-share/meta-share/imageFormat -->

    <owl:ObjectProperty rdf:about="http://w3id.org/meta-share/meta-share/imageFormat">
        <rdfs:domain rdf:resource="http://w3id.org/meta-share/meta-share/DatasetDistribution"/>
        <rdfs:range rdf:resource="http://w3id.org/meta-share/meta-share/ImageFormat"/>
        <rdfs:comment xml:lang="en">Provides information on each of the format(s) of the image part of a resource</rdfs:comment>
        <rdfs:label xml:lang="en">image format</rdfs:label>
    </owl:ObjectProperty>
    


    <!-- http://w3id.org/meta-share/meta-share/inputContentResource -->

    <owl:ObjectProperty rdf:about="http://w3id.org/meta-share/meta-share/inputContentResource">
        <rdfs:domain rdf:resource="http://w3id.org/meta-share/meta-share/ToolService"/>
        <rdfs:range rdf:resource="http://w3id.org/meta-share/meta-share/ProcessingResource"/>
        <rdfs:comment xml:lang="en">Specifies the requirements set by a tool/service for the (content) resource that it processes</rdfs:comment>
        <rdfs:label xml:lang="en">input content resource</rdfs:label>
    </owl:ObjectProperty>
    


    <!-- http://w3id.org/meta-share/meta-share/intendedApplication -->

    <owl:ObjectProperty rdf:about="http://w3id.org/meta-share/meta-share/intendedApplication">
        <rdfs:domain rdf:resource="http://w3id.org/meta-share/meta-share/LanguageResource"/>
        <rdfs:range rdf:resource="http://w3id.org/meta-share/omtd-share/Operation"/>
        <rdfs:comment xml:lang="en">Specifies an LT application for which the language resource has been created or for which it can be used or is recommended to be used</rdfs:comment>
        <rdfs:label xml:lang="en">intended application</rdfs:label>
    </owl:ObjectProperty>
    


    <!-- http://w3id.org/meta-share/meta-share/interactivity -->

    <owl:ObjectProperty rdf:about="http://w3id.org/meta-share/meta-share/interactivity">
        <rdfs:domain>
            <owl:Class>
                <owl:unionOf rdf:parseType="Collection">
                    <rdf:Description rdf:about="http://w3id.org/meta-share/meta-share/CorpusAudioPart"/>
                    <rdf:Description rdf:about="http://w3id.org/meta-share/meta-share/CorpusVideoPart"/>
                </owl:unionOf>
            </owl:Class>
        </rdfs:domain>
        <rdfs:range rdf:resource="http://w3id.org/meta-share/meta-share/Interactivity"/>
        <rdfs:comment xml:lang="en">Indicates the level of conversational interaction between speakers (for audio component) or participants (for video component)</rdfs:comment>
        <rdfs:label xml:lang="en">interactivity</rdfs:label>
    </owl:ObjectProperty>
    


    <!-- http://w3id.org/meta-share/meta-share/iprHolder -->

    <owl:ObjectProperty rdf:about="http://w3id.org/meta-share/meta-share/iprHolder">
        <rdfs:subPropertyOf rdf:resource="http://w3id.org/meta-share/meta-share/isRelatedToActor"/>
        <owl:inverseOf rdf:resource="http://w3id.org/meta-share/meta-share/isIprHolderOf"/>
        <rdfs:domain rdf:resource="http://w3id.org/meta-share/meta-share/LanguageResource"/>
        <rdfs:range rdf:resource="http://w3id.org/meta-share/meta-share/Actor"/>
        <rdfs:altLabel xml:lang="en">intellectual property rights holder</rdfs:altLabel>
        <rdfs:altLabel xml:lang="en">rights holder</rdfs:altLabel>
        <rdfs:comment xml:lang="en">A person or an organization who holds the full Intellectual Property Rights (Copyright, trademark , etc.) that subsist in the resource. The IPR holder could be different from the creator that may have assigned the rights to the IPR holder (e.g.,  an author as a creator assigns her rights to the publisher who is the IPR holder) and the distributor that holds a specific licence (i.e. a permission) to distribute the work via a specific distributor.</rdfs:comment>
        <rdfs:label xml:lang="en">IPR holder</rdfs:label>
    </owl:ObjectProperty>
    


    <!-- http://w3id.org/meta-share/meta-share/isAccessedBy -->

    <owl:ObjectProperty rdf:about="http://w3id.org/meta-share/meta-share/isAccessedBy">
        <rdfs:subPropertyOf rdf:resource="http://w3id.org/meta-share/meta-share/isRelatedToLT"/>
        <rdfs:domain>
            <owl:Class>
                <owl:unionOf rdf:parseType="Collection">
                    <rdf:Description rdf:about="http://w3id.org/meta-share/meta-share/DataLanguageResource"/>
                    <rdf:Description rdf:about="http://w3id.org/meta-share/meta-share/MediaPart"/>
                </owl:unionOf>
            </owl:Class>
        </rdfs:domain>
        <rdfs:range rdf:resource="http://w3id.org/meta-share/meta-share/ToolService"/>
        <rdfs:altLabel xml:lang="en">access tool</rdfs:altLabel>
        <rdfs:comment xml:lang="en">Links to a tool/service B that is (or can be) used for accessing LR A (the one being described), e.g.,  a corpus workbench, s/w for lexicon access</rdfs:comment>
        <rdfs:label xml:lang="en">is accessed by</rdfs:label>
    </owl:ObjectProperty>
    


    <!-- http://w3id.org/meta-share/meta-share/isAlignedVersionOf -->

    <owl:ObjectProperty rdf:about="http://w3id.org/meta-share/meta-share/isAlignedVersionOf">
        <rdfs:subPropertyOf rdf:resource="http://w3id.org/meta-share/meta-share/isVersionOf"/>
        <rdfs:domain rdf:resource="http://w3id.org/meta-share/meta-share/Corpus"/>
        <rdfs:range rdf:resource="http://w3id.org/meta-share/meta-share/Corpus"/>
        <rdfs:comment xml:lang="en">Links to a corpus B which is the aligned version of corpus A (the one being described)</rdfs:comment>
        <rdfs:label xml:lang="en">is aligned version of</rdfs:label>
    </owl:ObjectProperty>
    


    <!-- http://w3id.org/meta-share/meta-share/isAnalysedBy -->

    <owl:ObjectProperty rdf:about="http://w3id.org/meta-share/meta-share/isAnalysedBy">
        <rdfs:subPropertyOf rdf:resource="http://w3id.org/meta-share/meta-share/isRelatedToLT"/>
        <rdfs:domain>
            <owl:Class>
                <owl:unionOf rdf:parseType="Collection">
                    <rdf:Description rdf:about="http://w3id.org/meta-share/meta-share/DataLanguageResource"/>
                    <rdf:Description rdf:about="http://w3id.org/meta-share/meta-share/MediaPart"/>
                </owl:unionOf>
            </owl:Class>
        </rdfs:domain>
        <rdfs:range rdf:resource="http://w3id.org/meta-share/meta-share/ToolService"/>
        <rdfs:altLabel xml:lang="en">analysis tool</rdfs:altLabel>
        <rdfs:comment xml:lang="en">Links to a tool/service B that is (or can be or has been) used for analysing LR A (the one being described), e.g.,  a statistical tool</rdfs:comment>
        <rdfs:label xml:lang="en">is analysed by</rdfs:label>
    </owl:ObjectProperty>
    


    <!-- http://w3id.org/meta-share/meta-share/isAnnotatedBy -->

    <owl:ObjectProperty rdf:about="http://w3id.org/meta-share/meta-share/isAnnotatedBy">
        <rdfs:subPropertyOf rdf:resource="http://w3id.org/meta-share/meta-share/isRelatedToLT"/>
        <rdfs:domain rdf:resource="http://w3id.org/meta-share/meta-share/Annotation"/>
        <rdfs:range rdf:resource="http://w3id.org/meta-share/meta-share/ToolService"/>
        <rdfs:altLabel xml:lang="en">annotation tool</rdfs:altLabel>
        <rdfs:comment xml:lang="en">Links to a tool/service B that has been used for annotating LR A (the one being described), e.g.,  a tagger, NER , etc.</rdfs:comment>
        <rdfs:label xml:lang="en">is annotated by</rdfs:label>
    </owl:ObjectProperty>
    


    <!-- http://w3id.org/meta-share/meta-share/isAnnotatedVersionOf -->

    <owl:ObjectProperty rdf:about="http://w3id.org/meta-share/meta-share/isAnnotatedVersionOf">
        <rdfs:subPropertyOf rdf:resource="http://w3id.org/meta-share/meta-share/isVersionOf"/>
        <rdfs:domain rdf:resource="http://w3id.org/meta-share/meta-share/Corpus"/>
        <rdfs:range rdf:resource="http://w3id.org/meta-share/meta-share/Corpus"/>
        <rdfs:comment xml:lang="en">Links to a corpus B which is the raw corpus that has been annotated (corpus A, the one being described)</rdfs:comment>
        <rdfs:label xml:lang="en">is annotated version of</rdfs:label>
    </owl:ObjectProperty>
    


    <!-- http://w3id.org/meta-share/meta-share/isAnnotationResourceOf -->

    <owl:ObjectProperty rdf:about="http://w3id.org/meta-share/meta-share/isAnnotationResourceOf">
        <rdfs:subPropertyOf rdf:resource="http://w3id.org/meta-share/meta-share/dependentLR"/>
        <rdfs:domain rdf:resource="http://w3id.org/meta-share/meta-share/LexicalConceptualResource"/>
        <rdfs:range>
            <owl:Class>
                <owl:unionOf rdf:parseType="Collection">
                    <rdf:Description rdf:about="http://w3id.org/meta-share/meta-share/MLModel"/>
                    <rdf:Description rdf:about="http://w3id.org/meta-share/meta-share/ProcessingResource"/>
                    <rdf:Description rdf:about="http://w3id.org/meta-share/meta-share/ToolService"/>
                </owl:unionOf>
            </owl:Class>
        </rdfs:range>
        <rdfs:comment xml:lang="en">Links an annotation resource to the corpus where it has been used for annotating or to data of an annotation tool/service that has been or can be combined with</rdfs:comment>
        <rdfs:label xml:lang="en">is annotation resource of</rdfs:label>
    </owl:ObjectProperty>
    


    <!-- http://w3id.org/meta-share/meta-share/isAnnotationSchemaOf -->

    <owl:ObjectProperty rdf:about="http://w3id.org/meta-share/meta-share/isAnnotationSchemaOf">
        <rdfs:subPropertyOf rdf:resource="http://w3id.org/meta-share/meta-share/dependentLR"/>
        <rdfs:domain rdf:resource="http://w3id.org/meta-share/meta-share/LexicalConceptualResource"/>
        <rdfs:range>
            <owl:Class>
                <owl:unionOf rdf:parseType="Collection">
                    <rdf:Description rdf:about="http://w3id.org/meta-share/meta-share/MLModel"/>
                    <rdf:Description rdf:about="http://w3id.org/meta-share/meta-share/ProcessingResource"/>
                    <rdf:Description rdf:about="http://w3id.org/meta-share/meta-share/ToolService"/>
                </owl:unionOf>
            </owl:Class>
        </rdfs:range>
        <rdfs:comment xml:lang="en">Links an annotation schema  to the corpus where it has been used for annotating or to data of an annotation tool/service that has been or can be combined with</rdfs:comment>
        <rdfs:label xml:lang="en">is annotation schema of</rdfs:label>
    </owl:ObjectProperty>
    


    <!-- http://w3id.org/meta-share/meta-share/isAnnotatorOf -->

    <owl:ObjectProperty rdf:about="http://w3id.org/meta-share/meta-share/isAnnotatorOf">
        <rdfs:subPropertyOf rdf:resource="http://w3id.org/meta-share/meta-share/actorRelatedTo"/>
        <rdfs:domain rdf:resource="http://w3id.org/meta-share/meta-share/Actor"/>
        <rdfs:range rdf:resource="http://w3id.org/meta-share/meta-share/Annotation"/>
        <rdfs:comment xml:lang="en">Identifies the resource(s) that have been annotated by the person/organization</rdfs:comment>
        <rdfs:label xml:lang="en">is annotator of</rdfs:label>
    </owl:ObjectProperty>
    


    <!-- http://w3id.org/meta-share/meta-share/isArchivedBy -->

    <owl:ObjectProperty rdf:about="http://w3id.org/meta-share/meta-share/isArchivedBy">
        <rdfs:subPropertyOf rdf:resource="http://w3id.org/meta-share/meta-share/isRelatedToLT"/>
        <rdfs:domain rdf:resource="http://w3id.org/meta-share/meta-share/DataLanguageResource"/>
        <rdfs:range rdf:resource="http://w3id.org/meta-share/meta-share/ToolService"/>
        <rdfs:altLabel xml:lang="en">archiving tool</rdfs:altLabel>
        <rdfs:comment xml:lang="en">Links to a tool/service B that is (or can be or has been) used for archiving LR A (the one being described)</rdfs:comment>
        <rdfs:label xml:lang="en">is archived by</rdfs:label>
    </owl:ObjectProperty>
    


    <!-- http://w3id.org/meta-share/meta-share/isCitedBy -->

    <owl:ObjectProperty rdf:about="http://w3id.org/meta-share/meta-share/isCitedBy">
        <rdfs:subPropertyOf rdf:resource="http://w3id.org/meta-share/meta-share/isRelatedToDocument"/>
        <rdfs:domain rdf:resource="http://w3id.org/meta-share/meta-share/LanguageResource"/>
        <rdfs:range rdf:resource="http://w3id.org/meta-share/meta-share/Document"/>
        <rdfs:comment xml:lang="en">Links to a publication that cites the language resource described</rdfs:comment>
        <rdfs:label xml:lang="en">is cited by</rdfs:label>
    </owl:ObjectProperty>
    


    <!-- http://w3id.org/meta-share/meta-share/isCombinedWith -->

    <owl:ObjectProperty rdf:about="http://w3id.org/meta-share/meta-share/isCombinedWith">
        <rdfs:subPropertyOf rdf:resource="http://w3id.org/meta-share/meta-share/isRelatedToLR"/>
        <rdf:type rdf:resource="http://www.w3.org/2002/07/owl#SymmetricProperty"/>
        <rdfs:domain rdf:resource="http://w3id.org/meta-share/meta-share/LanguageResource"/>
        <rdfs:range rdf:resource="http://w3id.org/meta-share/meta-share/LanguageResource"/>
        <rdfs:comment xml:lang="en">Links to a LR B that has been used together with LR A (the one being described) to create LR C, e.g.,  two monolingual wordnets/corpora aligned to produce a bilingual resource</rdfs:comment>
        <rdfs:label xml:lang="en">is combined with</rdfs:label>
    </owl:ObjectProperty>
    


    <!-- http://w3id.org/meta-share/meta-share/isCompatibleWith -->

    <owl:ObjectProperty rdf:about="http://w3id.org/meta-share/meta-share/isCompatibleWith">
        <rdfs:subPropertyOf rdf:resource="http://w3id.org/meta-share/meta-share/dependsOn"/>
        <rdf:type rdf:resource="http://www.w3.org/2002/07/owl#SymmetricProperty"/>
        <rdfs:domain rdf:resource="http://w3id.org/meta-share/meta-share/LanguageResource"/>
        <rdfs:range rdf:resource="http://w3id.org/meta-share/meta-share/LanguageResource"/>
        <rdfs:comment xml:lang="en">Links to a LR B that can be used together with LR A (the one being described), e.g.,  a lexicon that is compatible with a grammar</rdfs:comment>
        <rdfs:label xml:lang="en">is compatible with</rdfs:label>
    </owl:ObjectProperty>
    


    <!-- http://w3id.org/meta-share/meta-share/isContactFor -->

    <owl:ObjectProperty rdf:about="http://w3id.org/meta-share/meta-share/isContactFor">
        <rdfs:subPropertyOf rdf:resource="http://w3id.org/meta-share/meta-share/actorRelatedTo"/>
        <rdfs:domain rdf:resource="http://w3id.org/meta-share/meta-share/Actor"/>
        <rdfs:range rdf:resource="http://w3id.org/meta-share/meta-share/LanguageResource"/>
        <rdfs:comment xml:lang="en">Links to the language resource(s) for which the person/organization/group can be contacted for further information</rdfs:comment>
        <rdfs:label xml:lang="en">is contact for</rdfs:label>
    </owl:ObjectProperty>
    


    <!-- http://w3id.org/meta-share/meta-share/isContinuationOf -->

    <owl:ObjectProperty rdf:about="http://w3id.org/meta-share/meta-share/isContinuationOf">
        <rdfs:subPropertyOf rdf:resource="http://w3id.org/meta-share/meta-share/isVersionOf"/>
        <owl:inverseOf rdf:resource="http://w3id.org/meta-share/meta-share/isContinuedBy"/>
        <rdfs:domain rdf:resource="http://w3id.org/meta-share/meta-share/LanguageResource"/>
        <rdfs:range rdf:resource="http://w3id.org/meta-share/meta-share/LanguageResource"/>
        <rdfs:comment xml:lang="en">Links to LR B that forms the basis of LR A (the one being described) upon which it has continued to extend / enrich</rdfs:comment>
        <rdfs:label xml:lang="en">is continuation of</rdfs:label>
    </owl:ObjectProperty>
    


    <!-- http://w3id.org/meta-share/meta-share/isContinuedBy -->

    <owl:ObjectProperty rdf:about="http://w3id.org/meta-share/meta-share/isContinuedBy">
        <rdfs:subPropertyOf rdf:resource="http://w3id.org/meta-share/meta-share/hasVersion"/>
        <rdfs:domain rdf:resource="http://w3id.org/meta-share/meta-share/LanguageResource"/>
        <rdfs:range rdf:resource="http://w3id.org/meta-share/meta-share/LanguageResource"/>
        <rdfs:comment xml:lang="en">Links to a LR B that extends / continues / enriches LR A (the one being described)</rdfs:comment>
        <rdfs:label xml:lang="en">is continued by</rdfs:label>
    </owl:ObjectProperty>
    


    <!-- http://w3id.org/meta-share/meta-share/isConvertedVersionOf -->

    <owl:ObjectProperty rdf:about="http://w3id.org/meta-share/meta-share/isConvertedVersionOf">
        <rdfs:subPropertyOf rdf:resource="http://w3id.org/meta-share/meta-share/isVersionOf"/>
        <rdfs:domain rdf:resource="http://w3id.org/meta-share/meta-share/DataLanguageResource"/>
        <rdfs:range rdf:resource="http://w3id.org/meta-share/meta-share/DataLanguageResource"/>
        <rdfs:comment xml:lang="en">Links to LR B that has been the outcome of a conversion procedure from LR A (the one being described), e.g.,  a PDF to text conversion</rdfs:comment>
        <rdfs:label xml:lang="en">is converted version of</rdfs:label>
    </owl:ObjectProperty>
    


    <!-- http://w3id.org/meta-share/meta-share/isCreatedBy -->

    <owl:ObjectProperty rdf:about="http://w3id.org/meta-share/meta-share/isCreatedBy">
        <rdfs:subPropertyOf rdf:resource="http://w3id.org/meta-share/meta-share/isRelatedToLT"/>
        <rdfs:domain>
            <owl:Class>
                <owl:unionOf rdf:parseType="Collection">
                    <rdf:Description rdf:about="http://w3id.org/meta-share/meta-share/DataLanguageResource"/>
                    <rdf:Description rdf:about="http://w3id.org/meta-share/meta-share/MediaPart"/>
                </owl:unionOf>
            </owl:Class>
        </rdfs:domain>
        <rdfs:range rdf:resource="http://w3id.org/meta-share/meta-share/ToolService"/>
        <rdfs:altLabel xml:lang="en">creation tool</rdfs:altLabel>
        <rdfs:altLabel xml:lang="en">derivation tool</rdfs:altLabel>
        <rdfs:comment xml:lang="en">Links to a tool/service B that has been used for creating LR A (the one being described)</rdfs:comment>
        <rdfs:label xml:lang="en">is created by</rdfs:label>
    </owl:ObjectProperty>
    


    <!-- http://w3id.org/meta-share/meta-share/isDescribedBy -->

    <owl:ObjectProperty rdf:about="http://w3id.org/meta-share/meta-share/isDescribedBy">
        <rdfs:subPropertyOf rdf:resource="http://w3id.org/meta-share/meta-share/isDocumentedBy"/>
        <rdfs:domain rdf:resource="http://w3id.org/meta-share/meta-share/LanguageResource"/>
        <rdfs:range rdf:resource="http://w3id.org/meta-share/meta-share/Document"/>
        <rdfs:comment xml:lang="en">Links to a document that describes the contents or operation of a language resource</rdfs:comment>
        <rdfs:label xml:lang="en">is described by</rdfs:label>
    </owl:ObjectProperty>
    


    <!-- http://w3id.org/meta-share/meta-share/isDisplayedBy -->

    <owl:ObjectProperty rdf:about="http://w3id.org/meta-share/meta-share/isDisplayedBy">
        <rdfs:subPropertyOf rdf:resource="http://w3id.org/meta-share/meta-share/isRelatedToLT"/>
        <rdfs:domain>
            <owl:Class>
                <owl:unionOf rdf:parseType="Collection">
                    <rdf:Description rdf:about="http://w3id.org/meta-share/meta-share/DataLanguageResource"/>
                    <rdf:Description rdf:about="http://w3id.org/meta-share/meta-share/MediaPart"/>
                </owl:unionOf>
            </owl:Class>
        </rdfs:domain>
        <rdfs:range rdf:resource="http://w3id.org/meta-share/meta-share/ToolService"/>
        <rdfs:altLabel xml:lang="en">display tool</rdfs:altLabel>
        <rdfs:altLabel xml:lang="en">visualization tool</rdfs:altLabel>
        <rdfs:comment xml:lang="en">Links to a tool/service B that is (or can be) used to display LR A (the one being described), e.g.,  a tool for visualizing relations in a lexicon, or annotations in a corpus</rdfs:comment>
        <rdfs:label xml:lang="en">is displayed by</rdfs:label>
    </owl:ObjectProperty>
    


    <!-- http://w3id.org/meta-share/meta-share/isDistributionRightsHolderOf -->

    <owl:ObjectProperty rdf:about="http://w3id.org/meta-share/meta-share/isDistributionRightsHolderOf">
        <rdfs:subPropertyOf rdf:resource="http://w3id.org/meta-share/meta-share/actorRelatedTo"/>
        <rdfs:domain rdf:resource="http://w3id.org/meta-share/meta-share/Actor"/>
        <rdfs:range rdf:resource="http://w3id.org/meta-share/meta-share/Distribution"/>
        <rdfs:comment xml:lang="en">Identifies the language resource for which a person or an organization holds the distribution rights. The range and scope of distribution rights is defined in the distribution agreement. The distributor in most cases only has a limited licence to distribute the work and collect royalties on behalf of the licensor or the IPR holder and cannot give to any recipient of the work permissions that exceed the scope of the distribution agreement (e.g.,  to allow uses of the work that are not defined in the distribution agreement)</rdfs:comment>
        <rdfs:label xml:lang="en">is distribution rights holder of</rdfs:label>
    </owl:ObjectProperty>
    


    <!-- http://w3id.org/meta-share/meta-share/isDivisionOf -->

    <owl:ObjectProperty rdf:about="http://w3id.org/meta-share/meta-share/isDivisionOf">
        <rdfs:domain rdf:resource="http://w3id.org/meta-share/meta-share/Division"/>
        <rdfs:range rdf:resource="http://w3id.org/meta-share/meta-share/Organization"/>
        <rdfs:comment xml:lang="en">Links a division to the organization to which it is associated</rdfs:comment>
        <rdfs:label xml:lang="en">is division of</rdfs:label>
    </owl:ObjectProperty>
    


    <!-- http://w3id.org/meta-share/meta-share/isDocumentedBy -->

    <owl:ObjectProperty rdf:about="http://w3id.org/meta-share/meta-share/isDocumentedBy">
        <rdfs:subPropertyOf rdf:resource="http://w3id.org/meta-share/meta-share/isRelatedToDocument"/>
        <rdfs:domain rdf:resource="http://w3id.org/meta-share/meta-share/LanguageResource"/>
        <rdfs:range rdf:resource="http://w3id.org/meta-share/meta-share/Document"/>
        <rdfs:altLabel xml:lang="en">documentation report</rdfs:altLabel>
        <rdfs:comment xml:lang="en">Links a language resource to a document (e.g.,  research paper describing its contents or its use in a project, user manual, etc.) or any other form of documentation (e.g.,  a URL with support information) that is related to the resource</rdfs:comment>
        <rdfs:label xml:lang="en">is documented by</rdfs:label>
    </owl:ObjectProperty>
    


    <!-- http://w3id.org/meta-share/meta-share/isEditedBy -->

    <owl:ObjectProperty rdf:about="http://w3id.org/meta-share/meta-share/isEditedBy">
        <rdfs:subPropertyOf rdf:resource="http://w3id.org/meta-share/meta-share/isRelatedToLT"/>
        <rdfs:domain>
            <owl:Class>
                <owl:unionOf rdf:parseType="Collection">
                    <rdf:Description rdf:about="http://w3id.org/meta-share/meta-share/DataLanguageResource"/>
                    <rdf:Description rdf:about="http://w3id.org/meta-share/meta-share/MediaPart"/>
                </owl:unionOf>
            </owl:Class>
        </rdfs:domain>
        <rdfs:range rdf:resource="http://w3id.org/meta-share/meta-share/ToolService"/>
        <rdfs:altLabel xml:lang="en">editing tool</rdfs:altLabel>
        <rdfs:comment xml:lang="en">Links to a tool/service B that is (or can be) used for editing LR A (the one being described)</rdfs:comment>
        <rdfs:label xml:lang="en">is edited by</rdfs:label>
    </owl:ObjectProperty>
    


    <!-- http://w3id.org/meta-share/meta-share/isElicitedBy -->

    <owl:ObjectProperty rdf:about="http://w3id.org/meta-share/meta-share/isElicitedBy">
        <rdfs:subPropertyOf rdf:resource="http://w3id.org/meta-share/meta-share/isRelatedToLT"/>
        <rdfs:domain>
            <owl:Class>
                <owl:unionOf rdf:parseType="Collection">
                    <rdf:Description rdf:about="http://w3id.org/meta-share/meta-share/DataLanguageResource"/>
                    <rdf:Description rdf:about="http://w3id.org/meta-share/meta-share/MediaPart"/>
                </owl:unionOf>
            </owl:Class>
        </rdfs:domain>
        <rdfs:range rdf:resource="http://w3id.org/meta-share/meta-share/ToolService"/>
        <rdfs:altLabel xml:lang="en">elicitation tool</rdfs:altLabel>
        <rdfs:comment xml:lang="en">Links to a tool/service B that is (or can be or has been) used for eliciting LR A (the one being described)</rdfs:comment>
        <rdfs:label xml:lang="en">is elicited by</rdfs:label>
    </owl:ObjectProperty>
    


    <!-- http://w3id.org/meta-share/meta-share/isEvaluatedBy -->

    <owl:ObjectProperty rdf:about="http://w3id.org/meta-share/meta-share/isEvaluatedBy">
        <rdfs:subPropertyOf rdf:resource="http://w3id.org/meta-share/meta-share/isRelatedToLT"/>
        <rdfs:domain rdf:resource="http://w3id.org/meta-share/meta-share/Evaluation"/>
        <rdfs:range rdf:resource="http://w3id.org/meta-share/meta-share/ToolService"/>
        <rdfs:altLabel xml:lang="en">evaluation tool</rdfs:altLabel>
        <rdfs:comment xml:lang="en">Links to a tool/service B that has been used to evaluate LR A (the one being described)</rdfs:comment>
        <rdfs:label xml:lang="en">is evaluated by</rdfs:label>
    </owl:ObjectProperty>
    


    <!-- http://w3id.org/meta-share/meta-share/isEvaluatorOf -->

    <owl:ObjectProperty rdf:about="http://w3id.org/meta-share/meta-share/isEvaluatorOf">
        <rdfs:subPropertyOf rdf:resource="http://w3id.org/meta-share/meta-share/actorRelatedTo"/>
        <rdfs:domain rdf:resource="http://w3id.org/meta-share/meta-share/Actor"/>
        <rdfs:range rdf:resource="http://w3id.org/meta-share/meta-share/Evaluation"/>
        <rdfs:comment xml:lang="en">Identifies the tool or service(s) that a person or organization that has evaluated</rdfs:comment>
        <rdfs:label xml:lang="en">is evaluator of</rdfs:label>
    </owl:ObjectProperty>
    


    <!-- http://w3id.org/meta-share/meta-share/isExactMatchWith -->

    <owl:ObjectProperty rdf:about="http://w3id.org/meta-share/meta-share/isExactMatchWith">
        <rdfs:subPropertyOf rdf:resource="http://w3id.org/meta-share/meta-share/isRelatedToLR"/>
        <rdf:type rdf:resource="http://www.w3.org/2002/07/owl#SymmetricProperty"/>
        <rdfs:domain rdf:resource="http://w3id.org/meta-share/meta-share/LanguageResource"/>
        <rdfs:range rdf:resource="http://w3id.org/meta-share/meta-share/LanguageResource"/>
        <rdfs:altLabel xml:lang="en">is identical with</rdfs:altLabel>
        <rdfs:altLabel xml:lang="en">is same as</rdfs:altLabel>
        <rdfs:comment xml:lang="en">Links to LR B that has the same contents with LR A; they may have different names or the same name and be stored on different locations</rdfs:comment>
        <rdfs:label xml:lang="en">is exact match with</rdfs:label>
    </owl:ObjectProperty>
    


    <!-- http://w3id.org/meta-share/meta-share/isFunderOf -->

    <owl:ObjectProperty rdf:about="http://w3id.org/meta-share/meta-share/isFunderOf">
        <rdfs:subPropertyOf rdf:resource="http://w3id.org/meta-share/meta-share/actorRelatedTo"/>
        <rdfs:domain rdf:resource="http://w3id.org/meta-share/meta-share/Actor"/>
        <rdfs:range rdf:resource="http://w3id.org/meta-share/meta-share/Project"/>
        <rdfs:comment xml:lang="en">Links to the projects) that the person/organization has financed</rdfs:comment>
        <rdfs:label xml:lang="en">is funder of</rdfs:label>
    </owl:ObjectProperty>
    


    <!-- http://w3id.org/meta-share/meta-share/isFundingProjectOf -->

    <owl:ObjectProperty rdf:about="http://w3id.org/meta-share/meta-share/isFundingProjectOf">
        <rdfs:subPropertyOf rdf:resource="http://w3id.org/meta-share/meta-share/projectRelatedTo"/>
        <rdfs:domain rdf:resource="http://w3id.org/meta-share/meta-share/Project"/>
        <rdfs:range rdf:resource="http://w3id.org/meta-share/meta-share/LanguageResource"/>
        <rdfs:comment xml:lang="en">Links a project to the language resource(s) that it has funded (e.g.,  creation, enrichment, extension , etc.)</rdfs:comment>
        <rdfs:label xml:lang="en">is funding project of</rdfs:label>
    </owl:ObjectProperty>
    


    <!-- http://w3id.org/meta-share/meta-share/isIprHolderOf -->

    <owl:ObjectProperty rdf:about="http://w3id.org/meta-share/meta-share/isIprHolderOf">
        <rdfs:subPropertyOf rdf:resource="http://w3id.org/meta-share/meta-share/actorRelatedTo"/>
        <rdfs:domain rdf:resource="http://w3id.org/meta-share/meta-share/Actor"/>
        <rdfs:range rdf:resource="http://w3id.org/meta-share/meta-share/LanguageResource"/>
        <rdfs:comment xml:lang="en">Links to the resource(s) for which a person or an organization holds the full Intellectual Property Rights (Copyright, trademark , etc.). The IPR holder could be different from the creator that may have assigned the rights to the IPR holder (e.g.,  an author as a creator assigns her rights to the publisher who is the IPR holder) and the distributor that holds a specific licence (i.e. a permission) to distribute the work via a specific distributor.</rdfs:comment>
        <rdfs:label xml:lang="en">is IPR holder of</rdfs:label>
    </owl:ObjectProperty>
    


    <!-- http://w3id.org/meta-share/meta-share/isLicensorOr -->

    <owl:ObjectProperty rdf:about="http://w3id.org/meta-share/meta-share/isLicensorOr">
        <rdfs:subPropertyOf rdf:resource="http://w3id.org/meta-share/meta-share/actorRelatedTo"/>
        <owl:inverseOf rdf:resource="http://w3id.org/meta-share/meta-share/licensor"/>
        <rdfs:domain rdf:resource="http://w3id.org/meta-share/meta-share/Actor"/>
        <rdfs:range rdf:resource="http://w3id.org/meta-share/meta-share/Distribution"/>
        <rdfs:comment xml:lang="en">Links to the resource(s) which a person or organisation is legally eligible to license and actually licenses. The licensor could be different from the creator, the distributor or the IPR holder. The licensor has the necessary rights or licences to license the work and is the party that actually licenses the resource that is distributed via the specific channel. She will have obtained the necessary rights or licences from the IPR holder and she may have a distribution agreement with a distributor that disseminates the work under a set of conditions defined in the specific  licence and collects revenue on the licensor&apos;s behalf. The attribution of the creator, separately from the attribution of the licensor, may be part of the licence under which the resource is distributed (as e.g.,  is the case with Creative Commons Licences).</rdfs:comment>
        <rdfs:label xml:lang="en">is licensor of</rdfs:label>
    </owl:ObjectProperty>
    


    <!-- http://w3id.org/meta-share/meta-share/isMLModelOf -->

    <owl:ObjectProperty rdf:about="http://w3id.org/meta-share/meta-share/isMLModelOf">
        <rdfs:subPropertyOf rdf:resource="http://w3id.org/meta-share/meta-share/dependentLR"/>
        <owl:inverseOf rdf:resource="http://w3id.org/meta-share/meta-share/mlModel"/>
        <rdfs:domain rdf:resource="http://w3id.org/meta-share/meta-share/MLModel"/>
        <rdfs:range rdf:resource="http://w3id.org/meta-share/meta-share/ToolService"/>
        <rdfs:altLabel xml:lang="en">is Machine Learning model of</rdfs:altLabel>
        <rdfs:comment xml:lang="en">Specifies the tool/service with which the ML model can be combined in order to perform the desired task</rdfs:comment>
        <rdfs:label xml:lang="en">is ML model of</rdfs:label>
    </owl:ObjectProperty>
    


    <!-- http://w3id.org/meta-share/meta-share/isMetadataCreatorOf -->

    <owl:ObjectProperty rdf:about="http://w3id.org/meta-share/meta-share/isMetadataCreatorOf">
        <rdfs:subPropertyOf rdf:resource="http://w3id.org/meta-share/meta-share/actorRelatedTo"/>
        <owl:inverseOf rdf:resource="http://w3id.org/meta-share/meta-share/metadataCreator"/>
        <rdfs:domain rdf:resource="http://w3id.org/meta-share/meta-share/Person"/>
        <rdfs:range rdf:resource="http://w3id.org/meta-share/meta-share/MetadataRecord"/>
        <rdfs:comment xml:lang="en">Links to the metadata record(s) that a person has created</rdfs:comment>
        <rdfs:label xml:lang="en">is metadata creator of</rdfs:label>
    </owl:ObjectProperty>
    


    <!-- http://w3id.org/meta-share/meta-share/isMetadataCuratorOf -->

    <owl:ObjectProperty rdf:about="http://w3id.org/meta-share/meta-share/isMetadataCuratorOf">
        <rdfs:subPropertyOf rdf:resource="http://w3id.org/meta-share/meta-share/actorRelatedTo"/>
        <owl:inverseOf rdf:resource="http://w3id.org/meta-share/meta-share/metadataCurator"/>
        <rdfs:domain rdf:resource="http://w3id.org/meta-share/meta-share/Person"/>
        <rdfs:range rdf:resource="http://w3id.org/meta-share/meta-share/MetadataRecord"/>
        <rdfs:comment xml:lang="en">Links to the metadata record(s) for which a person is responsible for creating, updating, enriching, etc.</rdfs:comment>
        <rdfs:label xml:lang="en">is metadata curator of</rdfs:label>
    </owl:ObjectProperty>
    


    <!-- http://w3id.org/meta-share/meta-share/isMetadataOf -->

    <owl:ObjectProperty rdf:about="http://w3id.org/meta-share/meta-share/isMetadataOf">
        <rdfs:subPropertyOf rdf:resource="http://w3id.org/meta-share/meta-share/MDRecordRelatedTo"/>
        <rdfs:domain rdf:resource="http://w3id.org/meta-share/meta-share/MetadataRecord"/>
        <rdfs:range rdf:resource="http://w3id.org/meta-share/meta-share/LanguageResource"/>
        <rdfs:comment xml:lang="en">Links an external metadata record (from another catalogue, repository, etc.) to the language resource described</rdfs:comment>
        <rdfs:label xml:lang="en">is metadata of</rdfs:label>
    </owl:ObjectProperty>
    


    <!-- http://w3id.org/meta-share/meta-share/isPartOf -->

    <owl:ObjectProperty rdf:about="http://w3id.org/meta-share/meta-share/isPartOf">
        <rdfs:subPropertyOf rdf:resource="http://w3id.org/meta-share/meta-share/isRelatedToLR"/>
        <rdfs:domain rdf:resource="http://w3id.org/meta-share/meta-share/LanguageResource"/>
        <rdfs:range rdf:resource="http://w3id.org/meta-share/meta-share/LanguageResource"/>
        <rdfs:comment xml:lang="en">Links to LR B which contains LR A (the one being described), e.g.,  a bilingual corpus that includes a monolingual corpus</rdfs:comment>
        <rdfs:label xml:lang="en">is part of</rdfs:label>
    </owl:ObjectProperty>
    


    <!-- http://w3id.org/meta-share/meta-share/isPartWith -->

    <owl:ObjectProperty rdf:about="http://w3id.org/meta-share/meta-share/isPartWith">
        <rdfs:subPropertyOf rdf:resource="http://w3id.org/meta-share/meta-share/isRelatedToLR"/>
        <rdf:type rdf:resource="http://www.w3.org/2002/07/owl#SymmetricProperty"/>
        <rdfs:domain rdf:resource="http://w3id.org/meta-share/meta-share/LanguageResource"/>
        <rdfs:range rdf:resource="http://w3id.org/meta-share/meta-share/LanguageResource"/>
        <rdfs:comment xml:lang="en">Links to LR B that together with LR A (the one being described) are parts of LR C</rdfs:comment>
        <rdfs:label xml:lang="en">is part with</rdfs:label>
    </owl:ObjectProperty>
    


    <!-- http://w3id.org/meta-share/meta-share/isParticipatingOrganizationIn -->

    <owl:ObjectProperty rdf:about="http://w3id.org/meta-share/meta-share/isParticipatingOrganizationIn">
        <rdfs:subPropertyOf rdf:resource="http://w3id.org/meta-share/meta-share/actorRelatedTo"/>
        <owl:inverseOf rdf:resource="http://w3id.org/meta-share/meta-share/participatingOrganization"/>
        <rdfs:domain rdf:resource="http://w3id.org/meta-share/meta-share/Organization"/>
        <rdfs:range rdf:resource="http://w3id.org/meta-share/meta-share/Project"/>
        <rdfs:comment xml:lang="en">Identifies the project(s) where an organization has officially participated or is participating</rdfs:comment>
        <rdfs:label xml:lang="en">is participating organization in</rdfs:label>
    </owl:ObjectProperty>
    


    <!-- http://w3id.org/meta-share/meta-share/isQueriedBy -->

    <owl:ObjectProperty rdf:about="http://w3id.org/meta-share/meta-share/isQueriedBy">
        <rdfs:subPropertyOf rdf:resource="http://w3id.org/meta-share/meta-share/isRelatedToLT"/>
        <owl:inverseOf rdf:resource="http://w3id.org/meta-share/meta-share/queries"/>
        <rdfs:domain rdf:resource="http://w3id.org/meta-share/meta-share/DataLanguageResource"/>
        <rdfs:range rdf:resource="http://w3id.org/meta-share/meta-share/ToolService"/>
        <rdfs:altLabel xml:lang="en">query tool</rdfs:altLabel>
        <rdfs:comment xml:lang="en">Links to a tool/service B that is (or can be) used for querying LR A (the one being described)</rdfs:comment>
        <rdfs:label xml:lang="en">is queried by</rdfs:label>
    </owl:ObjectProperty>
    


    <!-- http://w3id.org/meta-share/meta-share/isRecordedBy -->

    <owl:ObjectProperty rdf:about="http://w3id.org/meta-share/meta-share/isRecordedBy">
        <rdfs:subPropertyOf rdf:resource="http://w3id.org/meta-share/meta-share/isRelatedToLT"/>
        <rdfs:domain>
            <owl:Class>
                <owl:unionOf rdf:parseType="Collection">
                    <rdf:Description rdf:about="http://w3id.org/meta-share/meta-share/CorpusAudioPart"/>
                    <rdf:Description rdf:about="http://w3id.org/meta-share/meta-share/CorpusTextNumericalPart"/>
                    <rdf:Description rdf:about="http://w3id.org/meta-share/meta-share/CorpusVideoPart"/>
                </owl:unionOf>
            </owl:Class>
        </rdfs:domain>
        <rdfs:range rdf:resource="http://w3id.org/meta-share/meta-share/ToolService"/>
        <rdfs:altLabel xml:lang="en">recording platform software</rdfs:altLabel>
        <rdfs:altLabel xml:lang="en">recording tool</rdfs:altLabel>
        <rdfs:comment xml:lang="en">Links to a tool/service that has been used for recording a video or audio corpus part</rdfs:comment>
        <rdfs:label xml:lang="en">is recorded by</rdfs:label>
    </owl:ObjectProperty>
    


    <!-- http://w3id.org/meta-share/meta-share/isRecorderOf -->

    <owl:ObjectProperty rdf:about="http://w3id.org/meta-share/meta-share/isRecorderOf">
        <rdfs:subPropertyOf rdf:resource="http://w3id.org/meta-share/meta-share/actorRelatedTo"/>
        <owl:inverseOf rdf:resource="http://w3id.org/meta-share/meta-share/recorder"/>
        <rdfs:domain rdf:resource="http://w3id.org/meta-share/meta-share/Actor"/>
        <rdfs:range>
            <owl:Class>
                <owl:unionOf rdf:parseType="Collection">
                    <rdf:Description rdf:about="http://w3id.org/meta-share/meta-share/CorpusAudioPart"/>
                    <rdf:Description rdf:about="http://w3id.org/meta-share/meta-share/CorpusTextNumericalPart"/>
                    <rdf:Description rdf:about="http://w3id.org/meta-share/meta-share/CorpusVideoPart"/>
                </owl:unionOf>
            </owl:Class>
        </rdfs:range>
        <rdfs:comment xml:lang="en">Links to the audio or video part of the resource(s) that a person/organization has recorded</rdfs:comment>
        <rdfs:label xml:lang="en">is recorder of</rdfs:label>
    </owl:ObjectProperty>
    


    <!-- http://w3id.org/meta-share/meta-share/isRelatedTo -->

    <owl:ObjectProperty rdf:about="http://w3id.org/meta-share/meta-share/isRelatedTo">
        <rdfs:domain>
            <owl:Class>
                <owl:unionOf rdf:parseType="Collection">
                    <rdf:Description rdf:about="http://w3id.org/meta-share/meta-share/DescribedEntity"/>
                    <rdf:Description rdf:about="http://w3id.org/meta-share/meta-share/MetadataRecord"/>
                </owl:unionOf>
            </owl:Class>
        </rdfs:domain>
        <rdfs:range>
            <owl:Class>
                <owl:unionOf rdf:parseType="Collection">
                    <rdf:Description rdf:about="http://w3id.org/meta-share/meta-share/Actor"/>
                    <rdf:Description rdf:about="http://w3id.org/meta-share/meta-share/Document"/>
                    <rdf:Description rdf:about="http://w3id.org/meta-share/meta-share/LanguageResource"/>
                </owl:unionOf>
            </owl:Class>
        </rdfs:range>
        <rdfs:comment xml:lang="en">Identifies a relation holding between two language resources or a language resource and a document or actor or, in general, a satellite entity</rdfs:comment>
        <rdfs:label xml:lang="en">is related to</rdfs:label>
    </owl:ObjectProperty>
    


    <!-- http://w3id.org/meta-share/meta-share/isRelatedToActor -->

    <owl:ObjectProperty rdf:about="http://w3id.org/meta-share/meta-share/isRelatedToActor">
        <rdfs:subPropertyOf rdf:resource="http://w3id.org/meta-share/meta-share/isRelatedTo"/>
        <rdfs:domain>
            <owl:Class>
                <owl:unionOf rdf:parseType="Collection">
                    <rdf:Description rdf:about="http://w3id.org/meta-share/meta-share/Distribution"/>
                    <rdf:Description rdf:about="http://w3id.org/meta-share/meta-share/LanguageResource"/>
                    <rdf:Description rdf:about="http://w3id.org/meta-share/meta-share/MetadataRecord"/>
                </owl:unionOf>
            </owl:Class>
        </rdfs:domain>
        <rdfs:range rdf:resource="http://w3id.org/meta-share/meta-share/Actor"/>
        <rdfs:comment xml:lang="en">Links to the data of an actor that bears some relation to the language resource that is described</rdfs:comment>
        <rdfs:label xml:lang="en">is related to actor</rdfs:label>
    </owl:ObjectProperty>
    


    <!-- http://w3id.org/meta-share/meta-share/isRelatedToDocument -->

    <owl:ObjectProperty rdf:about="http://w3id.org/meta-share/meta-share/isRelatedToDocument">
        <rdfs:subPropertyOf rdf:resource="http://w3id.org/meta-share/meta-share/isRelatedTo"/>
        <rdfs:domain>
            <owl:Class>
                <owl:unionOf rdf:parseType="Collection">
                    <rdf:Description rdf:about="http://w3id.org/meta-share/meta-share/LanguageResource"/>
                    <rdf:Description rdf:about="http://w3id.org/meta-share/meta-share/Project"/>
                </owl:unionOf>
            </owl:Class>
        </rdfs:domain>
        <rdfs:range rdf:resource="http://w3id.org/meta-share/meta-share/Document"/>
        <rdfs:comment xml:lang="en">Links to a document that is somehow related to the entity that is described</rdfs:comment>
        <rdfs:label xml:lang="en">is related to document</rdfs:label>
    </owl:ObjectProperty>
    


    <!-- http://w3id.org/meta-share/meta-share/isRelatedToLR -->

    <owl:ObjectProperty rdf:about="http://w3id.org/meta-share/meta-share/isRelatedToLR">
        <rdfs:subPropertyOf rdf:resource="http://w3id.org/meta-share/meta-share/isRelatedTo"/>
        <rdfs:domain>
            <owl:Class>
                <owl:unionOf rdf:parseType="Collection">
                    <rdf:Description rdf:about="http://w3id.org/meta-share/meta-share/Division"/>
                    <rdf:Description rdf:about="http://w3id.org/meta-share/meta-share/Document"/>
                    <rdf:Description rdf:about="http://w3id.org/meta-share/meta-share/Group"/>
                    <rdf:Description rdf:about="http://w3id.org/meta-share/meta-share/LanguageResource"/>
                    <rdf:Description rdf:about="http://w3id.org/meta-share/meta-share/Organization"/>
                    <rdf:Description rdf:about="http://w3id.org/meta-share/meta-share/Person"/>
                    <rdf:Description rdf:about="http://w3id.org/meta-share/meta-share/Project"/>
                </owl:unionOf>
            </owl:Class>
        </rdfs:domain>
        <rdfs:range rdf:resource="http://w3id.org/meta-share/meta-share/LanguageResource"/>
        <rdfs:comment xml:lang="en">Links to a language resource that is related in any way to the entity being described</rdfs:comment>
        <rdfs:label xml:lang="en">is related to Language Resource</rdfs:label>
    </owl:ObjectProperty>
    


    <!-- http://w3id.org/meta-share/meta-share/isRelatedToLT -->

    <owl:ObjectProperty rdf:about="http://w3id.org/meta-share/meta-share/isRelatedToLT">
        <rdfs:subPropertyOf rdf:resource="http://w3id.org/meta-share/meta-share/isRelatedTo"/>
        <rdfs:domain rdf:resource="http://w3id.org/meta-share/meta-share/DataLanguageResource"/>
        <rdfs:range rdf:resource="http://w3id.org/meta-share/meta-share/ToolService"/>
        <rdfs:comment xml:lang="en">Links to a tool/service B that bears some relation to LR A (the one being described)</rdfs:comment>
        <rdfs:label xml:lang="en">is related to LT tool/service</rdfs:label>
    </owl:ObjectProperty>
    


    <!-- http://w3id.org/meta-share/meta-share/isRelatedToMDRecord -->

    <owl:ObjectProperty rdf:about="http://w3id.org/meta-share/meta-share/isRelatedToMDRecord">
        <rdfs:subPropertyOf rdf:resource="http://w3id.org/meta-share/meta-share/isRelatedTo"/>
        <rdfs:domain>
            <owl:Class>
                <owl:unionOf rdf:parseType="Collection">
                    <rdf:Description rdf:about="http://w3id.org/meta-share/meta-share/LanguageResource"/>
                    <rdf:Description rdf:about="http://w3id.org/meta-share/meta-share/MetadataRecord"/>
                </owl:unionOf>
            </owl:Class>
        </rdfs:domain>
        <rdfs:range rdf:resource="http://w3id.org/meta-share/meta-share/MetadataRecord"/>
        <rdfs:comment xml:lang="en">Links to an external metadata record that has some relation with the metadata record of the resource being described or the resource itself</rdfs:comment>
        <rdfs:label xml:lang="en">is related to metadata record</rdfs:label>
    </owl:ObjectProperty>
    


    <!-- http://w3id.org/meta-share/meta-share/isRelatedToProject -->

    <owl:ObjectProperty rdf:about="http://w3id.org/meta-share/meta-share/isRelatedToProject">
        <rdfs:subPropertyOf rdf:resource="http://w3id.org/meta-share/meta-share/isRelatedTo"/>
        <owl:inverseOf rdf:resource="http://w3id.org/meta-share/meta-share/projectRelatedTo"/>
        <rdfs:domain rdf:resource="http://w3id.org/meta-share/meta-share/LanguageResource"/>
        <rdfs:range rdf:resource="http://w3id.org/meta-share/meta-share/Project"/>
        <rdfs:comment xml:lang="en">Links to a project that has some relation with the language resource that is described (e.g.,  has funded its creation)</rdfs:comment>
        <rdfs:label xml:lang="en">is related to project</rdfs:label>
    </owl:ObjectProperty>
    


    <!-- http://w3id.org/meta-share/meta-share/isReplacedWith -->

    <owl:ObjectProperty rdf:about="http://w3id.org/meta-share/meta-share/isReplacedWith">
        <rdfs:subPropertyOf rdf:resource="http://w3id.org/meta-share/meta-share/hasVersion"/>
        <owl:inverseOf rdf:resource="http://w3id.org/meta-share/meta-share/replaces"/>
        <rdfs:domain rdf:resource="http://w3id.org/meta-share/meta-share/LanguageResource"/>
        <rdfs:range rdf:resource="http://w3id.org/meta-share/meta-share/LanguageResource"/>
        <rdfs:comment xml:lang="en">Links to LR B that is a newer version of LR A (the one being described) and replaces it</rdfs:comment>
        <rdfs:label xml:lang="en">is replaced with</rdfs:label>
    </owl:ObjectProperty>
    


    <!-- http://w3id.org/meta-share/meta-share/isRequiredLRBy -->

    <owl:ObjectProperty rdf:about="http://w3id.org/meta-share/meta-share/isRequiredLRBy">
        <rdfs:subPropertyOf rdf:resource="http://w3id.org/meta-share/meta-share/dependentLR"/>
        <owl:inverseOf rdf:resource="http://w3id.org/meta-share/meta-share/requiresLR"/>
        <rdfs:domain>
            <owl:Class>
                <owl:unionOf rdf:parseType="Collection">
                    <rdf:Description rdf:about="http://w3id.org/meta-share/meta-share/LanguageDescription"/>
                    <rdf:Description rdf:about="http://w3id.org/meta-share/meta-share/LexicalConceptualResource"/>
                </owl:unionOf>
            </owl:Class>
        </rdfs:domain>
        <rdfs:range>
            <owl:Class>
                <owl:unionOf rdf:parseType="Collection">
                    <rdf:Description rdf:about="http://w3id.org/meta-share/meta-share/LanguageDescription"/>
                    <rdf:Description rdf:about="http://w3id.org/meta-share/meta-share/ProcessingResource"/>
                    <rdf:Description rdf:about="http://w3id.org/meta-share/meta-share/ToolService"/>
                </owl:unionOf>
            </owl:Class>
        </rdfs:range>
        <rdfs:comment xml:lang="en">Links to a language resource that is required for the operation of a tool/service or computational grammar</rdfs:comment>
        <rdfs:label xml:lang="en">is required language resource by</rdfs:label>
    </owl:ObjectProperty>
    


    <!-- http://w3id.org/meta-share/meta-share/isResourceCreatorOf -->

    <owl:ObjectProperty rdf:about="http://w3id.org/meta-share/meta-share/isResourceCreatorOf">
        <rdfs:subPropertyOf rdf:resource="http://w3id.org/meta-share/meta-share/actorRelatedTo"/>
        <owl:inverseOf rdf:resource="http://w3id.org/meta-share/meta-share/resourceCreator"/>
        <rdfs:domain rdf:resource="http://w3id.org/meta-share/meta-share/Actor"/>
        <rdfs:range rdf:resource="http://w3id.org/meta-share/meta-share/LanguageResource"/>
        <rdfs:comment xml:lang="en">Links to the language resource(s) that a person/organization has created</rdfs:comment>
        <rdfs:label xml:lang="en">is resource creator of</rdfs:label>
    </owl:ObjectProperty>
    


    <!-- http://w3id.org/meta-share/meta-share/isResourceProviderOf -->

    <owl:ObjectProperty rdf:about="http://w3id.org/meta-share/meta-share/isResourceProviderOf">
        <rdfs:subPropertyOf rdf:resource="http://w3id.org/meta-share/meta-share/actorRelatedTo"/>
        <owl:inverseOf rdf:resource="http://w3id.org/meta-share/meta-share/resourceProvider"/>
        <rdfs:domain rdf:resource="http://w3id.org/meta-share/meta-share/Actor"/>
        <rdfs:range rdf:resource="http://w3id.org/meta-share/meta-share/LanguageResource"/>
        <rdfs:comment xml:lang="en">Links to a resource for which the person/organization is responsible of providing, curating and maintaining</rdfs:comment>
        <rdfs:label xml:lang="en">is resource provider of</rdfs:label>
    </owl:ObjectProperty>
    


    <!-- http://w3id.org/meta-share/meta-share/isReviewedBy -->

    <owl:ObjectProperty rdf:about="http://w3id.org/meta-share/meta-share/isReviewedBy">
        <rdfs:subPropertyOf rdf:resource="http://w3id.org/meta-share/meta-share/isDocumentedBy"/>
        <owl:inverseOf rdf:resource="http://w3id.org/meta-share/meta-share/reviews"/>
        <rdfs:domain rdf:resource="http://w3id.org/meta-share/meta-share/LanguageResource"/>
        <rdfs:range rdf:resource="http://w3id.org/meta-share/meta-share/Document"/>
        <rdfs:altLabel xml:lang="en">review</rdfs:altLabel>
        <rdfs:comment xml:lang="en">Links to a document that contains the review of LR A (the one being described)</rdfs:comment>
        <rdfs:label xml:lang="en">is reviewed by</rdfs:label>
    </owl:ObjectProperty>
    


    <!-- http://w3id.org/meta-share/meta-share/isSimilarTo -->

    <owl:ObjectProperty rdf:about="http://w3id.org/meta-share/meta-share/isSimilarTo">
        <rdfs:subPropertyOf rdf:resource="http://w3id.org/meta-share/meta-share/isRelatedToLR"/>
        <rdf:type rdf:resource="http://www.w3.org/2002/07/owl#SymmetricProperty"/>
        <rdfs:domain rdf:resource="http://w3id.org/meta-share/meta-share/LanguageResource"/>
        <rdfs:range rdf:resource="http://w3id.org/meta-share/meta-share/LanguageResource"/>
        <rdfs:altLabel xml:lang="en">is similar with</rdfs:altLabel>
        <rdfs:comment xml:lang="en">Links to LR B that bears resemblances to LR A (the one being described), e.g.,  they have been built with the same theoretical principles or are the same with different formats or processed at the same level with different tools</rdfs:comment>
        <rdfs:label xml:lang="en">is similar to</rdfs:label>
    </owl:ObjectProperty>
    


    <!-- http://w3id.org/meta-share/meta-share/isTypesystemOf -->

    <owl:ObjectProperty rdf:about="http://w3id.org/meta-share/meta-share/isTypesystemOf">
        <rdfs:subPropertyOf rdf:resource="http://w3id.org/meta-share/meta-share/dependentLR"/>
        <owl:inverseOf rdf:resource="http://w3id.org/meta-share/meta-share/typesystem"/>
        <rdfs:domain rdf:resource="http://w3id.org/meta-share/meta-share/LexicalConceptualResource"/>
        <rdfs:range>
            <owl:Class>
                <owl:unionOf rdf:parseType="Collection">
                    <rdf:Description rdf:about="http://w3id.org/meta-share/meta-share/MLModel"/>
                    <rdf:Description rdf:about="http://w3id.org/meta-share/meta-share/ProcessingResource"/>
                    <rdf:Description rdf:about="http://w3id.org/meta-share/meta-share/ToolService"/>
                </owl:unionOf>
            </owl:Class>
        </rdfs:range>
        <rdfs:comment xml:lang="en">Links a typesystem to the corpus where it has been used for annotating or to data of an annotation tool/service that has been or can be combined with</rdfs:comment>
        <rdfs:label xml:lang="en">is typesystem of</rdfs:label>
    </owl:ObjectProperty>
    


    <!-- http://w3id.org/meta-share/meta-share/isUsageProjectOf -->

    <owl:ObjectProperty rdf:about="http://w3id.org/meta-share/meta-share/isUsageProjectOf">
        <rdfs:subPropertyOf rdf:resource="http://w3id.org/meta-share/meta-share/projectRelatedTo"/>
        <owl:inverseOf rdf:resource="http://w3id.org/meta-share/meta-share/usageProject"/>
        <rdfs:domain rdf:resource="http://w3id.org/meta-share/meta-share/Project"/>
        <rdfs:range rdf:resource="http://w3id.org/meta-share/meta-share/ActualUse"/>
        <rdfs:comment xml:lang="en">Links a project where a language resource has been used to this LR</rdfs:comment>
        <rdfs:label xml:lang="en">is usage project of</rdfs:label>
    </owl:ObjectProperty>
    


    <!-- http://w3id.org/meta-share/meta-share/isValidatedBy -->

    <owl:ObjectProperty rdf:about="http://w3id.org/meta-share/meta-share/isValidatedBy">
        <rdfs:subPropertyOf rdf:resource="http://w3id.org/meta-share/meta-share/isRelatedToLT"/>
        <rdfs:domain rdf:resource="http://w3id.org/meta-share/meta-share/Validation"/>
        <rdfs:range rdf:resource="http://w3id.org/meta-share/meta-share/ToolService"/>
        <rdfs:altLabel xml:lang="en">validation tool</rdfs:altLabel>
        <rdfs:comment xml:lang="en">Links to a tool/service B that is (or can be) used for validating LR A (the one being described)</rdfs:comment>
        <rdfs:label xml:lang="en">is validated by</rdfs:label>
    </owl:ObjectProperty>
    


    <!-- http://w3id.org/meta-share/meta-share/isValidatorOf -->

    <owl:ObjectProperty rdf:about="http://w3id.org/meta-share/meta-share/isValidatorOf">
        <rdfs:subPropertyOf rdf:resource="http://w3id.org/meta-share/meta-share/actorRelatedTo"/>
        <owl:inverseOf rdf:resource="http://w3id.org/meta-share/meta-share/validator"/>
        <rdfs:domain rdf:resource="http://w3id.org/meta-share/meta-share/Actor"/>
        <rdfs:range rdf:resource="http://w3id.org/meta-share/meta-share/Validation"/>
        <rdfs:comment xml:lang="en">Links person(s), group(s) or organization(s) that have performed a specific validation of a language resource to the data of this validation</rdfs:comment>
        <rdfs:label xml:lang="en">is validator of</rdfs:label>
    </owl:ObjectProperty>
    


    <!-- http://w3id.org/meta-share/meta-share/isVersionOf -->

    <owl:ObjectProperty rdf:about="http://w3id.org/meta-share/meta-share/isVersionOf">
        <rdfs:subPropertyOf rdf:resource="http://w3id.org/meta-share/meta-share/isRelatedToLR"/>
        <rdfs:domain rdf:resource="http://w3id.org/meta-share/meta-share/LanguageResource"/>
        <rdfs:range rdf:resource="http://w3id.org/meta-share/meta-share/LanguageResource"/>
        <rdfs:comment xml:lang="en">Links to LR B that is a version (corrected, annotated, enriched, processed, etc.) of LR A (the one being described)</rdfs:comment>
        <rdfs:label xml:lang="en">is version of</rdfs:label>
    </owl:ObjectProperty>
    


    <!-- http://w3id.org/meta-share/meta-share/languageVariety -->

    <owl:ObjectProperty rdf:about="http://w3id.org/meta-share/meta-share/languageVariety">
        <rdfs:domain>
            <owl:Class>
                <owl:unionOf rdf:parseType="Collection">
                    <rdf:Description rdf:about="http://w3id.org/meta-share/meta-share/CorpusAudioPart"/>
                    <rdf:Description rdf:about="http://w3id.org/meta-share/meta-share/CorpusImagePart"/>
                    <rdf:Description rdf:about="http://w3id.org/meta-share/meta-share/CorpusTextPart"/>
                    <rdf:Description rdf:about="http://w3id.org/meta-share/meta-share/CorpusVideoPart"/>
                    <rdf:Description rdf:about="http://w3id.org/meta-share/meta-share/LanguageDescriptionImagePart"/>
                    <rdf:Description rdf:about="http://w3id.org/meta-share/meta-share/LanguageDescriptionTextPart"/>
                    <rdf:Description rdf:about="http://w3id.org/meta-share/meta-share/LanguageDescriptionVideoPart"/>
                    <rdf:Description rdf:about="http://w3id.org/meta-share/meta-share/LexicalConceptualResourceAudioPart"/>
                    <rdf:Description rdf:about="http://w3id.org/meta-share/meta-share/LexicalConceptualResourceImagePart"/>
                    <rdf:Description rdf:about="http://w3id.org/meta-share/meta-share/LexicalConceptualResourceTextPart"/>
                    <rdf:Description rdf:about="http://w3id.org/meta-share/meta-share/LexicalConceptualResourceVideoPart"/>
                </owl:unionOf>
            </owl:Class>
        </rdfs:domain>
        <rdfs:range rdf:resource="http://w3id.org/meta-share/meta-share/LanguageVariety"/>
        <rdfs:comment xml:lang="en">Relates a language resource that contains segments in a language variety (e.g.,  dialect, jargon) to it</rdfs:comment>
        <rdfs:label xml:lang="en">language variety</rdfs:label>
        <skos:note xml:lang="en">in MS we have language variety attached to language; check if this is ok; introduce a class Language after deciding on how to treat languages</skos:note>
    </owl:ObjectProperty>
    


    <!-- http://w3id.org/meta-share/meta-share/languageVarietyType -->

    <owl:ObjectProperty rdf:about="http://w3id.org/meta-share/meta-share/languageVarietyType">
        <rdfs:domain rdf:resource="http://w3id.org/meta-share/meta-share/LanguageVariety"/>
        <rdfs:range rdf:resource="http://w3id.org/meta-share/meta-share/LanguageVarietyType"/>
        <rdfs:comment xml:lang="en">Specifies the type of the language variety</rdfs:comment>
        <rdfs:label xml:lang="en">language variety type</rdfs:label>
    </owl:ObjectProperty>
    


    <!-- http://w3id.org/meta-share/meta-share/lcrSubclass -->

    <owl:ObjectProperty rdf:about="http://w3id.org/meta-share/meta-share/lcrSubclass">
        <rdfs:domain rdf:resource="http://w3id.org/meta-share/meta-share/LexicalConceptualResource"/>
        <rdfs:range rdf:resource="http://w3id.org/meta-share/meta-share/LCRSubclass"/>
        <rdfs:comment xml:lang="en">Introduces a classification of lexical/conceptual resources into types (used for descriptive reasons)</rdfs:comment>
        <rdfs:label xml:lang="en">lcr subclass</rdfs:label>
    </owl:ObjectProperty>
    


    <!-- http://w3id.org/meta-share/meta-share/ldTask -->

    <owl:ObjectProperty rdf:about="http://w3id.org/meta-share/meta-share/ldTask">
        <rdfs:domain rdf:resource="http://w3id.org/meta-share/meta-share/LanguageDescription"/>
        <rdfs:range rdf:resource="http://w3id.org/meta-share/meta-share/LDTask"/>
        <rdfs:comment xml:lang="en">Specifies the task performed by the language description</rdfs:comment>
        <rdfs:label xml:lang="en">language description task</rdfs:label>
    </owl:ObjectProperty>
    


    <!-- http://w3id.org/meta-share/meta-share/licenceCategory -->

    <owl:ObjectProperty rdf:about="http://w3id.org/meta-share/meta-share/licenceCategory">
        <rdfs:domain rdf:resource="http://w3id.org/meta-share/meta-share/LicenceTerms"/>
        <rdfs:range rdf:resource="http://w3id.org/meta-share/meta-share/LicenceCategory"/>
        <rdfs:comment xml:lang="en">Categorises a licence according to a classification scheme</rdfs:comment>
        <rdfs:label xml:lang="en">licence category</rdfs:label>
    </owl:ObjectProperty>
    


    <!-- http://w3id.org/meta-share/meta-share/licenceTerms -->

    <owl:ObjectProperty rdf:about="http://w3id.org/meta-share/meta-share/licenceTerms">
        <rdfs:subPropertyOf rdf:resource="http://purl.org/dc/terms/license"/>
        <rdfs:domain rdf:resource="http://w3id.org/meta-share/meta-share/Distribution"/>
        <rdfs:range rdf:resource="http://w3id.org/meta-share/meta-share/LicenceTerms"/>
        <rdfs:comment xml:lang="en">Links the distribution (distributable form) of a language resource to the licence or terms of use/service (a specific legal document) with which it is distributed</rdfs:comment>
        <rdfs:label xml:lang="en">licence/terms of use/service</rdfs:label>
    </owl:ObjectProperty>
    


    <!-- http://w3id.org/meta-share/meta-share/licensor -->

    <owl:ObjectProperty rdf:about="http://w3id.org/meta-share/meta-share/licensor">
        <rdfs:subPropertyOf rdf:resource="http://w3id.org/meta-share/meta-share/isRelatedToActor"/>
        <rdfs:domain rdf:resource="http://w3id.org/meta-share/meta-share/Distribution"/>
        <rdfs:range rdf:resource="http://w3id.org/meta-share/meta-share/Person"/>
        <rdfs:comment xml:lang="en">The person or organisation who is legally eligible to license and actually licenses the resource. The licensor could be different from the creator, the distributor or the IPR holder. The licensor has the necessary rights or licences to license the work and is the party that actually licenses the resource that is distributed via the specific channel. She will have obtained the necessary rights or licences from the IPR holder and she may have a distribution agreement with a distributor that disseminates the work under a set of conditions defined in the specific  licence and collects revenue on the licensor&apos;s behalf. The attribution of the creator, separately from the attribution of the licensor, may be part of the licence under which the resource is distributed (as e.g.,  is the case with Creative Commons Licences).</rdfs:comment>
        <rdfs:label xml:lang="en">licensor</rdfs:label>
    </owl:ObjectProperty>
    


    <!-- http://w3id.org/meta-share/meta-share/lingualityType -->

    <owl:ObjectProperty rdf:about="http://w3id.org/meta-share/meta-share/lingualityType">
        <rdfs:domain rdf:resource="http://w3id.org/meta-share/meta-share/MediaPart"/>
        <rdfs:range rdf:resource="http://w3id.org/meta-share/meta-share/LingualityType"/>
        <rdfs:comment xml:lang="en">Indicates whether the resource includes one, two or more languages</rdfs:comment>
        <rdfs:label xml:lang="en">linguality type</rdfs:label>
    </owl:ObjectProperty>
    


    <!-- http://w3id.org/meta-share/meta-share/linguisticInformation -->

    <owl:ObjectProperty rdf:about="http://w3id.org/meta-share/meta-share/linguisticInformation">
        <rdfs:domain rdf:resource="http://w3id.org/meta-share/meta-share/LexicalConceptualResource"/>
        <rdfs:range rdf:resource="http://w3id.org/meta-share/meta-share/ContentType"/>
        <rdfs:comment xml:lang="en">Provides a more detailed account of the linguistic information contained in the lexical/conceptual resource</rdfs:comment>
        <rdfs:label xml:lang="en">linguistic information</rdfs:label>
    </owl:ObjectProperty>
    


    <!-- http://w3id.org/meta-share/meta-share/linkToOtherMedia -->

    <owl:ObjectProperty rdf:about="http://w3id.org/meta-share/meta-share/linkToOtherMedia">
        <rdfs:domain>
            <owl:Class>
                <owl:unionOf rdf:parseType="Collection">
                    <rdf:Description rdf:about="http://w3id.org/meta-share/meta-share/CorpusMediaPart"/>
                    <rdf:Description rdf:about="http://w3id.org/meta-share/meta-share/LanguageDescriptionMediaPart"/>
                </owl:unionOf>
            </owl:Class>
        </rdfs:domain>
        <rdfs:range rdf:resource="http://w3id.org/meta-share/meta-share/LinkToOtherMedia"/>
        <rdfs:comment xml:lang="en">Describes the linking between different media parts of a resource (how they interact with or link to each other)</rdfs:comment>
        <rdfs:label xml:lang="en">link to other media</rdfs:label>
    </owl:ObjectProperty>
    


    <!-- http://w3id.org/meta-share/meta-share/mediaPart -->

    <owl:ObjectProperty rdf:about="http://w3id.org/meta-share/meta-share/mediaPart">
        <rdfs:domain rdf:resource="http://w3id.org/meta-share/meta-share/LanguageResource"/>
        <rdfs:range rdf:resource="http://w3id.org/meta-share/meta-share/MediaPart"/>
        <rdfs:comment xml:lang="en">Links a language resource to the parts it consists of (e.g.,  an oral corpus with the audio and its transcribed text part)</rdfs:comment>
        <rdfs:label xml:lang="en">media part</rdfs:label>
    </owl:ObjectProperty>
    


    <!-- http://w3id.org/meta-share/meta-share/mediaType -->

    <owl:ObjectProperty rdf:about="http://w3id.org/meta-share/meta-share/mediaType">
        <rdfs:domain>
            <owl:Class>
                <owl:unionOf rdf:parseType="Collection">
                    <rdf:Description rdf:about="http://w3id.org/meta-share/meta-share/MediaPart"/>
                    <rdf:Description rdf:about="http://w3id.org/meta-share/meta-share/ProcessingResourceType"/>
                </owl:unionOf>
            </owl:Class>
        </rdfs:domain>
        <rdfs:range rdf:resource="http://w3id.org/meta-share/meta-share/MediaType"/>
        <rdfs:comment xml:lang="en">Specifies the media type of a language resource (the physical medium of the contents representation) or of the input/output of a language processing tool/service; each media type is described through a distinctive set of technical features; a language resource may consist of different media parts</rdfs:comment>
        <rdfs:label xml:lang="en">media type</rdfs:label>
    </owl:ObjectProperty>
    


    <!-- http://w3id.org/meta-share/meta-share/memberOfAssociation -->

    <owl:ObjectProperty rdf:about="http://w3id.org/meta-share/meta-share/memberOfAssociation">
        <rdfs:domain>
            <owl:Class>
                <owl:unionOf rdf:parseType="Collection">
                    <rdf:Description rdf:about="http://w3id.org/meta-share/meta-share/Division"/>
                    <rdf:Description rdf:about="http://w3id.org/meta-share/meta-share/Organization"/>
                    <rdf:Description rdf:about="http://w3id.org/meta-share/meta-share/Person"/>
                </owl:unionOf>
            </owl:Class>
        </rdfs:domain>
        <rdfs:range rdf:resource="http://w3id.org/meta-share/meta-share/Organization"/>
        <rdfs:comment xml:lang="en">Links to an association or network that the organization or person is member of</rdfs:comment>
        <rdfs:label xml:lang="en">member of association</rdfs:label>
    </owl:ObjectProperty>
    


    <!-- http://w3id.org/meta-share/meta-share/membershipInstitution -->

    <owl:ObjectProperty rdf:about="http://w3id.org/meta-share/meta-share/membershipInstitution">
        <rdfs:domain rdf:resource="http://w3id.org/meta-share/meta-share/Distribution"/>
        <rdfs:range rdf:resource="http://w3id.org/meta-share/meta-share/MembershipInstitution"/>
        <rdfs:comment xml:lang="en">Introduces an institution with members that can benefit from specific conditions on the use of a resource (e.g. discount, unlimited access, etc.)</rdfs:comment>
        <rdfs:label xml:lang="en">membership institution</rdfs:label>
    </owl:ObjectProperty>
    


    <!-- http://w3id.org/meta-share/meta-share/metadataCreator -->

    <owl:ObjectProperty rdf:about="http://w3id.org/meta-share/meta-share/metadataCreator">
        <rdfs:subPropertyOf rdf:resource="http://w3id.org/meta-share/meta-share/isRelatedToActor"/>
        <rdfs:domain rdf:resource="http://w3id.org/meta-share/meta-share/MetadataRecord"/>
        <rdfs:range rdf:resource="http://w3id.org/meta-share/meta-share/Person"/>
        <rdfs:comment xml:lang="en">Introduces the person who has created the metadata record</rdfs:comment>
        <rdfs:label xml:lang="en">metadata creator</rdfs:label>
    </owl:ObjectProperty>
    


    <!-- http://w3id.org/meta-share/meta-share/metadataCurator -->

    <owl:ObjectProperty rdf:about="http://w3id.org/meta-share/meta-share/metadataCurator">
        <rdfs:subPropertyOf rdf:resource="http://w3id.org/meta-share/meta-share/isRelatedToActor"/>
        <rdfs:domain rdf:resource="http://w3id.org/meta-share/meta-share/MetadataRecord"/>
        <rdfs:range rdf:resource="http://w3id.org/meta-share/meta-share/Person"/>
        <rdfs:comment xml:lang="en">A person responsible for the creation, update, enrichment, etc. of a metadata record describing an entity</rdfs:comment>
        <rdfs:label xml:lang="en">metadata curator</rdfs:label>
    </owl:ObjectProperty>
    


    <!-- http://w3id.org/meta-share/meta-share/method -->

    <owl:ObjectProperty rdf:about="http://w3id.org/meta-share/meta-share/method">
        <rdfs:domain>
            <owl:Class>
                <owl:unionOf rdf:parseType="Collection">
                    <rdf:Description rdf:about="http://w3id.org/meta-share/meta-share/MLModel"/>
                    <rdf:Description rdf:about="http://w3id.org/meta-share/meta-share/ToolService"/>
                </owl:unionOf>
            </owl:Class>
        </rdfs:domain>
        <rdfs:range rdf:resource="http://w3id.org/meta-share/omtd-share/TdmMethod"/>
        <rdfs:comment xml:lang="en">Specifies the method used for the development of a tool/service or the ML model</rdfs:comment>
        <rdfs:label xml:lang="en">method</rdfs:label>
    </owl:ObjectProperty>
    


    <!-- http://w3id.org/meta-share/meta-share/metric -->

    <owl:ObjectProperty rdf:about="http://w3id.org/meta-share/meta-share/metric">
        <rdfs:domain rdf:resource="http://w3id.org/meta-share/meta-share/PerformanceIndicator"/>
        <rdfs:range rdf:resource="http://w3id.org/meta-share/meta-share/Metric"/>
        <rdfs:comment xml:lang="en">Identifies the metric used for the evaluation of the tool/service</rdfs:comment>
        <rdfs:label xml:lang="en">metric</rdfs:label>
    </owl:ObjectProperty>
    


    <!-- http://w3id.org/meta-share/meta-share/mlModel -->

    <owl:ObjectProperty rdf:about="http://w3id.org/meta-share/meta-share/mlModel">
        <rdfs:subPropertyOf rdf:resource="http://w3id.org/meta-share/meta-share/dependsOn"/>
        <rdfs:domain rdf:resource="http://w3id.org/meta-share/meta-share/ToolService"/>
        <rdfs:range rdf:resource="http://w3id.org/meta-share/meta-share/MLModel"/>
        <rdfs:comment xml:lang="en">Specifies the ML model that must be used together with the tool/service to perform the desired task</rdfs:comment>
        <rdfs:label xml:lang="en">ML model</rdfs:label>
    </owl:ObjectProperty>
    


    <!-- http://w3id.org/meta-share/meta-share/modalityType -->

    <owl:ObjectProperty rdf:about="http://w3id.org/meta-share/meta-share/modalityType">
        <rdfs:domain rdf:resource="http://w3id.org/meta-share/meta-share/MediaPart"/>
        <rdfs:range rdf:resource="http://w3id.org/meta-share/meta-share/ModalityType"/>
        <rdfs:comment xml:lang="en">Specifies the type of the modality represented in the resource or processed by a tool/service</rdfs:comment>
        <rdfs:label xml:lang="en">modality type</rdfs:label>
    </owl:ObjectProperty>
    


    <!-- http://w3id.org/meta-share/meta-share/multilingualityType -->

    <owl:ObjectProperty rdf:about="http://w3id.org/meta-share/meta-share/multilingualityType">
        <rdfs:domain rdf:resource="http://w3id.org/meta-share/meta-share/MediaPart"/>
        <rdfs:range rdf:resource="http://w3id.org/meta-share/meta-share/MultilingualityType"/>
        <rdfs:comment xml:lang="en">Indicates whether the resource (part) is parallel, comparable or mixed</rdfs:comment>
        <rdfs:label xml:lang="en">multilinguality type</rdfs:label>
    </owl:ObjectProperty>
    


    <!-- http://w3id.org/meta-share/meta-share/nationalMaxContribution -->

    <owl:ObjectProperty rdf:about="http://w3id.org/meta-share/meta-share/nationalMaxContribution">
        <rdfs:domain rdf:resource="http://w3id.org/meta-share/meta-share/Project"/>
        <rdfs:range rdf:resource="http://w3id.org/meta-share/meta-share/Cost"/>
        <rdfs:comment xml:lang="en">Introduces the maximum amount of money contributed from national funds</rdfs:comment>
        <rdfs:label xml:lang="en">national max contribution</rdfs:label>
    </owl:ObjectProperty>
    


    <!-- http://w3id.org/meta-share/meta-share/naturality -->

    <owl:ObjectProperty rdf:about="http://w3id.org/meta-share/meta-share/naturality">
        <rdfs:domain>
            <owl:Class>
                <owl:unionOf rdf:parseType="Collection">
                    <rdf:Description rdf:about="http://w3id.org/meta-share/meta-share/CorpusAudioPart"/>
                    <rdf:Description rdf:about="http://w3id.org/meta-share/meta-share/CorpusVideoPart"/>
                </owl:unionOf>
            </owl:Class>
        </rdfs:domain>
        <rdfs:range rdf:resource="http://w3id.org/meta-share/meta-share/Naturality"/>
        <rdfs:comment xml:lang="en">Specifies the level of naturality for multimodal/multimedia resources</rdfs:comment>
        <rdfs:label xml:lang="en">naturality</rdfs:label>
    </owl:ObjectProperty>
    


    <!-- http://w3id.org/meta-share/meta-share/noiseLevel -->

    <owl:ObjectProperty rdf:about="http://w3id.org/meta-share/meta-share/noiseLevel">
        <rdfs:domain>
            <owl:Class>
                <owl:unionOf rdf:parseType="Collection">
                    <rdf:Description rdf:about="http://w3id.org/meta-share/meta-share/CorpusAudioPart"/>
                    <rdf:Description rdf:about="http://w3id.org/meta-share/meta-share/LexicalConceptualResourceAudioPart"/>
                </owl:unionOf>
            </owl:Class>
        </rdfs:domain>
        <rdfs:range rdf:resource="http://w3id.org/meta-share/meta-share/NoiseLevel"/>
        <rdfs:comment xml:lang="en">Specifies the  level of background noise</rdfs:comment>
        <rdfs:label xml:lang="en">noise level</rdfs:label>
    </owl:ObjectProperty>
    


    <!-- http://w3id.org/meta-share/meta-share/nonSpeechItem -->

    <owl:ObjectProperty rdf:about="http://w3id.org/meta-share/meta-share/nonSpeechItem">
        <rdfs:domain>
            <owl:Class>
                <owl:unionOf rdf:parseType="Collection">
                    <rdf:Description rdf:about="http://w3id.org/meta-share/meta-share/CorpusAudioPart"/>
                    <rdf:Description rdf:about="http://w3id.org/meta-share/meta-share/LexicalConceptualResourceAudioPart"/>
                </owl:unionOf>
            </owl:Class>
        </rdfs:domain>
        <rdfs:range rdf:resource="http://w3id.org/meta-share/meta-share/NonSpeechItem"/>
        <rdfs:comment xml:lang="en">Specifies the distinct non-speech elements that maybe included in the audio part of a corpus or lexical/conceptual resource</rdfs:comment>
        <rdfs:label xml:lang="en">non-speech item</rdfs:label>
    </owl:ObjectProperty>
    


    <!-- http://w3id.org/meta-share/meta-share/operatingSystem -->

    <owl:ObjectProperty rdf:about="http://w3id.org/meta-share/meta-share/operatingSystem">
        <rdfs:domain rdf:resource="http://w3id.org/meta-share/meta-share/ToolService"/>
        <rdfs:range rdf:resource="http://w3id.org/meta-share/meta-share/OperatingSystem"/>
        <rdfs:comment xml:lang="en">Specifies the operating system on which a software object can run</rdfs:comment>
        <rdfs:label xml:lang="en">operating system</rdfs:label>
    </owl:ObjectProperty>
    


    <!-- http://w3id.org/meta-share/meta-share/organizationLegalStatus -->

    <owl:ObjectProperty rdf:about="http://w3id.org/meta-share/meta-share/organizationLegalStatus">
        <rdfs:domain rdf:resource="http://w3id.org/meta-share/meta-share/Organization"/>
        <rdfs:range rdf:resource="http://w3id.org/meta-share/meta-share/OrganizationLegalStatus"/>
        <rdfs:comment xml:lang="en">Classifies an organization according to its legal status</rdfs:comment>
        <rdfs:label xml:lang="en">organization legal status</rdfs:label>
    </owl:ObjectProperty>
    


    <!-- http://w3id.org/meta-share/meta-share/organizationRole -->

    <owl:ObjectProperty rdf:about="http://w3id.org/meta-share/meta-share/organizationRole">
        <rdfs:domain>
            <owl:Class>
                <owl:unionOf rdf:parseType="Collection">
                    <rdf:Description rdf:about="http://w3id.org/meta-share/meta-share/Division"/>
                    <rdf:Description rdf:about="http://w3id.org/meta-share/meta-share/Group"/>
                    <rdf:Description rdf:about="http://w3id.org/meta-share/meta-share/Organization"/>
                </owl:unionOf>
            </owl:Class>
        </rdfs:domain>
        <rdfs:range rdf:resource="http://w3id.org/meta-share/meta-share/OrganizationRole"/>
        <rdfs:comment xml:lang="en">Classifies an organization according to its role/mission</rdfs:comment>
        <rdfs:label xml:lang="en">organization role</rdfs:label>
    </owl:ObjectProperty>
    


    <!-- http://w3id.org/meta-share/meta-share/origin -->

    <owl:ObjectProperty rdf:about="http://w3id.org/meta-share/meta-share/origin">
        <rdfs:domain rdf:resource="http://w3id.org/meta-share/meta-share/Participant"/>
        <rdfs:range rdf:resource="http://w3id.org/meta-share/meta-share/Origin"/>
        <rdfs:comment xml:lang="en">Specifies the relation of the language of a participant with respect to the acquisition stage</rdfs:comment>
        <rdfs:label xml:lang="en">origin</rdfs:label>
    </owl:ObjectProperty>
    


    <!-- http://w3id.org/meta-share/meta-share/originOfParticipants -->

    <owl:ObjectProperty rdf:about="http://w3id.org/meta-share/meta-share/originOfParticipants">
        <rdfs:domain>
            <owl:Class>
                <owl:unionOf rdf:parseType="Collection">
                    <rdf:Description rdf:about="http://w3id.org/meta-share/meta-share/CorpusAudioPart"/>
                    <rdf:Description rdf:about="http://w3id.org/meta-share/meta-share/CorpusImagePart"/>
                    <rdf:Description rdf:about="http://w3id.org/meta-share/meta-share/CorpusTextNumericalPart"/>
                    <rdf:Description rdf:about="http://w3id.org/meta-share/meta-share/CorpusVideoPart"/>
                </owl:unionOf>
            </owl:Class>
        </rdfs:domain>
        <rdfs:range rdf:resource="http://w3id.org/meta-share/meta-share/Origin"/>
        <rdfs:comment xml:lang="en">Specifies the relation of the language of the group of participants with respect to the acquisition stage</rdfs:comment>
        <rdfs:label xml:lang="en">origin of participants</rdfs:label>
    </owl:ObjectProperty>
    


    <!-- http://w3id.org/meta-share/meta-share/otherMedia -->

    <owl:ObjectProperty rdf:about="http://w3id.org/meta-share/meta-share/otherMedia">
        <rdfs:domain rdf:resource="http://w3id.org/meta-share/meta-share/LinkToOtherMedia"/>
        <rdfs:range rdf:resource="http://w3id.org/meta-share/meta-share/MediaType"/>
        <rdfs:comment xml:lang="en">Specifies the media types that are linked to the media type described within the same resource</rdfs:comment>
        <rdfs:label xml:lang="en">other media</rdfs:label>
    </owl:ObjectProperty>
    


    <!-- http://w3id.org/meta-share/meta-share/outputResource -->

    <owl:ObjectProperty rdf:about="http://w3id.org/meta-share/meta-share/outputResource">
        <rdfs:domain rdf:resource="http://w3id.org/meta-share/meta-share/ToolService"/>
        <rdfs:range rdf:resource="http://w3id.org/meta-share/meta-share/ProcessingResource"/>
        <rdfs:comment xml:lang="en">Specifies the output results of a tool/service, i.e. the features of the processed (content) resource</rdfs:comment>
        <rdfs:label xml:lang="en">output resource</rdfs:label>
    </owl:ObjectProperty>
    


    <!-- http://w3id.org/meta-share/meta-share/parameter -->

    <owl:ObjectProperty rdf:about="http://w3id.org/meta-share/meta-share/parameter">
        <rdfs:domain rdf:resource="http://w3id.org/meta-share/meta-share/ToolService"/>
        <rdfs:range rdf:resource="http://w3id.org/meta-share/meta-share/Parameter"/>
        <rdfs:comment xml:lang="en">Introduces a parameter used for running a tool/service</rdfs:comment>
        <rdfs:label xml:lang="en">parameter</rdfs:label>
    </owl:ObjectProperty>
    


    <!-- http://w3id.org/meta-share/meta-share/parameterType -->

    <owl:ObjectProperty rdf:about="http://w3id.org/meta-share/meta-share/parameterType">
        <rdfs:domain rdf:resource="http://w3id.org/meta-share/meta-share/Parameter"/>
        <rdfs:range rdf:resource="http://w3id.org/meta-share/meta-share/ParameterType"/>
        <rdfs:comment xml:lang="en">Classifies the parameter according to a specific (not yet standardised)  typing system (e.g.,  whether it&apos;s boolean, string, integer, a document, mapping, etc.)</rdfs:comment>
        <rdfs:label xml:lang="en">parameter type</rdfs:label>
    </owl:ObjectProperty>
    


    <!-- http://w3id.org/meta-share/meta-share/participant -->

    <owl:ObjectProperty rdf:about="http://w3id.org/meta-share/meta-share/participant">
        <rdfs:domain>
            <owl:Class>
                <owl:unionOf rdf:parseType="Collection">
                    <rdf:Description rdf:about="http://w3id.org/meta-share/meta-share/CorpusAudioPart"/>
                    <rdf:Description rdf:about="http://w3id.org/meta-share/meta-share/CorpusImagePart"/>
                    <rdf:Description rdf:about="http://w3id.org/meta-share/meta-share/CorpusTextNumericalPart"/>
                    <rdf:Description rdf:about="http://w3id.org/meta-share/meta-share/CorpusVideoPart"/>
                </owl:unionOf>
            </owl:Class>
        </rdfs:domain>
        <rdfs:range rdf:resource="http://w3id.org/meta-share/meta-share/Participant"/>
        <rdfs:comment xml:lang="en">Introduces descriptive characteristics of a person that has participated in the audio, video, sensorimotor (textNumerical) part of the resource</rdfs:comment>
        <rdfs:label xml:lang="en">participant</rdfs:label>
    </owl:ObjectProperty>
    


    <!-- http://w3id.org/meta-share/meta-share/participatingOrganization -->

    <owl:ObjectProperty rdf:about="http://w3id.org/meta-share/meta-share/participatingOrganization">
        <rdfs:subPropertyOf rdf:resource="http://w3id.org/meta-share/meta-share/isRelatedToActor"/>
        <rdfs:domain rdf:resource="http://w3id.org/meta-share/meta-share/Project"/>
        <rdfs:range rdf:resource="http://w3id.org/meta-share/meta-share/Organization"/>
        <rdfs:comment xml:lang="en">Indicates the organization(s) that participate (or have participated) in a project</rdfs:comment>
        <rdfs:label xml:lang="en">participating organization</rdfs:label>
    </owl:ObjectProperty>
    


    <!-- http://w3id.org/meta-share/meta-share/performanceIndicator -->

    <owl:ObjectProperty rdf:about="http://w3id.org/meta-share/meta-share/performanceIndicator">
        <rdfs:domain rdf:resource="http://w3id.org/meta-share/meta-share/Evaluation"/>
        <rdfs:range rdf:resource="http://w3id.org/meta-share/meta-share/PerformanceIndicator"/>
        <rdfs:comment xml:lang="en">Describes the performance indicator used for the evaluation of a tool/service</rdfs:comment>
        <rdfs:label xml:lang="en">performance indicator</rdfs:label>
    </owl:ObjectProperty>
    


    <!-- http://w3id.org/meta-share/meta-share/previousAnnotationTypesPolicy -->

    <owl:ObjectProperty rdf:about="http://w3id.org/meta-share/meta-share/previousAnnotationTypesPolicy">
        <rdfs:domain rdf:resource="http://w3id.org/meta-share/meta-share/ToolService"/>
        <rdfs:range rdf:resource="http://w3id.org/meta-share/meta-share/PreviousAnnotationTypesPolicy"/>
        <rdfs:comment xml:lang="en">Specifies the policy that a tool/service has with respect to the annotation types included in the annotated resource that it takes as input (i.e. whether it keeps, modifies or drops them in the output resource)</rdfs:comment>
        <rdfs:label xml:lang="en">previous annotation types policy</rdfs:label>
    </owl:ObjectProperty>
    


    <!-- http://w3id.org/meta-share/meta-share/processMode -->

    <owl:ObjectProperty rdf:about="http://w3id.org/meta-share/meta-share/processMode">
        <rdfs:domain rdf:resource="http://www.w3.org/2002/07/owl#Thing"/>
        <rdfs:range rdf:resource="http://w3id.org/meta-share/meta-share/ProcessMode"/>
        <rdfs:comment xml:lang="en">Specifies the type of processing performed on a language resource</rdfs:comment>
        <rdfs:label xml:lang="en">process mode</rdfs:label>
    </owl:ObjectProperty>
    


    <!-- http://w3id.org/meta-share/meta-share/processingResourceType -->

    <owl:ObjectProperty rdf:about="http://w3id.org/meta-share/meta-share/processingResourceType">
        <rdfs:domain rdf:resource="http://w3id.org/meta-share/meta-share/ProcessingResource"/>
        <rdfs:range rdf:resource="http://w3id.org/meta-share/meta-share/ProcessingResourceType"/>
        <rdfs:comment xml:lang="en">Specifies the resource type that a tool/service takes as input or produces as output</rdfs:comment>
        <rdfs:label xml:lang="en">processing resource  type</rdfs:label>
    </owl:ObjectProperty>
    


    <!-- http://w3id.org/meta-share/meta-share/projectRelatedTo -->

    <owl:ObjectProperty rdf:about="http://w3id.org/meta-share/meta-share/projectRelatedTo">
        <rdfs:subPropertyOf rdf:resource="http://w3id.org/meta-share/meta-share/isRelatedTo"/>
        <rdfs:domain rdf:resource="http://w3id.org/meta-share/meta-share/Project"/>
        <rdfs:range rdf:resource="http://w3id.org/meta-share/meta-share/LanguageResource"/>
        <rdfs:comment xml:lang="en">Links a project to the language resource(s) it has some relation with (e.g.,  funded the creation of)</rdfs:comment>
        <rdfs:label xml:lang="en">project related to</rdfs:label>
    </owl:ObjectProperty>
    


    <!-- http://w3id.org/meta-share/meta-share/quality -->

    <owl:ObjectProperty rdf:about="http://w3id.org/meta-share/meta-share/quality">
        <rdfs:domain rdf:resource="http://w3id.org/meta-share/meta-share/ImageFormat"/>
        <rdfs:range rdf:resource="http://w3id.org/meta-share/meta-share/Quality"/>
        <rdfs:comment xml:lang="en">Specifies the quality level of image resource</rdfs:comment>
        <rdfs:label xml:lang="en">quality</rdfs:label>
    </owl:ObjectProperty>
    


    <!-- http://w3id.org/meta-share/meta-share/queries -->

    <owl:ObjectProperty rdf:about="http://w3id.org/meta-share/meta-share/queries">
        <rdfs:subPropertyOf rdf:resource="http://w3id.org/meta-share/meta-share/LΤRelatedTo"/>
        <rdfs:domain rdf:resource="http://w3id.org/meta-share/meta-share/ToolService"/>
        <rdfs:range rdf:resource="http://w3id.org/meta-share/meta-share/DataLanguageResource"/>
        <rdfs:comment xml:lang="en">Links a tool/service B that is (or can be) used for querying LR A to LR A</rdfs:comment>
        <rdfs:label xml:lang="en">queries</rdfs:label>
    </owl:ObjectProperty>
    


    <!-- http://w3id.org/meta-share/meta-share/rasterOrVectorGraphics -->

    <owl:ObjectProperty rdf:about="http://w3id.org/meta-share/meta-share/rasterOrVectorGraphics">
        <rdfs:domain rdf:resource="http://w3id.org/meta-share/meta-share/ImageFormat"/>
        <rdfs:range rdf:resource="http://w3id.org/meta-share/meta-share/RasterOrVectorGraphics"/>
        <rdfs:comment xml:lang="en">Indicates if the image is stored as raster or vector graphics</rdfs:comment>
        <rdfs:label xml:lang="en">raster or vector graphics</rdfs:label>
    </owl:ObjectProperty>
    


    <!-- http://w3id.org/meta-share/meta-share/recorder -->

    <owl:ObjectProperty rdf:about="http://w3id.org/meta-share/meta-share/recorder">
        <rdfs:subPropertyOf rdf:resource="http://w3id.org/meta-share/meta-share/isRelatedToActor"/>
        <rdfs:domain>
            <owl:Class>
                <owl:unionOf rdf:parseType="Collection">
                    <rdf:Description rdf:about="http://w3id.org/meta-share/meta-share/CorpusAudioPart"/>
                    <rdf:Description rdf:about="http://w3id.org/meta-share/meta-share/CorpusTextNumericalPart"/>
                    <rdf:Description rdf:about="http://w3id.org/meta-share/meta-share/CorpusVideoPart"/>
                </owl:unionOf>
            </owl:Class>
        </rdfs:domain>
        <rdfs:range rdf:resource="http://w3id.org/meta-share/meta-share/Actor"/>
        <rdfs:comment xml:lang="en">Links to the recorder(s) of the audio or video part of the resource</rdfs:comment>
        <rdfs:label xml:lang="en">recorder</rdfs:label>
    </owl:ObjectProperty>
    


    <!-- http://w3id.org/meta-share/meta-share/recordingDeviceType -->

    <owl:ObjectProperty rdf:about="http://w3id.org/meta-share/meta-share/recordingDeviceType">
        <rdfs:domain>
            <owl:Class>
                <owl:unionOf rdf:parseType="Collection">
                    <rdf:Description rdf:about="http://w3id.org/meta-share/meta-share/CorpusAudioPart"/>
                    <rdf:Description rdf:about="http://w3id.org/meta-share/meta-share/CorpusTextNumericalPart"/>
                    <rdf:Description rdf:about="http://w3id.org/meta-share/meta-share/CorpusVideoPart"/>
                </owl:unionOf>
            </owl:Class>
        </rdfs:domain>
        <rdfs:range rdf:resource="http://w3id.org/meta-share/meta-share/RecordingDeviceType"/>
        <rdfs:comment xml:lang="en">Specifies the nature of the recording platform hardware and the storage medium</rdfs:comment>
        <rdfs:label xml:lang="en">recording device type</rdfs:label>
    </owl:ObjectProperty>
    


    <!-- http://w3id.org/meta-share/meta-share/recordingEnvironment -->

    <owl:ObjectProperty rdf:about="http://w3id.org/meta-share/meta-share/recordingEnvironment">
        <rdfs:domain>
            <owl:Class>
                <owl:unionOf rdf:parseType="Collection">
                    <rdf:Description rdf:about="http://w3id.org/meta-share/meta-share/CorpusAudioPart"/>
                    <rdf:Description rdf:about="http://w3id.org/meta-share/meta-share/CorpusTextNumericalPart"/>
                    <rdf:Description rdf:about="http://w3id.org/meta-share/meta-share/CorpusVideoPart"/>
                </owl:unionOf>
            </owl:Class>
        </rdfs:domain>
        <rdfs:range rdf:resource="http://w3id.org/meta-share/meta-share/RecordingEnvironment"/>
        <rdfs:comment xml:lang="en">Specifies where the recording took place</rdfs:comment>
        <rdfs:label xml:lang="en">recording environment</rdfs:label>
    </owl:ObjectProperty>
    


    <!-- http://w3id.org/meta-share/meta-share/recordingQuality -->

    <owl:ObjectProperty rdf:about="http://w3id.org/meta-share/meta-share/recordingQuality">
        <rdfs:domain rdf:resource="http://w3id.org/meta-share/meta-share/AudioFormat"/>
        <rdfs:range rdf:resource="http://w3id.org/meta-share/meta-share/RecordingQuality"/>
        <rdfs:comment xml:lang="en">Indicates the audio or video recording quality</rdfs:comment>
        <rdfs:label xml:lang="en">recording quality</rdfs:label>
    </owl:ObjectProperty>
    


    <!-- http://w3id.org/meta-share/meta-share/relatedLR -->

    <owl:ObjectProperty rdf:about="http://w3id.org/meta-share/meta-share/relatedLR">
        <rdfs:domain rdf:resource="http://w3id.org/meta-share/meta-share/Relation"/>
        <rdfs:range rdf:resource="http://w3id.org/meta-share/meta-share/LanguageResource"/>
        <rdfs:comment xml:lang="en">Identifies the language resource with which a relation is holding with the one being described</rdfs:comment>
        <rdfs:label xml:lang="en">related language resource</rdfs:label>
    </owl:ObjectProperty>
    


    <!-- http://w3id.org/meta-share/meta-share/relatedLexiconType -->

    <owl:ObjectProperty rdf:about="http://w3id.org/meta-share/meta-share/relatedLexiconType">
        <rdfs:domain rdf:resource="http://w3id.org/meta-share/meta-share/LanguageDescription"/>
        <rdfs:range rdf:resource="http://w3id.org/meta-share/meta-share/RelatedLexiconType"/>
        <rdfs:comment xml:lang="en">Indicates the type of the lexica that must or can be used with the grammar</rdfs:comment>
        <rdfs:label xml:lang="en">related lexicon type</rdfs:label>
    </owl:ObjectProperty>
    


    <!-- http://w3id.org/meta-share/meta-share/relation -->

    <owl:ObjectProperty rdf:about="http://w3id.org/meta-share/meta-share/relation">
        <rdfs:domain rdf:resource="http://w3id.org/meta-share/meta-share/LanguageResource"/>
        <rdfs:range rdf:resource="http://w3id.org/meta-share/meta-share/Relation"/>
        <rdfs:comment xml:lang="en">Links a language resource to other related resources specifying also the type of relation</rdfs:comment>
        <rdfs:label xml:lang="en">relation</rdfs:label>
    </owl:ObjectProperty>
    


    <!-- http://w3id.org/meta-share/meta-share/replaces -->

    <owl:ObjectProperty rdf:about="http://w3id.org/meta-share/meta-share/replaces">
        <rdfs:subPropertyOf rdf:resource="http://w3id.org/meta-share/meta-share/isVersionOf"/>
        <rdfs:domain rdf:resource="http://w3id.org/meta-share/meta-share/LanguageResource"/>
        <rdfs:range rdf:resource="http://w3id.org/meta-share/meta-share/LanguageResource"/>
        <rdfs:comment xml:lang="en">Links to LR B that is an older version of LR A (the one being described) and has been replaced by it</rdfs:comment>
        <rdfs:label xml:lang="en">replaces</rdfs:label>
    </owl:ObjectProperty>
    


    <!-- http://w3id.org/meta-share/meta-share/requiredHardware -->

    <owl:ObjectProperty rdf:about="http://w3id.org/meta-share/meta-share/requiredHardware">
        <rdfs:domain>
            <owl:Class>
                <owl:unionOf rdf:parseType="Collection">
                    <rdf:Description rdf:about="http://w3id.org/meta-share/meta-share/LanguageDescription"/>
                    <rdf:Description rdf:about="http://w3id.org/meta-share/meta-share/ToolService"/>
                </owl:unionOf>
            </owl:Class>
        </rdfs:domain>
        <rdfs:range rdf:resource="http://w3id.org/meta-share/meta-share/RequiredHardware"/>
        <rdfs:comment xml:lang="en">Specifies the type of hardware required for running a tool and/or computational grammar</rdfs:comment>
        <rdfs:label xml:lang="en">required hardware</rdfs:label>
    </owl:ObjectProperty>
    


    <!-- http://w3id.org/meta-share/meta-share/requiresLR -->

    <owl:ObjectProperty rdf:about="http://w3id.org/meta-share/meta-share/requiresLR">
        <rdfs:subPropertyOf rdf:resource="http://w3id.org/meta-share/meta-share/dependsOn"/>
        <rdfs:domain>
            <owl:Class>
                <owl:unionOf rdf:parseType="Collection">
                    <rdf:Description rdf:about="http://w3id.org/meta-share/meta-share/LanguageDescription"/>
                    <rdf:Description rdf:about="http://w3id.org/meta-share/meta-share/ProcessingResource"/>
                    <rdf:Description rdf:about="http://w3id.org/meta-share/meta-share/ToolService"/>
                </owl:unionOf>
            </owl:Class>
        </rdfs:domain>
        <rdfs:range>
            <owl:Class>
                <owl:unionOf rdf:parseType="Collection">
                    <rdf:Description rdf:about="http://w3id.org/meta-share/meta-share/LanguageDescription"/>
                    <rdf:Description rdf:about="http://w3id.org/meta-share/meta-share/LexicalConceptualResource"/>
                </owl:unionOf>
            </owl:Class>
        </rdfs:range>
        <rdfs:comment xml:lang="en">LInks to LR B that is required for the operation of a tool/service or computational grammar (the one that is described)</rdfs:comment>
        <rdfs:label xml:lang="en">requires language resource</rdfs:label>
    </owl:ObjectProperty>
    


    <!-- http://w3id.org/meta-share/meta-share/resolution -->

    <owl:ObjectProperty rdf:about="http://w3id.org/meta-share/meta-share/resolution">
        <rdfs:domain>
            <owl:Class>
                <owl:unionOf rdf:parseType="Collection">
                    <rdf:Description rdf:about="http://w3id.org/meta-share/meta-share/ImageFormat"/>
                    <rdf:Description rdf:about="http://w3id.org/meta-share/meta-share/VideoFormat"/>
                </owl:unionOf>
            </owl:Class>
        </rdfs:domain>
        <rdfs:range rdf:resource="http://w3id.org/meta-share/meta-share/Resolution"/>
        <rdfs:comment xml:lang="en">Groups together information on the image resolution</rdfs:comment>
        <rdfs:label xml:lang="en">resolution</rdfs:label>
    </owl:ObjectProperty>
    


    <!-- http://w3id.org/meta-share/meta-share/resolutionStandard -->

    <owl:ObjectProperty rdf:about="http://w3id.org/meta-share/meta-share/resolutionStandard">
        <rdfs:domain rdf:resource="http://w3id.org/meta-share/meta-share/Resolution"/>
        <rdfs:range rdf:resource="http://w3id.org/meta-share/meta-share/ResolutionStandard"/>
        <rdfs:comment xml:lang="en">Specifies the standard to which  the resolution conforms</rdfs:comment>
        <rdfs:label xml:lang="en">resolution standard</rdfs:label>
    </owl:ObjectProperty>
    


    <!-- http://w3id.org/meta-share/meta-share/resourceCreator -->

    <owl:ObjectProperty rdf:about="http://w3id.org/meta-share/meta-share/resourceCreator">
        <rdfs:subPropertyOf rdf:resource="http://w3id.org/meta-share/meta-share/isRelatedToActor"/>
        <rdfs:domain rdf:resource="http://w3id.org/meta-share/meta-share/LanguageResource"/>
        <rdfs:range rdf:resource="http://w3id.org/meta-share/meta-share/Actor"/>
        <rdfs:comment xml:lang="en">Links a resource to the person, group or organisation that has created the resource</rdfs:comment>
        <rdfs:label xml:lang="en">resource creator</rdfs:label>
    </owl:ObjectProperty>
    


    <!-- http://w3id.org/meta-share/meta-share/resourceProvider -->

    <owl:ObjectProperty rdf:about="http://w3id.org/meta-share/meta-share/resourceProvider">
        <rdfs:subPropertyOf rdf:resource="http://w3id.org/meta-share/meta-share/isRelatedToActor"/>
        <rdfs:domain rdf:resource="http://w3id.org/meta-share/meta-share/LanguageResource"/>
        <rdfs:range rdf:resource="http://w3id.org/meta-share/meta-share/Actor"/>
        <rdfs:comment xml:lang="en">The person/organization responsible for providing, curating, maintaining and making available (publishing) the resource</rdfs:comment>
        <rdfs:label xml:lang="en">resource provider</rdfs:label>
    </owl:ObjectProperty>
    


    <!-- http://w3id.org/meta-share/meta-share/reviews -->

    <owl:ObjectProperty rdf:about="http://w3id.org/meta-share/meta-share/reviews">
        <rdfs:subPropertyOf rdf:resource="http://w3id.org/meta-share/meta-share/documents"/>
        <rdfs:domain rdf:resource="http://w3id.org/meta-share/meta-share/Document"/>
        <rdfs:range rdf:resource="http://w3id.org/meta-share/meta-share/LanguageResource"/>
        <rdfs:comment xml:lang="en">Links a document to the language resource it reviews</rdfs:comment>
        <rdfs:label xml:lang="en">reviews</rdfs:label>
    </owl:ObjectProperty>
    


    <!-- http://w3id.org/meta-share/meta-share/scenarioType -->

    <owl:ObjectProperty rdf:about="http://w3id.org/meta-share/meta-share/scenarioType">
        <rdfs:domain>
            <owl:Class>
                <owl:unionOf rdf:parseType="Collection">
                    <rdf:Description rdf:about="http://w3id.org/meta-share/meta-share/CorpusAudioPart"/>
                    <rdf:Description rdf:about="http://w3id.org/meta-share/meta-share/CorpusVideoPart"/>
                </owl:unionOf>
            </owl:Class>
        </rdfs:domain>
        <rdfs:range rdf:resource="http://w3id.org/meta-share/meta-share/ScenarioType"/>
        <rdfs:comment xml:lang="en">Indicates the task defined for the conversation or the interaction of participants</rdfs:comment>
        <rdfs:label xml:lang="en">scenario type</rdfs:label>
    </owl:ObjectProperty>
    


    <!-- http://w3id.org/meta-share/meta-share/sceneIllumination -->

    <owl:ObjectProperty rdf:about="http://w3id.org/meta-share/meta-share/sceneIllumination">
        <rdfs:domain>
            <owl:Class>
                <owl:unionOf rdf:parseType="Collection">
                    <rdf:Description rdf:about="http://w3id.org/meta-share/meta-share/CorpusAudioPart"/>
                    <rdf:Description rdf:about="http://w3id.org/meta-share/meta-share/CorpusImagePart"/>
                    <rdf:Description rdf:about="http://w3id.org/meta-share/meta-share/CorpusTextNumericalPart"/>
                    <rdf:Description rdf:about="http://w3id.org/meta-share/meta-share/CorpusVideoPart"/>
                </owl:unionOf>
            </owl:Class>
        </rdfs:domain>
        <rdfs:range rdf:resource="http://w3id.org/meta-share/meta-share/SceneIllumination"/>
        <rdfs:comment xml:lang="en">Provides information on the illumination of the scene</rdfs:comment>
        <rdfs:label xml:lang="en">scene illumination</rdfs:label>
        <skos:note xml:lang="en">needed for audio?</skos:note>
    </owl:ObjectProperty>
    


    <!-- http://w3id.org/meta-share/meta-share/segmentationLevel -->

    <owl:ObjectProperty rdf:about="http://w3id.org/meta-share/meta-share/segmentationLevel">
        <rdfs:domain rdf:resource="http://w3id.org/meta-share/meta-share/Annotation"/>
        <rdfs:range rdf:resource="http://w3id.org/meta-share/meta-share/SegmentationLevel"/>
        <rdfs:comment xml:lang="en">Specifies the segmentation unit in terms of which the resource has been segmented or the level of segmentation a tool/service requires/outputs</rdfs:comment>
        <rdfs:label xml:lang="en">segmentation level</rdfs:label>
    </owl:ObjectProperty>
    


    <!-- http://w3id.org/meta-share/meta-share/sex -->

    <owl:ObjectProperty rdf:about="http://w3id.org/meta-share/meta-share/sex">
        <rdfs:domain rdf:resource="http://w3id.org/meta-share/meta-share/Participant"/>
        <rdfs:range rdf:resource="http://w3id.org/meta-share/meta-share/Sex"/>
        <rdfs:comment xml:lang="en">Specifies the sex of a participant (either of the two major forms of individuals that occur in many species and that are distinguished respectively as female or male especially on the basis of their reproductive organs and structures [https://www.merriam-webster.com/dictionary/sex])</rdfs:comment>
        <rdfs:label xml:lang="en">sex</rdfs:label>
        <skos:note xml:lang="en">check with sociologists?</skos:note>
    </owl:ObjectProperty>
    


    <!-- http://w3id.org/meta-share/meta-share/sexOfParticipants -->

    <owl:ObjectProperty rdf:about="http://w3id.org/meta-share/meta-share/sexOfParticipants">
        <rdfs:domain>
            <owl:Class>
                <owl:unionOf rdf:parseType="Collection">
                    <rdf:Description rdf:about="http://w3id.org/meta-share/meta-share/CorpusAudioPart"/>
                    <rdf:Description rdf:about="http://w3id.org/meta-share/meta-share/CorpusImagePart"/>
                    <rdf:Description rdf:about="http://w3id.org/meta-share/meta-share/CorpusTextNumericalPart"/>
                    <rdf:Description rdf:about="http://w3id.org/meta-share/meta-share/CorpusVideoPart"/>
                </owl:unionOf>
            </owl:Class>
        </rdfs:domain>
        <rdfs:range rdf:resource="http://w3id.org/meta-share/meta-share/Sex"/>
        <rdfs:comment xml:lang="en">Specifies the sex of the participants (either of the two major forms of individuals that occur in many species and that are distinguished respectively as female or male especially on the basis of their reproductive organs and structures [https://www.merriam-webster.com/dictionary/sex])</rdfs:comment>
        <rdfs:label xml:lang="en">sex of participants</rdfs:label>
        <skos:note xml:lang="en">check with sociologists?</skos:note>
    </owl:ObjectProperty>
    


    <!-- http://w3id.org/meta-share/meta-share/signConvention -->

    <owl:ObjectProperty rdf:about="http://w3id.org/meta-share/meta-share/signConvention">
        <rdfs:domain rdf:resource="http://w3id.org/meta-share/meta-share/AudioFormat"/>
        <rdfs:range rdf:resource="http://w3id.org/meta-share/meta-share/SignConvention"/>
        <rdfs:comment xml:lang="en">Indicates the binary representation of numbers</rdfs:comment>
        <rdfs:label xml:lang="en">sign convention</rdfs:label>
    </owl:ObjectProperty>
    


    <!-- http://w3id.org/meta-share/meta-share/signalEncoding -->

    <owl:ObjectProperty rdf:about="http://w3id.org/meta-share/meta-share/signalEncoding">
        <rdfs:domain rdf:resource="http://w3id.org/meta-share/meta-share/CorpusAudioPart"/>
        <rdfs:range rdf:resource="http://w3id.org/meta-share/meta-share/SignalEncoding"/>
        <rdfs:comment xml:lang="en">Specifies the  encoding the audio type uses</rdfs:comment>
        <rdfs:label xml:lang="en">signal encoding</rdfs:label>
    </owl:ObjectProperty>
    


    <!-- http://w3id.org/meta-share/meta-share/size -->

    <owl:ObjectProperty rdf:about="http://w3id.org/meta-share/meta-share/size">
        <rdfs:domain rdf:resource="http://w3id.org/meta-share/meta-share/DatasetDistribution"/>
        <rdfs:range rdf:resource="http://w3id.org/meta-share/meta-share/Size"/>
        <rdfs:comment xml:lang="en">Specifies the size of the resource with regard to the SizeUnit measurement in form of a number</rdfs:comment>
        <rdfs:label xml:lang="en">size</rdfs:label>
    </owl:ObjectProperty>
    


    <!-- http://w3id.org/meta-share/meta-share/sizePerAnnotation -->

    <owl:ObjectProperty rdf:about="http://w3id.org/meta-share/meta-share/sizePerAnnotation">
        <rdfs:subPropertyOf rdf:resource="http://w3id.org/meta-share/meta-share/sizePerSubset"/>
        <rdfs:range rdf:resource="http://w3id.org/meta-share/meta-share/Size"/>
        <rdfs:comment xml:lang="en">Provides information on size for the annotated parts of the resource</rdfs:comment>
        <rdfs:label xml:lang="en">size per annotation</rdfs:label>
    </owl:ObjectProperty>
    


    <!-- http://w3id.org/meta-share/meta-share/sizePerAudioClassification -->

    <owl:ObjectProperty rdf:about="http://w3id.org/meta-share/meta-share/sizePerAudioClassification">
        <rdfs:subPropertyOf rdf:resource="http://w3id.org/meta-share/meta-share/sizePerSubset"/>
        <rdfs:range rdf:resource="http://w3id.org/meta-share/meta-share/Size"/>
        <rdfs:comment xml:lang="en">The size of the audio subparts of the resource in terms of classification criteria</rdfs:comment>
        <rdfs:label xml:lang="en">size per audio classification</rdfs:label>
    </owl:ObjectProperty>
    


    <!-- http://w3id.org/meta-share/meta-share/sizePerAudioFormat -->

    <owl:ObjectProperty rdf:about="http://w3id.org/meta-share/meta-share/sizePerAudioFormat">
        <rdfs:subPropertyOf rdf:resource="http://w3id.org/meta-share/meta-share/sizePerSubset"/>
        <rdfs:range rdf:resource="http://w3id.org/meta-share/meta-share/Size"/>
        <rdfs:comment xml:lang="en">Used to give info on size of parts of a resource that differ as to the format</rdfs:comment>
        <rdfs:label xml:lang="en">size per audio format</rdfs:label>
    </owl:ObjectProperty>
    


    <!-- http://w3id.org/meta-share/meta-share/sizePerCharacterEncoding -->

    <owl:ObjectProperty rdf:about="http://w3id.org/meta-share/meta-share/sizePerCharacterEncoding">
        <rdfs:subPropertyOf rdf:resource="http://w3id.org/meta-share/meta-share/sizePerSubset"/>
        <rdfs:range rdf:resource="http://w3id.org/meta-share/meta-share/Size"/>
        <rdfs:comment xml:lang="en">Provides information on the size of the resource parts with different character encoding</rdfs:comment>
        <rdfs:label xml:lang="en">size per character encoding</rdfs:label>
    </owl:ObjectProperty>
    


    <!-- http://w3id.org/meta-share/meta-share/sizePerDomain -->

    <owl:ObjectProperty rdf:about="http://w3id.org/meta-share/meta-share/sizePerDomain">
        <rdfs:subPropertyOf rdf:resource="http://w3id.org/meta-share/meta-share/sizePerSubset"/>
        <rdfs:range rdf:resource="http://w3id.org/meta-share/meta-share/Size"/>
        <rdfs:comment xml:lang="en">Specifies the size of resource parts per domain</rdfs:comment>
        <rdfs:label xml:lang="en">size per domain</rdfs:label>
    </owl:ObjectProperty>
    


    <!-- http://w3id.org/meta-share/meta-share/sizePerGeographicCoverage -->

    <owl:ObjectProperty rdf:about="http://w3id.org/meta-share/meta-share/sizePerGeographicCoverage">
        <rdfs:subPropertyOf rdf:resource="http://w3id.org/meta-share/meta-share/sizePerSubset"/>
        <rdfs:range rdf:resource="http://w3id.org/meta-share/meta-share/Size"/>
        <rdfs:comment xml:lang="en">Provides information on size per geographically distinct section of the resource</rdfs:comment>
        <rdfs:label xml:lang="en">size per geographic coverage</rdfs:label>
    </owl:ObjectProperty>
    


    <!-- http://w3id.org/meta-share/meta-share/sizePerImageClassification -->

    <owl:ObjectProperty rdf:about="http://w3id.org/meta-share/meta-share/sizePerImageClassification">
        <rdfs:subPropertyOf rdf:resource="http://w3id.org/meta-share/meta-share/sizePerSubset"/>
        <rdfs:range rdf:resource="http://w3id.org/meta-share/meta-share/Size"/>
        <rdfs:comment xml:lang="en">Provides information on size of parts with different image classification</rdfs:comment>
        <rdfs:label xml:lang="en">size per image classification</rdfs:label>
    </owl:ObjectProperty>
    


    <!-- http://w3id.org/meta-share/meta-share/sizePerImageFormat -->

    <owl:ObjectProperty rdf:about="http://w3id.org/meta-share/meta-share/sizePerImageFormat">
        <rdfs:subPropertyOf rdf:resource="http://w3id.org/meta-share/meta-share/sizePerSubset"/>
        <rdfs:range rdf:resource="http://w3id.org/meta-share/meta-share/Size"/>
        <rdfs:comment xml:lang="en">Used to give info on size of parts of a resource that differ as to the format</rdfs:comment>
        <rdfs:label xml:lang="en">size per image format</rdfs:label>
    </owl:ObjectProperty>
    


    <!-- http://w3id.org/meta-share/meta-share/sizePerLanguage -->

    <owl:ObjectProperty rdf:about="http://w3id.org/meta-share/meta-share/sizePerLanguage">
        <rdfs:subPropertyOf rdf:resource="http://w3id.org/meta-share/meta-share/sizePerSubset"/>
        <rdfs:range rdf:resource="http://w3id.org/meta-share/meta-share/Size"/>
        <rdfs:comment xml:lang="en">Provides information on the size per language component</rdfs:comment>
        <rdfs:label xml:lang="en">size per language</rdfs:label>
    </owl:ObjectProperty>
    


    <!-- http://w3id.org/meta-share/meta-share/sizePerLanguageVariety -->

    <owl:ObjectProperty rdf:about="http://w3id.org/meta-share/meta-share/sizePerLanguageVariety">
        <rdfs:subPropertyOf rdf:resource="http://w3id.org/meta-share/meta-share/sizePerSubset"/>
        <rdfs:range rdf:resource="http://w3id.org/meta-share/meta-share/Size"/>
        <rdfs:comment xml:lang="en">Provides information on the size per language variety component</rdfs:comment>
        <rdfs:label xml:lang="en">size per language variety</rdfs:label>
    </owl:ObjectProperty>
    


    <!-- http://w3id.org/meta-share/meta-share/sizePerModality -->

    <owl:ObjectProperty rdf:about="http://w3id.org/meta-share/meta-share/sizePerModality">
        <rdfs:subPropertyOf rdf:resource="http://w3id.org/meta-share/meta-share/sizePerSubset"/>
        <rdfs:range rdf:resource="http://w3id.org/meta-share/meta-share/Size"/>
        <rdfs:comment xml:lang="en">Provides information on the size per modality component</rdfs:comment>
        <rdfs:label xml:lang="en">size per modality</rdfs:label>
    </owl:ObjectProperty>
    


    <!-- http://w3id.org/meta-share/meta-share/sizePerSubset -->

    <owl:ObjectProperty rdf:about="http://w3id.org/meta-share/meta-share/sizePerSubset">
        <rdfs:domain rdf:resource="http://w3id.org/meta-share/meta-share/Subset"/>
        <rdfs:range rdf:resource="http://w3id.org/meta-share/meta-share/Size"/>
        <rdfs:comment xml:lang="en">Indicates the size of a subset of a language resource</rdfs:comment>
        <rdfs:label xml:lang="en">size per subset</rdfs:label>
    </owl:ObjectProperty>
    


    <!-- http://w3id.org/meta-share/meta-share/sizePerTextClassification -->

    <owl:ObjectProperty rdf:about="http://w3id.org/meta-share/meta-share/sizePerTextClassification">
        <rdfs:subPropertyOf rdf:resource="http://w3id.org/meta-share/meta-share/sizePerSubset"/>
        <rdfs:range rdf:resource="http://w3id.org/meta-share/meta-share/Size"/>
        <rdfs:comment xml:lang="en">Provides information on size of resource parts with different text classification</rdfs:comment>
        <rdfs:label xml:lang="en">size per text classification</rdfs:label>
    </owl:ObjectProperty>
    


    <!-- http://w3id.org/meta-share/meta-share/sizePerTextFormat -->

    <owl:ObjectProperty rdf:about="http://w3id.org/meta-share/meta-share/sizePerTextFormat">
        <rdfs:subPropertyOf rdf:resource="http://w3id.org/meta-share/meta-share/sizePerSubset"/>
        <rdfs:range rdf:resource="http://w3id.org/meta-share/meta-share/Size"/>
        <rdfs:comment xml:lang="en">Provides information on the size of the resource parts with different format</rdfs:comment>
        <rdfs:label xml:lang="en">size per text format</rdfs:label>
    </owl:ObjectProperty>
    


    <!-- http://w3id.org/meta-share/meta-share/sizePerTextNumericalFormat -->

    <owl:ObjectProperty rdf:about="http://w3id.org/meta-share/meta-share/sizePerTextNumericalFormat">
        <rdfs:subPropertyOf rdf:resource="http://w3id.org/meta-share/meta-share/sizePerSubset"/>
        <rdfs:range rdf:resource="http://w3id.org/meta-share/meta-share/Size"/>
        <rdfs:comment xml:lang="en">Gives information on the size of textNumerical resource parts with different format</rdfs:comment>
        <rdfs:label xml:lang="en">size per textNumerical format</rdfs:label>
    </owl:ObjectProperty>
    


    <!-- http://w3id.org/meta-share/meta-share/sizePerTimeCoverage -->

    <owl:ObjectProperty rdf:about="http://w3id.org/meta-share/meta-share/sizePerTimeCoverage">
        <rdfs:subPropertyOf rdf:resource="http://w3id.org/meta-share/meta-share/sizePerSubset"/>
        <rdfs:range rdf:resource="http://w3id.org/meta-share/meta-share/Size"/>
        <rdfs:comment xml:lang="en">Provides information on size per time period represented in the resource</rdfs:comment>
        <rdfs:label xml:lang="en">size per time coverage</rdfs:label>
    </owl:ObjectProperty>
    


    <!-- http://w3id.org/meta-share/meta-share/sizePerValidation -->

    <owl:ObjectProperty rdf:about="http://w3id.org/meta-share/meta-share/sizePerValidation">
        <rdfs:subPropertyOf rdf:resource="http://w3id.org/meta-share/meta-share/sizePerSubset"/>
        <rdfs:range rdf:resource="http://w3id.org/meta-share/meta-share/Size"/>
        <rdfs:comment xml:lang="en">Specifies the size of the validated part of a resource</rdfs:comment>
        <rdfs:label xml:lang="en">size per validation</rdfs:label>
    </owl:ObjectProperty>
    


    <!-- http://w3id.org/meta-share/meta-share/sizePerVideoClassification -->

    <owl:ObjectProperty rdf:about="http://w3id.org/meta-share/meta-share/sizePerVideoClassification">
        <rdfs:subPropertyOf rdf:resource="http://w3id.org/meta-share/meta-share/sizePerSubset"/>
        <rdfs:range rdf:resource="http://w3id.org/meta-share/meta-share/Size"/>
        <rdfs:comment xml:lang="en">Used to give info on size of parts with different video classification</rdfs:comment>
        <rdfs:label xml:lang="en">size per video classification</rdfs:label>
    </owl:ObjectProperty>
    


    <!-- http://w3id.org/meta-share/meta-share/sizePerVideoFormat -->

    <owl:ObjectProperty rdf:about="http://w3id.org/meta-share/meta-share/sizePerVideoFormat">
        <rdfs:subPropertyOf rdf:resource="http://w3id.org/meta-share/meta-share/sizePerSubset"/>
        <rdfs:range rdf:resource="http://w3id.org/meta-share/meta-share/Size"/>
        <rdfs:comment xml:lang="en">Used to give info on size of parts of a resource that differ as to the format</rdfs:comment>
        <rdfs:label xml:lang="en">size per video format</rdfs:label>
    </owl:ObjectProperty>
    


    <!-- http://w3id.org/meta-share/meta-share/sizeUnit -->

    <owl:ObjectProperty rdf:about="http://w3id.org/meta-share/meta-share/sizeUnit">
        <rdfs:domain rdf:resource="http://w3id.org/meta-share/meta-share/Size"/>
        <rdfs:range rdf:resource="http://w3id.org/meta-share/meta-share/SizeUnit"/>
        <rdfs:comment xml:lang="en">Specifies the unit that is used when providing information on the size of the resource or of resource parts</rdfs:comment>
        <rdfs:label xml:lang="en">size unit</rdfs:label>
    </owl:ObjectProperty>
    


    <!-- http://w3id.org/meta-share/meta-share/socialMediaOccupationalAccount -->

    <owl:ObjectProperty rdf:about="http://w3id.org/meta-share/meta-share/socialMediaOccupationalAccount">
        <rdfs:domain>
            <owl:Class>
                <owl:unionOf rdf:parseType="Collection">
                    <rdf:Description rdf:about="http://w3id.org/meta-share/meta-share/Division"/>
                    <rdf:Description rdf:about="http://w3id.org/meta-share/meta-share/Group"/>
                    <rdf:Description rdf:about="http://w3id.org/meta-share/meta-share/Organization"/>
                    <rdf:Description rdf:about="http://w3id.org/meta-share/meta-share/Person"/>
                    <rdf:Description rdf:about="http://w3id.org/meta-share/meta-share/Project"/>
                </owl:unionOf>
            </owl:Class>
        </rdfs:domain>
        <rdfs:range rdf:resource="http://w3id.org/meta-share/meta-share/SocialMediaOccupationalAccount"/>
        <rdfs:comment xml:lang="en">Introduces the social media or occupational account details of a person or organization</rdfs:comment>
        <rdfs:label xml:lang="en">social media occupational account</rdfs:label>
    </owl:ObjectProperty>
    


    <!-- http://w3id.org/meta-share/meta-share/socialMediaOccupationalAccountType -->

    <owl:ObjectProperty rdf:about="http://w3id.org/meta-share/meta-share/socialMediaOccupationalAccountType">
        <rdfs:domain rdf:resource="http://w3id.org/meta-share/meta-share/SocialMediaOccupationalAccount"/>
        <rdfs:range rdf:resource="http://w3id.org/meta-share/meta-share/SocialMediaOccupationalAccountType"/>
        <rdfs:comment xml:lang="en">Specifies the type of the social media or occupational account</rdfs:comment>
        <rdfs:label xml:lang="en">social media occupational account type</rdfs:label>
    </owl:ObjectProperty>
    


    <!-- http://w3id.org/meta-share/meta-share/sourceChannel -->

    <owl:ObjectProperty rdf:about="http://w3id.org/meta-share/meta-share/sourceChannel">
        <rdfs:domain>
            <owl:Class>
                <owl:unionOf rdf:parseType="Collection">
                    <rdf:Description rdf:about="http://w3id.org/meta-share/meta-share/CorpusAudioPart"/>
                    <rdf:Description rdf:about="http://w3id.org/meta-share/meta-share/CorpusTextNumericalPart"/>
                    <rdf:Description rdf:about="http://w3id.org/meta-share/meta-share/CorpusVideoPart"/>
                </owl:unionOf>
            </owl:Class>
        </rdfs:domain>
        <rdfs:range rdf:resource="http://w3id.org/meta-share/meta-share/SourceChannel"/>
        <rdfs:comment xml:lang="en">Specifies the source channel of the recording of a multimedia resource</rdfs:comment>
        <rdfs:label xml:lang="en">source channel</rdfs:label>
    </owl:ObjectProperty>
    


    <!-- http://w3id.org/meta-share/meta-share/sourceChannelType -->

    <owl:ObjectProperty rdf:about="http://w3id.org/meta-share/meta-share/sourceChannelType">
        <rdfs:domain>
            <owl:Class>
                <owl:unionOf rdf:parseType="Collection">
                    <rdf:Description rdf:about="http://w3id.org/meta-share/meta-share/CorpusAudioPart"/>
                    <rdf:Description rdf:about="http://w3id.org/meta-share/meta-share/CorpusTextNumericalPart"/>
                    <rdf:Description rdf:about="http://w3id.org/meta-share/meta-share/CorpusVideoPart"/>
                </owl:unionOf>
            </owl:Class>
        </rdfs:domain>
        <rdfs:range rdf:resource="http://w3id.org/meta-share/meta-share/SourceChannelType"/>
        <rdfs:comment xml:lang="en">Specifies the type of the source channel</rdfs:comment>
        <rdfs:label xml:lang="en">source channel type</rdfs:label>
    </owl:ObjectProperty>
    


    <!-- http://w3id.org/meta-share/meta-share/sourceMetadataRecord -->

    <owl:ObjectProperty rdf:about="http://w3id.org/meta-share/meta-share/sourceMetadataRecord">
        <rdfs:subPropertyOf rdf:resource="http://w3id.org/meta-share/meta-share/isRelatedToMDRecord"/>
        <owl:inverseOf rdf:resource="http://w3id.org/meta-share/meta-share/targetMetadataRecord"/>
        <rdfs:domain rdf:resource="http://w3id.org/meta-share/meta-share/MetadataRecord"/>
        <rdfs:range rdf:resource="http://w3id.org/meta-share/meta-share/MetadataRecord"/>
        <rdfs:comment xml:lang="en">Links, in some cases (e.g.,  harvesting, population from other catalogues, conversion from other metadata records, etc.), to the metadata record that has been used as the basis for the creation of the metadata record</rdfs:comment>
        <rdfs:label xml:lang="en">source metadata record</rdfs:label>
    </owl:ObjectProperty>
    


    <!-- http://w3id.org/meta-share/meta-share/sourceOfMetadataRecord -->

    <owl:ObjectProperty rdf:about="http://w3id.org/meta-share/meta-share/sourceOfMetadataRecord">
        <rdfs:domain rdf:resource="http://w3id.org/meta-share/meta-share/MetadataRecord"/>
        <rdfs:range rdf:resource="http://www.w3.org/ns/dcat#Catalog"/>
        <rdfs:comment xml:lang="en">Refers to the entity (repository, catalogue, archive, etc.) from which the metadata record has been imported into the new catalogue</rdfs:comment>
        <rdfs:label xml:lang="en">sourceOfMetadataRecord</rdfs:label>
        <skos:note xml:lang="en">for now dcat:catalog</skos:note>
    </owl:ObjectProperty>
    


    <!-- http://w3id.org/meta-share/meta-share/speakingImpairmentOfParticipants -->

    <owl:ObjectProperty rdf:about="http://w3id.org/meta-share/meta-share/speakingImpairmentOfParticipants">
        <rdfs:domain>
            <owl:Class>
                <owl:unionOf rdf:parseType="Collection">
                    <rdf:Description rdf:about="http://w3id.org/meta-share/meta-share/CorpusAudioPart"/>
                    <rdf:Description rdf:about="http://w3id.org/meta-share/meta-share/CorpusImagePart"/>
                    <rdf:Description rdf:about="http://w3id.org/meta-share/meta-share/CorpusTextNumericalPart"/>
                    <rdf:Description rdf:about="http://w3id.org/meta-share/meta-share/CorpusVideoPart"/>
                </owl:unionOf>
            </owl:Class>
        </rdfs:domain>
        <rdfs:range rdf:resource="http://w3id.org/meta-share/meta-share/SpeakingImpairmentOfParticipants"/>
        <rdfs:comment xml:lang="en">Indicates whether the group of participants contains persons with speaking impairments</rdfs:comment>
        <rdfs:label xml:lang="en">speaking impairment of participants</rdfs:label>
    </owl:ObjectProperty>
    


    <!-- http://w3id.org/meta-share/meta-share/speechInfluence -->

    <owl:ObjectProperty rdf:about="http://w3id.org/meta-share/meta-share/speechInfluence">
        <rdfs:domain>
            <owl:Class>
                <owl:unionOf rdf:parseType="Collection">
                    <rdf:Description rdf:about="http://w3id.org/meta-share/meta-share/CorpusAudioPart"/>
                    <rdf:Description rdf:about="http://w3id.org/meta-share/meta-share/CorpusImagePart"/>
                    <rdf:Description rdf:about="http://w3id.org/meta-share/meta-share/CorpusTextNumericalPart"/>
                    <rdf:Description rdf:about="http://w3id.org/meta-share/meta-share/CorpusVideoPart"/>
                </owl:unionOf>
            </owl:Class>
        </rdfs:domain>
        <rdfs:range rdf:resource="http://w3id.org/meta-share/meta-share/SpeechInfluence"/>
        <rdfs:comment xml:lang="en">Specifies the factors influencing speech</rdfs:comment>
        <rdfs:label xml:lang="en">speech influence</rdfs:label>
    </owl:ObjectProperty>
    


    <!-- http://w3id.org/meta-share/meta-share/speechItem -->

    <owl:ObjectProperty rdf:about="http://w3id.org/meta-share/meta-share/speechItem">
        <rdfs:domain>
            <owl:Class>
                <owl:unionOf rdf:parseType="Collection">
                    <rdf:Description rdf:about="http://w3id.org/meta-share/meta-share/CorpusAudioPart"/>
                    <rdf:Description rdf:about="http://w3id.org/meta-share/meta-share/LexicalConceptualResourceAudioPart"/>
                </owl:unionOf>
            </owl:Class>
        </rdfs:domain>
        <rdfs:range rdf:resource="http://w3id.org/meta-share/meta-share/SpeechItem"/>
        <rdfs:comment xml:lang="en">Specifies the distinct elements that are pronounced and annotated as such</rdfs:comment>
        <rdfs:label xml:lang="en">speech item</rdfs:label>
    </owl:ObjectProperty>
    


    <!-- http://w3id.org/meta-share/meta-share/staticElement -->

    <owl:ObjectProperty rdf:about="http://w3id.org/meta-share/meta-share/staticElement">
        <rdfs:domain>
            <owl:Class>
                <owl:unionOf rdf:parseType="Collection">
                    <rdf:Description rdf:about="http://w3id.org/meta-share/meta-share/CorpusImagePart"/>
                    <rdf:Description rdf:about="http://w3id.org/meta-share/meta-share/LanguageDescriptionImagePart"/>
                    <rdf:Description rdf:about="http://w3id.org/meta-share/meta-share/LexicalConceptualResourceImagePart"/>
                </owl:unionOf>
            </owl:Class>
        </rdfs:domain>
        <rdfs:range rdf:resource="http://w3id.org/meta-share/meta-share/StaticElement"/>
        <rdfs:comment xml:lang="en">Groups information on the static elements visible on images</rdfs:comment>
        <rdfs:label xml:lang="en">static element</rdfs:label>
    </owl:ObjectProperty>
    


    <!-- http://w3id.org/meta-share/meta-share/subject -->

    <owl:ObjectProperty rdf:about="http://w3id.org/meta-share/meta-share/subject">
        <rdfs:domain>
            <owl:Class>
                <owl:unionOf rdf:parseType="Collection">
                    <rdf:Description rdf:about="http://w3id.org/meta-share/meta-share/CorpusMediaPart"/>
                    <rdf:Description rdf:about="http://w3id.org/meta-share/meta-share/Document"/>
                    <rdf:Description rdf:about="http://w3id.org/meta-share/meta-share/Project"/>
                </owl:unionOf>
            </owl:Class>
        </rdfs:domain>
        <rdfs:range rdf:resource="http://w3id.org/meta-share/meta-share/Subject"/>
        <rdfs:altLabel xml:lang="en">topic</rdfs:altLabel>
        <rdfs:comment xml:lang="en">Specifies the subject/topic of a language resource</rdfs:comment>
        <rdfs:label xml:lang="en">subject</rdfs:label>
    </owl:ObjectProperty>
    


    <!-- http://w3id.org/meta-share/meta-share/tagset -->

    <owl:ObjectProperty rdf:about="http://w3id.org/meta-share/meta-share/tagset">
        <rdfs:domain>
            <owl:Class>
                <owl:unionOf rdf:parseType="Collection">
                    <rdf:Description rdf:about="http://w3id.org/meta-share/meta-share/Annotation"/>
                    <rdf:Description rdf:about="http://w3id.org/meta-share/meta-share/MLModel"/>
                </owl:unionOf>
            </owl:Class>
        </rdfs:domain>
        <rdfs:range rdf:resource="http://w3id.org/meta-share/meta-share/LexicalConceptualResource"/>
        <rdfs:comment xml:lang="en">The tagset used for annotating a resource or for the input resource (if annotated) of a tool/service or that should be used (dependency) for the annotation</rdfs:comment>
        <rdfs:label xml:lang="en">tagset</rdfs:label>
    </owl:ObjectProperty>
    


    <!-- http://w3id.org/meta-share/meta-share/targetMetadataRecord -->

    <owl:ObjectProperty rdf:about="http://w3id.org/meta-share/meta-share/targetMetadataRecord">
        <rdfs:subPropertyOf rdf:resource="http://w3id.org/meta-share/meta-share/MDRecordRelatedTo"/>
        <rdfs:domain rdf:resource="http://w3id.org/meta-share/meta-share/MetadataRecord"/>
        <rdfs:range rdf:resource="http://w3id.org/meta-share/meta-share/MetadataRecord"/>
        <rdfs:comment xml:lang="en">Links, in some cases (e.g.,  harvesting, population from other catalogues, conversion from other metadata records, etc.), an external metadata record that has been used as the basis for the creation of the internal metadata record to this internal metadata record</rdfs:comment>
        <rdfs:label xml:lang="en">target metadata record</rdfs:label>
    </owl:ObjectProperty>
    


    <!-- http://w3id.org/meta-share/meta-share/textIncludedInImage -->

    <owl:ObjectProperty rdf:about="http://w3id.org/meta-share/meta-share/textIncludedInImage">
        <rdfs:domain>
            <owl:Class>
                <owl:unionOf rdf:parseType="Collection">
                    <rdf:Description rdf:about="http://w3id.org/meta-share/meta-share/CorpusImagePart"/>
                    <rdf:Description rdf:about="http://w3id.org/meta-share/meta-share/LanguageDescriptionImagePart"/>
                    <rdf:Description rdf:about="http://w3id.org/meta-share/meta-share/LexicalConceptualResourceImagePart"/>
                </owl:unionOf>
            </owl:Class>
        </rdfs:domain>
        <rdfs:range rdf:resource="http://w3id.org/meta-share/meta-share/TextIncludedInImage"/>
        <rdfs:comment xml:lang="en">Provides information on the type of text that may be on the image</rdfs:comment>
        <rdfs:label xml:lang="en">text included in image</rdfs:label>
    </owl:ObjectProperty>
    


    <!-- http://w3id.org/meta-share/meta-share/textIncludedInVideo -->

    <owl:ObjectProperty rdf:about="http://w3id.org/meta-share/meta-share/textIncludedInVideo">
        <rdfs:domain>
            <owl:Class>
                <owl:unionOf rdf:parseType="Collection">
                    <rdf:Description rdf:about="http://w3id.org/meta-share/meta-share/CorpusVideoPart"/>
                    <rdf:Description rdf:about="http://w3id.org/meta-share/meta-share/LanguageDescriptionVideoPart"/>
                    <rdf:Description rdf:about="http://w3id.org/meta-share/meta-share/LexicalConceptualResourceVideoPart"/>
                </owl:unionOf>
            </owl:Class>
        </rdfs:domain>
        <rdfs:range rdf:resource="http://w3id.org/meta-share/meta-share/TextIncludedInVideo"/>
        <rdfs:comment xml:lang="en">Indicates if any text and what type is present in or in conjunction with the video</rdfs:comment>
        <rdfs:label xml:lang="en">text included in video</rdfs:label>
    </owl:ObjectProperty>
    


    <!-- http://w3id.org/meta-share/meta-share/textNumericalFormat -->

    <owl:ObjectProperty rdf:about="http://w3id.org/meta-share/meta-share/textNumericalFormat">
        <rdfs:domain rdf:resource="http://w3id.org/meta-share/meta-share/CorpusTextNumericalPart"/>
        <rdfs:range rdf:resource="http://w3id.org/meta-share/omtd-share/DataFormat"/>
        <rdfs:comment xml:lang="en">Groups information on the format(s) of the textNumerical part of the resource</rdfs:comment>
        <rdfs:label xml:lang="en">textNumerical format</rdfs:label>
    </owl:ObjectProperty>
    


    <!-- http://w3id.org/meta-share/meta-share/textType -->

    <owl:ObjectProperty rdf:about="http://w3id.org/meta-share/meta-share/textType">
        <rdfs:domain rdf:resource="http://w3id.org/meta-share/meta-share/CorpusTextPart"/>
        <rdfs:range rdf:resource="http://w3id.org/meta-share/meta-share/TextType"/>
        <rdfs:comment xml:lang="en">Specifies the text type (e.g.,  factual, literary, etc.) according to which a text corpus (part) is classified</rdfs:comment>
        <rdfs:label xml:lang="en">text type</rdfs:label>
    </owl:ObjectProperty>
    


    <!-- http://w3id.org/meta-share/meta-share/trl -->

    <owl:ObjectProperty rdf:about="http://w3id.org/meta-share/meta-share/trl">
        <rdfs:domain rdf:resource="http://w3id.org/meta-share/meta-share/ToolService"/>
        <rdfs:range rdf:resource="http://w3id.org/meta-share/meta-share/TRL"/>
        <rdfs:altLabel xml:lang="en">Technology Readiness Level</rdfs:altLabel>
        <rdfs:comment xml:lang="en">Specifies the TRL (Technology Readiness Level) of the technology according to the measurement system defined by the EC</rdfs:comment>
        <rdfs:label xml:lang="en">TRL</rdfs:label>
    </owl:ObjectProperty>
    


    <!-- http://w3id.org/meta-share/meta-share/typesystem -->

    <owl:ObjectProperty rdf:about="http://w3id.org/meta-share/meta-share/typesystem">
        <rdfs:subPropertyOf rdf:resource="http://w3id.org/meta-share/meta-share/dependsOn"/>
        <rdfs:domain>
            <owl:Class>
                <owl:unionOf rdf:parseType="Collection">
                    <rdf:Description rdf:about="http://w3id.org/meta-share/meta-share/MLModel"/>
                    <rdf:Description rdf:about="http://w3id.org/meta-share/meta-share/ProcessingResource"/>
                    <rdf:Description rdf:about="http://w3id.org/meta-share/meta-share/ToolService"/>
                </owl:unionOf>
            </owl:Class>
        </rdfs:domain>
        <rdfs:range rdf:resource="http://w3id.org/meta-share/meta-share/LexicalConceptualResource"/>
        <rdfs:comment xml:lang="en">Specifies the typesystem (preferrably through an identifier or URL) that has been used for the annotation of a resource or that is required for the input resource of a tool/service or that should be used (dependency) for the annotation or used in the training of a ML model</rdfs:comment>
        <rdfs:label xml:lang="en">typesystem</rdfs:label>
    </owl:ObjectProperty>
    


    <!-- http://w3id.org/meta-share/meta-share/usageProject -->

    <owl:ObjectProperty rdf:about="http://w3id.org/meta-share/meta-share/usageProject">
        <rdfs:subPropertyOf rdf:resource="http://w3id.org/meta-share/meta-share/isRelatedToProject"/>
        <rdfs:domain rdf:resource="http://w3id.org/meta-share/meta-share/ActualUse"/>
        <rdfs:range rdf:resource="http://w3id.org/meta-share/meta-share/Project"/>
        <rdfs:comment xml:lang="en">Links to a project in which the language resource has been used</rdfs:comment>
        <rdfs:label xml:lang="en">usage project</rdfs:label>
    </owl:ObjectProperty>
    


    <!-- http://w3id.org/meta-share/meta-share/usageReport -->

    <owl:ObjectProperty rdf:about="http://w3id.org/meta-share/meta-share/usageReport">
        <rdfs:subPropertyOf rdf:resource="http://w3id.org/meta-share/meta-share/isDocumentedBy"/>
        <rdfs:domain rdf:resource="http://w3id.org/meta-share/meta-share/ActualUse"/>
        <rdfs:range rdf:resource="http://w3id.org/meta-share/meta-share/Document"/>
        <rdfs:comment xml:lang="en">Links to a document (e.g.,  research article, report) describing a project, application, experiment or use case where the language resource has been used</rdfs:comment>
        <rdfs:label xml:lang="en">usage report</rdfs:label>
    </owl:ObjectProperty>
    


    <!-- http://w3id.org/meta-share/meta-share/usedInApplication -->

    <owl:ObjectProperty rdf:about="http://w3id.org/meta-share/meta-share/usedInApplication">
        <rdfs:domain rdf:resource="http://w3id.org/meta-share/meta-share/ActualUse"/>
        <rdfs:range rdf:resource="http://w3id.org/meta-share/omtd-share/Operation"/>
        <rdfs:comment xml:lang="en">Specifies an LT application where the language resource has been used in</rdfs:comment>
        <rdfs:label xml:lang="en">used in application</rdfs:label>
    </owl:ObjectProperty>
    


    <!-- http://w3id.org/meta-share/meta-share/userType -->

    <owl:ObjectProperty rdf:about="http://w3id.org/meta-share/meta-share/userType">
        <rdfs:domain rdf:resource="http://w3id.org/meta-share/meta-share/Distribution"/>
        <rdfs:range rdf:resource="http://w3id.org/meta-share/meta-share/UserType"/>
        <rdfs:comment xml:lang="en">Used to identify the type of user of the resource (affiliated with a commercial vs. academic institution); it is usually associated with licensing or pricing conditions on the use of a resource</rdfs:comment>
        <rdfs:label xml:lang="en">user type</rdfs:label>
    </owl:ObjectProperty>
    


    <!-- http://w3id.org/meta-share/meta-share/validation -->

    <owl:ObjectProperty rdf:about="http://w3id.org/meta-share/meta-share/validation">
        <rdfs:domain rdf:resource="http://w3id.org/meta-share/meta-share/LanguageResource"/>
        <rdfs:range rdf:resource="http://w3id.org/meta-share/meta-share/Validation"/>
        <rdfs:comment xml:lang="en">Provides information on each of the the validation procedure(s) a language resource may have undergone (e.g.,  formal validation of the whole resource, content validation of one part of the resource , etc.).</rdfs:comment>
        <rdfs:label xml:lang="en">validation</rdfs:label>
    </owl:ObjectProperty>
    


    <!-- http://w3id.org/meta-share/meta-share/validationExtent -->

    <owl:ObjectProperty rdf:about="http://w3id.org/meta-share/meta-share/validationExtent">
        <rdfs:domain rdf:resource="http://w3id.org/meta-share/meta-share/Validation"/>
        <rdfs:range rdf:resource="http://w3id.org/meta-share/meta-share/ValidationExtent"/>
        <rdfs:comment xml:lang="en">Specifies the coverage of the language resource that has been validated</rdfs:comment>
        <rdfs:label xml:lang="en">validation extent</rdfs:label>
    </owl:ObjectProperty>
    


    <!-- http://w3id.org/meta-share/meta-share/validationMode -->

    <owl:ObjectProperty rdf:about="http://w3id.org/meta-share/meta-share/validationMode">
        <rdfs:subPropertyOf rdf:resource="http://w3id.org/meta-share/meta-share/processMode"/>
        <rdfs:domain rdf:resource="http://w3id.org/meta-share/meta-share/Validation"/>
        <rdfs:range rdf:resource="http://w3id.org/meta-share/meta-share/ProcessMode"/>
        <rdfs:comment xml:lang="en">Specifies the type of processing applied for the validation of the language resource</rdfs:comment>
        <rdfs:label xml:lang="en">validation mode</rdfs:label>
    </owl:ObjectProperty>
    


    <!-- http://w3id.org/meta-share/meta-share/validationReport -->

    <owl:ObjectProperty rdf:about="http://w3id.org/meta-share/meta-share/validationReport">
        <rdfs:subPropertyOf rdf:resource="http://w3id.org/meta-share/meta-share/isDocumentedBy"/>
        <rdfs:domain rdf:resource="http://w3id.org/meta-share/meta-share/Validation"/>
        <rdfs:range rdf:resource="http://w3id.org/meta-share/meta-share/Document"/>
        <rdfs:comment xml:lang="en">Links to a document with detailed information on the validation process and results</rdfs:comment>
        <rdfs:label xml:lang="en">validation report</rdfs:label>
    </owl:ObjectProperty>
    


    <!-- http://w3id.org/meta-share/meta-share/validationType -->

    <owl:ObjectProperty rdf:about="http://w3id.org/meta-share/meta-share/validationType">
        <rdfs:domain rdf:resource="http://w3id.org/meta-share/meta-share/Validation"/>
        <rdfs:range rdf:resource="http://w3id.org/meta-share/meta-share/ValidationType"/>
        <rdfs:comment xml:lang="en">Specifies the type of validation that has been performed on a language resource</rdfs:comment>
        <rdfs:label xml:lang="en">validation type</rdfs:label>
    </owl:ObjectProperty>
    


    <!-- http://w3id.org/meta-share/meta-share/validator -->

    <owl:ObjectProperty rdf:about="http://w3id.org/meta-share/meta-share/validator">
        <rdfs:subPropertyOf rdf:resource="http://w3id.org/meta-share/meta-share/isRelatedToActor"/>
        <rdfs:domain rdf:resource="http://w3id.org/meta-share/meta-share/Validation"/>
        <rdfs:range rdf:resource="http://w3id.org/meta-share/meta-share/Actor"/>
        <rdfs:comment xml:lang="en">Links a validation to the person(s), group(s) or organization(s) that have performed a specific validation of a language resource</rdfs:comment>
        <rdfs:label xml:lang="en">validator</rdfs:label>
    </owl:ObjectProperty>
    


    <!-- http://w3id.org/meta-share/meta-share/versionType -->

    <owl:ObjectProperty rdf:about="http://w3id.org/meta-share/meta-share/versionType">
        <rdfs:domain>
            <owl:Class>
                <owl:unionOf rdf:parseType="Collection">
                    <rdf:Description rdf:about="http://w3id.org/meta-share/meta-share/Document"/>
                    <rdf:Description rdf:about="http://w3id.org/meta-share/meta-share/LanguageResource"/>
                </owl:unionOf>
            </owl:Class>
        </rdfs:domain>
        <rdfs:range rdf:resource="http://w3id.org/meta-share/meta-share/VersionType"/>
        <rdfs:comment xml:lang="en">Links scholarly works (mainly) to a type of versioning vocabulary related to the publication process</rdfs:comment>
        <rdfs:label xml:lang="en">version type</rdfs:label>
        <skos:note xml:lang="en">If we think this shouldn&apos; be used for LRTs, remove from XSD&apos;s</skos:note>
    </owl:ObjectProperty>
    


    <!-- http://w3id.org/meta-share/meta-share/videoFormat -->

    <owl:ObjectProperty rdf:about="http://w3id.org/meta-share/meta-share/videoFormat">
        <rdfs:domain rdf:resource="http://w3id.org/meta-share/meta-share/DatasetDistribution"/>
        <rdfs:range rdf:resource="http://w3id.org/meta-share/meta-share/VideoFormat"/>
        <rdfs:comment xml:lang="en">Groups information on the format(s) of a resource; repeated if parts of the resource are in different formats</rdfs:comment>
        <rdfs:label xml:lang="en">video format</rdfs:label>
        <skos:note xml:lang="en">see how data formats, audio &amp; video formats will be handled; must be on distribution</skos:note>
    </owl:ObjectProperty>
    


    <!-- http://w3id.org/meta-share/meta-share/visualModelling -->

    <owl:ObjectProperty rdf:about="http://w3id.org/meta-share/meta-share/visualModelling">
        <rdfs:domain>
            <owl:Class>
                <owl:unionOf rdf:parseType="Collection">
                    <rdf:Description rdf:about="http://w3id.org/meta-share/meta-share/ImageFormat"/>
                    <rdf:Description rdf:about="http://w3id.org/meta-share/meta-share/VideoFormat"/>
                </owl:unionOf>
            </owl:Class>
        </rdfs:domain>
        <rdfs:range rdf:resource="http://w3id.org/meta-share/meta-share/VisualModelling"/>
        <rdfs:comment xml:lang="en">Specifies the dimensional form applied on the video or image part(s) of a corpus</rdfs:comment>
        <rdfs:label xml:lang="en">visual modelling</rdfs:label>
    </owl:ObjectProperty>
    


    <!-- http://w3id.org/meta-share/meta-share/vocalTractCondition -->

    <owl:ObjectProperty rdf:about="http://w3id.org/meta-share/meta-share/vocalTractCondition">
        <rdfs:domain rdf:resource="http://w3id.org/meta-share/meta-share/Participant"/>
        <rdfs:range rdf:resource="http://w3id.org/meta-share/meta-share/VocalTractCondition"/>
        <rdfs:comment xml:lang="en">Provides information on the vocal tract conditions that may influence the speech of the participant</rdfs:comment>
        <rdfs:label xml:lang="en">vocal tract condition</rdfs:label>
    </owl:ObjectProperty>
    


    <!-- http://w3id.org/meta-share/meta-share/webServiceType -->

    <owl:ObjectProperty rdf:about="http://w3id.org/meta-share/meta-share/webServiceType">
        <rdfs:domain rdf:resource="http://w3id.org/meta-share/meta-share/SoftwareDistribution"/>
        <rdfs:range rdf:resource="http://w3id.org/meta-share/meta-share/WebServiceType"/>
        <rdfs:comment xml:lang="en">Identifies the type of a web service in accordance to a classification vocabulary that refers to the web service communication protocols</rdfs:comment>
        <rdfs:label xml:lang="en">web service type</rdfs:label>
        <skos:note xml:lang="en">try to restrict with instance &quot;webService&quot; on DistributionForm</skos:note>
    </owl:ObjectProperty>
    


    <!-- http://xmlns.com/foaf/0.1/primaryTopic -->

    <owl:ObjectProperty rdf:about="http://xmlns.com/foaf/0.1/primaryTopic"/>
    


    <!-- 
    ///////////////////////////////////////////////////////////////////////////////////////
    //
    // Data properties
    //
    ///////////////////////////////////////////////////////////////////////////////////////
     -->

    


    <!-- http://purl.org/dc/terms/alternative -->

    <owl:DatatypeProperty rdf:about="http://purl.org/dc/terms/alternative"/>
    


    <!-- http://purl.org/dc/terms/description -->

    <owl:DatatypeProperty rdf:about="http://purl.org/dc/terms/description">
        <rdfs:subPropertyOf rdf:resource="http://www.w3.org/2002/07/owl#topDataProperty"/>
    </owl:DatatypeProperty>
    


    <!-- http://purl.org/dc/terms/hasVersion -->

    <owl:DatatypeProperty rdf:about="http://purl.org/dc/terms/hasVersion"/>
    


    <!-- http://purl.org/dc/terms/issued -->

    <owl:DatatypeProperty rdf:about="http://purl.org/dc/terms/issued"/>
    


    <!-- http://purl.org/dc/terms/title -->

    <owl:DatatypeProperty rdf:about="http://purl.org/dc/terms/title"/>
    


    <!-- http://w3id.org/meta-share/meta-share/abstract -->

    <owl:DatatypeProperty rdf:about="http://w3id.org/meta-share/meta-share/abstract">
        <rdfs:domain rdf:resource="http://w3id.org/meta-share/meta-share/Document"/>
        <rdfs:range rdf:resource="http://www.w3.org/1999/02/22-rdf-syntax-ns#langString"/>
        <rdfs:comment xml:lang="en">Introduces a summary of the contents of a document</rdfs:comment>
        <rdfs:label xml:lang="en">abstract</rdfs:label>
    </owl:DatatypeProperty>
    


    <!-- http://w3id.org/meta-share/meta-share/accessLocation -->

    <owl:DatatypeProperty rdf:about="http://w3id.org/meta-share/meta-share/accessLocation">
        <rdfs:subPropertyOf rdf:resource="http://w3id.org/meta-share/meta-share/distributionLocation"/>
        <rdfs:domain rdf:resource="http://w3id.org/meta-share/meta-share/Distribution"/>
        <rdfs:range rdf:resource="http://www.w3.org/2001/XMLSchema#anyURI"/>
        <rdfs:comment xml:lang="en">A URL where the resource can be accessed from; it can be used for landing pages or for cases where the resource is accessible via an interface, i.e. cases where the resource itself is not provided with a direct link for downloading</rdfs:comment>
        <rdfs:label xml:lang="en">access location</rdfs:label>
    </owl:DatatypeProperty>
    


    <!-- http://w3id.org/meta-share/meta-share/actualUseDetails -->

    <owl:DatatypeProperty rdf:about="http://w3id.org/meta-share/meta-share/actualUseDetails">
        <rdfs:domain rdf:resource="http://w3id.org/meta-share/meta-share/ActualUse"/>
        <rdfs:range rdf:resource="http://www.w3.org/1999/02/22-rdf-syntax-ns#langString"/>
        <rdfs:comment xml:lang="en">Describes in free text specific use cases or situations where the language resource has been used</rdfs:comment>
        <rdfs:label xml:lang="en">actual use details</rdfs:label>
    </owl:DatatypeProperty>
    


    <!-- http://w3id.org/meta-share/meta-share/additionalHWRequirements -->

    <owl:DatatypeProperty rdf:about="http://w3id.org/meta-share/meta-share/additionalHWRequirements">
        <rdfs:domain rdf:resource="http://w3id.org/meta-share/meta-share/SoftwareDistribution"/>
        <rdfs:range rdf:resource="http://www.w3.org/2001/XMLSchema#string"/>
        <rdfs:altLabel xml:lang="en">additional hardware requirements</rdfs:altLabel>
        <rdfs:comment xml:lang="en">Specifies hardware requirements that are needed for running a tool/service</rdfs:comment>
        <rdfs:label xml:lang="en">additional h/w requirements</rdfs:label>
    </owl:DatatypeProperty>
    


    <!-- http://w3id.org/meta-share/meta-share/address -->

    <owl:DatatypeProperty rdf:about="http://w3id.org/meta-share/meta-share/address">
        <rdfs:domain rdf:resource="http://w3id.org/meta-share/meta-share/AddressSet"/>
        <rdfs:range rdf:resource="http://www.w3.org/1999/02/22-rdf-syntax-ns#langString"/>
        <rdfs:comment xml:lang="en">The street and the number of the postal address of a person or organization</rdfs:comment>
        <rdfs:label xml:lang="en">address</rdfs:label>
    </owl:DatatypeProperty>
    


    <!-- http://w3id.org/meta-share/meta-share/age -->

    <owl:DatatypeProperty rdf:about="http://w3id.org/meta-share/meta-share/age">
        <rdfs:domain rdf:resource="http://w3id.org/meta-share/meta-share/Participant"/>
        <rdfs:range rdf:resource="http://www.w3.org/2001/XMLSchema#int"/>
        <rdfs:comment xml:lang="en">Age of a person</rdfs:comment>
        <rdfs:label xml:lang="en">age</rdfs:label>
    </owl:DatatypeProperty>
    


    <!-- http://w3id.org/meta-share/meta-share/ageRangeEndOfParticipants -->

    <owl:DatatypeProperty rdf:about="http://w3id.org/meta-share/meta-share/ageRangeEndOfParticipants">
        <rdfs:domain>
            <owl:Class>
                <owl:unionOf rdf:parseType="Collection">
                    <rdf:Description rdf:about="http://w3id.org/meta-share/meta-share/CorpusAudioPart"/>
                    <rdf:Description rdf:about="http://w3id.org/meta-share/meta-share/CorpusImagePart"/>
                    <rdf:Description rdf:about="http://w3id.org/meta-share/meta-share/CorpusTextNumericalPart"/>
                    <rdf:Description rdf:about="http://w3id.org/meta-share/meta-share/CorpusVideoPart"/>
                </owl:unionOf>
            </owl:Class>
        </rdfs:domain>
        <rdfs:range rdf:resource="http://www.w3.org/2001/XMLSchema#int"/>
        <rdfs:comment xml:lang="en">End of age range of the group of participants</rdfs:comment>
        <rdfs:label xml:lang="en">age range end of participants</rdfs:label>
    </owl:DatatypeProperty>
    


    <!-- http://w3id.org/meta-share/meta-share/ageRangeStartOfParticipants -->

    <owl:DatatypeProperty rdf:about="http://w3id.org/meta-share/meta-share/ageRangeStartOfParticipants">
        <rdfs:domain>
            <owl:Class>
                <owl:unionOf rdf:parseType="Collection">
                    <rdf:Description rdf:about="http://w3id.org/meta-share/meta-share/CorpusAudioPart"/>
                    <rdf:Description rdf:about="http://w3id.org/meta-share/meta-share/CorpusImagePart"/>
                    <rdf:Description rdf:about="http://w3id.org/meta-share/meta-share/CorpusTextNumericalPart"/>
                    <rdf:Description rdf:about="http://w3id.org/meta-share/meta-share/CorpusVideoPart"/>
                </owl:unionOf>
            </owl:Class>
        </rdfs:domain>
        <rdfs:range rdf:resource="http://www.w3.org/2001/XMLSchema#int"/>
        <rdfs:comment xml:lang="en">Start of age range of the group of participants</rdfs:comment>
        <rdfs:label xml:lang="en">age range start of participants</rdfs:label>
    </owl:DatatypeProperty>
    


    <!-- http://w3id.org/meta-share/meta-share/algorithm -->

    <owl:DatatypeProperty rdf:about="http://w3id.org/meta-share/meta-share/algorithm">
        <rdfs:domain rdf:resource="http://w3id.org/meta-share/meta-share/MLModel"/>
        <rdfs:range rdf:resource="http://www.w3.org/1999/02/22-rdf-syntax-ns#langString"/>
        <rdfs:comment xml:lang="en">Identifies the training algorithm used for the model (e.g.,  maximum entropy, svm, etc.)</rdfs:comment>
        <rdfs:label xml:lang="en">algorithm</rdfs:label>
    </owl:DatatypeProperty>
    


    <!-- http://w3id.org/meta-share/meta-share/algorithmDetails -->

    <owl:DatatypeProperty rdf:about="http://w3id.org/meta-share/meta-share/algorithmDetails">
        <rdfs:domain rdf:resource="http://w3id.org/meta-share/meta-share/MLModel"/>
        <rdfs:range rdf:resource="http://www.w3.org/1999/02/22-rdf-syntax-ns#langString"/>
        <rdfs:comment xml:lang="en">Provides a detailed description of the algorithm, incl. info on whether it&apos;s supervised or not</rdfs:comment>
        <rdfs:label xml:lang="en">algorithm details</rdfs:label>
    </owl:DatatypeProperty>
    


    <!-- http://w3id.org/meta-share/meta-share/alias -->

    <owl:DatatypeProperty rdf:about="http://w3id.org/meta-share/meta-share/alias">
        <rdfs:domain rdf:resource="http://w3id.org/meta-share/meta-share/Participant"/>
        <rdfs:range rdf:resource="http://www.w3.org/1999/02/22-rdf-syntax-ns#langString"/>
        <rdfs:comment xml:lang="en">Introduces a name used for a participant of a multimedia resource instead of his/her real one</rdfs:comment>
        <rdfs:label xml:lang="en">alias</rdfs:label>
    </owl:DatatypeProperty>
    


    <!-- http://w3id.org/meta-share/meta-share/alternativeTitle -->

    <owl:DatatypeProperty rdf:about="http://w3id.org/meta-share/meta-share/alternativeTitle">
        <rdfs:subPropertyOf rdf:resource="http://purl.org/dc/terms/alternative"/>
        <rdfs:domain rdf:resource="http://w3id.org/meta-share/meta-share/Document"/>
        <rdfs:range rdf:resource="http://www.w3.org/1999/02/22-rdf-syntax-ns#langString"/>
        <rdfs:comment xml:lang="en">Introduces an alternative title (e.g. short title) used for the document being described</rdfs:comment>
        <rdfs:label xml:lang="en">alternative title</rdfs:label>
    </owl:DatatypeProperty>
    


    <!-- http://w3id.org/meta-share/meta-share/amount -->

    <owl:DatatypeProperty rdf:about="http://w3id.org/meta-share/meta-share/amount">
        <rdfs:domain>
            <owl:Class>
                <owl:unionOf rdf:parseType="Collection">
                    <rdf:Description rdf:about="http://w3id.org/meta-share/meta-share/Cost"/>
                    <rdf:Description rdf:about="http://w3id.org/meta-share/meta-share/Size"/>
                </owl:unionOf>
            </owl:Class>
        </rdfs:domain>
        <rdfs:range rdf:resource="http://www.w3.org/2001/XMLSchema#float"/>
        <rdfs:comment xml:lang="en">Specifies the number of units that constitute anything that can be measured (e.g. size of a data resource or cost, etc.)</rdfs:comment>
        <rdfs:label xml:lang="en">amount</rdfs:label>
    </owl:DatatypeProperty>
    


    <!-- http://w3id.org/meta-share/meta-share/annotationEndDate -->

    <owl:DatatypeProperty rdf:about="http://w3id.org/meta-share/meta-share/annotationEndDate">
        <rdfs:domain rdf:resource="http://w3id.org/meta-share/meta-share/Annotation"/>
        <rdfs:range rdf:resource="http://www.w3.org/2001/XMLSchema#date"/>
        <rdfs:comment xml:lang="en">The date in which the annotation process has ended</rdfs:comment>
        <rdfs:label xml:lang="en">annotation end date</rdfs:label>
    </owl:DatatypeProperty>
    


    <!-- http://w3id.org/meta-share/meta-share/annotationModeDetails -->

    <owl:DatatypeProperty rdf:about="http://w3id.org/meta-share/meta-share/annotationModeDetails">
        <rdfs:domain rdf:resource="http://w3id.org/meta-share/meta-share/Annotation"/>
        <rdfs:range rdf:resource="http://www.w3.org/1999/02/22-rdf-syntax-ns#langString"/>
        <rdfs:comment xml:lang="en">Provides further information on annotation process </rdfs:comment>
        <rdfs:label xml:lang="en">annotation mode details</rdfs:label>
    </owl:DatatypeProperty>
    


    <!-- http://w3id.org/meta-share/meta-share/annotationStandoff -->

    <owl:DatatypeProperty rdf:about="http://w3id.org/meta-share/meta-share/annotationStandoff">
        <rdfs:domain rdf:resource="http://w3id.org/meta-share/meta-share/Annotation"/>
        <rdfs:range rdf:resource="http://www.w3.org/2001/XMLSchema#boolean"/>
        <rdfs:comment xml:lang="en">Indicates whether the annotation is created inline or in a stand-off fashion</rdfs:comment>
        <rdfs:label xml:lang="en">annotation standoff</rdfs:label>
    </owl:DatatypeProperty>
    


    <!-- http://w3id.org/meta-share/meta-share/annotationStartDate -->

    <owl:DatatypeProperty rdf:about="http://w3id.org/meta-share/meta-share/annotationStartDate">
        <rdfs:domain rdf:resource="http://w3id.org/meta-share/meta-share/Annotation"/>
        <rdfs:range rdf:resource="http://www.w3.org/2001/XMLSchema#date"/>
        <rdfs:comment xml:lang="en">The date in which the annotation process has started</rdfs:comment>
        <rdfs:label xml:lang="en">annotation start date</rdfs:label>
    </owl:DatatypeProperty>
    


    <!-- http://w3id.org/meta-share/meta-share/anonymizationDetails -->

    <owl:DatatypeProperty rdf:about="http://w3id.org/meta-share/meta-share/anonymizationDetails">
        <rdfs:domain rdf:resource="http://w3id.org/meta-share/meta-share/DataLanguageResource"/>
        <rdfs:range rdf:resource="http://www.w3.org/1999/02/22-rdf-syntax-ns#langString"/>
        <rdfs:comment xml:lang="en">If the resource has been anonymized, this field can be used for entering more information, e.g.,  tool or method used for the anonymization, by whom it has been performed, whether there was any check of the results , etc.</rdfs:comment>
        <rdfs:label xml:lang="en">anonymization details</rdfs:label>
    </owl:DatatypeProperty>
    


    <!-- http://w3id.org/meta-share/meta-share/anonymized -->

    <owl:DatatypeProperty rdf:about="http://w3id.org/meta-share/meta-share/anonymized">
        <rdfs:domain rdf:resource="http://w3id.org/meta-share/meta-share/DataLanguageResource"/>
        <rdfs:range rdf:resource="http://www.w3.org/2001/XMLSchema#boolean"/>
        <rdfs:comment xml:lang="en">Indicates whether the language resource has been anonymized</rdfs:comment>
        <rdfs:label xml:lang="en">anonymized</rdfs:label>
    </owl:DatatypeProperty>
    


    <!-- http://w3id.org/meta-share/meta-share/artifactPart -->

    <owl:DatatypeProperty rdf:about="http://w3id.org/meta-share/meta-share/artifactPart">
        <rdfs:domain rdf:resource="http://w3id.org/meta-share/meta-share/StaticElement"/>
        <rdfs:range rdf:resource="http://www.w3.org/1999/02/22-rdf-syntax-ns#langString"/>
        <rdfs:comment xml:lang="en">Indicates the parts of the artifacts represented in the image corpus</rdfs:comment>
        <rdfs:label xml:lang="en">artifact part</rdfs:label>
    </owl:DatatypeProperty>
    


    <!-- http://w3id.org/meta-share/meta-share/attachedLexiconPosition -->

    <owl:DatatypeProperty rdf:about="http://w3id.org/meta-share/meta-share/attachedLexiconPosition">
        <rdfs:domain rdf:resource="http://w3id.org/meta-share/meta-share/LanguageDescription"/>
        <rdfs:range rdf:resource="http://www.w3.org/1999/02/22-rdf-syntax-ns#langString"/>
        <rdfs:comment xml:lang="en">Indicates the position of the lexicon, if attached to the grammar</rdfs:comment>
        <rdfs:label xml:lang="en">attached lexicon position</rdfs:label>
    </owl:DatatypeProperty>
    


    <!-- http://w3id.org/meta-share/meta-share/attributionText -->

    <owl:DatatypeProperty rdf:about="http://w3id.org/meta-share/meta-share/attributionText">
        <rdfs:domain rdf:resource="http://w3id.org/meta-share/meta-share/Distribution"/>
        <rdfs:range rdf:resource="http://www.w3.org/1999/02/22-rdf-syntax-ns#langString"/>
        <rdfs:comment xml:lang="en">The text that must be quoted for attribution purposes when using a resource - for cases where a resource is provided with a restriction on attribution</rdfs:comment>
        <rdfs:label xml:lang="en">attribution text</rdfs:label>
    </owl:DatatypeProperty>
    


    <!-- http://w3id.org/meta-share/meta-share/availabilityEndDate -->

    <owl:DatatypeProperty rdf:about="http://w3id.org/meta-share/meta-share/availabilityEndDate">
        <rdfs:domain rdf:resource="http://w3id.org/meta-share/meta-share/Distribution"/>
        <rdfs:range rdf:resource="http://www.w3.org/2001/XMLSchema#date"/>
        <rdfs:comment xml:lang="en">Specifies the end date of availability of a resource - only for cases where a resource is available for a restricted time period.</rdfs:comment>
        <rdfs:label xml:lang="en">availability end date</rdfs:label>
    </owl:DatatypeProperty>
    


    <!-- http://w3id.org/meta-share/meta-share/availabilityStartDate -->

    <owl:DatatypeProperty rdf:about="http://w3id.org/meta-share/meta-share/availabilityStartDate">
        <rdfs:domain rdf:resource="http://w3id.org/meta-share/meta-share/Distribution"/>
        <rdfs:range rdf:resource="http://www.w3.org/2001/XMLSchema#date"/>
        <rdfs:comment xml:lang="en">Specifies the start date of availability of a resource - only for cases where a resource is available for a restricted time period.</rdfs:comment>
        <rdfs:label xml:lang="en">availability start date</rdfs:label>
    </owl:DatatypeProperty>
    


    <!-- http://w3id.org/meta-share/meta-share/bibliographicRecord -->

    <owl:DatatypeProperty rdf:about="http://w3id.org/meta-share/meta-share/bibliographicRecord">
        <rdfs:domain rdf:resource="http://w3id.org/meta-share/meta-share/Document"/>
        <rdfs:range rdf:resource="http://www.w3.org/2001/XMLSchema#string"/>
        <rdfs:comment xml:lang="en">Specifies in the form of free text a set of bibliographic data (a bibliographic record) preferrably in bibtex form</rdfs:comment>
        <rdfs:label xml:lang="en">bibliographic record</rdfs:label>
    </owl:DatatypeProperty>
    


    <!-- http://w3id.org/meta-share/meta-share/bodyMovement -->

    <owl:DatatypeProperty rdf:about="http://w3id.org/meta-share/meta-share/bodyMovement">
        <rdfs:domain rdf:resource="http://w3id.org/meta-share/meta-share/DynamicElement"/>
        <rdfs:range rdf:resource="http://www.w3.org/1999/02/22-rdf-syntax-ns#langString"/>
        <rdfs:comment xml:lang="en">Indicates the body parts that move in the video part of the resource</rdfs:comment>
        <rdfs:label xml:lang="en">body movement</rdfs:label>
    </owl:DatatypeProperty>
    


    <!-- http://w3id.org/meta-share/meta-share/bookTitle -->

    <owl:DatatypeProperty rdf:about="http://w3id.org/meta-share/meta-share/bookTitle">
        <rdfs:subPropertyOf rdf:resource="http://purl.org/dc/terms/title"/>
        <rdfs:domain rdf:resource="http://w3id.org/meta-share/meta-share/Document"/>
        <rdfs:range rdf:resource="http://www.w3.org/1999/02/22-rdf-syntax-ns#langString"/>
        <rdfs:comment xml:lang="en">Introduces the human readable text that is used as the title of a book (differentiating from the title of an article)</rdfs:comment>
        <rdfs:label xml:lang="en">book title</rdfs:label>
    </owl:DatatypeProperty>
    


    <!-- http://w3id.org/meta-share/meta-share/capturingDetails -->

    <owl:DatatypeProperty rdf:about="http://w3id.org/meta-share/meta-share/capturingDetails">
        <rdfs:domain>
            <owl:Class>
                <owl:unionOf rdf:parseType="Collection">
                    <rdf:Description rdf:about="http://w3id.org/meta-share/meta-share/CorpusAudioPart"/>
                    <rdf:Description rdf:about="http://w3id.org/meta-share/meta-share/CorpusImagePart"/>
                    <rdf:Description rdf:about="http://w3id.org/meta-share/meta-share/CorpusTextNumericalPart"/>
                    <rdf:Description rdf:about="http://w3id.org/meta-share/meta-share/CorpusVideoPart"/>
                </owl:unionOf>
            </owl:Class>
        </rdfs:domain>
        <rdfs:range rdf:resource="http://www.w3.org/1999/02/22-rdf-syntax-ns#langString"/>
        <rdfs:comment xml:lang="en">Provides further information on the capturing method and procedure</rdfs:comment>
        <rdfs:label xml:lang="en">capturing details</rdfs:label>
    </owl:DatatypeProperty>
    


    <!-- http://w3id.org/meta-share/meta-share/capturingDeviceTypeDetails -->

    <owl:DatatypeProperty rdf:about="http://w3id.org/meta-share/meta-share/capturingDeviceTypeDetails">
        <rdfs:domain>
            <owl:Class>
                <owl:unionOf rdf:parseType="Collection">
                    <rdf:Description rdf:about="http://w3id.org/meta-share/meta-share/CorpusAudioPart"/>
                    <rdf:Description rdf:about="http://w3id.org/meta-share/meta-share/CorpusImagePart"/>
                    <rdf:Description rdf:about="http://w3id.org/meta-share/meta-share/CorpusTextNumericalPart"/>
                    <rdf:Description rdf:about="http://w3id.org/meta-share/meta-share/CorpusVideoPart"/>
                </owl:unionOf>
            </owl:Class>
        </rdfs:domain>
        <rdfs:range rdf:resource="http://www.w3.org/1999/02/22-rdf-syntax-ns#langString"/>
        <rdfs:comment xml:lang="en">Provides further information on the capturing device</rdfs:comment>
        <rdfs:label xml:lang="en">capturing device type details</rdfs:label>
    </owl:DatatypeProperty>
    


    <!-- http://w3id.org/meta-share/meta-share/categoryLabel -->

    <owl:DatatypeProperty rdf:about="http://w3id.org/meta-share/meta-share/categoryLabel">
        <rdfs:subPropertyOf rdf:resource="http://purl.org/dc/terms/title"/>
        <rdfs:domain rdf:resource="http://w3id.org/meta-share/meta-share/Classification"/>
        <rdfs:range rdf:resource="http://www.w3.org/1999/02/22-rdf-syntax-ns#langString"/>
        <rdfs:comment xml:lang="en">Introduces a human readable name (label) by which a classification category (e.g. text type, text genre, domain, etc.) is known</rdfs:comment>
        <rdfs:label xml:lang="en">category label</rdfs:label>
    </owl:DatatypeProperty>
    


    <!-- http://w3id.org/meta-share/meta-share/citationText -->

    <owl:DatatypeProperty rdf:about="http://w3id.org/meta-share/meta-share/citationText">
        <rdfs:domain rdf:resource="http://w3id.org/meta-share/meta-share/LanguageResource"/>
        <rdfs:range rdf:resource="http://www.w3.org/1999/02/22-rdf-syntax-ns#langString"/>
        <rdfs:comment xml:lang="en">The text that must be quoted for citation purposes when using a resource</rdfs:comment>
        <rdfs:label xml:lang="en">citation text</rdfs:label>
    </owl:DatatypeProperty>
    


    <!-- http://w3id.org/meta-share/meta-share/city -->

    <owl:DatatypeProperty rdf:about="http://w3id.org/meta-share/meta-share/city">
        <rdfs:domain rdf:resource="http://w3id.org/meta-share/meta-share/AddressSet"/>
        <rdfs:range rdf:resource="http://www.w3.org/1999/02/22-rdf-syntax-ns#langString"/>
        <rdfs:comment xml:lang="en">The name of the city, town or village as mentioned in the postal address of a person or organization </rdfs:comment>
        <rdfs:label xml:lang="en">city</rdfs:label>
    </owl:DatatypeProperty>
    


    <!-- http://w3id.org/meta-share/meta-share/colourDepth -->

    <owl:DatatypeProperty rdf:about="http://w3id.org/meta-share/meta-share/colourDepth">
        <rdfs:domain>
            <owl:Class>
                <owl:unionOf rdf:parseType="Collection">
                    <rdf:Description rdf:about="http://w3id.org/meta-share/meta-share/ImageFormat"/>
                    <rdf:Description rdf:about="http://w3id.org/meta-share/meta-share/VideoFormat"/>
                </owl:unionOf>
            </owl:Class>
        </rdfs:domain>
        <rdfs:range rdf:resource="http://www.w3.org/2001/XMLSchema#int"/>
        <rdfs:comment xml:lang="en">The number of bits used to represent the colour of a single pixel</rdfs:comment>
        <rdfs:label xml:lang="en">colour depth</rdfs:label>
    </owl:DatatypeProperty>
    


    <!-- http://w3id.org/meta-share/meta-share/command -->

    <owl:DatatypeProperty rdf:about="http://w3id.org/meta-share/meta-share/command">
        <rdfs:domain rdf:resource="http://w3id.org/meta-share/meta-share/SoftwareDistribution"/>
        <rdfs:range rdf:resource="http://www.w3.org/2001/XMLSchema#string"/>
        <rdfs:comment xml:lang="en">Specifies a command line used to invoke a software component</rdfs:comment>
        <rdfs:label xml:lang="en">command</rdfs:label>
    </owl:DatatypeProperty>
    


    <!-- http://w3id.org/meta-share/meta-share/compressed -->

    <owl:DatatypeProperty rdf:about="http://w3id.org/meta-share/meta-share/compressed">
        <rdfs:domain>
            <owl:Class>
                <owl:unionOf rdf:parseType="Collection">
                    <rdf:Description rdf:about="http://w3id.org/meta-share/meta-share/AudioFormat"/>
                    <rdf:Description rdf:about="http://w3id.org/meta-share/meta-share/ImageFormat"/>
                    <rdf:Description rdf:about="http://w3id.org/meta-share/meta-share/VideoFormat"/>
                </owl:unionOf>
            </owl:Class>
        </rdfs:domain>
        <rdfs:range rdf:resource="http://www.w3.org/2001/XMLSchema#boolean"/>
        <rdfs:comment xml:lang="en">Whether the audio, video or image is compressed or not</rdfs:comment>
        <rdfs:label xml:lang="en">compressed</rdfs:label>
    </owl:DatatypeProperty>
    


    <!-- http://w3id.org/meta-share/meta-share/compressionLoss -->

    <owl:DatatypeProperty rdf:about="http://w3id.org/meta-share/meta-share/compressionLoss">
        <rdfs:domain>
            <owl:Class>
                <owl:unionOf rdf:parseType="Collection">
                    <rdf:Description rdf:about="http://w3id.org/meta-share/meta-share/AudioFormat"/>
                    <rdf:Description rdf:about="http://w3id.org/meta-share/meta-share/ImageFormat"/>
                    <rdf:Description rdf:about="http://w3id.org/meta-share/meta-share/VideoFormat"/>
                </owl:unionOf>
            </owl:Class>
        </rdfs:domain>
        <rdfs:range rdf:resource="http://www.w3.org/2001/XMLSchema#boolean"/>
        <rdfs:comment xml:lang="en">Whether there is loss due to compression</rdfs:comment>
        <rdfs:label xml:lang="en">compression loss</rdfs:label>
    </owl:DatatypeProperty>
    


    <!-- http://w3id.org/meta-share/meta-share/conference -->

    <owl:DatatypeProperty rdf:about="http://w3id.org/meta-share/meta-share/conference">
        <rdfs:domain rdf:resource="http://w3id.org/meta-share/meta-share/Document"/>
        <rdfs:range rdf:resource="http://www.w3.org/1999/02/22-rdf-syntax-ns#langString"/>
        <rdfs:comment xml:lang="en">Introduces the name of the conference where the document being described was presented</rdfs:comment>
        <rdfs:label xml:lang="en">conference</rdfs:label>
    </owl:DatatypeProperty>
    


    <!-- http://w3id.org/meta-share/meta-share/copyrightStatement -->

    <owl:DatatypeProperty rdf:about="http://w3id.org/meta-share/meta-share/copyrightStatement">
        <rdfs:domain rdf:resource="http://w3id.org/meta-share/meta-share/Distribution"/>
        <rdfs:range rdf:resource="http://www.w3.org/1999/02/22-rdf-syntax-ns#langString"/>
        <rdfs:comment xml:lang="en">Introduces a free text statement that may be included with the language resource, usually containing the name(s) of copyright holders and licensing terms</rdfs:comment>
        <rdfs:label xml:lang="en">copyright notice</rdfs:label>
    </owl:DatatypeProperty>
    


    <!-- http://w3id.org/meta-share/meta-share/creationDetails -->

    <owl:DatatypeProperty rdf:about="http://w3id.org/meta-share/meta-share/creationDetails">
        <rdfs:domain>
            <owl:Class>
                <owl:unionOf rdf:parseType="Collection">
                    <rdf:Description rdf:about="http://w3id.org/meta-share/meta-share/LexicalConceptualResource"/>
                    <rdf:Description rdf:about="http://w3id.org/meta-share/meta-share/MediaPart"/>
                </owl:unionOf>
            </owl:Class>
        </rdfs:domain>
        <rdfs:range rdf:resource="http://www.w3.org/1999/02/22-rdf-syntax-ns#langString"/>
        <rdfs:comment xml:lang="en">Provides additional information on the creation of a language resource</rdfs:comment>
        <rdfs:label xml:lang="en">creation details</rdfs:label>
    </owl:DatatypeProperty>
    


    <!-- http://w3id.org/meta-share/meta-share/creationEndDate -->

    <owl:DatatypeProperty rdf:about="http://w3id.org/meta-share/meta-share/creationEndDate">
        <rdfs:domain rdf:resource="http://w3id.org/meta-share/meta-share/LanguageResource"/>
        <rdfs:range rdf:resource="http://www.w3.org/2001/XMLSchema#date"/>
        <rdfs:comment xml:lang="en">The date in which the process of creating a resource was completed</rdfs:comment>
        <rdfs:label xml:lang="en">creation end date</rdfs:label>
    </owl:DatatypeProperty>
    


    <!-- http://w3id.org/meta-share/meta-share/creationStartDate -->

    <owl:DatatypeProperty rdf:about="http://w3id.org/meta-share/meta-share/creationStartDate">
        <rdfs:domain rdf:resource="http://w3id.org/meta-share/meta-share/LanguageResource"/>
        <rdfs:range rdf:resource="http://www.w3.org/2001/XMLSchema#date"/>
        <rdfs:comment xml:lang="en">The date in which the process of creating the resource started</rdfs:comment>
        <rdfs:label xml:lang="en">creation start date</rdfs:label>
        <skos:note xml:lang="en">how do we handle cases where a resource was created, for instance, in 2000? Is this the start or end date?</skos:note>
    </owl:DatatypeProperty>
    


    <!-- http://w3id.org/meta-share/meta-share/defaultValue -->

    <owl:DatatypeProperty rdf:about="http://w3id.org/meta-share/meta-share/defaultValue">
        <rdfs:domain rdf:resource="http://w3id.org/meta-share/meta-share/Parameter"/>
        <rdfs:range rdf:resource="http://www.w3.org/2001/XMLSchema#string"/>
        <rdfs:comment xml:lang="en">Used for parameters that take a list of values in order to indicate the default value(s)</rdfs:comment>
        <rdfs:label xml:lang="en">default value</rdfs:label>
    </owl:DatatypeProperty>
    


    <!-- http://w3id.org/meta-share/meta-share/demoLocation -->

    <owl:DatatypeProperty rdf:about="http://w3id.org/meta-share/meta-share/demoLocation">
        <rdfs:domain rdf:resource="http://w3id.org/meta-share/meta-share/SoftwareDistribution"/>
        <rdfs:range rdf:resource="http://www.w3.org/2001/XMLSchema#anyURI"/>
        <rdfs:comment xml:lang="en">Specifies the URL where a user can access the demo of a tool/service</rdfs:comment>
        <rdfs:label xml:lang="en">demo location</rdfs:label>
    </owl:DatatypeProperty>
    


    <!-- http://w3id.org/meta-share/meta-share/description -->

    <owl:DatatypeProperty rdf:about="http://w3id.org/meta-share/meta-share/description">
        <rdfs:subPropertyOf rdf:resource="http://purl.org/dc/terms/description"/>
        <rdfs:domain rdf:resource="http://w3id.org/meta-share/meta-share/LanguageResource"/>
        <rdfs:range rdf:resource="http://www.w3.org/1999/02/22-rdf-syntax-ns#langString"/>
        <rdfs:comment xml:lang="en">Introduces a short free-text account that provides information about the resource (e.g.,  function, contents, technical information , etc.)</rdfs:comment>
        <rdfs:label xml:lang="en">description</rdfs:label>
        <skos:note xml:lang="en">Add some link to datacite:hasDescription and descriptionType:abstract (always for language resources). The rest of the values of descriptionType make sense mainly for publications, but this handling allows easier extension at a later time.

But note that there is no class datacite:Description; descriptionType is in range of anything that &quot;hasDescriptionType&quot;</skos:note>
    </owl:DatatypeProperty>
    


    <!-- http://w3id.org/meta-share/meta-share/dialectAccent -->

    <owl:DatatypeProperty rdf:about="http://w3id.org/meta-share/meta-share/dialectAccent">
        <rdfs:domain rdf:resource="http://w3id.org/meta-share/meta-share/Participant"/>
        <rdfs:range rdf:resource="http://www.w3.org/1999/02/22-rdf-syntax-ns#langString"/>
        <rdfs:comment xml:lang="en">Provides information on the dialect accent of the participant</rdfs:comment>
        <rdfs:label xml:lang="en">dialect accent</rdfs:label>
    </owl:DatatypeProperty>
    


    <!-- http://w3id.org/meta-share/meta-share/dialectAccentOfParticipants -->

    <owl:DatatypeProperty rdf:about="http://w3id.org/meta-share/meta-share/dialectAccentOfParticipants">
        <rdfs:domain>
            <owl:Class>
                <owl:unionOf rdf:parseType="Collection">
                    <rdf:Description rdf:about="http://w3id.org/meta-share/meta-share/CorpusAudioPart"/>
                    <rdf:Description rdf:about="http://w3id.org/meta-share/meta-share/CorpusImagePart"/>
                    <rdf:Description rdf:about="http://w3id.org/meta-share/meta-share/CorpusTextNumericalPart"/>
                    <rdf:Description rdf:about="http://w3id.org/meta-share/meta-share/CorpusVideoPart"/>
                </owl:unionOf>
            </owl:Class>
        </rdfs:domain>
        <rdfs:range rdf:resource="http://www.w3.org/1999/02/22-rdf-syntax-ns#langString"/>
        <rdfs:comment xml:lang="en">Provides information on the dialect accent of the group of participants</rdfs:comment>
        <rdfs:label xml:lang="en">dialect accent of participants</rdfs:label>
    </owl:DatatypeProperty>
    


    <!-- http://w3id.org/meta-share/meta-share/digest -->

    <owl:DatatypeProperty rdf:about="http://w3id.org/meta-share/meta-share/digest">
        <rdfs:domain rdf:resource="http://w3id.org/meta-share/meta-share/SoftwareDistribution"/>
        <rdfs:range rdf:resource="http://www.w3.org/2001/XMLSchema#string"/>
        <rdfs:comment xml:lang="en">Links a docker image to the sha256 hash (used for selecting the appropriate version)</rdfs:comment>
        <rdfs:label xml:lang="en">digest</rdfs:label>
    </owl:DatatypeProperty>
    


    <!-- http://w3id.org/meta-share/meta-share/discipline -->

    <owl:DatatypeProperty rdf:about="http://w3id.org/meta-share/meta-share/discipline">
        <rdfs:domain>
            <owl:Class>
                <owl:unionOf rdf:parseType="Collection">
                    <rdf:Description rdf:about="http://w3id.org/meta-share/meta-share/Division"/>
                    <rdf:Description rdf:about="http://w3id.org/meta-share/meta-share/Group"/>
                    <rdf:Description rdf:about="http://w3id.org/meta-share/meta-share/Organization"/>
                    <rdf:Description rdf:about="http://w3id.org/meta-share/meta-share/Person"/>
                </owl:unionOf>
            </owl:Class>
        </rdfs:domain>
        <rdfs:range rdf:resource="http://www.w3.org/1999/02/22-rdf-syntax-ns#langString"/>
        <rdfs:altLabel xml:lang="en">area of expertise</rdfs:altLabel>
        <rdfs:altLabel xml:lang="en">research area</rdfs:altLabel>
        <rdfs:comment xml:lang="en">Introduces a field of study or research area that a person or organization is expert in</rdfs:comment>
        <rdfs:label xml:lang="en">discipline</rdfs:label>
    </owl:DatatypeProperty>
    


    <!-- http://w3id.org/meta-share/meta-share/discussionURL -->

    <owl:DatatypeProperty rdf:about="http://w3id.org/meta-share/meta-share/discussionURL">
        <rdfs:domain rdf:resource="http://w3id.org/meta-share/meta-share/LanguageResource"/>
        <rdfs:range rdf:resource="http://www.w3.org/2001/XMLSchema#anyURI"/>
        <rdfs:comment xml:lang="en">Links to a URL where there&apos;s a discussion thread (e.g., user forum) about a resource</rdfs:comment>
        <rdfs:label xml:lang="en">discussion URL</rdfs:label>
    </owl:DatatypeProperty>
    


    <!-- http://w3id.org/meta-share/meta-share/distractor -->

    <owl:DatatypeProperty rdf:about="http://w3id.org/meta-share/meta-share/distractor">
        <rdfs:domain rdf:resource="http://w3id.org/meta-share/meta-share/DynamicElement"/>
        <rdfs:range rdf:resource="http://www.w3.org/1999/02/22-rdf-syntax-ns#langString"/>
        <rdfs:comment xml:lang="en">Identifies any distractors visible in the resource</rdfs:comment>
        <rdfs:label xml:lang="en">distractor</rdfs:label>
    </owl:DatatypeProperty>
    


    <!-- http://w3id.org/meta-share/meta-share/distributionLocation -->

    <owl:DatatypeProperty rdf:about="http://w3id.org/meta-share/meta-share/distributionLocation">
        <rdfs:domain rdf:resource="http://w3id.org/meta-share/meta-share/Distribution"/>
        <rdfs:range rdf:resource="http://www.w3.org/2001/XMLSchema#anyURI"/>
        <rdfs:comment xml:lang="en">A URL point from which a language resource can be directly accessed  (downloaded or executed)</rdfs:comment>
        <rdfs:label xml:lang="en">distribution location</rdfs:label>
    </owl:DatatypeProperty>
    


    <!-- http://w3id.org/meta-share/meta-share/divisionAlternativeName -->

    <owl:DatatypeProperty rdf:about="http://w3id.org/meta-share/meta-share/divisionAlternativeName">
        <rdfs:subPropertyOf rdf:resource="http://purl.org/dc/terms/alternative"/>
        <rdfs:domain rdf:resource="http://w3id.org/meta-share/meta-share/Division"/>
        <rdfs:range rdf:resource="http://www.w3.org/1999/02/22-rdf-syntax-ns#langString"/>
        <rdfs:comment xml:lang="en">Introduces an alternative name (other than the short name) used for a division</rdfs:comment>
        <rdfs:label xml:lang="en">division alternative name</rdfs:label>
    </owl:DatatypeProperty>
    


    <!-- http://w3id.org/meta-share/meta-share/divisionName -->

    <owl:DatatypeProperty rdf:about="http://w3id.org/meta-share/meta-share/divisionName">
        <rdfs:subPropertyOf rdf:resource="http://purl.org/dc/terms/title"/>
        <rdfs:domain rdf:resource="http://w3id.org/meta-share/meta-share/Division"/>
        <rdfs:range rdf:resource="http://www.w3.org/1999/02/22-rdf-syntax-ns#langString"/>
        <rdfs:comment xml:lang="en">The name of the department or unit (e.g.,  specific university faculty/department, department/unit of a research organization or private company , etc.)</rdfs:comment>
        <rdfs:label xml:lang="en">division name</rdfs:label>
    </owl:DatatypeProperty>
    


    <!-- http://w3id.org/meta-share/meta-share/divisionShortName -->

    <owl:DatatypeProperty rdf:about="http://w3id.org/meta-share/meta-share/divisionShortName">
        <rdfs:subPropertyOf rdf:resource="http://purl.org/dc/terms/alternative"/>
        <rdfs:domain rdf:resource="http://w3id.org/meta-share/meta-share/Division"/>
        <rdfs:range rdf:resource="http://www.w3.org/1999/02/22-rdf-syntax-ns#langString"/>
        <rdfs:comment xml:lang="en">Introduces the short name (abbreviation, acronym , etc.) used for the division of an organization</rdfs:comment>
        <rdfs:label xml:lang="en">division short name</rdfs:label>
    </owl:DatatypeProperty>
    


    <!-- http://w3id.org/meta-share/meta-share/dockerDownloadLocation -->

    <owl:DatatypeProperty rdf:about="http://w3id.org/meta-share/meta-share/dockerDownloadLocation">
        <rdfs:subPropertyOf rdf:resource="http://w3id.org/meta-share/meta-share/downloadLocation"/>
        <rdfs:domain rdf:resource="http://w3id.org/meta-share/meta-share/ToolService"/>
        <rdfs:range rdf:resource="http://www.w3.org/2001/XMLSchema#string"/>
        <rdfs:comment xml:lang="en">A location where the software in the form of a docker image can be downloaded from</rdfs:comment>
        <rdfs:label xml:lang="en">docker download location</rdfs:label>
    </owl:DatatypeProperty>
    


    <!-- http://w3id.org/meta-share/meta-share/downloadLocation -->

    <owl:DatatypeProperty rdf:about="http://w3id.org/meta-share/meta-share/downloadLocation">
        <rdfs:subPropertyOf rdf:resource="http://w3id.org/meta-share/meta-share/distributionLocation"/>
        <rdfs:domain rdf:resource="http://w3id.org/meta-share/meta-share/Distribution"/>
        <rdfs:range rdf:resource="http://www.w3.org/2001/XMLSchema#anyURI"/>
        <rdfs:comment xml:lang="en">A URL where the language resource (mainly data but also downloadable software programmes or forms) can be downloaded from</rdfs:comment>
        <rdfs:label xml:lang="en">download location</rdfs:label>
        <skos:note xml:lang="en">rule: must be filled in when SoftwareDistributionForm = downloadable; must not be filled in for web services; optional in all other cases</skos:note>
    </owl:DatatypeProperty>
    


    <!-- http://w3id.org/meta-share/meta-share/edition -->

    <owl:DatatypeProperty rdf:about="http://w3id.org/meta-share/meta-share/edition">
        <rdfs:domain rdf:resource="http://w3id.org/meta-share/meta-share/Document"/>
        <rdfs:range rdf:resource="http://www.w3.org/2001/XMLSchema#string"/>
        <rdfs:comment xml:lang="en">Introduces the number of the edition for the document that has been described</rdfs:comment>
        <rdfs:label xml:lang="en">edition</rdfs:label>
    </owl:DatatypeProperty>
    


    <!-- http://w3id.org/meta-share/meta-share/educationLevel -->

    <owl:DatatypeProperty rdf:about="http://w3id.org/meta-share/meta-share/educationLevel">
        <rdfs:domain rdf:resource="http://w3id.org/meta-share/meta-share/Participant"/>
        <rdfs:range rdf:resource="http://www.w3.org/1999/02/22-rdf-syntax-ns#langString"/>
        <rdfs:comment xml:lang="en">Provides information on the education level of the participant</rdfs:comment>
        <rdfs:label xml:lang="en">education level</rdfs:label>
    </owl:DatatypeProperty>
    


    <!-- http://w3id.org/meta-share/meta-share/email -->

    <owl:DatatypeProperty rdf:about="http://w3id.org/meta-share/meta-share/email">
        <rdfs:domain>
            <owl:Class>
                <owl:unionOf rdf:parseType="Collection">
                    <rdf:Description rdf:about="http://w3id.org/meta-share/meta-share/Affiliation"/>
                    <rdf:Description rdf:about="http://w3id.org/meta-share/meta-share/Division"/>
                    <rdf:Description rdf:about="http://w3id.org/meta-share/meta-share/Group"/>
                    <rdf:Description rdf:about="http://w3id.org/meta-share/meta-share/Organization"/>
                    <rdf:Description rdf:about="http://w3id.org/meta-share/meta-share/Person"/>
                </owl:unionOf>
            </owl:Class>
        </rdfs:domain>
        <rdfs:range rdf:resource="http://www.w3.org/2001/XMLSchema#string"/>
        <rdfs:comment xml:lang="en">Points to the email address of a person, organization or group</rdfs:comment>
        <rdfs:label xml:lang="en">email</rdfs:label>
    </owl:DatatypeProperty>
    


    <!-- http://w3id.org/meta-share/meta-share/evaluated -->

    <owl:DatatypeProperty rdf:about="http://w3id.org/meta-share/meta-share/evaluated">
        <rdfs:domain rdf:resource="http://w3id.org/meta-share/meta-share/ToolService"/>
        <rdfs:range rdf:resource="http://www.w3.org/2001/XMLSchema#boolean"/>
        <rdfs:comment xml:lang="en">Indicates whether the tool or service has been evaluated</rdfs:comment>
        <rdfs:label xml:lang="en">evaluated</rdfs:label>
    </owl:DatatypeProperty>
    


    <!-- http://w3id.org/meta-share/meta-share/evaluationDetails -->

    <owl:DatatypeProperty rdf:about="http://w3id.org/meta-share/meta-share/evaluationDetails">
        <rdfs:domain rdf:resource="http://w3id.org/meta-share/meta-share/Evaluation"/>
        <rdfs:range rdf:resource="http://www.w3.org/1999/02/22-rdf-syntax-ns#langString"/>
        <rdfs:comment xml:lang="en">Provides further information on the evaluation process of a tool or service</rdfs:comment>
        <rdfs:label xml:lang="en">evaluation details</rdfs:label>
    </owl:DatatypeProperty>
    


    <!-- http://w3id.org/meta-share/meta-share/eventDescription -->

    <owl:DatatypeProperty rdf:about="http://w3id.org/meta-share/meta-share/eventDescription">
        <rdfs:domain rdf:resource="http://w3id.org/meta-share/meta-share/StaticElement"/>
        <rdfs:range rdf:resource="http://www.w3.org/1999/02/22-rdf-syntax-ns#langString"/>
        <rdfs:comment xml:lang="en">Provides description of any events represented in the image corpus</rdfs:comment>
        <rdfs:label xml:lang="en">event description</rdfs:label>
    </owl:DatatypeProperty>
    


    <!-- http://w3id.org/meta-share/meta-share/executionLocation -->

    <owl:DatatypeProperty rdf:about="http://w3id.org/meta-share/meta-share/executionLocation">
        <rdfs:subPropertyOf rdf:resource="http://w3id.org/meta-share/meta-share/distributionLocation"/>
        <rdfs:domain rdf:resource="http://w3id.org/meta-share/meta-share/SoftwareDistribution"/>
        <rdfs:range rdf:resource="http://www.w3.org/2001/XMLSchema#anyURI"/>
        <rdfs:comment xml:lang="en">A URL where the resource (mainly software) can be directly executed</rdfs:comment>
        <rdfs:label xml:lang="en">execution location</rdfs:label>
        <skos:note xml:lang="en">rule: must be filled in when SoftwareDistributionMedium = webService; otherwise, not to be filled in</skos:note>
    </owl:DatatypeProperty>
    


    <!-- http://w3id.org/meta-share/meta-share/eyeMovement -->

    <owl:DatatypeProperty rdf:about="http://w3id.org/meta-share/meta-share/eyeMovement">
        <rdfs:domain rdf:resource="http://w3id.org/meta-share/meta-share/DynamicElement"/>
        <rdfs:range rdf:resource="http://www.w3.org/1999/02/22-rdf-syntax-ns#langString"/>
        <rdfs:comment xml:lang="en">Indicates the movement of the eyes visible in the resource</rdfs:comment>
        <rdfs:label xml:lang="en">eye movement</rdfs:label>
    </owl:DatatypeProperty>
    


    <!-- http://w3id.org/meta-share/meta-share/faceExpression -->

    <owl:DatatypeProperty rdf:about="http://w3id.org/meta-share/meta-share/faceExpression">
        <rdfs:domain>
            <owl:Class>
                <owl:unionOf rdf:parseType="Collection">
                    <rdf:Description rdf:about="http://w3id.org/meta-share/meta-share/DynamicElement"/>
                    <rdf:Description rdf:about="http://w3id.org/meta-share/meta-share/StaticElement"/>
                </owl:unionOf>
            </owl:Class>
        </rdfs:domain>
        <rdfs:range rdf:resource="http://www.w3.org/1999/02/22-rdf-syntax-ns#langString"/>
        <rdfs:comment xml:lang="en">Indicates the facial expressions visible in the resource</rdfs:comment>
        <rdfs:label xml:lang="en">face expression</rdfs:label>
    </owl:DatatypeProperty>
    


    <!-- http://w3id.org/meta-share/meta-share/faceView -->

    <owl:DatatypeProperty rdf:about="http://w3id.org/meta-share/meta-share/faceView">
        <rdfs:domain>
            <owl:Class>
                <owl:unionOf rdf:parseType="Collection">
                    <rdf:Description rdf:about="http://w3id.org/meta-share/meta-share/DynamicElement"/>
                    <rdf:Description rdf:about="http://w3id.org/meta-share/meta-share/StaticElement"/>
                </owl:unionOf>
            </owl:Class>
        </rdfs:domain>
        <rdfs:range rdf:resource="http://www.w3.org/1999/02/22-rdf-syntax-ns#langString"/>
        <rdfs:comment xml:lang="en">Indicates the view of the face(s) that appear in the video or on the image part of the resource</rdfs:comment>
        <rdfs:label xml:lang="en">face view</rdfs:label>
    </owl:DatatypeProperty>
    


    <!-- http://w3id.org/meta-share/meta-share/factor -->

    <owl:DatatypeProperty rdf:about="http://w3id.org/meta-share/meta-share/factor">
        <rdfs:domain rdf:resource="http://w3id.org/meta-share/meta-share/NGramModel"/>
        <rdfs:range rdf:resource="http://www.w3.org/2001/XMLSchema#string"/>
        <rdfs:comment xml:lang="en">A factor that has been used for the n-gram resource</rdfs:comment>
        <rdfs:label xml:lang="en">factor</rdfs:label>
    </owl:DatatypeProperty>
    


    <!-- http://w3id.org/meta-share/meta-share/faxNumber -->

    <owl:DatatypeProperty rdf:about="http://w3id.org/meta-share/meta-share/faxNumber">
        <rdfs:domain>
            <owl:Class>
                <owl:unionOf rdf:parseType="Collection">
                    <rdf:Description rdf:about="http://w3id.org/meta-share/meta-share/Division"/>
                    <rdf:Description rdf:about="http://w3id.org/meta-share/meta-share/Group"/>
                    <rdf:Description rdf:about="http://w3id.org/meta-share/meta-share/Organization"/>
                    <rdf:Description rdf:about="http://w3id.org/meta-share/meta-share/Person"/>
                </owl:unionOf>
            </owl:Class>
        </rdfs:domain>
        <rdfs:range rdf:resource="http://www.w3.org/2001/XMLSchema#string"/>
        <rdfs:comment xml:lang="en">The fax number of a person or an organization; recommended format: +_international code_city code_number</rdfs:comment>
        <rdfs:label xml:lang="en">fax number</rdfs:label>
    </owl:DatatypeProperty>
    


    <!-- http://w3id.org/meta-share/meta-share/fee -->

    <owl:DatatypeProperty rdf:about="http://w3id.org/meta-share/meta-share/fee">
        <rdfs:domain rdf:resource="http://w3id.org/meta-share/meta-share/Distribution"/>
        <rdfs:range rdf:resource="http://www.w3.org/1999/02/22-rdf-syntax-ns#langString"/>
        <rdfs:comment xml:lang="en">Describes in free the costs that are required to use the resource, a fragment of the resource or to use a tool or service</rdfs:comment>
        <rdfs:label xml:lang="en">fee</rdfs:label>
        <skos:note>pricing policy can be a more generic concept; discuss if we want to formalise this</skos:note>
    </owl:DatatypeProperty>
    


    <!-- http://w3id.org/meta-share/meta-share/fidelity -->

    <owl:DatatypeProperty rdf:about="http://w3id.org/meta-share/meta-share/fidelity">
        <rdfs:domain rdf:resource="http://w3id.org/meta-share/meta-share/VideoFormat"/>
        <rdfs:range rdf:resource="http://www.w3.org/2001/XMLSchema#boolean"/>
        <rdfs:comment xml:lang="en">Defines whether blur is present in the moving sequences</rdfs:comment>
        <rdfs:label xml:lang="en">fidelity</rdfs:label>
    </owl:DatatypeProperty>
    


    <!-- http://w3id.org/meta-share/meta-share/formalism -->

    <owl:DatatypeProperty rdf:about="http://w3id.org/meta-share/meta-share/formalism">
        <rdfs:domain>
            <owl:Class>
                <owl:unionOf rdf:parseType="Collection">
                    <rdf:Description rdf:about="http://w3id.org/meta-share/meta-share/LanguageDescription"/>
                    <rdf:Description rdf:about="http://w3id.org/meta-share/meta-share/ToolService"/>
                </owl:unionOf>
            </owl:Class>
        </rdfs:domain>
        <rdfs:range rdf:resource="http://www.w3.org/1999/02/22-rdf-syntax-ns#langString"/>
        <rdfs:comment xml:lang="en">Specifies the formalism (bibliographic reference, URL, name) used for the creation/enrichment of the resource (grammar or tool/service)</rdfs:comment>
        <rdfs:label xml:lang="en">formalism</rdfs:label>
    </owl:DatatypeProperty>
    


    <!-- http://w3id.org/meta-share/meta-share/frameRate -->

    <owl:DatatypeProperty rdf:about="http://w3id.org/meta-share/meta-share/frameRate">
        <rdfs:domain rdf:resource="http://w3id.org/meta-share/meta-share/VideoFormat"/>
        <rdfs:range rdf:resource="http://www.w3.org/2001/XMLSchema#int"/>
        <rdfs:comment xml:lang="en">The number of frames per second</rdfs:comment>
        <rdfs:label xml:lang="en">frame rate</rdfs:label>
    </owl:DatatypeProperty>
    


    <!-- http://w3id.org/meta-share/meta-share/fundingSchemeCategory -->

    <owl:DatatypeProperty rdf:about="http://w3id.org/meta-share/meta-share/fundingSchemeCategory">
        <rdfs:domain rdf:resource="http://w3id.org/meta-share/meta-share/Project"/>
        <rdfs:range rdf:resource="http://www.w3.org/2001/XMLSchema#string"/>
        <rdfs:comment xml:lang="en">Introduces a category (usually defined by the funding authority) of the funding scheme to which a project complies</rdfs:comment>
        <rdfs:label xml:lang="en">funding scheme category</rdfs:label>
    </owl:DatatypeProperty>
    


    <!-- http://w3id.org/meta-share/meta-share/geographicCoverage -->

    <owl:DatatypeProperty rdf:about="http://w3id.org/meta-share/meta-share/geographicCoverage">
        <rdfs:domain>
            <owl:Class>
                <owl:unionOf rdf:parseType="Collection">
                    <rdf:Description rdf:about="http://w3id.org/meta-share/meta-share/Corpus"/>
                    <rdf:Description rdf:about="http://w3id.org/meta-share/meta-share/LanguageDescription"/>
                    <rdf:Description rdf:about="http://w3id.org/meta-share/meta-share/LexicalConceptualResource"/>
                    <rdf:Description rdf:about="http://w3id.org/meta-share/meta-share/Subset"/>
                </owl:unionOf>
            </owl:Class>
        </rdfs:domain>
        <rdfs:range rdf:resource="http://www.w3.org/1999/02/22-rdf-syntax-ns#langString"/>
        <rdfs:comment xml:lang="en">Indicates the geographic region that the content of a resource is about; for countries, recommended use of ISO-3166</rdfs:comment>
        <rdfs:label xml:lang="en">geographic coverage</rdfs:label>
        <skos:note xml:lang="en">string or Location (iso3166) and geographic coordinates?</skos:note>
    </owl:DatatypeProperty>
    


    <!-- http://w3id.org/meta-share/meta-share/geographicDistributionOfParticipants -->

    <owl:DatatypeProperty rdf:about="http://w3id.org/meta-share/meta-share/geographicDistributionOfParticipants">
        <rdfs:domain>
            <owl:Class>
                <owl:unionOf rdf:parseType="Collection">
                    <rdf:Description rdf:about="http://w3id.org/meta-share/meta-share/CorpusAudioPart"/>
                    <rdf:Description rdf:about="http://w3id.org/meta-share/meta-share/CorpusImagePart"/>
                    <rdf:Description rdf:about="http://w3id.org/meta-share/meta-share/CorpusTextNumericalPart"/>
                    <rdf:Description rdf:about="http://w3id.org/meta-share/meta-share/CorpusVideoPart"/>
                </owl:unionOf>
            </owl:Class>
        </rdfs:domain>
        <rdfs:range rdf:resource="http://www.w3.org/1999/02/22-rdf-syntax-ns#langString"/>
        <rdfs:comment xml:lang="en">Gives information on the geographic distribution of the participants</rdfs:comment>
        <rdfs:label xml:lang="en">geographic distribution of participants</rdfs:label>
    </owl:DatatypeProperty>
    


    <!-- http://w3id.org/meta-share/meta-share/gesture -->

    <owl:DatatypeProperty rdf:about="http://w3id.org/meta-share/meta-share/gesture">
        <rdfs:domain rdf:resource="http://w3id.org/meta-share/meta-share/DynamicElement"/>
        <rdfs:range rdf:resource="http://www.w3.org/1999/02/22-rdf-syntax-ns#langString"/>
        <rdfs:comment xml:lang="en">Indicates the type of gestures visible in the resource</rdfs:comment>
        <rdfs:label xml:lang="en">gesture</rdfs:label>
    </owl:DatatypeProperty>
    


    <!-- http://w3id.org/meta-share/meta-share/givenName -->

    <owl:DatatypeProperty rdf:about="http://w3id.org/meta-share/meta-share/givenName">
        <rdfs:domain rdf:resource="http://w3id.org/meta-share/meta-share/Person"/>
        <rdfs:range rdf:resource="http://www.w3.org/1999/02/22-rdf-syntax-ns#langString"/>
        <rdfs:altLabel xml:lang="en">first name</rdfs:altLabel>
        <rdfs:altLabel xml:lang="en">forename</rdfs:altLabel>
        <rdfs:comment xml:lang="en">Introduces the given name (also known as &quot;first name&quot;) of a person</rdfs:comment>
        <rdfs:label xml:lang="en">given name</rdfs:label>
    </owl:DatatypeProperty>
    


    <!-- http://w3id.org/meta-share/meta-share/goldStandardLocation -->

    <owl:DatatypeProperty rdf:about="http://w3id.org/meta-share/meta-share/goldStandardLocation">
        <rdfs:subPropertyOf rdf:resource="http://w3id.org/meta-share/meta-share/url"/>
        <rdfs:domain rdf:resource="http://w3id.org/meta-share/meta-share/Evaluation"/>
        <rdfs:range rdf:resource="http://www.w3.org/2001/XMLSchema#anyURI"/>
        <rdfs:comment xml:lang="en">Links to the URL where a gold standard resource can be found in order to be used for evaluation purposes</rdfs:comment>
        <rdfs:label xml:lang="en">gold standard location</rdfs:label>
    </owl:DatatypeProperty>
    


    <!-- http://w3id.org/meta-share/meta-share/grantNumber -->

    <owl:DatatypeProperty rdf:about="http://w3id.org/meta-share/meta-share/grantNumber">
        <rdfs:domain rdf:resource="http://w3id.org/meta-share/meta-share/Project"/>
        <rdfs:range rdf:resource="http://www.w3.org/2001/XMLSchema#string"/>
        <rdfs:comment xml:lang="en">Specifies an identification number usually issued by the funding authority and referring uniquely to the project that has received the funding</rdfs:comment>
        <rdfs:label xml:lang="en">grant number</rdfs:label>
    </owl:DatatypeProperty>
    


    <!-- http://w3id.org/meta-share/meta-share/handArmMovement -->

    <owl:DatatypeProperty rdf:about="http://w3id.org/meta-share/meta-share/handArmMovement">
        <rdfs:domain rdf:resource="http://w3id.org/meta-share/meta-share/DynamicElement"/>
        <rdfs:range rdf:resource="http://www.w3.org/1999/02/22-rdf-syntax-ns#langString"/>
        <rdfs:comment xml:lang="en">Indicates the movement of hands and/or arms visible in the resource</rdfs:comment>
        <rdfs:label xml:lang="en">hand arm movement</rdfs:label>
    </owl:DatatypeProperty>
    


    <!-- http://w3id.org/meta-share/meta-share/handManipulation -->

    <owl:DatatypeProperty rdf:about="http://w3id.org/meta-share/meta-share/handManipulation">
        <rdfs:domain rdf:resource="http://w3id.org/meta-share/meta-share/DynamicElement"/>
        <rdfs:range rdf:resource="http://www.w3.org/1999/02/22-rdf-syntax-ns#langString"/>
        <rdfs:comment xml:lang="en">Gives information on the manipulation of objects by hand</rdfs:comment>
        <rdfs:label xml:lang="en">hand manipulation</rdfs:label>
    </owl:DatatypeProperty>
    


    <!-- http://w3id.org/meta-share/meta-share/headMovement -->

    <owl:DatatypeProperty rdf:about="http://w3id.org/meta-share/meta-share/headMovement">
        <rdfs:domain rdf:resource="http://w3id.org/meta-share/meta-share/DynamicElement"/>
        <rdfs:range rdf:resource="http://www.w3.org/1999/02/22-rdf-syntax-ns#langString"/>
        <rdfs:comment xml:lang="en">Indicates the movements of the head visible in the resource</rdfs:comment>
        <rdfs:label xml:lang="en">head movement</rdfs:label>
    </owl:DatatypeProperty>
    


    <!-- http://w3id.org/meta-share/meta-share/hearingImpairment -->

    <owl:DatatypeProperty rdf:about="http://w3id.org/meta-share/meta-share/hearingImpairment">
        <rdfs:domain rdf:resource="http://w3id.org/meta-share/meta-share/Participant"/>
        <rdfs:range rdf:resource="http://www.w3.org/1999/02/22-rdf-syntax-ns#langString"/>
        <rdfs:comment xml:lang="en">Provides information on any hearing impairment the participant may have</rdfs:comment>
        <rdfs:label xml:lang="en">hearing impairment</rdfs:label>
    </owl:DatatypeProperty>
    


    <!-- http://w3id.org/meta-share/meta-share/height -->

    <owl:DatatypeProperty rdf:about="http://w3id.org/meta-share/meta-share/height">
        <rdfs:domain rdf:resource="http://w3id.org/meta-share/meta-share/Participant"/>
        <rdfs:range rdf:resource="http://www.w3.org/2001/XMLSchema#int"/>
        <rdfs:comment xml:lang="en">Provides information on the height of the participant in cm</rdfs:comment>
        <rdfs:label xml:lang="en">height</rdfs:label>
    </owl:DatatypeProperty>
    


    <!-- http://w3id.org/meta-share/meta-share/homepage -->

    <owl:DatatypeProperty rdf:about="http://w3id.org/meta-share/meta-share/homepage">
        <rdfs:subPropertyOf rdf:resource="http://w3id.org/meta-share/meta-share/url"/>
        <rdfs:domain rdf:resource="http://w3id.org/meta-share/meta-share/Person"/>
        <rdfs:range rdf:resource="http://www.w3.org/2001/XMLSchema#anyURI"/>
        <rdfs:comment xml:lang="en">Links to a URL that includes information on a person (e.g.,  CV, publications, communication information, etc.)</rdfs:comment>
        <rdfs:label xml:lang="en">home page</rdfs:label>
    </owl:DatatypeProperty>
    


    <!-- http://w3id.org/meta-share/meta-share/honorificPrefix -->

    <owl:DatatypeProperty rdf:about="http://w3id.org/meta-share/meta-share/honorificPrefix">
        <rdfs:domain rdf:resource="http://w3id.org/meta-share/meta-share/Person"/>
        <rdfs:range rdf:resource="http://www.w3.org/1999/02/22-rdf-syntax-ns#langString"/>
        <rdfs:altLabel xml:lang="en">title</rdfs:altLabel>
        <rdfs:comment xml:lang="en">Introduces a honorific prefix (or  title) such as Dr./Mr/Ms. that precedes the name of a person</rdfs:comment>
        <rdfs:label xml:lang="en">honorific prefix</rdfs:label>
    </owl:DatatypeProperty>
    


    <!-- http://w3id.org/meta-share/meta-share/image3 -->

    <owl:DatatypeProperty rdf:about="http://w3id.org/meta-share/meta-share/image3">
        <rdfs:domain rdf:resource="http://w3id.org/meta-share/meta-share/Person"/>
        <rdfs:range rdf:resource="http://www.w3.org/2001/XMLSchema#anyURI"/>
        <rdfs:comment xml:lang="en">Links to a URL with an image file (e.g.,  a photo, or cartoon image) that is used for identifying a person (e.g.,  on a home page)</rdfs:comment>
        <rdfs:label xml:lang="en">image</rdfs:label>
    </owl:DatatypeProperty>
    


    <!-- http://w3id.org/meta-share/meta-share/implementationLanguage -->

    <owl:DatatypeProperty rdf:about="http://w3id.org/meta-share/meta-share/implementationLanguage">
        <rdfs:domain rdf:resource="http://w3id.org/meta-share/meta-share/ToolService"/>
        <rdfs:range rdf:resource="http://www.w3.org/2001/XMLSchema#string"/>
        <rdfs:comment xml:lang="en">The programming language(s) used for the development of a tool/service, which is needed for running the tools/services, in case no executables are available</rdfs:comment>
        <rdfs:label xml:lang="en">implementation language</rdfs:label>
    </owl:DatatypeProperty>
    


    <!-- http://w3id.org/meta-share/meta-share/interaction -->

    <owl:DatatypeProperty rdf:about="http://w3id.org/meta-share/meta-share/interaction">
        <rdfs:domain>
            <owl:Class>
                <owl:unionOf rdf:parseType="Collection">
                    <rdf:Description rdf:about="http://w3id.org/meta-share/meta-share/CorpusAudioPart"/>
                    <rdf:Description rdf:about="http://w3id.org/meta-share/meta-share/CorpusVideoPart"/>
                </owl:unionOf>
            </owl:Class>
        </rdfs:domain>
        <rdfs:range rdf:resource="http://www.w3.org/1999/02/22-rdf-syntax-ns#langString"/>
        <rdfs:comment xml:lang="en">Specifies the parts that interact in an audio or video component</rdfs:comment>
        <rdfs:label xml:lang="en">interaction</rdfs:label>
    </owl:DatatypeProperty>
    


    <!-- http://w3id.org/meta-share/meta-share/interactiveMedia -->

    <owl:DatatypeProperty rdf:about="http://w3id.org/meta-share/meta-share/interactiveMedia">
        <rdfs:domain rdf:resource="http://w3id.org/meta-share/meta-share/DynamicElement"/>
        <rdfs:range rdf:resource="http://www.w3.org/1999/02/22-rdf-syntax-ns#langString"/>
        <rdfs:comment xml:lang="en">Any interactive media visible in the resource</rdfs:comment>
        <rdfs:label xml:lang="en">interactive media</rdfs:label>
    </owl:DatatypeProperty>
    


    <!-- http://w3id.org/meta-share/meta-share/interannotatorAgreement -->

    <owl:DatatypeProperty rdf:about="http://w3id.org/meta-share/meta-share/interannotatorAgreement">
        <rdfs:domain rdf:resource="http://w3id.org/meta-share/meta-share/Annotation"/>
        <rdfs:range rdf:resource="http://www.w3.org/1999/02/22-rdf-syntax-ns#langString"/>
        <rdfs:comment xml:lang="en">Provides information on the inter-annotator agreement and the methods/metrics applied</rdfs:comment>
        <rdfs:label xml:lang="en">interannotator agreement</rdfs:label>
    </owl:DatatypeProperty>
    


    <!-- http://w3id.org/meta-share/meta-share/interpolated -->

    <owl:DatatypeProperty rdf:about="http://w3id.org/meta-share/meta-share/interpolated">
        <rdfs:domain rdf:resource="http://w3id.org/meta-share/meta-share/NGramModel"/>
        <rdfs:range rdf:resource="http://www.w3.org/2001/XMLSchema#boolean"/>
        <rdfs:comment xml:lang="en">Specifies whether the n-gram resource is interpolated (Interpolated language models are constructed by 2 or more corpora and each corpus is represented in the model according to a predefined weight)</rdfs:comment>
        <rdfs:label xml:lang="en">interpolated</rdfs:label>
    </owl:DatatypeProperty>
    


    <!-- http://w3id.org/meta-share/meta-share/intraannotatorAgreement -->

    <owl:DatatypeProperty rdf:about="http://w3id.org/meta-share/meta-share/intraannotatorAgreement">
        <rdfs:domain rdf:resource="http://w3id.org/meta-share/meta-share/Annotation"/>
        <rdfs:range rdf:resource="http://www.w3.org/1999/02/22-rdf-syntax-ns#langString"/>
        <rdfs:comment xml:lang="en">Provides information on the intra-annotator agreement and the methods/metrics applied  </rdfs:comment>
        <rdfs:label xml:lang="en">intra-annotator agreement</rdfs:label>
    </owl:DatatypeProperty>
    


    <!-- http://w3id.org/meta-share/meta-share/isFactored -->

    <owl:DatatypeProperty rdf:about="http://w3id.org/meta-share/meta-share/isFactored">
        <rdfs:domain rdf:resource="http://w3id.org/meta-share/meta-share/NGramModel"/>
        <rdfs:range rdf:resource="http://www.w3.org/2001/XMLSchema#boolean"/>
        <rdfs:comment xml:lang="en">Specifies whether the model is factored or not</rdfs:comment>
        <rdfs:label xml:lang="en">is factored</rdfs:label>
    </owl:DatatypeProperty>
    


    <!-- http://w3id.org/meta-share/meta-share/journal -->

    <owl:DatatypeProperty rdf:about="http://w3id.org/meta-share/meta-share/journal">
        <rdfs:domain rdf:resource="http://w3id.org/meta-share/meta-share/Document"/>
        <rdfs:range rdf:resource="http://www.w3.org/1999/02/22-rdf-syntax-ns#langString"/>
        <rdfs:comment xml:lang="en">Introduces the name of the journal where the document being described has been published</rdfs:comment>
        <rdfs:label xml:lang="en">journal</rdfs:label>
    </owl:DatatypeProperty>
    


    <!-- http://w3id.org/meta-share/meta-share/keyword -->

    <owl:DatatypeProperty rdf:about="http://w3id.org/meta-share/meta-share/keyword">
        <rdfs:domain>
            <owl:Class>
                <owl:unionOf rdf:parseType="Collection">
                    <rdf:Description rdf:about="http://w3id.org/meta-share/meta-share/Division"/>
                    <rdf:Description rdf:about="http://w3id.org/meta-share/meta-share/Document"/>
                    <rdf:Description rdf:about="http://w3id.org/meta-share/meta-share/Group"/>
                    <rdf:Description rdf:about="http://w3id.org/meta-share/meta-share/LanguageResource"/>
                    <rdf:Description rdf:about="http://w3id.org/meta-share/meta-share/Organization"/>
                    <rdf:Description rdf:about="http://w3id.org/meta-share/meta-share/Person"/>
                    <rdf:Description rdf:about="http://w3id.org/meta-share/meta-share/Project"/>
                </owl:unionOf>
            </owl:Class>
        </rdfs:domain>
        <rdfs:range rdf:resource="http://www.w3.org/1999/02/22-rdf-syntax-ns#langString"/>
        <rdfs:altLabel xml:lang="en">keyphrase</rdfs:altLabel>
        <rdfs:comment xml:lang="en">Introduces a word or phrase considered important for the description of a language resource, person or organization and thus used to index or classify it</rdfs:comment>
        <rdfs:label xml:lang="en">keyword</rdfs:label>
    </owl:DatatypeProperty>
    


    <!-- http://w3id.org/meta-share/meta-share/landingPage -->

    <owl:DatatypeProperty rdf:about="http://w3id.org/meta-share/meta-share/landingPage">
        <rdfs:subPropertyOf rdf:resource="http://w3id.org/meta-share/meta-share/url"/>
        <rdfs:domain rdf:resource="http://w3id.org/meta-share/meta-share/LanguageResource"/>
        <rdfs:range rdf:resource="http://www.w3.org/2001/XMLSchema#anyURI"/>
        <rdfs:comment xml:lang="en">Links to a web page that provides additional information about a language resource (e.g.,  its contents, acknowledgements, link to the access location, etc.)</rdfs:comment>
        <rdfs:label xml:lang="en">landing page</rdfs:label>
        <skos:note xml:lang="en">dcat:landingPage has range foaf:Document and is a subproperty of foaf:page; no distinction is made between physical and electronic documents. so I&apos;m not sure what the most appropriate relation is for us</skos:note>
    </owl:DatatypeProperty>
    


    <!-- http://w3id.org/meta-share/meta-share/landscapePart -->

    <owl:DatatypeProperty rdf:about="http://w3id.org/meta-share/meta-share/landscapePart">
        <rdfs:domain rdf:resource="http://w3id.org/meta-share/meta-share/StaticElement"/>
        <rdfs:range rdf:resource="http://www.w3.org/1999/02/22-rdf-syntax-ns#langString"/>
        <rdfs:comment xml:lang="en">Indicates the landscape parts represented in the image corpus</rdfs:comment>
        <rdfs:label xml:lang="en">landscape part</rdfs:label>
    </owl:DatatypeProperty>
    


    <!-- http://w3id.org/meta-share/meta-share/language -->

    <owl:DatatypeProperty rdf:about="http://w3id.org/meta-share/meta-share/language">
        <rdfs:domain>
            <owl:Class>
                <owl:unionOf rdf:parseType="Collection">
                    <rdf:Description rdf:about="http://w3id.org/meta-share/meta-share/CorpusAudioPart"/>
                    <rdf:Description rdf:about="http://w3id.org/meta-share/meta-share/CorpusImagePart"/>
                    <rdf:Description rdf:about="http://w3id.org/meta-share/meta-share/CorpusTextPart"/>
                    <rdf:Description rdf:about="http://w3id.org/meta-share/meta-share/CorpusVideoPart"/>
                    <rdf:Description rdf:about="http://w3id.org/meta-share/meta-share/LanguageDescriptionImagePart"/>
                    <rdf:Description rdf:about="http://w3id.org/meta-share/meta-share/LanguageDescriptionTextPart"/>
                    <rdf:Description rdf:about="http://w3id.org/meta-share/meta-share/LanguageDescriptionVideoPart"/>
                    <rdf:Description rdf:about="http://w3id.org/meta-share/meta-share/LexicalConceptualResourceAudioPart"/>
                    <rdf:Description rdf:about="http://w3id.org/meta-share/meta-share/LexicalConceptualResourceImagePart"/>
                    <rdf:Description rdf:about="http://w3id.org/meta-share/meta-share/LexicalConceptualResourceTextPart"/>
                    <rdf:Description rdf:about="http://w3id.org/meta-share/meta-share/LexicalConceptualResourceVideoPart"/>
                </owl:unionOf>
            </owl:Class>
        </rdfs:domain>
        <rdfs:range rdf:resource="http://www.w3.org/2001/XMLSchema#anyURI"/>
        <rdfs:comment xml:lang="en">Specifies the language that is used in the resource or supported by the tool/service</rdfs:comment>
        <rdfs:label xml:lang="en">language</rdfs:label>
        <skos:comment xml:lang="en">in the xsd, we have the full BCP47 recommendation combination, in ontology as a uri (to link with an ontology)</skos:comment>
    </owl:DatatypeProperty>
    


    <!-- http://w3id.org/meta-share/meta-share/languageDependent -->

    <owl:DatatypeProperty rdf:about="http://w3id.org/meta-share/meta-share/languageDependent">
        <rdfs:domain rdf:resource="http://w3id.org/meta-share/meta-share/ToolService"/>
        <rdfs:range rdf:resource="http://www.w3.org/2001/XMLSchema#boolean"/>
        <rdfs:comment xml:lang="en">Indicates whether the operation of the tool or service is language dependent or not</rdfs:comment>
        <rdfs:label xml:lang="en">language dependent</rdfs:label>
    </owl:DatatypeProperty>
    


    <!-- http://w3id.org/meta-share/meta-share/languageVarietyName -->

    <owl:DatatypeProperty rdf:about="http://w3id.org/meta-share/meta-share/languageVarietyName">
        <rdfs:domain rdf:resource="http://w3id.org/meta-share/meta-share/LanguageVariety"/>
        <rdfs:range rdf:resource="http://www.w3.org/1999/02/22-rdf-syntax-ns#langString"/>
        <rdfs:comment xml:lang="en">A textual string used for referring to a language variety</rdfs:comment>
        <rdfs:label xml:lang="en">language variety name</rdfs:label>
    </owl:DatatypeProperty>
    


    <!-- http://w3id.org/meta-share/meta-share/legend -->

    <owl:DatatypeProperty rdf:about="http://w3id.org/meta-share/meta-share/legend">
        <rdfs:domain>
            <owl:Class>
                <owl:unionOf rdf:parseType="Collection">
                    <rdf:Description rdf:about="http://w3id.org/meta-share/meta-share/CorpusAudioPart"/>
                    <rdf:Description rdf:about="http://w3id.org/meta-share/meta-share/LexicalConceptualResourceAudioPart"/>
                </owl:unionOf>
            </owl:Class>
        </rdfs:domain>
        <rdfs:range rdf:resource="http://www.w3.org/1999/02/22-rdf-syntax-ns#langString"/>
        <rdfs:comment xml:lang="en">Introduces the legend of the soundtrack</rdfs:comment>
        <rdfs:label xml:lang="en">legend</rdfs:label>
    </owl:DatatypeProperty>
    


    <!-- http://w3id.org/meta-share/meta-share/licenceTermsAlternativeName -->

    <owl:DatatypeProperty rdf:about="http://w3id.org/meta-share/meta-share/licenceTermsAlternativeName">
        <rdfs:subPropertyOf rdf:resource="http://purl.org/dc/terms/alternative"/>
        <rdfs:domain rdf:resource="http://w3id.org/meta-share/meta-share/LicenceTerms"/>
        <rdfs:range rdf:resource="http://www.w3.org/1999/02/22-rdf-syntax-ns#langString"/>
        <rdfs:comment xml:lang="en">Introduces an alternative name (other than the short name) used for a licence or terms of use</rdfs:comment>
        <rdfs:label xml:lang="en">licence/terms of use/service name</rdfs:label>
    </owl:DatatypeProperty>
    


    <!-- http://w3id.org/meta-share/meta-share/licenceTermsName -->

    <owl:DatatypeProperty rdf:about="http://w3id.org/meta-share/meta-share/licenceTermsName">
        <rdfs:subPropertyOf rdf:resource="http://purl.org/dc/terms/title"/>
        <rdfs:domain rdf:resource="http://w3id.org/meta-share/meta-share/LicenceTerms"/>
        <rdfs:range rdf:resource="http://www.w3.org/1999/02/22-rdf-syntax-ns#langString"/>
        <rdfs:comment xml:lang="en">The name by which a licence/terms of use/service is known</rdfs:comment>
        <rdfs:label xml:lang="en">licence/terms of use/service name</rdfs:label>
    </owl:DatatypeProperty>
    


    <!-- http://w3id.org/meta-share/meta-share/licenceTermsShortName -->

    <owl:DatatypeProperty rdf:about="http://w3id.org/meta-share/meta-share/licenceTermsShortName">
        <rdfs:subPropertyOf rdf:resource="http://purl.org/dc/terms/alternative"/>
        <rdfs:domain rdf:resource="http://w3id.org/meta-share/meta-share/LicenceTerms"/>
        <rdfs:range rdf:resource="http://www.w3.org/1999/02/22-rdf-syntax-ns#langString"/>
        <rdfs:comment xml:lang="en">Introduces the short name (abbreviation, acronym , etc.) used for a licence or terms of use document</rdfs:comment>
        <rdfs:label xml:lang="en">licence/Terms of use/service short name</rdfs:label>
    </owl:DatatypeProperty>
    


    <!-- http://w3id.org/meta-share/meta-share/licenceTermsURL -->

    <owl:DatatypeProperty rdf:about="http://w3id.org/meta-share/meta-share/licenceTermsURL">
        <rdfs:subPropertyOf rdf:resource="http://w3id.org/meta-share/meta-share/url"/>
        <rdfs:domain rdf:resource="http://w3id.org/meta-share/meta-share/LicenceTerms"/>
        <rdfs:range rdf:resource="http://www.w3.org/2001/XMLSchema#anyURI"/>
        <rdfs:comment xml:lang="en">Links to the URL where the text of a licence/terms of use/service is found</rdfs:comment>
        <rdfs:label xml:lang="en">licence/terms of use/service URL</rdfs:label>
    </owl:DatatypeProperty>
    


    <!-- http://w3id.org/meta-share/meta-share/logo -->

    <owl:DatatypeProperty rdf:about="http://w3id.org/meta-share/meta-share/logo">
        <rdfs:domain>
            <owl:Class>
                <owl:unionOf rdf:parseType="Collection">
                    <rdf:Description rdf:about="http://w3id.org/meta-share/meta-share/Division"/>
                    <rdf:Description rdf:about="http://w3id.org/meta-share/meta-share/Group"/>
                    <rdf:Description rdf:about="http://w3id.org/meta-share/meta-share/LanguageResource"/>
                    <rdf:Description rdf:about="http://w3id.org/meta-share/meta-share/LicenceTerms"/>
                    <rdf:Description rdf:about="http://w3id.org/meta-share/meta-share/Organization"/>
                    <rdf:Description rdf:about="http://w3id.org/meta-share/meta-share/Project"/>
                </owl:unionOf>
            </owl:Class>
        </rdfs:domain>
        <rdfs:range rdf:resource="http://www.w3.org/2001/XMLSchema#anyURI"/>
        <rdfs:comment xml:lang="en">Links to a URL with an image file containing a symbol or graphic object used to identify the entity</rdfs:comment>
        <rdfs:label xml:lang="en">logo</rdfs:label>
    </owl:DatatypeProperty>
    


    <!-- http://w3id.org/meta-share/meta-share/mailingListName -->

    <owl:DatatypeProperty rdf:about="http://w3id.org/meta-share/meta-share/mailingListName">
        <rdfs:domain rdf:resource="http://w3id.org/meta-share/meta-share/LanguageResource"/>
        <rdfs:range rdf:resource="http://www.w3.org/2001/XMLSchema#string"/>
        <rdfs:comment xml:lang="en">Indicates the name of a mailing list used in relation to a language resource</rdfs:comment>
        <rdfs:label xml:lang="en">mailing list name</rdfs:label>
    </owl:DatatypeProperty>
    


    <!-- http://w3id.org/meta-share/meta-share/measure -->

    <owl:DatatypeProperty rdf:about="http://w3id.org/meta-share/meta-share/measure">
        <rdfs:domain rdf:resource="http://w3id.org/meta-share/meta-share/PerformanceIndicator"/>
        <rdfs:range rdf:resource="http://www.w3.org/2001/XMLSchema#float"/>
        <rdfs:comment xml:lang="en">Defines the measure calculated for the metric</rdfs:comment>
        <rdfs:label xml:lang="en">measure</rdfs:label>
    </owl:DatatypeProperty>
    


    <!-- http://w3id.org/meta-share/meta-share/mediaTypeDetails -->

    <owl:DatatypeProperty rdf:about="http://w3id.org/meta-share/meta-share/mediaTypeDetails">
        <rdfs:domain rdf:resource="http://w3id.org/meta-share/meta-share/LinkToOtherMedia"/>
        <rdfs:range rdf:resource="http://www.w3.org/1999/02/22-rdf-syntax-ns#langString"/>
        <rdfs:comment xml:lang="en">Provides further information on the way the media types are linked and/or synchronized with each other within the same resource</rdfs:comment>
        <rdfs:label xml:lang="en">media type details</rdfs:label>
    </owl:DatatypeProperty>
    


    <!-- http://w3id.org/meta-share/meta-share/metadataCreationDate -->

    <owl:DatatypeProperty rdf:about="http://w3id.org/meta-share/meta-share/metadataCreationDate">
        <rdfs:domain rdf:resource="http://w3id.org/meta-share/meta-share/MetadataRecord"/>
        <rdfs:range rdf:resource="http://www.w3.org/2001/XMLSchema#date"/>
        <rdfs:comment xml:lang="en">Specifies the date when the metadata record was first created</rdfs:comment>
        <rdfs:label xml:lang="en">metadata creation date</rdfs:label>
    </owl:DatatypeProperty>
    


    <!-- http://w3id.org/meta-share/meta-share/metadataLastDateUpdated -->

    <owl:DatatypeProperty rdf:about="http://w3id.org/meta-share/meta-share/metadataLastDateUpdated">
        <rdfs:domain rdf:resource="http://w3id.org/meta-share/meta-share/MetadataRecord"/>
        <rdfs:range rdf:resource="http://www.w3.org/2001/XMLSchema#date"/>
        <rdfs:comment xml:lang="en">Specifies the date when the last update of the metadata record was made</rdfs:comment>
        <rdfs:label xml:lang="en">metadata last date updated</rdfs:label>
    </owl:DatatypeProperty>
    


    <!-- http://w3id.org/meta-share/meta-share/metalanguage -->

    <owl:DatatypeProperty rdf:about="http://w3id.org/meta-share/meta-share/metalanguage">
        <rdfs:domain>
            <owl:Class>
                <owl:unionOf rdf:parseType="Collection">
                    <rdf:Description rdf:about="http://w3id.org/meta-share/meta-share/LanguageDescriptionImagePart"/>
                    <rdf:Description rdf:about="http://w3id.org/meta-share/meta-share/LanguageDescriptionTextPart"/>
                    <rdf:Description rdf:about="http://w3id.org/meta-share/meta-share/LanguageDescriptionVideoPart"/>
                    <rdf:Description rdf:about="http://w3id.org/meta-share/meta-share/LexicalConceptualResourceAudioPart"/>
                    <rdf:Description rdf:about="http://w3id.org/meta-share/meta-share/LexicalConceptualResourceImagePart"/>
                    <rdf:Description rdf:about="http://w3id.org/meta-share/meta-share/LexicalConceptualResourceTextPart"/>
                    <rdf:Description rdf:about="http://w3id.org/meta-share/meta-share/LexicalConceptualResourceVideoPart"/>
                </owl:unionOf>
            </owl:Class>
        </rdfs:domain>
        <rdfs:range rdf:resource="http://www.w3.org/2001/XMLSchema#anyURI"/>
        <rdfs:comment xml:lang="en">Specifies the language that is used as support for the resource (e.g., a grammar of French described in English or a French dictionary with English definitions)</rdfs:comment>
        <rdfs:label xml:lang="en">metalanguage</rdfs:label>
        <skos:comment xml:lang="en">in the xsd, this is expressed with a BCP47 combination while in the ontology as a URI (to link with an ontology)</skos:comment>
    </owl:DatatypeProperty>
    


    <!-- http://w3id.org/meta-share/meta-share/mlFramework -->

    <owl:DatatypeProperty rdf:about="http://w3id.org/meta-share/meta-share/mlFramework">
        <rdfs:domain rdf:resource="http://w3id.org/meta-share/meta-share/MLModel"/>
        <rdfs:range rdf:resource="http://www.w3.org/2001/XMLSchema#string"/>
        <rdfs:altLabel xml:lang="en">Machine Learning framework</rdfs:altLabel>
        <rdfs:comment xml:lang="en">Specifies the framework that has been used for developing a model (e.g. keras, tensorflow, etc.)</rdfs:comment>
        <rdfs:label xml:lang="en">ML framework</rdfs:label>
    </owl:DatatypeProperty>
    


    <!-- http://w3id.org/meta-share/meta-share/modalityTypeDetails -->

    <owl:DatatypeProperty rdf:about="http://w3id.org/meta-share/meta-share/modalityTypeDetails">
        <rdfs:domain rdf:resource="http://w3id.org/meta-share/meta-share/MediaPart"/>
        <rdfs:range rdf:resource="http://www.w3.org/1999/02/22-rdf-syntax-ns#langString"/>
        <rdfs:comment xml:lang="en">Provides further information on the modalities represented in a language resource</rdfs:comment>
        <rdfs:label xml:lang="en">modality type details</rdfs:label>
    </owl:DatatypeProperty>
    


    <!-- http://w3id.org/meta-share/meta-share/modelVariant -->

    <owl:DatatypeProperty rdf:about="http://w3id.org/meta-share/meta-share/modelVariant">
        <rdfs:domain rdf:resource="http://w3id.org/meta-share/meta-share/MLModel"/>
        <rdfs:range rdf:resource="http://www.w3.org/2001/XMLSchema#string"/>
        <rdfs:comment xml:lang="en">Introduces a label that can be used to identify the variant of a ML model</rdfs:comment>
        <rdfs:label xml:lang="en">model variant</rdfs:label>
    </owl:DatatypeProperty>
    


    <!-- http://w3id.org/meta-share/meta-share/multiValue -->

    <owl:DatatypeProperty rdf:about="http://w3id.org/meta-share/meta-share/multiValue">
        <rdfs:domain rdf:resource="http://w3id.org/meta-share/meta-share/Parameter"/>
        <rdfs:range rdf:resource="http://www.w3.org/2001/XMLSchema#boolean"/>
        <rdfs:comment xml:lang="en">Specifies whether the parameter takes a list of values</rdfs:comment>
        <rdfs:label xml:lang="en">multi-value</rdfs:label>
    </owl:DatatypeProperty>
    


    <!-- http://w3id.org/meta-share/meta-share/multilingualityTypeDetails -->

    <owl:DatatypeProperty rdf:about="http://w3id.org/meta-share/meta-share/multilingualityTypeDetails">
        <rdfs:domain rdf:resource="http://w3id.org/meta-share/meta-share/MediaPart"/>
        <rdfs:range rdf:resource="http://www.w3.org/1999/02/22-rdf-syntax-ns#langString"/>
        <rdfs:comment xml:lang="en">Provides further information on multilinguality of a resource in free text</rdfs:comment>
        <rdfs:label>multilinguality type details</rdfs:label>
    </owl:DatatypeProperty>
    


    <!-- http://w3id.org/meta-share/meta-share/numberOfParticipants -->

    <owl:DatatypeProperty rdf:about="http://w3id.org/meta-share/meta-share/numberOfParticipants">
        <rdfs:domain>
            <owl:Class>
                <owl:unionOf rdf:parseType="Collection">
                    <rdf:Description rdf:about="http://w3id.org/meta-share/meta-share/CorpusAudioPart"/>
                    <rdf:Description rdf:about="http://w3id.org/meta-share/meta-share/CorpusImagePart"/>
                    <rdf:Description rdf:about="http://w3id.org/meta-share/meta-share/CorpusTextNumericalPart"/>
                    <rdf:Description rdf:about="http://w3id.org/meta-share/meta-share/CorpusVideoPart"/>
                </owl:unionOf>
            </owl:Class>
        </rdfs:domain>
        <rdfs:range rdf:resource="http://www.w3.org/2001/XMLSchema#int"/>
        <rdfs:comment xml:lang="en">The number of the persons participating in the audio or video part of the resource</rdfs:comment>
        <rdfs:label xml:lang="en">number of participants</rdfs:label>
    </owl:DatatypeProperty>
    


    <!-- http://w3id.org/meta-share/meta-share/numberOfTracks -->

    <owl:DatatypeProperty rdf:about="http://w3id.org/meta-share/meta-share/numberOfTracks">
        <rdfs:domain rdf:resource="http://w3id.org/meta-share/meta-share/AudioFormat"/>
        <rdfs:range rdf:resource="http://www.w3.org/2001/XMLSchema#int"/>
        <rdfs:comment xml:lang="en">Specifies the number of audio channels</rdfs:comment>
        <rdfs:label xml:lang="en">number of tracks</rdfs:label>
        <skos:note xml:lang="en">In MS it&apos;s a controlled vocabulary (1, 2, 4, 8) but I think it&apos;s too much</skos:note>
    </owl:DatatypeProperty>
    


    <!-- http://w3id.org/meta-share/meta-share/numberOfTrainedSpeakers -->

    <owl:DatatypeProperty rdf:about="http://w3id.org/meta-share/meta-share/numberOfTrainedSpeakers">
        <rdfs:domain>
            <owl:Class>
                <owl:unionOf rdf:parseType="Collection">
                    <rdf:Description rdf:about="http://w3id.org/meta-share/meta-share/CorpusAudioPart"/>
                    <rdf:Description rdf:about="http://w3id.org/meta-share/meta-share/CorpusImagePart"/>
                    <rdf:Description rdf:about="http://w3id.org/meta-share/meta-share/CorpusTextNumericalPart"/>
                    <rdf:Description rdf:about="http://w3id.org/meta-share/meta-share/CorpusVideoPart"/>
                </owl:unionOf>
            </owl:Class>
        </rdfs:domain>
        <rdfs:range rdf:resource="http://www.w3.org/2001/XMLSchema#int"/>
        <rdfs:comment xml:lang="en">The number of participants that have been trained for the specific task</rdfs:comment>
        <rdfs:label xml:lang="en">number of trained speakers</rdfs:label>
    </owl:DatatypeProperty>
    


    <!-- http://w3id.org/meta-share/meta-share/optional -->

    <owl:DatatypeProperty rdf:about="http://w3id.org/meta-share/meta-share/optional">
        <rdfs:domain rdf:resource="http://w3id.org/meta-share/meta-share/Parameter"/>
        <rdfs:range rdf:resource="http://www.w3.org/2001/XMLSchema#boolean"/>
        <rdfs:comment xml:lang="en">Specifies whether the parameter is mandatory or optional</rdfs:comment>
        <rdfs:label xml:lang="en">optional</rdfs:label>
    </owl:DatatypeProperty>
    


    <!-- http://w3id.org/meta-share/meta-share/order -->

    <owl:DatatypeProperty rdf:about="http://w3id.org/meta-share/meta-share/order">
        <rdfs:domain rdf:resource="http://w3id.org/meta-share/meta-share/NGramModel"/>
        <rdfs:range rdf:resource="http://www.w3.org/2001/XMLSchema#int"/>
        <rdfs:comment xml:lang="en">Specifies the maximum number of items in the sequence</rdfs:comment>
        <rdfs:label xml:lang="en">order</rdfs:label>
    </owl:DatatypeProperty>
    


    <!-- http://w3id.org/meta-share/meta-share/organizationAlternativeName -->

    <owl:DatatypeProperty rdf:about="http://w3id.org/meta-share/meta-share/organizationAlternativeName">
        <rdfs:subPropertyOf rdf:resource="http://purl.org/dc/terms/alternative"/>
        <rdfs:domain rdf:resource="http://w3id.org/meta-share/meta-share/Organization"/>
        <rdfs:range rdf:resource="http://www.w3.org/1999/02/22-rdf-syntax-ns#langString"/>
        <rdfs:comment xml:lang="en">Introduces an alternative name (other than the short name) used for an organization</rdfs:comment>
        <rdfs:label xml:lang="en">organization alternative name</rdfs:label>
    </owl:DatatypeProperty>
    


    <!-- http://w3id.org/meta-share/meta-share/organizationBio -->

    <owl:DatatypeProperty rdf:about="http://w3id.org/meta-share/meta-share/organizationBio">
        <rdfs:subPropertyOf rdf:resource="http://purl.org/dc/terms/description"/>
        <rdfs:domain>
            <owl:Class>
                <owl:unionOf rdf:parseType="Collection">
                    <rdf:Description rdf:about="http://w3id.org/meta-share/meta-share/Division"/>
                    <rdf:Description rdf:about="http://w3id.org/meta-share/meta-share/Group"/>
                    <rdf:Description rdf:about="http://w3id.org/meta-share/meta-share/Organization"/>
                </owl:unionOf>
            </owl:Class>
        </rdfs:domain>
        <rdfs:range rdf:resource="http://www.w3.org/1999/02/22-rdf-syntax-ns#langString"/>
        <rdfs:comment xml:lang="en">Introduces a short free-text account that provides information on an organization</rdfs:comment>
        <rdfs:label xml:lang="en">organization description</rdfs:label>
    </owl:DatatypeProperty>
    


    <!-- http://w3id.org/meta-share/meta-share/organizationDescription -->

    <owl:DatatypeProperty rdf:about="http://w3id.org/meta-share/meta-share/organizationDescription">
        <rdfs:domain rdf:resource="http://w3id.org/meta-share/meta-share/StaticElement"/>
        <rdfs:range rdf:resource="http://www.w3.org/1999/02/22-rdf-syntax-ns#langString"/>
        <rdfs:comment xml:lang="en">Provides description of the organizations that may appear in the image corpus</rdfs:comment>
        <rdfs:label xml:lang="en">organization description</rdfs:label>
    </owl:DatatypeProperty>
    


    <!-- http://w3id.org/meta-share/meta-share/organizationName -->

    <owl:DatatypeProperty rdf:about="http://w3id.org/meta-share/meta-share/organizationName">
        <rdfs:subPropertyOf rdf:resource="http://purl.org/dc/terms/title"/>
        <rdfs:domain>
            <owl:Class>
                <owl:unionOf rdf:parseType="Collection">
                    <rdf:Description rdf:about="http://w3id.org/meta-share/meta-share/Group"/>
                    <rdf:Description rdf:about="http://w3id.org/meta-share/meta-share/Organization"/>
                </owl:unionOf>
            </owl:Class>
        </rdfs:domain>
        <rdfs:range rdf:resource="http://www.w3.org/1999/02/22-rdf-syntax-ns#langString"/>
        <rdfs:comment xml:lang="en">The full name of an organization</rdfs:comment>
        <rdfs:label xml:lang="en">organization name</rdfs:label>
    </owl:DatatypeProperty>
    


    <!-- http://w3id.org/meta-share/meta-share/organizationShortName -->

    <owl:DatatypeProperty rdf:about="http://w3id.org/meta-share/meta-share/organizationShortName">
        <rdfs:subPropertyOf rdf:resource="http://purl.org/dc/terms/alternative"/>
        <rdfs:domain>
            <owl:Class>
                <owl:unionOf rdf:parseType="Collection">
                    <rdf:Description rdf:about="http://w3id.org/meta-share/meta-share/Group"/>
                    <rdf:Description rdf:about="http://w3id.org/meta-share/meta-share/Organization"/>
                </owl:unionOf>
            </owl:Class>
        </rdfs:domain>
        <rdfs:range rdf:resource="http://www.w3.org/1999/02/22-rdf-syntax-ns#langString"/>
        <rdfs:comment xml:lang="en">Introduces the short name (abbreviation, acronym , etc.) used for an organization</rdfs:comment>
        <rdfs:label xml:lang="en">organization short name</rdfs:label>
    </owl:DatatypeProperty>
    


    <!-- http://w3id.org/meta-share/meta-share/originalSourceDescription -->

    <owl:DatatypeProperty rdf:about="http://w3id.org/meta-share/meta-share/originalSourceDescription">
        <rdfs:domain>
            <owl:Class>
                <owl:unionOf rdf:parseType="Collection">
                    <rdf:Description rdf:about="http://w3id.org/meta-share/meta-share/LexicalConceptualResource"/>
                    <rdf:Description rdf:about="http://w3id.org/meta-share/meta-share/MediaPart"/>
                    <rdf:Description rdf:about="http://w3id.org/meta-share/meta-share/ToolService"/>
                </owl:unionOf>
            </owl:Class>
        </rdfs:domain>
        <rdfs:range rdf:resource="http://www.w3.org/1999/02/22-rdf-syntax-ns#langString"/>
        <rdfs:comment xml:lang="en">A description in free text of the source material that has been used for the creation of a language data resource</rdfs:comment>
        <rdfs:label xml:lang="en">original source description</rdfs:label>
    </owl:DatatypeProperty>
    


    <!-- http://w3id.org/meta-share/meta-share/output -->

    <owl:DatatypeProperty rdf:about="http://w3id.org/meta-share/meta-share/output">
        <rdfs:domain rdf:resource="http://w3id.org/meta-share/meta-share/LanguageDescription"/>
        <rdfs:range rdf:resource="http://www.w3.org/1999/02/22-rdf-syntax-ns#langString"/>
        <rdfs:comment xml:lang="en">Indicates whether the output of the operation of the grammar is a statement of grammaticality (grammatical/ungrammatical) or structures (interpretation of the input)</rdfs:comment>
        <rdfs:label xml:lang="en">output</rdfs:label>
    </owl:DatatypeProperty>
    


    <!-- http://w3id.org/meta-share/meta-share/pages -->

    <owl:DatatypeProperty rdf:about="http://w3id.org/meta-share/meta-share/pages">
        <rdfs:domain rdf:resource="http://w3id.org/meta-share/meta-share/Document"/>
        <rdfs:range rdf:resource="http://www.w3.org/2001/XMLSchema#string"/>
        <rdfs:comment xml:lang="en">Introduces the range of pages (preferrably with a dash between) on which a document is printed</rdfs:comment>
        <rdfs:label xml:lang="en">pages</rdfs:label>
    </owl:DatatypeProperty>
    


    <!-- http://w3id.org/meta-share/meta-share/parameterDescription -->

    <owl:DatatypeProperty rdf:about="http://w3id.org/meta-share/meta-share/parameterDescription">
        <rdfs:domain rdf:resource="http://w3id.org/meta-share/meta-share/Parameter"/>
        <rdfs:range rdf:resource="http://www.w3.org/1999/02/22-rdf-syntax-ns#langString"/>
        <rdfs:comment xml:lang="en">Provides a short account of he parameter (e.g.,  function it performs, input / output requirements, etc.) in free text</rdfs:comment>
        <rdfs:label xml:lang="en">parameter description</rdfs:label>
    </owl:DatatypeProperty>
    


    <!-- http://w3id.org/meta-share/meta-share/parameterLabel -->

    <owl:DatatypeProperty rdf:about="http://w3id.org/meta-share/meta-share/parameterLabel">
        <rdfs:domain rdf:resource="http://w3id.org/meta-share/meta-share/Parameter"/>
        <rdfs:range rdf:resource="http://www.w3.org/1999/02/22-rdf-syntax-ns#langString"/>
        <rdfs:comment xml:lang="en">Introduces a short free text used to show to the user for the parameter</rdfs:comment>
        <rdfs:label xml:lang="en">parameter label</rdfs:label>
    </owl:DatatypeProperty>
    


    <!-- http://w3id.org/meta-share/meta-share/parameterName -->

    <owl:DatatypeProperty rdf:about="http://w3id.org/meta-share/meta-share/parameterName">
        <rdfs:domain rdf:resource="http://w3id.org/meta-share/meta-share/Parameter"/>
        <rdfs:range rdf:resource="http://www.w3.org/2001/XMLSchema#string"/>
        <rdfs:comment xml:lang="en">Introduces a free text used to identify the parameter</rdfs:comment>
        <rdfs:label xml:lang="en">parameter name</rdfs:label>
    </owl:DatatypeProperty>
    


    <!-- http://w3id.org/meta-share/meta-share/perplexity -->

    <owl:DatatypeProperty rdf:about="http://w3id.org/meta-share/meta-share/perplexity">
        <rdfs:domain rdf:resource="http://w3id.org/meta-share/meta-share/NGramModel"/>
        <rdfs:range rdf:resource="http://www.w3.org/2001/XMLSchema#float"/>
        <rdfs:comment xml:lang="en">Provides information on the perplexity derived from running on test set taken from the same corpus</rdfs:comment>
        <rdfs:label xml:lang="en">perplexity</rdfs:label>
    </owl:DatatypeProperty>
    


    <!-- http://w3id.org/meta-share/meta-share/personDescription -->

    <owl:DatatypeProperty rdf:about="http://w3id.org/meta-share/meta-share/personDescription">
        <rdfs:domain rdf:resource="http://w3id.org/meta-share/meta-share/StaticElement"/>
        <rdfs:range rdf:resource="http://www.w3.org/1999/02/22-rdf-syntax-ns#langString"/>
        <rdfs:comment xml:lang="en">Provides descriptive features for the persons represented in the image corpus</rdfs:comment>
        <rdfs:label xml:lang="en">person description</rdfs:label>
    </owl:DatatypeProperty>
    


    <!-- http://w3id.org/meta-share/meta-share/personalDataDetails -->

    <owl:DatatypeProperty rdf:about="http://w3id.org/meta-share/meta-share/personalDataDetails">
        <rdfs:domain rdf:resource="http://w3id.org/meta-share/meta-share/DataLanguageResource"/>
        <rdfs:range rdf:resource="http://www.w3.org/1999/02/22-rdf-syntax-ns#langString"/>
        <rdfs:comment xml:lang="en">If the resource includes personal data, this field can be used for entering more information, e.g.,  whether special handling of the resource is required (e.g.,  anonymization, further request for use , etc.)</rdfs:comment>
        <rdfs:label xml:lang="en">personal data details</rdfs:label>
    </owl:DatatypeProperty>
    


    <!-- http://w3id.org/meta-share/meta-share/personalDataIncluded -->

    <owl:DatatypeProperty rdf:about="http://w3id.org/meta-share/meta-share/personalDataIncluded">
        <rdfs:domain rdf:resource="http://w3id.org/meta-share/meta-share/DataLanguageResource"/>
        <rdfs:range rdf:resource="http://www.w3.org/2001/XMLSchema#boolean"/>
        <rdfs:comment xml:lang="en">Specifies whether the language resource contains personal data (mainly in the sense falling under the GDPR)</rdfs:comment>
        <rdfs:label xml:lang="en">personal data included</rdfs:label>
    </owl:DatatypeProperty>
    


    <!-- http://w3id.org/meta-share/meta-share/placeOfBirth -->

    <owl:DatatypeProperty rdf:about="http://w3id.org/meta-share/meta-share/placeOfBirth">
        <rdfs:domain rdf:resource="http://w3id.org/meta-share/meta-share/Participant"/>
        <rdfs:range rdf:resource="http://www.w3.org/1999/02/22-rdf-syntax-ns#langString"/>
        <rdfs:comment xml:lang="en">The place in which the participant has been born</rdfs:comment>
        <rdfs:label xml:lang="en">place of birth</rdfs:label>
    </owl:DatatypeProperty>
    


    <!-- http://w3id.org/meta-share/meta-share/placeOfChildhood -->

    <owl:DatatypeProperty rdf:about="http://w3id.org/meta-share/meta-share/placeOfChildhood">
        <rdfs:domain rdf:resource="http://w3id.org/meta-share/meta-share/Participant"/>
        <rdfs:range rdf:resource="http://www.w3.org/1999/02/22-rdf-syntax-ns#langString"/>
        <rdfs:comment xml:lang="en">The place in which the participant lived as a child</rdfs:comment>
        <rdfs:label xml:lang="en">place of childhood</rdfs:label>
    </owl:DatatypeProperty>
    


    <!-- http://w3id.org/meta-share/meta-share/placeOfLiving -->

    <owl:DatatypeProperty rdf:about="http://w3id.org/meta-share/meta-share/placeOfLiving">
        <rdfs:domain rdf:resource="http://w3id.org/meta-share/meta-share/Participant"/>
        <rdfs:range rdf:resource="http://www.w3.org/1999/02/22-rdf-syntax-ns#langString"/>
        <rdfs:comment xml:lang="en">The place of living of a participant</rdfs:comment>
        <rdfs:label xml:lang="en">place of living</rdfs:label>
    </owl:DatatypeProperty>
    


    <!-- http://w3id.org/meta-share/meta-share/placeOfSecondEducation -->

    <owl:DatatypeProperty rdf:about="http://w3id.org/meta-share/meta-share/placeOfSecondEducation">
        <rdfs:domain rdf:resource="http://w3id.org/meta-share/meta-share/Participant"/>
        <rdfs:range rdf:resource="http://www.w3.org/1999/02/22-rdf-syntax-ns#langString"/>
        <rdfs:comment xml:lang="en">Specifies the place of the secondary education of the participant</rdfs:comment>
        <rdfs:label xml:lang="en">place of second education</rdfs:label>
    </owl:DatatypeProperty>
    


    <!-- http://w3id.org/meta-share/meta-share/posesPerSubject -->

    <owl:DatatypeProperty rdf:about="http://w3id.org/meta-share/meta-share/posesPerSubject">
        <rdfs:domain rdf:resource="http://w3id.org/meta-share/meta-share/DynamicElement"/>
        <rdfs:range rdf:resource="http://www.w3.org/2001/XMLSchema#int"/>
        <rdfs:comment xml:lang="en">Indicates the number of poses per subject that participates in the video part of the resource</rdfs:comment>
        <rdfs:label xml:lang="en">poses per subject</rdfs:label>
    </owl:DatatypeProperty>
    


    <!-- http://w3id.org/meta-share/meta-share/position -->

    <owl:DatatypeProperty rdf:about="http://w3id.org/meta-share/meta-share/position">
        <rdfs:domain rdf:resource="http://w3id.org/meta-share/meta-share/Affiliation"/>
        <rdfs:range rdf:resource="http://www.w3.org/1999/02/22-rdf-syntax-ns#langString"/>
        <rdfs:comment xml:lang="en">The position or the title of a person if affiliated to an organization </rdfs:comment>
        <rdfs:label xml:lang="en">position</rdfs:label>
    </owl:DatatypeProperty>
    


    <!-- http://w3id.org/meta-share/meta-share/profession -->

    <owl:DatatypeProperty rdf:about="http://w3id.org/meta-share/meta-share/profession">
        <rdfs:domain rdf:resource="http://w3id.org/meta-share/meta-share/Participant"/>
        <rdfs:range rdf:resource="http://www.w3.org/1999/02/22-rdf-syntax-ns#langString"/>
        <rdfs:comment xml:lang="en">Provides information on the participant&apos;s profession</rdfs:comment>
        <rdfs:label xml:lang="en">profession</rdfs:label>
    </owl:DatatypeProperty>
    


    <!-- http://w3id.org/meta-share/meta-share/projectAlternativeName -->

    <owl:DatatypeProperty rdf:about="http://w3id.org/meta-share/meta-share/projectAlternativeName">
        <rdfs:subPropertyOf rdf:resource="http://purl.org/dc/terms/alternative"/>
        <rdfs:domain rdf:resource="http://w3id.org/meta-share/meta-share/Project"/>
        <rdfs:range rdf:resource="http://www.w3.org/1999/02/22-rdf-syntax-ns#langString"/>
        <rdfs:comment xml:lang="en">Introduces an alternative name (other than the short name) used for a project</rdfs:comment>
        <rdfs:label xml:lang="en">project alternative name</rdfs:label>
    </owl:DatatypeProperty>
    


    <!-- http://w3id.org/meta-share/meta-share/projectEndDate -->

    <owl:DatatypeProperty rdf:about="http://w3id.org/meta-share/meta-share/projectEndDate">
        <rdfs:domain rdf:resource="http://w3id.org/meta-share/meta-share/Project"/>
        <rdfs:range rdf:resource="http://www.w3.org/2001/XMLSchema#date"/>
        <rdfs:comment xml:lang="en">The end date of a project</rdfs:comment>
        <rdfs:label xml:lang="en">project end date</rdfs:label>
    </owl:DatatypeProperty>
    


    <!-- http://w3id.org/meta-share/meta-share/projectName -->

    <owl:DatatypeProperty rdf:about="http://w3id.org/meta-share/meta-share/projectName">
        <rdfs:subPropertyOf rdf:resource="http://purl.org/dc/terms/title"/>
        <rdfs:domain rdf:resource="http://w3id.org/meta-share/meta-share/Project"/>
        <rdfs:range rdf:resource="http://www.w3.org/1999/02/22-rdf-syntax-ns#langString"/>
        <rdfs:altLabel xml:lang="en">project title</rdfs:altLabel>
        <rdfs:comment xml:lang="en">The full name (title) of a project</rdfs:comment>
        <rdfs:label xml:lang="en">project name</rdfs:label>
    </owl:DatatypeProperty>
    


    <!-- http://w3id.org/meta-share/meta-share/projectReport -->

    <owl:DatatypeProperty rdf:about="http://w3id.org/meta-share/meta-share/projectReport">
        <rdfs:domain rdf:resource="http://w3id.org/meta-share/meta-share/Project"/>
        <rdfs:range rdf:resource="http://www.w3.org/1999/02/22-rdf-syntax-ns#langString"/>
        <rdfs:comment xml:lang="en">Links to a report issued by a project</rdfs:comment>
        <rdfs:label xml:lang="en">project report</rdfs:label>
    </owl:DatatypeProperty>
    


    <!-- http://w3id.org/meta-share/meta-share/projectShortName -->

    <owl:DatatypeProperty rdf:about="http://w3id.org/meta-share/meta-share/projectShortName">
        <rdfs:subPropertyOf rdf:resource="http://purl.org/dc/terms/alternative"/>
        <rdfs:domain rdf:resource="http://w3id.org/meta-share/meta-share/Project"/>
        <rdfs:range rdf:resource="http://www.w3.org/1999/02/22-rdf-syntax-ns#langString"/>
        <rdfs:comment xml:lang="en">Introduces a short name (e.g.,  acronym, abbreviated form) by which a project is known</rdfs:comment>
        <rdfs:label xml:lang="en">project short name</rdfs:label>
    </owl:DatatypeProperty>
    


    <!-- http://w3id.org/meta-share/meta-share/projectStartDate -->

    <owl:DatatypeProperty rdf:about="http://w3id.org/meta-share/meta-share/projectStartDate">
        <rdfs:domain rdf:resource="http://w3id.org/meta-share/meta-share/Project"/>
        <rdfs:range rdf:resource="http://www.w3.org/2001/XMLSchema#date"/>
        <rdfs:comment xml:lang="en">The starting date of a project</rdfs:comment>
        <rdfs:label xml:lang="en">project start date</rdfs:label>
    </owl:DatatypeProperty>
    


    <!-- http://w3id.org/meta-share/meta-share/projectSummary -->

    <owl:DatatypeProperty rdf:about="http://w3id.org/meta-share/meta-share/projectSummary">
        <rdfs:domain rdf:resource="http://w3id.org/meta-share/meta-share/Project"/>
        <rdfs:range rdf:resource="http://www.w3.org/1999/02/22-rdf-syntax-ns#langString"/>
        <rdfs:comment xml:lang="en">Introduces a short description (in free text) of the main objectives, mission or contents of the project</rdfs:comment>
        <rdfs:label xml:lang="en">project summary</rdfs:label>
    </owl:DatatypeProperty>
    


    <!-- http://w3id.org/meta-share/meta-share/publicationDate -->

    <owl:DatatypeProperty rdf:about="http://w3id.org/meta-share/meta-share/publicationDate">
        <rdfs:subPropertyOf rdf:resource="http://purl.org/dc/terms/issued"/>
        <rdfs:domain>
            <owl:Class>
                <owl:unionOf rdf:parseType="Collection">
                    <rdf:Description rdf:about="http://w3id.org/meta-share/meta-share/Distribution"/>
                    <rdf:Description rdf:about="http://w3id.org/meta-share/meta-share/Document"/>
                    <rdf:Description rdf:about="http://w3id.org/meta-share/meta-share/LanguageResource"/>
                </owl:unionOf>
            </owl:Class>
        </rdfs:domain>
        <rdfs:range rdf:resource="http://www.w3.org/2001/XMLSchema#date"/>
        <rdfs:comment xml:lang="en">Specifies the date when a language resource has been made available to the public</rdfs:comment>
        <rdfs:label xml:lang="en">publication date</rdfs:label>
        <skos:note xml:lang="en">problem: when is the first publication date if a resource has been made available through zenodo, meta-share, clarin , etc.?? How can this be propagated? 
Important for citation purposes
should we also differentiate between distributions? e.g.,  a csv published at a different time from a database?</skos:note>
    </owl:DatatypeProperty>
    


    <!-- http://w3id.org/meta-share/meta-share/publisher -->

    <owl:DatatypeProperty rdf:about="http://w3id.org/meta-share/meta-share/publisher">
        <rdfs:domain rdf:resource="http://w3id.org/meta-share/meta-share/Document"/>
        <rdfs:range rdf:resource="http://www.w3.org/1999/02/22-rdf-syntax-ns#langString"/>
        <rdfs:comment xml:lang="en">Introduces the name of an organization that has published the document being described</rdfs:comment>
        <rdfs:label xml:lang="en">publisher</rdfs:label>
    </owl:DatatypeProperty>
    


    <!-- http://w3id.org/meta-share/meta-share/quantization -->

    <owl:DatatypeProperty rdf:about="http://w3id.org/meta-share/meta-share/quantization">
        <rdfs:domain rdf:resource="http://w3id.org/meta-share/meta-share/AudioFormat"/>
        <rdfs:range rdf:resource="http://www.w3.org/2001/XMLSchema#int"/>
        <rdfs:comment xml:lang="en">The number of bits for each audio sample</rdfs:comment>
        <rdfs:label xml:lang="en">quantization</rdfs:label>
        <skos:note xml:lang="en">In MS it&apos;s a controlled vocabulary (8, 16, 24, 32, 64) but I found it too much</skos:note>
    </owl:DatatypeProperty>
    


    <!-- http://w3id.org/meta-share/meta-share/recordingDeviceTypeDetails -->

    <owl:DatatypeProperty rdf:about="http://w3id.org/meta-share/meta-share/recordingDeviceTypeDetails">
        <rdfs:domain>
            <owl:Class>
                <owl:unionOf rdf:parseType="Collection">
                    <rdf:Description rdf:about="http://w3id.org/meta-share/meta-share/CorpusAudioPart"/>
                    <rdf:Description rdf:about="http://w3id.org/meta-share/meta-share/CorpusTextNumericalPart"/>
                    <rdf:Description rdf:about="http://w3id.org/meta-share/meta-share/CorpusVideoPart"/>
                </owl:unionOf>
            </owl:Class>
        </rdfs:domain>
        <rdfs:range rdf:resource="http://www.w3.org/1999/02/22-rdf-syntax-ns#langString"/>
        <rdfs:comment xml:lang="en">Free text description of the recording device</rdfs:comment>
        <rdfs:label xml:lang="en">recording device type details</rdfs:label>
    </owl:DatatypeProperty>
    


    <!-- http://w3id.org/meta-share/meta-share/recordingPlatformSoftware -->

    <owl:DatatypeProperty rdf:about="http://w3id.org/meta-share/meta-share/recordingPlatformSoftware">
        <rdfs:domain>
            <owl:Class>
                <owl:unionOf rdf:parseType="Collection">
                    <rdf:Description rdf:about="http://w3id.org/meta-share/meta-share/CorpusAudioPart"/>
                    <rdf:Description rdf:about="http://w3id.org/meta-share/meta-share/CorpusTextNumericalPart"/>
                    <rdf:Description rdf:about="http://w3id.org/meta-share/meta-share/CorpusVideoPart"/>
                </owl:unionOf>
            </owl:Class>
        </rdfs:domain>
        <rdfs:range rdf:resource="http://www.w3.org/2001/XMLSchema#string"/>
        <rdfs:comment xml:lang="en">Specifies the software used for the recording platform</rdfs:comment>
        <rdfs:label xml:lang="en">recording platform software</rdfs:label>
    </owl:DatatypeProperty>
    


    <!-- http://w3id.org/meta-share/meta-share/region -->

    <owl:DatatypeProperty rdf:about="http://w3id.org/meta-share/meta-share/region">
        <rdfs:domain rdf:resource="http://w3id.org/meta-share/meta-share/AddressSet"/>
        <rdfs:range rdf:resource="http://www.w3.org/1999/02/22-rdf-syntax-ns#langString"/>
        <rdfs:comment xml:lang="en">The name of the region, county or department as mentioned in the postal address of a person or organization</rdfs:comment>
        <rdfs:label xml:lang="en">region</rdfs:label>
    </owl:DatatypeProperty>
    


    <!-- http://w3id.org/meta-share/meta-share/register -->

    <owl:DatatypeProperty rdf:about="http://w3id.org/meta-share/meta-share/register">
        <rdfs:domain rdf:resource="http://w3id.org/meta-share/meta-share/CorpusTextPart"/>
        <rdfs:range rdf:resource="http://www.w3.org/1999/02/22-rdf-syntax-ns#langString"/>
        <rdfs:comment xml:lang="en">Specifies the type of register (any of the varieties of a language that a speaker uses in a particular social context [Merriam-Webster]) of the contents of a language resource</rdfs:comment>
        <rdfs:label xml:lang="en">register</rdfs:label>
    </owl:DatatypeProperty>
    


    <!-- http://w3id.org/meta-share/meta-share/relatedCall -->

    <owl:DatatypeProperty rdf:about="http://w3id.org/meta-share/meta-share/relatedCall">
        <rdfs:domain rdf:resource="http://w3id.org/meta-share/meta-share/Project"/>
        <rdfs:range rdf:resource="http://www.w3.org/2001/XMLSchema#string"/>
        <rdfs:comment xml:lang="en">Specifies the Call for proposals to which a project was submitted</rdfs:comment>
        <rdfs:label xml:lang="en">related call</rdfs:label>
    </owl:DatatypeProperty>
    


    <!-- http://w3id.org/meta-share/meta-share/relatedProgramme -->

    <owl:DatatypeProperty rdf:about="http://w3id.org/meta-share/meta-share/relatedProgramme">
        <rdfs:domain rdf:resource="http://w3id.org/meta-share/meta-share/Project"/>
        <rdfs:range rdf:resource="http://www.w3.org/2001/XMLSchema#string"/>
        <rdfs:comment xml:lang="en">Specifies the funding programme to which a project was submitted</rdfs:comment>
        <rdfs:label xml:lang="en">related programme</rdfs:label>
    </owl:DatatypeProperty>
    


    <!-- http://w3id.org/meta-share/meta-share/relatedSubprogramme -->

    <owl:DatatypeProperty rdf:about="http://w3id.org/meta-share/meta-share/relatedSubprogramme">
        <rdfs:domain rdf:resource="http://w3id.org/meta-share/meta-share/Project"/>
        <rdfs:range rdf:resource="http://www.w3.org/2001/XMLSchema#string"/>
        <rdfs:comment xml:lang="en">Specifies the funding subprogramme to which a project was submitted</rdfs:comment>
        <rdfs:label xml:lang="en">related subprogramme</rdfs:label>
    </owl:DatatypeProperty>
    


    <!-- http://w3id.org/meta-share/meta-share/relationType -->

    <owl:DatatypeProperty rdf:about="http://w3id.org/meta-share/meta-share/relationType">
        <rdfs:domain rdf:resource="http://w3id.org/meta-share/meta-share/Relation"/>
        <rdfs:range rdf:resource="http://www.w3.org/1999/02/22-rdf-syntax-ns#langString"/>
        <rdfs:comment xml:lang="en">Describes in a free text statement a relation holding between two Language Resources not yet covered by the schema</rdfs:comment>
        <rdfs:label xml:lang="en">relation type</rdfs:label>
    </owl:DatatypeProperty>
    


    <!-- http://w3id.org/meta-share/meta-share/requiresSoftware -->

    <owl:DatatypeProperty rdf:about="http://w3id.org/meta-share/meta-share/requiresSoftware">
        <rdfs:domain>
            <owl:Class>
                <owl:unionOf rdf:parseType="Collection">
                    <rdf:Description rdf:about="http://w3id.org/meta-share/meta-share/LanguageDescription"/>
                    <rdf:Description rdf:about="http://w3id.org/meta-share/meta-share/ToolService"/>
                </owl:unionOf>
            </owl:Class>
        </rdfs:domain>
        <rdfs:range rdf:resource="http://www.w3.org/2001/XMLSchema#string"/>
        <rdfs:comment xml:lang="en">Specifies software tools or libraries that are required for the operation of a tool/service or computational grammar</rdfs:comment>
        <rdfs:label xml:lang="en">requires software</rdfs:label>
        <skos:note xml:lang="en">left as a data property - it&apos;s for more general software than language processing tools, so difficult to restrict</skos:note>
    </owl:DatatypeProperty>
    


    <!-- http://w3id.org/meta-share/meta-share/resourceName -->

    <owl:DatatypeProperty rdf:about="http://w3id.org/meta-share/meta-share/resourceName">
        <rdfs:subPropertyOf rdf:resource="http://purl.org/dc/terms/title"/>
        <rdfs:domain rdf:resource="http://w3id.org/meta-share/meta-share/LanguageResource"/>
        <rdfs:range rdf:resource="http://www.w3.org/1999/02/22-rdf-syntax-ns#langString"/>
        <rdfs:altLabel xml:lang="en">resource title</rdfs:altLabel>
        <rdfs:comment xml:lang="en">Introduces a human-readable name or title by which the resource is known</rdfs:comment>
        <rdfs:label xml:lang="en">resource name</rdfs:label>
        <skos:example xml:lang="en">British National Corpus</skos:example>
    </owl:DatatypeProperty>
    


    <!-- http://w3id.org/meta-share/meta-share/resourceShortName -->

    <owl:DatatypeProperty rdf:about="http://w3id.org/meta-share/meta-share/resourceShortName">
        <rdfs:subPropertyOf rdf:resource="http://purl.org/dc/terms/alternative"/>
        <rdfs:domain rdf:resource="http://w3id.org/meta-share/meta-share/LanguageResource"/>
        <rdfs:range rdf:resource="http://www.w3.org/1999/02/22-rdf-syntax-ns#langString"/>
        <rdfs:comment xml:lang="en">Introduces a short form (e.g.,  abbreviation, acronym , etc.) used to refer to a language resource</rdfs:comment>
        <rdfs:label xml:lang="en">resource short name</rdfs:label>
    </owl:DatatypeProperty>
    


    <!-- http://w3id.org/meta-share/meta-share/revision -->

    <owl:DatatypeProperty rdf:about="http://w3id.org/meta-share/meta-share/revision">
        <rdfs:domain>
            <owl:Class>
                <owl:unionOf rdf:parseType="Collection">
                    <rdf:Description rdf:about="http://w3id.org/meta-share/meta-share/LanguageResource"/>
                    <rdf:Description rdf:about="http://w3id.org/meta-share/meta-share/MetadataRecord"/>
                </owl:unionOf>
            </owl:Class>
        </rdfs:domain>
        <rdfs:range rdf:resource="http://www.w3.org/1999/02/22-rdf-syntax-ns#langString"/>
        <rdfs:comment xml:lang="en">Provides an account of the revisions in free text or a link to a document with revisions</rdfs:comment>
        <rdfs:label xml:lang="en">revision</rdfs:label>
    </owl:DatatypeProperty>
    


    <!-- http://w3id.org/meta-share/meta-share/robustness -->

    <owl:DatatypeProperty rdf:about="http://w3id.org/meta-share/meta-share/robustness">
        <rdfs:domain rdf:resource="http://w3id.org/meta-share/meta-share/LanguageDescription"/>
        <rdfs:range rdf:resource="http://www.w3.org/1999/02/22-rdf-syntax-ns#langString"/>
        <rdfs:comment xml:lang="en">Introduces a free text statement on the robustness of the grammar (how well the grammar can cope with misspelt/unknown , etc. input, i.e. whether it can produce even partial interpretations of the input)</rdfs:comment>
        <rdfs:label xml:lang="en">robustness</rdfs:label>
    </owl:DatatypeProperty>
    


    <!-- http://w3id.org/meta-share/meta-share/runningEnvironmentDetails -->

    <owl:DatatypeProperty rdf:about="http://w3id.org/meta-share/meta-share/runningEnvironmentDetails">
        <rdfs:domain>
            <owl:Class>
                <owl:unionOf rdf:parseType="Collection">
                    <rdf:Description rdf:about="http://w3id.org/meta-share/meta-share/LanguageDescription"/>
                    <rdf:Description rdf:about="http://w3id.org/meta-share/meta-share/ToolService"/>
                </owl:unionOf>
            </owl:Class>
        </rdfs:domain>
        <rdfs:range rdf:resource="http://www.w3.org/1999/02/22-rdf-syntax-ns#langString"/>
        <rdfs:comment xml:lang="en">Provides further information on the running environment of a tool/service or of a language description</rdfs:comment>
        <rdfs:label xml:lang="en">running environment details</rdfs:label>
    </owl:DatatypeProperty>
    


    <!-- http://w3id.org/meta-share/meta-share/runningTime -->

    <owl:DatatypeProperty rdf:about="http://w3id.org/meta-share/meta-share/runningTime">
        <rdfs:domain rdf:resource="http://w3id.org/meta-share/meta-share/ToolService"/>
        <rdfs:range rdf:resource="http://www.w3.org/2001/XMLSchema#string"/>
        <rdfs:comment xml:lang="en">Gives information on the running time of a tool or service</rdfs:comment>
        <rdfs:label xml:lang="en">running time</rdfs:label>
    </owl:DatatypeProperty>
    


    <!-- http://w3id.org/meta-share/meta-share/samplesLocation -->

    <owl:DatatypeProperty rdf:about="http://w3id.org/meta-share/meta-share/samplesLocation">
        <rdfs:subPropertyOf rdf:resource="http://w3id.org/meta-share/meta-share/url"/>
        <rdfs:domain>
            <owl:Class>
                <owl:unionOf rdf:parseType="Collection">
                    <rdf:Description rdf:about="http://w3id.org/meta-share/meta-share/DataLanguageResource"/>
                    <rdf:Description rdf:about="http://w3id.org/meta-share/meta-share/ProcessingResource"/>
                </owl:unionOf>
            </owl:Class>
        </rdfs:domain>
        <rdfs:range rdf:resource="http://www.w3.org/2001/XMLSchema#anyURI"/>
        <rdfs:comment xml:lang="en">Links a resource to a url (or url&apos;s) with samples of a data resource or of the input of output resource of a tool/service</rdfs:comment>
        <rdfs:label xml:lang="en">samples location</rdfs:label>
    </owl:DatatypeProperty>
    


    <!-- http://w3id.org/meta-share/meta-share/samplingRate -->

    <owl:DatatypeProperty rdf:about="http://w3id.org/meta-share/meta-share/samplingRate">
        <rdfs:domain rdf:resource="http://w3id.org/meta-share/meta-share/AudioFormat"/>
        <rdfs:range rdf:resource="http://www.w3.org/2001/XMLSchema#int"/>
        <rdfs:comment xml:lang="en">Specifies the format of files contained in the resource in Hertz</rdfs:comment>
        <rdfs:label xml:lang="en">sampling rate</rdfs:label>
    </owl:DatatypeProperty>
    


    <!-- http://w3id.org/meta-share/meta-share/sensitiveDataDetails -->

    <owl:DatatypeProperty rdf:about="http://w3id.org/meta-share/meta-share/sensitiveDataDetails">
        <rdfs:domain rdf:resource="http://w3id.org/meta-share/meta-share/DataLanguageResource"/>
        <rdfs:range rdf:resource="http://www.w3.org/1999/02/22-rdf-syntax-ns#langString"/>
        <rdfs:comment xml:lang="en">If the resource includes sensitive data, this field can be used for entering more information, e.g.,  whether special handling of the resource is required (e.g.,  anonymization, further request for use , etc.)</rdfs:comment>
        <rdfs:label xml:lang="en">sensitive data details</rdfs:label>
    </owl:DatatypeProperty>
    


    <!-- http://w3id.org/meta-share/meta-share/sensitiveDataIncluded -->

    <owl:DatatypeProperty rdf:about="http://w3id.org/meta-share/meta-share/sensitiveDataIncluded">
        <rdfs:domain rdf:resource="http://w3id.org/meta-share/meta-share/DataLanguageResource"/>
        <rdfs:range rdf:resource="http://www.w3.org/2001/XMLSchema#boolean"/>
        <rdfs:comment xml:lang="en">Specifies whether the language resource contains sensitive data (e.g.,  medical/health-related, etc.) and thus requires special handling</rdfs:comment>
        <rdfs:label xml:lang="en">sensitive data included</rdfs:label>
    </owl:DatatypeProperty>
    


    <!-- http://w3id.org/meta-share/meta-share/sensorTechnology -->

    <owl:DatatypeProperty rdf:about="http://w3id.org/meta-share/meta-share/sensorTechnology">
        <rdfs:domain>
            <owl:Class>
                <owl:unionOf rdf:parseType="Collection">
                    <rdf:Description rdf:about="http://w3id.org/meta-share/meta-share/CorpusAudioPart"/>
                    <rdf:Description rdf:about="http://w3id.org/meta-share/meta-share/CorpusImagePart"/>
                    <rdf:Description rdf:about="http://w3id.org/meta-share/meta-share/CorpusTextNumericalPart"/>
                    <rdf:Description rdf:about="http://w3id.org/meta-share/meta-share/CorpusVideoPart"/>
                </owl:unionOf>
            </owl:Class>
        </rdfs:domain>
        <rdfs:range rdf:resource="http://www.w3.org/2001/XMLSchema#string"/>
        <rdfs:comment xml:lang="en">Specifies the type of image sensor or the sensing method used in the camera or the image-capture device</rdfs:comment>
        <rdfs:label xml:lang="en">sensor technology</rdfs:label>
    </owl:DatatypeProperty>
    


    <!-- http://w3id.org/meta-share/meta-share/series -->

    <owl:DatatypeProperty rdf:about="http://w3id.org/meta-share/meta-share/series">
        <rdfs:domain rdf:resource="http://w3id.org/meta-share/meta-share/Document"/>
        <rdfs:range rdf:resource="http://www.w3.org/1999/02/22-rdf-syntax-ns#langString"/>
        <rdfs:comment xml:lang="en">Introduces the title of the series of a book/journal where the document being described has been published</rdfs:comment>
        <rdfs:label xml:lang="en">series</rdfs:label>
    </owl:DatatypeProperty>
    


    <!-- http://w3id.org/meta-share/meta-share/serviceAdapterDownloadLocation -->

    <owl:DatatypeProperty rdf:about="http://w3id.org/meta-share/meta-share/serviceAdapterDownloadLocation">
        <rdfs:subPropertyOf rdf:resource="http://w3id.org/meta-share/meta-share/downloadLocation"/>
        <rdfs:domain rdf:resource="http://w3id.org/meta-share/meta-share/ToolService"/>
        <rdfs:range rdf:resource="http://www.w3.org/2001/XMLSchema#string"/>
        <rdfs:comment xml:lang="en">Τhe URL where the docker image of the service adapter can be downloaded from</rdfs:comment>
        <rdfs:label xml:lang="en">service adapter download location</rdfs:label>
    </owl:DatatypeProperty>
    


    <!-- http://w3id.org/meta-share/meta-share/serviceOffered -->

    <owl:DatatypeProperty rdf:about="http://w3id.org/meta-share/meta-share/serviceOffered">
        <rdfs:domain>
            <owl:Class>
                <owl:unionOf rdf:parseType="Collection">
                    <rdf:Description rdf:about="http://w3id.org/meta-share/meta-share/Division"/>
                    <rdf:Description rdf:about="http://w3id.org/meta-share/meta-share/Group"/>
                    <rdf:Description rdf:about="http://w3id.org/meta-share/meta-share/Organization"/>
                    <rdf:Description rdf:about="http://w3id.org/meta-share/meta-share/Person"/>
                </owl:unionOf>
            </owl:Class>
        </rdfs:domain>
        <rdfs:range rdf:resource="http://www.w3.org/1999/02/22-rdf-syntax-ns#langString"/>
        <rdfs:comment xml:lang="en">Lists the service(s) offered by an organization or person</rdfs:comment>
        <rdfs:label xml:lang="en">service offered</rdfs:label>
    </owl:DatatypeProperty>
    


    <!-- http://w3id.org/meta-share/meta-share/shallowness -->

    <owl:DatatypeProperty rdf:about="http://w3id.org/meta-share/meta-share/shallowness">
        <rdfs:domain rdf:resource="http://w3id.org/meta-share/meta-share/LanguageDescription"/>
        <rdfs:range rdf:resource="http://www.w3.org/1999/02/22-rdf-syntax-ns#langString"/>
        <rdfs:comment xml:lang="en">Introduces a free text statement on the shallowness of the grammar (how deep the syntactic analysis performed by the grammar can be)</rdfs:comment>
        <rdfs:label xml:lang="en">shallowness</rdfs:label>
    </owl:DatatypeProperty>
    


    <!-- http://w3id.org/meta-share/meta-share/shortBio -->

    <owl:DatatypeProperty rdf:about="http://w3id.org/meta-share/meta-share/shortBio">
        <rdfs:subPropertyOf rdf:resource="http://purl.org/dc/terms/description"/>
        <rdfs:domain rdf:resource="http://w3id.org/meta-share/meta-share/Person"/>
        <rdfs:range rdf:resource="http://www.w3.org/1999/02/22-rdf-syntax-ns#langString"/>
        <rdfs:comment xml:lang="en">Introduces a free text that can be used as a short bio for a person</rdfs:comment>
        <rdfs:label xml:lang="en">short bio</rdfs:label>
    </owl:DatatypeProperty>
    


    <!-- http://w3id.org/meta-share/meta-share/sizeHeight -->

    <owl:DatatypeProperty rdf:about="http://w3id.org/meta-share/meta-share/sizeHeight">
        <rdfs:domain rdf:resource="http://w3id.org/meta-share/meta-share/Resolution"/>
        <rdfs:range rdf:resource="http://www.w3.org/2001/XMLSchema#int"/>
        <rdfs:comment xml:lang="en">The frame height in pixels</rdfs:comment>
        <rdfs:label xml:lang="en">size height</rdfs:label>
    </owl:DatatypeProperty>
    


    <!-- http://w3id.org/meta-share/meta-share/sizeWidth -->

    <owl:DatatypeProperty rdf:about="http://w3id.org/meta-share/meta-share/sizeWidth">
        <rdfs:domain rdf:resource="http://w3id.org/meta-share/meta-share/Resolution"/>
        <rdfs:range rdf:resource="http://www.w3.org/2001/XMLSchema#int"/>
        <rdfs:comment xml:lang="en">The frame width in pixels</rdfs:comment>
        <rdfs:label xml:lang="en">size width</rdfs:label>
    </owl:DatatypeProperty>
    


    <!-- http://w3id.org/meta-share/meta-share/smokingHabit -->

    <owl:DatatypeProperty rdf:about="http://w3id.org/meta-share/meta-share/smokingHabit">
        <rdfs:domain rdf:resource="http://w3id.org/meta-share/meta-share/Participant"/>
        <rdfs:range rdf:resource="http://www.w3.org/1999/02/22-rdf-syntax-ns#langString"/>
        <rdfs:comment xml:lang="en">Provides information on whether the participant smokes and on his/her smoking habits in general</rdfs:comment>
        <rdfs:label xml:lang="en">smoking habit</rdfs:label>
    </owl:DatatypeProperty>
    


    <!-- http://w3id.org/meta-share/meta-share/smoothing -->

    <owl:DatatypeProperty rdf:about="http://w3id.org/meta-share/meta-share/smoothing">
        <rdfs:domain rdf:resource="http://w3id.org/meta-share/meta-share/NGramModel"/>
        <rdfs:range rdf:resource="http://www.w3.org/2001/XMLSchema#string"/>
        <rdfs:comment xml:lang="en">The technique used for giving unseen items some probability</rdfs:comment>
        <rdfs:label xml:lang="en">smoothing</rdfs:label>
    </owl:DatatypeProperty>
    


    <!-- http://w3id.org/meta-share/meta-share/sourceChannelDetails -->

    <owl:DatatypeProperty rdf:about="http://w3id.org/meta-share/meta-share/sourceChannelDetails">
        <rdfs:domain>
            <owl:Class>
                <owl:unionOf rdf:parseType="Collection">
                    <rdf:Description rdf:about="http://w3id.org/meta-share/meta-share/CorpusAudioPart"/>
                    <rdf:Description rdf:about="http://w3id.org/meta-share/meta-share/CorpusTextNumericalPart"/>
                    <rdf:Description rdf:about="http://w3id.org/meta-share/meta-share/CorpusVideoPart"/>
                </owl:unionOf>
            </owl:Class>
        </rdfs:domain>
        <rdfs:range rdf:resource="http://www.w3.org/1999/02/22-rdf-syntax-ns#langString"/>
        <rdfs:comment xml:lang="en">Provides information on the details of the channel equipment used (brand, type , etc.) in free text</rdfs:comment>
        <rdfs:label xml:lang="en">source channel details</rdfs:label>
    </owl:DatatypeProperty>
    


    <!-- http://w3id.org/meta-share/meta-share/sourceChannelName -->

    <owl:DatatypeProperty rdf:about="http://w3id.org/meta-share/meta-share/sourceChannelName">
        <rdfs:domain>
            <owl:Class>
                <owl:unionOf rdf:parseType="Collection">
                    <rdf:Description rdf:about="http://w3id.org/meta-share/meta-share/CorpusAudioPart"/>
                    <rdf:Description rdf:about="http://w3id.org/meta-share/meta-share/CorpusTextNumericalPart"/>
                    <rdf:Description rdf:about="http://w3id.org/meta-share/meta-share/CorpusVideoPart"/>
                </owl:unionOf>
            </owl:Class>
        </rdfs:domain>
        <rdfs:range rdf:resource="http://www.w3.org/1999/02/22-rdf-syntax-ns#langString"/>
        <rdfs:comment xml:lang="en">Introduces the name of the source channel through which the recording has been made</rdfs:comment>
        <rdfs:label xml:lang="en">source channel name</rdfs:label>
    </owl:DatatypeProperty>
    


    <!-- http://w3id.org/meta-share/meta-share/speakingImpairment -->

    <owl:DatatypeProperty rdf:about="http://w3id.org/meta-share/meta-share/speakingImpairment">
        <rdfs:domain rdf:resource="http://w3id.org/meta-share/meta-share/Participant"/>
        <rdfs:range rdf:resource="http://www.w3.org/1999/02/22-rdf-syntax-ns#langString"/>
        <rdfs:comment xml:lang="en">Provides information on any speaking impairment the participant may have</rdfs:comment>
        <rdfs:label xml:lang="en">speaking impairment</rdfs:label>
    </owl:DatatypeProperty>
    


    <!-- http://w3id.org/meta-share/meta-share/startup -->

    <owl:DatatypeProperty rdf:about="http://w3id.org/meta-share/meta-share/startup">
        <rdfs:domain>
            <owl:Class>
                <owl:unionOf rdf:parseType="Collection">
                    <rdf:Description rdf:about="http://w3id.org/meta-share/meta-share/Division"/>
                    <rdf:Description rdf:about="http://w3id.org/meta-share/meta-share/Organization"/>
                </owl:unionOf>
            </owl:Class>
        </rdfs:domain>
        <rdfs:range rdf:resource="http://www.w3.org/2001/XMLSchema#boolean"/>
        <rdfs:comment xml:lang="en">Indicates whether a company is a startup</rdfs:comment>
        <rdfs:label xml:lang="en">startup</rdfs:label>
    </owl:DatatypeProperty>
    


    <!-- http://w3id.org/meta-share/meta-share/status -->

    <owl:DatatypeProperty rdf:about="http://w3id.org/meta-share/meta-share/status">
        <rdfs:domain rdf:resource="http://w3id.org/meta-share/meta-share/Project"/>
        <rdfs:range rdf:resource="http://www.w3.org/2001/XMLSchema#string"/>
        <rdfs:comment xml:lang="en">Specifies the status in which a project is found in the course of a funding process (e.g. approved, signed, under negotiation, etc.)</rdfs:comment>
        <rdfs:label xml:lang="en">status</rdfs:label>
    </owl:DatatypeProperty>
    


    <!-- http://w3id.org/meta-share/meta-share/subtitle -->

    <owl:DatatypeProperty rdf:about="http://w3id.org/meta-share/meta-share/subtitle">
        <rdfs:subPropertyOf rdf:resource="http://purl.org/dc/terms/alternative"/>
        <rdfs:domain rdf:resource="http://w3id.org/meta-share/meta-share/Document"/>
        <rdfs:range rdf:resource="http://www.w3.org/1999/02/22-rdf-syntax-ns#langString"/>
        <rdfs:comment xml:lang="en">Introduces a secondary title used for a document</rdfs:comment>
        <rdfs:label xml:lang="en">subtitle</rdfs:label>
    </owl:DatatypeProperty>
    


    <!-- http://w3id.org/meta-share/meta-share/surname -->

    <owl:DatatypeProperty rdf:about="http://w3id.org/meta-share/meta-share/surname">
        <rdfs:domain rdf:resource="http://w3id.org/meta-share/meta-share/Person"/>
        <rdfs:range rdf:resource="http://www.w3.org/1999/02/22-rdf-syntax-ns#langString"/>
        <rdfs:altLabel xml:lang="en">family name</rdfs:altLabel>
        <rdfs:altLabel xml:lang="en">last name</rdfs:altLabel>
        <rdfs:comment xml:lang="en">Introduces the surname (i.e. the name shared by members of a family, also known as &quot;family name&quot; or &quot;last name&quot;) of a person</rdfs:comment>
        <rdfs:label xml:lang="en">surname</rdfs:label>
    </owl:DatatypeProperty>
    


    <!-- http://w3id.org/meta-share/meta-share/synchronizedWithAudio -->

    <owl:DatatypeProperty rdf:about="http://w3id.org/meta-share/meta-share/synchronizedWithAudio">
        <rdfs:domain rdf:resource="http://w3id.org/meta-share/meta-share/LinkToOtherMedia"/>
        <rdfs:range rdf:resource="http://www.w3.org/2001/XMLSchema#boolean"/>
        <rdfs:comment xml:lang="en">Whether the media part described is synchronized with audio within the same resource</rdfs:comment>
        <rdfs:label xml:lang="en">synchronized with audio</rdfs:label>
    </owl:DatatypeProperty>
    


    <!-- http://w3id.org/meta-share/meta-share/synchronizedWithImage -->

    <owl:DatatypeProperty rdf:about="http://w3id.org/meta-share/meta-share/synchronizedWithImage">
        <rdfs:domain rdf:resource="http://w3id.org/meta-share/meta-share/LinkToOtherMedia"/>
        <rdfs:range rdf:resource="http://www.w3.org/2001/XMLSchema#boolean"/>
        <rdfs:comment xml:lang="en">Whether the media part described is synchronized with image within the same resource</rdfs:comment>
        <rdfs:label xml:lang="en">synchronized with image</rdfs:label>
    </owl:DatatypeProperty>
    


    <!-- http://w3id.org/meta-share/meta-share/synchronizedWithText -->

    <owl:DatatypeProperty rdf:about="http://w3id.org/meta-share/meta-share/synchronizedWithText">
        <rdfs:domain rdf:resource="http://w3id.org/meta-share/meta-share/LinkToOtherMedia"/>
        <rdfs:range rdf:resource="http://www.w3.org/2001/XMLSchema#boolean"/>
        <rdfs:comment xml:lang="en">Whether video, text and textNumerical media type is synchronized with text within the same resource</rdfs:comment>
        <rdfs:label xml:lang="en">synchronized with text</rdfs:label>
    </owl:DatatypeProperty>
    


    <!-- http://w3id.org/meta-share/meta-share/synchronizedWithTextNumerical -->

    <owl:DatatypeProperty rdf:about="http://w3id.org/meta-share/meta-share/synchronizedWithTextNumerical">
        <rdfs:domain rdf:resource="http://w3id.org/meta-share/meta-share/LinkToOtherMedia"/>
        <rdfs:range rdf:resource="http://www.w3.org/2001/XMLSchema#boolean"/>
        <rdfs:comment xml:lang="en">Whether the media part described is synchronized with textNumerical within the same resource</rdfs:comment>
        <rdfs:label xml:lang="en">synchronized with textNumerical</rdfs:label>
    </owl:DatatypeProperty>
    


    <!-- http://w3id.org/meta-share/meta-share/synchronizedWithVideo -->

    <owl:DatatypeProperty rdf:about="http://w3id.org/meta-share/meta-share/synchronizedWithVideo">
        <rdfs:domain rdf:resource="http://w3id.org/meta-share/meta-share/LinkToOtherMedia"/>
        <rdfs:range rdf:resource="http://www.w3.org/2001/XMLSchema#boolean"/>
        <rdfs:comment xml:lang="en">Whether the media part described is synchronized with video within the same resource</rdfs:comment>
        <rdfs:label xml:lang="en">synchronized with video</rdfs:label>
    </owl:DatatypeProperty>
    


    <!-- http://w3id.org/meta-share/meta-share/syntheticData -->

    <owl:DatatypeProperty rdf:about="http://w3id.org/meta-share/meta-share/syntheticData">
        <rdfs:domain rdf:resource="http://w3id.org/meta-share/meta-share/CorpusMediaPart"/>
        <rdfs:range rdf:resource="http://www.w3.org/2001/XMLSchema#boolean"/>
        <rdfs:comment xml:lang="en">Specifies whether the contents of a corpus have been artificially generated (e.g.,  using a Machine Translation or NLG system) rather than having been created by humans (authentic/original data)</rdfs:comment>
        <rdfs:label xml:lang="en">synthetic data</rdfs:label>
    </owl:DatatypeProperty>
    


    <!-- http://w3id.org/meta-share/meta-share/telephoneNumber -->

    <owl:DatatypeProperty rdf:about="http://w3id.org/meta-share/meta-share/telephoneNumber">
        <rdfs:domain>
            <owl:Class>
                <owl:unionOf rdf:parseType="Collection">
                    <rdf:Description rdf:about="http://w3id.org/meta-share/meta-share/Division"/>
                    <rdf:Description rdf:about="http://w3id.org/meta-share/meta-share/Group"/>
                    <rdf:Description rdf:about="http://w3id.org/meta-share/meta-share/Organization"/>
                    <rdf:Description rdf:about="http://w3id.org/meta-share/meta-share/Person"/>
                </owl:unionOf>
            </owl:Class>
        </rdfs:domain>
        <rdfs:range rdf:resource="http://www.w3.org/2001/XMLSchema#string"/>
    </owl:DatatypeProperty>
    


    <!-- http://w3id.org/meta-share/meta-share/theoreticModel -->

    <owl:DatatypeProperty rdf:about="http://w3id.org/meta-share/meta-share/theoreticModel">
        <rdfs:domain>
            <owl:Class>
                <owl:unionOf rdf:parseType="Collection">
                    <rdf:Description rdf:about="http://w3id.org/meta-share/meta-share/Annotation"/>
                    <rdf:Description rdf:about="http://w3id.org/meta-share/meta-share/LanguageDescription"/>
                    <rdf:Description rdf:about="http://w3id.org/meta-share/meta-share/LexicalConceptualResource"/>
                </owl:unionOf>
            </owl:Class>
        </rdfs:domain>
        <rdfs:range rdf:resource="http://www.w3.org/1999/02/22-rdf-syntax-ns#langString"/>
        <rdfs:comment xml:lang="en">Indicates the theoretic model applied for the creation/enrichment of the resource, by name and/or by reference (URL or bibliographic reference) to informative material about the theoretic model used</rdfs:comment>
        <rdfs:label xml:lang="en">theoretic model</rdfs:label>
    </owl:DatatypeProperty>
    


    <!-- http://w3id.org/meta-share/meta-share/thingDescription -->

    <owl:DatatypeProperty rdf:about="http://w3id.org/meta-share/meta-share/thingDescription">
        <rdfs:domain rdf:resource="http://w3id.org/meta-share/meta-share/StaticElement"/>
        <rdfs:range rdf:resource="http://www.w3.org/1999/02/22-rdf-syntax-ns#langString"/>
        <rdfs:comment xml:lang="en">Provides description of the things represented in the image corpus</rdfs:comment>
        <rdfs:label xml:lang="en">thing description</rdfs:label>
    </owl:DatatypeProperty>
    


    <!-- http://w3id.org/meta-share/meta-share/timeCoverage -->

    <owl:DatatypeProperty rdf:about="http://w3id.org/meta-share/meta-share/timeCoverage">
        <rdfs:domain>
            <owl:Class>
                <owl:unionOf rdf:parseType="Collection">
                    <rdf:Description rdf:about="http://w3id.org/meta-share/meta-share/Corpus"/>
                    <rdf:Description rdf:about="http://w3id.org/meta-share/meta-share/LanguageDescription"/>
                    <rdf:Description rdf:about="http://w3id.org/meta-share/meta-share/LexicalConceptualResource"/>
                    <rdf:Description rdf:about="http://w3id.org/meta-share/meta-share/Subset"/>
                </owl:unionOf>
            </owl:Class>
        </rdfs:domain>
        <rdfs:range rdf:resource="http://www.w3.org/1999/02/22-rdf-syntax-ns#langString"/>
        <rdfs:comment xml:lang="en">Indicates the time period that the content of a resource is about</rdfs:comment>
        <rdfs:label xml:lang="en">time coverage</rdfs:label>
    </owl:DatatypeProperty>
    


    <!-- http://w3id.org/meta-share/meta-share/title -->

    <owl:DatatypeProperty rdf:about="http://w3id.org/meta-share/meta-share/title">
        <rdfs:subPropertyOf rdf:resource="http://purl.org/dc/terms/title"/>
        <rdfs:domain rdf:resource="http://w3id.org/meta-share/meta-share/Document"/>
        <rdfs:range rdf:resource="http://www.w3.org/1999/02/22-rdf-syntax-ns#langString"/>
        <rdfs:comment xml:lang="en">Introduces a human-readable text (typically short) used as a name for referring to the document being described</rdfs:comment>
        <rdfs:label xml:lang="en">title</rdfs:label>
    </owl:DatatypeProperty>
    


    <!-- http://w3id.org/meta-share/meta-share/trainedSpeaker -->

    <owl:DatatypeProperty rdf:about="http://w3id.org/meta-share/meta-share/trainedSpeaker">
        <rdfs:domain rdf:resource="http://w3id.org/meta-share/meta-share/Participant"/>
        <rdfs:range rdf:resource="http://www.w3.org/2001/XMLSchema#boolean"/>
        <rdfs:comment xml:lang="en">Provides information on whether the participant is trained in a specific task</rdfs:comment>
        <rdfs:label xml:lang="en">trained speaker</rdfs:label>
    </owl:DatatypeProperty>
    


    <!-- http://w3id.org/meta-share/meta-share/trainingCorpusDetails -->

    <owl:DatatypeProperty rdf:about="http://w3id.org/meta-share/meta-share/trainingCorpusDetails">
        <rdfs:domain rdf:resource="http://w3id.org/meta-share/meta-share/MLModel"/>
        <rdfs:range rdf:resource="http://www.w3.org/1999/02/22-rdf-syntax-ns#langString"/>
        <rdfs:comment xml:lang="en">Provides a detailed description of the training corpus (e.g.,  size, number of features , etc.)</rdfs:comment>
        <rdfs:label xml:lang="en">training corpus details</rdfs:label>
    </owl:DatatypeProperty>
    


    <!-- http://w3id.org/meta-share/meta-share/typeOfElement -->

    <owl:DatatypeProperty rdf:about="http://w3id.org/meta-share/meta-share/typeOfElement">
        <rdfs:domain>
            <owl:Class>
                <owl:unionOf rdf:parseType="Collection">
                    <rdf:Description rdf:about="http://w3id.org/meta-share/meta-share/DynamicElement"/>
                    <rdf:Description rdf:about="http://w3id.org/meta-share/meta-share/StaticElement"/>
                </owl:unionOf>
            </owl:Class>
        </rdfs:domain>
        <rdfs:range rdf:resource="http://www.w3.org/1999/02/22-rdf-syntax-ns#langString"/>
        <rdfs:comment xml:lang="en">Specifies the type of objects or people represented in the video or image part of the resource</rdfs:comment>
        <rdfs:label xml:lang="en">type of element</rdfs:label>
    </owl:DatatypeProperty>
    


    <!-- http://w3id.org/meta-share/meta-share/typeOfImageContent -->

    <owl:DatatypeProperty rdf:about="http://w3id.org/meta-share/meta-share/typeOfImageContent">
        <rdfs:domain>
            <owl:Class>
                <owl:unionOf rdf:parseType="Collection">
                    <rdf:Description rdf:about="http://w3id.org/meta-share/meta-share/CorpusImagePart"/>
                    <rdf:Description rdf:about="http://w3id.org/meta-share/meta-share/LanguageDescriptionImagePart"/>
                    <rdf:Description rdf:about="http://w3id.org/meta-share/meta-share/LexicalConceptualResourceImagePart"/>
                </owl:unionOf>
            </owl:Class>
        </rdfs:domain>
        <rdfs:range rdf:resource="http://www.w3.org/1999/02/22-rdf-syntax-ns#langString"/>
        <rdfs:comment xml:lang="en">The main types of object or people represented in the image corpus</rdfs:comment>
        <rdfs:label xml:lang="en">type of image content</rdfs:label>
    </owl:DatatypeProperty>
    


    <!-- http://w3id.org/meta-share/meta-share/typeOfTextNumericalContent -->

    <owl:DatatypeProperty rdf:about="http://w3id.org/meta-share/meta-share/typeOfTextNumericalContent">
        <rdfs:domain rdf:resource="http://w3id.org/meta-share/meta-share/CorpusTextNumericalPart"/>
        <rdfs:range rdf:resource="http://www.w3.org/1999/02/22-rdf-syntax-ns#langString"/>
        <rdfs:comment xml:lang="en">Specifies the content that is represented in the textNumerical part of the resource</rdfs:comment>
        <rdfs:label xml:lang="en">type of textNumerical content</rdfs:label>
    </owl:DatatypeProperty>
    


    <!-- http://w3id.org/meta-share/meta-share/typeOfVideoContent -->

    <owl:DatatypeProperty rdf:about="http://w3id.org/meta-share/meta-share/typeOfVideoContent">
        <rdfs:domain>
            <owl:Class>
                <owl:unionOf rdf:parseType="Collection">
                    <rdf:Description rdf:about="http://w3id.org/meta-share/meta-share/CorpusVideoPart"/>
                    <rdf:Description rdf:about="http://w3id.org/meta-share/meta-share/LanguageDescriptionVideoPart"/>
                    <rdf:Description rdf:about="http://w3id.org/meta-share/meta-share/LexicalConceptualResourceVideoPart"/>
                </owl:unionOf>
            </owl:Class>
        </rdfs:domain>
        <rdfs:range rdf:resource="http://www.w3.org/1999/02/22-rdf-syntax-ns#langString"/>
        <rdfs:comment xml:lang="en">Main type of object or people represented in the video</rdfs:comment>
        <rdfs:label xml:lang="en">type of video content</rdfs:label>
    </owl:DatatypeProperty>
    


    <!-- http://w3id.org/meta-share/meta-share/unitOfMeasureMetric -->

    <owl:DatatypeProperty rdf:about="http://w3id.org/meta-share/meta-share/unitOfMeasureMetric">
        <rdfs:domain rdf:resource="http://w3id.org/meta-share/meta-share/PerformanceIndicator"/>
        <rdfs:range rdf:resource="http://www.w3.org/2001/XMLSchema#string"/>
        <rdfs:comment xml:lang="en">Identifies the unit of measure used in the calculation of the metric (for the evaluation of a tool/service)</rdfs:comment>
        <rdfs:label xml:lang="en">unit of measure</rdfs:label>
    </owl:DatatypeProperty>
    


    <!-- http://w3id.org/meta-share/meta-share/updateFrequency -->

    <owl:DatatypeProperty rdf:about="http://w3id.org/meta-share/meta-share/updateFrequency">
        <rdfs:domain rdf:resource="http://w3id.org/meta-share/meta-share/LanguageResource"/>
        <rdfs:range rdf:resource="http://www.w3.org/1999/02/22-rdf-syntax-ns#langString"/>
        <rdfs:comment xml:lang="en">Specifies the frequency with which the resource is updated</rdfs:comment>
        <rdfs:label xml:lang="en">update frequency</rdfs:label>
    </owl:DatatypeProperty>
    


    <!-- http://w3id.org/meta-share/meta-share/url -->

    <owl:DatatypeProperty rdf:about="http://w3id.org/meta-share/meta-share/url">
        <rdfs:domain rdf:resource="http://www.w3.org/2002/07/owl#Thing"/>
        <rdfs:range rdf:resource="http://www.w3.org/2001/XMLSchema#anyURI"/>
        <rdfs:comment xml:lang="en">Links to a URL</rdfs:comment>
        <rdfs:label xml:lang="en">has URL</rdfs:label>
    </owl:DatatypeProperty>
    


    <!-- http://w3id.org/meta-share/meta-share/userQuery -->

    <owl:DatatypeProperty rdf:about="http://w3id.org/meta-share/meta-share/userQuery">
        <rdfs:domain rdf:resource="http://w3id.org/meta-share/meta-share/Corpus"/>
        <rdfs:range rdf:resource="http://www.w3.org/2001/XMLSchema#string"/>
        <rdfs:comment xml:lang="en">Introduces a query performed by a user that has resulted in the creation of the resource being described (e.g. a dataset created with a query aggregating texts from a database, or subset of a lexical resource, or a virtual collection of sentences from online corpora)</rdfs:comment>
        <rdfs:label xml:lang="en">user query</rdfs:label>
    </owl:DatatypeProperty>
    


    <!-- http://w3id.org/meta-share/meta-share/validated -->

    <owl:DatatypeProperty rdf:about="http://w3id.org/meta-share/meta-share/validated">
        <rdfs:domain rdf:resource="http://w3id.org/meta-share/meta-share/LanguageResource"/>
        <rdfs:range rdf:resource="http://www.w3.org/2001/XMLSchema#boolean"/>
        <rdfs:comment xml:lang="en">Specifies whether the resource has undergone a formal validation process</rdfs:comment>
        <rdfs:label xml:lang="en">validated</rdfs:label>
    </owl:DatatypeProperty>
    


    <!-- http://w3id.org/meta-share/meta-share/validationDetails -->

    <owl:DatatypeProperty rdf:about="http://w3id.org/meta-share/meta-share/validationDetails">
        <rdfs:domain rdf:resource="http://w3id.org/meta-share/meta-share/Validation"/>
        <rdfs:range rdf:resource="http://www.w3.org/1999/02/22-rdf-syntax-ns#langString"/>
        <rdfs:comment xml:lang="en">Provides additional information in the form of free text about the validation process of a language resource</rdfs:comment>
        <rdfs:label xml:lang="en">validation details</rdfs:label>
    </owl:DatatypeProperty>
    


    <!-- http://w3id.org/meta-share/meta-share/version -->

    <owl:DatatypeProperty rdf:about="http://w3id.org/meta-share/meta-share/version">
        <rdfs:subPropertyOf rdf:resource="http://purl.org/dc/terms/hasVersion"/>
        <rdfs:domain rdf:resource="http://w3id.org/meta-share/meta-share/LanguageResource"/>
        <rdfs:range rdf:resource="http://www.w3.org/2001/XMLSchema#string"/>
        <rdfs:comment xml:lang="en">Associates a language resource with a pattern that indicates its version; the recommended way is to follow the semantic versioning guidelines (http://semver.org) and use a numeric pattern of the form major_version.minor_version.patch</rdfs:comment>
        <rdfs:label xml:lang="en">version</rdfs:label>
    </owl:DatatypeProperty>
    


    <!-- http://w3id.org/meta-share/meta-share/versionDate -->

    <owl:DatatypeProperty rdf:about="http://w3id.org/meta-share/meta-share/versionDate">
        <rdfs:domain rdf:resource="http://w3id.org/meta-share/meta-share/LanguageResource"/>
        <rdfs:range rdf:resource="http://www.w3.org/2001/XMLSchema#date"/>
        <rdfs:comment xml:lang="en">Identifies the date associated with the version of the language resource being described (as a recommendation, of the latest update of the particular version)</rdfs:comment>
        <rdfs:label xml:lang="en">version date</rdfs:label>
    </owl:DatatypeProperty>
    


    <!-- http://w3id.org/meta-share/meta-share/volume -->

    <owl:DatatypeProperty rdf:about="http://w3id.org/meta-share/meta-share/volume">
        <rdfs:domain rdf:resource="http://w3id.org/meta-share/meta-share/Document"/>
        <rdfs:range rdf:resource="http://www.w3.org/2001/XMLSchema#string"/>
        <rdfs:comment xml:lang="en">Introduces the number used for the volume of a journal or a series of publications</rdfs:comment>
        <rdfs:label xml:lang="en">volume</rdfs:label>
    </owl:DatatypeProperty>
    


    <!-- http://w3id.org/meta-share/meta-share/website -->

    <owl:DatatypeProperty rdf:about="http://w3id.org/meta-share/meta-share/website">
        <rdfs:subPropertyOf rdf:resource="http://w3id.org/meta-share/meta-share/url"/>
        <rdfs:domain>
            <owl:Class>
                <owl:unionOf rdf:parseType="Collection">
                    <rdf:Description rdf:about="http://w3id.org/meta-share/meta-share/Division"/>
                    <rdf:Description rdf:about="http://w3id.org/meta-share/meta-share/Group"/>
                    <rdf:Description rdf:about="http://w3id.org/meta-share/meta-share/Organization"/>
                    <rdf:Description rdf:about="http://w3id.org/meta-share/meta-share/Project"/>
                </owl:unionOf>
            </owl:Class>
        </rdfs:domain>
        <rdfs:range rdf:resource="http://www.w3.org/2001/XMLSchema#anyURI"/>
        <rdfs:altLabel xml:lang="en">home page</rdfs:altLabel>
        <rdfs:comment xml:lang="en">Links to a URL that acts as the primary page (like a table of contents) introducing information about an organization (e.g.,  products, contact information, etc.) or project</rdfs:comment>
        <rdfs:label xml:lang="en">website</rdfs:label>
    </owl:DatatypeProperty>
    


    <!-- http://w3id.org/meta-share/meta-share/weight -->

    <owl:DatatypeProperty rdf:about="http://w3id.org/meta-share/meta-share/weight">
        <rdfs:domain rdf:resource="http://w3id.org/meta-share/meta-share/Participant"/>
        <rdfs:range rdf:resource="http://www.w3.org/2001/XMLSchema#int"/>
        <rdfs:comment xml:lang="en">Provides information on the weight of the participant</rdfs:comment>
        <rdfs:label xml:lang="en">weight</rdfs:label>
    </owl:DatatypeProperty>
    


    <!-- http://w3id.org/meta-share/meta-share/weightedGrammar -->

    <owl:DatatypeProperty rdf:about="http://w3id.org/meta-share/meta-share/weightedGrammar">
        <rdfs:domain rdf:resource="http://w3id.org/meta-share/meta-share/LanguageDescription"/>
        <rdfs:range rdf:resource="http://www.w3.org/2001/XMLSchema#boolean"/>
        <rdfs:comment xml:lang="en">Indicates whether the grammar contains numerical weights (incl. probabilities)</rdfs:comment>
        <rdfs:label xml:lang="en">weighted grammar</rdfs:label>
    </owl:DatatypeProperty>
    


    <!-- http://w3id.org/meta-share/meta-share/zipCode -->

    <owl:DatatypeProperty rdf:about="http://w3id.org/meta-share/meta-share/zipCode">
        <rdfs:domain rdf:resource="http://w3id.org/meta-share/meta-share/AddressSet"/>
        <rdfs:range rdf:resource="http://www.w3.org/2001/XMLSchema#string"/>
        <rdfs:comment xml:lang="en">The zip code of the postal address of a person or organization </rdfs:comment>
        <rdfs:label xml:lang="en">zip code</rdfs:label>
    </owl:DatatypeProperty>
    


    <!-- 
    ///////////////////////////////////////////////////////////////////////////////////////
    //
    // Classes
    //
    ///////////////////////////////////////////////////////////////////////////////////////
     -->

    


    <!-- http://creativecommons.org/ns#License -->

    <owl:Class rdf:about="http://creativecommons.org/ns#License"/>
    


    <!-- http://purl.org/spar/datacite/AgentIdentifier -->

    <owl:Class rdf:about="http://purl.org/spar/datacite/AgentIdentifier">
        <rdfs:subClassOf rdf:resource="http://purl.org/spar/datacite/Identifier"/>
    </owl:Class>
    


    <!-- http://purl.org/spar/datacite/AgentIdentifierScheme -->

    <owl:Class rdf:about="http://purl.org/spar/datacite/AgentIdentifierScheme">
        <rdfs:subClassOf rdf:resource="http://purl.org/spar/datacite/IdentifierScheme"/>
    </owl:Class>
    


    <!-- http://purl.org/spar/datacite/FunderIdentifier -->

    <owl:Class rdf:about="http://purl.org/spar/datacite/FunderIdentifier">
        <rdfs:subClassOf rdf:resource="http://purl.org/spar/datacite/AgentIdentifier"/>
        <rdfs:subClassOf>
            <owl:Restriction>
                <owl:onProperty rdf:resource="http://purl.org/spar/datacite/usesIdentifierScheme"/>
                <owl:allValuesFrom rdf:resource="http://purl.org/spar/datacite/FunderIdentifierScheme"/>
            </owl:Restriction>
        </rdfs:subClassOf>
    </owl:Class>
    


    <!-- http://purl.org/spar/datacite/FunderIdentifierScheme -->

    <owl:Class rdf:about="http://purl.org/spar/datacite/FunderIdentifierScheme">
        <rdfs:subClassOf rdf:resource="http://purl.org/spar/datacite/AgentIdentifierScheme"/>
    </owl:Class>
    


    <!-- http://purl.org/spar/datacite/Identifier -->

    <owl:Class rdf:about="http://purl.org/spar/datacite/Identifier"/>
    


    <!-- http://purl.org/spar/datacite/IdentifierScheme -->

    <owl:Class rdf:about="http://purl.org/spar/datacite/IdentifierScheme"/>
    


    <!-- http://purl.org/spar/datacite/OrganizationIdentifier -->

    <owl:Class rdf:about="http://purl.org/spar/datacite/OrganizationIdentifier">
        <rdfs:subClassOf rdf:resource="http://purl.org/spar/datacite/AgentIdentifier"/>
        <rdfs:subClassOf>
            <owl:Restriction>
                <owl:onProperty rdf:resource="http://purl.org/spar/datacite/usesIdentifierScheme"/>
                <owl:allValuesFrom rdf:resource="http://purl.org/spar/datacite/OrganizationIdentifierScheme"/>
            </owl:Restriction>
        </rdfs:subClassOf>
    </owl:Class>
    


    <!-- http://purl.org/spar/datacite/OrganizationIdentifierScheme -->

    <owl:Class rdf:about="http://purl.org/spar/datacite/OrganizationIdentifierScheme">
        <rdfs:subClassOf rdf:resource="http://purl.org/spar/datacite/AgentIdentifierScheme"/>
    </owl:Class>
    


    <!-- http://purl.org/spar/datacite/PersonalIdentifier -->

    <owl:Class rdf:about="http://purl.org/spar/datacite/PersonalIdentifier">
        <rdfs:subClassOf rdf:resource="http://purl.org/spar/datacite/AgentIdentifier"/>
        <rdfs:subClassOf>
            <owl:Restriction>
                <owl:onProperty rdf:resource="http://purl.org/spar/datacite/usesIdentifierScheme"/>
                <owl:allValuesFrom rdf:resource="http://purl.org/spar/datacite/PersonalIdentifierScheme"/>
            </owl:Restriction>
        </rdfs:subClassOf>
    </owl:Class>
    


    <!-- http://purl.org/spar/datacite/PersonalIdentifierScheme -->

    <owl:Class rdf:about="http://purl.org/spar/datacite/PersonalIdentifierScheme">
        <rdfs:subClassOf rdf:resource="http://purl.org/spar/datacite/AgentIdentifierScheme"/>
    </owl:Class>
    


    <!-- http://purl.org/spar/datacite/ResourceIdentifier -->

    <owl:Class rdf:about="http://purl.org/spar/datacite/ResourceIdentifier">
        <rdfs:subClassOf rdf:resource="http://purl.org/spar/datacite/Identifier"/>
    </owl:Class>
    


    <!-- http://purl.org/spar/datacite/ResourceIdentifierScheme -->

    <owl:Class rdf:about="http://purl.org/spar/datacite/ResourceIdentifierScheme">
        <rdfs:subClassOf rdf:resource="http://purl.org/spar/datacite/IdentifierScheme"/>
    </owl:Class>
    


    <!-- http://w3id.org/meta-share/meta-share/AccessRightsStatement -->

    <owl:Class rdf:about="http://w3id.org/meta-share/meta-share/AccessRightsStatement">
        <rdfs:subClassOf>
            <owl:Restriction>
                <owl:onProperty rdf:resource="http://purl.org/spar/datacite/hasIdentifier"/>
                <owl:allValuesFrom rdf:resource="http://w3id.org/meta-share/meta-share/AccessRightsStatementIdentifier"/>
            </owl:Restriction>
        </rdfs:subClassOf>
        <rdfs:comment xml:lang="en">A formal statement indicative of licensing terms for the use of a resource (e.g.,  open access, free to read , etc.); its semantics should be clear, preferrably formally expressed and documented at a URL</rdfs:comment>
        <rdfs:label xml:lang="en">Access rights statement</rdfs:label>
    </owl:Class>
    


    <!-- http://w3id.org/meta-share/meta-share/AccessRightsStatementIdentifier -->

    <owl:Class rdf:about="http://w3id.org/meta-share/meta-share/AccessRightsStatementIdentifier">
        <rdfs:subClassOf rdf:resource="http://purl.org/spar/datacite/Identifier"/>
        <rdfs:subClassOf>
            <owl:Restriction>
                <owl:onProperty rdf:resource="http://w3id.org/meta-share/meta-share/conformsTo"/>
                <owl:allValuesFrom rdf:resource="http://w3id.org/meta-share/meta-share/AccessRightsStatementScheme"/>
            </owl:Restriction>
        </rdfs:subClassOf>
        <rdfs:comment xml:lang="en">A string used to uniquely identify an access rights statement according to a specific scheme</rdfs:comment>
        <rdfs:label xml:lang="en">Access rights statement identifier</rdfs:label>
    </owl:Class>
    


    <!-- http://w3id.org/meta-share/meta-share/AccessRightsStatementScheme -->

    <owl:Class rdf:about="http://w3id.org/meta-share/meta-share/AccessRightsStatementScheme">
        <rdfs:subClassOf rdf:resource="http://w3id.org/meta-share/meta-share/ClassificationScheme"/>
        <rdfs:comment xml:lang="en">The name of the scheme according to which an access rights statement is assigned to a distribution</rdfs:comment>
        <rdfs:label xml:lang="en">Access rights statement scheme</rdfs:label>
    </owl:Class>
    


    <!-- http://w3id.org/meta-share/meta-share/Actor -->

    <owl:Class rdf:about="http://w3id.org/meta-share/meta-share/Actor">
        <rdfs:subClassOf rdf:resource="http://w3id.org/meta-share/meta-share/DescribedEntity"/>
        <rdfs:subClassOf rdf:resource="http://xmlns.com/foaf/0.1/Agent"/>
        <rdfs:comment xml:lang="en">A person, organization or group that participates in an event or process</rdfs:comment>
        <rdfs:label xml:lang="en">Actor</rdfs:label>
        <skos:comment xml:lang="en">Changed to subclass of foaf:agent because according to its definition (An agent (eg. person, group, software or physical artifact)), it might include entities that we do not consider at this time actors</skos:comment>
    </owl:Class>
    


    <!-- http://w3id.org/meta-share/meta-share/ActualUse -->

    <owl:Class rdf:about="http://w3id.org/meta-share/meta-share/ActualUse">
        <rdfs:comment xml:lang="en">Any activity where a language resource has been used (e.g.,  in a project, in an experiment, for a publication, etc.)</rdfs:comment>
        <rdfs:label xml:lang="en">Actual use</rdfs:label>
    </owl:Class>
    


    <!-- http://w3id.org/meta-share/meta-share/AddressSet -->

    <owl:Class rdf:about="http://w3id.org/meta-share/meta-share/AddressSet">
        <rdfs:comment xml:lang="en">A set of elements that describe the full address (i.e. including street address, zip code, etc.)</rdfs:comment>
        <rdfs:label xml:lang="en">Address</rdfs:label>
    </owl:Class>
    


    <!-- http://w3id.org/meta-share/meta-share/Affiliation -->

    <owl:Class rdf:about="http://w3id.org/meta-share/meta-share/Affiliation">
        <rdfs:comment xml:lang="en">Information the organization that a person works for (e.g.,  a company) or is affiliated with (e.g.,  university, etc.) and the data that are specific to this relation (e.g.,  position, professional contact information, etc.)</rdfs:comment>
        <rdfs:label xml:lang="en">Affiliation</rdfs:label>
    </owl:Class>
    


    <!-- http://w3id.org/meta-share/meta-share/AgeGroup -->

    <owl:Class rdf:about="http://w3id.org/meta-share/meta-share/AgeGroup">
        <rdfs:comment xml:lang="en">The age group to which the participant belongs</rdfs:comment>
        <rdfs:label xml:lang="en">Age group</rdfs:label>
    </owl:Class>
    


    <!-- http://w3id.org/meta-share/meta-share/AnnotatedElement -->

    <owl:Class rdf:about="http://w3id.org/meta-share/meta-share/AnnotatedElement">
        <rdfs:comment xml:lang="en">A type of element that can be annotated and may differ depending on the annotation level</rdfs:comment>
        <rdfs:label xml:lang="en">Annotated element</rdfs:label>
    </owl:Class>
    


    <!-- http://w3id.org/meta-share/meta-share/Annotation -->

    <owl:Class rdf:about="http://w3id.org/meta-share/meta-share/Annotation">
        <rdfs:comment xml:lang="en">The part of a corpus that contains annotations (interpretative linguistic information grounded in a knowledge resource that is added manually or automatically to a text or corpus respectively)</rdfs:comment>
        <rdfs:label xml:lang="en">Annotation</rdfs:label>
    </owl:Class>
    


    <!-- http://w3id.org/meta-share/meta-share/Application -->

    <owl:Class rdf:about="http://w3id.org/meta-share/meta-share/Application">
        <rdfs:subClassOf rdf:resource="http://w3id.org/meta-share/meta-share/ToolService"/>
        <rdfs:comment xml:lang="en">Any software program (or group of programs seen as a whole) intended for the end-user and addressing one or multiple related user needs.</rdfs:comment>
        <rdfs:label xml:lang="en">Application</rdfs:label>
    </owl:Class>
    


    <!-- http://w3id.org/meta-share/meta-share/Audience -->

    <owl:Class rdf:about="http://w3id.org/meta-share/meta-share/Audience">
        <rdfs:comment xml:lang="en">Indication of the intended audience size of a multimedia resource</rdfs:comment>
        <rdfs:label xml:lang="en">Audience</rdfs:label>
    </owl:Class>
    


    <!-- http://w3id.org/meta-share/meta-share/AudioFormat -->

    <owl:Class rdf:about="http://w3id.org/meta-share/meta-share/AudioFormat">
        <rdfs:comment xml:lang="en">The format of the audio part of a multimedia resource</rdfs:comment>
        <rdfs:label xml:lang="en">Audio format</rdfs:label>
    </owl:Class>
    


    <!-- http://w3id.org/meta-share/meta-share/AudioGenre -->

    <owl:Class rdf:about="http://w3id.org/meta-share/meta-share/AudioGenre">
        <rdfs:subClassOf rdf:resource="http://w3id.org/meta-share/meta-share/Genre"/>
        <rdfs:subClassOf>
            <owl:Restriction>
                <owl:onProperty rdf:resource="http://purl.org/spar/datacite/hasIdentifier"/>
                <owl:allValuesFrom rdf:resource="http://w3id.org/meta-share/meta-share/AudioGenreIdentifier"/>
            </owl:Restriction>
        </rdfs:subClassOf>
        <rdfs:subClassOf>
            <owl:Restriction>
                <owl:onProperty rdf:resource="http://w3id.org/meta-share/meta-share/genre"/>
                <owl:allValuesFrom rdf:resource="http://w3id.org/meta-share/meta-share/CorpusAudioPart"/>
            </owl:Restriction>
        </rdfs:subClassOf>
        <rdfs:comment xml:lang="en">A classification of audio parts based on extra-linguistic and internal linguistic criteria and reflected on the audio style, form or content</rdfs:comment>
        <rdfs:label xml:lang="en">Audio genre</rdfs:label>
    </owl:Class>
    


    <!-- http://w3id.org/meta-share/meta-share/AudioGenreClassificationScheme -->

    <owl:Class rdf:about="http://w3id.org/meta-share/meta-share/AudioGenreClassificationScheme">
        <rdfs:subClassOf rdf:resource="http://w3id.org/meta-share/meta-share/ClassificationScheme"/>
        <rdfs:comment xml:lang="en">A classification scheme devised for audio genres by an organization/authority</rdfs:comment>
        <rdfs:label xml:lang="en">Audio genre classification scheme</rdfs:label>
    </owl:Class>
    


    <!-- http://w3id.org/meta-share/meta-share/AudioGenreIdentifier -->

    <owl:Class rdf:about="http://w3id.org/meta-share/meta-share/AudioGenreIdentifier">
        <rdfs:subClassOf rdf:resource="http://purl.org/spar/datacite/Identifier"/>
        <rdfs:subClassOf>
            <owl:Restriction>
                <owl:onProperty rdf:resource="http://w3id.org/meta-share/meta-share/conformsTo"/>
                <owl:allValuesFrom rdf:resource="http://w3id.org/meta-share/meta-share/AudioGenreClassificationScheme"/>
            </owl:Restriction>
        </rdfs:subClassOf>
        <rdfs:comment xml:lang="en">A string used to uniquely identify an audio genre according to a specific classification scheme</rdfs:comment>
        <rdfs:label xml:lang="en">Audio genre identifier</rdfs:label>
    </owl:Class>
    


    <!-- http://w3id.org/meta-share/meta-share/AudioQualityMeasureIncluded -->

    <owl:Class rdf:about="http://w3id.org/meta-share/meta-share/AudioQualityMeasureIncluded">
        <rdfs:comment xml:lang="en">The audio quality measures included in audio format</rdfs:comment>
        <rdfs:label xml:lang="en">Audio quality measure included</rdfs:label>
    </owl:Class>
    


    <!-- http://w3id.org/meta-share/meta-share/AudioType -->

    <owl:Class rdf:about="http://w3id.org/meta-share/meta-share/AudioType">
        <rdfs:subClassOf rdf:resource="http://w3id.org/meta-share/meta-share/ContentType"/>
        <rdfs:comment xml:lang="en">A type of content included in a language resource pertaining to the audio level</rdfs:comment>
        <rdfs:label xml:lang="en">Audio type</rdfs:label>
    </owl:Class>
    


    <!-- http://w3id.org/meta-share/meta-share/Availability -->

    <owl:Class rdf:about="http://w3id.org/meta-share/meta-share/Availability">
        <rdfs:comment xml:lang="en">Availability status of the resource; conditionsOfUse can be further used to indicate the specific terms of availability</rdfs:comment>
        <rdfs:label xml:lang="en">Availability</rdfs:label>
        <skos:note xml:lang="en">Is there a point of keeping it? makes sense only for &quot;under negotiation&quot; and &apos;availableThroughOtherDistributors&apos; [change the value]; maybe also &quot;availableThroughOwnerOnly&quot;???</skos:note>
    </owl:Class>
    


    <!-- http://w3id.org/meta-share/meta-share/BaseItem -->

    <owl:Class rdf:about="http://w3id.org/meta-share/meta-share/BaseItem">
        <rdfs:comment xml:lang="en">Type of item that is represented in the n-gram resource</rdfs:comment>
        <rdfs:label xml:lang="en">Base item</rdfs:label>
    </owl:Class>
    


    <!-- http://w3id.org/meta-share/meta-share/BodyPart -->

    <owl:Class rdf:about="http://w3id.org/meta-share/meta-share/BodyPart">
        <rdfs:comment xml:lang="en">The body parts visible in the video or image part of the resource</rdfs:comment>
        <rdfs:label xml:lang="en">Body part</rdfs:label>
    </owl:Class>
    


    <!-- http://w3id.org/meta-share/meta-share/ByteOrder -->

    <owl:Class rdf:about="http://w3id.org/meta-share/meta-share/ByteOrder">
        <rdfs:comment xml:lang="en">The byte order of 2 or more bytes sample</rdfs:comment>
        <rdfs:label xml:lang="en">Byte order</rdfs:label>
    </owl:Class>
    


    <!-- http://w3id.org/meta-share/meta-share/CapturingDeviceType -->

    <owl:Class rdf:about="http://w3id.org/meta-share/meta-share/CapturingDeviceType">
        <rdfs:comment xml:lang="en">The type of transducers through which the data is captured</rdfs:comment>
        <rdfs:label xml:lang="en">Capturing device type</rdfs:label>
    </owl:Class>
    


    <!-- http://w3id.org/meta-share/meta-share/CapturingEnvironment -->

    <owl:Class rdf:about="http://w3id.org/meta-share/meta-share/CapturingEnvironment">
        <rdfs:comment xml:lang="en">The type of the capturing environment in terms of complexity</rdfs:comment>
        <rdfs:label xml:lang="en">Capturing environment</rdfs:label>
    </owl:Class>
    


    <!-- http://w3id.org/meta-share/meta-share/CharacterEncoding -->

    <owl:Class rdf:about="http://w3id.org/meta-share/meta-share/CharacterEncoding">
        <rdfs:comment xml:lang="en">The name of the character encoding used in the resource or accepted by the tool/service</rdfs:comment>
        <rdfs:label xml:lang="en">Character encoding</rdfs:label>
    </owl:Class>
    


    <!-- http://w3id.org/meta-share/meta-share/Classification -->

    <owl:Class rdf:about="http://w3id.org/meta-share/meta-share/Classification">
        <rdfs:comment xml:lang="en">A type of classifying (arranging in groups/categories) language resources</rdfs:comment>
        <rdfs:label xml:lang="en">Classification</rdfs:label>
    </owl:Class>
    


    <!-- http://w3id.org/meta-share/meta-share/ClassificationScheme -->

    <owl:Class rdf:about="http://w3id.org/meta-share/meta-share/ClassificationScheme">
        <rdfs:comment xml:lang="en">Scheme used for the classification of a language resource based on various criteria (e.g.,  domains, text types, genres , etc.)</rdfs:comment>
        <rdfs:label xml:lang="en">Classification scheme</rdfs:label>
    </owl:Class>
    


    <!-- http://w3id.org/meta-share/meta-share/ColourSpace -->

    <owl:Class rdf:about="http://w3id.org/meta-share/meta-share/ColourSpace">
        <rdfs:comment xml:lang="en">The colour space for the video and image part(s) of a resource</rdfs:comment>
        <rdfs:label xml:lang="en">Colour space</rdfs:label>
    </owl:Class>
    


    <!-- http://w3id.org/meta-share/meta-share/CompatibleLexiconType -->

    <owl:Class rdf:about="http://w3id.org/meta-share/meta-share/CompatibleLexiconType">
        <rdfs:comment xml:lang="en">A classification into types for lexical lexicon that can be used with the grammar being described</rdfs:comment>
        <rdfs:label xml:lang="en">Compatible lexicon type</rdfs:label>
    </owl:Class>
    


    <!-- http://w3id.org/meta-share/meta-share/Component -->

    <owl:Class rdf:about="http://w3id.org/meta-share/meta-share/Component">
        <rdfs:subClassOf rdf:resource="http://w3id.org/meta-share/meta-share/ToolService"/>
        <rdfs:comment xml:lang="en">A piece of software typically intended for a specific technical purpose, such as a particular implementation of a part-of-speech tagger (e.g TreeTagger), a tree parsing program (e.g.,  mstparser), etc. It is wrapped in a standard way within a particular component-oriented framework such as UIMA, GATE, etc. or as a specific type of web service.</rdfs:comment>
        <rdfs:label xml:lang="en">Component</rdfs:label>
    </owl:Class>
    


    <!-- http://w3id.org/meta-share/meta-share/CompressionName -->

    <owl:Class rdf:about="http://w3id.org/meta-share/meta-share/CompressionName">
        <rdfs:comment xml:lang="en">The name of the compression applied</rdfs:comment>
        <rdfs:label xml:lang="en">Compression name</rdfs:label>
    </owl:Class>
    


    <!-- http://w3id.org/meta-share/meta-share/ConditionOfUse -->

    <owl:Class rdf:about="http://w3id.org/meta-share/meta-share/ConditionOfUse">
        <dct:replaces rdf:resource="http://www.ilsp.gr/META-XMLSchema#restrictionsOfUse"/>
        <rdfs:comment xml:lang="en">A condition imposed via a specified licence on the use of a language resource (e.g.,  non-commercial use, no derivatives, etc.)</rdfs:comment>
        <rdfs:label xml:lang="en">Condition of use</rdfs:label>
    </owl:Class>
    


    <!-- http://w3id.org/meta-share/meta-share/ContentType -->

    <owl:Class rdf:about="http://w3id.org/meta-share/meta-share/ContentType">
        <rdfs:comment xml:lang="en">A more detailed account of the linguistic information contained in the lexical/conceptual resource</rdfs:comment>
        <rdfs:label xml:lang="en">Content type</rdfs:label>
        <skos:note xml:lang="en">could we organise them hierarchically?
for those that are used for annotation, align with annotationType values? or can we use annotationType together with these values as range for the property?
add definitions to all instances</skos:note>
    </owl:Class>
    


    <!-- http://w3id.org/meta-share/meta-share/ConversationalType -->

    <owl:Class rdf:about="http://w3id.org/meta-share/meta-share/ConversationalType">
        <rdfs:comment xml:lang="en">Classification of the conversation included in a multimedia resource based on the number of participants</rdfs:comment>
        <rdfs:label xml:lang="en">Conversational type</rdfs:label>
    </owl:Class>
    


    <!-- http://w3id.org/meta-share/meta-share/Corpus -->

    <owl:Class rdf:about="http://w3id.org/meta-share/meta-share/Corpus">
        <rdfs:subClassOf rdf:resource="http://w3id.org/meta-share/meta-share/DataLanguageResource"/>
        <rdfs:subClassOf>
            <owl:Restriction>
                <owl:onProperty rdf:resource="http://w3id.org/meta-share/meta-share/distribution"/>
                <owl:allValuesFrom rdf:resource="http://w3id.org/meta-share/meta-share/DatasetDistribution"/>
            </owl:Restriction>
        </rdfs:subClassOf>
        <rdfs:comment xml:lang="en">A structured collection of pieces of data (textual, audio, video, multimodal/multimedia, etc.) typically of considerable size and selected according to criteria external to the data (e.g.,  size, type of language, type of text producers or expected audience, etc.) to represent as comprehensively as possible the object of study</rdfs:comment>
        <rdfs:label xml:lang="en">Corpus</rdfs:label>
    </owl:Class>
    


    <!-- http://w3id.org/meta-share/meta-share/CorpusAudioPart -->

    <owl:Class rdf:about="http://w3id.org/meta-share/meta-share/CorpusAudioPart">
        <rdfs:subClassOf rdf:resource="http://w3id.org/meta-share/meta-share/CorpusMediaPart"/>
        <rdfs:comment xml:lang="en">The part of a corpus (or whole corpus) that consists of audio segments</rdfs:comment>
        <rdfs:label xml:lang="en">Corpus audio part</rdfs:label>
    </owl:Class>
    


    <!-- http://w3id.org/meta-share/meta-share/CorpusImagePart -->

    <owl:Class rdf:about="http://w3id.org/meta-share/meta-share/CorpusImagePart">
        <rdfs:subClassOf rdf:resource="http://w3id.org/meta-share/meta-share/CorpusMediaPart"/>
        <rdfs:comment xml:lang="en">The part of a corpus (or whole corpus) that consists of images (e.g., g a corpus of photographs and their captions)</rdfs:comment>
        <rdfs:label xml:lang="en">Corpus image part</rdfs:label>
    </owl:Class>
    


    <!-- http://w3id.org/meta-share/meta-share/CorpusMediaPart -->

    <owl:Class rdf:about="http://w3id.org/meta-share/meta-share/CorpusMediaPart">
        <rdfs:subClassOf rdf:resource="http://w3id.org/meta-share/meta-share/MediaPart"/>
        <rdfs:comment xml:lang="en">A part/segment of a corpus based on its media type classification</rdfs:comment>
        <rdfs:label xml:lang="en">Corpus media part</rdfs:label>
    </owl:Class>
    


    <!-- http://w3id.org/meta-share/meta-share/CorpusSubclass -->

    <owl:Class rdf:about="http://w3id.org/meta-share/meta-share/CorpusSubclass">
        <rdfs:comment xml:lang="en">A classification of corpora into types (used for descriptive reasons)</rdfs:comment>
        <rdfs:label xml:lang="en">Corpus subclass</rdfs:label>
    </owl:Class>
    


    <!-- http://w3id.org/meta-share/meta-share/CorpusTextNumericalPart -->

    <owl:Class rdf:about="http://w3id.org/meta-share/meta-share/CorpusTextNumericalPart">
        <rdfs:subClassOf rdf:resource="http://w3id.org/meta-share/meta-share/CorpusMediaPart"/>
        <rdfs:comment xml:lang="en">The part of a corpus (or whole corpus) that consists of sets of textual representations of measurements and observations linked to sensorimotor recordings</rdfs:comment>
        <rdfs:label xml:lang="en">Corpus text numerical part</rdfs:label>
    </owl:Class>
    


    <!-- http://w3id.org/meta-share/meta-share/CorpusTextPart -->

    <owl:Class rdf:about="http://w3id.org/meta-share/meta-share/CorpusTextPart">
        <rdfs:subClassOf rdf:resource="http://w3id.org/meta-share/meta-share/CorpusMediaPart"/>
        <rdfs:comment xml:lang="en">The part of a corpus (or a whole corpus) that consists of textual segments (e.g.,  a corpus of publications, or transcriptions of an oral corpus, or subtitles , etc.)</rdfs:comment>
        <rdfs:label xml:lang="en">Corpus text part</rdfs:label>
    </owl:Class>
    


    <!-- http://w3id.org/meta-share/meta-share/CorpusVideoPart -->

    <owl:Class rdf:about="http://w3id.org/meta-share/meta-share/CorpusVideoPart">
        <rdfs:subClassOf rdf:resource="http://w3id.org/meta-share/meta-share/CorpusMediaPart"/>
        <rdfs:comment xml:lang="en">The part of a corpus (or whole corpus) that consists of video files (e.g.,  a corpus of film documentaries)</rdfs:comment>
        <rdfs:label xml:lang="en">Corpus video part</rdfs:label>
    </owl:Class>
    


    <!-- http://w3id.org/meta-share/meta-share/Cost -->

    <owl:Class rdf:about="http://w3id.org/meta-share/meta-share/Cost">
        <rdfs:comment xml:lang="en">The cost for accessing a resource formally desribed as a set of amount and currency unit</rdfs:comment>
        <rdfs:label xml:lang="en">Cost</rdfs:label>
    </owl:Class>
    


    <!-- http://w3id.org/meta-share/meta-share/Country -->

    <owl:Class rdf:about="http://w3id.org/meta-share/meta-share/Country">
        <rdfs:comment xml:lang="en">The name of a country preferrably according to ISO 639</rdfs:comment>
        <rdfs:label xml:lang="en">Country</rdfs:label>
        <skos:note xml:lang="en">add here the dataset from EU NAL</skos:note>
    </owl:Class>
    


    <!-- http://w3id.org/meta-share/meta-share/Currency -->

    <owl:Class rdf:about="http://w3id.org/meta-share/meta-share/Currency">
        <rdfs:comment xml:lang="en">Any system of money used in a particular country</rdfs:comment>
        <rdfs:label xml:lang="en">Currency</rdfs:label>
    </owl:Class>
    


    <!-- http://w3id.org/meta-share/meta-share/DataLanguageResource -->

    <owl:Class rdf:about="http://w3id.org/meta-share/meta-share/DataLanguageResource">
        <rdfs:subClassOf rdf:resource="http://w3id.org/meta-share/meta-share/LanguageResource"/>
        <rdfs:comment xml:lang="en">A resource composed of linguistic material used to assist and augment language processing applications, but also, in a broader sense, in language and language-mediated research studies and applications; examples include data sets (textual, multimodal/multimedia and lexical data, grammars, language models, etc.) in machine readable form</rdfs:comment>
        <rdfs:label xml:lang="en">Data language resource</rdfs:label>
    </owl:Class>
    


    <!-- http://w3id.org/meta-share/meta-share/DatasetDistribution -->

    <owl:Class rdf:about="http://w3id.org/meta-share/meta-share/DatasetDistribution">
        <rdfs:subClassOf rdf:resource="http://w3id.org/meta-share/meta-share/Distribution"/>
        <rdfs:subClassOf>
            <owl:Restriction>
                <owl:onProperty rdf:resource="http://w3id.org/meta-share/meta-share/distributionForm"/>
                <owl:allValuesFrom rdf:resource="http://w3id.org/meta-share/meta-share/DatasetDistributionForm"/>
            </owl:Restriction>
        </rdfs:subClassOf>
        <rdfs:comment xml:lang="en">Any form with which a dataset is distributed, such as a downloadable form in a specific format (e.g.,  spreadsheet, plain text , etc.) or an API with which it can be accessed</rdfs:comment>
        <rdfs:label xml:lang="en">Dataset distribution</rdfs:label>
    </owl:Class>
    


    <!-- http://w3id.org/meta-share/meta-share/DatasetDistributionForm -->

    <owl:Class rdf:about="http://w3id.org/meta-share/meta-share/DatasetDistributionForm">
        <rdfs:subClassOf rdf:resource="http://w3id.org/meta-share/meta-share/DistributionForm"/>
        <rdfs:comment xml:lang="en">The form (medium/channel) used for distributing a language resource consisting of data (e.g.,  a corpus, a lexicon, etc.)</rdfs:comment>
        <rdfs:label xml:lang="en">Dataset distribution form</rdfs:label>
    </owl:Class>
    


    <!-- http://w3id.org/meta-share/meta-share/DescribedEntity -->

    <owl:Class rdf:about="http://w3id.org/meta-share/meta-share/DescribedEntity">
        <rdfs:comment xml:lang="en">The (type of) entity that is being described by a metadata record</rdfs:comment>
        <rdfs:label xml:lang="en">type of described entity</rdfs:label>
    </owl:Class>
    


    <!-- http://w3id.org/meta-share/meta-share/Distribution -->

    <owl:Class rdf:about="http://w3id.org/meta-share/meta-share/Distribution">
        <rdfs:comment xml:lang="en">Any form with which a language resource is distributed; for software, this can refer to web services, executable or code files, etc.; for datasets, it can be a downloadable form in a specific format (e.g.,  spreadsheet, plain text , etc.) or an API with which it can be accessed</rdfs:comment>
        <rdfs:label xml:lang="en">Distribution</rdfs:label>
    </owl:Class>
    


    <!-- http://w3id.org/meta-share/meta-share/DistributionAudioFeature -->

    <owl:Class rdf:about="http://w3id.org/meta-share/meta-share/DistributionAudioFeature">
        <rdfs:comment xml:lang="en">A feature that can be used for describing distinct distributable forms of audio resources/parts</rdfs:comment>
        <rdfs:label xml:lang="en">Distribution audio feature</rdfs:label>
    </owl:Class>
    


    <!-- http://w3id.org/meta-share/meta-share/DistributionForm -->

    <owl:Class rdf:about="http://w3id.org/meta-share/meta-share/DistributionForm">
        <rdfs:comment xml:lang="en">Τhe form used for distributing (delivering or providing access) to the resource</rdfs:comment>
        <rdfs:label xml:lang="en">Distribution form</rdfs:label>
    </owl:Class>
    


    <!-- http://w3id.org/meta-share/meta-share/DistributionImageFeature -->

    <owl:Class rdf:about="http://w3id.org/meta-share/meta-share/DistributionImageFeature">
        <rdfs:comment xml:lang="en">A feature that can be used for describing distinct distributable forms of image resources/parts</rdfs:comment>
        <rdfs:label xml:lang="en">Distribution image feature</rdfs:label>
    </owl:Class>
    


    <!-- http://w3id.org/meta-share/meta-share/DistributionTextFeature -->

    <owl:Class rdf:about="http://w3id.org/meta-share/meta-share/DistributionTextFeature">
        <rdfs:comment xml:lang="en">A feature that can be used for describing distinct distributable forms of text resources/parts</rdfs:comment>
        <rdfs:label xml:lang="en">Distribution text feature</rdfs:label>
    </owl:Class>
    


    <!-- http://w3id.org/meta-share/meta-share/DistributionTextNumericalFeature -->

    <owl:Class rdf:about="http://w3id.org/meta-share/meta-share/DistributionTextNumericalFeature">
        <rdfs:comment xml:lang="en">A feature that can be used for describing distinct distributable forms of numerical text resources/parts</rdfs:comment>
        <rdfs:label xml:lang="en">Distribution text numerical feature</rdfs:label>
    </owl:Class>
    


    <!-- http://w3id.org/meta-share/meta-share/DistributionVideoFeature -->

    <owl:Class rdf:about="http://w3id.org/meta-share/meta-share/DistributionVideoFeature">
        <rdfs:comment xml:lang="en">A feature that can be used for describing distinct distributable forms of video resources/parts</rdfs:comment>
        <rdfs:label xml:lang="en">Distribution video feature</rdfs:label>
    </owl:Class>
    


    <!-- http://w3id.org/meta-share/meta-share/Division -->

    <owl:Class rdf:about="http://w3id.org/meta-share/meta-share/Division">
        <rdfs:comment xml:lang="en">A section of a larger organization (e.g.,  school, faculty, department of a university, department or branch of a company, etc.)</rdfs:comment>
        <rdfs:label xml:lang="en">Division</rdfs:label>
    </owl:Class>
    


    <!-- http://w3id.org/meta-share/meta-share/DivisionCategory -->

    <owl:Class rdf:about="http://w3id.org/meta-share/meta-share/DivisionCategory">
        <rdfs:comment xml:lang="en">A controlled vocabulary used for classifying divisions</rdfs:comment>
        <rdfs:label xml:lang="en">Division category</rdfs:label>
    </owl:Class>
    


    <!-- http://w3id.org/meta-share/meta-share/Document -->

    <owl:Class rdf:about="http://w3id.org/meta-share/meta-share/Document">
        <rdfs:subClassOf rdf:resource="http://w3id.org/meta-share/meta-share/DescribedEntity"/>
        <rdfs:comment xml:lang="en">A piece of written, printed, or electronic matter that is primarily intended for reading</rdfs:comment>
        <rdfs:label xml:lang="en">Document</rdfs:label>
    </owl:Class>
    


    <!-- http://w3id.org/meta-share/meta-share/DocumentIdentifier -->

    <owl:Class rdf:about="http://w3id.org/meta-share/meta-share/DocumentIdentifier">
        <rdfs:subClassOf rdf:resource="http://purl.org/spar/datacite/ResourceIdentifier"/>
        <rdfs:subClassOf>
            <owl:Restriction>
                <owl:onProperty rdf:resource="http://purl.org/spar/datacite/usesIdentifierScheme"/>
                <owl:allValuesFrom rdf:resource="http://w3id.org/meta-share/meta-share/DocumentIdentifierScheme"/>
            </owl:Restriction>
        </rdfs:subClassOf>
        <rdfs:comment xml:lang="en">A string (e.g.,  PID, DOI, internal to an organization , etc.) used to uniquely identify a document (mainly intended for published documents)</rdfs:comment>
        <rdfs:label xml:lang="en">Document identifier</rdfs:label>
    </owl:Class>
    


    <!-- http://w3id.org/meta-share/meta-share/DocumentIdentifierScheme -->

    <owl:Class rdf:about="http://w3id.org/meta-share/meta-share/DocumentIdentifierScheme">
        <rdfs:subClassOf rdf:resource="http://purl.org/spar/datacite/ResourceIdentifierScheme"/>
        <rdfs:comment xml:lang="en">A scheme according to which an identifier is assigned by the authority that issues it (e.g.,  DOI, PubMed Central , etc.) specifically for publications</rdfs:comment>
        <rdfs:label xml:lang="en">Document identifier scheme</rdfs:label>
    </owl:Class>
    


    <!-- http://w3id.org/meta-share/meta-share/DocumentType -->

    <owl:Class rdf:about="http://w3id.org/meta-share/meta-share/DocumentType">
        <rdfs:comment xml:lang="en">A classification vocabulary for documents (e.g.,  article, book, etc.)</rdfs:comment>
        <rdfs:label xml:lang="en">Document type</rdfs:label>
    </owl:Class>
    


    <!-- http://w3id.org/meta-share/meta-share/DocumentationType -->

    <owl:Class rdf:about="http://w3id.org/meta-share/meta-share/DocumentationType">
        <rdfs:comment xml:lang="en">The type of the documentation vis-a-vis its relation with the language resource (e.g.,  general publication, user manual, etc.)</rdfs:comment>
        <rdfs:label xml:lang="en">Documentation type</rdfs:label>
    </owl:Class>
    


    <!-- http://w3id.org/meta-share/meta-share/Domain -->

    <owl:Class rdf:about="http://w3id.org/meta-share/meta-share/Domain">
        <rdfs:subClassOf rdf:resource="http://w3id.org/meta-share/meta-share/Classification"/>
        <rdfs:subClassOf>
            <owl:Restriction>
                <owl:onProperty rdf:resource="http://purl.org/spar/datacite/hasIdentifier"/>
                <owl:allValuesFrom rdf:resource="http://w3id.org/meta-share/meta-share/DomainIdentifier"/>
            </owl:Restriction>
        </rdfs:subClassOf>
        <rdfs:comment xml:lang="en">A particular field of thought, activity, or interest [adapted from https://www.collinsdictionary.com/dictionary/english/domain]</rdfs:comment>
        <rdfs:label xml:lang="en">Domain</rdfs:label>
    </owl:Class>
    


    <!-- http://w3id.org/meta-share/meta-share/DomainClassificationScheme -->

    <owl:Class rdf:about="http://w3id.org/meta-share/meta-share/DomainClassificationScheme">
        <rdfs:subClassOf rdf:resource="http://w3id.org/meta-share/meta-share/ClassificationScheme"/>
        <rdfs:comment xml:lang="en">A classification scheme devised by an authority for domains</rdfs:comment>
        <rdfs:label xml:lang="en">Domain classification scheme</rdfs:label>
    </owl:Class>
    


    <!-- http://w3id.org/meta-share/meta-share/DomainIdentifier -->

    <owl:Class rdf:about="http://w3id.org/meta-share/meta-share/DomainIdentifier">
        <rdfs:subClassOf rdf:resource="http://purl.org/spar/datacite/Identifier"/>
        <rdfs:subClassOf>
            <owl:Restriction>
                <owl:onProperty rdf:resource="http://w3id.org/meta-share/meta-share/conformsTo"/>
                <owl:allValuesFrom rdf:resource="http://w3id.org/meta-share/meta-share/DomainClassificationScheme"/>
            </owl:Restriction>
        </rdfs:subClassOf>
        <rdfs:comment xml:lang="en">A string used to uniquely identify a domain according to a specific classification scheme</rdfs:comment>
        <rdfs:label xml:lang="en">Domain identifier</rdfs:label>
    </owl:Class>
    


    <!-- http://w3id.org/meta-share/meta-share/Duration -->

    <owl:Class rdf:about="http://w3id.org/meta-share/meta-share/Duration">
        <rdfs:comment xml:lang="en">The time that an audio or video recording , etc. lasts</rdfs:comment>
        <rdfs:label xml:lang="en">Duration of audio</rdfs:label>
    </owl:Class>
    


    <!-- http://w3id.org/meta-share/meta-share/DurationUnit -->

    <owl:Class rdf:about="http://w3id.org/meta-share/meta-share/DurationUnit">
        <rdfs:comment xml:lang="en">A unit for measuring duration of audio / video parts</rdfs:comment>
        <rdfs:label xml:lang="en">Duration unit</rdfs:label>
    </owl:Class>
    


    <!-- http://w3id.org/meta-share/meta-share/DynamicElement -->

    <owl:Class rdf:about="http://w3id.org/meta-share/meta-share/DynamicElement">
        <rdfs:comment xml:lang="en">Element represented in the video part of a resource</rdfs:comment>
        <rdfs:label xml:lang="en">Dynamic element</rdfs:label>
    </owl:Class>
    


    <!-- http://w3id.org/meta-share/meta-share/EncodingLevel -->

    <owl:Class rdf:about="http://w3id.org/meta-share/meta-share/EncodingLevel">
        <rdfs:comment xml:lang="en">The linguistic level of analysis a lexical/conceptual resource or language description caters for as represented in its contents</rdfs:comment>
        <rdfs:label xml:lang="en">Encoding level</rdfs:label>
    </owl:Class>
    


    <!-- http://w3id.org/meta-share/meta-share/Evaluation -->

    <owl:Class rdf:about="http://w3id.org/meta-share/meta-share/Evaluation">
        <rdfs:comment xml:lang="en">Each of the procedures and outcomes followed for evaluating the performance and other features of a tool/service</rdfs:comment>
        <rdfs:label xml:lang="en">Evaluation</rdfs:label>
    </owl:Class>
    


    <!-- http://w3id.org/meta-share/meta-share/EvaluationCriterion -->

    <owl:Class rdf:about="http://w3id.org/meta-share/meta-share/EvaluationCriterion">
        <rdfs:comment xml:lang="en">The criterion of the evaluation of a tool</rdfs:comment>
        <rdfs:label xml:lang="en">Evaluation criterion</rdfs:label>
    </owl:Class>
    


    <!-- http://w3id.org/meta-share/meta-share/EvaluationLevel -->

    <owl:Class rdf:about="http://w3id.org/meta-share/meta-share/EvaluationLevel">
        <rdfs:comment xml:lang="en">The evaluation level</rdfs:comment>
        <rdfs:label xml:lang="en">Evaluation level</rdfs:label>
    </owl:Class>
    


    <!-- http://w3id.org/meta-share/meta-share/EvaluationMeasure -->

    <owl:Class rdf:about="http://w3id.org/meta-share/meta-share/EvaluationMeasure">
        <rdfs:comment xml:lang="en">The evaluation measure (human or automatic)</rdfs:comment>
        <rdfs:label xml:lang="en">Evaluation measure</rdfs:label>
    </owl:Class>
    


    <!-- http://w3id.org/meta-share/meta-share/EvaluationType -->

    <owl:Class rdf:about="http://w3id.org/meta-share/meta-share/EvaluationType">
        <rdfs:comment xml:lang="en">Indicates the type of evaluation performed on a tool/service</rdfs:comment>
        <rdfs:label xml:lang="en">Evaluation type</rdfs:label>
    </owl:Class>
    


    <!-- http://w3id.org/meta-share/meta-share/ExtratextualInformation -->

    <owl:Class rdf:about="http://w3id.org/meta-share/meta-share/ExtratextualInformation">
        <rdfs:comment xml:lang="en">The non-textual information contained in a lexical/conceptual resouce (e.g.,  images, videos, audios , etc.); it can be used as an alternative to fully describing them as a proper part of the resource when they are not as important as the textual part (e.g.,  cases of a dictionary with images attached to some lemmas)</rdfs:comment>
        <rdfs:label xml:lang="en">Extratextual information</rdfs:label>
    </owl:Class>
    


    <!-- http://w3id.org/meta-share/meta-share/ExtratextualInformationUnit -->

    <owl:Class rdf:about="http://w3id.org/meta-share/meta-share/ExtratextualInformationUnit">
        <rdfs:comment xml:lang="en">The unit on which the extratextual information in a lexical/conceptual resource is attached</rdfs:comment>
        <rdfs:label xml:lang="en">Extratextual information unit</rdfs:label>
    </owl:Class>
    


    <!-- http://w3id.org/meta-share/meta-share/Framework -->

    <owl:Class rdf:about="http://w3id.org/meta-share/meta-share/Framework">
        <rdfs:comment xml:lang="en">The implementation framework used for developing and running a tool/service</rdfs:comment>
        <rdfs:label xml:lang="en">Framework</rdfs:label>
    </owl:Class>
    


    <!-- http://w3id.org/meta-share/meta-share/FundingType -->

    <owl:Class rdf:about="http://w3id.org/meta-share/meta-share/FundingType">
        <rdfs:comment xml:lang="en">A classification of the funding of a project with regard to the source of the funds</rdfs:comment>
        <rdfs:label xml:lang="en">Funding type</rdfs:label>
    </owl:Class>
    


    <!-- http://w3id.org/meta-share/meta-share/Genre -->

    <owl:Class rdf:about="http://w3id.org/meta-share/meta-share/Genre">
        <rdfs:subClassOf rdf:resource="http://w3id.org/meta-share/meta-share/Classification"/>
        <rdfs:comment xml:lang="en">A way of classifying a language resource with regard to the style, form and content</rdfs:comment>
        <rdfs:label xml:lang="en">Genre</rdfs:label>
    </owl:Class>
    


    <!-- http://w3id.org/meta-share/meta-share/Grammar -->

    <owl:Class rdf:about="http://w3id.org/meta-share/meta-share/Grammar">
        <rdfs:subClassOf rdf:resource="http://w3id.org/meta-share/meta-share/LanguageDescription"/>
        <rdfs:comment xml:lang="en">A set of rules governing what strings are valid or allowable in a language or text [https://en.oxforddictionaries.com/definition/grammar]</rdfs:comment>
        <rdfs:label xml:lang="en">Grammar</rdfs:label>
    </owl:Class>
    


    <!-- http://w3id.org/meta-share/meta-share/GrammaticalPhenomenaCoverage -->

    <owl:Class rdf:about="http://w3id.org/meta-share/meta-share/GrammaticalPhenomenaCoverage">
        <rdfs:comment xml:lang="en">An indication of the grammatical phenomena covered by the grammar</rdfs:comment>
        <rdfs:label xml:lang="en">Grammatical phenomena coverage</rdfs:label>
    </owl:Class>
    


    <!-- http://w3id.org/meta-share/meta-share/Group -->

    <owl:Class rdf:about="http://w3id.org/meta-share/meta-share/Group">
        <rdfs:comment xml:lang="en">A set of persons related to some aspect of a language resource, that do not have a legal status (e.g.,  a group of software developers working on the same software)</rdfs:comment>
        <rdfs:label xml:lang="en">Group</rdfs:label>
    </owl:Class>
    


    <!-- http://w3id.org/meta-share/meta-share/GroupIdentifier -->

    <owl:Class rdf:about="http://w3id.org/meta-share/meta-share/GroupIdentifier">
        <rdfs:subClassOf rdf:resource="http://purl.org/spar/datacite/AgentIdentifier"/>
        <rdfs:subClassOf>
            <owl:Restriction>
                <owl:onProperty rdf:resource="http://purl.org/spar/datacite/usesIdentifierScheme"/>
                <owl:allValuesFrom rdf:resource="http://purl.org/spar/datacite/OrganizationIdentifierScheme"/>
            </owl:Restriction>
        </rdfs:subClassOf>
        <rdfs:comment xml:lang="en">A string used to uniquely identify a group</rdfs:comment>
        <rdfs:label xml:lang="en">Group identifier</rdfs:label>
    </owl:Class>
    


    <!-- http://w3id.org/meta-share/meta-share/HearingImpairmentOfParticipants -->

    <owl:Class rdf:about="http://w3id.org/meta-share/meta-share/HearingImpairmentOfParticipants">
        <rdfs:comment xml:lang="en">Whether the group of participants contains persons with hearing impairments</rdfs:comment>
        <rdfs:label xml:lang="en">Hearing impairment of participants</rdfs:label>
    </owl:Class>
    


    <!-- http://w3id.org/meta-share/meta-share/ImageFormat -->

    <owl:Class rdf:about="http://w3id.org/meta-share/meta-share/ImageFormat">
        <rdfs:comment xml:lang="en">The format used for the image part of a resource</rdfs:comment>
        <rdfs:label xml:lang="en">Image format</rdfs:label>
    </owl:Class>
    


    <!-- http://w3id.org/meta-share/meta-share/ImageGenre -->

    <owl:Class rdf:about="http://w3id.org/meta-share/meta-share/ImageGenre">
        <rdfs:subClassOf rdf:resource="http://w3id.org/meta-share/meta-share/Genre"/>
        <rdfs:subClassOf>
            <owl:Restriction>
                <owl:onProperty rdf:resource="http://purl.org/spar/datacite/hasIdentifier"/>
                <owl:allValuesFrom rdf:resource="http://w3id.org/meta-share/meta-share/ImageGenreIdentifier"/>
            </owl:Restriction>
        </rdfs:subClassOf>
        <rdfs:subClassOf>
            <owl:Restriction>
                <owl:onProperty rdf:resource="http://w3id.org/meta-share/meta-share/genre"/>
                <owl:allValuesFrom rdf:resource="http://w3id.org/meta-share/meta-share/CorpusImagePart"/>
            </owl:Restriction>
        </rdfs:subClassOf>
        <rdfs:comment xml:lang="en">A category of images characterized by a particular style, form, or content according to a specific classification scheme</rdfs:comment>
        <rdfs:label xml:lang="en">Image genre</rdfs:label>
    </owl:Class>
    


    <!-- http://w3id.org/meta-share/meta-share/ImageGenreClassificationScheme -->

    <owl:Class rdf:about="http://w3id.org/meta-share/meta-share/ImageGenreClassificationScheme">
        <rdfs:subClassOf rdf:resource="http://w3id.org/meta-share/meta-share/ClassificationScheme"/>
        <rdfs:comment xml:lang="en">A classification scheme devised by an authority for image genres</rdfs:comment>
        <rdfs:label xml:lang="en">Image genre classification scheme</rdfs:label>
    </owl:Class>
    


    <!-- http://w3id.org/meta-share/meta-share/ImageGenreIdentifier -->

    <owl:Class rdf:about="http://w3id.org/meta-share/meta-share/ImageGenreIdentifier">
        <rdfs:subClassOf rdf:resource="http://purl.org/spar/datacite/Identifier"/>
        <rdfs:subClassOf>
            <owl:Restriction>
                <owl:onProperty rdf:resource="http://w3id.org/meta-share/meta-share/conformsTo"/>
                <owl:allValuesFrom rdf:resource="http://w3id.org/meta-share/meta-share/ImageGenreClassificationScheme"/>
            </owl:Restriction>
        </rdfs:subClassOf>
        <rdfs:comment xml:lang="en">A string used to uniquely identify an image genre according to a specific classification scheme</rdfs:comment>
        <rdfs:label xml:lang="en">Image genre identifier</rdfs:label>
    </owl:Class>
    


    <!-- http://w3id.org/meta-share/meta-share/Interactivity -->

    <owl:Class rdf:about="http://w3id.org/meta-share/meta-share/Interactivity">
        <rdfs:comment xml:lang="en">The level of conversational interaction between speakers (for audio component) or participants (for video component)</rdfs:comment>
        <rdfs:label xml:lang="en">Interactivity</rdfs:label>
    </owl:Class>
    


    <!-- http://w3id.org/meta-share/meta-share/LCRSubclass -->

    <owl:Class rdf:about="http://w3id.org/meta-share/meta-share/LCRSubclass">
        <rdfs:comment xml:lang="en">A classification of lexical/conceptual resources into types (used for descriptive reasons)</rdfs:comment>
        <rdfs:label xml:lang="en">LCR subclass</rdfs:label>
    </owl:Class>
    


    <!-- http://w3id.org/meta-share/meta-share/LDTask -->

    <owl:Class rdf:about="http://w3id.org/meta-share/meta-share/LDTask">
        <rdfs:comment xml:lang="en">Identifies the task performed by the language description</rdfs:comment>
        <rdfs:label xml:lang="en">Language description task</rdfs:label>
        <skos:note xml:lang="en">add links to omtd-share operations</skos:note>
    </owl:Class>
    


    <!-- http://w3id.org/meta-share/meta-share/LRIdentifier -->

    <owl:Class rdf:about="http://w3id.org/meta-share/meta-share/LRIdentifier">
        <rdfs:subClassOf rdf:resource="http://purl.org/spar/datacite/ResourceIdentifier"/>
        <rdfs:subClassOf>
            <owl:Restriction>
                <owl:onProperty rdf:resource="http://purl.org/spar/datacite/usesIdentifierScheme"/>
                <owl:allValuesFrom rdf:resource="http://w3id.org/meta-share/meta-share/LRIdentifierScheme"/>
            </owl:Restriction>
        </rdfs:subClassOf>
        <rdfs:comment xml:lang="en">A string (e.g.,  PID, DOI, internal to an organization , etc.) used to uniquely identify a language resource</rdfs:comment>
        <rdfs:label xml:lang="en">Language Resource identifier</rdfs:label>
    </owl:Class>
    


    <!-- http://w3id.org/meta-share/meta-share/LRIdentifierScheme -->

    <owl:Class rdf:about="http://w3id.org/meta-share/meta-share/LRIdentifierScheme">
        <rdfs:subClassOf rdf:resource="http://purl.org/spar/datacite/ResourceIdentifierScheme"/>
        <rdfs:altLabel xml:lang="en">Language Resource identifier scheme</rdfs:altLabel>
        <rdfs:comment xml:lang="en">The name of the scheme according to which the LRT identifier is assigned by the authority that issues it (e.g.,  DOI, ISLRN , etc.)</rdfs:comment>
        <rdfs:label xml:lang="en">LR identifier scheme</rdfs:label>
    </owl:Class>
    


    <!-- http://w3id.org/meta-share/meta-share/LanguageDescription -->

    <owl:Class rdf:about="http://w3id.org/meta-share/meta-share/LanguageDescription">
        <rdfs:subClassOf rdf:resource="http://w3id.org/meta-share/meta-share/DataLanguageResource"/>
        <rdfs:subClassOf>
            <owl:Restriction>
                <owl:onProperty rdf:resource="http://w3id.org/meta-share/meta-share/distribution"/>
                <owl:allValuesFrom rdf:resource="http://w3id.org/meta-share/meta-share/DatasetDistribution"/>
            </owl:Restriction>
        </rdfs:subClassOf>
        <rdfs:comment xml:lang="en">A resource that describes a language or some aspect(s) of a language via a systematic documentation of linguistic structures</rdfs:comment>
        <rdfs:label xml:lang="en">Language description</rdfs:label>
    </owl:Class>
    


    <!-- http://w3id.org/meta-share/meta-share/LanguageDescriptionImagePart -->

    <owl:Class rdf:about="http://w3id.org/meta-share/meta-share/LanguageDescriptionImagePart">
        <rdfs:subClassOf rdf:resource="http://w3id.org/meta-share/meta-share/LanguageDescriptionMediaPart"/>
        <rdfs:comment xml:lang="en">The part (or whole set) of a language description that consists of images (e.g.,  a grammar part with photos or images for sign languages)</rdfs:comment>
        <rdfs:label xml:lang="en">Language description image part</rdfs:label>
    </owl:Class>
    


    <!-- http://w3id.org/meta-share/meta-share/LanguageDescriptionMediaPart -->

    <owl:Class rdf:about="http://w3id.org/meta-share/meta-share/LanguageDescriptionMediaPart">
        <rdfs:subClassOf rdf:resource="http://w3id.org/meta-share/meta-share/MediaPart"/>
        <rdfs:comment xml:lang="en">A part/segment of a language description based on its media type classification</rdfs:comment>
        <rdfs:label xml:lang="en">Language description media part</rdfs:label>
    </owl:Class>
    


    <!-- http://w3id.org/meta-share/meta-share/LanguageDescriptionTextPart -->

    <owl:Class rdf:about="http://w3id.org/meta-share/meta-share/LanguageDescriptionTextPart">
        <rdfs:subClassOf rdf:resource="http://w3id.org/meta-share/meta-share/LanguageDescriptionMediaPart"/>
        <rdfs:comment xml:lang="en">The textual part (or whole set) of a language description</rdfs:comment>
        <rdfs:label xml:lang="en">Language description text part</rdfs:label>
    </owl:Class>
    


    <!-- http://w3id.org/meta-share/meta-share/LanguageDescriptionVideoPart -->

    <owl:Class rdf:about="http://w3id.org/meta-share/meta-share/LanguageDescriptionVideoPart">
        <rdfs:subClassOf rdf:resource="http://w3id.org/meta-share/meta-share/LanguageDescriptionMediaPart"/>
        <rdfs:comment xml:lang="en">The part (or whole set) of a language description that consists of videos (e.g.,  a grammar part with videos for sign languages)</rdfs:comment>
        <rdfs:label xml:lang="en">Language description video part</rdfs:label>
    </owl:Class>
    


    <!-- http://w3id.org/meta-share/meta-share/LanguageModel -->

    <owl:Class rdf:about="http://w3id.org/meta-share/meta-share/LanguageModel">
        <rdfs:subClassOf rdf:resource="http://w3id.org/meta-share/meta-share/LanguageDescription"/>
        <rdfs:altLabel xml:lang="en">Statistical language model</rdfs:altLabel>
        <rdfs:comment xml:lang="en">A statistical language model is a probability distribution over sequences of words. Given such a sequence, say of length m, it assigns a probability P (w1, ..., wm) to the whole sequence. [from Wikipedia (https://en.wikipedia.org/wiki/Language_model)]</rdfs:comment>
        <rdfs:label xml:lang="en">Language model</rdfs:label>
    </owl:Class>
    


    <!-- http://w3id.org/meta-share/meta-share/LanguageResource -->

    <owl:Class rdf:about="http://w3id.org/meta-share/meta-share/LanguageResource">
        <rdfs:subClassOf rdf:resource="http://w3id.org/meta-share/meta-share/DescribedEntity"/>
        <rdfs:subClassOf>
            <owl:Restriction>
                <owl:onProperty rdf:resource="http://purl.org/spar/datacite/hasIdentifier"/>
                <owl:allValuesFrom rdf:resource="http://w3id.org/meta-share/meta-share/LRIdentifier"/>
            </owl:Restriction>
        </rdfs:subClassOf>
        <rdfs:altLabel xml:lang="en">LR</rdfs:altLabel>
        <rdfs:comment xml:lang="en">A resource composed of linguistic material used in the construction, improvement and/or evaluation of language processing applications, but also, in a broader sense, in language and language-mediated research studies and applications; the term is used with a broader meaning, encompassing (a) data sets (textual, multimodal/multimedia and lexical data, grammars, language models, etc.) in machine readable form, and (b) tools/technologies/services used for their processing and management.</rdfs:comment>
        <rdfs:label xml:lang="en">Language Resource</rdfs:label>
    </owl:Class>
    


    <!-- http://w3id.org/meta-share/meta-share/LanguageVariety -->

    <owl:Class rdf:about="http://w3id.org/meta-share/meta-share/LanguageVariety">
        <rdfs:comment xml:lang="en">A particular linguistic system used in a specific region or by a social group</rdfs:comment>
        <rdfs:label xml:lang="en">Language variety</rdfs:label>
    </owl:Class>
    


    <!-- http://w3id.org/meta-share/meta-share/LanguageVarietyType -->

    <owl:Class rdf:about="http://w3id.org/meta-share/meta-share/LanguageVarietyType">
        <rdfs:comment xml:lang="en">A classification for language varieties</rdfs:comment>
        <rdfs:label xml:lang="en">Language variety type</rdfs:label>
    </owl:Class>
    


    <!-- http://w3id.org/meta-share/meta-share/LemmaType -->

    <owl:Class rdf:about="http://w3id.org/meta-share/meta-share/LemmaType">
        <rdfs:subClassOf rdf:resource="http://w3id.org/meta-share/meta-share/ContentType"/>
        <rdfs:comment xml:lang="en">A type of content included in a language resource pertaining to the lemma</rdfs:comment>
        <rdfs:label xml:lang="en">Lemma type</rdfs:label>
    </owl:Class>
    


    <!-- http://w3id.org/meta-share/meta-share/LexicalConceptualResource -->

    <owl:Class rdf:about="http://w3id.org/meta-share/meta-share/LexicalConceptualResource">
        <rdfs:subClassOf rdf:resource="http://w3id.org/meta-share/meta-share/DataLanguageResource"/>
        <rdfs:subClassOf>
            <owl:Restriction>
                <owl:onProperty rdf:resource="http://w3id.org/meta-share/meta-share/distribution"/>
                <owl:allValuesFrom rdf:resource="http://w3id.org/meta-share/meta-share/DatasetDistribution"/>
            </owl:Restriction>
        </rdfs:subClassOf>
        <rdfs:subClassOf>
            <owl:Restriction>
                <owl:onProperty rdf:resource="http://w3id.org/meta-share/meta-share/mediaPart"/>
                <owl:allValuesFrom rdf:resource="http://w3id.org/meta-share/meta-share/LexicalConceptualResourceMediaPart"/>
            </owl:Restriction>
        </rdfs:subClassOf>
        <rdfs:comment xml:lang="en">A resource organised on the basis of lexical or conceptual entries (lexical items, terms, concepts , etc.) with their supplementary information (e.g.,  grammatical, semantic, statistical information, etc.)</rdfs:comment>
        <rdfs:label xml:lang="en">Lexical/Conceptual resource</rdfs:label>
    </owl:Class>
    


    <!-- http://w3id.org/meta-share/meta-share/LexicalConceptualResourceAudioPart -->

    <owl:Class rdf:about="http://w3id.org/meta-share/meta-share/LexicalConceptualResourceAudioPart">
        <rdfs:subClassOf rdf:resource="http://w3id.org/meta-share/meta-share/LexicalConceptualResourceMediaPart"/>
        <rdfs:comment xml:lang="en">The part (or whole set of) a lexical/conceptual resource that consists of audio elements (e.g.,  a set of audio files for a lexicon)</rdfs:comment>
        <rdfs:label xml:lang="en">Lexical/Conceptual resource audio part</rdfs:label>
    </owl:Class>
    


    <!-- http://w3id.org/meta-share/meta-share/LexicalConceptualResourceImagePart -->

    <owl:Class rdf:about="http://w3id.org/meta-share/meta-share/LexicalConceptualResourceImagePart">
        <rdfs:subClassOf rdf:resource="http://w3id.org/meta-share/meta-share/LexicalConceptualResourceMediaPart"/>
        <rdfs:comment xml:lang="en">A part (or whole set of) a lexical/conceptual resource that consists of images (e.g.,  a set of images used for a lexicon)</rdfs:comment>
        <rdfs:label xml:lang="en">Lexical/Conceptual resource image part</rdfs:label>
    </owl:Class>
    


    <!-- http://w3id.org/meta-share/meta-share/LexicalConceptualResourceMediaPart -->

    <owl:Class rdf:about="http://w3id.org/meta-share/meta-share/LexicalConceptualResourceMediaPart">
        <rdfs:subClassOf rdf:resource="http://w3id.org/meta-share/meta-share/MediaPart"/>
        <rdfs:comment xml:lang="en">A part/segment of a lexical/conceptual resource based on its media type classification</rdfs:comment>
        <rdfs:label xml:lang="en">Lexical conceptual resource media part</rdfs:label>
    </owl:Class>
    


    <!-- http://w3id.org/meta-share/meta-share/LexicalConceptualResourceTextPart -->

    <owl:Class rdf:about="http://w3id.org/meta-share/meta-share/LexicalConceptualResourceTextPart">
        <rdfs:subClassOf rdf:resource="http://w3id.org/meta-share/meta-share/LexicalConceptualResourceMediaPart"/>
        <rdfs:comment xml:lang="en">A part (or whole set) of a lexical/conceptual resource that consists of textual elements</rdfs:comment>
        <rdfs:label xml:lang="en">Lexical/Conceptual resource text part</rdfs:label>
    </owl:Class>
    


    <!-- http://w3id.org/meta-share/meta-share/LexicalConceptualResourceVideoPart -->

    <owl:Class rdf:about="http://w3id.org/meta-share/meta-share/LexicalConceptualResourceVideoPart">
        <rdfs:subClassOf rdf:resource="http://w3id.org/meta-share/meta-share/LexicalConceptualResourceMediaPart"/>
        <rdfs:comment xml:lang="en">The part (or whole set) of a lexical/conceptual resource that consists of videos (e.g.,  a set of video files for the lexicon of a sign language)</rdfs:comment>
        <rdfs:label xml:lang="en">Lexical/Conceptual resource video part</rdfs:label>
    </owl:Class>
    


    <!-- http://w3id.org/meta-share/meta-share/LicenceCategory -->

    <owl:Class rdf:about="http://w3id.org/meta-share/meta-share/LicenceCategory">
        <rdfs:subClassOf>
            <owl:Restriction>
                <owl:onProperty rdf:resource="http://w3id.org/meta-share/meta-share/conformsTo"/>
                <owl:allValuesFrom rdf:resource="http://w3id.org/meta-share/meta-share/LicenceCategoryScheme"/>
            </owl:Restriction>
        </rdfs:subClassOf>
        <rdfs:comment xml:lang="en">A classification scheme for licences</rdfs:comment>
        <rdfs:label xml:lang="en">Licence category</rdfs:label>
    </owl:Class>
    


    <!-- http://w3id.org/meta-share/meta-share/LicenceCategoryScheme -->

    <owl:Class rdf:about="http://w3id.org/meta-share/meta-share/LicenceCategoryScheme">
        <rdfs:comment xml:lang="en">The name of the scheme according to which a category is assigned to a licence</rdfs:comment>
        <rdfs:label xml:lang="en">Licence category scheme</rdfs:label>
    </owl:Class>
    


    <!-- http://w3id.org/meta-share/meta-share/LicenceIdentifier -->

    <owl:Class rdf:about="http://w3id.org/meta-share/meta-share/LicenceIdentifier">
        <rdfs:subClassOf rdf:resource="http://purl.org/spar/datacite/ResourceIdentifier"/>
        <rdfs:subClassOf>
            <owl:Restriction>
                <owl:onProperty rdf:resource="http://purl.org/spar/datacite/usesIdentifierScheme"/>
                <owl:allValuesFrom rdf:resource="http://w3id.org/meta-share/meta-share/LicenceIdentifierScheme"/>
            </owl:Restriction>
        </rdfs:subClassOf>
        <rdfs:comment xml:lang="en">A string used to uniquely identify a licence</rdfs:comment>
        <rdfs:label xml:lang="en-uk">Licence identifier</rdfs:label>
    </owl:Class>
    


    <!-- http://w3id.org/meta-share/meta-share/LicenceIdentifierScheme -->

    <owl:Class rdf:about="http://w3id.org/meta-share/meta-share/LicenceIdentifierScheme">
        <rdfs:subClassOf rdf:resource="http://purl.org/spar/datacite/ResourceIdentifierScheme"/>
        <rdfs:comment xml:lang="en">The name of the scheme according to which an identifier is assigned to a licence by the authority that issues it</rdfs:comment>
        <rdfs:label xml:lang="en">Licence identifier scheme</rdfs:label>
    </owl:Class>
    


    <!-- http://w3id.org/meta-share/meta-share/LicenceTerms -->

    <owl:Class rdf:about="http://w3id.org/meta-share/meta-share/LicenceTerms">
        <rdfs:subClassOf rdf:resource="http://creativecommons.org/ns#License"/>
        <rdfs:subClassOf rdf:resource="http://w3id.org/meta-share/meta-share/DescribedEntity"/>
        <rdfs:subClassOf>
            <owl:Restriction>
                <owl:onProperty rdf:resource="http://purl.org/spar/datacite/hasIdentifier"/>
                <owl:allValuesFrom rdf:resource="http://w3id.org/meta-share/meta-share/LicenceIdentifier"/>
            </owl:Restriction>
        </rdfs:subClassOf>
        <rdfs:comment xml:lang="en">A legal document (licence or terms of use/service) with which the language resource is distributed</rdfs:comment>
        <rdfs:label xml:lang="en-uk">Licence/Terms of use/service</rdfs:label>
        <skos:note xml:lang="en">Until now, this included an enumerated list of individuals; I think it&apos;s better to treat them as proper entities with name, identifier , etc. 

This means that for the editors we need to 
- add a set of well known licences using the SPDX codes (https://spdx.org/licenses/) and any set already in RDF form (e.g.,  https://github.com/creativecommons/cc.licenserdf/tree/master/cc/licenserdf/licenses and Victor&apos;s list) with our own extra elements
- allow them to add a new licence with the specific elements that we want
- add the clarin licence categories &amp; conditions of use with the ODRL representation


Note: I have created a file with the CC-rdf licences and its ontology so that I can edit them and add the supplementary features =&gt; under MS ontologies, file testrdflicencesCC.txt</skos:note>
    </owl:Class>
    


    <!-- http://w3id.org/meta-share/meta-share/LingualityType -->

    <owl:Class rdf:about="http://w3id.org/meta-share/meta-share/LingualityType">
        <rdfs:comment xml:lang="en">Classification of a resource (part) based on the number of languages it includes</rdfs:comment>
        <rdfs:label xml:lang="en">Linguality type</rdfs:label>
    </owl:Class>
    


    <!-- http://w3id.org/meta-share/meta-share/LinkToOtherMedia -->

    <owl:Class rdf:about="http://w3id.org/meta-share/meta-share/LinkToOtherMedia">
        <rdfs:comment xml:lang="en">The links between different media parts of a multimedia resource</rdfs:comment>
        <rdfs:label xml:lang="en">Link to other media</rdfs:label>
    </owl:Class>
    


    <!-- http://w3id.org/meta-share/meta-share/MLModel -->

    <owl:Class rdf:about="http://w3id.org/meta-share/meta-share/MLModel">
        <rdfs:subClassOf rdf:resource="http://w3id.org/meta-share/meta-share/LanguageDescription"/>
        <rdfs:altLabel xml:lang="en">ML model</rdfs:altLabel>
        <rdfs:comment xml:lang="en">The model artifact that is created through a training process involving an ML algorithm (that is, the learning algorithm) and the training data to learn from.</rdfs:comment>
        <rdfs:label xml:lang="en">Machine Learning model</rdfs:label>
    </owl:Class>
    


    <!-- http://w3id.org/meta-share/meta-share/MediaPart -->

    <owl:Class rdf:about="http://w3id.org/meta-share/meta-share/MediaPart">
        <rdfs:comment xml:lang="en">A part of a language resource based on the media type it belongs to (e.g.,  text, audio, video parts of a corpus or lexicon)</rdfs:comment>
        <rdfs:label xml:lang="en">Media part</rdfs:label>
    </owl:Class>
    


    <!-- http://w3id.org/meta-share/meta-share/MediaType -->

    <owl:Class rdf:about="http://w3id.org/meta-share/meta-share/MediaType">
        <rdfs:comment xml:lang="en">A classification of language resource parts based on the physical medium they are available in (e.g.,  text, video, audio)</rdfs:comment>
        <rdfs:label xml:lang="en">Media type</rdfs:label>
    </owl:Class>
    


    <!-- http://w3id.org/meta-share/meta-share/MembershipInstitution -->

    <owl:Class rdf:about="http://w3id.org/meta-share/meta-share/MembershipInstitution">
        <rdfs:comment xml:lang="en">An institution with members that can benefit from specific conditions on the use of a resource (e.g. discount, unlimited access, etc.)</rdfs:comment>
        <rdfs:label xml:lang="en">Membership institution</rdfs:label>
    </owl:Class>
    


    <!-- http://w3id.org/meta-share/meta-share/MetadataRecord -->

    <owl:Class rdf:about="http://w3id.org/meta-share/meta-share/MetadataRecord">
        <owl:equivalentClass rdf:resource="http://www.w3.org/ns/dcat#CatalogRecord"/>
        <rdfs:subClassOf>
            <owl:Restriction>
                <owl:onProperty rdf:resource="http://w3id.org/meta-share/meta-share/compliesWith"/>
                <owl:allValuesFrom rdf:resource="http://w3id.org/meta-share/meta-share/MetadataSchema"/>
            </owl:Restriction>
        </rdfs:subClassOf>
        <rdfs:comment xml:lang="en">A set of formalized structured information used  to describe the contents, structure, function, etc., of an entity, usually according to a specific set of rules (metadata schema)</rdfs:comment>
        <rdfs:label xml:lang="en">Metadata record</rdfs:label>
    </owl:Class>
    


    <!-- http://w3id.org/meta-share/meta-share/MetadataRecordIdentifier -->

    <owl:Class rdf:about="http://w3id.org/meta-share/meta-share/MetadataRecordIdentifier">
        <rdfs:subClassOf rdf:resource="http://purl.org/spar/datacite/ResourceIdentifier"/>
        <rdfs:subClassOf>
            <owl:Restriction>
                <owl:onProperty rdf:resource="http://purl.org/spar/datacite/usesIdentifierScheme"/>
                <owl:allValuesFrom rdf:resource="http://w3id.org/meta-share/meta-share/MetadataRecordIdentifierScheme"/>
            </owl:Restriction>
        </rdfs:subClassOf>
        <rdfs:comment xml:lang="en">A string (e.g.,  PID, DOI, internal to an organization , etc.) used to uniquely identify a metadata record</rdfs:comment>
        <rdfs:label xml:lang="en">Metadata record identifier</rdfs:label>
    </owl:Class>
    


    <!-- http://w3id.org/meta-share/meta-share/MetadataRecordIdentifierScheme -->

    <owl:Class rdf:about="http://w3id.org/meta-share/meta-share/MetadataRecordIdentifierScheme">
        <rdfs:subClassOf rdf:resource="http://purl.org/spar/datacite/ResourceIdentifierScheme"/>
        <rdfs:comment xml:lang="en">The name of the scheme according to which the metadata record identifier is assigned by the authority that issues it (e.g.,  DOI, URL, etc.)</rdfs:comment>
        <rdfs:label xml:lang="en">Metadata record identifier scheme</rdfs:label>
    </owl:Class>
    


    <!-- http://w3id.org/meta-share/meta-share/MetadataSchema -->

    <owl:Class rdf:about="http://w3id.org/meta-share/meta-share/MetadataSchema">
        <rdfs:comment xml:lang="en">A formal set of metadata elements organized in a specific way</rdfs:comment>
        <rdfs:label xml:lang="en">Metadata schema</rdfs:label>
    </owl:Class>
    


    <!-- http://w3id.org/meta-share/meta-share/Metric -->

    <owl:Class rdf:about="http://w3id.org/meta-share/meta-share/Metric">
        <rdfs:comment xml:lang="en">The metric used for the evaluation of the tool/service</rdfs:comment>
        <rdfs:label xml:lang="en">Metric</rdfs:label>
    </owl:Class>
    


    <!-- http://w3id.org/meta-share/meta-share/ModalityType -->

    <owl:Class rdf:about="http://w3id.org/meta-share/meta-share/ModalityType">
        <rdfs:comment xml:lang="en">A classification of modalities represented in the resource or processed by a tool/service</rdfs:comment>
        <rdfs:label xml:lang="en">Modality type</rdfs:label>
    </owl:Class>
    


    <!-- http://w3id.org/meta-share/meta-share/MorphologicalType -->

    <owl:Class rdf:about="http://w3id.org/meta-share/meta-share/MorphologicalType">
        <rdfs:subClassOf rdf:resource="http://w3id.org/meta-share/meta-share/ContentType"/>
        <rdfs:comment xml:lang="en">A type of content included in a language resource pertaining to the morphological level</rdfs:comment>
        <rdfs:label xml:lang="en">Morphological type</rdfs:label>
    </owl:Class>
    


    <!-- http://w3id.org/meta-share/meta-share/MultilingualityType -->

    <owl:Class rdf:about="http://w3id.org/meta-share/meta-share/MultilingualityType">
        <rdfs:comment xml:lang="en">A classification of a bi/multilingual resource (part) into parallel, comparable or mixed</rdfs:comment>
        <rdfs:label xml:lang="en">Multilinguality type</rdfs:label>
    </owl:Class>
    


    <!-- http://w3id.org/meta-share/meta-share/NGramModel -->

    <owl:Class rdf:about="http://w3id.org/meta-share/meta-share/NGramModel">
        <rdfs:subClassOf rdf:resource="http://w3id.org/meta-share/meta-share/LanguageDescription"/>
        <rdfs:comment xml:lang="en">A language model consisting of n-grams, i.e., specific sequences of a number of words</rdfs:comment>
        <rdfs:label xml:lang="en">N-gram model</rdfs:label>
    </owl:Class>
    


    <!-- http://w3id.org/meta-share/meta-share/Naturality -->

    <owl:Class rdf:about="http://w3id.org/meta-share/meta-share/Naturality">
        <rdfs:comment xml:lang="en">The level of naturality for multimodal/multimedia resources</rdfs:comment>
        <rdfs:label xml:lang="en">Naturality</rdfs:label>
    </owl:Class>
    


    <!-- http://w3id.org/meta-share/meta-share/NeuralNetwork -->

    <owl:Class rdf:about="http://w3id.org/meta-share/meta-share/NeuralNetwork">
        <rdfs:subClassOf rdf:resource="http://w3id.org/meta-share/meta-share/MLModel"/>
        <rdfs:comment xml:lang="en">A set of algorithms, modeled loosely after the human brain, designed to recognize patterns [adapted from https://skymind.ai/wiki/neural-network]</rdfs:comment>
        <rdfs:label xml:lang="en">Neural network</rdfs:label>
    </owl:Class>
    


    <!-- http://w3id.org/meta-share/meta-share/NoiseLevel -->

    <owl:Class rdf:about="http://w3id.org/meta-share/meta-share/NoiseLevel">
        <rdfs:comment xml:lang="en">The  level of background noise</rdfs:comment>
        <rdfs:label xml:lang="en">Noise level</rdfs:label>
    </owl:Class>
    


    <!-- http://w3id.org/meta-share/meta-share/NonSpeechItem -->

    <owl:Class rdf:about="http://w3id.org/meta-share/meta-share/NonSpeechItem">
        <rdfs:comment xml:lang="en">A non-speech element that maybe included in the audio corpus or lexical/conceptual resource</rdfs:comment>
        <rdfs:label xml:lang="en">Non-speech item</rdfs:label>
    </owl:Class>
    


    <!-- http://w3id.org/meta-share/meta-share/OperatingSystem -->

    <owl:Class rdf:about="http://w3id.org/meta-share/meta-share/OperatingSystem">
        <rdfs:comment xml:lang="en">The operating system on which the software is compatible with</rdfs:comment>
        <rdfs:label xml:lang="en">operating system</rdfs:label>
    </owl:Class>
    


    <!-- http://w3id.org/meta-share/meta-share/Organization -->

    <owl:Class rdf:about="http://w3id.org/meta-share/meta-share/Organization">
        <rdfs:subClassOf rdf:resource="http://xmlns.com/foaf/0.1/Organization"/>
        <rdfs:altLabel xml:lang="en-uk">Organisation</rdfs:altLabel>
        <rdfs:comment xml:lang="en-uk">A company or other group of people that works together for a particular purpose [https://dictionary.cambridge.org/dictionary/english/organization]</rdfs:comment>
        <rdfs:label xml:lang="en">Organization</rdfs:label>
    </owl:Class>
    


    <!-- http://w3id.org/meta-share/meta-share/OrganizationLegalStatus -->

    <owl:Class rdf:about="http://w3id.org/meta-share/meta-share/OrganizationLegalStatus">
        <rdfs:comment xml:lang="en">A classification vocabulary for organizations as legal entities</rdfs:comment>
        <rdfs:label xml:lang="en">Organization legal status</rdfs:label>
    </owl:Class>
    


    <!-- http://w3id.org/meta-share/meta-share/OrganizationRole -->

    <owl:Class rdf:about="http://w3id.org/meta-share/meta-share/OrganizationRole">
        <rdfs:comment xml:lang="en">A vocabulary for classifying organizations according to their role in relation to Language Technology</rdfs:comment>
        <rdfs:label xml:lang="en">Organization role</rdfs:label>
    </owl:Class>
    


    <!-- http://w3id.org/meta-share/meta-share/Origin -->

    <owl:Class rdf:about="http://w3id.org/meta-share/meta-share/Origin">
        <rdfs:comment xml:lang="en">The relation of the language of the group of participants with respect to the acquisition stage</rdfs:comment>
        <rdfs:label xml:lang="en">Origin</rdfs:label>
    </owl:Class>
    


    <!-- http://w3id.org/meta-share/meta-share/Parameter -->

    <owl:Class rdf:about="http://w3id.org/meta-share/meta-share/Parameter">
        <rdfs:comment xml:lang="en">A a special kind of variable in computer programming language that is used to pass information between functions or procedures [from https://www.techopedia.com/definition/3725/parameter-param]</rdfs:comment>
        <rdfs:label xml:lang="en">Parameter</rdfs:label>
    </owl:Class>
    


    <!-- http://w3id.org/meta-share/meta-share/ParameterType -->

    <owl:Class rdf:about="http://w3id.org/meta-share/meta-share/ParameterType">
        <rdfs:comment xml:lang="en">A specific (not yet standardised) typing system for parameters (e.g.,  whether it&apos;s boolean, string, integer, a document, mapping, etc.)</rdfs:comment>
        <rdfs:label xml:lang="en">Parameter type</rdfs:label>
    </owl:Class>
    


    <!-- http://w3id.org/meta-share/meta-share/Participant -->

    <owl:Class rdf:about="http://w3id.org/meta-share/meta-share/Participant">
        <rdfs:subClassOf rdf:resource="http://w3id.org/meta-share/meta-share/Person"/>
        <rdfs:comment xml:lang="en">A person that has participated in the recording of the audio, video, sensorimotor (textNumerical) part of the resource</rdfs:comment>
        <rdfs:label xml:lang="en">Participant</rdfs:label>
    </owl:Class>
    


    <!-- http://w3id.org/meta-share/meta-share/PerformanceIndicator -->

    <owl:Class rdf:about="http://w3id.org/meta-share/meta-share/PerformanceIndicator">
        <rdfs:comment xml:lang="en">The performance indicator used in the evaluation of a software given in the form of the metric used and reporting on the measure and unit of measure for this</rdfs:comment>
        <rdfs:label xml:lang="en">Performance indicator</rdfs:label>
    </owl:Class>
    


    <!-- http://w3id.org/meta-share/meta-share/Person -->

    <owl:Class rdf:about="http://w3id.org/meta-share/meta-share/Person">
        <rdfs:subClassOf rdf:resource="http://xmlns.com/foaf/0.1/Person"/>
        <rdfs:subClassOf>
            <owl:Restriction>
                <owl:onProperty rdf:resource="http://purl.org/spar/datacite/hasIdentifier"/>
                <owl:allValuesFrom rdf:resource="http://purl.org/spar/datacite/PersonalIdentifier"/>
            </owl:Restriction>
        </rdfs:subClassOf>
        <rdfs:comment xml:lang="en">A human being</rdfs:comment>
        <rdfs:label xml:lang="en">Person</rdfs:label>
        <skos:comment xml:lang="en">Subclass of foaf to exclude imaginary persons</skos:comment>
    </owl:Class>
    


    <!-- http://w3id.org/meta-share/meta-share/PreviousAnnotationTypesPolicy -->

    <owl:Class rdf:about="http://w3id.org/meta-share/meta-share/PreviousAnnotationTypesPolicy">
        <rdfs:comment xml:lang="en">Policy types that a tool/service has with respect to the annotation types included in the annotated resource that it takes as input (i.e. whether it keeps, modifies or drops them in the output resource)</rdfs:comment>
        <rdfs:label xml:lang="en">Previous annotation types policy</rdfs:label>
    </owl:Class>
    


    <!-- http://w3id.org/meta-share/meta-share/ProcessMode -->

    <owl:Class rdf:about="http://w3id.org/meta-share/meta-share/ProcessMode">
        <rdfs:comment xml:lang="en">Classification of the mode of operation applied when processing a resource</rdfs:comment>
        <rdfs:label xml:lang="en">Process mode</rdfs:label>
    </owl:Class>
    


    <!-- http://w3id.org/meta-share/meta-share/ProcessingResource -->

    <owl:Class rdf:about="http://w3id.org/meta-share/meta-share/ProcessingResource">
        <rdfs:comment xml:lang="en">A set of requirements posed on the resource that is input for processing by a tool/service</rdfs:comment>
        <rdfs:label xml:lang="en">Input content resource</rdfs:label>
    </owl:Class>
    


    <!-- http://w3id.org/meta-share/meta-share/ProcessingResourceType -->

    <owl:Class rdf:about="http://w3id.org/meta-share/meta-share/ProcessingResourceType">
        <rdfs:comment xml:lang="en">The type of the resource that a tool/service takes as input or produces as output</rdfs:comment>
        <rdfs:label xml:lang="en">Processing resource type</rdfs:label>
        <skos:note xml:lang="en">Unsure of the values for audio/video files</skos:note>
    </owl:Class>
    


    <!-- http://w3id.org/meta-share/meta-share/Project -->

    <owl:Class rdf:about="http://w3id.org/meta-share/meta-share/Project">
        <rdfs:subClassOf rdf:resource="http://w3id.org/meta-share/meta-share/DescribedEntity"/>
        <rdfs:subClassOf rdf:resource="http://xmlns.com/foaf/0.1/Project"/>
        <rdfs:subClassOf>
            <owl:Restriction>
                <owl:onProperty rdf:resource="http://purl.org/spar/datacite/hasIdentifier"/>
                <owl:allValuesFrom rdf:resource="http://w3id.org/meta-share/meta-share/ProjectIdentifier"/>
            </owl:Restriction>
        </rdfs:subClassOf>
        <rdfs:comment xml:lang="en">A set of operations undertaken as a whole by an individual or organization and related to some aspect of the lifecycle of the language resource (e.g.,  funding, deployment, etc.)</rdfs:comment>
        <rdfs:label xml:lang="en">Project</rdfs:label>
    </owl:Class>
    


    <!-- http://w3id.org/meta-share/meta-share/ProjectIdentifier -->

    <owl:Class rdf:about="http://w3id.org/meta-share/meta-share/ProjectIdentifier">
        <rdfs:subClassOf rdf:resource="http://purl.org/spar/datacite/ResourceIdentifier"/>
        <rdfs:subClassOf>
            <owl:Restriction>
                <owl:onProperty rdf:resource="http://purl.org/spar/datacite/usesIdentifierScheme"/>
                <owl:allValuesFrom rdf:resource="http://w3id.org/meta-share/meta-share/ProjectIdentifierScheme"/>
            </owl:Restriction>
        </rdfs:subClassOf>
        <rdfs:comment xml:lang="en">A string (e.g.,  PID, internal to an organization, issued by the funding authority , etc.) used to uniquely identify a project</rdfs:comment>
        <rdfs:label xml:lang="en">Project identifier</rdfs:label>
    </owl:Class>
    


    <!-- http://w3id.org/meta-share/meta-share/ProjectIdentifierScheme -->

    <owl:Class rdf:about="http://w3id.org/meta-share/meta-share/ProjectIdentifierScheme">
        <rdfs:subClassOf rdf:resource="http://purl.org/spar/datacite/ResourceIdentifierScheme"/>
        <rdfs:comment xml:lang="en">The name of the scheme according to which an identifier is assigned to a project by the authority that issues it</rdfs:comment>
        <rdfs:label xml:lang="en">Project identifier scheme</rdfs:label>
    </owl:Class>
    


    <!-- http://w3id.org/meta-share/meta-share/Quality -->

    <owl:Class rdf:about="http://w3id.org/meta-share/meta-share/Quality">
        <rdfs:comment xml:lang="en">The quality level of image part(s) of a resource</rdfs:comment>
        <rdfs:label xml:lang="en-uk">Quality</rdfs:label>
    </owl:Class>
    


    <!-- http://w3id.org/meta-share/meta-share/RasterOrVectorGraphics -->

    <owl:Class rdf:about="http://w3id.org/meta-share/meta-share/RasterOrVectorGraphics">
        <rdfs:comment xml:lang="en">Type of graphics of the image part(s) of a resource</rdfs:comment>
        <rdfs:label xml:lang="en">Raster or vector graphics</rdfs:label>
    </owl:Class>
    


    <!-- http://w3id.org/meta-share/meta-share/RecordingDeviceType -->

    <owl:Class rdf:about="http://w3id.org/meta-share/meta-share/RecordingDeviceType">
        <rdfs:comment xml:lang="en">The nature of the recording platform hardware and the storage medium</rdfs:comment>
        <rdfs:label xml:lang="en">Recording device type</rdfs:label>
    </owl:Class>
    


    <!-- http://w3id.org/meta-share/meta-share/RecordingEnvironment -->

    <owl:Class rdf:about="http://w3id.org/meta-share/meta-share/RecordingEnvironment">
        <rdfs:comment xml:lang="en">A setting where the recording of a multimedia resource took place</rdfs:comment>
        <rdfs:label xml:lang="en">Recording environment</rdfs:label>
    </owl:Class>
    


    <!-- http://w3id.org/meta-share/meta-share/RecordingQuality -->

    <owl:Class rdf:about="http://w3id.org/meta-share/meta-share/RecordingQuality">
        <rdfs:comment xml:lang="en">Indication of the audio or video recording quality</rdfs:comment>
        <rdfs:label xml:lang="en-uk">Recording quality</rdfs:label>
    </owl:Class>
    


    <!-- http://w3id.org/meta-share/meta-share/RelatedLexiconType -->

    <owl:Class rdf:about="http://w3id.org/meta-share/meta-share/RelatedLexiconType">
        <rdfs:comment xml:lang="en">Indicates the type for the lexica that must or can be used with the grammar</rdfs:comment>
        <rdfs:label xml:lang="en">Related lexicon type</rdfs:label>
    </owl:Class>
    


    <!-- http://w3id.org/meta-share/meta-share/Relation -->

    <owl:Class rdf:about="http://w3id.org/meta-share/meta-share/Relation">
        <rdfs:comment xml:lang="en">A relation holding between two language resources (e.g.,  a raw corpus and its annotated version, the annotation tool used for it, etc.)</rdfs:comment>
        <rdfs:label xml:lang="en">Relation</rdfs:label>
    </owl:Class>
    


    <!-- http://w3id.org/meta-share/meta-share/RequiredHardware -->

    <owl:Class rdf:about="http://w3id.org/meta-share/meta-share/RequiredHardware">
        <rdfs:comment xml:lang="en">Type of hardware required for running a tool and/or computational grammar</rdfs:comment>
        <rdfs:label xml:lang="en">Required hardware</rdfs:label>
    </owl:Class>
    


    <!-- http://w3id.org/meta-share/meta-share/Resolution -->

    <owl:Class rdf:about="http://w3id.org/meta-share/meta-share/Resolution">
        <rdfs:comment xml:lang="en">The image resolution used for the video/image part(s) of a resource</rdfs:comment>
        <rdfs:label xml:lang="en">Resolution</rdfs:label>
    </owl:Class>
    


    <!-- http://w3id.org/meta-share/meta-share/ResolutionStandard -->

    <owl:Class rdf:about="http://w3id.org/meta-share/meta-share/ResolutionStandard">
        <rdfs:comment xml:lang="en">The standard to which  the resolution conforms</rdfs:comment>
        <rdfs:label xml:lang="en">Resolution standard</rdfs:label>
    </owl:Class>
    


    <!-- http://w3id.org/meta-share/meta-share/ScenarioType -->

    <owl:Class rdf:about="http://w3id.org/meta-share/meta-share/ScenarioType">
        <rdfs:comment xml:lang="en">A classification of the task defined for the conversation or the interaction of participants in a multimedia resource</rdfs:comment>
        <rdfs:label xml:lang="en">Scenario type</rdfs:label>
    </owl:Class>
    


    <!-- http://w3id.org/meta-share/meta-share/SceneIllumination -->

    <owl:Class rdf:about="http://w3id.org/meta-share/meta-share/SceneIllumination">
        <rdfs:comment xml:lang="en">Information on the illumination of the scene</rdfs:comment>
        <rdfs:label xml:lang="en">Scene illumination</rdfs:label>
    </owl:Class>
    


    <!-- http://w3id.org/meta-share/meta-share/SegmentationLevel -->

    <owl:Class rdf:about="http://w3id.org/meta-share/meta-share/SegmentationLevel">
        <rdfs:comment xml:lang="en">The level at which a resource may be segmented (e.g.,  clause, word, unit , etc.)</rdfs:comment>
        <rdfs:label xml:lang="en">Segmentation level</rdfs:label>
    </owl:Class>
    


    <!-- http://w3id.org/meta-share/meta-share/SemanticType -->

    <owl:Class rdf:about="http://w3id.org/meta-share/meta-share/SemanticType">
        <rdfs:subClassOf rdf:resource="http://w3id.org/meta-share/meta-share/ContentType"/>
        <rdfs:comment xml:lang="en">A type of content included in a language resource pertaining to the semantic level</rdfs:comment>
        <rdfs:label xml:lang="en">Semantic type</rdfs:label>
    </owl:Class>
    


    <!-- http://w3id.org/meta-share/meta-share/Sex -->

    <owl:Class rdf:about="http://w3id.org/meta-share/meta-share/Sex">
        <rdfs:comment xml:lang="en">Either of the two major forms of individuals that occur in many species and that are distinguished respectively as female or male especially on the basis of their reproductive organs and structures [https://www.merriam-webster.com/dictionary/sex]</rdfs:comment>
        <rdfs:label xml:lang="en">Sex</rdfs:label>
    </owl:Class>
    


    <!-- http://w3id.org/meta-share/meta-share/SignConvention -->

    <owl:Class rdf:about="http://w3id.org/meta-share/meta-share/SignConvention">
        <rdfs:comment xml:lang="en">Binary representation of numbers</rdfs:comment>
        <rdfs:label xml:lang="en">Sign convention</rdfs:label>
    </owl:Class>
    


    <!-- http://w3id.org/meta-share/meta-share/SignalEncoding -->

    <owl:Class rdf:about="http://w3id.org/meta-share/meta-share/SignalEncoding">
        <rdfs:comment xml:lang="en">The encoding of the audio type of a multimedia resource</rdfs:comment>
        <rdfs:label xml:lang="en">Signal encoding</rdfs:label>
    </owl:Class>
    


    <!-- http://w3id.org/meta-share/meta-share/Size -->

    <owl:Class rdf:about="http://w3id.org/meta-share/meta-share/Size">
        <rdfs:comment xml:lang="en">The size of the resource with regard to the SizeUnit measurement in form of a number</rdfs:comment>
        <rdfs:label xml:lang="en">Size</rdfs:label>
    </owl:Class>
    


    <!-- http://w3id.org/meta-share/meta-share/SizeUnit -->

    <owl:Class rdf:about="http://w3id.org/meta-share/meta-share/SizeUnit">
        <rdfs:comment xml:lang="en">The unit of measurement used for determining and describing the size of a resource (part)</rdfs:comment>
        <rdfs:label xml:lang="en">Size unit</rdfs:label>
    </owl:Class>
    


    <!-- http://w3id.org/meta-share/meta-share/SocialMediaOccupationalAccount -->

    <owl:Class rdf:about="http://w3id.org/meta-share/meta-share/SocialMediaOccupationalAccount">
        <rdfs:comment xml:lang="en">The details for the social media or occupational account of a person or organization</rdfs:comment>
        <rdfs:label xml:lang="en">Social media occupational account</rdfs:label>
    </owl:Class>
    


    <!-- http://w3id.org/meta-share/meta-share/SocialMediaOccupationalAccountType -->

    <owl:Class rdf:about="http://w3id.org/meta-share/meta-share/SocialMediaOccupationalAccountType">
        <rdfs:comment xml:lang="en">A list of social media</rdfs:comment>
        <rdfs:label xml:lang="en">Social media account occupational type</rdfs:label>
    </owl:Class>
    


    <!-- http://w3id.org/meta-share/meta-share/SoftwareDistribution -->

    <owl:Class rdf:about="http://w3id.org/meta-share/meta-share/SoftwareDistribution">
        <rdfs:subClassOf rdf:resource="http://w3id.org/meta-share/meta-share/Distribution"/>
        <rdfs:subClassOf>
            <owl:Restriction>
                <owl:onProperty rdf:resource="http://w3id.org/meta-share/meta-share/distributionForm"/>
                <owl:allValuesFrom rdf:resource="http://w3id.org/meta-share/meta-share/SoftwareDistributionForm"/>
            </owl:Restriction>
        </rdfs:subClassOf>
        <rdfs:comment xml:lang="en">Any form with which software is distributed (e.g.,  web services, executable or code files, etc.)</rdfs:comment>
        <rdfs:label xml:lang="en">Software distribution</rdfs:label>
    </owl:Class>
    


    <!-- http://w3id.org/meta-share/meta-share/SoftwareDistributionForm -->

    <owl:Class rdf:about="http://w3id.org/meta-share/meta-share/SoftwareDistributionForm">
        <rdfs:subClassOf rdf:resource="http://w3id.org/meta-share/meta-share/DistributionForm"/>
        <rdfs:comment xml:lang="en">The medium, delivery channel or form (e.g.,  source code, API, web service , etc.) through which a software object is distributed</rdfs:comment>
        <rdfs:label xml:lang="en">Software distribution form</rdfs:label>
    </owl:Class>
    


    <!-- http://w3id.org/meta-share/meta-share/SourceChannel -->

    <owl:Class rdf:about="http://w3id.org/meta-share/meta-share/SourceChannel">
        <rdfs:comment xml:lang="en">Information on the source channel</rdfs:comment>
        <rdfs:label xml:lang="en">Source channel</rdfs:label>
    </owl:Class>
    


    <!-- http://w3id.org/meta-share/meta-share/SourceChannelType -->

    <owl:Class rdf:about="http://w3id.org/meta-share/meta-share/SourceChannelType">
        <rdfs:comment xml:lang="en">Type of the source channel</rdfs:comment>
        <rdfs:label xml:lang="en">Source channel type</rdfs:label>
    </owl:Class>
    


    <!-- http://w3id.org/meta-share/meta-share/SpeakingImpairmentOfParticipants -->

    <owl:Class rdf:about="http://w3id.org/meta-share/meta-share/SpeakingImpairmentOfParticipants">
        <rdfs:comment xml:lang="en">Whether the group of participants contains persons withwith speakingimpairments</rdfs:comment>
        <rdfs:label xml:lang="en">Speaking impairment of participants</rdfs:label>
    </owl:Class>
    


    <!-- http://w3id.org/meta-share/meta-share/SpeechGenre -->

    <owl:Class rdf:about="http://w3id.org/meta-share/meta-share/SpeechGenre">
        <rdfs:subClassOf rdf:resource="http://w3id.org/meta-share/meta-share/Genre"/>
        <rdfs:subClassOf>
            <owl:Restriction>
                <owl:onProperty rdf:resource="http://purl.org/spar/datacite/hasIdentifier"/>
                <owl:allValuesFrom rdf:resource="http://w3id.org/meta-share/meta-share/SpeechGenreIdentifier"/>
            </owl:Restriction>
        </rdfs:subClassOf>
        <rdfs:subClassOf>
            <owl:Restriction>
                <owl:onProperty rdf:resource="http://w3id.org/meta-share/meta-share/genre"/>
                <owl:allValuesFrom rdf:resource="http://w3id.org/meta-share/meta-share/CorpusAudioPart"/>
            </owl:Restriction>
        </rdfs:subClassOf>
        <rdfs:comment xml:lang="en">A category for the conventionalized discourse of the speech part of a language resource, based on extra-linguistic and internal linguistic criteria</rdfs:comment>
        <rdfs:label xml:lang="en">Speech genre</rdfs:label>
    </owl:Class>
    


    <!-- http://w3id.org/meta-share/meta-share/SpeechGenreClassificationScheme -->

    <owl:Class rdf:about="http://w3id.org/meta-share/meta-share/SpeechGenreClassificationScheme">
        <rdfs:subClassOf rdf:resource="http://w3id.org/meta-share/meta-share/ClassificationScheme"/>
        <rdfs:comment xml:lang="en">A classification scheme used for speech genres devised by an authority or organization</rdfs:comment>
        <rdfs:label xml:lang="en">Speech genre classification scheme</rdfs:label>
    </owl:Class>
    


    <!-- http://w3id.org/meta-share/meta-share/SpeechGenreIdentifier -->

    <owl:Class rdf:about="http://w3id.org/meta-share/meta-share/SpeechGenreIdentifier">
        <rdfs:subClassOf rdf:resource="http://purl.org/spar/datacite/Identifier"/>
        <rdfs:subClassOf>
            <owl:Restriction>
                <owl:onProperty rdf:resource="http://w3id.org/meta-share/meta-share/conformsTo"/>
                <owl:allValuesFrom rdf:resource="http://w3id.org/meta-share/meta-share/SpeechGenreClassificationScheme"/>
            </owl:Restriction>
        </rdfs:subClassOf>
        <rdfs:comment xml:lang="en">A string used to uniquely identify a speech genre according to a specific classification scheme</rdfs:comment>
        <rdfs:label xml:lang="en">Speech genre identifier</rdfs:label>
    </owl:Class>
    


    <!-- http://w3id.org/meta-share/meta-share/SpeechInfluence -->

    <owl:Class rdf:about="http://w3id.org/meta-share/meta-share/SpeechInfluence">
        <rdfs:comment xml:lang="en">A factor influencing speech</rdfs:comment>
        <rdfs:label xml:lang="en">Speech influence</rdfs:label>
    </owl:Class>
    


    <!-- http://w3id.org/meta-share/meta-share/SpeechItem -->

    <owl:Class rdf:about="http://w3id.org/meta-share/meta-share/SpeechItem">
        <rdfs:comment xml:lang="en">An element contained in an audio recording that is pronounced and annotated as such</rdfs:comment>
        <rdfs:label xml:lang="en">Speech item</rdfs:label>
    </owl:Class>
    


    <!-- http://w3id.org/meta-share/meta-share/StandardBestPractice -->

    <owl:Class rdf:about="http://w3id.org/meta-share/meta-share/StandardBestPractice">
        <rdfs:comment xml:lang="en">A standard or best practice widely used to which the lexical/conceptual resource or corpus conforms to</rdfs:comment>
        <rdfs:label xml:lang="en">Standard/Best practice</rdfs:label>
        <skos:note xml:lang="en">some of these are only formats rather than standards; how can we distinguish?</skos:note>
    </owl:Class>
    


    <!-- http://w3id.org/meta-share/meta-share/StaticElement -->

    <owl:Class rdf:about="http://w3id.org/meta-share/meta-share/StaticElement">
        <rdfs:comment xml:lang="en">The static elements visible on images</rdfs:comment>
        <rdfs:label xml:lang="en">Static element</rdfs:label>
    </owl:Class>
    


    <!-- http://w3id.org/meta-share/meta-share/Subject -->

    <owl:Class rdf:about="http://w3id.org/meta-share/meta-share/Subject">
        <rdfs:subClassOf rdf:resource="http://w3id.org/meta-share/meta-share/Classification"/>
        <rdfs:altLabel xml:lang="en">Topic</rdfs:altLabel>
        <rdfs:comment xml:lang="en">A situation, event, thing, etc. that is discussed in the contents of a language resource</rdfs:comment>
        <rdfs:label xml:lang="en">Subject</rdfs:label>
    </owl:Class>
    


    <!-- http://w3id.org/meta-share/meta-share/SubjectClassificationScheme -->

    <owl:Class rdf:about="http://w3id.org/meta-share/meta-share/SubjectClassificationScheme">
        <rdfs:subClassOf rdf:resource="http://w3id.org/meta-share/meta-share/ClassificationScheme"/>
        <rdfs:comment xml:lang="en">A classification scheme used for subjects/topics devised by an authority or organization</rdfs:comment>
        <rdfs:label xml:lang="en">Subject classification scheme</rdfs:label>
    </owl:Class>
    


    <!-- http://w3id.org/meta-share/meta-share/SubjectIdentifier -->

    <owl:Class rdf:about="http://w3id.org/meta-share/meta-share/SubjectIdentifier">
        <rdfs:subClassOf rdf:resource="http://purl.org/spar/datacite/Identifier"/>
        <rdfs:subClassOf>
            <owl:Restriction>
                <owl:onProperty rdf:resource="http://w3id.org/meta-share/meta-share/conformsTo"/>
                <owl:allValuesFrom rdf:resource="http://w3id.org/meta-share/meta-share/SubjectClassificationScheme"/>
            </owl:Restriction>
        </rdfs:subClassOf>
        <rdfs:comment xml:lang="en">A string used to uniquely identify a subject according to a specific classification scheme</rdfs:comment>
        <rdfs:label xml:lang="en">Subject identifier</rdfs:label>
    </owl:Class>
    


    <!-- http://w3id.org/meta-share/meta-share/Subset -->

    <owl:Class rdf:about="http://w3id.org/meta-share/meta-share/Subset">
        <rdfs:comment xml:lang="en">A subset of a language resource in terms of a specific parameter (e.g.,  per domain, time coverage, linguistic level of representation , etc.)</rdfs:comment>
        <rdfs:label xml:lang="en">Subset</rdfs:label>
    </owl:Class>
    


    <!-- http://w3id.org/meta-share/meta-share/SyntacticType -->

    <owl:Class rdf:about="http://w3id.org/meta-share/meta-share/SyntacticType">
        <rdfs:subClassOf rdf:resource="http://w3id.org/meta-share/meta-share/ContentType"/>
        <rdfs:comment xml:lang="en">A type of content included in a language resource pertaining to the syntactic level</rdfs:comment>
        <rdfs:label xml:lang="en">Syntactic type</rdfs:label>
    </owl:Class>
    


    <!-- http://w3id.org/meta-share/meta-share/SyntacticoSemanticType -->

    <owl:Class rdf:about="http://w3id.org/meta-share/meta-share/SyntacticoSemanticType">
        <rdfs:subClassOf rdf:resource="http://w3id.org/meta-share/meta-share/ContentType"/>
        <rdfs:comment xml:lang="en">A type of content included in a language resource pertaining to the syntactico-semantic level</rdfs:comment>
        <rdfs:label xml:lang="en">Syntactico-semantic type</rdfs:label>
    </owl:Class>
    


    <!-- http://w3id.org/meta-share/meta-share/TRL -->

    <owl:Class rdf:about="http://w3id.org/meta-share/meta-share/TRL">
        <rdfs:altLabel xml:lang="en">Technology Readiness Level</rdfs:altLabel>
        <rdfs:comment xml:lang="en">An indicator of the maturity level of particular technologies according to a measurement system defined by EC [adapted from https://ec.europa.eu/info/funding-tenders/opportunities/portal/screen/support/faq/2890]</rdfs:comment>
        <rdfs:label xml:lang="en">TRL</rdfs:label>
    </owl:Class>
    


    <!-- http://w3id.org/meta-share/meta-share/TextGenre -->

    <owl:Class rdf:about="http://w3id.org/meta-share/meta-share/TextGenre">
        <rdfs:subClassOf rdf:resource="http://w3id.org/meta-share/meta-share/Genre"/>
        <rdfs:subClassOf>
            <owl:Restriction>
                <owl:onProperty rdf:resource="http://purl.org/spar/datacite/hasIdentifier"/>
                <owl:allValuesFrom rdf:resource="http://w3id.org/meta-share/meta-share/TextGenreIdentifier"/>
            </owl:Restriction>
        </rdfs:subClassOf>
        <rdfs:subClassOf>
            <owl:Restriction>
                <owl:onProperty rdf:resource="http://w3id.org/meta-share/meta-share/genre"/>
                <owl:allValuesFrom rdf:resource="http://w3id.org/meta-share/meta-share/CorpusTextPart"/>
            </owl:Restriction>
        </rdfs:subClassOf>
        <rdfs:comment xml:lang="en">A category of text characterized by a particular style, form, or content according to a specific classification scheme</rdfs:comment>
        <rdfs:label xml:lang="en">Text genre</rdfs:label>
    </owl:Class>
    


    <!-- http://w3id.org/meta-share/meta-share/TextGenreClassificationScheme -->

    <owl:Class rdf:about="http://w3id.org/meta-share/meta-share/TextGenreClassificationScheme">
        <rdfs:subClassOf rdf:resource="http://w3id.org/meta-share/meta-share/ClassificationScheme"/>
        <rdfs:comment xml:lang="en">A classification scheme used for text genres devised by an authority or organization</rdfs:comment>
        <rdfs:label xml:lang="en">Text genre classification scheme</rdfs:label>
    </owl:Class>
    


    <!-- http://w3id.org/meta-share/meta-share/TextGenreIdentifier -->

    <owl:Class rdf:about="http://w3id.org/meta-share/meta-share/TextGenreIdentifier">
        <rdfs:subClassOf rdf:resource="http://purl.org/spar/datacite/Identifier"/>
        <rdfs:subClassOf>
            <owl:Restriction>
                <owl:onProperty rdf:resource="http://w3id.org/meta-share/meta-share/conformsTo"/>
                <owl:allValuesFrom rdf:resource="http://w3id.org/meta-share/meta-share/TextGenreClassificationScheme"/>
            </owl:Restriction>
        </rdfs:subClassOf>
        <rdfs:comment xml:lang="en">A string used to uniquely identify a text genre according to a specific classification scheme</rdfs:comment>
        <rdfs:label xml:lang="en">Text genre identifier</rdfs:label>
    </owl:Class>
    


    <!-- http://w3id.org/meta-share/meta-share/TextIncludedInImage -->

    <owl:Class rdf:about="http://w3id.org/meta-share/meta-share/TextIncludedInImage">
        <rdfs:comment xml:lang="en">Provides information on the type of text that may be on the image</rdfs:comment>
        <rdfs:label xml:lang="en">Text included in image</rdfs:label>
    </owl:Class>
    


    <!-- http://w3id.org/meta-share/meta-share/TextIncludedInVideo -->

    <owl:Class rdf:about="http://w3id.org/meta-share/meta-share/TextIncludedInVideo">
        <rdfs:comment xml:lang="en">The presence or not of text in or in conjunction with the video and, if yes, the type</rdfs:comment>
        <rdfs:label xml:lang="en">Text included in video</rdfs:label>
    </owl:Class>
    


    <!-- http://w3id.org/meta-share/meta-share/TextNumericalFormat -->

    <owl:Class rdf:about="http://w3id.org/meta-share/meta-share/TextNumericalFormat">
        <rdfs:comment xml:lang="en">The format(s) of the textNumerical part of the resource</rdfs:comment>
        <rdfs:label xml:lang="en">TextNumerical format</rdfs:label>
    </owl:Class>
    


    <!-- http://w3id.org/meta-share/meta-share/TextType -->

    <owl:Class rdf:about="http://w3id.org/meta-share/meta-share/TextType">
        <rdfs:subClassOf rdf:resource="http://w3id.org/meta-share/meta-share/Classification"/>
        <rdfs:subClassOf>
            <owl:Restriction>
                <owl:onProperty rdf:resource="http://purl.org/spar/datacite/hasIdentifier"/>
                <owl:allValuesFrom rdf:resource="http://w3id.org/meta-share/meta-share/TextTypeIdentifier"/>
            </owl:Restriction>
        </rdfs:subClassOf>
        <rdfs:comment xml:lang="en">An abstract category designed to characterize the main structure of a particular text or one of its parts according to its dominant properties [from https://www.lhn.uni-hamburg.de/node/121.html]</rdfs:comment>
        <rdfs:label xml:lang="en">Text type</rdfs:label>
    </owl:Class>
    


    <!-- http://w3id.org/meta-share/meta-share/TextTypeClassificationScheme -->

    <owl:Class rdf:about="http://w3id.org/meta-share/meta-share/TextTypeClassificationScheme">
        <rdfs:subClassOf rdf:resource="http://w3id.org/meta-share/meta-share/ClassificationScheme"/>
        <rdfs:comment xml:lang="en">A classification scheme used for text types devised by an authority or organization</rdfs:comment>
        <rdfs:label xml:lang="en">Text type classification scheme</rdfs:label>
    </owl:Class>
    


    <!-- http://w3id.org/meta-share/meta-share/TextTypeIdentifier -->

    <owl:Class rdf:about="http://w3id.org/meta-share/meta-share/TextTypeIdentifier">
        <rdfs:subClassOf rdf:resource="http://purl.org/spar/datacite/Identifier"/>
        <rdfs:subClassOf>
            <owl:Restriction>
                <owl:onProperty rdf:resource="http://w3id.org/meta-share/meta-share/conformsTo"/>
                <owl:allValuesFrom rdf:resource="http://w3id.org/meta-share/meta-share/TextTypeClassificationScheme"/>
            </owl:Restriction>
        </rdfs:subClassOf>
        <rdfs:comment xml:lang="en">A string used to uniquely identify a text type according to a specific classification scheme</rdfs:comment>
        <rdfs:label xml:lang="en">Text type identifier</rdfs:label>
    </owl:Class>
    


    <!-- http://w3id.org/meta-share/meta-share/ToolService -->

    <owl:Class rdf:about="http://w3id.org/meta-share/meta-share/ToolService">
        <rdfs:subClassOf rdf:resource="http://w3id.org/meta-share/meta-share/LanguageResource"/>
        <rdfs:altLabel xml:lang="en">LT tool/service</rdfs:altLabel>
        <rdfs:comment xml:lang="en">A tool/service/any piece of software that performs language processing and/or any Language Technology related operation.</rdfs:comment>
        <rdfs:label xml:lang="en">Language Technology tool/service</rdfs:label>
    </owl:Class>
    


    <!-- http://w3id.org/meta-share/meta-share/TranslationType -->

    <owl:Class rdf:about="http://w3id.org/meta-share/meta-share/TranslationType">
        <rdfs:subClassOf rdf:resource="http://w3id.org/meta-share/meta-share/ContentType"/>
        <rdfs:comment xml:lang="en">A type of content included in a language resource relevant to the translation procedure</rdfs:comment>
        <rdfs:label xml:lang="en">Translation type</rdfs:label>
    </owl:Class>
    


    <!-- http://w3id.org/meta-share/meta-share/UsageType -->

    <owl:Class rdf:about="http://w3id.org/meta-share/meta-share/UsageType">
        <rdfs:subClassOf rdf:resource="http://w3id.org/meta-share/meta-share/ContentType"/>
        <rdfs:comment xml:lang="en">A type of content included in a language resource encoding usage information</rdfs:comment>
        <rdfs:label xml:lang="en">Usage type</rdfs:label>
    </owl:Class>
    


    <!-- http://w3id.org/meta-share/meta-share/UserType -->

    <owl:Class rdf:about="http://w3id.org/meta-share/meta-share/UserType">
        <rdfs:comment xml:lang="en">Classification type for users of a language resource; usually required for assessing the licensing or pricing policies for the use of the resource</rdfs:comment>
        <rdfs:label xml:lang="en">User type</rdfs:label>
    </owl:Class>
    


    <!-- http://w3id.org/meta-share/meta-share/Validation -->

    <owl:Class rdf:about="http://w3id.org/meta-share/meta-share/Validation">
        <rdfs:comment xml:lang="en">Each of the procedures and outcomes followed for validating a language resource, i.e. confirming that its contents/structure/operation is as claimed after careful examination</rdfs:comment>
        <rdfs:label xml:lang="en">Validation</rdfs:label>
    </owl:Class>
    


    <!-- http://w3id.org/meta-share/meta-share/ValidationExtent -->

    <owl:Class rdf:about="http://w3id.org/meta-share/meta-share/ValidationExtent">
        <rdfs:comment xml:lang="en">The resource coverage in terms of validated data</rdfs:comment>
        <rdfs:label xml:lang="en">Validation extent</rdfs:label>
    </owl:Class>
    


    <!-- http://w3id.org/meta-share/meta-share/ValidationType -->

    <owl:Class rdf:about="http://w3id.org/meta-share/meta-share/ValidationType">
        <rdfs:comment xml:lang="en">Classification of validation that indicates whether the validation was made on the contents or on formal aspects of the resource</rdfs:comment>
        <rdfs:label xml:lang="en">Validation type</rdfs:label>
    </owl:Class>
    


    <!-- http://w3id.org/meta-share/meta-share/VersionType -->

    <owl:Class rdf:about="http://w3id.org/meta-share/meta-share/VersionType">
        <rdfs:comment xml:lang="en">A type of versioning vocabulary used mainly for works (e.g.,  scholarly articles, books , etc.) that go through a formal review process before final publication, marked with major changes across the versions</rdfs:comment>
        <rdfs:label xml:lang="en">Version type</rdfs:label>
        <skos:note xml:lang="en">When the COAR vocabulary is published (cf. https://www.coar-repositories.org/activities/repository-interoperability/coar-vocabularies/version-type-vocabulary/) check again</skos:note>
    </owl:Class>
    


    <!-- http://w3id.org/meta-share/meta-share/VideoFormat -->

    <owl:Class rdf:about="http://w3id.org/meta-share/meta-share/VideoFormat">
        <rdfs:comment xml:lang="en">The format(s) of a video (part of a) resource</rdfs:comment>
        <rdfs:label xml:lang="en">Video format</rdfs:label>
    </owl:Class>
    


    <!-- http://w3id.org/meta-share/meta-share/VideoGenre -->

    <owl:Class rdf:about="http://w3id.org/meta-share/meta-share/VideoGenre">
        <rdfs:subClassOf rdf:resource="http://w3id.org/meta-share/meta-share/Genre"/>
        <rdfs:subClassOf>
            <owl:Restriction>
                <owl:onProperty rdf:resource="http://purl.org/spar/datacite/hasIdentifier"/>
                <owl:allValuesFrom rdf:resource="http://w3id.org/meta-share/meta-share/VideoGenreIdentifier"/>
            </owl:Restriction>
        </rdfs:subClassOf>
        <rdfs:subClassOf>
            <owl:Restriction>
                <owl:onProperty rdf:resource="http://w3id.org/meta-share/meta-share/genre"/>
                <owl:allValuesFrom rdf:resource="http://w3id.org/meta-share/meta-share/CorpusVideoPart"/>
            </owl:Restriction>
        </rdfs:subClassOf>
        <rdfs:comment xml:lang="en">A classification of video parts based on extra-linguistic and internal linguistic criteria and reflected on the video style, form or content</rdfs:comment>
        <rdfs:label xml:lang="en">Video genre</rdfs:label>
    </owl:Class>
    


    <!-- http://w3id.org/meta-share/meta-share/VideoGenreClassificationScheme -->

    <owl:Class rdf:about="http://w3id.org/meta-share/meta-share/VideoGenreClassificationScheme">
        <rdfs:subClassOf rdf:resource="http://w3id.org/meta-share/meta-share/ClassificationScheme"/>
        <rdfs:comment xml:lang="en">A classification scheme devised by an authority for video genres</rdfs:comment>
        <rdfs:label xml:lang="en">Video genre classification scheme</rdfs:label>
    </owl:Class>
    


    <!-- http://w3id.org/meta-share/meta-share/VideoGenreIdentifier -->

    <owl:Class rdf:about="http://w3id.org/meta-share/meta-share/VideoGenreIdentifier">
        <rdfs:subClassOf rdf:resource="http://purl.org/spar/datacite/Identifier"/>
        <rdfs:subClassOf>
            <owl:Restriction>
                <owl:onProperty rdf:resource="http://w3id.org/meta-share/meta-share/conformsTo"/>
                <owl:allValuesFrom rdf:resource="http://w3id.org/meta-share/meta-share/VideoGenreClassificationScheme"/>
            </owl:Restriction>
        </rdfs:subClassOf>
        <rdfs:comment xml:lang="en">A string used to uniquely identify a video genre according to a specific classification scheme</rdfs:comment>
        <rdfs:label xml:lang="en">Video genre identifier</rdfs:label>
    </owl:Class>
    


    <!-- http://w3id.org/meta-share/meta-share/VisualModelling -->

    <owl:Class rdf:about="http://w3id.org/meta-share/meta-share/VisualModelling">
        <rdfs:comment xml:lang="en">The dimensional form applied on the video or image part(s) of a corpus</rdfs:comment>
        <rdfs:label xml:lang="en">Visual modelling</rdfs:label>
    </owl:Class>
    


    <!-- http://w3id.org/meta-share/meta-share/VocalTractCondition -->

    <owl:Class rdf:about="http://w3id.org/meta-share/meta-share/VocalTractCondition">
        <rdfs:comment xml:lang="en">The vocal tract condition that may influence the speech of the participant</rdfs:comment>
        <rdfs:label xml:lang="en">Vocal tract condition</rdfs:label>
    </owl:Class>
    


    <!-- http://w3id.org/meta-share/meta-share/WebServiceType -->

    <owl:Class rdf:about="http://w3id.org/meta-share/meta-share/WebServiceType">
        <rdfs:comment xml:lang="en">A classification of web services based on the protocol used for accessing them</rdfs:comment>
        <rdfs:label xml:lang="en">Web service type</rdfs:label>
    </owl:Class>
    


    <!-- http://w3id.org/meta-share/meta-share/WordEmbedding -->

    <owl:Class rdf:about="http://w3id.org/meta-share/meta-share/WordEmbedding">
        <rdfs:subClassOf rdf:resource="http://w3id.org/meta-share/meta-share/MLModel"/>
        <rdfs:comment xml:lang="en">Word embedding is the collective name for a set of language modeling and feature learning techniques in natural language processing where words or phrases from the vocabulary are mapped to vectors of real numbers. [wikipedia]</rdfs:comment>
        <rdfs:label xml:lang="en">Word embedding</rdfs:label>
    </owl:Class>
    


    <!-- http://w3id.org/meta-share/omtd-share/AnnotationType -->

    <owl:Class rdf:about="http://w3id.org/meta-share/omtd-share/AnnotationType"/>
    


    <!-- http://w3id.org/meta-share/omtd-share/DataFormat -->

    <owl:Class rdf:about="http://w3id.org/meta-share/omtd-share/DataFormat"/>
    


    <!-- http://w3id.org/meta-share/omtd-share/Operation -->

    <owl:Class rdf:about="http://w3id.org/meta-share/omtd-share/Operation"/>
    


    <!-- http://w3id.org/meta-share/omtd-share/TdmMethod -->

    <owl:Class rdf:about="http://w3id.org/meta-share/omtd-share/TdmMethod"/>
    


    <!-- http://www.w3.org/2004/02/skos/core#concept -->

    <owl:Class rdf:about="http://www.w3.org/2004/02/skos/core#concept"/>
    


    <!-- http://www.w3.org/ns/dcat#Catalog -->

    <owl:Class rdf:about="http://www.w3.org/ns/dcat#Catalog"/>
    


    <!-- http://www.w3.org/ns/dcat#CatalogRecord -->

    <owl:Class rdf:about="http://www.w3.org/ns/dcat#CatalogRecord"/>
    


    <!-- http://www.w3.org/ns/dcat#Dataset -->

    <owl:Class rdf:about="http://www.w3.org/ns/dcat#Dataset"/>
    


    <!-- http://www.w3.org/ns/odrl/2/Set -->

    <owl:Class rdf:about="http://www.w3.org/ns/odrl/2/Set"/>
    


    <!-- http://xmlns.com/foaf/0.1/Agent -->

    <owl:Class rdf:about="http://xmlns.com/foaf/0.1/Agent"/>
    


    <!-- http://xmlns.com/foaf/0.1/Organization -->

    <owl:Class rdf:about="http://xmlns.com/foaf/0.1/Organization">
        <rdfs:subClassOf>
            <owl:Restriction>
                <owl:onProperty rdf:resource="http://purl.org/spar/datacite/hasIdentifier"/>
                <owl:allValuesFrom rdf:resource="http://purl.org/spar/datacite/OrganizationIdentifier"/>
            </owl:Restriction>
        </rdfs:subClassOf>
    </owl:Class>
    


    <!-- http://xmlns.com/foaf/0.1/Person -->

    <owl:Class rdf:about="http://xmlns.com/foaf/0.1/Person"/>
    


    <!-- http://xmlns.com/foaf/0.1/Project -->

    <owl:Class rdf:about="http://xmlns.com/foaf/0.1/Project"/>
    


    <!-- 
    ///////////////////////////////////////////////////////////////////////////////////////
    //
    // Individuals
    //
    ///////////////////////////////////////////////////////////////////////////////////////
     -->

    


    <!-- http://purl.org/NET/rdflicense/cc-by4.0 -->

    <owl:NamedIndividual rdf:about="http://purl.org/NET/rdflicense/cc-by4.0"/>
    


    <!-- http://purl.org/coar/access_right/c_14cb -->

    <owl:NamedIndividual rdf:about="http://purl.org/coar/access_right/c_14cb">
        <rdf:type rdf:resource="http://w3id.org/meta-share/meta-share/AccessRightsStatementIdentifier"/>
        <ms:conformsTo rdf:resource="http://w3id.org/meta-share/meta-share/COARightsStatementScheme"/>
    </owl:NamedIndividual>
    


    <!-- http://purl.org/coar/access_right/c_16ec -->

    <owl:NamedIndividual rdf:about="http://purl.org/coar/access_right/c_16ec">
        <rdf:type rdf:resource="http://w3id.org/meta-share/meta-share/AccessRightsStatementIdentifier"/>
        <ms:conformsTo rdf:resource="http://w3id.org/meta-share/meta-share/COARightsStatementScheme"/>
    </owl:NamedIndividual>
    


    <!-- http://purl.org/coar/access_right/c_abf2 -->

    <owl:NamedIndividual rdf:about="http://purl.org/coar/access_right/c_abf2">
        <rdf:type rdf:resource="http://w3id.org/meta-share/meta-share/AccessRightsStatementIdentifier"/>
        <ms:conformsTo rdf:resource="http://w3id.org/meta-share/meta-share/COARightsStatementScheme"/>
    </owl:NamedIndividual>
    


    <!-- http://purl.org/coar/access_right/c_f1cf -->

    <owl:NamedIndividual rdf:about="http://purl.org/coar/access_right/c_f1cf">
        <rdf:type rdf:resource="http://w3id.org/meta-share/meta-share/AccessRightsStatementIdentifier"/>
        <ms:conformsTo rdf:resource="http://w3id.org/meta-share/meta-share/COARightsStatementScheme"/>
    </owl:NamedIndividual>
    


    <!-- http://purl.org/spar/datacite/ark -->

    <owl:NamedIndividual rdf:about="http://purl.org/spar/datacite/ark">
        <rdf:type rdf:resource="http://w3id.org/meta-share/meta-share/DocumentIdentifierScheme"/>
        <rdf:type rdf:resource="http://w3id.org/meta-share/meta-share/LRIdentifierScheme"/>
        <rdfs:comment xml:lang="en">Archival Resource Key</rdfs:comment>
        <rdfs:label xml:lang="en">ARK</rdfs:label>
    </owl:NamedIndividual>
    


    <!-- http://purl.org/spar/datacite/arxiv -->

    <owl:NamedIndividual rdf:about="http://purl.org/spar/datacite/arxiv">
        <rdf:type rdf:resource="http://w3id.org/meta-share/meta-share/DocumentIdentifierScheme"/>
        <rdf:type rdf:resource="http://w3id.org/meta-share/meta-share/LRIdentifierScheme"/>
        <rdfs:comment xml:lang="en">Identifier for ArXiv (http://arxiv.org/), a open access repository of preprints, having the format arXiv:1207.2147.</rdfs:comment>
        <rdfs:label xml:lang="en">ArXiv</rdfs:label>
    </owl:NamedIndividual>
    


    <!-- http://purl.org/spar/datacite/bibcode -->

    <owl:NamedIndividual rdf:about="http://purl.org/spar/datacite/bibcode">
        <rdf:type rdf:resource="http://w3id.org/meta-share/meta-share/DocumentIdentifierScheme"/>
        <rdf:type rdf:resource="http://w3id.org/meta-share/meta-share/LRIdentifierScheme"/>
        <rdfs:comment xml:lang="en">It is the Astrophysics Data System bibliographic codes, a standardized 19 character identifier according to the syntax &quot;yyyyjjjjjvvvvmppppa&quot;.</rdfs:comment>
        <rdfs:label xml:lang="en">bibcode</rdfs:label>
    </owl:NamedIndividual>
    


    <!-- http://purl.org/spar/datacite/doi -->

    <owl:NamedIndividual rdf:about="http://purl.org/spar/datacite/doi">
        <rdf:type rdf:resource="http://purl.org/spar/datacite/OrganizationIdentifierScheme"/>
        <rdf:type rdf:resource="http://w3id.org/meta-share/meta-share/DocumentIdentifierScheme"/>
        <rdf:type rdf:resource="http://w3id.org/meta-share/meta-share/LRIdentifierScheme"/>
        <rdfs:comment xml:lang="en">Digital Object Identifier</rdfs:comment>
        <rdfs:label xml:lang="en">DOI</rdfs:label>
    </owl:NamedIndividual>
    


    <!-- http://purl.org/spar/datacite/handle -->

    <owl:NamedIndividual rdf:about="http://purl.org/spar/datacite/handle">
        <rdf:type rdf:resource="http://w3id.org/meta-share/meta-share/DocumentIdentifierScheme"/>
        <rdf:type rdf:resource="http://w3id.org/meta-share/meta-share/LRIdentifierScheme"/>
        <rdf:type rdf:resource="http://w3id.org/meta-share/meta-share/MetadataRecordIdentifierScheme"/>
        <rdfs:comment xml:lang="en">The Handle system</rdfs:comment>
        <rdfs:label xml:lang="en">Handle</rdfs:label>
    </owl:NamedIndividual>
    


    <!-- http://purl.org/spar/datacite/isbn -->

    <owl:NamedIndividual rdf:about="http://purl.org/spar/datacite/isbn">
        <rdf:type rdf:resource="http://w3id.org/meta-share/meta-share/DocumentIdentifierScheme"/>
        <rdf:type rdf:resource="http://w3id.org/meta-share/meta-share/LRIdentifierScheme"/>
        <rdfs:comment xml:lang="en">International Standard Book Number</rdfs:comment>
        <rdfs:label xml:lang="en">ISBN</rdfs:label>
    </owl:NamedIndividual>
    


    <!-- http://purl.org/spar/datacite/openid -->

    <owl:NamedIndividual rdf:about="http://purl.org/spar/datacite/openid">
        <rdf:type rdf:resource="http://purl.org/spar/datacite/PersonalIdentifierScheme"/>
        <rdfs:comment xml:lang="en">OpenID is an open standard that describes how users can be authenticated in a decentralized manner, eliminating the need for centralized registration services.</rdfs:comment>
        <rdfs:label xml:lang="en">OpenID</rdfs:label>
    </owl:NamedIndividual>
    


    <!-- http://purl.org/spar/datacite/orcid -->

    <owl:NamedIndividual rdf:about="http://purl.org/spar/datacite/orcid">
        <rdf:type rdf:resource="http://purl.org/spar/datacite/PersonalIdentifierScheme"/>
        <rdfs:comment xml:lang="en">Open Researcher and Contributor Identifier.</rdfs:comment>
        <rdfs:label xml:lang="en">ORCID</rdfs:label>
    </owl:NamedIndividual>
    


    <!-- http://purl.org/spar/datacite/purl -->

    <owl:NamedIndividual rdf:about="http://purl.org/spar/datacite/purl">
        <rdf:type rdf:resource="http://w3id.org/meta-share/meta-share/DocumentIdentifierScheme"/>
        <rdf:type rdf:resource="http://w3id.org/meta-share/meta-share/LRIdentifierScheme"/>
        <rdf:type rdf:resource="http://w3id.org/meta-share/meta-share/MetadataRecordIdentifierScheme"/>
        <rdfs:comment xml:lang="en">Persistent Uniform Resource Locator</rdfs:comment>
        <rdfs:label xml:lang="en">PURL</rdfs:label>
    </owl:NamedIndividual>
    


    <!-- http://purl.org/spar/datacite/researcherid -->

    <owl:NamedIndividual rdf:about="http://purl.org/spar/datacite/researcherid">
        <rdf:type rdf:resource="http://purl.org/spar/datacite/PersonalIdentifierScheme"/>
        <rdfs:comment xml:lang="en">ResearcherID is an identifying system for scientific authors created and owned by Thomson Reuters.</rdfs:comment>
        <rdfs:label xml:lang="en">ResearcherID</rdfs:label>
    </owl:NamedIndividual>
    


    <!-- http://purl.org/spar/datacite/upc -->

    <owl:NamedIndividual rdf:about="http://purl.org/spar/datacite/upc">
        <rdf:type rdf:resource="http://w3id.org/meta-share/meta-share/DocumentIdentifierScheme"/>
        <rdf:type rdf:resource="http://w3id.org/meta-share/meta-share/LRIdentifierScheme"/>
        <rdfs:comment xml:lang="en">Universal Product Code</rdfs:comment>
        <rdfs:label xml:lang="en">UPC</rdfs:label>
    </owl:NamedIndividual>
    


    <!-- http://purl.org/spar/datacite/url -->

    <owl:NamedIndividual rdf:about="http://purl.org/spar/datacite/url">
        <rdf:type rdf:resource="http://w3id.org/meta-share/meta-share/DocumentIdentifierScheme"/>
        <rdf:type rdf:resource="http://w3id.org/meta-share/meta-share/LRIdentifierScheme"/>
        <rdf:type rdf:resource="http://w3id.org/meta-share/meta-share/MetadataRecordIdentifierScheme"/>
        <rdfs:comment xml:lang="en">Uniform Resource Locator</rdfs:comment>
        <rdfs:label xml:lang="en">URL</rdfs:label>
    </owl:NamedIndividual>
    


    <!-- http://purl.org/spar/datacite/urn -->

    <owl:NamedIndividual rdf:about="http://purl.org/spar/datacite/urn">
        <rdf:type rdf:resource="http://w3id.org/meta-share/meta-share/DocumentIdentifierScheme"/>
        <rdf:type rdf:resource="http://w3id.org/meta-share/meta-share/LRIdentifierScheme"/>
        <rdf:type rdf:resource="http://w3id.org/meta-share/meta-share/MetadataRecordIdentifierScheme"/>
        <rdfs:comment xml:lang="en">Uniform Resource Name</rdfs:comment>
        <rdfs:label xml:lang="en">URN</rdfs:label>
    </owl:NamedIndividual>
    


    <!-- http://rightsstatements.org/vocab/CNE/1.0/ -->

    <owl:NamedIndividual rdf:about="http://rightsstatements.org/vocab/CNE/1.0/">
        <rdf:type rdf:resource="http://w3id.org/meta-share/meta-share/AccessRightsStatementIdentifier"/>
        <ms:conformsTo rdf:resource="http://w3id.org/meta-share/meta-share/RightsStatementOrgScheme"/>
    </owl:NamedIndividual>
    


    <!-- http://rightsstatements.org/vocab/InC-EDU/1.0/ -->

    <owl:NamedIndividual rdf:about="http://rightsstatements.org/vocab/InC-EDU/1.0/">
        <rdf:type rdf:resource="http://w3id.org/meta-share/meta-share/AccessRightsStatementIdentifier"/>
        <ms:conformsTo rdf:resource="http://w3id.org/meta-share/meta-share/RightsStatementOrgScheme"/>
    </owl:NamedIndividual>
    


    <!-- http://rightsstatements.org/vocab/InC-NC/1.0/ -->

    <owl:NamedIndividual rdf:about="http://rightsstatements.org/vocab/InC-NC/1.0/">
        <rdf:type rdf:resource="http://w3id.org/meta-share/meta-share/AccessRightsStatementIdentifier"/>
        <ms:conformsTo rdf:resource="http://w3id.org/meta-share/meta-share/RightsStatementOrgScheme"/>
    </owl:NamedIndividual>
    


    <!-- http://rightsstatements.org/vocab/InC-OW-EU/1.0/ -->

    <owl:NamedIndividual rdf:about="http://rightsstatements.org/vocab/InC-OW-EU/1.0/">
        <rdf:type rdf:resource="http://w3id.org/meta-share/meta-share/AccessRightsStatementIdentifier"/>
        <ms:conformsTo rdf:resource="http://w3id.org/meta-share/meta-share/RightsStatementOrgScheme"/>
    </owl:NamedIndividual>
    


    <!-- http://rightsstatements.org/vocab/InC-RUU/1.0/ -->

    <owl:NamedIndividual rdf:about="http://rightsstatements.org/vocab/InC-RUU/1.0/">
        <rdf:type rdf:resource="http://w3id.org/meta-share/meta-share/AccessRightsStatementIdentifier"/>
        <ms:conformsTo rdf:resource="http://w3id.org/meta-share/meta-share/RightsStatementOrgScheme"/>
    </owl:NamedIndividual>
    


    <!-- http://rightsstatements.org/vocab/InC/1.0/ -->

    <owl:NamedIndividual rdf:about="http://rightsstatements.org/vocab/InC/1.0/">
        <rdf:type rdf:resource="http://w3id.org/meta-share/meta-share/AccessRightsStatementIdentifier"/>
        <ms:conformsTo rdf:resource="http://w3id.org/meta-share/meta-share/RightsStatementOrgScheme"/>
    </owl:NamedIndividual>
    


    <!-- http://rightsstatements.org/vocab/NKC/1.0/ -->

    <owl:NamedIndividual rdf:about="http://rightsstatements.org/vocab/NKC/1.0/">
        <rdf:type rdf:resource="http://w3id.org/meta-share/meta-share/AccessRightsStatementIdentifier"/>
        <ms:conformsTo rdf:resource="http://w3id.org/meta-share/meta-share/RightsStatementOrgScheme"/>
    </owl:NamedIndividual>
    


    <!-- http://rightsstatements.org/vocab/NoC-CR/1.0/ -->

    <owl:NamedIndividual rdf:about="http://rightsstatements.org/vocab/NoC-CR/1.0/">
        <rdf:type rdf:resource="http://w3id.org/meta-share/meta-share/AccessRightsStatementIdentifier"/>
        <ms:conformsTo rdf:resource="http://w3id.org/meta-share/meta-share/RightsStatementOrgScheme"/>
    </owl:NamedIndividual>
    


    <!-- http://rightsstatements.org/vocab/NoC-NC/1.0/ -->

    <owl:NamedIndividual rdf:about="http://rightsstatements.org/vocab/NoC-NC/1.0/">
        <rdf:type rdf:resource="http://w3id.org/meta-share/meta-share/AccessRightsStatementIdentifier"/>
        <ms:conformsTo rdf:resource="http://w3id.org/meta-share/meta-share/RightsStatementOrgScheme"/>
    </owl:NamedIndividual>
    


    <!-- http://rightsstatements.org/vocab/NoC-OKLR/1.0/ -->

    <owl:NamedIndividual rdf:about="http://rightsstatements.org/vocab/NoC-OKLR/1.0/">
        <rdf:type rdf:resource="http://w3id.org/meta-share/meta-share/AccessRightsStatementIdentifier"/>
        <ms:conformsTo rdf:resource="http://w3id.org/meta-share/meta-share/RightsStatementOrgScheme"/>
    </owl:NamedIndividual>
    


    <!-- http://rightsstatements.org/vocab/NoC-US/1.0/ -->

    <owl:NamedIndividual rdf:about="http://rightsstatements.org/vocab/NoC-US/1.0/">
        <rdf:type rdf:resource="http://w3id.org/meta-share/meta-share/AccessRightsStatementIdentifier"/>
        <ms:conformsTo rdf:resource="http://w3id.org/meta-share/meta-share/RightsStatementOrgScheme"/>
    </owl:NamedIndividual>
    


    <!-- http://rightsstatements.org/vocab/UND/1.0/ -->

    <owl:NamedIndividual rdf:about="http://rightsstatements.org/vocab/UND/1.0/">
        <rdf:type rdf:resource="http://w3id.org/meta-share/meta-share/AccessRightsStatementIdentifier"/>
        <ms:conformsTo rdf:resource="http://w3id.org/meta-share/meta-share/RightsStatementOrgScheme"/>
    </owl:NamedIndividual>
    


    <!-- http://w3id.org/meta-share/meta-share -->

    <owl:NamedIndividual rdf:about="http://w3id.org/meta-share/meta-share"/>
    


    <!-- http://w3id.org/meta-share/meta-share/ADPCM -->

    <owl:NamedIndividual rdf:about="http://w3id.org/meta-share/meta-share/ADPCM">
        <rdf:type rdf:resource="http://w3id.org/meta-share/meta-share/SignalEncoding"/>
        <rdfs:altLabel xml:lang="en">Adaptive differential pulse-code modulation</rdfs:altLabel>
        <rdfs:label xml:lang="en">ADPCM</rdfs:label>
    </owl:NamedIndividual>
    


    <!-- http://w3id.org/meta-share/meta-share/ANC_domainClassification -->

    <owl:NamedIndividual rdf:about="http://w3id.org/meta-share/meta-share/ANC_domainClassification">
        <rdf:type rdf:resource="http://w3id.org/meta-share/meta-share/DomainClassificationScheme"/>
        <rdfs:altLabel xml:lang="en">American National Corpus domain classification system</rdfs:altLabel>
        <rdfs:label xml:lang="en">ANC domain classification system</rdfs:label>
    </owl:NamedIndividual>
    


    <!-- http://w3id.org/meta-share/meta-share/ANC_genreClassification -->

    <owl:NamedIndividual rdf:about="http://w3id.org/meta-share/meta-share/ANC_genreClassification">
        <rdf:type rdf:resource="http://w3id.org/meta-share/meta-share/TextGenreClassificationScheme"/>
        <rdfs:altLabel xml:lang="en">American National Corpus genre classification scheme</rdfs:altLabel>
        <rdfs:label xml:lang="en">ANC genre classification scheme</rdfs:label>
    </owl:NamedIndividual>
    


    <!-- http://w3id.org/meta-share/meta-share/ART -->

    <owl:NamedIndividual rdf:about="http://w3id.org/meta-share/meta-share/ART">
        <rdf:type rdf:resource="http://w3id.org/meta-share/meta-share/Metric"/>
        <rdfs:altLabel xml:lang="en">Average Response Time</rdfs:altLabel>
        <rdfs:label xml:lang="en">ART</rdfs:label>
    </owl:NamedIndividual>
    


    <!-- http://w3id.org/meta-share/meta-share/AlvisNLP -->

    <owl:NamedIndividual rdf:about="http://w3id.org/meta-share/meta-share/AlvisNLP">
        <rdf:type rdf:resource="http://w3id.org/meta-share/meta-share/Framework"/>
        <rdfs:label xml:lang="en">AlvisNLP</rdfs:label>
    </owl:NamedIndividual>
    


    <!-- http://w3id.org/meta-share/meta-share/BML -->

    <owl:NamedIndividual rdf:about="http://w3id.org/meta-share/meta-share/BML">
        <rdf:type rdf:resource="http://w3id.org/meta-share/meta-share/StandardBestPractice"/>
        <ms:url>http://www.mindmakers.org/projects/bml-1-0/wiki#Introduction</ms:url>
        <rdfs:altLabel xml:lang="en">Behavior Markup Language</rdfs:altLabel>
        <rdfs:altLabel xml:lang="en">Behaviour Markup Language</rdfs:altLabel>
        <rdfs:label xml:lang="en">BML</rdfs:label>
    </owl:NamedIndividual>
    


    <!-- http://w3id.org/meta-share/meta-share/BNC_domainClassification -->

    <owl:NamedIndividual rdf:about="http://w3id.org/meta-share/meta-share/BNC_domainClassification">
        <rdf:type rdf:resource="http://w3id.org/meta-share/meta-share/DomainClassificationScheme"/>
        <rdfs:altLabel xml:lang="en">British National Corpus domain classification system</rdfs:altLabel>
        <rdfs:label xml:lang="en">BNC domain classification system</rdfs:label>
    </owl:NamedIndividual>
    


    <!-- http://w3id.org/meta-share/meta-share/BNC_textTypeClassification -->

    <owl:NamedIndividual rdf:about="http://w3id.org/meta-share/meta-share/BNC_textTypeClassification">
        <rdf:type rdf:resource="http://w3id.org/meta-share/meta-share/TextTypeClassificationScheme"/>
        <rdfs:label xml:lang="en">BNC text type classification scheme</rdfs:label>
    </owl:NamedIndividual>
    


    <!-- http://w3id.org/meta-share/meta-share/Big5 -->

    <owl:NamedIndividual rdf:about="http://w3id.org/meta-share/meta-share/Big5">
        <rdf:type rdf:resource="http://w3id.org/meta-share/meta-share/CharacterEncoding"/>
        <rdfs:label xml:lang="en">Big5</rdfs:label>
    </owl:NamedIndividual>
    


    <!-- http://w3id.org/meta-share/meta-share/Big5-HKSCS -->

    <owl:NamedIndividual rdf:about="http://w3id.org/meta-share/meta-share/Big5-HKSCS">
        <rdf:type rdf:resource="http://w3id.org/meta-share/meta-share/CharacterEncoding"/>
        <rdfs:label xml:lang="en">Big5-HKSCS</rdfs:label>
    </owl:NamedIndividual>
    


    <!-- http://w3id.org/meta-share/meta-share/Big5_Solaris -->

    <owl:NamedIndividual rdf:about="http://w3id.org/meta-share/meta-share/Big5_Solaris">
        <rdf:type rdf:resource="http://w3id.org/meta-share/meta-share/CharacterEncoding"/>
        <rdfs:label xml:lang="en">Big5_Solaris</rdfs:label>
    </owl:NamedIndividual>
    


    <!-- http://w3id.org/meta-share/meta-share/CD-ROM -->

    <owl:NamedIndividual rdf:about="http://w3id.org/meta-share/meta-share/CD-ROM">
        <rdf:type rdf:resource="http://w3id.org/meta-share/meta-share/DatasetDistributionForm"/>
        <rdfs:comment xml:lang="en">CD-ROM refers to a kind of distribution medium used for delivering a language resource; intended for resources delivered on CD-ROM</rdfs:comment>
        <rdfs:label xml:lang="en">CD-ROM</rdfs:label>
    </owl:NamedIndividual>
    


    <!-- http://w3id.org/meta-share/meta-share/CDMA -->

    <owl:NamedIndividual rdf:about="http://w3id.org/meta-share/meta-share/CDMA">
        <rdf:type rdf:resource="http://w3id.org/meta-share/meta-share/SourceChannelType"/>
        <rdfs:label xml:lang="en">CDMA</rdfs:label>
    </owl:NamedIndividual>
    


    <!-- http://w3id.org/meta-share/meta-share/CES -->

    <owl:NamedIndividual rdf:about="http://w3id.org/meta-share/meta-share/CES">
        <rdf:type rdf:resource="http://w3id.org/meta-share/meta-share/StandardBestPractice"/>
        <ms:url>https://www.cs.vassar.edu/CES/</ms:url>
        <rdfs:altLabel xml:lang="en">Corpus Encoding Standard</rdfs:altLabel>
        <rdfs:label xml:lang="en">CES</rdfs:label>
    </owl:NamedIndividual>
    


    <!-- http://w3id.org/meta-share/meta-share/CMYK -->

    <owl:NamedIndividual rdf:about="http://w3id.org/meta-share/meta-share/CMYK">
        <rdf:type rdf:resource="http://w3id.org/meta-share/meta-share/ColourSpace"/>
        <rdfs:label xml:lang="en">CMYK</rdfs:label>
    </owl:NamedIndividual>
    


    <!-- http://w3id.org/meta-share/meta-share/COARightsStatementScheme -->

    <owl:NamedIndividual rdf:about="http://w3id.org/meta-share/meta-share/COARightsStatementScheme">
        <rdf:type rdf:resource="http://w3id.org/meta-share/meta-share/AccessRightsStatementScheme"/>
        <rdfs:comment xml:lang="en">COAR access rights vocabulary (http://vocabularies.coar-repositories.org/documentation/access_rights/)</rdfs:comment>
        <rdfs:label xml:lang="en">COAR Rights Statement Scheme</rdfs:label>
    </owl:NamedIndividual>
    


    <!-- http://w3id.org/meta-share/meta-share/CORE -->

    <owl:NamedIndividual rdf:about="http://w3id.org/meta-share/meta-share/CORE">
        <rdf:type rdf:resource="http://w3id.org/meta-share/meta-share/MetadataRecordIdentifierScheme"/>
        <rdfs:label xml:lang="en">CORE</rdfs:label>
    </owl:NamedIndividual>
    


    <!-- http://w3id.org/meta-share/meta-share/ClarinEL_TextTypeClassification -->

    <owl:NamedIndividual rdf:about="http://w3id.org/meta-share/meta-share/ClarinEL_TextTypeClassification">
        <rdf:type rdf:resource="http://w3id.org/meta-share/meta-share/TextTypeClassificationScheme"/>
        <rdfs:label xml:lang="en">CLARIN_EL text type classification scheme</rdfs:label>
    </owl:NamedIndividual>
    


    <!-- http://w3id.org/meta-share/meta-share/ClarinEL_domainClassification -->

    <owl:NamedIndividual rdf:about="http://w3id.org/meta-share/meta-share/ClarinEL_domainClassification">
        <rdf:type rdf:resource="http://w3id.org/meta-share/meta-share/DomainClassificationScheme"/>
        <rdfs:label xml:lang="en">CLARIN-EL domain classification</rdfs:label>
    </owl:NamedIndividual>
    


    <!-- http://w3id.org/meta-share/meta-share/ClarinEl_TT001 -->

    <owl:NamedIndividual rdf:about="http://w3id.org/meta-share/meta-share/ClarinEl_TT001">
        <rdf:type rdf:resource="http://w3id.org/meta-share/meta-share/TextTypeIdentifier"/>
        <ms:conformsTo rdf:resource="http://w3id.org/meta-share/meta-share/ClarinEL_TextTypeClassification"/>
    </owl:NamedIndividual>
    


    <!-- http://w3id.org/meta-share/meta-share/ClarinEl_TT002 -->

    <owl:NamedIndividual rdf:about="http://w3id.org/meta-share/meta-share/ClarinEl_TT002">
        <rdf:type rdf:resource="http://w3id.org/meta-share/meta-share/TextTypeIdentifier"/>
        <ms:conformsTo rdf:resource="http://w3id.org/meta-share/meta-share/ClarinEL_TextTypeClassification"/>
    </owl:NamedIndividual>
    


    <!-- http://w3id.org/meta-share/meta-share/ClarinEl_TT003 -->

    <owl:NamedIndividual rdf:about="http://w3id.org/meta-share/meta-share/ClarinEl_TT003">
        <rdf:type rdf:resource="http://w3id.org/meta-share/meta-share/TextTypeIdentifier"/>
        <ms:conformsTo rdf:resource="http://w3id.org/meta-share/meta-share/ClarinEL_TextTypeClassification"/>
    </owl:NamedIndividual>
    


    <!-- http://w3id.org/meta-share/meta-share/ClarinEl_TT004 -->

    <owl:NamedIndividual rdf:about="http://w3id.org/meta-share/meta-share/ClarinEl_TT004">
        <rdf:type rdf:resource="http://w3id.org/meta-share/meta-share/TextTypeIdentifier"/>
        <ms:conformsTo rdf:resource="http://w3id.org/meta-share/meta-share/ClarinEL_TextTypeClassification"/>
    </owl:NamedIndividual>
    


    <!-- http://w3id.org/meta-share/meta-share/ClarinEl_TT005 -->

    <owl:NamedIndividual rdf:about="http://w3id.org/meta-share/meta-share/ClarinEl_TT005">
        <rdf:type rdf:resource="http://w3id.org/meta-share/meta-share/TextTypeIdentifier"/>
        <ms:conformsTo rdf:resource="http://w3id.org/meta-share/meta-share/ClarinEL_TextTypeClassification"/>
    </owl:NamedIndividual>
    


    <!-- http://w3id.org/meta-share/meta-share/ClarinEl_TT006 -->

    <owl:NamedIndividual rdf:about="http://w3id.org/meta-share/meta-share/ClarinEl_TT006">
        <rdf:type rdf:resource="http://w3id.org/meta-share/meta-share/TextTypeIdentifier"/>
        <ms:conformsTo rdf:resource="http://w3id.org/meta-share/meta-share/ClarinEL_TextTypeClassification"/>
    </owl:NamedIndividual>
    


    <!-- http://w3id.org/meta-share/meta-share/ClarinEl_TT007 -->

    <owl:NamedIndividual rdf:about="http://w3id.org/meta-share/meta-share/ClarinEl_TT007">
        <rdf:type rdf:resource="http://w3id.org/meta-share/meta-share/TextTypeIdentifier"/>
        <ms:conformsTo rdf:resource="http://w3id.org/meta-share/meta-share/ClarinEL_TextTypeClassification"/>
    </owl:NamedIndividual>
    


    <!-- http://w3id.org/meta-share/meta-share/ClarinEl_TT008 -->

    <owl:NamedIndividual rdf:about="http://w3id.org/meta-share/meta-share/ClarinEl_TT008">
        <rdf:type rdf:resource="http://w3id.org/meta-share/meta-share/TextTypeIdentifier"/>
        <ms:conformsTo rdf:resource="http://w3id.org/meta-share/meta-share/ClarinEL_TextTypeClassification"/>
    </owl:NamedIndividual>
    


    <!-- http://w3id.org/meta-share/meta-share/ClarinEl_TT009 -->

    <owl:NamedIndividual rdf:about="http://w3id.org/meta-share/meta-share/ClarinEl_TT009">
        <rdf:type rdf:resource="http://w3id.org/meta-share/meta-share/TextTypeIdentifier"/>
        <ms:conformsTo rdf:resource="http://w3id.org/meta-share/meta-share/ClarinEL_TextTypeClassification"/>
    </owl:NamedIndividual>
    


    <!-- http://w3id.org/meta-share/meta-share/ClarinEl_TT010 -->

    <owl:NamedIndividual rdf:about="http://w3id.org/meta-share/meta-share/ClarinEl_TT010">
        <rdf:type rdf:resource="http://w3id.org/meta-share/meta-share/TextTypeIdentifier"/>
        <ms:conformsTo rdf:resource="http://w3id.org/meta-share/meta-share/ClarinEL_TextTypeClassification"/>
    </owl:NamedIndividual>
    


    <!-- http://w3id.org/meta-share/meta-share/ClarinEl_TT011 -->

    <owl:NamedIndividual rdf:about="http://w3id.org/meta-share/meta-share/ClarinEl_TT011">
        <rdf:type rdf:resource="http://w3id.org/meta-share/meta-share/TextTypeIdentifier"/>
        <ms:conformsTo rdf:resource="http://w3id.org/meta-share/meta-share/ClarinEL_TextTypeClassification"/>
    </owl:NamedIndividual>
    


    <!-- http://w3id.org/meta-share/meta-share/ClarinEl_TT012 -->

    <owl:NamedIndividual rdf:about="http://w3id.org/meta-share/meta-share/ClarinEl_TT012">
        <rdf:type rdf:resource="http://w3id.org/meta-share/meta-share/TextTypeIdentifier"/>
        <ms:conformsTo rdf:resource="http://w3id.org/meta-share/meta-share/ClarinEL_TextTypeClassification"/>
    </owl:NamedIndividual>
    


    <!-- http://w3id.org/meta-share/meta-share/ClarinEl_TT013 -->

    <owl:NamedIndividual rdf:about="http://w3id.org/meta-share/meta-share/ClarinEl_TT013">
        <rdf:type rdf:resource="http://w3id.org/meta-share/meta-share/TextTypeIdentifier"/>
        <ms:conformsTo rdf:resource="http://w3id.org/meta-share/meta-share/ClarinEL_TextTypeClassification"/>
    </owl:NamedIndividual>
    


    <!-- http://w3id.org/meta-share/meta-share/ClarinEl_TT014 -->

    <owl:NamedIndividual rdf:about="http://w3id.org/meta-share/meta-share/ClarinEl_TT014">
        <rdf:type rdf:resource="http://w3id.org/meta-share/meta-share/TextTypeIdentifier"/>
        <ms:conformsTo rdf:resource="http://w3id.org/meta-share/meta-share/ClarinEL_TextTypeClassification"/>
    </owl:NamedIndividual>
    


    <!-- http://w3id.org/meta-share/meta-share/ClarinEl_TT015 -->

    <owl:NamedIndividual rdf:about="http://w3id.org/meta-share/meta-share/ClarinEl_TT015">
        <rdf:type rdf:resource="http://w3id.org/meta-share/meta-share/TextTypeIdentifier"/>
        <ms:conformsTo rdf:resource="http://w3id.org/meta-share/meta-share/ClarinEL_TextTypeClassification"/>
    </owl:NamedIndividual>
    


    <!-- http://w3id.org/meta-share/meta-share/ClarinEl_TT016 -->

    <owl:NamedIndividual rdf:about="http://w3id.org/meta-share/meta-share/ClarinEl_TT016">
        <rdf:type rdf:resource="http://w3id.org/meta-share/meta-share/TextTypeIdentifier"/>
        <ms:conformsTo rdf:resource="http://w3id.org/meta-share/meta-share/ClarinEL_TextTypeClassification"/>
    </owl:NamedIndividual>
    


    <!-- http://w3id.org/meta-share/meta-share/ClarinEl_TT017 -->

    <owl:NamedIndividual rdf:about="http://w3id.org/meta-share/meta-share/ClarinEl_TT017">
        <rdf:type rdf:resource="http://w3id.org/meta-share/meta-share/TextTypeIdentifier"/>
        <ms:conformsTo rdf:resource="http://w3id.org/meta-share/meta-share/ClarinEL_TextTypeClassification"/>
    </owl:NamedIndividual>
    


    <!-- http://w3id.org/meta-share/meta-share/ClarinEl_TT018 -->

    <owl:NamedIndividual rdf:about="http://w3id.org/meta-share/meta-share/ClarinEl_TT018">
        <rdf:type rdf:resource="http://w3id.org/meta-share/meta-share/TextTypeIdentifier"/>
        <ms:conformsTo rdf:resource="http://w3id.org/meta-share/meta-share/ClarinEL_TextTypeClassification"/>
    </owl:NamedIndividual>
    


    <!-- http://w3id.org/meta-share/meta-share/ClarinLicenceCategoryScheme -->

    <owl:NamedIndividual rdf:about="http://w3id.org/meta-share/meta-share/ClarinLicenceCategoryScheme">
        <rdf:type rdf:resource="http://w3id.org/meta-share/meta-share/LicenceCategoryScheme"/>
        <rdfs:label xml:lang="en">CLARIN licence category scheme</rdfs:label>
    </owl:NamedIndividual>
    


    <!-- http://w3id.org/meta-share/meta-share/Clarin_Domain001 -->

    <owl:NamedIndividual rdf:about="http://w3id.org/meta-share/meta-share/Clarin_Domain001">
        <rdf:type rdf:resource="http://w3id.org/meta-share/meta-share/DomainIdentifier"/>
        <ms:conformsTo rdf:resource="http://w3id.org/meta-share/meta-share/ClarinEL_domainClassification"/>
    </owl:NamedIndividual>
    


    <!-- http://w3id.org/meta-share/meta-share/Clarin_Domain002 -->

    <owl:NamedIndividual rdf:about="http://w3id.org/meta-share/meta-share/Clarin_Domain002">
        <rdf:type rdf:resource="http://w3id.org/meta-share/meta-share/DomainIdentifier"/>
        <ms:conformsTo rdf:resource="http://w3id.org/meta-share/meta-share/ClarinEL_domainClassification"/>
    </owl:NamedIndividual>
    


    <!-- http://w3id.org/meta-share/meta-share/Clarin_Domain003 -->

    <owl:NamedIndividual rdf:about="http://w3id.org/meta-share/meta-share/Clarin_Domain003">
        <rdf:type rdf:resource="http://w3id.org/meta-share/meta-share/DomainIdentifier"/>
        <ms:conformsTo rdf:resource="http://w3id.org/meta-share/meta-share/ClarinEL_domainClassification"/>
    </owl:NamedIndividual>
    


    <!-- http://w3id.org/meta-share/meta-share/Clarin_Domain004 -->

    <owl:NamedIndividual rdf:about="http://w3id.org/meta-share/meta-share/Clarin_Domain004">
        <rdf:type rdf:resource="http://w3id.org/meta-share/meta-share/DomainIdentifier"/>
        <ms:conformsTo rdf:resource="http://w3id.org/meta-share/meta-share/ClarinEL_domainClassification"/>
    </owl:NamedIndividual>
    


    <!-- http://w3id.org/meta-share/meta-share/Cp037 -->

    <owl:NamedIndividual rdf:about="http://w3id.org/meta-share/meta-share/Cp037">
        <rdf:type rdf:resource="http://w3id.org/meta-share/meta-share/CharacterEncoding"/>
        <rdfs:label xml:lang="en">Cp037</rdfs:label>
    </owl:NamedIndividual>
    


    <!-- http://w3id.org/meta-share/meta-share/Cp1006 -->

    <owl:NamedIndividual rdf:about="http://w3id.org/meta-share/meta-share/Cp1006">
        <rdf:type rdf:resource="http://w3id.org/meta-share/meta-share/CharacterEncoding"/>
        <rdfs:label xml:lang="en">Cp1006</rdfs:label>
    </owl:NamedIndividual>
    


    <!-- http://w3id.org/meta-share/meta-share/Cp1025 -->

    <owl:NamedIndividual rdf:about="http://w3id.org/meta-share/meta-share/Cp1025">
        <rdf:type rdf:resource="http://w3id.org/meta-share/meta-share/CharacterEncoding"/>
        <rdfs:label xml:lang="en">Cp1025</rdfs:label>
    </owl:NamedIndividual>
    


    <!-- http://w3id.org/meta-share/meta-share/Cp1026 -->

    <owl:NamedIndividual rdf:about="http://w3id.org/meta-share/meta-share/Cp1026">
        <rdf:type rdf:resource="http://w3id.org/meta-share/meta-share/CharacterEncoding"/>
        <rdfs:label xml:lang="en">Cp1026</rdfs:label>
    </owl:NamedIndividual>
    


    <!-- http://w3id.org/meta-share/meta-share/Cp1046 -->

    <owl:NamedIndividual rdf:about="http://w3id.org/meta-share/meta-share/Cp1046">
        <rdf:type rdf:resource="http://w3id.org/meta-share/meta-share/CharacterEncoding"/>
        <rdfs:label xml:lang="en">Cp1046</rdfs:label>
    </owl:NamedIndividual>
    


    <!-- http://w3id.org/meta-share/meta-share/Cp1047 -->

    <owl:NamedIndividual rdf:about="http://w3id.org/meta-share/meta-share/Cp1047">
        <rdf:type rdf:resource="http://w3id.org/meta-share/meta-share/CharacterEncoding"/>
        <rdfs:label xml:lang="en">Cp1047</rdfs:label>
    </owl:NamedIndividual>
    


    <!-- http://w3id.org/meta-share/meta-share/Cp1097 -->

    <owl:NamedIndividual rdf:about="http://w3id.org/meta-share/meta-share/Cp1097">
        <rdf:type rdf:resource="http://w3id.org/meta-share/meta-share/CharacterEncoding"/>
        <rdfs:label xml:lang="en">Cp1097</rdfs:label>
    </owl:NamedIndividual>
    


    <!-- http://w3id.org/meta-share/meta-share/Cp1098 -->

    <owl:NamedIndividual rdf:about="http://w3id.org/meta-share/meta-share/Cp1098">
        <rdf:type rdf:resource="http://w3id.org/meta-share/meta-share/CharacterEncoding"/>
        <rdfs:label xml:lang="en">Cp1098</rdfs:label>
    </owl:NamedIndividual>
    


    <!-- http://w3id.org/meta-share/meta-share/Cp1112 -->

    <owl:NamedIndividual rdf:about="http://w3id.org/meta-share/meta-share/Cp1112">
        <rdf:type rdf:resource="http://w3id.org/meta-share/meta-share/CharacterEncoding"/>
        <rdfs:label xml:lang="en">Cp1112</rdfs:label>
    </owl:NamedIndividual>
    


    <!-- http://w3id.org/meta-share/meta-share/Cp1122 -->

    <owl:NamedIndividual rdf:about="http://w3id.org/meta-share/meta-share/Cp1122">
        <rdf:type rdf:resource="http://w3id.org/meta-share/meta-share/CharacterEncoding"/>
        <rdfs:label xml:lang="en">Cp1122</rdfs:label>
    </owl:NamedIndividual>
    


    <!-- http://w3id.org/meta-share/meta-share/Cp1123 -->

    <owl:NamedIndividual rdf:about="http://w3id.org/meta-share/meta-share/Cp1123">
        <rdf:type rdf:resource="http://w3id.org/meta-share/meta-share/CharacterEncoding"/>
        <rdfs:label xml:lang="en">Cp1123</rdfs:label>
    </owl:NamedIndividual>
    


    <!-- http://w3id.org/meta-share/meta-share/Cp1124 -->

    <owl:NamedIndividual rdf:about="http://w3id.org/meta-share/meta-share/Cp1124">
        <rdf:type rdf:resource="http://w3id.org/meta-share/meta-share/CharacterEncoding"/>
        <rdfs:label xml:lang="en">Cp1124</rdfs:label>
    </owl:NamedIndividual>
    


    <!-- http://w3id.org/meta-share/meta-share/Cp1140 -->

    <owl:NamedIndividual rdf:about="http://w3id.org/meta-share/meta-share/Cp1140">
        <rdf:type rdf:resource="http://w3id.org/meta-share/meta-share/CharacterEncoding"/>
        <rdfs:label xml:lang="en">Cp1140</rdfs:label>
    </owl:NamedIndividual>
    


    <!-- http://w3id.org/meta-share/meta-share/Cp1141 -->

    <owl:NamedIndividual rdf:about="http://w3id.org/meta-share/meta-share/Cp1141">
        <rdf:type rdf:resource="http://w3id.org/meta-share/meta-share/CharacterEncoding"/>
        <rdfs:label xml:lang="en">Cp1141</rdfs:label>
    </owl:NamedIndividual>
    


    <!-- http://w3id.org/meta-share/meta-share/Cp1142 -->

    <owl:NamedIndividual rdf:about="http://w3id.org/meta-share/meta-share/Cp1142">
        <rdf:type rdf:resource="http://w3id.org/meta-share/meta-share/CharacterEncoding"/>
        <rdfs:label xml:lang="en">Cp1142</rdfs:label>
    </owl:NamedIndividual>
    


    <!-- http://w3id.org/meta-share/meta-share/Cp1143 -->

    <owl:NamedIndividual rdf:about="http://w3id.org/meta-share/meta-share/Cp1143">
        <rdf:type rdf:resource="http://w3id.org/meta-share/meta-share/CharacterEncoding"/>
        <rdfs:label xml:lang="en">Cp1143</rdfs:label>
    </owl:NamedIndividual>
    


    <!-- http://w3id.org/meta-share/meta-share/Cp1144 -->

    <owl:NamedIndividual rdf:about="http://w3id.org/meta-share/meta-share/Cp1144">
        <rdf:type rdf:resource="http://w3id.org/meta-share/meta-share/CharacterEncoding"/>
        <rdfs:label xml:lang="en">Cp1144</rdfs:label>
    </owl:NamedIndividual>
    


    <!-- http://w3id.org/meta-share/meta-share/Cp1145 -->

    <owl:NamedIndividual rdf:about="http://w3id.org/meta-share/meta-share/Cp1145">
        <rdf:type rdf:resource="http://w3id.org/meta-share/meta-share/CharacterEncoding"/>
        <rdfs:label xml:lang="en">Cp1145</rdfs:label>
    </owl:NamedIndividual>
    


    <!-- http://w3id.org/meta-share/meta-share/Cp1146 -->

    <owl:NamedIndividual rdf:about="http://w3id.org/meta-share/meta-share/Cp1146">
        <rdf:type rdf:resource="http://w3id.org/meta-share/meta-share/CharacterEncoding"/>
        <rdfs:label xml:lang="en">Cp1146</rdfs:label>
    </owl:NamedIndividual>
    


    <!-- http://w3id.org/meta-share/meta-share/Cp1147 -->

    <owl:NamedIndividual rdf:about="http://w3id.org/meta-share/meta-share/Cp1147">
        <rdf:type rdf:resource="http://w3id.org/meta-share/meta-share/CharacterEncoding"/>
        <rdfs:label xml:lang="en">Cp1147</rdfs:label>
    </owl:NamedIndividual>
    


    <!-- http://w3id.org/meta-share/meta-share/Cp1148 -->

    <owl:NamedIndividual rdf:about="http://w3id.org/meta-share/meta-share/Cp1148">
        <rdf:type rdf:resource="http://w3id.org/meta-share/meta-share/CharacterEncoding"/>
        <rdfs:label xml:lang="en">Cp1148</rdfs:label>
    </owl:NamedIndividual>
    


    <!-- http://w3id.org/meta-share/meta-share/Cp1149 -->

    <owl:NamedIndividual rdf:about="http://w3id.org/meta-share/meta-share/Cp1149">
        <rdf:type rdf:resource="http://w3id.org/meta-share/meta-share/CharacterEncoding"/>
        <rdfs:label xml:lang="en">Cp1149</rdfs:label>
    </owl:NamedIndividual>
    


    <!-- http://w3id.org/meta-share/meta-share/Cp1381 -->

    <owl:NamedIndividual rdf:about="http://w3id.org/meta-share/meta-share/Cp1381">
        <rdf:type rdf:resource="http://w3id.org/meta-share/meta-share/CharacterEncoding"/>
        <rdfs:label xml:lang="en">Cp1381</rdfs:label>
    </owl:NamedIndividual>
    


    <!-- http://w3id.org/meta-share/meta-share/Cp1383 -->

    <owl:NamedIndividual rdf:about="http://w3id.org/meta-share/meta-share/Cp1383">
        <rdf:type rdf:resource="http://w3id.org/meta-share/meta-share/CharacterEncoding"/>
        <rdfs:label xml:lang="en">Cp1383</rdfs:label>
    </owl:NamedIndividual>
    


    <!-- http://w3id.org/meta-share/meta-share/Cp273 -->

    <owl:NamedIndividual rdf:about="http://w3id.org/meta-share/meta-share/Cp273">
        <rdf:type rdf:resource="http://w3id.org/meta-share/meta-share/CharacterEncoding"/>
        <rdfs:label xml:lang="en">Cp273</rdfs:label>
    </owl:NamedIndividual>
    


    <!-- http://w3id.org/meta-share/meta-share/Cp277 -->

    <owl:NamedIndividual rdf:about="http://w3id.org/meta-share/meta-share/Cp277">
        <rdf:type rdf:resource="http://w3id.org/meta-share/meta-share/CharacterEncoding"/>
        <rdfs:label xml:lang="en">Cp277</rdfs:label>
    </owl:NamedIndividual>
    


    <!-- http://w3id.org/meta-share/meta-share/Cp278 -->

    <owl:NamedIndividual rdf:about="http://w3id.org/meta-share/meta-share/Cp278">
        <rdf:type rdf:resource="http://w3id.org/meta-share/meta-share/CharacterEncoding"/>
        <rdfs:label xml:lang="en">Cp278</rdfs:label>
    </owl:NamedIndividual>
    


    <!-- http://w3id.org/meta-share/meta-share/Cp280 -->

    <owl:NamedIndividual rdf:about="http://w3id.org/meta-share/meta-share/Cp280">
        <rdf:type rdf:resource="http://w3id.org/meta-share/meta-share/CharacterEncoding"/>
        <rdfs:label xml:lang="en">Cp280</rdfs:label>
    </owl:NamedIndividual>
    


    <!-- http://w3id.org/meta-share/meta-share/Cp284 -->

    <owl:NamedIndividual rdf:about="http://w3id.org/meta-share/meta-share/Cp284">
        <rdf:type rdf:resource="http://w3id.org/meta-share/meta-share/CharacterEncoding"/>
        <rdfs:label xml:lang="en">Cp284</rdfs:label>
    </owl:NamedIndividual>
    


    <!-- http://w3id.org/meta-share/meta-share/Cp285 -->

    <owl:NamedIndividual rdf:about="http://w3id.org/meta-share/meta-share/Cp285">
        <rdf:type rdf:resource="http://w3id.org/meta-share/meta-share/CharacterEncoding"/>
        <rdfs:label xml:lang="en">Cp285</rdfs:label>
    </owl:NamedIndividual>
    


    <!-- http://w3id.org/meta-share/meta-share/Cp297 -->

    <owl:NamedIndividual rdf:about="http://w3id.org/meta-share/meta-share/Cp297">
        <rdf:type rdf:resource="http://w3id.org/meta-share/meta-share/CharacterEncoding"/>
        <rdfs:label xml:lang="en">Cp297</rdfs:label>
    </owl:NamedIndividual>
    


    <!-- http://w3id.org/meta-share/meta-share/Cp33722 -->

    <owl:NamedIndividual rdf:about="http://w3id.org/meta-share/meta-share/Cp33722">
        <rdf:type rdf:resource="http://w3id.org/meta-share/meta-share/CharacterEncoding"/>
        <rdfs:label xml:lang="en">Cp33722</rdfs:label>
    </owl:NamedIndividual>
    


    <!-- http://w3id.org/meta-share/meta-share/Cp420 -->

    <owl:NamedIndividual rdf:about="http://w3id.org/meta-share/meta-share/Cp420">
        <rdf:type rdf:resource="http://w3id.org/meta-share/meta-share/CharacterEncoding"/>
        <rdfs:label xml:lang="en">Cp420</rdfs:label>
    </owl:NamedIndividual>
    


    <!-- http://w3id.org/meta-share/meta-share/Cp424 -->

    <owl:NamedIndividual rdf:about="http://w3id.org/meta-share/meta-share/Cp424">
        <rdf:type rdf:resource="http://w3id.org/meta-share/meta-share/CharacterEncoding"/>
        <rdfs:label xml:lang="en">Cp424</rdfs:label>
    </owl:NamedIndividual>
    


    <!-- http://w3id.org/meta-share/meta-share/Cp437 -->

    <owl:NamedIndividual rdf:about="http://w3id.org/meta-share/meta-share/Cp437">
        <rdf:type rdf:resource="http://w3id.org/meta-share/meta-share/CharacterEncoding"/>
        <rdfs:label xml:lang="en">Cp437</rdfs:label>
    </owl:NamedIndividual>
    


    <!-- http://w3id.org/meta-share/meta-share/Cp500 -->

    <owl:NamedIndividual rdf:about="http://w3id.org/meta-share/meta-share/Cp500">
        <rdf:type rdf:resource="http://w3id.org/meta-share/meta-share/CharacterEncoding"/>
        <rdfs:label xml:lang="en">Cp500</rdfs:label>
    </owl:NamedIndividual>
    


    <!-- http://w3id.org/meta-share/meta-share/Cp737 -->

    <owl:NamedIndividual rdf:about="http://w3id.org/meta-share/meta-share/Cp737">
        <rdf:type rdf:resource="http://w3id.org/meta-share/meta-share/CharacterEncoding"/>
        <rdfs:label xml:lang="en">Cp737</rdfs:label>
    </owl:NamedIndividual>
    


    <!-- http://w3id.org/meta-share/meta-share/Cp775 -->

    <owl:NamedIndividual rdf:about="http://w3id.org/meta-share/meta-share/Cp775">
        <rdf:type rdf:resource="http://w3id.org/meta-share/meta-share/CharacterEncoding"/>
        <rdfs:label xml:lang="en">Cp775</rdfs:label>
    </owl:NamedIndividual>
    


    <!-- http://w3id.org/meta-share/meta-share/Cp838 -->

    <owl:NamedIndividual rdf:about="http://w3id.org/meta-share/meta-share/Cp838">
        <rdf:type rdf:resource="http://w3id.org/meta-share/meta-share/CharacterEncoding"/>
        <rdfs:label xml:lang="en">Cp838</rdfs:label>
    </owl:NamedIndividual>
    


    <!-- http://w3id.org/meta-share/meta-share/Cp850 -->

    <owl:NamedIndividual rdf:about="http://w3id.org/meta-share/meta-share/Cp850">
        <rdf:type rdf:resource="http://w3id.org/meta-share/meta-share/CharacterEncoding"/>
        <rdfs:label xml:lang="en">Cp850</rdfs:label>
    </owl:NamedIndividual>
    


    <!-- http://w3id.org/meta-share/meta-share/Cp852 -->

    <owl:NamedIndividual rdf:about="http://w3id.org/meta-share/meta-share/Cp852">
        <rdf:type rdf:resource="http://w3id.org/meta-share/meta-share/CharacterEncoding"/>
        <rdfs:label xml:lang="en">Cp852</rdfs:label>
    </owl:NamedIndividual>
    


    <!-- http://w3id.org/meta-share/meta-share/Cp855 -->

    <owl:NamedIndividual rdf:about="http://w3id.org/meta-share/meta-share/Cp855">
        <rdf:type rdf:resource="http://w3id.org/meta-share/meta-share/CharacterEncoding"/>
        <rdfs:label xml:lang="en">Cp855</rdfs:label>
    </owl:NamedIndividual>
    


    <!-- http://w3id.org/meta-share/meta-share/Cp856 -->

    <owl:NamedIndividual rdf:about="http://w3id.org/meta-share/meta-share/Cp856">
        <rdf:type rdf:resource="http://w3id.org/meta-share/meta-share/CharacterEncoding"/>
        <rdfs:label xml:lang="en">Cp856</rdfs:label>
    </owl:NamedIndividual>
    


    <!-- http://w3id.org/meta-share/meta-share/Cp857 -->

    <owl:NamedIndividual rdf:about="http://w3id.org/meta-share/meta-share/Cp857">
        <rdf:type rdf:resource="http://w3id.org/meta-share/meta-share/CharacterEncoding"/>
        <rdfs:label xml:lang="en">Cp857</rdfs:label>
    </owl:NamedIndividual>
    


    <!-- http://w3id.org/meta-share/meta-share/Cp858 -->

    <owl:NamedIndividual rdf:about="http://w3id.org/meta-share/meta-share/Cp858">
        <rdf:type rdf:resource="http://w3id.org/meta-share/meta-share/CharacterEncoding"/>
        <rdfs:label xml:lang="en">Cp858</rdfs:label>
    </owl:NamedIndividual>
    


    <!-- http://w3id.org/meta-share/meta-share/Cp860 -->

    <owl:NamedIndividual rdf:about="http://w3id.org/meta-share/meta-share/Cp860">
        <rdf:type rdf:resource="http://w3id.org/meta-share/meta-share/CharacterEncoding"/>
        <rdfs:label xml:lang="en">Cp860</rdfs:label>
    </owl:NamedIndividual>
    


    <!-- http://w3id.org/meta-share/meta-share/Cp861 -->

    <owl:NamedIndividual rdf:about="http://w3id.org/meta-share/meta-share/Cp861">
        <rdf:type rdf:resource="http://w3id.org/meta-share/meta-share/CharacterEncoding"/>
        <rdfs:label xml:lang="en">Cp861</rdfs:label>
    </owl:NamedIndividual>
    


    <!-- http://w3id.org/meta-share/meta-share/Cp862 -->

    <owl:NamedIndividual rdf:about="http://w3id.org/meta-share/meta-share/Cp862">
        <rdf:type rdf:resource="http://w3id.org/meta-share/meta-share/CharacterEncoding"/>
        <rdfs:label xml:lang="en">Cp862</rdfs:label>
    </owl:NamedIndividual>
    


    <!-- http://w3id.org/meta-share/meta-share/Cp863 -->

    <owl:NamedIndividual rdf:about="http://w3id.org/meta-share/meta-share/Cp863">
        <rdf:type rdf:resource="http://w3id.org/meta-share/meta-share/CharacterEncoding"/>
        <rdfs:label xml:lang="en">Cp863</rdfs:label>
    </owl:NamedIndividual>
    


    <!-- http://w3id.org/meta-share/meta-share/Cp864 -->

    <owl:NamedIndividual rdf:about="http://w3id.org/meta-share/meta-share/Cp864">
        <rdf:type rdf:resource="http://w3id.org/meta-share/meta-share/CharacterEncoding"/>
        <rdfs:label xml:lang="en">Cp864</rdfs:label>
    </owl:NamedIndividual>
    


    <!-- http://w3id.org/meta-share/meta-share/Cp865 -->

    <owl:NamedIndividual rdf:about="http://w3id.org/meta-share/meta-share/Cp865">
        <rdf:type rdf:resource="http://w3id.org/meta-share/meta-share/CharacterEncoding"/>
        <rdfs:label xml:lang="en">Cp865</rdfs:label>
    </owl:NamedIndividual>
    


    <!-- http://w3id.org/meta-share/meta-share/Cp866 -->

    <owl:NamedIndividual rdf:about="http://w3id.org/meta-share/meta-share/Cp866">
        <rdf:type rdf:resource="http://w3id.org/meta-share/meta-share/CharacterEncoding"/>
        <rdfs:label xml:lang="en">Cp866</rdfs:label>
    </owl:NamedIndividual>
    


    <!-- http://w3id.org/meta-share/meta-share/Cp868 -->

    <owl:NamedIndividual rdf:about="http://w3id.org/meta-share/meta-share/Cp868">
        <rdf:type rdf:resource="http://w3id.org/meta-share/meta-share/CharacterEncoding"/>
        <rdfs:label xml:lang="en">Cp868</rdfs:label>
    </owl:NamedIndividual>
    


    <!-- http://w3id.org/meta-share/meta-share/Cp869 -->

    <owl:NamedIndividual rdf:about="http://w3id.org/meta-share/meta-share/Cp869">
        <rdf:type rdf:resource="http://w3id.org/meta-share/meta-share/CharacterEncoding"/>
        <rdfs:label xml:lang="en">Cp869</rdfs:label>
    </owl:NamedIndividual>
    


    <!-- http://w3id.org/meta-share/meta-share/Cp870 -->

    <owl:NamedIndividual rdf:about="http://w3id.org/meta-share/meta-share/Cp870">
        <rdf:type rdf:resource="http://w3id.org/meta-share/meta-share/CharacterEncoding"/>
        <rdfs:label xml:lang="en">Cp870</rdfs:label>
    </owl:NamedIndividual>
    


    <!-- http://w3id.org/meta-share/meta-share/Cp871 -->

    <owl:NamedIndividual rdf:about="http://w3id.org/meta-share/meta-share/Cp871">
        <rdf:type rdf:resource="http://w3id.org/meta-share/meta-share/CharacterEncoding"/>
        <rdfs:label xml:lang="en">Cp871</rdfs:label>
    </owl:NamedIndividual>
    


    <!-- http://w3id.org/meta-share/meta-share/Cp874 -->

    <owl:NamedIndividual rdf:about="http://w3id.org/meta-share/meta-share/Cp874">
        <rdf:type rdf:resource="http://w3id.org/meta-share/meta-share/CharacterEncoding"/>
        <rdfs:label xml:lang="en">Cp874</rdfs:label>
    </owl:NamedIndividual>
    


    <!-- http://w3id.org/meta-share/meta-share/Cp875 -->

    <owl:NamedIndividual rdf:about="http://w3id.org/meta-share/meta-share/Cp875">
        <rdf:type rdf:resource="http://w3id.org/meta-share/meta-share/CharacterEncoding"/>
        <rdfs:label xml:lang="en">Cp875</rdfs:label>
    </owl:NamedIndividual>
    


    <!-- http://w3id.org/meta-share/meta-share/Cp918 -->

    <owl:NamedIndividual rdf:about="http://w3id.org/meta-share/meta-share/Cp918">
        <rdf:type rdf:resource="http://w3id.org/meta-share/meta-share/CharacterEncoding"/>
        <rdfs:label xml:lang="en">Cp918</rdfs:label>
    </owl:NamedIndividual>
    


    <!-- http://w3id.org/meta-share/meta-share/Cp921 -->

    <owl:NamedIndividual rdf:about="http://w3id.org/meta-share/meta-share/Cp921">
        <rdf:type rdf:resource="http://w3id.org/meta-share/meta-share/CharacterEncoding"/>
        <rdfs:label xml:lang="en">Cp921</rdfs:label>
    </owl:NamedIndividual>
    


    <!-- http://w3id.org/meta-share/meta-share/Cp922 -->

    <owl:NamedIndividual rdf:about="http://w3id.org/meta-share/meta-share/Cp922">
        <rdf:type rdf:resource="http://w3id.org/meta-share/meta-share/CharacterEncoding"/>
        <rdfs:label xml:lang="en">Cp922</rdfs:label>
    </owl:NamedIndividual>
    


    <!-- http://w3id.org/meta-share/meta-share/Cp930 -->

    <owl:NamedIndividual rdf:about="http://w3id.org/meta-share/meta-share/Cp930">
        <rdf:type rdf:resource="http://w3id.org/meta-share/meta-share/CharacterEncoding"/>
        <rdfs:label xml:lang="en">Cp930</rdfs:label>
    </owl:NamedIndividual>
    


    <!-- http://w3id.org/meta-share/meta-share/Cp933 -->

    <owl:NamedIndividual rdf:about="http://w3id.org/meta-share/meta-share/Cp933">
        <rdf:type rdf:resource="http://w3id.org/meta-share/meta-share/CharacterEncoding"/>
        <rdfs:label xml:lang="en">Cp933</rdfs:label>
    </owl:NamedIndividual>
    


    <!-- http://w3id.org/meta-share/meta-share/Cp935 -->

    <owl:NamedIndividual rdf:about="http://w3id.org/meta-share/meta-share/Cp935">
        <rdf:type rdf:resource="http://w3id.org/meta-share/meta-share/CharacterEncoding"/>
        <rdfs:label xml:lang="en">Cp935</rdfs:label>
    </owl:NamedIndividual>
    


    <!-- http://w3id.org/meta-share/meta-share/Cp937 -->

    <owl:NamedIndividual rdf:about="http://w3id.org/meta-share/meta-share/Cp937">
        <rdf:type rdf:resource="http://w3id.org/meta-share/meta-share/CharacterEncoding"/>
        <rdfs:label xml:lang="en">Cp937</rdfs:label>
    </owl:NamedIndividual>
    


    <!-- http://w3id.org/meta-share/meta-share/Cp939 -->

    <owl:NamedIndividual rdf:about="http://w3id.org/meta-share/meta-share/Cp939">
        <rdf:type rdf:resource="http://w3id.org/meta-share/meta-share/CharacterEncoding"/>
        <rdfs:label xml:lang="en">Cp939</rdfs:label>
    </owl:NamedIndividual>
    


    <!-- http://w3id.org/meta-share/meta-share/Cp942 -->

    <owl:NamedIndividual rdf:about="http://w3id.org/meta-share/meta-share/Cp942">
        <rdf:type rdf:resource="http://w3id.org/meta-share/meta-share/CharacterEncoding"/>
        <rdfs:label xml:lang="en">Cp942</rdfs:label>
    </owl:NamedIndividual>
    


    <!-- http://w3id.org/meta-share/meta-share/Cp942C -->

    <owl:NamedIndividual rdf:about="http://w3id.org/meta-share/meta-share/Cp942C">
        <rdf:type rdf:resource="http://w3id.org/meta-share/meta-share/CharacterEncoding"/>
        <rdfs:label xml:lang="en">Cp942C</rdfs:label>
    </owl:NamedIndividual>
    


    <!-- http://w3id.org/meta-share/meta-share/Cp943 -->

    <owl:NamedIndividual rdf:about="http://w3id.org/meta-share/meta-share/Cp943">
        <rdf:type rdf:resource="http://w3id.org/meta-share/meta-share/CharacterEncoding"/>
        <rdfs:label xml:lang="en">Cp943</rdfs:label>
    </owl:NamedIndividual>
    


    <!-- http://w3id.org/meta-share/meta-share/Cp943C -->

    <owl:NamedIndividual rdf:about="http://w3id.org/meta-share/meta-share/Cp943C">
        <rdf:type rdf:resource="http://w3id.org/meta-share/meta-share/CharacterEncoding"/>
        <rdfs:label xml:lang="en">Cp943C</rdfs:label>
    </owl:NamedIndividual>
    


    <!-- http://w3id.org/meta-share/meta-share/Cp948 -->

    <owl:NamedIndividual rdf:about="http://w3id.org/meta-share/meta-share/Cp948">
        <rdf:type rdf:resource="http://w3id.org/meta-share/meta-share/CharacterEncoding"/>
        <rdfs:label xml:lang="en">Cp948</rdfs:label>
    </owl:NamedIndividual>
    


    <!-- http://w3id.org/meta-share/meta-share/Cp949 -->

    <owl:NamedIndividual rdf:about="http://w3id.org/meta-share/meta-share/Cp949">
        <rdf:type rdf:resource="http://w3id.org/meta-share/meta-share/CharacterEncoding"/>
        <rdfs:label xml:lang="en">Cp949</rdfs:label>
    </owl:NamedIndividual>
    


    <!-- http://w3id.org/meta-share/meta-share/Cp949C -->

    <owl:NamedIndividual rdf:about="http://w3id.org/meta-share/meta-share/Cp949C">
        <rdf:type rdf:resource="http://w3id.org/meta-share/meta-share/CharacterEncoding"/>
        <rdfs:label xml:lang="en">Cp949C</rdfs:label>
    </owl:NamedIndividual>
    


    <!-- http://w3id.org/meta-share/meta-share/Cp950 -->

    <owl:NamedIndividual rdf:about="http://w3id.org/meta-share/meta-share/Cp950">
        <rdf:type rdf:resource="http://w3id.org/meta-share/meta-share/CharacterEncoding"/>
        <rdfs:label xml:lang="en">Cp950</rdfs:label>
    </owl:NamedIndividual>
    


    <!-- http://w3id.org/meta-share/meta-share/Cp964 -->

    <owl:NamedIndividual rdf:about="http://w3id.org/meta-share/meta-share/Cp964">
        <rdf:type rdf:resource="http://w3id.org/meta-share/meta-share/CharacterEncoding"/>
        <rdfs:label xml:lang="en">Cp964</rdfs:label>
    </owl:NamedIndividual>
    


    <!-- http://w3id.org/meta-share/meta-share/Cp970 -->

    <owl:NamedIndividual rdf:about="http://w3id.org/meta-share/meta-share/Cp970">
        <rdf:type rdf:resource="http://w3id.org/meta-share/meta-share/CharacterEncoding"/>
        <rdfs:label xml:lang="en">Cp970</rdfs:label>
    </owl:NamedIndividual>
    


    <!-- http://w3id.org/meta-share/meta-share/DAT -->

    <owl:NamedIndividual rdf:about="http://w3id.org/meta-share/meta-share/DAT">
        <rdf:type rdf:resource="http://w3id.org/meta-share/meta-share/RecordingDeviceType"/>
        <rdfs:label xml:lang="en">DAT</rdfs:label>
    </owl:NamedIndividual>
    


    <!-- http://w3id.org/meta-share/meta-share/DDC000 -->

    <owl:NamedIndividual rdf:about="http://w3id.org/meta-share/meta-share/DDC000">
        <rdf:type rdf:resource="http://w3id.org/meta-share/meta-share/DomainIdentifier"/>
        <ms:conformsTo rdf:resource="http://w3id.org/meta-share/meta-share/DDC_classification"/>
    </owl:NamedIndividual>
    


    <!-- http://w3id.org/meta-share/meta-share/DDC070 -->

    <owl:NamedIndividual rdf:about="http://w3id.org/meta-share/meta-share/DDC070">
        <rdf:type rdf:resource="http://w3id.org/meta-share/meta-share/DomainIdentifier"/>
        <ms:conformsTo rdf:resource="http://w3id.org/meta-share/meta-share/DDC_classification"/>
    </owl:NamedIndividual>
    


    <!-- http://w3id.org/meta-share/meta-share/DDC100 -->

    <owl:NamedIndividual rdf:about="http://w3id.org/meta-share/meta-share/DDC100">
        <rdf:type rdf:resource="http://w3id.org/meta-share/meta-share/DomainIdentifier"/>
        <ms:conformsTo rdf:resource="http://w3id.org/meta-share/meta-share/DDC_classification"/>
    </owl:NamedIndividual>
    


    <!-- http://w3id.org/meta-share/meta-share/DDC150 -->

    <owl:NamedIndividual rdf:about="http://w3id.org/meta-share/meta-share/DDC150">
        <rdf:type rdf:resource="http://w3id.org/meta-share/meta-share/DomainIdentifier"/>
        <ms:conformsTo rdf:resource="http://w3id.org/meta-share/meta-share/DDC_classification"/>
    </owl:NamedIndividual>
    


    <!-- http://w3id.org/meta-share/meta-share/DDC200 -->

    <owl:NamedIndividual rdf:about="http://w3id.org/meta-share/meta-share/DDC200">
        <rdf:type rdf:resource="http://w3id.org/meta-share/meta-share/DomainIdentifier"/>
        <ms:conformsTo rdf:resource="http://w3id.org/meta-share/meta-share/DDC_classification"/>
    </owl:NamedIndividual>
    


    <!-- http://w3id.org/meta-share/meta-share/DDC300 -->

    <owl:NamedIndividual rdf:about="http://w3id.org/meta-share/meta-share/DDC300">
        <rdf:type rdf:resource="http://w3id.org/meta-share/meta-share/DomainIdentifier"/>
        <ms:conformsTo rdf:resource="http://w3id.org/meta-share/meta-share/DDC_classification"/>
    </owl:NamedIndividual>
    


    <!-- http://w3id.org/meta-share/meta-share/DDC301 -->

    <owl:NamedIndividual rdf:about="http://w3id.org/meta-share/meta-share/DDC301">
        <rdf:type rdf:resource="http://w3id.org/meta-share/meta-share/DomainIdentifier"/>
        <ms:conformsTo rdf:resource="http://w3id.org/meta-share/meta-share/DDC_classification"/>
    </owl:NamedIndividual>
    


    <!-- http://w3id.org/meta-share/meta-share/DDC310 -->

    <owl:NamedIndividual rdf:about="http://w3id.org/meta-share/meta-share/DDC310">
        <rdf:type rdf:resource="http://w3id.org/meta-share/meta-share/DomainIdentifier"/>
        <ms:conformsTo rdf:resource="http://w3id.org/meta-share/meta-share/DDC_classification"/>
    </owl:NamedIndividual>
    


    <!-- http://w3id.org/meta-share/meta-share/DDC320 -->

    <owl:NamedIndividual rdf:about="http://w3id.org/meta-share/meta-share/DDC320">
        <rdf:type rdf:resource="http://w3id.org/meta-share/meta-share/DomainIdentifier"/>
        <ms:conformsTo rdf:resource="http://w3id.org/meta-share/meta-share/DDC_classification"/>
    </owl:NamedIndividual>
    


    <!-- http://w3id.org/meta-share/meta-share/DDC330 -->

    <owl:NamedIndividual rdf:about="http://w3id.org/meta-share/meta-share/DDC330">
        <rdf:type rdf:resource="http://w3id.org/meta-share/meta-share/DomainIdentifier"/>
    </owl:NamedIndividual>
    


    <!-- http://w3id.org/meta-share/meta-share/DDC340 -->

    <owl:NamedIndividual rdf:about="http://w3id.org/meta-share/meta-share/DDC340">
        <rdf:type rdf:resource="http://w3id.org/meta-share/meta-share/DomainIdentifier"/>
        <ms:conformsTo rdf:resource="http://w3id.org/meta-share/meta-share/DDC_classification"/>
    </owl:NamedIndividual>
    


    <!-- http://w3id.org/meta-share/meta-share/DDC351 -->

    <owl:NamedIndividual rdf:about="http://w3id.org/meta-share/meta-share/DDC351">
        <rdf:type rdf:resource="http://w3id.org/meta-share/meta-share/DomainIdentifier"/>
        <ms:conformsTo rdf:resource="http://w3id.org/meta-share/meta-share/DDC_classification"/>
    </owl:NamedIndividual>
    


    <!-- http://w3id.org/meta-share/meta-share/DDC360 -->

    <owl:NamedIndividual rdf:about="http://w3id.org/meta-share/meta-share/DDC360">
        <rdf:type rdf:resource="http://w3id.org/meta-share/meta-share/DomainIdentifier"/>
        <ms:conformsTo rdf:resource="http://w3id.org/meta-share/meta-share/DDC_classification"/>
    </owl:NamedIndividual>
    


    <!-- http://w3id.org/meta-share/meta-share/DDC370 -->

    <owl:NamedIndividual rdf:about="http://w3id.org/meta-share/meta-share/DDC370">
        <rdf:type rdf:resource="http://w3id.org/meta-share/meta-share/DomainIdentifier"/>
    </owl:NamedIndividual>
    


    <!-- http://w3id.org/meta-share/meta-share/DDC381 -->

    <owl:NamedIndividual rdf:about="http://w3id.org/meta-share/meta-share/DDC381">
        <rdf:type rdf:resource="http://w3id.org/meta-share/meta-share/DomainIdentifier"/>
        <ms:conformsTo rdf:resource="http://w3id.org/meta-share/meta-share/DDC_classification"/>
    </owl:NamedIndividual>
    


    <!-- http://w3id.org/meta-share/meta-share/DDC384 -->

    <owl:NamedIndividual rdf:about="http://w3id.org/meta-share/meta-share/DDC384">
        <rdf:type rdf:resource="http://w3id.org/meta-share/meta-share/DomainIdentifier"/>
        <ms:conformsTo rdf:resource="http://w3id.org/meta-share/meta-share/DDC_classification"/>
        <rdfs:label>DDC384</rdfs:label>
    </owl:NamedIndividual>
    


    <!-- http://w3id.org/meta-share/meta-share/DDC388 -->

    <owl:NamedIndividual rdf:about="http://w3id.org/meta-share/meta-share/DDC388">
        <rdf:type rdf:resource="http://w3id.org/meta-share/meta-share/DomainIdentifier"/>
        <ms:conformsTo rdf:resource="http://w3id.org/meta-share/meta-share/DDC_classification"/>
        <rdfs:label xml:lang="en">DDC388</rdfs:label>
    </owl:NamedIndividual>
    


    <!-- http://w3id.org/meta-share/meta-share/DDC400 -->

    <owl:NamedIndividual rdf:about="http://w3id.org/meta-share/meta-share/DDC400">
        <rdf:type rdf:resource="http://w3id.org/meta-share/meta-share/DomainIdentifier"/>
        <ms:conformsTo rdf:resource="http://w3id.org/meta-share/meta-share/DDC_classification"/>
    </owl:NamedIndividual>
    


    <!-- http://w3id.org/meta-share/meta-share/DDC410 -->

    <owl:NamedIndividual rdf:about="http://w3id.org/meta-share/meta-share/DDC410">
        <rdf:type rdf:resource="http://w3id.org/meta-share/meta-share/DomainIdentifier"/>
        <ms:conformsTo rdf:resource="http://w3id.org/meta-share/meta-share/DDC_classification"/>
    </owl:NamedIndividual>
    


    <!-- http://w3id.org/meta-share/meta-share/DDC500 -->

    <owl:NamedIndividual rdf:about="http://w3id.org/meta-share/meta-share/DDC500">
        <rdf:type rdf:resource="http://w3id.org/meta-share/meta-share/DomainIdentifier"/>
        <ms:conformsTo rdf:resource="http://w3id.org/meta-share/meta-share/DDC_classification"/>
    </owl:NamedIndividual>
    


    <!-- http://w3id.org/meta-share/meta-share/DDC510 -->

    <owl:NamedIndividual rdf:about="http://w3id.org/meta-share/meta-share/DDC510">
        <rdf:type rdf:resource="http://w3id.org/meta-share/meta-share/DomainIdentifier"/>
        <ms:conformsTo rdf:resource="http://w3id.org/meta-share/meta-share/DDC_classification"/>
    </owl:NamedIndividual>
    


    <!-- http://w3id.org/meta-share/meta-share/DDC520 -->

    <owl:NamedIndividual rdf:about="http://w3id.org/meta-share/meta-share/DDC520">
        <rdf:type rdf:resource="http://w3id.org/meta-share/meta-share/DomainIdentifier"/>
        <ms:conformsTo rdf:resource="http://w3id.org/meta-share/meta-share/DDC_classification"/>
    </owl:NamedIndividual>
    


    <!-- http://w3id.org/meta-share/meta-share/DDC530 -->

    <owl:NamedIndividual rdf:about="http://w3id.org/meta-share/meta-share/DDC530">
        <rdf:type rdf:resource="http://w3id.org/meta-share/meta-share/DomainIdentifier"/>
        <ms:conformsTo rdf:resource="http://w3id.org/meta-share/meta-share/DDC_classification"/>
    </owl:NamedIndividual>
    


    <!-- http://w3id.org/meta-share/meta-share/DDC540 -->

    <owl:NamedIndividual rdf:about="http://w3id.org/meta-share/meta-share/DDC540">
        <rdf:type rdf:resource="http://w3id.org/meta-share/meta-share/DomainIdentifier"/>
        <ms:conformsTo rdf:resource="http://w3id.org/meta-share/meta-share/DDC_classification"/>
    </owl:NamedIndividual>
    


    <!-- http://w3id.org/meta-share/meta-share/DDC550 -->

    <owl:NamedIndividual rdf:about="http://w3id.org/meta-share/meta-share/DDC550">
        <rdf:type rdf:resource="http://w3id.org/meta-share/meta-share/DomainIdentifier"/>
        <ms:conformsTo rdf:resource="http://w3id.org/meta-share/meta-share/DDC_classification"/>
    </owl:NamedIndividual>
    


    <!-- http://w3id.org/meta-share/meta-share/DDC560 -->

    <owl:NamedIndividual rdf:about="http://w3id.org/meta-share/meta-share/DDC560">
        <rdf:type rdf:resource="http://w3id.org/meta-share/meta-share/DomainIdentifier"/>
        <ms:conformsTo rdf:resource="http://w3id.org/meta-share/meta-share/DDC_classification"/>
    </owl:NamedIndividual>
    


    <!-- http://w3id.org/meta-share/meta-share/DDC570 -->

    <owl:NamedIndividual rdf:about="http://w3id.org/meta-share/meta-share/DDC570">
        <rdf:type rdf:resource="http://w3id.org/meta-share/meta-share/DomainIdentifier"/>
    </owl:NamedIndividual>
    


    <!-- http://w3id.org/meta-share/meta-share/DDC572 -->

    <owl:NamedIndividual rdf:about="http://w3id.org/meta-share/meta-share/DDC572">
        <rdf:type rdf:resource="http://w3id.org/meta-share/meta-share/DomainIdentifier"/>
    </owl:NamedIndividual>
    


    <!-- http://w3id.org/meta-share/meta-share/DDC580 -->

    <owl:NamedIndividual rdf:about="http://w3id.org/meta-share/meta-share/DDC580">
        <rdf:type rdf:resource="http://w3id.org/meta-share/meta-share/DomainIdentifier"/>
        <ms:conformsTo rdf:resource="http://w3id.org/meta-share/meta-share/DDC_classification"/>
    </owl:NamedIndividual>
    


    <!-- http://w3id.org/meta-share/meta-share/DDC590 -->

    <owl:NamedIndividual rdf:about="http://w3id.org/meta-share/meta-share/DDC590">
        <rdf:type rdf:resource="http://w3id.org/meta-share/meta-share/DomainIdentifier"/>
        <ms:conformsTo rdf:resource="http://w3id.org/meta-share/meta-share/DDC_classification"/>
    </owl:NamedIndividual>
    


    <!-- http://w3id.org/meta-share/meta-share/DDC600 -->

    <owl:NamedIndividual rdf:about="http://w3id.org/meta-share/meta-share/DDC600">
        <rdf:type rdf:resource="http://w3id.org/meta-share/meta-share/DomainIdentifier"/>
        <ms:conformsTo rdf:resource="http://w3id.org/meta-share/meta-share/DDC_classification"/>
    </owl:NamedIndividual>
    


    <!-- http://w3id.org/meta-share/meta-share/DDC610 -->

    <owl:NamedIndividual rdf:about="http://w3id.org/meta-share/meta-share/DDC610">
        <rdf:type rdf:resource="http://w3id.org/meta-share/meta-share/DomainIdentifier"/>
    </owl:NamedIndividual>
    


    <!-- http://w3id.org/meta-share/meta-share/DDC620 -->

    <owl:NamedIndividual rdf:about="http://w3id.org/meta-share/meta-share/DDC620">
        <rdf:type rdf:resource="http://w3id.org/meta-share/meta-share/DomainIdentifier"/>
        <ms:conformsTo rdf:resource="http://w3id.org/meta-share/meta-share/DDC_classification"/>
    </owl:NamedIndividual>
    


    <!-- http://w3id.org/meta-share/meta-share/DDC621 -->

    <owl:NamedIndividual rdf:about="http://w3id.org/meta-share/meta-share/DDC621">
        <rdf:type rdf:resource="http://w3id.org/meta-share/meta-share/DomainIdentifier"/>
        <ms:conformsTo rdf:resource="http://w3id.org/meta-share/meta-share/DDC_classification"/>
    </owl:NamedIndividual>
    


    <!-- http://w3id.org/meta-share/meta-share/DDC630 -->

    <owl:NamedIndividual rdf:about="http://w3id.org/meta-share/meta-share/DDC630">
        <rdf:type rdf:resource="http://w3id.org/meta-share/meta-share/DomainIdentifier"/>
        <ms:conformsTo rdf:resource="http://w3id.org/meta-share/meta-share/DDC_classification"/>
        <rdfs:label xml:lang="en">DDC630</rdfs:label>
    </owl:NamedIndividual>
    


    <!-- http://w3id.org/meta-share/meta-share/DDC640 -->

    <owl:NamedIndividual rdf:about="http://w3id.org/meta-share/meta-share/DDC640">
        <rdf:type rdf:resource="http://w3id.org/meta-share/meta-share/DomainIdentifier"/>
        <ms:conformsTo rdf:resource="http://w3id.org/meta-share/meta-share/DDC_classification"/>
    </owl:NamedIndividual>
    


    <!-- http://w3id.org/meta-share/meta-share/DDC650 -->

    <owl:NamedIndividual rdf:about="http://w3id.org/meta-share/meta-share/DDC650">
        <rdf:type rdf:resource="http://w3id.org/meta-share/meta-share/DomainIdentifier"/>
    </owl:NamedIndividual>
    


    <!-- http://w3id.org/meta-share/meta-share/DDC659 -->

    <owl:NamedIndividual rdf:about="http://w3id.org/meta-share/meta-share/DDC659">
        <rdf:type rdf:resource="http://w3id.org/meta-share/meta-share/DomainIdentifier"/>
        <ms:conformsTo rdf:resource="http://w3id.org/meta-share/meta-share/DDC_classification"/>
        <rdfs:label xml:lang="en">DDC659</rdfs:label>
    </owl:NamedIndividual>
    


    <!-- http://w3id.org/meta-share/meta-share/DDC660 -->

    <owl:NamedIndividual rdf:about="http://w3id.org/meta-share/meta-share/DDC660">
        <rdf:type rdf:resource="http://w3id.org/meta-share/meta-share/DomainIdentifier"/>
        <ms:conformsTo rdf:resource="http://w3id.org/meta-share/meta-share/DDC_classification"/>
    </owl:NamedIndividual>
    


    <!-- http://w3id.org/meta-share/meta-share/DDC670 -->

    <owl:NamedIndividual rdf:about="http://w3id.org/meta-share/meta-share/DDC670">
        <rdf:type rdf:resource="http://w3id.org/meta-share/meta-share/DomainIdentifier"/>
        <ms:conformsTo rdf:resource="http://w3id.org/meta-share/meta-share/DDC_classification"/>
    </owl:NamedIndividual>
    


    <!-- http://w3id.org/meta-share/meta-share/DDC683 -->

    <owl:NamedIndividual rdf:about="http://w3id.org/meta-share/meta-share/DDC683">
        <rdf:type rdf:resource="http://w3id.org/meta-share/meta-share/DomainIdentifier"/>
        <ms:conformsTo rdf:resource="http://w3id.org/meta-share/meta-share/DDC_classification"/>
    </owl:NamedIndividual>
    


    <!-- http://w3id.org/meta-share/meta-share/DDC690 -->

    <owl:NamedIndividual rdf:about="http://w3id.org/meta-share/meta-share/DDC690">
        <rdf:type rdf:resource="http://w3id.org/meta-share/meta-share/DomainIdentifier"/>
    </owl:NamedIndividual>
    


    <!-- http://w3id.org/meta-share/meta-share/DDC700 -->

    <owl:NamedIndividual rdf:about="http://w3id.org/meta-share/meta-share/DDC700">
        <rdf:type rdf:resource="http://w3id.org/meta-share/meta-share/DomainIdentifier"/>
        <ms:conformsTo rdf:resource="http://w3id.org/meta-share/meta-share/DDC_classification"/>
    </owl:NamedIndividual>
    


    <!-- http://w3id.org/meta-share/meta-share/DDC720 -->

    <owl:NamedIndividual rdf:about="http://w3id.org/meta-share/meta-share/DDC720">
        <rdf:type rdf:resource="http://w3id.org/meta-share/meta-share/DomainIdentifier"/>
        <ms:conformsTo rdf:resource="http://w3id.org/meta-share/meta-share/DDC_classification"/>
    </owl:NamedIndividual>
    


    <!-- http://w3id.org/meta-share/meta-share/DDC730 -->

    <owl:NamedIndividual rdf:about="http://w3id.org/meta-share/meta-share/DDC730">
        <rdf:type rdf:resource="http://w3id.org/meta-share/meta-share/DomainIdentifier"/>
    </owl:NamedIndividual>
    


    <!-- http://w3id.org/meta-share/meta-share/DDC740 -->

    <owl:NamedIndividual rdf:about="http://w3id.org/meta-share/meta-share/DDC740">
        <rdf:type rdf:resource="http://w3id.org/meta-share/meta-share/DomainIdentifier"/>
        <ms:conformsTo rdf:resource="http://w3id.org/meta-share/meta-share/DDC_classification"/>
    </owl:NamedIndividual>
    


    <!-- http://w3id.org/meta-share/meta-share/DDC750 -->

    <owl:NamedIndividual rdf:about="http://w3id.org/meta-share/meta-share/DDC750">
        <rdf:type rdf:resource="http://w3id.org/meta-share/meta-share/DomainIdentifier"/>
        <ms:conformsTo rdf:resource="http://w3id.org/meta-share/meta-share/DDC_classification"/>
    </owl:NamedIndividual>
    


    <!-- http://w3id.org/meta-share/meta-share/DDC770 -->

    <owl:NamedIndividual rdf:about="http://w3id.org/meta-share/meta-share/DDC770">
        <rdf:type rdf:resource="http://w3id.org/meta-share/meta-share/DomainIdentifier"/>
    </owl:NamedIndividual>
    


    <!-- http://w3id.org/meta-share/meta-share/DDC780 -->

    <owl:NamedIndividual rdf:about="http://w3id.org/meta-share/meta-share/DDC780">
        <rdf:type rdf:resource="http://w3id.org/meta-share/meta-share/DomainIdentifier"/>
        <ms:conformsTo rdf:resource="http://w3id.org/meta-share/meta-share/DDC_classification"/>
    </owl:NamedIndividual>
    


    <!-- http://w3id.org/meta-share/meta-share/DDC790 -->

    <owl:NamedIndividual rdf:about="http://w3id.org/meta-share/meta-share/DDC790">
        <rdf:type rdf:resource="http://w3id.org/meta-share/meta-share/DomainIdentifier"/>
        <ms:conformsTo rdf:resource="http://w3id.org/meta-share/meta-share/DDC_classification"/>
    </owl:NamedIndividual>
    


    <!-- http://w3id.org/meta-share/meta-share/DDC800 -->

    <owl:NamedIndividual rdf:about="http://w3id.org/meta-share/meta-share/DDC800">
        <rdf:type rdf:resource="http://w3id.org/meta-share/meta-share/DomainIdentifier"/>
        <ms:conformsTo rdf:resource="http://w3id.org/meta-share/meta-share/DDC_classification"/>
    </owl:NamedIndividual>
    


    <!-- http://w3id.org/meta-share/meta-share/DDC900 -->

    <owl:NamedIndividual rdf:about="http://w3id.org/meta-share/meta-share/DDC900">
        <rdf:type rdf:resource="http://w3id.org/meta-share/meta-share/DomainIdentifier"/>
        <ms:conformsTo rdf:resource="http://w3id.org/meta-share/meta-share/DDC_classification"/>
    </owl:NamedIndividual>
    


    <!-- http://w3id.org/meta-share/meta-share/DDC910 -->

    <owl:NamedIndividual rdf:about="http://w3id.org/meta-share/meta-share/DDC910">
        <rdf:type rdf:resource="http://w3id.org/meta-share/meta-share/DomainIdentifier"/>
        <ms:conformsTo rdf:resource="http://w3id.org/meta-share/meta-share/DDC_classification"/>
    </owl:NamedIndividual>
    


    <!-- http://w3id.org/meta-share/meta-share/DDC_classification -->

    <owl:NamedIndividual rdf:about="http://w3id.org/meta-share/meta-share/DDC_classification">
        <rdf:type rdf:resource="http://w3id.org/meta-share/meta-share/DomainClassificationScheme"/>
        <ms:url>https://www.oclc.org/en/dewey/resources/summaries.html</ms:url>
        <rdfs:altLabel xml:lang="en">Dewey Decimal Classification</rdfs:altLabel>
        <rdfs:label xml:lang="en">DDC</rdfs:label>
    </owl:NamedIndividual>
    


    <!-- http://w3id.org/meta-share/meta-share/DK-5 -->

    <owl:NamedIndividual rdf:about="http://w3id.org/meta-share/meta-share/DK-5">
        <rdf:type rdf:resource="http://w3id.org/meta-share/meta-share/DomainClassificationScheme"/>
        <ms:url>http://metadata.dk/dk5-as-linked-data</ms:url>
        <rdfs:altLabel xml:lang="en">Danish Decimal Classification 5th edition</rdfs:altLabel>
        <rdfs:label xml:lang="en">DK-5</rdfs:label>
    </owl:NamedIndividual>
    


    <!-- http://w3id.org/meta-share/meta-share/DVB-C -->

    <owl:NamedIndividual rdf:about="http://w3id.org/meta-share/meta-share/DVB-C">
        <rdf:type rdf:resource="http://w3id.org/meta-share/meta-share/SourceChannelType"/>
        <rdfs:label xml:lang="en">DVB-C</rdfs:label>
    </owl:NamedIndividual>
    


    <!-- http://w3id.org/meta-share/meta-share/DVB-S -->

    <owl:NamedIndividual rdf:about="http://w3id.org/meta-share/meta-share/DVB-S">
        <rdf:type rdf:resource="http://w3id.org/meta-share/meta-share/SourceChannelType"/>
        <rdfs:label xml:lang="en">DVB-S</rdfs:label>
    </owl:NamedIndividual>
    


    <!-- http://w3id.org/meta-share/meta-share/DVB-T -->

    <owl:NamedIndividual rdf:about="http://w3id.org/meta-share/meta-share/DVB-T">
        <rdf:type rdf:resource="http://w3id.org/meta-share/meta-share/SourceChannelType"/>
        <rdfs:label xml:lang="en">DVB-T</rdfs:label>
    </owl:NamedIndividual>
    


    <!-- http://w3id.org/meta-share/meta-share/DVD-R -->

    <owl:NamedIndividual rdf:about="http://w3id.org/meta-share/meta-share/DVD-R">
        <rdf:type rdf:resource="http://w3id.org/meta-share/meta-share/DatasetDistributionForm"/>
        <rdfs:comment xml:lang="en">Value for data distribution medium, used for language resources delivered on a DVD-R</rdfs:comment>
        <rdfs:label xml:lang="en">DVD-R</rdfs:label>
    </owl:NamedIndividual>
    


    <!-- http://w3id.org/meta-share/meta-share/EAGLES -->

    <owl:NamedIndividual rdf:about="http://w3id.org/meta-share/meta-share/EAGLES">
        <rdf:type rdf:resource="http://w3id.org/meta-share/meta-share/StandardBestPractice"/>
        <ms:url>http://www.ilc.cnr.it/EAGLES/browse.html</ms:url>
        <rdfs:label xml:lang="en">EAGLES</rdfs:label>
    </owl:NamedIndividual>
    


    <!-- http://w3id.org/meta-share/meta-share/ELG-SHARE -->

    <owl:NamedIndividual rdf:about="http://w3id.org/meta-share/meta-share/ELG-SHARE">
        <rdf:type rdf:resource="http://w3id.org/meta-share/meta-share/StandardBestPractice"/>
        <rdfs:label xml:lang="en">ELG-SHARE</rdfs:label>
    </owl:NamedIndividual>
    


    <!-- http://w3id.org/meta-share/meta-share/ELG_Domain001 -->

    <owl:NamedIndividual rdf:about="http://w3id.org/meta-share/meta-share/ELG_Domain001">
        <rdf:type rdf:resource="http://w3id.org/meta-share/meta-share/DomainIdentifier"/>
        <ms:conformsTo rdf:resource="http://w3id.org/meta-share/meta-share/ELG_domainClassification"/>
    </owl:NamedIndividual>
    


    <!-- http://w3id.org/meta-share/meta-share/ELG_Domain002 -->

    <owl:NamedIndividual rdf:about="http://w3id.org/meta-share/meta-share/ELG_Domain002">
        <rdf:type rdf:resource="http://w3id.org/meta-share/meta-share/DomainIdentifier"/>
        <ms:conformsTo rdf:resource="http://w3id.org/meta-share/meta-share/ELG_domainClassification"/>
    </owl:NamedIndividual>
    


    <!-- http://w3id.org/meta-share/meta-share/ELG_Domain003 -->

    <owl:NamedIndividual rdf:about="http://w3id.org/meta-share/meta-share/ELG_Domain003">
        <rdf:type rdf:resource="http://w3id.org/meta-share/meta-share/DomainIdentifier"/>
        <ms:conformsTo rdf:resource="http://w3id.org/meta-share/meta-share/ELG_domainClassification"/>
    </owl:NamedIndividual>
    


    <!-- http://w3id.org/meta-share/meta-share/ELG_Domain004 -->

    <owl:NamedIndividual rdf:about="http://w3id.org/meta-share/meta-share/ELG_Domain004">
        <rdf:type rdf:resource="http://w3id.org/meta-share/meta-share/DomainIdentifier"/>
        <ms:conformsTo rdf:resource="http://w3id.org/meta-share/meta-share/ELG_domainClassification"/>
    </owl:NamedIndividual>
    


    <!-- http://w3id.org/meta-share/meta-share/ELG_Domain005 -->

    <owl:NamedIndividual rdf:about="http://w3id.org/meta-share/meta-share/ELG_Domain005">
        <rdf:type rdf:resource="http://w3id.org/meta-share/meta-share/DomainIdentifier"/>
        <ms:conformsTo rdf:resource="http://w3id.org/meta-share/meta-share/ELG_domainClassification"/>
    </owl:NamedIndividual>
    


    <!-- http://w3id.org/meta-share/meta-share/ELG_Domain006 -->

    <owl:NamedIndividual rdf:about="http://w3id.org/meta-share/meta-share/ELG_Domain006">
        <rdf:type rdf:resource="http://w3id.org/meta-share/meta-share/DomainIdentifier"/>
        <ms:conformsTo rdf:resource="http://w3id.org/meta-share/meta-share/ELG_domainClassification"/>
    </owl:NamedIndividual>
    


    <!-- http://w3id.org/meta-share/meta-share/ELG_Domain007 -->

    <owl:NamedIndividual rdf:about="http://w3id.org/meta-share/meta-share/ELG_Domain007">
        <rdf:type rdf:resource="http://w3id.org/meta-share/meta-share/DomainIdentifier"/>
        <ms:conformsTo rdf:resource="http://w3id.org/meta-share/meta-share/ELG_domainClassification"/>
    </owl:NamedIndividual>
    


    <!-- http://w3id.org/meta-share/meta-share/ELG_Domain008 -->

    <owl:NamedIndividual rdf:about="http://w3id.org/meta-share/meta-share/ELG_Domain008">
        <rdf:type rdf:resource="http://w3id.org/meta-share/meta-share/DomainIdentifier"/>
        <ms:conformsTo rdf:resource="http://w3id.org/meta-share/meta-share/ELG_domainClassification"/>
    </owl:NamedIndividual>
    


    <!-- http://w3id.org/meta-share/meta-share/ELG_Domain009 -->

    <owl:NamedIndividual rdf:about="http://w3id.org/meta-share/meta-share/ELG_Domain009">
        <rdf:type rdf:resource="http://w3id.org/meta-share/meta-share/DomainIdentifier"/>
        <ms:conformsTo rdf:resource="http://w3id.org/meta-share/meta-share/ELG_domainClassification"/>
    </owl:NamedIndividual>
    


    <!-- http://w3id.org/meta-share/meta-share/ELG_Domain010 -->

    <owl:NamedIndividual rdf:about="http://w3id.org/meta-share/meta-share/ELG_Domain010">
        <rdf:type rdf:resource="http://w3id.org/meta-share/meta-share/DomainIdentifier"/>
        <ms:conformsTo rdf:resource="http://w3id.org/meta-share/meta-share/ELG_domainClassification"/>
    </owl:NamedIndividual>
    


    <!-- http://w3id.org/meta-share/meta-share/ELG_Domain011 -->

    <owl:NamedIndividual rdf:about="http://w3id.org/meta-share/meta-share/ELG_Domain011">
        <rdf:type rdf:resource="http://w3id.org/meta-share/meta-share/DomainIdentifier"/>
        <ms:conformsTo rdf:resource="http://w3id.org/meta-share/meta-share/ELG_domainClassification"/>
    </owl:NamedIndividual>
    


    <!-- http://w3id.org/meta-share/meta-share/ELG_Domain012 -->

    <owl:NamedIndividual rdf:about="http://w3id.org/meta-share/meta-share/ELG_Domain012">
        <rdf:type rdf:resource="http://w3id.org/meta-share/meta-share/DomainIdentifier"/>
        <ms:conformsTo rdf:resource="http://w3id.org/meta-share/meta-share/ELG_domainClassification"/>
    </owl:NamedIndividual>
    


    <!-- http://w3id.org/meta-share/meta-share/ELG_Domain013 -->

    <owl:NamedIndividual rdf:about="http://w3id.org/meta-share/meta-share/ELG_Domain013">
        <rdf:type rdf:resource="http://w3id.org/meta-share/meta-share/DomainIdentifier"/>
        <ms:conformsTo rdf:resource="http://w3id.org/meta-share/meta-share/ELG_domainClassification"/>
    </owl:NamedIndividual>
    


    <!-- http://w3id.org/meta-share/meta-share/ELG_Domain014 -->

    <owl:NamedIndividual rdf:about="http://w3id.org/meta-share/meta-share/ELG_Domain014">
        <rdf:type rdf:resource="http://w3id.org/meta-share/meta-share/DomainIdentifier"/>
        <ms:conformsTo rdf:resource="http://w3id.org/meta-share/meta-share/ELG_domainClassification"/>
    </owl:NamedIndividual>
    


    <!-- http://w3id.org/meta-share/meta-share/ELG_Domain015 -->

    <owl:NamedIndividual rdf:about="http://w3id.org/meta-share/meta-share/ELG_Domain015">
        <rdf:type rdf:resource="http://w3id.org/meta-share/meta-share/DomainIdentifier"/>
        <ms:conformsTo rdf:resource="http://w3id.org/meta-share/meta-share/ELG_domainClassification"/>
    </owl:NamedIndividual>
    


    <!-- http://w3id.org/meta-share/meta-share/ELG_Domain016 -->

    <owl:NamedIndividual rdf:about="http://w3id.org/meta-share/meta-share/ELG_Domain016">
        <rdf:type rdf:resource="http://w3id.org/meta-share/meta-share/DomainIdentifier"/>
        <ms:conformsTo rdf:resource="http://w3id.org/meta-share/meta-share/ELG_domainClassification"/>
    </owl:NamedIndividual>
    


    <!-- http://w3id.org/meta-share/meta-share/ELG_Domain017 -->

    <owl:NamedIndividual rdf:about="http://w3id.org/meta-share/meta-share/ELG_Domain017">
        <rdf:type rdf:resource="http://w3id.org/meta-share/meta-share/DomainIdentifier"/>
        <ms:conformsTo rdf:resource="http://w3id.org/meta-share/meta-share/ELG_domainClassification"/>
    </owl:NamedIndividual>
    


    <!-- http://w3id.org/meta-share/meta-share/ELG_Domain018 -->

    <owl:NamedIndividual rdf:about="http://w3id.org/meta-share/meta-share/ELG_Domain018">
        <rdf:type rdf:resource="http://w3id.org/meta-share/meta-share/DomainIdentifier"/>
        <ms:conformsTo rdf:resource="http://w3id.org/meta-share/meta-share/ELG_domainClassification"/>
    </owl:NamedIndividual>
    


    <!-- http://w3id.org/meta-share/meta-share/ELG_domainClassification -->

    <owl:NamedIndividual rdf:about="http://w3id.org/meta-share/meta-share/ELG_domainClassification">
        <rdf:type rdf:resource="http://w3id.org/meta-share/meta-share/DomainClassificationScheme"/>
        <rdfs:label xml:lang="en">ELG domain classification</rdfs:label>
    </owl:NamedIndividual>
    


    <!-- http://w3id.org/meta-share/meta-share/ELRA -->

    <owl:NamedIndividual rdf:about="http://w3id.org/meta-share/meta-share/ELRA">
        <rdf:type rdf:resource="http://w3id.org/meta-share/meta-share/MembershipInstitution"/>
        <rdfs:comment xml:lang="en">European Language Resources Association (www.elra.eu)</rdfs:comment>
        <rdfs:label xml:lang="en">ELRA</rdfs:label>
    </owl:NamedIndividual>
    


    <!-- http://w3id.org/meta-share/meta-share/EMA -->

    <owl:NamedIndividual rdf:about="http://w3id.org/meta-share/meta-share/EMA">
        <rdf:type rdf:resource="http://w3id.org/meta-share/meta-share/SourceChannel"/>
        <rdfs:label xml:lang="en">EMA</rdfs:label>
    </owl:NamedIndividual>
    


    <!-- http://w3id.org/meta-share/meta-share/EML -->

    <owl:NamedIndividual rdf:about="http://w3id.org/meta-share/meta-share/EML">
        <rdf:type rdf:resource="http://w3id.org/meta-share/meta-share/StandardBestPractice"/>
        <ms:url>https://www.w3.org/TR/2009/WD-emotionml-20091029/</ms:url>
        <rdfs:altLabel xml:lang="en">EML</rdfs:altLabel>
        <rdfs:altLabel xml:lang="en">Emotion Markup Language</rdfs:altLabel>
        <rdfs:label xml:lang="en">EmotionML</rdfs:label>
    </owl:NamedIndividual>
    


    <!-- http://w3id.org/meta-share/meta-share/EMMA -->

    <owl:NamedIndividual rdf:about="http://w3id.org/meta-share/meta-share/EMMA">
        <rdf:type rdf:resource="http://w3id.org/meta-share/meta-share/StandardBestPractice"/>
        <ms:url>https://www.w3.org/TR/emma/</ms:url>
        <rdfs:altLabel xml:lang="en">Extensible MultiModal Annotation markup language</rdfs:altLabel>
        <rdfs:label xml:lang="en">EMMA</rdfs:label>
    </owl:NamedIndividual>
    


    <!-- http://w3id.org/meta-share/meta-share/EUC-JP -->

    <owl:NamedIndividual rdf:about="http://w3id.org/meta-share/meta-share/EUC-JP">
        <rdf:type rdf:resource="http://w3id.org/meta-share/meta-share/CharacterEncoding"/>
        <rdfs:label xml:lang="en">EUC-JP</rdfs:label>
    </owl:NamedIndividual>
    


    <!-- http://w3id.org/meta-share/meta-share/EUC-KR -->

    <owl:NamedIndividual rdf:about="http://w3id.org/meta-share/meta-share/EUC-KR">
        <rdf:type rdf:resource="http://w3id.org/meta-share/meta-share/CharacterEncoding"/>
        <rdfs:label xml:lang="en">EUC-KR</rdfs:label>
    </owl:NamedIndividual>
    


    <!-- http://w3id.org/meta-share/meta-share/EUROVOC -->

    <owl:NamedIndividual rdf:about="http://w3id.org/meta-share/meta-share/EUROVOC">
        <rdf:type rdf:resource="http://w3id.org/meta-share/meta-share/DomainClassificationScheme"/>
        <ms:url>https://eur-lex.europa.eu/browse/eurovoc.html</ms:url>
        <rdfs:label xml:lang="en">EUROVOC</rdfs:label>
    </owl:NamedIndividual>
    


    <!-- http://w3id.org/meta-share/meta-share/GATE -->

    <owl:NamedIndividual rdf:about="http://w3id.org/meta-share/meta-share/GATE">
        <rdf:type rdf:resource="http://w3id.org/meta-share/meta-share/Framework"/>
        <rdfs:label xml:lang="en">GATE</rdfs:label>
    </owl:NamedIndividual>
    


    <!-- http://w3id.org/meta-share/meta-share/GB18030 -->

    <owl:NamedIndividual rdf:about="http://w3id.org/meta-share/meta-share/GB18030">
        <rdf:type rdf:resource="http://w3id.org/meta-share/meta-share/CharacterEncoding"/>
        <rdfs:label xml:lang="en">GB18030</rdfs:label>
    </owl:NamedIndividual>
    


    <!-- http://w3id.org/meta-share/meta-share/GBK -->

    <owl:NamedIndividual rdf:about="http://w3id.org/meta-share/meta-share/GBK">
        <rdf:type rdf:resource="http://w3id.org/meta-share/meta-share/CharacterEncoding"/>
        <rdfs:label xml:lang="en">GBK</rdfs:label>
    </owl:NamedIndividual>
    


    <!-- http://w3id.org/meta-share/meta-share/GMX -->

    <owl:NamedIndividual rdf:about="http://w3id.org/meta-share/meta-share/GMX">
        <rdf:type rdf:resource="http://w3id.org/meta-share/meta-share/StandardBestPractice"/>
        <ms:url>https://xtm.cloud/manuals/gmx-v/GMX-V-2.0.html</ms:url>
        <rdfs:altLabel xml:lang="en">Global information management Metrics eXchange</rdfs:altLabel>
        <rdfs:label xml:lang="en">GMX</rdfs:label>
    </owl:NamedIndividual>
    


    <!-- http://w3id.org/meta-share/meta-share/GSM -->

    <owl:NamedIndividual rdf:about="http://w3id.org/meta-share/meta-share/GSM">
        <rdf:type rdf:resource="http://w3id.org/meta-share/meta-share/SourceChannelType"/>
        <rdfs:label xml:lang="en">GSM</rdfs:label>
    </owl:NamedIndividual>
    


    <!-- http://w3id.org/meta-share/meta-share/Galaxy -->

    <owl:NamedIndividual rdf:about="http://w3id.org/meta-share/meta-share/Galaxy">
        <rdf:type rdf:resource="http://w3id.org/meta-share/meta-share/Framework"/>
        <rdfs:label xml:lang="en">Galaxy</rdfs:label>
    </owl:NamedIndividual>
    


    <!-- http://w3id.org/meta-share/meta-share/GrAF -->

    <owl:NamedIndividual rdf:about="http://w3id.org/meta-share/meta-share/GrAF">
        <rdf:type rdf:resource="http://w3id.org/meta-share/meta-share/StandardBestPractice"/>
        <ms:url>http://www.xces.org/ns/GrAF/1.0/</ms:url>
        <rdfs:altLabel xml:lang="en">Graph Annotation Framework</rdfs:altLabel>
        <rdfs:label xml:lang="en">GrAF</rdfs:label>
    </owl:NamedIndividual>
    


    <!-- http://w3id.org/meta-share/meta-share/HD.1080 -->

    <owl:NamedIndividual rdf:about="http://w3id.org/meta-share/meta-share/HD.1080">
        <rdf:type rdf:resource="http://w3id.org/meta-share/meta-share/ResolutionStandard"/>
        <rdfs:label xml:lang="en">HD.1080</rdfs:label>
    </owl:NamedIndividual>
    


    <!-- http://w3id.org/meta-share/meta-share/HD.720 -->

    <owl:NamedIndividual rdf:about="http://w3id.org/meta-share/meta-share/HD.720">
        <rdf:type rdf:resource="http://w3id.org/meta-share/meta-share/ResolutionStandard"/>
        <rdfs:label xml:lang="en">HD.720</rdfs:label>
    </owl:NamedIndividual>
    


    <!-- http://w3id.org/meta-share/meta-share/HamNoSys -->

    <owl:NamedIndividual rdf:about="http://w3id.org/meta-share/meta-share/HamNoSys">
        <rdf:type rdf:resource="http://w3id.org/meta-share/meta-share/StandardBestPractice"/>
        <ms:url>https://www.sign-lang.uni-hamburg.de/dgs-korpus/index.php/hamnosys-97.html</ms:url>
        <rdfs:altLabel xml:lang="en">Hamburg Sign Language Notation System</rdfs:altLabel>
        <rdfs:label xml:lang="en">HamNoSys</rdfs:label>
    </owl:NamedIndividual>
    


    <!-- http://w3id.org/meta-share/meta-share/ISCII91 -->

    <owl:NamedIndividual rdf:about="http://w3id.org/meta-share/meta-share/ISCII91">
        <rdf:type rdf:resource="http://w3id.org/meta-share/meta-share/CharacterEncoding"/>
        <rdfs:label xml:lang="en">ISCII91</rdfs:label>
    </owl:NamedIndividual>
    


    <!-- http://w3id.org/meta-share/meta-share/ISDN -->

    <owl:NamedIndividual rdf:about="http://w3id.org/meta-share/meta-share/ISDN">
        <rdf:type rdf:resource="http://w3id.org/meta-share/meta-share/SourceChannelType"/>
        <rdfs:label xml:lang="en">ISDN</rdfs:label>
    </owl:NamedIndividual>
    


    <!-- http://w3id.org/meta-share/meta-share/ISO-2022-JP -->

    <owl:NamedIndividual rdf:about="http://w3id.org/meta-share/meta-share/ISO-2022-JP">
        <rdf:type rdf:resource="http://w3id.org/meta-share/meta-share/CharacterEncoding"/>
        <rdfs:label xml:lang="en">ISO-2022-JP</rdfs:label>
    </owl:NamedIndividual>
    


    <!-- http://w3id.org/meta-share/meta-share/ISO-2022-KR -->

    <owl:NamedIndividual rdf:about="http://w3id.org/meta-share/meta-share/ISO-2022-KR">
        <rdf:type rdf:resource="http://w3id.org/meta-share/meta-share/CharacterEncoding"/>
        <rdfs:label xml:lang="en">ISO-2022-KR</rdfs:label>
    </owl:NamedIndividual>
    


    <!-- http://w3id.org/meta-share/meta-share/ISO-8859-1 -->

    <owl:NamedIndividual rdf:about="http://w3id.org/meta-share/meta-share/ISO-8859-1">
        <rdf:type rdf:resource="http://w3id.org/meta-share/meta-share/CharacterEncoding"/>
        <rdfs:label xml:lang="en">ISO-8859-1</rdfs:label>
    </owl:NamedIndividual>
    


    <!-- http://w3id.org/meta-share/meta-share/ISO-8859-15 -->

    <owl:NamedIndividual rdf:about="http://w3id.org/meta-share/meta-share/ISO-8859-15">
        <rdf:type rdf:resource="http://w3id.org/meta-share/meta-share/CharacterEncoding"/>
        <rdfs:label xml:lang="en">ISO-8859-15</rdfs:label>
    </owl:NamedIndividual>
    


    <!-- http://w3id.org/meta-share/meta-share/ISO-8859-2 -->

    <owl:NamedIndividual rdf:about="http://w3id.org/meta-share/meta-share/ISO-8859-2">
        <rdf:type rdf:resource="http://w3id.org/meta-share/meta-share/CharacterEncoding"/>
        <rdfs:label xml:lang="en">ISO-8859-2</rdfs:label>
    </owl:NamedIndividual>
    


    <!-- http://w3id.org/meta-share/meta-share/ISO-8859-3 -->

    <owl:NamedIndividual rdf:about="http://w3id.org/meta-share/meta-share/ISO-8859-3">
        <rdf:type rdf:resource="http://w3id.org/meta-share/meta-share/CharacterEncoding"/>
        <rdfs:label xml:lang="en">ISO-8859-3</rdfs:label>
    </owl:NamedIndividual>
    


    <!-- http://w3id.org/meta-share/meta-share/ISO-8859-4 -->

    <owl:NamedIndividual rdf:about="http://w3id.org/meta-share/meta-share/ISO-8859-4">
        <rdf:type rdf:resource="http://w3id.org/meta-share/meta-share/CharacterEncoding"/>
        <rdfs:label xml:lang="en">ISO-8859-4</rdfs:label>
    </owl:NamedIndividual>
    


    <!-- http://w3id.org/meta-share/meta-share/ISO-8859-5 -->

    <owl:NamedIndividual rdf:about="http://w3id.org/meta-share/meta-share/ISO-8859-5">
        <rdf:type rdf:resource="http://w3id.org/meta-share/meta-share/CharacterEncoding"/>
        <rdfs:label xml:lang="en">ISO-8859-5</rdfs:label>
    </owl:NamedIndividual>
    


    <!-- http://w3id.org/meta-share/meta-share/ISO-8859-6 -->

    <owl:NamedIndividual rdf:about="http://w3id.org/meta-share/meta-share/ISO-8859-6">
        <rdf:type rdf:resource="http://w3id.org/meta-share/meta-share/CharacterEncoding"/>
        <rdfs:label xml:lang="en">ISO-8859-6</rdfs:label>
    </owl:NamedIndividual>
    


    <!-- http://w3id.org/meta-share/meta-share/ISO-8859-7 -->

    <owl:NamedIndividual rdf:about="http://w3id.org/meta-share/meta-share/ISO-8859-7">
        <rdf:type rdf:resource="http://w3id.org/meta-share/meta-share/CharacterEncoding"/>
        <rdfs:label xml:lang="en">ISO-8859-7</rdfs:label>
    </owl:NamedIndividual>
    


    <!-- http://w3id.org/meta-share/meta-share/ISO-8859-8 -->

    <owl:NamedIndividual rdf:about="http://w3id.org/meta-share/meta-share/ISO-8859-8">
        <rdf:type rdf:resource="http://w3id.org/meta-share/meta-share/CharacterEncoding"/>
        <rdfs:label xml:lang="en">ISO-8859-8</rdfs:label>
    </owl:NamedIndividual>
    


    <!-- http://w3id.org/meta-share/meta-share/ISO-8859-9 -->

    <owl:NamedIndividual rdf:about="http://w3id.org/meta-share/meta-share/ISO-8859-9">
        <rdf:type rdf:resource="http://w3id.org/meta-share/meta-share/CharacterEncoding"/>
        <rdfs:label xml:lang="en">ISO-8859-9</rdfs:label>
    </owl:NamedIndividual>
    


    <!-- http://w3id.org/meta-share/meta-share/ISO-8860-13 -->

    <owl:NamedIndividual rdf:about="http://w3id.org/meta-share/meta-share/ISO-8860-13">
        <rdf:type rdf:resource="http://w3id.org/meta-share/meta-share/CharacterEncoding"/>
        <rdfs:label xml:lang="en">ISO-8860-13</rdfs:label>
    </owl:NamedIndividual>
    


    <!-- http://w3id.org/meta-share/meta-share/ISO12620 -->

    <owl:NamedIndividual rdf:about="http://w3id.org/meta-share/meta-share/ISO12620">
        <rdf:type rdf:resource="http://w3id.org/meta-share/meta-share/StandardBestPractice"/>
        <ms:url>http://www.datcatinfo.net/#/</ms:url>
        <ms:url>http://www.iso.org/sites/dcr-redirect/dcr.html</ms:url>
        <rdfs:altLabel xml:lang="en">DCR</rdfs:altLabel>
        <rdfs:altLabel xml:lang="en">Data Category Repository</rdfs:altLabel>
        <rdfs:label xml:lang="en">ISO12620</rdfs:label>
    </owl:NamedIndividual>
    


    <!-- http://w3id.org/meta-share/meta-share/ISO16642 -->

    <owl:NamedIndividual rdf:about="http://w3id.org/meta-share/meta-share/ISO16642">
        <rdf:type rdf:resource="http://w3id.org/meta-share/meta-share/StandardBestPractice"/>
        <ms:url>http://xml.coverpages.org/ISO16642-200207.pdf</ms:url>
        <rdfs:altLabel xml:lang="en">TMF</rdfs:altLabel>
        <rdfs:altLabel xml:lang="en">Terminological Markup Framework</rdfs:altLabel>
        <rdfs:label xml:lang="en">ISO16642</rdfs:label>
    </owl:NamedIndividual>
    


    <!-- http://w3id.org/meta-share/meta-share/ISO1987 -->

    <owl:NamedIndividual rdf:about="http://w3id.org/meta-share/meta-share/ISO1987">
        <rdf:type rdf:resource="http://w3id.org/meta-share/meta-share/StandardBestPractice"/>
        <rdfs:label xml:lang="en">ISO 9001:1987</rdfs:label>
        <skos:comment xml:lang="en">Quality systems -- Model for quality assurance in design/development, production, installation and servicing</skos:comment>
    </owl:NamedIndividual>
    


    <!-- http://w3id.org/meta-share/meta-share/ISO2022_CN_CNS -->

    <owl:NamedIndividual rdf:about="http://w3id.org/meta-share/meta-share/ISO2022_CN_CNS">
        <rdf:type rdf:resource="http://w3id.org/meta-share/meta-share/CharacterEncoding"/>
        <rdfs:label xml:lang="en">ISO2022_CN_CNS</rdfs:label>
    </owl:NamedIndividual>
    


    <!-- http://w3id.org/meta-share/meta-share/ISO2022_CN_GB -->

    <owl:NamedIndividual rdf:about="http://w3id.org/meta-share/meta-share/ISO2022_CN_GB">
        <rdf:type rdf:resource="http://w3id.org/meta-share/meta-share/CharacterEncoding"/>
        <rdfs:label xml:lang="en">ISO2022_CN_GB</rdfs:label>
    </owl:NamedIndividual>
    


    <!-- http://w3id.org/meta-share/meta-share/ISO26162 -->

    <owl:NamedIndividual rdf:about="http://w3id.org/meta-share/meta-share/ISO26162">
        <rdf:type rdf:resource="http://w3id.org/meta-share/meta-share/StandardBestPractice"/>
        <ms:url>https://www.iso.org/standard/43427.html</ms:url>
        <rdfs:altLabel xml:lang="en">Systems to manage terminology, knowledge and content</rdfs:altLabel>
        <rdfs:label xml:lang="en">ISO 26162</rdfs:label>
    </owl:NamedIndividual>
    


    <!-- http://w3id.org/meta-share/meta-share/ISO30042 -->

    <owl:NamedIndividual rdf:about="http://w3id.org/meta-share/meta-share/ISO30042">
        <rdf:type rdf:resource="http://w3id.org/meta-share/meta-share/StandardBestPractice"/>
        <ms:url>https://www.iso.org/standard/45797.html</ms:url>
        <rdfs:altLabel xml:lang="en">TBX</rdfs:altLabel>
        <rdfs:altLabel xml:lang="en">TermBase eXchange</rdfs:altLabel>
        <rdfs:label xml:lang="en">ISO 30042</rdfs:label>
    </owl:NamedIndividual>
    


    <!-- http://w3id.org/meta-share/meta-share/ISO704 -->

    <owl:NamedIndividual rdf:about="http://w3id.org/meta-share/meta-share/ISO704">
        <rdf:type rdf:resource="http://w3id.org/meta-share/meta-share/StandardBestPractice"/>
        <ms:url>https://www.iso.org/standard/38109.html</ms:url>
        <rdfs:altLabel xml:lang="en">Terminology work</rdfs:altLabel>
        <rdfs:label xml:lang="en">ISO704</rdfs:label>
    </owl:NamedIndividual>
    


    <!-- http://w3id.org/meta-share/meta-share/InkML -->

    <owl:NamedIndividual rdf:about="http://w3id.org/meta-share/meta-share/InkML">
        <rdf:type rdf:resource="http://w3id.org/meta-share/meta-share/StandardBestPractice"/>
        <ms:url>https://www.w3.org/TR/InkML/</ms:url>
        <rdfs:altLabel xml:lang="en">Ink Markup Language</rdfs:altLabel>
        <rdfs:label xml:lang="en">Ink ML</rdfs:label>
    </owl:NamedIndividual>
    


    <!-- http://w3id.org/meta-share/meta-share/JISAutoDetect -->

    <owl:NamedIndividual rdf:about="http://w3id.org/meta-share/meta-share/JISAutoDetect">
        <rdf:type rdf:resource="http://w3id.org/meta-share/meta-share/CharacterEncoding"/>
        <rdfs:label xml:lang="en">JISAutoDetect</rdfs:label>
    </owl:NamedIndividual>
    


    <!-- http://w3id.org/meta-share/meta-share/KOI8-R -->

    <owl:NamedIndividual rdf:about="http://w3id.org/meta-share/meta-share/KOI8-R">
        <rdf:type rdf:resource="http://w3id.org/meta-share/meta-share/CharacterEncoding"/>
        <rdfs:label xml:lang="en">KOI8-R</rdfs:label>
    </owl:NamedIndividual>
    


    <!-- http://w3id.org/meta-share/meta-share/LAF -->

    <owl:NamedIndividual rdf:about="http://w3id.org/meta-share/meta-share/LAF">
        <rdf:type rdf:resource="http://w3id.org/meta-share/meta-share/StandardBestPractice"/>
        <ms:url>https://www.iso.org/standard/37326.html</ms:url>
        <rdfs:altLabel xml:lang="en">ISO 24612</rdfs:altLabel>
        <rdfs:altLabel xml:lang="en">Linguistic Annotation Framework</rdfs:altLabel>
        <rdfs:label xml:lang="en">LAF</rdfs:label>
    </owl:NamedIndividual>
    


    <!-- http://w3id.org/meta-share/meta-share/LDC -->

    <owl:NamedIndividual rdf:about="http://w3id.org/meta-share/meta-share/LDC">
        <rdf:type rdf:resource="http://w3id.org/meta-share/meta-share/MembershipInstitution"/>
        <rdfs:comment xml:lang="en">Linguistic Data Consortium</rdfs:comment>
        <rdfs:label xml:lang="en">LDC</rdfs:label>
    </owl:NamedIndividual>
    


    <!-- http://w3id.org/meta-share/meta-share/LMF -->

    <owl:NamedIndividual rdf:about="http://w3id.org/meta-share/meta-share/LMF">
        <rdf:type rdf:resource="http://w3id.org/meta-share/meta-share/StandardBestPractice"/>
        <ms:url>http://www.lexicalmarkupframework.org/</ms:url>
        <rdfs:altLabel xml:lang="en">Lexical Markup Framework</rdfs:altLabel>
        <rdfs:label xml:lang="en">LMF</rdfs:label>
    </owl:NamedIndividual>
    


    <!-- http://w3id.org/meta-share/meta-share/LTIntegrator -->

    <owl:NamedIndividual rdf:about="http://w3id.org/meta-share/meta-share/LTIntegrator">
        <rdf:type rdf:resource="http://w3id.org/meta-share/meta-share/OrganizationRole"/>
        <rdfs:altLabel xml:lang="en">Language Technology integrator</rdfs:altLabel>
        <rdfs:label xml:lang="en">LT integrator</rdfs:label>
    </owl:NamedIndividual>
    


    <!-- http://w3id.org/meta-share/meta-share/LTSupplier -->

    <owl:NamedIndividual rdf:about="http://w3id.org/meta-share/meta-share/LTSupplier">
        <rdf:type rdf:resource="http://w3id.org/meta-share/meta-share/OrganizationRole"/>
        <rdfs:altLabel xml:lang="en">Language Technology supplier</rdfs:altLabel>
        <rdfs:label xml:lang="en">LT supplier</rdfs:label>
    </owl:NamedIndividual>
    


    <!-- http://w3id.org/meta-share/meta-share/LTUser -->

    <owl:NamedIndividual rdf:about="http://w3id.org/meta-share/meta-share/LTUser">
        <rdf:type rdf:resource="http://w3id.org/meta-share/meta-share/OrganizationRole"/>
        <rdfs:altLabel xml:lang="en">Language Technology user</rdfs:altLabel>
        <rdfs:label xml:lang="en">LT user</rdfs:label>
    </owl:NamedIndividual>
    


    <!-- http://w3id.org/meta-share/meta-share/LanguageTechnology -->

    <owl:NamedIndividual rdf:about="http://w3id.org/meta-share/meta-share/LanguageTechnology">
        <rdf:type rdf:resource="http://w3id.org/meta-share/meta-share/Domain"/>
        <rdfs:altLabel xml:lang="en">HLT</rdfs:altLabel>
        <rdfs:altLabel xml:lang="en">Human Language Technology</rdfs:altLabel>
        <rdfs:altLabel xml:lang="en">LT</rdfs:altLabel>
        <rdfs:comment xml:lang="en">Language technology, often called human language technology, studies methods of how computer programs or electronic devices can analyze, produce, modify or respond to human texts and speech. It consists of natural language processing and computational linguistics on the one hand, and speech technology on the other. [Wikipedia]</rdfs:comment>
        <rdfs:label xml:lang="en">Language Technology</rdfs:label>
    </owl:NamedIndividual>
    


    <!-- http://w3id.org/meta-share/meta-share/MAD -->

    <owl:NamedIndividual rdf:about="http://w3id.org/meta-share/meta-share/MAD">
        <rdf:type rdf:resource="http://w3id.org/meta-share/meta-share/Metric"/>
        <rdfs:altLabel xml:lang="en">Mean Annotations per Document</rdfs:altLabel>
        <rdfs:label xml:lang="en">MAD</rdfs:label>
    </owl:NamedIndividual>
    


    <!-- http://w3id.org/meta-share/meta-share/MAF -->

    <owl:NamedIndividual rdf:about="http://w3id.org/meta-share/meta-share/MAF">
        <rdf:type rdf:resource="http://w3id.org/meta-share/meta-share/StandardBestPractice"/>
        <ms:url>https://www.iso.org/standard/51934.html</ms:url>
        <rdfs:altLabel xml:lang="en">ISO 24611</rdfs:altLabel>
        <rdfs:altLabel xml:lang="en">Morpho-syntactic Annotation Framework</rdfs:altLabel>
        <rdfs:label xml:lang="en">MAF</rdfs:label>
    </owl:NamedIndividual>
    


    <!-- http://w3id.org/meta-share/meta-share/MDTV -->

    <owl:NamedIndividual rdf:about="http://w3id.org/meta-share/meta-share/MDTV">
        <rdf:type rdf:resource="http://w3id.org/meta-share/meta-share/Metric"/>
        <rdfs:altLabel xml:lang="en">Mean Time per Document Volume</rdfs:altLabel>
        <rdfs:label xml:lang="en">MDTV</rdfs:label>
    </owl:NamedIndividual>
    


    <!-- http://w3id.org/meta-share/meta-share/MLIF -->

    <owl:NamedIndividual rdf:about="http://w3id.org/meta-share/meta-share/MLIF">
        <rdf:type rdf:resource="http://w3id.org/meta-share/meta-share/StandardBestPractice"/>
        <ms:url>https://www.iso.org/standard/37330.html</ms:url>
        <rdfs:altLabel xml:lang="en">ISO 24616</rdfs:altLabel>
        <rdfs:altLabel xml:lang="en">Multilingual Information Framework</rdfs:altLabel>
        <rdfs:label xml:lang="en">MLIF</rdfs:label>
    </owl:NamedIndividual>
    


    <!-- http://w3id.org/meta-share/meta-share/MMI -->

    <owl:NamedIndividual rdf:about="http://w3id.org/meta-share/meta-share/MMI">
        <rdf:type rdf:resource="http://w3id.org/meta-share/meta-share/StandardBestPractice"/>
        <ms:url>https://www.w3.org/TR/mmi-framework/</ms:url>
        <rdfs:altLabel xml:lang="en">Multi-Modal Interaction framework</rdfs:altLabel>
        <rdfs:label xml:lang="en">MMI</rdfs:label>
    </owl:NamedIndividual>
    


    <!-- http://w3id.org/meta-share/meta-share/MS874 -->

    <owl:NamedIndividual rdf:about="http://w3id.org/meta-share/meta-share/MS874">
        <rdf:type rdf:resource="http://w3id.org/meta-share/meta-share/CharacterEncoding"/>
        <rdfs:label xml:lang="en">MS874</rdfs:label>
    </owl:NamedIndividual>
    


    <!-- http://w3id.org/meta-share/meta-share/MS_AG001 -->

    <owl:NamedIndividual rdf:about="http://w3id.org/meta-share/meta-share/MS_AG001">
        <rdf:type rdf:resource="http://w3id.org/meta-share/meta-share/AudioGenreIdentifier"/>
        <ms:conformsTo rdf:resource="http://w3id.org/meta-share/meta-share/MS_audioGenreClassification"/>
    </owl:NamedIndividual>
    


    <!-- http://w3id.org/meta-share/meta-share/MS_AG002 -->

    <owl:NamedIndividual rdf:about="http://w3id.org/meta-share/meta-share/MS_AG002">
        <rdf:type rdf:resource="http://w3id.org/meta-share/meta-share/AudioGenreIdentifier"/>
        <ms:conformsTo rdf:resource="http://w3id.org/meta-share/meta-share/MS_audioGenreClassification"/>
    </owl:NamedIndividual>
    


    <!-- http://w3id.org/meta-share/meta-share/MS_AG003 -->

    <owl:NamedIndividual rdf:about="http://w3id.org/meta-share/meta-share/MS_AG003">
        <rdf:type rdf:resource="http://w3id.org/meta-share/meta-share/AudioGenreIdentifier"/>
        <ms:conformsTo rdf:resource="http://w3id.org/meta-share/meta-share/MS_audioGenreClassification"/>
    </owl:NamedIndividual>
    


    <!-- http://w3id.org/meta-share/meta-share/MS_AG004 -->

    <owl:NamedIndividual rdf:about="http://w3id.org/meta-share/meta-share/MS_AG004">
        <rdf:type rdf:resource="http://w3id.org/meta-share/meta-share/AudioGenreIdentifier"/>
        <ms:conformsTo rdf:resource="http://w3id.org/meta-share/meta-share/MS_audioGenreClassification"/>
    </owl:NamedIndividual>
    


    <!-- http://w3id.org/meta-share/meta-share/MS_AG005 -->

    <owl:NamedIndividual rdf:about="http://w3id.org/meta-share/meta-share/MS_AG005">
        <rdf:type rdf:resource="http://w3id.org/meta-share/meta-share/AudioGenreIdentifier"/>
        <ms:conformsTo rdf:resource="http://w3id.org/meta-share/meta-share/MS_audioGenreClassification"/>
    </owl:NamedIndividual>
    


    <!-- http://w3id.org/meta-share/meta-share/MS_AG006 -->

    <owl:NamedIndividual rdf:about="http://w3id.org/meta-share/meta-share/MS_AG006">
        <rdf:type rdf:resource="http://w3id.org/meta-share/meta-share/AudioGenreIdentifier"/>
        <ms:conformsTo rdf:resource="http://w3id.org/meta-share/meta-share/MS_audioGenreClassification"/>
    </owl:NamedIndividual>
    


    <!-- http://w3id.org/meta-share/meta-share/MS_SG001 -->

    <owl:NamedIndividual rdf:about="http://w3id.org/meta-share/meta-share/MS_SG001">
        <rdf:type rdf:resource="http://w3id.org/meta-share/meta-share/SpeechGenreIdentifier"/>
        <ms:conformsTo rdf:resource="http://w3id.org/meta-share/meta-share/MS_SpeechGenreClassification"/>
    </owl:NamedIndividual>
    


    <!-- http://w3id.org/meta-share/meta-share/MS_SG002 -->

    <owl:NamedIndividual rdf:about="http://w3id.org/meta-share/meta-share/MS_SG002">
        <rdf:type rdf:resource="http://w3id.org/meta-share/meta-share/SpeechGenreIdentifier"/>
        <ms:conformsTo rdf:resource="http://w3id.org/meta-share/meta-share/MS_SpeechGenreClassification"/>
    </owl:NamedIndividual>
    


    <!-- http://w3id.org/meta-share/meta-share/MS_SG003 -->

    <owl:NamedIndividual rdf:about="http://w3id.org/meta-share/meta-share/MS_SG003">
        <rdf:type rdf:resource="http://w3id.org/meta-share/meta-share/SpeechGenreIdentifier"/>
        <ms:conformsTo rdf:resource="http://w3id.org/meta-share/meta-share/MS_SpeechGenreClassification"/>
    </owl:NamedIndividual>
    


    <!-- http://w3id.org/meta-share/meta-share/MS_SG004 -->

    <owl:NamedIndividual rdf:about="http://w3id.org/meta-share/meta-share/MS_SG004">
        <rdf:type rdf:resource="http://w3id.org/meta-share/meta-share/SpeechGenreIdentifier"/>
        <ms:conformsTo rdf:resource="http://w3id.org/meta-share/meta-share/MS_SpeechGenreClassification"/>
    </owl:NamedIndividual>
    


    <!-- http://w3id.org/meta-share/meta-share/MS_SG005 -->

    <owl:NamedIndividual rdf:about="http://w3id.org/meta-share/meta-share/MS_SG005">
        <rdf:type rdf:resource="http://w3id.org/meta-share/meta-share/SpeechGenreIdentifier"/>
        <ms:conformsTo rdf:resource="http://w3id.org/meta-share/meta-share/MS_SpeechGenreClassification"/>
    </owl:NamedIndividual>
    


    <!-- http://w3id.org/meta-share/meta-share/MS_SG006 -->

    <owl:NamedIndividual rdf:about="http://w3id.org/meta-share/meta-share/MS_SG006">
        <rdf:type rdf:resource="http://w3id.org/meta-share/meta-share/SpeechGenreIdentifier"/>
        <ms:conformsTo rdf:resource="http://w3id.org/meta-share/meta-share/MS_SpeechGenreClassification"/>
    </owl:NamedIndividual>
    


    <!-- http://w3id.org/meta-share/meta-share/MS_SG007 -->

    <owl:NamedIndividual rdf:about="http://w3id.org/meta-share/meta-share/MS_SG007">
        <rdf:type rdf:resource="http://w3id.org/meta-share/meta-share/SpeechGenreIdentifier"/>
        <ms:conformsTo rdf:resource="http://w3id.org/meta-share/meta-share/MS_SpeechGenreClassification"/>
    </owl:NamedIndividual>
    


    <!-- http://w3id.org/meta-share/meta-share/MS_SG008 -->

    <owl:NamedIndividual rdf:about="http://w3id.org/meta-share/meta-share/MS_SG008">
        <rdf:type rdf:resource="http://w3id.org/meta-share/meta-share/SpeechGenreIdentifier"/>
        <ms:conformsTo rdf:resource="http://w3id.org/meta-share/meta-share/MS_SpeechGenreClassification"/>
    </owl:NamedIndividual>
    


    <!-- http://w3id.org/meta-share/meta-share/MS_SG009 -->

    <owl:NamedIndividual rdf:about="http://w3id.org/meta-share/meta-share/MS_SG009">
        <rdf:type rdf:resource="http://w3id.org/meta-share/meta-share/SpeechGenreIdentifier"/>
        <ms:conformsTo rdf:resource="http://w3id.org/meta-share/meta-share/MS_SpeechGenreClassification"/>
    </owl:NamedIndividual>
    


    <!-- http://w3id.org/meta-share/meta-share/MS_SG010 -->

    <owl:NamedIndividual rdf:about="http://w3id.org/meta-share/meta-share/MS_SG010">
        <rdf:type rdf:resource="http://w3id.org/meta-share/meta-share/SpeechGenreIdentifier"/>
    </owl:NamedIndividual>
    


    <!-- http://w3id.org/meta-share/meta-share/MS_SG011 -->

    <owl:NamedIndividual rdf:about="http://w3id.org/meta-share/meta-share/MS_SG011">
        <rdf:type rdf:resource="http://w3id.org/meta-share/meta-share/SpeechGenreIdentifier"/>
        <ms:conformsTo rdf:resource="http://w3id.org/meta-share/meta-share/MS_SpeechGenreClassification"/>
    </owl:NamedIndividual>
    


    <!-- http://w3id.org/meta-share/meta-share/MS_SG012 -->

    <owl:NamedIndividual rdf:about="http://w3id.org/meta-share/meta-share/MS_SG012">
        <rdf:type rdf:resource="http://w3id.org/meta-share/meta-share/SpeechGenreIdentifier"/>
        <ms:conformsTo rdf:resource="http://w3id.org/meta-share/meta-share/MS_SpeechGenreClassification"/>
    </owl:NamedIndividual>
    


    <!-- http://w3id.org/meta-share/meta-share/MS_SG013 -->

    <owl:NamedIndividual rdf:about="http://w3id.org/meta-share/meta-share/MS_SG013">
        <rdf:type rdf:resource="http://w3id.org/meta-share/meta-share/SpeechGenreIdentifier"/>
    </owl:NamedIndividual>
    


    <!-- http://w3id.org/meta-share/meta-share/MS_SpeechGenreClassification -->

    <owl:NamedIndividual rdf:about="http://w3id.org/meta-share/meta-share/MS_SpeechGenreClassification">
        <rdf:type rdf:resource="http://w3id.org/meta-share/meta-share/SpeechGenreClassificationScheme"/>
        <rdfs:label xml:lang="en">META-SHARE speech genre classification scheme</rdfs:label>
    </owl:NamedIndividual>
    


    <!-- http://w3id.org/meta-share/meta-share/MS_audioGenreClassification -->

    <owl:NamedIndividual rdf:about="http://w3id.org/meta-share/meta-share/MS_audioGenreClassification">
        <rdf:type rdf:resource="http://w3id.org/meta-share/meta-share/AudioGenreClassificationScheme"/>
        <rdfs:label xml:lang="en">META-SHARE audio genre classification scheme</rdfs:label>
    </owl:NamedIndividual>
    


    <!-- http://w3id.org/meta-share/meta-share/MTBF -->

    <owl:NamedIndividual rdf:about="http://w3id.org/meta-share/meta-share/MTBF">
        <rdf:type rdf:resource="http://w3id.org/meta-share/meta-share/Metric"/>
        <rdfs:altLabel xml:lang="en">Mean Time Between Failures</rdfs:altLabel>
        <rdfs:label xml:lang="en">MTBF</rdfs:label>
    </owl:NamedIndividual>
    


    <!-- http://w3id.org/meta-share/meta-share/MTSA -->

    <owl:NamedIndividual rdf:about="http://w3id.org/meta-share/meta-share/MTSA">
        <rdf:type rdf:resource="http://w3id.org/meta-share/meta-share/Metric"/>
        <rdfs:altLabel xml:lang="en">Mean Time Seek Annotations</rdfs:altLabel>
        <rdfs:label xml:lang="en">MTSA</rdfs:label>
    </owl:NamedIndividual>
    


    <!-- http://w3id.org/meta-share/meta-share/MTTR -->

    <owl:NamedIndividual rdf:about="http://w3id.org/meta-share/meta-share/MTTR">
        <rdf:type rdf:resource="http://w3id.org/meta-share/meta-share/Metric"/>
        <rdfs:altLabel xml:lang="en">Mean Time To Repair</rdfs:altLabel>
        <rdfs:label xml:lang="en">MTTR</rdfs:label>
    </owl:NamedIndividual>
    


    <!-- http://w3id.org/meta-share/meta-share/MULTEXT -->

    <owl:NamedIndividual rdf:about="http://w3id.org/meta-share/meta-share/MULTEXT">
        <rdf:type rdf:resource="http://w3id.org/meta-share/meta-share/StandardBestPractice"/>
        <ms:url>https://tei-c.org/activities/projects/multilingual-text-tools-and-corpora-multext/</ms:url>
        <rdfs:label xml:lang="en">MULTEXT</rdfs:label>
    </owl:NamedIndividual>
    


    <!-- http://w3id.org/meta-share/meta-share/MUMIN -->

    <owl:NamedIndividual rdf:about="http://w3id.org/meta-share/meta-share/MUMIN">
        <rdf:type rdf:resource="http://w3id.org/meta-share/meta-share/StandardBestPractice"/>
        <ms:url>https://cst.dk/mumin/</ms:url>
        <rdfs:altLabel xml:lang="en">MUltiModal INterfaces</rdfs:altLabel>
        <rdfs:label xml:lang="en">MUMIN</rdfs:label>
    </owl:NamedIndividual>
    


    <!-- http://w3id.org/meta-share/meta-share/MacArabic -->

    <owl:NamedIndividual rdf:about="http://w3id.org/meta-share/meta-share/MacArabic">
        <rdf:type rdf:resource="http://w3id.org/meta-share/meta-share/CharacterEncoding"/>
        <rdfs:label xml:lang="en">MacArabic</rdfs:label>
    </owl:NamedIndividual>
    


    <!-- http://w3id.org/meta-share/meta-share/MacCentralEurope -->

    <owl:NamedIndividual rdf:about="http://w3id.org/meta-share/meta-share/MacCentralEurope">
        <rdf:type rdf:resource="http://w3id.org/meta-share/meta-share/CharacterEncoding"/>
        <rdfs:label xml:lang="en">MacCentralEurope</rdfs:label>
    </owl:NamedIndividual>
    


    <!-- http://w3id.org/meta-share/meta-share/MacCroatian -->

    <owl:NamedIndividual rdf:about="http://w3id.org/meta-share/meta-share/MacCroatian">
        <rdf:type rdf:resource="http://w3id.org/meta-share/meta-share/CharacterEncoding"/>
        <rdfs:label xml:lang="en">MacCroatian</rdfs:label>
    </owl:NamedIndividual>
    


    <!-- http://w3id.org/meta-share/meta-share/MacCyrillic -->

    <owl:NamedIndividual rdf:about="http://w3id.org/meta-share/meta-share/MacCyrillic">
        <rdf:type rdf:resource="http://w3id.org/meta-share/meta-share/CharacterEncoding"/>
        <rdfs:label xml:lang="en">MacCyrillic</rdfs:label>
    </owl:NamedIndividual>
    


    <!-- http://w3id.org/meta-share/meta-share/MacDingbat -->

    <owl:NamedIndividual rdf:about="http://w3id.org/meta-share/meta-share/MacDingbat">
        <rdf:type rdf:resource="http://w3id.org/meta-share/meta-share/CharacterEncoding"/>
        <rdfs:label xml:lang="en">MacDingbat</rdfs:label>
    </owl:NamedIndividual>
    


    <!-- http://w3id.org/meta-share/meta-share/MacGreek -->

    <owl:NamedIndividual rdf:about="http://w3id.org/meta-share/meta-share/MacGreek">
        <rdf:type rdf:resource="http://w3id.org/meta-share/meta-share/CharacterEncoding"/>
        <rdfs:label xml:lang="en">MacGreek</rdfs:label>
    </owl:NamedIndividual>
    


    <!-- http://w3id.org/meta-share/meta-share/MacHebrew -->

    <owl:NamedIndividual rdf:about="http://w3id.org/meta-share/meta-share/MacHebrew">
        <rdf:type rdf:resource="http://w3id.org/meta-share/meta-share/CharacterEncoding"/>
        <rdfs:label xml:lang="en">MacHebrew</rdfs:label>
    </owl:NamedIndividual>
    


    <!-- http://w3id.org/meta-share/meta-share/MacIceland -->

    <owl:NamedIndividual rdf:about="http://w3id.org/meta-share/meta-share/MacIceland">
        <rdf:type rdf:resource="http://w3id.org/meta-share/meta-share/CharacterEncoding"/>
        <rdfs:label xml:lang="en">MacIceland</rdfs:label>
    </owl:NamedIndividual>
    


    <!-- http://w3id.org/meta-share/meta-share/MacRoman -->

    <owl:NamedIndividual rdf:about="http://w3id.org/meta-share/meta-share/MacRoman">
        <rdf:type rdf:resource="http://w3id.org/meta-share/meta-share/CharacterEncoding"/>
        <rdfs:label xml:lang="en">MacRoman</rdfs:label>
    </owl:NamedIndividual>
    


    <!-- http://w3id.org/meta-share/meta-share/MacRomania -->

    <owl:NamedIndividual rdf:about="http://w3id.org/meta-share/meta-share/MacRomania">
        <rdf:type rdf:resource="http://w3id.org/meta-share/meta-share/CharacterEncoding"/>
        <rdfs:label xml:lang="en">MacRomania</rdfs:label>
    </owl:NamedIndividual>
    


    <!-- http://w3id.org/meta-share/meta-share/MacSymbol -->

    <owl:NamedIndividual rdf:about="http://w3id.org/meta-share/meta-share/MacSymbol">
        <rdf:type rdf:resource="http://w3id.org/meta-share/meta-share/CharacterEncoding"/>
        <rdfs:label xml:lang="en">MacSymbol</rdfs:label>
    </owl:NamedIndividual>
    


    <!-- http://w3id.org/meta-share/meta-share/MacThai -->

    <owl:NamedIndividual rdf:about="http://w3id.org/meta-share/meta-share/MacThai">
        <rdf:type rdf:resource="http://w3id.org/meta-share/meta-share/CharacterEncoding"/>
        <rdfs:label xml:lang="en">MacThai</rdfs:label>
    </owl:NamedIndividual>
    


    <!-- http://w3id.org/meta-share/meta-share/MacTurkish -->

    <owl:NamedIndividual rdf:about="http://w3id.org/meta-share/meta-share/MacTurkish">
        <rdf:type rdf:resource="http://w3id.org/meta-share/meta-share/CharacterEncoding"/>
        <rdfs:label xml:lang="en">MacTurkish</rdfs:label>
    </owl:NamedIndividual>
    


    <!-- http://w3id.org/meta-share/meta-share/MacUkraine -->

    <owl:NamedIndividual rdf:about="http://w3id.org/meta-share/meta-share/MacUkraine">
        <rdf:type rdf:resource="http://w3id.org/meta-share/meta-share/CharacterEncoding"/>
        <rdfs:label xml:lang="en">MacUkraine</rdfs:label>
    </owl:NamedIndividual>
    


    <!-- http://w3id.org/meta-share/meta-share/MeSH_classification -->

    <owl:NamedIndividual rdf:about="http://w3id.org/meta-share/meta-share/MeSH_classification">
        <rdf:type rdf:resource="http://w3id.org/meta-share/meta-share/SubjectClassificationScheme"/>
        <ms:url>http://www.openclinical.org/medTermMesh.html</ms:url>
        <rdfs:altLabel xml:lang="en">Medical Subject Headings</rdfs:altLabel>
        <rdfs:label xml:lang="en">MeSH</rdfs:label>
    </owl:NamedIndividual>
    


    <!-- http://w3id.org/meta-share/meta-share/NLM_classification -->

    <owl:NamedIndividual rdf:about="http://w3id.org/meta-share/meta-share/NLM_classification">
        <rdf:type rdf:resource="http://w3id.org/meta-share/meta-share/SubjectClassificationScheme"/>
        <rdfs:comment xml:lang="en">Classification scheme of the National Library of Medicine (https://www.nlm.nih.gov/class/)</rdfs:comment>
        <rdfs:label xml:lang="en">NLM classification scheme</rdfs:label>
    </owl:NamedIndividual>
    


    <!-- http://w3id.org/meta-share/meta-share/OAXAL -->

    <owl:NamedIndividual rdf:about="http://w3id.org/meta-share/meta-share/OAXAL">
        <rdf:type rdf:resource="http://w3id.org/meta-share/meta-share/StandardBestPractice"/>
        <ms:url>https://www.oasis-open.org/committees/tc_home.php?wg_abbrev=oaxal</ms:url>
        <rdfs:altLabel xml:lang="en">OASIS Open Architecture for XML Authoring and Localization Reference Model</rdfs:altLabel>
        <rdfs:label xml:lang="en">OAXAL</rdfs:label>
    </owl:NamedIndividual>
    


    <!-- http://w3id.org/meta-share/meta-share/OMTDShareRightsStatementScheme -->

    <owl:NamedIndividual rdf:about="http://w3id.org/meta-share/meta-share/OMTDShareRightsStatementScheme">
        <rdf:type rdf:resource="http://w3id.org/meta-share/meta-share/AccessRightsStatementScheme"/>
        <rdfs:label xml:lang="en">OMTD-SHARE rights statement scheme</rdfs:label>
    </owl:NamedIndividual>
    


    <!-- http://w3id.org/meta-share/meta-share/OpenAIRE -->

    <owl:NamedIndividual rdf:about="http://w3id.org/meta-share/meta-share/OpenAIRE">
        <rdf:type rdf:resource="http://w3id.org/meta-share/meta-share/MetadataRecordIdentifierScheme"/>
        <rdfs:label xml:lang="en">OpenAIRE</rdfs:label>
    </owl:NamedIndividual>
    


    <!-- http://w3id.org/meta-share/meta-share/PAROLE_G001 -->

    <owl:NamedIndividual rdf:about="http://w3id.org/meta-share/meta-share/PAROLE_G001">
        <rdf:type rdf:resource="http://w3id.org/meta-share/meta-share/TextGenreIdentifier"/>
        <ms:conformsTo rdf:resource="http://w3id.org/meta-share/meta-share/PAROLE_genreClassification"/>
    </owl:NamedIndividual>
    


    <!-- http://w3id.org/meta-share/meta-share/PAROLE_G002 -->

    <owl:NamedIndividual rdf:about="http://w3id.org/meta-share/meta-share/PAROLE_G002">
        <rdf:type rdf:resource="http://w3id.org/meta-share/meta-share/TextGenreIdentifier"/>
        <ms:conformsTo rdf:resource="http://w3id.org/meta-share/meta-share/PAROLE_genreClassification"/>
    </owl:NamedIndividual>
    


    <!-- http://w3id.org/meta-share/meta-share/PAROLE_G003 -->

    <owl:NamedIndividual rdf:about="http://w3id.org/meta-share/meta-share/PAROLE_G003">
        <rdf:type rdf:resource="http://w3id.org/meta-share/meta-share/TextGenreIdentifier"/>
        <ms:conformsTo rdf:resource="http://w3id.org/meta-share/meta-share/PAROLE_genreClassification"/>
    </owl:NamedIndividual>
    


    <!-- http://w3id.org/meta-share/meta-share/PAROLE_G004 -->

    <owl:NamedIndividual rdf:about="http://w3id.org/meta-share/meta-share/PAROLE_G004">
        <rdf:type rdf:resource="http://w3id.org/meta-share/meta-share/TextGenreIdentifier"/>
        <ms:conformsTo rdf:resource="http://w3id.org/meta-share/meta-share/PAROLE_genreClassification"/>
    </owl:NamedIndividual>
    


    <!-- http://w3id.org/meta-share/meta-share/PAROLE_G005 -->

    <owl:NamedIndividual rdf:about="http://w3id.org/meta-share/meta-share/PAROLE_G005">
        <rdf:type rdf:resource="http://w3id.org/meta-share/meta-share/TextGenreIdentifier"/>
        <ms:conformsTo rdf:resource="http://w3id.org/meta-share/meta-share/PAROLE_genreClassification"/>
    </owl:NamedIndividual>
    


    <!-- http://w3id.org/meta-share/meta-share/PAROLE_G006 -->

    <owl:NamedIndividual rdf:about="http://w3id.org/meta-share/meta-share/PAROLE_G006">
        <rdf:type rdf:resource="http://w3id.org/meta-share/meta-share/TextGenreIdentifier"/>
        <ms:conformsTo rdf:resource="http://w3id.org/meta-share/meta-share/PAROLE_genreClassification"/>
    </owl:NamedIndividual>
    


    <!-- http://w3id.org/meta-share/meta-share/PAROLE_G007 -->

    <owl:NamedIndividual rdf:about="http://w3id.org/meta-share/meta-share/PAROLE_G007">
        <rdf:type rdf:resource="http://w3id.org/meta-share/meta-share/TextGenreIdentifier"/>
        <ms:conformsTo rdf:resource="http://w3id.org/meta-share/meta-share/PAROLE_genreClassification"/>
    </owl:NamedIndividual>
    


    <!-- http://w3id.org/meta-share/meta-share/PAROLE_G008 -->

    <owl:NamedIndividual rdf:about="http://w3id.org/meta-share/meta-share/PAROLE_G008">
        <rdf:type rdf:resource="http://w3id.org/meta-share/meta-share/TextGenreIdentifier"/>
        <ms:conformsTo rdf:resource="http://w3id.org/meta-share/meta-share/PAROLE_genreClassification"/>
    </owl:NamedIndividual>
    


    <!-- http://w3id.org/meta-share/meta-share/PAROLE_G009 -->

    <owl:NamedIndividual rdf:about="http://w3id.org/meta-share/meta-share/PAROLE_G009">
        <rdf:type rdf:resource="http://w3id.org/meta-share/meta-share/TextGenreIdentifier"/>
        <ms:conformsTo rdf:resource="http://w3id.org/meta-share/meta-share/PAROLE_genreClassification"/>
    </owl:NamedIndividual>
    


    <!-- http://w3id.org/meta-share/meta-share/PAROLE_genreClassification -->

    <owl:NamedIndividual rdf:about="http://w3id.org/meta-share/meta-share/PAROLE_genreClassification">
        <rdf:type rdf:resource="http://w3id.org/meta-share/meta-share/TextGenreClassificationScheme"/>
        <rdfs:label xml:lang="en">PAROLE_genre classification scheme</rdfs:label>
    </owl:NamedIndividual>
    


    <!-- http://w3id.org/meta-share/meta-share/PAROLE_topicClassification -->

    <owl:NamedIndividual rdf:about="http://w3id.org/meta-share/meta-share/PAROLE_topicClassification">
        <rdf:type rdf:resource="http://w3id.org/meta-share/meta-share/SubjectClassificationScheme"/>
        <rdfs:label xml:lang="en">PAROLE_topic classification scheme</rdfs:label>
    </owl:NamedIndividual>
    


    <!-- http://w3id.org/meta-share/meta-share/REST -->

    <owl:NamedIndividual rdf:about="http://w3id.org/meta-share/meta-share/REST">
        <rdf:type rdf:resource="http://w3id.org/meta-share/meta-share/WebServiceType"/>
        <rdfs:label xml:lang="en">REST</rdfs:label>
    </owl:NamedIndividual>
    


    <!-- http://w3id.org/meta-share/meta-share/RGB -->

    <owl:NamedIndividual rdf:about="http://w3id.org/meta-share/meta-share/RGB">
        <rdf:type rdf:resource="http://w3id.org/meta-share/meta-share/ColourSpace"/>
        <rdfs:label xml:lang="en">RGB</rdfs:label>
    </owl:NamedIndividual>
    


    <!-- http://w3id.org/meta-share/meta-share/RightsStatementOrgScheme -->

    <owl:NamedIndividual rdf:about="http://w3id.org/meta-share/meta-share/RightsStatementOrgScheme">
        <rdf:type rdf:resource="http://w3id.org/meta-share/meta-share/AccessRightsStatementScheme"/>
        <rdfs:label xml:lang="en">Rights_Statements_Org scheme</rdfs:label>
    </owl:NamedIndividual>
    


    <!-- http://w3id.org/meta-share/meta-share/SNR -->

    <owl:NamedIndividual rdf:about="http://w3id.org/meta-share/meta-share/SNR">
        <rdf:type rdf:resource="http://w3id.org/meta-share/meta-share/AudioQualityMeasureIncluded"/>
        <rdfs:label xml:lang="en">SNR</rdfs:label>
    </owl:NamedIndividual>
    


    <!-- http://w3id.org/meta-share/meta-share/SOAP -->

    <owl:NamedIndividual rdf:about="http://w3id.org/meta-share/meta-share/SOAP">
        <rdf:type rdf:resource="http://w3id.org/meta-share/meta-share/WebServiceType"/>
        <rdfs:label xml:lang="en">SOAP</rdfs:label>
    </owl:NamedIndividual>
    


    <!-- http://w3id.org/meta-share/meta-share/SPDX -->

    <owl:NamedIndividual rdf:about="http://w3id.org/meta-share/meta-share/SPDX">
        <rdf:type rdf:resource="http://w3id.org/meta-share/meta-share/LicenceIdentifierScheme"/>
        <ms:url>https://spdx.org/licenses/</ms:url>
        <rdfs:comment xml:lang="en">Value for LicenceIdentifierScheme referring to the codes (identifiers) for licences used by SPDX (https://spdx.org/licenses/))</rdfs:comment>
        <rdfs:label xml:lang="en">SPDX</rdfs:label>
    </owl:NamedIndividual>
    


    <!-- http://w3id.org/meta-share/meta-share/SRX -->

    <owl:NamedIndividual rdf:about="http://w3id.org/meta-share/meta-share/SRX">
        <rdf:type rdf:resource="http://w3id.org/meta-share/meta-share/StandardBestPractice"/>
        <ms:url>https://www.gala-global.org/srx-20-april-7-2008</ms:url>
        <rdfs:altLabel xml:lang="en">Segmentation Rules eXchange</rdfs:altLabel>
        <rdfs:label xml:lang="en">SRX</rdfs:label>
    </owl:NamedIndividual>
    


    <!-- http://w3id.org/meta-share/meta-share/SemAF -->

    <owl:NamedIndividual rdf:about="http://w3id.org/meta-share/meta-share/SemAF">
        <rdf:type rdf:resource="http://w3id.org/meta-share/meta-share/StandardBestPractice"/>
        <rdfs:label xml:lang="en">Semantic Annotation Framework</rdfs:label>
    </owl:NamedIndividual>
    


    <!-- http://w3id.org/meta-share/meta-share/SemAF-DA -->

    <owl:NamedIndividual rdf:about="http://w3id.org/meta-share/meta-share/SemAF-DA">
        <rdf:type rdf:resource="http://w3id.org/meta-share/meta-share/StandardBestPractice"/>
        <ms:url>https://www.iso.org/standard/76443.html</ms:url>
        <rdfs:altLabel xml:lang="en">Semantic Annotation Framework - Dialogue Acts</rdfs:altLabel>
        <rdfs:label xml:lang="en">SemAF-DA</rdfs:label>
    </owl:NamedIndividual>
    


    <!-- http://w3id.org/meta-share/meta-share/SemAF-DS -->

    <owl:NamedIndividual rdf:about="http://w3id.org/meta-share/meta-share/SemAF-DS">
        <rdf:type rdf:resource="http://w3id.org/meta-share/meta-share/StandardBestPractice"/>
        <ms:url>https://www.iso.org/obp/ui/#iso:std:iso:ts:24617:-5:ed-1:v1:en</ms:url>
        <rdfs:altLabel xml:lang="en">Semantic Annotation Framework - Discourse Structure</rdfs:altLabel>
        <rdfs:label xml:lang="en">SemAF-DS</rdfs:label>
    </owl:NamedIndividual>
    


    <!-- http://w3id.org/meta-share/meta-share/SemAF-NE -->

    <owl:NamedIndividual rdf:about="http://w3id.org/meta-share/meta-share/SemAF-NE">
        <rdf:type rdf:resource="http://w3id.org/meta-share/meta-share/StandardBestPractice"/>
        <ms:url>http://semanticweb.kaist.ac.kr/research/tc37sc4/new_doc/iso_tc37_sc4_N796_wg2_proposed_WD_24617-3_SemAF-NE.pdf</ms:url>
        <rdfs:altLabel xml:lang="en">Semantic Annotation Framework - Named Entities</rdfs:altLabel>
        <rdfs:label xml:lang="en">SemAF-NE</rdfs:label>
    </owl:NamedIndividual>
    


    <!-- http://w3id.org/meta-share/meta-share/SemAF-SR -->

    <owl:NamedIndividual rdf:about="http://w3id.org/meta-share/meta-share/SemAF-SR">
        <rdf:type rdf:resource="http://w3id.org/meta-share/meta-share/StandardBestPractice"/>
        <ms:url>https://www.iso.org/standard/56866.html</ms:url>
        <rdfs:altLabel xml:lang="en">Semantic Annotation Framework - Semantic Roles</rdfs:altLabel>
        <rdfs:label xml:lang="en">SemAF-SR</rdfs:label>
    </owl:NamedIndividual>
    


    <!-- http://w3id.org/meta-share/meta-share/Shift_JIS -->

    <owl:NamedIndividual rdf:about="http://w3id.org/meta-share/meta-share/Shift_JIS">
        <rdf:type rdf:resource="http://w3id.org/meta-share/meta-share/CharacterEncoding"/>
        <rdfs:label xml:lang="en">Shift_JIS</rdfs:label>
    </owl:NamedIndividual>
    


    <!-- http://w3id.org/meta-share/meta-share/SynAF -->

    <owl:NamedIndividual rdf:about="http://w3id.org/meta-share/meta-share/SynAF">
        <rdf:type rdf:resource="http://w3id.org/meta-share/meta-share/StandardBestPractice"/>
        <ms:url>https://www.iso.org/standard/62508.html</ms:url>
        <rdfs:altLabel xml:lang="en">Syntactic Annotation Framework</rdfs:altLabel>
        <rdfs:label xml:lang="en">SynAF</rdfs:label>
    </owl:NamedIndividual>
    


    <!-- http://w3id.org/meta-share/meta-share/T-HPair -->

    <owl:NamedIndividual rdf:about="http://w3id.org/meta-share/meta-share/T-HPair">
        <rdf:type rdf:resource="http://w3id.org/meta-share/meta-share/SizeUnit"/>
        <rdfs:label xml:lang="en">T-H pair</rdfs:label>
    </owl:NamedIndividual>
    


    <!-- http://w3id.org/meta-share/meta-share/TBX -->

    <owl:NamedIndividual rdf:about="http://w3id.org/meta-share/meta-share/TBX">
        <rdf:type rdf:resource="http://w3id.org/meta-share/meta-share/StandardBestPractice"/>
        <ms:url>https://www.tbxinfo.net/tbx-about/</ms:url>
        <rdfs:altLabel xml:lang="en">TermBase eXchange</rdfs:altLabel>
        <rdfs:label xml:lang="en">TBX</rdfs:label>
    </owl:NamedIndividual>
    


    <!-- http://w3id.org/meta-share/meta-share/TEI -->

    <owl:NamedIndividual rdf:about="http://w3id.org/meta-share/meta-share/TEI">
        <rdf:type rdf:resource="http://w3id.org/meta-share/meta-share/StandardBestPractice"/>
        <ms:url>https://tei-c.org/</ms:url>
        <rdfs:altLabel xml:lang="en">Text Encoding Initiative</rdfs:altLabel>
        <rdfs:label xml:lang="en">TEI</rdfs:label>
    </owl:NamedIndividual>
    


    <!-- http://w3id.org/meta-share/meta-share/TEI_P3 -->

    <owl:NamedIndividual rdf:about="http://w3id.org/meta-share/meta-share/TEI_P3">
        <rdf:type rdf:resource="http://w3id.org/meta-share/meta-share/StandardBestPractice"/>
        <ms:url>https://www.tei-c.org/Vault/GL/P3/index.htm</ms:url>
        <rdfs:altLabel xml:lang="en">Text Encoding Initiative P3</rdfs:altLabel>
        <rdfs:label xml:lang="en">TEI P3</rdfs:label>
    </owl:NamedIndividual>
    


    <!-- http://w3id.org/meta-share/meta-share/TEI_P4 -->

    <owl:NamedIndividual rdf:about="http://w3id.org/meta-share/meta-share/TEI_P4">
        <rdf:type rdf:resource="http://w3id.org/meta-share/meta-share/StandardBestPractice"/>
        <ms:url>https://tei-c.org/Vault/P4/doc/html/</ms:url>
        <rdfs:altLabel xml:lang="en">Text Encoding Initiative P4</rdfs:altLabel>
        <rdfs:label xml:lang="en">TEI P4</rdfs:label>
    </owl:NamedIndividual>
    


    <!-- http://w3id.org/meta-share/meta-share/TEI_P5 -->

    <owl:NamedIndividual rdf:about="http://w3id.org/meta-share/meta-share/TEI_P5">
        <rdf:type rdf:resource="http://w3id.org/meta-share/meta-share/StandardBestPractice"/>
        <ms:url>https://tei-c.org/guidelines/p5/</ms:url>
        <rdfs:altLabel xml:lang="en">Text Encoding Initiative P5</rdfs:altLabel>
        <rdfs:label xml:lang="en">TEI P5</rdfs:label>
    </owl:NamedIndividual>
    


    <!-- http://w3id.org/meta-share/meta-share/TIS-620 -->

    <owl:NamedIndividual rdf:about="http://w3id.org/meta-share/meta-share/TIS-620">
        <rdf:type rdf:resource="http://w3id.org/meta-share/meta-share/CharacterEncoding"/>
        <rdfs:label xml:lang="en">TIS-620</rdfs:label>
    </owl:NamedIndividual>
    


    <!-- http://w3id.org/meta-share/meta-share/TMX -->

    <owl:NamedIndividual rdf:about="http://w3id.org/meta-share/meta-share/TMX">
        <rdf:type rdf:resource="http://w3id.org/meta-share/meta-share/StandardBestPractice"/>
        <ms:url>http://www.opentag.com/tmx.htm</ms:url>
        <rdfs:altLabel xml:lang="en">Translation Memory eXchange</rdfs:altLabel>
        <rdfs:label xml:lang="en">TMX</rdfs:label>
    </owl:NamedIndividual>
    


    <!-- http://w3id.org/meta-share/meta-share/TST-CENTRALE -->

    <owl:NamedIndividual rdf:about="http://w3id.org/meta-share/meta-share/TST-CENTRALE">
        <rdf:type rdf:resource="http://w3id.org/meta-share/meta-share/MembershipInstitution"/>
        <rdfs:label xml:lang="en">TST-Centrale</rdfs:label>
    </owl:NamedIndividual>
    


    <!-- http://w3id.org/meta-share/meta-share/ThreeD -->

    <owl:NamedIndividual rdf:about="http://w3id.org/meta-share/meta-share/ThreeD">
        <rdf:type rdf:resource="http://w3id.org/meta-share/meta-share/VisualModelling"/>
        <rdfs:label xml:lang="en">3D</rdfs:label>
    </owl:NamedIndividual>
    


    <!-- http://w3id.org/meta-share/meta-share/ThreeG -->

    <owl:NamedIndividual rdf:about="http://w3id.org/meta-share/meta-share/ThreeG">
        <rdf:type rdf:resource="http://w3id.org/meta-share/meta-share/SourceChannelType"/>
        <rdfs:label xml:lang="en">3G</rdfs:label>
    </owl:NamedIndividual>
    


    <!-- http://w3id.org/meta-share/meta-share/TimeML -->

    <owl:NamedIndividual rdf:about="http://w3id.org/meta-share/meta-share/TimeML">
        <rdf:type rdf:resource="http://w3id.org/meta-share/meta-share/StandardBestPractice"/>
        <ms:url>http://www.timeml.org/</ms:url>
        <rdfs:altLabel xml:lang="en">Time Markup Language</rdfs:altLabel>
        <rdfs:label xml:lang="en">TimeML</rdfs:label>
    </owl:NamedIndividual>
    


    <!-- http://w3id.org/meta-share/meta-share/TwoD -->

    <owl:NamedIndividual rdf:about="http://w3id.org/meta-share/meta-share/TwoD">
        <rdf:type rdf:resource="http://w3id.org/meta-share/meta-share/VisualModelling"/>
        <rdfs:label xml:lang="en">2D</rdfs:label>
    </owl:NamedIndividual>
    


    <!-- http://w3id.org/meta-share/meta-share/UDC_classification -->

    <owl:NamedIndividual rdf:about="http://w3id.org/meta-share/meta-share/UDC_classification">
        <rdf:type rdf:resource="http://w3id.org/meta-share/meta-share/DomainClassificationScheme"/>
        <ms:url>http://www.udcc.org/</ms:url>
        <rdfs:altLabel xml:lang="en">Universal Decimal Classification</rdfs:altLabel>
        <rdfs:label xml:lang="en">UDC</rdfs:label>
    </owl:NamedIndividual>
    


    <!-- http://w3id.org/meta-share/meta-share/UIMA -->

    <owl:NamedIndividual rdf:about="http://w3id.org/meta-share/meta-share/UIMA">
        <rdf:type rdf:resource="http://w3id.org/meta-share/meta-share/Framework"/>
        <rdfs:label xml:lang="en">UIMA</rdfs:label>
    </owl:NamedIndividual>
    


    <!-- http://w3id.org/meta-share/meta-share/US-ASCII -->

    <owl:NamedIndividual rdf:about="http://w3id.org/meta-share/meta-share/US-ASCII">
        <rdf:type rdf:resource="http://w3id.org/meta-share/meta-share/CharacterEncoding"/>
        <rdfs:label xml:lang="en">US-ASCII</rdfs:label>
    </owl:NamedIndividual>
    


    <!-- http://w3id.org/meta-share/meta-share/UTF-16 -->

    <owl:NamedIndividual rdf:about="http://w3id.org/meta-share/meta-share/UTF-16">
        <rdf:type rdf:resource="http://w3id.org/meta-share/meta-share/CharacterEncoding"/>
        <rdfs:label xml:lang="en">UTF-16</rdfs:label>
    </owl:NamedIndividual>
    


    <!-- http://w3id.org/meta-share/meta-share/UTF-16BE -->

    <owl:NamedIndividual rdf:about="http://w3id.org/meta-share/meta-share/UTF-16BE">
        <rdf:type rdf:resource="http://w3id.org/meta-share/meta-share/CharacterEncoding"/>
        <rdfs:label xml:lang="en">UTF-16BE</rdfs:label>
    </owl:NamedIndividual>
    


    <!-- http://w3id.org/meta-share/meta-share/UTF-16LE -->

    <owl:NamedIndividual rdf:about="http://w3id.org/meta-share/meta-share/UTF-16LE">
        <rdf:type rdf:resource="http://w3id.org/meta-share/meta-share/CharacterEncoding"/>
        <rdfs:label xml:lang="en">UTF-16LE</rdfs:label>
    </owl:NamedIndividual>
    


    <!-- http://w3id.org/meta-share/meta-share/UTF-8 -->

    <owl:NamedIndividual rdf:about="http://w3id.org/meta-share/meta-share/UTF-8">
        <rdf:type rdf:resource="http://w3id.org/meta-share/meta-share/CharacterEncoding"/>
        <rdfs:label xml:lang="en">UTF-8</rdfs:label>
    </owl:NamedIndividual>
    


    <!-- http://w3id.org/meta-share/meta-share/VGA -->

    <owl:NamedIndividual rdf:about="http://w3id.org/meta-share/meta-share/VGA">
        <rdf:type rdf:resource="http://w3id.org/meta-share/meta-share/ResolutionStandard"/>
        <rdfs:label xml:lang="en">VGA</rdfs:label>
    </owl:NamedIndividual>
    


    <!-- http://w3id.org/meta-share/meta-share/VOIP -->

    <owl:NamedIndividual rdf:about="http://w3id.org/meta-share/meta-share/VOIP">
        <rdf:type rdf:resource="http://w3id.org/meta-share/meta-share/SourceChannelType"/>
        <rdfs:label xml:lang="en">VOIP</rdfs:label>
    </owl:NamedIndividual>
    


    <!-- http://w3id.org/meta-share/meta-share/XCES -->

    <owl:NamedIndividual rdf:about="http://w3id.org/meta-share/meta-share/XCES">
        <rdf:type rdf:resource="http://w3id.org/meta-share/meta-share/StandardBestPractice"/>
        <ms:url>http://www.xces.org/</ms:url>
        <rdfs:altLabel xml:lang="en">Corpus Encoding Standard for XML</rdfs:altLabel>
        <rdfs:label xml:lang="en">XCES</rdfs:label>
    </owl:NamedIndividual>
    


    <!-- http://w3id.org/meta-share/meta-share/XLIFF -->

    <owl:NamedIndividual rdf:about="http://w3id.org/meta-share/meta-share/XLIFF">
        <rdf:type rdf:resource="http://w3id.org/meta-share/meta-share/StandardBestPractice"/>
        <ms:url>http://docs.oasis-open.org/xliff/v1.2/os/xliff-core.html</ms:url>
        <rdfs:altLabel xml:lang="en">XML Localization Interchange File Format</rdfs:altLabel>
        <rdfs:label xml:lang="en">XLIFF</rdfs:label>
    </owl:NamedIndividual>
    


    <!-- http://w3id.org/meta-share/meta-share/YUV -->

    <owl:NamedIndividual rdf:about="http://w3id.org/meta-share/meta-share/YUV">
        <rdf:type rdf:resource="http://w3id.org/meta-share/meta-share/ColourSpace"/>
        <rdfs:label xml:lang="en">YUV</rdfs:label>
    </owl:NamedIndividual>
    


    <!-- http://w3id.org/meta-share/meta-share/aLaw -->

    <owl:NamedIndividual rdf:about="http://w3id.org/meta-share/meta-share/aLaw">
        <rdf:type rdf:resource="http://w3id.org/meta-share/meta-share/SignalEncoding"/>
        <rdfs:label xml:lang="en">A-law</rdfs:label>
    </owl:NamedIndividual>
    


    <!-- http://w3id.org/meta-share/meta-share/aac -->

    <owl:NamedIndividual rdf:about="http://w3id.org/meta-share/meta-share/aac">
        <rdf:type rdf:resource="http://w3id.org/meta-share/meta-share/CompressionName"/>
        <rdfs:altLabel xml:lang="en">Advanced Audio Coding</rdfs:altLabel>
        <rdfs:label xml:lang="en">AAC</rdfs:label>
    </owl:NamedIndividual>
    


    <!-- http://w3id.org/meta-share/meta-share/abbreviation -->

    <owl:NamedIndividual rdf:about="http://w3id.org/meta-share/meta-share/abbreviation">
        <rdf:type rdf:resource="http://w3id.org/meta-share/meta-share/LemmaType"/>
        <rdfs:label xml:lang="en">abbreviation</rdfs:label>
    </owl:NamedIndividual>
    


    <!-- http://w3id.org/meta-share/meta-share/academic -->

    <owl:NamedIndividual rdf:about="http://w3id.org/meta-share/meta-share/academic">
        <rdf:type rdf:resource="http://w3id.org/meta-share/meta-share/UserType"/>
        <rdfs:comment xml:lang="en">Value for &apos;user type&apos; reserved for individuals affiliated to academir or, in general, educational or research institutions and the respective organisations</rdfs:comment>
        <rdfs:label xml:lang="en">academic</rdfs:label>
    </owl:NamedIndividual>
    


    <!-- http://w3id.org/meta-share/meta-share/academic1 -->

    <owl:NamedIndividual rdf:about="http://w3id.org/meta-share/meta-share/academic1">
        <rdf:type rdf:resource="http://w3id.org/meta-share/meta-share/LicenceCategory"/>
        <ms:conformsTo rdf:resource="http://w3id.org/meta-share/meta-share/ClarinLicenceCategoryScheme"/>
        <rdfs:altLabel xml:lang="en">ACA</rdfs:altLabel>
        <rdfs:label xml:lang="en">academic</rdfs:label>
    </owl:NamedIndividual>
    


    <!-- http://w3id.org/meta-share/meta-share/academicInstitution -->

    <owl:NamedIndividual rdf:about="http://w3id.org/meta-share/meta-share/academicInstitution">
        <rdf:type rdf:resource="http://w3id.org/meta-share/meta-share/OrganizationLegalStatus"/>
        <rdfs:label xml:lang="en">academic institution</rdfs:label>
    </owl:NamedIndividual>
    


    <!-- http://w3id.org/meta-share/meta-share/academicText -->

    <owl:NamedIndividual rdf:about="http://w3id.org/meta-share/meta-share/academicText">
        <rdf:type rdf:resource="http://w3id.org/meta-share/meta-share/TextType"/>
        <datacite:hasIdentifier rdf:resource="http://w3id.org/meta-share/meta-share/ClarinEl_TT001"/>
        <rdfs:label xml:lang="en">academic text</rdfs:label>
    </owl:NamedIndividual>
    


    <!-- http://w3id.org/meta-share/meta-share/academicUser -->

    <owl:NamedIndividual rdf:about="http://w3id.org/meta-share/meta-share/academicUser">
        <rdf:type rdf:resource="http://w3id.org/meta-share/meta-share/ConditionOfUse"/>
        <rdfs:label xml:lang="en">academic user</rdfs:label>
    </owl:NamedIndividual>
    


    <!-- http://w3id.org/meta-share/meta-share/accentuation -->

    <owl:NamedIndividual rdf:about="http://w3id.org/meta-share/meta-share/accentuation">
        <rdf:type rdf:resource="http://w3id.org/meta-share/meta-share/AudioType"/>
        <rdfs:label xml:lang="en">accentuation</rdfs:label>
    </owl:NamedIndividual>
    


    <!-- http://w3id.org/meta-share/meta-share/accepted -->

    <owl:NamedIndividual rdf:about="http://w3id.org/meta-share/meta-share/accepted">
        <rdf:type rdf:resource="http://w3id.org/meta-share/meta-share/VersionType"/>
        <rdfs:comment xml:lang="en">Value for &apos;Version type&apos; used for versions as accepted for publication (following a reviewing process that may have introduced changes from the submitted version)</rdfs:comment>
        <rdfs:label xml:lang="en">accepted</rdfs:label>
    </owl:NamedIndividual>
    


    <!-- http://w3id.org/meta-share/meta-share/accessibleThroughInterface -->

    <owl:NamedIndividual rdf:about="http://w3id.org/meta-share/meta-share/accessibleThroughInterface">
        <rdf:type rdf:resource="http://w3id.org/meta-share/meta-share/DatasetDistributionForm"/>
        <rdfs:comment xml:lang="en">Value for distribution medium, used for corpora and lexical/conceptual resources that can be accessed via a human-intended interface (e.g.,  corpus workbench, lexicon browsing interface, etc.)</rdfs:comment>
        <rdfs:label xml:lang="en">accessible through interface</rdfs:label>
    </owl:NamedIndividual>
    


    <!-- http://w3id.org/meta-share/meta-share/accessibleThroughQuery -->

    <owl:NamedIndividual rdf:about="http://w3id.org/meta-share/meta-share/accessibleThroughQuery">
        <rdf:type rdf:resource="http://w3id.org/meta-share/meta-share/DatasetDistributionForm"/>
        <rdfs:comment xml:lang="en">Value for dataset distribution medium, used for lexical/conceptual resources that can be accessed via a SPARQL endpoint</rdfs:comment>
        <rdfs:label xml:lang="en">accessible through query</rdfs:label>
    </owl:NamedIndividual>
    


    <!-- http://w3id.org/meta-share/meta-share/administrativeText -->

    <owl:NamedIndividual rdf:about="http://w3id.org/meta-share/meta-share/administrativeText">
        <rdf:type rdf:resource="http://w3id.org/meta-share/meta-share/TextType"/>
        <datacite:hasIdentifier rdf:resource="http://w3id.org/meta-share/meta-share/ClarinEl_TT008"/>
        <rdfs:label xml:lang="en">administrative text</rdfs:label>
    </owl:NamedIndividual>
    


    <!-- http://w3id.org/meta-share/meta-share/adult -->

    <owl:NamedIndividual rdf:about="http://w3id.org/meta-share/meta-share/adult">
        <rdf:type rdf:resource="http://w3id.org/meta-share/meta-share/AgeGroup"/>
        <rdfs:label xml:lang="en">adult</rdfs:label>
    </owl:NamedIndividual>
    


    <!-- http://w3id.org/meta-share/meta-share/advertising -->

    <owl:NamedIndividual rdf:about="http://w3id.org/meta-share/meta-share/advertising">
        <rdf:type rdf:resource="http://w3id.org/meta-share/meta-share/TextGenre"/>
        <datacite:hasIdentifier rdf:resource="http://w3id.org/meta-share/meta-share/PAROLE_G002"/>
        <rdfs:label xml:lang="en">advertising</rdfs:label>
    </owl:NamedIndividual>
    


    <!-- http://w3id.org/meta-share/meta-share/advertisingAndPublicRelations -->

    <owl:NamedIndividual rdf:about="http://w3id.org/meta-share/meta-share/advertisingAndPublicRelations">
        <rdf:type rdf:resource="http://w3id.org/meta-share/meta-share/Domain"/>
        <datacite:hasIdentifier rdf:resource="http://w3id.org/meta-share/meta-share/DDC659"/>
        <rdfs:label xml:lang="en">Advertising &amp; Public Relations</rdfs:label>
    </owl:NamedIndividual>
    


    <!-- http://w3id.org/meta-share/meta-share/agriculture -->

    <owl:NamedIndividual rdf:about="http://w3id.org/meta-share/meta-share/agriculture">
        <rdf:type rdf:resource="http://w3id.org/meta-share/meta-share/Domain"/>
        <datacite:hasIdentifier rdf:resource="http://w3id.org/meta-share/meta-share/DDC630"/>
        <rdfs:comment xml:lang="en">The science, art, or practice of cultivating the soil, producing crops, and raising livestock and in varying degrees the preparation and marketing of the resulting products [https://www.merriam-webster.com/dictionary/agriculture]</rdfs:comment>
        <rdfs:label xml:lang="en">Agriculture</rdfs:label>
    </owl:NamedIndividual>
    


    <!-- http://w3id.org/meta-share/meta-share/airTrafficControl -->

    <owl:NamedIndividual rdf:about="http://w3id.org/meta-share/meta-share/airTrafficControl">
        <rdf:type rdf:resource="http://w3id.org/meta-share/meta-share/SpeechGenre"/>
        <datacite:hasIdentifier rdf:resource="http://w3id.org/meta-share/meta-share/MS_SG001"/>
        <rdfs:label xml:lang="en">air traffic control</rdfs:label>
    </owl:NamedIndividual>
    


    <!-- http://w3id.org/meta-share/meta-share/airflow -->

    <owl:NamedIndividual rdf:about="http://w3id.org/meta-share/meta-share/airflow">
        <rdf:type rdf:resource="http://w3id.org/meta-share/meta-share/SourceChannel"/>
        <rdfs:label xml:lang="en">airflow</rdfs:label>
    </owl:NamedIndividual>
    


    <!-- http://w3id.org/meta-share/meta-share/alcohol -->

    <owl:NamedIndividual rdf:about="http://w3id.org/meta-share/meta-share/alcohol">
        <rdf:type rdf:resource="http://w3id.org/meta-share/meta-share/SpeechInfluence"/>
        <rdfs:label xml:lang="en">alcohol</rdfs:label>
    </owl:NamedIndividual>
    


    <!-- http://w3id.org/meta-share/meta-share/analysis -->

    <owl:NamedIndividual rdf:about="http://w3id.org/meta-share/meta-share/analysis">
        <rdf:type rdf:resource="http://w3id.org/meta-share/meta-share/LDTask"/>
        <rdfs:label xml:lang="en">analysis</rdfs:label>
    </owl:NamedIndividual>
    


    <!-- http://w3id.org/meta-share/meta-share/anaphora -->

    <owl:NamedIndividual rdf:about="http://w3id.org/meta-share/meta-share/anaphora">
        <rdf:type rdf:resource="http://w3id.org/meta-share/meta-share/GrammaticalPhenomenaCoverage"/>
        <rdfs:label xml:lang="en">anaphora</rdfs:label>
    </owl:NamedIndividual>
    


    <!-- http://w3id.org/meta-share/meta-share/anaphoraResolution -->

    <owl:NamedIndividual rdf:about="http://w3id.org/meta-share/meta-share/anaphoraResolution">
        <rdf:type rdf:resource="http://w3id.org/meta-share/meta-share/LDTask"/>
        <rdfs:label xml:lang="en">anaphora resolution</rdfs:label>
    </owl:NamedIndividual>
    


    <!-- http://w3id.org/meta-share/meta-share/android -->

    <owl:NamedIndividual rdf:about="http://w3id.org/meta-share/meta-share/android">
        <rdf:type rdf:resource="http://w3id.org/meta-share/meta-share/OperatingSystem"/>
        <rdfs:label xml:lang="en">Android</rdfs:label>
    </owl:NamedIndividual>
    


    <!-- http://w3id.org/meta-share/meta-share/anechoicChamber -->

    <owl:NamedIndividual rdf:about="http://w3id.org/meta-share/meta-share/anechoicChamber">
        <rdf:type rdf:resource="http://w3id.org/meta-share/meta-share/RecordingEnvironment"/>
        <rdfs:label xml:lang="en">anechoic chamber</rdfs:label>
    </owl:NamedIndividual>
    


    <!-- http://w3id.org/meta-share/meta-share/animalVocalization -->

    <owl:NamedIndividual rdf:about="http://w3id.org/meta-share/meta-share/animalVocalization">
        <rdf:type rdf:resource="http://w3id.org/meta-share/meta-share/AudioGenre"/>
        <datacite:hasIdentifier rdf:resource="http://w3id.org/meta-share/meta-share/MS_AG006"/>
        <rdfs:label xml:lang="en">animal vocalization</rdfs:label>
    </owl:NamedIndividual>
    


    <!-- http://w3id.org/meta-share/meta-share/animalsZoology -->

    <owl:NamedIndividual rdf:about="http://w3id.org/meta-share/meta-share/animalsZoology">
        <rdf:type rdf:resource="http://w3id.org/meta-share/meta-share/Domain"/>
        <datacite:hasIdentifier rdf:resource="http://w3id.org/meta-share/meta-share/DDC590"/>
        <rdfs:label xml:lang="en">Animals (Zoology)</rdfs:label>
    </owl:NamedIndividual>
    


    <!-- http://w3id.org/meta-share/meta-share/annotatedCorpus -->

    <owl:NamedIndividual rdf:about="http://w3id.org/meta-share/meta-share/annotatedCorpus">
        <rdf:type rdf:resource="http://w3id.org/meta-share/meta-share/CorpusSubclass"/>
        <rdfs:comment xml:lang="en">A corpus that has been processed and thus includes the raw data and the automatic or manual annotations that have been added to them</rdfs:comment>
        <rdfs:label xml:lang="en">annotated corpus</rdfs:label>
    </owl:NamedIndividual>
    


    <!-- http://w3id.org/meta-share/meta-share/annotationScheme -->

    <owl:NamedIndividual rdf:about="http://w3id.org/meta-share/meta-share/annotationScheme">
        <rdf:type rdf:resource="http://w3id.org/meta-share/meta-share/LCRSubclass"/>
        <rdfs:comment xml:lang="en">A set of elements and values designed to annotate data. It usually consists in a formal representation. It aims to represent a specific level of information, such as morphological features of words, syntactic dependency relations between phrases, discourse level information , etc. It can consist of a flat structure of elements and values (e.g.,  part-of-speech tags) or it can be more complex with interrelated elements (e.g.,  specific morphological features to be used for each part-of-speech).</rdfs:comment>
        <rdfs:label xml:lang="en">annotation scheme</rdfs:label>
    </owl:NamedIndividual>
    


    <!-- http://w3id.org/meta-share/meta-share/annotationsCorpus -->

    <owl:NamedIndividual rdf:about="http://w3id.org/meta-share/meta-share/annotationsCorpus">
        <rdf:type rdf:resource="http://w3id.org/meta-share/meta-share/CorpusSubclass"/>
        <rdfs:comment xml:lang="en">A corpus of annotations without the raw data</rdfs:comment>
        <rdfs:label xml:lang="en">annotations corpus</rdfs:label>
    </owl:NamedIndividual>
    


    <!-- http://w3id.org/meta-share/meta-share/antonym -->

    <owl:NamedIndividual rdf:about="http://w3id.org/meta-share/meta-share/antonym">
        <rdf:type rdf:resource="http://w3id.org/meta-share/meta-share/SemanticType"/>
        <rdfs:label xml:lang="en">antonym</rdfs:label>
    </owl:NamedIndividual>
    


    <!-- http://w3id.org/meta-share/meta-share/apiSpecification -->

    <owl:NamedIndividual rdf:about="http://w3id.org/meta-share/meta-share/apiSpecification">
        <rdf:type rdf:resource="http://w3id.org/meta-share/meta-share/DocumentationType"/>
        <rdfs:comment xml:lang="en">Value for &apos;Documentation type&apos; used for the specification description of an API</rdfs:comment>
        <rdfs:label xml:lang="en">API specification</rdfs:label>
    </owl:NamedIndividual>
    


    <!-- http://w3id.org/meta-share/meta-share/applicationWord -->

    <owl:NamedIndividual rdf:about="http://w3id.org/meta-share/meta-share/applicationWord">
        <rdf:type rdf:resource="http://w3id.org/meta-share/meta-share/SpeechItem"/>
        <rdfs:label xml:lang="en">application word</rdfs:label>
    </owl:NamedIndividual>
    


    <!-- http://w3id.org/meta-share/meta-share/appliedPhysics -->

    <owl:NamedIndividual rdf:about="http://w3id.org/meta-share/meta-share/appliedPhysics">
        <rdf:type rdf:resource="http://w3id.org/meta-share/meta-share/Domain"/>
        <datacite:hasIdentifier rdf:resource="http://w3id.org/meta-share/meta-share/DDC621"/>
        <rdfs:label xml:lang="en">Applied Physics</rdfs:label>
    </owl:NamedIndividual>
    


    <!-- http://w3id.org/meta-share/meta-share/architecture -->

    <owl:NamedIndividual rdf:about="http://w3id.org/meta-share/meta-share/architecture">
        <rdf:type rdf:resource="http://w3id.org/meta-share/meta-share/Domain"/>
        <datacite:hasIdentifier rdf:resource="http://w3id.org/meta-share/meta-share/DDC720"/>
        <rdfs:label xml:lang="en">Architecture</rdfs:label>
    </owl:NamedIndividual>
    


    <!-- http://w3id.org/meta-share/meta-share/arm -->

    <owl:NamedIndividual rdf:about="http://w3id.org/meta-share/meta-share/arm">
        <rdf:type rdf:resource="http://w3id.org/meta-share/meta-share/BodyPart"/>
        <rdfs:label xml:lang="en">arm</rdfs:label>
    </owl:NamedIndividual>
    


    <!-- http://w3id.org/meta-share/meta-share/article -->

    <owl:NamedIndividual rdf:about="http://w3id.org/meta-share/meta-share/article">
        <rdf:type rdf:resource="http://w3id.org/meta-share/meta-share/SizeUnit"/>
        <rdfs:label xml:lang="en">article</rdfs:label>
    </owl:NamedIndividual>
    


    <!-- http://w3id.org/meta-share/meta-share/article1 -->

    <owl:NamedIndividual rdf:about="http://w3id.org/meta-share/meta-share/article1">
        <rdf:type rdf:resource="http://w3id.org/meta-share/meta-share/DocumentType"/>
        <rdfs:comment xml:lang="en">An article from a journal or magazine</rdfs:comment>
        <rdfs:label xml:lang="en">article</rdfs:label>
    </owl:NamedIndividual>
    


    <!-- http://w3id.org/meta-share/meta-share/artsAndRecreation -->

    <owl:NamedIndividual rdf:about="http://w3id.org/meta-share/meta-share/artsAndRecreation">
        <rdf:type rdf:resource="http://w3id.org/meta-share/meta-share/Domain"/>
        <datacite:hasIdentifier rdf:resource="http://w3id.org/meta-share/meta-share/DDC700"/>
        <rdfs:label xml:lang="en">Arts &amp; Recreation</rdfs:label>
    </owl:NamedIndividual>
    


    <!-- http://w3id.org/meta-share/meta-share/aspect -->

    <owl:NamedIndividual rdf:about="http://w3id.org/meta-share/meta-share/aspect">
        <rdf:type rdf:resource="http://w3id.org/meta-share/meta-share/MorphologicalType"/>
        <rdfs:label xml:lang="en">aspect</rdfs:label>
    </owl:NamedIndividual>
    


    <!-- http://w3id.org/meta-share/meta-share/assisted -->

    <owl:NamedIndividual rdf:about="http://w3id.org/meta-share/meta-share/assisted">
        <rdf:type rdf:resource="http://w3id.org/meta-share/meta-share/Naturality"/>
        <rdfs:label xml:lang="en">assisted</rdfs:label>
    </owl:NamedIndividual>
    


    <!-- http://w3id.org/meta-share/meta-share/association -->

    <owl:NamedIndividual rdf:about="http://w3id.org/meta-share/meta-share/association">
        <rdf:type rdf:resource="http://w3id.org/meta-share/meta-share/OrganizationLegalStatus"/>
        <rdfs:label xml:lang="en">association</rdfs:label>
    </owl:NamedIndividual>
    


    <!-- http://w3id.org/meta-share/meta-share/astronomy -->

    <owl:NamedIndividual rdf:about="http://w3id.org/meta-share/meta-share/astronomy">
        <rdf:type rdf:resource="http://w3id.org/meta-share/meta-share/Domain"/>
        <datacite:hasIdentifier rdf:resource="http://w3id.org/meta-share/meta-share/DDC520"/>
        <rdfs:label xml:lang="en">Astronomy</rdfs:label>
    </owl:NamedIndividual>
    


    <!-- http://w3id.org/meta-share/meta-share/atrac -->

    <owl:NamedIndividual rdf:about="http://w3id.org/meta-share/meta-share/atrac">
        <rdf:type rdf:resource="http://w3id.org/meta-share/meta-share/CompressionName"/>
        <rdfs:label xml:lang="en">altrac</rdfs:label>
    </owl:NamedIndividual>
    


    <!-- http://w3id.org/meta-share/meta-share/attached -->

    <owl:NamedIndividual rdf:about="http://w3id.org/meta-share/meta-share/attached">
        <rdf:type rdf:resource="http://w3id.org/meta-share/meta-share/RelatedLexiconType"/>
        <rdfs:label xml:lang="en">attached</rdfs:label>
    </owl:NamedIndividual>
    


    <!-- http://w3id.org/meta-share/meta-share/attribution -->

    <owl:NamedIndividual rdf:about="http://w3id.org/meta-share/meta-share/attribution">
        <rdf:type rdf:resource="http://w3id.org/meta-share/meta-share/ConditionOfUse"/>
        <rdf:type rdf:resource="http://www.w3.org/ns/odrl/2/Set"/>
        <rdfs:comment xml:lang="en">Value for &apos;ConditionOfUse&apos; that states that the use of a language resource must acknowledge it with an attribution note usually according to terms specified in the licensing document</rdfs:comment>
        <rdfs:label xml:lang="en">attribution</rdfs:label>
        <odrl:permission>
            <rdf:Description>
                <odrl:duty>
                    <rdf:Description>
                        <odrl:action rdf:resource="http://creativecommons.org/ns#Attribution"/>
                    </rdf:Description>
                </odrl:duty>
            </rdf:Description>
        </odrl:permission>
    </owl:NamedIndividual>
    


    <!-- http://w3id.org/meta-share/meta-share/audio -->

    <owl:NamedIndividual rdf:about="http://w3id.org/meta-share/meta-share/audio">
        <rdf:type rdf:resource="http://w3id.org/meta-share/meta-share/MediaType"/>
        <rdfs:comment xml:lang="en">Value for &apos;MediaType&apos; for the form of a language resource (part) composed of or relating to sound(s)</rdfs:comment>
        <rdfs:label xml:lang="en">audio</rdfs:label>
    </owl:NamedIndividual>
    


    <!-- http://w3id.org/meta-share/meta-share/automatic -->

    <owl:NamedIndividual rdf:about="http://w3id.org/meta-share/meta-share/automatic">
        <rdf:type rdf:resource="http://w3id.org/meta-share/meta-share/ProcessMode"/>
        <rdfs:comment xml:lang="en">Value for &apos;Process mode&apos; and its subclasses used for fully automatic processes where the results of the process have undergone no manual edits</rdfs:comment>
        <rdfs:label xml:lang="en">automatic</rdfs:label>
    </owl:NamedIndividual>
    


    <!-- http://w3id.org/meta-share/meta-share/automatic1 -->

    <owl:NamedIndividual rdf:about="http://w3id.org/meta-share/meta-share/automatic1">
        <rdf:type rdf:resource="http://w3id.org/meta-share/meta-share/EvaluationMeasure"/>
        <rdfs:label xml:lang="en">automatic</rdfs:label>
    </owl:NamedIndividual>
    


    <!-- http://w3id.org/meta-share/meta-share/auxiliary -->

    <owl:NamedIndividual rdf:about="http://w3id.org/meta-share/meta-share/auxiliary">
        <rdf:type rdf:resource="http://w3id.org/meta-share/meta-share/MorphologicalType"/>
        <rdfs:label xml:lang="en">auxiliary</rdfs:label>
    </owl:NamedIndividual>
    


    <!-- http://w3id.org/meta-share/meta-share/available -->

    <owl:NamedIndividual rdf:about="http://w3id.org/meta-share/meta-share/available">
        <rdf:type rdf:resource="http://w3id.org/meta-share/meta-share/Availability"/>
        <rdfs:comment xml:lang="en">For resources available through the infrastructure</rdfs:comment>
        <rdfs:label xml:lang="en">available</rdfs:label>
    </owl:NamedIndividual>
    


    <!-- http://w3id.org/meta-share/meta-share/availableThroughOtherDistributors -->

    <owl:NamedIndividual rdf:about="http://w3id.org/meta-share/meta-share/availableThroughOtherDistributors">
        <rdf:type rdf:resource="http://w3id.org/meta-share/meta-share/Availability"/>
        <rdfs:comment xml:lang="en">For resources that are available through other distribution channels</rdfs:comment>
        <rdfs:label xml:lang="en">available through other distributors</rdfs:label>
    </owl:NamedIndividual>
    


    <!-- http://w3id.org/meta-share/meta-share/avi -->

    <owl:NamedIndividual rdf:about="http://w3id.org/meta-share/meta-share/avi">
        <rdf:type rdf:resource="http://w3id.org/meta-share/meta-share/CompressionName"/>
        <rdfs:label xml:lang="en">avi</rdfs:label>
    </owl:NamedIndividual>
    


    <!-- http://w3id.org/meta-share/meta-share/backgroundNoise -->

    <owl:NamedIndividual rdf:about="http://w3id.org/meta-share/meta-share/backgroundNoise">
        <rdf:type rdf:resource="http://w3id.org/meta-share/meta-share/AudioQualityMeasureIncluded"/>
        <rdfs:label xml:lang="en">background noise</rdfs:label>
    </owl:NamedIndividual>
    


    <!-- http://w3id.org/meta-share/meta-share/backgroundNoise1 -->

    <owl:NamedIndividual rdf:about="http://w3id.org/meta-share/meta-share/backgroundNoise1">
        <rdf:type rdf:resource="http://w3id.org/meta-share/meta-share/AnnotatedElement"/>
        <rdfs:label xml:lang="en">background noise</rdfs:label>
    </owl:NamedIndividual>
    


    <!-- http://w3id.org/meta-share/meta-share/banking -->

    <owl:NamedIndividual rdf:about="http://w3id.org/meta-share/meta-share/banking">
        <rdf:type rdf:resource="http://w3id.org/meta-share/meta-share/Domain"/>
        <datacite:hasIdentifier rdf:resource="http://w3id.org/meta-share/meta-share/ELG_Domain014"/>
        <rdfs:label xml:lang="en">banking</rdfs:label>
    </owl:NamedIndividual>
    


    <!-- http://w3id.org/meta-share/meta-share/bigEndian -->

    <owl:NamedIndividual rdf:about="http://w3id.org/meta-share/meta-share/bigEndian">
        <rdf:type rdf:resource="http://w3id.org/meta-share/meta-share/ByteOrder"/>
        <rdfs:label xml:lang="en">Big Endian</rdfs:label>
    </owl:NamedIndividual>
    


    <!-- http://w3id.org/meta-share/meta-share/bigram -->

    <owl:NamedIndividual rdf:about="http://w3id.org/meta-share/meta-share/bigram">
        <rdf:type rdf:resource="http://w3id.org/meta-share/meta-share/SizeUnit"/>
        <rdfs:label xml:lang="en">bigram</rdfs:label>
    </owl:NamedIndividual>
    


    <!-- http://w3id.org/meta-share/meta-share/bilingual -->

    <owl:NamedIndividual rdf:about="http://w3id.org/meta-share/meta-share/bilingual">
        <rdf:type rdf:resource="http://w3id.org/meta-share/meta-share/LingualityType"/>
        <rdfs:comment xml:lang="en">Value for &apos;Linguality type&apos; for resource (parts) which include material in two languages</rdfs:comment>
        <rdfs:label xml:lang="en">bilingual</rdfs:label>
    </owl:NamedIndividual>
    


    <!-- http://w3id.org/meta-share/meta-share/biochemistry -->

    <owl:NamedIndividual rdf:about="http://w3id.org/meta-share/meta-share/biochemistry">
        <rdf:type rdf:resource="http://w3id.org/meta-share/meta-share/Domain"/>
        <datacite:hasIdentifier rdf:resource="http://w3id.org/meta-share/meta-share/DDC570"/>
        <rdfs:label xml:lang="en">Biochemistry</rdfs:label>
    </owl:NamedIndividual>
    


    <!-- http://w3id.org/meta-share/meta-share/biology -->

    <owl:NamedIndividual rdf:about="http://w3id.org/meta-share/meta-share/biology">
        <rdf:type rdf:resource="http://w3id.org/meta-share/meta-share/Domain"/>
        <datacite:hasIdentifier rdf:resource="http://w3id.org/meta-share/meta-share/DDC570"/>
        <rdfs:label xml:lang="en">Biology</rdfs:label>
    </owl:NamedIndividual>
    


    <!-- http://w3id.org/meta-share/meta-share/blackBox -->

    <owl:NamedIndividual rdf:about="http://w3id.org/meta-share/meta-share/blackBox">
        <rdf:type rdf:resource="http://w3id.org/meta-share/meta-share/EvaluationType"/>
        <rdfs:label xml:lang="en">black box</rdfs:label>
    </owl:NamedIndividual>
    


    <!-- http://w3id.org/meta-share/meta-share/blogText -->

    <owl:NamedIndividual rdf:about="http://w3id.org/meta-share/meta-share/blogText">
        <rdf:type rdf:resource="http://w3id.org/meta-share/meta-share/TextType"/>
        <datacite:hasIdentifier rdf:resource="http://w3id.org/meta-share/meta-share/ClarinEl_TT002"/>
        <rdfs:label xml:lang="en">blog text</rdfs:label>
    </owl:NamedIndividual>
    


    <!-- http://w3id.org/meta-share/meta-share/bluRay -->

    <owl:NamedIndividual rdf:about="http://w3id.org/meta-share/meta-share/bluRay">
        <rdf:type rdf:resource="http://w3id.org/meta-share/meta-share/DatasetDistributionForm"/>
        <rdfs:comment xml:lang="en">bluRay refers to a kind of distribution/access medium used for delivering a language resource; intended for resources delivered on bluRay disks</rdfs:comment>
        <rdfs:label xml:lang="en">bluRay</rdfs:label>
    </owl:NamedIndividual>
    


    <!-- http://w3id.org/meta-share/meta-share/bodyGesture -->

    <owl:NamedIndividual rdf:about="http://w3id.org/meta-share/meta-share/bodyGesture">
        <rdf:type rdf:resource="http://w3id.org/meta-share/meta-share/ModalityType"/>
        <rdfs:comment xml:lang="en">Value for &apos;ModalityType&apos; for body gestures represented in a language resource</rdfs:comment>
        <rdfs:label xml:lang="en">body gesture</rdfs:label>
    </owl:NamedIndividual>
    


    <!-- http://w3id.org/meta-share/meta-share/book -->

    <owl:NamedIndividual rdf:about="http://w3id.org/meta-share/meta-share/book">
        <rdf:type rdf:resource="http://w3id.org/meta-share/meta-share/DocumentType"/>
        <rdfs:label xml:lang="en">book</rdfs:label>
    </owl:NamedIndividual>
    


    <!-- http://w3id.org/meta-share/meta-share/booklet -->

    <owl:NamedIndividual rdf:about="http://w3id.org/meta-share/meta-share/booklet">
        <rdf:type rdf:resource="http://w3id.org/meta-share/meta-share/DocumentType"/>
        <rdfs:label xml:lang="en">booklet</rdfs:label>
    </owl:NamedIndividual>
    


    <!-- http://w3id.org/meta-share/meta-share/boolean -->

    <owl:NamedIndividual rdf:about="http://w3id.org/meta-share/meta-share/boolean">
        <rdf:type rdf:resource="http://w3id.org/meta-share/meta-share/ParameterType"/>
        <rdfs:label xml:lang="en">boolean</rdfs:label>
    </owl:NamedIndividual>
    


    <!-- http://w3id.org/meta-share/meta-share/branch -->

    <owl:NamedIndividual rdf:about="http://w3id.org/meta-share/meta-share/branch">
        <rdf:type rdf:resource="http://w3id.org/meta-share/meta-share/DivisionCategory"/>
        <rdfs:label xml:lang="en">branch</rdfs:label>
    </owl:NamedIndividual>
    


    <!-- http://w3id.org/meta-share/meta-share/broadcastNews -->

    <owl:NamedIndividual rdf:about="http://w3id.org/meta-share/meta-share/broadcastNews">
        <rdf:type rdf:resource="http://w3id.org/meta-share/meta-share/SpeechGenre"/>
        <datacite:hasIdentifier rdf:resource="http://w3id.org/meta-share/meta-share/MS_SG009"/>
        <rdfs:label xml:lang="en">broadcast news</rdfs:label>
    </owl:NamedIndividual>
    


    <!-- http://w3id.org/meta-share/meta-share/business -->

    <owl:NamedIndividual rdf:about="http://w3id.org/meta-share/meta-share/business">
        <rdf:type rdf:resource="http://w3id.org/meta-share/meta-share/Domain"/>
        <datacite:hasIdentifier rdf:resource="http://w3id.org/meta-share/meta-share/ELG_Domain011"/>
        <rdfs:label xml:lang="en">business</rdfs:label>
    </owl:NamedIndividual>
    


    <!-- http://w3id.org/meta-share/meta-share/byte -->

    <owl:NamedIndividual rdf:about="http://w3id.org/meta-share/meta-share/byte">
        <rdf:type rdf:resource="http://w3id.org/meta-share/meta-share/SizeUnit"/>
        <rdfs:label xml:lang="en">byte</rdfs:label>
    </owl:NamedIndividual>
    


    <!-- http://w3id.org/meta-share/meta-share/callIn -->

    <owl:NamedIndividual rdf:about="http://w3id.org/meta-share/meta-share/callIn">
        <rdf:type rdf:resource="http://w3id.org/meta-share/meta-share/SpeechGenre"/>
        <datacite:hasIdentifier rdf:resource="http://w3id.org/meta-share/meta-share/MS_SG002"/>
        <rdfs:label xml:lang="en">call-in</rdfs:label>
    </owl:NamedIndividual>
    


    <!-- http://w3id.org/meta-share/meta-share/camcorder -->

    <owl:NamedIndividual rdf:about="http://w3id.org/meta-share/meta-share/camcorder">
        <rdf:type rdf:resource="http://w3id.org/meta-share/meta-share/SourceChannel"/>
        <rdfs:label xml:lang="en">camcorder</rdfs:label>
    </owl:NamedIndividual>
    


    <!-- http://w3id.org/meta-share/meta-share/camera -->

    <owl:NamedIndividual rdf:about="http://w3id.org/meta-share/meta-share/camera">
        <rdf:type rdf:resource="http://w3id.org/meta-share/meta-share/CapturingDeviceType"/>
        <rdfs:label xml:lang="en">camera</rdfs:label>
    </owl:NamedIndividual>
    


    <!-- http://w3id.org/meta-share/meta-share/caption -->

    <owl:NamedIndividual rdf:about="http://w3id.org/meta-share/meta-share/caption">
        <rdf:type rdf:resource="http://w3id.org/meta-share/meta-share/TextIncludedInImage"/>
        <rdfs:label xml:lang="en">caption</rdfs:label>
    </owl:NamedIndividual>
    


    <!-- http://w3id.org/meta-share/meta-share/caption1 -->

    <owl:NamedIndividual rdf:about="http://w3id.org/meta-share/meta-share/caption1">
        <rdf:type rdf:resource="http://w3id.org/meta-share/meta-share/TextIncludedInVideo"/>
        <rdfs:label xml:lang="en">caption</rdfs:label>
    </owl:NamedIndividual>
    


    <!-- http://w3id.org/meta-share/meta-share/captureTime -->

    <owl:NamedIndividual rdf:about="http://w3id.org/meta-share/meta-share/captureTime">
        <rdf:type rdf:resource="http://w3id.org/meta-share/meta-share/TextIncludedInImage"/>
        <rdfs:label xml:lang="en">capture time</rdfs:label>
    </owl:NamedIndividual>
    


    <!-- http://w3id.org/meta-share/meta-share/case -->

    <owl:NamedIndividual rdf:about="http://w3id.org/meta-share/meta-share/case">
        <rdf:type rdf:resource="http://w3id.org/meta-share/meta-share/MorphologicalType"/>
        <rdfs:label xml:lang="en">case</rdfs:label>
    </owl:NamedIndividual>
    


    <!-- http://w3id.org/meta-share/meta-share/chatText -->

    <owl:NamedIndividual rdf:about="http://w3id.org/meta-share/meta-share/chatText">
        <rdf:type rdf:resource="http://w3id.org/meta-share/meta-share/TextType"/>
        <datacite:hasIdentifier rdf:resource="http://w3id.org/meta-share/meta-share/ClarinEl_TT014"/>
        <rdfs:label xml:lang="en">chat text</rdfs:label>
    </owl:NamedIndividual>
    


    <!-- http://w3id.org/meta-share/meta-share/chemicalEngineering -->

    <owl:NamedIndividual rdf:about="http://w3id.org/meta-share/meta-share/chemicalEngineering">
        <rdf:type rdf:resource="http://w3id.org/meta-share/meta-share/Domain"/>
        <datacite:hasIdentifier rdf:resource="http://w3id.org/meta-share/meta-share/DDC660"/>
        <rdfs:label xml:lang="en">Chemical Engineering</rdfs:label>
    </owl:NamedIndividual>
    


    <!-- http://w3id.org/meta-share/meta-share/chemistry -->

    <owl:NamedIndividual rdf:about="http://w3id.org/meta-share/meta-share/chemistry">
        <rdf:type rdf:resource="http://w3id.org/meta-share/meta-share/Domain"/>
        <datacite:hasIdentifier rdf:resource="http://w3id.org/meta-share/meta-share/DDC540"/>
        <rdfs:label xml:lang="en">Chemistry</rdfs:label>
    </owl:NamedIndividual>
    


    <!-- http://w3id.org/meta-share/meta-share/child -->

    <owl:NamedIndividual rdf:about="http://w3id.org/meta-share/meta-share/child">
        <rdf:type rdf:resource="http://w3id.org/meta-share/meta-share/AgeGroup"/>
        <rdfs:label xml:lang="en">child</rdfs:label>
    </owl:NamedIndividual>
    


    <!-- http://w3id.org/meta-share/meta-share/chunking -->

    <owl:NamedIndividual rdf:about="http://w3id.org/meta-share/meta-share/chunking">
        <rdf:type rdf:resource="http://w3id.org/meta-share/meta-share/LDTask"/>
        <rdfs:label xml:lang="en">chunking</rdfs:label>
    </owl:NamedIndividual>
    


    <!-- http://w3id.org/meta-share/meta-share/class -->

    <owl:NamedIndividual rdf:about="http://w3id.org/meta-share/meta-share/class">
        <rdf:type rdf:resource="http://w3id.org/meta-share/meta-share/SizeUnit"/>
        <rdfs:label xml:lang="en">class</rdfs:label>
    </owl:NamedIndividual>
    


    <!-- http://w3id.org/meta-share/meta-share/clause -->

    <owl:NamedIndividual rdf:about="http://w3id.org/meta-share/meta-share/clause">
        <rdf:type rdf:resource="http://w3id.org/meta-share/meta-share/SegmentationLevel"/>
        <rdfs:label xml:lang="en">clause</rdfs:label>
    </owl:NamedIndividual>
    


    <!-- http://w3id.org/meta-share/meta-share/clauseStructure -->

    <owl:NamedIndividual rdf:about="http://w3id.org/meta-share/meta-share/clauseStructure">
        <rdf:type rdf:resource="http://w3id.org/meta-share/meta-share/GrammaticalPhenomenaCoverage"/>
        <rdfs:label xml:lang="en">clause structure</rdfs:label>
    </owl:NamedIndividual>
    


    <!-- http://w3id.org/meta-share/meta-share/clippingRate -->

    <owl:NamedIndividual rdf:about="http://w3id.org/meta-share/meta-share/clippingRate">
        <rdf:type rdf:resource="http://w3id.org/meta-share/meta-share/AudioQualityMeasureIncluded"/>
        <rdfs:label xml:lang="en">clipping rate</rdfs:label>
    </owl:NamedIndividual>
    


    <!-- http://w3id.org/meta-share/meta-share/cliticForm -->

    <owl:NamedIndividual rdf:about="http://w3id.org/meta-share/meta-share/cliticForm">
        <rdf:type rdf:resource="http://w3id.org/meta-share/meta-share/LemmaType"/>
        <rdfs:altLabel xml:lang="en">inflectional form</rdfs:altLabel>
        <rdfs:label xml:lang="en">clitic form</rdfs:label>
    </owl:NamedIndividual>
    


    <!-- http://w3id.org/meta-share/meta-share/closeTalkMicrophone -->

    <owl:NamedIndividual rdf:about="http://w3id.org/meta-share/meta-share/closeTalkMicrophone">
        <rdf:type rdf:resource="http://w3id.org/meta-share/meta-share/CapturingDeviceType"/>
        <rdfs:label xml:lang="en">close talk microphone</rdfs:label>
    </owl:NamedIndividual>
    


    <!-- http://w3id.org/meta-share/meta-share/closedPublicPlace -->

    <owl:NamedIndividual rdf:about="http://w3id.org/meta-share/meta-share/closedPublicPlace">
        <rdf:type rdf:resource="http://w3id.org/meta-share/meta-share/RecordingEnvironment"/>
        <rdfs:label xml:lang="en">closed public place</rdfs:label>
    </owl:NamedIndividual>
    


    <!-- http://w3id.org/meta-share/meta-share/collocation -->

    <owl:NamedIndividual rdf:about="http://w3id.org/meta-share/meta-share/collocation">
        <rdf:type rdf:resource="http://w3id.org/meta-share/meta-share/UsageType"/>
        <rdfs:label xml:lang="en">collocation</rdfs:label>
    </owl:NamedIndividual>
    


    <!-- http://w3id.org/meta-share/meta-share/combinationOfModalities -->

    <owl:NamedIndividual rdf:about="http://w3id.org/meta-share/meta-share/combinationOfModalities">
        <rdf:type rdf:resource="http://w3id.org/meta-share/meta-share/ModalityType"/>
        <rdfs:comment xml:lang="en">Value for &apos;ModalityType&apos; for language resources that include various modalities</rdfs:comment>
        <rdfs:label xml:lang="en">combination of modalities</rdfs:label>
    </owl:NamedIndividual>
    


    <!-- http://w3id.org/meta-share/meta-share/commerceTrade -->

    <owl:NamedIndividual rdf:about="http://w3id.org/meta-share/meta-share/commerceTrade">
        <rdf:type rdf:resource="http://w3id.org/meta-share/meta-share/Domain"/>
        <datacite:hasIdentifier rdf:resource="http://w3id.org/meta-share/meta-share/DDC381"/>
        <rdfs:label xml:lang="en">Commerce (Trade)</rdfs:label>
    </owl:NamedIndividual>
    


    <!-- http://w3id.org/meta-share/meta-share/commercial -->

    <owl:NamedIndividual rdf:about="http://w3id.org/meta-share/meta-share/commercial">
        <rdf:type rdf:resource="http://w3id.org/meta-share/meta-share/UserType"/>
        <rdfs:comment xml:lang="en">Value for &apos;user type&apos; reserved for individuals affiliated with a commercial institution and the respective organisations</rdfs:comment>
        <rdfs:label xml:lang="en">commercial</rdfs:label>
    </owl:NamedIndividual>
    


    <!-- http://w3id.org/meta-share/meta-share/commercial1 -->

    <owl:NamedIndividual rdf:about="http://w3id.org/meta-share/meta-share/commercial1">
        <rdf:type rdf:resource="http://w3id.org/meta-share/meta-share/NonSpeechItem"/>
        <rdfs:comment xml:lang="en">Value for non-speech item, used for commercials (advertisements)</rdfs:comment>
        <rdfs:label xml:lang="en">commercial</rdfs:label>
    </owl:NamedIndividual>
    


    <!-- http://w3id.org/meta-share/meta-share/commercialUser -->

    <owl:NamedIndividual rdf:about="http://w3id.org/meta-share/meta-share/commercialUser">
        <rdf:type rdf:resource="http://w3id.org/meta-share/meta-share/ConditionOfUse"/>
        <rdfs:label xml:lang="en">commercial user</rdfs:label>
    </owl:NamedIndividual>
    


    <!-- http://w3id.org/meta-share/meta-share/communicate -->

    <owl:NamedIndividual rdf:about="http://w3id.org/meta-share/meta-share/communicate">
        <rdf:type rdf:resource="http://www.w3.org/2004/02/skos/core#concept"/>
        <rdfs:comment xml:lang="en">The Assigner permits/prohibits the Assignees to communicate the Asset to the public</rdfs:comment>
        <rdfs:label xml:lang="en">communicate</rdfs:label>
        <skos:closeMatch rdf:resource="http://www.w3.org/ns/odrl/2/present"/>
    </owl:NamedIndividual>
    


    <!-- http://w3id.org/meta-share/meta-share/communications -->

    <owl:NamedIndividual rdf:about="http://w3id.org/meta-share/meta-share/communications">
        <rdf:type rdf:resource="http://w3id.org/meta-share/meta-share/Domain"/>
        <datacite:hasIdentifier rdf:resource="http://w3id.org/meta-share/meta-share/DDC384"/>
        <rdfs:label xml:lang="en">Communications</rdfs:label>
    </owl:NamedIndividual>
    


    <!-- http://w3id.org/meta-share/meta-share/comparable -->

    <owl:NamedIndividual rdf:about="http://w3id.org/meta-share/meta-share/comparable">
        <rdf:type rdf:resource="http://w3id.org/meta-share/meta-share/MultilingualityType"/>
        <rdfs:comment xml:lang="en">Value for &apos;Multilinguality type&apos; for resource parts or resources that consist of the similar text segments in two or more languages (e.g.,  a corpus of legislation texts in Greek and English)</rdfs:comment>
        <rdfs:label xml:lang="en">comparable</rdfs:label>
    </owl:NamedIndividual>
    


    <!-- http://w3id.org/meta-share/meta-share/compatible -->

    <owl:NamedIndividual rdf:about="http://w3id.org/meta-share/meta-share/compatible">
        <rdf:type rdf:resource="http://w3id.org/meta-share/meta-share/RelatedLexiconType"/>
        <rdfs:label xml:lang="en">compatible</rdfs:label>
    </owl:NamedIndividual>
    


    <!-- http://w3id.org/meta-share/meta-share/complex -->

    <owl:NamedIndividual rdf:about="http://w3id.org/meta-share/meta-share/complex">
        <rdf:type rdf:resource="http://w3id.org/meta-share/meta-share/CapturingEnvironment"/>
        <rdfs:label xml:lang="en">complex</rdfs:label>
    </owl:NamedIndividual>
    


    <!-- http://w3id.org/meta-share/meta-share/component1 -->

    <owl:NamedIndividual rdf:about="http://w3id.org/meta-share/meta-share/component1">
        <rdf:type rdf:resource="http://w3id.org/meta-share/meta-share/ParameterType"/>
        <rdfs:label xml:lang="en">component</rdfs:label>
    </owl:NamedIndividual>
    


    <!-- http://w3id.org/meta-share/meta-share/compound -->

    <owl:NamedIndividual rdf:about="http://w3id.org/meta-share/meta-share/compound">
        <rdf:type rdf:resource="http://w3id.org/meta-share/meta-share/LemmaType"/>
        <rdfs:label xml:lang="en">compound</rdfs:label>
    </owl:NamedIndividual>
    


    <!-- http://w3id.org/meta-share/meta-share/computationalLexicon -->

    <owl:NamedIndividual rdf:about="http://w3id.org/meta-share/meta-share/computationalLexicon">
        <rdf:type rdf:resource="http://w3id.org/meta-share/meta-share/LCRSubclass"/>
        <rdfs:comment xml:lang="en">A lexicon which is intended for computational purposes and thus contains words associated with information relevant for the specific purposes</rdfs:comment>
        <rdfs:label xml:lang="en">computational lexicon</rdfs:label>
    </owl:NamedIndividual>
    


    <!-- http://w3id.org/meta-share/meta-share/computerScienceInformationGeneralWorks -->

    <owl:NamedIndividual rdf:about="http://w3id.org/meta-share/meta-share/computerScienceInformationGeneralWorks">
        <rdf:type rdf:resource="http://w3id.org/meta-share/meta-share/Domain"/>
        <datacite:hasIdentifier rdf:resource="http://w3id.org/meta-share/meta-share/DDC000"/>
        <rdfs:label xml:lang="en">Computer Science, Information &amp; General Works</rdfs:label>
    </owl:NamedIndividual>
    


    <!-- http://w3id.org/meta-share/meta-share/concept -->

    <owl:NamedIndividual rdf:about="http://w3id.org/meta-share/meta-share/concept">
        <rdf:type rdf:resource="http://w3id.org/meta-share/meta-share/SizeUnit"/>
        <rdfs:label xml:lang="en">concept</rdfs:label>
    </owl:NamedIndividual>
    


    <!-- http://w3id.org/meta-share/meta-share/conferenceRoom -->

    <owl:NamedIndividual rdf:about="http://w3id.org/meta-share/meta-share/conferenceRoom">
        <rdf:type rdf:resource="http://w3id.org/meta-share/meta-share/RecordingEnvironment"/>
        <rdfs:label xml:lang="en">conference room</rdfs:label>
    </owl:NamedIndividual>
    


    <!-- http://w3id.org/meta-share/meta-share/constructionOfBuildings -->

    <owl:NamedIndividual rdf:about="http://w3id.org/meta-share/meta-share/constructionOfBuildings">
        <rdf:type rdf:resource="http://w3id.org/meta-share/meta-share/Domain"/>
        <datacite:hasIdentifier rdf:resource="http://w3id.org/meta-share/meta-share/DDC690"/>
        <rdfs:label xml:lang="en">Construction of Buildings</rdfs:label>
    </owl:NamedIndividual>
    


    <!-- http://w3id.org/meta-share/meta-share/consultingFirm -->

    <owl:NamedIndividual rdf:about="http://w3id.org/meta-share/meta-share/consultingFirm">
        <rdf:type rdf:resource="http://w3id.org/meta-share/meta-share/OrganizationRole"/>
        <rdfs:label xml:lang="en">consulting firm</rdfs:label>
    </owl:NamedIndividual>
    


    <!-- http://w3id.org/meta-share/meta-share/content -->

    <owl:NamedIndividual rdf:about="http://w3id.org/meta-share/meta-share/content">
        <rdf:type rdf:resource="http://w3id.org/meta-share/meta-share/ValidationType"/>
        <rdfs:comment xml:lang="en">Value for &apos;Validation type&apos; indicating that the validation is performed on the contents of the resource</rdfs:comment>
        <rdfs:label xml:lang="en">content</rdfs:label>
    </owl:NamedIndividual>
    


    <!-- http://w3id.org/meta-share/meta-share/conversation -->

    <owl:NamedIndividual rdf:about="http://w3id.org/meta-share/meta-share/conversation">
        <rdf:type rdf:resource="http://w3id.org/meta-share/meta-share/SpeechGenre"/>
        <datacite:hasIdentifier rdf:resource="http://w3id.org/meta-share/meta-share/MS_SG012"/>
        <rdfs:label xml:lang="en">conversation</rdfs:label>
    </owl:NamedIndividual>
    


    <!-- http://w3id.org/meta-share/meta-share/coordination -->

    <owl:NamedIndividual rdf:about="http://w3id.org/meta-share/meta-share/coordination">
        <rdf:type rdf:resource="http://w3id.org/meta-share/meta-share/GrammaticalPhenomenaCoverage"/>
        <rdfs:label xml:lang="en">coordination</rdfs:label>
    </owl:NamedIndividual>
    


    <!-- http://w3id.org/meta-share/meta-share/copyrightNotEvaluated -->

    <owl:NamedIndividual rdf:about="http://w3id.org/meta-share/meta-share/copyrightNotEvaluated">
        <rdf:type rdf:resource="http://w3id.org/meta-share/meta-share/AccessRightsStatement"/>
        <datacite:hasIdentifier rdf:resource="http://rightsstatements.org/vocab/CNE/1.0/"/>
    </owl:NamedIndividual>
    


    <!-- http://w3id.org/meta-share/meta-share/copyrightUndetermined -->

    <owl:NamedIndividual rdf:about="http://w3id.org/meta-share/meta-share/copyrightUndetermined">
        <rdf:type rdf:resource="http://w3id.org/meta-share/meta-share/AccessRightsStatement"/>
        <datacite:hasIdentifier rdf:resource="http://rightsstatements.org/vocab/UND/1.0/"/>
    </owl:NamedIndividual>
    


    <!-- http://w3id.org/meta-share/meta-share/cordis -->

    <owl:NamedIndividual rdf:about="http://w3id.org/meta-share/meta-share/cordis">
        <rdf:type rdf:resource="http://w3id.org/meta-share/meta-share/ProjectIdentifierScheme"/>
        <rdfs:altLabel xml:lang="en">rcn</rdfs:altLabel>
        <rdfs:label xml:lang="en">cordis</rdfs:label>
    </owl:NamedIndividual>
    


    <!-- http://w3id.org/meta-share/meta-share/corpora -->

    <owl:NamedIndividual rdf:about="http://w3id.org/meta-share/meta-share/corpora">
        <rdf:type rdf:resource="http://w3id.org/meta-share/meta-share/ParameterType"/>
        <rdfs:label xml:lang="en">corpora</rdfs:label>
    </owl:NamedIndividual>
    


    <!-- http://w3id.org/meta-share/meta-share/corpus -->

    <owl:NamedIndividual rdf:about="http://w3id.org/meta-share/meta-share/corpus">
        <rdf:type rdf:resource="http://w3id.org/meta-share/meta-share/ProcessingResourceType"/>
        <rdfs:comment xml:lang="en">Value for &apos;Resource type&apos; for corpora, i.e. sets of datafiles (e.g.,  texts, audio recordings, videos, images, photographs, etc.)</rdfs:comment>
        <rdfs:label xml:lang="en">corpus</rdfs:label>
    </owl:NamedIndividual>
    


    <!-- http://w3id.org/meta-share/meta-share/creditCardNumber -->

    <owl:NamedIndividual rdf:about="http://w3id.org/meta-share/meta-share/creditCardNumber">
        <rdf:type rdf:resource="http://w3id.org/meta-share/meta-share/SpeechItem"/>
        <rdfs:label xml:lang="en">credit card number</rdfs:label>
    </owl:NamedIndividual>
    


    <!-- http://w3id.org/meta-share/meta-share/crossReference -->

    <owl:NamedIndividual rdf:about="http://w3id.org/meta-share/meta-share/crossReference">
        <rdf:type rdf:resource="http://w3id.org/meta-share/meta-share/SemanticType"/>
        <rdfs:label xml:lang="en">cross-reference</rdfs:label>
    </owl:NamedIndividual>
    


    <!-- http://w3id.org/meta-share/meta-share/crossTalk -->

    <owl:NamedIndividual rdf:about="http://w3id.org/meta-share/meta-share/crossTalk">
        <rdf:type rdf:resource="http://w3id.org/meta-share/meta-share/AudioQualityMeasureIncluded"/>
        <rdfs:label xml:lang="en">cross talk</rdfs:label>
    </owl:NamedIndividual>
    


    <!-- http://w3id.org/meta-share/meta-share/culture -->

    <owl:NamedIndividual rdf:about="http://w3id.org/meta-share/meta-share/culture">
        <rdf:type rdf:resource="http://w3id.org/meta-share/meta-share/Domain"/>
        <datacite:hasIdentifier rdf:resource="http://w3id.org/meta-share/meta-share/Clarin_Domain004"/>
        <rdfs:label xml:lang="en">culture</rdfs:label>
    </owl:NamedIndividual>
    


    <!-- http://w3id.org/meta-share/meta-share/data -->

    <owl:NamedIndividual rdf:about="http://w3id.org/meta-share/meta-share/data">
        <rdf:type rdf:resource="http://w3id.org/meta-share/meta-share/ParameterType"/>
        <rdfs:label xml:lang="en">data</rdfs:label>
    </owl:NamedIndividual>
    


    <!-- http://w3id.org/meta-share/meta-share/dataEvaluator -->

    <owl:NamedIndividual rdf:about="http://w3id.org/meta-share/meta-share/dataEvaluator">
        <rdf:type rdf:resource="http://w3id.org/meta-share/meta-share/OrganizationRole"/>
        <rdfs:label xml:lang="en">data evaluator</rdfs:label>
    </owl:NamedIndividual>
    


    <!-- http://w3id.org/meta-share/meta-share/daylight -->

    <owl:NamedIndividual rdf:about="http://w3id.org/meta-share/meta-share/daylight">
        <rdf:type rdf:resource="http://w3id.org/meta-share/meta-share/SceneIllumination"/>
        <rdfs:label xml:lang="en">daylight</rdfs:label>
    </owl:NamedIndividual>
    


    <!-- http://w3id.org/meta-share/meta-share/debate -->

    <owl:NamedIndividual rdf:about="http://w3id.org/meta-share/meta-share/debate">
        <rdf:type rdf:resource="http://w3id.org/meta-share/meta-share/SpeechGenre"/>
        <datacite:hasIdentifier rdf:resource="http://w3id.org/meta-share/meta-share/MS_SG013"/>
        <rdfs:label xml:lang="en">debate</rdfs:label>
    </owl:NamedIndividual>
    


    <!-- http://w3id.org/meta-share/meta-share/defence -->

    <owl:NamedIndividual rdf:about="http://w3id.org/meta-share/meta-share/defence">
        <rdf:type rdf:resource="http://w3id.org/meta-share/meta-share/Domain"/>
        <datacite:hasIdentifier rdf:resource="http://w3id.org/meta-share/meta-share/ELG_Domain010"/>
        <rdfs:label xml:lang="en">defence</rdfs:label>
    </owl:NamedIndividual>
    


    <!-- http://w3id.org/meta-share/meta-share/definition -->

    <owl:NamedIndividual rdf:about="http://w3id.org/meta-share/meta-share/definition">
        <rdf:type rdf:resource="http://w3id.org/meta-share/meta-share/SemanticType"/>
        <rdfs:altLabel xml:lang="en">gloss</rdfs:altLabel>
        <rdfs:label xml:lang="en">definition</rdfs:label>
    </owl:NamedIndividual>
    


    <!-- http://w3id.org/meta-share/meta-share/definitionsParsing -->

    <owl:NamedIndividual rdf:about="http://w3id.org/meta-share/meta-share/definitionsParsing">
        <rdf:type rdf:resource="http://w3id.org/meta-share/meta-share/LDTask"/>
        <rdfs:label xml:lang="en">parsing of definitions</rdfs:label>
    </owl:NamedIndividual>
    


    <!-- http://w3id.org/meta-share/meta-share/degree -->

    <owl:NamedIndividual rdf:about="http://w3id.org/meta-share/meta-share/degree">
        <rdf:type rdf:resource="http://w3id.org/meta-share/meta-share/MorphologicalType"/>
        <rdfs:label xml:lang="en">degree</rdfs:label>
    </owl:NamedIndividual>
    


    <!-- http://w3id.org/meta-share/meta-share/demoResource -->

    <owl:NamedIndividual rdf:about="http://w3id.org/meta-share/meta-share/demoResource">
        <rdf:type rdf:resource="http://w3id.org/meta-share/meta-share/DocumentationType"/>
        <rdfs:comment xml:lang="en">Value for &apos;DocumentationType&apos; used for demos of a resource available usually through the internet (e.g.,  video demos)</rdfs:comment>
        <rdfs:label xml:lang="en">demo resource</rdfs:label>
    </owl:NamedIndividual>
    


    <!-- http://w3id.org/meta-share/meta-share/dentalProsthesis -->

    <owl:NamedIndividual rdf:about="http://w3id.org/meta-share/meta-share/dentalProsthesis">
        <rdf:type rdf:resource="http://w3id.org/meta-share/meta-share/VocalTractCondition"/>
        <rdfs:label xml:lang="en">dental prosthesis</rdfs:label>
    </owl:NamedIndividual>
    


    <!-- http://w3id.org/meta-share/meta-share/department -->

    <owl:NamedIndividual rdf:about="http://w3id.org/meta-share/meta-share/department">
        <rdf:type rdf:resource="http://w3id.org/meta-share/meta-share/DivisionCategory"/>
        <rdfs:label xml:lang="en">department</rdfs:label>
    </owl:NamedIndividual>
    


    <!-- http://w3id.org/meta-share/meta-share/derivation -->

    <owl:NamedIndividual rdf:about="http://w3id.org/meta-share/meta-share/derivation">
        <rdf:type rdf:resource="http://w3id.org/meta-share/meta-share/MorphologicalType"/>
        <rdfs:label xml:lang="en">derivation</rdfs:label>
    </owl:NamedIndividual>
    


    <!-- http://w3id.org/meta-share/meta-share/diagnostic -->

    <owl:NamedIndividual rdf:about="http://w3id.org/meta-share/meta-share/diagnostic">
        <rdf:type rdf:resource="http://w3id.org/meta-share/meta-share/EvaluationLevel"/>
        <rdfs:label xml:lang="en">diagnostic</rdfs:label>
    </owl:NamedIndividual>
    


    <!-- http://w3id.org/meta-share/meta-share/dialect -->

    <owl:NamedIndividual rdf:about="http://w3id.org/meta-share/meta-share/dialect">
        <rdf:type rdf:resource="http://w3id.org/meta-share/meta-share/LanguageVarietyType"/>
        <rdfs:comment xml:lang="en">Value for &apos;LanguageVarietyType&apos; used for a particular form of a language which is peculiar to a specific region or social group</rdfs:comment>
        <rdfs:label xml:lang="en">dialect</rdfs:label>
    </owl:NamedIndividual>
    


    <!-- http://w3id.org/meta-share/meta-share/dialogue -->

    <owl:NamedIndividual rdf:about="http://w3id.org/meta-share/meta-share/dialogue">
        <rdf:type rdf:resource="http://w3id.org/meta-share/meta-share/ConversationalType"/>
        <rdfs:label xml:lang="en">dialogue</rdfs:label>
    </owl:NamedIndividual>
    


    <!-- http://w3id.org/meta-share/meta-share/dictionary -->

    <owl:NamedIndividual rdf:about="http://w3id.org/meta-share/meta-share/dictionary">
        <rdf:type rdf:resource="http://w3id.org/meta-share/meta-share/LCRSubclass"/>
        <rdfs:comment xml:lang="en">A book or electronic resource that contains a list of words (usually in alphabetical order) and explains their meanings, or gives a word for them in another language and other information (e.g.,  spelling, pronunciation, etc.)</rdfs:comment>
        <rdfs:label xml:lang="en">dictionary</rdfs:label>
    </owl:NamedIndividual>
    


    <!-- http://w3id.org/meta-share/meta-share/diphone -->

    <owl:NamedIndividual rdf:about="http://w3id.org/meta-share/meta-share/diphone">
        <rdf:type rdf:resource="http://w3id.org/meta-share/meta-share/SegmentationLevel"/>
        <rdfs:label xml:lang="en">diphone</rdfs:label>
    </owl:NamedIndividual>
    


    <!-- http://w3id.org/meta-share/meta-share/diphone1 -->

    <owl:NamedIndividual rdf:about="http://w3id.org/meta-share/meta-share/diphone1">
        <rdf:type rdf:resource="http://w3id.org/meta-share/meta-share/SizeUnit"/>
        <rdfs:label xml:lang="en">diphone</rdfs:label>
    </owl:NamedIndividual>
    


    <!-- http://w3id.org/meta-share/meta-share/disasterManagement -->

    <owl:NamedIndividual rdf:about="http://w3id.org/meta-share/meta-share/disasterManagement">
        <rdf:type rdf:resource="http://w3id.org/meta-share/meta-share/Domain"/>
        <datacite:hasIdentifier rdf:resource="http://w3id.org/meta-share/meta-share/ELG_Domain005"/>
        <rdfs:label xml:lang="en">disaster management</rdfs:label>
    </owl:NamedIndividual>
    


    <!-- http://w3id.org/meta-share/meta-share/discourseMarker -->

    <owl:NamedIndividual rdf:about="http://w3id.org/meta-share/meta-share/discourseMarker">
        <rdf:type rdf:resource="http://w3id.org/meta-share/meta-share/AnnotatedElement"/>
        <rdfs:label xml:lang="en">discourse marker</rdfs:label>
    </owl:NamedIndividual>
    


    <!-- http://w3id.org/meta-share/meta-share/discussion -->

    <owl:NamedIndividual rdf:about="http://w3id.org/meta-share/meta-share/discussion">
        <rdf:type rdf:resource="http://w3id.org/meta-share/meta-share/TextGenre"/>
        <datacite:hasIdentifier rdf:resource="http://w3id.org/meta-share/meta-share/PAROLE_G005"/>
        <rdfs:label xml:lang="en">discussion</rdfs:label>
    </owl:NamedIndividual>
    


    <!-- http://w3id.org/meta-share/meta-share/dockerImage -->

    <owl:NamedIndividual rdf:about="http://w3id.org/meta-share/meta-share/dockerImage">
        <rdf:type rdf:resource="http://w3id.org/meta-share/meta-share/SoftwareDistributionForm"/>
        <rdfs:comment xml:lang="en">Value for software distribution form, used for software objects distributed as Docker images, i.e. packaged together with all their dependencies  and ready to be executed</rdfs:comment>
        <rdfs:label xml:lang="en">docker image</rdfs:label>
    </owl:NamedIndividual>
    


    <!-- http://w3id.org/meta-share/meta-share/document2 -->

    <owl:NamedIndividual rdf:about="http://w3id.org/meta-share/meta-share/document2">
        <rdf:type rdf:resource="http://w3id.org/meta-share/meta-share/ParameterType"/>
        <rdfs:label xml:lang="en">document</rdfs:label>
    </owl:NamedIndividual>
    


    <!-- http://w3id.org/meta-share/meta-share/domain1 -->

    <owl:NamedIndividual rdf:about="http://w3id.org/meta-share/meta-share/domain1">
        <rdf:type rdf:resource="http://w3id.org/meta-share/meta-share/SemanticType"/>
        <rdfs:label xml:lang="en">domain</rdfs:label>
    </owl:NamedIndividual>
    


    <!-- http://w3id.org/meta-share/meta-share/downloadable -->

    <owl:NamedIndividual rdf:about="http://w3id.org/meta-share/meta-share/downloadable">
        <rdf:type rdf:resource="http://w3id.org/meta-share/meta-share/DatasetDistributionForm"/>
        <rdfs:comment xml:lang="en">Value for distribution medium, used for language resources that can be downloaded from a remote location</rdfs:comment>
        <rdfs:label xml:lang="en">downloadable</rdfs:label>
    </owl:NamedIndividual>
    


    <!-- http://w3id.org/meta-share/meta-share/draft -->

    <owl:NamedIndividual rdf:about="http://w3id.org/meta-share/meta-share/draft">
        <rdf:type rdf:resource="http://w3id.org/meta-share/meta-share/VersionType"/>
        <rdfs:comment xml:lang="en">Value for &apos;Version type&apos; used for versions during the writing up process</rdfs:comment>
        <rdfs:label xml:lang="en">draft</rdfs:label>
    </owl:NamedIndividual>
    


    <!-- http://w3id.org/meta-share/meta-share/drop -->

    <owl:NamedIndividual rdf:about="http://w3id.org/meta-share/meta-share/drop">
        <rdf:type rdf:resource="http://w3id.org/meta-share/meta-share/PreviousAnnotationTypesPolicy"/>
        <rdfs:label xml:lang="en">drop</rdfs:label>
    </owl:NamedIndividual>
    


    <!-- http://w3id.org/meta-share/meta-share/dv -->

    <owl:NamedIndividual rdf:about="http://w3id.org/meta-share/meta-share/dv">
        <rdf:type rdf:resource="http://w3id.org/meta-share/meta-share/RecordingDeviceType"/>
        <rdfs:label xml:lang="en">DV</rdfs:label>
    </owl:NamedIndividual>
    


    <!-- http://w3id.org/meta-share/meta-share/ean13 -->

    <owl:NamedIndividual rdf:about="http://w3id.org/meta-share/meta-share/ean13">
        <rdf:type rdf:resource="http://w3id.org/meta-share/meta-share/DocumentIdentifierScheme"/>
        <ms:url>https://en.wikipedia.org/wiki/International_Article_Number</ms:url>
        <rdfs:altLabel xml:lang="en">European Article Number 13 standard</rdfs:altLabel>
        <rdfs:comment xml:lang="en">Value for resourceIdentifierSchemeName, referring to EAN (International Article Number, also known as European Article Number) and more specifically to the EAN 13 standard (cf. https://en.wikipedia.org/wiki/International_Article_Number)</rdfs:comment>
        <rdfs:label xml:lang="en">EAN 13</rdfs:label>
    </owl:NamedIndividual>
    


    <!-- http://w3id.org/meta-share/meta-share/earthSciencesGeology -->

    <owl:NamedIndividual rdf:about="http://w3id.org/meta-share/meta-share/earthSciencesGeology">
        <rdf:type rdf:resource="http://w3id.org/meta-share/meta-share/Domain"/>
        <datacite:hasIdentifier rdf:resource="http://w3id.org/meta-share/meta-share/DDC550"/>
        <rdfs:label xml:lang="en">Earth Sciences &amp; Geology</rdfs:label>
    </owl:NamedIndividual>
    


    <!-- http://w3id.org/meta-share/meta-share/economics -->

    <owl:NamedIndividual rdf:about="http://w3id.org/meta-share/meta-share/economics">
        <rdf:type rdf:resource="http://w3id.org/meta-share/meta-share/Domain"/>
        <datacite:hasIdentifier rdf:resource="http://w3id.org/meta-share/meta-share/DDC330"/>
        <rdfs:label xml:lang="en">Economics</rdfs:label>
    </owl:NamedIndividual>
    


    <!-- http://w3id.org/meta-share/meta-share/education -->

    <owl:NamedIndividual rdf:about="http://w3id.org/meta-share/meta-share/education">
        <rdf:type rdf:resource="http://w3id.org/meta-share/meta-share/Domain"/>
        <datacite:hasIdentifier rdf:resource="http://w3id.org/meta-share/meta-share/DDC370"/>
        <rdfs:label xml:lang="en">Education</rdfs:label>
    </owl:NamedIndividual>
    


    <!-- http://w3id.org/meta-share/meta-share/eissn -->

    <owl:NamedIndividual rdf:about="http://w3id.org/meta-share/meta-share/eissn">
        <rdf:type rdf:resource="http://w3id.org/meta-share/meta-share/DocumentIdentifierScheme"/>
        <ms:url>https://en.wikipedia.org/wiki/International_Standard_Serial_Number</ms:url>
        <rdfs:comment xml:lang="en">Value for resourceIdentifierSchemeName, referring to the e-ISSN (electronic International Standard Serial Number, https://en.wikipedia.org/wiki/International_Standard_Serial_Number)</rdfs:comment>
        <rdfs:label xml:lang="en">e-ISSN</rdfs:label>
    </owl:NamedIndividual>
    


    <!-- http://w3id.org/meta-share/meta-share/elderly -->

    <owl:NamedIndividual rdf:about="http://w3id.org/meta-share/meta-share/elderly">
        <rdf:type rdf:resource="http://w3id.org/meta-share/meta-share/AgeGroup"/>
        <rdfs:label xml:lang="en">elderly</rdfs:label>
    </owl:NamedIndividual>
    


    <!-- http://w3id.org/meta-share/meta-share/element -->

    <owl:NamedIndividual rdf:about="http://w3id.org/meta-share/meta-share/element">
        <rdf:type rdf:resource="http://w3id.org/meta-share/meta-share/SizeUnit"/>
        <rdfs:label xml:lang="en">element</rdfs:label>
    </owl:NamedIndividual>
    


    <!-- http://w3id.org/meta-share/meta-share/elg -->

    <owl:NamedIndividual rdf:about="http://w3id.org/meta-share/meta-share/elg">
        <rdf:type rdf:resource="http://purl.org/spar/datacite/AgentIdentifierScheme"/>
        <rdf:type rdf:resource="http://purl.org/spar/datacite/FunderIdentifierScheme"/>
        <rdf:type rdf:resource="http://purl.org/spar/datacite/OrganizationIdentifierScheme"/>
        <rdf:type rdf:resource="http://purl.org/spar/datacite/PersonalIdentifierScheme"/>
        <rdf:type rdf:resource="http://w3id.org/meta-share/meta-share/DocumentIdentifierScheme"/>
        <rdf:type rdf:resource="http://w3id.org/meta-share/meta-share/LRIdentifierScheme"/>
        <rdf:type rdf:resource="http://w3id.org/meta-share/meta-share/LicenceIdentifierScheme"/>
        <rdf:type rdf:resource="http://w3id.org/meta-share/meta-share/MetadataRecordIdentifierScheme"/>
        <rdf:type rdf:resource="http://w3id.org/meta-share/meta-share/ProjectIdentifierScheme"/>
        <rdfs:comment xml:lang="en">European Language Grid</rdfs:comment>
        <rdfs:label xml:lang="en">ELG</rdfs:label>
    </owl:NamedIndividual>
    


    <!-- http://w3id.org/meta-share/meta-share/elicited -->

    <owl:NamedIndividual rdf:about="http://w3id.org/meta-share/meta-share/elicited">
        <rdf:type rdf:resource="http://w3id.org/meta-share/meta-share/Naturality"/>
        <rdfs:label xml:lang="en">elicited</rdfs:label>
    </owl:NamedIndividual>
    


    <!-- http://w3id.org/meta-share/meta-share/emailText -->

    <owl:NamedIndividual rdf:about="http://w3id.org/meta-share/meta-share/emailText">
        <rdf:type rdf:resource="http://w3id.org/meta-share/meta-share/TextType"/>
        <datacite:hasIdentifier rdf:resource="http://w3id.org/meta-share/meta-share/ClarinEl_TT016"/>
        <rdfs:label xml:lang="en">email text</rdfs:label>
    </owl:NamedIndividual>
    


    <!-- http://w3id.org/meta-share/meta-share/embargoedAccess -->

    <owl:NamedIndividual rdf:about="http://w3id.org/meta-share/meta-share/embargoedAccess">
        <rdf:type rdf:resource="http://w3id.org/meta-share/meta-share/AccessRightsStatement"/>
        <datacite:hasIdentifier rdf:resource="http://purl.org/coar/access_right/c_f1cf"/>
    </owl:NamedIndividual>
    


    <!-- http://w3id.org/meta-share/meta-share/embeddedMicrophone -->

    <owl:NamedIndividual rdf:about="http://w3id.org/meta-share/meta-share/embeddedMicrophone">
        <rdf:type rdf:resource="http://w3id.org/meta-share/meta-share/CapturingDeviceType"/>
        <rdfs:label xml:lang="en">embedded microphone</rdfs:label>
    </owl:NamedIndividual>
    


    <!-- http://w3id.org/meta-share/meta-share/emotionalExpressive -->

    <owl:NamedIndividual rdf:about="http://w3id.org/meta-share/meta-share/emotionalExpressive">
        <rdf:type rdf:resource="http://w3id.org/meta-share/meta-share/SpeechGenre"/>
        <datacite:hasIdentifier rdf:resource="http://w3id.org/meta-share/meta-share/MS_SG007"/>
        <rdfs:label xml:lang="en">emotional expressive</rdfs:label>
    </owl:NamedIndividual>
    


    <!-- http://w3id.org/meta-share/meta-share/encyclopaedicText -->

    <owl:NamedIndividual rdf:about="http://w3id.org/meta-share/meta-share/encyclopaedicText">
        <rdf:type rdf:resource="http://w3id.org/meta-share/meta-share/TextType"/>
        <datacite:hasIdentifier rdf:resource="http://w3id.org/meta-share/meta-share/ClarinEl_TT003"/>
        <rdfs:label xml:lang="en">encyclopaedic text</rdfs:label>
    </owl:NamedIndividual>
    


    <!-- http://w3id.org/meta-share/meta-share/energy -->

    <owl:NamedIndividual rdf:about="http://w3id.org/meta-share/meta-share/energy">
        <rdf:type rdf:resource="http://w3id.org/meta-share/meta-share/Domain"/>
        <datacite:hasIdentifier rdf:resource="http://w3id.org/meta-share/meta-share/ELG_Domain002"/>
        <rdfs:label xml:lang="en">energy</rdfs:label>
    </owl:NamedIndividual>
    


    <!-- http://w3id.org/meta-share/meta-share/energy1 -->

    <owl:NamedIndividual rdf:about="http://w3id.org/meta-share/meta-share/energy1">
        <rdf:type rdf:resource="http://w3id.org/meta-share/meta-share/Domain"/>
        <datacite:hasIdentifier rdf:resource="http://w3id.org/meta-share/meta-share/Clarin_Domain001"/>
        <rdfs:label xml:lang="en">Energy</rdfs:label>
    </owl:NamedIndividual>
    


    <!-- http://w3id.org/meta-share/meta-share/engineering -->

    <owl:NamedIndividual rdf:about="http://w3id.org/meta-share/meta-share/engineering">
        <rdf:type rdf:resource="http://w3id.org/meta-share/meta-share/Domain"/>
        <datacite:hasIdentifier rdf:resource="http://w3id.org/meta-share/meta-share/DDC620"/>
        <rdfs:label xml:lang="en">Engineering</rdfs:label>
    </owl:NamedIndividual>
    


    <!-- http://w3id.org/meta-share/meta-share/entry -->

    <owl:NamedIndividual rdf:about="http://w3id.org/meta-share/meta-share/entry">
        <rdf:type rdf:resource="http://w3id.org/meta-share/meta-share/SizeUnit"/>
        <rdfs:label xml:lang="en">entry</rdfs:label>
    </owl:NamedIndividual>
    


    <!-- http://w3id.org/meta-share/meta-share/environment -->

    <owl:NamedIndividual rdf:about="http://w3id.org/meta-share/meta-share/environment">
        <rdf:type rdf:resource="http://w3id.org/meta-share/meta-share/Domain"/>
        <datacite:hasIdentifier rdf:resource="http://w3id.org/meta-share/meta-share/Clarin_Domain002"/>
        <rdfs:label xml:lang="en">Environment</rdfs:label>
    </owl:NamedIndividual>
    


    <!-- http://w3id.org/meta-share/meta-share/euFunds -->

    <owl:NamedIndividual rdf:about="http://w3id.org/meta-share/meta-share/euFunds">
        <rdf:type rdf:resource="http://w3id.org/meta-share/meta-share/FundingType"/>
        <rdfs:comment xml:lang="en">Value for &apos;Funding type&apos; for projects with EU funds</rdfs:comment>
        <rdfs:label xml:lang="en">EU funds</rdfs:label>
    </owl:NamedIndividual>
    


    <!-- http://w3id.org/meta-share/meta-share/euro -->

    <owl:NamedIndividual rdf:about="http://w3id.org/meta-share/meta-share/euro">
        <rdf:type rdf:resource="http://w3id.org/meta-share/meta-share/Currency"/>
        <rdfs:label xml:lang="en">euro</rdfs:label>
    </owl:NamedIndividual>
    


    <!-- http://w3id.org/meta-share/meta-share/evaluationUse -->

    <owl:NamedIndividual rdf:about="http://w3id.org/meta-share/meta-share/evaluationUse">
        <rdf:type rdf:resource="http://w3id.org/meta-share/meta-share/ConditionOfUse"/>
        <rdfs:comment xml:lang="en">Value for &apos;ConditionOfUse&apos; that states that the language resource can only be used for evaluation purposes</rdfs:comment>
        <rdfs:label xml:lang="en">evaluation use</rdfs:label>
        <skos:note xml:lang="en">add odrl</skos:note>
    </owl:NamedIndividual>
    


    <!-- http://w3id.org/meta-share/meta-share/eventType -->

    <owl:NamedIndividual rdf:about="http://w3id.org/meta-share/meta-share/eventType">
        <rdf:type rdf:resource="http://w3id.org/meta-share/meta-share/SemanticType"/>
        <rdfs:label xml:lang="en">event type</rdfs:label>
    </owl:NamedIndividual>
    


    <!-- http://w3id.org/meta-share/meta-share/example -->

    <owl:NamedIndividual rdf:about="http://w3id.org/meta-share/meta-share/example">
        <rdf:type rdf:resource="http://w3id.org/meta-share/meta-share/ExtratextualInformationUnit"/>
        <rdfs:label xml:lang="en">example</rdfs:label>
    </owl:NamedIndividual>
    


    <!-- http://w3id.org/meta-share/meta-share/example1 -->

    <owl:NamedIndividual rdf:about="http://w3id.org/meta-share/meta-share/example1">
        <rdf:type rdf:resource="http://w3id.org/meta-share/meta-share/UsageType"/>
        <rdfs:label xml:lang="en">example</rdfs:label>
    </owl:NamedIndividual>
    


    <!-- http://w3id.org/meta-share/meta-share/executableCode -->

    <owl:NamedIndividual rdf:about="http://w3id.org/meta-share/meta-share/executableCode">
        <rdf:type rdf:resource="http://w3id.org/meta-share/meta-share/SoftwareDistributionForm"/>
        <rdfs:comment xml:lang="en">Value for software distribution form, used for software objects available as binary files already compiled and ready to be executed</rdfs:comment>
        <rdfs:label xml:lang="en">executable code</rdfs:label>
    </owl:NamedIndividual>
    


    <!-- http://w3id.org/meta-share/meta-share/expression -->

    <owl:NamedIndividual rdf:about="http://w3id.org/meta-share/meta-share/expression">
        <rdf:type rdf:resource="http://w3id.org/meta-share/meta-share/SizeUnit"/>
        <rdfs:label xml:lang="en">expression</rdfs:label>
    </owl:NamedIndividual>
    


    <!-- http://w3id.org/meta-share/meta-share/extrinsic -->

    <owl:NamedIndividual rdf:about="http://w3id.org/meta-share/meta-share/extrinsic">
        <rdf:type rdf:resource="http://w3id.org/meta-share/meta-share/EvaluationCriterion"/>
        <rdfs:label xml:lang="en">extrinsic</rdfs:label>
    </owl:NamedIndividual>
    


    <!-- http://w3id.org/meta-share/meta-share/face -->

    <owl:NamedIndividual rdf:about="http://w3id.org/meta-share/meta-share/face">
        <rdf:type rdf:resource="http://w3id.org/meta-share/meta-share/BodyPart"/>
        <rdfs:label xml:lang="en">face</rdfs:label>
    </owl:NamedIndividual>
    


    <!-- http://w3id.org/meta-share/meta-share/faceToFaceConversation -->

    <owl:NamedIndividual rdf:about="http://w3id.org/meta-share/meta-share/faceToFaceConversation">
        <rdf:type rdf:resource="http://w3id.org/meta-share/meta-share/TextType"/>
        <datacite:hasIdentifier rdf:resource="http://w3id.org/meta-share/meta-share/ClarinEl_TT013"/>
        <rdfs:altLabel xml:lang="en">face-to-face conversation</rdfs:altLabel>
        <rdfs:label xml:lang="en">face to face conversation</rdfs:label>
    </owl:NamedIndividual>
    


    <!-- http://w3id.org/meta-share/meta-share/facebook -->

    <owl:NamedIndividual rdf:about="http://w3id.org/meta-share/meta-share/facebook">
        <rdf:type rdf:resource="http://w3id.org/meta-share/meta-share/SocialMediaOccupationalAccountType"/>
        <rdfs:label xml:lang="en">facebook</rdfs:label>
    </owl:NamedIndividual>
    


    <!-- http://w3id.org/meta-share/meta-share/facialExpression -->

    <owl:NamedIndividual rdf:about="http://w3id.org/meta-share/meta-share/facialExpression">
        <rdf:type rdf:resource="http://w3id.org/meta-share/meta-share/ModalityType"/>
        <rdfs:comment xml:lang="en">Value for &apos;ModalityType&apos; for facial expressions represented in a language resource</rdfs:comment>
        <rdfs:label xml:lang="en">facial expression</rdfs:label>
    </owl:NamedIndividual>
    


    <!-- http://w3id.org/meta-share/meta-share/faculty -->

    <owl:NamedIndividual rdf:about="http://w3id.org/meta-share/meta-share/faculty">
        <rdf:type rdf:resource="http://w3id.org/meta-share/meta-share/DivisionCategory"/>
        <rdfs:label xml:lang="en">faculty</rdfs:label>
    </owl:NamedIndividual>
    


    <!-- http://w3id.org/meta-share/meta-share/farfieldMicrophone -->

    <owl:NamedIndividual rdf:about="http://w3id.org/meta-share/meta-share/farfieldMicrophone">
        <rdf:type rdf:resource="http://w3id.org/meta-share/meta-share/CapturingDeviceType"/>
        <rdfs:label xml:lang="en">farfield microphone</rdfs:label>
    </owl:NamedIndividual>
    


    <!-- http://w3id.org/meta-share/meta-share/feature -->

    <owl:NamedIndividual rdf:about="http://w3id.org/meta-share/meta-share/feature">
        <rdf:type rdf:resource="http://w3id.org/meta-share/meta-share/TextGenre"/>
        <datacite:hasIdentifier rdf:resource="http://w3id.org/meta-share/meta-share/PAROLE_G001"/>
        <rdfs:label xml:lang="en">feature</rdfs:label>
    </owl:NamedIndividual>
    


    <!-- http://w3id.org/meta-share/meta-share/female -->

    <owl:NamedIndividual rdf:about="http://w3id.org/meta-share/meta-share/female">
        <rdf:type rdf:resource="http://w3id.org/meta-share/meta-share/Sex"/>
        <rdfs:label xml:lang="en">female</rdfs:label>
    </owl:NamedIndividual>
    


    <!-- http://w3id.org/meta-share/meta-share/few -->

    <owl:NamedIndividual rdf:about="http://w3id.org/meta-share/meta-share/few">
        <rdf:type rdf:resource="http://w3id.org/meta-share/meta-share/Audience"/>
        <rdfs:label xml:lang="en">few</rdfs:label>
    </owl:NamedIndividual>
    


    <!-- http://w3id.org/meta-share/meta-share/fiction -->

    <owl:NamedIndividual rdf:about="http://w3id.org/meta-share/meta-share/fiction">
        <rdf:type rdf:resource="http://w3id.org/meta-share/meta-share/TextGenre"/>
        <datacite:hasIdentifier rdf:resource="http://w3id.org/meta-share/meta-share/PAROLE_G006"/>
        <rdfs:label xml:lang="en">fiction</rdfs:label>
    </owl:NamedIndividual>
    


    <!-- http://w3id.org/meta-share/meta-share/file -->

    <owl:NamedIndividual rdf:about="http://w3id.org/meta-share/meta-share/file">
        <rdf:type rdf:resource="http://w3id.org/meta-share/meta-share/SizeUnit"/>
        <rdfs:label xml:lang="en">file</rdfs:label>
    </owl:NamedIndividual>
    


    <!-- http://w3id.org/meta-share/meta-share/file1 -->

    <owl:NamedIndividual rdf:about="http://w3id.org/meta-share/meta-share/file1">
        <rdf:type rdf:resource="http://w3id.org/meta-share/meta-share/ProcessingResourceType"/>
        <rdfs:label xml:lang="en">file</rdfs:label>
    </owl:NamedIndividual>
    


    <!-- http://w3id.org/meta-share/meta-share/finance -->

    <owl:NamedIndividual rdf:about="http://w3id.org/meta-share/meta-share/finance">
        <rdf:type rdf:resource="http://w3id.org/meta-share/meta-share/Domain"/>
        <datacite:hasIdentifier rdf:resource="http://w3id.org/meta-share/meta-share/ELG_Domain016"/>
        <rdfs:label xml:lang="en">finance</rdfs:label>
    </owl:NamedIndividual>
    


    <!-- http://w3id.org/meta-share/meta-share/five-gram -->

    <owl:NamedIndividual rdf:about="http://w3id.org/meta-share/meta-share/five-gram">
        <rdf:type rdf:resource="http://w3id.org/meta-share/meta-share/SizeUnit"/>
        <rdfs:label xml:lang="en">5-gram</rdfs:label>
    </owl:NamedIndividual>
    


    <!-- http://w3id.org/meta-share/meta-share/fix -->

    <owl:NamedIndividual rdf:about="http://w3id.org/meta-share/meta-share/fix">
        <rdf:type rdf:resource="http://w3id.org/meta-share/meta-share/SceneIllumination"/>
        <rdfs:label xml:lang="en">fix</rdfs:label>
    </owl:NamedIndividual>
    


    <!-- http://w3id.org/meta-share/meta-share/flac -->

    <owl:NamedIndividual rdf:about="http://w3id.org/meta-share/meta-share/flac">
        <rdf:type rdf:resource="http://w3id.org/meta-share/meta-share/CompressionName"/>
        <rdfs:altLabel xml:lang="en">Free Lossless Audio Codec</rdfs:altLabel>
        <rdfs:label xml:lang="en">FLAC</rdfs:label>
    </owl:NamedIndividual>
    


    <!-- http://w3id.org/meta-share/meta-share/flash -->

    <owl:NamedIndividual rdf:about="http://w3id.org/meta-share/meta-share/flash">
        <rdf:type rdf:resource="http://w3id.org/meta-share/meta-share/RecordingDeviceType"/>
        <rdfs:label xml:lang="en">flash</rdfs:label>
    </owl:NamedIndividual>
    


    <!-- http://w3id.org/meta-share/meta-share/float -->

    <owl:NamedIndividual rdf:about="http://w3id.org/meta-share/meta-share/float">
        <rdf:type rdf:resource="http://w3id.org/meta-share/meta-share/ParameterType"/>
        <rdfs:label xml:lang="en">float</rdfs:label>
    </owl:NamedIndividual>
    


    <!-- http://w3id.org/meta-share/meta-share/floatingPoint -->

    <owl:NamedIndividual rdf:about="http://w3id.org/meta-share/meta-share/floatingPoint">
        <rdf:type rdf:resource="http://w3id.org/meta-share/meta-share/SignConvention"/>
        <rdfs:label xml:lang="en">floating point</rdfs:label>
    </owl:NamedIndividual>
    


    <!-- http://w3id.org/meta-share/meta-share/foot -->

    <owl:NamedIndividual rdf:about="http://w3id.org/meta-share/meta-share/foot">
        <rdf:type rdf:resource="http://w3id.org/meta-share/meta-share/BodyPart"/>
        <rdfs:label xml:lang="en">foot</rdfs:label>
    </owl:NamedIndividual>
    


    <!-- http://w3id.org/meta-share/meta-share/foreignAffairs -->

    <owl:NamedIndividual rdf:about="http://w3id.org/meta-share/meta-share/foreignAffairs">
        <rdf:type rdf:resource="http://w3id.org/meta-share/meta-share/Domain"/>
        <datacite:hasIdentifier rdf:resource="http://w3id.org/meta-share/meta-share/ELG_Domain012"/>
        <rdfs:label xml:lang="en">foreign affairs</rdfs:label>
    </owl:NamedIndividual>
    


    <!-- http://w3id.org/meta-share/meta-share/formal -->

    <owl:NamedIndividual rdf:about="http://w3id.org/meta-share/meta-share/formal">
        <rdf:type rdf:resource="http://w3id.org/meta-share/meta-share/ValidationType"/>
        <rdfs:comment xml:lang="en">Value for &apos;Validation type&apos; indicating that the validation is performed on formal aspects of the resource (e.g.,  size, syntactic validation , etc.)</rdfs:comment>
        <rdfs:label xml:lang="en">formal</rdfs:label>
    </owl:NamedIndividual>
    


    <!-- http://w3id.org/meta-share/meta-share/four-gram -->

    <owl:NamedIndividual rdf:about="http://w3id.org/meta-share/meta-share/four-gram">
        <rdf:type rdf:resource="http://w3id.org/meta-share/meta-share/SizeUnit"/>
        <rdfs:label xml:lang="en">4-gram</rdfs:label>
    </owl:NamedIndividual>
    


    <!-- http://w3id.org/meta-share/meta-share/frame -->

    <owl:NamedIndividual rdf:about="http://w3id.org/meta-share/meta-share/frame">
        <rdf:type rdf:resource="http://w3id.org/meta-share/meta-share/SegmentationLevel"/>
        <rdfs:label xml:lang="en">frame</rdfs:label>
    </owl:NamedIndividual>
    


    <!-- http://w3id.org/meta-share/meta-share/frame1 -->

    <owl:NamedIndividual rdf:about="http://w3id.org/meta-share/meta-share/frame1">
        <rdf:type rdf:resource="http://w3id.org/meta-share/meta-share/SizeUnit"/>
        <rdfs:label xml:lang="en">frame</rdfs:label>
    </owl:NamedIndividual>
    


    <!-- http://w3id.org/meta-share/meta-share/frameNet -->

    <owl:NamedIndividual rdf:about="http://w3id.org/meta-share/meta-share/frameNet">
        <rdf:type rdf:resource="http://w3id.org/meta-share/meta-share/CompatibleLexiconType"/>
        <rdf:type rdf:resource="http://w3id.org/meta-share/meta-share/LCRSubclass"/>
        <rdfs:comment xml:lang="en">A lexical database based on annotating examples of how words are used in actual texts in accordance to the notion of &apos;semantic frame&apos; (schematic representation of a situation involving various participants, props and other conceptual roles); originally built for English and extended to other languages according to the same design principles</rdfs:comment>
        <rdfs:label xml:lang="en">FrameNet</rdfs:label>
    </owl:NamedIndividual>
    


    <!-- http://w3id.org/meta-share/meta-share/freeSpeech -->

    <owl:NamedIndividual rdf:about="http://w3id.org/meta-share/meta-share/freeSpeech">
        <rdf:type rdf:resource="http://w3id.org/meta-share/meta-share/SpeechItem"/>
        <rdfs:label xml:lang="en">free speech</rdfs:label>
    </owl:NamedIndividual>
    


    <!-- http://w3id.org/meta-share/meta-share/frequency -->

    <owl:NamedIndividual rdf:about="http://w3id.org/meta-share/meta-share/frequency">
        <rdf:type rdf:resource="http://w3id.org/meta-share/meta-share/UsageType"/>
        <rdfs:label xml:lang="en">frequency</rdfs:label>
    </owl:NamedIndividual>
    


    <!-- http://w3id.org/meta-share/meta-share/frogStory -->

    <owl:NamedIndividual rdf:about="http://w3id.org/meta-share/meta-share/frogStory">
        <rdf:type rdf:resource="http://w3id.org/meta-share/meta-share/ScenarioType"/>
        <rdfs:label xml:lang="en">frog story</rdfs:label>
    </owl:NamedIndividual>
    


    <!-- http://w3id.org/meta-share/meta-share/full -->

    <owl:NamedIndividual rdf:about="http://w3id.org/meta-share/meta-share/full">
        <rdf:type rdf:resource="http://w3id.org/meta-share/meta-share/ValidationExtent"/>
        <rdfs:label xml:lang="en">full</rdfs:label>
    </owl:NamedIndividual>
    


    <!-- http://w3id.org/meta-share/meta-share/fundingAuthority -->

    <owl:NamedIndividual rdf:about="http://w3id.org/meta-share/meta-share/fundingAuthority">
        <rdf:type rdf:resource="http://w3id.org/meta-share/meta-share/OrganizationLegalStatus"/>
        <rdfs:label xml:lang="en">funding authority</rdfs:label>
    </owl:NamedIndividual>
    


    <!-- http://w3id.org/meta-share/meta-share/galaxyWorkflow -->

    <owl:NamedIndividual rdf:about="http://w3id.org/meta-share/meta-share/galaxyWorkflow">
        <rdf:type rdf:resource="http://w3id.org/meta-share/meta-share/SoftwareDistributionForm"/>
        <rdfs:comment xml:lang="en">Value for software distribution form, used for software workflows created with the Galaxy workflow engine</rdfs:comment>
        <rdfs:label xml:lang="en">galaxy workflow</rdfs:label>
    </owl:NamedIndividual>
    


    <!-- http://w3id.org/meta-share/meta-share/gb -->

    <owl:NamedIndividual rdf:about="http://w3id.org/meta-share/meta-share/gb">
        <rdf:type rdf:resource="http://w3id.org/meta-share/meta-share/SizeUnit"/>
        <rdfs:altLabel xml:lang="en">gigabyte</rdfs:altLabel>
        <rdfs:label xml:lang="en">gb</rdfs:label>
    </owl:NamedIndividual>
    


    <!-- http://w3id.org/meta-share/meta-share/gender -->

    <owl:NamedIndividual rdf:about="http://w3id.org/meta-share/meta-share/gender">
        <rdf:type rdf:resource="http://w3id.org/meta-share/meta-share/MorphologicalType"/>
        <rdfs:label xml:lang="en">gender</rdfs:label>
    </owl:NamedIndividual>
    


    <!-- http://w3id.org/meta-share/meta-share/general -->

    <owl:NamedIndividual rdf:about="http://w3id.org/meta-share/meta-share/general">
        <rdf:type rdf:resource="http://w3id.org/meta-share/meta-share/Domain"/>
        <datacite:hasIdentifier rdf:resource="http://w3id.org/meta-share/meta-share/Clarin_Domain003"/>
        <rdfs:label xml:lang="en">General</rdfs:label>
    </owl:NamedIndividual>
    


    <!-- http://w3id.org/meta-share/meta-share/generalDocumenation -->

    <owl:NamedIndividual rdf:about="http://w3id.org/meta-share/meta-share/generalDocumenation">
        <rdf:type rdf:resource="http://w3id.org/meta-share/meta-share/DocumentationType"/>
        <rdfs:comment xml:lang="en">Value for &apos;Documentation type&apos; used for documents that describe a language resource or some aspect of it</rdfs:comment>
        <rdfs:label xml:lang="en">general documentation</rdfs:label>
    </owl:NamedIndividual>
    


    <!-- http://w3id.org/meta-share/meta-share/generation -->

    <owl:NamedIndividual rdf:about="http://w3id.org/meta-share/meta-share/generation">
        <rdf:type rdf:resource="http://w3id.org/meta-share/meta-share/LDTask"/>
        <rdfs:label xml:lang="en">generation</rdfs:label>
    </owl:NamedIndividual>
    


    <!-- http://w3id.org/meta-share/meta-share/geographyAndTravel -->

    <owl:NamedIndividual rdf:about="http://w3id.org/meta-share/meta-share/geographyAndTravel">
        <rdf:type rdf:resource="http://w3id.org/meta-share/meta-share/Domain"/>
        <datacite:hasIdentifier rdf:resource="http://w3id.org/meta-share/meta-share/DDC910"/>
        <rdfs:label xml:lang="en">Geography &amp; Travel</rdfs:label>
    </owl:NamedIndividual>
    


    <!-- http://w3id.org/meta-share/meta-share/github -->

    <owl:NamedIndividual rdf:about="http://w3id.org/meta-share/meta-share/github">
        <rdf:type rdf:resource="http://w3id.org/meta-share/meta-share/SocialMediaOccupationalAccountType"/>
        <rdfs:label xml:lang="en">GitHub</rdfs:label>
    </owl:NamedIndividual>
    


    <!-- http://w3id.org/meta-share/meta-share/gitlab -->

    <owl:NamedIndividual rdf:about="http://w3id.org/meta-share/meta-share/gitlab">
        <rdf:type rdf:resource="http://w3id.org/meta-share/meta-share/SocialMediaOccupationalAccountType"/>
        <rdfs:label xml:lang="en">GitLab</rdfs:label>
    </owl:NamedIndividual>
    


    <!-- http://w3id.org/meta-share/meta-share/glassBox -->

    <owl:NamedIndividual rdf:about="http://w3id.org/meta-share/meta-share/glassBox">
        <rdf:type rdf:resource="http://w3id.org/meta-share/meta-share/EvaluationType"/>
        <rdfs:label xml:lang="en">glass box</rdfs:label>
    </owl:NamedIndividual>
    


    <!-- http://w3id.org/meta-share/meta-share/googleChromeOS -->

    <owl:NamedIndividual rdf:about="http://w3id.org/meta-share/meta-share/googleChromeOS">
        <rdf:type rdf:resource="http://w3id.org/meta-share/meta-share/OperatingSystem"/>
        <rdfs:label xml:lang="en">Google Chrome OS</rdfs:label>
    </owl:NamedIndividual>
    


    <!-- http://w3id.org/meta-share/meta-share/graphicArtsAndDecorativeArts -->

    <owl:NamedIndividual rdf:about="http://w3id.org/meta-share/meta-share/graphicArtsAndDecorativeArts">
        <rdf:type rdf:resource="http://w3id.org/meta-share/meta-share/Domain"/>
        <datacite:hasIdentifier rdf:resource="http://w3id.org/meta-share/meta-share/DDC740"/>
        <rdfs:label xml:lang="en">Graphic Arts &amp; Decorative Arts</rdfs:label>
    </owl:NamedIndividual>
    


    <!-- http://w3id.org/meta-share/meta-share/graphicCard -->

    <owl:NamedIndividual rdf:about="http://w3id.org/meta-share/meta-share/graphicCard">
        <rdf:type rdf:resource="http://w3id.org/meta-share/meta-share/RequiredHardware"/>
        <rdfs:label xml:lang="en">graphic card</rdfs:label>
    </owl:NamedIndividual>
    


    <!-- http://w3id.org/meta-share/meta-share/grid -->

    <owl:NamedIndividual rdf:about="http://w3id.org/meta-share/meta-share/grid">
        <rdf:type rdf:resource="http://purl.org/spar/datacite/OrganizationIdentifierScheme"/>
        <ms:url>https://www.grid.ac/</ms:url>
        <rdfs:comment xml:lang="en">Value for organizationIdentifierSchemeName, referring to the GRID (Global Research Identifier Database, https://www.grid.ac/)</rdfs:comment>
        <rdfs:label xml:lang="en">GRID</rdfs:label>
    </owl:NamedIndividual>
    


    <!-- http://w3id.org/meta-share/meta-share/group -->

    <owl:NamedIndividual rdf:about="http://w3id.org/meta-share/meta-share/group">
        <rdf:type rdf:resource="http://w3id.org/meta-share/meta-share/DivisionCategory"/>
        <rdfs:label xml:lang="en">group</rdfs:label>
    </owl:NamedIndividual>
    


    <!-- http://w3id.org/meta-share/meta-share/guidelines -->

    <owl:NamedIndividual rdf:about="http://w3id.org/meta-share/meta-share/guidelines">
        <rdf:type rdf:resource="http://w3id.org/meta-share/meta-share/DocumentationType"/>
    </owl:NamedIndividual>
    


    <!-- http://w3id.org/meta-share/meta-share/hand -->

    <owl:NamedIndividual rdf:about="http://w3id.org/meta-share/meta-share/hand">
        <rdf:type rdf:resource="http://w3id.org/meta-share/meta-share/BodyPart"/>
        <rdfs:label xml:lang="en">hand</rdfs:label>
    </owl:NamedIndividual>
    


    <!-- http://w3id.org/meta-share/meta-share/hardDisk -->

    <owl:NamedIndividual rdf:about="http://w3id.org/meta-share/meta-share/hardDisk">
        <rdf:type rdf:resource="http://w3id.org/meta-share/meta-share/DatasetDistributionForm"/>
        <rdfs:comment xml:lang="en">Value for data distribution medium, used for resources that are delivered on a hard disk</rdfs:comment>
        <rdfs:label xml:lang="en">hard disk</rdfs:label>
    </owl:NamedIndividual>
    


    <!-- http://w3id.org/meta-share/meta-share/hardDisk1 -->

    <owl:NamedIndividual rdf:about="http://w3id.org/meta-share/meta-share/hardDisk1">
        <rdf:type rdf:resource="http://w3id.org/meta-share/meta-share/RecordingDeviceType"/>
        <rdfs:label xml:lang="en">hard disk</rdfs:label>
    </owl:NamedIndividual>
    


    <!-- http://w3id.org/meta-share/meta-share/hardwareAndHouseholdAppliances -->

    <owl:NamedIndividual rdf:about="http://w3id.org/meta-share/meta-share/hardwareAndHouseholdAppliances">
        <rdf:type rdf:resource="http://w3id.org/meta-share/meta-share/Domain"/>
        <datacite:hasIdentifier rdf:resource="http://w3id.org/meta-share/meta-share/DDC683"/>
        <rdfs:label xml:lang="en">Hardware &amp; Household Appliances</rdfs:label>
    </owl:NamedIndividual>
    


    <!-- http://w3id.org/meta-share/meta-share/head -->

    <owl:NamedIndividual rdf:about="http://w3id.org/meta-share/meta-share/head">
        <rdf:type rdf:resource="http://w3id.org/meta-share/meta-share/BodyPart"/>
        <rdfs:label xml:lang="en">head</rdfs:label>
    </owl:NamedIndividual>
    


    <!-- http://w3id.org/meta-share/meta-share/health -->

    <owl:NamedIndividual rdf:about="http://w3id.org/meta-share/meta-share/health">
        <rdf:type rdf:resource="http://w3id.org/meta-share/meta-share/Domain"/>
        <datacite:hasIdentifier rdf:resource="http://w3id.org/meta-share/meta-share/ELG_Domain009"/>
        <rdfs:label xml:lang="en">health</rdfs:label>
    </owl:NamedIndividual>
    


    <!-- http://w3id.org/meta-share/meta-share/high -->

    <owl:NamedIndividual rdf:about="http://w3id.org/meta-share/meta-share/high">
        <rdf:type rdf:resource="http://w3id.org/meta-share/meta-share/RecordingQuality"/>
        <rdfs:label xml:lang="en">high</rdfs:label>
    </owl:NamedIndividual>
    


    <!-- http://w3id.org/meta-share/meta-share/high1 -->

    <owl:NamedIndividual rdf:about="http://w3id.org/meta-share/meta-share/high1">
        <rdf:type rdf:resource="http://w3id.org/meta-share/meta-share/Quality"/>
        <rdfs:label xml:lang="en">high</rdfs:label>
    </owl:NamedIndividual>
    


    <!-- http://w3id.org/meta-share/meta-share/high2 -->

    <owl:NamedIndividual rdf:about="http://w3id.org/meta-share/meta-share/high2">
        <rdf:type rdf:resource="http://w3id.org/meta-share/meta-share/NoiseLevel"/>
        <rdfs:label xml:lang="en">high</rdfs:label>
    </owl:NamedIndividual>
    


    <!-- http://w3id.org/meta-share/meta-share/history -->

    <owl:NamedIndividual rdf:about="http://w3id.org/meta-share/meta-share/history">
        <rdf:type rdf:resource="http://w3id.org/meta-share/meta-share/Domain"/>
        <datacite:hasIdentifier rdf:resource="http://w3id.org/meta-share/meta-share/DDC900"/>
        <rdfs:label xml:lang="en">History</rdfs:label>
    </owl:NamedIndividual>
    


    <!-- http://w3id.org/meta-share/meta-share/homeAndFamilyManagement -->

    <owl:NamedIndividual rdf:about="http://w3id.org/meta-share/meta-share/homeAndFamilyManagement">
        <rdf:type rdf:resource="http://w3id.org/meta-share/meta-share/Domain"/>
        <datacite:hasIdentifier rdf:resource="http://w3id.org/meta-share/meta-share/DDC640"/>
        <rdfs:label xml:lang="en">Home &amp; Family Management</rdfs:label>
    </owl:NamedIndividual>
    


    <!-- http://w3id.org/meta-share/meta-share/hour -->

    <owl:NamedIndividual rdf:about="http://w3id.org/meta-share/meta-share/hour">
        <rdf:type rdf:resource="http://w3id.org/meta-share/meta-share/DurationUnit"/>
        <rdfs:label xml:lang="en">hour</rdfs:label>
    </owl:NamedIndividual>
    


    <!-- http://w3id.org/meta-share/meta-share/hour1 -->

    <owl:NamedIndividual rdf:about="http://w3id.org/meta-share/meta-share/hour1">
        <rdf:type rdf:resource="http://w3id.org/meta-share/meta-share/SizeUnit"/>
        <rdfs:label xml:lang="en">hour</rdfs:label>
    </owl:NamedIndividual>
    


    <!-- http://w3id.org/meta-share/meta-share/human -->

    <owl:NamedIndividual rdf:about="http://w3id.org/meta-share/meta-share/human">
        <rdf:type rdf:resource="http://w3id.org/meta-share/meta-share/EvaluationMeasure"/>
        <rdfs:label xml:lang="en">human</rdfs:label>
    </owl:NamedIndividual>
    


    <!-- http://w3id.org/meta-share/meta-share/humanNonSpeech -->

    <owl:NamedIndividual rdf:about="http://w3id.org/meta-share/meta-share/humanNonSpeech">
        <rdf:type rdf:resource="http://w3id.org/meta-share/meta-share/AudioGenre"/>
        <datacite:hasIdentifier rdf:resource="http://w3id.org/meta-share/meta-share/MS_AG001"/>
        <rdfs:label xml:lang="en">human non speech</rdfs:label>
    </owl:NamedIndividual>
    


    <!-- http://w3id.org/meta-share/meta-share/hyperbaric -->

    <owl:NamedIndividual rdf:about="http://w3id.org/meta-share/meta-share/hyperbaric">
        <rdf:type rdf:resource="http://w3id.org/meta-share/meta-share/SpeechInfluence"/>
        <rdfs:label xml:lang="en">hyperbaric</rdfs:label>
    </owl:NamedIndividual>
    


    <!-- http://w3id.org/meta-share/meta-share/hyperonym -->

    <owl:NamedIndividual rdf:about="http://w3id.org/meta-share/meta-share/hyperonym">
        <rdf:type rdf:resource="http://w3id.org/meta-share/meta-share/SemanticType"/>
        <rdfs:label xml:lang="en">hyperonym</rdfs:label>
    </owl:NamedIndividual>
    


    <!-- http://w3id.org/meta-share/meta-share/hyponym -->

    <owl:NamedIndividual rdf:about="http://w3id.org/meta-share/meta-share/hyponym">
        <rdf:type rdf:resource="http://w3id.org/meta-share/meta-share/SemanticType"/>
        <rdfs:label xml:lang="en">hyponym</rdfs:label>
    </owl:NamedIndividual>
    


    <!-- http://w3id.org/meta-share/meta-share/iOS -->

    <owl:NamedIndividual rdf:about="http://w3id.org/meta-share/meta-share/iOS">
        <rdf:type rdf:resource="http://w3id.org/meta-share/meta-share/OperatingSystem"/>
        <rdfs:label xml:lang="en">iOS</rdfs:label>
    </owl:NamedIndividual>
    


    <!-- http://w3id.org/meta-share/meta-share/idiomaticExpression -->

    <owl:NamedIndividual rdf:about="http://w3id.org/meta-share/meta-share/idiomaticExpression">
        <rdf:type rdf:resource="http://w3id.org/meta-share/meta-share/SizeUnit"/>
        <rdfs:label xml:lang="en">idiomatic expression</rdfs:label>
    </owl:NamedIndividual>
    


    <!-- http://w3id.org/meta-share/meta-share/image -->

    <owl:NamedIndividual rdf:about="http://w3id.org/meta-share/meta-share/image">
        <rdf:type rdf:resource="http://w3id.org/meta-share/meta-share/MediaType"/>
        <rdfs:comment xml:lang="en">Value for &apos;Media type&apos; for the for of a language resource (part) consisting of visual representations (e.g.,  pictures, photos)</rdfs:comment>
        <rdfs:label xml:lang="en">image</rdfs:label>
    </owl:NamedIndividual>
    


    <!-- http://w3id.org/meta-share/meta-share/image1 -->

    <owl:NamedIndividual rdf:about="http://w3id.org/meta-share/meta-share/image1">
        <rdf:type rdf:resource="http://w3id.org/meta-share/meta-share/ExtratextualInformation"/>
        <rdfs:label xml:lang="en">image</rdfs:label>
    </owl:NamedIndividual>
    


    <!-- http://w3id.org/meta-share/meta-share/image2 -->

    <owl:NamedIndividual rdf:about="http://w3id.org/meta-share/meta-share/image2">
        <rdf:type rdf:resource="http://w3id.org/meta-share/meta-share/SizeUnit"/>
        <rdfs:label xml:lang="en">image</rdfs:label>
    </owl:NamedIndividual>
    


    <!-- http://w3id.org/meta-share/meta-share/impact -->

    <owl:NamedIndividual rdf:about="http://w3id.org/meta-share/meta-share/impact">
        <rdf:type rdf:resource="http://w3id.org/meta-share/meta-share/EvaluationLevel"/>
        <rdfs:label xml:lang="en">impact</rdfs:label>
    </owl:NamedIndividual>
    


    <!-- http://w3id.org/meta-share/meta-share/inBook -->

    <owl:NamedIndividual rdf:about="http://w3id.org/meta-share/meta-share/inBook">
        <rdf:type rdf:resource="http://w3id.org/meta-share/meta-share/DocumentType"/>
        <rdfs:label xml:lang="en">in book</rdfs:label>
    </owl:NamedIndividual>
    


    <!-- http://w3id.org/meta-share/meta-share/inCar -->

    <owl:NamedIndividual rdf:about="http://w3id.org/meta-share/meta-share/inCar">
        <rdf:type rdf:resource="http://w3id.org/meta-share/meta-share/RecordingEnvironment"/>
        <rdfs:label xml:lang="en">in car</rdfs:label>
    </owl:NamedIndividual>
    


    <!-- http://w3id.org/meta-share/meta-share/inCollection -->

    <owl:NamedIndividual rdf:about="http://w3id.org/meta-share/meta-share/inCollection">
        <rdf:type rdf:resource="http://w3id.org/meta-share/meta-share/DocumentType"/>
        <rdfs:label xml:lang="en">in collection</rdfs:label>
    </owl:NamedIndividual>
    


    <!-- http://w3id.org/meta-share/meta-share/inCopyright -->

    <owl:NamedIndividual rdf:about="http://w3id.org/meta-share/meta-share/inCopyright">
        <rdf:type rdf:resource="http://w3id.org/meta-share/meta-share/AccessRightsStatement"/>
        <datacite:hasIdentifier rdf:resource="http://rightsstatements.org/vocab/InC/1.0/"/>
    </owl:NamedIndividual>
    


    <!-- http://w3id.org/meta-share/meta-share/inCopyrightEUOrphan -->

    <owl:NamedIndividual rdf:about="http://w3id.org/meta-share/meta-share/inCopyrightEUOrphan">
        <rdf:type rdf:resource="http://w3id.org/meta-share/meta-share/AccessRightsStatement"/>
        <datacite:hasIdentifier rdf:resource="http://rightsstatements.org/vocab/InC-OW-EU/1.0/"/>
    </owl:NamedIndividual>
    


    <!-- http://w3id.org/meta-share/meta-share/inCopyrightEdu -->

    <owl:NamedIndividual rdf:about="http://w3id.org/meta-share/meta-share/inCopyrightEdu">
        <rdf:type rdf:resource="http://w3id.org/meta-share/meta-share/AccessRightsStatement"/>
        <datacite:hasIdentifier rdf:resource="http://rightsstatements.org/vocab/InC-EDU/1.0/"/>
    </owl:NamedIndividual>
    


    <!-- http://w3id.org/meta-share/meta-share/inCopyrightNCPermitted -->

    <owl:NamedIndividual rdf:about="http://w3id.org/meta-share/meta-share/inCopyrightNCPermitted">
        <rdf:type rdf:resource="http://w3id.org/meta-share/meta-share/AccessRightsStatement"/>
        <datacite:hasIdentifier rdf:resource="http://rightsstatements.org/vocab/InC-NC/1.0/"/>
    </owl:NamedIndividual>
    


    <!-- http://w3id.org/meta-share/meta-share/inCopyrightRightsHoldersUnlocatable -->

    <owl:NamedIndividual rdf:about="http://w3id.org/meta-share/meta-share/inCopyrightRightsHoldersUnlocatable">
        <rdf:type rdf:resource="http://w3id.org/meta-share/meta-share/AccessRightsStatement"/>
        <datacite:hasIdentifier rdf:resource="http://rightsstatements.org/vocab/InC-RUU/1.0/"/>
    </owl:NamedIndividual>
    


    <!-- http://w3id.org/meta-share/meta-share/inProceedings -->

    <owl:NamedIndividual rdf:about="http://w3id.org/meta-share/meta-share/inProceedings">
        <rdf:type rdf:resource="http://w3id.org/meta-share/meta-share/DocumentType"/>
        <rdfs:label xml:lang="en">in proceedings</rdfs:label>
    </owl:NamedIndividual>
    


    <!-- http://w3id.org/meta-share/meta-share/included -->

    <owl:NamedIndividual rdf:about="http://w3id.org/meta-share/meta-share/included">
        <rdf:type rdf:resource="http://w3id.org/meta-share/meta-share/RelatedLexiconType"/>
        <rdfs:label xml:lang="en">included</rdfs:label>
    </owl:NamedIndividual>
    


    <!-- http://w3id.org/meta-share/meta-share/incorporate -->

    <owl:NamedIndividual rdf:about="http://w3id.org/meta-share/meta-share/incorporate">
        <rdf:type rdf:resource="http://www.w3.org/2004/02/skos/core#concept"/>
        <rdfs:comment xml:lang="en">The Assigner permits/prohibits the Assignees to incorporate the Asset unmodified into a Collective Work.</rdfs:comment>
        <rdfs:label xml:lang="en">incorporate</rdfs:label>
        <skos:broaderTransitive rdf:resource="http://www.w3.org/ns/odrl/2/use"/>
    </owl:NamedIndividual>
    


    <!-- http://w3id.org/meta-share/meta-share/industrial -->

    <owl:NamedIndividual rdf:about="http://w3id.org/meta-share/meta-share/industrial">
        <rdf:type rdf:resource="http://w3id.org/meta-share/meta-share/RecordingEnvironment"/>
        <rdfs:label xml:lang="en">industrial</rdfs:label>
    </owl:NamedIndividual>
    


    <!-- http://w3id.org/meta-share/meta-share/inflection -->

    <owl:NamedIndividual rdf:about="http://w3id.org/meta-share/meta-share/inflection">
        <rdf:type rdf:resource="http://w3id.org/meta-share/meta-share/MorphologicalType"/>
        <rdfs:label xml:lang="en">inflection</rdfs:label>
    </owl:NamedIndividual>
    


    <!-- http://w3id.org/meta-share/meta-share/informLicensor -->

    <owl:NamedIndividual rdf:about="http://w3id.org/meta-share/meta-share/informLicensor">
        <rdf:type rdf:resource="http://w3id.org/meta-share/meta-share/ConditionOfUse"/>
        <rdf:type rdf:resource="http://www.w3.org/ns/odrl/2/Set"/>
        <rdfs:comment xml:lang="en">Value for &apos;ConditionOfUse&apos; which states that users must inform the licensor as to the kind of use they intend to make of the resource</rdfs:comment>
        <rdfs:label xml:lang="en">inform licensor</rdfs:label>
        <odrl:permission>
            <rdf:Description>
                <odrl:duty>
                    <rdf:Description>
                        <odrl:action rdf:resource="http://creativecommons.org/ns#Notify"/>
                    </rdf:Description>
                </odrl:duty>
            </rdf:Description>
        </odrl:permission>
    </owl:NamedIndividual>
    


    <!-- http://w3id.org/meta-share/meta-share/information -->

    <owl:NamedIndividual rdf:about="http://w3id.org/meta-share/meta-share/information">
        <rdf:type rdf:resource="http://w3id.org/meta-share/meta-share/TextGenre"/>
        <datacite:hasIdentifier rdf:resource="http://w3id.org/meta-share/meta-share/PAROLE_G003"/>
        <rdfs:label xml:lang="en">information</rdfs:label>
    </owl:NamedIndividual>
    


    <!-- http://w3id.org/meta-share/meta-share/installationManual -->

    <owl:NamedIndividual rdf:about="http://w3id.org/meta-share/meta-share/installationManual">
        <rdf:type rdf:resource="http://w3id.org/meta-share/meta-share/DocumentationType"/>
        <rdfs:comment xml:lang="en">Value for &apos;Documentation type&apos; used for documents that contain instructions on how to install a software</rdfs:comment>
        <rdfs:label xml:lang="en">installation manual</rdfs:label>
    </owl:NamedIndividual>
    


    <!-- http://w3id.org/meta-share/meta-share/institute -->

    <owl:NamedIndividual rdf:about="http://w3id.org/meta-share/meta-share/institute">
        <rdf:type rdf:resource="http://w3id.org/meta-share/meta-share/DivisionCategory"/>
        <rdfs:label xml:lang="en">institute</rdfs:label>
    </owl:NamedIndividual>
    


    <!-- http://w3id.org/meta-share/meta-share/instruction -->

    <owl:NamedIndividual rdf:about="http://w3id.org/meta-share/meta-share/instruction">
        <rdf:type rdf:resource="http://w3id.org/meta-share/meta-share/TextGenre"/>
        <datacite:hasIdentifier rdf:resource="http://w3id.org/meta-share/meta-share/PAROLE_G004"/>
        <rdfs:label xml:lang="en">instruction</rdfs:label>
    </owl:NamedIndividual>
    


    <!-- http://w3id.org/meta-share/meta-share/instrumentalMusic -->

    <owl:NamedIndividual rdf:about="http://w3id.org/meta-share/meta-share/instrumentalMusic">
        <rdf:type rdf:resource="http://w3id.org/meta-share/meta-share/AudioGenre"/>
        <datacite:hasIdentifier rdf:resource="http://w3id.org/meta-share/meta-share/MS_AG005"/>
        <rdfs:label xml:lang="en">instrumental music</rdfs:label>
    </owl:NamedIndividual>
    


    <!-- http://w3id.org/meta-share/meta-share/insurance -->

    <owl:NamedIndividual rdf:about="http://w3id.org/meta-share/meta-share/insurance">
        <rdf:type rdf:resource="http://w3id.org/meta-share/meta-share/Domain"/>
        <datacite:hasIdentifier rdf:resource="http://w3id.org/meta-share/meta-share/ELG_Domain006"/>
        <rdfs:label xml:lang="en">insurance</rdfs:label>
    </owl:NamedIndividual>
    


    <!-- http://w3id.org/meta-share/meta-share/integer -->

    <owl:NamedIndividual rdf:about="http://w3id.org/meta-share/meta-share/integer">
        <rdf:type rdf:resource="http://w3id.org/meta-share/meta-share/ParameterType"/>
        <rdfs:label xml:lang="en">integer</rdfs:label>
    </owl:NamedIndividual>
    


    <!-- http://w3id.org/meta-share/meta-share/interactive -->

    <owl:NamedIndividual rdf:about="http://w3id.org/meta-share/meta-share/interactive">
        <rdf:type rdf:resource="http://w3id.org/meta-share/meta-share/ProcessMode"/>
        <rdfs:comment xml:lang="en">Value for &apos;Process mode&apos; and its subclasses used for processes that include some interaction between the processing tool and the human agent performing the process</rdfs:comment>
        <rdfs:label xml:lang="en">interactive</rdfs:label>
    </owl:NamedIndividual>
    


    <!-- http://w3id.org/meta-share/meta-share/interactive1 -->

    <owl:NamedIndividual rdf:about="http://w3id.org/meta-share/meta-share/interactive1">
        <rdf:type rdf:resource="http://w3id.org/meta-share/meta-share/Interactivity"/>
        <rdfs:label xml:lang="en">interactive</rdfs:label>
    </owl:NamedIndividual>
    


    <!-- http://w3id.org/meta-share/meta-share/internet -->

    <owl:NamedIndividual rdf:about="http://w3id.org/meta-share/meta-share/internet">
        <rdf:type rdf:resource="http://w3id.org/meta-share/meta-share/SourceChannel"/>
        <rdfs:label xml:lang="en">internet</rdfs:label>
    </owl:NamedIndividual>
    


    <!-- http://w3id.org/meta-share/meta-share/interview -->

    <owl:NamedIndividual rdf:about="http://w3id.org/meta-share/meta-share/interview">
        <rdf:type rdf:resource="http://w3id.org/meta-share/meta-share/TextType"/>
        <datacite:hasIdentifier rdf:resource="http://w3id.org/meta-share/meta-share/ClarinEl_TT006"/>
        <rdfs:label xml:lang="en">interview</rdfs:label>
    </owl:NamedIndividual>
    


    <!-- http://w3id.org/meta-share/meta-share/interview1 -->

    <owl:NamedIndividual rdf:about="http://w3id.org/meta-share/meta-share/interview1">
        <rdf:type rdf:resource="http://w3id.org/meta-share/meta-share/SpeechGenre"/>
        <datacite:hasIdentifier rdf:resource="http://w3id.org/meta-share/meta-share/MS_SG006"/>
        <rdfs:label xml:lang="en">interview</rdfs:label>
    </owl:NamedIndividual>
    


    <!-- http://w3id.org/meta-share/meta-share/intrinsic -->

    <owl:NamedIndividual rdf:about="http://w3id.org/meta-share/meta-share/intrinsic">
        <rdf:type rdf:resource="http://w3id.org/meta-share/meta-share/EvaluationCriterion"/>
        <rdfs:label xml:lang="en">intrinsic</rdfs:label>
    </owl:NamedIndividual>
    


    <!-- http://w3id.org/meta-share/meta-share/irregularForm -->

    <owl:NamedIndividual rdf:about="http://w3id.org/meta-share/meta-share/irregularForm">
        <rdf:type rdf:resource="http://w3id.org/meta-share/meta-share/MorphologicalType"/>
        <rdfs:label xml:lang="en">irregular form</rdfs:label>
    </owl:NamedIndividual>
    


    <!-- http://w3id.org/meta-share/meta-share/islrn -->

    <owl:NamedIndividual rdf:about="http://w3id.org/meta-share/meta-share/islrn">
        <rdf:type rdf:resource="http://w3id.org/meta-share/meta-share/LRIdentifierScheme"/>
        <ms:url>http://www.islrn.org</ms:url>
        <rdfs:comment xml:lang="en">Value for LRTIdentifierScheme referring to ISLRN (International Standard Language Resource Number, http://www.islrn.org/)</rdfs:comment>
        <rdfs:label>ISLRN</rdfs:label>
    </owl:NamedIndividual>
    


    <!-- http://w3id.org/meta-share/meta-share/isolatedDigit -->

    <owl:NamedIndividual rdf:about="http://w3id.org/meta-share/meta-share/isolatedDigit">
        <rdf:type rdf:resource="http://w3id.org/meta-share/meta-share/SpeechItem"/>
        <rdfs:label xml:lang="en">isolated digit</rdfs:label>
    </owl:NamedIndividual>
    


    <!-- http://w3id.org/meta-share/meta-share/isolatedWord -->

    <owl:NamedIndividual rdf:about="http://w3id.org/meta-share/meta-share/isolatedWord">
        <rdf:type rdf:resource="http://w3id.org/meta-share/meta-share/SpeechItem"/>
        <rdfs:label xml:lang="en">isolated word</rdfs:label>
    </owl:NamedIndividual>
    


    <!-- http://w3id.org/meta-share/meta-share/issn -->

    <owl:NamedIndividual rdf:about="http://w3id.org/meta-share/meta-share/issn">
        <rdf:type rdf:resource="http://w3id.org/meta-share/meta-share/DocumentIdentifierScheme"/>
        <ms:url>http://www.issn.org</ms:url>
        <rdfs:altLabel xml:lang="en">International Standard Serial Number</rdfs:altLabel>
        <rdfs:comment xml:lang="en">Value for resourceIdentifierSchemeName, referring to the ISSN (International Standard Serial Number, http://www.issn.org/)</rdfs:comment>
        <rdfs:label xml:lang="en">ISSN</rdfs:label>
    </owl:NamedIndividual>
    


    <!-- http://w3id.org/meta-share/meta-share/issueTracker -->

    <owl:NamedIndividual rdf:about="http://w3id.org/meta-share/meta-share/issueTracker">
        <rdf:type rdf:resource="http://w3id.org/meta-share/meta-share/DocumentationType"/>
        <rdfs:comment xml:lang="en">Value for &apos;DocumentationType&apos; for issue-tracking tools used by software developers usually available through a dedicated web page</rdfs:comment>
        <rdfs:label xml:lang="en">issue tracker</rdfs:label>
    </owl:NamedIndividual>
    


    <!-- http://w3id.org/meta-share/meta-share/istc -->

    <owl:NamedIndividual rdf:about="http://w3id.org/meta-share/meta-share/istc">
        <rdf:type rdf:resource="http://w3id.org/meta-share/meta-share/DocumentIdentifierScheme"/>
        <ms:url>http://www.istc-international.org/</ms:url>
        <rdfs:altLabel xml:lang="en">International Standard Text Code</rdfs:altLabel>
        <rdfs:comment xml:lang="en">Value for resourceIdentifierSchemeName, referring to the ISTC (International Standard Text Code, http://www.istc-international.org/)</rdfs:comment>
        <rdfs:label xml:lang="en">ISTC</rdfs:label>
    </owl:NamedIndividual>
    


    <!-- http://w3id.org/meta-share/meta-share/item -->

    <owl:NamedIndividual rdf:about="http://w3id.org/meta-share/meta-share/item">
        <rdf:type rdf:resource="http://w3id.org/meta-share/meta-share/SizeUnit"/>
        <rdfs:label xml:lang="en">item</rdfs:label>
    </owl:NamedIndividual>
    


    <!-- http://w3id.org/meta-share/meta-share/jargon -->

    <owl:NamedIndividual rdf:about="http://w3id.org/meta-share/meta-share/jargon">
        <rdf:type rdf:resource="http://w3id.org/meta-share/meta-share/LanguageVarietyType"/>
        <rdfs:comment xml:lang="en">Value for &apos;LanguageVarietyType&apos; used for a particular type of language mainly used in a specific context (e.g.,  by a professional or social group) which may not be well understood outside that context</rdfs:comment>
        <rdfs:label xml:lang="en">jargon</rdfs:label>
    </owl:NamedIndividual>
    


    <!-- http://w3id.org/meta-share/meta-share/journalisticText -->

    <owl:NamedIndividual rdf:about="http://w3id.org/meta-share/meta-share/journalisticText">
        <rdf:type rdf:resource="http://w3id.org/meta-share/meta-share/TextType"/>
        <datacite:hasIdentifier rdf:resource="http://w3id.org/meta-share/meta-share/ClarinEl_TT018"/>
        <rdfs:label xml:lang="en">journalistic text</rdfs:label>
    </owl:NamedIndividual>
    


    <!-- http://w3id.org/meta-share/meta-share/kb -->

    <owl:NamedIndividual rdf:about="http://w3id.org/meta-share/meta-share/kb">
        <rdf:type rdf:resource="http://w3id.org/meta-share/meta-share/SizeUnit"/>
        <rdfs:altLabel xml:lang="en">kb</rdfs:altLabel>
        <rdfs:label xml:lang="en">kilobyte</rdfs:label>
    </owl:NamedIndividual>
    


    <!-- http://w3id.org/meta-share/meta-share/keep -->

    <owl:NamedIndividual rdf:about="http://w3id.org/meta-share/meta-share/keep">
        <rdf:type rdf:resource="http://w3id.org/meta-share/meta-share/PreviousAnnotationTypesPolicy"/>
        <rdfs:label xml:lang="en">keep</rdfs:label>
    </owl:NamedIndividual>
    


    <!-- http://w3id.org/meta-share/meta-share/keyword1 -->

    <owl:NamedIndividual rdf:about="http://w3id.org/meta-share/meta-share/keyword1">
        <rdf:type rdf:resource="http://w3id.org/meta-share/meta-share/SizeUnit"/>
        <rdfs:label xml:lang="en">keyword</rdfs:label>
    </owl:NamedIndividual>
    


    <!-- http://w3id.org/meta-share/meta-share/laboratory -->

    <owl:NamedIndividual rdf:about="http://w3id.org/meta-share/meta-share/laboratory">
        <rdf:type rdf:resource="http://w3id.org/meta-share/meta-share/DivisionCategory"/>
        <rdfs:label xml:lang="en">laboratory</rdfs:label>
    </owl:NamedIndividual>
    


    <!-- http://w3id.org/meta-share/meta-share/language1 -->

    <owl:NamedIndividual rdf:about="http://w3id.org/meta-share/meta-share/language1">
        <rdf:type rdf:resource="http://w3id.org/meta-share/meta-share/Domain"/>
        <datacite:hasIdentifier rdf:resource="http://w3id.org/meta-share/meta-share/DDC400"/>
        <rdfs:label xml:lang="en">Language</rdfs:label>
    </owl:NamedIndividual>
    


    <!-- http://w3id.org/meta-share/meta-share/languageDescription -->

    <owl:NamedIndividual rdf:about="http://w3id.org/meta-share/meta-share/languageDescription">
        <rdf:type rdf:resource="http://w3id.org/meta-share/meta-share/ProcessingResourceType"/>
        <rdfs:comment xml:lang="en">Value for &apos;Resource type&apos; for language descriptions, e.g.,  grammars, machine learning models , etc., i.e. language resources that formally describe a language</rdfs:comment>
        <rdfs:label xml:lang="en">language description</rdfs:label>
    </owl:NamedIndividual>
    


    <!-- http://w3id.org/meta-share/meta-share/languageEngineeringResearchUse -->

    <owl:NamedIndividual rdf:about="http://w3id.org/meta-share/meta-share/languageEngineeringResearchUse">
        <rdf:type rdf:resource="http://w3id.org/meta-share/meta-share/ConditionOfUse"/>
        <dct:replaces xml:lang="en">Value for &apos;ConditionOfUse&apos; which states that the resource can only be used for research purposes in the Language Enginnering / Language Technology domain.</dct:replaces>
        <rdfs:label xml:lang="en">language engineering research use</rdfs:label>
    </owl:NamedIndividual>
    


    <!-- http://w3id.org/meta-share/meta-share/languageServiceProvider -->

    <owl:NamedIndividual rdf:about="http://w3id.org/meta-share/meta-share/languageServiceProvider">
        <rdf:type rdf:resource="http://w3id.org/meta-share/meta-share/OrganizationRole"/>
        <rdfs:label xml:lang="en">language service provider</rdfs:label>
    </owl:NamedIndividual>
    


    <!-- http://w3id.org/meta-share/meta-share/largeCompany -->

    <owl:NamedIndividual rdf:about="http://w3id.org/meta-share/meta-share/largeCompany">
        <rdf:type rdf:resource="http://w3id.org/meta-share/meta-share/OrganizationLegalStatus"/>
        <rdfs:label xml:lang="en">large company</rdfs:label>
    </owl:NamedIndividual>
    


    <!-- http://w3id.org/meta-share/meta-share/largeMembraneMicrophone -->

    <owl:NamedIndividual rdf:about="http://w3id.org/meta-share/meta-share/largeMembraneMicrophone">
        <rdf:type rdf:resource="http://w3id.org/meta-share/meta-share/CapturingDeviceType"/>
        <rdfs:label xml:lang="en">large membrane microphone</rdfs:label>
    </owl:NamedIndividual>
    


    <!-- http://w3id.org/meta-share/meta-share/largePublic -->

    <owl:NamedIndividual rdf:about="http://w3id.org/meta-share/meta-share/largePublic">
        <rdf:type rdf:resource="http://w3id.org/meta-share/meta-share/Audience"/>
        <rdfs:label xml:lang="en">large public</rdfs:label>
    </owl:NamedIndividual>
    


    <!-- http://w3id.org/meta-share/meta-share/laryngograph -->

    <owl:NamedIndividual rdf:about="http://w3id.org/meta-share/meta-share/laryngograph">
        <rdf:type rdf:resource="http://w3id.org/meta-share/meta-share/SourceChannel"/>
        <rdfs:label xml:lang="en">laryngograph</rdfs:label>
    </owl:NamedIndividual>
    


    <!-- http://w3id.org/meta-share/meta-share/laryngograph1 -->

    <owl:NamedIndividual rdf:about="http://w3id.org/meta-share/meta-share/laryngograph1">
        <rdf:type rdf:resource="http://w3id.org/meta-share/meta-share/CapturingDeviceType"/>
        <rdfs:label xml:lang="en">laryngograph</rdfs:label>
    </owl:NamedIndividual>
    


    <!-- http://w3id.org/meta-share/meta-share/lavalierMicrophone -->

    <owl:NamedIndividual rdf:about="http://w3id.org/meta-share/meta-share/lavalierMicrophone">
        <rdf:type rdf:resource="http://w3id.org/meta-share/meta-share/CapturingDeviceType"/>
        <rdfs:label xml:lang="en">lavalier microphone</rdfs:label>
    </owl:NamedIndividual>
    


    <!-- http://w3id.org/meta-share/meta-share/law -->

    <owl:NamedIndividual rdf:about="http://w3id.org/meta-share/meta-share/law">
        <rdf:type rdf:resource="http://w3id.org/meta-share/meta-share/Domain"/>
        <datacite:hasIdentifier rdf:resource="http://w3id.org/meta-share/meta-share/DDC340"/>
        <rdfs:label xml:lang="en">Law</rdfs:label>
    </owl:NamedIndividual>
    


    <!-- http://w3id.org/meta-share/meta-share/law1 -->

    <owl:NamedIndividual rdf:about="http://w3id.org/meta-share/meta-share/law1">
        <rdf:type rdf:resource="http://w3id.org/meta-share/meta-share/Domain"/>
        <datacite:hasIdentifier rdf:resource="http://w3id.org/meta-share/meta-share/ELG_Domain018"/>
        <rdfs:label xml:lang="en">law</rdfs:label>
    </owl:NamedIndividual>
    


    <!-- http://w3id.org/meta-share/meta-share/lecture -->

    <owl:NamedIndividual rdf:about="http://w3id.org/meta-share/meta-share/lecture">
        <rdf:type rdf:resource="http://w3id.org/meta-share/meta-share/SpeechGenre"/>
        <datacite:hasIdentifier rdf:resource="http://w3id.org/meta-share/meta-share/MS_SG010"/>
        <rdfs:label xml:lang="en">lecture</rdfs:label>
    </owl:NamedIndividual>
    


    <!-- http://w3id.org/meta-share/meta-share/lectureRoom -->

    <owl:NamedIndividual rdf:about="http://w3id.org/meta-share/meta-share/lectureRoom">
        <rdf:type rdf:resource="http://w3id.org/meta-share/meta-share/RecordingEnvironment"/>
        <rdfs:label xml:lang="en">lecture room</rdfs:label>
    </owl:NamedIndividual>
    


    <!-- http://w3id.org/meta-share/meta-share/leg -->

    <owl:NamedIndividual rdf:about="http://w3id.org/meta-share/meta-share/leg">
        <rdf:type rdf:resource="http://w3id.org/meta-share/meta-share/BodyPart"/>
        <rdfs:label xml:lang="en">leg</rdfs:label>
    </owl:NamedIndividual>
    


    <!-- http://w3id.org/meta-share/meta-share/lemma -->

    <owl:NamedIndividual rdf:about="http://w3id.org/meta-share/meta-share/lemma">
        <rdf:type rdf:resource="http://w3id.org/meta-share/meta-share/LemmaType"/>
        <rdfs:label xml:lang="en">lemma</rdfs:label>
    </owl:NamedIndividual>
    


    <!-- http://w3id.org/meta-share/meta-share/lemma1 -->

    <owl:NamedIndividual rdf:about="http://w3id.org/meta-share/meta-share/lemma1">
        <rdf:type rdf:resource="http://w3id.org/meta-share/meta-share/ExtratextualInformationUnit"/>
        <rdfs:label xml:lang="en">lemma</rdfs:label>
    </owl:NamedIndividual>
    


    <!-- http://w3id.org/meta-share/meta-share/letter -->

    <owl:NamedIndividual rdf:about="http://w3id.org/meta-share/meta-share/letter">
        <rdf:type rdf:resource="http://w3id.org/meta-share/meta-share/BaseItem"/>
        <rdfs:label xml:lang="en">letter</rdfs:label>
    </owl:NamedIndividual>
    


    <!-- http://w3id.org/meta-share/meta-share/letter1 -->

    <owl:NamedIndividual rdf:about="http://w3id.org/meta-share/meta-share/letter1">
        <rdf:type rdf:resource="http://w3id.org/meta-share/meta-share/TextType"/>
        <datacite:hasIdentifier rdf:resource="http://w3id.org/meta-share/meta-share/ClarinEl_TT004"/>
        <rdfs:label xml:lang="en">letter</rdfs:label>
    </owl:NamedIndividual>
    


    <!-- http://w3id.org/meta-share/meta-share/lexicalConceptualResource -->

    <owl:NamedIndividual rdf:about="http://w3id.org/meta-share/meta-share/lexicalConceptualResource">
        <rdf:type rdf:resource="http://w3id.org/meta-share/meta-share/ProcessingResourceType"/>
        <rdfs:comment xml:lang="en">Value for &apos;Processing resource type&apos; for lexical and conceptual resources (e.g.,  lexica, ontologies, gazetteers, terminological lists, dictionaries, thesauri, etc.)</rdfs:comment>
        <rdfs:label xml:lang="en">lexical/conceptual resource</rdfs:label>
    </owl:NamedIndividual>
    


    <!-- http://w3id.org/meta-share/meta-share/lexicalType -->

    <owl:NamedIndividual rdf:about="http://w3id.org/meta-share/meta-share/lexicalType">
        <rdf:type rdf:resource="http://w3id.org/meta-share/meta-share/SizeUnit"/>
        <rdfs:label xml:lang="en">lexical type</rdfs:label>
    </owl:NamedIndividual>
    


    <!-- http://w3id.org/meta-share/meta-share/lexicalUnit -->

    <owl:NamedIndividual rdf:about="http://w3id.org/meta-share/meta-share/lexicalUnit">
        <rdf:type rdf:resource="http://w3id.org/meta-share/meta-share/ExtratextualInformationUnit"/>
        <rdfs:label xml:lang="en">lexical unit</rdfs:label>
    </owl:NamedIndividual>
    


    <!-- http://w3id.org/meta-share/meta-share/lexicon -->

    <owl:NamedIndividual rdf:about="http://w3id.org/meta-share/meta-share/lexicon">
        <rdf:type rdf:resource="http://w3id.org/meta-share/meta-share/LCRSubclass"/>
        <rdfs:comment xml:lang="en">(a list of) all the words used in a particular language or subject, or a dictionary [https://dictionary.cambridge.org/dictionary/english/lexicon]</rdfs:comment>
        <rdfs:label xml:lang="en">lexicon</rdfs:label>
    </owl:NamedIndividual>
    


    <!-- http://w3id.org/meta-share/meta-share/libraryOfCongress_Classification -->

    <owl:NamedIndividual rdf:about="http://w3id.org/meta-share/meta-share/libraryOfCongress_Classification">
        <rdf:type rdf:resource="http://w3id.org/meta-share/meta-share/DomainClassificationScheme"/>
        <rdfs:altLabel xml:lang="en">Library of Congress classification system</rdfs:altLabel>
        <rdfs:label xml:lang="en">LCC</rdfs:label>
    </owl:NamedIndividual>
    


    <!-- http://w3id.org/meta-share/meta-share/libraryofCongressSubjectHeadings_classification -->

    <owl:NamedIndividual rdf:about="http://w3id.org/meta-share/meta-share/libraryofCongressSubjectHeadings_classification">
        <rdf:type rdf:resource="http://w3id.org/meta-share/meta-share/SubjectClassificationScheme"/>
        <rdfs:altLabel xml:lang="en">Library of Congress Subject Headings</rdfs:altLabel>
        <rdfs:label xml:lang="en">LCSH</rdfs:label>
    </owl:NamedIndividual>
    


    <!-- http://w3id.org/meta-share/meta-share/lifeSciences -->

    <owl:NamedIndividual rdf:about="http://w3id.org/meta-share/meta-share/lifeSciences">
        <rdf:type rdf:resource="http://w3id.org/meta-share/meta-share/Domain"/>
        <rdfs:comment xml:lang="en">A branch of science (such as biology, medicine, and sometimes anthropology or sociology) that deals with living organisms and life processes —usually used in plural</rdfs:comment>
        <rdfs:label xml:lang="en">life sciences</rdfs:label>
    </owl:NamedIndividual>
    


    <!-- http://w3id.org/meta-share/meta-share/linearPCM -->

    <owl:NamedIndividual rdf:about="http://w3id.org/meta-share/meta-share/linearPCM">
        <rdf:type rdf:resource="http://w3id.org/meta-share/meta-share/SignalEncoding"/>
        <rdfs:label xml:lang="en">linear PCM</rdfs:label>
    </owl:NamedIndividual>
    


    <!-- http://w3id.org/meta-share/meta-share/linguistics -->

    <owl:NamedIndividual rdf:about="http://w3id.org/meta-share/meta-share/linguistics">
        <rdf:type rdf:resource="http://w3id.org/meta-share/meta-share/Domain"/>
        <datacite:hasIdentifier rdf:resource="http://w3id.org/meta-share/meta-share/DDC410"/>
        <rdfs:label xml:lang="en">Linguistics</rdfs:label>
    </owl:NamedIndividual>
    


    <!-- http://w3id.org/meta-share/meta-share/linkedIn -->

    <owl:NamedIndividual rdf:about="http://w3id.org/meta-share/meta-share/linkedIn">
        <rdf:type rdf:resource="http://w3id.org/meta-share/meta-share/SocialMediaOccupationalAccountType"/>
        <rdfs:label xml:lang="en">linkedIn</rdfs:label>
    </owl:NamedIndividual>
    


    <!-- http://w3id.org/meta-share/meta-share/linux -->

    <owl:NamedIndividual rdf:about="http://w3id.org/meta-share/meta-share/linux">
        <rdf:type rdf:resource="http://w3id.org/meta-share/meta-share/OperatingSystem"/>
        <rdfs:label xml:lang="en">Linux</rdfs:label>
    </owl:NamedIndividual>
    


    <!-- http://w3id.org/meta-share/meta-share/lissn -->

    <owl:NamedIndividual rdf:about="http://w3id.org/meta-share/meta-share/lissn">
        <rdf:type rdf:resource="http://w3id.org/meta-share/meta-share/DocumentIdentifierScheme"/>
        <rdfs:altLabel xml:lang="en">ISSN-L</rdfs:altLabel>
        <rdfs:comment xml:lang="en">Value for resourceIdentifierSchemeName, referring to the linking ISSN or ISSN-L</rdfs:comment>
        <rdfs:label xml:lang="en">LISSN</rdfs:label>
    </owl:NamedIndividual>
    


    <!-- http://w3id.org/meta-share/meta-share/literaryText -->

    <owl:NamedIndividual rdf:about="http://w3id.org/meta-share/meta-share/literaryText">
        <rdf:type rdf:resource="http://w3id.org/meta-share/meta-share/TextType"/>
        <datacite:hasIdentifier rdf:resource="http://w3id.org/meta-share/meta-share/ClarinEl_TT012"/>
        <rdfs:label xml:lang="en">literary text</rdfs:label>
    </owl:NamedIndividual>
    


    <!-- http://w3id.org/meta-share/meta-share/literatureRhetoricAndCriticism -->

    <owl:NamedIndividual rdf:about="http://w3id.org/meta-share/meta-share/literatureRhetoricAndCriticism">
        <rdf:type rdf:resource="http://w3id.org/meta-share/meta-share/Domain"/>
        <datacite:hasIdentifier rdf:resource="http://w3id.org/meta-share/meta-share/DDC800"/>
        <rdfs:label xml:lang="en">Literature, Rhetoric &amp; Criticism</rdfs:label>
    </owl:NamedIndividual>
    


    <!-- http://w3id.org/meta-share/meta-share/littleEndian -->

    <owl:NamedIndividual rdf:about="http://w3id.org/meta-share/meta-share/littleEndian">
        <rdf:type rdf:resource="http://w3id.org/meta-share/meta-share/ByteOrder"/>
        <rdfs:label xml:lang="en">Little Endian</rdfs:label>
    </owl:NamedIndividual>
    


    <!-- http://w3id.org/meta-share/meta-share/low -->

    <owl:NamedIndividual rdf:about="http://w3id.org/meta-share/meta-share/low">
        <rdf:type rdf:resource="http://w3id.org/meta-share/meta-share/RecordingQuality"/>
        <rdfs:label xml:lang="en">low</rdfs:label>
    </owl:NamedIndividual>
    


    <!-- http://w3id.org/meta-share/meta-share/low1 -->

    <owl:NamedIndividual rdf:about="http://w3id.org/meta-share/meta-share/low1">
        <rdf:type rdf:resource="http://w3id.org/meta-share/meta-share/Quality"/>
        <rdfs:label xml:lang="en">low</rdfs:label>
    </owl:NamedIndividual>
    


    <!-- http://w3id.org/meta-share/meta-share/low2 -->

    <owl:NamedIndividual rdf:about="http://w3id.org/meta-share/meta-share/low2">
        <rdf:type rdf:resource="http://w3id.org/meta-share/meta-share/NoiseLevel"/>
        <rdfs:label xml:lang="en">low</rdfs:label>
    </owl:NamedIndividual>
    


    <!-- http://w3id.org/meta-share/meta-share/lsid -->

    <owl:NamedIndividual rdf:about="http://w3id.org/meta-share/meta-share/lsid">
        <rdf:type rdf:resource="http://w3id.org/meta-share/meta-share/DocumentIdentifierScheme"/>
        <ms:url>http://www.webcitation.org/getfile?fileid=27fcd073ea70199946ace15c6868520be2cab2ab</ms:url>
        <rdfs:altLabel xml:lang="en">Life Sciences Identifier</rdfs:altLabel>
        <rdfs:comment xml:lang="en">Value for resourceIdentifierSchemeName, referring to the LSID (Life Sciences Identifier, http://www.webcitation.org/getfile?fileid=27fcd073ea70199946ace15c6868520be2cab2ab)</rdfs:comment>
        <rdfs:label xml:lang="en">LSID</rdfs:label>
    </owl:NamedIndividual>
    


    <!-- http://w3id.org/meta-share/meta-share/mac-OS -->

    <owl:NamedIndividual rdf:about="http://w3id.org/meta-share/meta-share/mac-OS">
        <rdf:type rdf:resource="http://w3id.org/meta-share/meta-share/OperatingSystem"/>
        <rdfs:label xml:lang="en">MAC-OS</rdfs:label>
    </owl:NamedIndividual>
    


    <!-- http://w3id.org/meta-share/meta-share/machineReadableDictionary -->

    <owl:NamedIndividual rdf:about="http://w3id.org/meta-share/meta-share/machineReadableDictionary">
        <rdf:type rdf:resource="http://w3id.org/meta-share/meta-share/LCRSubclass"/>
        <rdfs:altLabel xml:lang="en">MRD</rdfs:altLabel>
        <rdfs:comment xml:lang="en">a dictionary usually meant for humans in a form that a computer can process</rdfs:comment>
        <rdfs:label xml:lang="en">Machine Readable Dictionary</rdfs:label>
    </owl:NamedIndividual>
    


    <!-- http://w3id.org/meta-share/meta-share/male -->

    <owl:NamedIndividual rdf:about="http://w3id.org/meta-share/meta-share/male">
        <rdf:type rdf:resource="http://w3id.org/meta-share/meta-share/Sex"/>
        <rdfs:label xml:lang="en">male</rdfs:label>
    </owl:NamedIndividual>
    


    <!-- http://w3id.org/meta-share/meta-share/managementAndPublicRelations -->

    <owl:NamedIndividual rdf:about="http://w3id.org/meta-share/meta-share/managementAndPublicRelations">
        <rdf:type rdf:resource="http://w3id.org/meta-share/meta-share/Domain"/>
        <datacite:hasIdentifier rdf:resource="http://w3id.org/meta-share/meta-share/DDC650"/>
        <rdfs:label xml:lang="en">Management &amp; Public Relations</rdfs:label>
    </owl:NamedIndividual>
    


    <!-- http://w3id.org/meta-share/meta-share/manual -->

    <owl:NamedIndividual rdf:about="http://w3id.org/meta-share/meta-share/manual">
        <rdf:type rdf:resource="http://w3id.org/meta-share/meta-share/ProcessMode"/>
        <rdfs:comment xml:lang="en">Value for &apos;Process mode&apos; and its subclasses used for processes that are performed manually</rdfs:comment>
        <rdfs:label xml:lang="en">manual</rdfs:label>
    </owl:NamedIndividual>
    


    <!-- http://w3id.org/meta-share/meta-share/manual1 -->

    <owl:NamedIndividual rdf:about="http://w3id.org/meta-share/meta-share/manual1">
        <rdf:type rdf:resource="http://w3id.org/meta-share/meta-share/DocumentType"/>
        <rdfs:label xml:lang="en">manual</rdfs:label>
    </owl:NamedIndividual>
    


    <!-- http://w3id.org/meta-share/meta-share/manufacturing -->

    <owl:NamedIndividual rdf:about="http://w3id.org/meta-share/meta-share/manufacturing">
        <rdf:type rdf:resource="http://w3id.org/meta-share/meta-share/Domain"/>
        <datacite:hasIdentifier rdf:resource="http://w3id.org/meta-share/meta-share/DDC670"/>
        <rdfs:label xml:lang="en">Manufacturing</rdfs:label>
    </owl:NamedIndividual>
    


    <!-- http://w3id.org/meta-share/meta-share/mapTask -->

    <owl:NamedIndividual rdf:about="http://w3id.org/meta-share/meta-share/mapTask">
        <rdf:type rdf:resource="http://w3id.org/meta-share/meta-share/ScenarioType"/>
        <rdfs:label xml:lang="en">map task</rdfs:label>
    </owl:NamedIndividual>
    


    <!-- http://w3id.org/meta-share/meta-share/mappingOfResources -->

    <owl:NamedIndividual rdf:about="http://w3id.org/meta-share/meta-share/mappingOfResources">
        <rdf:type rdf:resource="http://w3id.org/meta-share/meta-share/LCRSubclass"/>
        <rdfs:comment xml:lang="en">a resource consisting of mapping values and/or rules between two resources</rdfs:comment>
        <rdfs:label xml:lang="en">mapping of resources</rdfs:label>
    </owl:NamedIndividual>
    


    <!-- http://w3id.org/meta-share/meta-share/mastersThesis -->

    <owl:NamedIndividual rdf:about="http://w3id.org/meta-share/meta-share/mastersThesis">
        <rdf:type rdf:resource="http://w3id.org/meta-share/meta-share/DocumentType"/>
        <rdfs:label xml:lang="en">masters thesis</rdfs:label>
    </owl:NamedIndividual>
    


    <!-- http://w3id.org/meta-share/meta-share/mathematics -->

    <owl:NamedIndividual rdf:about="http://w3id.org/meta-share/meta-share/mathematics">
        <rdf:type rdf:resource="http://w3id.org/meta-share/meta-share/Domain"/>
        <datacite:hasIdentifier rdf:resource="http://w3id.org/meta-share/meta-share/DDC510"/>
        <rdfs:label xml:lang="en">Mathematics</rdfs:label>
    </owl:NamedIndividual>
    


    <!-- http://w3id.org/meta-share/meta-share/maven -->

    <owl:NamedIndividual rdf:about="http://w3id.org/meta-share/meta-share/maven">
        <rdf:type rdf:resource="http://w3id.org/meta-share/meta-share/LRIdentifierScheme"/>
        <ms:url>https://maven.apache.org/pom.html#Maven_Coordinates</ms:url>
        <rdfs:comment xml:lang="en">Value for LRTIdentifierScheme referring to the Maven coordinates (cf. Maven POM, https://maven.apache.org/pom.html#Maven_Coordinates)</rdfs:comment>
        <rdfs:label xml:lang="en">maven</rdfs:label>
    </owl:NamedIndividual>
    


    <!-- http://w3id.org/meta-share/meta-share/mb -->

    <owl:NamedIndividual rdf:about="http://w3id.org/meta-share/meta-share/mb">
        <rdf:type rdf:resource="http://w3id.org/meta-share/meta-share/SizeUnit"/>
        <rdfs:altLabel xml:lang="en">megabyte</rdfs:altLabel>
        <rdfs:label xml:lang="en">mb</rdfs:label>
    </owl:NamedIndividual>
    


    <!-- http://w3id.org/meta-share/meta-share/media -->

    <owl:NamedIndividual rdf:about="http://w3id.org/meta-share/meta-share/media">
        <rdf:type rdf:resource="http://w3id.org/meta-share/meta-share/Domain"/>
        <datacite:hasIdentifier rdf:resource="http://w3id.org/meta-share/meta-share/ELG_Domain008"/>
        <rdfs:label xml:lang="en">media</rdfs:label>
    </owl:NamedIndividual>
    


    <!-- http://w3id.org/meta-share/meta-share/medication -->

    <owl:NamedIndividual rdf:about="http://w3id.org/meta-share/meta-share/medication">
        <rdf:type rdf:resource="http://w3id.org/meta-share/meta-share/SpeechInfluence"/>
        <rdfs:label xml:lang="en">medication</rdfs:label>
    </owl:NamedIndividual>
    


    <!-- http://w3id.org/meta-share/meta-share/medicineAndHealth -->

    <owl:NamedIndividual rdf:about="http://w3id.org/meta-share/meta-share/medicineAndHealth">
        <rdf:type rdf:resource="http://w3id.org/meta-share/meta-share/Domain"/>
        <datacite:hasIdentifier rdf:resource="http://w3id.org/meta-share/meta-share/DDC610"/>
        <rdfs:label xml:lang="en">Medicine &amp; Health</rdfs:label>
    </owl:NamedIndividual>
    


    <!-- http://w3id.org/meta-share/meta-share/medium -->

    <owl:NamedIndividual rdf:about="http://w3id.org/meta-share/meta-share/medium">
        <rdf:type rdf:resource="http://w3id.org/meta-share/meta-share/RecordingQuality"/>
        <rdfs:label xml:lang="en">medium</rdfs:label>
    </owl:NamedIndividual>
    


    <!-- http://w3id.org/meta-share/meta-share/medium1 -->

    <owl:NamedIndividual rdf:about="http://w3id.org/meta-share/meta-share/medium1">
        <rdf:type rdf:resource="http://w3id.org/meta-share/meta-share/Quality"/>
        <rdfs:label xml:lang="en">medium</rdfs:label>
    </owl:NamedIndividual>
    


    <!-- http://w3id.org/meta-share/meta-share/medium2 -->

    <owl:NamedIndividual rdf:about="http://w3id.org/meta-share/meta-share/medium2">
        <rdf:type rdf:resource="http://w3id.org/meta-share/meta-share/NoiseLevel"/>
        <rdfs:label xml:lang="en">medium</rdfs:label>
    </owl:NamedIndividual>
    


    <!-- http://w3id.org/meta-share/meta-share/meeting -->

    <owl:NamedIndividual rdf:about="http://w3id.org/meta-share/meta-share/meeting">
        <rdf:type rdf:resource="http://w3id.org/meta-share/meta-share/SpeechGenre"/>
        <datacite:hasIdentifier rdf:resource="http://w3id.org/meta-share/meta-share/MS_SG011"/>
        <rdfs:label xml:lang="en">meeting</rdfs:label>
    </owl:NamedIndividual>
    


    <!-- http://w3id.org/meta-share/meta-share/meetingProceedings -->

    <owl:NamedIndividual rdf:about="http://w3id.org/meta-share/meta-share/meetingProceedings">
        <rdf:type rdf:resource="http://w3id.org/meta-share/meta-share/TextType"/>
        <datacite:hasIdentifier rdf:resource="http://w3id.org/meta-share/meta-share/ClarinEl_TT009"/>
        <rdfs:label xml:lang="en">meeting proceedings</rdfs:label>
    </owl:NamedIndividual>
    


    <!-- http://w3id.org/meta-share/meta-share/memberOfAssociation1 -->

    <owl:NamedIndividual rdf:about="http://w3id.org/meta-share/meta-share/memberOfAssociation1">
        <rdf:type rdf:resource="http://w3id.org/meta-share/meta-share/ConditionOfUse"/>
        <rdfs:label xml:lang="en">member of association</rdfs:label>
    </owl:NamedIndividual>
    


    <!-- http://w3id.org/meta-share/meta-share/meronym -->

    <owl:NamedIndividual rdf:about="http://w3id.org/meta-share/meta-share/meronym">
        <rdf:type rdf:resource="http://w3id.org/meta-share/meta-share/SemanticType"/>
        <rdfs:label xml:lang="en">meronym</rdfs:label>
    </owl:NamedIndividual>
    


    <!-- http://w3id.org/meta-share/meta-share/metaShare -->

    <owl:NamedIndividual rdf:about="http://w3id.org/meta-share/meta-share/metaShare">
        <rdf:type rdf:resource="http://w3id.org/meta-share/meta-share/LRIdentifierScheme"/>
        <ms:url>http://www.meta-share.org</ms:url>
        <rdfs:comment xml:lang="en">Value for LRTIdentifierScheme referring to the identifier assigned by META-SHARE (http://www.meta-share.org/)</rdfs:comment>
        <rdfs:label xml:lang="en">META-SHARE</rdfs:label>
        <skos:note xml:lang="en">in MS, we had MetaShareId and not the scheme; in general, discuss the use of &quot;local resource identifier scheme&quot; from DataCite as a value</skos:note>
    </owl:NamedIndividual>
    


    <!-- http://w3id.org/meta-share/meta-share/metadataOnlyAccess -->

    <owl:NamedIndividual rdf:about="http://w3id.org/meta-share/meta-share/metadataOnlyAccess">
        <rdf:type rdf:resource="http://w3id.org/meta-share/meta-share/AccessRightsStatement"/>
        <datacite:hasIdentifier rdf:resource="http://purl.org/coar/access_right/c_14cb"/>
    </owl:NamedIndividual>
    


    <!-- http://w3id.org/meta-share/meta-share/microphone -->

    <owl:NamedIndividual rdf:about="http://w3id.org/meta-share/meta-share/microphone">
        <rdf:type rdf:resource="http://w3id.org/meta-share/meta-share/RequiredHardware"/>
        <rdfs:label xml:lang="en">microphone</rdfs:label>
    </owl:NamedIndividual>
    


    <!-- http://w3id.org/meta-share/meta-share/microphone1 -->

    <owl:NamedIndividual rdf:about="http://w3id.org/meta-share/meta-share/microphone1">
        <rdf:type rdf:resource="http://w3id.org/meta-share/meta-share/CapturingDeviceType"/>
        <rdfs:label xml:lang="en">microphone</rdfs:label>
    </owl:NamedIndividual>
    


    <!-- http://w3id.org/meta-share/meta-share/microphoneArray -->

    <owl:NamedIndividual rdf:about="http://w3id.org/meta-share/meta-share/microphoneArray">
        <rdf:type rdf:resource="http://w3id.org/meta-share/meta-share/CapturingDeviceType"/>
        <rdfs:label xml:lang="en">microphone array</rdfs:label>
    </owl:NamedIndividual>
    


    <!-- http://w3id.org/meta-share/meta-share/minute -->

    <owl:NamedIndividual rdf:about="http://w3id.org/meta-share/meta-share/minute">
        <rdf:type rdf:resource="http://w3id.org/meta-share/meta-share/SizeUnit"/>
        <rdfs:label xml:lang="en">minute</rdfs:label>
    </owl:NamedIndividual>
    


    <!-- http://w3id.org/meta-share/meta-share/minute1 -->

    <owl:NamedIndividual rdf:about="http://w3id.org/meta-share/meta-share/minute1">
        <rdf:type rdf:resource="http://w3id.org/meta-share/meta-share/DurationUnit"/>
        <rdfs:label xml:lang="en">minute</rdfs:label>
    </owl:NamedIndividual>
    


    <!-- http://w3id.org/meta-share/meta-share/mispronunciation -->

    <owl:NamedIndividual rdf:about="http://w3id.org/meta-share/meta-share/mispronunciation">
        <rdf:type rdf:resource="http://w3id.org/meta-share/meta-share/AnnotatedElement"/>
        <rdfs:label xml:lang="en">mispronunciation</rdfs:label>
    </owl:NamedIndividual>
    


    <!-- http://w3id.org/meta-share/meta-share/mixed -->

    <owl:NamedIndividual rdf:about="http://w3id.org/meta-share/meta-share/mixed">
        <rdf:type rdf:resource="http://w3id.org/meta-share/meta-share/ProcessMode"/>
        <rdfs:comment xml:lang="en">Value for &apos;Process mode&apos; and its subclasses used for mixed processes, usually involving an automatic processing followed by human edits</rdfs:comment>
        <rdfs:label xml:lang="en">mixed</rdfs:label>
    </owl:NamedIndividual>
    


    <!-- http://w3id.org/meta-share/meta-share/mixedH -->

    <owl:NamedIndividual rdf:about="http://w3id.org/meta-share/meta-share/mixedH">
        <rdf:type rdf:resource="http://w3id.org/meta-share/meta-share/HearingImpairmentOfParticipants"/>
        <rdfs:label xml:lang="en">mixed</rdfs:label>
    </owl:NamedIndividual>
    


    <!-- http://w3id.org/meta-share/meta-share/mixedS -->

    <owl:NamedIndividual rdf:about="http://w3id.org/meta-share/meta-share/mixedS">
        <rdf:type rdf:resource="http://w3id.org/meta-share/meta-share/SpeakingImpairmentOfParticipants"/>
        <rdfs:label xml:lang="en">mixed</rdfs:label>
    </owl:NamedIndividual>
    


    <!-- http://w3id.org/meta-share/meta-share/modify -->

    <owl:NamedIndividual rdf:about="http://w3id.org/meta-share/meta-share/modify">
        <rdf:type rdf:resource="http://w3id.org/meta-share/meta-share/PreviousAnnotationTypesPolicy"/>
        <rdfs:label xml:lang="en">modify</rdfs:label>
    </owl:NamedIndividual>
    


    <!-- http://w3id.org/meta-share/meta-share/moneyAmount -->

    <owl:NamedIndividual rdf:about="http://w3id.org/meta-share/meta-share/moneyAmount">
        <rdf:type rdf:resource="http://w3id.org/meta-share/meta-share/SpeechItem"/>
        <rdfs:label xml:lang="en">money amount</rdfs:label>
    </owl:NamedIndividual>
    


    <!-- http://w3id.org/meta-share/meta-share/monolingual -->

    <owl:NamedIndividual rdf:about="http://w3id.org/meta-share/meta-share/monolingual">
        <rdf:type rdf:resource="http://w3id.org/meta-share/meta-share/LingualityType"/>
        <rdfs:comment xml:lang="en">Value for &apos;Linguality type&apos; for resource (parts) which include material in one language</rdfs:comment>
        <rdfs:label xml:lang="en">monolingual</rdfs:label>
    </owl:NamedIndividual>
    


    <!-- http://w3id.org/meta-share/meta-share/monologue -->

    <owl:NamedIndividual rdf:about="http://w3id.org/meta-share/meta-share/monologue">
        <rdf:type rdf:resource="http://w3id.org/meta-share/meta-share/ConversationalType"/>
        <rdfs:label xml:lang="en">monologue</rdfs:label>
    </owl:NamedIndividual>
    


    <!-- http://w3id.org/meta-share/meta-share/mood -->

    <owl:NamedIndividual rdf:about="http://w3id.org/meta-share/meta-share/mood">
        <rdf:type rdf:resource="http://w3id.org/meta-share/meta-share/MorphologicalType"/>
        <rdfs:label xml:lang="en">mood</rdfs:label>
    </owl:NamedIndividual>
    


    <!-- http://w3id.org/meta-share/meta-share/morphologicalLexicon -->

    <owl:NamedIndividual rdf:about="http://w3id.org/meta-share/meta-share/morphologicalLexicon">
        <rdf:type rdf:resource="http://w3id.org/meta-share/meta-share/CompatibleLexiconType"/>
        <rdf:type rdf:resource="http://w3id.org/meta-share/meta-share/LCRSubclass"/>
        <rdfs:comment xml:lang="en">a lexicon with morphological information associated with its entries</rdfs:comment>
        <rdfs:label xml:lang="en">morphological lexicon</rdfs:label>
    </owl:NamedIndividual>
    


    <!-- http://w3id.org/meta-share/meta-share/morphology -->

    <owl:NamedIndividual rdf:about="http://w3id.org/meta-share/meta-share/morphology">
        <rdf:type rdf:resource="http://w3id.org/meta-share/meta-share/EncodingLevel"/>
        <rdfs:comment xml:lang="en">Value for &apos;EncodingLevel&apos; for the particular linguistic level that relates to the study of word formation (such as inflection, derivation and compounding)</rdfs:comment>
        <rdfs:label xml:lang="en">morphology</rdfs:label>
    </owl:NamedIndividual>
    


    <!-- http://w3id.org/meta-share/meta-share/mouth -->

    <owl:NamedIndividual rdf:about="http://w3id.org/meta-share/meta-share/mouth">
        <rdf:type rdf:resource="http://w3id.org/meta-share/meta-share/BodyPart"/>
        <rdfs:label xml:lang="en">mouth</rdfs:label>
    </owl:NamedIndividual>
    


    <!-- http://w3id.org/meta-share/meta-share/mov -->

    <owl:NamedIndividual rdf:about="http://w3id.org/meta-share/meta-share/mov">
        <rdf:type rdf:resource="http://w3id.org/meta-share/meta-share/CompressionName"/>
        <rdfs:label xml:lang="en">mov</rdfs:label>
    </owl:NamedIndividual>
    


    <!-- http://w3id.org/meta-share/meta-share/mp3 -->

    <owl:NamedIndividual rdf:about="http://w3id.org/meta-share/meta-share/mp3">
        <rdf:type rdf:resource="http://w3id.org/meta-share/meta-share/CompressionName"/>
        <rdfs:label xml:lang="en">mp3</rdfs:label>
    </owl:NamedIndividual>
    


    <!-- http://w3id.org/meta-share/meta-share/mpeg -->

    <owl:NamedIndividual rdf:about="http://w3id.org/meta-share/meta-share/mpeg">
        <rdf:type rdf:resource="http://w3id.org/meta-share/meta-share/CompressionName"/>
        <rdfs:label xml:lang="en">mpeg</rdfs:label>
    </owl:NamedIndividual>
    


    <!-- http://w3id.org/meta-share/meta-share/mpg -->

    <owl:NamedIndividual rdf:about="http://w3id.org/meta-share/meta-share/mpg">
        <rdf:type rdf:resource="http://w3id.org/meta-share/meta-share/CompressionName"/>
        <rdfs:label xml:lang="en">mpg</rdfs:label>
    </owl:NamedIndividual>
    


    <!-- http://w3id.org/meta-share/meta-share/mu-law -->

    <owl:NamedIndividual rdf:about="http://w3id.org/meta-share/meta-share/mu-law">
        <rdf:type rdf:resource="http://w3id.org/meta-share/meta-share/SignalEncoding"/>
        <rdfs:label xml:lang="en">mu-law</rdfs:label>
    </owl:NamedIndividual>
    


    <!-- http://w3id.org/meta-share/meta-share/multiWordUnit -->

    <owl:NamedIndividual rdf:about="http://w3id.org/meta-share/meta-share/multiWordUnit">
        <rdf:type rdf:resource="http://w3id.org/meta-share/meta-share/SizeUnit"/>
        <rdfs:altLabel xml:lang="en">multi-word expression</rdfs:altLabel>
        <rdfs:label xml:lang="en">multi-word unit</rdfs:label>
    </owl:NamedIndividual>
    


    <!-- http://w3id.org/meta-share/meta-share/multiWordUnit1 -->

    <owl:NamedIndividual rdf:about="http://w3id.org/meta-share/meta-share/multiWordUnit1">
        <rdf:type rdf:resource="http://w3id.org/meta-share/meta-share/LemmaType"/>
        <rdfs:altLabel xml:lang="en">multi-word expression</rdfs:altLabel>
        <rdfs:label xml:lang="en">multi-word unit</rdfs:label>
    </owl:NamedIndividual>
    


    <!-- http://w3id.org/meta-share/meta-share/multilingual -->

    <owl:NamedIndividual rdf:about="http://w3id.org/meta-share/meta-share/multilingual">
        <rdf:type rdf:resource="http://w3id.org/meta-share/meta-share/LingualityType"/>
        <rdfs:comment xml:lang="en">Value for &apos;Linguality type&apos; for resource (parts) which include material in three or more languages</rdfs:comment>
        <rdfs:label xml:lang="en">multilingual</rdfs:label>
    </owl:NamedIndividual>
    


    <!-- http://w3id.org/meta-share/meta-share/multilingualSingleText -->

    <owl:NamedIndividual rdf:about="http://w3id.org/meta-share/meta-share/multilingualSingleText">
        <rdf:type rdf:resource="http://w3id.org/meta-share/meta-share/MultilingualityType"/>
        <rdfs:comment xml:lang="en">Value for &apos;Multilinguality type&apos; for resource parts or resources that consist of segments including text in two or more languages (e.g.,  the transcription of a European Parliament session with MPs speaking in their native language)</rdfs:comment>
        <rdfs:label xml:lang="en">multilingual single text</rdfs:label>
    </owl:NamedIndividual>
    


    <!-- http://w3id.org/meta-share/meta-share/multilogue -->

    <owl:NamedIndividual rdf:about="http://w3id.org/meta-share/meta-share/multilogue">
        <rdf:type rdf:resource="http://w3id.org/meta-share/meta-share/ConversationalType"/>
        <rdfs:label xml:lang="en">multilogue</rdfs:label>
    </owl:NamedIndividual>
    


    <!-- http://w3id.org/meta-share/meta-share/multipleSources -->

    <owl:NamedIndividual rdf:about="http://w3id.org/meta-share/meta-share/multipleSources">
        <rdf:type rdf:resource="http://w3id.org/meta-share/meta-share/SceneIllumination"/>
        <rdfs:label xml:lang="en">multiple sources</rdfs:label>
    </owl:NamedIndividual>
    


    <!-- http://w3id.org/meta-share/meta-share/music -->

    <owl:NamedIndividual rdf:about="http://w3id.org/meta-share/meta-share/music">
        <rdf:type rdf:resource="http://w3id.org/meta-share/meta-share/NonSpeechItem"/>
        <rdfs:label xml:lang="en">music</rdfs:label>
    </owl:NamedIndividual>
    


    <!-- http://w3id.org/meta-share/meta-share/music1 -->

    <owl:NamedIndividual rdf:about="http://w3id.org/meta-share/meta-share/music1">
        <rdf:type rdf:resource="http://w3id.org/meta-share/meta-share/Domain"/>
        <datacite:hasIdentifier rdf:resource="http://w3id.org/meta-share/meta-share/DDC780"/>
        <rdfs:label xml:lang="en">Music</rdfs:label>
    </owl:NamedIndividual>
    


    <!-- http://w3id.org/meta-share/meta-share/narrative -->

    <owl:NamedIndividual rdf:about="http://w3id.org/meta-share/meta-share/narrative">
        <rdf:type rdf:resource="http://w3id.org/meta-share/meta-share/SpeechGenre"/>
        <datacite:hasIdentifier rdf:resource="http://w3id.org/meta-share/meta-share/MS_SG008"/>
        <rdfs:label xml:lang="en">narrative</rdfs:label>
    </owl:NamedIndividual>
    


    <!-- http://w3id.org/meta-share/meta-share/nationalFunds -->

    <owl:NamedIndividual rdf:about="http://w3id.org/meta-share/meta-share/nationalFunds">
        <rdf:type rdf:resource="http://w3id.org/meta-share/meta-share/FundingType"/>
        <rdfs:comment xml:lang="en">Value for &apos;Funding type&apos; for projects funded by national authorities</rdfs:comment>
        <rdfs:label xml:lang="en">national funds</rdfs:label>
    </owl:NamedIndividual>
    


    <!-- http://w3id.org/meta-share/meta-share/nationalSecurity -->

    <owl:NamedIndividual rdf:about="http://w3id.org/meta-share/meta-share/nationalSecurity">
        <rdf:type rdf:resource="http://w3id.org/meta-share/meta-share/Domain"/>
        <datacite:hasIdentifier rdf:resource="http://w3id.org/meta-share/meta-share/ELG_Domain015"/>
        <rdfs:label xml:lang="en">national security</rdfs:label>
    </owl:NamedIndividual>
    


    <!-- http://w3id.org/meta-share/meta-share/native -->

    <owl:NamedIndividual rdf:about="http://w3id.org/meta-share/meta-share/native">
        <rdf:type rdf:resource="http://w3id.org/meta-share/meta-share/Origin"/>
        <rdfs:label xml:lang="en">native</rdfs:label>
    </owl:NamedIndividual>
    


    <!-- http://w3id.org/meta-share/meta-share/natural -->

    <owl:NamedIndividual rdf:about="http://w3id.org/meta-share/meta-share/natural">
        <rdf:type rdf:resource="http://w3id.org/meta-share/meta-share/Naturality"/>
        <rdfs:label xml:lang="en">natural</rdfs:label>
    </owl:NamedIndividual>
    


    <!-- http://w3id.org/meta-share/meta-share/naturalNumber -->

    <owl:NamedIndividual rdf:about="http://w3id.org/meta-share/meta-share/naturalNumber">
        <rdf:type rdf:resource="http://w3id.org/meta-share/meta-share/SpeechItem"/>
        <rdfs:label xml:lang="en">natural number</rdfs:label>
    </owl:NamedIndividual>
    


    <!-- http://w3id.org/meta-share/meta-share/neologism -->

    <owl:NamedIndividual rdf:about="http://w3id.org/meta-share/meta-share/neologism">
        <rdf:type rdf:resource="http://w3id.org/meta-share/meta-share/SizeUnit"/>
        <rdfs:label xml:lang="en">neologism</rdfs:label>
    </owl:NamedIndividual>
    


    <!-- http://w3id.org/meta-share/meta-share/network -->

    <owl:NamedIndividual rdf:about="http://w3id.org/meta-share/meta-share/network">
        <rdf:type rdf:resource="http://w3id.org/meta-share/meta-share/OrganizationLegalStatus"/>
        <rdfs:label xml:lang="en">network</rdfs:label>
    </owl:NamedIndividual>
    


    <!-- http://w3id.org/meta-share/meta-share/newsMediaJournalismAndPublishing -->

    <owl:NamedIndividual rdf:about="http://w3id.org/meta-share/meta-share/newsMediaJournalismAndPublishing">
        <rdf:type rdf:resource="http://w3id.org/meta-share/meta-share/Domain"/>
        <datacite:hasIdentifier rdf:resource="http://w3id.org/meta-share/meta-share/DDC070"/>
        <rdfs:label xml:lang="en">News, Media, Journalism &amp; Publishing</rdfs:label>
    </owl:NamedIndividual>
    


    <!-- http://w3id.org/meta-share/meta-share/no -->

    <owl:NamedIndividual rdf:about="http://w3id.org/meta-share/meta-share/no">
        <rdf:type rdf:resource="http://w3id.org/meta-share/meta-share/SpeakingImpairmentOfParticipants"/>
        <rdfs:label xml:lang="en">no</rdfs:label>
    </owl:NamedIndividual>
    


    <!-- http://w3id.org/meta-share/meta-share/noCopyright -->

    <owl:NamedIndividual rdf:about="http://w3id.org/meta-share/meta-share/noCopyright">
        <rdf:type rdf:resource="http://w3id.org/meta-share/meta-share/AccessRightsStatement"/>
        <datacite:hasIdentifier rdf:resource="http://rightsstatements.org/vocab/NoC-OKLR/1.0/"/>
    </owl:NamedIndividual>
    


    <!-- http://w3id.org/meta-share/meta-share/noCopyrightContract -->

    <owl:NamedIndividual rdf:about="http://w3id.org/meta-share/meta-share/noCopyrightContract">
        <rdf:type rdf:resource="http://w3id.org/meta-share/meta-share/AccessRightsStatement"/>
        <datacite:hasIdentifier rdf:resource="http://rightsstatements.org/vocab/NoC-CR/1.0/"/>
    </owl:NamedIndividual>
    


    <!-- http://w3id.org/meta-share/meta-share/noCopyrightNC -->

    <owl:NamedIndividual rdf:about="http://w3id.org/meta-share/meta-share/noCopyrightNC">
        <rdf:type rdf:resource="http://w3id.org/meta-share/meta-share/AccessRightsStatement"/>
        <datacite:hasIdentifier rdf:resource="http://rightsstatements.org/vocab/NoC-NC/1.0/"/>
    </owl:NamedIndividual>
    


    <!-- http://w3id.org/meta-share/meta-share/noCopyrightUS -->

    <owl:NamedIndividual rdf:about="http://w3id.org/meta-share/meta-share/noCopyrightUS">
        <rdf:type rdf:resource="http://w3id.org/meta-share/meta-share/AccessRightsStatement"/>
        <datacite:hasIdentifier rdf:resource="http://rightsstatements.org/vocab/NoC-US/1.0/"/>
    </owl:NamedIndividual>
    


    <!-- http://w3id.org/meta-share/meta-share/noDerivatives -->

    <owl:NamedIndividual rdf:about="http://w3id.org/meta-share/meta-share/noDerivatives">
        <rdf:type rdf:resource="http://w3id.org/meta-share/meta-share/ConditionOfUse"/>
        <rdf:type rdf:resource="http://www.w3.org/ns/odrl/2/Set"/>
        <rdfs:comment xml:lang="en">Value for &apos;ConditionOfUse&apos; which states that the users of the resource are not allowed to share derivatives of the resource</rdfs:comment>
        <rdfs:label xml:lang="en">no derivatives</rdfs:label>
        <odrl:prohibition>
            <rdf:Description>
                <odrl:action rdf:resource="http://creativecommons.org/ns#DerivativeWorks"/>
            </rdf:Description>
        </odrl:prohibition>
    </owl:NamedIndividual>
    


    <!-- http://w3id.org/meta-share/meta-share/noH -->

    <owl:NamedIndividual rdf:about="http://w3id.org/meta-share/meta-share/noH">
        <rdf:type rdf:resource="http://w3id.org/meta-share/meta-share/HearingImpairmentOfParticipants"/>
        <rdfs:label xml:lang="en">no</rdfs:label>
    </owl:NamedIndividual>
    


    <!-- http://w3id.org/meta-share/meta-share/noKnownCopyright -->

    <owl:NamedIndividual rdf:about="http://w3id.org/meta-share/meta-share/noKnownCopyright">
        <rdf:type rdf:resource="http://w3id.org/meta-share/meta-share/AccessRightsStatement"/>
        <datacite:hasIdentifier rdf:resource="http://rightsstatements.org/vocab/NKC/1.0/"/>
    </owl:NamedIndividual>
    


    <!-- http://w3id.org/meta-share/meta-share/noRedistribution -->

    <owl:NamedIndividual rdf:about="http://w3id.org/meta-share/meta-share/noRedistribution">
        <rdf:type rdf:resource="http://w3id.org/meta-share/meta-share/ConditionOfUse"/>
        <rdfs:comment xml:lang="en">Value for &apos;ConditionOfUse&apos; which states that users are not allowed to redistribute the resource</rdfs:comment>
        <rdfs:label xml:lang="en">no redistribution</rdfs:label>
        <odrl:prohibition>
            <rdf:Description>
                <odrl:action rdf:resource="http://creativecommons.org/ns#Reproduction"/>
            </rdf:Description>
        </odrl:prohibition>
    </owl:NamedIndividual>
    


    <!-- http://w3id.org/meta-share/meta-share/noise -->

    <owl:NamedIndividual rdf:about="http://w3id.org/meta-share/meta-share/noise">
        <rdf:type rdf:resource="http://w3id.org/meta-share/meta-share/NonSpeechItem"/>
        <rdfs:label xml:lang="en">noise</rdfs:label>
    </owl:NamedIndividual>
    


    <!-- http://w3id.org/meta-share/meta-share/noise1 -->

    <owl:NamedIndividual rdf:about="http://w3id.org/meta-share/meta-share/noise1">
        <rdf:type rdf:resource="http://w3id.org/meta-share/meta-share/AudioGenre"/>
        <datacite:hasIdentifier rdf:resource="http://w3id.org/meta-share/meta-share/MS_AG002"/>
        <rdfs:label xml:lang="en">noise</rdfs:label>
    </owl:NamedIndividual>
    


    <!-- http://w3id.org/meta-share/meta-share/nonCommercialUse -->

    <owl:NamedIndividual rdf:about="http://w3id.org/meta-share/meta-share/nonCommercialUse">
        <rdf:type rdf:resource="http://w3id.org/meta-share/meta-share/ConditionOfUse"/>
        <rdf:type rdf:resource="http://www.w3.org/ns/odrl/2/Set"/>
        <rdfs:comment xml:lang="en">Value for &apos;ConditionOfUse&apos; which states that the language resource cannot be used for commercial purposes, i.e. where there is some direct profit from using it</rdfs:comment>
        <rdfs:label xml:lang="en">non-commercial use</rdfs:label>
        <odrl:prohibition>
            <rdf:Description>
                <odrl:action rdf:resource="https://creativecommons.org/ns#CommercialUse"/>
            </rdf:Description>
        </odrl:prohibition>
    </owl:NamedIndividual>
    


    <!-- http://w3id.org/meta-share/meta-share/nonFiction -->

    <owl:NamedIndividual rdf:about="http://w3id.org/meta-share/meta-share/nonFiction">
        <rdf:type rdf:resource="http://w3id.org/meta-share/meta-share/TextGenre"/>
        <datacite:hasIdentifier rdf:resource="http://w3id.org/meta-share/meta-share/PAROLE_G008"/>
        <rdfs:label xml:lang="en">non fiction</rdfs:label>
    </owl:NamedIndividual>
    


    <!-- http://w3id.org/meta-share/meta-share/nonInteractive -->

    <owl:NamedIndividual rdf:about="http://w3id.org/meta-share/meta-share/nonInteractive">
        <rdf:type rdf:resource="http://w3id.org/meta-share/meta-share/Interactivity"/>
        <rdfs:label xml:lang="en">non interactive</rdfs:label>
    </owl:NamedIndividual>
    


    <!-- http://w3id.org/meta-share/meta-share/nonNative -->

    <owl:NamedIndividual rdf:about="http://w3id.org/meta-share/meta-share/nonNative">
        <rdf:type rdf:resource="http://w3id.org/meta-share/meta-share/Origin"/>
        <rdfs:label xml:lang="en">nonNative</rdfs:label>
    </owl:NamedIndividual>
    


    <!-- http://w3id.org/meta-share/meta-share/none -->

    <owl:NamedIndividual rdf:about="http://w3id.org/meta-share/meta-share/none">
        <rdf:type rdf:resource="http://w3id.org/meta-share/meta-share/BodyPart"/>
        <rdfs:label xml:lang="en">none</rdfs:label>
    </owl:NamedIndividual>
    


    <!-- http://w3id.org/meta-share/meta-share/none1 -->

    <owl:NamedIndividual rdf:about="http://w3id.org/meta-share/meta-share/none1">
        <rdf:type rdf:resource="http://w3id.org/meta-share/meta-share/TextIncludedInVideo"/>
        <rdfs:label xml:lang="en">none</rdfs:label>
    </owl:NamedIndividual>
    


    <!-- http://w3id.org/meta-share/meta-share/none2 -->

    <owl:NamedIndividual rdf:about="http://w3id.org/meta-share/meta-share/none2">
        <rdf:type rdf:resource="http://w3id.org/meta-share/meta-share/TextIncludedInImage"/>
        <rdfs:label xml:lang="en">none</rdfs:label>
    </owl:NamedIndividual>
    


    <!-- http://w3id.org/meta-share/meta-share/none3 -->

    <owl:NamedIndividual rdf:about="http://w3id.org/meta-share/meta-share/none3">
        <rdf:type rdf:resource="http://w3id.org/meta-share/meta-share/Audience"/>
        <rdfs:label xml:lang="en">none</rdfs:label>
    </owl:NamedIndividual>
    


    <!-- http://w3id.org/meta-share/meta-share/none4 -->

    <owl:NamedIndividual rdf:about="http://w3id.org/meta-share/meta-share/none4">
        <rdf:type rdf:resource="http://w3id.org/meta-share/meta-share/RelatedLexiconType"/>
        <rdfs:label xml:lang="en">none</rdfs:label>
    </owl:NamedIndividual>
    


    <!-- http://w3id.org/meta-share/meta-share/none5 -->

    <owl:NamedIndividual rdf:about="http://w3id.org/meta-share/meta-share/none5">
        <rdf:type rdf:resource="http://w3id.org/meta-share/meta-share/RequiredHardware"/>
        <rdfs:label xml:lang="en">none</rdfs:label>
    </owl:NamedIndividual>
    


    <!-- http://w3id.org/meta-share/meta-share/note -->

    <owl:NamedIndividual rdf:about="http://w3id.org/meta-share/meta-share/note">
        <rdf:type rdf:resource="http://w3id.org/meta-share/meta-share/NonSpeechItem"/>
        <rdfs:label xml:lang="en">note</rdfs:label>
    </owl:NamedIndividual>
    


    <!-- http://w3id.org/meta-share/meta-share/note1 -->

    <owl:NamedIndividual rdf:about="http://w3id.org/meta-share/meta-share/note1">
        <rdf:type rdf:resource="http://w3id.org/meta-share/meta-share/UsageType"/>
        <rdfs:label xml:lang="en">note</rdfs:label>
    </owl:NamedIndividual>
    


    <!-- http://w3id.org/meta-share/meta-share/npRecognition -->

    <owl:NamedIndividual rdf:about="http://w3id.org/meta-share/meta-share/npRecognition">
        <rdf:type rdf:resource="http://w3id.org/meta-share/meta-share/LDTask"/>
        <rdfs:label xml:lang="en">recognition of noun phrases</rdfs:label>
    </owl:NamedIndividual>
    


    <!-- http://w3id.org/meta-share/meta-share/npStructure -->

    <owl:NamedIndividual rdf:about="http://w3id.org/meta-share/meta-share/npStructure">
        <rdf:type rdf:resource="http://w3id.org/meta-share/meta-share/GrammaticalPhenomenaCoverage"/>
        <rdfs:altLabel xml:lang="en">Structure of noun phrases</rdfs:altLabel>
        <rdfs:label xml:lang="en">NP structure</rdfs:label>
    </owl:NamedIndividual>
    


    <!-- http://w3id.org/meta-share/meta-share/number -->

    <owl:NamedIndividual rdf:about="http://w3id.org/meta-share/meta-share/number">
        <rdf:type rdf:resource="http://w3id.org/meta-share/meta-share/MorphologicalType"/>
        <rdfs:label xml:lang="en">number</rdfs:label>
    </owl:NamedIndividual>
    


    <!-- http://w3id.org/meta-share/meta-share/oai -->

    <owl:NamedIndividual rdf:about="http://w3id.org/meta-share/meta-share/oai">
        <rdf:type rdf:resource="http://w3id.org/meta-share/meta-share/LRIdentifierScheme"/>
        <ms:url>http://www.openarchives.org/OAI/2.0/guidelines-oai-identifier.htm</ms:url>
        <rdfs:comment xml:lang="en">Value for LRTIdentifierScheme referring to the OAI identifier (Open Archives Initiative, http://www.openarchives.org/OAI/2.0/guidelines-oai-identifier.htm)</rdfs:comment>
        <rdfs:label xml:lang="en">OAI</rdfs:label>
    </owl:NamedIndividual>
    


    <!-- http://w3id.org/meta-share/meta-share/ocrSystem -->

    <owl:NamedIndividual rdf:about="http://w3id.org/meta-share/meta-share/ocrSystem">
        <rdf:type rdf:resource="http://w3id.org/meta-share/meta-share/RequiredHardware"/>
        <rdfs:label xml:lang="en">OCR system</rdfs:label>
    </owl:NamedIndividual>
    


    <!-- http://w3id.org/meta-share/meta-share/office -->

    <owl:NamedIndividual rdf:about="http://w3id.org/meta-share/meta-share/office">
        <rdf:type rdf:resource="http://w3id.org/meta-share/meta-share/RecordingEnvironment"/>
        <rdfs:label xml:lang="en">office</rdfs:label>
    </owl:NamedIndividual>
    


    <!-- http://w3id.org/meta-share/meta-share/official -->

    <owl:NamedIndividual rdf:about="http://w3id.org/meta-share/meta-share/official">
        <rdf:type rdf:resource="http://w3id.org/meta-share/meta-share/TextGenre"/>
        <datacite:hasIdentifier rdf:resource="http://w3id.org/meta-share/meta-share/PAROLE_G009"/>
        <rdfs:label xml:lang="en">official</rdfs:label>
    </owl:NamedIndividual>
    


    <!-- http://w3id.org/meta-share/meta-share/oggVorbis -->

    <owl:NamedIndividual rdf:about="http://w3id.org/meta-share/meta-share/oggVorbis">
        <rdf:type rdf:resource="http://w3id.org/meta-share/meta-share/CompressionName"/>
        <rdfs:label xml:lang="en">Ogg Vorbis</rdfs:label>
    </owl:NamedIndividual>
    


    <!-- http://w3id.org/meta-share/meta-share/omtd -->

    <owl:NamedIndividual rdf:about="http://w3id.org/meta-share/meta-share/omtd">
        <rdf:type rdf:resource="http://w3id.org/meta-share/meta-share/LRIdentifierScheme"/>
        <rdf:type rdf:resource="http://w3id.org/meta-share/meta-share/MetadataRecordIdentifierScheme"/>
        <ms:url>https://services.openminted.eu/home</ms:url>
        <rdfs:comment xml:lang="en">Value for LRTIdentifierScheme referring to the identifier assigned by the OpenMinTeD platform (https://services.openminted.eu/home)</rdfs:comment>
        <rdfs:label xml:lang="en">OMTD</rdfs:label>
    </owl:NamedIndividual>
    


    <!-- http://w3id.org/meta-share/meta-share/omtdAccess1 -->

    <owl:NamedIndividual rdf:about="http://w3id.org/meta-share/meta-share/omtdAccess1">
        <rdf:type rdf:resource="http://w3id.org/meta-share/meta-share/AccessRightsStatementIdentifier"/>
        <ms:conformsTo rdf:resource="http://w3id.org/meta-share/meta-share/OMTDShareRightsStatementScheme"/>
    </owl:NamedIndividual>
    


    <!-- http://w3id.org/meta-share/meta-share/omtdAccess2 -->

    <owl:NamedIndividual rdf:about="http://w3id.org/meta-share/meta-share/omtdAccess2">
        <rdf:type rdf:resource="http://w3id.org/meta-share/meta-share/AccessRightsStatementIdentifier"/>
        <ms:conformsTo rdf:resource="http://w3id.org/meta-share/meta-share/OMTDShareRightsStatementScheme"/>
    </owl:NamedIndividual>
    


    <!-- http://w3id.org/meta-share/meta-share/omtdDocker -->

    <owl:NamedIndividual rdf:about="http://w3id.org/meta-share/meta-share/omtdDocker">
        <rdf:type rdf:resource="http://w3id.org/meta-share/meta-share/LRIdentifierScheme"/>
        <ms:url>https://guidelines.openminted.eu/components_resourceIdentifier.html</ms:url>
        <rdfs:comment xml:lang="en">Value for LRTIdentifierScheme referring to the recommended by OpenMinTeD use of identifiers for Docker images uploaded to the registry (https://guidelines.openminted.eu/components_resourceIdentifier.html)</rdfs:comment>
        <rdfs:label xml:lang="en">OMTD-Docker</rdfs:label>
    </owl:NamedIndividual>
    


    <!-- http://w3id.org/meta-share/meta-share/onLineHelpURL -->

    <owl:NamedIndividual rdf:about="http://w3id.org/meta-share/meta-share/onLineHelpURL">
        <rdf:type rdf:resource="http://w3id.org/meta-share/meta-share/DocumentationType"/>
        <rdfs:comment xml:lang="en">Value for &apos;Documentation type&apos; for the online help site of a language resource</rdfs:comment>
        <rdfs:label xml:lang="en">online help URL</rdfs:label>
    </owl:NamedIndividual>
    


    <!-- http://w3id.org/meta-share/meta-share/onlineEducationalGame -->

    <owl:NamedIndividual rdf:about="http://w3id.org/meta-share/meta-share/onlineEducationalGame">
        <rdf:type rdf:resource="http://w3id.org/meta-share/meta-share/ScenarioType"/>
        <rdfs:label xml:lang="en">online educational game</rdfs:label>
    </owl:NamedIndividual>
    


    <!-- http://w3id.org/meta-share/meta-share/onlyMSmembers -->

    <owl:NamedIndividual rdf:about="http://w3id.org/meta-share/meta-share/onlyMSmembers">
        <rdf:type rdf:resource="http://w3id.org/meta-share/meta-share/ConditionOfUse"/>
        <rdf:type rdf:resource="http://www.w3.org/ns/odrl/2/Set"/>
        <rdfs:comment xml:lang="en">Value for &apos;ConditionsOfUse&apos; which states that the language resource can only be used by members of the MetaShare network</rdfs:comment>
        <rdfs:label xml:lang="en">only META-SHARE members</rdfs:label>
        <skos:note xml:lang="en">should we also add something more generic for restricting a resource to specific group members (as for spatial constraint)? and I don&apos;t think the odrl is ok.</skos:note>
        <odrl:permission>
            <rdf:Description>
                <odrl:constraint>
                    <rdf:Description>
                        <odrl:operator rdf:resource="http://www.w3.org/ns/odrl/2/eq"/>
                        <odrl:recipient rdf:resource="http://w3id.org/meta-share/meta-share/onlyMSmembers"/>
                    </rdf:Description>
                </odrl:constraint>
            </rdf:Description>
        </odrl:permission>
    </owl:NamedIndividual>
    


    <!-- http://w3id.org/meta-share/meta-share/ontology -->

    <owl:NamedIndividual rdf:about="http://w3id.org/meta-share/meta-share/ontology">
        <rdf:type rdf:resource="http://w3id.org/meta-share/meta-share/CompatibleLexiconType"/>
        <rdf:type rdf:resource="http://w3id.org/meta-share/meta-share/LCRSubclass"/>
        <rdfs:comment xml:lang="en">a set of concepts and categories in a subject area or domain that shows their properties and the relations between them [https://en.oxforddictionaries.com/definition/ontology]</rdfs:comment>
        <rdfs:label xml:lang="en">ontology</rdfs:label>
    </owl:NamedIndividual>
    


    <!-- http://w3id.org/meta-share/meta-share/openAccess -->

    <owl:NamedIndividual rdf:about="http://w3id.org/meta-share/meta-share/openAccess">
        <rdf:type rdf:resource="http://w3id.org/meta-share/meta-share/AccessRightsStatement"/>
        <datacite:hasIdentifier rdf:resource="http://w3id.org/meta-share/meta-share/omtdAccess2"/>
        <rdfs:comment xml:lang="en">The free and online availability of literature, which allows to read, download, copy, distribute, print, search, or link to the ful text, crawl articles for indexing, pass them as data to software, or use them for any other useful purpose. An availability that is granted without financial, legal, or technical barriers other than those inseparable from gaining access to the internet itself, and those related to giving authors control over the integrity of their work and the right to be properly acknowledged and cited.</rdfs:comment>
        <rdfs:label xml:lang="en">open access</rdfs:label>
        <skos:closeMatch rdf:resource="http://purl.org/coar/access_right/c_abf2"/>
        <skos:closeMatch rdf:resource="http://purl.org/eprint/accessRights/OpenAccess"/>
    </owl:NamedIndividual>
    


    <!-- http://w3id.org/meta-share/meta-share/openAccess1 -->

    <owl:NamedIndividual rdf:about="http://w3id.org/meta-share/meta-share/openAccess1">
        <rdf:type rdf:resource="http://w3id.org/meta-share/meta-share/AccessRightsStatement"/>
        <datacite:hasIdentifier rdf:resource="http://purl.org/coar/access_right/c_abf2"/>
    </owl:NamedIndividual>
    


    <!-- http://w3id.org/meta-share/meta-share/openPublicPlace -->

    <owl:NamedIndividual rdf:about="http://w3id.org/meta-share/meta-share/openPublicPlace">
        <rdf:type rdf:resource="http://w3id.org/meta-share/meta-share/RecordingEnvironment"/>
        <rdfs:label xml:lang="en">open public place</rdfs:label>
    </owl:NamedIndividual>
    


    <!-- http://w3id.org/meta-share/meta-share/os-independent -->

    <owl:NamedIndividual rdf:about="http://w3id.org/meta-share/meta-share/os-independent">
        <rdf:type rdf:resource="http://w3id.org/meta-share/meta-share/OperatingSystem"/>
        <rdfs:label xml:lang="en">OS-independent</rdfs:label>
    </owl:NamedIndividual>
    


    <!-- http://w3id.org/meta-share/meta-share/other -->

    <owl:NamedIndividual rdf:about="http://w3id.org/meta-share/meta-share/other">
        <rdf:type rdf:resource="http://purl.org/spar/datacite/FunderIdentifierScheme"/>
        <rdf:type rdf:resource="http://purl.org/spar/datacite/OrganizationIdentifierScheme"/>
        <rdf:type rdf:resource="http://purl.org/spar/datacite/PersonalIdentifierScheme"/>
        <rdf:type rdf:resource="http://w3id.org/meta-share/meta-share/AnnotatedElement"/>
        <rdf:type rdf:resource="http://w3id.org/meta-share/meta-share/AudioGenre"/>
        <rdf:type rdf:resource="http://w3id.org/meta-share/meta-share/AudioGenreClassificationScheme"/>
        <rdf:type rdf:resource="http://w3id.org/meta-share/meta-share/AudioQualityMeasureIncluded"/>
        <rdf:type rdf:resource="http://w3id.org/meta-share/meta-share/BaseItem"/>
        <rdf:type rdf:resource="http://w3id.org/meta-share/meta-share/CapturingDeviceType"/>
        <rdf:type rdf:resource="http://w3id.org/meta-share/meta-share/CompatibleLexiconType"/>
        <rdf:type rdf:resource="http://w3id.org/meta-share/meta-share/CompressionName"/>
        <rdf:type rdf:resource="http://w3id.org/meta-share/meta-share/ConditionOfUse"/>
        <rdf:type rdf:resource="http://w3id.org/meta-share/meta-share/ContentType"/>
        <rdf:type rdf:resource="http://w3id.org/meta-share/meta-share/DatasetDistributionForm"/>
        <rdf:type rdf:resource="http://w3id.org/meta-share/meta-share/DivisionCategory"/>
        <rdf:type rdf:resource="http://w3id.org/meta-share/meta-share/DocumentIdentifierScheme"/>
        <rdf:type rdf:resource="http://w3id.org/meta-share/meta-share/DocumentType"/>
        <rdf:type rdf:resource="http://w3id.org/meta-share/meta-share/Domain"/>
        <rdf:type rdf:resource="http://w3id.org/meta-share/meta-share/DomainClassificationScheme"/>
        <rdf:type rdf:resource="http://w3id.org/meta-share/meta-share/EncodingLevel"/>
        <rdf:type rdf:resource="http://w3id.org/meta-share/meta-share/ExtratextualInformation"/>
        <rdf:type rdf:resource="http://w3id.org/meta-share/meta-share/ExtratextualInformationUnit"/>
        <rdf:type rdf:resource="http://w3id.org/meta-share/meta-share/Framework"/>
        <rdf:type rdf:resource="http://w3id.org/meta-share/meta-share/FundingType"/>
        <rdf:type rdf:resource="http://w3id.org/meta-share/meta-share/GrammaticalPhenomenaCoverage"/>
        <rdf:type rdf:resource="http://w3id.org/meta-share/meta-share/ImageGenreClassificationScheme"/>
        <rdf:type rdf:resource="http://w3id.org/meta-share/meta-share/Interactivity"/>
        <rdf:type rdf:resource="http://w3id.org/meta-share/meta-share/LCRSubclass"/>
        <rdf:type rdf:resource="http://w3id.org/meta-share/meta-share/LDTask"/>
        <rdf:type rdf:resource="http://w3id.org/meta-share/meta-share/LRIdentifierScheme"/>
        <rdf:type rdf:resource="http://w3id.org/meta-share/meta-share/LanguageVarietyType"/>
        <rdf:type rdf:resource="http://w3id.org/meta-share/meta-share/LicenceIdentifierScheme"/>
        <rdf:type rdf:resource="http://w3id.org/meta-share/meta-share/MembershipInstitution"/>
        <rdf:type rdf:resource="http://w3id.org/meta-share/meta-share/MetadataRecordIdentifierScheme"/>
        <rdf:type rdf:resource="http://w3id.org/meta-share/meta-share/Metric"/>
        <rdf:type rdf:resource="http://w3id.org/meta-share/meta-share/ModalityType"/>
        <rdf:type rdf:resource="http://w3id.org/meta-share/meta-share/MultilingualityType"/>
        <rdf:type rdf:resource="http://w3id.org/meta-share/meta-share/Naturality"/>
        <rdf:type rdf:resource="http://w3id.org/meta-share/meta-share/NonSpeechItem"/>
        <rdf:type rdf:resource="http://w3id.org/meta-share/meta-share/OperatingSystem"/>
        <rdf:type rdf:resource="http://w3id.org/meta-share/meta-share/OrganizationLegalStatus"/>
        <rdf:type rdf:resource="http://w3id.org/meta-share/meta-share/OrganizationRole"/>
        <rdf:type rdf:resource="http://w3id.org/meta-share/meta-share/ParameterType"/>
        <rdf:type rdf:resource="http://w3id.org/meta-share/meta-share/ProcessingResourceType"/>
        <rdf:type rdf:resource="http://w3id.org/meta-share/meta-share/ProjectIdentifierScheme"/>
        <rdf:type rdf:resource="http://w3id.org/meta-share/meta-share/RecordingDeviceType"/>
        <rdf:type rdf:resource="http://w3id.org/meta-share/meta-share/RecordingEnvironment"/>
        <rdf:type rdf:resource="http://w3id.org/meta-share/meta-share/RequiredHardware"/>
        <rdf:type rdf:resource="http://w3id.org/meta-share/meta-share/ScenarioType"/>
        <rdf:type rdf:resource="http://w3id.org/meta-share/meta-share/SceneIllumination"/>
        <rdf:type rdf:resource="http://w3id.org/meta-share/meta-share/SegmentationLevel"/>
        <rdf:type rdf:resource="http://w3id.org/meta-share/meta-share/SignalEncoding"/>
        <rdf:type rdf:resource="http://w3id.org/meta-share/meta-share/SizeUnit"/>
        <rdf:type rdf:resource="http://w3id.org/meta-share/meta-share/SocialMediaOccupationalAccountType"/>
        <rdf:type rdf:resource="http://w3id.org/meta-share/meta-share/SoftwareDistributionForm"/>
        <rdf:type rdf:resource="http://w3id.org/meta-share/meta-share/SourceChannel"/>
        <rdf:type rdf:resource="http://w3id.org/meta-share/meta-share/SourceChannelType"/>
        <rdf:type rdf:resource="http://w3id.org/meta-share/meta-share/SpeechGenre"/>
        <rdf:type rdf:resource="http://w3id.org/meta-share/meta-share/SpeechGenreClassificationScheme"/>
        <rdf:type rdf:resource="http://w3id.org/meta-share/meta-share/SpeechInfluence"/>
        <rdf:type rdf:resource="http://w3id.org/meta-share/meta-share/SpeechItem"/>
        <rdf:type rdf:resource="http://w3id.org/meta-share/meta-share/StandardBestPractice"/>
        <rdf:type rdf:resource="http://w3id.org/meta-share/meta-share/SubjectClassificationScheme"/>
        <rdf:type rdf:resource="http://w3id.org/meta-share/meta-share/TextGenre"/>
        <rdf:type rdf:resource="http://w3id.org/meta-share/meta-share/TextGenreClassificationScheme"/>
        <rdf:type rdf:resource="http://w3id.org/meta-share/meta-share/TextType"/>
        <rdf:type rdf:resource="http://w3id.org/meta-share/meta-share/TextTypeClassificationScheme"/>
        <rdf:type rdf:resource="http://w3id.org/meta-share/meta-share/VideoGenreClassificationScheme"/>
        <rdf:type rdf:resource="http://w3id.org/meta-share/meta-share/VocalTractCondition"/>
        <rdf:type rdf:resource="http://w3id.org/meta-share/meta-share/WebServiceType"/>
        <rdfs:label xml:lang="en">other</rdfs:label>
    </owl:NamedIndividual>
    


    <!-- http://w3id.org/meta-share/meta-share/outputText -->

    <owl:NamedIndividual rdf:about="http://w3id.org/meta-share/meta-share/outputText">
        <rdf:type rdf:resource="http://w3id.org/meta-share/meta-share/ProcessingResourceType"/>
        <rdfs:label xml:lang="en">output text</rdfs:label>
    </owl:NamedIndividual>
    


    <!-- http://w3id.org/meta-share/meta-share/overlapping -->

    <owl:NamedIndividual rdf:about="http://w3id.org/meta-share/meta-share/overlapping">
        <rdf:type rdf:resource="http://w3id.org/meta-share/meta-share/Interactivity"/>
        <rdfs:label xml:lang="en">overlapping</rdfs:label>
    </owl:NamedIndividual>
    


    <!-- http://w3id.org/meta-share/meta-share/ownFunds -->

    <owl:NamedIndividual rdf:about="http://w3id.org/meta-share/meta-share/ownFunds">
        <rdf:type rdf:resource="http://w3id.org/meta-share/meta-share/FundingType"/>
        <rdfs:comment xml:lang="en">Value for &apos;Funding type&apos; for self-funded projects</rdfs:comment>
        <rdfs:label xml:lang="en">own funds</rdfs:label>
    </owl:NamedIndividual>
    


    <!-- http://w3id.org/meta-share/meta-share/painting -->

    <owl:NamedIndividual rdf:about="http://w3id.org/meta-share/meta-share/painting">
        <rdf:type rdf:resource="http://w3id.org/meta-share/meta-share/Domain"/>
        <datacite:hasIdentifier rdf:resource="http://w3id.org/meta-share/meta-share/DDC750"/>
        <rdfs:label xml:lang="en">Painting</rdfs:label>
    </owl:NamedIndividual>
    


    <!-- http://w3id.org/meta-share/meta-share/paleontology -->

    <owl:NamedIndividual rdf:about="http://w3id.org/meta-share/meta-share/paleontology">
        <rdf:type rdf:resource="http://w3id.org/meta-share/meta-share/Domain"/>
        <datacite:hasIdentifier rdf:resource="http://w3id.org/meta-share/meta-share/DDC560"/>
        <rdfs:label xml:lang="en">Paleontology</rdfs:label>
    </owl:NamedIndividual>
    


    <!-- http://w3id.org/meta-share/meta-share/paperCopy -->

    <owl:NamedIndividual rdf:about="http://w3id.org/meta-share/meta-share/paperCopy">
        <rdf:type rdf:resource="http://w3id.org/meta-share/meta-share/DatasetDistributionForm"/>
        <rdfs:comment xml:lang="en">Value for data distribution medium, used for language resources that are delivered in paper format</rdfs:comment>
        <rdfs:label xml:lang="en">paper copy</rdfs:label>
    </owl:NamedIndividual>
    


    <!-- http://w3id.org/meta-share/meta-share/paragraph -->

    <owl:NamedIndividual rdf:about="http://w3id.org/meta-share/meta-share/paragraph">
        <rdf:type rdf:resource="http://w3id.org/meta-share/meta-share/SegmentationLevel"/>
        <rdfs:label xml:lang="en">paragraph</rdfs:label>
    </owl:NamedIndividual>
    


    <!-- http://w3id.org/meta-share/meta-share/parallel -->

    <owl:NamedIndividual rdf:about="http://w3id.org/meta-share/meta-share/parallel">
        <rdf:type rdf:resource="http://w3id.org/meta-share/meta-share/MultilingualityType"/>
        <rdfs:comment xml:lang="en">Value for &apos;Multilinguality type&apos; for resource parts or resources that consist of the equivalent text segments in two or more languages (e.g.,  an original and its translation equivalents)</rdfs:comment>
        <rdfs:label xml:lang="en">parallel</rdfs:label>
    </owl:NamedIndividual>
    


    <!-- http://w3id.org/meta-share/meta-share/parsing -->

    <owl:NamedIndividual rdf:about="http://w3id.org/meta-share/meta-share/parsing">
        <rdf:type rdf:resource="http://w3id.org/meta-share/meta-share/LDTask"/>
        <rdfs:label xml:lang="en">parsing</rdfs:label>
    </owl:NamedIndividual>
    


    <!-- http://w3id.org/meta-share/meta-share/partOfSpeech -->

    <owl:NamedIndividual rdf:about="http://w3id.org/meta-share/meta-share/partOfSpeech">
        <rdf:type rdf:resource="http://w3id.org/meta-share/meta-share/MorphologicalType"/>
        <rdfs:label xml:lang="en">part of speech</rdfs:label>
    </owl:NamedIndividual>
    


    <!-- http://w3id.org/meta-share/meta-share/partial -->

    <owl:NamedIndividual rdf:about="http://w3id.org/meta-share/meta-share/partial">
        <rdf:type rdf:resource="http://w3id.org/meta-share/meta-share/ValidationExtent"/>
        <rdfs:label xml:lang="en">partial</rdfs:label>
    </owl:NamedIndividual>
    


    <!-- http://w3id.org/meta-share/meta-share/pearStory -->

    <owl:NamedIndividual rdf:about="http://w3id.org/meta-share/meta-share/pearStory">
        <rdf:type rdf:resource="http://w3id.org/meta-share/meta-share/ScenarioType"/>
        <rdfs:label xml:lang="en">pear story</rdfs:label>
    </owl:NamedIndividual>
    


    <!-- http://w3id.org/meta-share/meta-share/pennTreeBank -->

    <owl:NamedIndividual rdf:about="http://w3id.org/meta-share/meta-share/pennTreeBank">
        <rdf:type rdf:resource="http://w3id.org/meta-share/meta-share/StandardBestPractice"/>
        <ms:url>https://link.springer.com/chapter/10.1007/978-94-010-0201-1_1</ms:url>
        <rdfs:label xml:lang="en">Penn treebank</rdfs:label>
    </owl:NamedIndividual>
    


    <!-- http://w3id.org/meta-share/meta-share/person1 -->

    <owl:NamedIndividual rdf:about="http://w3id.org/meta-share/meta-share/person1">
        <rdf:type rdf:resource="http://w3id.org/meta-share/meta-share/MorphologicalType"/>
        <rdfs:label xml:lang="en">person</rdfs:label>
    </owl:NamedIndividual>
    


    <!-- http://w3id.org/meta-share/meta-share/pharmaceutics -->

    <owl:NamedIndividual rdf:about="http://w3id.org/meta-share/meta-share/pharmaceutics">
        <rdf:type rdf:resource="http://w3id.org/meta-share/meta-share/Domain"/>
        <datacite:hasIdentifier rdf:resource="http://w3id.org/meta-share/meta-share/ELG_Domain003"/>
        <rdfs:label xml:lang="en">pharmaceutics</rdfs:label>
    </owl:NamedIndividual>
    


    <!-- http://w3id.org/meta-share/meta-share/phdThesis -->

    <owl:NamedIndividual rdf:about="http://w3id.org/meta-share/meta-share/phdThesis">
        <rdf:type rdf:resource="http://w3id.org/meta-share/meta-share/DocumentType"/>
        <rdfs:label xml:lang="en">PhD thesis</rdfs:label>
    </owl:NamedIndividual>
    


    <!-- http://w3id.org/meta-share/meta-share/philosophy -->

    <owl:NamedIndividual rdf:about="http://w3id.org/meta-share/meta-share/philosophy">
        <rdf:type rdf:resource="http://w3id.org/meta-share/meta-share/Domain"/>
        <datacite:hasIdentifier rdf:resource="http://w3id.org/meta-share/meta-share/DDC100"/>
        <rdfs:label xml:lang="en">Philosophy</rdfs:label>
    </owl:NamedIndividual>
    


    <!-- http://w3id.org/meta-share/meta-share/phoneme -->

    <owl:NamedIndividual rdf:about="http://w3id.org/meta-share/meta-share/phoneme">
        <rdf:type rdf:resource="http://w3id.org/meta-share/meta-share/BaseItem"/>
        <rdfs:label xml:lang="en">phoneme</rdfs:label>
    </owl:NamedIndividual>
    


    <!-- http://w3id.org/meta-share/meta-share/phoneme1 -->

    <owl:NamedIndividual rdf:about="http://w3id.org/meta-share/meta-share/phoneme1">
        <rdf:type rdf:resource="http://w3id.org/meta-share/meta-share/SegmentationLevel"/>
        <rdfs:label xml:lang="en">phoneme</rdfs:label>
    </owl:NamedIndividual>
    


    <!-- http://w3id.org/meta-share/meta-share/phoneme2 -->

    <owl:NamedIndividual rdf:about="http://w3id.org/meta-share/meta-share/phoneme2">
        <rdf:type rdf:resource="http://w3id.org/meta-share/meta-share/SizeUnit"/>
        <rdfs:label xml:lang="en">phoneme</rdfs:label>
    </owl:NamedIndividual>
    


    <!-- http://w3id.org/meta-share/meta-share/phoneticUnit -->

    <owl:NamedIndividual rdf:about="http://w3id.org/meta-share/meta-share/phoneticUnit">
        <rdf:type rdf:resource="http://w3id.org/meta-share/meta-share/SizeUnit"/>
        <rdfs:label xml:lang="en">phonetic unit</rdfs:label>
    </owl:NamedIndividual>
    


    <!-- http://w3id.org/meta-share/meta-share/phoneticallyBalancedSentence -->

    <owl:NamedIndividual rdf:about="http://w3id.org/meta-share/meta-share/phoneticallyBalancedSentence">
        <rdf:type rdf:resource="http://w3id.org/meta-share/meta-share/SpeechItem"/>
        <rdfs:label xml:lang="en">phonetically balanced sentence</rdfs:label>
    </owl:NamedIndividual>
    


    <!-- http://w3id.org/meta-share/meta-share/phoneticallyRichSentence -->

    <owl:NamedIndividual rdf:about="http://w3id.org/meta-share/meta-share/phoneticallyRichSentence">
        <rdf:type rdf:resource="http://w3id.org/meta-share/meta-share/SpeechItem"/>
        <rdfs:label xml:lang="en">phonetically rich sentence</rdfs:label>
    </owl:NamedIndividual>
    


    <!-- http://w3id.org/meta-share/meta-share/phoneticallyRichWord -->

    <owl:NamedIndividual rdf:about="http://w3id.org/meta-share/meta-share/phoneticallyRichWord">
        <rdf:type rdf:resource="http://w3id.org/meta-share/meta-share/SpeechItem"/>
        <rdfs:label xml:lang="en">phonetically rich word</rdfs:label>
    </owl:NamedIndividual>
    


    <!-- http://w3id.org/meta-share/meta-share/phonetics -->

    <owl:NamedIndividual rdf:about="http://w3id.org/meta-share/meta-share/phonetics">
        <rdf:type rdf:resource="http://w3id.org/meta-share/meta-share/EncodingLevel"/>
        <rdfs:comment xml:lang="en">Value for &apos;EncodingLevel&apos; for the particular linguistic level that relates to the study of speech sounds</rdfs:comment>
        <rdfs:label xml:lang="en">phonetics</rdfs:label>
    </owl:NamedIndividual>
    


    <!-- http://w3id.org/meta-share/meta-share/phonology -->

    <owl:NamedIndividual rdf:about="http://w3id.org/meta-share/meta-share/phonology">
        <rdf:type rdf:resource="http://w3id.org/meta-share/meta-share/EncodingLevel"/>
        <rdfs:comment xml:lang="en">Value for &apos;EncodingLevel&apos; for the particular linguistic level that relates to the study of speech sounds that constitute the fundamental components of a language</rdfs:comment>
        <rdfs:label xml:lang="en">phonology</rdfs:label>
    </owl:NamedIndividual>
    


    <!-- http://w3id.org/meta-share/meta-share/photographyComputerArtFilmVideo -->

    <owl:NamedIndividual rdf:about="http://w3id.org/meta-share/meta-share/photographyComputerArtFilmVideo">
        <rdf:type rdf:resource="http://w3id.org/meta-share/meta-share/Domain"/>
        <datacite:hasIdentifier rdf:resource="http://w3id.org/meta-share/meta-share/DDC770"/>
        <rdfs:label xml:lang="en">Photography, Computer Art, Film, Video</rdfs:label>
    </owl:NamedIndividual>
    


    <!-- http://w3id.org/meta-share/meta-share/phrase -->

    <owl:NamedIndividual rdf:about="http://w3id.org/meta-share/meta-share/phrase">
        <rdf:type rdf:resource="http://w3id.org/meta-share/meta-share/SegmentationLevel"/>
        <rdfs:label xml:lang="en">phrase</rdfs:label>
    </owl:NamedIndividual>
    


    <!-- http://w3id.org/meta-share/meta-share/physics -->

    <owl:NamedIndividual rdf:about="http://w3id.org/meta-share/meta-share/physics">
        <rdf:type rdf:resource="http://w3id.org/meta-share/meta-share/Domain"/>
        <datacite:hasIdentifier rdf:resource="http://w3id.org/meta-share/meta-share/DDC530"/>
        <rdfs:label xml:lang="en">Physics</rdfs:label>
    </owl:NamedIndividual>
    


    <!-- http://w3id.org/meta-share/meta-share/plain -->

    <owl:NamedIndividual rdf:about="http://w3id.org/meta-share/meta-share/plain">
        <rdf:type rdf:resource="http://w3id.org/meta-share/meta-share/CapturingEnvironment"/>
        <rdfs:label xml:lang="en">plain</rdfs:label>
    </owl:NamedIndividual>
    


    <!-- http://w3id.org/meta-share/meta-share/planned -->

    <owl:NamedIndividual rdf:about="http://w3id.org/meta-share/meta-share/planned">
        <rdf:type rdf:resource="http://w3id.org/meta-share/meta-share/Naturality"/>
        <rdfs:label xml:lang="en">planned</rdfs:label>
    </owl:NamedIndividual>
    


    <!-- http://w3id.org/meta-share/meta-share/plants -->

    <owl:NamedIndividual rdf:about="http://w3id.org/meta-share/meta-share/plants">
        <rdf:type rdf:resource="http://w3id.org/meta-share/meta-share/Domain"/>
        <datacite:hasIdentifier rdf:resource="http://w3id.org/meta-share/meta-share/DDC580"/>
        <rdfs:label xml:lang="en">Plants</rdfs:label>
    </owl:NamedIndividual>
    


    <!-- http://w3id.org/meta-share/meta-share/pmcid -->

    <owl:NamedIndividual rdf:about="http://w3id.org/meta-share/meta-share/pmcid">
        <rdf:type rdf:resource="http://w3id.org/meta-share/meta-share/DocumentIdentifierScheme"/>
        <ms:url>https://www.ncbi.nlm.nih.gov/pmc/pmctopmid/</ms:url>
        <rdfs:altLabel xml:lang="en">PubMed Central Identifier</rdfs:altLabel>
        <rdfs:comment xml:lang="en">Value for resourceIdentifierSchemeName, referring to the PMCID (PubMed Central Identifier, https://www.ncbi.nlm.nih.gov/pmc/pmctopmid/)</rdfs:comment>
        <rdfs:label xml:lang="en">PMCID</rdfs:label>
    </owl:NamedIndividual>
    


    <!-- http://w3id.org/meta-share/meta-share/pmid -->

    <owl:NamedIndividual rdf:about="http://w3id.org/meta-share/meta-share/pmid">
        <rdf:type rdf:resource="http://w3id.org/meta-share/meta-share/DocumentIdentifierScheme"/>
        <ms:url>https://www.ncbi.nlm.nih.gov/pmc/pmctopmid/</ms:url>
        <rdfs:altLabel xml:lang="en">PubMed Identifier</rdfs:altLabel>
        <rdfs:comment xml:lang="en">Value for resourceIdentifierSchemeName, referring to the PMID (PubMed Identifier, https://www.ncbi.nlm.nih.gov/pmc/pmctopmid/)</rdfs:comment>
        <rdfs:label xml:lang="en">PMID</rdfs:label>
    </owl:NamedIndividual>
    


    <!-- http://w3id.org/meta-share/meta-share/politicalScience -->

    <owl:NamedIndividual rdf:about="http://w3id.org/meta-share/meta-share/politicalScience">
        <rdf:type rdf:resource="http://w3id.org/meta-share/meta-share/Domain"/>
        <datacite:hasIdentifier rdf:resource="http://w3id.org/meta-share/meta-share/DDC320"/>
        <rdfs:label xml:lang="en">Political Science</rdfs:label>
    </owl:NamedIndividual>
    


    <!-- http://w3id.org/meta-share/meta-share/politics -->

    <owl:NamedIndividual rdf:about="http://w3id.org/meta-share/meta-share/politics">
        <rdf:type rdf:resource="http://w3id.org/meta-share/meta-share/Domain"/>
        <datacite:hasIdentifier rdf:resource="http://w3id.org/meta-share/meta-share/ELG_Domain017"/>
        <rdfs:label xml:lang="en">politics</rdfs:label>
    </owl:NamedIndividual>
    


    <!-- http://w3id.org/meta-share/meta-share/ppAttachment -->

    <owl:NamedIndividual rdf:about="http://w3id.org/meta-share/meta-share/ppAttachment">
        <rdf:type rdf:resource="http://w3id.org/meta-share/meta-share/GrammaticalPhenomenaCoverage"/>
        <rdfs:altLabel xml:lang="en">Attachment of Prepositional phrases</rdfs:altLabel>
        <rdfs:label xml:lang="en">PP attachment</rdfs:label>
    </owl:NamedIndividual>
    


    <!-- http://w3id.org/meta-share/meta-share/pragmatics -->

    <owl:NamedIndividual rdf:about="http://w3id.org/meta-share/meta-share/pragmatics">
        <rdf:type rdf:resource="http://w3id.org/meta-share/meta-share/EncodingLevel"/>
        <rdfs:comment xml:lang="en">Value for &apos;EncodingLevel&apos; for the particular linguistic level of analysis that studies the relationship of sentences to the environment in which they occur</rdfs:comment>
        <rdfs:label xml:lang="en">pragmatics</rdfs:label>
    </owl:NamedIndividual>
    


    <!-- http://w3id.org/meta-share/meta-share/pragueTreebank -->

    <owl:NamedIndividual rdf:about="http://w3id.org/meta-share/meta-share/pragueTreebank">
        <rdf:type rdf:resource="http://w3id.org/meta-share/meta-share/StandardBestPractice"/>
        <ms:url>http://ufal.mff.cuni.cz/pdt2.0/</ms:url>
        <rdfs:altLabel xml:lang="en">PDT</rdfs:altLabel>
        <rdfs:altLabel xml:lang="en">Prague Dependency Treebank</rdfs:altLabel>
        <rdfs:label xml:lang="en">Prague treebank</rdfs:label>
    </owl:NamedIndividual>
    


    <!-- http://w3id.org/meta-share/meta-share/predicate -->

    <owl:NamedIndividual rdf:about="http://w3id.org/meta-share/meta-share/predicate">
        <rdf:type rdf:resource="http://w3id.org/meta-share/meta-share/SizeUnit"/>
        <rdfs:label xml:lang="en">predicate</rdfs:label>
    </owl:NamedIndividual>
    


    <!-- http://w3id.org/meta-share/meta-share/presentation -->

    <owl:NamedIndividual rdf:about="http://w3id.org/meta-share/meta-share/presentation">
        <rdf:type rdf:resource="http://w3id.org/meta-share/meta-share/SpeechGenre"/>
        <datacite:hasIdentifier rdf:resource="http://w3id.org/meta-share/meta-share/MS_SG003"/>
        <rdfs:label xml:lang="en">presentation</rdfs:label>
    </owl:NamedIndividual>
    


    <!-- http://w3id.org/meta-share/meta-share/private -->

    <owl:NamedIndividual rdf:about="http://w3id.org/meta-share/meta-share/private">
        <rdf:type rdf:resource="http://w3id.org/meta-share/meta-share/TextGenre"/>
        <datacite:hasIdentifier rdf:resource="http://w3id.org/meta-share/meta-share/PAROLE_G007"/>
        <rdfs:label xml:lang="en">private</rdfs:label>
    </owl:NamedIndividual>
    


    <!-- http://w3id.org/meta-share/meta-share/proceedings -->

    <owl:NamedIndividual rdf:about="http://w3id.org/meta-share/meta-share/proceedings">
        <rdf:type rdf:resource="http://w3id.org/meta-share/meta-share/DocumentType"/>
        <rdfs:label xml:lang="en">proceedings</rdfs:label>
    </owl:NamedIndividual>
    


    <!-- http://w3id.org/meta-share/meta-share/prompted -->

    <owl:NamedIndividual rdf:about="http://w3id.org/meta-share/meta-share/prompted">
        <rdf:type rdf:resource="http://w3id.org/meta-share/meta-share/Naturality"/>
        <rdfs:label xml:lang="en">prompted</rdfs:label>
    </owl:NamedIndividual>
    


    <!-- http://w3id.org/meta-share/meta-share/properNoun -->

    <owl:NamedIndividual rdf:about="http://w3id.org/meta-share/meta-share/properNoun">
        <rdf:type rdf:resource="http://w3id.org/meta-share/meta-share/SpeechItem"/>
        <rdfs:label xml:lang="en">proper noun</rdfs:label>
    </owl:NamedIndividual>
    


    <!-- http://w3id.org/meta-share/meta-share/prosodicBoundary -->

    <owl:NamedIndividual rdf:about="http://w3id.org/meta-share/meta-share/prosodicBoundary">
        <rdf:type rdf:resource="http://w3id.org/meta-share/meta-share/SegmentationLevel"/>
        <rdfs:label xml:lang="en">prosodic boundary</rdfs:label>
    </owl:NamedIndividual>
    


    <!-- http://w3id.org/meta-share/meta-share/psychology -->

    <owl:NamedIndividual rdf:about="http://w3id.org/meta-share/meta-share/psychology">
        <rdf:type rdf:resource="http://w3id.org/meta-share/meta-share/Domain"/>
        <datacite:hasIdentifier rdf:resource="http://w3id.org/meta-share/meta-share/DDC150"/>
        <rdfs:label xml:lang="en">Psychology</rdfs:label>
    </owl:NamedIndividual>
    


    <!-- http://w3id.org/meta-share/meta-share/public -->

    <owl:NamedIndividual rdf:about="http://w3id.org/meta-share/meta-share/public">
        <rdf:type rdf:resource="http://w3id.org/meta-share/meta-share/LicenceCategory"/>
        <ms:conformsTo rdf:resource="http://w3id.org/meta-share/meta-share/ClarinLicenceCategoryScheme"/>
        <rdfs:altLabel xml:lang="en">PUB</rdfs:altLabel>
        <rdfs:label xml:lang="en">public</rdfs:label>
    </owl:NamedIndividual>
    


    <!-- http://w3id.org/meta-share/meta-share/publicAdministration -->

    <owl:NamedIndividual rdf:about="http://w3id.org/meta-share/meta-share/publicAdministration">
        <rdf:type rdf:resource="http://w3id.org/meta-share/meta-share/Domain"/>
        <datacite:hasIdentifier rdf:resource="http://w3id.org/meta-share/meta-share/ELG_Domain007"/>
        <rdfs:label xml:lang="en">public administration</rdfs:label>
    </owl:NamedIndividual>
    


    <!-- http://w3id.org/meta-share/meta-share/publicAdministration1 -->

    <owl:NamedIndividual rdf:about="http://w3id.org/meta-share/meta-share/publicAdministration1">
        <rdf:type rdf:resource="http://w3id.org/meta-share/meta-share/Domain"/>
        <datacite:hasIdentifier rdf:resource="http://w3id.org/meta-share/meta-share/DDC351"/>
        <rdfs:label xml:lang="en">Public Administration</rdfs:label>
    </owl:NamedIndividual>
    


    <!-- http://w3id.org/meta-share/meta-share/publicOrganization -->

    <owl:NamedIndividual rdf:about="http://w3id.org/meta-share/meta-share/publicOrganization">
        <rdf:type rdf:resource="http://w3id.org/meta-share/meta-share/OrganizationLegalStatus"/>
        <rdfs:label xml:lang="en">public organization</rdfs:label>
    </owl:NamedIndividual>
    


    <!-- http://w3id.org/meta-share/meta-share/publication -->

    <owl:NamedIndividual rdf:about="http://w3id.org/meta-share/meta-share/publication">
        <rdf:type rdf:resource="http://w3id.org/meta-share/meta-share/DocumentationType"/>
        <rdfs:comment xml:lang="en">Value for &apos;Documentation type&apos; used for published documents about a language resource (mainly meant for documents that describe the resource itself rather than its deployment)</rdfs:comment>
        <rdfs:label xml:lang="en">publication</rdfs:label>
    </owl:NamedIndividual>
    


    <!-- http://w3id.org/meta-share/meta-share/publicationForCitation -->

    <owl:NamedIndividual rdf:about="http://w3id.org/meta-share/meta-share/publicationForCitation">
        <rdf:type rdf:resource="http://w3id.org/meta-share/meta-share/DocumentationType"/>
        <rdfs:comment xml:lang="en">Value for &apos;Documentation type&apos; for a published document describing the language resource and which is recommended by the resource creator(s) to be used for citation purposes when the resource is mentioned in another publication</rdfs:comment>
        <rdfs:label xml:lang="en">publication for citation</rdfs:label>
    </owl:NamedIndividual>
    


    <!-- http://w3id.org/meta-share/meta-share/published -->

    <owl:NamedIndividual rdf:about="http://w3id.org/meta-share/meta-share/published">
        <rdf:type rdf:resource="http://w3id.org/meta-share/meta-share/VersionType"/>
        <rdfs:comment xml:lang="en">Value for &apos;Version type&apos; used for versions as published in digital or print form</rdfs:comment>
        <rdfs:label xml:lang="en">published</rdfs:label>
    </owl:NamedIndividual>
    


    <!-- http://w3id.org/meta-share/meta-share/publishing -->

    <owl:NamedIndividual rdf:about="http://w3id.org/meta-share/meta-share/publishing">
        <rdf:type rdf:resource="http://w3id.org/meta-share/meta-share/Domain"/>
        <datacite:hasIdentifier rdf:resource="http://w3id.org/meta-share/meta-share/ELG_Domain001"/>
        <rdfs:label xml:lang="en">publishing</rdfs:label>
    </owl:NamedIndividual>
    


    <!-- http://w3id.org/meta-share/meta-share/qualiaStructure -->

    <owl:NamedIndividual rdf:about="http://w3id.org/meta-share/meta-share/qualiaStructure">
        <rdf:type rdf:resource="http://w3id.org/meta-share/meta-share/SemanticType"/>
        <rdfs:label xml:lang="en">qualia structure</rdfs:label>
    </owl:NamedIndividual>
    


    <!-- http://w3id.org/meta-share/meta-share/question -->

    <owl:NamedIndividual rdf:about="http://w3id.org/meta-share/meta-share/question">
        <rdf:type rdf:resource="http://w3id.org/meta-share/meta-share/SizeUnit"/>
        <rdfs:label xml:lang="en">question</rdfs:label>
    </owl:NamedIndividual>
    


    <!-- http://w3id.org/meta-share/meta-share/questionAnswer -->

    <owl:NamedIndividual rdf:about="http://w3id.org/meta-share/meta-share/questionAnswer">
        <rdf:type rdf:resource="http://w3id.org/meta-share/meta-share/SpeechGenre"/>
        <datacite:hasIdentifier rdf:resource="http://w3id.org/meta-share/meta-share/MS_SG004"/>
        <rdfs:label xml:lang="en">question answer</rdfs:label>
    </owl:NamedIndividual>
    


    <!-- http://w3id.org/meta-share/meta-share/radio -->

    <owl:NamedIndividual rdf:about="http://w3id.org/meta-share/meta-share/radio">
        <rdf:type rdf:resource="http://w3id.org/meta-share/meta-share/SourceChannel"/>
        <rdfs:label xml:lang="en">radio</rdfs:label>
    </owl:NamedIndividual>
    


    <!-- http://w3id.org/meta-share/meta-share/raster -->

    <owl:NamedIndividual rdf:about="http://w3id.org/meta-share/meta-share/raster">
        <rdf:type rdf:resource="http://w3id.org/meta-share/meta-share/RasterOrVectorGraphics"/>
        <rdfs:label xml:lang="en">raster</rdfs:label>
    </owl:NamedIndividual>
    


    <!-- http://w3id.org/meta-share/meta-share/rawCorpus -->

    <owl:NamedIndividual rdf:about="http://w3id.org/meta-share/meta-share/rawCorpus">
        <rdf:type rdf:resource="http://w3id.org/meta-share/meta-share/CorpusSubclass"/>
        <rdfs:comment xml:lang="en">The form of the corpus that has not been enriched with annotations</rdfs:comment>
        <rdfs:label xml:lang="en">raw corpus</rdfs:label>
    </owl:NamedIndividual>
    


    <!-- http://w3id.org/meta-share/meta-share/readSpeech -->

    <owl:NamedIndividual rdf:about="http://w3id.org/meta-share/meta-share/readSpeech">
        <rdf:type rdf:resource="http://w3id.org/meta-share/meta-share/Naturality"/>
        <rdfs:label xml:lang="en">read speech</rdfs:label>
    </owl:NamedIndividual>
    


    <!-- http://w3id.org/meta-share/meta-share/realAudio -->

    <owl:NamedIndividual rdf:about="http://w3id.org/meta-share/meta-share/realAudio">
        <rdf:type rdf:resource="http://w3id.org/meta-share/meta-share/CompressionName"/>
        <rdfs:label xml:lang="en">real audio</rdfs:label>
    </owl:NamedIndividual>
    


    <!-- http://w3id.org/meta-share/meta-share/redeposit -->

    <owl:NamedIndividual rdf:about="http://w3id.org/meta-share/meta-share/redeposit">
        <rdf:type rdf:resource="http://w3id.org/meta-share/meta-share/ConditionOfUse"/>
        <rdf:type rdf:resource="http://www.w3.org/ns/odrl/2/Set"/>
        <rdfs:comment xml:lang="en">Value for &apos;ConditionsOfUse&apos; which states that users are encouraged to deposit any modified versions of the resource they make to the distribution channel through which they have acquired the resource</rdfs:comment>
        <rdfs:label xml:lang="en">redeposit</rdfs:label>
        <odrl:permission>
            <rdf:Description>
                <odrl:duty>
                    <rdf:Description>
                        <odrl:action rdf:resource="http://w3id.org/meta-share/meta-share/redeposit"/>
                    </rdf:Description>
                </odrl:duty>
            </rdf:Description>
        </odrl:permission>
    </owl:NamedIndividual>
    


    <!-- http://w3id.org/meta-share/meta-share/reflexivity -->

    <owl:NamedIndividual rdf:about="http://w3id.org/meta-share/meta-share/reflexivity">
        <rdf:type rdf:resource="http://w3id.org/meta-share/meta-share/MorphologicalType"/>
        <rdfs:label xml:lang="en">reflexivity</rdfs:label>
    </owl:NamedIndividual>
    


    <!-- http://w3id.org/meta-share/meta-share/register1 -->

    <owl:NamedIndividual rdf:about="http://w3id.org/meta-share/meta-share/register1">
        <rdf:type rdf:resource="http://w3id.org/meta-share/meta-share/UsageType"/>
        <rdfs:label xml:lang="en">register</rdfs:label>
    </owl:NamedIndividual>
    


    <!-- http://w3id.org/meta-share/meta-share/religion -->

    <owl:NamedIndividual rdf:about="http://w3id.org/meta-share/meta-share/religion">
        <rdf:type rdf:resource="http://w3id.org/meta-share/meta-share/Domain"/>
        <datacite:hasIdentifier rdf:resource="http://w3id.org/meta-share/meta-share/DDC200"/>
        <rdfs:label xml:lang="en">Religion</rdfs:label>
    </owl:NamedIndividual>
    


    <!-- http://w3id.org/meta-share/meta-share/requestPlan -->

    <owl:NamedIndividual rdf:about="http://w3id.org/meta-share/meta-share/requestPlan">
        <rdf:type rdf:resource="http://w3id.org/meta-share/meta-share/ConditionOfUse"/>
        <rdfs:comment xml:lang="en">Value for &apos;ConditionOfUse&apos; that states that the licensor requires the submission of a research plan in order to grant access to the language resource</rdfs:comment>
        <rdfs:label xml:lang="en">request plan</rdfs:label>
    </owl:NamedIndividual>
    


    <!-- http://w3id.org/meta-share/meta-share/researchOrganization -->

    <owl:NamedIndividual rdf:about="http://w3id.org/meta-share/meta-share/researchOrganization">
        <rdf:type rdf:resource="http://w3id.org/meta-share/meta-share/OrganizationRole"/>
        <rdfs:label xml:lang="en">research organization</rdfs:label>
    </owl:NamedIndividual>
    


    <!-- http://w3id.org/meta-share/meta-share/researchUse -->

    <owl:NamedIndividual rdf:about="http://w3id.org/meta-share/meta-share/researchUse">
        <rdf:type rdf:resource="http://w3id.org/meta-share/meta-share/ConditionOfUse"/>
        <rdfs:comment xml:lang="en">Value for &apos;ConditionOfUse&apos; stating that the resource can be used only for research purposes</rdfs:comment>
        <rdfs:label xml:lang="en">research use</rdfs:label>
        <skos:note xml:lang="en">add ODRL</skos:note>
    </owl:NamedIndividual>
    


    <!-- http://w3id.org/meta-share/meta-share/restricted -->

    <owl:NamedIndividual rdf:about="http://w3id.org/meta-share/meta-share/restricted">
        <rdf:type rdf:resource="http://w3id.org/meta-share/meta-share/LicenceCategory"/>
        <ms:conformsTo rdf:resource="http://w3id.org/meta-share/meta-share/ClarinLicenceCategoryScheme"/>
        <rdfs:altLabel xml:lang="en">RES</rdfs:altLabel>
        <rdfs:label xml:lang="en">restricted</rdfs:label>
    </owl:NamedIndividual>
    


    <!-- http://w3id.org/meta-share/meta-share/restrictedAccess -->

    <owl:NamedIndividual rdf:about="http://w3id.org/meta-share/meta-share/restrictedAccess">
        <rdf:type rdf:resource="http://w3id.org/meta-share/meta-share/AccessRightsStatement"/>
        <datacite:hasIdentifier rdf:resource="http://w3id.org/meta-share/meta-share/omtdAccess1"/>
        <rdfs:comment xml:lang="en">Access is subject to restrictions or controls regarding users (e.g.,  limited to researchers or members of a specific group) or use (e.g.,  for research only, noncommercial use , etc.); subscription or registration may also be required and access may incur financial costs</rdfs:comment>
        <rdfs:label xml:lang="en">restricted access</rdfs:label>
        <skos:closeMatch rdf:resource="http://purl.org/coar/access_right/c_16ec"/>
        <skos:closeMatch rdf:resource="http://purl.org/eprint/accessRights/RestrictedAccess"/>
    </owl:NamedIndividual>
    


    <!-- http://w3id.org/meta-share/meta-share/restrictedAccess1 -->

    <owl:NamedIndividual rdf:about="http://w3id.org/meta-share/meta-share/restrictedAccess1">
        <rdf:type rdf:resource="http://w3id.org/meta-share/meta-share/AccessRightsStatement"/>
        <datacite:hasIdentifier rdf:resource="http://purl.org/coar/access_right/c_16ec"/>
    </owl:NamedIndividual>
    


    <!-- http://w3id.org/meta-share/meta-share/review -->

    <owl:NamedIndividual rdf:about="http://w3id.org/meta-share/meta-share/review">
        <rdf:type rdf:resource="http://w3id.org/meta-share/meta-share/TextType"/>
        <datacite:hasIdentifier rdf:resource="http://w3id.org/meta-share/meta-share/ClarinEl_TT017"/>
        <rdfs:label xml:lang="en">review</rdfs:label>
    </owl:NamedIndividual>
    


    <!-- http://w3id.org/meta-share/meta-share/rolePlay -->

    <owl:NamedIndividual rdf:about="http://w3id.org/meta-share/meta-share/rolePlay">
        <rdf:type rdf:resource="http://w3id.org/meta-share/meta-share/ScenarioType"/>
        <rdfs:label xml:lang="en">role play</rdfs:label>
    </owl:NamedIndividual>
    


    <!-- http://w3id.org/meta-share/meta-share/roundtable -->

    <owl:NamedIndividual rdf:about="http://w3id.org/meta-share/meta-share/roundtable">
        <rdf:type rdf:resource="http://w3id.org/meta-share/meta-share/SpeechGenre"/>
        <datacite:hasIdentifier rdf:resource="http://w3id.org/meta-share/meta-share/MS_SG005"/>
        <rdfs:label xml:lang="en">roundtable</rdfs:label>
    </owl:NamedIndividual>
    


    <!-- http://w3id.org/meta-share/meta-share/rule -->

    <owl:NamedIndividual rdf:about="http://w3id.org/meta-share/meta-share/rule">
        <rdf:type rdf:resource="http://w3id.org/meta-share/meta-share/SizeUnit"/>
        <rdfs:label xml:lang="en">rule</rdfs:label>
    </owl:NamedIndividual>
    


    <!-- http://w3id.org/meta-share/meta-share/samples -->

    <owl:NamedIndividual rdf:about="http://w3id.org/meta-share/meta-share/samples">
        <rdf:type rdf:resource="http://w3id.org/meta-share/meta-share/DocumentationType"/>
        <rdfs:comment xml:lang="en">Value for &apos;DocumentationType&apos; used for samples of a language resource</rdfs:comment>
        <rdfs:label xml:lang="en">samples</rdfs:label>
    </owl:NamedIndividual>
    


    <!-- http://w3id.org/meta-share/meta-share/scene -->

    <owl:NamedIndividual rdf:about="http://w3id.org/meta-share/meta-share/scene">
        <rdf:type rdf:resource="http://w3id.org/meta-share/meta-share/SegmentationLevel"/>
        <rdfs:label xml:lang="en">scene</rdfs:label>
    </owl:NamedIndividual>
    


    <!-- http://w3id.org/meta-share/meta-share/scholarlyCommunication -->

    <owl:NamedIndividual rdf:about="http://w3id.org/meta-share/meta-share/scholarlyCommunication">
        <rdf:type rdf:resource="http://w3id.org/meta-share/meta-share/Domain"/>
        <rdfs:comment xml:lang="en">Scholarly communication can be defined as “the system through which research and other scholarly writings are created, evaluated for quality, disseminated to the scholarly community, and preserved for future use. The system includes both formal means of communication, such as publication in peer-reviewed journals, and informal channels, such as electronic listservs.” (Association of College &amp; Research Libraries, “Principles and Strategies for the Reform of Scholarly Communication 1,” 2003)</rdfs:comment>
        <rdfs:label xml:lang="en">scholarly communication</rdfs:label>
    </owl:NamedIndividual>
    


    <!-- http://w3id.org/meta-share/meta-share/school -->

    <owl:NamedIndividual rdf:about="http://w3id.org/meta-share/meta-share/school">
        <rdf:type rdf:resource="http://w3id.org/meta-share/meta-share/DivisionCategory"/>
        <rdfs:label xml:lang="en">school</rdfs:label>
    </owl:NamedIndividual>
    


    <!-- http://w3id.org/meta-share/meta-share/science -->

    <owl:NamedIndividual rdf:about="http://w3id.org/meta-share/meta-share/science">
        <rdf:type rdf:resource="http://w3id.org/meta-share/meta-share/Domain"/>
        <datacite:hasIdentifier rdf:resource="http://w3id.org/meta-share/meta-share/DDC500"/>
        <rdfs:label xml:lang="en">Science</rdfs:label>
    </owl:NamedIndividual>
    


    <!-- http://w3id.org/meta-share/meta-share/scopusId -->

    <owl:NamedIndividual rdf:about="http://w3id.org/meta-share/meta-share/scopusId">
        <rdf:type rdf:resource="http://purl.org/spar/datacite/PersonalIdentifierScheme"/>
        <rdfs:comment xml:lang="en">Value for personIdentifierSchemeName, referring to the Scopus identifier for authors (https://www.scopus.com)</rdfs:comment>
        <rdfs:label xml:lang="en">Scopus ID</rdfs:label>
    </owl:NamedIndividual>
    


    <!-- http://w3id.org/meta-share/meta-share/script -->

    <owl:NamedIndividual rdf:about="http://w3id.org/meta-share/meta-share/script">
        <rdf:type rdf:resource="http://w3id.org/meta-share/meta-share/TextType"/>
        <datacite:hasIdentifier rdf:resource="http://w3id.org/meta-share/meta-share/ClarinEl_TT010"/>
        <rdfs:label xml:lang="en">script</rdfs:label>
    </owl:NamedIndividual>
    


    <!-- http://w3id.org/meta-share/meta-share/sculptureCeramicsAndMetalwork -->

    <owl:NamedIndividual rdf:about="http://w3id.org/meta-share/meta-share/sculptureCeramicsAndMetalwork">
        <rdf:type rdf:resource="http://w3id.org/meta-share/meta-share/Domain"/>
        <datacite:hasIdentifier rdf:resource="http://w3id.org/meta-share/meta-share/DDC730"/>
        <rdfs:label xml:lang="en">Sculpture, Ceramics and Metalwork</rdfs:label>
    </owl:NamedIndividual>
    


    <!-- http://w3id.org/meta-share/meta-share/second -->

    <owl:NamedIndividual rdf:about="http://w3id.org/meta-share/meta-share/second">
        <rdf:type rdf:resource="http://w3id.org/meta-share/meta-share/SizeUnit"/>
        <rdfs:label xml:lang="en">second</rdfs:label>
    </owl:NamedIndividual>
    


    <!-- http://w3id.org/meta-share/meta-share/second1 -->

    <owl:NamedIndividual rdf:about="http://w3id.org/meta-share/meta-share/second1">
        <rdf:type rdf:resource="http://w3id.org/meta-share/meta-share/DurationUnit"/>
        <rdfs:label xml:lang="en">second</rdfs:label>
    </owl:NamedIndividual>
    


    <!-- http://w3id.org/meta-share/meta-share/semanticClass -->

    <owl:NamedIndividual rdf:about="http://w3id.org/meta-share/meta-share/semanticClass">
        <rdf:type rdf:resource="http://w3id.org/meta-share/meta-share/SemanticType"/>
        <rdfs:label xml:lang="en">semantic class</rdfs:label>
    </owl:NamedIndividual>
    


    <!-- http://w3id.org/meta-share/meta-share/semanticFeature -->

    <owl:NamedIndividual rdf:about="http://w3id.org/meta-share/meta-share/semanticFeature">
        <rdf:type rdf:resource="http://w3id.org/meta-share/meta-share/SemanticType"/>
        <rdfs:altLabel xml:lang="en">semantic trait</rdfs:altLabel>
        <rdfs:label xml:lang="en">semantic feature</rdfs:label>
    </owl:NamedIndividual>
    


    <!-- http://w3id.org/meta-share/meta-share/semanticRelation -->

    <owl:NamedIndividual rdf:about="http://w3id.org/meta-share/meta-share/semanticRelation">
        <rdf:type rdf:resource="http://w3id.org/meta-share/meta-share/SemanticType"/>
        <rdfs:label xml:lang="en">semantic relation</rdfs:label>
    </owl:NamedIndividual>
    


    <!-- http://w3id.org/meta-share/meta-share/semanticRole -->

    <owl:NamedIndividual rdf:about="http://w3id.org/meta-share/meta-share/semanticRole">
        <rdf:type rdf:resource="http://w3id.org/meta-share/meta-share/SemanticType"/>
        <rdfs:label xml:lang="en">semantic role</rdfs:label>
    </owl:NamedIndividual>
    


    <!-- http://w3id.org/meta-share/meta-share/semanticUnit -->

    <owl:NamedIndividual rdf:about="http://w3id.org/meta-share/meta-share/semanticUnit">
        <rdf:type rdf:resource="http://w3id.org/meta-share/meta-share/ExtratextualInformationUnit"/>
        <rdfs:label xml:lang="en">semantic unit</rdfs:label>
    </owl:NamedIndividual>
    


    <!-- http://w3id.org/meta-share/meta-share/semanticUnit1 -->

    <owl:NamedIndividual rdf:about="http://w3id.org/meta-share/meta-share/semanticUnit1">
        <rdf:type rdf:resource="http://w3id.org/meta-share/meta-share/SizeUnit"/>
        <rdfs:label xml:lang="en">semantic unit</rdfs:label>
    </owl:NamedIndividual>
    


    <!-- http://w3id.org/meta-share/meta-share/semantics -->

    <owl:NamedIndividual rdf:about="http://w3id.org/meta-share/meta-share/semantics">
        <rdf:type rdf:resource="http://w3id.org/meta-share/meta-share/EncodingLevel"/>
        <rdfs:comment xml:lang="en">Value for &apos;EncodingLevel&apos; for the particular linguistic level of analysis that relates to the meaning of a word, phrase, etc.</rdfs:comment>
        <rdfs:label xml:lang="en">semantics</rdfs:label>
    </owl:NamedIndividual>
    


    <!-- http://w3id.org/meta-share/meta-share/semiInteractive -->

    <owl:NamedIndividual rdf:about="http://w3id.org/meta-share/meta-share/semiInteractive">
        <rdf:type rdf:resource="http://w3id.org/meta-share/meta-share/Interactivity"/>
        <rdfs:label xml:lang="en">semi-interactive</rdfs:label>
    </owl:NamedIndividual>
    


    <!-- http://w3id.org/meta-share/meta-share/semiPlanned -->

    <owl:NamedIndividual rdf:about="http://w3id.org/meta-share/meta-share/semiPlanned">
        <rdf:type rdf:resource="http://w3id.org/meta-share/meta-share/Naturality"/>
        <rdfs:label xml:lang="en">semi-planned</rdfs:label>
    </owl:NamedIndividual>
    


    <!-- http://w3id.org/meta-share/meta-share/sentence -->

    <owl:NamedIndividual rdf:about="http://w3id.org/meta-share/meta-share/sentence">
        <rdf:type rdf:resource="http://w3id.org/meta-share/meta-share/SegmentationLevel"/>
        <rdfs:label xml:lang="en">sentence</rdfs:label>
    </owl:NamedIndividual>
    


    <!-- http://w3id.org/meta-share/meta-share/sentence1 -->

    <owl:NamedIndividual rdf:about="http://w3id.org/meta-share/meta-share/sentence1">
        <rdf:type rdf:resource="http://w3id.org/meta-share/meta-share/SizeUnit"/>
        <rdfs:label xml:lang="en">sentence</rdfs:label>
    </owl:NamedIndividual>
    


    <!-- http://w3id.org/meta-share/meta-share/shareAlike -->

    <owl:NamedIndividual rdf:about="http://w3id.org/meta-share/meta-share/shareAlike">
        <rdf:type rdf:resource="http://w3id.org/meta-share/meta-share/ConditionOfUse"/>
        <rdf:type rdf:resource="http://www.w3.org/ns/odrl/2/Set"/>
        <rdfs:comment xml:lang="en">Value for &apos;ConditionOfUse&apos; that states that the derivatives of the language resource must be distributed with the same or a compatible licence</rdfs:comment>
        <rdfs:label xml:lang="en">share alike</rdfs:label>
        <odrl:permission>
            <rdf:Description>
                <odrl:duty>
                    <rdf:Description>
                        <odrl:action rdf:resource="http://creativecommons.org/ns#ShareALike"/>
                    </rdf:Description>
                </odrl:duty>
            </rdf:Description>
        </odrl:permission>
    </owl:NamedIndividual>
    


    <!-- http://w3id.org/meta-share/meta-share/shorten -->

    <owl:NamedIndividual rdf:about="http://w3id.org/meta-share/meta-share/shorten">
        <rdf:type rdf:resource="http://w3id.org/meta-share/meta-share/CompressionName"/>
        <rdfs:label xml:lang="en">shorten</rdfs:label>
    </owl:NamedIndividual>
    


    <!-- http://w3id.org/meta-share/meta-share/shot -->

    <owl:NamedIndividual rdf:about="http://w3id.org/meta-share/meta-share/shot">
        <rdf:type rdf:resource="http://w3id.org/meta-share/meta-share/SegmentationLevel"/>
        <rdfs:label xml:lang="en">shot</rdfs:label>
    </owl:NamedIndividual>
    


    <!-- http://w3id.org/meta-share/meta-share/shot1 -->

    <owl:NamedIndividual rdf:about="http://w3id.org/meta-share/meta-share/shot1">
        <rdf:type rdf:resource="http://w3id.org/meta-share/meta-share/SizeUnit"/>
        <rdfs:label xml:lang="en">shot</rdfs:label>
    </owl:NamedIndividual>
    


    <!-- http://w3id.org/meta-share/meta-share/signLanguage -->

    <owl:NamedIndividual rdf:about="http://w3id.org/meta-share/meta-share/signLanguage">
        <rdf:type rdf:resource="http://w3id.org/meta-share/meta-share/ModalityType"/>
        <rdfs:comment xml:lang="en">Value for &apos;ModalityType&apos; for sign languages represented in a language resource</rdfs:comment>
        <rdfs:label xml:lang="en">sign language</rdfs:label>
    </owl:NamedIndividual>
    


    <!-- http://w3id.org/meta-share/meta-share/signal -->

    <owl:NamedIndividual rdf:about="http://w3id.org/meta-share/meta-share/signal">
        <rdf:type rdf:resource="http://w3id.org/meta-share/meta-share/SegmentationLevel"/>
        <rdfs:label xml:lang="en">signal</rdfs:label>
    </owl:NamedIndividual>
    


    <!-- http://w3id.org/meta-share/meta-share/signedInteger -->

    <owl:NamedIndividual rdf:about="http://w3id.org/meta-share/meta-share/signedInteger">
        <rdf:type rdf:resource="http://w3id.org/meta-share/meta-share/SignConvention"/>
        <rdfs:label xml:lang="en">signed integer</rdfs:label>
    </owl:NamedIndividual>
    


    <!-- http://w3id.org/meta-share/meta-share/singleSource -->

    <owl:NamedIndividual rdf:about="http://w3id.org/meta-share/meta-share/singleSource">
        <rdf:type rdf:resource="http://w3id.org/meta-share/meta-share/SceneIllumination"/>
        <rdfs:label xml:lang="en">single source</rdfs:label>
    </owl:NamedIndividual>
    


    <!-- http://w3id.org/meta-share/meta-share/sleepDeprivation -->

    <owl:NamedIndividual rdf:about="http://w3id.org/meta-share/meta-share/sleepDeprivation">
        <rdf:type rdf:resource="http://w3id.org/meta-share/meta-share/SpeechInfluence"/>
        <rdfs:label xml:lang="en">sleep deprivation</rdfs:label>
    </owl:NamedIndividual>
    


    <!-- http://w3id.org/meta-share/meta-share/sme -->

    <owl:NamedIndividual rdf:about="http://w3id.org/meta-share/meta-share/sme">
        <rdf:type rdf:resource="http://w3id.org/meta-share/meta-share/OrganizationLegalStatus"/>
        <rdfs:label xml:lang="en">SME</rdfs:label>
    </owl:NamedIndividual>
    


    <!-- http://w3id.org/meta-share/meta-share/socialProblemsAndSocialServices -->

    <owl:NamedIndividual rdf:about="http://w3id.org/meta-share/meta-share/socialProblemsAndSocialServices">
        <rdf:type rdf:resource="http://w3id.org/meta-share/meta-share/Domain"/>
        <datacite:hasIdentifier rdf:resource="http://w3id.org/meta-share/meta-share/DDC360"/>
        <rdfs:label xml:lang="en">Social Problems &amp; Social Services</rdfs:label>
    </owl:NamedIndividual>
    


    <!-- http://w3id.org/meta-share/meta-share/socialSciences -->

    <owl:NamedIndividual rdf:about="http://w3id.org/meta-share/meta-share/socialSciences">
        <rdf:type rdf:resource="http://w3id.org/meta-share/meta-share/Domain"/>
        <datacite:hasIdentifier rdf:resource="http://w3id.org/meta-share/meta-share/DDC300"/>
        <rdfs:comment xml:lang="en">The social sciences are academic disciplines concerned with the study of the social life of human groups and individuals including anthropology, economics, geography, history, political science, psychology, social studies, and sociology. The social sciences consist of the scientific study of the human aspects of the world.[https://en.wikipedia.org/wiki/Category:Social_sciences</rdfs:comment>
        <rdfs:label xml:lang="en">Social Sciences</rdfs:label>
    </owl:NamedIndividual>
    


    <!-- http://w3id.org/meta-share/meta-share/society -->

    <owl:NamedIndividual rdf:about="http://w3id.org/meta-share/meta-share/society">
        <rdf:type rdf:resource="http://w3id.org/meta-share/meta-share/OrganizationLegalStatus"/>
        <rdfs:label xml:lang="en">society</rdfs:label>
    </owl:NamedIndividual>
    


    <!-- http://w3id.org/meta-share/meta-share/sociologyAndAnthropology -->

    <owl:NamedIndividual rdf:about="http://w3id.org/meta-share/meta-share/sociologyAndAnthropology">
        <rdf:type rdf:resource="http://w3id.org/meta-share/meta-share/Domain"/>
        <datacite:hasIdentifier rdf:resource="http://w3id.org/meta-share/meta-share/DDC301"/>
        <rdfs:label xml:lang="en">Sociology &amp; Anthropology</rdfs:label>
    </owl:NamedIndividual>
    


    <!-- http://w3id.org/meta-share/meta-share/some -->

    <owl:NamedIndividual rdf:about="http://w3id.org/meta-share/meta-share/some">
        <rdf:type rdf:resource="http://w3id.org/meta-share/meta-share/Audience"/>
        <rdfs:label xml:lang="en">some</rdfs:label>
    </owl:NamedIndividual>
    


    <!-- http://w3id.org/meta-share/meta-share/song -->

    <owl:NamedIndividual rdf:about="http://w3id.org/meta-share/meta-share/song">
        <rdf:type rdf:resource="http://w3id.org/meta-share/meta-share/AudioGenre"/>
        <datacite:hasIdentifier rdf:resource="http://w3id.org/meta-share/meta-share/MS_AG004"/>
        <rdfs:label xml:lang="en">song</rdfs:label>
    </owl:NamedIndividual>
    


    <!-- http://w3id.org/meta-share/meta-share/sound -->

    <owl:NamedIndividual rdf:about="http://w3id.org/meta-share/meta-share/sound">
        <rdf:type rdf:resource="http://w3id.org/meta-share/meta-share/NonSpeechItem"/>
        <rdfs:label xml:lang="en">sound</rdfs:label>
    </owl:NamedIndividual>
    


    <!-- http://w3id.org/meta-share/meta-share/soundBlasterCard -->

    <owl:NamedIndividual rdf:about="http://w3id.org/meta-share/meta-share/soundBlasterCard">
        <rdf:type rdf:resource="http://w3id.org/meta-share/meta-share/RecordingDeviceType"/>
        <rdfs:label xml:lang="en">Sound blaster card</rdfs:label>
    </owl:NamedIndividual>
    


    <!-- http://w3id.org/meta-share/meta-share/soundRecording -->

    <owl:NamedIndividual rdf:about="http://w3id.org/meta-share/meta-share/soundRecording">
        <rdf:type rdf:resource="http://w3id.org/meta-share/meta-share/ExtratextualInformation"/>
        <rdfs:label xml:lang="en">sound recording</rdfs:label>
    </owl:NamedIndividual>
    


    <!-- http://w3id.org/meta-share/meta-share/sourceAndExecutableCode -->

    <owl:NamedIndividual rdf:about="http://w3id.org/meta-share/meta-share/sourceAndExecutableCode">
        <rdf:type rdf:resource="http://w3id.org/meta-share/meta-share/SoftwareDistributionForm"/>
        <rdfs:comment xml:lang="en">Value for software distribution form, used for software that is available from the same location both as source code and executable program</rdfs:comment>
        <rdfs:label xml:lang="en">source and executable code</rdfs:label>
    </owl:NamedIndividual>
    


    <!-- http://w3id.org/meta-share/meta-share/sourceCode -->

    <owl:NamedIndividual rdf:about="http://w3id.org/meta-share/meta-share/sourceCode">
        <rdf:type rdf:resource="http://w3id.org/meta-share/meta-share/SoftwareDistributionForm"/>
        <rdfs:comment xml:lang="en">Value for software distribution form, used for software objects in the form of source code, i.e. as files with the commands ready to be compiled or assembled into an executable computer program</rdfs:comment>
        <rdfs:label xml:lang="en">source code</rdfs:label>
    </owl:NamedIndividual>
    


    <!-- http://w3id.org/meta-share/meta-share/spatialConstraint -->

    <owl:NamedIndividual rdf:about="http://w3id.org/meta-share/meta-share/spatialConstraint">
        <rdf:type rdf:resource="http://w3id.org/meta-share/meta-share/ConditionOfUse"/>
        <rdfs:comment xml:lang="en">Value for &apos;ConditionsOfUse&apos; which is used for resources with spatial restrictions, e.g.,  in cases where the content is available or can be used only at a single location, center, or site</rdfs:comment>
        <rdfs:label xml:lang="en">spatial constraint</rdfs:label>
    </owl:NamedIndividual>
    


    <!-- http://w3id.org/meta-share/meta-share/speakerNoise -->

    <owl:NamedIndividual rdf:about="http://w3id.org/meta-share/meta-share/speakerNoise">
        <rdf:type rdf:resource="http://w3id.org/meta-share/meta-share/AnnotatedElement"/>
        <rdfs:label xml:lang="en">speaker noise</rdfs:label>
    </owl:NamedIndividual>
    


    <!-- http://w3id.org/meta-share/meta-share/specialHardwareEquipment -->

    <owl:NamedIndividual rdf:about="http://w3id.org/meta-share/meta-share/specialHardwareEquipment">
        <rdf:type rdf:resource="http://w3id.org/meta-share/meta-share/RequiredHardware"/>
        <rdfs:label xml:lang="en">special hardware equipment</rdfs:label>
    </owl:NamedIndividual>
    


    <!-- http://w3id.org/meta-share/meta-share/speech -->

    <owl:NamedIndividual rdf:about="http://w3id.org/meta-share/meta-share/speech">
        <rdf:type rdf:resource="http://w3id.org/meta-share/meta-share/AudioGenre"/>
        <datacite:hasIdentifier rdf:resource="http://w3id.org/meta-share/meta-share/MS_AG003"/>
        <rdfs:label xml:lang="en">speech</rdfs:label>
    </owl:NamedIndividual>
    


    <!-- http://w3id.org/meta-share/meta-share/spokenLanguage -->

    <owl:NamedIndividual rdf:about="http://w3id.org/meta-share/meta-share/spokenLanguage">
        <rdf:type rdf:resource="http://w3id.org/meta-share/meta-share/ModalityType"/>
        <rdfs:comment xml:lang="en">Value for &apos;ModalityType&apos; for language resources including spoken language words and expressions</rdfs:comment>
        <rdfs:label xml:lang="en">spoken language</rdfs:label>
    </owl:NamedIndividual>
    


    <!-- http://w3id.org/meta-share/meta-share/spontaneous -->

    <owl:NamedIndividual rdf:about="http://w3id.org/meta-share/meta-share/spontaneous">
        <rdf:type rdf:resource="http://w3id.org/meta-share/meta-share/Naturality"/>
        <rdfs:label xml:lang="en">spontaneous</rdfs:label>
    </owl:NamedIndividual>
    


    <!-- http://w3id.org/meta-share/meta-share/sportsGamesAndEntertainment -->

    <owl:NamedIndividual rdf:about="http://w3id.org/meta-share/meta-share/sportsGamesAndEntertainment">
        <rdf:type rdf:resource="http://w3id.org/meta-share/meta-share/Domain"/>
        <datacite:hasIdentifier rdf:resource="http://w3id.org/meta-share/meta-share/DDC790"/>
        <rdfs:label xml:lang="en">Sports, Games &amp; Entertainment</rdfs:label>
    </owl:NamedIndividual>
    


    <!-- http://w3id.org/meta-share/meta-share/standardizationBody -->

    <owl:NamedIndividual rdf:about="http://w3id.org/meta-share/meta-share/standardizationBody">
        <rdf:type rdf:resource="http://w3id.org/meta-share/meta-share/OrganizationRole"/>
        <rdfs:label xml:lang="en">standardization body</rdfs:label>
    </owl:NamedIndividual>
    


    <!-- http://w3id.org/meta-share/meta-share/statisticalProperty -->

    <owl:NamedIndividual rdf:about="http://w3id.org/meta-share/meta-share/statisticalProperty">
        <rdf:type rdf:resource="http://w3id.org/meta-share/meta-share/ContentType"/>
        <rdfs:label xml:lang="en">statistical property</rdfs:label>
    </owl:NamedIndividual>
    


    <!-- http://w3id.org/meta-share/meta-share/statistics -->

    <owl:NamedIndividual rdf:about="http://w3id.org/meta-share/meta-share/statistics">
        <rdf:type rdf:resource="http://w3id.org/meta-share/meta-share/Domain"/>
        <datacite:hasIdentifier rdf:resource="http://w3id.org/meta-share/meta-share/DDC310"/>
        <rdfs:label xml:lang="en">Statistics</rdfs:label>
    </owl:NamedIndividual>
    


    <!-- http://w3id.org/meta-share/meta-share/string -->

    <owl:NamedIndividual rdf:about="http://w3id.org/meta-share/meta-share/string">
        <rdf:type rdf:resource="http://w3id.org/meta-share/meta-share/ParameterType"/>
        <rdfs:label xml:lang="en">string</rdfs:label>
    </owl:NamedIndividual>
    


    <!-- http://w3id.org/meta-share/meta-share/studio -->

    <owl:NamedIndividual rdf:about="http://w3id.org/meta-share/meta-share/studio">
        <rdf:type rdf:resource="http://w3id.org/meta-share/meta-share/RecordingEnvironment"/>
        <rdfs:label xml:lang="en">studio</rdfs:label>
    </owl:NamedIndividual>
    


    <!-- http://w3id.org/meta-share/meta-share/studioEquipment -->

    <owl:NamedIndividual rdf:about="http://w3id.org/meta-share/meta-share/studioEquipment">
        <rdf:type rdf:resource="http://w3id.org/meta-share/meta-share/CapturingDeviceType"/>
        <rdfs:label xml:lang="en">studio equipment</rdfs:label>
    </owl:NamedIndividual>
    


    <!-- http://w3id.org/meta-share/meta-share/subcatFrame -->

    <owl:NamedIndividual rdf:about="http://w3id.org/meta-share/meta-share/subcatFrame">
        <rdf:type rdf:resource="http://w3id.org/meta-share/meta-share/SyntacticType"/>
        <rdfs:label xml:lang="en">subcategorization frame</rdfs:label>
    </owl:NamedIndividual>
    


    <!-- http://w3id.org/meta-share/meta-share/submitted -->

    <owl:NamedIndividual rdf:about="http://w3id.org/meta-share/meta-share/submitted">
        <rdf:type rdf:resource="http://w3id.org/meta-share/meta-share/VersionType"/>
        <rdfs:comment xml:lang="en">Value for &apos;Version type&apos; used for versions as submitted for publication</rdfs:comment>
        <rdfs:label xml:lang="en">submitted</rdfs:label>
    </owl:NamedIndividual>
    


    <!-- http://w3id.org/meta-share/meta-share/subsidiary -->

    <owl:NamedIndividual rdf:about="http://w3id.org/meta-share/meta-share/subsidiary">
        <rdf:type rdf:resource="http://w3id.org/meta-share/meta-share/DivisionCategory"/>
        <rdfs:label xml:lang="en">subsidiary</rdfs:label>
    </owl:NamedIndividual>
    


    <!-- http://w3id.org/meta-share/meta-share/subtitle1 -->

    <owl:NamedIndividual rdf:about="http://w3id.org/meta-share/meta-share/subtitle1">
        <rdf:type rdf:resource="http://w3id.org/meta-share/meta-share/TextIncludedInVideo"/>
        <rdfs:label xml:lang="en">subtitle</rdfs:label>
    </owl:NamedIndividual>
    


    <!-- http://w3id.org/meta-share/meta-share/subtitle2 -->

    <owl:NamedIndividual rdf:about="http://w3id.org/meta-share/meta-share/subtitle2">
        <rdf:type rdf:resource="http://w3id.org/meta-share/meta-share/TextIncludedInImage"/>
        <rdfs:label xml:lang="en">subtitle</rdfs:label>
    </owl:NamedIndividual>
    


    <!-- http://w3id.org/meta-share/meta-share/subtitle3 -->

    <owl:NamedIndividual rdf:about="http://w3id.org/meta-share/meta-share/subtitle3">
        <rdf:type rdf:resource="http://w3id.org/meta-share/meta-share/TextType"/>
        <datacite:hasIdentifier rdf:resource="http://w3id.org/meta-share/meta-share/ClarinEl_TT015"/>
        <rdfs:label xml:lang="en">subtitle</rdfs:label>
    </owl:NamedIndividual>
    


    <!-- http://w3id.org/meta-share/meta-share/syllable -->

    <owl:NamedIndividual rdf:about="http://w3id.org/meta-share/meta-share/syllable">
        <rdf:type rdf:resource="http://w3id.org/meta-share/meta-share/BaseItem"/>
        <rdfs:label xml:lang="en">syllable</rdfs:label>
    </owl:NamedIndividual>
    


    <!-- http://w3id.org/meta-share/meta-share/syllable1 -->

    <owl:NamedIndividual rdf:about="http://w3id.org/meta-share/meta-share/syllable1">
        <rdf:type rdf:resource="http://w3id.org/meta-share/meta-share/SegmentationLevel"/>
        <rdfs:label xml:lang="en">syllable</rdfs:label>
    </owl:NamedIndividual>
    


    <!-- http://w3id.org/meta-share/meta-share/syllable2 -->

    <owl:NamedIndividual rdf:about="http://w3id.org/meta-share/meta-share/syllable2">
        <rdf:type rdf:resource="http://w3id.org/meta-share/meta-share/SizeUnit"/>
        <rdfs:label xml:lang="en">syllable</rdfs:label>
    </owl:NamedIndividual>
    


    <!-- http://w3id.org/meta-share/meta-share/synonym -->

    <owl:NamedIndividual rdf:about="http://w3id.org/meta-share/meta-share/synonym">
        <rdf:type rdf:resource="http://w3id.org/meta-share/meta-share/SemanticType"/>
        <rdfs:label xml:lang="en">synonym</rdfs:label>
    </owl:NamedIndividual>
    


    <!-- http://w3id.org/meta-share/meta-share/synset -->

    <owl:NamedIndividual rdf:about="http://w3id.org/meta-share/meta-share/synset">
        <rdf:type rdf:resource="http://w3id.org/meta-share/meta-share/SizeUnit"/>
        <rdfs:label xml:lang="en">synset</rdfs:label>
    </owl:NamedIndividual>
    


    <!-- http://w3id.org/meta-share/meta-share/syntacticUnit -->

    <owl:NamedIndividual rdf:about="http://w3id.org/meta-share/meta-share/syntacticUnit">
        <rdf:type rdf:resource="http://w3id.org/meta-share/meta-share/ExtratextualInformationUnit"/>
        <rdfs:label xml:lang="en">syntactic unit</rdfs:label>
    </owl:NamedIndividual>
    


    <!-- http://w3id.org/meta-share/meta-share/syntacticUnit1 -->

    <owl:NamedIndividual rdf:about="http://w3id.org/meta-share/meta-share/syntacticUnit1">
        <rdf:type rdf:resource="http://w3id.org/meta-share/meta-share/SizeUnit"/>
        <rdfs:label xml:lang="en">syntactic unit</rdfs:label>
    </owl:NamedIndividual>
    


    <!-- http://w3id.org/meta-share/meta-share/syntacticoSemanticLink -->

    <owl:NamedIndividual rdf:about="http://w3id.org/meta-share/meta-share/syntacticoSemanticLink">
        <rdf:type rdf:resource="http://w3id.org/meta-share/meta-share/SyntacticoSemanticType"/>
        <rdfs:label xml:lang="en">syntactico-semantic link</rdfs:label>
    </owl:NamedIndividual>
    


    <!-- http://w3id.org/meta-share/meta-share/syntax -->

    <owl:NamedIndividual rdf:about="http://w3id.org/meta-share/meta-share/syntax">
        <rdf:type rdf:resource="http://w3id.org/meta-share/meta-share/EncodingLevel"/>
        <rdfs:comment xml:lang="en">Value for &apos;EncodingLevel&apos; for the particular linguistic level that relates to the study of the structure of linguistic units (phrases, sentences)</rdfs:comment>
        <rdfs:label xml:lang="en">syntax</rdfs:label>
    </owl:NamedIndividual>
    


    <!-- http://w3id.org/meta-share/meta-share/systemEvaluator -->

    <owl:NamedIndividual rdf:about="http://w3id.org/meta-share/meta-share/systemEvaluator">
        <rdf:type rdf:resource="http://w3id.org/meta-share/meta-share/OrganizationRole"/>
        <rdfs:label xml:lang="en">system evaluator</rdfs:label>
    </owl:NamedIndividual>
    


    <!-- http://w3id.org/meta-share/meta-share/tagset1 -->

    <owl:NamedIndividual rdf:about="http://w3id.org/meta-share/meta-share/tagset1">
        <rdf:type rdf:resource="http://w3id.org/meta-share/meta-share/CompatibleLexiconType"/>
        <rdf:type rdf:resource="http://w3id.org/meta-share/meta-share/LCRSubclass"/>
        <rdfs:comment xml:lang="en">a flat list of valid values (tags) designed to annotate data; it usually corresponds to a specific annotation type or set of annotation types</rdfs:comment>
        <rdfs:label xml:lang="en">tagset</rdfs:label>
    </owl:NamedIndividual>
    


    <!-- http://w3id.org/meta-share/meta-share/tapeVHS -->

    <owl:NamedIndividual rdf:about="http://w3id.org/meta-share/meta-share/tapeVHS">
        <rdf:type rdf:resource="http://w3id.org/meta-share/meta-share/RecordingDeviceType"/>
        <rdfs:label xml:lang="en">VHS tape</rdfs:label>
    </owl:NamedIndividual>
    


    <!-- http://w3id.org/meta-share/meta-share/tb -->

    <owl:NamedIndividual rdf:about="http://w3id.org/meta-share/meta-share/tb">
        <rdf:type rdf:resource="http://w3id.org/meta-share/meta-share/SizeUnit"/>
        <rdfs:altLabel xml:lang="en">tb</rdfs:altLabel>
        <rdfs:label xml:lang="en">terabyte</rdfs:label>
    </owl:NamedIndividual>
    


    <!-- http://w3id.org/meta-share/meta-share/techReport -->

    <owl:NamedIndividual rdf:about="http://w3id.org/meta-share/meta-share/techReport">
        <rdf:type rdf:resource="http://w3id.org/meta-share/meta-share/DocumentType"/>
        <rdfs:label xml:lang="en">technical report</rdfs:label>
    </owl:NamedIndividual>
    


    <!-- http://w3id.org/meta-share/meta-share/technicalText -->

    <owl:NamedIndividual rdf:about="http://w3id.org/meta-share/meta-share/technicalText">
        <rdf:type rdf:resource="http://w3id.org/meta-share/meta-share/TextType"/>
        <datacite:hasIdentifier rdf:resource="http://w3id.org/meta-share/meta-share/ClarinEl_TT011"/>
        <rdfs:label xml:lang="en">technical text</rdfs:label>
    </owl:NamedIndividual>
    


    <!-- http://w3id.org/meta-share/meta-share/technological -->

    <owl:NamedIndividual rdf:about="http://w3id.org/meta-share/meta-share/technological">
        <rdf:type rdf:resource="http://w3id.org/meta-share/meta-share/EvaluationLevel"/>
        <rdfs:label xml:lang="en">technological</rdfs:label>
    </owl:NamedIndividual>
    


    <!-- http://w3id.org/meta-share/meta-share/technology -->

    <owl:NamedIndividual rdf:about="http://w3id.org/meta-share/meta-share/technology">
        <rdf:type rdf:resource="http://w3id.org/meta-share/meta-share/Domain"/>
        <datacite:hasIdentifier rdf:resource="http://w3id.org/meta-share/meta-share/DDC600"/>
        <rdfs:label xml:lang="en">Technology</rdfs:label>
    </owl:NamedIndividual>
    


    <!-- http://w3id.org/meta-share/meta-share/teenager -->

    <owl:NamedIndividual rdf:about="http://w3id.org/meta-share/meta-share/teenager">
        <rdf:type rdf:resource="http://w3id.org/meta-share/meta-share/AgeGroup"/>
        <rdfs:label xml:lang="en">teenager</rdfs:label>
    </owl:NamedIndividual>
    


    <!-- http://w3id.org/meta-share/meta-share/telecommunications -->

    <owl:NamedIndividual rdf:about="http://w3id.org/meta-share/meta-share/telecommunications">
        <rdf:type rdf:resource="http://w3id.org/meta-share/meta-share/Domain"/>
        <datacite:hasIdentifier rdf:resource="http://w3id.org/meta-share/meta-share/ELG_Domain004"/>
        <rdfs:label xml:lang="en">telecommunications</rdfs:label>
    </owl:NamedIndividual>
    


    <!-- http://w3id.org/meta-share/meta-share/telephone -->

    <owl:NamedIndividual rdf:about="http://w3id.org/meta-share/meta-share/telephone">
        <rdf:type rdf:resource="http://w3id.org/meta-share/meta-share/SourceChannel"/>
        <rdfs:label xml:lang="en">telephone</rdfs:label>
    </owl:NamedIndividual>
    


    <!-- http://w3id.org/meta-share/meta-share/telephoneConversation -->

    <owl:NamedIndividual rdf:about="http://w3id.org/meta-share/meta-share/telephoneConversation">
        <rdf:type rdf:resource="http://w3id.org/meta-share/meta-share/TextType"/>
        <datacite:hasIdentifier rdf:resource="http://w3id.org/meta-share/meta-share/ClarinEl_TT005"/>
        <rdfs:label xml:lang="en">telephone conversation</rdfs:label>
    </owl:NamedIndividual>
    


    <!-- http://w3id.org/meta-share/meta-share/telephoneFixed -->

    <owl:NamedIndividual rdf:about="http://w3id.org/meta-share/meta-share/telephoneFixed">
        <rdf:type rdf:resource="http://w3id.org/meta-share/meta-share/CapturingDeviceType"/>
        <rdfs:label xml:lang="en">fixed telephone</rdfs:label>
    </owl:NamedIndividual>
    


    <!-- http://w3id.org/meta-share/meta-share/telephoneIP -->

    <owl:NamedIndividual rdf:about="http://w3id.org/meta-share/meta-share/telephoneIP">
        <rdf:type rdf:resource="http://w3id.org/meta-share/meta-share/CapturingDeviceType"/>
        <rdfs:label xml:lang="en">IP telephone</rdfs:label>
    </owl:NamedIndividual>
    


    <!-- http://w3id.org/meta-share/meta-share/telephoneMobile -->

    <owl:NamedIndividual rdf:about="http://w3id.org/meta-share/meta-share/telephoneMobile">
        <rdf:type rdf:resource="http://w3id.org/meta-share/meta-share/CapturingDeviceType"/>
        <rdfs:label xml:lang="en">mobile telephone</rdfs:label>
    </owl:NamedIndividual>
    


    <!-- http://w3id.org/meta-share/meta-share/telephoneNumber -->

    <owl:NamedIndividual rdf:about="http://w3id.org/meta-share/meta-share/telephoneNumber">
        <rdf:type rdf:resource="http://w3id.org/meta-share/meta-share/SpeechItem"/>
    </owl:NamedIndividual>
    


    <!-- http://w3id.org/meta-share/meta-share/tempo -->

    <owl:NamedIndividual rdf:about="http://w3id.org/meta-share/meta-share/tempo">
        <rdf:type rdf:resource="http://w3id.org/meta-share/meta-share/NonSpeechItem"/>
        <rdfs:label xml:lang="en">tempo</rdfs:label>
    </owl:NamedIndividual>
    


    <!-- http://w3id.org/meta-share/meta-share/tense -->

    <owl:NamedIndividual rdf:about="http://w3id.org/meta-share/meta-share/tense">
        <rdf:type rdf:resource="http://w3id.org/meta-share/meta-share/MorphologicalType"/>
        <rdfs:label xml:lang="en">tense</rdfs:label>
    </owl:NamedIndividual>
    


    <!-- http://w3id.org/meta-share/meta-share/term -->

    <owl:NamedIndividual rdf:about="http://w3id.org/meta-share/meta-share/term">
        <rdf:type rdf:resource="http://w3id.org/meta-share/meta-share/SizeUnit"/>
        <rdfs:label xml:lang="en">term</rdfs:label>
    </owl:NamedIndividual>
    


    <!-- http://w3id.org/meta-share/meta-share/terminologicalResource -->

    <owl:NamedIndividual rdf:about="http://w3id.org/meta-share/meta-share/terminologicalResource">
        <rdf:type rdf:resource="http://w3id.org/meta-share/meta-share/LCRSubclass"/>
        <rdfs:altLabel xml:lang="en">term list</rdfs:altLabel>
        <rdfs:comment xml:lang="en">A lexical resource that lists concepts pertaining to a specific domain</rdfs:comment>
        <rdfs:label xml:lang="en">terminological resource</rdfs:label>
    </owl:NamedIndividual>
    


    <!-- http://w3id.org/meta-share/meta-share/text -->

    <owl:NamedIndividual rdf:about="http://w3id.org/meta-share/meta-share/text">
        <rdf:type rdf:resource="http://w3id.org/meta-share/meta-share/MediaType"/>
        <rdfs:comment xml:lang="en">Value for &apos;MediaType&apos; for the written or printed form of a language resource (part)</rdfs:comment>
        <rdfs:label xml:lang="en">text</rdfs:label>
    </owl:NamedIndividual>
    


    <!-- http://w3id.org/meta-share/meta-share/text1 -->

    <owl:NamedIndividual rdf:about="http://w3id.org/meta-share/meta-share/text1">
        <rdf:type rdf:resource="http://w3id.org/meta-share/meta-share/SizeUnit"/>
        <rdfs:label xml:lang="en">text</rdfs:label>
    </owl:NamedIndividual>
    


    <!-- http://w3id.org/meta-share/meta-share/textNumerical -->

    <owl:NamedIndividual rdf:about="http://w3id.org/meta-share/meta-share/textNumerical">
        <rdf:type rdf:resource="http://w3id.org/meta-share/meta-share/MediaType"/>
        <rdfs:label xml:lang="en">numerical text</rdfs:label>
    </owl:NamedIndividual>
    


    <!-- http://w3id.org/meta-share/meta-share/thesaurus -->

    <owl:NamedIndividual rdf:about="http://w3id.org/meta-share/meta-share/thesaurus">
        <rdf:type rdf:resource="http://w3id.org/meta-share/meta-share/LCRSubclass"/>
        <rdfs:comment xml:lang="en">A reference work that lists words grouped together according to similarity of meaning (containing synonyms and sometimes antonyms) [https://en.wikipedia.org/wiki/Thesaurus]</rdfs:comment>
        <rdfs:label xml:lang="en">thesaurus</rdfs:label>
    </owl:NamedIndividual>
    


    <!-- http://w3id.org/meta-share/meta-share/titlesParsing -->

    <owl:NamedIndividual rdf:about="http://w3id.org/meta-share/meta-share/titlesParsing">
        <rdf:type rdf:resource="http://w3id.org/meta-share/meta-share/LDTask"/>
        <rdfs:label xml:lang="en">parsing of titles</rdfs:label>
    </owl:NamedIndividual>
    


    <!-- http://w3id.org/meta-share/meta-share/token -->

    <owl:NamedIndividual rdf:about="http://w3id.org/meta-share/meta-share/token">
        <rdf:type rdf:resource="http://w3id.org/meta-share/meta-share/SizeUnit"/>
        <rdfs:label xml:lang="en">token</rdfs:label>
    </owl:NamedIndividual>
    


    <!-- http://w3id.org/meta-share/meta-share/token1 -->

    <owl:NamedIndividual rdf:about="http://w3id.org/meta-share/meta-share/token1">
        <rdf:type rdf:resource="http://w3id.org/meta-share/meta-share/SegmentationLevel"/>
        <rdfs:label xml:lang="en">token</rdfs:label>
    </owl:NamedIndividual>
    


    <!-- http://w3id.org/meta-share/meta-share/trainingResource -->

    <owl:NamedIndividual rdf:about="http://w3id.org/meta-share/meta-share/trainingResource">
        <rdf:type rdf:resource="http://w3id.org/meta-share/meta-share/DocumentationType"/>
        <rdfs:comment xml:lang="en">Value for &apos;DocumentationType&apos; used for the training material of a resource (e.g.,  video tutorials, screencasts, guided tours, etc.)</rdfs:comment>
        <rdfs:label xml:lang="en">training resource</rdfs:label>
    </owl:NamedIndividual>
    


    <!-- http://w3id.org/meta-share/meta-share/trainingUse -->

    <owl:NamedIndividual rdf:about="http://w3id.org/meta-share/meta-share/trainingUse">
        <rdf:type rdf:resource="http://w3id.org/meta-share/meta-share/ConditionOfUse"/>
        <rdfs:comment xml:lang="en">Value for &apos;ConditionOfUse&apos; which states that the resource can only be used for training purposes</rdfs:comment>
        <rdfs:label xml:lang="en">training use</rdfs:label>
        <skos:note xml:lang="en">add ODRL representation</skos:note>
    </owl:NamedIndividual>
    


    <!-- http://w3id.org/meta-share/meta-share/transcription -->

    <owl:NamedIndividual rdf:about="http://w3id.org/meta-share/meta-share/transcription">
        <rdf:type rdf:resource="http://w3id.org/meta-share/meta-share/AudioType"/>
        <rdfs:label xml:lang="en">phonetic transcription</rdfs:label>
    </owl:NamedIndividual>
    


    <!-- http://w3id.org/meta-share/meta-share/translationEquivalent -->

    <owl:NamedIndividual rdf:about="http://w3id.org/meta-share/meta-share/translationEquivalent">
        <rdf:type rdf:resource="http://w3id.org/meta-share/meta-share/TranslationType"/>
        <rdfs:label xml:lang="en">translation equivalent</rdfs:label>
    </owl:NamedIndividual>
    


    <!-- http://w3id.org/meta-share/meta-share/translationUnit -->

    <owl:NamedIndividual rdf:about="http://w3id.org/meta-share/meta-share/translationUnit">
        <rdf:type rdf:resource="http://w3id.org/meta-share/meta-share/SizeUnit"/>
        <rdfs:altLabel xml:lang="en">tu</rdfs:altLabel>
        <rdfs:label xml:lang="en">translation unit</rdfs:label>
    </owl:NamedIndividual>
    


    <!-- http://w3id.org/meta-share/meta-share/transport -->

    <owl:NamedIndividual rdf:about="http://w3id.org/meta-share/meta-share/transport">
        <rdf:type rdf:resource="http://w3id.org/meta-share/meta-share/RecordingEnvironment"/>
        <rdfs:label xml:lang="en">transport</rdfs:label>
    </owl:NamedIndividual>
    


    <!-- http://w3id.org/meta-share/meta-share/transportation -->

    <owl:NamedIndividual rdf:about="http://w3id.org/meta-share/meta-share/transportation">
        <rdf:type rdf:resource="http://w3id.org/meta-share/meta-share/Domain"/>
        <datacite:hasIdentifier rdf:resource="http://w3id.org/meta-share/meta-share/DDC388"/>
        <rdfs:label xml:lang="en">Transportation</rdfs:label>
    </owl:NamedIndividual>
    


    <!-- http://w3id.org/meta-share/meta-share/travelIndustry -->

    <owl:NamedIndividual rdf:about="http://w3id.org/meta-share/meta-share/travelIndustry">
        <rdf:type rdf:resource="http://w3id.org/meta-share/meta-share/Domain"/>
        <datacite:hasIdentifier rdf:resource="http://w3id.org/meta-share/meta-share/ELG_Domain013"/>
        <rdfs:label xml:lang="en">travel industry</rdfs:label>
    </owl:NamedIndividual>
    


    <!-- http://w3id.org/meta-share/meta-share/trigram -->

    <owl:NamedIndividual rdf:about="http://w3id.org/meta-share/meta-share/trigram">
        <rdf:type rdf:resource="http://w3id.org/meta-share/meta-share/SizeUnit"/>
        <rdfs:label xml:lang="en">trigram</rdfs:label>
    </owl:NamedIndividual>
    


    <!-- http://w3id.org/meta-share/meta-share/trl1 -->

    <owl:NamedIndividual rdf:about="http://w3id.org/meta-share/meta-share/trl1">
        <rdf:type rdf:resource="http://w3id.org/meta-share/meta-share/TRL"/>
        <rdfs:comment xml:lang="en">Basic principles observed</rdfs:comment>
        <rdfs:label xml:lang="en">TRL1</rdfs:label>
    </owl:NamedIndividual>
    


    <!-- http://w3id.org/meta-share/meta-share/trl2 -->

    <owl:NamedIndividual rdf:about="http://w3id.org/meta-share/meta-share/trl2">
        <rdf:type rdf:resource="http://w3id.org/meta-share/meta-share/TRL"/>
        <rdfs:comment xml:lang="en">Technology concept formulated</rdfs:comment>
        <rdfs:label xml:lang="en">TRL2</rdfs:label>
    </owl:NamedIndividual>
    


    <!-- http://w3id.org/meta-share/meta-share/trl3 -->

    <owl:NamedIndividual rdf:about="http://w3id.org/meta-share/meta-share/trl3">
        <rdf:type rdf:resource="http://w3id.org/meta-share/meta-share/TRL"/>
        <rdfs:comment xml:lang="en">Experimental proof of concept</rdfs:comment>
        <rdfs:label xml:lang="en">TRL3</rdfs:label>
    </owl:NamedIndividual>
    


    <!-- http://w3id.org/meta-share/meta-share/trl4 -->

    <owl:NamedIndividual rdf:about="http://w3id.org/meta-share/meta-share/trl4">
        <rdf:type rdf:resource="http://w3id.org/meta-share/meta-share/TRL"/>
        <rdfs:comment xml:lang="en">Technology validated in lab</rdfs:comment>
        <rdfs:label xml:lang="en">TRL4</rdfs:label>
    </owl:NamedIndividual>
    


    <!-- http://w3id.org/meta-share/meta-share/trl5 -->

    <owl:NamedIndividual rdf:about="http://w3id.org/meta-share/meta-share/trl5">
        <rdf:type rdf:resource="http://w3id.org/meta-share/meta-share/TRL"/>
        <rdfs:comment xml:lang="en">Technology  validated  in  relevant  environment  (industrially relevant environment in the case of key enabling technologies)</rdfs:comment>
        <rdfs:label xml:lang="en">TRL5</rdfs:label>
    </owl:NamedIndividual>
    


    <!-- http://w3id.org/meta-share/meta-share/trl6 -->

    <owl:NamedIndividual rdf:about="http://w3id.org/meta-share/meta-share/trl6">
        <rdf:type rdf:resource="http://w3id.org/meta-share/meta-share/TRL"/>
        <rdfs:comment xml:lang="en">Technology  demonstrated  in  relevant  environment  (industrially relevant environment in the case of key enabling technologies)</rdfs:comment>
        <rdfs:label xml:lang="en">TRL6</rdfs:label>
    </owl:NamedIndividual>
    


    <!-- http://w3id.org/meta-share/meta-share/trl7 -->

    <owl:NamedIndividual rdf:about="http://w3id.org/meta-share/meta-share/trl7">
        <rdf:type rdf:resource="http://w3id.org/meta-share/meta-share/TRL"/>
        <rdfs:comment xml:lang="en">System prototype demonstration in operational environment</rdfs:comment>
        <rdfs:label xml:lang="en">TRL7</rdfs:label>
    </owl:NamedIndividual>
    


    <!-- http://w3id.org/meta-share/meta-share/trl8 -->

    <owl:NamedIndividual rdf:about="http://w3id.org/meta-share/meta-share/trl8">
        <rdf:type rdf:resource="http://w3id.org/meta-share/meta-share/TRL"/>
        <rdfs:comment xml:lang="en">System complete and qualified</rdfs:comment>
        <rdfs:label xml:lang="en">TRL8</rdfs:label>
    </owl:NamedIndividual>
    


    <!-- http://w3id.org/meta-share/meta-share/trl9 -->

    <owl:NamedIndividual rdf:about="http://w3id.org/meta-share/meta-share/trl9">
        <rdf:type rdf:resource="http://w3id.org/meta-share/meta-share/TRL"/>
        <rdfs:comment xml:lang="en">Actual system proven in operational environment (competitive manufacturing in the case of key enabling technologies; or in space)</rdfs:comment>
        <rdfs:label xml:lang="en">TRL9</rdfs:label>
    </owl:NamedIndividual>
    


    <!-- http://w3id.org/meta-share/meta-share/troponym -->

    <owl:NamedIndividual rdf:about="http://w3id.org/meta-share/meta-share/troponym">
        <rdf:type rdf:resource="http://w3id.org/meta-share/meta-share/SemanticType"/>
        <rdfs:label xml:lang="en">troponym</rdfs:label>
    </owl:NamedIndividual>
    


    <!-- http://w3id.org/meta-share/meta-share/truncation -->

    <owl:NamedIndividual rdf:about="http://w3id.org/meta-share/meta-share/truncation">
        <rdf:type rdf:resource="http://w3id.org/meta-share/meta-share/AnnotatedElement"/>
        <rdfs:label xml:lang="en">truncation</rdfs:label>
    </owl:NamedIndividual>
    


    <!-- http://w3id.org/meta-share/meta-share/turn -->

    <owl:NamedIndividual rdf:about="http://w3id.org/meta-share/meta-share/turn">
        <rdf:type rdf:resource="http://w3id.org/meta-share/meta-share/SizeUnit"/>
        <rdfs:label xml:lang="en">turn</rdfs:label>
    </owl:NamedIndividual>
    


    <!-- http://w3id.org/meta-share/meta-share/tv -->

    <owl:NamedIndividual rdf:about="http://w3id.org/meta-share/meta-share/tv">
        <rdf:type rdf:resource="http://w3id.org/meta-share/meta-share/SourceChannel"/>
        <rdfs:label xml:lang="en">tv</rdfs:label>
    </owl:NamedIndividual>
    


    <!-- http://w3id.org/meta-share/meta-share/tweet -->

    <owl:NamedIndividual rdf:about="http://w3id.org/meta-share/meta-share/tweet">
        <rdf:type rdf:resource="http://w3id.org/meta-share/meta-share/TextType"/>
        <datacite:hasIdentifier rdf:resource="http://w3id.org/meta-share/meta-share/ClarinEl_TT007"/>
        <rdfs:label xml:lang="en">tweet</rdfs:label>
    </owl:NamedIndividual>
    


    <!-- http://w3id.org/meta-share/meta-share/twitter -->

    <owl:NamedIndividual rdf:about="http://w3id.org/meta-share/meta-share/twitter">
        <rdf:type rdf:resource="http://w3id.org/meta-share/meta-share/SocialMediaOccupationalAccountType"/>
        <rdfs:label xml:lang="en">twitter</rdfs:label>
    </owl:NamedIndividual>
    


    <!-- http://w3id.org/meta-share/meta-share/typesystem1 -->

    <owl:NamedIndividual rdf:about="http://w3id.org/meta-share/meta-share/typesystem1">
        <rdf:type rdf:resource="http://w3id.org/meta-share/meta-share/LCRSubclass"/>
        <rdfs:comment xml:lang="en">A set of elements designed to annotate data; it typically contains only a list of annotation types, i.e. specific labels that are used for the annotation (e.g.,  part-of-speech, person, organization, etc.), and is usually inbuilt in the annotation software</rdfs:comment>
        <rdfs:label xml:lang="en">typesystem</rdfs:label>
    </owl:NamedIndividual>
    


    <!-- http://w3id.org/meta-share/meta-share/underNegotiation -->

    <owl:NamedIndividual rdf:about="http://w3id.org/meta-share/meta-share/underNegotiation">
        <rdf:type rdf:resource="http://w3id.org/meta-share/meta-share/Availability"/>
        <rdfs:comment xml:lang="en">For resources whose availability is still pending.</rdfs:comment>
        <rdfs:label xml:lang="en">under negotiation</rdfs:label>
    </owl:NamedIndividual>
    


    <!-- http://w3id.org/meta-share/meta-share/unigram -->

    <owl:NamedIndividual rdf:about="http://w3id.org/meta-share/meta-share/unigram">
        <rdf:type rdf:resource="http://w3id.org/meta-share/meta-share/SizeUnit"/>
        <rdfs:label xml:lang="en">unigram</rdfs:label>
    </owl:NamedIndividual>
    


    <!-- http://w3id.org/meta-share/meta-share/unit -->

    <owl:NamedIndividual rdf:about="http://w3id.org/meta-share/meta-share/unit">
        <rdf:type rdf:resource="http://w3id.org/meta-share/meta-share/SizeUnit"/>
        <rdfs:label xml:lang="en">unit</rdfs:label>
    </owl:NamedIndividual>
    


    <!-- http://w3id.org/meta-share/meta-share/unit1 -->

    <owl:NamedIndividual rdf:about="http://w3id.org/meta-share/meta-share/unit1">
        <rdf:type rdf:resource="http://w3id.org/meta-share/meta-share/DivisionCategory"/>
        <rdfs:label xml:lang="en">unit</rdfs:label>
    </owl:NamedIndividual>
    


    <!-- http://w3id.org/meta-share/meta-share/unix -->

    <owl:NamedIndividual rdf:about="http://w3id.org/meta-share/meta-share/unix">
        <rdf:type rdf:resource="http://w3id.org/meta-share/meta-share/OperatingSystem"/>
        <rdfs:label xml:lang="en">UNIX</rdfs:label>
    </owl:NamedIndividual>
    


    <!-- http://w3id.org/meta-share/meta-share/unknown -->

    <owl:NamedIndividual rdf:about="http://w3id.org/meta-share/meta-share/unknown">
        <rdf:type rdf:resource="http://w3id.org/meta-share/meta-share/Origin"/>
        <rdfs:label xml:lang="en">unknown</rdfs:label>
    </owl:NamedIndividual>
    


    <!-- http://w3id.org/meta-share/meta-share/unknown1 -->

    <owl:NamedIndividual rdf:about="http://w3id.org/meta-share/meta-share/unknown1">
        <rdf:type rdf:resource="http://w3id.org/meta-share/meta-share/Sex"/>
        <rdfs:label xml:lang="en">unknown</rdfs:label>
    </owl:NamedIndividual>
    


    <!-- http://w3id.org/meta-share/meta-share/unpublished -->

    <owl:NamedIndividual rdf:about="http://w3id.org/meta-share/meta-share/unpublished">
        <rdf:type rdf:resource="http://w3id.org/meta-share/meta-share/DocumentType"/>
        <rdfs:label xml:lang="en">unpublished</rdfs:label>
    </owl:NamedIndividual>
    


    <!-- http://w3id.org/meta-share/meta-share/unsignedInteger -->

    <owl:NamedIndividual rdf:about="http://w3id.org/meta-share/meta-share/unsignedInteger">
        <rdf:type rdf:resource="http://w3id.org/meta-share/meta-share/SignConvention"/>
        <rdfs:label xml:lang="en">unsigned integer</rdfs:label>
    </owl:NamedIndividual>
    


    <!-- http://w3id.org/meta-share/meta-share/updated -->

    <owl:NamedIndividual rdf:about="http://w3id.org/meta-share/meta-share/updated">
        <rdf:type rdf:resource="http://w3id.org/meta-share/meta-share/VersionType"/>
        <rdfs:comment xml:lang="en">Value for &apos;Version type&apos; used for versions that have been updated vis-a-vis the previous published version</rdfs:comment>
        <rdfs:label xml:lang="en">updated</rdfs:label>
    </owl:NamedIndividual>
    


    <!-- http://w3id.org/meta-share/meta-share/url1 -->

    <owl:NamedIndividual rdf:about="http://w3id.org/meta-share/meta-share/url1">
        <rdf:type rdf:resource="http://w3id.org/meta-share/meta-share/ParameterType"/>
        <rdfs:label xml:lang="en">url</rdfs:label>
    </owl:NamedIndividual>
    


    <!-- http://w3id.org/meta-share/meta-share/usage -->

    <owl:NamedIndividual rdf:about="http://w3id.org/meta-share/meta-share/usage">
        <rdf:type rdf:resource="http://w3id.org/meta-share/meta-share/EvaluationLevel"/>
        <rdfs:label xml:lang="en">usage</rdfs:label>
    </owl:NamedIndividual>
    


    <!-- http://w3id.org/meta-share/meta-share/userIdentified -->

    <owl:NamedIndividual rdf:about="http://w3id.org/meta-share/meta-share/userIdentified">
        <rdf:type rdf:resource="http://w3id.org/meta-share/meta-share/ConditionOfUse"/>
        <rdfs:comment xml:lang="en">Value for &apos;ConditionOfUse&apos; which states that the resource can only be accessed by identified/authenticated users</rdfs:comment>
        <rdfs:label xml:lang="en">user identified</rdfs:label>
    </owl:NamedIndividual>
    


    <!-- http://w3id.org/meta-share/meta-share/userInputText -->

    <owl:NamedIndividual rdf:about="http://w3id.org/meta-share/meta-share/userInputText">
        <rdf:type rdf:resource="http://w3id.org/meta-share/meta-share/ProcessingResourceType"/>
        <rdfs:label xml:lang="en">user input text</rdfs:label>
    </owl:NamedIndividual>
    


    <!-- http://w3id.org/meta-share/meta-share/userManual -->

    <owl:NamedIndividual rdf:about="http://w3id.org/meta-share/meta-share/userManual">
        <rdf:type rdf:resource="http://w3id.org/meta-share/meta-share/DocumentationType"/>
        <rdfs:comment xml:lang="en">Value for &apos;Documentation type&apos; for documents that include instructions and examples on the usage of a tool/service (or resource in general)</rdfs:comment>
        <rdfs:label xml:lang="en">user manual</rdfs:label>
    </owl:NamedIndividual>
    


    <!-- http://w3id.org/meta-share/meta-share/utterance -->

    <owl:NamedIndividual rdf:about="http://w3id.org/meta-share/meta-share/utterance">
        <rdf:type rdf:resource="http://w3id.org/meta-share/meta-share/SegmentationLevel"/>
        <rdfs:label xml:lang="en">utterance</rdfs:label>
    </owl:NamedIndividual>
    


    <!-- http://w3id.org/meta-share/meta-share/utterance1 -->

    <owl:NamedIndividual rdf:about="http://w3id.org/meta-share/meta-share/utterance1">
        <rdf:type rdf:resource="http://w3id.org/meta-share/meta-share/SizeUnit"/>
        <rdfs:label xml:lang="en">utterance</rdfs:label>
    </owl:NamedIndividual>
    


    <!-- http://w3id.org/meta-share/meta-share/variable -->

    <owl:NamedIndividual rdf:about="http://w3id.org/meta-share/meta-share/variable">
        <rdf:type rdf:resource="http://w3id.org/meta-share/meta-share/SceneIllumination"/>
        <rdfs:label xml:lang="en">variable</rdfs:label>
    </owl:NamedIndividual>
    


    <!-- http://w3id.org/meta-share/meta-share/variant1 -->

    <owl:NamedIndividual rdf:about="http://w3id.org/meta-share/meta-share/variant1">
        <rdf:type rdf:resource="http://w3id.org/meta-share/meta-share/LemmaType"/>
        <rdfs:label xml:lang="en">variant</rdfs:label>
    </owl:NamedIndividual>
    


    <!-- http://w3id.org/meta-share/meta-share/vcvSequence -->

    <owl:NamedIndividual rdf:about="http://w3id.org/meta-share/meta-share/vcvSequence">
        <rdf:type rdf:resource="http://w3id.org/meta-share/meta-share/SpeechItem"/>
        <rdfs:label xml:lang="en">VCV sequence</rdfs:label>
    </owl:NamedIndividual>
    


    <!-- http://w3id.org/meta-share/meta-share/vector -->

    <owl:NamedIndividual rdf:about="http://w3id.org/meta-share/meta-share/vector">
        <rdf:type rdf:resource="http://w3id.org/meta-share/meta-share/RasterOrVectorGraphics"/>
        <rdfs:label xml:lang="en">vector</rdfs:label>
    </owl:NamedIndividual>
    


    <!-- http://w3id.org/meta-share/meta-share/veryHigh -->

    <owl:NamedIndividual rdf:about="http://w3id.org/meta-share/meta-share/veryHigh">
        <rdf:type rdf:resource="http://w3id.org/meta-share/meta-share/RecordingQuality"/>
        <rdfs:label xml:lang="en">very high</rdfs:label>
    </owl:NamedIndividual>
    


    <!-- http://w3id.org/meta-share/meta-share/veryHigh1 -->

    <owl:NamedIndividual rdf:about="http://w3id.org/meta-share/meta-share/veryHigh1">
        <rdf:type rdf:resource="http://w3id.org/meta-share/meta-share/Quality"/>
        <rdfs:label xml:lang="en">very high</rdfs:label>
    </owl:NamedIndividual>
    


    <!-- http://w3id.org/meta-share/meta-share/veryLow -->

    <owl:NamedIndividual rdf:about="http://w3id.org/meta-share/meta-share/veryLow">
        <rdf:type rdf:resource="http://w3id.org/meta-share/meta-share/RecordingQuality"/>
        <rdfs:label xml:lang="en">very low</rdfs:label>
    </owl:NamedIndividual>
    


    <!-- http://w3id.org/meta-share/meta-share/veryLow1 -->

    <owl:NamedIndividual rdf:about="http://w3id.org/meta-share/meta-share/veryLow1">
        <rdf:type rdf:resource="http://w3id.org/meta-share/meta-share/Quality"/>
        <rdfs:label xml:lang="en">very low</rdfs:label>
    </owl:NamedIndividual>
    


    <!-- http://w3id.org/meta-share/meta-share/video -->

    <owl:NamedIndividual rdf:about="http://w3id.org/meta-share/meta-share/video">
        <rdf:type rdf:resource="http://w3id.org/meta-share/meta-share/MediaType"/>
        <rdfs:comment xml:lang="en">Value for &apos;Media type&apos; for the audiovisual form of a language resource (part)</rdfs:comment>
        <rdfs:label xml:lang="en">video</rdfs:label>
    </owl:NamedIndividual>
    


    <!-- http://w3id.org/meta-share/meta-share/video1 -->

    <owl:NamedIndividual rdf:about="http://w3id.org/meta-share/meta-share/video1">
        <rdf:type rdf:resource="http://w3id.org/meta-share/meta-share/ExtratextualInformation"/>
        <rdfs:label xml:lang="en">video</rdfs:label>
    </owl:NamedIndividual>
    


    <!-- http://w3id.org/meta-share/meta-share/voice -->

    <owl:NamedIndividual rdf:about="http://w3id.org/meta-share/meta-share/voice">
        <rdf:type rdf:resource="http://w3id.org/meta-share/meta-share/ModalityType"/>
        <rdfs:comment xml:lang="en">Value for &apos;ModalityType&apos; for voice</rdfs:comment>
        <rdfs:label xml:lang="en">voice</rdfs:label>
    </owl:NamedIndividual>
    


    <!-- http://w3id.org/meta-share/meta-share/voice1 -->

    <owl:NamedIndividual rdf:about="http://w3id.org/meta-share/meta-share/voice1">
        <rdf:type rdf:resource="http://w3id.org/meta-share/meta-share/MorphologicalType"/>
        <rdfs:label xml:lang="en">voice</rdfs:label>
    </owl:NamedIndividual>
    


    <!-- http://w3id.org/meta-share/meta-share/webCam -->

    <owl:NamedIndividual rdf:about="http://w3id.org/meta-share/meta-share/webCam">
        <rdf:type rdf:resource="http://w3id.org/meta-share/meta-share/SourceChannel"/>
        <rdfs:label xml:lang="en">webcam</rdfs:label>
    </owl:NamedIndividual>
    


    <!-- http://w3id.org/meta-share/meta-share/webService -->

    <owl:NamedIndividual rdf:about="http://w3id.org/meta-share/meta-share/webService">
        <rdf:type rdf:resource="http://w3id.org/meta-share/meta-share/SoftwareDistributionForm"/>
        <rdfs:comment xml:lang="en">Value for software distribution form, used for software objects that can be accessed through remote invocation typically using some REST-style APIs or SOAP protocols</rdfs:comment>
        <rdfs:label xml:lang="en">web service</rdfs:label>
    </owl:NamedIndividual>
    


    <!-- http://w3id.org/meta-share/meta-share/webcam -->

    <owl:NamedIndividual rdf:about="http://w3id.org/meta-share/meta-share/webcam">
        <rdf:type rdf:resource="http://w3id.org/meta-share/meta-share/CapturingDeviceType"/>
        <rdfs:label xml:lang="en">webcam</rdfs:label>
    </owl:NamedIndividual>
    


    <!-- http://w3id.org/meta-share/meta-share/wholeBody -->

    <owl:NamedIndividual rdf:about="http://w3id.org/meta-share/meta-share/wholeBody">
        <rdf:type rdf:resource="http://w3id.org/meta-share/meta-share/BodyPart"/>
        <rdfs:label xml:lang="en">whole body</rdfs:label>
    </owl:NamedIndividual>
    


    <!-- http://w3id.org/meta-share/meta-share/windows -->

    <owl:NamedIndividual rdf:about="http://w3id.org/meta-share/meta-share/windows">
        <rdf:type rdf:resource="http://w3id.org/meta-share/meta-share/OperatingSystem"/>
        <rdfs:label xml:lang="en">Windows</rdfs:label>
    </owl:NamedIndividual>
    


    <!-- http://w3id.org/meta-share/meta-share/windows-1250 -->

    <owl:NamedIndividual rdf:about="http://w3id.org/meta-share/meta-share/windows-1250">
        <rdf:type rdf:resource="http://w3id.org/meta-share/meta-share/CharacterEncoding"/>
        <rdfs:label xml:lang="en">windows-1250</rdfs:label>
    </owl:NamedIndividual>
    


    <!-- http://w3id.org/meta-share/meta-share/windows-1251 -->

    <owl:NamedIndividual rdf:about="http://w3id.org/meta-share/meta-share/windows-1251">
        <rdf:type rdf:resource="http://w3id.org/meta-share/meta-share/CharacterEncoding"/>
        <rdfs:label xml:lang="en">windows-1251</rdfs:label>
    </owl:NamedIndividual>
    


    <!-- http://w3id.org/meta-share/meta-share/windows-1252 -->

    <owl:NamedIndividual rdf:about="http://w3id.org/meta-share/meta-share/windows-1252">
        <rdf:type rdf:resource="http://w3id.org/meta-share/meta-share/CharacterEncoding"/>
        <rdfs:label xml:lang="en">windows-1252</rdfs:label>
    </owl:NamedIndividual>
    


    <!-- http://w3id.org/meta-share/meta-share/windows-1253 -->

    <owl:NamedIndividual rdf:about="http://w3id.org/meta-share/meta-share/windows-1253">
        <rdf:type rdf:resource="http://w3id.org/meta-share/meta-share/CharacterEncoding"/>
        <rdfs:label xml:lang="en">windows-1253</rdfs:label>
    </owl:NamedIndividual>
    


    <!-- http://w3id.org/meta-share/meta-share/windows-1254 -->

    <owl:NamedIndividual rdf:about="http://w3id.org/meta-share/meta-share/windows-1254">
        <rdf:type rdf:resource="http://w3id.org/meta-share/meta-share/CharacterEncoding"/>
        <rdfs:label xml:lang="en">windows-1254</rdfs:label>
    </owl:NamedIndividual>
    


    <!-- http://w3id.org/meta-share/meta-share/windows-1255 -->

    <owl:NamedIndividual rdf:about="http://w3id.org/meta-share/meta-share/windows-1255">
        <rdf:type rdf:resource="http://w3id.org/meta-share/meta-share/CharacterEncoding"/>
        <rdfs:label xml:lang="en">windows-1255</rdfs:label>
    </owl:NamedIndividual>
    


    <!-- http://w3id.org/meta-share/meta-share/windows-1256 -->

    <owl:NamedIndividual rdf:about="http://w3id.org/meta-share/meta-share/windows-1256">
        <rdf:type rdf:resource="http://w3id.org/meta-share/meta-share/CharacterEncoding"/>
        <rdfs:label xml:lang="en">windows-1256</rdfs:label>
    </owl:NamedIndividual>
    


    <!-- http://w3id.org/meta-share/meta-share/windows-1257 -->

    <owl:NamedIndividual rdf:about="http://w3id.org/meta-share/meta-share/windows-1257">
        <rdf:type rdf:resource="http://w3id.org/meta-share/meta-share/CharacterEncoding"/>
        <rdfs:label xml:lang="en">windows-1257</rdfs:label>
    </owl:NamedIndividual>
    


    <!-- http://w3id.org/meta-share/meta-share/windows-1258 -->

    <owl:NamedIndividual rdf:about="http://w3id.org/meta-share/meta-share/windows-1258">
        <rdf:type rdf:resource="http://w3id.org/meta-share/meta-share/CharacterEncoding"/>
        <rdfs:label xml:lang="en">windows-1258</rdfs:label>
    </owl:NamedIndividual>
    


    <!-- http://w3id.org/meta-share/meta-share/windows-31j -->

    <owl:NamedIndividual rdf:about="http://w3id.org/meta-share/meta-share/windows-31j">
        <rdf:type rdf:resource="http://w3id.org/meta-share/meta-share/CharacterEncoding"/>
        <rdfs:label xml:lang="en">windows-31j</rdfs:label>
    </owl:NamedIndividual>
    


    <!-- http://w3id.org/meta-share/meta-share/wizardOfOz -->

    <owl:NamedIndividual rdf:about="http://w3id.org/meta-share/meta-share/wizardOfOz">
        <rdf:type rdf:resource="http://w3id.org/meta-share/meta-share/ScenarioType"/>
        <rdfs:label xml:lang="en">wizard of Oz</rdfs:label>
    </owl:NamedIndividual>
    


    <!-- http://w3id.org/meta-share/meta-share/word -->

    <owl:NamedIndividual rdf:about="http://w3id.org/meta-share/meta-share/word">
        <rdf:type rdf:resource="http://w3id.org/meta-share/meta-share/BaseItem"/>
        <rdfs:label xml:lang="en">word</rdfs:label>
    </owl:NamedIndividual>
    


    <!-- http://w3id.org/meta-share/meta-share/word1 -->

    <owl:NamedIndividual rdf:about="http://w3id.org/meta-share/meta-share/word1">
        <rdf:type rdf:resource="http://w3id.org/meta-share/meta-share/SegmentationLevel"/>
        <rdfs:label xml:lang="en">word</rdfs:label>
    </owl:NamedIndividual>
    


    <!-- http://w3id.org/meta-share/meta-share/word2 -->

    <owl:NamedIndividual rdf:about="http://w3id.org/meta-share/meta-share/word2">
        <rdf:type rdf:resource="http://w3id.org/meta-share/meta-share/ExtratextualInformationUnit"/>
        <rdfs:label xml:lang="en">word</rdfs:label>
    </owl:NamedIndividual>
    


    <!-- http://w3id.org/meta-share/meta-share/word3 -->

    <owl:NamedIndividual rdf:about="http://w3id.org/meta-share/meta-share/word3">
        <rdf:type rdf:resource="http://w3id.org/meta-share/meta-share/SizeUnit"/>
        <rdfs:label xml:lang="en">word</rdfs:label>
    </owl:NamedIndividual>
    


    <!-- http://w3id.org/meta-share/meta-share/wordGame -->

    <owl:NamedIndividual rdf:about="http://w3id.org/meta-share/meta-share/wordGame">
        <rdf:type rdf:resource="http://w3id.org/meta-share/meta-share/ScenarioType"/>
        <rdfs:label xml:lang="en">word game</rdfs:label>
    </owl:NamedIndividual>
    


    <!-- http://w3id.org/meta-share/meta-share/wordGroup -->

    <owl:NamedIndividual rdf:about="http://w3id.org/meta-share/meta-share/wordGroup">
        <rdf:type rdf:resource="http://w3id.org/meta-share/meta-share/SegmentationLevel"/>
        <rdfs:label xml:lang="en">word group</rdfs:label>
    </owl:NamedIndividual>
    


    <!-- http://w3id.org/meta-share/meta-share/wordNet -->

    <owl:NamedIndividual rdf:about="http://w3id.org/meta-share/meta-share/wordNet">
        <rdf:type rdf:resource="http://w3id.org/meta-share/meta-share/CompatibleLexiconType"/>
        <rdf:type rdf:resource="http://w3id.org/meta-share/meta-share/LCRSubclass"/>
        <rdf:type rdf:resource="http://w3id.org/meta-share/meta-share/StandardBestPractice"/>
        <rdfs:comment xml:lang="en">A lexical database originally created for English and extended to other languages, which groups words into sets of synonyms called synsets, provides short definitions and usage examples, and records a number of relations among these synonym sets or their members</rdfs:comment>
        <rdfs:label xml:lang="en">WordNet</rdfs:label>
    </owl:NamedIndividual>
    


    <!-- http://w3id.org/meta-share/meta-share/wordlist -->

    <owl:NamedIndividual rdf:about="http://w3id.org/meta-share/meta-share/wordlist">
        <rdf:type rdf:resource="http://w3id.org/meta-share/meta-share/CompatibleLexiconType"/>
        <rdf:type rdf:resource="http://w3id.org/meta-share/meta-share/LCRSubclass"/>
        <rdfs:comment xml:lang="en">A written collection of all words derived from a particular source, or sharing some other characteristic [https://www.yourdictionary.com/wordlist]</rdfs:comment>
        <rdfs:label xml:lang="en">wordlist</rdfs:label>
    </owl:NamedIndividual>
    


    <!-- http://w3id.org/meta-share/meta-share/workflowFile -->

    <owl:NamedIndividual rdf:about="http://w3id.org/meta-share/meta-share/workflowFile">
        <rdf:type rdf:resource="http://w3id.org/meta-share/meta-share/SoftwareDistributionForm"/>
        <rdfs:comment xml:lang="en">Value for software distribution form, used for software workflows that are made available in the form of the workflow description file</rdfs:comment>
        <rdfs:label xml:lang="en">workflow file</rdfs:label>
    </owl:NamedIndividual>
    


    <!-- http://w3id.org/meta-share/meta-share/writtenLanguage -->

    <owl:NamedIndividual rdf:about="http://w3id.org/meta-share/meta-share/writtenLanguage">
        <rdf:type rdf:resource="http://w3id.org/meta-share/meta-share/ModalityType"/>
        <rdfs:comment xml:lang="en">Value for &apos;ModalityType&apos; for texts with written language</rdfs:comment>
        <rdfs:label xml:lang="en">written language</rdfs:label>
    </owl:NamedIndividual>
    


    <!-- http://w3id.org/meta-share/meta-share/x-EUC-CN -->

    <owl:NamedIndividual rdf:about="http://w3id.org/meta-share/meta-share/x-EUC-CN">
        <rdf:type rdf:resource="http://w3id.org/meta-share/meta-share/CharacterEncoding"/>
        <rdfs:label xml:lang="en">x-EUC-CN</rdfs:label>
    </owl:NamedIndividual>
    


    <!-- http://w3id.org/meta-share/meta-share/x-EUC-JP-LINUX -->

    <owl:NamedIndividual rdf:about="http://w3id.org/meta-share/meta-share/x-EUC-JP-LINUX">
        <rdf:type rdf:resource="http://w3id.org/meta-share/meta-share/CharacterEncoding"/>
        <rdfs:label xml:lang="en">x-EUC-JP-LINUX</rdfs:label>
    </owl:NamedIndividual>
    


    <!-- http://w3id.org/meta-share/meta-share/x-EUC-TW -->

    <owl:NamedIndividual rdf:about="http://w3id.org/meta-share/meta-share/x-EUC-TW">
        <rdf:type rdf:resource="http://w3id.org/meta-share/meta-share/CharacterEncoding"/>
        <rdfs:label xml:lang="en">x-EUC-TW</rdfs:label>
    </owl:NamedIndividual>
    


    <!-- http://w3id.org/meta-share/meta-share/x-MS950-HKSCS -->

    <owl:NamedIndividual rdf:about="http://w3id.org/meta-share/meta-share/x-MS950-HKSCS">
        <rdf:type rdf:resource="http://w3id.org/meta-share/meta-share/CharacterEncoding"/>
        <rdfs:label xml:lang="en">x-MS950-HKSCS</rdfs:label>
    </owl:NamedIndividual>
    


    <!-- http://w3id.org/meta-share/meta-share/x-mswin-936 -->

    <owl:NamedIndividual rdf:about="http://w3id.org/meta-share/meta-share/x-mswin-936">
        <rdf:type rdf:resource="http://w3id.org/meta-share/meta-share/CharacterEncoding"/>
        <rdfs:label xml:lang="en">x-mswin-936</rdfs:label>
    </owl:NamedIndividual>
    


    <!-- http://w3id.org/meta-share/meta-share/x-windows-949 -->

    <owl:NamedIndividual rdf:about="http://w3id.org/meta-share/meta-share/x-windows-949">
        <rdf:type rdf:resource="http://w3id.org/meta-share/meta-share/CharacterEncoding"/>
        <rdfs:label xml:lang="en">x-windows-949</rdfs:label>
    </owl:NamedIndividual>
    


    <!-- http://w3id.org/meta-share/meta-share/x-windows-950 -->

    <owl:NamedIndividual rdf:about="http://w3id.org/meta-share/meta-share/x-windows-950">
        <rdf:type rdf:resource="http://w3id.org/meta-share/meta-share/CharacterEncoding"/>
        <rdfs:label xml:lang="en">x-windows-950</rdfs:label>
    </owl:NamedIndividual>
    


    <!-- http://w3id.org/meta-share/meta-share/yes -->

    <owl:NamedIndividual rdf:about="http://w3id.org/meta-share/meta-share/yes">
        <rdf:type rdf:resource="http://w3id.org/meta-share/meta-share/SpeakingImpairmentOfParticipants"/>
        <rdfs:label xml:lang="en">yes</rdfs:label>
    </owl:NamedIndividual>
    


    <!-- http://w3id.org/meta-share/meta-share/yesH -->

    <owl:NamedIndividual rdf:about="http://w3id.org/meta-share/meta-share/yesH">
        <rdf:type rdf:resource="http://w3id.org/meta-share/meta-share/HearingImpairmentOfParticipants"/>
        <rdfs:label xml:lang="en">yes</rdfs:label>
    </owl:NamedIndividual>
    


    <!-- http://w3id.org/meta-share/meta-share/yesNoQuestion -->

    <owl:NamedIndividual rdf:about="http://w3id.org/meta-share/meta-share/yesNoQuestion">
        <rdf:type rdf:resource="http://w3id.org/meta-share/meta-share/SpeechItem"/>
        <rdfs:label xml:lang="en">yes/no question</rdfs:label>
    </owl:NamedIndividual>
    


    <!-- http://w3id.org/meta-share/meta-share/youtube -->

    <owl:NamedIndividual rdf:about="http://w3id.org/meta-share/meta-share/youtube">
        <rdf:type rdf:resource="http://w3id.org/meta-share/meta-share/SocialMediaOccupationalAccountType"/>
        <rdfs:label>youtube</rdfs:label>
    </owl:NamedIndividual>
    


    <!-- http://w3id.org/meta-share/meta-share/4:2:24four_2_2 -->

    <owl:NamedIndividual rdf:about="http://w3id.org/meta-share/meta-share/4:2:24four_2_2">
        <rdf:type rdf:resource="http://w3id.org/meta-share/meta-share/ColourSpace"/>
        <rdfs:label xml:lang="en">4:2:2</rdfs:label>
    </owl:NamedIndividual>
    <rdf:Description>
        <odrl:action rdf:resource="http://creativecommons.org/ns#Reproduction"/>
    </rdf:Description>
    <rdf:Description>
        <odrl:constraint>
            <rdf:Description>
                <odrl:operator rdf:resource="http://www.w3.org/ns/odrl/2/eq"/>
                <odrl:purpose rdf:resource="http://w3id.org/meta-share/meta-share/academic"/>
            </rdf:Description>
        </odrl:constraint>
    </rdf:Description>
    <rdf:Description>
        <odrl:action rdf:resource="http://creativecommons.org/ns#CommercialUse"/>
    </rdf:Description>
    <rdf:Description>
        <odrl:action rdf:resource="http://creativecommons.org/ns#CommericalUse"/>
        <odrl:action rdf:resource="http://creativecommons.org/ns#Distribution"/>
    </rdf:Description>
    


    <!-- 
    ///////////////////////////////////////////////////////////////////////////////////////
    //
    // Annotations
    //
    ///////////////////////////////////////////////////////////////////////////////////////
     -->

    <rdf:Description rdf:about="http://w3id.org/meta-share/meta-share/CharacterEncodingSet">
        <dct:replaces rdf:resource="http://www.ilsp.gr/META-XMLSchema#characterEncoding"/>
    </rdf:Description>
    <rdf:Description rdf:about="http://w3id.org/meta-share/meta-share/DomainClassification">
        <dct:replaces rdf:resource="http://www.ilsp.gr/META-XMLSchema#domainInfo"/>
    </rdf:Description>
    <rdf:Description rdf:about="http://w3id.org/meta-share/meta-share/GeographicCoverageClassification">
        <dct:replaces rdf:resource="http://www.ilsp.gr/META-XMLSchema#geographicCoverageInfo"/>
    </rdf:Description>
    <rdf:Description rdf:about="http://w3id.org/meta-share/meta-share/LicenseInfo">
        <rdfs:comment xml:lang="en">Links a resource to the licence under which it is distributed; values are taken from a list of standard licences</rdfs:comment>
    </rdf:Description>
    <rdf:Description rdf:about="http://w3id.org/meta-share/meta-share/TimeCoverageClassification">
        <dct:replaces rdf:resource="http://www.ilsp.gr/META-XMLSchema#timeCoverageInfo"/>
    </rdf:Description>
    <rdf:Description rdf:about="http://w3id.org/meta-share/meta-share/availableThroughOtherDistributor">
        <dct:replaces rdf:resource="http://www.ilsp.gr/META-XMLSchema#notAvailableThroughMetashare"/>
        <rdfs:label xml:lang="en">Available Through Other Distributor</rdfs:label>
        <rdfs:comment xml:lang="en">For resources that are documented in the catalogue but the contents of which can only be accessed through other distribution channels.</rdfs:comment>
    </rdf:Description>
    <rdf:Description rdf:about="http://w3id.org/meta-share/meta-share/guidelines">
        <rdfs:comment xml:lang="en">Links to the document used as guidelines for the creation or annotation of a corpus</rdfs:comment>
        <rdfs:label xml:lang="en">guidelines</rdfs:label>
    </rdf:Description>
    <rdf:Description rdf:about="http://w3id.org/meta-share/meta-share/licenseInfo">
        <rdfs:comment xml:lang="en">Links a resource to the licence under which it is distributed; values are taken from a list of standard licences</rdfs:comment>
    </rdf:Description>
    <rdf:Description rdf:about="http://w3id.org/meta-share/meta-share/telephoneNumber">
        <rdfs:comment xml:lang="en">The telephone number of a person or an organization; recommended format: +_international code_city code_number</rdfs:comment>
        <rdfs:label xml:lang="en">telephone number</rdfs:label>
    </rdf:Description>
    <rdf:Description rdf:about="http://w3id.org/meta-share/meta-share/2.0.0/copyrightNotEvaluated">
        <rdfs:label xml:lang="en">Copyright Not Evaluated</rdfs:label>
    </rdf:Description>
    <rdf:Description rdf:about="http://w3id.org/meta-share/meta-share/2.0.0/copyrightUndetermined">
        <rdfs:label xml:lang="en">Copyright Undetermined</rdfs:label>
    </rdf:Description>
    <rdf:Description rdf:about="http://w3id.org/meta-share/meta-share/2.0.0/embargoedAccess">
        <rdfs:label xml:lang="en">embargoed access</rdfs:label>
        <rdfs:comment xml:lang="en">Embargoed access refers to a resource that is metadata only access until released for open access on a certain date. Embargoes can be required by publishers and funders policies, or set by the author (e.g such as in the case of theses and dissertations).</rdfs:comment>
    </rdf:Description>
    <rdf:Description rdf:about="http://w3id.org/meta-share/meta-share/2.0.0/inCopyright">
        <rdfs:label xml:lang="en">In Copyright</rdfs:label>
    </rdf:Description>
    <rdf:Description rdf:about="http://w3id.org/meta-share/meta-share/2.0.0/inCopyrightEUOrphan">
        <rdfs:label xml:lang="en">In Copyright - EU Orphan Work</rdfs:label>
    </rdf:Description>
    <rdf:Description rdf:about="http://w3id.org/meta-share/meta-share/2.0.0/inCopyrightEdu">
        <rdfs:label xml:lang="en">In Copyright - Educational Use Permitted</rdfs:label>
    </rdf:Description>
    <rdf:Description rdf:about="http://w3id.org/meta-share/meta-share/2.0.0/inCopyrightNCPermitted">
        <rdfs:label xml:lang="en">In Copyright - Non-Commercial Use Permitted</rdfs:label>
    </rdf:Description>
    <rdf:Description rdf:about="http://w3id.org/meta-share/meta-share/2.0.0/inCopyrightRightsHoldersUnlocatable">
        <rdfs:label xml:lang="en">In Copyright - Rights-holder(s) Unlocatable or Unidentifiable</rdfs:label>
    </rdf:Description>
    <rdf:Description rdf:about="http://w3id.org/meta-share/meta-share/2.0.0/metadataOnlyAccess">
        <rdfs:comment xml:lang="en">Metadata only access refers to a resource in which access is limited to metadata only. The resource itself is described by the metadata, but neither is directly available through the system or platform nor can be referenced to an open access copy in an external journal or trustworthy archive.</rdfs:comment>
        <rdfs:label>metadata only access</rdfs:label>
    </rdf:Description>
    <rdf:Description rdf:about="http://w3id.org/meta-share/meta-share/2.0.0/noCopyright">
        <rdfs:label xml:lang="en">No Copyright - Other Known Legal Restrictions</rdfs:label>
    </rdf:Description>
    <rdf:Description rdf:about="http://w3id.org/meta-share/meta-share/2.0.0/noCopyrightContract">
        <rdfs:label xml:lang="en">No Copyright - Contractual Restrictions</rdfs:label>
    </rdf:Description>
    <rdf:Description rdf:about="http://w3id.org/meta-share/meta-share/2.0.0/noCopyrightNC">
        <rdfs:label xml:lang="en">No Copyright - Non-Commercial Use Only</rdfs:label>
    </rdf:Description>
    <rdf:Description rdf:about="http://w3id.org/meta-share/meta-share/2.0.0/noCopyrightUS">
        <rdfs:label xml:lang="en">No Copyright - United States</rdfs:label>
    </rdf:Description>
    <rdf:Description rdf:about="http://w3id.org/meta-share/meta-share/2.0.0/noKnownCopyright">
        <rdfs:label xml:lang="en">No Known Copyright</rdfs:label>
    </rdf:Description>
    <rdf:Description rdf:about="http://w3id.org/meta-share/meta-share/2.0.0/openAccess1">
        <rdfs:comment xml:lang="en">Open access refers to a resource that is immediately and permanently online, and free for all on the Web, without financial and technical barriers.The resource is either stored in the repository or referenced to an external journal or trustworthy archive.</rdfs:comment>
        <rdfs:label xml:lang="en">open access</rdfs:label>
    </rdf:Description>
    <rdf:Description rdf:about="http://w3id.org/meta-share/meta-share/2.0.0/restrictedAccess1">
        <rdfs:label xml:lang="en">restricted access</rdfs:label>
        <rdfs:comment xml:lang="en">Restricted access refers to a resource that is available in a system but with some type of restriction for full open access. This type of access can occur in a number of different situations. Some examples are described below: The user must log-in to the system in order to access the resource The user must send an email to the author or system administrator to access the resource Access to the resource is restricted to a specific community (e.g.,  limited to a university community)</rdfs:comment>
    </rdf:Description>
</rdf:RDF>



<!-- Generated by the OWL API (version 4.2.8.20170104-2310) https://github.com/owlcs/owlapi -->

