@prefix : <http://w3id.org/meta-share/meta-share> .
@prefix cc: <http://creativecommons.org/ns#> .
@prefix dc: <http://purl.org/dc/elements/1.1/> .
@prefix ms: <http://w3id.org/meta-share/meta-share/> .
@prefix dct: <http://purl.org/dc/terms/> .
@prefix owl: <http://www.w3.org/2002/07/owl#> .
@prefix rdf: <http://www.w3.org/1999/02/22-rdf-syntax-ns#> .
@prefix xml: <http://www.w3.org/XML/1998/namespace> .
@prefix xsd: <http://www.w3.org/2001/XMLSchema#> .
@prefix dcat: <http://www.w3.org/ns/dcat#> .
@prefix foaf: <http://xmlns.com/foaf/0.1/> .
@prefix odrl: <http://www.w3.org/ns/odrl/2/> .
@prefix omtd: <http://w3id.org/meta-share/omtd-share/> .
@prefix rdfs: <http://www.w3.org/2000/01/rdf-schema#> .
@prefix skos: <http://www.w3.org/2004/02/skos/core#> .
@prefix swrc: <http://swrc.ontoware.org/ontology#> .
@prefix vann: <http://purl.org/vocab/vann/> .
@prefix msxml: <http://www.ilsp.gr/META-XMLSchema#> .
@prefix datacite: <http://purl.org/spar/datacite/> .
@base <http://w3id.org/meta-share/meta-share> .

<http://w3id.org/meta-share/meta-share> rdf:type owl:Ontology ;
                                         owl:versionIRI <http://w3id.org/meta-share/meta-share/2.0.0> ;
                                         dc:description """Meta-Share ontology v2. The ontology caters for the description of Language resources (corpora, lexical/conceptual resources, models, grammars, etc. and language processing tools and services) for Language Technology needs. 
It is also related to the OMTD-SHARE ontology (http://w3id.org/meta-share/omtd-share/) which caters for specific features (LT operation/area, data format, method, annotation type)."""@en ;
                                         dc:title "META-SHARE ontology"@en ;
                                         dct:creator <http://john.mccr.ae/> ,
                                                     "Dimitris Galanis" ,
                                                     "John P. McCrae" ,
                                                     "Jorge Gracia" ,
                                                     "Katerina Gkirtzou" ,
                                                     "Marta Villegas" ,
                                                     "Penny Labropoulou" ,
                                                     "Philipp Cimiano" ,
                                                     "Victor Rodriguez Doncel" ;
                                         dct:license <http://purl.org/NET/rdflicense/cc-by4.0> ;
                                         dct:modified "2020-03-20" ;
                                         vann:preferredNamespacePrefix "ms" ;
                                         vann:preferredNamespaceUri ms: ;
                                         owl:priorVersion <http://lodserver.iula.upf.edu/Metashare/ontology/> ,
                                                          <http://purl.org/ms-lod/MetaShareRights.ttl#> ;
                                         owl:versionInfo "v2.0.0 pre-release"@en .

#################################################################
#    Annotation properties
#################################################################

###  http://purl.org/dc/elements/1.1/description
dc:description rdf:type owl:AnnotationProperty .


###  http://purl.org/dc/elements/1.1/source
dc:source rdf:type owl:AnnotationProperty .


###  http://purl.org/dc/elements/1.1/title
dc:title rdf:type owl:AnnotationProperty .


###  http://purl.org/dc/terms/contributor
dct:contributor rdf:type owl:AnnotationProperty .


###  http://purl.org/dc/terms/creator
dct:creator rdf:type owl:AnnotationProperty .


###  http://purl.org/dc/terms/license
dct:license rdf:type owl:AnnotationProperty .


###  http://purl.org/dc/terms/modified
dct:modified rdf:type owl:AnnotationProperty .


###  http://purl.org/dc/terms/replaces
dct:replaces rdf:type owl:AnnotationProperty .


###  http://purl.org/dc/terms/source
dct:source rdf:type owl:AnnotationProperty .


###  http://purl.org/vocab/vann/preferredNamespacePrefix
vann:preferredNamespacePrefix rdf:type owl:AnnotationProperty .


###  http://purl.org/vocab/vann/preferredNamespaceUri
vann:preferredNamespaceUri rdf:type owl:AnnotationProperty .


###  http://www.w3.org/2002/07/owl#equivalentProperty
owl:equivalentProperty rdf:type owl:AnnotationProperty .


###  http://www.w3.org/2002/07/owl#sameAs
owl:sameAs rdf:type owl:AnnotationProperty .


###  http://www.w3.org/2004/02/skos/core#altLabel
skos:altLabel rdf:type owl:AnnotationProperty .


###  http://www.w3.org/2004/02/skos/core#broader
skos:broader rdf:type owl:AnnotationProperty .


###  http://www.w3.org/2004/02/skos/core#broaderTransitive
skos:broaderTransitive rdf:type owl:AnnotationProperty .


###  http://www.w3.org/2004/02/skos/core#closeMatch
skos:closeMatch rdf:type owl:AnnotationProperty .


###  http://www.w3.org/2004/02/skos/core#comment
skos:comment rdf:type owl:AnnotationProperty .


###  http://www.w3.org/2004/02/skos/core#example
skos:example rdf:type owl:AnnotationProperty .


###  http://www.w3.org/2004/02/skos/core#hasTopConcept
skos:hasTopConcept rdf:type owl:AnnotationProperty .


###  http://www.w3.org/2004/02/skos/core#inScheme
skos:inScheme rdf:type owl:AnnotationProperty .


###  http://www.w3.org/2004/02/skos/core#note
skos:note rdf:type owl:AnnotationProperty .


###  http://www.w3.org/2004/02/skos/core#prefLabel
skos:prefLabel rdf:type owl:AnnotationProperty .


###  http://www.w3.org/ns/odrl/2/action
odrl:action rdf:type owl:AnnotationProperty .


###  http://www.w3.org/ns/odrl/2/constraint
odrl:constraint rdf:type owl:AnnotationProperty .


###  http://www.w3.org/ns/odrl/2/duty
odrl:duty rdf:type owl:AnnotationProperty .


###  http://www.w3.org/ns/odrl/2/operator
odrl:operator rdf:type owl:AnnotationProperty .


###  http://www.w3.org/ns/odrl/2/permission
odrl:permission rdf:type owl:AnnotationProperty .


###  http://www.w3.org/ns/odrl/2/prohibition
odrl:prohibition rdf:type owl:AnnotationProperty .


###  http://www.w3.org/ns/odrl/2/recipient
odrl:recipient rdf:type owl:AnnotationProperty .


#################################################################
#    Datatypes
#################################################################

###  http://www.w3.org/1999/02/22-rdf-syntax-ns#langString
rdf:langString rdf:type rdfs:Datatype .


###  http://www.w3.org/2001/XMLSchema#date
xsd:date rdf:type rdfs:Datatype .


#################################################################
#    Object Properties
#################################################################

###  http://purl.org/dc/terms/license
dct:license rdf:type owl:ObjectProperty .


###  http://purl.org/dc/terms/publisher
dct:publisher rdf:type owl:ObjectProperty ;
              owl:equivalentProperty ms:resourceProvider .


###  http://purl.org/dc/terms/spatial
dct:spatial rdf:type owl:ObjectProperty ;
            rdfs:domain [ rdf:type owl:Class ;
                          owl:unionOf ( ms:Corpus
                                        ms:LanguageDescription
                                        ms:LexicalConceptualResource
                                        ms:Subset
                                      )
                        ] ;
            rdfs:range dct:Location ;
            rdfs:comment "Spatial characteristics of the resource"@en ;
            rdfs:label "spatial"@en .


###  http://purl.org/dc/terms/temporal
dct:temporal rdf:type owl:ObjectProperty ;
             rdfs:domain [ rdf:type owl:Class ;
                           owl:unionOf ( ms:Corpus
                                         ms:LanguageDescription
                                         ms:LexicalConceptualResource
                                         ms:Subset
                                       )
                         ] ;
             rdfs:range dct:PeriodOfTime ;
             rdfs:comment "Temporal characteristics of the resource"@en ;
             rdfs:label "temporal"@en .


###  http://purl.org/spar/datacite/hasIdentifier
datacite:hasIdentifier rdf:type owl:ObjectProperty ;
                       rdfs:domain owl:Thing ;
                       rdfs:range datacite:Identifier ;
                       rdfs:comment "Associates an entity to an identifier, i.e. a string used to uniquely identify it"@en ;
                       rdfs:label "has identifier"@en .


###  http://purl.org/spar/datacite/usesIdentifierScheme
datacite:usesIdentifierScheme rdf:type owl:ObjectProperty ;
                              rdfs:domain datacite:Identifier ;
                              rdfs:range datacite:IdentifierScheme ;
                              rdfs:comment "Indicates the scheme used to provide the identifier for an entity"@en ;
                              rdfs:label "uses identifier scheme"@en .


###  http://w3id.org/meta-share/meta-share/LTArea
ms:LTArea rdf:type owl:ObjectProperty ;
          rdfs:domain [ rdf:type owl:Class ;
                        owl:unionOf ( ms:Division
                                      ms:Document
                                      ms:Group
                                      ms:Organization
                                      ms:Person
                                      ms:Project
                                    )
                      ] ;
          rdfs:range [ owl:intersectionOf ( skos:Concept
                                            [ rdf:type owl:Restriction ;
                                              owl:onProperty skos:inScheme ;
                                              owl:hasValue omtd:OperationTypeScheme
                                            ]
                                          ) ;
                       rdf:type owl:Class
                     ] ;
          rdfs:comment "Introduces a Language Technology-related area associated with the activities or domain of interest of an entity"@en ;
          rdfs:label "LT area"@en ;
          skos:altLabel "Language Technology area"@en .


###  http://w3id.org/meta-share/meta-share/LΤRelatedTo
ms:LΤRelatedTo rdf:type owl:ObjectProperty ;
               rdfs:subPropertyOf ms:isRelatedTo ;
               owl:inverseOf ms:isRelatedToLT ;
               rdfs:domain ms:ToolService ;
               rdfs:range ms:DataLanguageResource ;
               rdfs:comment "Links a tool/service (the one being described) to a language resource that bears some relation to it"@en ;
               rdfs:label "LT tool/service related to"@en .


###  http://w3id.org/meta-share/meta-share/MDRecordRelatedTo
ms:MDRecordRelatedTo rdf:type owl:ObjectProperty ;
                     rdfs:subPropertyOf ms:isRelatedTo ;
                     owl:inverseOf ms:isRelatedToMDRecord ;
                     rdfs:domain ms:MetadataRecord ;
                     rdfs:range [ rdf:type owl:Class ;
                                  owl:unionOf ( ms:LanguageResource
                                                ms:MetadataRecord
                                              )
                                ] ;
                     rdfs:comment "Links an external metadata record that has some relation with the metadata record of the resource being described or the resource itself"@en ;
                     rdfs:label "metadata record related to"@en .


###  http://w3id.org/meta-share/meta-share/accessRights
ms:accessRights rdf:type owl:ObjectProperty ;
                rdfs:domain ms:Distribution ;
                rdfs:range ms:AccessRightsStatement ;
                rdfs:comment "Specifies the rights for accessing the distributable form(s) of a language resource (preferrably in accordance to a formalised vocabulary)"@en ;
                rdfs:label "access rights"@en .


###  http://w3id.org/meta-share/meta-share/accesses
ms:accesses rdf:type owl:ObjectProperty ;
            rdfs:subPropertyOf ms:LΤRelatedTo ;
            owl:inverseOf ms:isAccessedBy ;
            rdfs:domain ms:ToolService ;
            rdfs:range [ rdf:type owl:Class ;
                         owl:unionOf ( ms:DataLanguageResource
                                       ms:MediaPart
                                     )
                       ] ;
            rdfs:comment "Links a tool/service B that is (or can be) used for accessing LR A (e.g., a corpus workbench, s/w for lexicon access) to the LR A"@en ;
            rdfs:label "accesses"@en .


###  http://w3id.org/meta-share/meta-share/actorRelatedTo
ms:actorRelatedTo rdf:type owl:ObjectProperty ;
                  rdfs:subPropertyOf ms:isRelatedTo ;
                  owl:inverseOf ms:isRelatedToActor ;
                  rdfs:domain ms:Actor ;
                  rdfs:range ms:LanguageResource ;
                  rdfs:comment "Links actors to a language resource with which they have some relation"@en ;
                  rdfs:label "actor related to"@en .


###  http://w3id.org/meta-share/meta-share/actualUse
ms:actualUse rdf:type owl:ObjectProperty ;
             rdfs:domain ms:LanguageResource ;
             rdfs:range ms:ActualUse ;
             rdfs:comment "Provides information on how the resource has been used (e.g., in a project, for a publication, for testing a tool/service, etc.)"@en ;
             rdfs:label "actual use"@en .


###  http://w3id.org/meta-share/meta-share/addressSet
ms:addressSet rdf:type owl:ObjectProperty ;
              rdfs:domain [ rdf:type owl:Class ;
                            owl:unionOf ( ms:Affiliation
                                          ms:Division
                                          ms:Group
                                          ms:Organization
                                          ms:Person
                                        )
                          ] ;
              rdfs:range ms:AddressSet ;
              rdfs:comment "Links to the physical address of an organization, group or person represented as a set of distinct elements (street, number, zip code, city, etc.)"@en ;
              rdfs:label "address"@en .


###  http://w3id.org/meta-share/meta-share/affiliatedOrganization
ms:affiliatedOrganization rdf:type owl:ObjectProperty ;
                          rdfs:domain ms:Affiliation ;
                          rdfs:range ms:Organization ;
                          rdfs:comment "Specifies the organization that a person is affiliated with or works for"@en ;
                          rdfs:label "affiliated organization"@en .


###  http://w3id.org/meta-share/meta-share/affiliation
ms:affiliation rdf:type owl:ObjectProperty ;
               rdfs:domain ms:Person ;
               rdfs:range ms:Affiliation ;
               rdfs:comment "Introduces information on an organization to whom the person is affiliated and the data relevant to this relation (i.e. position, email, etc.)"@en ;
               rdfs:label "affiliation"@en .


###  http://w3id.org/meta-share/meta-share/ageGroup
ms:ageGroup rdf:type owl:ObjectProperty ;
            rdfs:domain ms:Participant ;
            rdfs:range ms:AgeGroup ;
            rdfs:comment "The age group to which the participant belongs"@en ;
            rdfs:label "age group"@en .


###  http://w3id.org/meta-share/meta-share/ageGroupOfParticipants
ms:ageGroupOfParticipants rdf:type owl:ObjectProperty ;
                          rdfs:domain [ rdf:type owl:Class ;
                                        owl:unionOf ( ms:CorpusAudioPart
                                                      ms:CorpusImagePart
                                                      ms:CorpusTextNumericalPart
                                                      ms:CorpusVideoPart
                                                    )
                                      ] ;
                          rdfs:range ms:AgeGroup ;
                          rdfs:comment "The age range of the group of participants"@en ;
                          rdfs:label "age group of participants"@en .


###  http://w3id.org/meta-share/meta-share/annotatedElement
ms:annotatedElement rdf:type owl:ObjectProperty ;
                    rdfs:domain ms:Annotation ;
                    rdfs:range ms:AnnotatedElement ;
                    rdfs:comment "Specifies the elements annotated at each annotation level"@en ;
                    rdfs:label "annotated element"@en .


###  http://w3id.org/meta-share/meta-share/annotation
ms:annotation rdf:type owl:ObjectProperty ;
              rdfs:domain ms:CorpusMediaPart ;
              rdfs:range ms:Annotation ;
              rdfs:comment "Links a corpus to its annotated part(s)"@en ;
              rdfs:label "annotation"@en .


###  http://w3id.org/meta-share/meta-share/annotationMode
ms:annotationMode rdf:type owl:ObjectProperty ;
                  rdfs:subPropertyOf ms:processMode ;
                  rdfs:domain ms:Annotation ;
                  rdfs:range ms:ProcessMode ;
                  rdfs:comment "Indicates whether the resource is annotated manually or by automatic processes"@en ;
                  rdfs:label "annotation mode"@en .


###  http://w3id.org/meta-share/meta-share/annotationReport
ms:annotationReport rdf:type owl:ObjectProperty ;
                    rdfs:subPropertyOf ms:isDocumentedBy ;
                    owl:inverseOf ms:documentsAnnotation ;
                    rdfs:domain ms:Annotation ;
                    rdfs:range ms:Document ;
                    rdfs:comment "Links to a report describing the annotation process, tool, method, etc. of the language resource"@en ;
                    rdfs:label "annotation report"@en .


###  http://w3id.org/meta-share/meta-share/annotationResource
ms:annotationResource rdf:type owl:ObjectProperty ;
                      rdfs:subPropertyOf ms:dependsOn ;
                      owl:inverseOf ms:isAnnotationResourceOf ;
                      rdfs:domain [ rdf:type owl:Class ;
                                    owl:unionOf ( ms:MLModel
                                                  ms:ProcessingResource
                                                  ms:ToolService
                                                )
                                  ] ;
                      rdfs:range ms:LexicalConceptualResource ;
                      rdfs:comment "Specifies the annotation resource used for annotating a corpus or that has been used for the input resource of a tool/service or that should be used (dependency) for the annotation"@en ;
                      rdfs:label "annotation resource"@en .


###  http://w3id.org/meta-share/meta-share/annotationSchema
ms:annotationSchema rdf:type owl:ObjectProperty ;
                    rdfs:subPropertyOf ms:dependsOn ;
                    owl:inverseOf ms:isAnnotationSchemaOf ;
                    rdfs:domain [ rdf:type owl:Class ;
                                  owl:unionOf ( ms:MLModel
                                                ms:ProcessingResource
                                                ms:ToolService
                                              )
                                ] ;
                    rdfs:range ms:LexicalConceptualResource ;
                    rdfs:comment "The annotation schema used for annotating a resource or for the input resource (if annotated) of a tool/service or that should be used (dependency) for the annotation"@en ;
                    rdfs:label "annotation schema"@en .


###  http://w3id.org/meta-share/meta-share/annotationType
ms:annotationType rdf:type owl:ObjectProperty ;
                  rdfs:domain ms:Annotation ;
                  rdfs:range [ owl:intersectionOf ( skos:Concept
                                                    [ rdf:type owl:Restriction ;
                                                      owl:onProperty skos:inScheme ;
                                                      owl:hasValue omtd:AnnotationTypeScheme
                                                    ]
                                                  ) ;
                               rdf:type owl:Class
                             ] ;
                  rdfs:comment "Specifies the annotation type of the annotated version(s) of a resource or the annotation type a tool/ service requires or produces as an output"@en ;
                  rdfs:label "annotation type"@en .


###  http://w3id.org/meta-share/meta-share/annotator
ms:annotator rdf:type owl:ObjectProperty ;
             rdfs:subPropertyOf ms:isRelatedToActor ;
             owl:inverseOf ms:isAnnotatorOf ;
             rdfs:domain ms:Annotation ;
             rdfs:range ms:Actor ;
             rdfs:comment "Identifies the person or organisation responsible for the annotation of a resource"@en ;
             rdfs:label "annotator"@en .


###  http://w3id.org/meta-share/meta-share/anonymized
ms:anonymized rdf:type owl:ObjectProperty ;
              rdfs:domain ms:DataLanguageResource ;
              rdfs:range ms:Anonymized ;
              rdfs:comment "Indicates whether the language resource has been anonymized"@en ;
              rdfs:label "anonymized"@en .


###  http://w3id.org/meta-share/meta-share/attributedAgent
ms:attributedAgent rdf:type owl:ObjectProperty ;
                   rdfs:subPropertyOf ms:isRelatedToActor ;
                   rdfs:domain ms:Attribution ;
                   rdfs:range ms:Actor ;
                   rdfs:comment "agent for attribution"@en ;
                   rdfs:label "attributed agent"@en .


###  http://w3id.org/meta-share/meta-share/audience
ms:audience rdf:type owl:ObjectProperty ;
            rdfs:domain [ rdf:type owl:Class ;
                          owl:unionOf ( ms:CorpusAudioPart
                                        ms:CorpusVideoPart
                                      )
                        ] ;
            rdfs:range ms:Audience ;
            rdfs:comment "Indicates the intended audience size of a multimedia resource"@en ;
            rdfs:label "audience"@en .


###  http://w3id.org/meta-share/meta-share/audioFormat
ms:audioFormat rdf:type owl:ObjectProperty ;
               rdfs:domain ms:DistributionAudioFeature ;
               rdfs:range ms:AudioFormat ;
               rdfs:comment "Specifies the features of the format of the audio part of a language resource"@en ;
               rdfs:label "detailed audio format"@en ;
               owl:deprecated ""@en .


###  http://w3id.org/meta-share/meta-share/audioQualityMeasureIncluded
ms:audioQualityMeasureIncluded rdf:type owl:ObjectProperty ;
                               rdfs:domain ms:AudioFormat ;
                               rdfs:range ms:AudioQualityMeasureIncluded ;
                               rdfs:comment "Specifies the audio quality measures"@en ;
                               rdfs:label "audio quality measure included"@en .


###  http://w3id.org/meta-share/meta-share/author
ms:author rdf:type owl:ObjectProperty ;
          rdfs:domain ms:Document ;
          rdfs:range ms:Person ;
          rdfs:comment "Introduces the details for a person that has created the document being described"@en ;
          rdfs:label "author"@en .


###  http://w3id.org/meta-share/meta-share/availability
ms:availability rdf:type owl:ObjectProperty ;
                rdfs:domain ms:Distribution ;
                rdfs:range ms:Availability ;
                rdfs:comment "Specifies the availability status of the resource"@en ;
                rdfs:label "availability"@en .


###  http://w3id.org/meta-share/meta-share/baseItem
ms:baseItem rdf:type owl:ObjectProperty ;
            rdfs:domain ms:NGramModel ;
            rdfs:range ms:BaseItem ;
            rdfs:comment "Type of item that is represented in the n-gram resource"@en ;
            rdfs:label "base item"@en .


###  http://w3id.org/meta-share/meta-share/bodyPart
ms:bodyPart rdf:type owl:ObjectProperty ;
            rdfs:domain [ rdf:type owl:Class ;
                          owl:unionOf ( ms:DynamicElement
                                        ms:StaticElement
                                      )
                        ] ;
            rdfs:range ms:BodyPart ;
            rdfs:comment "Specifies the body parts visible in the video or image part of the resource"@en ;
            rdfs:label "body part"@en .


###  http://w3id.org/meta-share/meta-share/byteOrder
ms:byteOrder rdf:type owl:ObjectProperty ;
             rdfs:domain ms:AudioFormat ;
             rdfs:range ms:ByteOrder ;
             rdfs:comment "Specifies the byte order of 2 or more bytes sample"@en ;
             rdfs:label "byte order"@en .


###  http://w3id.org/meta-share/meta-share/capturingDeviceType
ms:capturingDeviceType rdf:type owl:ObjectProperty ;
                       rdfs:domain [ rdf:type owl:Class ;
                                     owl:unionOf ( ms:CorpusAudioPart
                                                   ms:CorpusImagePart
                                                   ms:CorpusTextNumericalPart
                                                   ms:CorpusVideoPart
                                                 )
                                   ] ;
                       rdfs:range ms:CapturingDeviceType ;
                       rdfs:comment "Provides information on the type of the transducers through which the data is captured"@en ;
                       rdfs:label "capturing device type"@en .


###  http://w3id.org/meta-share/meta-share/capturingEnvironment
ms:capturingEnvironment rdf:type owl:ObjectProperty ;
                        rdfs:domain [ rdf:type owl:Class ;
                                      owl:unionOf ( ms:CorpusAudioPart
                                                    ms:CorpusImagePart
                                                    ms:CorpusTextNumericalPart
                                                    ms:CorpusVideoPart
                                                  )
                                    ] ;
                        rdfs:range ms:CapturingEnvironment ;
                        rdfs:comment "Specifies the type of the capturing environment"@en ;
                        rdfs:label "capturing environment"@en .


###  http://w3id.org/meta-share/meta-share/characterEncoding
ms:characterEncoding rdf:type owl:ObjectProperty ;
                     rdfs:domain ms:DistributionTextFeature ;
                     rdfs:range ms:CharacterEncoding ;
                     rdfs:comment "Specifies the character encoding used for a language resource data distribution"@en ;
                     rdfs:label "character encoding"@en .


###  http://w3id.org/meta-share/meta-share/cites
ms:cites rdf:type owl:ObjectProperty ;
         rdfs:subPropertyOf ms:documentRelatedTo ;
         owl:inverseOf ms:isCitedBy ;
         rdfs:domain ms:Document ;
         rdfs:range ms:LanguageResource ;
         rdfs:comment "Links to the language resource(s) that a publication includes in its citations"@en ;
         rdfs:label "cites"@en .


###  http://w3id.org/meta-share/meta-share/colourSpace
ms:colourSpace rdf:type owl:ObjectProperty ;
               rdfs:domain [ rdf:type owl:Class ;
                             owl:unionOf ( ms:ImageFormat
                                           ms:VideoFormat
                                         )
                           ] ;
               rdfs:range ms:ColourSpace ;
               rdfs:comment "Defines the colour space for the video"@en ;
               rdfs:label "colour space"@en .


###  http://w3id.org/meta-share/meta-share/compatibleLexiconType
ms:compatibleLexiconType rdf:type owl:ObjectProperty ;
                         rdfs:domain ms:LanguageDescription ;
                         rdfs:range ms:CompatibleLexiconType ;
                         rdfs:comment "Specifies the type of (external) lexicon that can be used with the grammar"@en ;
                         rdfs:label "compatible lexicon type"@en .


###  http://w3id.org/meta-share/meta-share/compliesWith
ms:compliesWith rdf:type owl:ObjectProperty ;
                rdfs:domain [ rdf:type owl:Class ;
                              owl:unionOf ( ms:LanguageResource
                                            ms:MetadataRecord
                                          )
                            ] ;
                rdfs:range ms:StandardBestPractice ;
                rdfs:comment "Specifies the vocabulary/standard/best practice to which a resource is compliant with"@en ;
                rdfs:label "complies with"@en .


###  http://w3id.org/meta-share/meta-share/compressionName
ms:compressionName rdf:type owl:ObjectProperty ;
                   rdfs:domain [ rdf:type owl:Class ;
                                 owl:unionOf ( ms:AudioFormat
                                               ms:ImageFormat
                                               ms:VideoFormat
                                             )
                               ] ;
                   rdfs:range ms:CompressionName ;
                   rdfs:comment "The name of the compression applied"@en ;
                   rdfs:label "compression name"@en .


###  http://w3id.org/meta-share/meta-share/conditionOfUse
ms:conditionOfUse rdf:type owl:ObjectProperty ;
                  rdfs:domain ms:LicenceTerms ;
                  rdfs:range ms:ConditionOfUse ;
                  rdfs:comment "Links a licence with a specific condition/term of use imposed for accessing a language resource. It is an optional element and only to be taken as providing brief human readable information on the fact that the language resource is provided under a specific set of conditions. These correspond to the most frequently used conditions imposed by the licensor (via the specified licence). The proper exposition of all conditions and possible exceptions is to be found inside the licence text. Depositors should, hence, carefully choose the values of this field to match the licence chosen and users should carefully read that licence before using the language resource."@en ;
                  rdfs:label "condition of use"@en .


###  http://w3id.org/meta-share/meta-share/conformsTo
ms:conformsTo rdf:type owl:ObjectProperty ;
              rdfs:domain ms:Classification ;
              rdfs:range ms:ClassificationScheme ;
              rdfs:comment "Specifies the vocabulary/scheme to which a value (e.g., as of text genre, domain, etc.) conforms to"@en ;
              rdfs:label "conforms to"@en .


###  http://w3id.org/meta-share/meta-share/contact
ms:contact rdf:type owl:ObjectProperty ;
           rdfs:subPropertyOf ms:isRelatedToActor ;
           owl:inverseOf ms:isContactFor ;
           rdfs:domain ms:LanguageResource ;
           rdfs:range ms:Actor ;
           rdfs:comment "Specifies the data of the person/organization/group that can be contacted for information about a language resource"@en ;
           rdfs:label "contact"@en .


###  http://w3id.org/meta-share/meta-share/contributor
ms:contributor rdf:type owl:ObjectProperty ;
               rdfs:domain ms:Document ;
               rdfs:range ms:Person ;
               rdfs:comment "Introduces the details for a person that has contributed in some way to the production of a document or resource"@en ;
               rdfs:label "contributor"@en .


###  http://w3id.org/meta-share/meta-share/conversationalType
ms:conversationalType rdf:type owl:ObjectProperty ;
                      rdfs:domain [ rdf:type owl:Class ;
                                    owl:unionOf ( ms:CorpusAudioPart
                                                  ms:CorpusVideoPart
                                                )
                                  ] ;
                      rdfs:range ms:ConversationalType ;
                      rdfs:comment "Specifies the conversational type of a multimedia resource"@en ;
                      rdfs:label "conversational type"@en .


###  http://w3id.org/meta-share/meta-share/coordinator
ms:coordinator rdf:type owl:ObjectProperty ;
               rdfs:subPropertyOf ms:isRelatedToActor ;
               owl:inverseOf ms:isCoordinatorOf ;
               rdfs:domain ms:Project ;
               rdfs:range ms:Organization ;
               rdfs:comment "Introduces the organization that coordinates the project being described"@en ;
               rdfs:label "coordinator"@en ;
               skos:altLabel "co-ordinator"@en .


###  http://w3id.org/meta-share/meta-share/corpusSubclass
ms:corpusSubclass rdf:type owl:ObjectProperty ;
                  rdfs:domain ms:Corpus ;
                  rdfs:range ms:CorpusSubclass ;
                  rdfs:comment "Introduces a classification of corpora into types (used for descriptive reasons)"@en ;
                  rdfs:label "corpus subclass"@en .


###  http://w3id.org/meta-share/meta-share/cost
ms:cost rdf:type owl:ObjectProperty ;
        rdfs:domain [ rdf:type owl:Class ;
                      owl:unionOf ( ms:Distribution
                                    ms:Project
                                  )
                    ] ;
        rdfs:range ms:Cost ;
        rdfs:comment "Introduces the cost for accessing a resource or the overall budget of a project, formally described as a set of amount and currency unit"@en ;
        rdfs:label "cost"@en .


###  http://w3id.org/meta-share/meta-share/country
ms:country rdf:type owl:ObjectProperty ;
           rdfs:domain ms:AddressSet ;
           rdfs:range ms:Country ;
           rdfs:comment "Introduces the name of the country mentioned in the postal address of a person or organization as defined in the list of values of ISO 3166"@en ;
           rdfs:label "country"@en .


###  http://w3id.org/meta-share/meta-share/countryOfRegistration
ms:countryOfRegistration rdf:type owl:ObjectProperty ;
                         rdfs:domain [ rdf:type owl:Class ;
                                       owl:unionOf ( ms:Division
                                                     ms:Organization
                                                   )
                                     ] ;
                         rdfs:range ms:Country ;
                         rdfs:comment "Introduces the country in which an organization was officially registered for the first time as a legal entity"@en ;
                         rdfs:label "country of registration"@en .


###  http://w3id.org/meta-share/meta-share/creationMode
ms:creationMode rdf:type owl:ObjectProperty ;
                rdfs:subPropertyOf ms:processMode ;
                rdfs:domain [ rdf:type owl:Class ;
                              owl:unionOf ( ms:LexicalConceptualResource
                                            ms:MediaPart
                                          )
                            ] ;
                rdfs:range ms:ProcessMode ;
                rdfs:comment "Specifies whether the resource was created automatically or in a manual or interactive mode"@en ;
                rdfs:label "creation mode"@en .


###  http://w3id.org/meta-share/meta-share/currency
ms:currency rdf:type owl:ObjectProperty ;
            rdfs:domain ms:Cost ;
            rdfs:range ms:Currency ;
            rdfs:comment "Specifies the currency used for describing the cost of a resource"@en ;
            rdfs:label "currency"@en .


###  http://w3id.org/meta-share/meta-share/dataFormat
ms:dataFormat rdf:type owl:ObjectProperty ;
              rdfs:domain [ rdf:type owl:Class ;
                            owl:unionOf ( ms:AudioFormat
                                          ms:ImageFormat
                                          ms:Parameter
                                          ms:VideoFormat
                                        )
                          ] ;
              rdfs:range [ owl:intersectionOf ( skos:Concept
                                                [ rdf:type owl:Restriction ;
                                                  owl:onProperty skos:inScheme ;
                                                  owl:hasValue omtd:DataFormatScheme
                                                ]
                                              ) ;
                           rdf:type owl:Class
                         ] ;
              rdfs:comment "Indicates the format(s) of a data resource"@en ;
              rdfs:label "data format"@en .


###  http://w3id.org/meta-share/meta-share/dependentLR
ms:dependentLR rdf:type owl:ObjectProperty ;
               rdfs:subPropertyOf ms:isRelatedToLR ;
               owl:inverseOf ms:dependsOn ;
               rdfs:domain ms:LanguageResource ;
               rdfs:range ms:LanguageResource ;
               rdfs:comment "Links to LR B that requires LR A (the one being described) for its operation or that has been processed with LR A"@en ;
               rdfs:label "dependent language resource"@en .


###  http://w3id.org/meta-share/meta-share/dependsOn
ms:dependsOn rdf:type owl:ObjectProperty ;
             rdfs:subPropertyOf ms:isRelatedToLR ;
             rdf:type owl:SymmetricProperty ;
             rdfs:domain ms:LanguageResource ;
             rdfs:range ms:LanguageResource ;
             rdfs:comment "Links to LR B that is required for the operation of LR A (the one being described) or that has been used in its processing"@en ;
             rdfs:label "depends on"@en ;
             skos:altLabel "supporting resource"@en .


###  http://w3id.org/meta-share/meta-share/depositingParty
ms:depositingParty rdf:type owl:ObjectProperty ;
                   rdfs:subPropertyOf odrl:function ;
                   rdfs:domain ms:Organization ;
                   rdfs:range ms:LanguageResource ;
                   rdfs:label "depositing party"@en ;
                   skos:comment "An entity where one can deposit (upload) a resource"@en .


###  http://w3id.org/meta-share/meta-share/describedEntity
ms:describedEntity rdf:type owl:ObjectProperty ;
                   rdfs:domain ms:MetadataRecord ;
                   rdfs:range ms:DescribedEntity ;
                   rdfs:comment "Links to the entity that is being described by a metadata record"@en ;
                   rdfs:label "type of described entity"@en ;
                   skos:note "foaf:primaryTopic in DCAT"@en .


###  http://w3id.org/meta-share/meta-share/describes
ms:describes rdf:type owl:ObjectProperty ;
             rdfs:subPropertyOf ms:documents ;
             owl:inverseOf ms:isDescribedBy ;
             rdfs:domain ms:Document ;
             rdfs:range ms:LanguageResource ;
             rdfs:comment "Links to the language resource(s) that are described (contents, operation, etc.) in a document"@en ;
             rdfs:label "describes"@en .


###  http://w3id.org/meta-share/meta-share/developmentFramework
ms:developmentFramework rdf:type owl:ObjectProperty ;
                        rdfs:domain [ rdf:type owl:Class ;
                                      owl:unionOf ( ms:MLModel
                                                    ms:ToolService
                                                  )
                                    ] ;
                        rdfs:range ms:DevelopmentFramework ;
                        rdfs:comment "Introduces a framework used in the development of the resource"@en ;
                        rdfs:label "development framework"@en .


###  http://w3id.org/meta-share/meta-share/displays
ms:displays rdf:type owl:ObjectProperty ;
            rdfs:subPropertyOf ms:LΤRelatedTo ;
            owl:inverseOf ms:isDisplayedBy ;
            rdfs:domain ms:ToolService ;
            rdfs:range [ rdf:type owl:Class ;
                         owl:unionOf ( ms:DataLanguageResource
                                       ms:MediaPart
                                     )
                       ] ;
            rdfs:comment "Links a tool/service B that is (or can be) used to display LR A (e.g., a tool for visualizing relations in a lexicon, or annotations in a corpus) to the LR A"@en ;
            rdfs:label "displays"@en ;
            skos:altLabel "visualises"@en ,
                          "visualizes"@en .


###  http://w3id.org/meta-share/meta-share/distribution
ms:distribution rdf:type owl:ObjectProperty ;
                rdfs:domain ms:LanguageResource ;
                rdfs:range ms:Distribution ;
                rdfs:comment "Links a language resource to the various forms with which it is distributed"@en ;
                rdfs:label "distribution"@en ;
                skos:closeMatch <dcat:distribution> .


###  http://w3id.org/meta-share/meta-share/distributionAudioFeature
ms:distributionAudioFeature rdf:type owl:ObjectProperty ;
                            rdfs:domain ms:DatasetDistribution ;
                            rdfs:range ms:DistributionAudioFeature ;
                            rdfs:comment "Links to a feature that can be used for describing distinct distributable forms of audio resources/parts"@en ;
                            rdfs:label "audio feature"@en ;
                            owl:deprecated "" .


###  http://w3id.org/meta-share/meta-share/distributionFeature
ms:distributionFeature rdf:type owl:ObjectProperty ;
                       rdfs:domain ms:DatasetDistribution ;
                       rdfs:range [ rdf:type owl:Class ;
                                    owl:unionOf ( ms:DistributionAudioFeature
                                                  ms:DistributionImageFeature
                                                  ms:DistributionTextFeature
                                                  ms:DistributionTextNumericalFeature
                                                  ms:DistributionVideoFeature
                                                )
                                  ] ;
                       rdfs:label "distribution feature"@en ;
                       owl:backwardCompatibleWith "Links to a set of features that can be used for describing distinct distributable forms of resources/parts"@en .


###  http://w3id.org/meta-share/meta-share/distributionForm
ms:distributionForm rdf:type owl:ObjectProperty ;
                    rdfs:domain ms:Distribution ;
                    rdfs:range ms:DistributionForm ;
                    rdfs:comment "Specifies the form (medium/channel) with which a resource is distributed (delivered or provided access to)"@en ;
                    rdfs:label "distribution form"@en .


###  http://w3id.org/meta-share/meta-share/distributionImageFeature
ms:distributionImageFeature rdf:type owl:ObjectProperty ;
                            rdfs:domain ms:DatasetDistribution ;
                            rdfs:range ms:DistributionImageFeature ;
                            rdfs:comment "Links to a feature that can be used for describing distinct distributable forms of image resources/parts"@en ;
                            rdfs:label "image feature"@en ;
                            owl:deprecated "" .


###  http://w3id.org/meta-share/meta-share/distributionRightsHolder
ms:distributionRightsHolder rdf:type owl:ObjectProperty ;
                            rdfs:subPropertyOf ms:isRelatedToActor ;
                            owl:inverseOf ms:isDistributionRightsHolderOf ;
                            rdfs:domain ms:Distribution ;
                            rdfs:range ms:Actor ;
                            rdfs:comment "Identifies a person or an organization that holds the distribution rights. The range and scope of distribution rights is defined in the distribution agreement. The distributor in most cases only has a limited licence to distribute the work and collect royalties on behalf of the licensor or the IPR holder and cannot give to any recipient of the work permissions that exceed the scope of the distribution agreement (e.g., to allow uses of the work that are not defined in the distribution agreement)"@en ;
                            rdfs:label "distribution rights holder"@en .


###  http://w3id.org/meta-share/meta-share/distributionTextFeature
ms:distributionTextFeature rdf:type owl:ObjectProperty ;
                           rdfs:label "distribution text feature"@en ;
                           owl:deprecated "" .


###  http://w3id.org/meta-share/meta-share/distributionTextNumericalFeature
ms:distributionTextNumericalFeature rdf:type owl:ObjectProperty ;
                                    rdfs:domain ms:DatasetDistribution ;
                                    rdfs:range ms:DistributionTextNumericalFeature ;
                                    rdfs:comment "Links to a feature that can be used for describing distinct distributable forms of numerical text resources/parts"@en ;
                                    rdfs:label "numerical text feature"@en ;
                                    owl:deprecated "" .


###  http://w3id.org/meta-share/meta-share/distributionVideoFeature
ms:distributionVideoFeature rdf:type owl:ObjectProperty ;
                            rdfs:domain ms:DatasetDistribution ;
                            rdfs:range ms:DistributionVideoFeature ;
                            rdfs:comment "Links to a feature that can be used for describing distinct distributable forms of video resources/parts"@en ;
                            rdfs:label "video feature"@en ;
                            owl:deprecated "" .


###  http://w3id.org/meta-share/meta-share/divisionCategory
ms:divisionCategory rdf:type owl:ObjectProperty ;
                    rdfs:subPropertyOf ms:durationOfAudio ;
                    rdfs:domain ms:Division ;
                    rdfs:range ms:DivisionCategory ;
                    rdfs:comment "Classifies the division of an organization according to a controlled vocabulary"@en ;
                    rdfs:label "division category"@en .


###  http://w3id.org/meta-share/meta-share/documentRelatedTo
ms:documentRelatedTo rdf:type owl:ObjectProperty ;
                     rdfs:subPropertyOf ms:isRelatedTo ;
                     owl:inverseOf ms:isRelatedToDocument ;
                     rdfs:domain ms:Document ;
                     rdfs:range [ rdf:type owl:Class ;
                                  owl:unionOf ( ms:LanguageResource
                                                ms:Project
                                              )
                                ] ;
                     rdfs:comment "Links to the entity (language resource, project, part of a language resource) that is somehow related to the document that is described"@en ;
                     rdfs:label "document related to"@en .


###  http://w3id.org/meta-share/meta-share/documentType
ms:documentType rdf:type owl:ObjectProperty ;
                rdfs:domain ms:Document ;
                rdfs:range ms:DocumentType ;
                rdfs:comment "Specifies the type of the document (e.g., article, book, etc.) provided with or related to the language resource"@en ;
                rdfs:label "document type"@en .


###  http://w3id.org/meta-share/meta-share/documentationType
ms:documentationType rdf:type owl:ObjectProperty ;
                     rdfs:domain ms:Document ;
                     rdfs:range ms:DocumentationType ;
                     rdfs:comment "Classifies the documentation vis-a-vis its relation with the language resource (e.g., general publication, user manual, url for online help, etc.)"@en ;
                     rdfs:label "documentation type"@en .


###  http://w3id.org/meta-share/meta-share/documents
ms:documents rdf:type owl:ObjectProperty ;
             rdfs:subPropertyOf ms:documentRelatedTo ;
             owl:inverseOf ms:isDocumentedBy ;
             rdfs:domain ms:Document ;
             rdfs:range ms:LanguageResource ;
             rdfs:comment "Links a document to a language resource (e.g., research paper describing its contents or its use in a project, user manual, etc.)"@en ;
             rdfs:label "documents"@en .


###  http://w3id.org/meta-share/meta-share/documentsAnnotation
ms:documentsAnnotation rdf:type owl:ObjectProperty ;
                       rdfs:subPropertyOf ms:documents ;
                       rdfs:domain ms:Document ;
                       rdfs:range ms:Annotation ;
                       rdfs:comment "Links a report to the annotation process, tool, method, etc. of a language resource that it describes"@en ;
                       rdfs:label "documents annotation"@en .


###  http://w3id.org/meta-share/meta-share/documentsEvaluation
ms:documentsEvaluation rdf:type owl:ObjectProperty ;
                       rdfs:subPropertyOf ms:documents ;
                       owl:inverseOf ms:evaluationReport ;
                       rdfs:domain ms:Document ;
                       rdfs:range ms:Evaluation ;
                       rdfs:comment "Links a report to the evaluation process, tool, method, etc. of the tool or service it purports to describe"@en ;
                       rdfs:label "documents evaluation"@en .


###  http://w3id.org/meta-share/meta-share/documentsGuidelines
ms:documentsGuidelines rdf:type owl:ObjectProperty ;
                       rdfs:subPropertyOf ms:documents ;
                       owl:inverseOf ms:guidelines ;
                       rdfs:domain ms:Document ;
                       rdfs:range [ rdf:type owl:Class ;
                                    owl:unionOf ( ms:Annotation
                                                  ms:LanguageResource
                                                )
                                  ] ;
                       rdfs:comment "Links the guidelines used for the creation or annotation of a language resource to this language resource"@en ;
                       rdfs:label "documents guidelines"@en .


###  http://w3id.org/meta-share/meta-share/documentsUsage
ms:documentsUsage rdf:type owl:ObjectProperty ;
                  rdfs:subPropertyOf ms:documents ;
                  owl:inverseOf ms:usageReport ;
                  rdfs:domain ms:Document ;
                  rdfs:range ms:ActualUse ;
                  rdfs:comment "Links a document (e.g., research article, report) describing the use of a language resource (e.g., in a project, application, experiment or use case) to the data of this use"@en ;
                  rdfs:label "documents usage"@en .


###  http://w3id.org/meta-share/meta-share/documentsValidation
ms:documentsValidation rdf:type owl:ObjectProperty ;
                       rdfs:subPropertyOf ms:documents ;
                       owl:inverseOf ms:validationReport ;
                       rdfs:domain ms:Document ;
                       rdfs:range ms:Validation ;
                       rdfs:comment "Links a document with detailed information on the validation process and results to the data of this validation"@en ;
                       rdfs:label "documents validation"@en .


###  http://w3id.org/meta-share/meta-share/domain
ms:domain rdf:type owl:ObjectProperty ;
          rdfs:domain [ rdf:type owl:Class ;
                        owl:unionOf ( ms:Actor
                                      ms:Division
                                      ms:Document
                                      ms:LanguageResource
                                      ms:ProcessingResource
                                      ms:Project
                                    )
                      ] ;
          rdfs:range ms:Domain ;
          rdfs:comment "Identifies the domain according to which an entity is classified"@en ;
          rdfs:label "domain"@en .


###  http://w3id.org/meta-share/meta-share/durationOfAudio
ms:durationOfAudio rdf:type owl:ObjectProperty ;
                   rdfs:domain ms:DistributionAudioFeature ;
                   rdfs:range ms:Duration ;
                   rdfs:comment "Specifies the duration of the audio recording including silences, music, pauses, etc."@en ;
                   rdfs:label "duration of audio"@en .


###  http://w3id.org/meta-share/meta-share/durationOfEffectiveSpeech
ms:durationOfEffectiveSpeech rdf:type owl:ObjectProperty ;
                             rdfs:domain ms:DistributionAudioFeature ;
                             rdfs:range ms:Duration ;
                             rdfs:comment "Specifies the duration of effective speech of the audio (part of a) resource"@en ;
                             rdfs:label "duration of effective speech"@en .


###  http://w3id.org/meta-share/meta-share/durationUnit
ms:durationUnit rdf:type owl:ObjectProperty ;
                rdfs:domain ms:Duration ;
                rdfs:range ms:DurationUnit ;
                rdfs:comment "Specifies the unit used for measuring the duration of a resource"@en ;
                rdfs:label "duration unit"@en .


###  http://w3id.org/meta-share/meta-share/dynamicElement
ms:dynamicElement rdf:type owl:ObjectProperty ;
                  rdfs:domain [ rdf:type owl:Class ;
                                owl:unionOf ( ms:CorpusVideoPart
                                              ms:LanguageDescriptionVideoPart
                                              ms:LexicalConceptualResourceVideoPart
                                            )
                              ] ;
                  rdfs:range ms:DynamicElement ;
                  rdfs:comment "Groups information on the dynamic elements that are represented in the video part of the resource"@en ;
                  rdfs:label "dynamic element"@en ;
                  skos:note "it was like this in MS-OWL v1, although it's not multiple; helps to organise the elements though"@en .


###  http://w3id.org/meta-share/meta-share/ecMaxContribution
ms:ecMaxContribution rdf:type owl:ObjectProperty ;
                     rdfs:domain ms:Project ;
                     rdfs:range ms:Cost ;
                     rdfs:comment "Introduces the maximum amount of money contributed from EC funds"@en ;
                     rdfs:label "EC max contribution"@en .


###  http://w3id.org/meta-share/meta-share/editor
ms:editor rdf:type owl:ObjectProperty ;
          rdfs:domain ms:Document ;
          rdfs:range ms:Person ;
          rdfs:comment "Introduces the details for a person that has edited the document being described"@en ;
          rdfs:label "editor"@en .


###  http://w3id.org/meta-share/meta-share/edits
ms:edits rdf:type owl:ObjectProperty ;
         rdfs:subPropertyOf ms:LΤRelatedTo ;
         owl:inverseOf ms:isEditedBy ;
         rdfs:domain ms:ToolService ;
         rdfs:range [ rdf:type owl:Class ;
                      owl:unionOf ( ms:DataLanguageResource
                                    ms:MediaPart
                                  )
                    ] ;
         rdfs:comment "Links a tool/service B that is (or can be) used for editing LR A (the one being described) to LR A"@en ;
         rdfs:label "edits"@en .


###  http://w3id.org/meta-share/meta-share/encodingLevel
ms:encodingLevel rdf:type owl:ObjectProperty ;
                 rdfs:domain [ rdf:type owl:Class ;
                               owl:unionOf ( ms:LanguageDescription
                                             ms:LexicalConceptualResource
                                           )
                             ] ;
                 rdfs:range ms:EncodingLevel ;
                 rdfs:comment "Classifies the contents of a lexical/conceptual resource or language description as regards the linguistic level of analysis it caters for"@en ;
                 rdfs:label "encoding level" .


###  http://w3id.org/meta-share/meta-share/enumerationValue
ms:enumerationValue rdf:type owl:ObjectProperty ;
                    rdfs:domain ms:Parameter ;
                    rdfs:range ms:EnumerationValue ;
                    rdfs:comment "Introduces a value of a list used inside parameters"@en ;
                    rdfs:label "enumeration value"@en .


###  http://w3id.org/meta-share/meta-share/evaluation
ms:evaluation rdf:type owl:ObjectProperty ;
              rdfs:domain ms:ToolService ;
              rdfs:range ms:Evaluation ;
              rdfs:comment "Provides information on the evaluation process and results for a tool/service"@en ;
              rdfs:label "evaluation"@en .


###  http://w3id.org/meta-share/meta-share/evaluationCriterion
ms:evaluationCriterion rdf:type owl:ObjectProperty ;
                       rdfs:domain ms:Evaluation ;
                       rdfs:range ms:EvaluationCriterion ;
                       rdfs:comment "Defines the criterion(s) of the evaluation of a tool"@en ;
                       rdfs:label "evaluation criterion"@en .


###  http://w3id.org/meta-share/meta-share/evaluationLevel
ms:evaluationLevel rdf:type owl:ObjectProperty ;
                   rdfs:domain ms:Evaluation ;
                   rdfs:range ms:EvaluationLevel ;
                   rdfs:comment "Indicates the evaluation level"@en ;
                   rdfs:label "evaluation level"@en .


###  http://w3id.org/meta-share/meta-share/evaluationMeasure
ms:evaluationMeasure rdf:type owl:ObjectProperty ;
                     rdfs:domain ms:Evaluation ;
                     rdfs:range ms:EvaluationMeasure ;
                     rdfs:comment "Defines whether the evaluation measure is human or automatic"@en ;
                     rdfs:label "evaluation measure"@en .


###  http://w3id.org/meta-share/meta-share/evaluationReport
ms:evaluationReport rdf:type owl:ObjectProperty ;
                    rdfs:subPropertyOf ms:isDocumentedBy ;
                    rdfs:domain ms:Evaluation ;
                    rdfs:range ms:Document ;
                    rdfs:comment "Links to a report describing the evaluation process, tool, method, etc. of the tool or service"@en ;
                    rdfs:label "evaluation report"@en .


###  http://w3id.org/meta-share/meta-share/evaluationType
ms:evaluationType rdf:type owl:ObjectProperty ;
                  rdfs:domain ms:Evaluation ;
                  rdfs:range ms:EvaluationType ;
                  rdfs:comment "Indicates the evaluation type"@en ;
                  rdfs:label "evaluation type"@en .


###  http://w3id.org/meta-share/meta-share/evaluator
ms:evaluator rdf:type owl:ObjectProperty ;
             rdfs:subPropertyOf ms:isRelatedToActor ;
             owl:inverseOf ms:isEvaluatorOf ;
             rdfs:domain ms:Evaluation ;
             rdfs:range ms:Actor ;
             rdfs:comment "Describes the person or organization that evaluated the tool or service"@en ;
             rdfs:label "evaluator"@en .


###  http://w3id.org/meta-share/meta-share/externalReference
ms:externalReference rdf:type owl:ObjectProperty ;
                     rdfs:domain ms:LexicalConceptualResource ;
                     rdfs:range ms:LexicalConceptualResource ;
                     rdfs:comment "Provides reference to another resource to which the lexicalConceptualResource is linked (e.g., link to a wordnet or ontology)"@en ;
                     rdfs:label "external reference"@en .


###  http://w3id.org/meta-share/meta-share/extratextualInformation
ms:extratextualInformation rdf:type owl:ObjectProperty ;
                           rdfs:domain ms:LexicalConceptualResource ;
                           rdfs:range ms:ExtratextualInformation ;
                           rdfs:comment "Indicates the extratextual information contained in a lexical/conceptual resource; it can be used as an alternative to the representation of the audio, image, video, etc. part(s) of the resource when these are not considered important enough to fully describe"@en ;
                           rdfs:label "extratextual information"@en .


###  http://w3id.org/meta-share/meta-share/extratextualInformationUnit
ms:extratextualInformationUnit rdf:type owl:ObjectProperty ;
                               rdfs:domain ms:LexicalConceptualResource ;
                               rdfs:range ms:ExtratextualInformationUnit ;
                               rdfs:comment "Indicates the unit on which the extratextual information is attached to in the lexical conceptual resource"@en ;
                               rdfs:label "extratextual information unit"@en .


###  http://w3id.org/meta-share/meta-share/format
ms:format rdf:type owl:ObjectProperty ;
          rdfs:domain [ rdf:type owl:Class ;
                        owl:unionOf ( ms:DistributionAudioFeature
                                      ms:DistributionImageFeature
                                      ms:DistributionTextFeature
                                      ms:DistributionTextNumericalFeature
                                      ms:DistributionVideoFeature
                                    )
                      ] ;
          rdfs:range [ rdf:type owl:Class ;
                       owl:unionOf ( ms:AudioFormat
                                     ms:ImageFormat
                                     ms:VideoFormat
                                     omtd:DataFormat
                                   )
                     ] ;
          rdfs:comment "Indicates the format of a resource or resource part"@en ;
          rdfs:label "format"@en .


###  http://w3id.org/meta-share/meta-share/framework
ms:framework rdf:type owl:ObjectProperty ;
             rdfs:domain ms:ToolService ;
             rdfs:range ms:Framework ;
             rdfs:comment "Specifies the implementation framework used for developing and running a tool/service"@en ;
             rdfs:label "wrapping framework"@en .


###  http://w3id.org/meta-share/meta-share/function
ms:function rdf:type owl:ObjectProperty ;
            rdfs:domain ms:ToolService ;
            rdfs:range [ owl:intersectionOf ( skos:Concept
                                              [ rdf:type owl:Restriction ;
                                                owl:onProperty skos:inScheme ;
                                                owl:hasValue omtd:OperationScheme
                                              ]
                                            ) ;
                         rdf:type owl:Class
                       ] ;
            rdfs:comment "Specifies the operation/function/task that a software object performs"@en ;
            rdfs:label "function"@en ;
            skos:altLabel "operation" ,
                          "task" .


###  http://w3id.org/meta-share/meta-share/funder
ms:funder rdf:type owl:ObjectProperty ;
          rdfs:subPropertyOf ms:isRelatedToActor ;
          owl:inverseOf ms:isFunderOf ;
          rdfs:domain ms:Project ;
          rdfs:range ms:Actor ;
          rdfs:comment "Identifies the person or organization or group that has financed the project"@en ;
          rdfs:label "funder"@en .


###  http://w3id.org/meta-share/meta-share/fundingCountry
ms:fundingCountry rdf:type owl:ObjectProperty ;
                  rdfs:domain ms:Project ;
                  rdfs:range ms:Country ;
                  rdfs:comment "Specifies the name of the funding country, in case of national funding as mentioned in ISO3166"@en ;
                  rdfs:label "funding country"@en .


###  http://w3id.org/meta-share/meta-share/fundingProject
ms:fundingProject rdf:type owl:ObjectProperty ;
                  rdfs:subPropertyOf ms:isRelatedToProject ;
                  owl:inverseOf ms:isFundingProjectOf ;
                  rdfs:domain ms:LanguageResource ;
                  rdfs:range ms:Project ;
                  rdfs:comment "Links a language resource to the project that has funded its creation, enrichment, extension, etc."@en ;
                  rdfs:label "funded by"@en ;
                  skos:altLabel "funding project"@en .


###  http://w3id.org/meta-share/meta-share/fundingType
ms:fundingType rdf:type owl:ObjectProperty ;
               rdfs:domain ms:Project ;
               rdfs:range ms:FundingType ;
               rdfs:comment "Specifies the type of funding of a project with regard to the source of the funding"@en ;
               rdfs:label "funding type"@en .


###  http://w3id.org/meta-share/meta-share/genre
ms:genre rdf:type owl:ObjectProperty ;
         rdfs:domain ms:CorpusMediaPart ;
         rdfs:range ms:Genre ;
         rdfs:comment "Links a language resource (part) to the genre it belongs to"@en ;
         rdfs:label "genre"@en .


###  http://w3id.org/meta-share/meta-share/grammaticalPhenomenaCoverage
ms:grammaticalPhenomenaCoverage rdf:type owl:ObjectProperty ;
                                rdfs:domain ms:LanguageDescription ;
                                rdfs:range ms:GrammaticalPhenomenaCoverage ;
                                rdfs:comment "Gives an indication of the grammatical phenomena covered by the grammar"@en ;
                                rdfs:label "grammatical phenomena coverage"@en .


###  http://w3id.org/meta-share/meta-share/guidelines
ms:guidelines rdf:type owl:ObjectProperty ;
              rdfs:subPropertyOf ms:isDocumentedBy ;
              rdfs:domain [ rdf:type owl:Class ;
                            owl:unionOf ( ms:Annotation
                                          ms:LanguageResource
                                        )
                          ] ;
              rdfs:range ms:Document .


###  http://w3id.org/meta-share/meta-share/hadRole
ms:hadRole rdf:type owl:ObjectProperty ;
           rdfs:domain ms:Attribution ;
           rdfs:range ms:Role ;
           rdfs:comment "Links to the role with which an agent is attributed for a certain activity"@en ;
           rdfs:label "had role"@en .


###  http://w3id.org/meta-share/meta-share/hasAlignedVersion
ms:hasAlignedVersion rdf:type owl:ObjectProperty ;
                     rdfs:subPropertyOf ms:hasVersion ;
                     owl:inverseOf ms:isAlignedVersionOf ;
                     rdfs:domain ms:Corpus ;
                     rdfs:range ms:Corpus ;
                     rdfs:comment "Links to a corpus B which contains an aligned version of corpus A (the one being described)"@en ;
                     rdfs:label "has aligned version"@en .


###  http://w3id.org/meta-share/meta-share/hasAnalysed
ms:hasAnalysed rdf:type owl:ObjectProperty ;
               rdfs:subPropertyOf ms:LΤRelatedTo ;
               owl:inverseOf ms:isAnalysedBy ;
               rdfs:domain ms:ToolService ;
               rdfs:range [ rdf:type owl:Class ;
                            owl:unionOf ( ms:DataLanguageResource
                                          ms:MediaPart
                                        )
                          ] ;
               rdfs:comment "Links a tool/service B that is (or can be or has been) used for analysing LR A (e.g., a statistical tool) to LR A"@en ;
               rdfs:label "has analysed"@en .


###  http://w3id.org/meta-share/meta-share/hasAnnotated
ms:hasAnnotated rdf:type owl:ObjectProperty ;
                rdfs:subPropertyOf ms:LΤRelatedTo ;
                owl:inverseOf ms:isAnnotatedBy ;
                rdfs:domain ms:ToolService ;
                rdfs:range [ rdf:type owl:Class ;
                             owl:unionOf ( ms:Annotation
                                           ms:Corpus
                                         )
                           ] ;
                rdfs:comment "Links a tool/service B that has been used for annotating LR A (e.g., a tagger, NER, etc.) to LR A"@en ;
                rdfs:label "has annotated"@en .


###  http://w3id.org/meta-share/meta-share/hasAnnotatedVersion
ms:hasAnnotatedVersion rdf:type owl:ObjectProperty ;
                       rdfs:subPropertyOf ms:hasVersion ;
                       owl:inverseOf ms:isAnnotatedVersionOf ;
                       rdfs:domain ms:Corpus ;
                       rdfs:range ms:Corpus ;
                       rdfs:comment "Links to a corpus B which contains the annotations of corpus A (the one being described)"@en ;
                       rdfs:label "has annotated version"@en .


###  http://w3id.org/meta-share/meta-share/hasArchived
ms:hasArchived rdf:type owl:ObjectProperty ;
               rdfs:subPropertyOf ms:LΤRelatedTo ;
               owl:inverseOf ms:isArchivedBy ;
               rdfs:domain ms:ToolService ;
               rdfs:range ms:DataLanguageResource ;
               rdfs:comment "Links a tool/service B that is (or can be or has been) used for archiving LR A to LR A"@en ;
               rdfs:label "has archived"@en .


###  http://w3id.org/meta-share/meta-share/hasConvertedVersion
ms:hasConvertedVersion rdf:type owl:ObjectProperty ;
                       rdfs:subPropertyOf ms:hasVersion ;
                       owl:inverseOf ms:isConvertedVersionOf ;
                       rdfs:domain ms:DataLanguageResource ;
                       rdfs:range ms:DataLanguageResource ;
                       rdfs:comment "Links to LR B that has been used for creating LR A (the one being described) through a conversion procedure, e.g., a PDF to text conversion"@en ;
                       rdfs:label "has converted version"@en .


###  http://w3id.org/meta-share/meta-share/hasCreated
ms:hasCreated rdf:type owl:ObjectProperty ;
              rdfs:subPropertyOf ms:LΤRelatedTo ;
              owl:inverseOf ms:isCreatedBy ;
              rdfs:domain ms:ToolService ;
              rdfs:range [ rdf:type owl:Class ;
                           owl:unionOf ( ms:DataLanguageResource
                                         ms:MediaPart
                                       )
                         ] ;
              rdfs:comment "Links a tool/service B that is (or can be or has been) used for creating LR A to LR A"@en ;
              rdfs:label "has created"@en .


###  http://w3id.org/meta-share/meta-share/hasDivision
ms:hasDivision rdf:type owl:ObjectProperty ;
               rdfs:subPropertyOf ms:isRelatedTo ;
               owl:inverseOf ms:isDivisionOf ;
               rdfs:domain ms:Organization ;
               rdfs:range ms:Division ;
               rdfs:comment "Links an organization to the division(s) (e.g., company branch, university faculty or department, etc.) it consists of"@en ;
               rdfs:label "has division"@en .


###  http://w3id.org/meta-share/meta-share/hasElicited
ms:hasElicited rdf:type owl:ObjectProperty ;
               rdfs:subPropertyOf ms:LΤRelatedTo ;
               owl:inverseOf ms:isElicitedBy ;
               rdfs:domain ms:ToolService ;
               rdfs:range [ rdf:type owl:Class ;
                            owl:unionOf ( ms:DataLanguageResource
                                          ms:MediaPart
                                        )
                          ] ;
               rdfs:comment "Links a tool/service B that is (or can be or has been) used for eliciting LR A to LR A"@en ;
               rdfs:label "has elicited"@en .


###  http://w3id.org/meta-share/meta-share/hasEvaluated
ms:hasEvaluated rdf:type owl:ObjectProperty ;
                rdfs:subPropertyOf ms:LΤRelatedTo ;
                owl:inverseOf ms:isEvaluatedBy ;
                rdfs:domain ms:ToolService ;
                rdfs:range [ rdf:type owl:Class ;
                             owl:unionOf ( ms:Evaluation
                                           ms:LanguageResource
                                         )
                           ] ;
                rdfs:comment "Links a tool/service that has been used for evaluating an LR A to the data of this evaluation"@en ;
                rdfs:label "has evaluated"@en .


###  http://w3id.org/meta-share/meta-share/hasMetadata
ms:hasMetadata rdf:type owl:ObjectProperty ;
               rdfs:subPropertyOf ms:isRelatedToMDRecord ;
               owl:inverseOf ms:isMetadataOf ;
               rdfs:domain ms:LanguageResource ;
               rdfs:range ms:MetadataRecord ;
               rdfs:comment "Links to an external metadata record that describes the same language resource in another catalogue, repository, etc."@en ;
               rdfs:label "has metadata"@en .


###  http://w3id.org/meta-share/meta-share/hasOriginalSource
ms:hasOriginalSource rdf:type owl:ObjectProperty ;
                     rdfs:subPropertyOf ms:isRelatedToLR ;
                     owl:inverseOf ms:hasOutcome ;
                     rdfs:domain [ rdf:type owl:Class ;
                                   owl:unionOf ( ms:LanguageResource
                                                 ms:MediaPart
                                               )
                                 ] ;
                     rdfs:range ms:LanguageResource ;
                     rdfs:comment "Links a language resource to the original source that has been used for its creation, where it's derived or elicited from"@en ;
                     rdfs:label "has original source"@en .


###  http://w3id.org/meta-share/meta-share/hasOutcome
ms:hasOutcome rdf:type owl:ObjectProperty ;
              rdfs:subPropertyOf ms:isRelatedToLR ;
              rdfs:domain ms:ActualUse ;
              rdfs:range ms:LanguageResource ;
              rdfs:comment "Links to LR B which is created / extracted from LR A (the one being described), i.e. LR A has been used as the basis/initial/source material for LR B"@en ;
              rdfs:label "has outcome"@en ;
              skos:altLabel "is source of"@en .


###  http://w3id.org/meta-share/meta-share/hasPart
ms:hasPart rdf:type owl:ObjectProperty ;
           rdfs:subPropertyOf ms:isRelatedToLR ;
           owl:inverseOf ms:isPartOf ;
           rdfs:domain ms:LanguageResource ;
           rdfs:range ms:LanguageResource ;
           rdfs:comment "Links to LR B which is contained in LR A (the one being described), e.g., a monolingual corpus part of a bilingual corpus"@en ;
           rdfs:label "has part"@en .


###  http://w3id.org/meta-share/meta-share/hasRecorded
ms:hasRecorded rdf:type owl:ObjectProperty ;
               rdfs:subPropertyOf ms:LΤRelatedTo ;
               owl:inverseOf ms:isRecordedBy ;
               rdfs:domain ms:ToolService ;
               rdfs:range [ rdf:type owl:Class ;
                            owl:unionOf ( ms:CorpusAudioPart
                                          ms:CorpusTextNumericalPart
                                          ms:CorpusVideoPart
                                        )
                          ] ;
               rdfs:comment "Links a tool/service to the data of the language resource (e.g., audio or video part of a corpus) it has recorded"@en ;
               rdfs:label "has recorded"@en .


###  http://w3id.org/meta-share/meta-share/hasSubset
ms:hasSubset rdf:type owl:ObjectProperty ;
             rdfs:domain ms:MediaPart ;
             rdfs:range ms:Subset ;
             rdfs:comment "Links to a subset of the resource that is described in order to add specific information on the subset (e.g. size per language for multilingual corpora, size per domain for lexica with multiple domains, etc.)"@en ;
             rdfs:label "has subset"@en ;
             skos:note "introduced to cater for all sizePer properties; decided not to use the isPartOf because I wanted to keep this for \"whole\" language resources"@en .


###  http://w3id.org/meta-share/meta-share/hasValidated
ms:hasValidated rdf:type owl:ObjectProperty ;
                rdfs:subPropertyOf ms:LΤRelatedTo ;
                owl:inverseOf ms:isValidatedBy ;
                rdfs:domain ms:ToolService ;
                rdfs:range [ rdf:type owl:Class ;
                             owl:unionOf ( ms:LanguageResource
                                           ms:Validation
                                         )
                           ] ;
                rdfs:comment "Links a tool/service B that is (or can be) used for validating LR A to the data of this validation"@en ;
                rdfs:label "has validated"@en .


###  http://w3id.org/meta-share/meta-share/hasVersion
ms:hasVersion rdf:type owl:ObjectProperty ;
              rdfs:subPropertyOf ms:isRelatedToLR ;
              owl:inverseOf ms:isVersionOf ;
              rdfs:domain ms:LanguageResource ;
              rdfs:range ms:LanguageResource ;
              rdfs:comment "Links to LR B that is a version of LR A (the one being described)"@en ;
              rdfs:label "has version"@en .


###  http://w3id.org/meta-share/meta-share/headOfficeAddress
ms:headOfficeAddress rdf:type owl:ObjectProperty ;
                     rdfs:subPropertyOf ms:addressSet ;
                     rdfs:domain [ rdf:type owl:Class ;
                                   owl:unionOf ( ms:Affiliation
                                                 ms:Division
                                                 ms:Group
                                                 ms:Organization
                                               )
                                 ] ;
                     rdfs:range ms:AddressSet ;
                     rdfs:comment "Links to the physical address of the head office of an organization or group represented as a set of distinct elements (street, zip code, city, etc.)"@en ;
                     rdfs:label "address (head office)"@en .


###  http://w3id.org/meta-share/meta-share/hearingImpairmentOfParticipants
ms:hearingImpairmentOfParticipants rdf:type owl:ObjectProperty ;
                                   rdfs:domain [ rdf:type owl:Class ;
                                                 owl:unionOf ( ms:CorpusAudioPart
                                                               ms:CorpusImagePart
                                                               ms:CorpusTextNumericalPart
                                                               ms:CorpusVideoPart
                                                             )
                                               ] ;
                                   rdfs:range ms:HearingImpairmentOfParticipants ;
                                   rdfs:comment "Specifies whether the group of participants contains persons with hearing impairments"@en ;
                                   rdfs:label "hearing impairment of participants"@en .


###  http://w3id.org/meta-share/meta-share/imageFormat
ms:imageFormat rdf:type owl:ObjectProperty ;
               rdfs:domain ms:DatasetDistribution ;
               rdfs:range ms:ImageFormat ;
               rdfs:comment "Provides information on each of the format(s) of the image part of a resource"@en ;
               rdfs:label "detailed image format"@en ;
               owl:deprecated ""@en .


###  http://w3id.org/meta-share/meta-share/inputContentResource
ms:inputContentResource rdf:type owl:ObjectProperty ;
                        rdfs:domain ms:ToolService ;
                        rdfs:range ms:ProcessingResource ;
                        rdfs:comment "Specifies the requirements set by a tool/service for the (content) resource that it processes"@en ;
                        rdfs:label "input content resource"@en .


###  http://w3id.org/meta-share/meta-share/intendedApplication
ms:intendedApplication rdf:type owl:ObjectProperty ;
                       rdfs:domain ms:LanguageResource ;
                       rdfs:range [ owl:intersectionOf ( skos:Concept
                                                         [ rdf:type owl:Restriction ;
                                                           owl:onProperty skos:inScheme ;
                                                           owl:hasValue omtd:OperationScheme
                                                         ]
                                                       ) ;
                                    rdf:type owl:Class
                                  ] ;
                       rdfs:comment "Specifies an LT application for which the language resource has been created or for which it can be used or is recommended to be used"@en ;
                       rdfs:label "intended application"@en .


###  http://w3id.org/meta-share/meta-share/interactivity
ms:interactivity rdf:type owl:ObjectProperty ;
                 rdfs:domain [ rdf:type owl:Class ;
                               owl:unionOf ( ms:CorpusAudioPart
                                             ms:CorpusVideoPart
                                           )
                             ] ;
                 rdfs:range ms:Interactivity ;
                 rdfs:comment "Indicates the level of conversational interaction between speakers (for audio component) or participants (for video component)"@en ;
                 rdfs:label "interactivity"@en .


###  http://w3id.org/meta-share/meta-share/iprHolder
ms:iprHolder rdf:type owl:ObjectProperty ;
             rdfs:subPropertyOf ms:isRelatedToActor ;
             owl:inverseOf ms:isIprHolderOf ;
             rdfs:domain ms:LanguageResource ;
             rdfs:range ms:Actor ;
             rdfs:comment "A person or an organization who holds the full Intellectual Property Rights (Copyright, trademark, etc.) that subsist in the resource. The IPR holder could be different from the creator that may have assigned the rights to the IPR holder (e.g., an author as a creator assigns her rights to the publisher who is the IPR holder) and the distributor that holds a specific licence (i.e. a permission) to distribute the work via a specific distributor."@en ;
             rdfs:label "IPR holder"@en ;
             skos:altLabel "intellectual property rights holder"@en ,
                           "rights holder"@en .


###  http://w3id.org/meta-share/meta-share/isAccessedBy
ms:isAccessedBy rdf:type owl:ObjectProperty ;
                rdfs:subPropertyOf ms:isRelatedToLT ;
                rdfs:domain [ rdf:type owl:Class ;
                              owl:unionOf ( ms:DataLanguageResource
                                            ms:DatasetDistribution
                                            ms:MediaPart
                                          )
                            ] ;
                rdfs:range ms:ToolService ;
                rdfs:comment "Links to a tool/service B that is (or can be) used for accessing LR A (the one being described), e.g., a corpus workbench, s/w for lexicon access"@en ;
                rdfs:label "is accessed by"@en ;
                skos:altLabel "access tool"@en .


###  http://w3id.org/meta-share/meta-share/isAlignedVersionOf
ms:isAlignedVersionOf rdf:type owl:ObjectProperty ;
                      rdfs:subPropertyOf ms:isVersionOf ;
                      rdfs:domain ms:Corpus ;
                      rdfs:range ms:Corpus ;
                      rdfs:comment "Links to a corpus B which is the aligned version of corpus A (the one being described)"@en ;
                      rdfs:label "is aligned version of"@en .


###  http://w3id.org/meta-share/meta-share/isAnalysedBy
ms:isAnalysedBy rdf:type owl:ObjectProperty ;
                rdfs:subPropertyOf ms:isRelatedToLT ;
                rdfs:domain [ rdf:type owl:Class ;
                              owl:unionOf ( ms:DataLanguageResource
                                            ms:MediaPart
                                          )
                            ] ;
                rdfs:range ms:ToolService ;
                rdfs:comment "Links to a tool/service B that is (or can be or has been) used for analysing LR A (the one being described), e.g., a statistical tool"@en ;
                rdfs:label "is analysed by"@en ;
                skos:altLabel "analysis tool"@en .


###  http://w3id.org/meta-share/meta-share/isAnnotatedBy
ms:isAnnotatedBy rdf:type owl:ObjectProperty ;
                 rdfs:subPropertyOf ms:isRelatedToLT ;
                 rdfs:domain ms:Annotation ;
                 rdfs:range ms:ToolService ;
                 rdfs:comment "Links to a tool/service B that has been used for annotating LR A (the one being described), e.g., a tagger, NER, etc."@en ;
                 rdfs:label "is annotated by"@en ;
                 skos:altLabel "annotation tool"@en .


###  http://w3id.org/meta-share/meta-share/isAnnotatedVersionOf
ms:isAnnotatedVersionOf rdf:type owl:ObjectProperty ;
                        rdfs:subPropertyOf ms:isVersionOf ;
                        rdfs:domain ms:Corpus ;
                        rdfs:range ms:Corpus ;
                        rdfs:comment "Links to a corpus B which is the raw corpus that has been annotated (corpus A, the one being described)"@en ;
                        rdfs:label "is annotated version of"@en .


###  http://w3id.org/meta-share/meta-share/isAnnotationResourceOf
ms:isAnnotationResourceOf rdf:type owl:ObjectProperty ;
                          rdfs:subPropertyOf ms:dependentLR ;
                          rdfs:domain ms:LexicalConceptualResource ;
                          rdfs:range [ rdf:type owl:Class ;
                                       owl:unionOf ( ms:MLModel
                                                     ms:ProcessingResource
                                                     ms:ToolService
                                                   )
                                     ] ;
                          rdfs:comment "Links an annotation resource to the corpus where it has been used for annotating or to data of an annotation tool/service that has been or can be combined with"@en ;
                          rdfs:label "is annotation resource of"@en .


###  http://w3id.org/meta-share/meta-share/isAnnotationSchemaOf
ms:isAnnotationSchemaOf rdf:type owl:ObjectProperty ;
                        rdfs:subPropertyOf ms:dependentLR ;
                        rdfs:domain ms:LexicalConceptualResource ;
                        rdfs:range [ rdf:type owl:Class ;
                                     owl:unionOf ( ms:MLModel
                                                   ms:ProcessingResource
                                                   ms:ToolService
                                                 )
                                   ] ;
                        rdfs:comment "Links an annotation schema to the corpus where it has been used for annotating or to data of an annotation tool/service that has been or can be combined with"@en ;
                        rdfs:label "is annotation schema of"@en .


###  http://w3id.org/meta-share/meta-share/isAnnotatorOf
ms:isAnnotatorOf rdf:type owl:ObjectProperty ;
                 rdfs:subPropertyOf ms:actorRelatedTo ;
                 rdfs:domain ms:Actor ;
                 rdfs:range ms:Annotation ;
                 rdfs:comment "Identifies the resource(s) that have been annotated by the person/organization"@en ;
                 rdfs:label "is annotator of"@en .


###  http://w3id.org/meta-share/meta-share/isArchivedBy
ms:isArchivedBy rdf:type owl:ObjectProperty ;
                rdfs:subPropertyOf ms:isRelatedToLT ;
                rdfs:domain ms:DataLanguageResource ;
                rdfs:range ms:ToolService ;
                rdfs:comment "Links to a tool/service B that is (or can be or has been) used for archiving LR A (the one being described)"@en ;
                rdfs:label "is archived by"@en ;
                skos:altLabel "archiving tool"@en .


###  http://w3id.org/meta-share/meta-share/isCitedBy
ms:isCitedBy rdf:type owl:ObjectProperty ;
             rdfs:subPropertyOf ms:isRelatedToDocument ;
             rdfs:domain ms:LanguageResource ;
             rdfs:range ms:Document ;
             rdfs:comment "Links to a publication that cites the language resource described"@en ;
             rdfs:label "is cited by"@en .


###  http://w3id.org/meta-share/meta-share/isCombinedWith
ms:isCombinedWith rdf:type owl:ObjectProperty ;
                  rdfs:subPropertyOf ms:isRelatedToLR ;
                  rdf:type owl:SymmetricProperty ;
                  rdfs:domain ms:LanguageResource ;
                  rdfs:range ms:LanguageResource ;
                  rdfs:comment "Links to a LR B that has been used together with LR A (the one being described) to create LR C, e.g., two monolingual wordnets/corpora aligned to produce a bilingual resource"@en ;
                  rdfs:label "is combined with"@en .


###  http://w3id.org/meta-share/meta-share/isCompatibleWith
ms:isCompatibleWith rdf:type owl:ObjectProperty ;
                    rdfs:subPropertyOf ms:dependsOn ;
                    rdf:type owl:SymmetricProperty ;
                    rdfs:domain ms:LanguageResource ;
                    rdfs:range ms:LanguageResource ;
                    rdfs:comment "Links to a LR B that can be used together with LR A (the one being described), e.g., a lexicon that is compatible with a grammar"@en ;
                    rdfs:label "is compatible with"@en .


###  http://w3id.org/meta-share/meta-share/isContactFor
ms:isContactFor rdf:type owl:ObjectProperty ;
                rdfs:subPropertyOf ms:actorRelatedTo ;
                rdfs:domain ms:Actor ;
                rdfs:range ms:LanguageResource ;
                rdfs:comment "Links to the language resource(s) for which the person/organization/group can be contacted for further information"@en ;
                rdfs:label "is contact for"@en .


###  http://w3id.org/meta-share/meta-share/isContinuationOf
ms:isContinuationOf rdf:type owl:ObjectProperty ;
                    rdfs:subPropertyOf ms:isVersionOf ;
                    owl:inverseOf ms:isContinuedBy ;
                    rdfs:domain ms:LanguageResource ;
                    rdfs:range ms:LanguageResource ;
                    rdfs:comment "Links to LR B that forms the basis of LR A (the one being described) upon which it has continued to extend / enrich"@en ;
                    rdfs:label "is continuation of"@en .


###  http://w3id.org/meta-share/meta-share/isContinuedBy
ms:isContinuedBy rdf:type owl:ObjectProperty ;
                 rdfs:subPropertyOf ms:hasVersion ;
                 rdfs:domain ms:LanguageResource ;
                 rdfs:range ms:LanguageResource ;
                 rdfs:comment "Links to a LR B that extends / continues / enriches LR A (the one being described)"@en ;
                 rdfs:label "is continued by"@en .


###  http://w3id.org/meta-share/meta-share/isConvertedVersionOf
ms:isConvertedVersionOf rdf:type owl:ObjectProperty ;
                        rdfs:subPropertyOf ms:isVersionOf ;
                        rdfs:domain ms:DataLanguageResource ;
                        rdfs:range ms:DataLanguageResource ;
                        rdfs:comment "Links to LR B that has been the outcome of a conversion procedure from LR A (the one being described), e.g., a PDF to text conversion"@en ;
                        rdfs:label "is converted version of"@en .


###  http://w3id.org/meta-share/meta-share/isCoordinatorOf
ms:isCoordinatorOf rdf:type owl:ObjectProperty ;
                   rdfs:subPropertyOf ms:actorRelatedTo ;
                   rdfs:comment "Introduces the project that an organization coordinates"@en ;
                   rdfs:label "is coordinator of"@en .


###  http://w3id.org/meta-share/meta-share/isCreatedBy
ms:isCreatedBy rdf:type owl:ObjectProperty ;
               rdfs:subPropertyOf ms:isRelatedToLT ;
               rdfs:domain [ rdf:type owl:Class ;
                             owl:unionOf ( ms:DataLanguageResource
                                           ms:MediaPart
                                         )
                           ] ;
               rdfs:range ms:ToolService ;
               rdfs:comment "Links to a tool/service B that has been used for creating LR A (the one being described)"@en ;
               rdfs:label "is created by"@en ;
               skos:altLabel "creation tool"@en ,
                             "derivation tool"@en .


###  http://w3id.org/meta-share/meta-share/isDescribedBy
ms:isDescribedBy rdf:type owl:ObjectProperty ;
                 rdfs:subPropertyOf ms:isDocumentedBy ;
                 rdfs:domain ms:LanguageResource ;
                 rdfs:range ms:Document ;
                 rdfs:comment "Links to a document that describes the contents or operation of a language resource"@en ;
                 rdfs:label "is described by"@en .


###  http://w3id.org/meta-share/meta-share/isDisplayedBy
ms:isDisplayedBy rdf:type owl:ObjectProperty ;
                 rdfs:subPropertyOf ms:isRelatedToLT ;
                 rdfs:domain [ rdf:type owl:Class ;
                               owl:unionOf ( ms:DataLanguageResource
                                             ms:DatasetDistribution
                                             ms:MediaPart
                                           )
                             ] ;
                 rdfs:range ms:ToolService ;
                 rdfs:comment "Links to a tool/service B that is (or can be) used to display LR A (the one being described), e.g., a tool for visualizing relations in a lexicon, or annotations in a corpus"@en ;
                 rdfs:label "is displayed by"@en ;
                 skos:altLabel "display tool"@en ,
                               "visualization tool"@en .


###  http://w3id.org/meta-share/meta-share/isDistributionRightsHolderOf
ms:isDistributionRightsHolderOf rdf:type owl:ObjectProperty ;
                                rdfs:subPropertyOf ms:actorRelatedTo ;
                                rdfs:domain ms:Actor ;
                                rdfs:range ms:Distribution ;
                                rdfs:comment "Identifies the language resource for which a person or an organization holds the distribution rights. The range and scope of distribution rights is defined in the distribution agreement. The distributor in most cases only has a limited licence to distribute the work and collect royalties on behalf of the licensor or the IPR holder and cannot give to any recipient of the work permissions that exceed the scope of the distribution agreement (e.g., to allow uses of the work that are not defined in the distribution agreement)"@en ;
                                rdfs:label "is distribution rights holder of"@en .


###  http://w3id.org/meta-share/meta-share/isDivisionOf
ms:isDivisionOf rdf:type owl:ObjectProperty ;
                rdfs:subPropertyOf ms:isRelatedTo ;
                rdfs:domain ms:Division ;
                rdfs:range ms:Organization ;
                rdfs:comment "Links a division (e.g., company branch, university department or faculty) to the organization to which it belongs"@en ;
                rdfs:label "is division of"@en .


###  http://w3id.org/meta-share/meta-share/isDocumentedBy
ms:isDocumentedBy rdf:type owl:ObjectProperty ;
                  rdfs:subPropertyOf ms:isRelatedToDocument ;
                  rdfs:domain ms:LanguageResource ;
                  rdfs:range ms:Document ;
                  rdfs:comment "Links a language resource to a document (e.g., research paper describing its contents or its use in a project, user manual, etc.) or any other form of documentation (e.g., a URL with support information) that is related to the resource"@en ;
                  rdfs:label "is documented by"@en ;
                  skos:altLabel "documentation report"@en .


###  http://w3id.org/meta-share/meta-share/isEditedBy
ms:isEditedBy rdf:type owl:ObjectProperty ;
              rdfs:subPropertyOf ms:isRelatedToLT ;
              rdfs:domain [ rdf:type owl:Class ;
                            owl:unionOf ( ms:DataLanguageResource
                                          ms:MediaPart
                                        )
                          ] ;
              rdfs:range ms:ToolService ;
              rdfs:comment "Links to a tool/service B that is (or can be) used for editing LR A (the one being described)"@en ;
              rdfs:label "is edited by"@en ;
              skos:altLabel "editing tool"@en .


###  http://w3id.org/meta-share/meta-share/isElicitedBy
ms:isElicitedBy rdf:type owl:ObjectProperty ;
                rdfs:subPropertyOf ms:isRelatedToLT ;
                rdfs:domain [ rdf:type owl:Class ;
                              owl:unionOf ( ms:DataLanguageResource
                                            ms:MediaPart
                                          )
                            ] ;
                rdfs:range ms:ToolService ;
                rdfs:comment "Links to a tool/service B that is (or can be or has been) used for eliciting LR A (the one being described)"@en ;
                rdfs:label "is elicited by"@en ;
                skos:altLabel "elicitation tool"@en .


###  http://w3id.org/meta-share/meta-share/isEvaluatedBy
ms:isEvaluatedBy rdf:type owl:ObjectProperty ;
                 rdfs:subPropertyOf ms:isRelatedToLT ;
                 rdfs:domain ms:Evaluation ;
                 rdfs:range ms:ToolService ;
                 rdfs:comment "Links to a tool/service B that has been used to evaluate LR A (the one being described)"@en ;
                 rdfs:label "is evaluated by"@en ;
                 skos:altLabel "evaluation tool"@en .


###  http://w3id.org/meta-share/meta-share/isEvaluatorOf
ms:isEvaluatorOf rdf:type owl:ObjectProperty ;
                 rdfs:subPropertyOf ms:actorRelatedTo ;
                 rdfs:domain ms:Actor ;
                 rdfs:range ms:Evaluation ;
                 rdfs:comment "Identifies the tool or service(s) that a person or organization that has evaluated"@en ;
                 rdfs:label "is evaluator of"@en .


###  http://w3id.org/meta-share/meta-share/isExactMatchWith
ms:isExactMatchWith rdf:type owl:ObjectProperty ;
                    rdfs:subPropertyOf ms:isRelatedToLR ;
                    rdf:type owl:SymmetricProperty ;
                    rdfs:domain ms:LanguageResource ;
                    rdfs:range ms:LanguageResource ;
                    rdfs:comment "Links to LR B that has the same contents with LR A; they may have different names or the same name and be stored on different locations"@en ;
                    rdfs:label "is exact match with"@en ;
                    skos:altLabel "is identical with"@en ,
                                  "is same as"@en .


###  http://w3id.org/meta-share/meta-share/isFunderOf
ms:isFunderOf rdf:type owl:ObjectProperty ;
              rdfs:subPropertyOf ms:actorRelatedTo ;
              rdfs:domain ms:Actor ;
              rdfs:range ms:Project ;
              rdfs:comment "Links to the projects) that the person/organization has financed"@en ;
              rdfs:label "is funder of"@en .


###  http://w3id.org/meta-share/meta-share/isFundingProjectOf
ms:isFundingProjectOf rdf:type owl:ObjectProperty ;
                      rdfs:subPropertyOf ms:projectRelatedTo ;
                      rdfs:domain ms:Project ;
                      rdfs:range ms:LanguageResource ;
                      rdfs:comment "Links a project to the language resource(s) that it has funded (e.g., creation, enrichment, extension, etc.)"@en ;
                      rdfs:label "is funding project of"@en .


###  http://w3id.org/meta-share/meta-share/isIprHolderOf
ms:isIprHolderOf rdf:type owl:ObjectProperty ;
                 rdfs:subPropertyOf ms:actorRelatedTo ;
                 rdfs:domain ms:Actor ;
                 rdfs:range ms:LanguageResource ;
                 rdfs:comment "Links to the resource(s) for which a person or an organization holds the full Intellectual Property Rights (Copyright, trademark, etc.). The IPR holder could be different from the creator that may have assigned the rights to the IPR holder (e.g., an author as a creator assigns her rights to the publisher who is the IPR holder) and the distributor that holds a specific licence (i.e. a permission) to distribute the work via a specific distributor."@en ;
                 rdfs:label "is IPR holder of"@en .


###  http://w3id.org/meta-share/meta-share/isLicensorOr
ms:isLicensorOr rdf:type owl:ObjectProperty ;
                rdfs:subPropertyOf ms:actorRelatedTo ;
                owl:inverseOf ms:licensor ;
                rdfs:domain ms:Actor ;
                rdfs:range ms:Distribution ;
                rdfs:comment "Links to the resource(s) which a person or organisation is legally eligible to license and actually licenses. The licensor could be different from the creator, the distributor or the IPR holder. The licensor has the necessary rights or licences to license the work and is the party that actually licenses the resource that is distributed via the specific channel. She will have obtained the necessary rights or licences from the IPR holder and she may have a distribution agreement with a distributor that disseminates the work under a set of conditions defined in the specific licence and collects revenue on the licensor's behalf. The attribution of the creator, separately from the attribution of the licensor, may be part of the licence under which the resource is distributed (as e.g., is the case with Creative Commons Licences)."@en ;
                rdfs:label "is licensor of"@en .


###  http://w3id.org/meta-share/meta-share/isMLModelOf
ms:isMLModelOf rdf:type owl:ObjectProperty ;
               rdfs:subPropertyOf ms:dependentLR ;
               owl:inverseOf ms:mlModel ;
               rdfs:domain ms:MLModel ;
               rdfs:range ms:ToolService ;
               rdfs:comment "Specifies the tool/service with which the ML model can be combined in order to perform the desired task"@en ;
               rdfs:label "is ML model of"@en ;
               skos:altLabel "is Machine Learning model of"@en .


###  http://w3id.org/meta-share/meta-share/isMetadataCreatorOf
ms:isMetadataCreatorOf rdf:type owl:ObjectProperty ;
                       rdfs:subPropertyOf ms:actorRelatedTo ;
                       owl:inverseOf ms:metadataCreator ;
                       rdfs:domain ms:Person ;
                       rdfs:range ms:MetadataRecord ;
                       rdfs:comment "Links to the metadata record(s) that a person has created"@en ;
                       rdfs:label "is metadata creator of"@en .


###  http://w3id.org/meta-share/meta-share/isMetadataCuratorOf
ms:isMetadataCuratorOf rdf:type owl:ObjectProperty ;
                       rdfs:subPropertyOf ms:actorRelatedTo ;
                       owl:inverseOf ms:metadataCurator ;
                       rdfs:domain ms:Person ;
                       rdfs:range ms:MetadataRecord ;
                       rdfs:comment "Links to the metadata record(s) for which a person is responsible for creating, updating, enriching, etc."@en ;
                       rdfs:label "is metadata curator of"@en .


###  http://w3id.org/meta-share/meta-share/isMetadataOf
ms:isMetadataOf rdf:type owl:ObjectProperty ;
                rdfs:subPropertyOf ms:MDRecordRelatedTo ;
                rdfs:domain ms:MetadataRecord ;
                rdfs:range ms:LanguageResource ;
                rdfs:comment "Links an external metadata record (from another catalogue, repository, etc.) to the language resource described"@en ;
                rdfs:label "is metadata of"@en .


###  http://w3id.org/meta-share/meta-share/isPartOf
ms:isPartOf rdf:type owl:ObjectProperty ;
            rdfs:subPropertyOf ms:isRelatedToLR ;
            rdfs:domain ms:LanguageResource ;
            rdfs:range ms:LanguageResource ;
            rdfs:comment "Links to LR B which contains LR A (the one being described), e.g., a bilingual corpus that includes a monolingual corpus"@en ;
            rdfs:label "is part of"@en .


###  http://w3id.org/meta-share/meta-share/isPartWith
ms:isPartWith rdf:type owl:ObjectProperty ;
              rdfs:subPropertyOf ms:isRelatedToLR ;
              rdf:type owl:SymmetricProperty ;
              rdfs:domain ms:LanguageResource ;
              rdfs:range ms:LanguageResource ;
              rdfs:comment "Links to LR B that together with LR A (the one being described) are parts of LR C"@en ;
              rdfs:label "is part with"@en .


###  http://w3id.org/meta-share/meta-share/isParticipatingOrganizationIn
ms:isParticipatingOrganizationIn rdf:type owl:ObjectProperty ;
                                 rdfs:subPropertyOf ms:actorRelatedTo ;
                                 owl:inverseOf ms:participatingOrganization ;
                                 rdfs:domain ms:Organization ;
                                 rdfs:range ms:Project ;
                                 rdfs:comment "Identifies the project(s) where an organization has officially participated or participates in"@en ;
                                 rdfs:label "participant in"@en ;
                                 skos:example "European Language Technology Project, Machine Translation for Elderly People, ..."@en .


###  http://w3id.org/meta-share/meta-share/isQueriedBy
ms:isQueriedBy rdf:type owl:ObjectProperty ;
               rdfs:subPropertyOf ms:isRelatedToLT ;
               owl:inverseOf ms:queries ;
               rdfs:domain [ rdf:type owl:Class ;
                             owl:unionOf ( ms:DataLanguageResource
                                           ms:DatasetDistribution
                                           ms:MediaPart
                                         )
                           ] ;
               rdfs:range ms:ToolService ;
               rdfs:comment "Links to a tool/service B that is (or can be) used for querying LR A (the one being described)"@en ;
               rdfs:label "is queried by"@en ;
               skos:altLabel "query tool"@en .


###  http://w3id.org/meta-share/meta-share/isRecordedBy
ms:isRecordedBy rdf:type owl:ObjectProperty ;
                rdfs:subPropertyOf ms:isRelatedToLT ;
                rdfs:domain [ rdf:type owl:Class ;
                              owl:unionOf ( ms:CorpusAudioPart
                                            ms:CorpusTextNumericalPart
                                            ms:CorpusVideoPart
                                          )
                            ] ;
                rdfs:range ms:ToolService ;
                rdfs:comment "Links to a tool/service that has been used for recording a video or audio corpus part"@en ;
                rdfs:label "is recorded by"@en ;
                skos:altLabel "recording platform software"@en ,
                              "recording tool"@en .


###  http://w3id.org/meta-share/meta-share/isRecorderOf
ms:isRecorderOf rdf:type owl:ObjectProperty ;
                rdfs:subPropertyOf ms:actorRelatedTo ;
                owl:inverseOf ms:recorder ;
                rdfs:domain ms:Actor ;
                rdfs:range [ rdf:type owl:Class ;
                             owl:unionOf ( ms:CorpusAudioPart
                                           ms:CorpusTextNumericalPart
                                           ms:CorpusVideoPart
                                         )
                           ] ;
                rdfs:comment "Links to the audio or video part of the resource(s) that a person/organization has recorded"@en ;
                rdfs:label "is recorder of"@en .


###  http://w3id.org/meta-share/meta-share/isRelatedTo
ms:isRelatedTo rdf:type owl:ObjectProperty ;
               rdfs:domain [ rdf:type owl:Class ;
                             owl:unionOf ( ms:DescribedEntity
                                           ms:MetadataRecord
                                         )
                           ] ;
               rdfs:range [ rdf:type owl:Class ;
                            owl:unionOf ( ms:Actor
                                          ms:Document
                                          ms:LanguageResource
                                        )
                          ] ;
               rdfs:comment "Identifies a relation holding between two language resources or a language resource and a document or actor or, in general, a satellite entity"@en ;
               rdfs:label "is related to"@en .


###  http://w3id.org/meta-share/meta-share/isRelatedToActor
ms:isRelatedToActor rdf:type owl:ObjectProperty ;
                    rdfs:subPropertyOf ms:isRelatedTo ;
                    rdfs:domain [ rdf:type owl:Class ;
                                  owl:unionOf ( ms:Distribution
                                                ms:LanguageResource
                                                ms:MetadataRecord
                                              )
                                ] ;
                    rdfs:range ms:Actor ;
                    rdfs:comment "Links to the data of an actor that bears some relation to the language resource that is described"@en ;
                    rdfs:label "is related to actor"@en .


###  http://w3id.org/meta-share/meta-share/isRelatedToDocument
ms:isRelatedToDocument rdf:type owl:ObjectProperty ;
                       rdfs:subPropertyOf ms:isRelatedTo ;
                       rdfs:domain [ rdf:type owl:Class ;
                                     owl:unionOf ( ms:LanguageResource
                                                   ms:Project
                                                 )
                                   ] ;
                       rdfs:range ms:Document ;
                       rdfs:comment "Links to a document that is somehow related to the entity that is described"@en ;
                       rdfs:label "is related to document"@en .


###  http://w3id.org/meta-share/meta-share/isRelatedToLR
ms:isRelatedToLR rdf:type owl:ObjectProperty ;
                 rdfs:subPropertyOf ms:isRelatedTo ;
                 rdfs:domain [ rdf:type owl:Class ;
                               owl:unionOf ( ms:Division
                                             ms:Document
                                             ms:Group
                                             ms:LanguageResource
                                             ms:Organization
                                             ms:Person
                                             ms:Project
                                           )
                             ] ;
                 rdfs:range ms:LanguageResource ;
                 rdfs:comment "Links to a language resource that holds a relation with the entity being described (without further specification of the relation type)"@en ;
                 rdfs:label "is related to Language Resource"@en .


###  http://w3id.org/meta-share/meta-share/isRelatedToLT
ms:isRelatedToLT rdf:type owl:ObjectProperty ;
                 rdfs:subPropertyOf ms:isRelatedTo ;
                 rdfs:domain ms:DataLanguageResource ;
                 rdfs:range ms:ToolService ;
                 rdfs:comment "Links to a tool/service B that bears some relation to LR A (the one being described)"@en ;
                 rdfs:label "is related to LT tool/service"@en .


###  http://w3id.org/meta-share/meta-share/isRelatedToMDRecord
ms:isRelatedToMDRecord rdf:type owl:ObjectProperty ;
                       rdfs:subPropertyOf ms:isRelatedTo ;
                       rdfs:domain [ rdf:type owl:Class ;
                                     owl:unionOf ( ms:LanguageResource
                                                   ms:MetadataRecord
                                                 )
                                   ] ;
                       rdfs:range ms:MetadataRecord ;
                       rdfs:comment "Links to an external metadata record that has some relation with the metadata record of the resource being described or the resource itself"@en ;
                       rdfs:label "is related to metadata record"@en .


###  http://w3id.org/meta-share/meta-share/isRelatedToProject
ms:isRelatedToProject rdf:type owl:ObjectProperty ;
                      rdfs:subPropertyOf ms:isRelatedTo ;
                      owl:inverseOf ms:projectRelatedTo ;
                      rdfs:domain ms:LanguageResource ;
                      rdfs:range ms:Project ;
                      rdfs:comment "Links to a project that has some relation with the language resource that is described (e.g., has funded its creation)"@en ;
                      rdfs:label "is related to project"@en .


###  http://w3id.org/meta-share/meta-share/isReplacedWith
ms:isReplacedWith rdf:type owl:ObjectProperty ;
                  rdfs:subPropertyOf ms:hasVersion ;
                  owl:inverseOf ms:replaces ;
                  rdfs:domain ms:LanguageResource ;
                  rdfs:range ms:LanguageResource ;
                  rdfs:comment "Links to LR B that is a newer version of LR A (the one being described) and replaces it"@en ;
                  rdfs:label "is replaced with"@en .


###  http://w3id.org/meta-share/meta-share/isRequiredLRBy
ms:isRequiredLRBy rdf:type owl:ObjectProperty ;
                  rdfs:subPropertyOf ms:dependentLR ;
                  owl:inverseOf ms:requiresLR ;
                  rdfs:domain [ rdf:type owl:Class ;
                                owl:unionOf ( ms:LanguageDescription
                                              ms:LexicalConceptualResource
                                            )
                              ] ;
                  rdfs:range [ rdf:type owl:Class ;
                               owl:unionOf ( ms:LanguageDescription
                                             ms:ProcessingResource
                                             ms:ToolService
                                           )
                             ] ;
                  rdfs:comment "Links to a language resource that is required for the operation of a tool/service or computational grammar"@en ;
                  rdfs:label "is required language resource by"@en .


###  http://w3id.org/meta-share/meta-share/isResourceCreatorOf
ms:isResourceCreatorOf rdf:type owl:ObjectProperty ;
                       rdfs:subPropertyOf ms:actorRelatedTo ;
                       owl:inverseOf ms:resourceCreator ;
                       rdfs:domain ms:Actor ;
                       rdfs:range ms:LanguageResource ;
                       rdfs:comment "Links to the language resource(s) that a person/organization has created"@en ;
                       rdfs:label "is resource creator of"@en .


###  http://w3id.org/meta-share/meta-share/isResourceProviderOf
ms:isResourceProviderOf rdf:type owl:ObjectProperty ;
                        rdfs:subPropertyOf ms:actorRelatedTo ;
                        owl:inverseOf ms:resourceProvider ;
                        rdfs:domain ms:Actor ;
                        rdfs:range ms:LanguageResource ;
                        rdfs:comment "Links to a resource for which the person/organization is responsible of providing, curating and maintaining"@en ;
                        rdfs:label "is resource provider of"@en .


###  http://w3id.org/meta-share/meta-share/isReviewedBy
ms:isReviewedBy rdf:type owl:ObjectProperty ;
                rdfs:subPropertyOf ms:isDocumentedBy ;
                owl:inverseOf ms:reviews ;
                rdfs:domain ms:LanguageResource ;
                rdfs:range ms:Document ;
                rdfs:comment "Links to a document that contains the review of LR A (the one being described)"@en ;
                rdfs:label "is reviewed by"@en ;
                skos:altLabel "review"@en .


###  http://w3id.org/meta-share/meta-share/isSimilarTo
ms:isSimilarTo rdf:type owl:ObjectProperty ;
               rdfs:subPropertyOf ms:isRelatedToLR ;
               rdf:type owl:SymmetricProperty ;
               rdfs:domain ms:LanguageResource ;
               rdfs:range ms:LanguageResource ;
               rdfs:comment "Links to LR B that bears resemblances to LR A (the one being described), e.g., they have been built with the same theoretical principles or are the same with different formats or processed at the same level with different tools"@en ;
               rdfs:label "is similar to"@en ;
               skos:altLabel "is similar with"@en .


###  http://w3id.org/meta-share/meta-share/isSupplementTo
ms:isSupplementTo rdf:type owl:ObjectProperty ;
                  rdfs:subPropertyOf ms:isRelatedToLR ;
                  owl:inverseOf ms:isSupplementedBy ;
                  rdfs:label "is supplement to"@en .


###  http://w3id.org/meta-share/meta-share/isSupplementedBy
ms:isSupplementedBy rdf:type owl:ObjectProperty ;
                    rdfs:subPropertyOf ms:isRelatedToLR ;
                    rdfs:label "is supplemented by"@en .


###  http://w3id.org/meta-share/meta-share/isTagsetOf
ms:isTagsetOf rdf:type owl:ObjectProperty ;
              rdfs:subPropertyOf ms:dependentLR ;
              owl:inverseOf ms:tagset ;
              rdfs:domain ms:LexicalConceptualResource ;
              rdfs:range [ rdf:type owl:Class ;
                           owl:unionOf ( ms:Annotation
                                         ms:LanguageResource
                                         ms:MLModel
                                       )
                         ] ;
              rdfs:comment "Links a tagset to the resource where it has been used for annotating or to a tool/service or that should be used (dependency) for the annotation"@en ;
              rdfs:label "is tagset for"@en .


###  http://w3id.org/meta-share/meta-share/isToBeCitedBy
ms:isToBeCitedBy rdf:type owl:ObjectProperty ;
                 rdfs:subPropertyOf ms:isRelatedToDocument ;
                 rdfs:domain ms:LanguageResource ;
                 rdfs:range ms:Document ;
                 rdfs:comment "Links to the publication that must be used when citing the language resource"@en ;
                 rdfs:label "is to be cited by"@en .


###  http://w3id.org/meta-share/meta-share/isTypesystemOf
ms:isTypesystemOf rdf:type owl:ObjectProperty ;
                  rdfs:subPropertyOf ms:dependentLR ;
                  owl:inverseOf ms:typesystem ;
                  rdfs:domain ms:LexicalConceptualResource ;
                  rdfs:range [ rdf:type owl:Class ;
                               owl:unionOf ( ms:MLModel
                                             ms:ProcessingResource
                                             ms:ToolService
                                           )
                             ] ;
                  rdfs:comment "Links a typesystem to the corpus where it has been used for annotating or to data of an annotation tool/service that has been or can be combined with"@en ;
                  rdfs:label "is typesystem of"@en .


###  http://w3id.org/meta-share/meta-share/isUsageProjectOf
ms:isUsageProjectOf rdf:type owl:ObjectProperty ;
                    rdfs:subPropertyOf ms:projectRelatedTo ;
                    owl:inverseOf ms:usageProject ;
                    rdfs:domain ms:Project ;
                    rdfs:range ms:ActualUse ;
                    rdfs:comment "Links a project where a language resource has been used to this LR"@en ;
                    rdfs:label "is usage project of"@en .


###  http://w3id.org/meta-share/meta-share/isValidatedBy
ms:isValidatedBy rdf:type owl:ObjectProperty ;
                 rdfs:subPropertyOf ms:isRelatedToLT ;
                 rdfs:domain ms:Validation ;
                 rdfs:range ms:ToolService ;
                 rdfs:comment "Links to a tool/service B that is (or can be) used for validating LR A (the one being described)"@en ;
                 rdfs:label "is validated by"@en ;
                 skos:altLabel "validation tool"@en .


###  http://w3id.org/meta-share/meta-share/isValidatorOf
ms:isValidatorOf rdf:type owl:ObjectProperty ;
                 rdfs:subPropertyOf ms:actorRelatedTo ;
                 owl:inverseOf ms:validator ;
                 rdfs:domain ms:Actor ;
                 rdfs:range ms:Validation ;
                 rdfs:comment "Links person(s), group(s) or organization(s) that have performed a specific validation of a language resource to the data of this validation"@en ;
                 rdfs:label "is validator of"@en .


###  http://w3id.org/meta-share/meta-share/isVersionOf
ms:isVersionOf rdf:type owl:ObjectProperty ;
               rdfs:subPropertyOf ms:isRelatedToLR ;
               rdfs:domain ms:LanguageResource ;
               rdfs:range ms:LanguageResource ;
               rdfs:comment "Links to LR B that is a version (corrected, annotated, enriched, processed, etc.) of LR A (the one being described)"@en ;
               rdfs:label "is version of"@en .


###  http://w3id.org/meta-share/meta-share/languageVariety
ms:languageVariety rdf:type owl:ObjectProperty ;
                   rdfs:domain [ rdf:type owl:Class ;
                                 owl:unionOf ( ms:CorpusAudioPart
                                               ms:CorpusImagePart
                                               ms:CorpusTextPart
                                               ms:CorpusVideoPart
                                               ms:LanguageDescriptionImagePart
                                               ms:LanguageDescriptionTextPart
                                               ms:LanguageDescriptionVideoPart
                                               ms:LexicalConceptualResourceAudioPart
                                               ms:LexicalConceptualResourceImagePart
                                               ms:LexicalConceptualResourceTextPart
                                               ms:LexicalConceptualResourceVideoPart
                                             )
                               ] ;
                   rdfs:range ms:LanguageVariety ;
                   rdfs:comment "Relates a language resource that contains segments in a language variety (e.g., dialect, jargon) to it"@en ;
                   rdfs:label "language variety"@en ;
                   skos:note "in MS we have language variety attached to language; check if this is ok; introduce a class Language after deciding on how to treat languages"@en .


###  http://w3id.org/meta-share/meta-share/languageVarietyType
ms:languageVarietyType rdf:type owl:ObjectProperty ;
                       rdfs:domain ms:LanguageVariety ;
                       rdfs:range ms:LanguageVarietyType ;
                       rdfs:comment "Specifies the type of the language variety"@en ;
                       rdfs:label "language variety type"@en .


###  http://w3id.org/meta-share/meta-share/lcrSubclass
ms:lcrSubclass rdf:type owl:ObjectProperty ;
               rdfs:domain ms:LexicalConceptualResource ;
               rdfs:range ms:LCRSubclass ;
               rdfs:comment "Introduces a classification of lexical/conceptual resources into types (used for descriptive reasons)"@en ;
               rdfs:label "LCR subclass"@en .


###  http://w3id.org/meta-share/meta-share/ldSubclass
ms:ldSubclass rdf:type owl:ObjectProperty ;
              rdfs:domain ms:LanguageDescription ;
              rdfs:range ms:LDSubclass ;
              rdfs:comment "A classification of language descriptions into models, grammars etc."@en ;
              rdfs:label "Language Description subclass"@en .


###  http://w3id.org/meta-share/meta-share/ldTask
ms:ldTask rdf:type owl:ObjectProperty ;
          rdfs:domain ms:LanguageDescription ;
          rdfs:range ms:LDTask ;
          rdfs:comment "Specifies the task performed by the language description"@en ;
          rdfs:label "language description task"@en .


###  http://w3id.org/meta-share/meta-share/licenceCategory
ms:licenceCategory rdf:type owl:ObjectProperty ;
                   rdfs:domain ms:LicenceTerms ;
                   rdfs:range ms:LicenceCategory ;
                   rdfs:comment "Categorises a licence according to a classification scheme"@en ;
                   rdfs:label "licence category"@en .


###  http://w3id.org/meta-share/meta-share/licenceTerms
ms:licenceTerms rdf:type owl:ObjectProperty ;
                rdfs:subPropertyOf dct:license ;
                rdfs:domain ms:Distribution ;
                rdfs:range ms:LicenceTerms ;
                rdfs:comment "Links the distribution (distributable form) of a language resource to the licence or terms of use/service (a specific legal document) with which it is distributed"@en ;
                rdfs:label "licence"@en .


###  http://w3id.org/meta-share/meta-share/licensor
ms:licensor rdf:type owl:ObjectProperty ;
            rdfs:subPropertyOf ms:isRelatedToActor ;
            rdfs:domain ms:Distribution ;
            rdfs:range ms:Person ;
            rdfs:comment "The person or organisation who is legally eligible to license and actually licenses the resource. The licensor could be different from the creator, the distributor or the IPR holder. The licensor has the necessary rights or licences to license the work and is the party that actually licenses the resource that is distributed via the specific channel. She will have obtained the necessary rights or licences from the IPR holder and she may have a distribution agreement with a distributor that disseminates the work under a set of conditions defined in the specific licence and collects revenue on the licensor's behalf. The attribution of the creator, separately from the attribution of the licensor, may be part of the licence under which the resource is distributed (as e.g., is the case with Creative Commons Licences)."@en ;
            rdfs:label "licensor"@en .


###  http://w3id.org/meta-share/meta-share/lingualityType
ms:lingualityType rdf:type owl:ObjectProperty ;
                  rdfs:domain ms:MediaPart ;
                  rdfs:range ms:LingualityType ;
                  rdfs:comment "Indicates whether the resource includes one, two or more languages"@en ;
                  rdfs:label "linguality type"@en .


###  http://w3id.org/meta-share/meta-share/linguisticInformation
ms:linguisticInformation rdf:type owl:ObjectProperty ;
                         rdfs:domain ms:LexicalConceptualResource ;
                         rdfs:range [ owl:intersectionOf ( skos:Concept
                                                           [ rdf:type owl:Restriction ;
                                                             owl:onProperty skos:inScheme ;
                                                             owl:hasValue ms:ContentTypeScheme
                                                           ]
                                                         ) ;
                                      rdf:type owl:Class
                                    ] ;
                         rdfs:comment "Provides a more detailed account of the linguistic information contained in the lexical/conceptual resource"@en ;
                         rdfs:label "linguistic information"@en .


###  http://w3id.org/meta-share/meta-share/linkToOtherMedia
ms:linkToOtherMedia rdf:type owl:ObjectProperty ;
                    rdfs:domain [ rdf:type owl:Class ;
                                  owl:unionOf ( ms:CorpusMediaPart
                                                ms:LanguageDescriptionMediaPart
                                              )
                                ] ;
                    rdfs:range ms:LinkToOtherMedia ;
                    rdfs:comment "Describes the linking between different media parts of a resource (how they interact with or link to each other)"@en ;
                    rdfs:label "link to other media"@en .


###  http://w3id.org/meta-share/meta-share/mediaPart
ms:mediaPart rdf:type owl:ObjectProperty ;
             rdfs:domain ms:LanguageResource ;
             rdfs:range ms:MediaPart ;
             rdfs:comment "Links a language resource to the parts it consists of (e.g., an oral corpus with the audio and its transcribed text part)"@en ;
             rdfs:label "media part"@en .


###  http://w3id.org/meta-share/meta-share/mediaType
ms:mediaType rdf:type owl:ObjectProperty ;
             rdfs:domain [ rdf:type owl:Class ;
                           owl:unionOf ( ms:MediaPart
                                         ms:ProcessingResourceType
                                       )
                         ] ;
             rdfs:range ms:MediaType ;
             rdfs:comment "Specifies the media type of a language resource (the physical medium of the contents representation) or of the input/output of a language processing tool/service; each media type is described through a distinctive set of technical features; a language resource may consist of different media parts"@en ;
             rdfs:label "media type"@en .


###  http://w3id.org/meta-share/meta-share/memberOfAssociation
ms:memberOfAssociation rdf:type owl:ObjectProperty ;
                       rdfs:domain [ rdf:type owl:Class ;
                                     owl:unionOf ( ms:Division
                                                   ms:Organization
                                                   ms:Person
                                                 )
                                   ] ;
                       rdfs:range ms:Organization ;
                       rdfs:comment "Links to an association or network that the organization or person is member of"@en ;
                       rdfs:label "member of association"@en .


###  http://w3id.org/meta-share/meta-share/membershipInstitution
ms:membershipInstitution rdf:type owl:ObjectProperty ;
                         rdfs:domain ms:Distribution ;
                         rdfs:range ms:MembershipInstitution ;
                         rdfs:comment "Introduces an institution with members that can benefit from specific conditions on the use of a resource (e.g. discount, unlimited access, etc.)"@en ;
                         rdfs:label "membership institution"@en .


###  http://w3id.org/meta-share/meta-share/metadataCreator
ms:metadataCreator rdf:type owl:ObjectProperty ;
                   rdfs:subPropertyOf ms:isRelatedToActor ;
                   rdfs:domain ms:MetadataRecord ;
                   rdfs:range ms:Person ;
                   rdfs:comment "Introduces the person who has created the metadata record"@en ;
                   rdfs:label "metadata creator"@en .


###  http://w3id.org/meta-share/meta-share/metadataCurator
ms:metadataCurator rdf:type owl:ObjectProperty ;
                   rdfs:subPropertyOf ms:isRelatedToActor ;
                   rdfs:domain ms:MetadataRecord ;
                   rdfs:range ms:Person ;
                   rdfs:comment "A person responsible for the creation, update, enrichment, etc. of a metadata record describing an entity"@en ;
                   rdfs:label "metadata curator"@en .


###  http://w3id.org/meta-share/meta-share/method
ms:method rdf:type owl:ObjectProperty ;
          rdfs:domain [ rdf:type owl:Class ;
                        owl:unionOf ( ms:MLModel
                                      ms:ToolService
                                    )
                      ] ;
          rdfs:range [ owl:intersectionOf ( skos:Concept
                                            [ rdf:type owl:Restriction ;
                                              owl:onProperty skos:inScheme ;
                                              owl:hasValue omtd:TdmMethodScheme
                                            ]
                                          ) ;
                       rdf:type owl:Class
                     ] ;
          rdfs:comment "Specifies the method used for the development of a tool/service or the ML model"@en ;
          rdfs:label "method"@en .


###  http://w3id.org/meta-share/meta-share/metric
ms:metric rdf:type owl:ObjectProperty ;
          rdfs:domain ms:PerformanceIndicator ;
          rdfs:range ms:Metric ;
          rdfs:comment "Identifies the metric used for the evaluation of the tool/service"@en ;
          rdfs:label "metric"@en .


###  http://w3id.org/meta-share/meta-share/mimetype
ms:mimetype rdf:type owl:ObjectProperty ;
            rdfs:domain [ rdf:type owl:Class ;
                          owl:unionOf ( ms:DatasetDistribution
                                        ms:DistributionAudioFeature
                                        ms:DistributionImageFeature
                                        ms:DistributionTextFeature
                                        ms:DistributionTextNumericalFeature
                                        ms:DistributionVideoFeature
                                        ms:ProcessingResource
                                      )
                        ] ;
            rdfs:range dct:MediaType ;
            rdfs:comment "The format of the resource expressed with one of the values from the IANA mimetypes (https://www.iana.org/assignments/media-types/media-types.xhtml)."@en ;
            rdfs:label "format (as mimetype value)"@en .


###  http://w3id.org/meta-share/meta-share/mlFramework1
ms:mlFramework1 rdf:type owl:ObjectProperty ;
                rdfs:domain [ rdf:type owl:Class ;
                              owl:unionOf ( ms:MLModel
                                            ms:ToolService
                                          )
                            ] ;
                rdfs:range ms:MLFramework ;
                dct:replaces ms:mlFramework ;
                rdfs:comment "Specifies the framework that has been used for developing a model (e.g. keras, tensorflow, etc.)"@en ;
                rdfs:label "ML framework"@en ;
                skos:altLabel "Machine Learning framework"@en .


###  http://w3id.org/meta-share/meta-share/mlModel
ms:mlModel rdf:type owl:ObjectProperty ;
           rdfs:subPropertyOf ms:dependsOn ;
           rdfs:domain ms:ToolService ;
           rdfs:range ms:Model ;
           rdfs:comment "Specifies the ML model that must be used together with the tool/service to perform the desired task"@en ;
           rdfs:label "ML model"@en .


###  http://w3id.org/meta-share/meta-share/modalityType
ms:modalityType rdf:type owl:ObjectProperty ;
                rdfs:domain ms:MediaPart ;
                rdfs:range ms:ModalityType ;
                rdfs:comment "Specifies the type of the modality represented in the resource or processed by a tool/service"@en ;
                rdfs:label "modality type"@en .


###  http://w3id.org/meta-share/meta-share/modelFunction
ms:modelFunction rdf:type owl:ObjectProperty ;
                 rdfs:domain ms:Model ;
                 rdfs:range [ owl:intersectionOf ( skos:Concept
                                                   [ rdf:type owl:Restriction ;
                                                     owl:onProperty skos:inScheme ;
                                                     owl:hasValue omtd:ModelFunctionScheme
                                                   ]
                                                 ) ;
                              rdf:type owl:Class
                            ] ;
                 rdfs:comment "The function/task/operation a model performs"@en ;
                 rdfs:label "model function"@en .


###  http://w3id.org/meta-share/meta-share/modelType
ms:modelType rdf:type owl:ObjectProperty ;
             rdfs:domain ms:Model ;
             rdfs:range ms:ModelType ;
             rdfs:comment "A classificaiton of models based on their algorithm"@en ;
             rdfs:label "model type"@en .


###  http://w3id.org/meta-share/meta-share/multilingualityType
ms:multilingualityType rdf:type owl:ObjectProperty ;
                       rdfs:domain ms:MediaPart ;
                       rdfs:range ms:MultilingualityType ;
                       rdfs:comment "Indicates whether the resource (part) is parallel, comparable or mixed"@en ;
                       rdfs:label "multilinguality type"@en .


###  http://w3id.org/meta-share/meta-share/nationalMaxContribution
ms:nationalMaxContribution rdf:type owl:ObjectProperty ;
                           rdfs:domain ms:Project ;
                           rdfs:range ms:Cost ;
                           rdfs:comment "Introduces the maximum amount of money contributed from national funds"@en ;
                           rdfs:label "national max contribution"@en .


###  http://w3id.org/meta-share/meta-share/naturality
ms:naturality rdf:type owl:ObjectProperty ;
              rdfs:domain [ rdf:type owl:Class ;
                            owl:unionOf ( ms:CorpusAudioPart
                                          ms:CorpusVideoPart
                                        )
                          ] ;
              rdfs:range ms:Naturality ;
              rdfs:comment "Specifies the level of naturality for multimodal/multimedia resources"@en ;
              rdfs:label "naturality"@en .


###  http://w3id.org/meta-share/meta-share/noiseLevel
ms:noiseLevel rdf:type owl:ObjectProperty ;
              rdfs:domain [ rdf:type owl:Class ;
                            owl:unionOf ( ms:CorpusAudioPart
                                          ms:LexicalConceptualResourceAudioPart
                                        )
                          ] ;
              rdfs:range ms:NoiseLevel ;
              rdfs:comment "Specifies the level of background noise"@en ;
              rdfs:label "noise level"@en .


###  http://w3id.org/meta-share/meta-share/nonSpeechItem
ms:nonSpeechItem rdf:type owl:ObjectProperty ;
                 rdfs:domain [ rdf:type owl:Class ;
                               owl:unionOf ( ms:CorpusAudioPart
                                             ms:LexicalConceptualResourceAudioPart
                                           )
                             ] ;
                 rdfs:range ms:NonSpeechItem ;
                 rdfs:comment "Specifies the distinct non-speech elements that maybe included in the audio part of a corpus or lexical/conceptual resource"@en ;
                 rdfs:label "non-speech item"@en .


###  http://w3id.org/meta-share/meta-share/operatingSystem
ms:operatingSystem rdf:type owl:ObjectProperty ;
                   rdfs:domain ms:ToolService ;
                   rdfs:range ms:OperatingSystem ;
                   rdfs:comment "Specifies the operating system on which a software object can run"@en ;
                   rdfs:label "operating system"@en .


###  http://w3id.org/meta-share/meta-share/organizationLegalStatus
ms:organizationLegalStatus rdf:type owl:ObjectProperty ;
                           rdfs:domain ms:Organization ;
                           rdfs:range ms:OrganizationLegalStatus ;
                           rdfs:comment "Classifies an organization according to its legal status"@en ;
                           rdfs:label "organization legal status"@en .


###  http://w3id.org/meta-share/meta-share/organizationRole
ms:organizationRole rdf:type owl:ObjectProperty ;
                    rdfs:domain [ rdf:type owl:Class ;
                                  owl:unionOf ( ms:Division
                                                ms:Group
                                                ms:Organization
                                              )
                                ] ;
                    rdfs:range ms:OrganizationRole ;
                    rdfs:comment "Classifies an organization according to its role/mission"@en ;
                    rdfs:label "organization role"@en .


###  http://w3id.org/meta-share/meta-share/origin
ms:origin rdf:type owl:ObjectProperty ;
          rdfs:domain ms:Participant ;
          rdfs:range ms:Origin ;
          rdfs:comment "Specifies the relation of the language of a participant with respect to the acquisition stage"@en ;
          rdfs:label "origin"@en .


###  http://w3id.org/meta-share/meta-share/originOfParticipants
ms:originOfParticipants rdf:type owl:ObjectProperty ;
                        rdfs:domain [ rdf:type owl:Class ;
                                      owl:unionOf ( ms:CorpusAudioPart
                                                    ms:CorpusImagePart
                                                    ms:CorpusTextNumericalPart
                                                    ms:CorpusVideoPart
                                                  )
                                    ] ;
                        rdfs:range ms:Origin ;
                        rdfs:comment "Specifies the relation of the language of the group of participants with respect to the acquisition stage"@en ;
                        rdfs:label "origin of participants"@en .


###  http://w3id.org/meta-share/meta-share/otherMedia
ms:otherMedia rdf:type owl:ObjectProperty ;
              rdfs:domain ms:LinkToOtherMedia ;
              rdfs:range ms:MediaType ;
              rdfs:comment "Specifies the media types that are linked to the media type described within the same resource"@en ;
              rdfs:label "other media"@en .


###  http://w3id.org/meta-share/meta-share/otherOfficeAddress
ms:otherOfficeAddress rdf:type owl:ObjectProperty ;
                      rdfs:subPropertyOf ms:addressSet ;
                      rdfs:domain [ rdf:type owl:Class ;
                                    owl:unionOf ( ms:Affiliation
                                                  ms:Division
                                                  ms:Group
                                                  ms:Organization
                                                )
                                  ] ;
                      rdfs:range ms:AddressSet ;
                      rdfs:comment "Links to the physical address of an office (other than the principal one) of an organization or group represented as a set of distinct elements (street, zip code, city, etc.)"@en ;
                      rdfs:label "address (other offices)"@en .


###  http://w3id.org/meta-share/meta-share/outputResource
ms:outputResource rdf:type owl:ObjectProperty ;
                  rdfs:domain ms:ToolService ;
                  rdfs:range ms:ProcessingResource ;
                  rdfs:comment "Specifies the output results of a tool/service, i.e. the features of the processed (content) resource"@en ;
                  rdfs:label "output resource"@en .


###  http://w3id.org/meta-share/meta-share/packageFormat
ms:packageFormat rdf:type owl:ObjectProperty ;
                 rdfs:domain [ rdf:type owl:Class ;
                               owl:unionOf ( ms:DatasetDistribution
                                             ms:SoftwareDistribution
                                           )
                             ] ;
                 rdfs:range omtd:PackageFormat ;
                 rdfs:comment "Specifies the format of the package (zipped file) that contains the resource files"@en ;
                 rdfs:label "package format"@en .


###  http://w3id.org/meta-share/meta-share/parameter
ms:parameter rdf:type owl:ObjectProperty ;
             rdfs:domain ms:ToolService ;
             rdfs:range ms:Parameter ;
             rdfs:comment "Introduces a parameter used for running a tool/service"@en ;
             rdfs:label "parameter"@en .


###  http://w3id.org/meta-share/meta-share/parameterType
ms:parameterType rdf:type owl:ObjectProperty ;
                 rdfs:domain ms:Parameter ;
                 rdfs:range ms:ParameterType ;
                 rdfs:comment "Classifies the parameter according to a specific (not yet standardised) typing system (e.g., whether it's boolean, string, integer, a document, mapping, etc.)"@en ;
                 rdfs:label "parameter type"@en .


###  http://w3id.org/meta-share/meta-share/participant
ms:participant rdf:type owl:ObjectProperty ;
               rdfs:domain [ rdf:type owl:Class ;
                             owl:unionOf ( ms:CorpusAudioPart
                                           ms:CorpusImagePart
                                           ms:CorpusTextNumericalPart
                                           ms:CorpusVideoPart
                                         )
                           ] ;
               rdfs:range ms:Participant ;
               rdfs:comment "Introduces descriptive characteristics of a person that has participated in the audio, video, sensorimotor (textNumerical) part of the resource"@en ;
               rdfs:label "participant"@en .


###  http://w3id.org/meta-share/meta-share/participatingOrganization
ms:participatingOrganization rdf:type owl:ObjectProperty ;
                             rdfs:subPropertyOf ms:isRelatedToActor ;
                             rdfs:domain ms:Project ;
                             rdfs:range ms:Organization ;
                             rdfs:comment "Indicates the organization(s) that participate (or have participated) in a project"@en ;
                             rdfs:label "participating organization"@en .


###  http://w3id.org/meta-share/meta-share/performanceIndicator
ms:performanceIndicator rdf:type owl:ObjectProperty ;
                        rdfs:domain ms:Evaluation ;
                        rdfs:range ms:PerformanceIndicator ;
                        rdfs:comment "Describes the performance indicator used for the evaluation of a tool/service"@en ;
                        rdfs:label "performance indicator"@en .


###  http://w3id.org/meta-share/meta-share/personalDataIncluded
ms:personalDataIncluded rdf:type owl:ObjectProperty ;
                        rdfs:domain ms:DataLanguageResource ;
                        rdfs:range ms:PersonalDataIncluded ;
                        rdfs:comment "Specifies whether the language resource contains personal data (mainly in the sense falling under the GDPR)"@en ;
                        rdfs:label "personal data included"@en .


###  http://w3id.org/meta-share/meta-share/pivotLanguage
ms:pivotLanguage rdf:type owl:ObjectProperty ;
                 rdfs:domain [ rdf:type owl:Class ;
                               owl:unionOf ( ms:CorpusAudioPart
                                             ms:CorpusImagePart
                                             ms:CorpusTextPart
                                             ms:CorpusVideoPart
                                             ms:LanguageDescriptionImagePart
                                             ms:LanguageDescriptionTextPart
                                             ms:LanguageDescriptionVideoPart
                                             ms:LexicalConceptualResourceAudioPart
                                             ms:LexicalConceptualResourceImagePart
                                             ms:LexicalConceptualResourceTextPart
                                             ms:LexicalConceptualResourceVideoPart
                                           )
                             ] ;
                 rdfs:range dct:LinguisticSystem ;
                 rdfs:comment "The language acting as an intermediary for translations between many languages"@en ;
                 rdfs:label "pivot language"@en .


###  http://w3id.org/meta-share/meta-share/previousAnnotationTypesPolicy
ms:previousAnnotationTypesPolicy rdf:type owl:ObjectProperty ;
                                 rdfs:domain ms:ToolService ;
                                 rdfs:range ms:PreviousAnnotationTypesPolicy ;
                                 rdfs:comment "Specifies the policy that a tool/service has with respect to the annotation types included in the annotated resource that it takes as input (i.e. whether it keeps, modifies or drops them in the output resource)"@en ;
                                 rdfs:label "previous annotation types policy"@en .


###  http://w3id.org/meta-share/meta-share/processMode
ms:processMode rdf:type owl:ObjectProperty ;
               rdfs:domain owl:Thing ;
               rdfs:range ms:ProcessMode ;
               rdfs:comment "Specifies the type of processing performed on a language resource"@en ;
               rdfs:label "process mode"@en .


###  http://w3id.org/meta-share/meta-share/processingResourceType
ms:processingResourceType rdf:type owl:ObjectProperty ;
                          rdfs:domain ms:ProcessingResource ;
                          rdfs:range ms:ProcessingResourceType ;
                          rdfs:comment "Specifies the resource type that a tool/service takes as input or produces as output"@en ;
                          rdfs:label "processing resource type"@en .


###  http://w3id.org/meta-share/meta-share/projectRelatedTo
ms:projectRelatedTo rdf:type owl:ObjectProperty ;
                    rdfs:subPropertyOf ms:isRelatedTo ;
                    rdfs:domain ms:Project ;
                    rdfs:range ms:LanguageResource ;
                    rdfs:comment "Links a project to the language resource(s) it has some relation with (e.g., funded the creation of)"@en ;
                    rdfs:label "project related to"@en .


###  http://w3id.org/meta-share/meta-share/qualifiedAttribution
ms:qualifiedAttribution rdf:type owl:ObjectProperty ;
                        rdfs:domain ms:LanguageResource ;
                        rdfs:range ms:Attribution ;
                        rdfs:comment "Used for relations to agents not covered by the classic relations (e.g., funders, contributors, etc.)"@en ;
                        rdfs:label "attribution"@en .


###  http://w3id.org/meta-share/meta-share/quality
ms:quality rdf:type owl:ObjectProperty ;
           rdfs:domain ms:ImageFormat ;
           rdfs:range ms:Quality ;
           rdfs:comment "Specifies the quality level of image resource"@en ;
           rdfs:label "quality"@en .


###  http://w3id.org/meta-share/meta-share/queries
ms:queries rdf:type owl:ObjectProperty ;
           rdfs:subPropertyOf ms:LΤRelatedTo ;
           rdfs:domain ms:ToolService ;
           rdfs:range ms:DataLanguageResource ;
           rdfs:comment "Links a tool/service B that is (or can be) used for querying LR A to LR A"@en ;
           rdfs:label "queries"@en .


###  http://w3id.org/meta-share/meta-share/rasterOrVectorGraphics
ms:rasterOrVectorGraphics rdf:type owl:ObjectProperty ;
                          rdfs:domain ms:ImageFormat ;
                          rdfs:range ms:RasterOrVectorGraphics ;
                          rdfs:comment "Indicates if the image is stored as raster or vector graphics"@en ;
                          rdfs:label "raster or vector graphics"@en .


###  http://w3id.org/meta-share/meta-share/recorder
ms:recorder rdf:type owl:ObjectProperty ;
            rdfs:subPropertyOf ms:isRelatedToActor ;
            rdfs:domain [ rdf:type owl:Class ;
                          owl:unionOf ( ms:CorpusAudioPart
                                        ms:CorpusTextNumericalPart
                                        ms:CorpusVideoPart
                                      )
                        ] ;
            rdfs:range ms:Actor ;
            rdfs:comment "Links to the recorder(s) of the audio or video part of the resource"@en ;
            rdfs:label "recorder"@en .


###  http://w3id.org/meta-share/meta-share/recordingDeviceType
ms:recordingDeviceType rdf:type owl:ObjectProperty ;
                       rdfs:domain [ rdf:type owl:Class ;
                                     owl:unionOf ( ms:CorpusAudioPart
                                                   ms:CorpusTextNumericalPart
                                                   ms:CorpusVideoPart
                                                 )
                                   ] ;
                       rdfs:range ms:RecordingDeviceType ;
                       rdfs:comment "Specifies the nature of the recording platform hardware and the storage medium"@en ;
                       rdfs:label "recording device type"@en .


###  http://w3id.org/meta-share/meta-share/recordingEnvironment
ms:recordingEnvironment rdf:type owl:ObjectProperty ;
                        rdfs:domain [ rdf:type owl:Class ;
                                      owl:unionOf ( ms:CorpusAudioPart
                                                    ms:CorpusTextNumericalPart
                                                    ms:CorpusVideoPart
                                                  )
                                    ] ;
                        rdfs:range ms:RecordingEnvironment ;
                        rdfs:comment "Specifies where the recording took place"@en ;
                        rdfs:label "recording environment"@en .


###  http://w3id.org/meta-share/meta-share/recordingQuality
ms:recordingQuality rdf:type owl:ObjectProperty ;
                    rdfs:domain ms:AudioFormat ;
                    rdfs:range ms:RecordingQuality ;
                    rdfs:comment "Indicates the audio or video recording quality"@en ;
                    rdfs:label "recording quality"@en .


###  http://w3id.org/meta-share/meta-share/relatedLR
ms:relatedLR rdf:type owl:ObjectProperty ;
             rdfs:domain ms:Relation ;
             rdfs:range ms:LanguageResource ;
             rdfs:comment "Identifies the language resource with which a relation is holding with the one being described"@en ;
             rdfs:label "related language resource"@en .


###  http://w3id.org/meta-share/meta-share/relatedLexiconType
ms:relatedLexiconType rdf:type owl:ObjectProperty ;
                      rdfs:domain ms:LanguageDescription ;
                      rdfs:range ms:RelatedLexiconType ;
                      rdfs:comment "Indicates the type of the lexica that must or can be used with the grammar"@en ;
                      rdfs:label "related lexicon type"@en .


###  http://w3id.org/meta-share/meta-share/relation
ms:relation rdf:type owl:ObjectProperty ;
            rdfs:domain ms:LanguageResource ;
            rdfs:range ms:Relation ;
            rdfs:comment "Links a language resource to other related resources specifying also the type of relation"@en ;
            rdfs:label "relation"@en .


###  http://w3id.org/meta-share/meta-share/replaces
ms:replaces rdf:type owl:ObjectProperty ;
            rdfs:subPropertyOf ms:isVersionOf ;
            rdfs:domain ms:LanguageResource ;
            rdfs:range ms:LanguageResource ;
            rdfs:comment "Links to LR B that is an older version of LR A (the one being described) and has been replaced by it"@en ;
            rdfs:label "replaces"@en .


###  http://w3id.org/meta-share/meta-share/replacesOrganization
ms:replacesOrganization rdf:type owl:ObjectProperty ;
                        rdfs:domain ms:Organization ;
                        rdfs:range ms:Organization ;
                        rdfs:comment "Specified an organization that has been replaced by the organization which is described (e.g. following a merge or acquisition action)"@en ;
                        rdfs:label "replaces organization"@en .


###  http://w3id.org/meta-share/meta-share/replacesProject
ms:replacesProject rdf:type owl:ObjectProperty ;
                   rdfs:domain ms:Project ;
                   rdfs:range ms:Project ;
                   rdfs:comment "Specifies a project that has been replaced by the project described"@en ;
                   rdfs:label "Replaces project"@en .


###  http://w3id.org/meta-share/meta-share/requiredHardware
ms:requiredHardware rdf:type owl:ObjectProperty ;
                    rdfs:domain [ rdf:type owl:Class ;
                                  owl:unionOf ( ms:LanguageDescription
                                                ms:ToolService
                                              )
                                ] ;
                    rdfs:range ms:RequiredHardware ;
                    rdfs:comment "Specifies the type of hardware required for running a tool and/or computational grammar"@en ;
                    rdfs:label "required hardware"@en .


###  http://w3id.org/meta-share/meta-share/requiresLR
ms:requiresLR rdf:type owl:ObjectProperty ;
              rdfs:subPropertyOf ms:dependsOn ;
              rdfs:domain [ rdf:type owl:Class ;
                            owl:unionOf ( ms:LanguageDescription
                                          ms:ProcessingResource
                                          ms:ToolService
                                        )
                          ] ;
              rdfs:range [ rdf:type owl:Class ;
                           owl:unionOf ( ms:LanguageDescription
                                         ms:LexicalConceptualResource
                                       )
                         ] ;
              rdfs:comment "Links to LR B that is required for the operation of a tool/service or computational grammar (the one that is described)"@en ;
              rdfs:label "requires language resource"@en .


###  http://w3id.org/meta-share/meta-share/resolution
ms:resolution rdf:type owl:ObjectProperty ;
              rdfs:domain [ rdf:type owl:Class ;
                            owl:unionOf ( ms:ImageFormat
                                          ms:VideoFormat
                                        )
                          ] ;
              rdfs:range ms:Resolution ;
              rdfs:comment "Groups together information on the image resolution"@en ;
              rdfs:label "resolution"@en .


###  http://w3id.org/meta-share/meta-share/resolutionStandard
ms:resolutionStandard rdf:type owl:ObjectProperty ;
                      rdfs:domain ms:Resolution ;
                      rdfs:range ms:ResolutionStandard ;
                      rdfs:comment "Specifies the standard to which the resolution conforms"@en ;
                      rdfs:label "resolution standard"@en .


###  http://w3id.org/meta-share/meta-share/resourceCreator
ms:resourceCreator rdf:type owl:ObjectProperty ;
                   rdfs:subPropertyOf ms:isRelatedToActor ;
                   rdfs:domain ms:LanguageResource ;
                   rdfs:range ms:Actor ;
                   rdfs:comment "Links a resource to the person, group or organisation that has created the resource"@en ;
                   rdfs:label "resource creator"@en .


###  http://w3id.org/meta-share/meta-share/resourceProvider
ms:resourceProvider rdf:type owl:ObjectProperty ;
                    rdfs:subPropertyOf ms:isRelatedToActor ;
                    rdfs:domain ms:LanguageResource ;
                    rdfs:range ms:Actor ;
                    rdfs:comment "The person/organization responsible for providing, curating, maintaining and making available (publishing) the resource"@en ;
                    rdfs:label "resource provider"@en .


###  http://w3id.org/meta-share/meta-share/reviews
ms:reviews rdf:type owl:ObjectProperty ;
           rdfs:subPropertyOf ms:documents ;
           rdfs:domain ms:Document ;
           rdfs:range ms:LanguageResource ;
           rdfs:comment "Links a document to the language resource it reviews"@en ;
           rdfs:label "reviews"@en .


###  http://w3id.org/meta-share/meta-share/sample
ms:sample rdf:type owl:ObjectProperty ;
          rdfs:domain ms:ProcessingResource ;
          rdfs:range ms:Sample ;
          rdfs:comment "Introduces a combination of the sample text(s) or sample file(s) and optional tags that can be used for feeding a processing service for testing purposes"@en ;
          rdfs:label "sample"@en .


###  http://w3id.org/meta-share/meta-share/scenarioType
ms:scenarioType rdf:type owl:ObjectProperty ;
                rdfs:domain [ rdf:type owl:Class ;
                              owl:unionOf ( ms:CorpusAudioPart
                                            ms:CorpusVideoPart
                                          )
                            ] ;
                rdfs:range ms:ScenarioType ;
                rdfs:comment "Indicates the task defined for the conversation or the interaction of participants"@en ;
                rdfs:label "scenario type"@en .


###  http://w3id.org/meta-share/meta-share/sceneIllumination
ms:sceneIllumination rdf:type owl:ObjectProperty ;
                     rdfs:domain [ rdf:type owl:Class ;
                                   owl:unionOf ( ms:CorpusAudioPart
                                                 ms:CorpusImagePart
                                                 ms:CorpusTextNumericalPart
                                                 ms:CorpusVideoPart
                                               )
                                 ] ;
                     rdfs:range ms:SceneIllumination ;
                     rdfs:comment "Provides information on the illumination of the scene"@en ;
                     rdfs:label "scene illumination"@en ;
                     skos:note "needed for audio?"@en .


###  http://w3id.org/meta-share/meta-share/segmentationLevel
ms:segmentationLevel rdf:type owl:ObjectProperty ;
                     rdfs:domain ms:Annotation ;
                     rdfs:range ms:SegmentationLevel ;
                     rdfs:comment "Specifies the segmentation unit in terms of which the resource has been segmented or the level of segmentation a tool/service requires/outputs"@en ;
                     rdfs:label "segmentation level"@en .


###  http://w3id.org/meta-share/meta-share/sensitiveDataIncluded
ms:sensitiveDataIncluded rdf:type owl:ObjectProperty ;
                         rdfs:domain ms:DataLanguageResource ;
                         rdfs:range ms:SensitiveDataIncluded ;
                         rdfs:comment "Specifies whether the language resource contains sensitive data (e.g., medical/health-related, etc.) and thus requires special handling"@en ;
                         rdfs:label "sensitive data included"@en .


###  http://w3id.org/meta-share/meta-share/sex
ms:sex rdf:type owl:ObjectProperty ;
       rdfs:domain ms:Participant ;
       rdfs:range ms:Sex ;
       rdfs:comment "Specifies the sex of a participant (either of the two major forms of individuals that occur in many species and that are distinguished respectively as female or male especially on the basis of their reproductive organs and structures [https://www.merriam-webster.com/dictionary/sex])"@en ;
       rdfs:label "sex"@en ;
       skos:note "check with sociologists?"@en .


###  http://w3id.org/meta-share/meta-share/sexOfParticipants
ms:sexOfParticipants rdf:type owl:ObjectProperty ;
                     rdfs:domain [ rdf:type owl:Class ;
                                   owl:unionOf ( ms:CorpusAudioPart
                                                 ms:CorpusImagePart
                                                 ms:CorpusTextNumericalPart
                                                 ms:CorpusVideoPart
                                               )
                                 ] ;
                     rdfs:range ms:SexOfParticipants ;
                     rdfs:comment "Specifies the sex of the participants (either of the two major forms of individuals that occur in many species and that are distinguished respectively as female or male especially on the basis of their reproductive organs and structures [https://www.merriam-webster.com/dictionary/sex])"@en ;
                     rdfs:label "sex of participants"@en ;
                     skos:note "check with sociologists?"@en .


###  http://w3id.org/meta-share/meta-share/signConvention
ms:signConvention rdf:type owl:ObjectProperty ;
                  rdfs:domain ms:AudioFormat ;
                  rdfs:range ms:SignConvention ;
                  rdfs:comment "Indicates the binary representation of numbers"@en ;
                  rdfs:label "sign convention"@en .


###  http://w3id.org/meta-share/meta-share/signalEncoding
ms:signalEncoding rdf:type owl:ObjectProperty ;
                  rdfs:domain ms:CorpusAudioPart ;
                  rdfs:range ms:SignalEncoding ;
                  rdfs:comment "Specifies the encoding the audio type uses"@en ;
                  rdfs:label "signal encoding"@en .


###  http://w3id.org/meta-share/meta-share/size
ms:size rdf:type owl:ObjectProperty ;
        rdfs:domain ms:DistributionTextFeature ,
                    [ rdf:type owl:Class ;
                      owl:unionOf ( ms:DistributionAudioFeature
                                    ms:DistributionImageFeature
                                    ms:DistributionTextFeature
                                    ms:DistributionTextNumericalFeature
                                    ms:DistributionVideoFeature
                                  )
                    ] ;
        rdfs:range ms:Size ;
        rdfs:comment "Specifies the size of a countable entity with regard to the SizeUnit measurement in form of a number"@en ;
        rdfs:label "size"@en .


###  http://w3id.org/meta-share/meta-share/sizePerAnnotation
ms:sizePerAnnotation rdf:type owl:ObjectProperty ;
                     rdfs:subPropertyOf ms:sizePerSubset ;
                     rdfs:range ms:Size ;
                     rdfs:comment "Provides information on size for the annotated parts of the resource"@en ;
                     rdfs:label "size per annotation"@en .


###  http://w3id.org/meta-share/meta-share/sizePerAudioClassification
ms:sizePerAudioClassification rdf:type owl:ObjectProperty ;
                              rdfs:subPropertyOf ms:sizePerSubset ;
                              rdfs:range ms:Size ;
                              rdfs:comment "The size of the audio subparts of the resource in terms of classification criteria"@en ;
                              rdfs:label "size per audio classification"@en .


###  http://w3id.org/meta-share/meta-share/sizePerAudioFormat
ms:sizePerAudioFormat rdf:type owl:ObjectProperty ;
                      rdfs:subPropertyOf ms:sizePerSubset ;
                      rdfs:range ms:Size ;
                      rdfs:comment "Used to give info on size of parts of a resource that differ as to the format"@en ;
                      rdfs:label "size per audio format"@en .


###  http://w3id.org/meta-share/meta-share/sizePerCharacterEncoding
ms:sizePerCharacterEncoding rdf:type owl:ObjectProperty ;
                            rdfs:subPropertyOf ms:sizePerSubset ;
                            rdfs:range ms:Size ;
                            rdfs:comment "Provides information on the size of the resource parts with different character encoding"@en ;
                            rdfs:label "size per character encoding"@en .


###  http://w3id.org/meta-share/meta-share/sizePerDomain
ms:sizePerDomain rdf:type owl:ObjectProperty ;
                 rdfs:subPropertyOf ms:sizePerSubset ;
                 rdfs:range ms:Size ;
                 rdfs:comment "Specifies the size of resource parts per domain"@en ;
                 rdfs:label "size per domain"@en .


###  http://w3id.org/meta-share/meta-share/sizePerGeographicCoverage
ms:sizePerGeographicCoverage rdf:type owl:ObjectProperty ;
                             rdfs:subPropertyOf ms:sizePerSubset ;
                             rdfs:range ms:Size ;
                             rdfs:comment "Provides information on size per geographically distinct section of the resource"@en ;
                             rdfs:label "size per geographic coverage"@en .


###  http://w3id.org/meta-share/meta-share/sizePerImageClassification
ms:sizePerImageClassification rdf:type owl:ObjectProperty ;
                              rdfs:subPropertyOf ms:sizePerSubset ;
                              rdfs:range ms:Size ;
                              rdfs:comment "Provides information on size of parts with different image classification"@en ;
                              rdfs:label "size per image classification"@en .


###  http://w3id.org/meta-share/meta-share/sizePerImageFormat
ms:sizePerImageFormat rdf:type owl:ObjectProperty ;
                      rdfs:subPropertyOf ms:sizePerSubset ;
                      rdfs:range ms:Size ;
                      rdfs:comment "Used to give info on size of parts of a resource that differ as to the format"@en ;
                      rdfs:label "size per image format"@en .


###  http://w3id.org/meta-share/meta-share/sizePerLanguage
ms:sizePerLanguage rdf:type owl:ObjectProperty ;
                   rdfs:subPropertyOf ms:sizePerSubset ;
                   rdfs:range ms:Size ;
                   rdfs:comment "Provides information on the size per language component"@en ;
                   rdfs:label "size per language"@en .


###  http://w3id.org/meta-share/meta-share/sizePerLanguageVariety
ms:sizePerLanguageVariety rdf:type owl:ObjectProperty ;
                          rdfs:subPropertyOf ms:sizePerSubset ;
                          rdfs:range ms:Size ;
                          rdfs:comment "Provides information on the size per language variety component"@en ;
                          rdfs:label "size per language variety"@en .


###  http://w3id.org/meta-share/meta-share/sizePerModality
ms:sizePerModality rdf:type owl:ObjectProperty ;
                   rdfs:subPropertyOf ms:sizePerSubset ;
                   rdfs:range ms:Size ;
                   rdfs:comment "Provides information on the size per modality component"@en ;
                   rdfs:label "size per modality"@en .


###  http://w3id.org/meta-share/meta-share/sizePerSubset
ms:sizePerSubset rdf:type owl:ObjectProperty ;
                 rdfs:domain ms:Subset ;
                 rdfs:range ms:Size ;
                 rdfs:comment "Indicates the size of a subset of a language resource"@en ;
                 rdfs:label "size per subset"@en .


###  http://w3id.org/meta-share/meta-share/sizePerTextClassification
ms:sizePerTextClassification rdf:type owl:ObjectProperty ;
                             rdfs:subPropertyOf ms:sizePerSubset ;
                             rdfs:range ms:Size ;
                             rdfs:comment "Provides information on size of resource parts with different text classification"@en ;
                             rdfs:label "size per text classification"@en .


###  http://w3id.org/meta-share/meta-share/sizePerTextFormat
ms:sizePerTextFormat rdf:type owl:ObjectProperty ;
                     rdfs:subPropertyOf ms:sizePerSubset ;
                     rdfs:range ms:Size ;
                     rdfs:comment "Provides information on the size of the resource parts with different format"@en ;
                     rdfs:label "size per text format"@en .


###  http://w3id.org/meta-share/meta-share/sizePerTextNumericalFormat
ms:sizePerTextNumericalFormat rdf:type owl:ObjectProperty ;
                              rdfs:subPropertyOf ms:sizePerSubset ;
                              rdfs:range ms:Size ;
                              rdfs:comment "Gives information on the size of textNumerical resource parts with different format"@en ;
                              rdfs:label "size per textNumerical format"@en .


###  http://w3id.org/meta-share/meta-share/sizePerTimeCoverage
ms:sizePerTimeCoverage rdf:type owl:ObjectProperty ;
                       rdfs:subPropertyOf ms:sizePerSubset ;
                       rdfs:range ms:Size ;
                       rdfs:comment "Provides information on size per time period represented in the resource"@en ;
                       rdfs:label "size per time coverage"@en .


###  http://w3id.org/meta-share/meta-share/sizePerValidation
ms:sizePerValidation rdf:type owl:ObjectProperty ;
                     rdfs:subPropertyOf ms:sizePerSubset ;
                     rdfs:range ms:Size ;
                     rdfs:comment "Specifies the size of the validated part of a resource"@en ;
                     rdfs:label "size per validation"@en .


###  http://w3id.org/meta-share/meta-share/sizePerVideoClassification
ms:sizePerVideoClassification rdf:type owl:ObjectProperty ;
                              rdfs:subPropertyOf ms:sizePerSubset ;
                              rdfs:range ms:Size ;
                              rdfs:comment "Used to give info on size of parts with different video classification"@en ;
                              rdfs:label "size per video classification"@en .


###  http://w3id.org/meta-share/meta-share/sizePerVideoFormat
ms:sizePerVideoFormat rdf:type owl:ObjectProperty ;
                      rdfs:subPropertyOf ms:sizePerSubset ;
                      rdfs:range ms:Size ;
                      rdfs:comment "Used to give info on size of parts of a resource that differ as to the format"@en ;
                      rdfs:label "size per video format"@en .


###  http://w3id.org/meta-share/meta-share/sizeUnit
ms:sizeUnit rdf:type owl:ObjectProperty ;
            rdfs:domain ms:Size ;
            rdfs:range ms:SizeUnit ;
            rdfs:comment "Specifies the unit that is used when providing information on the size of the resource or of resource parts"@en ;
            rdfs:label "size unit"@en .


###  http://w3id.org/meta-share/meta-share/socialMediaOccupationalAccount
ms:socialMediaOccupationalAccount rdf:type owl:ObjectProperty ;
                                  rdfs:domain [ rdf:type owl:Class ;
                                                owl:unionOf ( ms:Division
                                                              ms:Group
                                                              ms:Organization
                                                              ms:Person
                                                              ms:Project
                                                            )
                                              ] ;
                                  rdfs:range ms:SocialMediaOccupationalAccount ;
                                  rdfs:comment "Introduces the social media or occupational account details of an entity"@en ;
                                  rdfs:label "social media occupational account"@en .


###  http://w3id.org/meta-share/meta-share/socialMediaOccupationalAccountType
ms:socialMediaOccupationalAccountType rdf:type owl:ObjectProperty ;
                                      rdfs:domain ms:SocialMediaOccupationalAccount ;
                                      rdfs:range ms:SocialMediaOccupationalAccountType ;
                                      rdfs:comment "Specifies the type of the social media or occupational account"@en ;
                                      rdfs:label "social media occupational account type"@en .


###  http://w3id.org/meta-share/meta-share/sourceChannel
ms:sourceChannel rdf:type owl:ObjectProperty ;
                 rdfs:domain [ rdf:type owl:Class ;
                               owl:unionOf ( ms:CorpusAudioPart
                                             ms:CorpusTextNumericalPart
                                             ms:CorpusVideoPart
                                           )
                             ] ;
                 rdfs:range ms:SourceChannel ;
                 rdfs:comment "Specifies the source channel of the recording of a multimedia resource"@en ;
                 rdfs:label "source channel"@en .


###  http://w3id.org/meta-share/meta-share/sourceChannelType
ms:sourceChannelType rdf:type owl:ObjectProperty ;
                     rdfs:domain [ rdf:type owl:Class ;
                                   owl:unionOf ( ms:CorpusAudioPart
                                                 ms:CorpusTextNumericalPart
                                                 ms:CorpusVideoPart
                                               )
                                 ] ;
                     rdfs:range ms:SourceChannelType ;
                     rdfs:comment "Specifies the type of the source channel"@en ;
                     rdfs:label "source channel type"@en .


###  http://w3id.org/meta-share/meta-share/sourceLanguage
ms:sourceLanguage rdf:type owl:ObjectProperty ;
                  rdfs:domain [ rdf:type owl:Class ;
                                owl:unionOf ( ms:CorpusAudioPart
                                              ms:CorpusImagePart
                                              ms:CorpusTextPart
                                              ms:CorpusVideoPart
                                              ms:LanguageDescriptionImagePart
                                              ms:LanguageDescriptionTextPart
                                              ms:LanguageDescriptionVideoPart
                                              ms:LexicalConceptualResourceAudioPart
                                              ms:LexicalConceptualResourceImagePart
                                              ms:LexicalConceptualResourceTextPart
                                              ms:LexicalConceptualResourceVideoPart
                                            )
                              ] ;
                  rdfs:range dct:LinguisticSystem ;
                  rdfs:comment "The language from which a translation is made."@en ;
                  rdfs:label "source language"@en .


###  http://w3id.org/meta-share/meta-share/sourceMetadataRecord
ms:sourceMetadataRecord rdf:type owl:ObjectProperty ;
                        rdfs:subPropertyOf ms:isRelatedToMDRecord ;
                        owl:inverseOf ms:targetMetadataRecord ;
                        rdfs:domain ms:MetadataRecord ;
                        rdfs:range ms:MetadataRecord ;
                        rdfs:comment "Links, in some cases (e.g., harvesting, population from other catalogues, conversion from other metadata records, etc.), to the metadata record that has been used as the basis for the creation of the metadata record"@en ;
                        rdfs:label "source metadata record"@en .


###  http://w3id.org/meta-share/meta-share/sourceOfMetadataRecord
ms:sourceOfMetadataRecord rdf:type owl:ObjectProperty ;
                          rdfs:domain ms:MetadataRecord ;
                          rdfs:range dcat:Catalog ;
                          rdfs:comment "Refers to the entity (repository, catalogue, archive, etc.) from which the metadata record has been imported into the new catalogue"@en ;
                          rdfs:label "source of metadata record"@en ;
                          skos:note "for now dcat:catalog"@en .


###  http://w3id.org/meta-share/meta-share/speakingImpairmentOfParticipants
ms:speakingImpairmentOfParticipants rdf:type owl:ObjectProperty ;
                                    rdfs:domain [ rdf:type owl:Class ;
                                                  owl:unionOf ( ms:CorpusAudioPart
                                                                ms:CorpusImagePart
                                                                ms:CorpusTextNumericalPart
                                                                ms:CorpusVideoPart
                                                              )
                                                ] ;
                                    rdfs:range ms:SpeakingImpairmentOfParticipants ;
                                    rdfs:comment "Indicates whether the group of participants contains persons with speaking impairments"@en ;
                                    rdfs:label "speaking impairment of participants"@en .


###  http://w3id.org/meta-share/meta-share/speechInfluence
ms:speechInfluence rdf:type owl:ObjectProperty ;
                   rdfs:domain [ rdf:type owl:Class ;
                                 owl:unionOf ( ms:CorpusAudioPart
                                               ms:CorpusImagePart
                                               ms:CorpusTextNumericalPart
                                               ms:CorpusVideoPart
                                             )
                               ] ;
                   rdfs:range ms:SpeechInfluence ;
                   rdfs:comment "Specifies the factors influencing speech"@en ;
                   rdfs:label "speech influence"@en .


###  http://w3id.org/meta-share/meta-share/speechItem
ms:speechItem rdf:type owl:ObjectProperty ;
              rdfs:domain [ rdf:type owl:Class ;
                            owl:unionOf ( ms:CorpusAudioPart
                                          ms:LexicalConceptualResourceAudioPart
                                        )
                          ] ;
              rdfs:range ms:SpeechItem ;
              rdfs:comment "Specifies the distinct elements that are pronounced and annotated as such"@en ;
              rdfs:label "speech item"@en .


###  http://w3id.org/meta-share/meta-share/staticElement
ms:staticElement rdf:type owl:ObjectProperty ;
                 rdfs:domain [ rdf:type owl:Class ;
                               owl:unionOf ( ms:CorpusImagePart
                                             ms:LanguageDescriptionImagePart
                                             ms:LexicalConceptualResourceImagePart
                                           )
                             ] ;
                 rdfs:range ms:StaticElement ;
                 rdfs:comment "Groups information on the static elements visible on images"@en ;
                 rdfs:label "static element"@en .


###  http://w3id.org/meta-share/meta-share/subject
ms:subject rdf:type owl:ObjectProperty ;
           rdfs:domain [ rdf:type owl:Class ;
                         owl:unionOf ( ms:Corpus
                                       ms:Document
                                       ms:LanguageDescription
                                       ms:LexicalConceptualResource
                                       ms:Project
                                     )
                       ] ;
           rdfs:range ms:Subject ;
           rdfs:comment "Specifies the subject/topic of a language resource"@en ;
           rdfs:label "subject"@en ;
           skos:altLabel "topic"@en .


###  http://w3id.org/meta-share/meta-share/supportType
ms:supportType rdf:type owl:ObjectProperty ;
               rdfs:domain ms:LanguageResource ;
               rdfs:range ms:SupportType ;
               rdfs:comment "Specifies whether some type of support (commercial, free, etc.) is provided for the resource installation or use"@en ;
               rdfs:label "support type"@en .


###  http://w3id.org/meta-share/meta-share/tagset
ms:tagset rdf:type owl:ObjectProperty ;
          rdfs:subPropertyOf ms:dependsOn ;
          rdfs:domain [ rdf:type owl:Class ;
                        owl:unionOf ( ms:Annotation
                                      ms:MLModel
                                    )
                      ] ;
          rdfs:range ms:LexicalConceptualResource ;
          rdfs:comment "The tagset used for annotating a resource or for the input resource (if annotated) of a tool/service or that should be used (dependency) for the annotation"@en ;
          rdfs:label "tagset"@en .


###  http://w3id.org/meta-share/meta-share/targetLanguage
ms:targetLanguage rdf:type owl:ObjectProperty ;
                  rdfs:domain [ rdf:type owl:Class ;
                                owl:unionOf ( ms:CorpusAudioPart
                                              ms:CorpusImagePart
                                              ms:CorpusTextPart
                                              ms:CorpusVideoPart
                                              ms:LanguageDescriptionImagePart
                                              ms:LanguageDescriptionTextPart
                                              ms:LanguageDescriptionVideoPart
                                              ms:LexicalConceptualResourceAudioPart
                                              ms:LexicalConceptualResourceImagePart
                                              ms:LexicalConceptualResourceTextPart
                                              ms:LexicalConceptualResourceVideoPart
                                            )
                              ] ;
                  rdfs:range dct:LinguisticSystem ;
                  rdfs:comment "The language into which a translation is made"@en ;
                  rdfs:label "target language"@en .


###  http://w3id.org/meta-share/meta-share/targetMetadataRecord
ms:targetMetadataRecord rdf:type owl:ObjectProperty ;
                        rdfs:subPropertyOf ms:MDRecordRelatedTo ;
                        rdfs:domain ms:MetadataRecord ;
                        rdfs:range ms:MetadataRecord ;
                        rdfs:comment "Links, in some cases (e.g., harvesting, population from other catalogues, conversion from other metadata records, etc.), an external metadata record that has been used as the basis for the creation of the internal metadata record to this internal metadata record"@en ;
                        rdfs:label "target metadata record"@en .


###  http://w3id.org/meta-share/meta-share/textIncludedInImage
ms:textIncludedInImage rdf:type owl:ObjectProperty ;
                       rdfs:domain [ rdf:type owl:Class ;
                                     owl:unionOf ( ms:CorpusImagePart
                                                   ms:LanguageDescriptionImagePart
                                                   ms:LexicalConceptualResourceImagePart
                                                 )
                                   ] ;
                       rdfs:range ms:TextIncludedInImage ;
                       rdfs:comment "Provides information on the type of text that may be on the image"@en ;
                       rdfs:label "text included in image"@en .


###  http://w3id.org/meta-share/meta-share/textIncludedInVideo
ms:textIncludedInVideo rdf:type owl:ObjectProperty ;
                       rdfs:domain [ rdf:type owl:Class ;
                                     owl:unionOf ( ms:CorpusVideoPart
                                                   ms:LanguageDescriptionVideoPart
                                                   ms:LexicalConceptualResourceVideoPart
                                                 )
                                   ] ;
                       rdfs:range ms:TextIncludedInVideo ;
                       rdfs:comment "Indicates if any text and what type is present in or in conjunction with the video"@en ;
                       rdfs:label "text included in video"@en .


###  http://w3id.org/meta-share/meta-share/textNumericalFormat
ms:textNumericalFormat rdf:type owl:ObjectProperty ;
                       rdfs:domain ms:CorpusTextNumericalPart ;
                       rdfs:comment "Groups information on the format(s) of the textNumerical part of the resource"@en ;
                       rdfs:label "detailed numerical text format"@en ;
                       owl:deprecated ""@en .


###  http://w3id.org/meta-share/meta-share/textType
ms:textType rdf:type owl:ObjectProperty ;
            rdfs:domain ms:CorpusTextPart ;
            rdfs:range ms:TextType ;
            rdfs:comment "Specifies the text type (e.g., factual, literary, etc.) according to which a text corpus (part) is classified"@en ;
            rdfs:label "text type"@en .


###  http://w3id.org/meta-share/meta-share/trl
ms:trl rdf:type owl:ObjectProperty ;
       rdfs:domain ms:ToolService ;
       rdfs:range ms:TRL ;
       rdfs:comment "Specifies the TRL (Technology Readiness Level) of the technology according to the measurement system defined by the EC"@en ;
       rdfs:label "TRL"@en ;
       skos:altLabel "Technology Readiness Level"@en .


###  http://w3id.org/meta-share/meta-share/typesystem
ms:typesystem rdf:type owl:ObjectProperty ;
              rdfs:subPropertyOf ms:dependsOn ;
              rdfs:domain [ rdf:type owl:Class ;
                            owl:unionOf ( ms:MLModel
                                          ms:ProcessingResource
                                          ms:ToolService
                                        )
                          ] ;
              rdfs:range ms:LexicalConceptualResource ;
              rdfs:comment "Specifies the typesystem (preferrably through an identifier or URL) that has been used for the annotation of a resource or that is required for the input resource of a tool/service or that should be used (dependency) for the annotation or used in the training of a ML model"@en ;
              rdfs:label "typesystem"@en .


###  http://w3id.org/meta-share/meta-share/usageProject
ms:usageProject rdf:type owl:ObjectProperty ;
                rdfs:subPropertyOf ms:isRelatedToProject ;
                rdfs:domain ms:ActualUse ;
                rdfs:range ms:Project ;
                rdfs:comment "Links to a project in which the language resource has been used"@en ;
                rdfs:label "usage project"@en .


###  http://w3id.org/meta-share/meta-share/usageReport
ms:usageReport rdf:type owl:ObjectProperty ;
               rdfs:subPropertyOf ms:isDocumentedBy ;
               rdfs:domain ms:ActualUse ;
               rdfs:range ms:Document ;
               rdfs:comment "Links to a document (e.g., research article, report) describing a project, application, experiment or use case where the language resource has been used"@en ;
               rdfs:label "usage report"@en .


###  http://w3id.org/meta-share/meta-share/usedInApplication
ms:usedInApplication rdf:type owl:ObjectProperty ;
                     rdfs:domain ms:ActualUse ;
                     rdfs:range [ owl:intersectionOf ( skos:Concept
                                                       [ rdf:type owl:Restriction ;
                                                         owl:onProperty skos:inScheme ;
                                                         owl:hasValue omtd:OperationScheme
                                                       ]
                                                     ) ;
                                  rdf:type owl:Class
                                ] ;
                     rdfs:comment "Specifies an LT application where the language resource has been used in"@en ;
                     rdfs:label "used in application"@en .


###  http://w3id.org/meta-share/meta-share/userType
ms:userType rdf:type owl:ObjectProperty ;
            rdfs:domain [ rdf:type owl:Class ;
                          owl:unionOf ( ms:Distribution
                                        ms:Organization
                                        ms:Person
                                      )
                        ] ;
            rdfs:range ms:UserType ;
            rdfs:comment "Used to identify the type of user of the resource (affiliated with a commercial vs. academic institution); it is usually associated with licensing or pricing conditions on the use of a resource"@en ;
            rdfs:label "user type"@en .


###  http://w3id.org/meta-share/meta-share/validation
ms:validation rdf:type owl:ObjectProperty ;
              rdfs:domain ms:LanguageResource ;
              rdfs:range ms:Validation ;
              rdfs:comment "Provides information on each of the the validation procedure(s) a language resource may have undergone (e.g., formal validation of the whole resource, content validation of one part of the resource, etc.)."@en ;
              rdfs:label "validation"@en .


###  http://w3id.org/meta-share/meta-share/validationExtent
ms:validationExtent rdf:type owl:ObjectProperty ;
                    rdfs:domain ms:Validation ;
                    rdfs:range ms:ValidationExtent ;
                    rdfs:comment "Specifies the coverage of the language resource that has been validated"@en ;
                    rdfs:label "validation extent"@en .


###  http://w3id.org/meta-share/meta-share/validationMode
ms:validationMode rdf:type owl:ObjectProperty ;
                  rdfs:subPropertyOf ms:processMode ;
                  rdfs:domain ms:Validation ;
                  rdfs:range ms:ProcessMode ;
                  rdfs:comment "Specifies the type of processing applied for the validation of the language resource"@en ;
                  rdfs:label "validation mode"@en .


###  http://w3id.org/meta-share/meta-share/validationReport
ms:validationReport rdf:type owl:ObjectProperty ;
                    rdfs:subPropertyOf ms:isDocumentedBy ;
                    rdfs:domain ms:Validation ;
                    rdfs:range ms:Document ;
                    rdfs:comment "Links to a document with detailed information on the validation process and results"@en ;
                    rdfs:label "validation report"@en .


###  http://w3id.org/meta-share/meta-share/validationType
ms:validationType rdf:type owl:ObjectProperty ;
                  rdfs:domain ms:Validation ;
                  rdfs:range ms:ValidationType ;
                  rdfs:comment "Specifies the type of validation that has been performed on a language resource"@en ;
                  rdfs:label "validation type"@en .


###  http://w3id.org/meta-share/meta-share/validator
ms:validator rdf:type owl:ObjectProperty ;
             rdfs:subPropertyOf ms:isRelatedToActor ;
             rdfs:domain ms:Validation ;
             rdfs:range ms:Actor ;
             rdfs:comment "Links a validation to the person(s), group(s) or organization(s) that have performed a specific validation of a language resource"@en ;
             rdfs:label "validator"@en .


###  http://w3id.org/meta-share/meta-share/versionType
ms:versionType rdf:type owl:ObjectProperty ;
               rdfs:domain [ rdf:type owl:Class ;
                             owl:unionOf ( ms:Document
                                           ms:LanguageResource
                                         )
                           ] ;
               rdfs:range ms:VersionType ;
               rdfs:comment "Links scholarly works (mainly) to a type of versioning vocabulary related to the publication process"@en ;
               rdfs:label "version type"@en ;
               skos:note "If we think this shouldn' be used for LRTs, remove from XSD's"@en .


###  http://w3id.org/meta-share/meta-share/videoFormat
ms:videoFormat rdf:type owl:ObjectProperty ;
               rdfs:domain ms:DatasetDistribution ;
               rdfs:range ms:VideoFormat ;
               rdfs:comment "Groups information on the format(s) of a resource; repeated if parts of the resource are in different formats"@en ;
               rdfs:label "detailed video format"@en ;
               owl:deprecated ""@en ;
               skos:note "see how data formats, audio & video formats will be handled; must be on distribution"@en .


###  http://w3id.org/meta-share/meta-share/visualModelling
ms:visualModelling rdf:type owl:ObjectProperty ;
                   rdfs:domain [ rdf:type owl:Class ;
                                 owl:unionOf ( ms:ImageFormat
                                               ms:VideoFormat
                                             )
                               ] ;
                   rdfs:range ms:VisualModelling ;
                   rdfs:comment "Specifies the dimensional form applied on the video or image part(s) of a corpus"@en ;
                   rdfs:label "visual modelling"@en .


###  http://w3id.org/meta-share/meta-share/vocalTractCondition
ms:vocalTractCondition rdf:type owl:ObjectProperty ;
                       rdfs:domain ms:Participant ;
                       rdfs:range ms:VocalTractCondition ;
                       rdfs:comment "Provides information on the vocal tract conditions that may influence the speech of the participant"@en ;
                       rdfs:label "vocal tract condition"@en .


###  http://w3id.org/meta-share/meta-share/webServiceType
ms:webServiceType rdf:type owl:ObjectProperty ;
                  rdfs:domain ms:SoftwareDistribution ;
                  rdfs:range ms:WebServiceType ;
                  rdfs:comment "Identifies the type of a web service in accordance to a classification vocabulary that refers to the web service communication protocols"@en ;
                  rdfs:label "web service type"@en ;
                  skos:note "try to restrict with instance \"webService\" on DistributionForm"@en .


###  http://www.w3.org/ns/locn#geographicName
<http://www.w3.org/ns/locn#geographicName> rdf:type owl:ObjectProperty ;
                                           rdfs:domain dct:Location ;
                                           rdfs:range skos:Concept ;
                                           skos:note "geographicIdentifier is also a property for location represented as \"rdfs:seeAls\""@en .


###  http://www.w3.org/ns/odrl/2/function
odrl:function rdf:type owl:ObjectProperty .


###  http://xmlns.com/foaf/0.1/primaryTopic
foaf:primaryTopic rdf:type owl:ObjectProperty .


#################################################################
#    Data properties
#################################################################

###  http://purl.org/dc/terms/alternative
dct:alternative rdf:type owl:DatatypeProperty .


###  http://purl.org/dc/terms/description
dct:description rdf:type owl:DatatypeProperty ;
                rdfs:subPropertyOf owl:topDataProperty .


###  http://purl.org/dc/terms/hasVersion
dct:hasVersion rdf:type owl:DatatypeProperty .


###  http://purl.org/dc/terms/issued
dct:issued rdf:type owl:DatatypeProperty .


###  http://purl.org/dc/terms/title
dct:title rdf:type owl:DatatypeProperty ;
          rdfs:domain owl:Thing ;
          rdfs:range rdfs:Literal .


###  http://w3id.org/meta-share/meta-share/abstract
ms:abstract rdf:type owl:DatatypeProperty ;
            rdfs:domain ms:Document ;
            rdfs:range rdf:langString ;
            rdfs:comment "Introduces a summary of the contents of a document"@en ;
            rdfs:label "abstract"@en .


###  http://w3id.org/meta-share/meta-share/accessLocation
ms:accessLocation rdf:type owl:DatatypeProperty ;
                  rdfs:subPropertyOf ms:distributionLocation ;
                  rdfs:domain ms:Distribution ;
                  rdfs:range xsd:anyURI ;
                  rdfs:comment "A URL where the resource can be accessed from; it can be used for landing pages or for cases where the resource is accessible via an interface, i.e. cases where the resource itself is not provided with a direct link for downloading"@en ;
                  rdfs:label "access location"@en .


###  http://w3id.org/meta-share/meta-share/actualUseDetails
ms:actualUseDetails rdf:type owl:DatatypeProperty ;
                    rdfs:domain ms:ActualUse ;
                    rdfs:range rdf:langString ;
                    rdfs:comment "Describes in free text specific use cases or situations where the language resource has been used"@en ;
                    rdfs:label "actual use details"@en .


###  http://w3id.org/meta-share/meta-share/additionalHWRequirements
ms:additionalHWRequirements rdf:type owl:DatatypeProperty ;
                            rdfs:domain [ rdf:type owl:Class ;
                                          owl:unionOf ( ms:LanguageDescription
                                                        ms:SoftwareDistribution
                                                      )
                                        ] ;
                            rdfs:range xsd:string ;
                            rdfs:comment "Specifies hardware requirements that are needed for running a tool/service or model"@en ;
                            rdfs:label "hardware requirements"@en ;
                            skos:altLabel "h/w requirements"@en .


###  http://w3id.org/meta-share/meta-share/address
ms:address rdf:type owl:DatatypeProperty ;
           rdfs:domain ms:AddressSet ;
           rdfs:range rdf:langString ;
           rdfs:comment "The street and the number of the postal address of a person or organization"@en ;
           rdfs:label "address"@en .


###  http://w3id.org/meta-share/meta-share/age
ms:age rdf:type owl:DatatypeProperty ;
       rdfs:domain ms:Participant ;
       rdfs:range xsd:int ;
       rdfs:comment "Age of a person"@en ;
       rdfs:label "age"@en .


###  http://w3id.org/meta-share/meta-share/ageRangeEndOfParticipants
ms:ageRangeEndOfParticipants rdf:type owl:DatatypeProperty ;
                             rdfs:domain [ rdf:type owl:Class ;
                                           owl:unionOf ( ms:CorpusAudioPart
                                                         ms:CorpusImagePart
                                                         ms:CorpusTextNumericalPart
                                                         ms:CorpusVideoPart
                                                       )
                                         ] ;
                             rdfs:range xsd:int ;
                             rdfs:comment "End of age range of the group of participants"@en ;
                             rdfs:label "age range end of participants"@en .


###  http://w3id.org/meta-share/meta-share/ageRangeStartOfParticipants
ms:ageRangeStartOfParticipants rdf:type owl:DatatypeProperty ;
                               rdfs:domain [ rdf:type owl:Class ;
                                             owl:unionOf ( ms:CorpusAudioPart
                                                           ms:CorpusImagePart
                                                           ms:CorpusTextNumericalPart
                                                           ms:CorpusVideoPart
                                                         )
                                           ] ;
                               rdfs:range xsd:int ;
                               rdfs:comment "Start of age range of the group of participants"@en ;
                               rdfs:label "age range start of participants"@en .


###  http://w3id.org/meta-share/meta-share/algorithm
ms:algorithm rdf:type owl:DatatypeProperty ;
             rdfs:domain ms:MLModel ;
             rdfs:range rdf:langString ;
             rdfs:comment "Identifies the training algorithm used for the model (e.g., maximum entropy, svm, etc.)"@en ;
             rdfs:label "algorithm"@en .


###  http://w3id.org/meta-share/meta-share/algorithmDetails
ms:algorithmDetails rdf:type owl:DatatypeProperty ;
                    rdfs:domain ms:MLModel ;
                    rdfs:range rdf:langString ;
                    rdfs:comment "Provides a detailed description of the algorithm, incl. info on whether it's supervised or not"@en ;
                    rdfs:label "algorithm details"@en .


###  http://w3id.org/meta-share/meta-share/alias
ms:alias rdf:type owl:DatatypeProperty ;
         rdfs:domain ms:Participant ;
         rdfs:range rdf:langString ;
         rdfs:comment "Introduces a name used for a participant of a multimedia resource instead of his/her real one"@en ;
         rdfs:label "alias"@en .


###  http://w3id.org/meta-share/meta-share/alternativeTitle
ms:alternativeTitle rdf:type owl:DatatypeProperty ;
                    rdfs:subPropertyOf dct:alternative ;
                    rdfs:domain ms:Document ;
                    rdfs:range rdf:langString ;
                    rdfs:comment "Introduces an alternative title (e.g. short title) used for the document being described"@en ;
                    rdfs:label "alternative title"@en .


###  http://w3id.org/meta-share/meta-share/amount
ms:amount rdf:type owl:DatatypeProperty ;
          rdfs:domain [ rdf:type owl:Class ;
                        owl:unionOf ( ms:Cost
                                      ms:Duration
                                      ms:Size
                                    )
                      ] ;
          rdfs:range xsd:float ;
          rdfs:comment "Specifies the number of units that constitute anything that can be measured (e.g. size of a data resource or cost, etc.)"@en ;
          rdfs:label "amount"@en .


###  http://w3id.org/meta-share/meta-share/annotationEndDate
ms:annotationEndDate rdf:type owl:DatatypeProperty ;
                     rdfs:domain ms:Annotation ;
                     rdfs:range xsd:date ;
                     rdfs:comment "The date in which the annotation process has ended"@en ;
                     rdfs:label "annotation end date"@en .


###  http://w3id.org/meta-share/meta-share/annotationModeDetails
ms:annotationModeDetails rdf:type owl:DatatypeProperty ;
                         rdfs:domain ms:Annotation ;
                         rdfs:range rdf:langString ;
                         rdfs:comment "Provides further information on annotation process "@en ;
                         rdfs:label "annotation mode details"@en .


###  http://w3id.org/meta-share/meta-share/annotationStandoff
ms:annotationStandoff rdf:type owl:DatatypeProperty ;
                      rdfs:domain ms:Annotation ;
                      rdfs:range xsd:boolean ;
                      rdfs:comment "Indicates whether the annotation is created inline or in a stand-off fashion"@en ;
                      rdfs:label "annotation standoff"@en .


###  http://w3id.org/meta-share/meta-share/annotationStartDate
ms:annotationStartDate rdf:type owl:DatatypeProperty ;
                       rdfs:domain ms:Annotation ;
                       rdfs:range xsd:date ;
                       rdfs:comment "The date in which the annotation process has started"@en ;
                       rdfs:label "annotation start date"@en .


###  http://w3id.org/meta-share/meta-share/anonymizationDetails
ms:anonymizationDetails rdf:type owl:DatatypeProperty ;
                        rdfs:domain ms:DataLanguageResource ;
                        rdfs:range rdf:langString ;
                        rdfs:comment "If the resource has been anonymized, this field can be used for entering more information, e.g., tool or method used for the anonymization, by whom it has been performed, whether there was any check of the results, etc."@en ;
                        rdfs:label "anonymization details"@en .


###  http://w3id.org/meta-share/meta-share/artifactPart
ms:artifactPart rdf:type owl:DatatypeProperty ;
                rdfs:domain ms:StaticElement ;
                rdfs:range rdf:langString ;
                rdfs:comment "Indicates the parts of the artifacts represented in the image corpus"@en ;
                rdfs:label "artifact part"@en .


###  http://w3id.org/meta-share/meta-share/attachedLexiconPosition
ms:attachedLexiconPosition rdf:type owl:DatatypeProperty ;
                           rdfs:domain ms:LanguageDescription ;
                           rdfs:range rdf:langString ;
                           rdfs:comment "Indicates the position of the lexicon, if attached to the grammar"@en ;
                           rdfs:label "attached lexicon position"@en .


###  http://w3id.org/meta-share/meta-share/attributionText
ms:attributionText rdf:type owl:DatatypeProperty ;
                   rdfs:domain ms:Distribution ;
                   rdfs:range rdf:langString ;
                   rdfs:comment "The text that must be quoted for attribution purposes when using a resource - for cases where a resource is provided with a restriction on attribution"@en ;
                   rdfs:label "attribution text"@en .


###  http://w3id.org/meta-share/meta-share/availabilityEndDate
ms:availabilityEndDate rdf:type owl:DatatypeProperty ;
                       rdfs:domain ms:Distribution ;
                       rdfs:range xsd:date ;
                       rdfs:comment "Specifies the end date of availability of a resource - only for cases where a resource is available for a restricted time period."@en ;
                       rdfs:label "availability end date"@en .


###  http://w3id.org/meta-share/meta-share/availabilityStartDate
ms:availabilityStartDate rdf:type owl:DatatypeProperty ;
                         rdfs:domain ms:Distribution ;
                         rdfs:range xsd:date ;
                         rdfs:comment "Specifies the start date of availability of a resource - only for cases where a resource is available for a restricted time period."@en ;
                         rdfs:label "availability start date"@en .


###  http://w3id.org/meta-share/meta-share/biasDetails
ms:biasDetails rdf:type owl:DatatypeProperty ;
               rdfs:domain ms:LanguageResource ;
               rdfs:range rdf:langString ;
               rdfs:comment "Provides a free text account on bias considerations of a model"@en ;
               rdfs:label "bias details"@en .


###  http://w3id.org/meta-share/meta-share/bibliographicRecord
ms:bibliographicRecord rdf:type owl:DatatypeProperty ;
                       rdfs:domain ms:Document ;
                       rdfs:range xsd:string ;
                       rdfs:comment "Specifies in the form of free text a set of bibliographic data (a bibliographic record) preferrably in bibtex form"@en ;
                       rdfs:label "bibliographic record"@en .


###  http://w3id.org/meta-share/meta-share/bodyMovement
ms:bodyMovement rdf:type owl:DatatypeProperty ;
                rdfs:domain ms:DynamicElement ;
                rdfs:range rdf:langString ;
                rdfs:comment "Indicates the body parts that move in the video part of the resource"@en ;
                rdfs:label "body movement"@en .


###  http://w3id.org/meta-share/meta-share/bookTitle
ms:bookTitle rdf:type owl:DatatypeProperty ;
             rdfs:subPropertyOf dct:title ;
             rdfs:domain ms:Document ;
             rdfs:range rdf:langString ;
             rdfs:comment "Introduces the human readable text that is used as the title of a book (differentiating from the title of an article)"@en ;
             rdfs:label "book title"@en .


###  http://w3id.org/meta-share/meta-share/capturingDetails
ms:capturingDetails rdf:type owl:DatatypeProperty ;
                    rdfs:domain [ rdf:type owl:Class ;
                                  owl:unionOf ( ms:CorpusAudioPart
                                                ms:CorpusImagePart
                                                ms:CorpusTextNumericalPart
                                                ms:CorpusVideoPart
                                              )
                                ] ;
                    rdfs:range rdf:langString ;
                    rdfs:comment "Provides further information on the capturing method and procedure"@en ;
                    rdfs:label "capturing details"@en .


###  http://w3id.org/meta-share/meta-share/capturingDeviceTypeDetails
ms:capturingDeviceTypeDetails rdf:type owl:DatatypeProperty ;
                              rdfs:domain [ rdf:type owl:Class ;
                                            owl:unionOf ( ms:CorpusAudioPart
                                                          ms:CorpusImagePart
                                                          ms:CorpusTextNumericalPart
                                                          ms:CorpusVideoPart
                                                        )
                                          ] ;
                              rdfs:range rdf:langString ;
                              rdfs:comment "Provides further information on the capturing device"@en ;
                              rdfs:label "capturing device type details"@en .


###  http://w3id.org/meta-share/meta-share/categoryLabel
ms:categoryLabel rdf:type owl:DatatypeProperty ;
                 rdfs:subPropertyOf dct:title ;
                 rdfs:domain ms:Classification ;
                 rdfs:range rdf:langString ;
                 rdfs:comment "Introduces a human readable name (label) by which a classification category (e.g. text type, text genre, domain, etc.) is known"@en ;
                 rdfs:label "category label"@en .


###  http://w3id.org/meta-share/meta-share/citationText
ms:citationText rdf:type owl:DatatypeProperty ;
                rdfs:domain ms:LanguageResource ;
                rdfs:range rdf:langString ;
                rdfs:comment "Provides the text that must be quoted for citation purposes when using a language resource"@en ;
                rdfs:label "citation text"@en .


###  http://w3id.org/meta-share/meta-share/city
ms:city rdf:type owl:DatatypeProperty ;
        rdfs:domain ms:AddressSet ;
        rdfs:range rdf:langString ;
        rdfs:comment "The name of the city, town or village as mentioned in the postal address of a person or organization "@en ;
        rdfs:label "city"@en .


###  http://w3id.org/meta-share/meta-share/colourDepth
ms:colourDepth rdf:type owl:DatatypeProperty ;
               rdfs:domain [ rdf:type owl:Class ;
                             owl:unionOf ( ms:ImageFormat
                                           ms:VideoFormat
                                         )
                           ] ;
               rdfs:range xsd:int ;
               rdfs:comment "The number of bits used to represent the colour of a single pixel"@en ;
               rdfs:label "colour depth"@en .


###  http://w3id.org/meta-share/meta-share/command
ms:command rdf:type owl:DatatypeProperty ;
           rdfs:domain ms:SoftwareDistribution ;
           rdfs:range xsd:string ;
           rdfs:comment "Specifies a command line used to invoke a software component"@en ;
           rdfs:label "command"@en .


###  http://w3id.org/meta-share/meta-share/compressed
ms:compressed rdf:type owl:DatatypeProperty ;
              rdfs:domain [ rdf:type owl:Class ;
                            owl:unionOf ( ms:AudioFormat
                                          ms:ImageFormat
                                          ms:VideoFormat
                                        )
                          ] ;
              rdfs:range xsd:boolean ;
              rdfs:comment "Whether the audio, video or image is compressed or not"@en ;
              rdfs:label "compressed"@en .


###  http://w3id.org/meta-share/meta-share/compressionLoss
ms:compressionLoss rdf:type owl:DatatypeProperty ;
                   rdfs:domain [ rdf:type owl:Class ;
                                 owl:unionOf ( ms:AudioFormat
                                               ms:ImageFormat
                                               ms:VideoFormat
                                             )
                               ] ;
                   rdfs:range xsd:boolean ;
                   rdfs:comment "Whether there is loss due to compression"@en ;
                   rdfs:label "compression loss"@en .


###  http://w3id.org/meta-share/meta-share/conference
ms:conference rdf:type owl:DatatypeProperty ;
              rdfs:domain ms:Document ;
              rdfs:range rdf:langString ;
              rdfs:comment "Introduces the name of the conference where the document being described was presented"@en ;
              rdfs:label "conference"@en .


###  http://w3id.org/meta-share/meta-share/copyrightStatement
ms:copyrightStatement rdf:type owl:DatatypeProperty ;
                      rdfs:domain ms:Distribution ;
                      rdfs:range rdf:langString ;
                      rdfs:comment "Introduces a free text statement that may be included with the language resource, usually containing the name(s) of copyright holders and licensing terms"@en ;
                      rdfs:label "copyright notice"@en .


###  http://w3id.org/meta-share/meta-share/creationDetails
ms:creationDetails rdf:type owl:DatatypeProperty ;
                   rdfs:domain [ rdf:type owl:Class ;
                                 owl:unionOf ( ms:LexicalConceptualResource
                                               ms:MediaPart
                                             )
                               ] ;
                   rdfs:range rdf:langString ;
                   rdfs:comment "Provides additional information on the creation of a language resource"@en ;
                   rdfs:label "creation details"@en .


###  http://w3id.org/meta-share/meta-share/creationEndDate
ms:creationEndDate rdf:type owl:DatatypeProperty ;
                   rdfs:domain ms:LanguageResource ;
                   rdfs:range xsd:date ;
                   rdfs:comment "The date in which the process of creating a resource was completed"@en ;
                   rdfs:label "creation end date"@en .


###  http://w3id.org/meta-share/meta-share/creationStartDate
ms:creationStartDate rdf:type owl:DatatypeProperty ;
                     rdfs:domain ms:LanguageResource ;
                     rdfs:range xsd:date ;
                     rdfs:comment "The date in which the process of creating the resource started"@en ;
                     rdfs:label "creation start date"@en ;
                     skos:note "how do we handle cases where a resource was created, for instance, in 2000? Is this the start or end date?"@en .


###  http://w3id.org/meta-share/meta-share/defaultValue
ms:defaultValue rdf:type owl:DatatypeProperty ;
                rdfs:domain ms:Parameter ;
                rdfs:range xsd:string ;
                rdfs:comment "Specifies the initial value that user interfaces should use when prompting the user for a parameter taking a list of values"@en ;
                rdfs:label "default value"@en .


###  http://w3id.org/meta-share/meta-share/demoLocation
ms:demoLocation rdf:type owl:DatatypeProperty ;
                rdfs:domain ms:SoftwareDistribution ;
                rdfs:range xsd:anyURI ;
                rdfs:comment "Specifies the URL where a user can access the demo of a tool/service"@en ;
                rdfs:label "demo location"@en .


###  http://w3id.org/meta-share/meta-share/description
ms:description rdf:type owl:DatatypeProperty ;
               rdfs:subPropertyOf dct:description ;
               rdfs:domain ms:LanguageResource ;
               rdfs:range rdf:langString ;
               rdfs:comment "Introduces a short free-text account that provides information about the resource (e.g., function, contents, technical information, etc.)"@en ;
               rdfs:label "description"@en ;
               skos:note """Add some link to datacite:hasDescription and descriptionType:abstract (always for language resources). The rest of the values of descriptionType make sense mainly for publications, but this handling allows easier extension at a later time.

But note that there is no class datacite:Description; descriptionType is in range of anything that \"hasDescriptionType\""""@en .


###  http://w3id.org/meta-share/meta-share/dialectAccent
ms:dialectAccent rdf:type owl:DatatypeProperty ;
                 rdfs:domain ms:Participant ;
                 rdfs:range rdf:langString ;
                 rdfs:comment "Provides information on the dialect accent of the participant"@en ;
                 rdfs:label "dialect accent"@en .


###  http://w3id.org/meta-share/meta-share/dialectAccentOfParticipants
ms:dialectAccentOfParticipants rdf:type owl:DatatypeProperty ;
                               rdfs:domain [ rdf:type owl:Class ;
                                             owl:unionOf ( ms:CorpusAudioPart
                                                           ms:CorpusImagePart
                                                           ms:CorpusTextNumericalPart
                                                           ms:CorpusVideoPart
                                                         )
                                           ] ;
                               rdfs:range rdf:langString ;
                               rdfs:comment "Provides information on the dialect accent of the group of participants"@en ;
                               rdfs:label "dialect accent of participants"@en .


###  http://w3id.org/meta-share/meta-share/digest
ms:digest rdf:type owl:DatatypeProperty ;
          rdfs:domain ms:SoftwareDistribution ;
          rdfs:range xsd:string ;
          rdfs:comment "Links a docker image to the sha256 hash (used for selecting the appropriate version)"@en ;
          rdfs:label "digest"@en .


###  http://w3id.org/meta-share/meta-share/discipline
ms:discipline rdf:type owl:DatatypeProperty ;
              rdfs:domain [ rdf:type owl:Class ;
                            owl:unionOf ( ms:Division
                                          ms:Group
                                          ms:Organization
                                          ms:Person
                                        )
                          ] ;
              rdfs:range rdf:langString ;
              rdfs:comment "Introduces an academic field of study or research area that a person, group or organization is expert in"@en ;
              rdfs:label "discipline"@en ;
              skos:altLabel "area of expertise"@en ,
                            "research area"@en ;
              skos:example "computer programming, translation and interpreting, linguistics, ..."@en .


###  http://w3id.org/meta-share/meta-share/discussionURL
ms:discussionURL rdf:type owl:DatatypeProperty ;
                 rdfs:domain ms:LanguageResource ;
                 rdfs:range xsd:anyURI ;
                 rdfs:comment "Links to a URL where there's a discussion thread (e.g., user forum) about a resource"@en ;
                 rdfs:label "discussion URL"@en .


###  http://w3id.org/meta-share/meta-share/distractor
ms:distractor rdf:type owl:DatatypeProperty ;
              rdfs:domain ms:DynamicElement ;
              rdfs:range rdf:langString ;
              rdfs:comment "Identifies any distractors visible in the resource"@en ;
              rdfs:label "distractor"@en .


###  http://w3id.org/meta-share/meta-share/distributionLocation
ms:distributionLocation rdf:type owl:DatatypeProperty ;
                        rdfs:domain ms:Distribution ;
                        rdfs:range xsd:anyURI ;
                        rdfs:comment "A URL point from which a language resource can be directly accessed (downloaded or executed)"@en ;
                        rdfs:label "distribution location"@en .


###  http://w3id.org/meta-share/meta-share/divisionAlternativeName
ms:divisionAlternativeName rdf:type owl:DatatypeProperty ;
                           rdfs:subPropertyOf dct:alternative ;
                           rdfs:domain ms:Division ;
                           rdfs:range rdf:langString ;
                           rdfs:comment "Introduces an alternative name (other than the short name) used for a division"@en ;
                           rdfs:label "division alternative name"@en .


###  http://w3id.org/meta-share/meta-share/divisionName
ms:divisionName rdf:type owl:DatatypeProperty ;
                rdfs:subPropertyOf dct:title ;
                rdfs:domain ms:Division ;
                rdfs:range rdf:langString ;
                rdfs:comment "The official title of a unit of an organization (e.g., faculty or department of a university, department of a research organization or private company, etc.)"@en ;
                rdfs:label "division name"@en .


###  http://w3id.org/meta-share/meta-share/divisionShortName
ms:divisionShortName rdf:type owl:DatatypeProperty ;
                     rdfs:subPropertyOf dct:alternative ;
                     rdfs:domain ms:Division ;
                     rdfs:range rdf:langString ;
                     rdfs:comment "Introduces the short name (abbreviation, acronym, etc.) used for the division of an organization"@en ;
                     rdfs:label "division short name"@en .


###  http://w3id.org/meta-share/meta-share/dockerDownloadLocation
ms:dockerDownloadLocation rdf:type owl:DatatypeProperty ;
                          rdfs:subPropertyOf ms:downloadLocation ;
                          rdfs:domain ms:ToolService ;
                          rdfs:range xsd:string ;
                          rdfs:comment "A location where the software in the form of a docker image can be downloaded from"@en ;
                          rdfs:label "docker download location"@en .


###  http://w3id.org/meta-share/meta-share/downloadLocation
ms:downloadLocation rdf:type owl:DatatypeProperty ;
                    rdfs:subPropertyOf ms:distributionLocation ;
                    rdfs:domain ms:Distribution ;
                    rdfs:range xsd:anyURI ;
                    rdfs:comment "A URL where the language resource (mainly data but also downloadable software programmes or forms) can be downloaded from"@en ;
                    rdfs:label "download location"@en ;
                    skos:note "rule: must be filled in when SoftwareDistributionForm = downloadable; must not be filled in for web services; optional in all other cases"@en .


###  http://w3id.org/meta-share/meta-share/edition
ms:edition rdf:type owl:DatatypeProperty ;
           rdfs:domain ms:Document ;
           rdfs:range xsd:string ;
           rdfs:comment "Introduces the number of the edition for the document that has been described"@en ;
           rdfs:label "edition"@en .


###  http://w3id.org/meta-share/meta-share/educationLevel
ms:educationLevel rdf:type owl:DatatypeProperty ;
                  rdfs:domain ms:Participant ;
                  rdfs:range rdf:langString ;
                  rdfs:comment "Provides information on the education level of the participant"@en ;
                  rdfs:label "education level"@en .


###  http://w3id.org/meta-share/meta-share/email
ms:email rdf:type owl:DatatypeProperty ;
         rdfs:domain [ rdf:type owl:Class ;
                       owl:unionOf ( ms:Affiliation
                                     ms:Division
                                     ms:Group
                                     ms:LanguageResource
                                     ms:Organization
                                     ms:Person
                                   )
                     ] ;
         rdfs:range xsd:string ;
         rdfs:comment "Points to the email address of a person, organization or group"@en ;
         rdfs:label "email"@en ;
         skos:example "john.smith@example.com, ..."@en .


###  http://w3id.org/meta-share/meta-share/evaluated
ms:evaluated rdf:type owl:DatatypeProperty ;
             rdfs:domain ms:ToolService ;
             rdfs:range xsd:boolean ;
             rdfs:comment "Indicates whether the tool or service has been evaluated"@en ;
             rdfs:label "evaluated"@en .


###  http://w3id.org/meta-share/meta-share/evaluationDetails
ms:evaluationDetails rdf:type owl:DatatypeProperty ;
                     rdfs:domain ms:Evaluation ;
                     rdfs:range rdf:langString ;
                     rdfs:comment "Provides further information on the evaluation process of a tool or service"@en ;
                     rdfs:label "evaluation details"@en .


###  http://w3id.org/meta-share/meta-share/eventDescription
ms:eventDescription rdf:type owl:DatatypeProperty ;
                    rdfs:domain ms:StaticElement ;
                    rdfs:range rdf:langString ;
                    rdfs:comment "Provides description of any events represented in the image corpus"@en ;
                    rdfs:label "event description"@en .


###  http://w3id.org/meta-share/meta-share/executionLocation
ms:executionLocation rdf:type owl:DatatypeProperty ;
                     rdfs:subPropertyOf ms:distributionLocation ;
                     rdfs:domain ms:SoftwareDistribution ;
                     rdfs:range xsd:anyURI ;
                     rdfs:comment "A URL where the resource (mainly software) can be directly executed"@en ;
                     rdfs:label "execution location"@en ;
                     skos:note "rule: must be filled in when SoftwareDistributionMedium = webService; otherwise, not to be filled in"@en .


###  http://w3id.org/meta-share/meta-share/eyeMovement
ms:eyeMovement rdf:type owl:DatatypeProperty ;
               rdfs:domain ms:DynamicElement ;
               rdfs:range rdf:langString ;
               rdfs:comment "Indicates the movement of the eyes visible in the resource"@en ;
               rdfs:label "eye movement"@en .


###  http://w3id.org/meta-share/meta-share/faceExpression
ms:faceExpression rdf:type owl:DatatypeProperty ;
                  rdfs:domain [ rdf:type owl:Class ;
                                owl:unionOf ( ms:DynamicElement
                                              ms:StaticElement
                                            )
                              ] ;
                  rdfs:range rdf:langString ;
                  rdfs:comment "Indicates the facial expressions visible in the resource"@en ;
                  rdfs:label "face expression"@en .


###  http://w3id.org/meta-share/meta-share/faceView
ms:faceView rdf:type owl:DatatypeProperty ;
            rdfs:domain [ rdf:type owl:Class ;
                          owl:unionOf ( ms:DynamicElement
                                        ms:StaticElement
                                      )
                        ] ;
            rdfs:range rdf:langString ;
            rdfs:comment "Indicates the view of the face(s) that appear in the video or on the image part of the resource"@en ;
            rdfs:label "face view"@en .


###  http://w3id.org/meta-share/meta-share/factor
ms:factor rdf:type owl:DatatypeProperty ;
          rdfs:domain ms:NGramModel ;
          rdfs:range xsd:string ;
          rdfs:comment "A factor that has been used for the n-gram resource"@en ;
          rdfs:label "factor"@en .


###  http://w3id.org/meta-share/meta-share/faxNumber
ms:faxNumber rdf:type owl:DatatypeProperty ;
             rdfs:domain [ rdf:type owl:Class ;
                           owl:unionOf ( ms:Division
                                         ms:Group
                                         ms:Organization
                                         ms:Person
                                       )
                         ] ;
             rdfs:range xsd:string ;
             rdfs:comment "Introduces the fax number of a person, group or organization; recommended format: +_international code_city code_number without spaces"@en ;
             rdfs:label "fax number"@en ;
             skos:example "+123456789012"@en .


###  http://w3id.org/meta-share/meta-share/fee
ms:fee rdf:type owl:DatatypeProperty ;
       rdfs:domain ms:Distribution ;
       rdfs:range rdf:langString ;
       rdfs:comment "Describes in free the costs that are required to use the resource, a fragment of the resource or to use a tool or service"@en ;
       rdfs:label "fee"@en ;
       skos:note "pricing policy can be a more generic concept; discuss if we want to formalise this" .


###  http://w3id.org/meta-share/meta-share/fidelity
ms:fidelity rdf:type owl:DatatypeProperty ;
            rdfs:domain ms:VideoFormat ;
            rdfs:range xsd:boolean ;
            rdfs:comment "Defines whether blur is present in the moving sequences"@en ;
            rdfs:label "fidelity"@en .


###  http://w3id.org/meta-share/meta-share/formalism
ms:formalism rdf:type owl:DatatypeProperty ;
             rdfs:domain [ rdf:type owl:Class ;
                           owl:unionOf ( ms:LanguageDescription
                                         ms:ToolService
                                       )
                         ] ;
             rdfs:range rdf:langString ;
             rdfs:comment "Specifies the formalism (bibliographic reference, URL, name) used for the creation/enrichment of the resource (grammar or tool/service)"@en ;
             rdfs:label "formalism"@en .


###  http://w3id.org/meta-share/meta-share/frameRate
ms:frameRate rdf:type owl:DatatypeProperty ;
             rdfs:domain ms:VideoFormat ;
             rdfs:range xsd:int ;
             rdfs:comment "The number of frames per second"@en ;
             rdfs:label "frame rate"@en .


###  http://w3id.org/meta-share/meta-share/fundingSchemeCategory
ms:fundingSchemeCategory rdf:type owl:DatatypeProperty ;
                         rdfs:domain ms:Project ;
                         rdfs:range xsd:string ;
                         rdfs:comment "Introduces a category (usually defined by the funding authority) of the funding scheme to which a project complies"@en ;
                         rdfs:label "funding scheme category"@en .


###  http://w3id.org/meta-share/meta-share/geographicCoverage
ms:geographicCoverage rdf:type owl:DatatypeProperty ;
                      rdfs:domain [ rdf:type owl:Class ;
                                    owl:unionOf ( ms:Corpus
                                                  ms:LanguageDescription
                                                  ms:LexicalConceptualResource
                                                  ms:Subset
                                                )
                                  ] ;
                      rdfs:range rdf:langString ;
                      rdfs:comment "Indicates the geographic region that the content of a resource is about; for countries, recommended use of ISO-3166"@en ;
                      rdfs:label "geographic coverage"@en ;
                      skos:note "string or Location (iso3166) and geographic coordinates?"@en .


###  http://w3id.org/meta-share/meta-share/geographicDistributionOfParticipants
ms:geographicDistributionOfParticipants rdf:type owl:DatatypeProperty ;
                                        rdfs:domain [ rdf:type owl:Class ;
                                                      owl:unionOf ( ms:CorpusAudioPart
                                                                    ms:CorpusImagePart
                                                                    ms:CorpusTextNumericalPart
                                                                    ms:CorpusVideoPart
                                                                  )
                                                    ] ;
                                        rdfs:range rdf:langString ;
                                        rdfs:comment "Gives information on the geographic distribution of the participants"@en ;
                                        rdfs:label "geographic distribution of participants"@en .


###  http://w3id.org/meta-share/meta-share/gesture
ms:gesture rdf:type owl:DatatypeProperty ;
           rdfs:domain ms:DynamicElement ;
           rdfs:range rdf:langString ;
           rdfs:comment "Indicates the type of gestures visible in the resource"@en ;
           rdfs:label "gesture"@en .


###  http://w3id.org/meta-share/meta-share/givenName
ms:givenName rdf:type owl:DatatypeProperty ;
             rdfs:domain ms:Person ;
             rdfs:range rdf:langString ;
             rdfs:comment "Introduces the given name (also known as \"first name\") of a person"@en ;
             rdfs:label "given name"@en ;
             skos:altLabel "first name"@en ,
                           "forename"@en .


###  http://w3id.org/meta-share/meta-share/goldStandardLocation
ms:goldStandardLocation rdf:type owl:DatatypeProperty ;
                        rdfs:subPropertyOf ms:url ;
                        rdfs:domain ms:Evaluation ;
                        rdfs:range xsd:anyURI ;
                        rdfs:comment "Links to the URL where a gold standard resource can be found in order to be used for evaluation purposes"@en ;
                        rdfs:label "gold standard location"@en .


###  http://w3id.org/meta-share/meta-share/grantNumber
ms:grantNumber rdf:type owl:DatatypeProperty ;
               rdfs:domain ms:Project ;
               rdfs:range xsd:string ;
               rdfs:comment "Specifies an identification number usually issued by the funding authority and referring uniquely to the project that has received the funding"@en ;
               rdfs:label "grant number"@en .


###  http://w3id.org/meta-share/meta-share/handArmMovement
ms:handArmMovement rdf:type owl:DatatypeProperty ;
                   rdfs:domain ms:DynamicElement ;
                   rdfs:range rdf:langString ;
                   rdfs:comment "Indicates the movement of hands and/or arms visible in the resource"@en ;
                   rdfs:label "hand arm movement"@en .


###  http://w3id.org/meta-share/meta-share/handManipulation
ms:handManipulation rdf:type owl:DatatypeProperty ;
                    rdfs:domain ms:DynamicElement ;
                    rdfs:range rdf:langString ;
                    rdfs:comment "Gives information on the manipulation of objects by hand"@en ;
                    rdfs:label "hand manipulation"@en .


###  http://w3id.org/meta-share/meta-share/headMovement
ms:headMovement rdf:type owl:DatatypeProperty ;
                rdfs:domain ms:DynamicElement ;
                rdfs:range rdf:langString ;
                rdfs:comment "Indicates the movements of the head visible in the resource"@en ;
                rdfs:label "head movement"@en .


###  http://w3id.org/meta-share/meta-share/hearingImpairment
ms:hearingImpairment rdf:type owl:DatatypeProperty ;
                     rdfs:domain ms:Participant ;
                     rdfs:range rdf:langString ;
                     rdfs:comment "Provides information on any hearing impairment the participant may have"@en ;
                     rdfs:label "hearing impairment"@en .


###  http://w3id.org/meta-share/meta-share/height
ms:height rdf:type owl:DatatypeProperty ;
          rdfs:domain ms:Participant ;
          rdfs:range xsd:int ;
          rdfs:comment "Provides information on the height of the participant in cm"@en ;
          rdfs:label "height"@en .


###  http://w3id.org/meta-share/meta-share/homepage
ms:homepage rdf:type owl:DatatypeProperty ;
            rdfs:subPropertyOf ms:url ;
            rdfs:domain ms:Person ;
            rdfs:range xsd:anyURI ;
            rdfs:comment "Links to a URL that includes information on a person (e.g., CV, publications, communication information, etc.)"@en ;
            rdfs:label "home page"@en .


###  http://w3id.org/meta-share/meta-share/honorificPrefix
ms:honorificPrefix rdf:type owl:DatatypeProperty ;
                   rdfs:domain ms:Person ;
                   rdfs:range rdf:langString ;
                   rdfs:comment "Introduces a honorific prefix (or title) such as Dr./Mr/Ms. that precedes the name of a person"@en ;
                   rdfs:label "honorific prefix"@en ;
                   skos:altLabel "title"@en .


###  http://w3id.org/meta-share/meta-share/image3
ms:image3 rdf:type owl:DatatypeProperty ;
          rdfs:domain ms:Person ;
          rdfs:range xsd:anyURI .


###  http://w3id.org/meta-share/meta-share/implementationLanguage
ms:implementationLanguage rdf:type owl:DatatypeProperty ;
                          rdfs:domain ms:ToolService ;
                          rdfs:range xsd:string ;
                          rdfs:comment "The programming language(s) used for the development of a tool/service, which is needed for running the tools/services, in case no executables are available"@en ;
                          rdfs:label "implementation language"@en .


###  http://w3id.org/meta-share/meta-share/interaction
ms:interaction rdf:type owl:DatatypeProperty ;
               rdfs:domain [ rdf:type owl:Class ;
                             owl:unionOf ( ms:CorpusAudioPart
                                           ms:CorpusVideoPart
                                         )
                           ] ;
               rdfs:range rdf:langString ;
               rdfs:comment "Specifies the parts that interact in an audio or video component"@en ;
               rdfs:label "interaction"@en .


###  http://w3id.org/meta-share/meta-share/interactiveMedia
ms:interactiveMedia rdf:type owl:DatatypeProperty ;
                    rdfs:domain ms:DynamicElement ;
                    rdfs:range rdf:langString ;
                    rdfs:comment "Any interactive media visible in the resource"@en ;
                    rdfs:label "interactive media"@en .


###  http://w3id.org/meta-share/meta-share/interannotatorAgreement
ms:interannotatorAgreement rdf:type owl:DatatypeProperty ;
                           rdfs:domain ms:Annotation ;
                           rdfs:range rdf:langString ;
                           rdfs:comment "Provides information on the inter-annotator agreement and the methods/metrics applied"@en ;
                           rdfs:label "interannotator agreement"@en .


###  http://w3id.org/meta-share/meta-share/interpolated
ms:interpolated rdf:type owl:DatatypeProperty ;
                rdfs:domain ms:NGramModel ;
                rdfs:range xsd:boolean ;
                rdfs:comment "Specifies whether the n-gram resource is interpolated (Interpolated language models are constructed by 2 or more corpora and each corpus is represented in the model according to a predefined weight)"@en ;
                rdfs:label "interpolated"@en .


###  http://w3id.org/meta-share/meta-share/intraannotatorAgreement
ms:intraannotatorAgreement rdf:type owl:DatatypeProperty ;
                           rdfs:domain ms:Annotation ;
                           rdfs:range rdf:langString ;
                           rdfs:comment "Provides information on the intra-annotator agreement and the methods/metrics applied "@en ;
                           rdfs:label "intra-annotator agreement"@en .


###  http://w3id.org/meta-share/meta-share/isFactored
ms:isFactored rdf:type owl:DatatypeProperty ;
              rdfs:domain ms:NGramModel ;
              rdfs:range xsd:boolean ;
              rdfs:comment "Specifies whether the model is factored or not"@en ;
              rdfs:label "is factored"@en .


###  http://w3id.org/meta-share/meta-share/journal
ms:journal rdf:type owl:DatatypeProperty ;
           rdfs:domain ms:Document ;
           rdfs:range rdf:langString ;
           rdfs:comment "Introduces the name of the journal where the document being described has been published"@en ;
           rdfs:label "journal"@en .


###  http://w3id.org/meta-share/meta-share/keyword
ms:keyword rdf:type owl:DatatypeProperty ;
           rdfs:domain [ rdf:type owl:Class ;
                         owl:unionOf ( ms:Division
                                       ms:Document
                                       ms:Group
                                       ms:LanguageResource
                                       ms:Organization
                                       ms:Person
                                       ms:Project
                                     )
                       ] ;
           rdfs:range rdf:langString ;
           rdfs:comment "Introduces a word or phrase considered important for the description of an entity and thus used to index or classify it"@en ;
           rdfs:label "keyword"@en ;
           skos:altLabel "keyphrase"@en ;
           skos:example "crisis management, speech synthesis, subtitling, ..."@en .


###  http://w3id.org/meta-share/meta-share/landingPage
ms:landingPage rdf:type owl:DatatypeProperty ;
               rdfs:subPropertyOf ms:url ;
               rdfs:domain ms:LanguageResource ;
               rdfs:range xsd:anyURI ;
               rdfs:comment "Links to a web page that provides additional information about a language resource (e.g., its contents, acknowledgements, link to the access location, etc.)"@en ;
               rdfs:label "landing page"@en ;
               skos:note "dcat:landingPage has range foaf:Document and is a subproperty of foaf:page; no distinction is made between physical and electronic documents. so I'm not sure what the most appropriate relation is for us"@en .


###  http://w3id.org/meta-share/meta-share/landscapePart
ms:landscapePart rdf:type owl:DatatypeProperty ;
                 rdfs:domain ms:StaticElement ;
                 rdfs:range rdf:langString ;
                 rdfs:comment "Indicates the landscape parts represented in the image corpus"@en ;
                 rdfs:label "landscape part"@en .


###  http://w3id.org/meta-share/meta-share/language
ms:language rdf:type owl:DatatypeProperty ;
            rdfs:domain [ rdf:type owl:Class ;
                          owl:unionOf ( ms:CorpusAudioPart
                                        ms:CorpusImagePart
                                        ms:CorpusTextPart
                                        ms:CorpusVideoPart
                                        ms:LanguageDescriptionImagePart
                                        ms:LanguageDescriptionTextPart
                                        ms:LanguageDescriptionVideoPart
                                        ms:LexicalConceptualResourceAudioPart
                                        ms:LexicalConceptualResourceImagePart
                                        ms:LexicalConceptualResourceTextPart
                                        ms:LexicalConceptualResourceVideoPart
                                      )
                        ] ;
            rdfs:range xsd:anyURI ;
            rdfs:comment "Specifies the language that is used in the resource or supported by the tool/service"@en ;
            rdfs:label "language"@en ;
            skos:note "in the xsd, we have the full BCP47 recommendation combination, in ontology as a uri (to link with an ontology)"@en .


###  http://w3id.org/meta-share/meta-share/languageDependent
ms:languageDependent rdf:type owl:DatatypeProperty ;
                     rdfs:domain ms:ToolService ;
                     rdfs:range xsd:boolean ;
                     rdfs:comment "Indicates whether the operation of the tool or service is language dependent or not"@en ;
                     rdfs:label "language dependent"@en .


###  http://w3id.org/meta-share/meta-share/languageVarietyName
ms:languageVarietyName rdf:type owl:DatatypeProperty ;
                       rdfs:domain ms:LanguageVariety ;
                       rdfs:range rdf:langString ;
                       rdfs:comment "A textual string used for referring to a language variety"@en ;
                       rdfs:label "language variety name"@en .


###  http://w3id.org/meta-share/meta-share/legend
ms:legend rdf:type owl:DatatypeProperty ;
          rdfs:domain [ rdf:type owl:Class ;
                        owl:unionOf ( ms:CorpusAudioPart
                                      ms:LexicalConceptualResourceAudioPart
                                    )
                      ] ;
          rdfs:range rdf:langString ;
          rdfs:comment "Introduces the legend of the soundtrack"@en ;
          rdfs:label "legend"@en .


###  http://w3id.org/meta-share/meta-share/licenceTermsAlternativeName
ms:licenceTermsAlternativeName rdf:type owl:DatatypeProperty ;
                               rdfs:subPropertyOf dct:alternative ;
                               rdfs:domain ms:LicenceTerms ;
                               rdfs:range rdf:langString ;
                               rdfs:comment "Introduces an alternative name (other than the short name) used for a licence or terms of use"@en ;
                               rdfs:label "licence/terms of use/service name"@en .


###  http://w3id.org/meta-share/meta-share/licenceTermsName
ms:licenceTermsName rdf:type owl:DatatypeProperty ;
                    rdfs:subPropertyOf dct:title ;
                    rdfs:domain ms:LicenceTerms ;
                    rdfs:range rdf:langString ;
                    rdfs:comment "The name by which a legal document (e.g., licence, terms of use, terms of service) is known"@en ;
                    rdfs:label "licence/terms of use/service name"@en .


###  http://w3id.org/meta-share/meta-share/licenceTermsShortName
ms:licenceTermsShortName rdf:type owl:DatatypeProperty ;
                         rdfs:subPropertyOf dct:alternative ;
                         rdfs:domain ms:LicenceTerms ;
                         rdfs:range rdf:langString ;
                         rdfs:comment "Introduces the short name (abbreviation, acronym, etc.) used for a licence or terms of use document"@en ;
                         rdfs:label "licence/Terms of use/service short name"@en .


###  http://w3id.org/meta-share/meta-share/licenceTermsURL
ms:licenceTermsURL rdf:type owl:DatatypeProperty ;
                   rdfs:subPropertyOf ms:url ;
                   rdfs:domain ms:LicenceTerms ;
                   rdfs:range xsd:anyURI ;
                   rdfs:comment "Links to the URL where the text of a licence/terms of use/service is found"@en ;
                   rdfs:label "licence/terms of use/service URL"@en .


###  http://w3id.org/meta-share/meta-share/logo
ms:logo rdf:type owl:DatatypeProperty ;
        rdfs:domain [ rdf:type owl:Class ;
                      owl:unionOf ( ms:Division
                                    ms:Group
                                    ms:LanguageResource
                                    ms:LicenceTerms
                                    ms:Organization
                                    ms:Project
                                  )
                    ] ;
        rdfs:range xsd:anyURI ;
        rdfs:comment "Links to a symbol or graphic object used to identify an entity; please, add a URL with an image file"@en ;
        rdfs:label "logo"@en ;
        skos:example "https://www.logo.eu"@en .


###  http://w3id.org/meta-share/meta-share/mailingListName
ms:mailingListName rdf:type owl:DatatypeProperty ;
                   rdfs:domain ms:LanguageResource ;
                   rdfs:range xsd:string ;
                   rdfs:comment "Indicates the name of a mailing list used in relation to a language resource"@en ;
                   rdfs:label "mailing list name"@en .


###  http://w3id.org/meta-share/meta-share/measure
ms:measure rdf:type owl:DatatypeProperty ;
           rdfs:domain ms:PerformanceIndicator ;
           rdfs:range xsd:float ;
           rdfs:comment "Defines the measure calculated for the metric"@en ;
           rdfs:label "measure"@en .


###  http://w3id.org/meta-share/meta-share/mediaTypeDetails
ms:mediaTypeDetails rdf:type owl:DatatypeProperty ;
                    rdfs:domain ms:LinkToOtherMedia ;
                    rdfs:range rdf:langString ;
                    rdfs:comment "Provides further information on the way the media types are linked and/or synchronized with each other within the same resource"@en ;
                    rdfs:label "media type details"@en .


###  http://w3id.org/meta-share/meta-share/metadataCreationDate
ms:metadataCreationDate rdf:type owl:DatatypeProperty ;
                        rdfs:domain ms:MetadataRecord ;
                        rdfs:range xsd:date ;
                        rdfs:comment "Specifies the date when the metadata record was first created"@en ;
                        rdfs:label "metadata creation date"@en .


###  http://w3id.org/meta-share/meta-share/metadataLastDateUpdated
ms:metadataLastDateUpdated rdf:type owl:DatatypeProperty ;
                           rdfs:domain ms:MetadataRecord ;
                           rdfs:range xsd:date ;
                           rdfs:comment "Specifies the date when the last update of the metadata record was made"@en ;
                           rdfs:label "metadata last date updated"@en .


###  http://w3id.org/meta-share/meta-share/metalanguage
ms:metalanguage rdf:type owl:DatatypeProperty ;
                rdfs:domain [ rdf:type owl:Class ;
                              owl:unionOf ( ms:LanguageDescriptionImagePart
                                            ms:LanguageDescriptionTextPart
                                            ms:LanguageDescriptionVideoPart
                                            ms:LexicalConceptualResourceAudioPart
                                            ms:LexicalConceptualResourceImagePart
                                            ms:LexicalConceptualResourceTextPart
                                            ms:LexicalConceptualResourceVideoPart
                                          )
                            ] ;
                rdfs:range xsd:anyURI ;
                rdfs:comment "Specifies the language that is used as support for the resource (e.g., English for a grammar of French described in English or for a French dictionary with English definitions)"@en ;
                rdfs:label "metalanguage"@en ;
                skos:note "in the xsd, this is expressed with a BCP47 combination while in the ontology as a URI (to link with an ontology)"@en .


###  http://w3id.org/meta-share/meta-share/mlFramework
ms:mlFramework rdf:type owl:DatatypeProperty ;
               rdfs:domain ms:MLModel ;
               rdfs:range xsd:string ;
               rdfs:comment "Specifies the framework that has been used for developing a model (e.g. keras, tensorflow, etc.)"@en ;
               rdfs:label "ML framework"@en ;
               owl:deprecated "" ;
               skos:altLabel "Machine Learning framework"@en .


###  http://w3id.org/meta-share/meta-share/modalityTypeDetails
ms:modalityTypeDetails rdf:type owl:DatatypeProperty ;
                       rdfs:domain ms:MediaPart ;
                       rdfs:range rdf:langString ;
                       rdfs:comment "Provides further information on the modalities represented in a language resource"@en ;
                       rdfs:label "modality type details"@en .


###  http://w3id.org/meta-share/meta-share/modelVariant
ms:modelVariant rdf:type owl:DatatypeProperty ;
                rdfs:domain ms:MLModel ;
                rdfs:range xsd:string ;
                rdfs:comment "Introduces a label that can be used to identify the variant of a ML model"@en ;
                rdfs:label "model variant"@en .


###  http://w3id.org/meta-share/meta-share/multiValue
ms:multiValue rdf:type owl:DatatypeProperty ;
              rdfs:domain ms:Parameter ;
              rdfs:range xsd:boolean ;
              rdfs:comment "Specifies whether the parameter takes a list of values"@en ;
              rdfs:label "multi-value"@en .


###  http://w3id.org/meta-share/meta-share/multilingualityTypeDetails
ms:multilingualityTypeDetails rdf:type owl:DatatypeProperty ;
                              rdfs:domain ms:MediaPart ;
                              rdfs:range rdf:langString ;
                              rdfs:comment "Provides further information on multilinguality of a resource in free text"@en ;
                              rdfs:label "multilinguality type details" .


###  http://w3id.org/meta-share/meta-share/name
ms:name rdf:type owl:DatatypeProperty ;
        rdfs:domain ms:Person ;
        rdfs:range rdf:langString ;
        rdfs:comment "Introduces the full name of a person; recommended format \"surname, givenName\""@en ;
        rdfs:label "name"@en .


###  http://w3id.org/meta-share/meta-share/numberOfParticipants
ms:numberOfParticipants rdf:type owl:DatatypeProperty ;
                        rdfs:domain [ rdf:type owl:Class ;
                                      owl:unionOf ( ms:CorpusAudioPart
                                                    ms:CorpusImagePart
                                                    ms:CorpusTextNumericalPart
                                                    ms:CorpusVideoPart
                                                  )
                                    ] ;
                        rdfs:range xsd:int ;
                        rdfs:comment "The number of the persons participating in the audio or video part of the resource"@en ;
                        rdfs:label "number of participants"@en .


###  http://w3id.org/meta-share/meta-share/numberOfTracks
ms:numberOfTracks rdf:type owl:DatatypeProperty ;
                  rdfs:domain ms:AudioFormat ;
                  rdfs:range xsd:int ;
                  rdfs:comment "Specifies the number of audio channels"@en ;
                  rdfs:label "number of tracks"@en ;
                  skos:note "In MS it's a controlled vocabulary (1, 2, 4, 8) but I think it's too much"@en .


###  http://w3id.org/meta-share/meta-share/numberOfTrainedSpeakers
ms:numberOfTrainedSpeakers rdf:type owl:DatatypeProperty ;
                           rdfs:domain [ rdf:type owl:Class ;
                                         owl:unionOf ( ms:CorpusAudioPart
                                                       ms:CorpusImagePart
                                                       ms:CorpusTextNumericalPart
                                                       ms:CorpusVideoPart
                                                     )
                                       ] ;
                           rdfs:range xsd:int ;
                           rdfs:comment "The number of participants that have been trained for the specific task"@en ;
                           rdfs:label "number of trained speakers"@en .


###  http://w3id.org/meta-share/meta-share/optional
ms:optional rdf:type owl:DatatypeProperty ;
            rdfs:domain ms:Parameter ;
            rdfs:range xsd:boolean ;
            rdfs:comment "Specifies whether the parameter should be treated as mandatory or optional by user interfaces"@en ;
            rdfs:label "optional"@en .


###  http://w3id.org/meta-share/meta-share/order
ms:order rdf:type owl:DatatypeProperty ;
         rdfs:domain ms:NGramModel ;
         rdfs:range xsd:int ;
         rdfs:comment "Specifies the maximum number of items in the sequence"@en ;
         rdfs:label "order"@en .


###  http://w3id.org/meta-share/meta-share/organizationAlternativeName
ms:organizationAlternativeName rdf:type owl:DatatypeProperty ;
                               rdfs:subPropertyOf dct:alternative ;
                               rdfs:domain ms:Organization ;
                               rdfs:range rdf:langString ;
                               rdfs:comment "Introduces an alternative name (other than the official title or the short name) used for an organization"@en ;
                               rdfs:label "organization alternative name"@en .


###  http://w3id.org/meta-share/meta-share/organizationBio
ms:organizationBio rdf:type owl:DatatypeProperty ;
                   rdfs:subPropertyOf dct:description ;
                   rdfs:domain [ rdf:type owl:Class ;
                                 owl:unionOf ( ms:Division
                                               ms:Group
                                               ms:Organization
                                             )
                               ] ;
                   rdfs:range rdf:langString ;
                   rdfs:comment "Introduces a short free-text account that provides information on an organization"@en ;
                   rdfs:label "organization description"@en .


###  http://w3id.org/meta-share/meta-share/organizationDescription
ms:organizationDescription rdf:type owl:DatatypeProperty ;
                           rdfs:domain ms:StaticElement ;
                           rdfs:range rdf:langString ;
                           rdfs:comment "Provides description of the organizations that may appear in the image corpus"@en ;
                           rdfs:label "organization description"@en .


###  http://w3id.org/meta-share/meta-share/organizationName
ms:organizationName rdf:type owl:DatatypeProperty ;
                    rdfs:subPropertyOf dct:title ;
                    rdfs:domain [ rdf:type owl:Class ;
                                  owl:unionOf ( ms:Group
                                                ms:Organization
                                              )
                                ] ;
                    rdfs:range rdf:langString ;
                    rdfs:comment "The official title of an organization"@en ;
                    rdfs:label "organization name"@en .


###  http://w3id.org/meta-share/meta-share/organizationShortName
ms:organizationShortName rdf:type owl:DatatypeProperty ;
                         rdfs:subPropertyOf dct:alternative ;
                         rdfs:domain [ rdf:type owl:Class ;
                                       owl:unionOf ( ms:Group
                                                     ms:Organization
                                                   )
                                     ] ;
                         rdfs:range rdf:langString ;
                         rdfs:comment "Introduces the short name (abbreviation, acronym, etc.) used for an organization"@en ;
                         rdfs:label "organization short name"@en .


###  http://w3id.org/meta-share/meta-share/originalSourceDescription
ms:originalSourceDescription rdf:type owl:DatatypeProperty ;
                             rdfs:domain [ rdf:type owl:Class ;
                                           owl:unionOf ( ms:LexicalConceptualResource
                                                         ms:MediaPart
                                                         ms:ToolService
                                                       )
                                         ] ;
                             rdfs:range rdf:langString ;
                             rdfs:comment "A description in free text of the source material that has been used for the creation of a language data resource"@en ;
                             rdfs:label "original source description"@en .


###  http://w3id.org/meta-share/meta-share/output
ms:output rdf:type owl:DatatypeProperty ;
          rdfs:domain ms:LanguageDescription ;
          rdfs:range rdf:langString ;
          rdfs:comment "Indicates whether the output of the operation of the grammar is a statement of grammaticality (grammatical/ungrammatical) or structures (interpretation of the input)"@en ;
          rdfs:label "output"@en .


###  http://w3id.org/meta-share/meta-share/pages
ms:pages rdf:type owl:DatatypeProperty ;
         rdfs:domain ms:Document ;
         rdfs:range xsd:string ;
         rdfs:comment "Introduces the range of pages (preferrably with a dash between) on which a document is printed"@en ;
         rdfs:label "pages"@en .


###  http://w3id.org/meta-share/meta-share/parameterDescription
ms:parameterDescription rdf:type owl:DatatypeProperty ;
                        rdfs:domain ms:Parameter ;
                        rdfs:range rdf:langString ;
                        rdfs:comment "Provides a short account of he parameter (e.g., function it performs, input / output requirements, etc.) in free text"@en ;
                        rdfs:label "parameter description"@en .


###  http://w3id.org/meta-share/meta-share/parameterLabel
ms:parameterLabel rdf:type owl:DatatypeProperty ;
                  rdfs:domain ms:Parameter ;
                  rdfs:range rdf:langString ;
                  rdfs:comment "Introduces a short name for a parameter suitable for use as a field label in a user interface"@en ;
                  rdfs:label "parameter label"@en .


###  http://w3id.org/meta-share/meta-share/parameterName
ms:parameterName rdf:type owl:DatatypeProperty ;
                 rdfs:domain ms:Parameter ;
                 rdfs:range xsd:string ;
                 rdfs:comment "Introduces the name of the paramter as sent to a processing service"@en ;
                 rdfs:label "parameter name"@en .


###  http://w3id.org/meta-share/meta-share/perplexity
ms:perplexity rdf:type owl:DatatypeProperty ;
              rdfs:domain ms:NGramModel ;
              rdfs:range xsd:float ;
              rdfs:comment "Provides information on the perplexity derived from running on test set taken from the same corpus"@en ;
              rdfs:label "perplexity"@en .


###  http://w3id.org/meta-share/meta-share/personDescription
ms:personDescription rdf:type owl:DatatypeProperty ;
                     rdfs:domain ms:StaticElement ;
                     rdfs:range rdf:langString ;
                     rdfs:comment "Provides descriptive features for the persons represented in the image corpus"@en ;
                     rdfs:label "person description"@en .


###  http://w3id.org/meta-share/meta-share/personalDataDetails
ms:personalDataDetails rdf:type owl:DatatypeProperty ;
                       rdfs:domain ms:DataLanguageResource ;
                       rdfs:range rdf:langString ;
                       rdfs:comment "If the resource includes personal data, this field can be used for entering more information, e.g., whether special handling of the resource is required (e.g., anonymization, further request for use, etc.)"@en ;
                       rdfs:label "personal data details"@en .


###  http://w3id.org/meta-share/meta-share/placeOfBirth
ms:placeOfBirth rdf:type owl:DatatypeProperty ;
                rdfs:domain ms:Participant ;
                rdfs:range rdf:langString ;
                rdfs:comment "The place in which the participant has been born"@en ;
                rdfs:label "place of birth"@en .


###  http://w3id.org/meta-share/meta-share/placeOfChildhood
ms:placeOfChildhood rdf:type owl:DatatypeProperty ;
                    rdfs:domain ms:Participant ;
                    rdfs:range rdf:langString ;
                    rdfs:comment "The place in which the participant lived as a child"@en ;
                    rdfs:label "place of childhood"@en .


###  http://w3id.org/meta-share/meta-share/placeOfLiving
ms:placeOfLiving rdf:type owl:DatatypeProperty ;
                 rdfs:domain ms:Participant ;
                 rdfs:range rdf:langString ;
                 rdfs:comment "The place of living of a participant"@en ;
                 rdfs:label "place of living"@en .


###  http://w3id.org/meta-share/meta-share/placeOfSecondEducation
ms:placeOfSecondEducation rdf:type owl:DatatypeProperty ;
                          rdfs:domain ms:Participant ;
                          rdfs:range rdf:langString ;
                          rdfs:comment "Specifies the place of the secondary education of the participant"@en ;
                          rdfs:label "place of second education"@en .


###  http://w3id.org/meta-share/meta-share/posesPerSubject
ms:posesPerSubject rdf:type owl:DatatypeProperty ;
                   rdfs:domain ms:DynamicElement ;
                   rdfs:range xsd:int ;
                   rdfs:comment "Indicates the number of poses per subject that participates in the video part of the resource"@en ;
                   rdfs:label "poses per subject"@en .


###  http://w3id.org/meta-share/meta-share/position
ms:position rdf:type owl:DatatypeProperty ;
            rdfs:domain ms:Affiliation ;
            rdfs:range rdf:langString ;
            rdfs:comment "The position or the title of a person if affiliated to an organization "@en ;
            rdfs:label "position"@en .


###  http://w3id.org/meta-share/meta-share/privateResource
ms:privateResource rdf:type owl:DatatypeProperty ;
                   rdfs:domain [ rdf:type owl:Class ;
                                 owl:unionOf ( ms:DatasetDistribution
                                               ms:SoftwareDistribution
                                             )
                               ] ;
                   rdfs:range xsd:boolean ;
                   rdfs:comment "Specifies whether the resource is private so that its access/download location remains hidden"@en ;
                   rdfs:label "private"@en .


###  http://w3id.org/meta-share/meta-share/profession
ms:profession rdf:type owl:DatatypeProperty ;
              rdfs:domain ms:Participant ;
              rdfs:range rdf:langString ;
              rdfs:comment "Provides information on the participant's profession"@en ;
              rdfs:label "profession"@en .


###  http://w3id.org/meta-share/meta-share/projectAlternativeName
ms:projectAlternativeName rdf:type owl:DatatypeProperty ;
                          rdfs:subPropertyOf dct:alternative ;
                          rdfs:domain ms:Project ;
                          rdfs:range rdf:langString ;
                          rdfs:comment "Introduces an alternative name (other than the short name) used for a project"@en ;
                          rdfs:label "project alternative name"@en .


###  http://w3id.org/meta-share/meta-share/projectEndDate
ms:projectEndDate rdf:type owl:DatatypeProperty ;
                  rdfs:domain ms:Project ;
                  rdfs:range xsd:date ;
                  rdfs:comment "The end date of a project"@en ;
                  rdfs:label "project end date"@en .


###  http://w3id.org/meta-share/meta-share/projectName
ms:projectName rdf:type owl:DatatypeProperty ;
               rdfs:subPropertyOf dct:title ;
               rdfs:domain ms:Project ;
               rdfs:range rdf:langString ;
               rdfs:comment "The official title of a project"@en ;
               rdfs:label "project name"@en ;
               skos:altLabel "project title"@en .


###  http://w3id.org/meta-share/meta-share/projectReport
ms:projectReport rdf:type owl:DatatypeProperty ;
                 rdfs:domain ms:Project ;
                 rdfs:range rdf:langString ;
                 rdfs:comment "Links to a report issued by a project"@en ;
                 rdfs:label "project report"@en .


###  http://w3id.org/meta-share/meta-share/projectShortName
ms:projectShortName rdf:type owl:DatatypeProperty ;
                    rdfs:subPropertyOf dct:alternative ;
                    rdfs:domain ms:Project ;
                    rdfs:range rdf:langString ;
                    rdfs:comment "Introduces a short name (e.g., acronym, abbreviated form) by which a project is known"@en ;
                    rdfs:label "project short name"@en .


###  http://w3id.org/meta-share/meta-share/projectStartDate
ms:projectStartDate rdf:type owl:DatatypeProperty ;
                    rdfs:domain ms:Project ;
                    rdfs:range xsd:date ;
                    rdfs:comment "The starting date of a project"@en ;
                    rdfs:label "project start date"@en .


###  http://w3id.org/meta-share/meta-share/projectSummary
ms:projectSummary rdf:type owl:DatatypeProperty ;
                  rdfs:domain ms:Project ;
                  rdfs:range rdf:langString ;
                  rdfs:comment "Introduces a short description (in free text) of the main objectives, mission or contents of the project"@en ;
                  rdfs:label "project summary"@en .


###  http://w3id.org/meta-share/meta-share/publicationDate
ms:publicationDate rdf:type owl:DatatypeProperty ;
                   rdfs:subPropertyOf dct:issued ;
                   rdfs:domain [ rdf:type owl:Class ;
                                 owl:unionOf ( ms:Distribution
                                               ms:Document
                                               ms:LanguageResource
                                             )
                               ] ;
                   rdfs:range xsd:date ;
                   rdfs:comment "Specifies the date when a language resource has been made available to the public"@en ;
                   rdfs:label "publication date"@en ;
                   skos:note """problem: when is the first publication date if a resource has been made available through zenodo, meta-share, clarin, etc.?? How can this be propagated? 
Important for citation purposes
should we also differentiate between distributions? e.g., a csv published at a different time from a database?"""@en .


###  http://w3id.org/meta-share/meta-share/publisher
ms:publisher rdf:type owl:DatatypeProperty ;
             rdfs:domain ms:Document ;
             rdfs:range rdf:langString ;
             rdfs:comment "Introduces the name of an organization that has published the document being described"@en ;
             rdfs:label "publisher"@en .


###  http://w3id.org/meta-share/meta-share/quantization
ms:quantization rdf:type owl:DatatypeProperty ;
                rdfs:domain ms:AudioFormat ;
                rdfs:range xsd:int ;
                rdfs:comment "The number of bits for each audio sample"@en ;
                rdfs:label "quantization"@en ;
                skos:note "In MS it's a controlled vocabulary (8, 16, 24, 32, 64) but I found it too much"@en .


###  http://w3id.org/meta-share/meta-share/recordingDeviceTypeDetails
ms:recordingDeviceTypeDetails rdf:type owl:DatatypeProperty ;
                              rdfs:domain [ rdf:type owl:Class ;
                                            owl:unionOf ( ms:CorpusAudioPart
                                                          ms:CorpusTextNumericalPart
                                                          ms:CorpusVideoPart
                                                        )
                                          ] ;
                              rdfs:range rdf:langString ;
                              rdfs:comment "Free text description of the recording device"@en ;
                              rdfs:label "recording device type details"@en .


###  http://w3id.org/meta-share/meta-share/recordingPlatformSoftware
ms:recordingPlatformSoftware rdf:type owl:DatatypeProperty ;
                             rdfs:domain [ rdf:type owl:Class ;
                                           owl:unionOf ( ms:CorpusAudioPart
                                                         ms:CorpusTextNumericalPart
                                                         ms:CorpusVideoPart
                                                       )
                                         ] ;
                             rdfs:range xsd:string ;
                             rdfs:comment "Specifies the software used for the recording platform"@en ;
                             rdfs:label "recording platform software"@en .


###  http://w3id.org/meta-share/meta-share/region
ms:region rdf:type owl:DatatypeProperty ;
          rdfs:domain ms:AddressSet ;
          rdfs:range rdf:langString ;
          rdfs:comment "The name of the region, county or department as mentioned in the postal address of a person or organization"@en ;
          rdfs:label "region"@en .


###  http://w3id.org/meta-share/meta-share/register
ms:register rdf:type owl:DatatypeProperty ;
            rdfs:domain ms:CorpusTextPart ;
            rdfs:range rdf:langString ;
            rdfs:comment "Specifies the type of register (any of the varieties of a language that a speaker uses in a particular social context [Merriam-Webster]) of the contents of a language resource"@en ;
            rdfs:label "register"@en .


###  http://w3id.org/meta-share/meta-share/relatedCall
ms:relatedCall rdf:type owl:DatatypeProperty ;
               rdfs:domain ms:Project ;
               rdfs:range xsd:string ;
               rdfs:comment "Specifies the Call for proposals to which a project was submitted"@en ;
               rdfs:label "related call"@en .


###  http://w3id.org/meta-share/meta-share/relatedProgramme
ms:relatedProgramme rdf:type owl:DatatypeProperty ;
                    rdfs:domain ms:Project ;
                    rdfs:range xsd:string ;
                    rdfs:comment "Specifies the funding programme to which a project was submitted"@en ;
                    rdfs:label "related programme"@en ;
                    skos:altLabel "program"@en .


###  http://w3id.org/meta-share/meta-share/relatedSubprogramme
ms:relatedSubprogramme rdf:type owl:DatatypeProperty ;
                       rdfs:domain ms:Project ;
                       rdfs:range xsd:string ;
                       rdfs:comment "Specifies the funding subprogramme to which a project was submitted"@en ;
                       rdfs:label "related subprogramme"@en .


###  http://w3id.org/meta-share/meta-share/relationType
ms:relationType rdf:type owl:DatatypeProperty ;
                rdfs:domain ms:Relation ;
                rdfs:range rdf:langString ;
                rdfs:comment "Describes in a free text statement a relation holding between two Language Resources not yet covered by the schema"@en ;
                rdfs:label "relation type"@en .


###  http://w3id.org/meta-share/meta-share/requiresSoftware
ms:requiresSoftware rdf:type owl:DatatypeProperty ;
                    rdfs:domain [ rdf:type owl:Class ;
                                  owl:unionOf ( ms:LanguageDescription
                                                ms:ToolService
                                              )
                                ] ;
                    rdfs:range xsd:string ;
                    rdfs:comment "Specifies software tools or libraries that are required for the operation of a tool/service or computational grammar"@en ;
                    rdfs:label "requires software"@en ;
                    skos:note "left as a data property - it's for more general software than language processing tools, so difficult to restrict"@en .


###  http://w3id.org/meta-share/meta-share/resourceName
ms:resourceName rdf:type owl:DatatypeProperty ;
                rdfs:subPropertyOf dct:title ;
                rdfs:domain ms:LanguageResource ;
                rdfs:range rdf:langString ;
                rdfs:comment "Introduces a human-readable name or title by which the resource is known"@en ;
                rdfs:label "resource name"@en ;
                skos:altLabel "resource title"@en ;
                skos:example "British National Corpus"@en .


###  http://w3id.org/meta-share/meta-share/resourceShortName
ms:resourceShortName rdf:type owl:DatatypeProperty ;
                     rdfs:subPropertyOf dct:alternative ;
                     rdfs:domain ms:LanguageResource ;
                     rdfs:range rdf:langString ;
                     rdfs:comment "Introduces a short form (e.g., abbreviation, acronym, etc.) used to refer to a language resource"@en ;
                     rdfs:label "resource short name"@en .


###  http://w3id.org/meta-share/meta-share/revision
ms:revision rdf:type owl:DatatypeProperty ;
            rdfs:domain [ rdf:type owl:Class ;
                          owl:unionOf ( ms:LanguageResource
                                        ms:MetadataRecord
                                      )
                        ] ;
            rdfs:range rdf:langString ;
            rdfs:comment "Provides an account of the revisions in free text or a link to a document with revisions"@en ;
            rdfs:label "revision"@en .


###  http://w3id.org/meta-share/meta-share/robustness
ms:robustness rdf:type owl:DatatypeProperty ;
              rdfs:domain ms:LanguageDescription ;
              rdfs:range rdf:langString ;
              rdfs:comment "Introduces a free text statement on the robustness of the grammar (how well the grammar can cope with misspelt/unknown, etc. input, i.e. whether it can produce even partial interpretations of the input)"@en ;
              rdfs:label "robustness"@en .


###  http://w3id.org/meta-share/meta-share/runningEnvironmentDetails
ms:runningEnvironmentDetails rdf:type owl:DatatypeProperty ;
                             rdfs:domain [ rdf:type owl:Class ;
                                           owl:unionOf ( ms:LanguageDescription
                                                         ms:ToolService
                                                       )
                                         ] ;
                             rdfs:range rdf:langString ;
                             rdfs:comment "Provides further information on the running environment of a tool/service or of a language description"@en ;
                             rdfs:label "running environment details"@en .


###  http://w3id.org/meta-share/meta-share/runningTime
ms:runningTime rdf:type owl:DatatypeProperty ;
               rdfs:domain ms:ToolService ;
               rdfs:range xsd:string ;
               rdfs:comment "Gives information on the running time of a tool or service"@en ;
               rdfs:label "running time"@en .


###  http://w3id.org/meta-share/meta-share/sampleText
ms:sampleText rdf:type owl:DatatypeProperty ;
              rdfs:domain ms:Sample ;
              rdfs:range xsd:string ;
              rdfs:comment "Introduces a short text that can be used to feed a service in order to test it"@en ;
              rdfs:label "sample text"@en .


###  http://w3id.org/meta-share/meta-share/samplesLocation
ms:samplesLocation rdf:type owl:DatatypeProperty ;
                   rdfs:subPropertyOf ms:url ;
                   rdfs:domain [ rdf:type owl:Class ;
                                 owl:unionOf ( ms:DataLanguageResource
                                               ms:DatasetDistribution
                                               ms:ProcessingResource
                                               ms:Sample
                                             )
                               ] ;
                   rdfs:range xsd:anyURI ;
                   rdfs:comment "Links a resource to a url (or url's) with samples of a data resource or of the input of output resource of a tool/service"@en ;
                   rdfs:label "samples location"@en .


###  http://w3id.org/meta-share/meta-share/samplingRate
ms:samplingRate rdf:type owl:DatatypeProperty ;
                rdfs:domain ms:AudioFormat ;
                rdfs:range xsd:int ;
                rdfs:comment "Specifies the format of files contained in the resource in Hertz"@en ;
                rdfs:label "sampling rate"@en .


###  http://w3id.org/meta-share/meta-share/sensitiveDataDetails
ms:sensitiveDataDetails rdf:type owl:DatatypeProperty ;
                        rdfs:domain ms:DataLanguageResource ;
                        rdfs:range rdf:langString ;
                        rdfs:comment "If the resource includes sensitive data, this field can be used for entering more information, e.g., whether special handling of the resource is required (e.g., anonymization, further request for use, etc.)"@en ;
                        rdfs:label "sensitive data details"@en .


###  http://w3id.org/meta-share/meta-share/sensorTechnology
ms:sensorTechnology rdf:type owl:DatatypeProperty ;
                    rdfs:domain [ rdf:type owl:Class ;
                                  owl:unionOf ( ms:CorpusAudioPart
                                                ms:CorpusImagePart
                                                ms:CorpusTextNumericalPart
                                                ms:CorpusVideoPart
                                              )
                                ] ;
                    rdfs:range xsd:string ;
                    rdfs:comment "Specifies the type of image sensor or the sensing method used in the camera or the image-capture device"@en ;
                    rdfs:label "sensor technology"@en .


###  http://w3id.org/meta-share/meta-share/series
ms:series rdf:type owl:DatatypeProperty ;
          rdfs:domain ms:Document ;
          rdfs:range rdf:langString ;
          rdfs:comment "Introduces the title of the series of a book/journal where the document being described has been published"@en ;
          rdfs:label "series"@en .


###  http://w3id.org/meta-share/meta-share/serviceAdapterDownloadLocation
ms:serviceAdapterDownloadLocation rdf:type owl:DatatypeProperty ;
                                  rdfs:subPropertyOf ms:downloadLocation ;
                                  rdfs:domain ms:ToolService ;
                                  rdfs:range xsd:string ;
                                  rdfs:comment "Τhe URL where the docker image of the service adapter can be downloaded from"@en ;
                                  rdfs:label "service adapter download location"@en .


###  http://w3id.org/meta-share/meta-share/serviceOffered
ms:serviceOffered rdf:type owl:DatatypeProperty ;
                  rdfs:domain [ rdf:type owl:Class ;
                                owl:unionOf ( ms:Division
                                              ms:Group
                                              ms:Organization
                                              ms:Person
                                            )
                              ] ;
                  rdfs:range rdf:langString ;
                  rdfs:comment "Lists the service(s) offered by an organization or person"@en ;
                  rdfs:label "service offered"@en .


###  http://w3id.org/meta-share/meta-share/shallowness
ms:shallowness rdf:type owl:DatatypeProperty ;
               rdfs:domain ms:LanguageDescription ;
               rdfs:range rdf:langString ;
               rdfs:comment "Introduces a free text statement on the shallowness of the grammar (how deep the syntactic analysis performed by the grammar can be)"@en ;
               rdfs:label "shallowness"@en .


###  http://w3id.org/meta-share/meta-share/shortBio
ms:shortBio rdf:type owl:DatatypeProperty ;
            rdfs:subPropertyOf dct:description ;
            rdfs:domain ms:Person ;
            rdfs:range rdf:langString ;
            rdfs:comment "Introduces a free text that can be used as a short bio for a person"@en ;
            rdfs:label "short bio"@en .


###  http://w3id.org/meta-share/meta-share/sizeHeight
ms:sizeHeight rdf:type owl:DatatypeProperty ;
              rdfs:domain ms:Resolution ;
              rdfs:range xsd:int ;
              rdfs:comment "The frame height in pixels"@en ;
              rdfs:label "size height"@en .


###  http://w3id.org/meta-share/meta-share/sizeText
ms:sizeText rdf:type owl:DatatypeProperty ;
            rdfs:domain ms:Size ;
            rdfs:range rdf:langString ;
            rdfs:comment "Specifies the size of a resource in the form of a free text"@en ;
            rdfs:label "size (free text)"@en .


###  http://w3id.org/meta-share/meta-share/sizeWidth
ms:sizeWidth rdf:type owl:DatatypeProperty ;
             rdfs:domain ms:Resolution ;
             rdfs:range xsd:int ;
             rdfs:comment "The frame width in pixels"@en ;
             rdfs:label "size width"@en .


###  http://w3id.org/meta-share/meta-share/smokingHabit
ms:smokingHabit rdf:type owl:DatatypeProperty ;
                rdfs:domain ms:Participant ;
                rdfs:range rdf:langString ;
                rdfs:comment "Provides information on whether the participant smokes and on his/her smoking habits in general"@en ;
                rdfs:label "smoking habit"@en .


###  http://w3id.org/meta-share/meta-share/smoothing
ms:smoothing rdf:type owl:DatatypeProperty ;
             rdfs:domain ms:NGramModel ;
             rdfs:range xsd:string ;
             rdfs:comment "The technique used for giving unseen items some probability"@en ;
             rdfs:label "smoothing"@en .


###  http://w3id.org/meta-share/meta-share/sourceChannelDetails
ms:sourceChannelDetails rdf:type owl:DatatypeProperty ;
                        rdfs:domain [ rdf:type owl:Class ;
                                      owl:unionOf ( ms:CorpusAudioPart
                                                    ms:CorpusTextNumericalPart
                                                    ms:CorpusVideoPart
                                                  )
                                    ] ;
                        rdfs:range rdf:langString ;
                        rdfs:comment "Provides information on the details of the channel equipment used (brand, type, etc.) in free text"@en ;
                        rdfs:label "source channel details"@en .


###  http://w3id.org/meta-share/meta-share/sourceChannelName
ms:sourceChannelName rdf:type owl:DatatypeProperty ;
                     rdfs:domain [ rdf:type owl:Class ;
                                   owl:unionOf ( ms:CorpusAudioPart
                                                 ms:CorpusTextNumericalPart
                                                 ms:CorpusVideoPart
                                               )
                                 ] ;
                     rdfs:range rdf:langString ;
                     rdfs:comment "Introduces the name of the source channel through which the recording has been made"@en ;
                     rdfs:label "source channel name"@en .


###  http://w3id.org/meta-share/meta-share/speakingImpairment
ms:speakingImpairment rdf:type owl:DatatypeProperty ;
                      rdfs:domain ms:Participant ;
                      rdfs:range rdf:langString ;
                      rdfs:comment "Provides information on any speaking impairment the participant may have"@en ;
                      rdfs:label "speaking impairment"@en .


###  http://w3id.org/meta-share/meta-share/startup
ms:startup rdf:type owl:DatatypeProperty ;
           rdfs:domain [ rdf:type owl:Class ;
                         owl:unionOf ( ms:Division
                                       ms:Organization
                                     )
                       ] ;
           rdfs:range xsd:boolean ;
           rdfs:comment "Indicates whether a company is a startup"@en ;
           rdfs:label "startup"@en .


###  http://w3id.org/meta-share/meta-share/status
ms:status rdf:type owl:DatatypeProperty ;
          rdfs:domain ms:Project ;
          rdfs:range xsd:string ;
          rdfs:comment "Specifies the status in which a project is found in the course of a funding process (e.g. approved, signed, under negotiation, etc.)"@en ;
          rdfs:label "status"@en .


###  http://w3id.org/meta-share/meta-share/subtitle
ms:subtitle rdf:type owl:DatatypeProperty ;
            rdfs:subPropertyOf dct:alternative ;
            rdfs:domain ms:Document ;
            rdfs:range rdf:langString ;
            rdfs:comment "Introduces a secondary title used for a document"@en ;
            rdfs:label "subtitle"@en .


###  http://w3id.org/meta-share/meta-share/surname
ms:surname rdf:type owl:DatatypeProperty ;
           rdfs:domain ms:Person ;
           rdfs:range rdf:langString ;
           rdfs:comment "Introduces the surname (i.e. the name shared by members of a family, also known as \"family name\" or \"last name\") of a person"@en ;
           rdfs:label "surname"@en ;
           skos:altLabel "family name"@en ,
                         "last name"@en .


###  http://w3id.org/meta-share/meta-share/synchronizedWithAudio
ms:synchronizedWithAudio rdf:type owl:DatatypeProperty ;
                         rdfs:domain ms:LinkToOtherMedia ;
                         rdfs:range xsd:boolean ;
                         rdfs:comment "Whether the media part described is synchronized with audio within the same resource"@en ;
                         rdfs:label "synchronized with audio"@en .


###  http://w3id.org/meta-share/meta-share/synchronizedWithImage
ms:synchronizedWithImage rdf:type owl:DatatypeProperty ;
                         rdfs:domain ms:LinkToOtherMedia ;
                         rdfs:range xsd:boolean ;
                         rdfs:comment "Whether the media part described is synchronized with image within the same resource"@en ;
                         rdfs:label "synchronized with image"@en .


###  http://w3id.org/meta-share/meta-share/synchronizedWithText
ms:synchronizedWithText rdf:type owl:DatatypeProperty ;
                        rdfs:domain ms:LinkToOtherMedia ;
                        rdfs:range xsd:boolean ;
                        rdfs:comment "Whether video, text and textNumerical media type is synchronized with text within the same resource"@en ;
                        rdfs:label "synchronized with text"@en .


###  http://w3id.org/meta-share/meta-share/synchronizedWithTextNumerical
ms:synchronizedWithTextNumerical rdf:type owl:DatatypeProperty ;
                                 rdfs:domain ms:LinkToOtherMedia ;
                                 rdfs:range xsd:boolean ;
                                 rdfs:comment "Whether the media part described is synchronized with textNumerical within the same resource"@en ;
                                 rdfs:label "synchronized with textNumerical"@en .


###  http://w3id.org/meta-share/meta-share/synchronizedWithVideo
ms:synchronizedWithVideo rdf:type owl:DatatypeProperty ;
                         rdfs:domain ms:LinkToOtherMedia ;
                         rdfs:range xsd:boolean ;
                         rdfs:comment "Whether the media part described is synchronized with video within the same resource"@en ;
                         rdfs:label "synchronized with video"@en .


###  http://w3id.org/meta-share/meta-share/syntheticData
ms:syntheticData rdf:type owl:DatatypeProperty ;
                 rdfs:domain ms:CorpusMediaPart ;
                 rdfs:range xsd:boolean ;
                 rdfs:comment "Specifies whether the contents of a corpus have been artificially generated (e.g., using a Machine Translation or NLG system) rather than having been created by humans (authentic/original data)"@en ;
                 rdfs:label "synthetic data"@en .


###  http://w3id.org/meta-share/meta-share/tag
ms:tag rdf:type owl:DatatypeProperty ;
       rdfs:domain ms:Sample ;
       rdfs:range xsd:string ;
       rdfs:comment "Introduces a tag that can be used as a criterion for selecting different samples for testing (e.g. the language value for Machine Translation services that operate on multiple languages)"@en ;
       rdfs:label "tag"@en .


###  http://w3id.org/meta-share/meta-share/telephoneNumber
ms:telephoneNumber rdf:type owl:DatatypeProperty ;
                   rdfs:domain [ rdf:type owl:Class ;
                                 owl:unionOf ( ms:Division
                                               ms:Group
                                               ms:Organization
                                               ms:Person
                                             )
                               ] ;
                   rdfs:range xsd:string .


###  http://w3id.org/meta-share/meta-share/theoreticModel
ms:theoreticModel rdf:type owl:DatatypeProperty ;
                  rdfs:domain [ rdf:type owl:Class ;
                                owl:unionOf ( ms:Annotation
                                              ms:LanguageDescription
                                              ms:LexicalConceptualResource
                                            )
                              ] ;
                  rdfs:range rdf:langString ;
                  rdfs:comment "Indicates the theoretic model applied for the creation/enrichment of the resource, by name and/or by reference (URL or bibliographic reference) to informative material about the theoretic model used"@en ;
                  rdfs:label "theoretic model"@en .


###  http://w3id.org/meta-share/meta-share/thingDescription
ms:thingDescription rdf:type owl:DatatypeProperty ;
                    rdfs:domain ms:StaticElement ;
                    rdfs:range rdf:langString ;
                    rdfs:comment "Provides description of the things represented in the image corpus"@en ;
                    rdfs:label "thing description"@en .


###  http://w3id.org/meta-share/meta-share/timeCoverage
ms:timeCoverage rdf:type owl:DatatypeProperty ;
                rdfs:domain [ rdf:type owl:Class ;
                              owl:unionOf ( ms:Corpus
                                            ms:LanguageDescription
                                            ms:LexicalConceptualResource
                                            ms:Subset
                                          )
                            ] ;
                rdfs:range rdf:langString ;
                rdfs:comment "Indicates the time period that the content of a resource is about"@en ;
                rdfs:label "time coverage"@en .


###  http://w3id.org/meta-share/meta-share/title
ms:title rdf:type owl:DatatypeProperty ;
         rdfs:subPropertyOf dct:title ;
         rdfs:domain ms:Document ;
         rdfs:range rdf:langString ;
         rdfs:comment "Introduces a human-readable text (typically short) used as a name for referring to the document being described"@en ;
         rdfs:label "title"@en .


###  http://w3id.org/meta-share/meta-share/trainedSpeaker
ms:trainedSpeaker rdf:type owl:DatatypeProperty ;
                  rdfs:domain ms:Participant ;
                  rdfs:range xsd:boolean ;
                  rdfs:comment "Provides information on whether the participant is trained in a specific task"@en ;
                  rdfs:label "trained speaker"@en .


###  http://w3id.org/meta-share/meta-share/trainingCorpusDetails
ms:trainingCorpusDetails rdf:type owl:DatatypeProperty ;
                         rdfs:domain ms:MLModel ;
                         rdfs:range rdf:langString ;
                         rdfs:comment "Provides a detailed description of the training corpus (e.g., size, number of features, etc.)"@en ;
                         rdfs:label "training corpus details"@en .


###  http://w3id.org/meta-share/meta-share/trainingProcessDetails
ms:trainingProcessDetails rdf:type owl:DatatypeProperty ;
                          rdfs:domain ms:MLModel ;
                          rdfs:range rdf:langString ;
                          rdfs:comment "Provides a detailed description of the training process (pre-processing, pretraining, etc.)"@en ;
                          rdfs:label "training process details"@en .


###  http://w3id.org/meta-share/meta-share/typeOfElement
ms:typeOfElement rdf:type owl:DatatypeProperty ;
                 rdfs:domain [ rdf:type owl:Class ;
                               owl:unionOf ( ms:DynamicElement
                                             ms:StaticElement
                                           )
                             ] ;
                 rdfs:range rdf:langString ;
                 rdfs:comment "Specifies the type of objects or people represented in the video or image part of the resource"@en ;
                 rdfs:label "type of element"@en .


###  http://w3id.org/meta-share/meta-share/typeOfImageContent
ms:typeOfImageContent rdf:type owl:DatatypeProperty ;
                      rdfs:domain [ rdf:type owl:Class ;
                                    owl:unionOf ( ms:CorpusImagePart
                                                  ms:LanguageDescriptionImagePart
                                                  ms:LexicalConceptualResourceImagePart
                                                )
                                  ] ;
                      rdfs:range rdf:langString ;
                      rdfs:comment "The main types of object or people represented in the image corpus"@en ;
                      rdfs:label "type of image content"@en .


###  http://w3id.org/meta-share/meta-share/typeOfTextNumericalContent
ms:typeOfTextNumericalContent rdf:type owl:DatatypeProperty ;
                              rdfs:domain ms:CorpusTextNumericalPart ;
                              rdfs:range rdf:langString ;
                              rdfs:comment "Specifies the content that is represented in the textNumerical part of the resource"@en ;
                              rdfs:label "type of textNumerical content"@en .


###  http://w3id.org/meta-share/meta-share/typeOfVideoContent
ms:typeOfVideoContent rdf:type owl:DatatypeProperty ;
                      rdfs:domain [ rdf:type owl:Class ;
                                    owl:unionOf ( ms:CorpusVideoPart
                                                  ms:LanguageDescriptionVideoPart
                                                  ms:LexicalConceptualResourceVideoPart
                                                )
                                  ] ;
                      rdfs:range rdf:langString ;
                      rdfs:comment "Main type of object or people represented in the video"@en ;
                      rdfs:label "type of video content"@en .


###  http://w3id.org/meta-share/meta-share/unitOfMeasureMetric
ms:unitOfMeasureMetric rdf:type owl:DatatypeProperty ;
                       rdfs:domain ms:PerformanceIndicator ;
                       rdfs:range xsd:string ;
                       rdfs:comment "Identifies the unit of measure used in the calculation of the metric (for the evaluation of a tool/service)"@en ;
                       rdfs:label "unit of measure"@en .


###  http://w3id.org/meta-share/meta-share/updateFrequency
ms:updateFrequency rdf:type owl:DatatypeProperty ;
                   rdfs:domain ms:LanguageResource ;
                   rdfs:range rdf:langString ;
                   rdfs:comment "Specifies the frequency with which the resource is updated"@en ;
                   rdfs:label "update frequency"@en .


###  http://w3id.org/meta-share/meta-share/url
ms:url rdf:type owl:DatatypeProperty ;
       rdfs:domain owl:Thing ;
       rdfs:range xsd:anyURI ;
       rdfs:comment "Links to a URL"@en ;
       rdfs:label "has URL"@en .


###  http://w3id.org/meta-share/meta-share/userQuery
ms:userQuery rdf:type owl:DatatypeProperty ;
             rdfs:domain ms:Corpus ;
             rdfs:range xsd:string ;
             rdfs:comment "Introduces a query performed by a user that has resulted in the creation of the resource being described (e.g. a dataset created with a query aggregating texts from a database, or subset of a lexical resource, or a virtual collection of sentences from online corpora)"@en ;
             rdfs:label "user query"@en .


###  http://w3id.org/meta-share/meta-share/validated
ms:validated rdf:type owl:DatatypeProperty ;
             rdfs:domain ms:LanguageResource ;
             rdfs:range xsd:boolean ;
             rdfs:comment "Specifies whether the resource has undergone a formal validation process"@en ;
             rdfs:label "validated"@en .


###  http://w3id.org/meta-share/meta-share/validationDetails
ms:validationDetails rdf:type owl:DatatypeProperty ;
                     rdfs:domain ms:Validation ;
                     rdfs:range rdf:langString ;
                     rdfs:comment "Provides additional information in the form of free text about the validation process of a language resource"@en ;
                     rdfs:label "validation details"@en .


###  http://w3id.org/meta-share/meta-share/valueDescription
ms:valueDescription rdf:type owl:DatatypeProperty ;
                    rdfs:domain ms:EnumerationValue ;
                    rdfs:range rdf:langString ;
                    rdfs:comment "Introduces a short free text used to show to the user as a tip for the value of a list used in parameters"@en ;
                    rdfs:label "value description"@en .


###  http://w3id.org/meta-share/meta-share/valueLabel
ms:valueLabel rdf:type owl:DatatypeProperty ;
              rdfs:domain ms:EnumerationValue ;
              rdfs:range rdf:langString ;
              rdfs:comment "Introduces a short free text used to show to the user for the value of a list used in parameters"@en ;
              rdfs:label "value label"@en .


###  http://w3id.org/meta-share/meta-share/valueName
ms:valueName rdf:type owl:DatatypeProperty ;
             rdfs:domain ms:EnumerationValue ;
             rdfs:range xsd:string ;
             rdfs:comment "Introduces a free text used to identify the value of a list inside parameters"@en ;
             rdfs:label "value name"@en .


###  http://w3id.org/meta-share/meta-share/version
ms:version rdf:type owl:DatatypeProperty ;
           rdfs:subPropertyOf dct:hasVersion ;
           rdfs:domain ms:LanguageResource ;
           rdfs:range xsd:string ;
           rdfs:comment "Associates a language resource with a pattern that indicates its version; the recommended way is to follow the semantic versioning guidelines (http://semver.org) and use a numeric pattern of the form major_version.minor_version.patch"@en ;
           rdfs:label "version"@en .


###  http://w3id.org/meta-share/meta-share/versionDate
ms:versionDate rdf:type owl:DatatypeProperty ;
               rdfs:domain ms:LanguageResource ;
               rdfs:range xsd:date ;
               rdfs:comment "Identifies the date associated with the version of the language resource being described (as a recommendation, of the latest update of the particular version)"@en ;
               rdfs:label "version date"@en .


###  http://w3id.org/meta-share/meta-share/volume
ms:volume rdf:type owl:DatatypeProperty ;
          rdfs:domain ms:Document ;
          rdfs:range xsd:string ;
          rdfs:comment "Introduces the number used for the volume of a journal or a series of publications"@en ;
          rdfs:label "volume"@en .


###  http://w3id.org/meta-share/meta-share/website
ms:website rdf:type owl:DatatypeProperty ;
           rdfs:subPropertyOf ms:url ;
           rdfs:domain [ rdf:type owl:Class ;
                         owl:unionOf ( ms:Division
                                       ms:Group
                                       ms:Organization
                                       ms:Project
                                     )
                       ] ;
           rdfs:range xsd:anyURI ;
           rdfs:comment "Links to a URL that acts as the primary page (like a table of contents) introducing information about an organization (e.g., products, contact information, etc.) or project"@en ;
           rdfs:label "website"@en ;
           skos:altLabel "home page"@en .


###  http://w3id.org/meta-share/meta-share/weight
ms:weight rdf:type owl:DatatypeProperty ;
          rdfs:domain ms:Participant ;
          rdfs:range xsd:int ;
          rdfs:comment "Provides information on the weight of the participant"@en ;
          rdfs:label "weight"@en .


###  http://w3id.org/meta-share/meta-share/weightedGrammar
ms:weightedGrammar rdf:type owl:DatatypeProperty ;
                   rdfs:domain ms:LanguageDescription ;
                   rdfs:range xsd:boolean ;
                   rdfs:comment "Indicates whether the grammar contains numerical weights (incl. probabilities)"@en ;
                   rdfs:label "weighted grammar"@en .


###  http://w3id.org/meta-share/meta-share/zipCode
ms:zipCode rdf:type owl:DatatypeProperty ;
           rdfs:domain ms:AddressSet ;
           rdfs:range xsd:string ;
           rdfs:comment "The zip code of the postal address of a person or organization "@en ;
           rdfs:label "zip code"@en .


###  http://www.w3.org/ns/dcat#endDate
dcat:endDate rdf:type owl:DatatypeProperty ;
             rdfs:domain dct:PeriodOfTime ;
             rdfs:range xsd:date ;
             rdfs:comment "The end date of an activity"@en ;
             rdfs:label "end date"@en .


###  http://www.w3.org/ns/dcat#startDate
dcat:startDate rdf:type owl:DatatypeProperty ;
               rdfs:domain dct:PeriodOfTime ;
               rdfs:range xsd:date ;
               rdfs:comment "The start date of an activity"@en ;
               rdfs:label "start date"@en .


#################################################################
#    Classes
#################################################################

###  http://creativecommons.org/ns#License
cc:License rdf:type owl:Class .


###  http://purl.org/dc/terms/LinguisticSystem
dct:LinguisticSystem rdf:type owl:Class .


###  http://purl.org/dc/terms/Location
dct:Location rdf:type owl:Class ;
             rdfs:label "Location"@en .


###  http://purl.org/dc/terms/MediaType
dct:MediaType rdf:type owl:Class .


###  http://purl.org/dc/terms/PeriodOfTime
dct:PeriodOfTime rdf:type owl:Class ;
                 rdfs:label "Period of time"@en .


###  http://purl.org/spar/datacite/AgentIdentifier
datacite:AgentIdentifier rdf:type owl:Class ;
                         rdfs:subClassOf datacite:Identifier .


###  http://purl.org/spar/datacite/AgentIdentifierScheme
datacite:AgentIdentifierScheme rdf:type owl:Class ;
                               rdfs:subClassOf datacite:IdentifierScheme .


###  http://purl.org/spar/datacite/FunderIdentifier
datacite:FunderIdentifier rdf:type owl:Class ;
                          rdfs:subClassOf datacite:AgentIdentifier ,
                                          [ rdf:type owl:Restriction ;
                                            owl:onProperty datacite:usesIdentifierScheme ;
                                            owl:allValuesFrom datacite:FunderIdentifierScheme
                                          ] .


###  http://purl.org/spar/datacite/FunderIdentifierScheme
datacite:FunderIdentifierScheme rdf:type owl:Class ;
                                rdfs:subClassOf datacite:AgentIdentifierScheme ;
                                rdfs:comment "The name of the scheme used to identify a funder"@en ;
                                rdfs:label "Funder identfier scheme"@en .


###  http://purl.org/spar/datacite/Identifier
datacite:Identifier rdf:type owl:Class .


###  http://purl.org/spar/datacite/IdentifierScheme
datacite:IdentifierScheme rdf:type owl:Class .


###  http://purl.org/spar/datacite/OrganizationIdentifier
datacite:OrganizationIdentifier rdf:type owl:Class ;
                                rdfs:subClassOf datacite:AgentIdentifier ,
                                                [ rdf:type owl:Restriction ;
                                                  owl:onProperty datacite:usesIdentifierScheme ;
                                                  owl:allValuesFrom datacite:OrganizationIdentifierScheme
                                                ] ;
                                rdfs:comment "A string used to uniquely identify an organization"@en ;
                                rdfs:label "Organization identifier"@en ;
                                skos:altLabel "Organisation identifier"@en-uk .


###  http://purl.org/spar/datacite/OrganizationIdentifierScheme
datacite:OrganizationIdentifierScheme rdf:type owl:Class ;
                                      rdfs:subClassOf datacite:AgentIdentifierScheme ;
                                      rdfs:comment "The name of the scheme used to identify an organization"@en ;
                                      rdfs:label "Organization identifier scheme"@en .


###  http://purl.org/spar/datacite/PersonalIdentifier
datacite:PersonalIdentifier rdf:type owl:Class ;
                            rdfs:subClassOf datacite:AgentIdentifier ,
                                            [ rdf:type owl:Restriction ;
                                              owl:onProperty datacite:usesIdentifierScheme ;
                                              owl:allValuesFrom datacite:PersonalIdentifierScheme
                                            ] ;
                            rdfs:comment "A string (e.g., PID, DOI, internal to an organization, etc.) used to uniquely identify a person"@en ;
                            rdfs:label "Person identifier"@en .


###  http://purl.org/spar/datacite/PersonalIdentifierScheme
datacite:PersonalIdentifierScheme rdf:type owl:Class ;
                                  rdfs:subClassOf datacite:AgentIdentifierScheme ;
                                  rdfs:comment "The name of the scheme used to identify a person"@en ;
                                  rdfs:label "Person identfier scheme"@en .


###  http://purl.org/spar/datacite/ResourceIdentifier
datacite:ResourceIdentifier rdf:type owl:Class ;
                            rdfs:subClassOf datacite:Identifier .


###  http://purl.org/spar/datacite/ResourceIdentifierScheme
datacite:ResourceIdentifierScheme rdf:type owl:Class ;
                                  rdfs:subClassOf datacite:IdentifierScheme ;
                                  rdfs:comment "The name of the scheme used to identify a resource"@en ;
                                  rdfs:label "Resource identifier scheme"@en .


###  http://w3id.org/meta-share/meta-share/AcademicUse
ms:AcademicUse rdf:type owl:Class ;
               rdfs:subClassOf odrl:RightOperand ;
               rdfs:comment "The use of a resource only for academic purposes (academic research, educational purposes)"@en ;
               rdfs:label "Academic use"@en .


###  http://w3id.org/meta-share/meta-share/AccessRightsStatement
ms:AccessRightsStatement rdf:type owl:Class ;
                         rdfs:subClassOf skos:Concept ,
                                         [ rdf:type owl:Restriction ;
                                           owl:onProperty datacite:hasIdentifier ;
                                           owl:allValuesFrom ms:AccessRightsStatementIdentifier
                                         ] ;
                         rdfs:comment "A formal statement indicative of licensing terms for the use of a resource (e.g., open access, free to read, etc.); its semantics should be clear, preferably formally expressed and documented at a URL"@en ;
                         rdfs:label "Access rights statement"@en ;
                         skos:inScheme ms:AccessRightsStatements .


###  http://w3id.org/meta-share/meta-share/AccessRightsStatementIdentifier
ms:AccessRightsStatementIdentifier rdf:type owl:Class ;
                                   rdfs:subClassOf datacite:Identifier ,
                                                   [ rdf:type owl:Restriction ;
                                                     owl:onProperty ms:conformsTo ;
                                                     owl:allValuesFrom ms:AccessRightsStatementScheme
                                                   ] ;
                                   rdfs:comment "A string used to uniquely identify an access rights statement according to a specific scheme"@en ;
                                   rdfs:label "Access rights statement identifier"@en .


###  http://w3id.org/meta-share/meta-share/AccessRightsStatementScheme
ms:AccessRightsStatementScheme rdf:type owl:Class ;
                               rdfs:subClassOf ms:ClassificationScheme ;
                               rdfs:comment "The name of the scheme according to which an access rights statement is assigned to a distribution"@en ;
                               rdfs:label "Access rights statement scheme"@en .


###  http://w3id.org/meta-share/meta-share/Actor
ms:Actor rdf:type owl:Class ;
         rdfs:subClassOf ms:DescribedEntity ;
         rdfs:comment "A person, organization or group that participates in an event or process"@en ;
         rdfs:label "Actor"@en ;
         skos:note "Changed to subclass of foaf:agent because according to its definition (An agent (eg. person, group, software or physical artifact)), it might include entities that we do not consider at this time actors"@en .


###  http://w3id.org/meta-share/meta-share/ActualUse
ms:ActualUse rdf:type owl:Class ;
             rdfs:comment "Any activity where a language resource has been used (e.g., in a project, in an experiment, for a publication, etc.)"@en ;
             rdfs:label "Actual use"@en .


###  http://w3id.org/meta-share/meta-share/AddressSet
ms:AddressSet rdf:type owl:Class ;
              rdfs:comment "The physical address of an organization, group or person expressed in the form of distinct elements (street address, zip code, city, etc.)"@en ;
              rdfs:label "Address"@en .


###  http://w3id.org/meta-share/meta-share/Affiliation
ms:Affiliation rdf:type owl:Class ;
               rdfs:comment "Information the organization that a person works for (e.g., a company) or is affiliated with (e.g., university, etc.) and the data that are specific to this relation (e.g., position, professional contact information, etc.)"@en ;
               rdfs:label "Affiliation"@en .


###  http://w3id.org/meta-share/meta-share/AgeGroup
ms:AgeGroup rdf:type owl:Class ;
            rdfs:comment "The age group to which the participant belongs"@en ;
            rdfs:label "Age group"@en .


###  http://w3id.org/meta-share/meta-share/AnnotatedElement
ms:AnnotatedElement rdf:type owl:Class ;
                    rdfs:comment "A type of element that can be annotated and may differ depending on the annotation level"@en ;
                    rdfs:label "Annotated element"@en .


###  http://w3id.org/meta-share/meta-share/Annotation
ms:Annotation rdf:type owl:Class ;
              rdfs:comment "The part of a corpus that contains annotations (interpretative linguistic information grounded in a knowledge resource that is added manually or automatically to a text or corpus respectively)"@en ;
              rdfs:label "Annotation"@en .


###  http://w3id.org/meta-share/meta-share/Anonymized
ms:Anonymized rdf:type owl:Class ;
              rdfs:comment "Indication of whether the language resource has been anonymized"@en ;
              rdfs:label "Anonymized"@en .


###  http://w3id.org/meta-share/meta-share/Application
ms:Application rdf:type owl:Class ;
               rdfs:subClassOf ms:ToolService ;
               rdfs:comment "Any software program (or group of programs seen as a whole) intended for the end-user and addressing one or multiple related user needs."@en ;
               rdfs:label "Application"@en .


###  http://w3id.org/meta-share/meta-share/Attribution
ms:Attribution rdf:type owl:Class ;
               rdfs:comment "Relation of attribution between language resource and an agent"@en ;
               rdfs:label "Attribution"@en .


###  http://w3id.org/meta-share/meta-share/Audience
ms:Audience rdf:type owl:Class ;
            rdfs:comment "Indication of the intended audience size of a multimedia resource"@en ;
            rdfs:label "Audience"@en .


###  http://w3id.org/meta-share/meta-share/AudioFormat
ms:AudioFormat rdf:type owl:Class ;
               rdfs:comment "The format of the audio part of a multimedia resource"@en ;
               rdfs:label "Detailed audio format"@en .


###  http://w3id.org/meta-share/meta-share/AudioGenre
ms:AudioGenre rdf:type owl:Class ;
              rdfs:subClassOf ms:Genre ,
                              [ rdf:type owl:Restriction ;
                                owl:onProperty datacite:hasIdentifier ;
                                owl:allValuesFrom ms:AudioGenreIdentifier
                              ] ,
                              [ rdf:type owl:Restriction ;
                                owl:onProperty ms:genre ;
                                owl:allValuesFrom ms:CorpusAudioPart
                              ] ;
              rdfs:comment "A classification of audio parts based on extra-linguistic and internal linguistic criteria and reflected on the audio style, form or content"@en ;
              rdfs:label "Audio genre"@en .


###  http://w3id.org/meta-share/meta-share/AudioGenreClassificationScheme
ms:AudioGenreClassificationScheme rdf:type owl:Class ;
                                  rdfs:subClassOf ms:ClassificationScheme ;
                                  rdfs:comment "A classification scheme devised for audio genres by an organization/authority"@en ;
                                  rdfs:label "Audio genre classification scheme"@en .


###  http://w3id.org/meta-share/meta-share/AudioGenreIdentifier
ms:AudioGenreIdentifier rdf:type owl:Class ;
                        rdfs:subClassOf datacite:Identifier ,
                                        [ rdf:type owl:Restriction ;
                                          owl:onProperty ms:conformsTo ;
                                          owl:allValuesFrom ms:AudioGenreClassificationScheme
                                        ] ;
                        rdfs:comment "A string used to uniquely identify an audio genre according to a specific classification scheme"@en ;
                        rdfs:label "Audio genre identifier"@en .


###  http://w3id.org/meta-share/meta-share/AudioQualityMeasureIncluded
ms:AudioQualityMeasureIncluded rdf:type owl:Class ;
                               rdfs:comment "The audio quality measures included in audio format"@en ;
                               rdfs:label "Audio quality measure included"@en .


###  http://w3id.org/meta-share/meta-share/Authorize
ms:Authorize rdf:type owl:Class ;
             rdfs:comment "Authorize the use of a resource by an individual"@en ;
             rdfs:label "Authorize"@en .


###  http://w3id.org/meta-share/meta-share/Availability
ms:Availability rdf:type owl:Class ;
                rdfs:comment "Availability status of the resource; conditionsOfUse can be further used to indicate the specific terms of availability"@en ;
                rdfs:label "Availability"@en ;
                skos:note "Is there a point of keeping it? makes sense only for \"under negotiation\" and 'availableThroughOtherDistributors' [change the value]; maybe also \"availableThroughOwnerOnly\"???"@en .


###  http://w3id.org/meta-share/meta-share/BaseItem
ms:BaseItem rdf:type owl:Class ;
            rdfs:comment "Type of item that is represented in the n-gram resource"@en ;
            rdfs:label "Base item"@en .


###  http://w3id.org/meta-share/meta-share/BodyPart
ms:BodyPart rdf:type owl:Class ;
            rdfs:comment "The body parts visible in the video or image part of the resource"@en ;
            rdfs:label "Body part"@en .


###  http://w3id.org/meta-share/meta-share/ByteOrder
ms:ByteOrder rdf:type owl:Class ;
             rdfs:comment "The byte order of 2 or more bytes sample"@en ;
             rdfs:label "Byte order"@en .


###  http://w3id.org/meta-share/meta-share/CapturingDeviceType
ms:CapturingDeviceType rdf:type owl:Class ;
                       rdfs:comment "The type of transducers through which the data is captured"@en ;
                       rdfs:label "Capturing device type"@en .


###  http://w3id.org/meta-share/meta-share/CapturingEnvironment
ms:CapturingEnvironment rdf:type owl:Class ;
                        rdfs:comment "The type of the capturing environment in terms of complexity"@en ;
                        rdfs:label "Capturing environment"@en .


###  http://w3id.org/meta-share/meta-share/CharacterEncoding
ms:CharacterEncoding rdf:type owl:Class ;
                     rdfs:comment "The name of the character encoding used in the resource or accepted by the tool/service"@en ;
                     rdfs:label "Character encoding"@en .


###  http://w3id.org/meta-share/meta-share/Classification
ms:Classification rdf:type owl:Class ;
                  rdfs:comment "A type of classifying (arranging in groups/categories) language resources"@en ;
                  rdfs:label "Classification"@en .


###  http://w3id.org/meta-share/meta-share/ClassificationScheme
ms:ClassificationScheme rdf:type owl:Class ;
                        rdfs:comment "Scheme used for the classification of a language resource based on various criteria (e.g., domains, text types, genres, etc.)"@en ;
                        rdfs:label "Classification scheme"@en .


###  http://w3id.org/meta-share/meta-share/ColourSpace
ms:ColourSpace rdf:type owl:Class ;
               rdfs:comment "The colour space for the video and image part(s) of a resource"@en ;
               rdfs:label "Colour space"@en .


###  http://w3id.org/meta-share/meta-share/Combine
ms:Combine rdf:type owl:Class ;
           rdfs:subClassOf odrl:Action ;
           rdfs:comment "Combine two or more resources of different resource types (e.g. a model and a tool/service) in order to deploy them together"@en ;
           rdfs:label "Combine"@en .


###  http://w3id.org/meta-share/meta-share/CompatibleLexiconType
ms:CompatibleLexiconType rdf:type owl:Class ;
                         rdfs:comment "A classification into types for lexical lexicon that can be used with the grammar being described"@en ;
                         rdfs:label "Compatible lexicon type"@en .


###  http://w3id.org/meta-share/meta-share/Component
ms:Component rdf:type owl:Class ;
             rdfs:subClassOf ms:ToolService ;
             rdfs:comment "A piece of software typically intended for a specific technical purpose, such as a particular implementation of a part-of-speech tagger (e.g TreeTagger), a tree parsing program (e.g., mstparser), etc. It is wrapped in a standard way within a particular component-oriented framework such as UIMA, GATE, etc. or as a specific type of web service."@en ;
             rdfs:label "Component"@en .


###  http://w3id.org/meta-share/meta-share/CompressionName
ms:CompressionName rdf:type owl:Class ;
                   rdfs:comment "The name of the compression applied"@en ;
                   rdfs:label "Compression name"@en .


###  http://w3id.org/meta-share/meta-share/ConditionOfUse
ms:ConditionOfUse rdf:type owl:Class ;
                  dct:replaces msxml:restrictionsOfUse ;
                  rdfs:comment "A condition imposed via a specified licence on the use of a language resource (e.g., non-commercial use, no derivatives, etc.)"@en ;
                  rdfs:label "Condition of use"@en .


###  http://w3id.org/meta-share/meta-share/ConversationalType
ms:ConversationalType rdf:type owl:Class ;
                      rdfs:comment "Classification of the conversation included in a multimedia resource based on the number of participants"@en ;
                      rdfs:label "Conversational type"@en .


###  http://w3id.org/meta-share/meta-share/Corpus
ms:Corpus rdf:type owl:Class ;
          rdfs:subClassOf ms:DataLanguageResource ,
                          [ rdf:type owl:Restriction ;
                            owl:onProperty ms:distribution ;
                            owl:allValuesFrom ms:DatasetDistribution
                          ] ;
          rdfs:comment "A structured collection of pieces of data (textual, audio, video, multimodal/multimedia, etc.) typically of considerable size and selected according to criteria external to the data (e.g., size, type of language, type of text producers or expected audience, etc.) to represent as comprehensively as possible the object of study"@en ;
          rdfs:label "Corpus"@en .


###  http://w3id.org/meta-share/meta-share/CorpusAudioPart
ms:CorpusAudioPart rdf:type owl:Class ;
                   rdfs:subClassOf ms:CorpusMediaPart ;
                   rdfs:comment "The part of a corpus (or whole corpus) that consists of audio segments"@en ;
                   rdfs:label "Corpus audio part"@en .


###  http://w3id.org/meta-share/meta-share/CorpusImagePart
ms:CorpusImagePart rdf:type owl:Class ;
                   rdfs:subClassOf ms:CorpusMediaPart ;
                   rdfs:comment "The part of a corpus (or whole corpus) that consists of images (e.g., g a corpus of photographs and their captions)"@en ;
                   rdfs:label "Corpus image part"@en .


###  http://w3id.org/meta-share/meta-share/CorpusMediaPart
ms:CorpusMediaPart rdf:type owl:Class ;
                   rdfs:subClassOf ms:MediaPart ;
                   rdfs:comment "A part/segment of a corpus based on its media type classification"@en ;
                   rdfs:label "Corpus part"@en .


###  http://w3id.org/meta-share/meta-share/CorpusSubclass
ms:CorpusSubclass rdf:type owl:Class ;
                  rdfs:comment "A classification of corpora into types (used for descriptive reasons)"@en ;
                  rdfs:label "Corpus subclass"@en .


###  http://w3id.org/meta-share/meta-share/CorpusTextNumericalPart
ms:CorpusTextNumericalPart rdf:type owl:Class ;
                           rdfs:subClassOf ms:CorpusMediaPart ;
                           rdfs:comment "The part of a corpus (or whole corpus) that consists of sets of textual representations of measurements and observations linked to sensorimotor recordings"@en ;
                           rdfs:label "Corpus text numerical part"@en .


###  http://w3id.org/meta-share/meta-share/CorpusTextPart
ms:CorpusTextPart rdf:type owl:Class ;
                  rdfs:subClassOf ms:CorpusMediaPart ;
                  rdfs:comment "The part of a corpus (or a whole corpus) that consists of textual segments (e.g., a corpus of publications, or transcriptions of an oral corpus, or subtitles, etc.)"@en ;
                  rdfs:label "Corpus text part"@en .


###  http://w3id.org/meta-share/meta-share/CorpusVideoPart
ms:CorpusVideoPart rdf:type owl:Class ;
                   rdfs:subClassOf ms:CorpusMediaPart ;
                   rdfs:comment "The part of a corpus (or whole corpus) that consists of video files (e.g., a corpus of film documentaries)"@en ;
                   rdfs:label "Corpus video part"@en .


###  http://w3id.org/meta-share/meta-share/Cost
ms:Cost rdf:type owl:Class ;
        rdfs:comment "The cost for accessing a resource formally desribed as a set of amount and currency unit"@en ;
        rdfs:label "Cost"@en .


###  http://w3id.org/meta-share/meta-share/Country
ms:Country rdf:type owl:Class ;
           rdfs:comment "The name of a country preferrably according to ISO 639"@en ;
           rdfs:label "Country"@en ;
           skos:note "add here the dataset from EU NAL"@en .


###  http://w3id.org/meta-share/meta-share/Currency
ms:Currency rdf:type owl:Class ;
            rdfs:comment "Any system of money used in a particular country"@en ;
            rdfs:label "Currency"@en .


###  http://w3id.org/meta-share/meta-share/DataLanguageResource
ms:DataLanguageResource rdf:type owl:Class ;
                        rdfs:subClassOf ms:LanguageResource ;
                        rdfs:comment "A resource composed of linguistic material used to assist and augment language processing applications, but also, in a broader sense, in language and language-mediated research studies and applications; examples include data sets (textual, multimodal/multimedia and lexical data, grammars, language models, etc.) in machine readable form"@en ;
                        rdfs:label "Data language resource"@en .


###  http://w3id.org/meta-share/meta-share/DatasetDistribution
ms:DatasetDistribution rdf:type owl:Class ;
                       rdfs:subClassOf ms:Distribution ,
                                       [ rdf:type owl:Restriction ;
                                         owl:onProperty ms:distributionForm ;
                                         owl:allValuesFrom ms:DatasetDistributionForm
                                       ] ;
                       rdfs:comment "Any form with which a dataset is distributed, such as a downloadable form in a specific format (e.g., spreadsheet, plain text, etc.) or an API with which it can be accessed"@en ;
                       rdfs:label "Dataset distribution"@en .


###  http://w3id.org/meta-share/meta-share/DatasetDistributionForm
ms:DatasetDistributionForm rdf:type owl:Class ;
                           rdfs:subClassOf ms:DistributionForm ;
                           rdfs:comment "The form (medium/channel) used for distributing a language resource consisting of data (e.g., a corpus, a lexicon, etc.)"@en ;
                           rdfs:label "Dataset distribution form"@en .


###  http://w3id.org/meta-share/meta-share/Deposit
ms:Deposit rdf:type owl:Class ;
           rdfs:subClassOf odrl:Action ;
           rdfs:comment "The action of uploading a resource to a hosting entity (repository), e.g. for preservation purposes"@en ;
           rdfs:label "Deposit"@en .


###  http://w3id.org/meta-share/meta-share/DescribedEntity
ms:DescribedEntity rdf:type owl:Class ;
                   rdfs:comment "The (type of) entity that is being described by a metadata record"@en ;
                   rdfs:label "type of described entity"@en .


###  http://w3id.org/meta-share/meta-share/DevelopmentFramework
ms:DevelopmentFramework rdf:type owl:Class ;
                        rdfs:comment "A framework or toolkit (Machine Learning model, NLP toolkit) used in the development of a resource"@en ;
                        rdfs:label "Development framework"@en .


###  http://w3id.org/meta-share/meta-share/Distribution
ms:Distribution rdf:type owl:Class ;
                rdfs:subClassOf owl:Thing ;
                rdfs:comment "Any form with which a language resource is distributed; for software, this can refer to web services, executable or code files, etc.; for datasets, it can be a downloadable form in a specific format (e.g., spreadsheet, plain text, etc.) or an API with which it can be accessed"@en ;
                rdfs:label "Distribution"@en .


###  http://w3id.org/meta-share/meta-share/DistributionAudioFeature
ms:DistributionAudioFeature rdf:type owl:Class ;
                            rdfs:comment "A feature that can be used for describing distinct distributable forms of audio resources/parts"@en ;
                            rdfs:label "Audio feature"@en .


###  http://w3id.org/meta-share/meta-share/DistributionForm
ms:DistributionForm rdf:type owl:Class ;
                    rdfs:comment "Τhe form used for distributing (delivering or providing access) to the resource"@en ;
                    rdfs:label "Distribution form"@en .


###  http://w3id.org/meta-share/meta-share/DistributionImageFeature
ms:DistributionImageFeature rdf:type owl:Class ;
                            rdfs:comment "A feature that can be used for describing distinct distributable forms of image resources/parts"@en ;
                            rdfs:label "Image feature"@en .


###  http://w3id.org/meta-share/meta-share/DistributionTextFeature
ms:DistributionTextFeature rdf:type owl:Class ;
                           rdfs:subClassOf [ rdf:type owl:Restriction ;
                                             owl:onProperty ms:format ;
                                             owl:allValuesFrom omtd:DataFormat
                                           ] ;
                           rdfs:comment "A feature that can be used for describing distinct distributable forms of text resources/parts"@en ;
                           rdfs:label "Text feature"@en .


###  http://w3id.org/meta-share/meta-share/DistributionTextNumericalFeature
ms:DistributionTextNumericalFeature rdf:type owl:Class ;
                                    rdfs:subClassOf [ rdf:type owl:Restriction ;
                                                      owl:onProperty ms:format ;
                                                      owl:allValuesFrom omtd:DataFormat
                                                    ] ;
                                    rdfs:comment "A feature that can be used for describing distinct distributable forms of numerical text resources/parts"@en ;
                                    rdfs:label "Numerical text feature"@en .


###  http://w3id.org/meta-share/meta-share/DistributionVideoFeature
ms:DistributionVideoFeature rdf:type owl:Class ;
                            rdfs:comment "A feature that can be used for describing distinct distributable forms of video resources/parts"@en ;
                            rdfs:label "Video feature"@en .


###  http://w3id.org/meta-share/meta-share/Division
ms:Division rdf:type owl:Class ;
            rdfs:comment "Section of a larger organization (e.g., school, faculty, department of a university, department or branch of a company, etc.)"@en ;
            rdfs:label "Division"@en .


###  http://w3id.org/meta-share/meta-share/DivisionCategory
ms:DivisionCategory rdf:type owl:Class ;
                    rdfs:comment "A controlled vocabulary used for classifying divisions"@en ;
                    rdfs:label "Division category"@en .


###  http://w3id.org/meta-share/meta-share/Document
ms:Document rdf:type owl:Class ;
            rdfs:subClassOf ms:DescribedEntity ;
            rdfs:comment "A piece of written, printed, or electronic matter that is primarily intended for reading"@en ;
            rdfs:label "Document"@en .


###  http://w3id.org/meta-share/meta-share/DocumentIdentifier
ms:DocumentIdentifier rdf:type owl:Class ;
                      rdfs:subClassOf datacite:ResourceIdentifier ,
                                      [ rdf:type owl:Restriction ;
                                        owl:onProperty datacite:usesIdentifierScheme ;
                                        owl:allValuesFrom ms:DocumentIdentifierScheme
                                      ] ;
                      rdfs:comment "A string (e.g., PID, DOI, internal to an organization, etc.) used to uniquely identify a document (mainly intended for published documents)"@en ;
                      rdfs:label "Document identifier"@en .


###  http://w3id.org/meta-share/meta-share/DocumentIdentifierScheme
ms:DocumentIdentifierScheme rdf:type owl:Class ;
                            rdfs:subClassOf datacite:ResourceIdentifierScheme ;
                            rdfs:comment "A scheme according to which an identifier is assigned by the authority that issues it (e.g., DOI, PubMed Central, etc.) specifically for publications"@en ;
                            rdfs:label "Document identifier scheme"@en .


###  http://w3id.org/meta-share/meta-share/DocumentType
ms:DocumentType rdf:type owl:Class ;
                rdfs:comment "A classification vocabulary for documents (e.g., article, book, etc.)"@en ;
                rdfs:label "Document type"@en .


###  http://w3id.org/meta-share/meta-share/DocumentationType
ms:DocumentationType rdf:type owl:Class ;
                     rdfs:comment "The type of the documentation vis-a-vis its relation with the language resource (e.g., general publication, user manual, etc.)"@en ;
                     rdfs:label "Documentation type"@en .


###  http://w3id.org/meta-share/meta-share/Domain
ms:Domain rdf:type owl:Class ;
          rdfs:subClassOf ms:Classification ,
                          [ rdf:type owl:Restriction ;
                            owl:onProperty datacite:hasIdentifier ;
                            owl:allValuesFrom ms:DomainIdentifier
                          ] ;
          rdfs:comment "A particular field of thought, activity, or interest related to a language resource, organization or person activities, etc."@en ;
          rdfs:label "Domain"@en ;
          skos:example "health, law, banking, ..."@en ;
          skos:note "Adapted from https://www.collinsdictionary.com/dictionary/english/domain"@en .


###  http://w3id.org/meta-share/meta-share/DomainClassificationScheme
ms:DomainClassificationScheme rdf:type owl:Class ;
                              rdfs:subClassOf ms:ClassificationScheme ;
                              rdfs:comment "A classification scheme devised by an authority for domains"@en ;
                              rdfs:label "Domain classification scheme"@en .


###  http://w3id.org/meta-share/meta-share/DomainIdentifier
ms:DomainIdentifier rdf:type owl:Class ;
                    rdfs:subClassOf datacite:Identifier ,
                                    [ rdf:type owl:Restriction ;
                                      owl:onProperty ms:conformsTo ;
                                      owl:allValuesFrom ms:DomainClassificationScheme
                                    ] ;
                    rdfs:comment "A string used to uniquely identify a domain according to a specific classification scheme"@en ;
                    rdfs:label "Domain identifier"@en .


###  http://w3id.org/meta-share/meta-share/Download
ms:Download rdf:type owl:Class ;
            rdfs:subClassOf odrl:Action ;
            rdfs:comment "Download of a content file (with data or executable file) on one's local system"@en ;
            rdfs:label "Download"@en .


###  http://w3id.org/meta-share/meta-share/Duration
ms:Duration rdf:type owl:Class ;
            rdfs:comment "The time that an audio or video recording, etc. lasts"@en ;
            rdfs:label "Duration of audio"@en .


###  http://w3id.org/meta-share/meta-share/DurationUnit
ms:DurationUnit rdf:type owl:Class ;
                rdfs:comment "A unit for measuring duration of audio / video parts"@en ;
                rdfs:label "Duration unit"@en .


###  http://w3id.org/meta-share/meta-share/DynamicElement
ms:DynamicElement rdf:type owl:Class ;
                  rdfs:comment "Element represented in the video part of a resource"@en ;
                  rdfs:label "Dynamic element"@en .


###  http://w3id.org/meta-share/meta-share/EncodingLevel
ms:EncodingLevel rdf:type owl:Class ;
                 rdfs:comment "The linguistic level of analysis a lexical/conceptual resource or language description caters for as represented in its contents"@en ;
                 rdfs:label "Encoding level"@en .


###  http://w3id.org/meta-share/meta-share/EnumerationValue
ms:EnumerationValue rdf:type owl:Class ;
                    rdfs:comment "The value of a list used inside parameters"@en ;
                    rdfs:label "Enumeration value"@en .


###  http://w3id.org/meta-share/meta-share/Evaluation
ms:Evaluation rdf:type owl:Class ;
              rdfs:comment "Each of the procedures and outcomes followed for evaluating the performance and other features of a tool/service"@en ;
              rdfs:label "Evaluation"@en .


###  http://w3id.org/meta-share/meta-share/Evaluation1
ms:Evaluation1 rdf:type owl:Class ;
               rdfs:subClassOf odrl:RightOperand ;
               rdfs:comment "The use of a resource for evaluation purposes"@en ;
               rdfs:label "Evaluation"@en .


###  http://w3id.org/meta-share/meta-share/EvaluationCriterion
ms:EvaluationCriterion rdf:type owl:Class ;
                       rdfs:comment "The criterion of the evaluation of a tool"@en ;
                       rdfs:label "Evaluation criterion"@en .


###  http://w3id.org/meta-share/meta-share/EvaluationLevel
ms:EvaluationLevel rdf:type owl:Class ;
                   rdfs:comment "The evaluation level"@en ;
                   rdfs:label "Evaluation level"@en .


###  http://w3id.org/meta-share/meta-share/EvaluationMeasure
ms:EvaluationMeasure rdf:type owl:Class ;
                     rdfs:comment "The evaluation measure (human or automatic)"@en ;
                     rdfs:label "Evaluation measure"@en .


###  http://w3id.org/meta-share/meta-share/EvaluationType
ms:EvaluationType rdf:type owl:Class ;
                  rdfs:comment "Indicates the type of evaluation performed on a tool/service"@en ;
                  rdfs:label "Evaluation type"@en .


###  http://w3id.org/meta-share/meta-share/ExtratextualInformation
ms:ExtratextualInformation rdf:type owl:Class ;
                           rdfs:comment "The non-textual information contained in a lexical/conceptual resouce (e.g., images, videos, audios, etc.); it can be used as an alternative to fully describing them as a proper part of the resource when they are not as important as the textual part (e.g., cases of a dictionary with images attached to some lemmas)"@en ;
                           rdfs:label "Extratextual information"@en .


###  http://w3id.org/meta-share/meta-share/ExtratextualInformationUnit
ms:ExtratextualInformationUnit rdf:type owl:Class ;
                               rdfs:comment "The unit on which the extratextual information in a lexical/conceptual resource is attached"@en ;
                               rdfs:label "Extratextual information unit"@en .


###  http://w3id.org/meta-share/meta-share/Framework
ms:Framework rdf:type owl:Class ;
             rdfs:comment "The implementation framework used for developing and running a tool/service"@en ;
             rdfs:label "Wrapping framework"@en .


###  http://w3id.org/meta-share/meta-share/FundingType
ms:FundingType rdf:type owl:Class ;
               rdfs:comment "A classification of the funding of a project with regard to the source of the funds"@en ;
               rdfs:label "Funding type"@en .


###  http://w3id.org/meta-share/meta-share/Genre
ms:Genre rdf:type owl:Class ;
         rdfs:subClassOf ms:Classification ;
         rdfs:comment "A way of classifying a language resource with regard to the style, form and content"@en ;
         rdfs:label "Genre"@en .


###  http://w3id.org/meta-share/meta-share/Grammar
ms:Grammar rdf:type owl:Class ;
           rdfs:subClassOf ms:LanguageDescription ;
           rdfs:comment "A set of rules governing what strings are valid or allowable in a language or text [https://en.oxforddictionaries.com/definition/grammar]"@en ;
           rdfs:label "Grammar"@en .


###  http://w3id.org/meta-share/meta-share/GrammaticalPhenomenaCoverage
ms:GrammaticalPhenomenaCoverage rdf:type owl:Class ;
                                rdfs:comment "An indication of the grammatical phenomena covered by the grammar"@en ;
                                rdfs:label "Grammatical phenomena coverage"@en .


###  http://w3id.org/meta-share/meta-share/Group
ms:Group rdf:type owl:Class ;
         rdfs:comment "A set of persons related to some aspect of a language resource, that do not have a legal status (e.g., a group of software developers working on the same software)"@en ;
         rdfs:label "Group"@en .


###  http://w3id.org/meta-share/meta-share/GroupIdentifier
ms:GroupIdentifier rdf:type owl:Class ;
                   rdfs:subClassOf datacite:AgentIdentifier ,
                                   [ rdf:type owl:Restriction ;
                                     owl:onProperty datacite:usesIdentifierScheme ;
                                     owl:allValuesFrom datacite:OrganizationIdentifierScheme
                                   ] ;
                   rdfs:comment "A string used to uniquely identify a group"@en ;
                   rdfs:label "Group identifier"@en .


###  http://w3id.org/meta-share/meta-share/HearingImpairmentOfParticipants
ms:HearingImpairmentOfParticipants rdf:type owl:Class ;
                                   rdfs:comment "Whether the group of participants contains persons with hearing impairments"@en ;
                                   rdfs:label "Hearing impairment of participants"@en .


###  http://w3id.org/meta-share/meta-share/ImageFormat
ms:ImageFormat rdf:type owl:Class ;
               rdfs:comment "The format used for the image part of a resource"@en ;
               rdfs:label "Detailed image format"@en .


###  http://w3id.org/meta-share/meta-share/ImageGenre
ms:ImageGenre rdf:type owl:Class ;
              rdfs:subClassOf ms:Genre ,
                              [ rdf:type owl:Restriction ;
                                owl:onProperty datacite:hasIdentifier ;
                                owl:allValuesFrom ms:ImageGenreIdentifier
                              ] ,
                              [ rdf:type owl:Restriction ;
                                owl:onProperty ms:genre ;
                                owl:allValuesFrom ms:CorpusImagePart
                              ] ;
              rdfs:comment "A category of images characterized by a particular style, form, or content according to a specific classification scheme"@en ;
              rdfs:label "Image genre"@en .


###  http://w3id.org/meta-share/meta-share/ImageGenreClassificationScheme
ms:ImageGenreClassificationScheme rdf:type owl:Class ;
                                  rdfs:subClassOf ms:ClassificationScheme ;
                                  rdfs:comment "A classification scheme devised by an authority for image genres"@en ;
                                  rdfs:label "Image genre classification scheme"@en .


###  http://w3id.org/meta-share/meta-share/ImageGenreIdentifier
ms:ImageGenreIdentifier rdf:type owl:Class ;
                        rdfs:subClassOf datacite:Identifier ,
                                        [ rdf:type owl:Restriction ;
                                          owl:onProperty ms:conformsTo ;
                                          owl:allValuesFrom ms:ImageGenreClassificationScheme
                                        ] ;
                        rdfs:comment "A string used to uniquely identify an image genre according to a specific classification scheme"@en ;
                        rdfs:label "Image genre identifier"@en .


###  http://w3id.org/meta-share/meta-share/Interactivity
ms:Interactivity rdf:type owl:Class ;
                 rdfs:comment "The level of conversational interaction between speakers (for audio component) or participants (for video component)"@en ;
                 rdfs:label "Interactivity"@en .


###  http://w3id.org/meta-share/meta-share/LCRSubclass
ms:LCRSubclass rdf:type owl:Class ;
               rdfs:subClassOf skos:Concept ;
               rdfs:comment "A classification of lexical/conceptual resources into types (used for descriptive reasons)"@en ;
               rdfs:label "LCR subclass"@en .


###  http://w3id.org/meta-share/meta-share/LDSubclass
ms:LDSubclass rdf:type owl:Class ;
              rdfs:subClassOf skos:Concept ;
              rdfs:label "Language description subclass"@en .


###  http://w3id.org/meta-share/meta-share/LDTask
ms:LDTask rdf:type owl:Class ;
          rdfs:comment "Identifies the task performed by the language description"@en ;
          rdfs:label "Language description task"@en ;
          skos:note "add links to omtd-share operations"@en .


###  http://w3id.org/meta-share/meta-share/LRIdentifier
ms:LRIdentifier rdf:type owl:Class ;
                rdfs:subClassOf datacite:ResourceIdentifier ,
                                [ rdf:type owl:Restriction ;
                                  owl:onProperty datacite:usesIdentifierScheme ;
                                  owl:allValuesFrom ms:LRIdentifierScheme
                                ] ;
                rdfs:comment "A string (e.g., PID, DOI, internal to an organization, etc.) used to uniquely identify a language resource"@en ;
                rdfs:label "Language Resource identifier"@en .


###  http://w3id.org/meta-share/meta-share/LRIdentifierScheme
ms:LRIdentifierScheme rdf:type owl:Class ;
                      rdfs:subClassOf datacite:ResourceIdentifierScheme ;
                      rdfs:comment "The name of the scheme according to which the LRT identifier is assigned by the authority that issues it (e.g., DOI, ISLRN, etc.)"@en ;
                      rdfs:label "LR identifier scheme"@en ;
                      skos:altLabel "Language Resource identifier scheme"@en .


###  http://w3id.org/meta-share/meta-share/LanguageDescription
ms:LanguageDescription rdf:type owl:Class ;
                       rdfs:subClassOf ms:DataLanguageResource ,
                                       [ rdf:type owl:Restriction ;
                                         owl:onProperty ms:distribution ;
                                         owl:allValuesFrom ms:DatasetDistribution
                                       ] ;
                       rdfs:comment "A resource that describes a language or some aspect(s) of a language via a systematic documentation of linguistic structures"@en ;
                       rdfs:label "Language description"@en .


###  http://w3id.org/meta-share/meta-share/LanguageDescriptionImagePart
ms:LanguageDescriptionImagePart rdf:type owl:Class ;
                                rdfs:subClassOf ms:LanguageDescriptionMediaPart ;
                                rdfs:comment "The part (or whole set) of a language description that consists of images (e.g., a grammar part with photos or images for sign languages)"@en ;
                                rdfs:label "Language description image part"@en .


###  http://w3id.org/meta-share/meta-share/LanguageDescriptionMediaPart
ms:LanguageDescriptionMediaPart rdf:type owl:Class ;
                                rdfs:subClassOf ms:MediaPart ;
                                rdfs:comment "A part/segment of a language description based on its media type classification"@en ;
                                rdfs:label "Language description part"@en .


###  http://w3id.org/meta-share/meta-share/LanguageDescriptionTextPart
ms:LanguageDescriptionTextPart rdf:type owl:Class ;
                               rdfs:subClassOf ms:LanguageDescriptionMediaPart ;
                               rdfs:comment "The textual part (or whole set) of a language description"@en ;
                               rdfs:label "Language description text part"@en .


###  http://w3id.org/meta-share/meta-share/LanguageDescriptionVideoPart
ms:LanguageDescriptionVideoPart rdf:type owl:Class ;
                                rdfs:subClassOf ms:LanguageDescriptionMediaPart ;
                                rdfs:comment "The part (or whole set) of a language description that consists of videos (e.g., a grammar part with videos for sign languages)"@en ;
                                rdfs:label "Language description video part"@en .


###  http://w3id.org/meta-share/meta-share/LanguageEngineeringResearch
ms:LanguageEngineeringResearch rdf:type owl:Class ;
                               rdfs:subClassOf odrl:RightOperand ;
                               rdfs:comment "The use of a resource for research in the Language Technology (Language engineering) area"@en ;
                               rdfs:label "Language engineering research"@en .


###  http://w3id.org/meta-share/meta-share/LanguageModel
ms:LanguageModel rdf:type owl:Class ;
                 rdfs:subClassOf ms:LanguageDescription ;
                 rdfs:comment "A statistical language model is a probability distribution over sequences of words. Given such a sequence, say of length m, it assigns a probability P (w1, ..., wm) to the whole sequence. [from Wikipedia (https://en.wikipedia.org/wiki/Language_model)]"@en ;
                 rdfs:label "Language model"@en ;
                 skos:altLabel "Statistical language model"@en .


###  http://w3id.org/meta-share/meta-share/LanguageResource
ms:LanguageResource rdf:type owl:Class ;
                    rdfs:subClassOf ms:DescribedEntity ,
                                    [ rdf:type owl:Restriction ;
                                      owl:onProperty datacite:hasIdentifier ;
                                      owl:allValuesFrom ms:LRIdentifier
                                    ] ;
                    rdfs:comment "A resource composed of linguistic material used in the construction, improvement and/or evaluation of language processing applications, but also, in a broader sense, in language and language-mediated research studies and applications; the term is used with a broader meaning, encompassing (a) data sets (textual, multimodal/multimedia and lexical data, grammars, language models, etc.) in machine readable form, and (b) tools/technologies/services used for their processing and management."@en ;
                    rdfs:label "Language Resource"@en ;
                    skos:altLabel "LR"@en .


###  http://w3id.org/meta-share/meta-share/LanguageVariety
ms:LanguageVariety rdf:type owl:Class ;
                   rdfs:comment "A particular linguistic system used in a specific region or by a social group"@en ;
                   rdfs:label "Language variety"@en .


###  http://w3id.org/meta-share/meta-share/LanguageVarietyType
ms:LanguageVarietyType rdf:type owl:Class ;
                       rdfs:comment "A classification for language varieties"@en ;
                       rdfs:label "Language variety type"@en .


###  http://w3id.org/meta-share/meta-share/LexicalConceptualResource
ms:LexicalConceptualResource rdf:type owl:Class ;
                             rdfs:subClassOf ms:DataLanguageResource ,
                                             [ rdf:type owl:Restriction ;
                                               owl:onProperty ms:distribution ;
                                               owl:allValuesFrom ms:DatasetDistribution
                                             ] ,
                                             [ rdf:type owl:Restriction ;
                                               owl:onProperty ms:mediaPart ;
                                               owl:allValuesFrom ms:LexicalConceptualResourceMediaPart
                                             ] ;
                             rdfs:comment "A resource organised on the basis of lexical or conceptual entries (lexical items, terms, concepts, etc.) with their supplementary information (e.g., grammatical, semantic, statistical information, etc.)"@en ;
                             rdfs:label "Lexical/Conceptual resource"@en .


###  http://w3id.org/meta-share/meta-share/LexicalConceptualResourceAudioPart
ms:LexicalConceptualResourceAudioPart rdf:type owl:Class ;
                                      rdfs:subClassOf ms:LexicalConceptualResourceMediaPart ;
                                      rdfs:comment "The part (or whole set of) a lexical/conceptual resource that consists of audio elements (e.g., a set of audio files for a lexicon)"@en ;
                                      rdfs:label "Lexical/Conceptual resource audio part"@en .


###  http://w3id.org/meta-share/meta-share/LexicalConceptualResourceImagePart
ms:LexicalConceptualResourceImagePart rdf:type owl:Class ;
                                      rdfs:subClassOf ms:LexicalConceptualResourceMediaPart ;
                                      rdfs:comment "A part (or whole set of) a lexical/conceptual resource that consists of images (e.g., a set of images used for a lexicon)"@en ;
                                      rdfs:label "Lexical/Conceptual resource image part"@en .


###  http://w3id.org/meta-share/meta-share/LexicalConceptualResourceMediaPart
ms:LexicalConceptualResourceMediaPart rdf:type owl:Class ;
                                      rdfs:subClassOf ms:MediaPart ;
                                      rdfs:comment "A part/segment of a lexical/conceptual resource based on its media type classification"@en ;
                                      rdfs:label "Lexical/ Conceptual resource part"@en .


###  http://w3id.org/meta-share/meta-share/LexicalConceptualResourceTextPart
ms:LexicalConceptualResourceTextPart rdf:type owl:Class ;
                                     rdfs:subClassOf ms:LexicalConceptualResourceMediaPart ;
                                     rdfs:comment "A part (or whole set) of a lexical/conceptual resource that consists of textual elements"@en ;
                                     rdfs:label "Lexical/Conceptual resource text part"@en .


###  http://w3id.org/meta-share/meta-share/LexicalConceptualResourceVideoPart
ms:LexicalConceptualResourceVideoPart rdf:type owl:Class ;
                                      rdfs:subClassOf ms:LexicalConceptualResourceMediaPart ;
                                      rdfs:comment "The part (or whole set) of a lexical/conceptual resource that consists of videos (e.g., a set of video files for the lexicon of a sign language)"@en ;
                                      rdfs:label "Lexical/Conceptual resource video part"@en .


###  http://w3id.org/meta-share/meta-share/LicenceCategory
ms:LicenceCategory rdf:type owl:Class ;
                   rdfs:subClassOf [ rdf:type owl:Restriction ;
                                     owl:onProperty ms:conformsTo ;
                                     owl:allValuesFrom ms:LicenceCategoryScheme
                                   ] ;
                   rdfs:comment "A classification scheme for licences"@en ;
                   rdfs:label "Licence category"@en .


###  http://w3id.org/meta-share/meta-share/LicenceCategoryScheme
ms:LicenceCategoryScheme rdf:type owl:Class ;
                         rdfs:comment "The name of the scheme according to which a category is assigned to a licence"@en ;
                         rdfs:label "Licence category scheme"@en .


###  http://w3id.org/meta-share/meta-share/LicenceIdentifier
ms:LicenceIdentifier rdf:type owl:Class ;
                     rdfs:subClassOf datacite:ResourceIdentifier ,
                                     [ rdf:type owl:Restriction ;
                                       owl:onProperty datacite:usesIdentifierScheme ;
                                       owl:allValuesFrom ms:LicenceIdentifierScheme
                                     ] ;
                     rdfs:comment "A string used to uniquely identify a licence"@en ;
                     rdfs:label "Licence identifier"@en-uk .


###  http://w3id.org/meta-share/meta-share/LicenceIdentifierScheme
ms:LicenceIdentifierScheme rdf:type owl:Class ;
                           rdfs:subClassOf datacite:ResourceIdentifierScheme ;
                           rdfs:comment "The name of the scheme according to which an identifier is assigned to a licence by the authority that issues it"@en ;
                           rdfs:label "Licence identifier scheme"@en .


###  http://w3id.org/meta-share/meta-share/LicenceTerms
ms:LicenceTerms rdf:type owl:Class ;
                rdfs:subClassOf cc:License ,
                                ms:DescribedEntity ,
                                [ rdf:type owl:Restriction ;
                                  owl:onProperty datacite:hasIdentifier ;
                                  owl:allValuesFrom ms:LicenceIdentifier
                                ] ;
                rdfs:comment "A legal document (licence or terms of use/service) with which the language resource is distributed"@en ;
                rdfs:label "Licence"@en-uk ;
                skos:note "Kanella test"@en ,
                          """Until now, this included an enumerated list of individuals; I think it's better to treat them as proper entities with name, identifier, etc. 

This means that for the editors we need to 
- add a set of well known licences using the SPDX codes (https://spdx.org/licenses/) and any set already in RDF form (e.g., https://github.com/creativecommons/cc.licenserdf/tree/master/cc/licenserdf/licenses and Victor's list) with our own extra elements
- allow them to add a new licence with the specific elements that we want
- add the clarin licence categories & conditions of use with the ODRL representation


Note: I have created a file with the CC-rdf licences and its ontology so that I can edit them and add the supplementary features => under MS ontologies, file testrdflicencesCC.txt"""@en .


###  http://w3id.org/meta-share/meta-share/LingualityType
ms:LingualityType rdf:type owl:Class ;
                  rdfs:comment "Classification of a resource (part) based on the number of languages it includes"@en ;
                  rdfs:label "Linguality type"@en .


###  http://w3id.org/meta-share/meta-share/LinkToOtherMedia
ms:LinkToOtherMedia rdf:type owl:Class ;
                    rdfs:comment "The links between different media parts of a multimedia resource"@en ;
                    rdfs:label "Link to other media"@en .


###  http://w3id.org/meta-share/meta-share/MLFramework
ms:MLFramework rdf:type owl:Class ;
               rdfs:subClassOf ms:DevelopmentFramework ;
               rdfs:comment "The framework (e.g. keras, tensorflow, etc.) that has been used for developing a Machine Learning model and the tool/service that uses it"@en ;
               rdfs:label "ML framework"@en ;
               skos:altLabel "Machine Learning framework"@en .


###  http://w3id.org/meta-share/meta-share/MLModel
ms:MLModel rdf:type owl:Class ;
           rdfs:subClassOf ms:Model ;
           rdfs:comment "The model artifact that is created through a training process involving an ML algorithm (that is, the learning algorithm) and the training data to learn from."@en ;
           rdfs:label "Machine Learning model"@en ;
           skos:altLabel "ML model"@en .


###  http://w3id.org/meta-share/meta-share/MediaPart
ms:MediaPart rdf:type owl:Class ;
             rdfs:comment "A part of a language resource based on the media type it belongs to (e.g., text, audio, video parts of a corpus or lexicon)"@en ;
             rdfs:label "Media part"@en .


###  http://w3id.org/meta-share/meta-share/MediaType
ms:MediaType rdf:type owl:Class ;
             rdfs:comment "A classification of language resource parts based on the physical medium they are available in (e.g., text, video, audio)"@en ;
             rdfs:label "Media type"@en .


###  http://w3id.org/meta-share/meta-share/MembershipInstitution
ms:MembershipInstitution rdf:type owl:Class ;
                         rdfs:comment "An institution with members that can benefit from specific conditions on the use of a resource (e.g. discount, unlimited access, etc.)"@en ;
                         rdfs:label "Membership institution"@en .


###  http://w3id.org/meta-share/meta-share/MetadataRecord
ms:MetadataRecord rdf:type owl:Class ;
                  owl:equivalentClass dcat:CatalogRecord ;
                  rdfs:subClassOf [ rdf:type owl:Restriction ;
                                    owl:onProperty ms:compliesWith ;
                                    owl:allValuesFrom ms:MetadataSchema
                                  ] ;
                  rdfs:comment "A set of formalized structured information used to describe the contents, structure, function, etc., of an entity, usually according to a specific set of rules (metadata schema)"@en ;
                  rdfs:label "Metadata record"@en .


###  http://w3id.org/meta-share/meta-share/MetadataRecordIdentifier
ms:MetadataRecordIdentifier rdf:type owl:Class ;
                            rdfs:subClassOf datacite:ResourceIdentifier ,
                                            [ rdf:type owl:Restriction ;
                                              owl:onProperty datacite:usesIdentifierScheme ;
                                              owl:allValuesFrom ms:MetadataRecordIdentifierScheme
                                            ] ;
                            rdfs:comment "A string (e.g., PID, DOI, internal to an organization, etc.) used to uniquely identify a metadata record"@en ;
                            rdfs:label "Metadata record identifier"@en .


###  http://w3id.org/meta-share/meta-share/MetadataRecordIdentifierScheme
ms:MetadataRecordIdentifierScheme rdf:type owl:Class ;
                                  rdfs:subClassOf datacite:ResourceIdentifierScheme ;
                                  rdfs:comment "The name of the scheme according to which the metadata record identifier is assigned by the authority that issues it (e.g., DOI, URL, etc.)"@en ;
                                  rdfs:label "Metadata record identifier scheme"@en .


###  http://w3id.org/meta-share/meta-share/MetadataSchema
ms:MetadataSchema rdf:type owl:Class ;
                  rdfs:comment "A formal set of metadata elements organized in a specific way"@en ;
                  rdfs:label "Metadata schema"@en .


###  http://w3id.org/meta-share/meta-share/Metric
ms:Metric rdf:type owl:Class ;
          rdfs:comment "The metric used for the evaluation of the tool/service"@en ;
          rdfs:label "Metric"@en .


###  http://w3id.org/meta-share/meta-share/ModalityType
ms:ModalityType rdf:type owl:Class ;
                rdfs:comment "A classification of modalities represented in the resource or processed by a tool/service"@en ;
                rdfs:label "Modality type"@en .


###  http://w3id.org/meta-share/meta-share/Model
ms:Model rdf:type owl:Class ;
         rdfs:subClassOf ms:LanguageDescription ;
         rdfs:label "Model"@en .


###  http://w3id.org/meta-share/meta-share/ModelType
ms:ModelType rdf:type owl:Class ;
             rdfs:subClassOf skos:Concept ;
             rdfs:comment "A classification of models into types based on their algorithm"@en ;
             rdfs:label "Model type"@en .


###  http://w3id.org/meta-share/meta-share/MultilingualityType
ms:MultilingualityType rdf:type owl:Class ;
                       rdfs:comment "A classification of a bi/multilingual resource (part) into parallel, comparable or mixed"@en ;
                       rdfs:label "Multilinguality type"@en .


###  http://w3id.org/meta-share/meta-share/NGramModel
ms:NGramModel rdf:type owl:Class ;
              rdfs:subClassOf ms:Model ;
              rdfs:comment "A language model consisting of n-grams, i.e., specific sequences of a number of words"@en ;
              rdfs:label "N-gram model"@en .


###  http://w3id.org/meta-share/meta-share/NLPFramework
ms:NLPFramework rdf:type owl:Class ;
                rdfs:subClassOf ms:DevelopmentFramework ;
                rdfs:label "NLP framework"@en .


###  http://w3id.org/meta-share/meta-share/Naturality
ms:Naturality rdf:type owl:Class ;
              rdfs:comment "The level of naturality for multimodal/multimedia resources"@en ;
              rdfs:label "Naturality"@en .


###  http://w3id.org/meta-share/meta-share/NeuralNetwork
ms:NeuralNetwork rdf:type owl:Class ;
                 rdfs:subClassOf ms:MLModel ;
                 rdfs:comment "A set of algorithms, modeled loosely after the human brain, designed to recognize patterns [adapted from https://skymind.ai/wiki/neural-network]"@en ;
                 rdfs:label "Neural network"@en .


###  http://w3id.org/meta-share/meta-share/NoiseLevel
ms:NoiseLevel rdf:type owl:Class ;
              rdfs:comment "The level of background noise"@en ;
              rdfs:label "Noise level"@en .


###  http://w3id.org/meta-share/meta-share/NonSpeechItem
ms:NonSpeechItem rdf:type owl:Class ;
                 rdfs:comment "A non-speech element that maybe included in the audio corpus or lexical/conceptual resource"@en ;
                 rdfs:label "Non-speech item"@en .


###  http://w3id.org/meta-share/meta-share/ObjectOfReport
ms:ObjectOfReport rdf:type owl:Class ;
                  rdfs:subClassOf odrl:LeftOperand ;
                  rdfs:comment "The output of a report"@en ;
                  rdfs:label "Object of report"@en .


###  http://w3id.org/meta-share/meta-share/OperatingSystem
ms:OperatingSystem rdf:type owl:Class ;
                   rdfs:comment "The operating system on which the software is compatible with"@en ;
                   rdfs:label "operating system"@en .


###  http://w3id.org/meta-share/meta-share/Organization
ms:Organization rdf:type owl:Class ;
                rdfs:subClassOf ms:Actor ,
                                [ rdf:type owl:Restriction ;
                                  owl:onProperty datacite:hasIdentifier ;
                                  owl:allValuesFrom datacite:OrganizationIdentifier
                                ] ;
                rdfs:comment "A company or other group of people that works together for a particular purpose [https://dictionary.cambridge.org/dictionary/english/organization]"@en-uk ;
                rdfs:label "Organization"@en ;
                skos:altLabel "Organisation"@en-uk .


###  http://w3id.org/meta-share/meta-share/OrganizationLegalStatus
ms:OrganizationLegalStatus rdf:type owl:Class ;
                           rdfs:comment "A classification vocabulary for organizations as legal entities"@en ;
                           rdfs:label "Organization legal status"@en .


###  http://w3id.org/meta-share/meta-share/OrganizationRole
ms:OrganizationRole rdf:type owl:Class ;
                    rdfs:comment "A vocabulary for classifying organizations according to their role in relation to Language Technology"@en ;
                    rdfs:label "Organization role"@en .


###  http://w3id.org/meta-share/meta-share/Origin
ms:Origin rdf:type owl:Class ;
          rdfs:comment "The relation of the language of the group of participants with respect to the acquisition stage"@en ;
          rdfs:label "Origin"@en .


###  http://w3id.org/meta-share/meta-share/Parameter
ms:Parameter rdf:type owl:Class ;
             rdfs:comment "A a special kind of variable in computer programming language that is used to pass information between functions or procedures [from https://www.techopedia.com/definition/3725/parameter-param]"@en ;
             rdfs:label "Parameter"@en .


###  http://w3id.org/meta-share/meta-share/ParameterType
ms:ParameterType rdf:type owl:Class ;
                 rdfs:comment "A specific (not yet standardised) typing system for parameters (e.g., whether it's boolean, string, integer, a document, mapping, etc.)"@en ;
                 rdfs:label "Parameter type"@en .


###  http://w3id.org/meta-share/meta-share/Participant
ms:Participant rdf:type owl:Class ;
               rdfs:subClassOf ms:Person ;
               rdfs:comment "A person that has participated in the recording of the audio, video, sensorimotor (textNumerical) part of the resource"@en ;
               rdfs:label "Participant"@en .


###  http://w3id.org/meta-share/meta-share/PerformanceIndicator
ms:PerformanceIndicator rdf:type owl:Class ;
                        rdfs:comment "The performance indicator used in the evaluation of a software given in the form of the metric used and reporting on the measure and unit of measure for this"@en ;
                        rdfs:label "Performance indicator"@en .


###  http://w3id.org/meta-share/meta-share/Person
ms:Person rdf:type owl:Class ;
          rdfs:subClassOf ms:Actor ,
                          [ rdf:type owl:Restriction ;
                            owl:onProperty datacite:hasIdentifier ;
                            owl:allValuesFrom datacite:PersonalIdentifier
                          ] ;
          rdfs:comment "A human being"@en ;
          rdfs:label "Person"@en ;
          skos:note "Subclass of foaf to exclude imaginary persons"@en .


###  http://w3id.org/meta-share/meta-share/PersonalDataIncluded
ms:PersonalDataIncluded rdf:type owl:Class ;
                        rdfs:comment "Specification of whether the language resource contains personal data (mainly in the sense falling under the GDPR)"@en ;
                        rdfs:label "Personal data included"@en .


###  http://w3id.org/meta-share/meta-share/PreviousAnnotationTypesPolicy
ms:PreviousAnnotationTypesPolicy rdf:type owl:Class ;
                                 rdfs:comment "Policy types that a tool/service has with respect to the annotation types included in the annotated resource that it takes as input (i.e. whether it keeps, modifies or drops them in the output resource)"@en ;
                                 rdfs:label "Previous annotation types policy"@en .


###  http://w3id.org/meta-share/meta-share/Process
ms:Process rdf:type owl:Class ;
           rdfs:subClassOf odrl:Action ;
           rdfs:comment "To process a data resource with a language processing service (e.g. to create an annotated version, or to extract elements from it)"@en ;
           rdfs:label "Process"@en .


###  http://w3id.org/meta-share/meta-share/ProcessMode
ms:ProcessMode rdf:type owl:Class ;
               rdfs:comment "Classification of the mode of operation applied when processing a resource"@en ;
               rdfs:label "Process mode"@en .


###  http://w3id.org/meta-share/meta-share/ProcessingResource
ms:ProcessingResource rdf:type owl:Class ;
                      rdfs:comment "A set of requirements posed on the resource that is input for processing by a tool/service"@en ;
                      rdfs:label "Input content resource"@en .


###  http://w3id.org/meta-share/meta-share/ProcessingResourceType
ms:ProcessingResourceType rdf:type owl:Class ;
                          rdfs:comment "The type of the resource that a tool/service takes as input or produces as output"@en ;
                          rdfs:label "Processing resource type"@en ;
                          skos:note "Unsure of the values for audio/video files"@en .


###  http://w3id.org/meta-share/meta-share/Project
ms:Project rdf:type owl:Class ;
           rdfs:subClassOf ms:DescribedEntity ,
                           foaf:Project ,
                           [ rdf:type owl:Restriction ;
                             owl:onProperty datacite:hasIdentifier ;
                             owl:allValuesFrom ms:ProjectIdentifier
                           ] ;
           rdfs:comment "A set of operations undertaken as a whole by an individual or organization and related to some aspect of the lifecycle of the language resource (e.g., funding, deployment, etc.)"@en ;
           rdfs:label "Project"@en .


###  http://w3id.org/meta-share/meta-share/ProjectIdentifier
ms:ProjectIdentifier rdf:type owl:Class ;
                     rdfs:subClassOf datacite:ResourceIdentifier ,
                                     [ rdf:type owl:Restriction ;
                                       owl:onProperty datacite:usesIdentifierScheme ;
                                       owl:allValuesFrom ms:ProjectIdentifierScheme
                                     ] ;
                     rdfs:comment "A string (e.g., PID, internal to an organization, issued by the funding authority, etc.) used to uniquely identify a project"@en ;
                     rdfs:label "Project identifier"@en .


###  http://w3id.org/meta-share/meta-share/ProjectIdentifierScheme
ms:ProjectIdentifierScheme rdf:type owl:Class ;
                           rdfs:subClassOf datacite:ResourceIdentifierScheme ;
                           rdfs:comment "The name of the scheme according to which an identifier is assigned to a project by the authority that issues it"@en ;
                           rdfs:label "Project identifier scheme"@en .


###  http://w3id.org/meta-share/meta-share/Quality
ms:Quality rdf:type owl:Class ;
           rdfs:comment "The quality level of image part(s) of a resource"@en ;
           rdfs:label "Quality"@en-uk .


###  http://w3id.org/meta-share/meta-share/RasterOrVectorGraphics
ms:RasterOrVectorGraphics rdf:type owl:Class ;
                          rdfs:comment "Type of graphics of the image part(s) of a resource"@en ;
                          rdfs:label "Raster or vector graphics"@en .


###  http://w3id.org/meta-share/meta-share/RecordingDeviceType
ms:RecordingDeviceType rdf:type owl:Class ;
                       rdfs:comment "The nature of the recording platform hardware and the storage medium"@en ;
                       rdfs:label "Recording device type"@en .


###  http://w3id.org/meta-share/meta-share/RecordingEnvironment
ms:RecordingEnvironment rdf:type owl:Class ;
                        rdfs:comment "A setting where the recording of a multimedia resource took place"@en ;
                        rdfs:label "Recording environment"@en .


###  http://w3id.org/meta-share/meta-share/RecordingQuality
ms:RecordingQuality rdf:type owl:Class ;
                    rdfs:comment "Indication of the audio or video recording quality"@en ;
                    rdfs:label "Recording quality"@en-uk .


###  http://w3id.org/meta-share/meta-share/RelatedLexiconType
ms:RelatedLexiconType rdf:type owl:Class ;
                      rdfs:comment "Indicates the type for the lexica that must or can be used with the grammar"@en ;
                      rdfs:label "Related lexicon type"@en .


###  http://w3id.org/meta-share/meta-share/Relation
ms:Relation rdf:type owl:Class ;
            rdfs:comment "A relation holding between two language resources (e.g., a raw corpus and its annotated version, the annotation tool used for it, etc.)"@en ;
            rdfs:label "Relation"@en .


###  http://w3id.org/meta-share/meta-share/Report
ms:Report rdf:type owl:Class ;
          rdfs:subClassOf odrl:Action ;
          rdfs:comment "Give an account of an event related to the resource (e.g. a research plan, the use of the resource in a project or publication, etc.)"@en ;
          rdfs:label "Report"@en .


###  http://w3id.org/meta-share/meta-share/RepositoryIdentifier
ms:RepositoryIdentifier rdf:type owl:Class ;
                        rdfs:subClassOf datacite:AgentIdentifier ,
                                        [ rdf:type owl:Restriction ;
                                          owl:onProperty datacite:usesIdentifierScheme ;
                                          owl:allValuesFrom ms:RepositoryIdentifierScheme
                                        ] ;
                        rdfs:comment "A string (e.g., PID, DOI, internal to an organization, etc.) used to uniquely identify a repository"@en ;
                        rdfs:label "Repository identifier"@en .


###  http://w3id.org/meta-share/meta-share/RepositoryIdentifierScheme
ms:RepositoryIdentifierScheme rdf:type owl:Class ;
                              rdfs:subClassOf datacite:AgentIdentifierScheme ;
                              rdfs:comment "The name of the scheme used to identify a repository"@en ;
                              rdfs:label "Repository identifier scheme"@en .


###  http://w3id.org/meta-share/meta-share/RequiredHardware
ms:RequiredHardware rdf:type owl:Class ;
                    rdfs:comment "Type of hardware required for running a tool and/or computational grammar"@en ;
                    rdfs:label "Required hardware"@en .


###  http://w3id.org/meta-share/meta-share/Research
ms:Research rdf:type owl:Class ;
            rdfs:subClassOf odrl:RightOperand ;
            rdfs:comment "The use of a reseach for research purposes"@en ;
            rdfs:label "Research"@en .


###  http://w3id.org/meta-share/meta-share/ResearchPlan
ms:ResearchPlan rdf:type owl:Class ;
                rdfs:subClassOf odrl:RightOperand ;
                rdfs:comment "The plan for conducting research using a specific resource; this may be required by a resource provider to allow access to the resource"@en ;
                rdfs:label "Research plan"@en .


###  http://w3id.org/meta-share/meta-share/Resolution
ms:Resolution rdf:type owl:Class ;
              rdfs:comment "The image resolution used for the video/image part(s) of a resource"@en ;
              rdfs:label "Resolution"@en .


###  http://w3id.org/meta-share/meta-share/ResolutionStandard
ms:ResolutionStandard rdf:type owl:Class ;
                      rdfs:comment "The standard to which the resolution conforms"@en ;
                      rdfs:label "Resolution standard"@en .


###  http://w3id.org/meta-share/meta-share/Role
ms:Role rdf:type owl:Class ;
        rdfs:comment "The role of an agent with regard to an activity (e.g. contributor, funder, software developer, etc.)"@en ;
        rdfs:label "Role"@en .


###  http://w3id.org/meta-share/meta-share/RoleIdentifier
ms:RoleIdentifier rdf:type owl:Class ;
                  rdfs:subClassOf datacite:Identifier ,
                                  [ rdf:type owl:Restriction ;
                                    owl:onProperty ms:conformsTo ;
                                    owl:allValuesFrom ms:RoleIdentifierScheme
                                  ] ;
                  rdfs:comment "A string used to uniquely identify a role according to a specific scheme"@en ;
                  rdfs:label "Role identifier"@en .


###  http://w3id.org/meta-share/meta-share/RoleIdentifierScheme
ms:RoleIdentifierScheme rdf:type owl:Class ;
                        rdfs:subClassOf datacite:IdentifierScheme ;
                        rdfs:comment "The name of the scheme used to identify a role"@en ;
                        rdfs:label "Role identifier scheme"@en .


###  http://w3id.org/meta-share/meta-share/Sample
ms:Sample rdf:type owl:Class ;
          rdfs:comment "A combination of the sample text(s) or sample file(s) and optional tags that can be used for feeding a processing service for testing purposes"@en ;
          rdfs:label "Sample"@en .


###  http://w3id.org/meta-share/meta-share/ScenarioType
ms:ScenarioType rdf:type owl:Class ;
                rdfs:comment "A classification of the task defined for the conversation or the interaction of participants in a multimedia resource"@en ;
                rdfs:label "Scenario type"@en .


###  http://w3id.org/meta-share/meta-share/SceneIllumination
ms:SceneIllumination rdf:type owl:Class ;
                     rdfs:comment "Information on the illumination of the scene"@en ;
                     rdfs:label "Scene illumination"@en .


###  http://w3id.org/meta-share/meta-share/SegmentationLevel
ms:SegmentationLevel rdf:type owl:Class ;
                     rdfs:comment "The level at which a resource may be segmented (e.g., clause, word, unit, etc.)"@en ;
                     rdfs:label "Segmentation level"@en .


###  http://w3id.org/meta-share/meta-share/SensitiveDataIncluded
ms:SensitiveDataIncluded rdf:type owl:Class ;
                         rdfs:comment "Specification of whether the language resource contains sensitive data (e.g., medical/health-related, etc.) and thus requires special handling"@en ;
                         rdfs:label "Sensitive data included"@en .


###  http://w3id.org/meta-share/meta-share/Sex
ms:Sex rdf:type owl:Class ;
       rdfs:comment "Either of the two major forms of individuals that occur in many species and that are distinguished respectively as female or male especially on the basis of their reproductive organs and structures [https://www.merriam-webster.com/dictionary/sex]"@en ;
       rdfs:label "Sex"@en .


###  http://w3id.org/meta-share/meta-share/SexOfParticipants
ms:SexOfParticipants rdf:type owl:Class ;
                     rdfs:comment "The constitution of a group as regards the sex of the members"@en ;
                     rdfs:label "Sex of participants"@en .


###  http://w3id.org/meta-share/meta-share/SignConvention
ms:SignConvention rdf:type owl:Class ;
                  rdfs:comment "Binary representation of numbers"@en ;
                  rdfs:label "Sign convention"@en .


###  http://w3id.org/meta-share/meta-share/SignIn
ms:SignIn rdf:type owl:Class ;
          rdfs:subClassOf odrl:Action ;
          rdfs:comment "To sign in a system or application"@en ;
          rdfs:label "Sign in"@en .


###  http://w3id.org/meta-share/meta-share/SignLicence
ms:SignLicence rdf:type owl:Class ;
               rdfs:subClassOf odrl:Action ;
               rdfs:comment "The obligation of the assignee to sign a licence before being allowed to use a resource"@en ;
               rdfs:label "Sign licence"@en .


###  http://w3id.org/meta-share/meta-share/SignalEncoding
ms:SignalEncoding rdf:type owl:Class ;
                  rdfs:comment "The encoding of the audio type of a multimedia resource"@en ;
                  rdfs:label "Signal encoding"@en .


###  http://w3id.org/meta-share/meta-share/Size
ms:Size rdf:type owl:Class ;
        rdfs:comment "The size of the resource with regard to the SizeUnit measurement in form of a number"@en ;
        rdfs:label "Size"@en .


###  http://w3id.org/meta-share/meta-share/SizeUnit
ms:SizeUnit rdf:type owl:Class ;
            rdfs:comment "The unit of measurement used for determining and describing the size of a resource (part)"@en ;
            rdfs:label "Size unit"@en .


###  http://w3id.org/meta-share/meta-share/SocialMediaOccupationalAccount
ms:SocialMediaOccupationalAccount rdf:type owl:Class ;
                                  rdfs:comment "The details for the social media or occupational account of a person or organization"@en ;
                                  rdfs:label "Social media occupational account"@en .


###  http://w3id.org/meta-share/meta-share/SocialMediaOccupationalAccountType
ms:SocialMediaOccupationalAccountType rdf:type owl:Class ;
                                      rdfs:comment "A list of social media"@en ;
                                      rdfs:label "Social media account occupational type"@en .


###  http://w3id.org/meta-share/meta-share/SoftwareDistribution
ms:SoftwareDistribution rdf:type owl:Class ;
                        rdfs:subClassOf ms:Distribution ,
                                        [ rdf:type owl:Restriction ;
                                          owl:onProperty ms:distributionForm ;
                                          owl:allValuesFrom ms:SoftwareDistributionForm
                                        ] ;
                        rdfs:comment "Any form with which software is distributed (e.g., web services, executable or code files, etc.)"@en ;
                        rdfs:label "Software distribution"@en .


###  http://w3id.org/meta-share/meta-share/SoftwareDistributionForm
ms:SoftwareDistributionForm rdf:type owl:Class ;
                            rdfs:subClassOf ms:DistributionForm ;
                            rdfs:comment "The medium, delivery channel or form (e.g., source code, API, web service, etc.) through which a software object is distributed"@en ;
                            rdfs:label "Software distribution form"@en .


###  http://w3id.org/meta-share/meta-share/SourceChannel
ms:SourceChannel rdf:type owl:Class ;
                 rdfs:comment "Information on the source channel"@en ;
                 rdfs:label "Source channel"@en .


###  http://w3id.org/meta-share/meta-share/SourceChannelType
ms:SourceChannelType rdf:type owl:Class ;
                     rdfs:comment "Type of the source channel"@en ;
                     rdfs:label "Source channel type"@en .


###  http://w3id.org/meta-share/meta-share/SpeakingImpairmentOfParticipants
ms:SpeakingImpairmentOfParticipants rdf:type owl:Class ;
                                    rdfs:comment "Whether the group of participants contains persons withwith speakingimpairments"@en ;
                                    rdfs:label "Speaking impairment of participants"@en .


###  http://w3id.org/meta-share/meta-share/SpeechGenre
ms:SpeechGenre rdf:type owl:Class ;
               rdfs:subClassOf ms:Genre ,
                               [ rdf:type owl:Restriction ;
                                 owl:onProperty datacite:hasIdentifier ;
                                 owl:allValuesFrom ms:SpeechGenreIdentifier
                               ] ,
                               [ rdf:type owl:Restriction ;
                                 owl:onProperty ms:genre ;
                                 owl:allValuesFrom ms:CorpusAudioPart
                               ] ;
               rdfs:comment "A category for the conventionalized discourse of the speech part of a language resource, based on extra-linguistic and internal linguistic criteria"@en ;
               rdfs:label "Speech genre"@en .


###  http://w3id.org/meta-share/meta-share/SpeechGenreClassificationScheme
ms:SpeechGenreClassificationScheme rdf:type owl:Class ;
                                   rdfs:subClassOf ms:ClassificationScheme ;
                                   rdfs:comment "A classification scheme used for speech genres devised by an authority or organization"@en ;
                                   rdfs:label "Speech genre classification scheme"@en .


###  http://w3id.org/meta-share/meta-share/SpeechGenreIdentifier
ms:SpeechGenreIdentifier rdf:type owl:Class ;
                         rdfs:subClassOf datacite:Identifier ,
                                         [ rdf:type owl:Restriction ;
                                           owl:onProperty ms:conformsTo ;
                                           owl:allValuesFrom ms:SpeechGenreClassificationScheme
                                         ] ;
                         rdfs:comment "A string used to uniquely identify a speech genre according to a specific classification scheme"@en ;
                         rdfs:label "Speech genre identifier"@en .


###  http://w3id.org/meta-share/meta-share/SpeechInfluence
ms:SpeechInfluence rdf:type owl:Class ;
                   rdfs:comment "A factor influencing speech"@en ;
                   rdfs:label "Speech influence"@en .


###  http://w3id.org/meta-share/meta-share/SpeechItem
ms:SpeechItem rdf:type owl:Class ;
              rdfs:comment "An element contained in an audio recording that is pronounced and annotated as such"@en ;
              rdfs:label "Speech item"@en .


###  http://w3id.org/meta-share/meta-share/StandardBestPractice
ms:StandardBestPractice rdf:type owl:Class ;
                        rdfs:comment "A standard or best practice widely used to which the lexical/conceptual resource or corpus conforms to"@en ;
                        rdfs:label "Standard/Best practice"@en ;
                        skos:note "some of these are only formats rather than standards; how can we distinguish?"@en .


###  http://w3id.org/meta-share/meta-share/StaticElement
ms:StaticElement rdf:type owl:Class ;
                 rdfs:comment "The static elements visible on images"@en ;
                 rdfs:label "Static element"@en .


###  http://w3id.org/meta-share/meta-share/Subject
ms:Subject rdf:type owl:Class ;
           rdfs:subClassOf ms:Classification ;
           rdfs:comment "A situation, event, thing, etc. that is discussed in the contents of a language resource"@en ;
           rdfs:label "Subject"@en ;
           skos:altLabel "Topic"@en .


###  http://w3id.org/meta-share/meta-share/SubjectClassificationScheme
ms:SubjectClassificationScheme rdf:type owl:Class ;
                               rdfs:subClassOf ms:ClassificationScheme ;
                               rdfs:comment "A classification scheme used for subjects/topics devised by an authority or organization"@en ;
                               rdfs:label "Subject classification scheme"@en .


###  http://w3id.org/meta-share/meta-share/SubjectIdentifier
ms:SubjectIdentifier rdf:type owl:Class ;
                     rdfs:subClassOf datacite:Identifier ,
                                     [ rdf:type owl:Restriction ;
                                       owl:onProperty ms:conformsTo ;
                                       owl:allValuesFrom ms:SubjectClassificationScheme
                                     ] ;
                     rdfs:comment "A string used to uniquely identify a subject according to a specific classification scheme"@en ;
                     rdfs:label "Subject identifier"@en .


###  http://w3id.org/meta-share/meta-share/Subset
ms:Subset rdf:type owl:Class ;
          rdfs:comment "A subset of a language resource in terms of a specific parameter (e.g., per domain, time coverage, linguistic level of representation, etc.)"@en ;
          rdfs:label "Subset"@en .


###  http://w3id.org/meta-share/meta-share/SupportType
ms:SupportType rdf:type owl:Class ;
               rdfs:comment "The type of support provided for the use of a resource"@en ;
               rdfs:label "Support type"@en .


###  http://w3id.org/meta-share/meta-share/TRL
ms:TRL rdf:type owl:Class ;
       rdfs:comment "An indicator of the maturity level of particular technologies according to a measurement system defined by EC [adapted from https://ec.europa.eu/info/funding-tenders/opportunities/portal/screen/support/faq/2890]"@en ;
       rdfs:label "TRL"@en ;
       skos:altLabel "Technology Readiness Level"@en .


###  http://w3id.org/meta-share/meta-share/TextGenre
ms:TextGenre rdf:type owl:Class ;
             rdfs:subClassOf ms:Genre ,
                             [ rdf:type owl:Restriction ;
                               owl:onProperty datacite:hasIdentifier ;
                               owl:allValuesFrom ms:TextGenreIdentifier
                             ] ,
                             [ rdf:type owl:Restriction ;
                               owl:onProperty ms:genre ;
                               owl:allValuesFrom ms:CorpusTextPart
                             ] ;
             rdfs:comment "A category of text characterized by a particular style, form, or content according to a specific classification scheme"@en ;
             rdfs:label "Text genre"@en .


###  http://w3id.org/meta-share/meta-share/TextGenreClassificationScheme
ms:TextGenreClassificationScheme rdf:type owl:Class ;
                                 rdfs:subClassOf ms:ClassificationScheme ;
                                 rdfs:comment "A classification scheme used for text genres devised by an authority or organization"@en ;
                                 rdfs:label "Text genre classification scheme"@en .


###  http://w3id.org/meta-share/meta-share/TextGenreIdentifier
ms:TextGenreIdentifier rdf:type owl:Class ;
                       rdfs:subClassOf datacite:Identifier ,
                                       [ rdf:type owl:Restriction ;
                                         owl:onProperty ms:conformsTo ;
                                         owl:allValuesFrom ms:TextGenreClassificationScheme
                                       ] ;
                       rdfs:comment "A string used to uniquely identify a text genre according to a specific classification scheme"@en ;
                       rdfs:label "Text genre identifier"@en .


###  http://w3id.org/meta-share/meta-share/TextIncludedInImage
ms:TextIncludedInImage rdf:type owl:Class ;
                       rdfs:comment "Provides information on the type of text that may be on the image"@en ;
                       rdfs:label "Text included in image"@en .


###  http://w3id.org/meta-share/meta-share/TextIncludedInVideo
ms:TextIncludedInVideo rdf:type owl:Class ;
                       rdfs:comment "The presence or not of text in or in conjunction with the video and, if yes, the type"@en ;
                       rdfs:label "Text included in video"@en .


###  http://w3id.org/meta-share/meta-share/TextNumericalFormat
ms:TextNumericalFormat rdf:type owl:Class ;
                       rdfs:comment "The format(s) of the textNumerical part of the resource"@en ;
                       rdfs:label "TextNumerical format"@en ;
                       owl:deprecated "" .


###  http://w3id.org/meta-share/meta-share/TextType
ms:TextType rdf:type owl:Class ;
            rdfs:subClassOf ms:Classification ,
                            [ rdf:type owl:Restriction ;
                              owl:onProperty datacite:hasIdentifier ;
                              owl:allValuesFrom ms:TextTypeIdentifier
                            ] ;
            rdfs:comment "An abstract category designed to characterize the main structure of a particular text or one of its parts according to its dominant properties [from https://www.lhn.uni-hamburg.de/node/121.html]"@en ;
            rdfs:label "Text type"@en .


###  http://w3id.org/meta-share/meta-share/TextTypeClassificationScheme
ms:TextTypeClassificationScheme rdf:type owl:Class ;
                                rdfs:subClassOf ms:ClassificationScheme ;
                                rdfs:comment "A classification scheme used for text types devised by an authority or organization"@en ;
                                rdfs:label "Text type classification scheme"@en .


###  http://w3id.org/meta-share/meta-share/TextTypeIdentifier
ms:TextTypeIdentifier rdf:type owl:Class ;
                      rdfs:subClassOf datacite:Identifier ,
                                      [ rdf:type owl:Restriction ;
                                        owl:onProperty ms:conformsTo ;
                                        owl:allValuesFrom ms:TextTypeClassificationScheme
                                      ] ;
                      rdfs:comment "A string used to uniquely identify a text type according to a specific classification scheme"@en ;
                      rdfs:label "Text type identifier"@en .


###  http://w3id.org/meta-share/meta-share/ToolService
ms:ToolService rdf:type owl:Class ;
               rdfs:subClassOf ms:LanguageResource ;
               rdfs:comment "A tool/service/any piece of software that performs language processing and/or any Language Technology related operation."@en ;
               rdfs:label "Language Technology tool/service"@en ;
               skos:altLabel "LT tool/service"@en .


###  http://w3id.org/meta-share/meta-share/Toolkit
ms:Toolkit rdf:type owl:Class ;
           rdfs:subClassOf ms:DevelopmentFramework ;
           rdfs:label "Tooolkit"@en .


###  http://w3id.org/meta-share/meta-share/UserType
ms:UserType rdf:type owl:Class ;
            rdfs:subClassOf odrl:LeftOperand ;
            rdfs:comment "Classification type for users of a language resource; usually required for assessing the licensing or pricing policies for the use of the resource"@en ;
            rdfs:label "User type"@en .


###  http://w3id.org/meta-share/meta-share/Validation
ms:Validation rdf:type owl:Class ;
              rdfs:comment "Each of the procedures and outcomes followed for validating a language resource, i.e. confirming that its contents/structure/operation is as claimed after careful examination"@en ;
              rdfs:label "Validation"@en .


###  http://w3id.org/meta-share/meta-share/ValidationExtent
ms:ValidationExtent rdf:type owl:Class ;
                    rdfs:comment "The resource coverage in terms of validated data"@en ;
                    rdfs:label "Validation extent"@en .


###  http://w3id.org/meta-share/meta-share/ValidationType
ms:ValidationType rdf:type owl:Class ;
                  rdfs:comment "Classification of validation that indicates whether the validation was made on the contents or on formal aspects of the resource"@en ;
                  rdfs:label "Validation type"@en .


###  http://w3id.org/meta-share/meta-share/VersionType
ms:VersionType rdf:type owl:Class ;
               rdfs:comment "A type of versioning vocabulary used mainly for works (e.g., scholarly articles, books, etc.) that go through a formal review process before final publication, marked with major changes across the versions"@en ;
               rdfs:label "Version type"@en ;
               skos:note "When the COAR vocabulary is published (cf. https://www.coar-repositories.org/activities/repository-interoperability/coar-vocabularies/version-type-vocabulary/) check again"@en .


###  http://w3id.org/meta-share/meta-share/VideoFormat
ms:VideoFormat rdf:type owl:Class ;
               rdfs:label "Detailed video format"@en ;
               owl:backwardCompatibleWith "The format of a video (part of a) resource"@en .


###  http://w3id.org/meta-share/meta-share/VideoGenre
ms:VideoGenre rdf:type owl:Class ;
              rdfs:subClassOf ms:Genre ,
                              [ rdf:type owl:Restriction ;
                                owl:onProperty datacite:hasIdentifier ;
                                owl:allValuesFrom ms:VideoGenreIdentifier
                              ] ,
                              [ rdf:type owl:Restriction ;
                                owl:onProperty ms:genre ;
                                owl:allValuesFrom ms:CorpusVideoPart
                              ] ;
              rdfs:comment "A classification of video parts based on extra-linguistic and internal linguistic criteria and reflected on the video style, form or content"@en ;
              rdfs:label "Video genre"@en .


###  http://w3id.org/meta-share/meta-share/VideoGenreClassificationScheme
ms:VideoGenreClassificationScheme rdf:type owl:Class ;
                                  rdfs:subClassOf ms:ClassificationScheme ;
                                  rdfs:comment "A classification scheme devised by an authority for video genres"@en ;
                                  rdfs:label "Video genre classification scheme"@en .


###  http://w3id.org/meta-share/meta-share/VideoGenreIdentifier
ms:VideoGenreIdentifier rdf:type owl:Class ;
                        rdfs:subClassOf datacite:Identifier ,
                                        [ rdf:type owl:Restriction ;
                                          owl:onProperty ms:conformsTo ;
                                          owl:allValuesFrom ms:VideoGenreClassificationScheme
                                        ] ;
                        rdfs:comment "A string used to uniquely identify a video genre according to a specific classification scheme"@en ;
                        rdfs:label "Video genre identifier"@en .


###  http://w3id.org/meta-share/meta-share/VisualModelling
ms:VisualModelling rdf:type owl:Class ;
                   rdfs:comment "The dimensional form applied on the video or image part(s) of a corpus"@en ;
                   rdfs:label "Visual modelling"@en .


###  http://w3id.org/meta-share/meta-share/VocalTractCondition
ms:VocalTractCondition rdf:type owl:Class ;
                       rdfs:comment "The vocal tract condition that may influence the speech of the participant"@en ;
                       rdfs:label "Vocal tract condition"@en .


###  http://w3id.org/meta-share/meta-share/WebServiceType
ms:WebServiceType rdf:type owl:Class ;
                  rdfs:comment "A classification of web services based on the protocol used for accessing them"@en ;
                  rdfs:label "Web service type"@en .


###  http://w3id.org/meta-share/meta-share/WordEmbedding
ms:WordEmbedding rdf:type owl:Class ;
                 rdfs:subClassOf ms:MLModel ;
                 rdfs:comment "Word embedding is the collective name for a set of language modeling and feature learning techniques in natural language processing where words or phrases from the vocabulary are mapped to vectors of real numbers. [wikipedia]"@en ;
                 rdfs:label "Word embedding"@en .


###  http://w3id.org/meta-share/omtd-share/AnnotationType
omtd:AnnotationType rdf:type owl:Class .


###  http://w3id.org/meta-share/omtd-share/DataFormat
omtd:DataFormat rdf:type owl:Class .


###  http://w3id.org/meta-share/omtd-share/Operation
omtd:Operation rdf:type owl:Class .


###  http://w3id.org/meta-share/omtd-share/PackageFormat
omtd:PackageFormat rdf:type owl:Class .


###  http://w3id.org/meta-share/omtd-share/TdmMethod
omtd:TdmMethod rdf:type owl:Class .


###  http://www.w3.org/2004/02/skos/core#Concept
skos:Concept rdf:type owl:Class .


###  http://www.w3.org/2004/02/skos/core#ConceptScheme
skos:ConceptScheme rdf:type owl:Class .


###  http://www.w3.org/ns/dcat#Catalog
dcat:Catalog rdf:type owl:Class .


###  http://www.w3.org/ns/dcat#CatalogRecord
dcat:CatalogRecord rdf:type owl:Class .


###  http://www.w3.org/ns/dcat#Dataset
dcat:Dataset rdf:type owl:Class .


###  http://www.w3.org/ns/odrl/2/Action
odrl:Action rdf:type owl:Class ;
            rdfs:comment "To be formally allowed to access and make use of a resource"@en ;
            rdfs:label "Authorize"@en .


###  http://www.w3.org/ns/odrl/2/LeftOperand
odrl:LeftOperand rdf:type owl:Class .


###  http://www.w3.org/ns/odrl/2/RightOperand
odrl:RightOperand rdf:type owl:Class .


###  http://www.w3.org/ns/odrl/2/Set
odrl:Set rdf:type owl:Class .


###  http://xmlns.com/foaf/0.1/Project
foaf:Project rdf:type owl:Class .


#################################################################
#    Individuals
#################################################################

###  http://purl.org/NET/rdflicense/cc-by4.0
<http://purl.org/NET/rdflicense/cc-by4.0> rdf:type owl:NamedIndividual .


###  http://purl.org/coar/access_right/c_14cb
<http://purl.org/coar/access_right/c_14cb> rdf:type owl:NamedIndividual ,
                                                    ms:AccessRightsStatementIdentifier ;
                                           ms:conformsTo ms:COARightsStatementScheme .


###  http://purl.org/coar/access_right/c_16ec
<http://purl.org/coar/access_right/c_16ec> rdf:type owl:NamedIndividual ,
                                                    ms:AccessRightsStatementIdentifier ;
                                           owl:sameAs ms:restrictedAccess ;
                                           ms:conformsTo ms:COARightsStatementScheme .


###  http://purl.org/coar/access_right/c_abf2
<http://purl.org/coar/access_right/c_abf2> rdf:type owl:NamedIndividual ,
                                                    ms:AccessRightsStatementIdentifier ;
                                           owl:sameAs ms:openAccess ;
                                           ms:conformsTo ms:COARightsStatementScheme .


###  http://purl.org/coar/access_right/c_f1cf
<http://purl.org/coar/access_right/c_f1cf> rdf:type owl:NamedIndividual ,
                                                    ms:AccessRightsStatementIdentifier ;
                                           ms:conformsTo ms:COARightsStatementScheme .


###  http://purl.org/eprint/accessRights/OpenAccess
<http://purl.org/eprint/accessRights/OpenAccess> rdf:type owl:NamedIndividual ;
                                                 owl:sameAs ms:openAccess .


###  http://purl.org/eprint/accessRights/RestrictedAccess
<http://purl.org/eprint/accessRights/RestrictedAccess> rdf:type owl:NamedIndividual ;
                                                       owl:sameAs ms:restrictedAccess .


###  http://purl.org/spar/datacite/ark
datacite:ark rdf:type owl:NamedIndividual ,
                      ms:DocumentIdentifierScheme ,
                      ms:LRIdentifierScheme ;
             rdfs:comment "Archival Resource Key"@en ;
             rdfs:label "ARK"@en .


###  http://purl.org/spar/datacite/arxiv
datacite:arxiv rdf:type owl:NamedIndividual ,
                        ms:DocumentIdentifierScheme ,
                        ms:LRIdentifierScheme ;
               rdfs:comment "Identifier for ArXiv (http://arxiv.org/), a open access repository of preprints, having the format arXiv:1207.2147."@en ;
               rdfs:label "ArXiv"@en .


###  http://purl.org/spar/datacite/bibcode
datacite:bibcode rdf:type owl:NamedIndividual ,
                          ms:DocumentIdentifierScheme ,
                          ms:LRIdentifierScheme ;
                 rdfs:comment "It is the Astrophysics Data System bibliographic codes, a standardized 19 character identifier according to the syntax \"yyyyjjjjjvvvvmppppa\"."@en ;
                 rdfs:label "bibcode"@en .


###  http://purl.org/spar/datacite/doi
datacite:doi rdf:type owl:NamedIndividual ,
                      datacite:OrganizationIdentifierScheme ,
                      ms:DocumentIdentifierScheme ,
                      ms:LRIdentifierScheme ;
             rdfs:comment "Digital Object Identifier scheme (https://www.doi.org/)"@en ;
             rdfs:label "DOI"@en .


###  http://purl.org/spar/datacite/handle
datacite:handle rdf:type owl:NamedIndividual ,
                         ms:DocumentIdentifierScheme ,
                         ms:LRIdentifierScheme ,
                         ms:MetadataRecordIdentifierScheme ,
                         ms:RepositoryIdentifierScheme ;
                rdfs:comment "the Handle system"@en ;
                rdfs:label "Handle"@en .


###  http://purl.org/spar/datacite/isbn
datacite:isbn rdf:type owl:NamedIndividual ,
                       ms:DocumentIdentifierScheme ,
                       ms:LRIdentifierScheme ;
              rdfs:comment "International Standard Book Number"@en ;
              rdfs:label "ISBN"@en .


###  http://purl.org/spar/datacite/openid
datacite:openid rdf:type owl:NamedIndividual ,
                         datacite:PersonalIdentifierScheme ;
                rdfs:comment "OpenID is an open standard that describes how users can be authenticated in a decentralized manner, eliminating the need for centralized registration services."@en ;
                rdfs:label "OpenID"@en .


###  http://purl.org/spar/datacite/orcid
datacite:orcid rdf:type owl:NamedIndividual ,
                        datacite:PersonalIdentifierScheme ;
               rdfs:comment "Open Researcher and Contributor Identifier."@en ;
               rdfs:label "ORCID"@en .


###  http://purl.org/spar/datacite/purl
datacite:purl rdf:type owl:NamedIndividual ,
                       ms:DocumentIdentifierScheme ,
                       ms:LRIdentifierScheme ,
                       ms:MetadataRecordIdentifierScheme ;
              rdfs:comment "Persistent Uniform Resource Locator"@en ;
              rdfs:label "PURL"@en .


###  http://purl.org/spar/datacite/researcherid
datacite:researcherid rdf:type owl:NamedIndividual ,
                               datacite:PersonalIdentifierScheme ;
                      rdfs:comment "ResearcherID is an identifying system for scientific authors created and owned by Thomson Reuters."@en ;
                      rdfs:label "ResearcherID"@en .


###  http://purl.org/spar/datacite/upc
datacite:upc rdf:type owl:NamedIndividual ,
                      ms:DocumentIdentifierScheme ,
                      ms:LRIdentifierScheme ;
             rdfs:comment "Universal Product Code"@en ;
             rdfs:label "UPC"@en .


###  http://purl.org/spar/datacite/url
datacite:url rdf:type owl:NamedIndividual ,
                      ms:DocumentIdentifierScheme ,
                      ms:LRIdentifierScheme ,
                      ms:MetadataRecordIdentifierScheme ;
             rdfs:comment "Uniform Resource Locator"@en ;
             rdfs:label "URL"@en .


###  http://purl.org/spar/datacite/urn
datacite:urn rdf:type owl:NamedIndividual ,
                      ms:DocumentIdentifierScheme ,
                      ms:LRIdentifierScheme ,
                      ms:MetadataRecordIdentifierScheme ;
             rdfs:comment "Uniform Resource Name"@en ;
             rdfs:label "URN"@en .


###  http://rightsstatements.org/vocab/CNE/1.0/
<http://rightsstatements.org/vocab/CNE/1.0/> rdf:type owl:NamedIndividual ,
                                                      ms:AccessRightsStatementIdentifier ;
                                             ms:conformsTo ms:RightsStatementOrgScheme .


###  http://rightsstatements.org/vocab/InC-EDU/1.0/
<http://rightsstatements.org/vocab/InC-EDU/1.0/> rdf:type owl:NamedIndividual ,
                                                          ms:AccessRightsStatementIdentifier ;
                                                 ms:conformsTo ms:RightsStatementOrgScheme .


###  http://rightsstatements.org/vocab/InC-NC/1.0/
<http://rightsstatements.org/vocab/InC-NC/1.0/> rdf:type owl:NamedIndividual ,
                                                         ms:AccessRightsStatementIdentifier ;
                                                ms:conformsTo ms:RightsStatementOrgScheme .


###  http://rightsstatements.org/vocab/InC-OW-EU/1.0/
<http://rightsstatements.org/vocab/InC-OW-EU/1.0/> rdf:type owl:NamedIndividual ,
                                                            ms:AccessRightsStatementIdentifier ;
                                                   ms:conformsTo ms:RightsStatementOrgScheme .


###  http://rightsstatements.org/vocab/InC-RUU/1.0/
<http://rightsstatements.org/vocab/InC-RUU/1.0/> rdf:type owl:NamedIndividual ,
                                                          ms:AccessRightsStatementIdentifier ;
                                                 ms:conformsTo ms:RightsStatementOrgScheme .


###  http://rightsstatements.org/vocab/InC/1.0/
<http://rightsstatements.org/vocab/InC/1.0/> rdf:type owl:NamedIndividual ,
                                                      ms:AccessRightsStatementIdentifier ;
                                             ms:conformsTo ms:RightsStatementOrgScheme .


###  http://rightsstatements.org/vocab/NKC/1.0/
<http://rightsstatements.org/vocab/NKC/1.0/> rdf:type owl:NamedIndividual ,
                                                      ms:AccessRightsStatementIdentifier ;
                                             ms:conformsTo ms:RightsStatementOrgScheme .


###  http://rightsstatements.org/vocab/NoC-CR/1.0/
<http://rightsstatements.org/vocab/NoC-CR/1.0/> rdf:type owl:NamedIndividual ,
                                                         ms:AccessRightsStatementIdentifier ;
                                                ms:conformsTo ms:RightsStatementOrgScheme .


###  http://rightsstatements.org/vocab/NoC-NC/1.0/
<http://rightsstatements.org/vocab/NoC-NC/1.0/> rdf:type owl:NamedIndividual ,
                                                         ms:AccessRightsStatementIdentifier ;
                                                ms:conformsTo ms:RightsStatementOrgScheme .


###  http://rightsstatements.org/vocab/NoC-OKLR/1.0/
<http://rightsstatements.org/vocab/NoC-OKLR/1.0/> rdf:type owl:NamedIndividual ,
                                                           ms:AccessRightsStatementIdentifier ;
                                                  ms:conformsTo ms:RightsStatementOrgScheme .


###  http://rightsstatements.org/vocab/NoC-US/1.0/
<http://rightsstatements.org/vocab/NoC-US/1.0/> rdf:type owl:NamedIndividual ,
                                                         ms:AccessRightsStatementIdentifier ;
                                                ms:conformsTo ms:RightsStatementOrgScheme .


###  http://rightsstatements.org/vocab/UND/1.0/
<http://rightsstatements.org/vocab/UND/1.0/> rdf:type owl:NamedIndividual ,
                                                      ms:AccessRightsStatementIdentifier ;
                                             ms:conformsTo ms:RightsStatementOrgScheme .


###  http://w3id.org/meta-share/meta-share
<http://w3id.org/meta-share/meta-share> rdf:type owl:NamedIndividual .


###  http://w3id.org/meta-share/meta-share/ADPCM
ms:ADPCM rdf:type owl:NamedIndividual ,
                  ms:SignalEncoding ;
         rdfs:label "ADPCM"@en ;
         skos:altLabel "Adaptive differential pulse-code modulation"@en .


###  http://w3id.org/meta-share/meta-share/ANC_domainClassification
ms:ANC_domainClassification rdf:type owl:NamedIndividual ,
                                     ms:DomainClassificationScheme ;
                            rdfs:label "ANC domain classification system"@en ;
                            skos:altLabel "American National Corpus domain classification system"@en .


###  http://w3id.org/meta-share/meta-share/ANC_genreClassification
ms:ANC_genreClassification rdf:type owl:NamedIndividual ,
                                    ms:TextGenreClassificationScheme ;
                           rdfs:label "ANC genre classification scheme"@en ;
                           skos:altLabel "American National Corpus genre classification scheme"@en .


###  http://w3id.org/meta-share/meta-share/ART
ms:ART rdf:type owl:NamedIndividual ,
                ms:Metric ;
       rdfs:label "ART"@en ;
       skos:altLabel "Average Response Time"@en .


###  http://w3id.org/meta-share/meta-share/AllenNLP
ms:AllenNLP rdf:type owl:NamedIndividual ,
                     ms:NLPFramework ;
            rdfs:comment "NLP framework based on deep learning; it includes reference implementations of high quality models for both core NLP problems (e.g. semantic role labeling) and NLP applications (e.g. textual entailment); built on PyTorch"@en ;
            rdfs:label "AllenNLP"@en .


###  http://w3id.org/meta-share/meta-share/AlvisNLP
ms:AlvisNLP rdf:type owl:NamedIndividual ,
                     ms:Framework ;
            rdfs:label "AlvisNLP"@en .


###  http://w3id.org/meta-share/meta-share/Asteroid
ms:Asteroid rdf:type owl:NamedIndividual ,
                     ms:Toolkit ;
            rdfs:comment "A speech processing toolkit based on PyTorch"@en ;
            rdfs:label "Asteroid"@en .


###  http://w3id.org/meta-share/meta-share/AudioType
ms:AudioType rdf:type owl:NamedIndividual ,
                      skos:Concept ;
             rdfs:comment "A type of content included in a language resource pertaining to the audio level"@en ;
             rdfs:label "Audio type"@en ;
             skos:inScheme ms:ContentTypeScheme .


###  http://w3id.org/meta-share/meta-share/BML
ms:BML rdf:type owl:NamedIndividual ,
                ms:StandardBestPractice ;
       ms:url "http://www.mindmakers.org/projects/bml-1-0/wiki#Introduction" ;
       rdfs:label "BML"@en ;
       skos:altLabel "Behavior Markup Language"@en ,
                     "Behaviour Markup Language"@en .


###  http://w3id.org/meta-share/meta-share/BNC_domainClassification
ms:BNC_domainClassification rdf:type owl:NamedIndividual ,
                                     ms:DomainClassificationScheme ;
                            rdfs:label "BNC domain classification system"@en ;
                            skos:altLabel "British National Corpus domain classification system"@en .


###  http://w3id.org/meta-share/meta-share/BNC_textTypeClassification
ms:BNC_textTypeClassification rdf:type owl:NamedIndividual ,
                                       ms:TextTypeClassificationScheme ;
                              rdfs:label "BNC text type classification scheme"@en .


###  http://w3id.org/meta-share/meta-share/Big5
ms:Big5 rdf:type owl:NamedIndividual ,
                 ms:CharacterEncoding ;
        rdfs:label "Big5"@en .


###  http://w3id.org/meta-share/meta-share/Big5-HKSCS
ms:Big5-HKSCS rdf:type owl:NamedIndividual ,
                       ms:CharacterEncoding ;
              rdfs:label "Big5-HKSCS"@en .


###  http://w3id.org/meta-share/meta-share/Big5_Solaris
ms:Big5_Solaris rdf:type owl:NamedIndividual ,
                         ms:CharacterEncoding ;
                rdfs:label "Big5_Solaris"@en .


###  http://w3id.org/meta-share/meta-share/CD-ROM
ms:CD-ROM rdf:type owl:NamedIndividual ,
                   ms:DatasetDistributionForm ;
          rdfs:comment "CD-ROM refers to a kind of distribution medium used for delivering a language resource; intended for resources delivered on CD-ROM"@en ;
          rdfs:label "CD-ROM"@en .


###  http://w3id.org/meta-share/meta-share/CDMA
ms:CDMA rdf:type owl:NamedIndividual ,
                 ms:SourceChannelType ;
        rdfs:label "CDMA"@en .


###  http://w3id.org/meta-share/meta-share/CES
ms:CES rdf:type owl:NamedIndividual ,
                ms:StandardBestPractice ;
       ms:url "https://www.cs.vassar.edu/CES/" ;
       rdfs:label "CES"@en ;
       skos:altLabel "Corpus Encoding Standard"@en .


###  http://w3id.org/meta-share/meta-share/CLARIN-SHARE
ms:CLARIN-SHARE rdf:type owl:NamedIndividual ,
                         ms:StandardBestPractice ;
                rdfs:label "CLARIN-SHARE"@en .


###  http://w3id.org/meta-share/meta-share/CMYK
ms:CMYK rdf:type owl:NamedIndividual ,
                 ms:ColourSpace ;
        rdfs:label "CMYK"@en .


###  http://w3id.org/meta-share/meta-share/COARightsStatementScheme
ms:COARightsStatementScheme rdf:type owl:NamedIndividual ,
                                     ms:AccessRightsStatementScheme ;
                            rdfs:comment "COAR access rights vocabulary (http://vocabularies.coar-repositories.org/documentation/access_rights/)"@en ;
                            rdfs:label "COAR Rights Statement Scheme"@en .


###  http://w3id.org/meta-share/meta-share/CORE
ms:CORE rdf:type owl:NamedIndividual ,
                 ms:MetadataRecordIdentifierScheme ;
        rdfs:label "CORE"@en .


###  http://w3id.org/meta-share/meta-share/Caffe
ms:Caffe rdf:type owl:NamedIndividual ,
                  ms:MLFramework ;
         rdfs:label "Caffe"@en .


###  http://w3id.org/meta-share/meta-share/ClarinEL_TextTypeClassification
ms:ClarinEL_TextTypeClassification rdf:type owl:NamedIndividual ,
                                            ms:TextTypeClassificationScheme ;
                                   rdfs:label "CLARIN_EL text type classification scheme"@en .


###  http://w3id.org/meta-share/meta-share/ClarinEL_domainClassification
ms:ClarinEL_domainClassification rdf:type owl:NamedIndividual ,
                                          ms:DomainClassificationScheme ;
                                 rdfs:label "CLARIN-EL domain classification"@en .


###  http://w3id.org/meta-share/meta-share/ClarinEl_TT001
ms:ClarinEl_TT001 rdf:type owl:NamedIndividual ,
                           ms:TextTypeIdentifier ;
                  ms:conformsTo ms:ClarinEL_TextTypeClassification .


###  http://w3id.org/meta-share/meta-share/ClarinEl_TT002
ms:ClarinEl_TT002 rdf:type owl:NamedIndividual ,
                           ms:TextTypeIdentifier ;
                  ms:conformsTo ms:ClarinEL_TextTypeClassification .


###  http://w3id.org/meta-share/meta-share/ClarinEl_TT003
ms:ClarinEl_TT003 rdf:type owl:NamedIndividual ,
                           ms:TextTypeIdentifier ;
                  ms:conformsTo ms:ClarinEL_TextTypeClassification .


###  http://w3id.org/meta-share/meta-share/ClarinEl_TT004
ms:ClarinEl_TT004 rdf:type owl:NamedIndividual ,
                           ms:TextTypeIdentifier ;
                  ms:conformsTo ms:ClarinEL_TextTypeClassification .


###  http://w3id.org/meta-share/meta-share/ClarinEl_TT005
ms:ClarinEl_TT005 rdf:type owl:NamedIndividual ,
                           ms:TextTypeIdentifier ;
                  ms:conformsTo ms:ClarinEL_TextTypeClassification .


###  http://w3id.org/meta-share/meta-share/ClarinEl_TT006
ms:ClarinEl_TT006 rdf:type owl:NamedIndividual ,
                           ms:TextTypeIdentifier ;
                  ms:conformsTo ms:ClarinEL_TextTypeClassification .


###  http://w3id.org/meta-share/meta-share/ClarinEl_TT007
ms:ClarinEl_TT007 rdf:type owl:NamedIndividual ,
                           ms:TextTypeIdentifier ;
                  ms:conformsTo ms:ClarinEL_TextTypeClassification .


###  http://w3id.org/meta-share/meta-share/ClarinEl_TT008
ms:ClarinEl_TT008 rdf:type owl:NamedIndividual ,
                           ms:TextTypeIdentifier ;
                  ms:conformsTo ms:ClarinEL_TextTypeClassification .


###  http://w3id.org/meta-share/meta-share/ClarinEl_TT009
ms:ClarinEl_TT009 rdf:type owl:NamedIndividual ,
                           ms:TextTypeIdentifier ;
                  ms:conformsTo ms:ClarinEL_TextTypeClassification .


###  http://w3id.org/meta-share/meta-share/ClarinEl_TT010
ms:ClarinEl_TT010 rdf:type owl:NamedIndividual ,
                           ms:TextTypeIdentifier ;
                  ms:conformsTo ms:ClarinEL_TextTypeClassification .


###  http://w3id.org/meta-share/meta-share/ClarinEl_TT011
ms:ClarinEl_TT011 rdf:type owl:NamedIndividual ,
                           ms:TextTypeIdentifier ;
                  ms:conformsTo ms:ClarinEL_TextTypeClassification .


###  http://w3id.org/meta-share/meta-share/ClarinEl_TT012
ms:ClarinEl_TT012 rdf:type owl:NamedIndividual ,
                           ms:TextTypeIdentifier ;
                  ms:conformsTo ms:ClarinEL_TextTypeClassification .


###  http://w3id.org/meta-share/meta-share/ClarinEl_TT013
ms:ClarinEl_TT013 rdf:type owl:NamedIndividual ,
                           ms:TextTypeIdentifier ;
                  ms:conformsTo ms:ClarinEL_TextTypeClassification .


###  http://w3id.org/meta-share/meta-share/ClarinEl_TT014
ms:ClarinEl_TT014 rdf:type owl:NamedIndividual ,
                           ms:TextTypeIdentifier ;
                  ms:conformsTo ms:ClarinEL_TextTypeClassification .


###  http://w3id.org/meta-share/meta-share/ClarinEl_TT015
ms:ClarinEl_TT015 rdf:type owl:NamedIndividual ,
                           ms:TextTypeIdentifier ;
                  ms:conformsTo ms:ClarinEL_TextTypeClassification .


###  http://w3id.org/meta-share/meta-share/ClarinEl_TT016
ms:ClarinEl_TT016 rdf:type owl:NamedIndividual ,
                           ms:TextTypeIdentifier ;
                  ms:conformsTo ms:ClarinEL_TextTypeClassification .


###  http://w3id.org/meta-share/meta-share/ClarinEl_TT017
ms:ClarinEl_TT017 rdf:type owl:NamedIndividual ,
                           ms:TextTypeIdentifier ;
                  ms:conformsTo ms:ClarinEL_TextTypeClassification .


###  http://w3id.org/meta-share/meta-share/ClarinEl_TT018
ms:ClarinEl_TT018 rdf:type owl:NamedIndividual ,
                           ms:TextTypeIdentifier ;
                  ms:conformsTo ms:ClarinEL_TextTypeClassification .


###  http://w3id.org/meta-share/meta-share/ClarinLicenceCategoryScheme
ms:ClarinLicenceCategoryScheme rdf:type owl:NamedIndividual ,
                                        ms:LicenceCategoryScheme ;
                               rdfs:label "CLARIN licence category scheme"@en .


###  http://w3id.org/meta-share/meta-share/Clarin_Domain001
ms:Clarin_Domain001 rdf:type owl:NamedIndividual ,
                             ms:DomainIdentifier ;
                    ms:conformsTo ms:ClarinEL_domainClassification .


###  http://w3id.org/meta-share/meta-share/Clarin_Domain002
ms:Clarin_Domain002 rdf:type owl:NamedIndividual ,
                             ms:DomainIdentifier ;
                    ms:conformsTo ms:ClarinEL_domainClassification .


###  http://w3id.org/meta-share/meta-share/Clarin_Domain003
ms:Clarin_Domain003 rdf:type owl:NamedIndividual ,
                             ms:DomainIdentifier ;
                    ms:conformsTo ms:ClarinEL_domainClassification .


###  http://w3id.org/meta-share/meta-share/Clarin_Domain004
ms:Clarin_Domain004 rdf:type owl:NamedIndividual ,
                             ms:DomainIdentifier ;
                    ms:conformsTo ms:ClarinEL_domainClassification .


###  http://w3id.org/meta-share/meta-share/Clarin_Domain005
ms:Clarin_Domain005 rdf:type owl:NamedIndividual ,
                             ms:DomainIdentifier ;
                    ms:conformsTo ms:ClarinEL_domainClassification .


###  http://w3id.org/meta-share/meta-share/Clarin_Domain006
ms:Clarin_Domain006 rdf:type owl:NamedIndividual ,
                             ms:DomainIdentifier ;
                    ms:conformsTo ms:ClarinEL_domainClassification .


###  http://w3id.org/meta-share/meta-share/ContentType
ms:ContentType rdf:type owl:NamedIndividual ,
                        skos:Concept ;
               rdfs:comment "A more detailed account of the linguistic information contained in the lexical/conceptual resource"@en ;
               rdfs:label "Content type"@en ;
               skos:inScheme ms:ContentTypeScheme ;
               skos:note """could we organise them hierarchically?
for those that are used for annotation, align with annotationType values? or can we use annotationType together with these values as range for the property?
add definitions to all instances"""@en .


###  http://w3id.org/meta-share/meta-share/ContentTypeScheme
ms:ContentTypeScheme rdf:type owl:NamedIndividual ,
                              skos:ConceptScheme ;
                     rdfs:label "Content types vocabulary"@en ;
                     skos:hasTopConcept ms:ContentType ;
                     skos:prefLabel "Content types vocabulary"@en .


###  http://w3id.org/meta-share/meta-share/Cp037
ms:Cp037 rdf:type owl:NamedIndividual ,
                  ms:CharacterEncoding ;
         rdfs:label "Cp037"@en .


###  http://w3id.org/meta-share/meta-share/Cp1006
ms:Cp1006 rdf:type owl:NamedIndividual ,
                   ms:CharacterEncoding ;
          rdfs:label "Cp1006"@en .


###  http://w3id.org/meta-share/meta-share/Cp1025
ms:Cp1025 rdf:type owl:NamedIndividual ,
                   ms:CharacterEncoding ;
          rdfs:label "Cp1025"@en .


###  http://w3id.org/meta-share/meta-share/Cp1026
ms:Cp1026 rdf:type owl:NamedIndividual ,
                   ms:CharacterEncoding ;
          rdfs:label "Cp1026"@en .


###  http://w3id.org/meta-share/meta-share/Cp1046
ms:Cp1046 rdf:type owl:NamedIndividual ,
                   ms:CharacterEncoding ;
          rdfs:label "Cp1046"@en .


###  http://w3id.org/meta-share/meta-share/Cp1047
ms:Cp1047 rdf:type owl:NamedIndividual ,
                   ms:CharacterEncoding ;
          rdfs:label "Cp1047"@en .


###  http://w3id.org/meta-share/meta-share/Cp1097
ms:Cp1097 rdf:type owl:NamedIndividual ,
                   ms:CharacterEncoding ;
          rdfs:label "Cp1097"@en .


###  http://w3id.org/meta-share/meta-share/Cp1098
ms:Cp1098 rdf:type owl:NamedIndividual ,
                   ms:CharacterEncoding ;
          rdfs:label "Cp1098"@en .


###  http://w3id.org/meta-share/meta-share/Cp1112
ms:Cp1112 rdf:type owl:NamedIndividual ,
                   ms:CharacterEncoding ;
          rdfs:label "Cp1112"@en .


###  http://w3id.org/meta-share/meta-share/Cp1122
ms:Cp1122 rdf:type owl:NamedIndividual ,
                   ms:CharacterEncoding ;
          rdfs:label "Cp1122"@en .


###  http://w3id.org/meta-share/meta-share/Cp1123
ms:Cp1123 rdf:type owl:NamedIndividual ,
                   ms:CharacterEncoding ;
          rdfs:label "Cp1123"@en .


###  http://w3id.org/meta-share/meta-share/Cp1124
ms:Cp1124 rdf:type owl:NamedIndividual ,
                   ms:CharacterEncoding ;
          rdfs:label "Cp1124"@en .


###  http://w3id.org/meta-share/meta-share/Cp1140
ms:Cp1140 rdf:type owl:NamedIndividual ,
                   ms:CharacterEncoding ;
          rdfs:label "Cp1140"@en .


###  http://w3id.org/meta-share/meta-share/Cp1141
ms:Cp1141 rdf:type owl:NamedIndividual ,
                   ms:CharacterEncoding ;
          rdfs:label "Cp1141"@en .


###  http://w3id.org/meta-share/meta-share/Cp1142
ms:Cp1142 rdf:type owl:NamedIndividual ,
                   ms:CharacterEncoding ;
          rdfs:label "Cp1142"@en .


###  http://w3id.org/meta-share/meta-share/Cp1143
ms:Cp1143 rdf:type owl:NamedIndividual ,
                   ms:CharacterEncoding ;
          rdfs:label "Cp1143"@en .


###  http://w3id.org/meta-share/meta-share/Cp1144
ms:Cp1144 rdf:type owl:NamedIndividual ,
                   ms:CharacterEncoding ;
          rdfs:label "Cp1144"@en .


###  http://w3id.org/meta-share/meta-share/Cp1145
ms:Cp1145 rdf:type owl:NamedIndividual ,
                   ms:CharacterEncoding ;
          rdfs:label "Cp1145"@en .


###  http://w3id.org/meta-share/meta-share/Cp1146
ms:Cp1146 rdf:type owl:NamedIndividual ,
                   ms:CharacterEncoding ;
          rdfs:label "Cp1146"@en .


###  http://w3id.org/meta-share/meta-share/Cp1147
ms:Cp1147 rdf:type owl:NamedIndividual ,
                   ms:CharacterEncoding ;
          rdfs:label "Cp1147"@en .


###  http://w3id.org/meta-share/meta-share/Cp1148
ms:Cp1148 rdf:type owl:NamedIndividual ,
                   ms:CharacterEncoding ;
          rdfs:label "Cp1148"@en .


###  http://w3id.org/meta-share/meta-share/Cp1149
ms:Cp1149 rdf:type owl:NamedIndividual ,
                   ms:CharacterEncoding ;
          rdfs:label "Cp1149"@en .


###  http://w3id.org/meta-share/meta-share/Cp1381
ms:Cp1381 rdf:type owl:NamedIndividual ,
                   ms:CharacterEncoding ;
          rdfs:label "Cp1381"@en .


###  http://w3id.org/meta-share/meta-share/Cp1383
ms:Cp1383 rdf:type owl:NamedIndividual ,
                   ms:CharacterEncoding ;
          rdfs:label "Cp1383"@en .


###  http://w3id.org/meta-share/meta-share/Cp273
ms:Cp273 rdf:type owl:NamedIndividual ,
                  ms:CharacterEncoding ;
         rdfs:label "Cp273"@en .


###  http://w3id.org/meta-share/meta-share/Cp277
ms:Cp277 rdf:type owl:NamedIndividual ,
                  ms:CharacterEncoding ;
         rdfs:label "Cp277"@en .


###  http://w3id.org/meta-share/meta-share/Cp278
ms:Cp278 rdf:type owl:NamedIndividual ,
                  ms:CharacterEncoding ;
         rdfs:label "Cp278"@en .


###  http://w3id.org/meta-share/meta-share/Cp280
ms:Cp280 rdf:type owl:NamedIndividual ,
                  ms:CharacterEncoding ;
         rdfs:label "Cp280"@en .


###  http://w3id.org/meta-share/meta-share/Cp284
ms:Cp284 rdf:type owl:NamedIndividual ,
                  ms:CharacterEncoding ;
         rdfs:label "Cp284"@en .


###  http://w3id.org/meta-share/meta-share/Cp285
ms:Cp285 rdf:type owl:NamedIndividual ,
                  ms:CharacterEncoding ;
         rdfs:label "Cp285"@en .


###  http://w3id.org/meta-share/meta-share/Cp297
ms:Cp297 rdf:type owl:NamedIndividual ,
                  ms:CharacterEncoding ;
         rdfs:label "Cp297"@en .


###  http://w3id.org/meta-share/meta-share/Cp33722
ms:Cp33722 rdf:type owl:NamedIndividual ,
                    ms:CharacterEncoding ;
           rdfs:label "Cp33722"@en .


###  http://w3id.org/meta-share/meta-share/Cp420
ms:Cp420 rdf:type owl:NamedIndividual ,
                  ms:CharacterEncoding ;
         rdfs:label "Cp420"@en .


###  http://w3id.org/meta-share/meta-share/Cp424
ms:Cp424 rdf:type owl:NamedIndividual ,
                  ms:CharacterEncoding ;
         rdfs:label "Cp424"@en .


###  http://w3id.org/meta-share/meta-share/Cp437
ms:Cp437 rdf:type owl:NamedIndividual ,
                  ms:CharacterEncoding ;
         rdfs:label "Cp437"@en .


###  http://w3id.org/meta-share/meta-share/Cp500
ms:Cp500 rdf:type owl:NamedIndividual ,
                  ms:CharacterEncoding ;
         rdfs:label "Cp500"@en .


###  http://w3id.org/meta-share/meta-share/Cp737
ms:Cp737 rdf:type owl:NamedIndividual ,
                  ms:CharacterEncoding ;
         rdfs:label "Cp737"@en .


###  http://w3id.org/meta-share/meta-share/Cp775
ms:Cp775 rdf:type owl:NamedIndividual ,
                  ms:CharacterEncoding ;
         rdfs:label "Cp775"@en .


###  http://w3id.org/meta-share/meta-share/Cp838
ms:Cp838 rdf:type owl:NamedIndividual ,
                  ms:CharacterEncoding ;
         rdfs:label "Cp838"@en .


###  http://w3id.org/meta-share/meta-share/Cp850
ms:Cp850 rdf:type owl:NamedIndividual ,
                  ms:CharacterEncoding ;
         rdfs:label "Cp850"@en .


###  http://w3id.org/meta-share/meta-share/Cp852
ms:Cp852 rdf:type owl:NamedIndividual ,
                  ms:CharacterEncoding ;
         rdfs:label "Cp852"@en .


###  http://w3id.org/meta-share/meta-share/Cp855
ms:Cp855 rdf:type owl:NamedIndividual ,
                  ms:CharacterEncoding ;
         rdfs:label "Cp855"@en .


###  http://w3id.org/meta-share/meta-share/Cp856
ms:Cp856 rdf:type owl:NamedIndividual ,
                  ms:CharacterEncoding ;
         rdfs:label "Cp856"@en .


###  http://w3id.org/meta-share/meta-share/Cp857
ms:Cp857 rdf:type owl:NamedIndividual ,
                  ms:CharacterEncoding ;
         rdfs:label "Cp857"@en .


###  http://w3id.org/meta-share/meta-share/Cp858
ms:Cp858 rdf:type owl:NamedIndividual ,
                  ms:CharacterEncoding ;
         rdfs:label "Cp858"@en .


###  http://w3id.org/meta-share/meta-share/Cp860
ms:Cp860 rdf:type owl:NamedIndividual ,
                  ms:CharacterEncoding ;
         rdfs:label "Cp860"@en .


###  http://w3id.org/meta-share/meta-share/Cp861
ms:Cp861 rdf:type owl:NamedIndividual ,
                  ms:CharacterEncoding ;
         rdfs:label "Cp861"@en .


###  http://w3id.org/meta-share/meta-share/Cp862
ms:Cp862 rdf:type owl:NamedIndividual ,
                  ms:CharacterEncoding ;
         rdfs:label "Cp862"@en .


###  http://w3id.org/meta-share/meta-share/Cp863
ms:Cp863 rdf:type owl:NamedIndividual ,
                  ms:CharacterEncoding ;
         rdfs:label "Cp863"@en .


###  http://w3id.org/meta-share/meta-share/Cp864
ms:Cp864 rdf:type owl:NamedIndividual ,
                  ms:CharacterEncoding ;
         rdfs:label "Cp864"@en .


###  http://w3id.org/meta-share/meta-share/Cp865
ms:Cp865 rdf:type owl:NamedIndividual ,
                  ms:CharacterEncoding ;
         rdfs:label "Cp865"@en .


###  http://w3id.org/meta-share/meta-share/Cp866
ms:Cp866 rdf:type owl:NamedIndividual ,
                  ms:CharacterEncoding ;
         rdfs:label "Cp866"@en .


###  http://w3id.org/meta-share/meta-share/Cp868
ms:Cp868 rdf:type owl:NamedIndividual ,
                  ms:CharacterEncoding ;
         rdfs:label "Cp868"@en .


###  http://w3id.org/meta-share/meta-share/Cp869
ms:Cp869 rdf:type owl:NamedIndividual ,
                  ms:CharacterEncoding ;
         rdfs:label "Cp869"@en .


###  http://w3id.org/meta-share/meta-share/Cp870
ms:Cp870 rdf:type owl:NamedIndividual ,
                  ms:CharacterEncoding ;
         rdfs:label "Cp870"@en .


###  http://w3id.org/meta-share/meta-share/Cp871
ms:Cp871 rdf:type owl:NamedIndividual ,
                  ms:CharacterEncoding ;
         rdfs:label "Cp871"@en .


###  http://w3id.org/meta-share/meta-share/Cp874
ms:Cp874 rdf:type owl:NamedIndividual ,
                  ms:CharacterEncoding ;
         rdfs:label "Cp874"@en .


###  http://w3id.org/meta-share/meta-share/Cp875
ms:Cp875 rdf:type owl:NamedIndividual ,
                  ms:CharacterEncoding ;
         rdfs:label "Cp875"@en .


###  http://w3id.org/meta-share/meta-share/Cp918
ms:Cp918 rdf:type owl:NamedIndividual ,
                  ms:CharacterEncoding ;
         rdfs:label "Cp918"@en .


###  http://w3id.org/meta-share/meta-share/Cp921
ms:Cp921 rdf:type owl:NamedIndividual ,
                  ms:CharacterEncoding ;
         rdfs:label "Cp921"@en .


###  http://w3id.org/meta-share/meta-share/Cp922
ms:Cp922 rdf:type owl:NamedIndividual ,
                  ms:CharacterEncoding ;
         rdfs:label "Cp922"@en .


###  http://w3id.org/meta-share/meta-share/Cp930
ms:Cp930 rdf:type owl:NamedIndividual ,
                  ms:CharacterEncoding ;
         rdfs:label "Cp930"@en .


###  http://w3id.org/meta-share/meta-share/Cp933
ms:Cp933 rdf:type owl:NamedIndividual ,
                  ms:CharacterEncoding ;
         rdfs:label "Cp933"@en .


###  http://w3id.org/meta-share/meta-share/Cp935
ms:Cp935 rdf:type owl:NamedIndividual ,
                  ms:CharacterEncoding ;
         rdfs:label "Cp935"@en .


###  http://w3id.org/meta-share/meta-share/Cp937
ms:Cp937 rdf:type owl:NamedIndividual ,
                  ms:CharacterEncoding ;
         rdfs:label "Cp937"@en .


###  http://w3id.org/meta-share/meta-share/Cp939
ms:Cp939 rdf:type owl:NamedIndividual ,
                  ms:CharacterEncoding ;
         rdfs:label "Cp939"@en .


###  http://w3id.org/meta-share/meta-share/Cp942
ms:Cp942 rdf:type owl:NamedIndividual ,
                  ms:CharacterEncoding ;
         rdfs:label "Cp942"@en .


###  http://w3id.org/meta-share/meta-share/Cp942C
ms:Cp942C rdf:type owl:NamedIndividual ,
                   ms:CharacterEncoding ;
          rdfs:label "Cp942C"@en .


###  http://w3id.org/meta-share/meta-share/Cp943
ms:Cp943 rdf:type owl:NamedIndividual ,
                  ms:CharacterEncoding ;
         rdfs:label "Cp943"@en .


###  http://w3id.org/meta-share/meta-share/Cp943C
ms:Cp943C rdf:type owl:NamedIndividual ,
                   ms:CharacterEncoding ;
          rdfs:label "Cp943C"@en .


###  http://w3id.org/meta-share/meta-share/Cp948
ms:Cp948 rdf:type owl:NamedIndividual ,
                  ms:CharacterEncoding ;
         rdfs:label "Cp948"@en .


###  http://w3id.org/meta-share/meta-share/Cp949
ms:Cp949 rdf:type owl:NamedIndividual ,
                  ms:CharacterEncoding ;
         rdfs:label "Cp949"@en .


###  http://w3id.org/meta-share/meta-share/Cp949C
ms:Cp949C rdf:type owl:NamedIndividual ,
                   ms:CharacterEncoding ;
          rdfs:label "Cp949C"@en .


###  http://w3id.org/meta-share/meta-share/Cp950
ms:Cp950 rdf:type owl:NamedIndividual ,
                  ms:CharacterEncoding ;
         rdfs:label "Cp950"@en .


###  http://w3id.org/meta-share/meta-share/Cp964
ms:Cp964 rdf:type owl:NamedIndividual ,
                  ms:CharacterEncoding ;
         rdfs:label "Cp964"@en .


###  http://w3id.org/meta-share/meta-share/Cp970
ms:Cp970 rdf:type owl:NamedIndividual ,
                  ms:CharacterEncoding ;
         rdfs:label "Cp970"@en .


###  http://w3id.org/meta-share/meta-share/DAT
ms:DAT rdf:type owl:NamedIndividual ,
                ms:RecordingDeviceType ;
       rdfs:label "DAT"@en .


###  http://w3id.org/meta-share/meta-share/DDC000
ms:DDC000 rdf:type owl:NamedIndividual ,
                   ms:DomainIdentifier ;
          ms:conformsTo ms:DDC_classification .


###  http://w3id.org/meta-share/meta-share/DDC070
ms:DDC070 rdf:type owl:NamedIndividual ,
                   ms:DomainIdentifier ;
          ms:conformsTo ms:DDC_classification .


###  http://w3id.org/meta-share/meta-share/DDC100
ms:DDC100 rdf:type owl:NamedIndividual ,
                   ms:DomainIdentifier ;
          ms:conformsTo ms:DDC_classification .


###  http://w3id.org/meta-share/meta-share/DDC150
ms:DDC150 rdf:type owl:NamedIndividual ,
                   ms:DomainIdentifier ;
          ms:conformsTo ms:DDC_classification .


###  http://w3id.org/meta-share/meta-share/DDC200
ms:DDC200 rdf:type owl:NamedIndividual ,
                   ms:DomainIdentifier ;
          ms:conformsTo ms:DDC_classification .


###  http://w3id.org/meta-share/meta-share/DDC300
ms:DDC300 rdf:type owl:NamedIndividual ,
                   ms:DomainIdentifier ;
          ms:conformsTo ms:DDC_classification .


###  http://w3id.org/meta-share/meta-share/DDC301
ms:DDC301 rdf:type owl:NamedIndividual ,
                   ms:DomainIdentifier ;
          ms:conformsTo ms:DDC_classification .


###  http://w3id.org/meta-share/meta-share/DDC310
ms:DDC310 rdf:type owl:NamedIndividual ,
                   ms:DomainIdentifier ;
          ms:conformsTo ms:DDC_classification .


###  http://w3id.org/meta-share/meta-share/DDC320
ms:DDC320 rdf:type owl:NamedIndividual ,
                   ms:DomainIdentifier ;
          ms:conformsTo ms:DDC_classification .


###  http://w3id.org/meta-share/meta-share/DDC330
ms:DDC330 rdf:type owl:NamedIndividual ,
                   ms:DomainIdentifier .


###  http://w3id.org/meta-share/meta-share/DDC340
ms:DDC340 rdf:type owl:NamedIndividual ,
                   ms:DomainIdentifier ;
          ms:conformsTo ms:DDC_classification .


###  http://w3id.org/meta-share/meta-share/DDC351
ms:DDC351 rdf:type owl:NamedIndividual ,
                   ms:DomainIdentifier ;
          ms:conformsTo ms:DDC_classification .


###  http://w3id.org/meta-share/meta-share/DDC360
ms:DDC360 rdf:type owl:NamedIndividual ,
                   ms:DomainIdentifier ;
          ms:conformsTo ms:DDC_classification .


###  http://w3id.org/meta-share/meta-share/DDC370
ms:DDC370 rdf:type owl:NamedIndividual ,
                   ms:DomainIdentifier .


###  http://w3id.org/meta-share/meta-share/DDC381
ms:DDC381 rdf:type owl:NamedIndividual ,
                   ms:DomainIdentifier ;
          ms:conformsTo ms:DDC_classification .


###  http://w3id.org/meta-share/meta-share/DDC384
ms:DDC384 rdf:type owl:NamedIndividual ,
                   ms:DomainIdentifier ;
          ms:conformsTo ms:DDC_classification ;
          rdfs:label "DDC384" .


###  http://w3id.org/meta-share/meta-share/DDC388
ms:DDC388 rdf:type owl:NamedIndividual ,
                   ms:DomainIdentifier ;
          ms:conformsTo ms:DDC_classification ;
          rdfs:label "DDC388"@en .


###  http://w3id.org/meta-share/meta-share/DDC400
ms:DDC400 rdf:type owl:NamedIndividual ,
                   ms:DomainIdentifier ;
          ms:conformsTo ms:DDC_classification .


###  http://w3id.org/meta-share/meta-share/DDC410
ms:DDC410 rdf:type owl:NamedIndividual ,
                   ms:DomainIdentifier ;
          ms:conformsTo ms:DDC_classification .


###  http://w3id.org/meta-share/meta-share/DDC500
ms:DDC500 rdf:type owl:NamedIndividual ,
                   ms:DomainIdentifier ;
          ms:conformsTo ms:DDC_classification .


###  http://w3id.org/meta-share/meta-share/DDC510
ms:DDC510 rdf:type owl:NamedIndividual ,
                   ms:DomainIdentifier ;
          ms:conformsTo ms:DDC_classification .


###  http://w3id.org/meta-share/meta-share/DDC520
ms:DDC520 rdf:type owl:NamedIndividual ,
                   ms:DomainIdentifier ;
          ms:conformsTo ms:DDC_classification .


###  http://w3id.org/meta-share/meta-share/DDC530
ms:DDC530 rdf:type owl:NamedIndividual ,
                   ms:DomainIdentifier ;
          ms:conformsTo ms:DDC_classification .


###  http://w3id.org/meta-share/meta-share/DDC540
ms:DDC540 rdf:type owl:NamedIndividual ,
                   ms:DomainIdentifier ;
          ms:conformsTo ms:DDC_classification .


###  http://w3id.org/meta-share/meta-share/DDC550
ms:DDC550 rdf:type owl:NamedIndividual ,
                   ms:DomainIdentifier ;
          ms:conformsTo ms:DDC_classification .


###  http://w3id.org/meta-share/meta-share/DDC560
ms:DDC560 rdf:type owl:NamedIndividual ,
                   ms:DomainIdentifier ;
          ms:conformsTo ms:DDC_classification .


###  http://w3id.org/meta-share/meta-share/DDC570
ms:DDC570 rdf:type owl:NamedIndividual ,
                   ms:DomainIdentifier .


###  http://w3id.org/meta-share/meta-share/DDC572
ms:DDC572 rdf:type owl:NamedIndividual ,
                   ms:DomainIdentifier .


###  http://w3id.org/meta-share/meta-share/DDC580
ms:DDC580 rdf:type owl:NamedIndividual ,
                   ms:DomainIdentifier ;
          ms:conformsTo ms:DDC_classification .


###  http://w3id.org/meta-share/meta-share/DDC590
ms:DDC590 rdf:type owl:NamedIndividual ,
                   ms:DomainIdentifier ;
          ms:conformsTo ms:DDC_classification .


###  http://w3id.org/meta-share/meta-share/DDC600
ms:DDC600 rdf:type owl:NamedIndividual ,
                   ms:DomainIdentifier ;
          ms:conformsTo ms:DDC_classification .


###  http://w3id.org/meta-share/meta-share/DDC610
ms:DDC610 rdf:type owl:NamedIndividual ,
                   ms:DomainIdentifier .


###  http://w3id.org/meta-share/meta-share/DDC620
ms:DDC620 rdf:type owl:NamedIndividual ,
                   ms:DomainIdentifier ;
          ms:conformsTo ms:DDC_classification .


###  http://w3id.org/meta-share/meta-share/DDC621
ms:DDC621 rdf:type owl:NamedIndividual ,
                   ms:DomainIdentifier ;
          ms:conformsTo ms:DDC_classification .


###  http://w3id.org/meta-share/meta-share/DDC630
ms:DDC630 rdf:type owl:NamedIndividual ,
                   ms:DomainIdentifier ;
          ms:conformsTo ms:DDC_classification ;
          rdfs:label "DDC630"@en .


###  http://w3id.org/meta-share/meta-share/DDC640
ms:DDC640 rdf:type owl:NamedIndividual ,
                   ms:DomainIdentifier ;
          ms:conformsTo ms:DDC_classification .


###  http://w3id.org/meta-share/meta-share/DDC650
ms:DDC650 rdf:type owl:NamedIndividual ,
                   ms:DomainIdentifier .


###  http://w3id.org/meta-share/meta-share/DDC659
ms:DDC659 rdf:type owl:NamedIndividual ,
                   ms:DomainIdentifier ;
          ms:conformsTo ms:DDC_classification ;
          rdfs:label "DDC659"@en .


###  http://w3id.org/meta-share/meta-share/DDC660
ms:DDC660 rdf:type owl:NamedIndividual ,
                   ms:DomainIdentifier ;
          ms:conformsTo ms:DDC_classification .


###  http://w3id.org/meta-share/meta-share/DDC670
ms:DDC670 rdf:type owl:NamedIndividual ,
                   ms:DomainIdentifier ;
          ms:conformsTo ms:DDC_classification .


###  http://w3id.org/meta-share/meta-share/DDC683
ms:DDC683 rdf:type owl:NamedIndividual ,
                   ms:DomainIdentifier ;
          ms:conformsTo ms:DDC_classification .


###  http://w3id.org/meta-share/meta-share/DDC690
ms:DDC690 rdf:type owl:NamedIndividual ,
                   ms:DomainIdentifier .


###  http://w3id.org/meta-share/meta-share/DDC700
ms:DDC700 rdf:type owl:NamedIndividual ,
                   ms:DomainIdentifier ;
          ms:conformsTo ms:DDC_classification .


###  http://w3id.org/meta-share/meta-share/DDC720
ms:DDC720 rdf:type owl:NamedIndividual ,
                   ms:DomainIdentifier ;
          ms:conformsTo ms:DDC_classification .


###  http://w3id.org/meta-share/meta-share/DDC730
ms:DDC730 rdf:type owl:NamedIndividual ,
                   ms:DomainIdentifier .


###  http://w3id.org/meta-share/meta-share/DDC740
ms:DDC740 rdf:type owl:NamedIndividual ,
                   ms:DomainIdentifier ;
          ms:conformsTo ms:DDC_classification .


###  http://w3id.org/meta-share/meta-share/DDC750
ms:DDC750 rdf:type owl:NamedIndividual ,
                   ms:DomainIdentifier ;
          ms:conformsTo ms:DDC_classification .


###  http://w3id.org/meta-share/meta-share/DDC770
ms:DDC770 rdf:type owl:NamedIndividual ,
                   ms:DomainIdentifier .


###  http://w3id.org/meta-share/meta-share/DDC780
ms:DDC780 rdf:type owl:NamedIndividual ,
                   ms:DomainIdentifier ;
          ms:conformsTo ms:DDC_classification .


###  http://w3id.org/meta-share/meta-share/DDC790
ms:DDC790 rdf:type owl:NamedIndividual ,
                   ms:DomainIdentifier ;
          ms:conformsTo ms:DDC_classification .


###  http://w3id.org/meta-share/meta-share/DDC800
ms:DDC800 rdf:type owl:NamedIndividual ,
                   ms:DomainIdentifier ;
          ms:conformsTo ms:DDC_classification .


###  http://w3id.org/meta-share/meta-share/DDC900
ms:DDC900 rdf:type owl:NamedIndividual ,
                   ms:DomainIdentifier ;
          ms:conformsTo ms:DDC_classification .


###  http://w3id.org/meta-share/meta-share/DDC910
ms:DDC910 rdf:type owl:NamedIndividual ,
                   ms:DomainIdentifier ;
          ms:conformsTo ms:DDC_classification .


###  http://w3id.org/meta-share/meta-share/DDC_classification
ms:DDC_classification rdf:type owl:NamedIndividual ,
                               ms:DomainClassificationScheme ;
                      ms:url "https://www.oclc.org/en/dewey/resources/summaries.html" ;
                      rdfs:label "DDC"@en ;
                      skos:altLabel "Dewey Decimal Classification"@en .


###  http://w3id.org/meta-share/meta-share/DK-5
ms:DK-5 rdf:type owl:NamedIndividual ,
                 ms:DomainClassificationScheme ;
        ms:url "http://metadata.dk/dk5-as-linked-data" ;
        rdfs:label "DK-5"@en ;
        skos:altLabel "Danish Decimal Classification 5th edition"@en .


###  http://w3id.org/meta-share/meta-share/DVB-C
ms:DVB-C rdf:type owl:NamedIndividual ,
                  ms:SourceChannelType ;
         rdfs:label "DVB-C"@en .


###  http://w3id.org/meta-share/meta-share/DVB-S
ms:DVB-S rdf:type owl:NamedIndividual ,
                  ms:SourceChannelType ;
         rdfs:label "DVB-S"@en .


###  http://w3id.org/meta-share/meta-share/DVB-T
ms:DVB-T rdf:type owl:NamedIndividual ,
                  ms:SourceChannelType ;
         rdfs:label "DVB-T"@en .


###  http://w3id.org/meta-share/meta-share/DVD-R
ms:DVD-R rdf:type owl:NamedIndividual ,
                  ms:DatasetDistributionForm ;
         rdfs:comment "Value for data distribution medium, used for language resources delivered on a DVD-R"@en ;
         rdfs:label "DVD-R"@en .


###  http://w3id.org/meta-share/meta-share/DataCite
ms:DataCite rdf:type owl:NamedIndividual ,
                     ms:RoleIdentifierScheme ;
            rdfs:label "DataCite"@en .


###  http://w3id.org/meta-share/meta-share/DeepLearningModel
ms:DeepLearningModel rdf:type owl:NamedIndividual ,
                              ms:ModelType ;
                     rdfs:label "Deep Learning model"@en ;
                     skos:altLabel "DL model"@en .


###  http://w3id.org/meta-share/meta-share/EAGLES
ms:EAGLES rdf:type owl:NamedIndividual ,
                   ms:StandardBestPractice ;
          ms:url "http://www.ilc.cnr.it/EAGLES/browse.html" ;
          rdfs:label "EAGLES"@en .


###  http://w3id.org/meta-share/meta-share/ELERightsStatementScheme
ms:ELERightsStatementScheme rdf:type owl:NamedIndividual ,
                                     ms:AccessRightsStatementScheme ;
                            rdfs:comment "ELE access rights vocabulary"@en ;
                            rdfs:label "ELE access rights statements scheme"@en .


###  http://w3id.org/meta-share/meta-share/ELG-SHARE
ms:ELG-SHARE rdf:type owl:NamedIndividual ,
                      ms:StandardBestPractice ;
             rdfs:label "ELG-SHARE"@en .


###  http://w3id.org/meta-share/meta-share/ELG_Domain001
ms:ELG_Domain001 rdf:type owl:NamedIndividual ,
                          ms:DomainIdentifier ;
                 ms:conformsTo ms:ELG_domainClassification .


###  http://w3id.org/meta-share/meta-share/ELG_Domain002
ms:ELG_Domain002 rdf:type owl:NamedIndividual ,
                          ms:DomainIdentifier ;
                 ms:conformsTo ms:ELG_domainClassification .


###  http://w3id.org/meta-share/meta-share/ELG_Domain003
ms:ELG_Domain003 rdf:type owl:NamedIndividual ,
                          ms:DomainIdentifier ;
                 ms:conformsTo ms:ELG_domainClassification .


###  http://w3id.org/meta-share/meta-share/ELG_Domain004
ms:ELG_Domain004 rdf:type owl:NamedIndividual ,
                          ms:DomainIdentifier ;
                 ms:conformsTo ms:ELG_domainClassification .


###  http://w3id.org/meta-share/meta-share/ELG_Domain005
ms:ELG_Domain005 rdf:type owl:NamedIndividual ,
                          ms:DomainIdentifier ;
                 ms:conformsTo ms:ELG_domainClassification .


###  http://w3id.org/meta-share/meta-share/ELG_Domain006
ms:ELG_Domain006 rdf:type owl:NamedIndividual ,
                          ms:DomainIdentifier ;
                 ms:conformsTo ms:ELG_domainClassification .


###  http://w3id.org/meta-share/meta-share/ELG_Domain007
ms:ELG_Domain007 rdf:type owl:NamedIndividual ,
                          ms:DomainIdentifier ;
                 ms:conformsTo ms:ELG_domainClassification .


###  http://w3id.org/meta-share/meta-share/ELG_Domain008
ms:ELG_Domain008 rdf:type owl:NamedIndividual ,
                          ms:DomainIdentifier ;
                 ms:conformsTo ms:ELG_domainClassification .


###  http://w3id.org/meta-share/meta-share/ELG_Domain009
ms:ELG_Domain009 rdf:type owl:NamedIndividual ,
                          ms:DomainIdentifier ;
                 ms:conformsTo ms:ELG_domainClassification .


###  http://w3id.org/meta-share/meta-share/ELG_Domain010
ms:ELG_Domain010 rdf:type owl:NamedIndividual ,
                          ms:DomainIdentifier ;
                 ms:conformsTo ms:ELG_domainClassification .


###  http://w3id.org/meta-share/meta-share/ELG_Domain011
ms:ELG_Domain011 rdf:type owl:NamedIndividual ,
                          ms:DomainIdentifier ;
                 ms:conformsTo ms:ELG_domainClassification .


###  http://w3id.org/meta-share/meta-share/ELG_Domain012
ms:ELG_Domain012 rdf:type owl:NamedIndividual ,
                          ms:DomainIdentifier ;
                 ms:conformsTo ms:ELG_domainClassification .


###  http://w3id.org/meta-share/meta-share/ELG_Domain013
ms:ELG_Domain013 rdf:type owl:NamedIndividual ,
                          ms:DomainIdentifier ;
                 ms:conformsTo ms:ELG_domainClassification .


###  http://w3id.org/meta-share/meta-share/ELG_Domain014
ms:ELG_Domain014 rdf:type owl:NamedIndividual ,
                          ms:DomainIdentifier ;
                 ms:conformsTo ms:ELG_domainClassification .


###  http://w3id.org/meta-share/meta-share/ELG_Domain015
ms:ELG_Domain015 rdf:type owl:NamedIndividual ,
                          ms:DomainIdentifier ;
                 ms:conformsTo ms:ELG_domainClassification .


###  http://w3id.org/meta-share/meta-share/ELG_Domain016
ms:ELG_Domain016 rdf:type owl:NamedIndividual ,
                          ms:DomainIdentifier ;
                 ms:conformsTo ms:ELG_domainClassification .


###  http://w3id.org/meta-share/meta-share/ELG_Domain017
ms:ELG_Domain017 rdf:type owl:NamedIndividual ,
                          ms:DomainIdentifier ;
                 ms:conformsTo ms:ELG_domainClassification .


###  http://w3id.org/meta-share/meta-share/ELG_Domain018
ms:ELG_Domain018 rdf:type owl:NamedIndividual ,
                          ms:DomainIdentifier ;
                 ms:conformsTo ms:ELG_domainClassification .


###  http://w3id.org/meta-share/meta-share/ELG_domainClassification
ms:ELG_domainClassification rdf:type owl:NamedIndividual ,
                                     ms:DomainClassificationScheme ;
                            rdfs:label "ELG domain classification"@en .


###  http://w3id.org/meta-share/meta-share/ELRA
ms:ELRA rdf:type owl:NamedIndividual ,
                 ms:MembershipInstitution ;
        rdfs:comment "European Language Resources Association (www.elra.eu)"@en ;
        rdfs:label "ELRA"@en .


###  http://w3id.org/meta-share/meta-share/EMA
ms:EMA rdf:type owl:NamedIndividual ,
                ms:SourceChannel ;
       rdfs:label "EMA"@en .


###  http://w3id.org/meta-share/meta-share/EML
ms:EML rdf:type owl:NamedIndividual ,
                ms:StandardBestPractice ;
       ms:url "https://www.w3.org/TR/2009/WD-emotionml-20091029/" ;
       rdfs:label "EmotionML"@en ;
       skos:altLabel "EML"@en ,
                     "Emotion Markup Language"@en .


###  http://w3id.org/meta-share/meta-share/EMMA
ms:EMMA rdf:type owl:NamedIndividual ,
                 ms:StandardBestPractice ;
        ms:url "https://www.w3.org/TR/emma/" ;
        rdfs:label "EMMA"@en ;
        skos:altLabel "Extensible MultiModal Annotation markup language"@en .


###  http://w3id.org/meta-share/meta-share/ESPnet
ms:ESPnet rdf:type owl:NamedIndividual ,
                   ms:Toolkit ;
          rdfs:comment "A speech processing toolkit, mainly focusing on end-to-end speech recognition and end-to-end text-to-speech using Chainer and PyTorch as a main deep learning engine"@en .


###  http://w3id.org/meta-share/meta-share/EUC-JP
ms:EUC-JP rdf:type owl:NamedIndividual ,
                   ms:CharacterEncoding ;
          rdfs:label "EUC-JP"@en .


###  http://w3id.org/meta-share/meta-share/EUC-KR
ms:EUC-KR rdf:type owl:NamedIndividual ,
                   ms:CharacterEncoding ;
          rdfs:label "EUC-KR"@en .


###  http://w3id.org/meta-share/meta-share/EUROVOC
ms:EUROVOC rdf:type owl:NamedIndividual ,
                    ms:DomainClassificationScheme ;
           ms:url "https://eur-lex.europa.eu/browse/eurovoc.html" ;
           rdfs:label "EUROVOC"@en .


###  http://w3id.org/meta-share/meta-share/FiveG
ms:FiveG rdf:type owl:NamedIndividual ,
                  ms:SourceChannelType ;
         rdfs:label "5G"@en .


###  http://w3id.org/meta-share/meta-share/Flair
ms:Flair rdf:type owl:NamedIndividual ,
                  ms:NLPFramework ;
         rdfs:label "Flair"@en .


###  http://w3id.org/meta-share/meta-share/FourG
ms:FourG rdf:type owl:NamedIndividual ,
                  ms:SourceChannelType ;
         rdfs:label "4G"@en .


###  http://w3id.org/meta-share/meta-share/GATE
ms:GATE rdf:type owl:NamedIndividual ,
                 ms:Framework ;
        rdfs:label "GATE"@en .


###  http://w3id.org/meta-share/meta-share/GB18030
ms:GB18030 rdf:type owl:NamedIndividual ,
                    ms:CharacterEncoding ;
           rdfs:label "GB18030"@en .


###  http://w3id.org/meta-share/meta-share/GBK
ms:GBK rdf:type owl:NamedIndividual ,
                ms:CharacterEncoding ;
       rdfs:label "GBK"@en .


###  http://w3id.org/meta-share/meta-share/GMX
ms:GMX rdf:type owl:NamedIndividual ,
                ms:StandardBestPractice ;
       ms:url "https://xtm.cloud/manuals/gmx-v/GMX-V-2.0.html" ;
       rdfs:label "GMX"@en ;
       skos:altLabel "Global information management Metrics eXchange"@en .


###  http://w3id.org/meta-share/meta-share/GSM
ms:GSM rdf:type owl:NamedIndividual ,
                ms:SourceChannelType ;
       rdfs:label "GSM"@en .


###  http://w3id.org/meta-share/meta-share/Galaxy
ms:Galaxy rdf:type owl:NamedIndividual ,
                   ms:Framework ;
          rdfs:label "Galaxy"@en .


###  http://w3id.org/meta-share/meta-share/GrAF
ms:GrAF rdf:type owl:NamedIndividual ,
                 ms:StandardBestPractice ;
        ms:url "http://www.xces.org/ns/GrAF/1.0/" ;
        rdfs:label "GrAF"@en ;
        skos:altLabel "Graph Annotation Framework"@en .


###  http://w3id.org/meta-share/meta-share/H2O
ms:H2O rdf:type owl:NamedIndividual ,
                ms:MLFramework ;
       rdfs:label "H2O"@en .


###  http://w3id.org/meta-share/meta-share/HD.1080
ms:HD.1080 rdf:type owl:NamedIndividual ,
                    ms:ResolutionStandard ;
           rdfs:label "HD.1080"@en .


###  http://w3id.org/meta-share/meta-share/HD.720
ms:HD.720 rdf:type owl:NamedIndividual ,
                   ms:ResolutionStandard ;
          rdfs:label "HD.720"@en .


###  http://w3id.org/meta-share/meta-share/HamNoSys
ms:HamNoSys rdf:type owl:NamedIndividual ,
                     ms:StandardBestPractice ;
            ms:url "https://www.sign-lang.uni-hamburg.de/dgs-korpus/index.php/hamnosys-97.html" ;
            rdfs:label "HamNoSys"@en ;
            skos:altLabel "Hamburg Sign Language Notation System"@en .


###  http://w3id.org/meta-share/meta-share/ISCII91
ms:ISCII91 rdf:type owl:NamedIndividual ,
                    ms:CharacterEncoding ;
           rdfs:label "ISCII91"@en .


###  http://w3id.org/meta-share/meta-share/ISDN
ms:ISDN rdf:type owl:NamedIndividual ,
                 ms:SourceChannelType ;
        rdfs:label "ISDN"@en .


###  http://w3id.org/meta-share/meta-share/ISO-2022-JP
ms:ISO-2022-JP rdf:type owl:NamedIndividual ,
                        ms:CharacterEncoding ;
               rdfs:label "ISO-2022-JP"@en .


###  http://w3id.org/meta-share/meta-share/ISO-2022-KR
ms:ISO-2022-KR rdf:type owl:NamedIndividual ,
                        ms:CharacterEncoding ;
               rdfs:label "ISO-2022-KR"@en .


###  http://w3id.org/meta-share/meta-share/ISO-8859-1
ms:ISO-8859-1 rdf:type owl:NamedIndividual ,
                       ms:CharacterEncoding ;
              rdfs:label "ISO-8859-1"@en .


###  http://w3id.org/meta-share/meta-share/ISO-8859-15
ms:ISO-8859-15 rdf:type owl:NamedIndividual ,
                        ms:CharacterEncoding ;
               rdfs:label "ISO-8859-15"@en .


###  http://w3id.org/meta-share/meta-share/ISO-8859-2
ms:ISO-8859-2 rdf:type owl:NamedIndividual ,
                       ms:CharacterEncoding ;
              rdfs:label "ISO-8859-2"@en .


###  http://w3id.org/meta-share/meta-share/ISO-8859-3
ms:ISO-8859-3 rdf:type owl:NamedIndividual ,
                       ms:CharacterEncoding ;
              rdfs:label "ISO-8859-3"@en .


###  http://w3id.org/meta-share/meta-share/ISO-8859-4
ms:ISO-8859-4 rdf:type owl:NamedIndividual ,
                       ms:CharacterEncoding ;
              rdfs:label "ISO-8859-4"@en .


###  http://w3id.org/meta-share/meta-share/ISO-8859-5
ms:ISO-8859-5 rdf:type owl:NamedIndividual ,
                       ms:CharacterEncoding ;
              rdfs:label "ISO-8859-5"@en .


###  http://w3id.org/meta-share/meta-share/ISO-8859-6
ms:ISO-8859-6 rdf:type owl:NamedIndividual ,
                       ms:CharacterEncoding ;
              rdfs:label "ISO-8859-6"@en .


###  http://w3id.org/meta-share/meta-share/ISO-8859-7
ms:ISO-8859-7 rdf:type owl:NamedIndividual ,
                       ms:CharacterEncoding ;
              rdfs:label "ISO-8859-7"@en .


###  http://w3id.org/meta-share/meta-share/ISO-8859-8
ms:ISO-8859-8 rdf:type owl:NamedIndividual ,
                       ms:CharacterEncoding ;
              rdfs:label "ISO-8859-8"@en .


###  http://w3id.org/meta-share/meta-share/ISO-8859-9
ms:ISO-8859-9 rdf:type owl:NamedIndividual ,
                       ms:CharacterEncoding ;
              rdfs:label "ISO-8859-9"@en .


###  http://w3id.org/meta-share/meta-share/ISO-8860-13
ms:ISO-8860-13 rdf:type owl:NamedIndividual ,
                        ms:CharacterEncoding ;
               rdfs:label "ISO-8860-13"@en .


###  http://w3id.org/meta-share/meta-share/ISO12620
ms:ISO12620 rdf:type owl:NamedIndividual ,
                     ms:StandardBestPractice ;
            ms:url "http://www.datcatinfo.net/#/" ,
                   "http://www.iso.org/sites/dcr-redirect/dcr.html" ;
            rdfs:label "ISO12620"@en ;
            skos:altLabel "DCR"@en ,
                          "Data Category Repository"@en .


###  http://w3id.org/meta-share/meta-share/ISO16642
ms:ISO16642 rdf:type owl:NamedIndividual ,
                     ms:StandardBestPractice ;
            ms:url "http://xml.coverpages.org/ISO16642-200207.pdf" ;
            rdfs:label "ISO16642"@en ;
            skos:altLabel "TMF"@en ,
                          "Terminological Markup Framework"@en .


###  http://w3id.org/meta-share/meta-share/ISO1987
ms:ISO1987 rdf:type owl:NamedIndividual ,
                    ms:StandardBestPractice ;
           rdfs:comment "Quality systems -- Model for quality assurance in design/development, production, installation and servicing"@en ;
           rdfs:label "ISO 9001:1987"@en .


###  http://w3id.org/meta-share/meta-share/ISO2022_CN_CNS
ms:ISO2022_CN_CNS rdf:type owl:NamedIndividual ,
                           ms:CharacterEncoding ;
                  rdfs:label "ISO2022_CN_CNS"@en .


###  http://w3id.org/meta-share/meta-share/ISO2022_CN_GB
ms:ISO2022_CN_GB rdf:type owl:NamedIndividual ,
                          ms:CharacterEncoding ;
                 rdfs:label "ISO2022_CN_GB"@en .


###  http://w3id.org/meta-share/meta-share/ISO26162
ms:ISO26162 rdf:type owl:NamedIndividual ,
                     ms:StandardBestPractice ;
            ms:url "https://www.iso.org/standard/43427.html" ;
            rdfs:label "ISO 26162"@en ;
            skos:altLabel "Systems to manage terminology, knowledge and content"@en .


###  http://w3id.org/meta-share/meta-share/ISO30042
ms:ISO30042 rdf:type owl:NamedIndividual ,
                     ms:StandardBestPractice ;
            ms:url "https://www.iso.org/standard/45797.html" ;
            rdfs:label "ISO 30042"@en ;
            skos:altLabel "TBX"@en ,
                          "TermBase eXchange"@en .


###  http://w3id.org/meta-share/meta-share/ISO704
ms:ISO704 rdf:type owl:NamedIndividual ,
                   ms:StandardBestPractice ;
          ms:url "https://www.iso.org/standard/38109.html" ;
          rdfs:label "ISO704"@en ;
          skos:altLabel "Terminology work"@en .


###  http://w3id.org/meta-share/meta-share/InkML
ms:InkML rdf:type owl:NamedIndividual ,
                  ms:StandardBestPractice ;
         ms:url "https://www.w3.org/TR/InkML/" ;
         rdfs:label "Ink ML"@en ;
         skos:altLabel "Ink Markup Language"@en .


###  http://w3id.org/meta-share/meta-share/JAX
ms:JAX rdf:type owl:NamedIndividual ,
                ms:MLFramework ;
       rdfs:label "JAX"@en .


###  http://w3id.org/meta-share/meta-share/JISAutoDetect
ms:JISAutoDetect rdf:type owl:NamedIndividual ,
                          ms:CharacterEncoding ;
                 rdfs:label "JISAutoDetect"@en .


###  http://w3id.org/meta-share/meta-share/Joblib
ms:Joblib rdf:type owl:NamedIndividual ,
                   ms:DevelopmentFramework ;
          rdfs:comment "A python framework for running pipelines"@en ;
          rdfs:label "Joblib"@en .


###  http://w3id.org/meta-share/meta-share/KOI8-R
ms:KOI8-R rdf:type owl:NamedIndividual ,
                   ms:CharacterEncoding ;
          rdfs:label "KOI8-R"@en .


###  http://w3id.org/meta-share/meta-share/Keras
ms:Keras rdf:type owl:NamedIndividual ,
                  ms:MLFramework ;
         rdfs:label "Keras"@en .


###  http://w3id.org/meta-share/meta-share/LAF
ms:LAF rdf:type owl:NamedIndividual ,
                ms:StandardBestPractice ;
       ms:url "https://www.iso.org/standard/37326.html" ;
       rdfs:label "LAF"@en ;
       skos:altLabel "ISO 24612"@en ,
                     "Linguistic Annotation Framework"@en .


###  http://w3id.org/meta-share/meta-share/LDC
ms:LDC rdf:type owl:NamedIndividual ,
                ms:MembershipInstitution ;
       rdfs:comment "Linguistic Data Consortium"@en ;
       rdfs:label "LDC"@en .


###  http://w3id.org/meta-share/meta-share/LMF
ms:LMF rdf:type owl:NamedIndividual ,
                ms:StandardBestPractice ;
       ms:url "http://www.lexicalmarkupframework.org/" ;
       rdfs:label "LMF"@en ;
       skos:altLabel "Lexical Markup Framework"@en .


###  http://w3id.org/meta-share/meta-share/LTIntegrator
ms:LTIntegrator rdf:type owl:NamedIndividual ,
                         ms:OrganizationRole ;
                rdfs:label "LT integrator"@en ;
                skos:altLabel "Language Technology integrator"@en .


###  http://w3id.org/meta-share/meta-share/LTSupplier
ms:LTSupplier rdf:type owl:NamedIndividual ,
                       ms:OrganizationRole ;
              rdfs:label "LT supplier"@en ;
              skos:altLabel "Language Technology supplier"@en .


###  http://w3id.org/meta-share/meta-share/LTUser
ms:LTUser rdf:type owl:NamedIndividual ,
                   ms:OrganizationRole ;
          rdfs:label "LT user"@en ;
          skos:altLabel "Language Technology user"@en .


###  http://w3id.org/meta-share/meta-share/LemmaType
ms:LemmaType rdf:type owl:NamedIndividual ,
                      skos:Concept ;
             rdfs:comment "A type of content included in a language resource pertaining to the lemma"@en ;
             rdfs:label "Lemma type"@en ;
             skos:broader ms:ContentType ;
             skos:inScheme ms:ContentTypeScheme .


###  http://w3id.org/meta-share/meta-share/LemonOntolex
ms:LemonOntolex rdf:type owl:NamedIndividual ,
                         ms:StandardBestPractice ;
                rdfs:label "Lemon-Ontolex"@en .


###  http://w3id.org/meta-share/meta-share/MAD
ms:MAD rdf:type owl:NamedIndividual ,
                ms:Metric ;
       rdfs:label "MAD"@en ;
       skos:altLabel "Mean Annotations per Document"@en .


###  http://w3id.org/meta-share/meta-share/MAF
ms:MAF rdf:type owl:NamedIndividual ,
                ms:StandardBestPractice ;
       ms:url "https://www.iso.org/standard/51934.html" ;
       rdfs:label "MAF"@en ;
       skos:altLabel "ISO 24611"@en ,
                     "Morpho-syntactic Annotation Framework"@en .


###  http://w3id.org/meta-share/meta-share/MARC
ms:MARC rdf:type owl:NamedIndividual ,
                 ms:RoleIdentifierScheme ;
        rdfs:label "MARC"@en .


###  http://w3id.org/meta-share/meta-share/MDTV
ms:MDTV rdf:type owl:NamedIndividual ,
                 ms:Metric ;
        rdfs:label "MDTV"@en ;
        skos:altLabel "Mean Time per Document Volume"@en .


###  http://w3id.org/meta-share/meta-share/META-SHARE
ms:META-SHARE rdf:type owl:NamedIndividual ,
                       ms:MembershipInstitution ;
              rdfs:label "META-SHARE"@en .


###  http://w3id.org/meta-share/meta-share/MLIF
ms:MLIF rdf:type owl:NamedIndividual ,
                 ms:StandardBestPractice ;
        ms:url "https://www.iso.org/standard/37330.html" ;
        rdfs:label "MLIF"@en ;
        skos:altLabel "ISO 24616"@en ,
                      "Multilingual Information Framework"@en .


###  http://w3id.org/meta-share/meta-share/MMI
ms:MMI rdf:type owl:NamedIndividual ,
                ms:StandardBestPractice ;
       ms:url "https://www.w3.org/TR/mmi-framework/" ;
       rdfs:label "MMI"@en ;
       skos:altLabel "Multi-Modal Interaction framework"@en .


###  http://w3id.org/meta-share/meta-share/MS874
ms:MS874 rdf:type owl:NamedIndividual ,
                  ms:CharacterEncoding ;
         rdfs:label "MS874"@en .


###  http://w3id.org/meta-share/meta-share/MS_AG001
ms:MS_AG001 rdf:type owl:NamedIndividual ,
                     ms:AudioGenreIdentifier ;
            ms:conformsTo ms:MS_audioGenreClassification .


###  http://w3id.org/meta-share/meta-share/MS_AG002
ms:MS_AG002 rdf:type owl:NamedIndividual ,
                     ms:AudioGenreIdentifier ;
            ms:conformsTo ms:MS_audioGenreClassification .


###  http://w3id.org/meta-share/meta-share/MS_AG003
ms:MS_AG003 rdf:type owl:NamedIndividual ,
                     ms:AudioGenreIdentifier ;
            ms:conformsTo ms:MS_audioGenreClassification .


###  http://w3id.org/meta-share/meta-share/MS_AG004
ms:MS_AG004 rdf:type owl:NamedIndividual ,
                     ms:AudioGenreIdentifier ;
            ms:conformsTo ms:MS_audioGenreClassification .


###  http://w3id.org/meta-share/meta-share/MS_AG005
ms:MS_AG005 rdf:type owl:NamedIndividual ,
                     ms:AudioGenreIdentifier ;
            ms:conformsTo ms:MS_audioGenreClassification .


###  http://w3id.org/meta-share/meta-share/MS_AG006
ms:MS_AG006 rdf:type owl:NamedIndividual ,
                     ms:AudioGenreIdentifier ;
            ms:conformsTo ms:MS_audioGenreClassification .


###  http://w3id.org/meta-share/meta-share/MS_SG001
ms:MS_SG001 rdf:type owl:NamedIndividual ,
                     ms:SpeechGenreIdentifier ;
            ms:conformsTo ms:MS_SpeechGenreClassification .


###  http://w3id.org/meta-share/meta-share/MS_SG002
ms:MS_SG002 rdf:type owl:NamedIndividual ,
                     ms:SpeechGenreIdentifier ;
            ms:conformsTo ms:MS_SpeechGenreClassification .


###  http://w3id.org/meta-share/meta-share/MS_SG003
ms:MS_SG003 rdf:type owl:NamedIndividual ,
                     ms:SpeechGenreIdentifier ;
            ms:conformsTo ms:MS_SpeechGenreClassification .


###  http://w3id.org/meta-share/meta-share/MS_SG004
ms:MS_SG004 rdf:type owl:NamedIndividual ,
                     ms:SpeechGenreIdentifier ;
            ms:conformsTo ms:MS_SpeechGenreClassification .


###  http://w3id.org/meta-share/meta-share/MS_SG005
ms:MS_SG005 rdf:type owl:NamedIndividual ,
                     ms:SpeechGenreIdentifier ;
            ms:conformsTo ms:MS_SpeechGenreClassification .


###  http://w3id.org/meta-share/meta-share/MS_SG006
ms:MS_SG006 rdf:type owl:NamedIndividual ,
                     ms:SpeechGenreIdentifier ;
            ms:conformsTo ms:MS_SpeechGenreClassification .


###  http://w3id.org/meta-share/meta-share/MS_SG007
ms:MS_SG007 rdf:type owl:NamedIndividual ,
                     ms:SpeechGenreIdentifier ;
            ms:conformsTo ms:MS_SpeechGenreClassification .


###  http://w3id.org/meta-share/meta-share/MS_SG008
ms:MS_SG008 rdf:type owl:NamedIndividual ,
                     ms:SpeechGenreIdentifier ;
            ms:conformsTo ms:MS_SpeechGenreClassification .


###  http://w3id.org/meta-share/meta-share/MS_SG009
ms:MS_SG009 rdf:type owl:NamedIndividual ,
                     ms:SpeechGenreIdentifier ;
            ms:conformsTo ms:MS_SpeechGenreClassification .


###  http://w3id.org/meta-share/meta-share/MS_SG010
ms:MS_SG010 rdf:type owl:NamedIndividual ,
                     ms:SpeechGenreIdentifier .


###  http://w3id.org/meta-share/meta-share/MS_SG011
ms:MS_SG011 rdf:type owl:NamedIndividual ,
                     ms:SpeechGenreIdentifier ;
            ms:conformsTo ms:MS_SpeechGenreClassification .


###  http://w3id.org/meta-share/meta-share/MS_SG012
ms:MS_SG012 rdf:type owl:NamedIndividual ,
                     ms:SpeechGenreIdentifier ;
            ms:conformsTo ms:MS_SpeechGenreClassification .


###  http://w3id.org/meta-share/meta-share/MS_SG013
ms:MS_SG013 rdf:type owl:NamedIndividual ,
                     ms:SpeechGenreIdentifier .


###  http://w3id.org/meta-share/meta-share/MS_SpeechGenreClassification
ms:MS_SpeechGenreClassification rdf:type owl:NamedIndividual ,
                                         ms:SpeechGenreClassificationScheme ;
                                rdfs:label "META-SHARE speech genre classification scheme"@en .


###  http://w3id.org/meta-share/meta-share/MS_audioGenreClassification
ms:MS_audioGenreClassification rdf:type owl:NamedIndividual ,
                                        ms:AudioGenreClassificationScheme ;
                               rdfs:label "META-SHARE audio genre classification scheme"@en .


###  http://w3id.org/meta-share/meta-share/MTBF
ms:MTBF rdf:type owl:NamedIndividual ,
                 ms:Metric ;
        rdfs:label "MTBF"@en ;
        skos:altLabel "Mean Time Between Failures"@en .


###  http://w3id.org/meta-share/meta-share/MTSA
ms:MTSA rdf:type owl:NamedIndividual ,
                 ms:Metric ;
        rdfs:label "MTSA"@en ;
        skos:altLabel "Mean Time Seek Annotations"@en .


###  http://w3id.org/meta-share/meta-share/MTTR
ms:MTTR rdf:type owl:NamedIndividual ,
                 ms:Metric ;
        rdfs:label "MTTR"@en ;
        skos:altLabel "Mean Time To Repair"@en .


###  http://w3id.org/meta-share/meta-share/MULTEXT
ms:MULTEXT rdf:type owl:NamedIndividual ,
                    ms:StandardBestPractice ;
           ms:url "https://tei-c.org/activities/projects/multilingual-text-tools-and-corpora-multext/" ;
           rdfs:label "MULTEXT"@en .


###  http://w3id.org/meta-share/meta-share/MUMIN
ms:MUMIN rdf:type owl:NamedIndividual ,
                  ms:StandardBestPractice ;
         ms:url "https://cst.dk/mumin/" ;
         rdfs:label "MUMIN"@en ;
         skos:altLabel "MUltiModal INterfaces"@en .


###  http://w3id.org/meta-share/meta-share/MXNet
ms:MXNet rdf:type owl:NamedIndividual ,
                  ms:MLFramework ;
         rdfs:label "MXNet"@en .


###  http://w3id.org/meta-share/meta-share/MacArabic
ms:MacArabic rdf:type owl:NamedIndividual ,
                      ms:CharacterEncoding ;
             rdfs:label "MacArabic"@en .


###  http://w3id.org/meta-share/meta-share/MacCentralEurope
ms:MacCentralEurope rdf:type owl:NamedIndividual ,
                             ms:CharacterEncoding ;
                    rdfs:label "MacCentralEurope"@en .


###  http://w3id.org/meta-share/meta-share/MacCroatian
ms:MacCroatian rdf:type owl:NamedIndividual ,
                        ms:CharacterEncoding ;
               rdfs:label "MacCroatian"@en .


###  http://w3id.org/meta-share/meta-share/MacCyrillic
ms:MacCyrillic rdf:type owl:NamedIndividual ,
                        ms:CharacterEncoding ;
               rdfs:label "MacCyrillic"@en .


###  http://w3id.org/meta-share/meta-share/MacDingbat
ms:MacDingbat rdf:type owl:NamedIndividual ,
                       ms:CharacterEncoding ;
              rdfs:label "MacDingbat"@en .


###  http://w3id.org/meta-share/meta-share/MacGreek
ms:MacGreek rdf:type owl:NamedIndividual ,
                     ms:CharacterEncoding ;
            rdfs:label "MacGreek"@en .


###  http://w3id.org/meta-share/meta-share/MacHebrew
ms:MacHebrew rdf:type owl:NamedIndividual ,
                      ms:CharacterEncoding ;
             rdfs:label "MacHebrew"@en .


###  http://w3id.org/meta-share/meta-share/MacIceland
ms:MacIceland rdf:type owl:NamedIndividual ,
                       ms:CharacterEncoding ;
              rdfs:label "MacIceland"@en .


###  http://w3id.org/meta-share/meta-share/MacRoman
ms:MacRoman rdf:type owl:NamedIndividual ,
                     ms:CharacterEncoding ;
            rdfs:label "MacRoman"@en .


###  http://w3id.org/meta-share/meta-share/MacRomania
ms:MacRomania rdf:type owl:NamedIndividual ,
                       ms:CharacterEncoding ;
              rdfs:label "MacRomania"@en .


###  http://w3id.org/meta-share/meta-share/MacSymbol
ms:MacSymbol rdf:type owl:NamedIndividual ,
                      ms:CharacterEncoding ;
             rdfs:label "MacSymbol"@en .


###  http://w3id.org/meta-share/meta-share/MacThai
ms:MacThai rdf:type owl:NamedIndividual ,
                    ms:CharacterEncoding ;
           rdfs:label "MacThai"@en .


###  http://w3id.org/meta-share/meta-share/MacTurkish
ms:MacTurkish rdf:type owl:NamedIndividual ,
                       ms:CharacterEncoding ;
              rdfs:label "MacTurkish"@en .


###  http://w3id.org/meta-share/meta-share/MacUkraine
ms:MacUkraine rdf:type owl:NamedIndividual ,
                       ms:CharacterEncoding ;
              rdfs:label "MacUkraine"@en .


###  http://w3id.org/meta-share/meta-share/MeSH_classification
ms:MeSH_classification rdf:type owl:NamedIndividual ,
                                ms:SubjectClassificationScheme ;
                       ms:url "http://www.openclinical.org/medTermMesh.html" ;
                       rdfs:label "MeSH"@en ;
                       skos:altLabel "Medical Subject Headings"@en .


###  http://w3id.org/meta-share/meta-share/MicrosoftCognitiveToolkit
ms:MicrosoftCognitiveToolkit rdf:type owl:NamedIndividual ,
                                      ms:MLFramework ;
                             rdfs:label "Microsoft Cognitive Toolkit"@en .


###  http://w3id.org/meta-share/meta-share/MorphologicalType
ms:MorphologicalType rdf:type owl:NamedIndividual ,
                              skos:Concept ;
                     rdfs:comment "A type of content included in a language resource pertaining to the morphological level"@en ;
                     rdfs:label "Morphological type"@en ;
                     skos:inScheme ms:ContentTypeScheme .


###  http://w3id.org/meta-share/meta-share/NLM_classification
ms:NLM_classification rdf:type owl:NamedIndividual ,
                               ms:SubjectClassificationScheme ;
                      rdfs:comment "Classification scheme of the National Library of Medicine (https://www.nlm.nih.gov/class/)"@en ;
                      rdfs:label "NLM classification scheme"@en .


###  http://w3id.org/meta-share/meta-share/OAXAL
ms:OAXAL rdf:type owl:NamedIndividual ,
                  ms:StandardBestPractice ;
         ms:url "https://www.oasis-open.org/committees/tc_home.php?wg_abbrev=oaxal" ;
         rdfs:label "OAXAL"@en ;
         skos:altLabel "OASIS Open Architecture for XML Authoring and Localization Reference Model"@en .


###  http://w3id.org/meta-share/meta-share/OMTDShareRightsStatementScheme
ms:OMTDShareRightsStatementScheme rdf:type owl:NamedIndividual ,
                                           ms:AccessRightsStatementScheme ;
                                  rdfs:label "OMTD-SHARE rights statement scheme"@en .


###  http://w3id.org/meta-share/meta-share/OpenAIRE
ms:OpenAIRE rdf:type owl:NamedIndividual ,
                     ms:MetadataRecordIdentifierScheme ,
                     ms:ProjectIdentifierScheme ;
            rdfs:label "OpenAIRE"@en .


###  http://w3id.org/meta-share/meta-share/PAROLE_G001
ms:PAROLE_G001 rdf:type owl:NamedIndividual ,
                        ms:TextGenreIdentifier ;
               ms:conformsTo ms:PAROLE_genreClassification .


###  http://w3id.org/meta-share/meta-share/PAROLE_G002
ms:PAROLE_G002 rdf:type owl:NamedIndividual ,
                        ms:TextGenreIdentifier ;
               ms:conformsTo ms:PAROLE_genreClassification .


###  http://w3id.org/meta-share/meta-share/PAROLE_G003
ms:PAROLE_G003 rdf:type owl:NamedIndividual ,
                        ms:TextGenreIdentifier ;
               ms:conformsTo ms:PAROLE_genreClassification .


###  http://w3id.org/meta-share/meta-share/PAROLE_G004
ms:PAROLE_G004 rdf:type owl:NamedIndividual ,
                        ms:TextGenreIdentifier ;
               ms:conformsTo ms:PAROLE_genreClassification .


###  http://w3id.org/meta-share/meta-share/PAROLE_G005
ms:PAROLE_G005 rdf:type owl:NamedIndividual ,
                        ms:TextGenreIdentifier ;
               ms:conformsTo ms:PAROLE_genreClassification .


###  http://w3id.org/meta-share/meta-share/PAROLE_G006
ms:PAROLE_G006 rdf:type owl:NamedIndividual ,
                        ms:TextGenreIdentifier ;
               ms:conformsTo ms:PAROLE_genreClassification .


###  http://w3id.org/meta-share/meta-share/PAROLE_G007
ms:PAROLE_G007 rdf:type owl:NamedIndividual ,
                        ms:TextGenreIdentifier ;
               ms:conformsTo ms:PAROLE_genreClassification .


###  http://w3id.org/meta-share/meta-share/PAROLE_G008
ms:PAROLE_G008 rdf:type owl:NamedIndividual ,
                        ms:TextGenreIdentifier ;
               ms:conformsTo ms:PAROLE_genreClassification .


###  http://w3id.org/meta-share/meta-share/PAROLE_G009
ms:PAROLE_G009 rdf:type owl:NamedIndividual ,
                        ms:TextGenreIdentifier ;
               ms:conformsTo ms:PAROLE_genreClassification .


###  http://w3id.org/meta-share/meta-share/PAROLE_genreClassification
ms:PAROLE_genreClassification rdf:type owl:NamedIndividual ,
                                       ms:TextGenreClassificationScheme ;
                              rdfs:label "PAROLE_genre classification scheme"@en .


###  http://w3id.org/meta-share/meta-share/PAROLE_topicClassification
ms:PAROLE_topicClassification rdf:type owl:NamedIndividual ,
                                       ms:SubjectClassificationScheme ;
                              rdfs:label "PAROLE_topic classification scheme"@en .


###  http://w3id.org/meta-share/meta-share/PyTorch
ms:PyTorch rdf:type owl:NamedIndividual ,
                    ms:MLFramework ;
           rdfs:label "PyTorch"@en .


###  http://w3id.org/meta-share/meta-share/Pyannote
ms:Pyannote rdf:type owl:NamedIndividual ,
                     ms:Toolkit ;
            rdfs:comment "Framework for multimedia processing"@en ;
            rdfs:label "Pyannote"@en .


###  http://w3id.org/meta-share/meta-share/REST
ms:REST rdf:type owl:NamedIndividual ,
                 ms:WebServiceType ;
        rdfs:label "REST"@en .


###  http://w3id.org/meta-share/meta-share/RGB
ms:RGB rdf:type owl:NamedIndividual ,
                ms:ColourSpace ;
       rdfs:label "RGB"@en .


###  http://w3id.org/meta-share/meta-share/RightsStatementOrgScheme
ms:RightsStatementOrgScheme rdf:type owl:NamedIndividual ,
                                     ms:AccessRightsStatementScheme ;
                            rdfs:label "Rights_Statements_Org scheme"@en .


###  http://w3id.org/meta-share/meta-share/Rust
ms:Rust rdf:type owl:NamedIndividual ,
                 ms:DevelopmentFramework ;
        rdfs:comment "Programming language designed for performance and safety, especially safe concurrency"@en ;
        rdfs:label "Rust"@en .


###  http://w3id.org/meta-share/meta-share/SNR
ms:SNR rdf:type owl:NamedIndividual ,
                ms:AudioQualityMeasureIncluded ;
       rdfs:label "SNR"@en .


###  http://w3id.org/meta-share/meta-share/SOAP
ms:SOAP rdf:type owl:NamedIndividual ,
                 ms:WebServiceType ;
        rdfs:label "SOAP"@en .


###  http://w3id.org/meta-share/meta-share/SPDX
ms:SPDX rdf:type owl:NamedIndividual ,
                 ms:LicenceIdentifierScheme ;
        ms:url "https://spdx.org/licenses/" ;
        rdfs:comment "Value for LicenceIdentifierScheme referring to the codes (identifiers) for licences used by SPDX (https://spdx.org/licenses/))"@en ;
        rdfs:label "SPDX"@en .


###  http://w3id.org/meta-share/meta-share/SRX
ms:SRX rdf:type owl:NamedIndividual ,
                ms:StandardBestPractice ;
       ms:url "https://www.gala-global.org/srx-20-april-7-2008" ;
       rdfs:label "SRX"@en ;
       skos:altLabel "Segmentation Rules eXchange"@en .


###  http://w3id.org/meta-share/meta-share/Scikit-Learn
ms:Scikit-Learn rdf:type owl:NamedIndividual ,
                         ms:MLFramework ;
                rdfs:label "Scikit-Learn"@en .


###  http://w3id.org/meta-share/meta-share/SemAF
ms:SemAF rdf:type owl:NamedIndividual ,
                  ms:StandardBestPractice ;
         rdfs:label "Semantic Annotation Framework"@en .


###  http://w3id.org/meta-share/meta-share/SemAF-DA
ms:SemAF-DA rdf:type owl:NamedIndividual ,
                     ms:StandardBestPractice ;
            ms:url "https://www.iso.org/standard/76443.html" ;
            rdfs:label "SemAF-DA"@en ;
            skos:altLabel "Semantic Annotation Framework - Dialogue Acts"@en .


###  http://w3id.org/meta-share/meta-share/SemAF-DS
ms:SemAF-DS rdf:type owl:NamedIndividual ,
                     ms:StandardBestPractice ;
            ms:url "https://www.iso.org/obp/ui/#iso:std:iso:ts:24617:-5:ed-1:v1:en" ;
            rdfs:label "SemAF-DS"@en ;
            skos:altLabel "Semantic Annotation Framework - Discourse Structure"@en .


###  http://w3id.org/meta-share/meta-share/SemAF-NE
ms:SemAF-NE rdf:type owl:NamedIndividual ,
                     ms:StandardBestPractice ;
            ms:url "http://semanticweb.kaist.ac.kr/research/tc37sc4/new_doc/iso_tc37_sc4_N796_wg2_proposed_WD_24617-3_SemAF-NE.pdf" ;
            rdfs:label "SemAF-NE"@en ;
            skos:altLabel "Semantic Annotation Framework - Named Entities"@en .


###  http://w3id.org/meta-share/meta-share/SemAF-SR
ms:SemAF-SR rdf:type owl:NamedIndividual ,
                     ms:StandardBestPractice ;
            ms:url "https://www.iso.org/standard/56866.html" ;
            rdfs:label "SemAF-SR"@en ;
            skos:altLabel "Semantic Annotation Framework - Semantic Roles"@en .


###  http://w3id.org/meta-share/meta-share/SemanticType
ms:SemanticType rdf:type owl:NamedIndividual ,
                         skos:Concept ;
                rdfs:comment "A type of content included in a language resource pertaining to the semantic level"@en ;
                rdfs:label "Semantic type"@en ;
                skos:inScheme ms:ContentTypeScheme .


###  http://w3id.org/meta-share/meta-share/Shift_JIS
ms:Shift_JIS rdf:type owl:NamedIndividual ,
                      ms:CharacterEncoding ;
             rdfs:label "Shift_JIS"@en .


###  http://w3id.org/meta-share/meta-share/Speechbrain
ms:Speechbrain rdf:type owl:NamedIndividual ,
                        ms:Toolkit ;
               rdfs:comment "A speech processing toolkit"@en ;
               rdfs:label "Speechbrain"@en .


###  http://w3id.org/meta-share/meta-share/SynAF
ms:SynAF rdf:type owl:NamedIndividual ,
                  ms:StandardBestPractice ;
         ms:url "https://www.iso.org/standard/62508.html" ;
         rdfs:label "SynAF"@en ;
         skos:altLabel "Syntactic Annotation Framework"@en .


###  http://w3id.org/meta-share/meta-share/SyntacticType
ms:SyntacticType rdf:type owl:NamedIndividual ,
                          skos:Concept ;
                 rdfs:comment "A type of content included in a language resource pertaining to the syntactic level"@en ;
                 rdfs:label "Syntactic type"@en ;
                 skos:inScheme ms:ContentTypeScheme .


###  http://w3id.org/meta-share/meta-share/SyntacticoSemanticType
ms:SyntacticoSemanticType rdf:type owl:NamedIndividual ,
                                   skos:Concept ;
                          rdfs:comment "A type of content included in a language resource pertaining to the syntactico-semantic level"@en ;
                          rdfs:label "Syntactico-semantic type"@en ;
                          skos:inScheme ms:ContentTypeScheme .


###  http://w3id.org/meta-share/meta-share/T-HPair
ms:T-HPair rdf:type owl:NamedIndividual ,
                    ms:SizeUnit ;
           rdfs:label "T-H pair"@en .


###  http://w3id.org/meta-share/meta-share/TBX
ms:TBX rdf:type owl:NamedIndividual ,
                ms:StandardBestPractice ;
       ms:url "https://www.tbxinfo.net/tbx-about/" ;
       rdfs:label "TBX"@en ;
       skos:altLabel "TermBase eXchange"@en .


###  http://w3id.org/meta-share/meta-share/TEI
ms:TEI rdf:type owl:NamedIndividual ,
                ms:StandardBestPractice ;
       ms:url "https://tei-c.org/" ;
       rdfs:label "TEI"@en ;
       skos:altLabel "Text Encoding Initiative"@en .


###  http://w3id.org/meta-share/meta-share/TEI_P3
ms:TEI_P3 rdf:type owl:NamedIndividual ,
                   ms:StandardBestPractice ;
          ms:url "https://www.tei-c.org/Vault/GL/P3/index.htm" ;
          rdfs:label "TEI P3"@en ;
          skos:altLabel "Text Encoding Initiative P3"@en .


###  http://w3id.org/meta-share/meta-share/TEI_P4
ms:TEI_P4 rdf:type owl:NamedIndividual ,
                   ms:StandardBestPractice ;
          ms:url "https://tei-c.org/Vault/P4/doc/html/" ;
          rdfs:label "TEI P4"@en ;
          skos:altLabel "Text Encoding Initiative P4"@en .


###  http://w3id.org/meta-share/meta-share/TEI_P5
ms:TEI_P5 rdf:type owl:NamedIndividual ,
                   ms:StandardBestPractice ;
          ms:url "https://tei-c.org/guidelines/p5/" ;
          rdfs:label "TEI P5"@en ;
          skos:altLabel "Text Encoding Initiative P5"@en .


###  http://w3id.org/meta-share/meta-share/TFLite
ms:TFLite rdf:type owl:NamedIndividual ,
                   ms:MLFramework ;
          rdfs:label "Tensor Flow lite"@en ;
          skos:altLabel "TF lite"@en .


###  http://w3id.org/meta-share/meta-share/TIS-620
ms:TIS-620 rdf:type owl:NamedIndividual ,
                    ms:CharacterEncoding ;
           rdfs:label "TIS-620"@en .


###  http://w3id.org/meta-share/meta-share/TMX
ms:TMX rdf:type owl:NamedIndividual ,
                ms:StandardBestPractice ;
       ms:url "http://www.opentag.com/tmx.htm" ;
       rdfs:label "TMX"@en ;
       skos:altLabel "Translation Memory eXchange"@en .


###  http://w3id.org/meta-share/meta-share/TST-CENTRALE
ms:TST-CENTRALE rdf:type owl:NamedIndividual ,
                         ms:MembershipInstitution ;
                rdfs:label "TST-Centrale"@en .


###  http://w3id.org/meta-share/meta-share/TensorFlow
ms:TensorFlow rdf:type owl:NamedIndividual ,
                       ms:MLFramework ;
              rdfs:label "TensorFlow"@en .


###  http://w3id.org/meta-share/meta-share/TensorFlowTTS
ms:TensorFlowTTS rdf:type owl:NamedIndividual ,
                          ms:Toolkit ;
                 rdfs:comment "A speech processing toolkit based on TensorFlow"@en ;
                 rdfs:label "TensorFlowTTS"@en .


###  http://w3id.org/meta-share/meta-share/ThreeD
ms:ThreeD rdf:type owl:NamedIndividual ,
                   ms:VisualModelling ;
          rdfs:label "3D"@en .


###  http://w3id.org/meta-share/meta-share/ThreeG
ms:ThreeG rdf:type owl:NamedIndividual ,
                   ms:SourceChannelType ;
          rdfs:label "3G"@en .


###  http://w3id.org/meta-share/meta-share/TimeML
ms:TimeML rdf:type owl:NamedIndividual ,
                   ms:StandardBestPractice ;
          ms:url "http://www.timeml.org/" ;
          rdfs:label "TimeML"@en ;
          skos:altLabel "Time Markup Language"@en .


###  http://w3id.org/meta-share/meta-share/Timm
ms:Timm rdf:type owl:NamedIndividual ,
                 ms:MLFramework ;
        rdfs:comment "A deep learning framework/library for vision; a deep-learning library created by Ross Wightman; it is a collection of SOTA computer vision models, layers, utilities, optimizers, schedulers, data-loaders, augmentations and also training/validating scripts with ability to reproduce ImageNet training results"@en ;
        rdfs:label "timm"@en .


###  http://w3id.org/meta-share/meta-share/TranslationType
ms:TranslationType rdf:type owl:NamedIndividual ,
                            skos:Concept ;
                   rdfs:comment "A type of content included in a language resource relevant to the translation procedure"@en ;
                   rdfs:label "Translation type"@en ;
                   skos:inScheme ms:ContentTypeScheme .


###  http://w3id.org/meta-share/meta-share/TwoD
ms:TwoD rdf:type owl:NamedIndividual ,
                 ms:VisualModelling ;
        rdfs:label "2D"@en .


###  http://w3id.org/meta-share/meta-share/UDC_classification
ms:UDC_classification rdf:type owl:NamedIndividual ,
                               ms:DomainClassificationScheme ;
                      ms:url "http://www.udcc.org/" ;
                      rdfs:label "UDC"@en ;
                      skos:altLabel "Universal Decimal Classification"@en .


###  http://w3id.org/meta-share/meta-share/UIMA
ms:UIMA rdf:type owl:NamedIndividual ,
                 ms:Framework ;
        rdfs:label "UIMA"@en .


###  http://w3id.org/meta-share/meta-share/US-ASCII
ms:US-ASCII rdf:type owl:NamedIndividual ,
                     ms:CharacterEncoding ;
            rdfs:label "US-ASCII"@en .


###  http://w3id.org/meta-share/meta-share/UTF-16
ms:UTF-16 rdf:type owl:NamedIndividual ,
                   ms:CharacterEncoding ;
          rdfs:label "UTF-16"@en .


###  http://w3id.org/meta-share/meta-share/UTF-16BE
ms:UTF-16BE rdf:type owl:NamedIndividual ,
                     ms:CharacterEncoding ;
            rdfs:label "UTF-16BE"@en .


###  http://w3id.org/meta-share/meta-share/UTF-16LE
ms:UTF-16LE rdf:type owl:NamedIndividual ,
                     ms:CharacterEncoding ;
            rdfs:label "UTF-16LE"@en .


###  http://w3id.org/meta-share/meta-share/UTF-8
ms:UTF-8 rdf:type owl:NamedIndividual ,
                  ms:CharacterEncoding ;
         rdfs:label "UTF-8"@en .


###  http://w3id.org/meta-share/meta-share/UsageType
ms:UsageType rdf:type owl:NamedIndividual ,
                      skos:Concept ;
             rdfs:comment "A type of content included in a language resource encoding usage information"@en ;
             rdfs:label "Usage type"@en ;
             skos:inScheme ms:ContentTypeScheme .


###  http://w3id.org/meta-share/meta-share/VGA
ms:VGA rdf:type owl:NamedIndividual ,
                ms:ResolutionStandard ;
       rdfs:label "VGA"@en .


###  http://w3id.org/meta-share/meta-share/VOIP
ms:VOIP rdf:type owl:NamedIndividual ,
                 ms:SourceChannelType ;
        rdfs:label "VOIP"@en .


###  http://w3id.org/meta-share/meta-share/XCES
ms:XCES rdf:type owl:NamedIndividual ,
                 ms:StandardBestPractice ;
        ms:url "http://www.xces.org/" ;
        rdfs:label "XCES"@en ;
        skos:altLabel "Corpus Encoding Standard for XML"@en .


###  http://w3id.org/meta-share/meta-share/XLIFF
ms:XLIFF rdf:type owl:NamedIndividual ,
                  ms:StandardBestPractice ;
         ms:url "http://docs.oasis-open.org/xliff/v1.2/os/xliff-core.html" ;
         rdfs:label "XLIFF"@en ;
         skos:altLabel "XML Localization Interchange File Format"@en .


###  http://w3id.org/meta-share/meta-share/YUV
ms:YUV rdf:type owl:NamedIndividual ,
                ms:ColourSpace ;
       rdfs:label "YUV"@en .


###  http://w3id.org/meta-share/meta-share/aLaw
ms:aLaw rdf:type owl:NamedIndividual ,
                 ms:SignalEncoding ;
        rdfs:label "A-law"@en .


###  http://w3id.org/meta-share/meta-share/aac
ms:aac rdf:type owl:NamedIndividual ,
                ms:CompressionName ;
       rdfs:label "AAC"@en ;
       skos:altLabel "Advanced Audio Coding"@en .


###  http://w3id.org/meta-share/meta-share/abbreviation
ms:abbreviation rdf:type owl:NamedIndividual ,
                         skos:Concept ;
                rdfs:label "abbreviation"@en ;
                skos:broader ms:LemmaType ;
                skos:inScheme ms:ContentTypeScheme .


###  http://w3id.org/meta-share/meta-share/academic
ms:academic rdf:type owl:NamedIndividual ,
                     ms:UserType ;
            rdfs:comment "Value for 'user type' reserved for individuals affiliated to academir or, in general, educational or research institutions and the respective organisations"@en ;
            rdfs:label "academic"@en .


###  http://w3id.org/meta-share/meta-share/academic1
ms:academic1 rdf:type owl:NamedIndividual ,
                      ms:LicenceCategory ;
             ms:conformsTo ms:ClarinLicenceCategoryScheme ;
             rdfs:label "academic"@en ;
             skos:altLabel "ACA"@en .


###  http://w3id.org/meta-share/meta-share/academicInstitution
ms:academicInstitution rdf:type owl:NamedIndividual ,
                                ms:OrganizationLegalStatus ;
                       rdfs:label "academic institution"@en .


###  http://w3id.org/meta-share/meta-share/academicText
ms:academicText rdf:type owl:NamedIndividual ,
                         ms:TextType ;
                datacite:hasIdentifier ms:ClarinEl_TT001 ;
                rdfs:label "academic text"@en .


###  http://w3id.org/meta-share/meta-share/academicUseOnly
ms:academicUseOnly rdf:type owl:NamedIndividual ,
                            ms:ConditionOfUse ;
                   rdfs:comment "Value for 'ConditionOfUse' that states that the language resource can only be used for academic purposes only (research, teaching, etc.)"@en ;
                   rdfs:label "academic use only"@en .


###  http://w3id.org/meta-share/meta-share/academicUser
ms:academicUser rdf:type owl:NamedIndividual ,
                         ms:ConditionOfUse ;
                rdfs:label "academic user"@en .


###  http://w3id.org/meta-share/meta-share/accentuation
ms:accentuation rdf:type owl:NamedIndividual ,
                         skos:Concept ;
                rdfs:label "accentuation"@en ;
                skos:broader ms:AudioType ;
                skos:inScheme ms:ContentTypeScheme .


###  http://w3id.org/meta-share/meta-share/accepted
ms:accepted rdf:type owl:NamedIndividual ,
                     ms:VersionType ;
            rdfs:comment "Value for 'Version type' used for versions as accepted for publication (following a reviewing process that may have introduced changes from the submitted version)"@en ;
            rdfs:label "accepted"@en .


###  http://w3id.org/meta-share/meta-share/accessibleThroughInterface
ms:accessibleThroughInterface rdf:type owl:NamedIndividual ,
                                       ms:DatasetDistributionForm ;
                              rdfs:comment "Value for distribution medium, used for corpora and lexical/conceptual resources that can be accessed via a human-intended interface (e.g., corpus workbench, lexicon browsing interface, etc.)"@en ;
                              rdfs:label "accessible through interface"@en .


###  http://w3id.org/meta-share/meta-share/accessibleThroughQuery
ms:accessibleThroughQuery rdf:type owl:NamedIndividual ,
                                   ms:DatasetDistributionForm ;
                          rdfs:comment "Value for dataset distribution medium, used for lexical/conceptual resources that can be accessed via a SPARQL endpoint"@en ;
                          rdfs:label "accessible through query"@en .


###  http://w3id.org/meta-share/meta-share/adapterTransformer
ms:adapterTransformer rdf:type owl:NamedIndividual ,
                               ms:MLFramework ;
                      rdfs:label "adapter transformer"@en .


###  http://w3id.org/meta-share/meta-share/administrativeText
ms:administrativeText rdf:type owl:NamedIndividual ,
                               ms:TextType ;
                      datacite:hasIdentifier ms:ClarinEl_TT008 ;
                      rdfs:label "administrative text"@en .


###  http://w3id.org/meta-share/meta-share/adult
ms:adult rdf:type owl:NamedIndividual ,
                  ms:AgeGroup ;
         rdfs:label "adult"@en .


###  http://w3id.org/meta-share/meta-share/advertising
ms:advertising rdf:type owl:NamedIndividual ,
                        ms:TextGenre ;
               datacite:hasIdentifier ms:PAROLE_G002 ;
               rdfs:label "advertising"@en .


###  http://w3id.org/meta-share/meta-share/advertisingAndPublicRelations
ms:advertisingAndPublicRelations rdf:type owl:NamedIndividual ,
                                          ms:Domain ;
                                 datacite:hasIdentifier ms:DDC659 ;
                                 rdfs:label "Advertising & Public Relations"@en .


###  http://w3id.org/meta-share/meta-share/agriculture
ms:agriculture rdf:type owl:NamedIndividual ,
                        ms:Domain ;
               datacite:hasIdentifier ms:DDC630 ;
               rdfs:comment "The science, art, or practice of cultivating the soil, producing crops, and raising livestock and in varying degrees the preparation and marketing of the resulting products [https://www.merriam-webster.com/dictionary/agriculture]"@en ;
               rdfs:label "Agriculture"@en .


###  http://w3id.org/meta-share/meta-share/airTrafficControl
ms:airTrafficControl rdf:type owl:NamedIndividual ,
                              ms:SpeechGenre ;
                     datacite:hasIdentifier ms:MS_SG001 ;
                     rdfs:label "air traffic control"@en .


###  http://w3id.org/meta-share/meta-share/airflow
ms:airflow rdf:type owl:NamedIndividual ,
                    ms:SourceChannel ;
           rdfs:label "airflow"@en .


###  http://w3id.org/meta-share/meta-share/alcohol
ms:alcohol rdf:type owl:NamedIndividual ,
                    ms:SpeechInfluence ;
           rdfs:label "alcohol"@en .


###  http://w3id.org/meta-share/meta-share/allowsAccessWithSignature
ms:allowsAccessWithSignature rdf:type owl:NamedIndividual ,
                                      ms:LicenceCategory ;
                             rdfs:comment "Value for licence category; for licences that allow access to resources only after signing the agreement"@en ;
                             rdfs:label "allows access with signature"@en .


###  http://w3id.org/meta-share/meta-share/allowsDirectAccess
ms:allowsDirectAccess rdf:type owl:NamedIndividual ,
                               ms:LicenceCategory ;
                      rdfs:comment "Value for licence category; for licences that allow access to resources without any interactions with the user"@en ;
                      rdfs:label "allows direct access"@en .


###  http://w3id.org/meta-share/meta-share/allowsProcessing
ms:allowsProcessing rdf:type owl:NamedIndividual ,
                             ms:LicenceCategory ;
                    rdfs:comment "Value for licence category; for licences that permit processing of data resources that produce research outputs (e.g., training of models, annotations, etc.)"@en ;
                    rdfs:label "allows processing"@en .


###  http://w3id.org/meta-share/meta-share/analysis
ms:analysis rdf:type owl:NamedIndividual ,
                     ms:LDTask ;
            rdfs:label "analysis"@en .


###  http://w3id.org/meta-share/meta-share/anaphora
ms:anaphora rdf:type owl:NamedIndividual ,
                     ms:GrammaticalPhenomenaCoverage ;
            rdfs:label "anaphora"@en .


###  http://w3id.org/meta-share/meta-share/anaphoraResolution
ms:anaphoraResolution rdf:type owl:NamedIndividual ,
                               ms:LDTask ;
                      rdfs:label "anaphora resolution"@en .


###  http://w3id.org/meta-share/meta-share/android
ms:android rdf:type owl:NamedIndividual ,
                    ms:OperatingSystem ;
           rdfs:label "Android"@en .


###  http://w3id.org/meta-share/meta-share/anechoicChamber
ms:anechoicChamber rdf:type owl:NamedIndividual ,
                            ms:RecordingEnvironment ;
                   rdfs:label "anechoic chamber"@en .


###  http://w3id.org/meta-share/meta-share/animalVocalization
ms:animalVocalization rdf:type owl:NamedIndividual ,
                               ms:AudioGenre ;
                      datacite:hasIdentifier ms:MS_AG006 ;
                      rdfs:label "animal vocalization"@en .


###  http://w3id.org/meta-share/meta-share/animalsZoology
ms:animalsZoology rdf:type owl:NamedIndividual ,
                           ms:Domain ;
                  datacite:hasIdentifier ms:DDC590 ;
                  rdfs:label "Animals (Zoology)"@en .


###  http://w3id.org/meta-share/meta-share/annotatedCorpus
ms:annotatedCorpus rdf:type owl:NamedIndividual ,
                            ms:CorpusSubclass ;
                   rdfs:comment "A corpus that has been processed and thus includes the raw data and the automatic or manual annotations that have been added to them"@en ;
                   rdfs:label "annotated corpus"@en .


###  http://w3id.org/meta-share/meta-share/annotationScheme
ms:annotationScheme rdf:type owl:NamedIndividual ,
                             ms:LCRSubclass ;
                    rdfs:comment "A set of elements and values designed to annotate data. It usually consists in a formal representation. It aims to represent a specific level of information, such as morphological features of words, syntactic dependency relations between phrases, discourse level information, etc. It can consist of a flat structure of elements and values (e.g., part-of-speech tags) or it can be more complex with interrelated elements (e.g., specific morphological features to be used for each part-of-speech)."@en ;
                    rdfs:label "annotation scheme"@en .


###  http://w3id.org/meta-share/meta-share/annotationsCorpus
ms:annotationsCorpus rdf:type owl:NamedIndividual ,
                              ms:CorpusSubclass ;
                     rdfs:comment "A corpus of annotations without the raw data"@en ;
                     rdfs:label "annotations corpus"@en .


###  http://w3id.org/meta-share/meta-share/antonym
ms:antonym rdf:type owl:NamedIndividual ,
                    skos:Concept ;
           rdfs:label "antonym"@en ;
           skos:broader ms:SemanticType ;
           skos:inScheme ms:ContentTypeScheme .


###  http://w3id.org/meta-share/meta-share/apiSpecification
ms:apiSpecification rdf:type owl:NamedIndividual ,
                             ms:DocumentationType ;
                    rdfs:comment "Value for 'Documentation type' used for the specification description of an API"@en ;
                    rdfs:label "API specification"@en .


###  http://w3id.org/meta-share/meta-share/applicationWord
ms:applicationWord rdf:type owl:NamedIndividual ,
                            ms:SpeechItem ;
                   rdfs:label "application word"@en .


###  http://w3id.org/meta-share/meta-share/appliedPhysics
ms:appliedPhysics rdf:type owl:NamedIndividual ,
                           ms:Domain ;
                  datacite:hasIdentifier ms:DDC621 ;
                  rdfs:label "Applied Physics"@en .


###  http://w3id.org/meta-share/meta-share/architecture
ms:architecture rdf:type owl:NamedIndividual ,
                         ms:Domain ;
                datacite:hasIdentifier ms:DDC720 ;
                rdfs:label "Architecture"@en .


###  http://w3id.org/meta-share/meta-share/arm
ms:arm rdf:type owl:NamedIndividual ,
                ms:BodyPart ;
       rdfs:label "arm"@en .


###  http://w3id.org/meta-share/meta-share/article
ms:article rdf:type owl:NamedIndividual ,
                    ms:SizeUnit ;
           rdfs:label "article"@en .


###  http://w3id.org/meta-share/meta-share/article1
ms:article1 rdf:type owl:NamedIndividual ,
                     ms:DocumentType ;
            rdfs:comment "An article from a journal or magazine"@en ;
            rdfs:label "article"@en .


###  http://w3id.org/meta-share/meta-share/artsAndRecreation
ms:artsAndRecreation rdf:type owl:NamedIndividual ,
                              ms:Domain ;
                     datacite:hasIdentifier ms:DDC700 ;
                     rdfs:label "Arts & Recreation"@en .


###  http://w3id.org/meta-share/meta-share/aspect
ms:aspect rdf:type owl:NamedIndividual ,
                   skos:Concept ;
          rdfs:label "aspect"@en ;
          skos:broader ms:MorphologicalType ;
          skos:inScheme ms:ContentTypeScheme .


###  http://w3id.org/meta-share/meta-share/assisted
ms:assisted rdf:type owl:NamedIndividual ,
                     ms:Naturality ;
            rdfs:label "assisted"@en .


###  http://w3id.org/meta-share/meta-share/association
ms:association rdf:type owl:NamedIndividual ,
                        ms:OrganizationLegalStatus ;
               rdfs:label "association"@en .


###  http://w3id.org/meta-share/meta-share/astronomy
ms:astronomy rdf:type owl:NamedIndividual ,
                      ms:Domain ;
             datacite:hasIdentifier ms:DDC520 ;
             rdfs:label "Astronomy"@en .


###  http://w3id.org/meta-share/meta-share/atrac
ms:atrac rdf:type owl:NamedIndividual ,
                  ms:CompressionName ;
         rdfs:label "altrac"@en .


###  http://w3id.org/meta-share/meta-share/attached
ms:attached rdf:type owl:NamedIndividual ,
                     ms:RelatedLexiconType ;
            rdfs:label "attached"@en .


###  http://w3id.org/meta-share/meta-share/attribution
ms:attribution rdf:type owl:NamedIndividual ,
                        ms:ConditionOfUse ,
                        odrl:Set ;
               rdfs:comment "Value for 'ConditionOfUse' that states that the use of a language resource must acknowledge it with an attribution note usually according to terms specified in the licensing document"@en ;
               rdfs:label "attribution"@en ;
               odrl:permission [ odrl:duty [ odrl:action cc:Attribution
                                           ]
                               ] .


###  http://w3id.org/meta-share/meta-share/audio
ms:audio rdf:type owl:NamedIndividual ,
                  ms:MediaType ;
         rdfs:comment "Value for 'MediaType' for the form of a language resource (part) composed of or relating to sound(s)"@en ;
         rdfs:label "audio"@en .


###  http://w3id.org/meta-share/meta-share/automatic
ms:automatic rdf:type owl:NamedIndividual ,
                      ms:ProcessMode ;
             rdfs:comment "Value for 'Process mode' and its subclasses used for fully automatic processes where the results of the process have undergone no manual edits"@en ;
             rdfs:label "automatic"@en .


###  http://w3id.org/meta-share/meta-share/automatic1
ms:automatic1 rdf:type owl:NamedIndividual ,
                       ms:EvaluationMeasure ;
              rdfs:label "automatic"@en .


###  http://w3id.org/meta-share/meta-share/auxiliary
ms:auxiliary rdf:type owl:NamedIndividual ,
                      skos:Concept ;
             rdfs:label "auxiliary"@en ;
             skos:broader ms:MorphologicalType ;
             skos:inScheme ms:ContentTypeScheme .


###  http://w3id.org/meta-share/meta-share/available
ms:available rdf:type owl:NamedIndividual ,
                      ms:Availability ;
             rdfs:comment "For resources available through the infrastructure"@en ;
             rdfs:label "available"@en .


###  http://w3id.org/meta-share/meta-share/availableThroughOtherDistributors
ms:availableThroughOtherDistributors rdf:type owl:NamedIndividual ,
                                              ms:Availability ;
                                     rdfs:comment "For resources that are available through other distribution channels"@en ;
                                     rdfs:label "available through other distributors"@en .


###  http://w3id.org/meta-share/meta-share/avi
ms:avi rdf:type owl:NamedIndividual ,
                ms:CompressionName ;
       rdfs:label "avi"@en .


###  http://w3id.org/meta-share/meta-share/backgroundNoise
ms:backgroundNoise rdf:type owl:NamedIndividual ,
                            ms:AudioQualityMeasureIncluded ;
                   rdfs:label "background noise"@en .


###  http://w3id.org/meta-share/meta-share/backgroundNoise1
ms:backgroundNoise1 rdf:type owl:NamedIndividual ,
                             ms:AnnotatedElement ;
                    rdfs:label "background noise"@en .


###  http://w3id.org/meta-share/meta-share/banking
ms:banking rdf:type owl:NamedIndividual ,
                    ms:Domain ;
           datacite:hasIdentifier ms:ELG_Domain014 ;
           rdfs:label "banking"@en .


###  http://w3id.org/meta-share/meta-share/bayesianNetwork
ms:bayesianNetwork rdf:type owl:NamedIndividual ,
                            ms:ModelType ;
                   rdfs:label "bayesian network"@en ;
                   skos:broader ms:nonDeepLearningModel .


###  http://w3id.org/meta-share/meta-share/biDirectionalRNN
ms:biDirectionalRNN rdf:type owl:NamedIndividual ,
                             ms:ModelType ;
                    rdfs:label "bidirectional recurrent neural network"@en ;
                    skos:altLabel "bidirectional RNN"@en ;
                    skos:broader ms:recurrentNeuralNetwork .


###  http://w3id.org/meta-share/meta-share/bigEndian
ms:bigEndian rdf:type owl:NamedIndividual ,
                      ms:ByteOrder ;
             rdfs:label "Big Endian"@en .


###  http://w3id.org/meta-share/meta-share/bigram
ms:bigram rdf:type owl:NamedIndividual ,
                   ms:SizeUnit ;
          rdfs:label "bigram"@en .


###  http://w3id.org/meta-share/meta-share/bilingual
ms:bilingual rdf:type owl:NamedIndividual ,
                      ms:LingualityType ;
             rdfs:comment "Value for 'Linguality type' for resource (parts) which include material in two languages"@en ;
             rdfs:label "bilingual"@en .


###  http://w3id.org/meta-share/meta-share/biochemistry
ms:biochemistry rdf:type owl:NamedIndividual ,
                         ms:Domain ;
                datacite:hasIdentifier ms:DDC572 ;
                rdfs:label "Biochemistry"@en .


###  http://w3id.org/meta-share/meta-share/biology
ms:biology rdf:type owl:NamedIndividual ,
                    ms:Domain ;
           datacite:hasIdentifier ms:DDC570 ;
           rdfs:label "Biology"@en .


###  http://w3id.org/meta-share/meta-share/blackBox
ms:blackBox rdf:type owl:NamedIndividual ,
                     ms:EvaluationType ;
            rdfs:label "black box"@en .


###  http://w3id.org/meta-share/meta-share/blogText
ms:blogText rdf:type owl:NamedIndividual ,
                     ms:TextType ;
            datacite:hasIdentifier ms:ClarinEl_TT002 ;
            rdfs:label "blog text"@en .


###  http://w3id.org/meta-share/meta-share/bluRay
ms:bluRay rdf:type owl:NamedIndividual ,
                   ms:DatasetDistributionForm ;
          rdfs:comment "bluRay refers to a kind of distribution/access medium used for delivering a language resource; intended for resources delivered on bluRay disks"@en ;
          rdfs:label "bluRay"@en .


###  http://w3id.org/meta-share/meta-share/bodyGesture
ms:bodyGesture rdf:type owl:NamedIndividual ,
                        ms:ModalityType ;
               rdfs:comment "Value for 'ModalityType' for body gestures represented in a language resource"@en ;
               rdfs:label "body gesture"@en .


###  http://w3id.org/meta-share/meta-share/book
ms:book rdf:type owl:NamedIndividual ,
                 ms:DocumentType ;
        rdfs:label "book"@en .


###  http://w3id.org/meta-share/meta-share/booklet
ms:booklet rdf:type owl:NamedIndividual ,
                    ms:DocumentType ;
           rdfs:label "booklet"@en .


###  http://w3id.org/meta-share/meta-share/boolean
ms:boolean rdf:type owl:NamedIndividual ,
                    ms:ParameterType ;
           rdfs:label "boolean"@en .


###  http://w3id.org/meta-share/meta-share/branch
ms:branch rdf:type owl:NamedIndividual ,
                   ms:DivisionCategory ;
          rdfs:label "branch"@en .


###  http://w3id.org/meta-share/meta-share/broadcastNews
ms:broadcastNews rdf:type owl:NamedIndividual ,
                          ms:SpeechGenre ;
                 datacite:hasIdentifier ms:MS_SG009 ;
                 rdfs:label "broadcast news"@en .


###  http://w3id.org/meta-share/meta-share/business
ms:business rdf:type owl:NamedIndividual ,
                     ms:Domain ;
            datacite:hasIdentifier ms:ELG_Domain011 ;
            rdfs:label "business"@en .


###  http://w3id.org/meta-share/meta-share/byte
ms:byte rdf:type owl:NamedIndividual ,
                 ms:SizeUnit ;
        rdfs:label "byte"@en .


###  http://w3id.org/meta-share/meta-share/callIn
ms:callIn rdf:type owl:NamedIndividual ,
                   ms:SpeechGenre ;
          datacite:hasIdentifier ms:MS_SG002 ;
          rdfs:label "call-in"@en .


###  http://w3id.org/meta-share/meta-share/camcorder
ms:camcorder rdf:type owl:NamedIndividual ,
                      ms:SourceChannel ;
             rdfs:label "camcorder"@en .


###  http://w3id.org/meta-share/meta-share/camera
ms:camera rdf:type owl:NamedIndividual ,
                   ms:CapturingDeviceType ;
          rdfs:label "camera"@en .


###  http://w3id.org/meta-share/meta-share/caption
ms:caption rdf:type owl:NamedIndividual ,
                    ms:TextIncludedInImage ;
           rdfs:label "caption"@en .


###  http://w3id.org/meta-share/meta-share/caption1
ms:caption1 rdf:type owl:NamedIndividual ,
                     ms:TextIncludedInVideo ;
            rdfs:label "caption"@en .


###  http://w3id.org/meta-share/meta-share/captureTime
ms:captureTime rdf:type owl:NamedIndividual ,
                        ms:TextIncludedInImage ;
               rdfs:label "capture time"@en .


###  http://w3id.org/meta-share/meta-share/case
ms:case rdf:type owl:NamedIndividual ,
                 skos:Concept ;
        rdfs:label "case"@en ;
        skos:broader ms:MorphologicalType ;
        skos:inScheme ms:ContentTypeScheme .


###  http://w3id.org/meta-share/meta-share/chart
ms:chart rdf:type owl:NamedIndividual ,
                  ms:ProcessingResourceType ;
         rdfs:label "chart"@en .


###  http://w3id.org/meta-share/meta-share/chatText
ms:chatText rdf:type owl:NamedIndividual ,
                     ms:TextType ;
            datacite:hasIdentifier ms:ClarinEl_TT014 ;
            rdfs:label "chat text"@en .


###  http://w3id.org/meta-share/meta-share/chemicalEngineering
ms:chemicalEngineering rdf:type owl:NamedIndividual ,
                                ms:Domain ;
                       datacite:hasIdentifier ms:DDC660 ;
                       rdfs:label "Chemical Engineering"@en .


###  http://w3id.org/meta-share/meta-share/chemistry
ms:chemistry rdf:type owl:NamedIndividual ,
                      ms:Domain ;
             datacite:hasIdentifier ms:DDC540 ;
             rdfs:label "Chemistry"@en .


###  http://w3id.org/meta-share/meta-share/child
ms:child rdf:type owl:NamedIndividual ,
                  ms:AgeGroup ;
         rdfs:label "child"@en .


###  http://w3id.org/meta-share/meta-share/chunking
ms:chunking rdf:type owl:NamedIndividual ,
                     ms:LDTask ;
            rdfs:label "chunking"@en .


###  http://w3id.org/meta-share/meta-share/class
ms:class rdf:type owl:NamedIndividual ,
                  ms:SizeUnit ;
         rdfs:label "class"@en .


###  http://w3id.org/meta-share/meta-share/clause
ms:clause rdf:type owl:NamedIndividual ,
                   ms:SegmentationLevel ;
          rdfs:label "clause"@en .


###  http://w3id.org/meta-share/meta-share/clauseStructure
ms:clauseStructure rdf:type owl:NamedIndividual ,
                            ms:GrammaticalPhenomenaCoverage ;
                   rdfs:label "clause structure"@en .


###  http://w3id.org/meta-share/meta-share/clippingRate
ms:clippingRate rdf:type owl:NamedIndividual ,
                         ms:AudioQualityMeasureIncluded ;
                rdfs:label "clipping rate"@en .


###  http://w3id.org/meta-share/meta-share/cliticForm
ms:cliticForm rdf:type owl:NamedIndividual ,
                       skos:Concept ;
              rdfs:label "clitic form"@en ;
              skos:altLabel "inflectional form"@en ;
              skos:broader ms:LemmaType ;
              skos:inScheme ms:ContentTypeScheme .


###  http://w3id.org/meta-share/meta-share/closeTalkMicrophone
ms:closeTalkMicrophone rdf:type owl:NamedIndividual ,
                                ms:CapturingDeviceType ;
                       rdfs:label "close talk microphone"@en .


###  http://w3id.org/meta-share/meta-share/closedPublicPlace
ms:closedPublicPlace rdf:type owl:NamedIndividual ,
                              ms:RecordingEnvironment ;
                     rdfs:label "closed public place"@en .


###  http://w3id.org/meta-share/meta-share/cognates
ms:cognates rdf:type owl:NamedIndividual ,
                     ms:LCRSubclass ;
            rdfs:label "cognates"@en .


###  http://w3id.org/meta-share/meta-share/collocation
ms:collocation rdf:type owl:NamedIndividual ,
                        skos:Concept ;
               rdfs:label "collocation"@en ;
               skos:broader ms:UsageType ;
               skos:inScheme ms:ContentTypeScheme .


###  http://w3id.org/meta-share/meta-share/combinationOfModalities
ms:combinationOfModalities rdf:type owl:NamedIndividual ,
                                    ms:ModalityType ;
                           rdfs:comment "Value for 'ModalityType' for language resources that include various modalities"@en ;
                           rdfs:label "combination of modalities"@en .


###  http://w3id.org/meta-share/meta-share/commerceTrade
ms:commerceTrade rdf:type owl:NamedIndividual ,
                          ms:Domain ;
                 datacite:hasIdentifier ms:DDC381 ;
                 rdfs:label "Commerce (Trade)"@en .


###  http://w3id.org/meta-share/meta-share/commercial
ms:commercial rdf:type owl:NamedIndividual ,
                       ms:UserType ;
              rdfs:comment "Value for 'user type' reserved for individuals affiliated with a commercial institution and the respective organisations"@en ;
              rdfs:label "commercial"@en .


###  http://w3id.org/meta-share/meta-share/commercial1
ms:commercial1 rdf:type owl:NamedIndividual ,
                        ms:NonSpeechItem ;
               rdfs:comment "Value for non-speech item, used for commercials (advertisements)"@en ;
               rdfs:label "commercial"@en .


###  http://w3id.org/meta-share/meta-share/commercialSupport
ms:commercialSupport rdf:type owl:NamedIndividual ,
                              ms:SupportType ;
                     rdfs:label "commercial support"@en .


###  http://w3id.org/meta-share/meta-share/commercialUser
ms:commercialUser rdf:type owl:NamedIndividual ,
                           ms:ConditionOfUse ;
                  rdfs:label "commercial user"@en .


###  http://w3id.org/meta-share/meta-share/communicate
ms:communicate rdf:type owl:NamedIndividual ,
                        skos:Concept ;
               rdfs:comment "The Assigner permits/prohibits the Assignees to communicate the Asset to the public"@en ;
               rdfs:label "communicate"@en ;
               skos:closeMatch odrl:present .


###  http://w3id.org/meta-share/meta-share/communications
ms:communications rdf:type owl:NamedIndividual ,
                           ms:Domain ;
                  datacite:hasIdentifier ms:DDC384 ;
                  rdfs:label "Communications"@en .


###  http://w3id.org/meta-share/meta-share/comparable
ms:comparable rdf:type owl:NamedIndividual ,
                       ms:MultilingualityType ;
              rdfs:comment "Value for 'Multilinguality type' for resource parts or resources that consist of the similar text segments in two or more languages (e.g., a corpus of legislation texts in Greek and English)"@en ;
              rdfs:label "comparable"@en .


###  http://w3id.org/meta-share/meta-share/compatible
ms:compatible rdf:type owl:NamedIndividual ,
                       ms:RelatedLexiconType ;
              rdfs:label "compatible"@en .


###  http://w3id.org/meta-share/meta-share/complex
ms:complex rdf:type owl:NamedIndividual ,
                    ms:CapturingEnvironment ;
           rdfs:label "complex"@en .


###  http://w3id.org/meta-share/meta-share/component1
ms:component1 rdf:type owl:NamedIndividual ,
                       ms:ParameterType ;
              rdfs:label "component"@en .


###  http://w3id.org/meta-share/meta-share/compound
ms:compound rdf:type owl:NamedIndividual ,
                     skos:Concept ;
            rdfs:label "compound"@en ;
            skos:broader ms:LemmaType ;
            skos:inScheme ms:ContentTypeScheme .


###  http://w3id.org/meta-share/meta-share/computationalLexicon
ms:computationalLexicon rdf:type owl:NamedIndividual ,
                                 ms:LCRSubclass ;
                        rdfs:comment "A lexicon which is intended for computational purposes and thus contains words associated with information relevant for the specific purposes"@en ;
                        rdfs:label "computational lexicon"@en .


###  http://w3id.org/meta-share/meta-share/computerScienceInformationGeneralWorks
ms:computerScienceInformationGeneralWorks rdf:type owl:NamedIndividual ,
                                                   ms:Domain ;
                                          datacite:hasIdentifier ms:DDC000 ;
                                          rdfs:label "Computer Science, Information & General Works"@en .


###  http://w3id.org/meta-share/meta-share/concept
ms:concept rdf:type owl:NamedIndividual ,
                    ms:SizeUnit ;
           rdfs:label "concept"@en .


###  http://w3id.org/meta-share/meta-share/conferenceRoom
ms:conferenceRoom rdf:type owl:NamedIndividual ,
                           ms:RecordingEnvironment ;
                  rdfs:label "conference room"@en .


###  http://w3id.org/meta-share/meta-share/constructionOfBuildings
ms:constructionOfBuildings rdf:type owl:NamedIndividual ,
                                    ms:Domain ;
                           datacite:hasIdentifier ms:DDC690 ;
                           rdfs:label "Construction of Buildings"@en .


###  http://w3id.org/meta-share/meta-share/consultingFirm
ms:consultingFirm rdf:type owl:NamedIndividual ,
                           ms:OrganizationRole ;
                  rdfs:label "consulting firm"@en .


###  http://w3id.org/meta-share/meta-share/content
ms:content rdf:type owl:NamedIndividual ,
                    ms:ValidationType ;
           rdfs:comment "Value for 'Validation type' indicating that the validation is performed on the contents of the resource"@en ;
           rdfs:label "content"@en .


###  http://w3id.org/meta-share/meta-share/conversation
ms:conversation rdf:type owl:NamedIndividual ,
                         ms:SpeechGenre ;
                datacite:hasIdentifier ms:MS_SG012 ;
                rdfs:label "conversation"@en .


###  http://w3id.org/meta-share/meta-share/convolutionalNeuralNetwork
ms:convolutionalNeuralNetwork rdf:type owl:NamedIndividual ,
                                       ms:ModelType ;
                              rdfs:label "convolutional neural network"@en ;
                              skos:altLabel "CNN"@en ;
                              skos:broader ms:DeepLearningModel .


###  http://w3id.org/meta-share/meta-share/coordination
ms:coordination rdf:type owl:NamedIndividual ,
                         ms:GrammaticalPhenomenaCoverage ;
                rdfs:label "coordination"@en .


###  http://w3id.org/meta-share/meta-share/copyrightNotEvaluated
ms:copyrightNotEvaluated rdf:type owl:NamedIndividual ,
                                  ms:AccessRightsStatement ;
                         datacite:hasIdentifier <http://rightsstatements.org/vocab/CNE/1.0/> .


###  http://w3id.org/meta-share/meta-share/copyrightUndetermined
ms:copyrightUndetermined rdf:type owl:NamedIndividual ,
                                  ms:AccessRightsStatement ;
                         datacite:hasIdentifier <http://rightsstatements.org/vocab/UND/1.0/> .


###  http://w3id.org/meta-share/meta-share/cordis
ms:cordis rdf:type owl:NamedIndividual ,
                   ms:ProjectIdentifierScheme ;
          rdfs:label "cordis"@en ;
          skos:altLabel "rcn"@en .


###  http://w3id.org/meta-share/meta-share/corpora
ms:corpora rdf:type owl:NamedIndividual ,
                    ms:ParameterType ;
           rdfs:label "corpora"@en .


###  http://w3id.org/meta-share/meta-share/corpus
ms:corpus rdf:type owl:NamedIndividual ,
                   ms:ProcessingResourceType ;
          rdfs:comment "Value for 'Resource type' for corpora, i.e. sets of datafiles (e.g., texts, audio recordings, videos, images, photographs, etc.)"@en ;
          rdfs:label "corpus"@en .


###  http://w3id.org/meta-share/meta-share/creditCardNumber
ms:creditCardNumber rdf:type owl:NamedIndividual ,
                             ms:SpeechItem ;
                    rdfs:label "credit card number"@en .


###  http://w3id.org/meta-share/meta-share/crossReference
ms:crossReference rdf:type owl:NamedIndividual ,
                           skos:Concept ;
                  rdfs:label "cross-reference"@en ;
                  skos:broader ms:SemanticType ;
                  skos:inScheme ms:ContentTypeScheme .


###  http://w3id.org/meta-share/meta-share/crossTalk
ms:crossTalk rdf:type owl:NamedIndividual ,
                      ms:AudioQualityMeasureIncluded ;
             rdfs:label "cross talk"@en .


###  http://w3id.org/meta-share/meta-share/culture
ms:culture rdf:type owl:NamedIndividual ,
                    ms:Domain ;
           datacite:hasIdentifier ms:Clarin_Domain004 ;
           rdfs:label "culture"@en .


###  http://w3id.org/meta-share/meta-share/data
ms:data rdf:type owl:NamedIndividual ,
                 ms:ParameterType ;
        rdfs:label "data"@en .


###  http://w3id.org/meta-share/meta-share/dataEvaluator
ms:dataEvaluator rdf:type owl:NamedIndividual ,
                          ms:OrganizationRole ;
                 rdfs:label "data evaluator"@en .


###  http://w3id.org/meta-share/meta-share/daylight
ms:daylight rdf:type owl:NamedIndividual ,
                     ms:SceneIllumination ;
            rdfs:label "daylight"@en .


###  http://w3id.org/meta-share/meta-share/debate
ms:debate rdf:type owl:NamedIndividual ,
                   ms:SpeechGenre ;
          datacite:hasIdentifier ms:MS_SG013 ;
          rdfs:label "debate"@en .


###  http://w3id.org/meta-share/meta-share/defence
ms:defence rdf:type owl:NamedIndividual ,
                    ms:Domain ;
           datacite:hasIdentifier ms:ELG_Domain010 ;
           rdfs:label "defence"@en .


###  http://w3id.org/meta-share/meta-share/definition
ms:definition rdf:type owl:NamedIndividual ,
                       skos:Concept ;
              rdfs:label "definition"@en ;
              skos:altLabel "gloss"@en ;
              skos:broader ms:SemanticType ;
              skos:inScheme ms:ContentTypeScheme .


###  http://w3id.org/meta-share/meta-share/definitionsParsing
ms:definitionsParsing rdf:type owl:NamedIndividual ,
                               ms:LDTask ;
                      rdfs:label "parsing of definitions"@en .


###  http://w3id.org/meta-share/meta-share/degree
ms:degree rdf:type owl:NamedIndividual ,
                   skos:Concept ;
          rdfs:label "degree"@en ;
          skos:broader ms:MorphologicalType ;
          skos:inScheme ms:ContentTypeScheme .


###  http://w3id.org/meta-share/meta-share/demoResource
ms:demoResource rdf:type owl:NamedIndividual ,
                         ms:DocumentationType ;
                rdfs:comment "Value for 'DocumentationType' used for demos of a resource available usually through the internet (e.g., video demos)"@en ;
                rdfs:label "demo resource"@en .


###  http://w3id.org/meta-share/meta-share/dentalProsthesis
ms:dentalProsthesis rdf:type owl:NamedIndividual ,
                             ms:VocalTractCondition ;
                    rdfs:label "dental prosthesis"@en .


###  http://w3id.org/meta-share/meta-share/department
ms:department rdf:type owl:NamedIndividual ,
                       ms:DivisionCategory ;
              rdfs:label "department"@en .


###  http://w3id.org/meta-share/meta-share/derivation
ms:derivation rdf:type owl:NamedIndividual ,
                       skos:Concept ;
              rdfs:label "derivation"@en ;
              skos:broader ms:MorphologicalType ;
              skos:inScheme ms:ContentTypeScheme .


###  http://w3id.org/meta-share/meta-share/diagnostic
ms:diagnostic rdf:type owl:NamedIndividual ,
                       ms:EvaluationLevel ;
              rdfs:label "diagnostic"@en .


###  http://w3id.org/meta-share/meta-share/diagram
ms:diagram rdf:type owl:NamedIndividual ,
                    ms:ProcessingResourceType ;
           rdfs:label "diagram"@en .


###  http://w3id.org/meta-share/meta-share/dialect
ms:dialect rdf:type owl:NamedIndividual ,
                    ms:LanguageVarietyType ;
           rdfs:comment "Value for 'LanguageVarietyType' used for a particular form of a language which is peculiar to a specific region or social group"@en ;
           rdfs:label "dialect"@en .


###  http://w3id.org/meta-share/meta-share/dialogue
ms:dialogue rdf:type owl:NamedIndividual ,
                     ms:ConversationalType ;
            rdfs:label "dialogue"@en .


###  http://w3id.org/meta-share/meta-share/dictionary
ms:dictionary rdf:type owl:NamedIndividual ,
                       ms:LCRSubclass ;
              rdfs:comment "A book or electronic resource that contains a list of words (usually in alphabetical order) and explains their meanings, or gives a word for them in another language and other information (e.g., spelling, pronunciation, etc.)"@en ;
              rdfs:label "dictionary"@en .


###  http://w3id.org/meta-share/meta-share/diphone
ms:diphone rdf:type owl:NamedIndividual ,
                    ms:SegmentationLevel ;
           rdfs:label "diphone"@en .


###  http://w3id.org/meta-share/meta-share/diphone1
ms:diphone1 rdf:type owl:NamedIndividual ,
                     ms:SizeUnit ;
            rdfs:label "diphone"@en .


###  http://w3id.org/meta-share/meta-share/directlyAccessible
ms:directlyAccessible rdf:type owl:NamedIndividual ,
                               ms:AccessRightsStatement ;
                      rdfs:comment "Value for access rights statements; for resources that can be accessed without interactions with the user (e.g., for resources that can be directly downloaded by users without logging into a system or signing a contract)"@en ;
                      rdfs:label "directly accessible"@en .


###  http://w3id.org/meta-share/meta-share/disasterManagement
ms:disasterManagement rdf:type owl:NamedIndividual ,
                               ms:Domain ;
                      datacite:hasIdentifier ms:ELG_Domain005 ;
                      rdfs:label "disaster management"@en .


###  http://w3id.org/meta-share/meta-share/discourseMarker
ms:discourseMarker rdf:type owl:NamedIndividual ,
                            ms:AnnotatedElement ;
                   rdfs:label "discourse marker"@en .


###  http://w3id.org/meta-share/meta-share/discussion
ms:discussion rdf:type owl:NamedIndividual ,
                       ms:TextGenre ;
              datacite:hasIdentifier ms:PAROLE_G005 ;
              rdfs:label "discussion"@en .


###  http://w3id.org/meta-share/meta-share/discussionForum
ms:discussionForum rdf:type owl:NamedIndividual ,
                            ms:SupportType ;
                   rdfs:label "discussion forum"@en .


###  http://w3id.org/meta-share/meta-share/dockerImage
ms:dockerImage rdf:type owl:NamedIndividual ,
                        ms:SoftwareDistributionForm ;
               rdfs:comment "Value for software distribution form, used for software objects distributed as Docker images, i.e. packaged together with all their dependencies and ready to be executed"@en ;
               rdfs:label "docker image"@en .


###  http://w3id.org/meta-share/meta-share/document2
ms:document2 rdf:type owl:NamedIndividual ,
                      ms:ParameterType ;
             rdfs:label "document"@en .


###  http://w3id.org/meta-share/meta-share/domain1
ms:domain1 rdf:type owl:NamedIndividual ,
                    skos:Concept ;
           rdfs:label "domain"@en ;
           skos:broader ms:SemanticType ;
           skos:inScheme ms:ContentTypeScheme .


###  http://w3id.org/meta-share/meta-share/downloadable
ms:downloadable rdf:type owl:NamedIndividual ,
                         ms:DatasetDistributionForm ;
                rdfs:comment "Value for distribution medium, used for language resources that can be downloaded from a remote location"@en ;
                rdfs:label "downloadable"@en .


###  http://w3id.org/meta-share/meta-share/draft
ms:draft rdf:type owl:NamedIndividual ,
                  ms:VersionType ;
         rdfs:comment "Value for 'Version type' used for versions during the writing up process"@en ;
         rdfs:label "draft"@en .


###  http://w3id.org/meta-share/meta-share/drop
ms:drop rdf:type owl:NamedIndividual ,
                 ms:PreviousAnnotationTypesPolicy ;
        rdfs:label "drop"@en .


###  http://w3id.org/meta-share/meta-share/dv
ms:dv rdf:type owl:NamedIndividual ,
               ms:RecordingDeviceType ;
      rdfs:label "DV"@en .


###  http://w3id.org/meta-share/meta-share/ean13
ms:ean13 rdf:type owl:NamedIndividual ,
                  ms:DocumentIdentifierScheme ;
         ms:url "https://en.wikipedia.org/wiki/International_Article_Number" ;
         rdfs:comment "Value for resourceIdentifierSchemeName, referring to EAN (International Article Number, also known as European Article Number) and more specifically to the EAN 13 standard (cf. https://en.wikipedia.org/wiki/International_Article_Number)"@en ;
         rdfs:label "EAN 13"@en ;
         skos:altLabel "European Article Number 13 standard"@en .


###  http://w3id.org/meta-share/meta-share/earthSciencesGeology
ms:earthSciencesGeology rdf:type owl:NamedIndividual ,
                                 ms:Domain ;
                        datacite:hasIdentifier ms:DDC550 ;
                        rdfs:label "Earth Sciences & Geology"@en .


###  http://w3id.org/meta-share/meta-share/economics
ms:economics rdf:type owl:NamedIndividual ,
                      ms:Domain ;
             datacite:hasIdentifier ms:DDC330 ;
             rdfs:label "Economics"@en .


###  http://w3id.org/meta-share/meta-share/education
ms:education rdf:type owl:NamedIndividual ,
                      ms:Domain ;
             datacite:hasIdentifier ms:DDC370 ;
             rdfs:label "Education"@en .


###  http://w3id.org/meta-share/meta-share/eissn
ms:eissn rdf:type owl:NamedIndividual ,
                  ms:DocumentIdentifierScheme ;
         ms:url "https://en.wikipedia.org/wiki/International_Standard_Serial_Number" ;
         rdfs:comment "Value for resourceIdentifierSchemeName, referring to the e-ISSN (electronic International Standard Serial Number, https://en.wikipedia.org/wiki/International_Standard_Serial_Number)"@en ;
         rdfs:label "e-ISSN"@en .


###  http://w3id.org/meta-share/meta-share/elderly
ms:elderly rdf:type owl:NamedIndividual ,
                    ms:AgeGroup ;
           rdfs:label "elderly"@en .


###  http://w3id.org/meta-share/meta-share/eleAccess1
ms:eleAccess1 rdf:type owl:NamedIndividual ,
                       ms:AccessRightsStatementIdentifier ;
              ms:conformsTo ms:ELERightsStatementScheme .


###  http://w3id.org/meta-share/meta-share/eleAccess2
ms:eleAccess2 rdf:type owl:NamedIndividual ,
                       ms:AccessRightsStatementIdentifier ;
              ms:conformsTo ms:ELERightsStatementScheme .


###  http://w3id.org/meta-share/meta-share/eleAccess3
ms:eleAccess3 rdf:type owl:NamedIndividual ,
                       ms:AccessRightsStatementIdentifier ;
              ms:conformsTo ms:ELERightsStatementScheme .


###  http://w3id.org/meta-share/meta-share/element
ms:element rdf:type owl:NamedIndividual ,
                    ms:SizeUnit ;
           rdfs:label "element"@en .


###  http://w3id.org/meta-share/meta-share/elg
ms:elg rdf:type owl:NamedIndividual ,
                datacite:AgentIdentifierScheme ,
                datacite:FunderIdentifierScheme ,
                datacite:OrganizationIdentifierScheme ,
                datacite:PersonalIdentifierScheme ,
                ms:DocumentIdentifierScheme ,
                ms:LRIdentifierScheme ,
                ms:LicenceIdentifierScheme ,
                ms:MetadataRecordIdentifierScheme ,
                ms:ProjectIdentifierScheme ,
                ms:RepositoryIdentifierScheme ,
                ms:RoleIdentifierScheme ;
       rdfs:comment "European Language Grid identifier scheme (used for internal purposes)"@en ;
       rdfs:label "ELG"@en .


###  http://w3id.org/meta-share/meta-share/elicited
ms:elicited rdf:type owl:NamedIndividual ,
                     ms:Naturality ;
            rdfs:label "elicited"@en .


###  http://w3id.org/meta-share/meta-share/emailText
ms:emailText rdf:type owl:NamedIndividual ,
                      ms:TextType ;
             datacite:hasIdentifier ms:ClarinEl_TT016 ;
             rdfs:label "email text"@en .


###  http://w3id.org/meta-share/meta-share/embargoedAccess
ms:embargoedAccess rdf:type owl:NamedIndividual ,
                            ms:AccessRightsStatement ;
                   datacite:hasIdentifier <http://purl.org/coar/access_right/c_f1cf> .


###  http://w3id.org/meta-share/meta-share/embeddedMicrophone
ms:embeddedMicrophone rdf:type owl:NamedIndividual ,
                               ms:CapturingDeviceType ;
                      rdfs:label "embedded microphone"@en .


###  http://w3id.org/meta-share/meta-share/embeddings
ms:embeddings rdf:type owl:NamedIndividual ,
                       ms:ModelType ;
              rdfs:label "embeddings"@en ;
              skos:broader ms:DeepLearningModel .


###  http://w3id.org/meta-share/meta-share/emotionalExpressive
ms:emotionalExpressive rdf:type owl:NamedIndividual ,
                                ms:SpeechGenre ;
                       datacite:hasIdentifier ms:MS_SG007 ;
                       rdfs:label "emotional expressive"@en .


###  http://w3id.org/meta-share/meta-share/encyclopaedicText
ms:encyclopaedicText rdf:type owl:NamedIndividual ,
                              ms:TextType ;
                     datacite:hasIdentifier ms:ClarinEl_TT003 ;
                     rdfs:label "encyclopaedic text"@en .


###  http://w3id.org/meta-share/meta-share/energy
ms:energy rdf:type owl:NamedIndividual ,
                   ms:Domain ;
          datacite:hasIdentifier ms:ELG_Domain002 ;
          rdfs:label "energy"@en .


###  http://w3id.org/meta-share/meta-share/energy1
ms:energy1 rdf:type owl:NamedIndividual ,
                    ms:Domain ;
           datacite:hasIdentifier ms:Clarin_Domain001 ;
           rdfs:label "Energy"@en .


###  http://w3id.org/meta-share/meta-share/engineering
ms:engineering rdf:type owl:NamedIndividual ,
                        ms:Domain ;
               datacite:hasIdentifier ms:DDC620 ;
               rdfs:label "Engineering"@en .


###  http://w3id.org/meta-share/meta-share/entry
ms:entry rdf:type owl:NamedIndividual ,
                  ms:SizeUnit ;
         rdfs:label "entry"@en .


###  http://w3id.org/meta-share/meta-share/enumeration
ms:enumeration rdf:type owl:NamedIndividual ,
                        ms:ParameterType ;
               rdfs:label "enumeration"@en .


###  http://w3id.org/meta-share/meta-share/environment
ms:environment rdf:type owl:NamedIndividual ,
                        ms:Domain ;
               datacite:hasIdentifier ms:Clarin_Domain002 ;
               rdfs:label "Environment"@en .


###  http://w3id.org/meta-share/meta-share/euFunds
ms:euFunds rdf:type owl:NamedIndividual ,
                    ms:FundingType ;
           rdfs:comment "Value for 'Funding type' for projects with EU funds"@en ;
           rdfs:label "EU funds"@en .


###  http://w3id.org/meta-share/meta-share/euro
ms:euro rdf:type owl:NamedIndividual ,
                 ms:Currency ;
        rdfs:label "euro"@en .


###  http://w3id.org/meta-share/meta-share/evaluationUse
ms:evaluationUse rdf:type owl:NamedIndividual ,
                          ms:ConditionOfUse ;
                 rdfs:comment "Value for 'ConditionOfUse' that states that the language resource can only be used for evaluation purposes"@en ;
                 rdfs:label "evaluation use"@en ;
                 skos:note "add odrl"@en .


###  http://w3id.org/meta-share/meta-share/eventType
ms:eventType rdf:type owl:NamedIndividual ,
                      skos:Concept ;
             rdfs:label "event type"@en ;
             skos:broader ms:SemanticType ;
             skos:inScheme ms:ContentTypeScheme .


###  http://w3id.org/meta-share/meta-share/example
ms:example rdf:type owl:NamedIndividual ,
                    ms:ExtratextualInformationUnit ;
           rdfs:label "example"@en .


###  http://w3id.org/meta-share/meta-share/example1
ms:example1 rdf:type owl:NamedIndividual ,
                     skos:Concept ;
            rdfs:label "example"@en ;
            skos:broader ms:UsageType ;
            skos:inScheme ms:ContentTypeScheme .


###  http://w3id.org/meta-share/meta-share/executableCode
ms:executableCode rdf:type owl:NamedIndividual ,
                           ms:SoftwareDistributionForm ;
                  rdfs:comment "Value for software distribution form, used for software objects available as binary files already compiled and ready to be executed"@en ;
                  rdfs:label "executable code"@en .


###  http://w3id.org/meta-share/meta-share/expression
ms:expression rdf:type owl:NamedIndividual ,
                       ms:SizeUnit ;
              rdfs:label "expression"@en .


###  http://w3id.org/meta-share/meta-share/extrinsic
ms:extrinsic rdf:type owl:NamedIndividual ,
                      ms:EvaluationCriterion ;
             rdfs:label "extrinsic"@en .


###  http://w3id.org/meta-share/meta-share/face
ms:face rdf:type owl:NamedIndividual ,
                 ms:BodyPart ;
        rdfs:label "face"@en .


###  http://w3id.org/meta-share/meta-share/faceToFaceConversation
ms:faceToFaceConversation rdf:type owl:NamedIndividual ,
                                   ms:TextType ;
                          datacite:hasIdentifier ms:ClarinEl_TT013 ;
                          rdfs:label "face to face conversation"@en ;
                          skos:altLabel "face-to-face conversation"@en .


###  http://w3id.org/meta-share/meta-share/facebook
ms:facebook rdf:type owl:NamedIndividual ,
                     ms:SocialMediaOccupationalAccountType ;
            rdfs:label "facebook"@en .


###  http://w3id.org/meta-share/meta-share/facialExpression
ms:facialExpression rdf:type owl:NamedIndividual ,
                             ms:ModalityType ;
                    rdfs:comment "Value for 'ModalityType' for facial expressions represented in a language resource"@en ;
                    rdfs:label "facial expression"@en .


###  http://w3id.org/meta-share/meta-share/faculty
ms:faculty rdf:type owl:NamedIndividual ,
                    ms:DivisionCategory ;
           rdfs:label "faculty"@en .


###  http://w3id.org/meta-share/meta-share/farfieldMicrophone
ms:farfieldMicrophone rdf:type owl:NamedIndividual ,
                               ms:CapturingDeviceType ;
                      rdfs:label "farfield microphone"@en .


###  http://w3id.org/meta-share/meta-share/feature
ms:feature rdf:type owl:NamedIndividual ,
                    ms:TextGenre ;
           datacite:hasIdentifier ms:PAROLE_G001 ;
           rdfs:label "feature"@en .


###  http://w3id.org/meta-share/meta-share/female
ms:female rdf:type owl:NamedIndividual ,
                   ms:Sex ,
                   ms:SexOfParticipants ;
          rdfs:label "female"@en .


###  http://w3id.org/meta-share/meta-share/few
ms:few rdf:type owl:NamedIndividual ,
                ms:Audience ;
       rdfs:label "few"@en .


###  http://w3id.org/meta-share/meta-share/fiction
ms:fiction rdf:type owl:NamedIndividual ,
                    ms:TextGenre ;
           datacite:hasIdentifier ms:PAROLE_G006 ;
           rdfs:label "fiction"@en .


###  http://w3id.org/meta-share/meta-share/file
ms:file rdf:type owl:NamedIndividual ,
                 ms:SizeUnit ;
        rdfs:label "file"@en .


###  http://w3id.org/meta-share/meta-share/file1
ms:file1 rdf:type owl:NamedIndividual ,
                  ms:ProcessingResourceType ;
         rdfs:label "file"@en .


###  http://w3id.org/meta-share/meta-share/finance
ms:finance rdf:type owl:NamedIndividual ,
                    ms:Domain ;
           datacite:hasIdentifier ms:ELG_Domain016 ;
           rdfs:label "finance"@en .


###  http://w3id.org/meta-share/meta-share/five-gram
ms:five-gram rdf:type owl:NamedIndividual ,
                      ms:SizeUnit ;
             rdfs:label "5-gram"@en .


###  http://w3id.org/meta-share/meta-share/fix
ms:fix rdf:type owl:NamedIndividual ,
                ms:SceneIllumination ;
       rdfs:label "fix"@en .


###  http://w3id.org/meta-share/meta-share/flac
ms:flac rdf:type owl:NamedIndividual ,
                 ms:CompressionName ;
        rdfs:label "FLAC"@en ;
        skos:altLabel "Free Lossless Audio Codec"@en .


###  http://w3id.org/meta-share/meta-share/flash
ms:flash rdf:type owl:NamedIndividual ,
                  ms:RecordingDeviceType ;
         rdfs:label "flash"@en .


###  http://w3id.org/meta-share/meta-share/float
ms:float rdf:type owl:NamedIndividual ,
                  ms:ParameterType ;
         rdfs:label "float"@en .


###  http://w3id.org/meta-share/meta-share/floatingPoint
ms:floatingPoint rdf:type owl:NamedIndividual ,
                          ms:SignConvention ;
                 rdfs:label "floating point"@en .


###  http://w3id.org/meta-share/meta-share/foot
ms:foot rdf:type owl:NamedIndividual ,
                 ms:BodyPart ;
        rdfs:label "foot"@en .


###  http://w3id.org/meta-share/meta-share/foreignAffairs
ms:foreignAffairs rdf:type owl:NamedIndividual ,
                           ms:Domain ;
                  datacite:hasIdentifier ms:ELG_Domain012 ;
                  rdfs:label "foreign affairs"@en .


###  http://w3id.org/meta-share/meta-share/formal
ms:formal rdf:type owl:NamedIndividual ,
                   ms:ValidationType ;
          rdfs:comment "Value for 'Validation type' indicating that the validation is performed on formal aspects of the resource (e.g., size, syntactic validation, etc.)"@en ;
          rdfs:label "formal"@en .


###  http://w3id.org/meta-share/meta-share/four-gram
ms:four-gram rdf:type owl:NamedIndividual ,
                      ms:SizeUnit ;
             rdfs:label "4-gram"@en .


###  http://w3id.org/meta-share/meta-share/four_2_2
ms:four_2_2 rdf:type owl:NamedIndividual ,
                     ms:ColourSpace ;
            rdfs:label "4:2:2"@en .


###  http://w3id.org/meta-share/meta-share/frame
ms:frame rdf:type owl:NamedIndividual ,
                  ms:SegmentationLevel ;
         rdfs:label "frame"@en .


###  http://w3id.org/meta-share/meta-share/frame1
ms:frame1 rdf:type owl:NamedIndividual ,
                   ms:SizeUnit ;
          rdfs:label "frame"@en .


###  http://w3id.org/meta-share/meta-share/frameNet
ms:frameNet rdf:type owl:NamedIndividual ,
                     ms:CompatibleLexiconType ,
                     ms:LCRSubclass ;
            rdfs:comment "A lexical database based on annotating examples of how words are used in actual texts in accordance to the notion of 'semantic frame' (schematic representation of a situation involving various participants, props and other conceptual roles); originally built for English and extended to other languages according to the same design principles"@en ;
            rdfs:label "FrameNet"@en .


###  http://w3id.org/meta-share/meta-share/freeSpeech
ms:freeSpeech rdf:type owl:NamedIndividual ,
                       ms:SpeechItem ;
              rdfs:label "free speech"@en .


###  http://w3id.org/meta-share/meta-share/freeSupport
ms:freeSupport rdf:type owl:NamedIndividual ,
                        ms:SupportType ;
               rdfs:label "free support"@en .


###  http://w3id.org/meta-share/meta-share/frequency
ms:frequency rdf:type owl:NamedIndividual ,
                      skos:Concept ;
             rdfs:label "frequency"@en ;
             skos:broader ms:UsageType ;
             skos:inScheme ms:ContentTypeScheme .


###  http://w3id.org/meta-share/meta-share/frogStory
ms:frogStory rdf:type owl:NamedIndividual ,
                      ms:ScenarioType ;
             rdfs:label "frog story"@en .


###  http://w3id.org/meta-share/meta-share/full
ms:full rdf:type owl:NamedIndividual ,
                 ms:ValidationExtent ;
        rdfs:label "full"@en .


###  http://w3id.org/meta-share/meta-share/fundingAuthority
ms:fundingAuthority rdf:type owl:NamedIndividual ,
                             ms:OrganizationLegalStatus ;
                    rdfs:label "funding authority"@en .


###  http://w3id.org/meta-share/meta-share/gatedRecurrentUnits
ms:gatedRecurrentUnits rdf:type owl:NamedIndividual ,
                                ms:ModelType ;
                       rdfs:label "gated recurrent units"@en ;
                       skos:altLabel "GRUs"@en ;
                       skos:broader ms:recurrentNeuralNetwork .


###  http://w3id.org/meta-share/meta-share/gb
ms:gb rdf:type owl:NamedIndividual ,
               ms:SizeUnit ;
      rdfs:label "gb"@en ;
      skos:altLabel "gigabyte"@en .


###  http://w3id.org/meta-share/meta-share/gender
ms:gender rdf:type owl:NamedIndividual ,
                   skos:Concept ;
          rdfs:label "gender"@en ;
          skos:broader ms:MorphologicalType ;
          skos:inScheme ms:ContentTypeScheme .


###  http://w3id.org/meta-share/meta-share/general
ms:general rdf:type owl:NamedIndividual ,
                    ms:Domain ;
           datacite:hasIdentifier ms:Clarin_Domain003 ;
           rdfs:label "General"@en .


###  http://w3id.org/meta-share/meta-share/generalDocumenation
ms:generalDocumenation rdf:type owl:NamedIndividual ,
                                ms:DocumentationType ;
                       rdfs:comment "Value for 'Documentation type' used for documents that describe a language resource or some aspect of it"@en ;
                       rdfs:label "general documentation"@en .


###  http://w3id.org/meta-share/meta-share/generation
ms:generation rdf:type owl:NamedIndividual ,
                       ms:LDTask ;
              rdfs:label "generation"@en .


###  http://w3id.org/meta-share/meta-share/geographyAndTravel
ms:geographyAndTravel rdf:type owl:NamedIndividual ,
                               ms:Domain ;
                      datacite:hasIdentifier ms:DDC910 ;
                      rdfs:label "Geography & Travel"@en .


###  http://w3id.org/meta-share/meta-share/github
ms:github rdf:type owl:NamedIndividual ,
                   ms:SocialMediaOccupationalAccountType ;
          rdfs:label "GitHub"@en .


###  http://w3id.org/meta-share/meta-share/gitlab
ms:gitlab rdf:type owl:NamedIndividual ,
                   ms:SocialMediaOccupationalAccountType ;
          rdfs:label "GitLab"@en .


###  http://w3id.org/meta-share/meta-share/glassBox
ms:glassBox rdf:type owl:NamedIndividual ,
                     ms:EvaluationType ;
            rdfs:label "glass box"@en .


###  http://w3id.org/meta-share/meta-share/googleChromeOS
ms:googleChromeOS rdf:type owl:NamedIndividual ,
                           ms:OperatingSystem ;
                  rdfs:label "Google Chrome OS"@en .


###  http://w3id.org/meta-share/meta-share/grammar
ms:grammar rdf:type owl:NamedIndividual ,
                    ms:LDSubclass ;
           rdfs:label "grammar"@en .


###  http://w3id.org/meta-share/meta-share/graph
ms:graph rdf:type owl:NamedIndividual ,
                  ms:ProcessingResourceType ;
         rdfs:label "graph"@en .


###  http://w3id.org/meta-share/meta-share/graphicArtsAndDecorativeArts
ms:graphicArtsAndDecorativeArts rdf:type owl:NamedIndividual ,
                                         ms:Domain ;
                                datacite:hasIdentifier ms:DDC740 ;
                                rdfs:label "Graphic Arts & Decorative Arts"@en .


###  http://w3id.org/meta-share/meta-share/graphicCard
ms:graphicCard rdf:type owl:NamedIndividual ,
                        ms:RequiredHardware ;
               rdfs:label "graphic card"@en .


###  http://w3id.org/meta-share/meta-share/grid
ms:grid rdf:type owl:NamedIndividual ,
                 datacite:OrganizationIdentifierScheme ;
        ms:url "https://www.grid.ac/" ;
        rdfs:comment "GRID identifier scheme (Global Research Identifier Database, https://www.grid.ac/)"@en ;
        rdfs:label "GRID"@en .


###  http://w3id.org/meta-share/meta-share/group
ms:group rdf:type owl:NamedIndividual ,
                  ms:DivisionCategory ;
         rdfs:label "group"@en .


###  http://w3id.org/meta-share/meta-share/guidelines
ms:guidelines rdf:type owl:NamedIndividual ,
                       ms:DocumentationType .


###  http://w3id.org/meta-share/meta-share/hand
ms:hand rdf:type owl:NamedIndividual ,
                 ms:BodyPart ;
        rdfs:label "hand"@en .


###  http://w3id.org/meta-share/meta-share/hardDisk
ms:hardDisk rdf:type owl:NamedIndividual ,
                     ms:DatasetDistributionForm ;
            rdfs:comment "Value for data distribution medium, used for resources that are delivered on a hard disk"@en ;
            rdfs:label "hard disk"@en .


###  http://w3id.org/meta-share/meta-share/hardDisk1
ms:hardDisk1 rdf:type owl:NamedIndividual ,
                      ms:RecordingDeviceType ;
             rdfs:label "hard disk"@en .


###  http://w3id.org/meta-share/meta-share/hardwareAndHouseholdAppliances
ms:hardwareAndHouseholdAppliances rdf:type owl:NamedIndividual ,
                                           ms:Domain ;
                                  datacite:hasIdentifier ms:DDC683 ;
                                  rdfs:label "Hardware & Household Appliances"@en .


###  http://w3id.org/meta-share/meta-share/head
ms:head rdf:type owl:NamedIndividual ,
                 ms:BodyPart ;
        rdfs:label "head"@en .


###  http://w3id.org/meta-share/meta-share/health
ms:health rdf:type owl:NamedIndividual ,
                   ms:Domain ;
          datacite:hasIdentifier ms:ELG_Domain009 ;
          rdfs:label "health"@en .


###  http://w3id.org/meta-share/meta-share/hiddenMarkovModels
ms:hiddenMarkovModels rdf:type owl:NamedIndividual ,
                               ms:ModelType ;
                      rdfs:label "Hidden Markov Models"@en ;
                      skos:altLabel "HMM"@en ;
                      skos:broader ms:nonDeepLearningModel .


###  http://w3id.org/meta-share/meta-share/high
ms:high rdf:type owl:NamedIndividual ,
                 ms:RecordingQuality ;
        rdfs:label "high"@en .


###  http://w3id.org/meta-share/meta-share/high1
ms:high1 rdf:type owl:NamedIndividual ,
                  ms:Quality ;
         rdfs:label "high"@en .


###  http://w3id.org/meta-share/meta-share/high2
ms:high2 rdf:type owl:NamedIndividual ,
                  ms:NoiseLevel ;
         rdfs:label "high"@en .


###  http://w3id.org/meta-share/meta-share/history
ms:history rdf:type owl:NamedIndividual ,
                    ms:Domain ;
           datacite:hasIdentifier ms:DDC900 ;
           rdfs:label "History"@en .


###  http://w3id.org/meta-share/meta-share/homeAndFamilyManagement
ms:homeAndFamilyManagement rdf:type owl:NamedIndividual ,
                                    ms:Domain ;
                           datacite:hasIdentifier ms:DDC640 ;
                           rdfs:label "Home & Family Management"@en .


###  http://w3id.org/meta-share/meta-share/hour
ms:hour rdf:type owl:NamedIndividual ,
                 ms:DurationUnit ;
        rdfs:label "hour"@en .


###  http://w3id.org/meta-share/meta-share/hour1
ms:hour1 rdf:type owl:NamedIndividual ,
                  ms:SizeUnit ;
         rdfs:label "hour"@en .


###  http://w3id.org/meta-share/meta-share/human
ms:human rdf:type owl:NamedIndividual ,
                  ms:EvaluationMeasure ;
         rdfs:label "human"@en .


###  http://w3id.org/meta-share/meta-share/humanNonSpeech
ms:humanNonSpeech rdf:type owl:NamedIndividual ,
                           ms:AudioGenre ;
                  datacite:hasIdentifier ms:MS_AG001 ;
                  rdfs:label "human non speech"@en .


###  http://w3id.org/meta-share/meta-share/hyperbaric
ms:hyperbaric rdf:type owl:NamedIndividual ,
                       ms:SpeechInfluence ;
              rdfs:label "hyperbaric"@en .


###  http://w3id.org/meta-share/meta-share/hyperonym
ms:hyperonym rdf:type owl:NamedIndividual ,
                      skos:Concept ;
             rdfs:label "hyperonym"@en ;
             skos:broader ms:SemanticType ;
             skos:inScheme ms:ContentTypeScheme .


###  http://w3id.org/meta-share/meta-share/hyponym
ms:hyponym rdf:type owl:NamedIndividual ,
                    skos:Concept ;
           rdfs:label "hyponym"@en ;
           skos:broader ms:SemanticType ;
           skos:inScheme ms:ContentTypeScheme .


###  http://w3id.org/meta-share/meta-share/iOS
ms:iOS rdf:type owl:NamedIndividual ,
                ms:OperatingSystem ;
       rdfs:label "iOS"@en .


###  http://w3id.org/meta-share/meta-share/idiomaticExpression
ms:idiomaticExpression rdf:type owl:NamedIndividual ,
                                ms:SizeUnit ;
                       rdfs:label "idiomatic expression"@en .


###  http://w3id.org/meta-share/meta-share/image
ms:image rdf:type owl:NamedIndividual ,
                  ms:MediaType ;
         rdfs:comment "Value for 'Media type' for the for of a language resource (part) consisting of visual representations (e.g., pictures, photos)"@en ;
         rdfs:label "image"@en .


###  http://w3id.org/meta-share/meta-share/image1
ms:image1 rdf:type owl:NamedIndividual ,
                   ms:ExtratextualInformation ;
          rdfs:label "image"@en .


###  http://w3id.org/meta-share/meta-share/image2
ms:image2 rdf:type owl:NamedIndividual ,
                   ms:SizeUnit ;
          rdfs:label "image"@en .


###  http://w3id.org/meta-share/meta-share/image3
ms:image3 rdf:type owl:NamedIndividual .


###  http://w3id.org/meta-share/meta-share/impact
ms:impact rdf:type owl:NamedIndividual ,
                   ms:EvaluationLevel ;
          rdfs:label "impact"@en .


###  http://w3id.org/meta-share/meta-share/inBook
ms:inBook rdf:type owl:NamedIndividual ,
                   ms:DocumentType ;
          rdfs:label "in book"@en .


###  http://w3id.org/meta-share/meta-share/inCar
ms:inCar rdf:type owl:NamedIndividual ,
                  ms:RecordingEnvironment ;
         rdfs:label "in car"@en .


###  http://w3id.org/meta-share/meta-share/inCollection
ms:inCollection rdf:type owl:NamedIndividual ,
                         ms:DocumentType ;
                rdfs:label "in collection"@en .


###  http://w3id.org/meta-share/meta-share/inCopyright
ms:inCopyright rdf:type owl:NamedIndividual ,
                        ms:AccessRightsStatement ;
               datacite:hasIdentifier <http://rightsstatements.org/vocab/InC/1.0/> .


###  http://w3id.org/meta-share/meta-share/inCopyrightEUOrphan
ms:inCopyrightEUOrphan rdf:type owl:NamedIndividual ,
                                ms:AccessRightsStatement ;
                       datacite:hasIdentifier <http://rightsstatements.org/vocab/InC-OW-EU/1.0/> .


###  http://w3id.org/meta-share/meta-share/inCopyrightEdu
ms:inCopyrightEdu rdf:type owl:NamedIndividual ,
                           ms:AccessRightsStatement ;
                  datacite:hasIdentifier <http://rightsstatements.org/vocab/InC-EDU/1.0/> .


###  http://w3id.org/meta-share/meta-share/inCopyrightNCPermitted
ms:inCopyrightNCPermitted rdf:type owl:NamedIndividual ,
                                   ms:AccessRightsStatement ;
                          datacite:hasIdentifier <http://rightsstatements.org/vocab/InC-NC/1.0/> .


###  http://w3id.org/meta-share/meta-share/inCopyrightRightsHoldersUnlocatable
ms:inCopyrightRightsHoldersUnlocatable rdf:type owl:NamedIndividual ,
                                                ms:AccessRightsStatement ;
                                       datacite:hasIdentifier <http://rightsstatements.org/vocab/InC-RUU/1.0/> .


###  http://w3id.org/meta-share/meta-share/inProceedings
ms:inProceedings rdf:type owl:NamedIndividual ,
                          ms:DocumentType ;
                 rdfs:label "in proceedings"@en .


###  http://w3id.org/meta-share/meta-share/included
ms:included rdf:type owl:NamedIndividual ,
                     ms:RelatedLexiconType ;
            rdfs:label "included"@en .


###  http://w3id.org/meta-share/meta-share/incorporate
ms:incorporate rdf:type owl:NamedIndividual ,
                        skos:Concept ;
               rdfs:comment "The Assigner permits/prohibits the Assignees to incorporate the Asset unmodified into a Collective Work."@en ;
               rdfs:label "incorporate"@en ;
               skos:broader odrl:use .


###  http://w3id.org/meta-share/meta-share/industrial
ms:industrial rdf:type owl:NamedIndividual ,
                       ms:RecordingEnvironment ;
              rdfs:label "industrial"@en .


###  http://w3id.org/meta-share/meta-share/inflection
ms:inflection rdf:type owl:NamedIndividual ,
                       skos:Concept ;
              rdfs:label "inflection"@en ;
              skos:broader ms:MorphologicalType ;
              skos:inScheme ms:ContentTypeScheme .


###  http://w3id.org/meta-share/meta-share/informLicensor
ms:informLicensor rdf:type owl:NamedIndividual ,
                           ms:ConditionOfUse ,
                           odrl:Set ;
                  rdfs:comment "Value for 'ConditionOfUse' which states that users must inform the licensor as to the kind of use they intend to make of the resource"@en ;
                  rdfs:label "inform licensor"@en ;
                  odrl:permission [ odrl:duty [ odrl:action cc:Notify
                                              ]
                                  ] .


###  http://w3id.org/meta-share/meta-share/information
ms:information rdf:type owl:NamedIndividual ,
                        ms:TextGenre ;
               datacite:hasIdentifier ms:PAROLE_G003 ;
               rdfs:label "information"@en .


###  http://w3id.org/meta-share/meta-share/ingestedRecord
ms:ingestedRecord rdf:type owl:NamedIndividual ,
                           ms:SizeUnit ;
                  rdfs:label "ingested record"@en .


###  http://w3id.org/meta-share/meta-share/installationManual
ms:installationManual rdf:type owl:NamedIndividual ,
                               ms:DocumentationType ;
                      rdfs:comment "Value for 'Documentation type' used for documents that contain instructions on how to install a software"@en ;
                      rdfs:label "installation manual"@en .


###  http://w3id.org/meta-share/meta-share/institute
ms:institute rdf:type owl:NamedIndividual ,
                      ms:DivisionCategory ;
             rdfs:label "institute"@en .


###  http://w3id.org/meta-share/meta-share/instruction
ms:instruction rdf:type owl:NamedIndividual ,
                        ms:TextGenre ;
               datacite:hasIdentifier ms:PAROLE_G004 ;
               rdfs:label "instruction"@en .


###  http://w3id.org/meta-share/meta-share/instrumentalMusic
ms:instrumentalMusic rdf:type owl:NamedIndividual ,
                              ms:AudioGenre ;
                     datacite:hasIdentifier ms:MS_AG005 ;
                     rdfs:label "instrumental music"@en .


###  http://w3id.org/meta-share/meta-share/insurance
ms:insurance rdf:type owl:NamedIndividual ,
                      ms:Domain ;
             datacite:hasIdentifier ms:ELG_Domain006 ;
             rdfs:label "insurance"@en .


###  http://w3id.org/meta-share/meta-share/integer
ms:integer rdf:type owl:NamedIndividual ,
                    ms:ParameterType ;
           rdfs:label "integer"@en .


###  http://w3id.org/meta-share/meta-share/interactive
ms:interactive rdf:type owl:NamedIndividual ,
                        ms:ProcessMode ;
               rdfs:comment "Value for 'Process mode' and its subclasses used for processes that include some interaction between the processing tool and the human agent performing the process"@en ;
               rdfs:label "interactive"@en .


###  http://w3id.org/meta-share/meta-share/interactive1
ms:interactive1 rdf:type owl:NamedIndividual ,
                         ms:Interactivity ;
                rdfs:label "interactive"@en .


###  http://w3id.org/meta-share/meta-share/internal
ms:internal rdf:type owl:NamedIndividual ,
                     datacite:AgentIdentifierScheme ,
                     datacite:FunderIdentifierScheme ,
                     datacite:OrganizationIdentifierScheme ,
                     datacite:PersonalIdentifierScheme ,
                     ms:DocumentIdentifierScheme ,
                     ms:LRIdentifierScheme ,
                     ms:LicenceIdentifierScheme ,
                     ms:MetadataRecordIdentifierScheme ,
                     ms:ProjectIdentifierScheme ,
                     ms:RepositoryIdentifierScheme ,
                     ms:RoleIdentifierScheme ;
            rdfs:comment "Value for identifier scheme; for identifiers created and used by systems for internal purposes"@en ;
            rdfs:label "internal"@en .


###  http://w3id.org/meta-share/meta-share/internalRecord
ms:internalRecord rdf:type owl:NamedIndividual ,
                           ms:SizeUnit ;
                  rdfs:label "internal record"@en .


###  http://w3id.org/meta-share/meta-share/internet
ms:internet rdf:type owl:NamedIndividual ,
                     ms:SourceChannel ;
            rdfs:label "internet"@en .


###  http://w3id.org/meta-share/meta-share/interview
ms:interview rdf:type owl:NamedIndividual ,
                      ms:TextType ;
             datacite:hasIdentifier ms:ClarinEl_TT006 ;
             rdfs:label "interview"@en .


###  http://w3id.org/meta-share/meta-share/interview1
ms:interview1 rdf:type owl:NamedIndividual ,
                       ms:SpeechGenre ;
              datacite:hasIdentifier ms:MS_SG006 ;
              rdfs:label "interview"@en .


###  http://w3id.org/meta-share/meta-share/intrinsic
ms:intrinsic rdf:type owl:NamedIndividual ,
                      ms:EvaluationCriterion ;
             rdfs:label "intrinsic"@en .


###  http://w3id.org/meta-share/meta-share/irregularForm
ms:irregularForm rdf:type owl:NamedIndividual ,
                          skos:Concept ;
                 rdfs:label "irregular form"@en ;
                 skos:broader ms:MorphologicalType ;
                 skos:inScheme ms:ContentTypeScheme .


###  http://w3id.org/meta-share/meta-share/islrn
ms:islrn rdf:type owl:NamedIndividual ,
                  ms:LRIdentifierScheme ;
         ms:url "http://www.islrn.org" ;
         rdfs:comment "Value for LRTIdentifierScheme referring to ISLRN (International Standard Language Resource Number, http://www.islrn.org/)"@en ;
         rdfs:label "ISLRN" .


###  http://w3id.org/meta-share/meta-share/isolatedDigit
ms:isolatedDigit rdf:type owl:NamedIndividual ,
                          ms:SpeechItem ;
                 rdfs:label "isolated digit"@en .


###  http://w3id.org/meta-share/meta-share/isolatedWord
ms:isolatedWord rdf:type owl:NamedIndividual ,
                         ms:SpeechItem ;
                rdfs:label "isolated word"@en .


###  http://w3id.org/meta-share/meta-share/issn
ms:issn rdf:type owl:NamedIndividual ,
                 ms:DocumentIdentifierScheme ;
        ms:url "http://www.issn.org" ;
        rdfs:comment "Value for resourceIdentifierSchemeName, referring to the ISSN (International Standard Serial Number, http://www.issn.org/)"@en ;
        rdfs:label "ISSN"@en ;
        skos:altLabel "International Standard Serial Number"@en .


###  http://w3id.org/meta-share/meta-share/issueTracker
ms:issueTracker rdf:type owl:NamedIndividual ,
                         ms:DocumentationType ;
                rdfs:comment "Value for 'DocumentationType' for issue-tracking tools used by software developers usually available through a dedicated web page"@en ;
                rdfs:label "issue tracker"@en .


###  http://w3id.org/meta-share/meta-share/istc
ms:istc rdf:type owl:NamedIndividual ,
                 ms:DocumentIdentifierScheme ;
        ms:url "http://www.istc-international.org/" ;
        rdfs:comment "Value for resourceIdentifierSchemeName, referring to the ISTC (International Standard Text Code, http://www.istc-international.org/)"@en ;
        rdfs:label "ISTC"@en ;
        skos:altLabel "International Standard Text Code"@en .


###  http://w3id.org/meta-share/meta-share/item
ms:item rdf:type owl:NamedIndividual ,
                 ms:SizeUnit ;
        rdfs:label "item"@en .


###  http://w3id.org/meta-share/meta-share/jargon
ms:jargon rdf:type owl:NamedIndividual ,
                   ms:LanguageVarietyType ;
          rdfs:comment "Value for 'LanguageVarietyType' used for a particular type of language mainly used in a specific context (e.g., by a professional or social group) which may not be well understood outside that context"@en ;
          rdfs:label "jargon"@en .


###  http://w3id.org/meta-share/meta-share/journalisticText
ms:journalisticText rdf:type owl:NamedIndividual ,
                             ms:TextType ;
                    datacite:hasIdentifier ms:ClarinEl_TT018 ;
                    rdfs:label "journalistic text"@en .


###  http://w3id.org/meta-share/meta-share/kNearestNeighbours
ms:kNearestNeighbours rdf:type owl:NamedIndividual ,
                               ms:ModelType ;
                      rdfs:label "k-nearest neighbours"@en ;
                      skos:altLabel "k-NN"@en ;
                      skos:broader ms:nonDeepLearningModel .


###  http://w3id.org/meta-share/meta-share/kb
ms:kb rdf:type owl:NamedIndividual ,
               ms:SizeUnit ;
      rdfs:label "kilobyte"@en ;
      skos:altLabel "kb"@en .


###  http://w3id.org/meta-share/meta-share/keep
ms:keep rdf:type owl:NamedIndividual ,
                 ms:PreviousAnnotationTypesPolicy ;
        rdfs:label "keep"@en .


###  http://w3id.org/meta-share/meta-share/keyword1
ms:keyword1 rdf:type owl:NamedIndividual ,
                     ms:SizeUnit ;
            rdfs:label "keyword"@en .


###  http://w3id.org/meta-share/meta-share/laboratory
ms:laboratory rdf:type owl:NamedIndividual ,
                       ms:DivisionCategory ;
              rdfs:label "laboratory"@en .


###  http://w3id.org/meta-share/meta-share/language1
ms:language1 rdf:type owl:NamedIndividual ,
                      ms:Domain ;
             datacite:hasIdentifier ms:DDC400 ;
             rdfs:label "Language"@en .


###  http://w3id.org/meta-share/meta-share/languageDescription
ms:languageDescription rdf:type owl:NamedIndividual ,
                                ms:ProcessingResourceType ;
                       rdfs:comment "Value for 'Resource type' for language descriptions, e.g., grammars, machine learning models, etc., i.e. language resources that formally describe a language"@en ;
                       rdfs:label "language description"@en .


###  http://w3id.org/meta-share/meta-share/languageEngineeringResearchUse
ms:languageEngineeringResearchUse rdf:type owl:NamedIndividual ,
                                           ms:ConditionOfUse ;
                                  dct:replaces "Value for 'ConditionOfUse' which states that the resource can only be used for research purposes in the Language Enginnering / Language Technology domain."@en ;
                                  rdfs:label "language engineering research use"@en .


###  http://w3id.org/meta-share/meta-share/languageServiceProvider
ms:languageServiceProvider rdf:type owl:NamedIndividual ,
                                    ms:OrganizationRole ;
                           rdfs:label "language service provider"@en .


###  http://w3id.org/meta-share/meta-share/largeCompany
ms:largeCompany rdf:type owl:NamedIndividual ,
                         ms:OrganizationLegalStatus ;
                rdfs:label "large company"@en .


###  http://w3id.org/meta-share/meta-share/largeMembraneMicrophone
ms:largeMembraneMicrophone rdf:type owl:NamedIndividual ,
                                    ms:CapturingDeviceType ;
                           rdfs:label "large membrane microphone"@en .


###  http://w3id.org/meta-share/meta-share/largePublic
ms:largePublic rdf:type owl:NamedIndividual ,
                        ms:Audience ;
               rdfs:label "large public"@en .


###  http://w3id.org/meta-share/meta-share/laryngograph
ms:laryngograph rdf:type owl:NamedIndividual ,
                         ms:SourceChannel ;
                rdfs:label "laryngograph"@en .


###  http://w3id.org/meta-share/meta-share/laryngograph1
ms:laryngograph1 rdf:type owl:NamedIndividual ,
                          ms:CapturingDeviceType ;
                 rdfs:label "laryngograph"@en .


###  http://w3id.org/meta-share/meta-share/lavalierMicrophone
ms:lavalierMicrophone rdf:type owl:NamedIndividual ,
                               ms:CapturingDeviceType ;
                      rdfs:label "lavalier microphone"@en .


###  http://w3id.org/meta-share/meta-share/law
ms:law rdf:type owl:NamedIndividual ,
                ms:Domain ;
       datacite:hasIdentifier ms:DDC340 ;
       rdfs:label "Law"@en .


###  http://w3id.org/meta-share/meta-share/law1
ms:law1 rdf:type owl:NamedIndividual ,
                 ms:Domain ;
        datacite:hasIdentifier ms:ELG_Domain018 ;
        rdfs:label "law"@en .


###  http://w3id.org/meta-share/meta-share/lecture
ms:lecture rdf:type owl:NamedIndividual ,
                    ms:SpeechGenre ;
           datacite:hasIdentifier ms:MS_SG010 ;
           rdfs:label "lecture"@en .


###  http://w3id.org/meta-share/meta-share/lectureRoom
ms:lectureRoom rdf:type owl:NamedIndividual ,
                        ms:RecordingEnvironment ;
               rdfs:label "lecture room"@en .


###  http://w3id.org/meta-share/meta-share/leg
ms:leg rdf:type owl:NamedIndividual ,
                ms:BodyPart ;
       rdfs:label "leg"@en .


###  http://w3id.org/meta-share/meta-share/lemma
ms:lemma rdf:type owl:NamedIndividual ,
                  skos:Concept ;
         rdfs:label "lemma"@en ;
         skos:broader ms:LemmaType ;
         skos:inScheme ms:ContentTypeScheme .


###  http://w3id.org/meta-share/meta-share/lemma1
ms:lemma1 rdf:type owl:NamedIndividual ,
                   ms:ExtratextualInformationUnit ;
          rdfs:label "lemma"@en .


###  http://w3id.org/meta-share/meta-share/letter
ms:letter rdf:type owl:NamedIndividual ,
                   ms:BaseItem ;
          rdfs:label "letter"@en .


###  http://w3id.org/meta-share/meta-share/letter1
ms:letter1 rdf:type owl:NamedIndividual ,
                    ms:TextType ;
           datacite:hasIdentifier ms:ClarinEl_TT004 ;
           rdfs:label "letter"@en .


###  http://w3id.org/meta-share/meta-share/lexicalConceptualResource
ms:lexicalConceptualResource rdf:type owl:NamedIndividual ,
                                      ms:ProcessingResourceType ;
                             rdfs:comment "Value for 'Processing resource type' for lexical and conceptual resources (e.g., lexica, ontologies, gazetteers, terminological lists, dictionaries, thesauri, etc.)"@en ;
                             rdfs:label "lexical/conceptual resource"@en .


###  http://w3id.org/meta-share/meta-share/lexicalType
ms:lexicalType rdf:type owl:NamedIndividual ,
                        ms:SizeUnit ;
               rdfs:label "lexical type"@en .


###  http://w3id.org/meta-share/meta-share/lexicalUnit
ms:lexicalUnit rdf:type owl:NamedIndividual ,
                        ms:ExtratextualInformationUnit ;
               rdfs:label "lexical unit"@en .


###  http://w3id.org/meta-share/meta-share/lexicon
ms:lexicon rdf:type owl:NamedIndividual ,
                    ms:LCRSubclass ;
           rdfs:comment "(a list of) all the words used in a particular language or subject, or a dictionary [https://dictionary.cambridge.org/dictionary/english/lexicon]"@en ;
           rdfs:label "lexicon"@en .


###  http://w3id.org/meta-share/meta-share/library
ms:library rdf:type owl:NamedIndividual ,
                    ms:SoftwareDistributionForm ;
           rdfs:comment "Value for software distribution form, used for software objects in the form of libraries (e.g. Java, python libraries)"@en ;
           rdfs:label "library"@en .


###  http://w3id.org/meta-share/meta-share/libraryOfCongress_Classification
ms:libraryOfCongress_Classification rdf:type owl:NamedIndividual ,
                                             ms:DomainClassificationScheme ;
                                    rdfs:label "LCC"@en ;
                                    skos:altLabel "Library of Congress classification system"@en .


###  http://w3id.org/meta-share/meta-share/libraryofCongressSubjectHeadings_classification
ms:libraryofCongressSubjectHeadings_classification rdf:type owl:NamedIndividual ,
                                                            ms:SubjectClassificationScheme ;
                                                   rdfs:label "LCSH"@en ;
                                                   skos:altLabel "Library of Congress Subject Headings"@en .


###  http://w3id.org/meta-share/meta-share/licensedWithAFee
ms:licensedWithAFee rdf:type owl:NamedIndividual ,
                             ms:AccessRightsStatement ;
                    datacite:hasIdentifier ms:eleAccess3 ;
                    rdfs:label "licensed with a fee"@en .


###  http://w3id.org/meta-share/meta-share/licensedWithoutAFeeForAllUses
ms:licensedWithoutAFeeForAllUses rdf:type owl:NamedIndividual ,
                                          ms:AccessRightsStatement ;
                                 datacite:hasIdentifier ms:eleAccess1 ;
                                 rdfs:label "licensed without a fee for all uses"@en .


###  http://w3id.org/meta-share/meta-share/licensedWithoutAFeeForSpecificUses
ms:licensedWithoutAFeeForSpecificUses rdf:type owl:NamedIndividual ,
                                               ms:AccessRightsStatement ;
                                      datacite:hasIdentifier ms:eleAccess2 ;
                                      rdfs:label "licensed without a fee for specific uses"@en .


###  http://w3id.org/meta-share/meta-share/lifeSciences
ms:lifeSciences rdf:type owl:NamedIndividual ,
                         ms:Domain ;
                datacite:hasIdentifier ms:Clarin_Domain005 ;
                rdfs:comment "A branch of science (such as biology, medicine, and sometimes anthropology or sociology) that deals with living organisms and life processes —usually used in plural"@en ;
                rdfs:label "life sciences"@en .


###  http://w3id.org/meta-share/meta-share/linearPCM
ms:linearPCM rdf:type owl:NamedIndividual ,
                      ms:SignalEncoding ;
             rdfs:label "linear PCM"@en .


###  http://w3id.org/meta-share/meta-share/linguistics
ms:linguistics rdf:type owl:NamedIndividual ,
                        ms:Domain ;
               datacite:hasIdentifier ms:DDC410 ;
               rdfs:label "Linguistics"@en .


###  http://w3id.org/meta-share/meta-share/linkedIn
ms:linkedIn rdf:type owl:NamedIndividual ,
                     ms:SocialMediaOccupationalAccountType ;
            rdfs:label "linkedIn"@en .


###  http://w3id.org/meta-share/meta-share/linux
ms:linux rdf:type owl:NamedIndividual ,
                  ms:OperatingSystem ;
         rdfs:label "Linux"@en .


###  http://w3id.org/meta-share/meta-share/lissn
ms:lissn rdf:type owl:NamedIndividual ,
                  ms:DocumentIdentifierScheme ;
         rdfs:comment "Value for resourceIdentifierSchemeName, referring to the linking ISSN or ISSN-L"@en ;
         rdfs:label "LISSN"@en ;
         skos:altLabel "ISSN-L"@en .


###  http://w3id.org/meta-share/meta-share/literaryText
ms:literaryText rdf:type owl:NamedIndividual ,
                         ms:TextType ;
                datacite:hasIdentifier ms:ClarinEl_TT012 ;
                rdfs:label "literary text"@en .


###  http://w3id.org/meta-share/meta-share/literatureRhetoricAndCriticism
ms:literatureRhetoricAndCriticism rdf:type owl:NamedIndividual ,
                                           ms:Domain ;
                                  datacite:hasIdentifier ms:DDC800 ;
                                  rdfs:label "Literature, Rhetoric & Criticism"@en .


###  http://w3id.org/meta-share/meta-share/littleEndian
ms:littleEndian rdf:type owl:NamedIndividual ,
                         ms:ByteOrder ;
                rdfs:label "Little Endian"@en .


###  http://w3id.org/meta-share/meta-share/logisticRegression
ms:logisticRegression rdf:type owl:NamedIndividual ,
                               ms:ModelType ;
                      rdfs:label "logistic regression"@en ;
                      skos:broader ms:nonDeepLearningModel .


###  http://w3id.org/meta-share/meta-share/longShortTermMemory
ms:longShortTermMemory rdf:type owl:NamedIndividual ,
                                ms:ModelType ;
                       rdfs:label "Long short-term memory"@en ;
                       skos:altLabel "LSTM"@en ;
                       skos:broader ms:recurrentNeuralNetwork .


###  http://w3id.org/meta-share/meta-share/low
ms:low rdf:type owl:NamedIndividual ,
                ms:RecordingQuality ;
       rdfs:label "low"@en .


###  http://w3id.org/meta-share/meta-share/low1
ms:low1 rdf:type owl:NamedIndividual ,
                 ms:Quality ;
        rdfs:label "low"@en .


###  http://w3id.org/meta-share/meta-share/low2
ms:low2 rdf:type owl:NamedIndividual ,
                 ms:NoiseLevel ;
        rdfs:label "low"@en .


###  http://w3id.org/meta-share/meta-share/lsid
ms:lsid rdf:type owl:NamedIndividual ,
                 ms:DocumentIdentifierScheme ;
        ms:url "http://www.webcitation.org/getfile?fileid=27fcd073ea70199946ace15c6868520be2cab2ab" ;
        rdfs:comment "Value for resourceIdentifierSchemeName, referring to the LSID (Life Sciences Identifier, http://www.webcitation.org/getfile?fileid=27fcd073ea70199946ace15c6868520be2cab2ab)"@en ;
        rdfs:label "LSID"@en ;
        skos:altLabel "Life Sciences Identifier"@en .


###  http://w3id.org/meta-share/meta-share/mac-OS
ms:mac-OS rdf:type owl:NamedIndividual ,
                   ms:OperatingSystem ;
          rdfs:label "MAC-OS"@en .


###  http://w3id.org/meta-share/meta-share/machineReadableDictionary
ms:machineReadableDictionary rdf:type owl:NamedIndividual ,
                                      ms:LCRSubclass ;
                             rdfs:comment "a dictionary usually meant for humans in a form that a computer can process"@en ;
                             rdfs:label "Machine Readable Dictionary"@en ;
                             skos:altLabel "MRD"@en .


###  http://w3id.org/meta-share/meta-share/male
ms:male rdf:type owl:NamedIndividual ,
                 ms:Sex ,
                 ms:SexOfParticipants ;
        rdfs:label "male"@en .


###  http://w3id.org/meta-share/meta-share/managementAndPublicRelations
ms:managementAndPublicRelations rdf:type owl:NamedIndividual ,
                                         ms:Domain ;
                                datacite:hasIdentifier ms:DDC650 ;
                                rdfs:label "Management & Public Relations"@en .


###  http://w3id.org/meta-share/meta-share/manual
ms:manual rdf:type owl:NamedIndividual ,
                   ms:ProcessMode ;
          rdfs:comment "Value for 'Process mode' and its subclasses used for processes that are performed manually"@en ;
          rdfs:label "manual"@en .


###  http://w3id.org/meta-share/meta-share/manual1
ms:manual1 rdf:type owl:NamedIndividual ,
                    ms:DocumentType ;
           rdfs:label "manual"@en .


###  http://w3id.org/meta-share/meta-share/manufacturing
ms:manufacturing rdf:type owl:NamedIndividual ,
                          ms:Domain ;
                 datacite:hasIdentifier ms:DDC670 ;
                 rdfs:label "Manufacturing"@en .


###  http://w3id.org/meta-share/meta-share/mapTask
ms:mapTask rdf:type owl:NamedIndividual ,
                    ms:ScenarioType ;
           rdfs:label "map task"@en .


###  http://w3id.org/meta-share/meta-share/mappingOfResources
ms:mappingOfResources rdf:type owl:NamedIndividual ,
                               ms:LCRSubclass ;
                      rdfs:comment "a resource consisting of mapping values and/or rules between two resources"@en ;
                      rdfs:label "mapping of resources"@en .


###  http://w3id.org/meta-share/meta-share/mastersThesis
ms:mastersThesis rdf:type owl:NamedIndividual ,
                          ms:DocumentType ;
                 rdfs:label "masters thesis"@en .


###  http://w3id.org/meta-share/meta-share/mathematics
ms:mathematics rdf:type owl:NamedIndividual ,
                        ms:Domain ;
               datacite:hasIdentifier ms:DDC510 ;
               rdfs:label "Mathematics"@en .


###  http://w3id.org/meta-share/meta-share/maven
ms:maven rdf:type owl:NamedIndividual ,
                  ms:LRIdentifierScheme ;
         ms:url "https://maven.apache.org/pom.html#Maven_Coordinates" ;
         rdfs:comment "Value for LRTIdentifierScheme referring to the Maven coordinates (cf. Maven POM, https://maven.apache.org/pom.html#Maven_Coordinates)"@en ;
         rdfs:label "maven"@en .


###  http://w3id.org/meta-share/meta-share/mb
ms:mb rdf:type owl:NamedIndividual ,
               ms:SizeUnit ;
      rdfs:label "mb"@en ;
      skos:altLabel "megabyte"@en .


###  http://w3id.org/meta-share/meta-share/media
ms:media rdf:type owl:NamedIndividual ,
                  ms:Domain ;
         datacite:hasIdentifier ms:ELG_Domain008 ;
         rdfs:label "media"@en .


###  http://w3id.org/meta-share/meta-share/medication
ms:medication rdf:type owl:NamedIndividual ,
                       ms:SpeechInfluence ;
              rdfs:label "medication"@en .


###  http://w3id.org/meta-share/meta-share/medicineAndHealth
ms:medicineAndHealth rdf:type owl:NamedIndividual ,
                              ms:Domain ;
                     datacite:hasIdentifier ms:DDC610 ;
                     rdfs:label "Medicine & Health"@en .


###  http://w3id.org/meta-share/meta-share/medium
ms:medium rdf:type owl:NamedIndividual ,
                   ms:RecordingQuality ;
          rdfs:label "medium"@en .


###  http://w3id.org/meta-share/meta-share/medium1
ms:medium1 rdf:type owl:NamedIndividual ,
                    ms:Quality ;
           rdfs:label "medium"@en .


###  http://w3id.org/meta-share/meta-share/medium2
ms:medium2 rdf:type owl:NamedIndividual ,
                    ms:NoiseLevel ;
           rdfs:label "medium"@en .


###  http://w3id.org/meta-share/meta-share/meeting
ms:meeting rdf:type owl:NamedIndividual ,
                    ms:SpeechGenre ;
           datacite:hasIdentifier ms:MS_SG011 ;
           rdfs:label "meeting"@en .


###  http://w3id.org/meta-share/meta-share/meetingProceedings
ms:meetingProceedings rdf:type owl:NamedIndividual ,
                               ms:TextType ;
                      datacite:hasIdentifier ms:ClarinEl_TT009 ;
                      rdfs:label "meeting proceedings"@en .


###  http://w3id.org/meta-share/meta-share/memberOfAssociation1
ms:memberOfAssociation1 rdf:type owl:NamedIndividual ,
                                 ms:ConditionOfUse ;
                        rdfs:label "member of association"@en .


###  http://w3id.org/meta-share/meta-share/meronym
ms:meronym rdf:type owl:NamedIndividual ,
                    skos:Concept ;
           rdfs:label "meronym"@en ;
           skos:broader ms:SemanticType ;
           skos:inScheme ms:ContentTypeScheme .


###  http://w3id.org/meta-share/meta-share/metaShare
ms:metaShare rdf:type owl:NamedIndividual ,
                      ms:LRIdentifierScheme ;
             ms:url "http://www.meta-share.org" ;
             rdfs:comment "Value for LRTIdentifierScheme referring to the identifier assigned by META-SHARE (http://www.meta-share.org/)"@en ;
             rdfs:label "META-SHARE"@en ;
             skos:note "in MS, we had MetaShareId and not the scheme; in general, discuss the use of \"local resource identifier scheme\" from DataCite as a value"@en .


###  http://w3id.org/meta-share/meta-share/metadataOnlyAccess
ms:metadataOnlyAccess rdf:type owl:NamedIndividual ,
                               ms:AccessRightsStatement ;
                      datacite:hasIdentifier <http://purl.org/coar/access_right/c_14cb> .


###  http://w3id.org/meta-share/meta-share/microphone
ms:microphone rdf:type owl:NamedIndividual ,
                       ms:RequiredHardware ;
              rdfs:label "microphone"@en .


###  http://w3id.org/meta-share/meta-share/microphone1
ms:microphone1 rdf:type owl:NamedIndividual ,
                        ms:CapturingDeviceType ;
               rdfs:label "microphone"@en .


###  http://w3id.org/meta-share/meta-share/microphoneArray
ms:microphoneArray rdf:type owl:NamedIndividual ,
                            ms:CapturingDeviceType ;
                   rdfs:label "microphone array"@en .


###  http://w3id.org/meta-share/meta-share/minute
ms:minute rdf:type owl:NamedIndividual ,
                   ms:SizeUnit ;
          rdfs:label "minute"@en .


###  http://w3id.org/meta-share/meta-share/minute1
ms:minute1 rdf:type owl:NamedIndividual ,
                    ms:DurationUnit ;
           rdfs:label "minute"@en .


###  http://w3id.org/meta-share/meta-share/mispronunciation
ms:mispronunciation rdf:type owl:NamedIndividual ,
                             ms:AnnotatedElement ;
                    rdfs:label "mispronunciation"@en .


###  http://w3id.org/meta-share/meta-share/mixed
ms:mixed rdf:type owl:NamedIndividual ,
                  ms:ProcessMode ;
         rdfs:comment "Value for 'Process mode' and its subclasses used for mixed processes, usually involving an automatic processing followed by human edits"@en ;
         rdfs:label "mixed"@en .


###  http://w3id.org/meta-share/meta-share/mixed1
ms:mixed1 rdf:type owl:NamedIndividual ,
                   ms:SexOfParticipants .


###  http://w3id.org/meta-share/meta-share/mixedH
ms:mixedH rdf:type owl:NamedIndividual ,
                   ms:HearingImpairmentOfParticipants ;
          rdfs:label "mixed"@en .


###  http://w3id.org/meta-share/meta-share/mixedO
ms:mixedO rdf:type owl:NamedIndividual ,
                   ms:Origin ;
          rdfs:label "mixed"@en .


###  http://w3id.org/meta-share/meta-share/mixedS
ms:mixedS rdf:type owl:NamedIndividual ,
                   ms:SpeakingImpairmentOfParticipants ;
          rdfs:label "mixed"@en .


###  http://w3id.org/meta-share/meta-share/model
ms:model rdf:type owl:NamedIndividual ,
                  ms:LDSubclass ;
         rdfs:label "model"@en .


###  http://w3id.org/meta-share/meta-share/modify
ms:modify rdf:type owl:NamedIndividual ,
                   ms:PreviousAnnotationTypesPolicy ;
          rdfs:label "modify"@en .


###  http://w3id.org/meta-share/meta-share/moneyAmount
ms:moneyAmount rdf:type owl:NamedIndividual ,
                        ms:SpeechItem ;
               rdfs:label "money amount"@en .


###  http://w3id.org/meta-share/meta-share/monolingual
ms:monolingual rdf:type owl:NamedIndividual ,
                        ms:LingualityType ;
               rdfs:comment "Value for 'Linguality type' for resource (parts) which include material in one language"@en ;
               rdfs:label "monolingual"@en .


###  http://w3id.org/meta-share/meta-share/monologue
ms:monologue rdf:type owl:NamedIndividual ,
                      ms:ConversationalType ;
             rdfs:label "monologue"@en .


###  http://w3id.org/meta-share/meta-share/mood
ms:mood rdf:type owl:NamedIndividual ,
                 skos:Concept ;
        rdfs:label "mood"@en ;
        skos:broader ms:MorphologicalType ;
        skos:inScheme ms:ContentTypeScheme .


###  http://w3id.org/meta-share/meta-share/morphologicalLexicon
ms:morphologicalLexicon rdf:type owl:NamedIndividual ,
                                 ms:CompatibleLexiconType ,
                                 ms:LCRSubclass ;
                        rdfs:comment "a lexicon with morphological information associated with its entries"@en ;
                        rdfs:label "morphological lexicon"@en .


###  http://w3id.org/meta-share/meta-share/morphology
ms:morphology rdf:type owl:NamedIndividual ,
                       ms:EncodingLevel ;
              rdfs:comment "Value for 'EncodingLevel' for the particular linguistic level that relates to the study of word formation (such as inflection, derivation and compounding)"@en ;
              rdfs:label "morphology"@en .


###  http://w3id.org/meta-share/meta-share/mouth
ms:mouth rdf:type owl:NamedIndividual ,
                  ms:BodyPart ;
         rdfs:label "mouth"@en .


###  http://w3id.org/meta-share/meta-share/mov
ms:mov rdf:type owl:NamedIndividual ,
                ms:CompressionName ;
       rdfs:label "mov"@en .


###  http://w3id.org/meta-share/meta-share/mp3
ms:mp3 rdf:type owl:NamedIndividual ,
                ms:CompressionName ;
       rdfs:label "mp3"@en .


###  http://w3id.org/meta-share/meta-share/mpeg
ms:mpeg rdf:type owl:NamedIndividual ,
                 ms:CompressionName ;
        rdfs:label "mpeg"@en .


###  http://w3id.org/meta-share/meta-share/mpg
ms:mpg rdf:type owl:NamedIndividual ,
                ms:CompressionName ;
       rdfs:label "mpg"@en .


###  http://w3id.org/meta-share/meta-share/mu-law
ms:mu-law rdf:type owl:NamedIndividual ,
                   ms:SignalEncoding ;
          rdfs:label "mu-law"@en .


###  http://w3id.org/meta-share/meta-share/multiWordUnit
ms:multiWordUnit rdf:type owl:NamedIndividual ,
                          ms:SizeUnit ;
                 rdfs:label "multi-word unit"@en ;
                 skos:altLabel "multi-word expression"@en .


###  http://w3id.org/meta-share/meta-share/multiWordUnit1
ms:multiWordUnit1 rdf:type owl:NamedIndividual ,
                           skos:Concept ;
                  rdfs:label "multi-word unit"@en ;
                  skos:altLabel "multi-word expression"@en ;
                  skos:broader ms:LemmaType ;
                  skos:inScheme ms:ContentTypeScheme .


###  http://w3id.org/meta-share/meta-share/multilingual
ms:multilingual rdf:type owl:NamedIndividual ,
                         ms:LingualityType ;
                rdfs:comment "Value for 'Linguality type' for resource (parts) which include material in three or more languages"@en ;
                rdfs:label "multilingual"@en .


###  http://w3id.org/meta-share/meta-share/multilingualSingleText
ms:multilingualSingleText rdf:type owl:NamedIndividual ,
                                   ms:MultilingualityType ;
                          rdfs:comment "Value for 'Multilinguality type' for resource parts or resources that consist of segments including text in two or more languages (e.g., the transcription of a European Parliament session with MPs speaking in their native language)"@en ;
                          rdfs:label "multilingual single text"@en .


###  http://w3id.org/meta-share/meta-share/multilogue
ms:multilogue rdf:type owl:NamedIndividual ,
                       ms:ConversationalType ;
              rdfs:label "multilogue"@en .


###  http://w3id.org/meta-share/meta-share/multipleSources
ms:multipleSources rdf:type owl:NamedIndividual ,
                            ms:SceneIllumination ;
                   rdfs:label "multiple sources"@en .


###  http://w3id.org/meta-share/meta-share/music
ms:music rdf:type owl:NamedIndividual ,
                  ms:NonSpeechItem ;
         rdfs:label "music"@en .


###  http://w3id.org/meta-share/meta-share/music1
ms:music1 rdf:type owl:NamedIndividual ,
                   ms:Domain ;
          datacite:hasIdentifier ms:DDC780 ;
          rdfs:label "Music"@en .


###  http://w3id.org/meta-share/meta-share/naiveBayes
ms:naiveBayes rdf:type owl:NamedIndividual ,
                       ms:ModelType ;
              rdfs:label "naive Bayes"@en ;
              skos:broader ms:nonDeepLearningModel .


###  http://w3id.org/meta-share/meta-share/narrative
ms:narrative rdf:type owl:NamedIndividual ,
                      ms:SpeechGenre ;
             datacite:hasIdentifier ms:MS_SG008 ;
             rdfs:label "narrative"@en .


###  http://w3id.org/meta-share/meta-share/nationalFunds
ms:nationalFunds rdf:type owl:NamedIndividual ,
                          ms:FundingType ;
                 rdfs:comment "Value for 'Funding type' for projects funded by national authorities"@en ;
                 rdfs:label "national funds"@en .


###  http://w3id.org/meta-share/meta-share/nationalSecurity
ms:nationalSecurity rdf:type owl:NamedIndividual ,
                             ms:Domain ;
                    datacite:hasIdentifier ms:ELG_Domain015 ;
                    rdfs:label "national security"@en .


###  http://w3id.org/meta-share/meta-share/native
ms:native rdf:type owl:NamedIndividual ,
                   ms:Origin ;
          rdfs:label "native"@en .


###  http://w3id.org/meta-share/meta-share/natural
ms:natural rdf:type owl:NamedIndividual ,
                    ms:Naturality ;
           rdfs:label "natural"@en .


###  http://w3id.org/meta-share/meta-share/naturalNumber
ms:naturalNumber rdf:type owl:NamedIndividual ,
                          ms:SpeechItem ;
                 rdfs:label "natural number"@en .


###  http://w3id.org/meta-share/meta-share/neologism
ms:neologism rdf:type owl:NamedIndividual ,
                      ms:SizeUnit ;
             rdfs:label "neologism"@en .


###  http://w3id.org/meta-share/meta-share/network
ms:network rdf:type owl:NamedIndividual ,
                    ms:OrganizationLegalStatus ;
           rdfs:label "network"@en .


###  http://w3id.org/meta-share/meta-share/newsMediaJournalismAndPublishing
ms:newsMediaJournalismAndPublishing rdf:type owl:NamedIndividual ,
                                             ms:Domain ;
                                    datacite:hasIdentifier ms:DDC070 ;
                                    rdfs:label "News, Media, Journalism & Publishing"@en .


###  http://w3id.org/meta-share/meta-share/ngramModel
ms:ngramModel rdf:type owl:NamedIndividual ,
                       ms:ModelType ;
              rdfs:label "n-gram model"@en ;
              skos:broader ms:nonDeepLearningModel .


###  http://w3id.org/meta-share/meta-share/no
ms:no rdf:type owl:NamedIndividual ,
               ms:SpeakingImpairmentOfParticipants ;
      rdfs:label "no"@en .


###  http://w3id.org/meta-share/meta-share/noA
ms:noA rdf:type owl:NamedIndividual ,
                ms:Anonymized ;
       rdfs:label "no"@en .


###  http://w3id.org/meta-share/meta-share/noConditions
ms:noConditions rdf:type owl:NamedIndividual ,
                         ms:ConditionOfUse ;
                rdfs:comment "Value for 'ConditionsOfUse' which states that the licence imposes no conditions"@en ;
                rdfs:label "no conditions"@en .


###  http://w3id.org/meta-share/meta-share/noCopyright
ms:noCopyright rdf:type owl:NamedIndividual ,
                        ms:AccessRightsStatement ;
               datacite:hasIdentifier <http://rightsstatements.org/vocab/NoC-OKLR/1.0/> .


###  http://w3id.org/meta-share/meta-share/noCopyrightContract
ms:noCopyrightContract rdf:type owl:NamedIndividual ,
                                ms:AccessRightsStatement ;
                       datacite:hasIdentifier <http://rightsstatements.org/vocab/NoC-CR/1.0/> .


###  http://w3id.org/meta-share/meta-share/noCopyrightNC
ms:noCopyrightNC rdf:type owl:NamedIndividual ,
                          ms:AccessRightsStatement ;
                 datacite:hasIdentifier <http://rightsstatements.org/vocab/NoC-NC/1.0/> .


###  http://w3id.org/meta-share/meta-share/noCopyrightUS
ms:noCopyrightUS rdf:type owl:NamedIndividual ,
                          ms:AccessRightsStatement ;
                 datacite:hasIdentifier <http://rightsstatements.org/vocab/NoC-US/1.0/> .


###  http://w3id.org/meta-share/meta-share/noDerivatives
ms:noDerivatives rdf:type owl:NamedIndividual ,
                          ms:ConditionOfUse ,
                          odrl:Set ;
                 rdfs:comment "Value for 'ConditionOfUse' which states that the users of the resource are not allowed to share derivatives of the resource"@en ;
                 rdfs:label "no derivatives"@en ;
                 odrl:prohibition [ odrl:action cc:DerivativeWorks
                                  ] .


###  http://w3id.org/meta-share/meta-share/noH
ms:noH rdf:type owl:NamedIndividual ,
                ms:HearingImpairmentOfParticipants ;
       rdfs:label "no"@en .


###  http://w3id.org/meta-share/meta-share/noKnownCopyright
ms:noKnownCopyright rdf:type owl:NamedIndividual ,
                             ms:AccessRightsStatement ;
                    datacite:hasIdentifier <http://rightsstatements.org/vocab/NKC/1.0/> .


###  http://w3id.org/meta-share/meta-share/noP
ms:noP rdf:type owl:NamedIndividual ,
                ms:PersonalDataIncluded ;
       rdfs:label "no"@en .


###  http://w3id.org/meta-share/meta-share/noRedistribution
ms:noRedistribution rdf:type owl:NamedIndividual ,
                             ms:ConditionOfUse ;
                    rdfs:comment "Value for 'ConditionOfUse' which states that users are not allowed to redistribute the resource"@en ;
                    rdfs:label "no redistribution"@en ;
                    odrl:prohibition [ odrl:action cc:Reproduction
                                     ] .


###  http://w3id.org/meta-share/meta-share/noS
ms:noS rdf:type owl:NamedIndividual ,
                ms:SensitiveDataIncluded ;
       rdfs:label "no"@en .


###  http://w3id.org/meta-share/meta-share/noise
ms:noise rdf:type owl:NamedIndividual ,
                  ms:NonSpeechItem ;
         rdfs:label "noise"@en .


###  http://w3id.org/meta-share/meta-share/noise1
ms:noise1 rdf:type owl:NamedIndividual ,
                   ms:AudioGenre ;
          datacite:hasIdentifier ms:MS_AG002 ;
          rdfs:label "noise"@en .


###  http://w3id.org/meta-share/meta-share/nonCommercialUse
ms:nonCommercialUse rdf:type owl:NamedIndividual ,
                             ms:ConditionOfUse ,
                             odrl:Set ;
                    rdfs:comment "Value for 'ConditionOfUse' which states that the language resource cannot be used for commercial purposes, i.e. where there is some direct profit from using it"@en ;
                    rdfs:label "non-commercial use"@en ;
                    odrl:prohibition [ odrl:action <https://creativecommons.org/ns#CommercialUse>
                                     ] .


###  http://w3id.org/meta-share/meta-share/nonDeepLearningModel
ms:nonDeepLearningModel rdf:type owl:NamedIndividual ,
                                 ms:ModelType ;
                        rdfs:label "non-deep learning model"@en ;
                        skos:altLabel "shallow learning model"@en .


###  http://w3id.org/meta-share/meta-share/nonFiction
ms:nonFiction rdf:type owl:NamedIndividual ,
                       ms:TextGenre ;
              datacite:hasIdentifier ms:PAROLE_G008 ;
              rdfs:label "non fiction"@en .


###  http://w3id.org/meta-share/meta-share/nonInteractive
ms:nonInteractive rdf:type owl:NamedIndividual ,
                           ms:Interactivity ;
                  rdfs:label "non interactive"@en .


###  http://w3id.org/meta-share/meta-share/nonNative
ms:nonNative rdf:type owl:NamedIndividual ,
                      ms:Origin ;
             rdfs:label "nonNative"@en .


###  http://w3id.org/meta-share/meta-share/none
ms:none rdf:type owl:NamedIndividual ,
                 ms:BodyPart ;
        rdfs:label "none"@en .


###  http://w3id.org/meta-share/meta-share/none1
ms:none1 rdf:type owl:NamedIndividual ,
                  ms:TextIncludedInVideo ;
         rdfs:label "none"@en .


###  http://w3id.org/meta-share/meta-share/none2
ms:none2 rdf:type owl:NamedIndividual ,
                  ms:TextIncludedInImage ;
         rdfs:label "none"@en .


###  http://w3id.org/meta-share/meta-share/none3
ms:none3 rdf:type owl:NamedIndividual ,
                  ms:Audience ;
         rdfs:label "none"@en .


###  http://w3id.org/meta-share/meta-share/none4
ms:none4 rdf:type owl:NamedIndividual ,
                  ms:RelatedLexiconType ;
         rdfs:label "none"@en .


###  http://w3id.org/meta-share/meta-share/none5
ms:none5 rdf:type owl:NamedIndividual ,
                  ms:RequiredHardware ;
         rdfs:label "none"@en .


###  http://w3id.org/meta-share/meta-share/note
ms:note rdf:type owl:NamedIndividual ,
                 ms:NonSpeechItem ;
        rdfs:label "note"@en .


###  http://w3id.org/meta-share/meta-share/note1
ms:note1 rdf:type owl:NamedIndividual ,
                  skos:Concept ;
         rdfs:label "note"@en ;
         skos:broader ms:UsageType ;
         skos:inScheme ms:ContentTypeScheme .


###  http://w3id.org/meta-share/meta-share/npRecognition
ms:npRecognition rdf:type owl:NamedIndividual ,
                          ms:LDTask ;
                 rdfs:label "recognition of noun phrases"@en .


###  http://w3id.org/meta-share/meta-share/npStructure
ms:npStructure rdf:type owl:NamedIndividual ,
                        ms:GrammaticalPhenomenaCoverage ;
               rdfs:label "NP structure"@en ;
               skos:altLabel "Structure of noun phrases"@en .


###  http://w3id.org/meta-share/meta-share/number
ms:number rdf:type owl:NamedIndividual ,
                   skos:Concept ;
          rdfs:label "number"@en ;
          skos:broader ms:MorphologicalType ;
          skos:inScheme ms:ContentTypeScheme .


###  http://w3id.org/meta-share/meta-share/oai
ms:oai rdf:type owl:NamedIndividual ,
                ms:LRIdentifierScheme ;
       ms:url "http://www.openarchives.org/OAI/2.0/guidelines-oai-identifier.htm" ;
       rdfs:comment "Value for LRTIdentifierScheme referring to the OAI identifier (Open Archives Initiative, http://www.openarchives.org/OAI/2.0/guidelines-oai-identifier.htm)"@en ;
       rdfs:label "OAI"@en .


###  http://w3id.org/meta-share/meta-share/ocrSystem
ms:ocrSystem rdf:type owl:NamedIndividual ,
                      ms:RequiredHardware ;
             rdfs:label "OCR system"@en .


###  http://w3id.org/meta-share/meta-share/office
ms:office rdf:type owl:NamedIndividual ,
                   ms:RecordingEnvironment ;
          rdfs:label "office"@en .


###  http://w3id.org/meta-share/meta-share/official
ms:official rdf:type owl:NamedIndividual ,
                     ms:TextGenre ;
            datacite:hasIdentifier ms:PAROLE_G009 ;
            rdfs:label "official"@en .


###  http://w3id.org/meta-share/meta-share/oggVorbis
ms:oggVorbis rdf:type owl:NamedIndividual ,
                      ms:CompressionName ;
             rdfs:label "Ogg Vorbis"@en .


###  http://w3id.org/meta-share/meta-share/omtd
ms:omtd rdf:type owl:NamedIndividual ,
                 ms:LRIdentifierScheme ,
                 ms:MetadataRecordIdentifierScheme ;
        ms:url "https://services.openminted.eu/home" ;
        rdfs:comment "Value for LRTIdentifierScheme referring to the identifier assigned by the OpenMinTeD platform (https://services.openminted.eu/home)"@en ;
        rdfs:label "OMTD"@en .


###  http://w3id.org/meta-share/meta-share/omtdAccess1
ms:omtdAccess1 rdf:type owl:NamedIndividual ,
                        ms:AccessRightsStatementIdentifier ;
               ms:conformsTo ms:OMTDShareRightsStatementScheme .


###  http://w3id.org/meta-share/meta-share/omtdAccess2
ms:omtdAccess2 rdf:type owl:NamedIndividual ,
                        ms:AccessRightsStatementIdentifier ;
               ms:conformsTo ms:OMTDShareRightsStatementScheme .


###  http://w3id.org/meta-share/meta-share/omtdDocker
ms:omtdDocker rdf:type owl:NamedIndividual ,
                       ms:LRIdentifierScheme ;
              ms:url "https://guidelines.openminted.eu/components_resourceIdentifier.html" ;
              rdfs:comment "Value for LRTIdentifierScheme referring to the recommended by OpenMinTeD use of identifiers for Docker images uploaded to the registry (https://guidelines.openminted.eu/components_resourceIdentifier.html)"@en ;
              rdfs:label "OMTD-Docker"@en .


###  http://w3id.org/meta-share/meta-share/onLineHelpURL
ms:onLineHelpURL rdf:type owl:NamedIndividual ,
                          ms:DocumentationType ;
                 rdfs:comment "Value for 'Documentation type' for the online help site of a language resource"@en ;
                 rdfs:label "online help URL"@en .


###  http://w3id.org/meta-share/meta-share/onlineEducationalGame
ms:onlineEducationalGame rdf:type owl:NamedIndividual ,
                                  ms:ScenarioType ;
                         rdfs:label "online educational game"@en .


###  http://w3id.org/meta-share/meta-share/onlyMSmembers
ms:onlyMSmembers rdf:type owl:NamedIndividual ,
                          ms:ConditionOfUse ,
                          odrl:Set ;
                 rdfs:comment "Value for 'ConditionsOfUse' which states that the language resource can only be used by members of the MetaShare network"@en ;
                 rdfs:label "only META-SHARE members"@en ;
                 skos:note "should we also add something more generic for restricting a resource to specific group members (as for spatial constraint)? and I don't think the odrl is ok."@en ;
                 odrl:permission [ odrl:constraint [ odrl:operator odrl:eq ;
                                                     odrl:recipient ms:onlyMSmembers
                                                   ]
                                 ] .


###  http://w3id.org/meta-share/meta-share/ontology
ms:ontology rdf:type owl:NamedIndividual ,
                     ms:CompatibleLexiconType ,
                     ms:LCRSubclass ;
            rdfs:comment "a set of concepts and categories in a subject area or domain that shows their properties and the relations between them [https://en.oxforddictionaries.com/definition/ontology]"@en ;
            rdfs:label "ontology"@en .


###  http://w3id.org/meta-share/meta-share/openAccess
ms:openAccess rdf:type owl:NamedIndividual ,
                       ms:AccessRightsStatement ;
              datacite:hasIdentifier ms:omtdAccess2 ;
              rdfs:comment "The free and online availability of literature, which allows to read, download, copy, distribute, print, search, or link to the ful text, crawl articles for indexing, pass them as data to software, or use them for any other useful purpose. An availability that is granted without financial, legal, or technical barriers other than those inseparable from gaining access to the internet itself, and those related to giving authors control over the integrity of their work and the right to be properly acknowledged and cited."@en ;
              rdfs:label "open access"@en .


###  http://w3id.org/meta-share/meta-share/openAccess1
ms:openAccess1 rdf:type owl:NamedIndividual ,
                        ms:AccessRightsStatement ;
               datacite:hasIdentifier <http://purl.org/coar/access_right/c_abf2> .


###  http://w3id.org/meta-share/meta-share/openPublicPlace
ms:openPublicPlace rdf:type owl:NamedIndividual ,
                            ms:RecordingEnvironment ;
                   rdfs:label "open public place"@en .


###  http://w3id.org/meta-share/meta-share/os-independent
ms:os-independent rdf:type owl:NamedIndividual ,
                           ms:OperatingSystem ;
                  rdfs:label "OS-independent"@en .


###  http://w3id.org/meta-share/meta-share/other
ms:other rdf:type owl:NamedIndividual ,
                  datacite:FunderIdentifierScheme ,
                  datacite:OrganizationIdentifierScheme ,
                  datacite:PersonalIdentifierScheme ,
                  ms:AnnotatedElement ,
                  ms:AudioGenre ,
                  ms:AudioGenreClassificationScheme ,
                  ms:AudioQualityMeasureIncluded ,
                  ms:BaseItem ,
                  ms:CapturingDeviceType ,
                  ms:CompatibleLexiconType ,
                  ms:CompressionName ,
                  ms:ConditionOfUse ,
                  ms:Currency ,
                  ms:DatasetDistributionForm ,
                  ms:DivisionCategory ,
                  ms:DocumentIdentifierScheme ,
                  ms:DocumentType ,
                  ms:Domain ,
                  ms:DomainClassificationScheme ,
                  ms:EncodingLevel ,
                  ms:ExtratextualInformation ,
                  ms:ExtratextualInformationUnit ,
                  ms:Framework ,
                  ms:FundingType ,
                  ms:GrammaticalPhenomenaCoverage ,
                  ms:ImageGenreClassificationScheme ,
                  ms:Interactivity ,
                  ms:LCRSubclass ,
                  ms:LDSubclass ,
                  ms:LDTask ,
                  ms:LRIdentifierScheme ,
                  ms:LanguageVarietyType ,
                  ms:LicenceIdentifierScheme ,
                  ms:MembershipInstitution ,
                  ms:MetadataRecordIdentifierScheme ,
                  ms:Metric ,
                  ms:ModalityType ,
                  ms:ModelType ,
                  ms:MultilingualityType ,
                  ms:Naturality ,
                  ms:NonSpeechItem ,
                  ms:OperatingSystem ,
                  ms:OrganizationLegalStatus ,
                  ms:OrganizationRole ,
                  ms:ParameterType ,
                  ms:ProcessingResourceType ,
                  ms:ProjectIdentifierScheme ,
                  ms:RecordingDeviceType ,
                  ms:RecordingEnvironment ,
                  ms:RepositoryIdentifierScheme ,
                  ms:RequiredHardware ,
                  ms:RoleIdentifierScheme ,
                  ms:ScenarioType ,
                  ms:SceneIllumination ,
                  ms:SegmentationLevel ,
                  ms:SignalEncoding ,
                  ms:SizeUnit ,
                  ms:SocialMediaOccupationalAccountType ,
                  ms:SoftwareDistributionForm ,
                  ms:SourceChannel ,
                  ms:SourceChannelType ,
                  ms:SpeechGenre ,
                  ms:SpeechGenreClassificationScheme ,
                  ms:SpeechInfluence ,
                  ms:SpeechItem ,
                  ms:StandardBestPractice ,
                  ms:SubjectClassificationScheme ,
                  ms:SupportType ,
                  ms:TextGenre ,
                  ms:TextGenreClassificationScheme ,
                  ms:TextType ,
                  ms:TextTypeClassificationScheme ,
                  ms:VideoGenreClassificationScheme ,
                  ms:VocalTractCondition ,
                  ms:WebServiceType ;
         rdfs:comment "Value used when none of the recommended values of an element is appropriate for an item"@en ;
         rdfs:label "other"@en .


###  http://w3id.org/meta-share/meta-share/otherSpecificRestrictions
ms:otherSpecificRestrictions rdf:type owl:NamedIndividual ,
                                      ms:ConditionOfUse ;
                             rdfs:comment "Value for 'ConditionOfUse' that states that the language resource can only be used with unspecified restrictions (not covered by the controlled vocabulary)"@en ;
                             rdfs:label "other specific restrictions"@en .


###  http://w3id.org/meta-share/meta-share/outputText
ms:outputText rdf:type owl:NamedIndividual ,
                       ms:ProcessingResourceType ;
              rdfs:label "output text"@en .


###  http://w3id.org/meta-share/meta-share/overlapping
ms:overlapping rdf:type owl:NamedIndividual ,
                        ms:Interactivity ;
               rdfs:label "overlapping"@en .


###  http://w3id.org/meta-share/meta-share/ownFunds
ms:ownFunds rdf:type owl:NamedIndividual ,
                     ms:FundingType ;
            rdfs:comment "Value for 'Funding type' for self-funded projects"@en ;
            rdfs:label "own funds"@en .


###  http://w3id.org/meta-share/meta-share/painting
ms:painting rdf:type owl:NamedIndividual ,
                     ms:Domain ;
            datacite:hasIdentifier ms:DDC750 ;
            rdfs:label "Painting"@en .


###  http://w3id.org/meta-share/meta-share/paleontology
ms:paleontology rdf:type owl:NamedIndividual ,
                         ms:Domain ;
                datacite:hasIdentifier ms:DDC560 ;
                rdfs:label "Paleontology"@en .


###  http://w3id.org/meta-share/meta-share/paperCopy
ms:paperCopy rdf:type owl:NamedIndividual ,
                      ms:DatasetDistributionForm ;
             rdfs:comment "Value for data distribution medium, used for language resources that are delivered in paper format"@en ;
             rdfs:label "paper copy"@en .


###  http://w3id.org/meta-share/meta-share/paragraph
ms:paragraph rdf:type owl:NamedIndividual ,
                      ms:SegmentationLevel ;
             rdfs:label "paragraph"@en .


###  http://w3id.org/meta-share/meta-share/parallel
ms:parallel rdf:type owl:NamedIndividual ,
                     ms:MultilingualityType ;
            rdfs:comment "Value for 'Multilinguality type' for resource parts or resources that consist of the equivalent text segments in two or more languages (e.g., an original and its translation equivalents)"@en ;
            rdfs:label "parallel"@en .


###  http://w3id.org/meta-share/meta-share/parsing
ms:parsing rdf:type owl:NamedIndividual ,
                    ms:LDTask ;
           rdfs:label "parsing"@en .


###  http://w3id.org/meta-share/meta-share/partOfSpeech
ms:partOfSpeech rdf:type owl:NamedIndividual ,
                         skos:Concept ;
                rdfs:label "part of speech"@en ;
                skos:broader ms:MorphologicalType ;
                skos:inScheme ms:ContentTypeScheme .


###  http://w3id.org/meta-share/meta-share/partial
ms:partial rdf:type owl:NamedIndividual ,
                    ms:ValidationExtent ;
           rdfs:label "partial"@en .


###  http://w3id.org/meta-share/meta-share/pearStory
ms:pearStory rdf:type owl:NamedIndividual ,
                      ms:ScenarioType ;
             rdfs:label "pear story"@en .


###  http://w3id.org/meta-share/meta-share/pennTreeBank
ms:pennTreeBank rdf:type owl:NamedIndividual ,
                         ms:StandardBestPractice ;
                ms:url "https://link.springer.com/chapter/10.1007/978-94-010-0201-1_1" ;
                rdfs:label "Penn treebank"@en .


###  http://w3id.org/meta-share/meta-share/person1
ms:person1 rdf:type owl:NamedIndividual ,
                    skos:Concept ;
           rdfs:label "person"@en ;
           skos:broader ms:MorphologicalType ;
           skos:inScheme ms:ContentTypeScheme .


###  http://w3id.org/meta-share/meta-share/pharmaceutics
ms:pharmaceutics rdf:type owl:NamedIndividual ,
                          ms:Domain ;
                 datacite:hasIdentifier ms:ELG_Domain003 ;
                 rdfs:label "pharmaceutics"@en .


###  http://w3id.org/meta-share/meta-share/phdThesis
ms:phdThesis rdf:type owl:NamedIndividual ,
                      ms:DocumentType ;
             rdfs:label "PhD thesis"@en .


###  http://w3id.org/meta-share/meta-share/philosophy
ms:philosophy rdf:type owl:NamedIndividual ,
                       ms:Domain ;
              datacite:hasIdentifier ms:DDC100 ;
              rdfs:label "Philosophy"@en .


###  http://w3id.org/meta-share/meta-share/phoneme
ms:phoneme rdf:type owl:NamedIndividual ,
                    ms:BaseItem ;
           rdfs:label "phoneme"@en .


###  http://w3id.org/meta-share/meta-share/phoneme1
ms:phoneme1 rdf:type owl:NamedIndividual ,
                     ms:SegmentationLevel ;
            rdfs:label "phoneme"@en .


###  http://w3id.org/meta-share/meta-share/phoneme2
ms:phoneme2 rdf:type owl:NamedIndividual ,
                     ms:SizeUnit ;
            rdfs:label "phoneme"@en .


###  http://w3id.org/meta-share/meta-share/phoneticUnit
ms:phoneticUnit rdf:type owl:NamedIndividual ,
                         ms:SizeUnit ;
                rdfs:label "phonetic unit"@en .


###  http://w3id.org/meta-share/meta-share/phoneticallyBalancedSentence
ms:phoneticallyBalancedSentence rdf:type owl:NamedIndividual ,
                                         ms:SpeechItem ;
                                rdfs:label "phonetically balanced sentence"@en .


###  http://w3id.org/meta-share/meta-share/phoneticallyRichSentence
ms:phoneticallyRichSentence rdf:type owl:NamedIndividual ,
                                     ms:SpeechItem ;
                            rdfs:label "phonetically rich sentence"@en .


###  http://w3id.org/meta-share/meta-share/phoneticallyRichWord
ms:phoneticallyRichWord rdf:type owl:NamedIndividual ,
                                 ms:SpeechItem ;
                        rdfs:label "phonetically rich word"@en .


###  http://w3id.org/meta-share/meta-share/phonetics
ms:phonetics rdf:type owl:NamedIndividual ,
                      ms:EncodingLevel ;
             rdfs:comment "Value for 'EncodingLevel' for the particular linguistic level that relates to the study of speech sounds"@en ;
             rdfs:label "phonetics"@en .


###  http://w3id.org/meta-share/meta-share/phonology
ms:phonology rdf:type owl:NamedIndividual ,
                      ms:EncodingLevel ;
             rdfs:comment "Value for 'EncodingLevel' for the particular linguistic level that relates to the study of speech sounds that constitute the fundamental components of a language"@en ;
             rdfs:label "phonology"@en .


###  http://w3id.org/meta-share/meta-share/photographyComputerArtFilmVideo
ms:photographyComputerArtFilmVideo rdf:type owl:NamedIndividual ,
                                            ms:Domain ;
                                   datacite:hasIdentifier ms:DDC770 ;
                                   rdfs:label "Photography, Computer Art, Film, Video"@en .


###  http://w3id.org/meta-share/meta-share/phrase
ms:phrase rdf:type owl:NamedIndividual ,
                   ms:SegmentationLevel ;
          rdfs:label "phrase"@en .


###  http://w3id.org/meta-share/meta-share/phrase1
ms:phrase1 rdf:type owl:NamedIndividual ,
                    ms:SizeUnit ;
           rdfs:label "phrase"@en .


###  http://w3id.org/meta-share/meta-share/physics
ms:physics rdf:type owl:NamedIndividual ,
                    ms:Domain ;
           datacite:hasIdentifier ms:DDC530 ;
           rdfs:label "Physics"@en .


###  http://w3id.org/meta-share/meta-share/plain
ms:plain rdf:type owl:NamedIndividual ,
                  ms:CapturingEnvironment ;
         rdfs:label "plain"@en .


###  http://w3id.org/meta-share/meta-share/planned
ms:planned rdf:type owl:NamedIndividual ,
                    ms:Naturality ;
           rdfs:label "planned"@en .


###  http://w3id.org/meta-share/meta-share/plants
ms:plants rdf:type owl:NamedIndividual ,
                   ms:Domain ;
          datacite:hasIdentifier ms:DDC580 ;
          rdfs:label "Plants"@en .


###  http://w3id.org/meta-share/meta-share/plugin
ms:plugin rdf:type owl:NamedIndividual ,
                   ms:SoftwareDistributionForm ;
          rdfs:comment "Value for software distribution form, used for software objects in the form of plugins (e.g. Chrome browser extension)"@en ;
          rdfs:label "plugin"@en .


###  http://w3id.org/meta-share/meta-share/pmcid
ms:pmcid rdf:type owl:NamedIndividual ,
                  ms:DocumentIdentifierScheme ;
         ms:url "https://www.ncbi.nlm.nih.gov/pmc/pmctopmid/" ;
         rdfs:comment "Value for resourceIdentifierSchemeName, referring to the PMCID (PubMed Central Identifier, https://www.ncbi.nlm.nih.gov/pmc/pmctopmid/)"@en ;
         rdfs:label "PMCID"@en ;
         skos:altLabel "PubMed Central Identifier"@en .


###  http://w3id.org/meta-share/meta-share/pmid
ms:pmid rdf:type owl:NamedIndividual ,
                 ms:DocumentIdentifierScheme ;
        ms:url "https://www.ncbi.nlm.nih.gov/pmc/pmctopmid/" ;
        rdfs:comment "Value for resourceIdentifierSchemeName, referring to the PMID (PubMed Identifier, https://www.ncbi.nlm.nih.gov/pmc/pmctopmid/)"@en ;
        rdfs:label "PMID"@en ;
        skos:altLabel "PubMed Identifier"@en .


###  http://w3id.org/meta-share/meta-share/politicalScience
ms:politicalScience rdf:type owl:NamedIndividual ,
                             ms:Domain ;
                    datacite:hasIdentifier ms:DDC320 ;
                    rdfs:label "Political Science"@en .


###  http://w3id.org/meta-share/meta-share/politics
ms:politics rdf:type owl:NamedIndividual ,
                     ms:Domain ;
            datacite:hasIdentifier ms:ELG_Domain017 ;
            rdfs:label "politics"@en .


###  http://w3id.org/meta-share/meta-share/ppAttachment
ms:ppAttachment rdf:type owl:NamedIndividual ,
                         ms:GrammaticalPhenomenaCoverage ;
                rdfs:label "PP attachment"@en ;
                skos:altLabel "Attachment of Prepositional phrases"@en .


###  http://w3id.org/meta-share/meta-share/pragmatics
ms:pragmatics rdf:type owl:NamedIndividual ,
                       ms:EncodingLevel ;
              rdfs:comment "Value for 'EncodingLevel' for the particular linguistic level of analysis that studies the relationship of sentences to the environment in which they occur"@en ;
              rdfs:label "pragmatics"@en .


###  http://w3id.org/meta-share/meta-share/pragueTreebank
ms:pragueTreebank rdf:type owl:NamedIndividual ,
                           ms:StandardBestPractice ;
                  ms:url "http://ufal.mff.cuni.cz/pdt2.0/" ;
                  rdfs:label "Prague treebank"@en ;
                  skos:altLabel "PDT"@en ,
                                "Prague Dependency Treebank"@en .


###  http://w3id.org/meta-share/meta-share/predicate
ms:predicate rdf:type owl:NamedIndividual ,
                      ms:SizeUnit ;
             rdfs:label "predicate"@en .


###  http://w3id.org/meta-share/meta-share/presentation
ms:presentation rdf:type owl:NamedIndividual ,
                         ms:SpeechGenre ;
                datacite:hasIdentifier ms:MS_SG003 ;
                rdfs:label "presentation"@en .


###  http://w3id.org/meta-share/meta-share/private
ms:private rdf:type owl:NamedIndividual ,
                    ms:TextGenre ;
           datacite:hasIdentifier ms:PAROLE_G007 ;
           rdfs:label "private"@en .


###  http://w3id.org/meta-share/meta-share/proceedings
ms:proceedings rdf:type owl:NamedIndividual ,
                        ms:DocumentType ;
               rdfs:label "proceedings"@en .


###  http://w3id.org/meta-share/meta-share/processable
ms:processable rdf:type owl:NamedIndividual ,
                        ms:AccessRightsStatement ;
               rdfs:comment "Value for access rights; for data resources whose licence permits their processing (resulting in research outputs)"@en ;
               rdfs:label "processable"@en .


###  http://w3id.org/meta-share/meta-share/prompted
ms:prompted rdf:type owl:NamedIndividual ,
                     ms:Naturality ;
            rdfs:label "prompted"@en .


###  http://w3id.org/meta-share/meta-share/properNoun
ms:properNoun rdf:type owl:NamedIndividual ,
                       ms:SpeechItem ;
              rdfs:label "proper noun"@en .


###  http://w3id.org/meta-share/meta-share/prosodicBoundary
ms:prosodicBoundary rdf:type owl:NamedIndividual ,
                             ms:SegmentationLevel ;
                    rdfs:label "prosodic boundary"@en .


###  http://w3id.org/meta-share/meta-share/psychology
ms:psychology rdf:type owl:NamedIndividual ,
                       ms:Domain ;
              datacite:hasIdentifier ms:DDC150 ;
              rdfs:label "Psychology"@en .


###  http://w3id.org/meta-share/meta-share/public
ms:public rdf:type owl:NamedIndividual ,
                   ms:LicenceCategory ;
          ms:conformsTo ms:ClarinLicenceCategoryScheme ;
          rdfs:label "public"@en ;
          skos:altLabel "PUB"@en .


###  http://w3id.org/meta-share/meta-share/publicAdministration
ms:publicAdministration rdf:type owl:NamedIndividual ,
                                 ms:Domain ;
                        datacite:hasIdentifier ms:ELG_Domain007 ;
                        rdfs:label "public administration"@en .


###  http://w3id.org/meta-share/meta-share/publicAdministration1
ms:publicAdministration1 rdf:type owl:NamedIndividual ,
                                  ms:Domain ;
                         datacite:hasIdentifier ms:DDC351 ;
                         rdfs:label "Public Administration"@en .


###  http://w3id.org/meta-share/meta-share/publicOrganization
ms:publicOrganization rdf:type owl:NamedIndividual ,
                               ms:OrganizationLegalStatus ;
                      rdfs:label "public organization"@en .


###  http://w3id.org/meta-share/meta-share/publication
ms:publication rdf:type owl:NamedIndividual ,
                        ms:DocumentationType ;
               rdfs:comment "Value for 'Documentation type' used for published documents about a language resource (mainly meant for documents that describe the resource itself rather than its deployment)"@en ,
                            "Value for licence category; for licences that allow access to resources only for logged in users that have fulfilled further requirements (e.g. paid the fees for a commercial licence)"@en ;
               rdfs:label "publication"@en .


###  http://w3id.org/meta-share/meta-share/publicationForCitation
ms:publicationForCitation rdf:type owl:NamedIndividual ,
                                   ms:DocumentationType ;
                          rdfs:comment "Value for 'Documentation type' for a published document describing the language resource and which is recommended by the resource creator(s) to be used for citation purposes when the resource is mentioned in another publication"@en ;
                          rdfs:label "publication for citation"@en .


###  http://w3id.org/meta-share/meta-share/published
ms:published rdf:type owl:NamedIndividual ,
                      ms:VersionType ;
             rdfs:comment "Value for 'Version type' used for versions as published in digital or print form"@en ;
             rdfs:label "published"@en .


###  http://w3id.org/meta-share/meta-share/publishedRecord
ms:publishedRecord rdf:type owl:NamedIndividual ,
                            ms:SizeUnit ;
                   rdfs:label "published record"@en .


###  http://w3id.org/meta-share/meta-share/publishing
ms:publishing rdf:type owl:NamedIndividual ,
                       ms:Domain ;
              datacite:hasIdentifier ms:ELG_Domain001 ;
              rdfs:label "publishing"@en .


###  http://w3id.org/meta-share/meta-share/qualiaStructure
ms:qualiaStructure rdf:type owl:NamedIndividual ,
                            skos:Concept ;
                   rdfs:label "qualia structure"@en ;
                   skos:broader ms:SemanticType ;
                   skos:inScheme ms:ContentTypeScheme .


###  http://w3id.org/meta-share/meta-share/question
ms:question rdf:type owl:NamedIndividual ,
                     ms:SizeUnit ;
            rdfs:label "question"@en .


###  http://w3id.org/meta-share/meta-share/questionAnswer
ms:questionAnswer rdf:type owl:NamedIndividual ,
                           ms:SpeechGenre ;
                  datacite:hasIdentifier ms:MS_SG004 ;
                  rdfs:label "question answer"@en .


###  http://w3id.org/meta-share/meta-share/radio
ms:radio rdf:type owl:NamedIndividual ,
                  ms:SourceChannel ;
         rdfs:label "radio"@en .


###  http://w3id.org/meta-share/meta-share/randomForest
ms:randomForest rdf:type owl:NamedIndividual ,
                         ms:ModelType ;
                rdfs:label "random forest"@en ;
                skos:altLabel "random decision forest"@en ;
                skos:broader ms:nonDeepLearningModel .


###  http://w3id.org/meta-share/meta-share/raster
ms:raster rdf:type owl:NamedIndividual ,
                   ms:RasterOrVectorGraphics ;
          rdfs:label "raster"@en .


###  http://w3id.org/meta-share/meta-share/rawCorpus
ms:rawCorpus rdf:type owl:NamedIndividual ,
                      ms:CorpusSubclass ;
             rdfs:comment "The form of the corpus that has not been enriched with annotations"@en ;
             rdfs:label "raw corpus"@en .


###  http://w3id.org/meta-share/meta-share/re3data
ms:re3data rdf:type owl:NamedIndividual ,
                    ms:RepositoryIdentifierScheme ;
           rdfs:label "re3data"@en .


###  http://w3id.org/meta-share/meta-share/readSpeech
ms:readSpeech rdf:type owl:NamedIndividual ,
                       ms:Naturality ;
              rdfs:label "read speech"@en .


###  http://w3id.org/meta-share/meta-share/realAudio
ms:realAudio rdf:type owl:NamedIndividual ,
                      ms:CompressionName ;
             rdfs:label "real audio"@en .


###  http://w3id.org/meta-share/meta-share/recurrentNeuralNetwork
ms:recurrentNeuralNetwork rdf:type owl:NamedIndividual ,
                                   ms:ModelType ;
                          rdfs:label "recurrent neural network"@en ;
                          skos:altLabel "RNN"@en ;
                          skos:broader ms:DeepLearningModel .


###  http://w3id.org/meta-share/meta-share/redeposit
ms:redeposit rdf:type owl:NamedIndividual ,
                      ms:ConditionOfUse ,
                      odrl:Set ;
             rdfs:comment "Value for 'ConditionsOfUse' which states that users are encouraged to deposit any modified versions of the resource they make to the distribution channel through which they have acquired the resource"@en ;
             rdfs:label "redeposit"@en ;
             odrl:permission [ odrl:duty [ odrl:action ms:redeposit
                                         ]
                             ] .


###  http://w3id.org/meta-share/meta-share/reflexivity
ms:reflexivity rdf:type owl:NamedIndividual ,
                        skos:Concept ;
               rdfs:label "reflexivity"@en ;
               skos:broader ms:MorphologicalType ;
               skos:inScheme ms:ContentTypeScheme .


###  http://w3id.org/meta-share/meta-share/regionalFunds
ms:regionalFunds rdf:type owl:NamedIndividual ,
                          ms:FundingType ;
                 rdfs:comment "Value for 'Funding type' for projects financed by regional authorities"@en ;
                 rdfs:label "regional funds"@en .


###  http://w3id.org/meta-share/meta-share/register1
ms:register1 rdf:type owl:NamedIndividual ,
                      skos:Concept ;
             rdfs:label "register"@en ;
             skos:broader ms:UsageType ;
             skos:inScheme ms:ContentTypeScheme .


###  http://w3id.org/meta-share/meta-share/religion
ms:religion rdf:type owl:NamedIndividual ,
                     ms:Domain ;
            datacite:hasIdentifier ms:DDC200 ;
            rdfs:label "Religion"@en .


###  http://w3id.org/meta-share/meta-share/requestPlan
ms:requestPlan rdf:type owl:NamedIndividual ,
                        ms:ConditionOfUse ;
               rdfs:comment "Value for 'ConditionOfUse' that states that the licensor requires the submission of a research plan in order to grant access to the language resource"@en ;
               rdfs:label "request plan"@en .


###  http://w3id.org/meta-share/meta-share/requiresUserAuthentication
ms:requiresUserAuthentication rdf:type owl:NamedIndividual ,
                                       ms:LicenceCategory ;
                              rdfs:comment "Value for licence category; for licences for resources that can be access only by logged in users"@en ;
                              rdfs:label "requires user authentication"@en .


###  http://w3id.org/meta-share/meta-share/requiresUserAuthorization
ms:requiresUserAuthorization rdf:type owl:NamedIndividual ,
                                      ms:LicenceCategory .


###  http://w3id.org/meta-share/meta-share/researchOrganization
ms:researchOrganization rdf:type owl:NamedIndividual ,
                                 ms:OrganizationRole ;
                        rdfs:label "research organization"@en .


###  http://w3id.org/meta-share/meta-share/researchUse
ms:researchUse rdf:type owl:NamedIndividual ,
                        ms:ConditionOfUse ;
               rdfs:comment "Value for 'ConditionOfUse' stating that the resource can be used only for research purposes"@en ;
               rdfs:label "research use"@en ;
               skos:note "add ODRL"@en .


###  http://w3id.org/meta-share/meta-share/restricted
ms:restricted rdf:type owl:NamedIndividual ,
                       ms:LicenceCategory ;
              ms:conformsTo ms:ClarinLicenceCategoryScheme ;
              rdfs:label "restricted"@en ;
              skos:altLabel "RES"@en .


###  http://w3id.org/meta-share/meta-share/restrictedAccess
ms:restrictedAccess rdf:type owl:NamedIndividual ,
                             ms:AccessRightsStatement ;
                    datacite:hasIdentifier ms:omtdAccess1 ;
                    rdfs:comment "Access is subject to restrictions or controls regarding users (e.g., limited to researchers or members of a specific group) or use (e.g., for research only, noncommercial use, etc.); subscription or registration may also be required and access may incur financial costs"@en ;
                    rdfs:label "restricted access"@en .


###  http://w3id.org/meta-share/meta-share/restrictedAccess1
ms:restrictedAccess1 rdf:type owl:NamedIndividual ,
                              ms:AccessRightsStatement ;
                     datacite:hasIdentifier <http://purl.org/coar/access_right/c_16ec> .


###  http://w3id.org/meta-share/meta-share/review
ms:review rdf:type owl:NamedIndividual ,
                   ms:TextType ;
          datacite:hasIdentifier ms:ClarinEl_TT017 ;
          rdfs:label "review"@en .


###  http://w3id.org/meta-share/meta-share/rolePlay
ms:rolePlay rdf:type owl:NamedIndividual ,
                     ms:ScenarioType ;
            rdfs:label "role play"@en .


###  http://w3id.org/meta-share/meta-share/roundtable
ms:roundtable rdf:type owl:NamedIndividual ,
                       ms:SpeechGenre ;
              datacite:hasIdentifier ms:MS_SG005 ;
              rdfs:label "roundtable"@en .


###  http://w3id.org/meta-share/meta-share/rule
ms:rule rdf:type owl:NamedIndividual ,
                 ms:SizeUnit ;
        rdfs:label "rule"@en .


###  http://w3id.org/meta-share/meta-share/samples
ms:samples rdf:type owl:NamedIndividual ,
                    ms:DocumentationType ;
           rdfs:comment "Value for 'DocumentationType' used for samples of a language resource"@en ;
           rdfs:label "samples"@en .


###  http://w3id.org/meta-share/meta-share/scene
ms:scene rdf:type owl:NamedIndividual ,
                  ms:SegmentationLevel ;
         rdfs:label "scene"@en .


###  http://w3id.org/meta-share/meta-share/scholarlyCommunication
ms:scholarlyCommunication rdf:type owl:NamedIndividual ,
                                   ms:Domain ;
                          datacite:hasIdentifier ms:Clarin_Domain006 ;
                          rdfs:comment "Scholarly communication can be defined as “the system through which research and other scholarly writings are created, evaluated for quality, disseminated to the scholarly community, and preserved for future use. The system includes both formal means of communication, such as publication in peer-reviewed journals, and informal channels, such as electronic listservs.” (Association of College & Research Libraries, “Principles and Strategies for the Reform of Scholarly Communication 1,” 2003)"@en ;
                          rdfs:label "scholarly communication"@en .


###  http://w3id.org/meta-share/meta-share/school
ms:school rdf:type owl:NamedIndividual ,
                   ms:DivisionCategory ;
          rdfs:label "school"@en .


###  http://w3id.org/meta-share/meta-share/science
ms:science rdf:type owl:NamedIndividual ,
                    ms:Domain ;
           datacite:hasIdentifier ms:DDC500 ;
           rdfs:label "Science"@en .


###  http://w3id.org/meta-share/meta-share/scopusId
ms:scopusId rdf:type owl:NamedIndividual ,
                     datacite:PersonalIdentifierScheme ;
            rdfs:comment "Value for personIdentifierSchemeName, referring to the Scopus identifier for authors (https://www.scopus.com)"@en ;
            rdfs:label "Scopus ID"@en .


###  http://w3id.org/meta-share/meta-share/script
ms:script rdf:type owl:NamedIndividual ,
                   ms:TextType ;
          datacite:hasIdentifier ms:ClarinEl_TT010 ;
          rdfs:label "script"@en .


###  http://w3id.org/meta-share/meta-share/sculptureCeramicsAndMetalwork
ms:sculptureCeramicsAndMetalwork rdf:type owl:NamedIndividual ,
                                          ms:Domain ;
                                 datacite:hasIdentifier ms:DDC730 ;
                                 rdfs:label "Sculpture, Ceramics and Metalwork"@en .


###  http://w3id.org/meta-share/meta-share/second
ms:second rdf:type owl:NamedIndividual ,
                   ms:SizeUnit ;
          rdfs:label "second"@en .


###  http://w3id.org/meta-share/meta-share/second1
ms:second1 rdf:type owl:NamedIndividual ,
                    ms:DurationUnit ;
           rdfs:label "second"@en .


###  http://w3id.org/meta-share/meta-share/segment
ms:segment rdf:type owl:NamedIndividual ,
                    ms:SizeUnit ;
           rdfs:label "segment"@en .


###  http://w3id.org/meta-share/meta-share/semanticClass
ms:semanticClass rdf:type owl:NamedIndividual ,
                          skos:Concept ;
                 rdfs:label "semantic class"@en ;
                 skos:broader ms:SemanticType ;
                 skos:inScheme ms:ContentTypeScheme .


###  http://w3id.org/meta-share/meta-share/semanticFeature
ms:semanticFeature rdf:type owl:NamedIndividual ,
                            skos:Concept ;
                   rdfs:label "semantic feature"@en ;
                   skos:altLabel "semantic trait"@en ;
                   skos:broader ms:SemanticType ;
                   skos:inScheme ms:ContentTypeScheme .


###  http://w3id.org/meta-share/meta-share/semanticRelation
ms:semanticRelation rdf:type owl:NamedIndividual ,
                             skos:Concept ;
                    rdfs:label "semantic relation"@en ;
                    skos:broader ms:SemanticType ;
                    skos:inScheme ms:ContentTypeScheme .


###  http://w3id.org/meta-share/meta-share/semanticRole
ms:semanticRole rdf:type owl:NamedIndividual ,
                         skos:Concept ;
                rdfs:label "semantic role"@en ;
                skos:broader ms:SemanticType ;
                skos:inScheme ms:ContentTypeScheme .


###  http://w3id.org/meta-share/meta-share/semanticUnit
ms:semanticUnit rdf:type owl:NamedIndividual ,
                         ms:ExtratextualInformationUnit ;
                rdfs:label "semantic unit"@en .


###  http://w3id.org/meta-share/meta-share/semanticUnit1
ms:semanticUnit1 rdf:type owl:NamedIndividual ,
                          ms:SizeUnit ;
                 rdfs:label "semantic unit"@en .


###  http://w3id.org/meta-share/meta-share/semantics
ms:semantics rdf:type owl:NamedIndividual ,
                      ms:EncodingLevel ;
             rdfs:comment "Value for 'EncodingLevel' for the particular linguistic level of analysis that relates to the meaning of a word, phrase, etc."@en ;
             rdfs:label "semantics"@en .


###  http://w3id.org/meta-share/meta-share/semiInteractive
ms:semiInteractive rdf:type owl:NamedIndividual ,
                            ms:Interactivity ;
                   rdfs:label "semi-interactive"@en .


###  http://w3id.org/meta-share/meta-share/semiPlanned
ms:semiPlanned rdf:type owl:NamedIndividual ,
                        ms:Naturality ;
               rdfs:label "semi-planned"@en .


###  http://w3id.org/meta-share/meta-share/sentence
ms:sentence rdf:type owl:NamedIndividual ,
                     ms:SegmentationLevel ;
            rdfs:label "sentence"@en .


###  http://w3id.org/meta-share/meta-share/sentence1
ms:sentence1 rdf:type owl:NamedIndividual ,
                      ms:SizeUnit ;
             rdfs:label "sentence"@en .


###  http://w3id.org/meta-share/meta-share/sentenceTransformer
ms:sentenceTransformer rdf:type owl:NamedIndividual ,
                                ms:MLFramework ;
                       rdfs:comment "Special case of transformers tuned for sentences"@en ;
                       rdfs:label "sentence transformer"@en .


###  http://w3id.org/meta-share/meta-share/serviceContract
ms:serviceContract rdf:type owl:NamedIndividual ,
                            ms:FundingType ;
                   rdfs:comment "Value for 'Funding type' for projects financed under service contracts"@en ;
                   rdfs:label "service contract"@en .


###  http://w3id.org/meta-share/meta-share/shareAlike
ms:shareAlike rdf:type owl:NamedIndividual ,
                       ms:ConditionOfUse ,
                       odrl:Set ;
              rdfs:comment "Value for 'ConditionOfUse' that states that the derivatives of the language resource must be distributed with the same or a compatible licence"@en ;
              rdfs:label "share alike"@en ;
              odrl:permission [ odrl:duty [ odrl:action cc:ShareALike
                                          ]
                              ] .


###  http://w3id.org/meta-share/meta-share/shorten
ms:shorten rdf:type owl:NamedIndividual ,
                    ms:CompressionName ;
           rdfs:label "shorten"@en .


###  http://w3id.org/meta-share/meta-share/shot
ms:shot rdf:type owl:NamedIndividual ,
                 ms:SegmentationLevel ;
        rdfs:label "shot"@en .


###  http://w3id.org/meta-share/meta-share/shot1
ms:shot1 rdf:type owl:NamedIndividual ,
                  ms:SizeUnit ;
         rdfs:label "shot"@en .


###  http://w3id.org/meta-share/meta-share/signLanguage
ms:signLanguage rdf:type owl:NamedIndividual ,
                         ms:ModalityType ;
                rdfs:comment "Value for 'ModalityType' for sign languages represented in a language resource"@en ;
                rdfs:label "sign language"@en .


###  http://w3id.org/meta-share/meta-share/signal
ms:signal rdf:type owl:NamedIndividual ,
                   ms:SegmentationLevel ;
          rdfs:label "signal"@en .


###  http://w3id.org/meta-share/meta-share/signedInteger
ms:signedInteger rdf:type owl:NamedIndividual ,
                          ms:SignConvention ;
                 rdfs:label "signed integer"@en .


###  http://w3id.org/meta-share/meta-share/singleSource
ms:singleSource rdf:type owl:NamedIndividual ,
                         ms:SceneIllumination ;
                rdfs:label "single source"@en .


###  http://w3id.org/meta-share/meta-share/sleepDeprivation
ms:sleepDeprivation rdf:type owl:NamedIndividual ,
                             ms:SpeechInfluence ;
                    rdfs:label "sleep deprivation"@en .


###  http://w3id.org/meta-share/meta-share/sme
ms:sme rdf:type owl:NamedIndividual ,
                ms:OrganizationLegalStatus ;
       rdfs:label "SME"@en .


###  http://w3id.org/meta-share/meta-share/socialProblemsAndSocialServices
ms:socialProblemsAndSocialServices rdf:type owl:NamedIndividual ,
                                            ms:Domain ;
                                   datacite:hasIdentifier ms:DDC360 ;
                                   rdfs:label "Social Problems & Social Services"@en .


###  http://w3id.org/meta-share/meta-share/socialSciences
ms:socialSciences rdf:type owl:NamedIndividual ,
                           ms:Domain ;
                  datacite:hasIdentifier ms:DDC300 ;
                  rdfs:comment "The social sciences are academic disciplines concerned with the study of the social life of human groups and individuals including anthropology, economics, geography, history, political science, psychology, social studies, and sociology. The social sciences consist of the scientific study of the human aspects of the world.[https://en.wikipedia.org/wiki/Category:Social_sciences"@en ;
                  rdfs:label "Social Sciences"@en .


###  http://w3id.org/meta-share/meta-share/society
ms:society rdf:type owl:NamedIndividual ,
                    ms:OrganizationLegalStatus ;
           rdfs:label "society"@en .


###  http://w3id.org/meta-share/meta-share/sociologyAndAnthropology
ms:sociologyAndAnthropology rdf:type owl:NamedIndividual ,
                                     ms:Domain ;
                            datacite:hasIdentifier ms:DDC301 ;
                            rdfs:label "Sociology & Anthropology"@en .


###  http://w3id.org/meta-share/meta-share/some
ms:some rdf:type owl:NamedIndividual ,
                 ms:Audience ;
        rdfs:label "some"@en .


###  http://w3id.org/meta-share/meta-share/song
ms:song rdf:type owl:NamedIndividual ,
                 ms:AudioGenre ;
        datacite:hasIdentifier ms:MS_AG004 ;
        rdfs:label "song"@en .


###  http://w3id.org/meta-share/meta-share/sound
ms:sound rdf:type owl:NamedIndividual ,
                  ms:NonSpeechItem ;
         rdfs:label "sound"@en .


###  http://w3id.org/meta-share/meta-share/soundBlasterCard
ms:soundBlasterCard rdf:type owl:NamedIndividual ,
                             ms:RecordingDeviceType ;
                    rdfs:label "Sound blaster card"@en .


###  http://w3id.org/meta-share/meta-share/soundRecording
ms:soundRecording rdf:type owl:NamedIndividual ,
                           ms:ExtratextualInformation ;
                  rdfs:label "sound recording"@en .


###  http://w3id.org/meta-share/meta-share/sourceAndExecutableCode
ms:sourceAndExecutableCode rdf:type owl:NamedIndividual ,
                                    ms:SoftwareDistributionForm ;
                           rdfs:comment "Value for software distribution form, used for software that is available from the same location both as source code and executable program"@en ;
                           rdfs:label "source and executable code"@en .


###  http://w3id.org/meta-share/meta-share/sourceCode
ms:sourceCode rdf:type owl:NamedIndividual ,
                       ms:SoftwareDistributionForm ;
              rdfs:comment "Value for software distribution form, used for software objects in the form of source code, i.e. as files with the commands ready to be compiled or assembled into an executable computer program"@en ;
              rdfs:label "source code"@en .


###  http://w3id.org/meta-share/meta-share/spaCy
ms:spaCy rdf:type owl:NamedIndividual ,
                  ms:NLPFramework .


###  http://w3id.org/meta-share/meta-share/spatialConstraint
ms:spatialConstraint rdf:type owl:NamedIndividual ,
                              ms:ConditionOfUse ;
                     rdfs:comment "Value for 'ConditionsOfUse' which is used for resources with spatial restrictions, e.g., in cases where the content is available or can be used only at a single location, center, or site"@en ;
                     rdfs:label "spatial constraint"@en .


###  http://w3id.org/meta-share/meta-share/speakerNoise
ms:speakerNoise rdf:type owl:NamedIndividual ,
                         ms:AnnotatedElement ;
                rdfs:label "speaker noise"@en .


###  http://w3id.org/meta-share/meta-share/specialHardwareEquipment
ms:specialHardwareEquipment rdf:type owl:NamedIndividual ,
                                     ms:RequiredHardware ;
                            rdfs:label "special hardware equipment"@en .


###  http://w3id.org/meta-share/meta-share/speech
ms:speech rdf:type owl:NamedIndividual ,
                   ms:AudioGenre ;
          datacite:hasIdentifier ms:MS_AG003 ;
          rdfs:label "speech"@en .


###  http://w3id.org/meta-share/meta-share/spokenLanguage
ms:spokenLanguage rdf:type owl:NamedIndividual ,
                           ms:ModalityType ;
                  rdfs:comment "Value for 'ModalityType' for language resources including spoken language words and expressions"@en ;
                  rdfs:label "spoken language"@en .


###  http://w3id.org/meta-share/meta-share/spontaneous
ms:spontaneous rdf:type owl:NamedIndividual ,
                        ms:Naturality ;
               rdfs:label "spontaneous"@en .


###  http://w3id.org/meta-share/meta-share/sportsGamesAndEntertainment
ms:sportsGamesAndEntertainment rdf:type owl:NamedIndividual ,
                                        ms:Domain ;
                               datacite:hasIdentifier ms:DDC790 ;
                               rdfs:label "Sports, Games & Entertainment"@en .


###  http://w3id.org/meta-share/meta-share/standardizationBody
ms:standardizationBody rdf:type owl:NamedIndividual ,
                                ms:OrganizationRole ;
                       rdfs:label "standardization body"@en .


###  http://w3id.org/meta-share/meta-share/statisticalProperty
ms:statisticalProperty rdf:type owl:NamedIndividual ,
                                skos:Concept ;
                       rdfs:label "statistical property"@en ;
                       skos:inScheme ms:ContentTypeScheme .


###  http://w3id.org/meta-share/meta-share/statistics
ms:statistics rdf:type owl:NamedIndividual ,
                       ms:Domain ;
              datacite:hasIdentifier ms:DDC310 ;
              rdfs:label "Statistics"@en .


###  http://w3id.org/meta-share/meta-share/string
ms:string rdf:type owl:NamedIndividual ,
                   ms:ParameterType ;
          rdfs:label "string"@en .


###  http://w3id.org/meta-share/meta-share/studio
ms:studio rdf:type owl:NamedIndividual ,
                   ms:RecordingEnvironment ;
          rdfs:label "studio"@en .


###  http://w3id.org/meta-share/meta-share/studioEquipment
ms:studioEquipment rdf:type owl:NamedIndividual ,
                            ms:CapturingDeviceType ;
                   rdfs:label "studio equipment"@en .


###  http://w3id.org/meta-share/meta-share/subcatFrame
ms:subcatFrame rdf:type owl:NamedIndividual ,
                        skos:Concept ;
               rdfs:label "subcategorization frame"@en ;
               skos:broader ms:SyntacticType ;
               skos:inScheme ms:ContentTypeScheme .


###  http://w3id.org/meta-share/meta-share/submitted
ms:submitted rdf:type owl:NamedIndividual ,
                      ms:VersionType ;
             rdfs:comment "Value for 'Version type' used for versions as submitted for publication"@en ;
             rdfs:label "submitted"@en .


###  http://w3id.org/meta-share/meta-share/subsidiary
ms:subsidiary rdf:type owl:NamedIndividual ,
                       ms:DivisionCategory ;
              rdfs:label "subsidiary"@en .


###  http://w3id.org/meta-share/meta-share/subtitle1
ms:subtitle1 rdf:type owl:NamedIndividual ,
                      ms:TextIncludedInVideo ;
             rdfs:label "subtitle"@en .


###  http://w3id.org/meta-share/meta-share/subtitle2
ms:subtitle2 rdf:type owl:NamedIndividual ,
                      ms:TextIncludedInImage ;
             rdfs:label "subtitle"@en .


###  http://w3id.org/meta-share/meta-share/subtitle3
ms:subtitle3 rdf:type owl:NamedIndividual ,
                      ms:TextType ;
             datacite:hasIdentifier ms:ClarinEl_TT015 ;
             rdfs:label "subtitle"@en .


###  http://w3id.org/meta-share/meta-share/supportVectorMachine
ms:supportVectorMachine rdf:type owl:NamedIndividual ,
                                 ms:ModelType ;
                        rdfs:label "support vector machine"@en ;
                        skos:altLabel "SVM"@en ,
                                      "support vector network"@en ;
                        skos:broader ms:nonDeepLearningModel .


###  http://w3id.org/meta-share/meta-share/syllable
ms:syllable rdf:type owl:NamedIndividual ,
                     ms:BaseItem ;
            rdfs:label "syllable"@en .


###  http://w3id.org/meta-share/meta-share/syllable1
ms:syllable1 rdf:type owl:NamedIndividual ,
                      ms:SegmentationLevel ;
             rdfs:label "syllable"@en .


###  http://w3id.org/meta-share/meta-share/syllable2
ms:syllable2 rdf:type owl:NamedIndividual ,
                      ms:SizeUnit ;
             rdfs:label "syllable"@en .


###  http://w3id.org/meta-share/meta-share/synonym
ms:synonym rdf:type owl:NamedIndividual ,
                    skos:Concept ;
           rdfs:label "synonym"@en ;
           skos:broader ms:SemanticType ;
           skos:inScheme ms:ContentTypeScheme .


###  http://w3id.org/meta-share/meta-share/synset
ms:synset rdf:type owl:NamedIndividual ,
                   ms:SizeUnit ;
          rdfs:label "synset"@en .


###  http://w3id.org/meta-share/meta-share/syntacticUnit
ms:syntacticUnit rdf:type owl:NamedIndividual ,
                          ms:ExtratextualInformationUnit ;
                 rdfs:label "syntactic unit"@en .


###  http://w3id.org/meta-share/meta-share/syntacticUnit1
ms:syntacticUnit1 rdf:type owl:NamedIndividual ,
                           ms:SizeUnit ;
                  rdfs:label "syntactic unit"@en .


###  http://w3id.org/meta-share/meta-share/syntacticoSemanticLink
ms:syntacticoSemanticLink rdf:type owl:NamedIndividual ,
                                   skos:Concept ;
                          rdfs:label "syntactico-semantic link"@en ;
                          skos:broader ms:SyntacticoSemanticType ;
                          skos:inScheme ms:ContentTypeScheme .


###  http://w3id.org/meta-share/meta-share/syntax
ms:syntax rdf:type owl:NamedIndividual ,
                   ms:EncodingLevel ;
          rdfs:comment "Value for 'EncodingLevel' for the particular linguistic level that relates to the study of the structure of linguistic units (phrases, sentences)"@en ;
          rdfs:label "syntax"@en .


###  http://w3id.org/meta-share/meta-share/systemEvaluator
ms:systemEvaluator rdf:type owl:NamedIndividual ,
                            ms:OrganizationRole ;
                   rdfs:label "system evaluator"@en .


###  http://w3id.org/meta-share/meta-share/tagset1
ms:tagset1 rdf:type owl:NamedIndividual ,
                    ms:CompatibleLexiconType ,
                    ms:LCRSubclass ;
           rdfs:comment "a flat list of valid values (tags) designed to annotate data; it usually corresponds to a specific annotation type or set of annotation types"@en ;
           rdfs:label "tagset"@en .


###  http://w3id.org/meta-share/meta-share/tapeVHS
ms:tapeVHS rdf:type owl:NamedIndividual ,
                    ms:RecordingDeviceType ;
           rdfs:label "VHS tape"@en .


###  http://w3id.org/meta-share/meta-share/tb
ms:tb rdf:type owl:NamedIndividual ,
               ms:SizeUnit ;
      rdfs:label "terabyte"@en ;
      skos:altLabel "tb"@en .


###  http://w3id.org/meta-share/meta-share/techReport
ms:techReport rdf:type owl:NamedIndividual ,
                       ms:DocumentType ;
              rdfs:label "technical report"@en .


###  http://w3id.org/meta-share/meta-share/technicalText
ms:technicalText rdf:type owl:NamedIndividual ,
                          ms:TextType ;
                 datacite:hasIdentifier ms:ClarinEl_TT011 ;
                 rdfs:label "technical text"@en .


###  http://w3id.org/meta-share/meta-share/technological
ms:technological rdf:type owl:NamedIndividual ,
                          ms:EvaluationLevel ;
                 rdfs:label "technological"@en .


###  http://w3id.org/meta-share/meta-share/technology
ms:technology rdf:type owl:NamedIndividual ,
                       ms:Domain ;
              datacite:hasIdentifier ms:DDC600 ;
              rdfs:label "Technology"@en .


###  http://w3id.org/meta-share/meta-share/teenager
ms:teenager rdf:type owl:NamedIndividual ,
                     ms:AgeGroup ;
            rdfs:label "teenager"@en .


###  http://w3id.org/meta-share/meta-share/telecommunications
ms:telecommunications rdf:type owl:NamedIndividual ,
                               ms:Domain ;
                      datacite:hasIdentifier ms:ELG_Domain004 ;
                      rdfs:label "telecommunications"@en .


###  http://w3id.org/meta-share/meta-share/telephone
ms:telephone rdf:type owl:NamedIndividual ,
                      ms:SourceChannel ;
             rdfs:label "telephone"@en .


###  http://w3id.org/meta-share/meta-share/telephoneConversation
ms:telephoneConversation rdf:type owl:NamedIndividual ,
                                  ms:TextType ;
                         datacite:hasIdentifier ms:ClarinEl_TT005 ;
                         rdfs:label "telephone conversation"@en .


###  http://w3id.org/meta-share/meta-share/telephoneFixed
ms:telephoneFixed rdf:type owl:NamedIndividual ,
                           ms:CapturingDeviceType ;
                  rdfs:label "fixed telephone"@en .


###  http://w3id.org/meta-share/meta-share/telephoneIP
ms:telephoneIP rdf:type owl:NamedIndividual ,
                        ms:CapturingDeviceType ;
               rdfs:label "IP telephone"@en .


###  http://w3id.org/meta-share/meta-share/telephoneMobile
ms:telephoneMobile rdf:type owl:NamedIndividual ,
                            ms:CapturingDeviceType ;
                   rdfs:label "mobile telephone"@en .


###  http://w3id.org/meta-share/meta-share/telephoneNumber
ms:telephoneNumber rdf:type owl:NamedIndividual ,
                            ms:SpeechItem .


###  http://w3id.org/meta-share/meta-share/tempo
ms:tempo rdf:type owl:NamedIndividual ,
                  ms:NonSpeechItem ;
         rdfs:label "tempo"@en .


###  http://w3id.org/meta-share/meta-share/tense
ms:tense rdf:type owl:NamedIndividual ,
                  skos:Concept ;
         rdfs:label "tense"@en ;
         skos:broader ms:MorphologicalType ;
         skos:inScheme ms:ContentTypeScheme .


###  http://w3id.org/meta-share/meta-share/term
ms:term rdf:type owl:NamedIndividual ,
                 ms:SizeUnit ;
        rdfs:label "term"@en .


###  http://w3id.org/meta-share/meta-share/terminologicalResource
ms:terminologicalResource rdf:type owl:NamedIndividual ,
                                   ms:LCRSubclass ;
                          rdfs:comment "A lexical resource that lists concepts pertaining to a specific domain"@en ;
                          rdfs:label "terminological resource"@en ;
                          skos:altLabel "term list"@en .


###  http://w3id.org/meta-share/meta-share/text
ms:text rdf:type owl:NamedIndividual ,
                 ms:MediaType ;
        rdfs:comment "Value for 'MediaType' for the written or printed form of a language resource (part)"@en ;
        rdfs:label "text"@en .


###  http://w3id.org/meta-share/meta-share/text1
ms:text1 rdf:type owl:NamedIndividual ,
                  ms:SizeUnit ;
         rdfs:label "text"@en .


###  http://w3id.org/meta-share/meta-share/textNumerical
ms:textNumerical rdf:type owl:NamedIndividual ,
                          ms:MediaType ;
                 rdfs:label "numerical text"@en .


###  http://w3id.org/meta-share/meta-share/thesaurus
ms:thesaurus rdf:type owl:NamedIndividual ,
                      ms:LCRSubclass ;
             rdfs:comment "A reference work that lists words grouped together according to similarity of meaning (containing synonyms and sometimes antonyms) [https://en.wikipedia.org/wiki/Thesaurus]"@en ;
             rdfs:label "thesaurus"@en .


###  http://w3id.org/meta-share/meta-share/titlesParsing
ms:titlesParsing rdf:type owl:NamedIndividual ,
                          ms:LDTask ;
                 rdfs:label "parsing of titles"@en .


###  http://w3id.org/meta-share/meta-share/token
ms:token rdf:type owl:NamedIndividual ,
                  ms:SizeUnit ;
         rdfs:label "token"@en .


###  http://w3id.org/meta-share/meta-share/token1
ms:token1 rdf:type owl:NamedIndividual ,
                   ms:SegmentationLevel ;
          rdfs:label "token"@en .


###  http://w3id.org/meta-share/meta-share/trainingResource
ms:trainingResource rdf:type owl:NamedIndividual ,
                             ms:DocumentationType ;
                    rdfs:comment "Value for 'DocumentationType' used for the training material of a resource (e.g., video tutorials, screencasts, guided tours, etc.)"@en ;
                    rdfs:label "training resource"@en .


###  http://w3id.org/meta-share/meta-share/trainingUse
ms:trainingUse rdf:type owl:NamedIndividual ,
                        ms:ConditionOfUse ;
               rdfs:comment "Value for 'ConditionOfUse' which states that the resource can only be used for training purposes"@en ;
               rdfs:label "training use"@en ;
               skos:note "add ODRL representation"@en .


###  http://w3id.org/meta-share/meta-share/transcription
ms:transcription rdf:type owl:NamedIndividual ,
                          skos:Concept ;
                 rdfs:label "phonetic transcription"@en ;
                 skos:broader ms:AudioType ;
                 skos:inScheme ms:ContentTypeScheme .


###  http://w3id.org/meta-share/meta-share/transformer
ms:transformer rdf:type owl:NamedIndividual ,
                        ms:MLFramework ;
               rdfs:comment """A transformer is a deep learning model that adopts the mechanism of attention, 
differentially weighing the significance of each part of the input data. It is used primarily in the field of natural language processing (NLP) and in computer vision (CV)"""@en ;
               rdfs:label "transformer"@en ;
               skos:note "https://en.wikipedia.org/wiki/Transformer_(machine_learning_model)"@en .


###  http://w3id.org/meta-share/meta-share/transformer1
ms:transformer1 rdf:type owl:NamedIndividual ,
                         ms:ModelType ;
                rdfs:label "transformer"@en ;
                skos:broader ms:DeepLearningModel .


###  http://w3id.org/meta-share/meta-share/translationEquivalent
ms:translationEquivalent rdf:type owl:NamedIndividual ,
                                  skos:Concept ;
                         rdfs:label "translation equivalent"@en ;
                         skos:broader ms:TranslationType ;
                         skos:inScheme ms:ContentTypeScheme .


###  http://w3id.org/meta-share/meta-share/translationUnit
ms:translationUnit rdf:type owl:NamedIndividual ,
                            ms:SizeUnit ;
                   rdfs:label "translation unit"@en ;
                   skos:altLabel "tu"@en .


###  http://w3id.org/meta-share/meta-share/transport
ms:transport rdf:type owl:NamedIndividual ,
                      ms:RecordingEnvironment ;
             rdfs:label "transport"@en .


###  http://w3id.org/meta-share/meta-share/transportation
ms:transportation rdf:type owl:NamedIndividual ,
                           ms:Domain ;
                  datacite:hasIdentifier ms:DDC388 ;
                  rdfs:label "Transportation"@en .


###  http://w3id.org/meta-share/meta-share/travelIndustry
ms:travelIndustry rdf:type owl:NamedIndividual ,
                           ms:Domain ;
                  datacite:hasIdentifier ms:ELG_Domain013 ;
                  rdfs:label "travel industry"@en .


###  http://w3id.org/meta-share/meta-share/trigram
ms:trigram rdf:type owl:NamedIndividual ,
                    ms:SizeUnit ;
           rdfs:label "trigram"@en .


###  http://w3id.org/meta-share/meta-share/triple
ms:triple rdf:type owl:NamedIndividual ,
                   ms:SizeUnit .


###  http://w3id.org/meta-share/meta-share/trl1
ms:trl1 rdf:type owl:NamedIndividual ,
                 ms:TRL ;
        rdfs:comment "Basic principles observed"@en ;
        rdfs:label "TRL1"@en .


###  http://w3id.org/meta-share/meta-share/trl2
ms:trl2 rdf:type owl:NamedIndividual ,
                 ms:TRL ;
        rdfs:comment "Technology concept formulated"@en ;
        rdfs:label "TRL2"@en .


###  http://w3id.org/meta-share/meta-share/trl3
ms:trl3 rdf:type owl:NamedIndividual ,
                 ms:TRL ;
        rdfs:comment "Experimental proof of concept"@en ;
        rdfs:label "TRL3"@en .


###  http://w3id.org/meta-share/meta-share/trl4
ms:trl4 rdf:type owl:NamedIndividual ,
                 ms:TRL ;
        rdfs:comment "Technology validated in lab"@en ;
        rdfs:label "TRL4"@en .


###  http://w3id.org/meta-share/meta-share/trl5
ms:trl5 rdf:type owl:NamedIndividual ,
                 ms:TRL ;
        rdfs:comment "Technology validated in relevant environment (industrially relevant environment in the case of key enabling technologies)"@en ;
        rdfs:label "TRL5"@en .


###  http://w3id.org/meta-share/meta-share/trl6
ms:trl6 rdf:type owl:NamedIndividual ,
                 ms:TRL ;
        rdfs:comment "Technology demonstrated in relevant environment (industrially relevant environment in the case of key enabling technologies)"@en ;
        rdfs:label "TRL6"@en .


###  http://w3id.org/meta-share/meta-share/trl7
ms:trl7 rdf:type owl:NamedIndividual ,
                 ms:TRL ;
        rdfs:comment "System prototype demonstration in operational environment"@en ;
        rdfs:label "TRL7"@en .


###  http://w3id.org/meta-share/meta-share/trl8
ms:trl8 rdf:type owl:NamedIndividual ,
                 ms:TRL ;
        rdfs:comment "System complete and qualified"@en ;
        rdfs:label "TRL8"@en .


###  http://w3id.org/meta-share/meta-share/trl9
ms:trl9 rdf:type owl:NamedIndividual ,
                 ms:TRL ;
        rdfs:comment "Actual system proven in operational environment (competitive manufacturing in the case of key enabling technologies; or in space)"@en ;
        rdfs:label "TRL9"@en .


###  http://w3id.org/meta-share/meta-share/troponym
ms:troponym rdf:type owl:NamedIndividual ,
                     skos:Concept ;
            rdfs:label "troponym"@en ;
            skos:broader ms:SemanticType ;
            skos:inScheme ms:ContentTypeScheme .


###  http://w3id.org/meta-share/meta-share/truncation
ms:truncation rdf:type owl:NamedIndividual ,
                       ms:AnnotatedElement ;
              rdfs:label "truncation"@en .


###  http://w3id.org/meta-share/meta-share/turn
ms:turn rdf:type owl:NamedIndividual ,
                 ms:SizeUnit ;
        rdfs:label "turn"@en .


###  http://w3id.org/meta-share/meta-share/tv
ms:tv rdf:type owl:NamedIndividual ,
               ms:SourceChannel ;
      rdfs:label "tv"@en .


###  http://w3id.org/meta-share/meta-share/tweet
ms:tweet rdf:type owl:NamedIndividual ,
                  ms:TextType ;
         datacite:hasIdentifier ms:ClarinEl_TT007 ;
         rdfs:label "tweet"@en .


###  http://w3id.org/meta-share/meta-share/twitter
ms:twitter rdf:type owl:NamedIndividual ,
                    ms:SocialMediaOccupationalAccountType ;
           rdfs:label "twitter"@en .


###  http://w3id.org/meta-share/meta-share/typesystem1
ms:typesystem1 rdf:type owl:NamedIndividual ,
                        ms:LCRSubclass ;
               rdfs:comment "A set of elements designed to annotate data; it typically contains only a list of annotation types, i.e. specific labels that are used for the annotation (e.g., part-of-speech, person, organization, etc.), and is usually inbuilt in the annotation software"@en ;
               rdfs:label "typesystem"@en .


###  http://w3id.org/meta-share/meta-share/underNegotiation
ms:underNegotiation rdf:type owl:NamedIndividual ,
                             ms:Availability ;
                    rdfs:comment "For resources whose availability is still pending."@en ;
                    rdfs:label "under negotiation"@en .


###  http://w3id.org/meta-share/meta-share/unigram
ms:unigram rdf:type owl:NamedIndividual ,
                    ms:SizeUnit ;
           rdfs:label "unigram"@en .


###  http://w3id.org/meta-share/meta-share/unit
ms:unit rdf:type owl:NamedIndividual ,
                 ms:SizeUnit ;
        rdfs:label "unit"@en .


###  http://w3id.org/meta-share/meta-share/unit1
ms:unit1 rdf:type owl:NamedIndividual ,
                  ms:DivisionCategory ;
         rdfs:label "unit"@en .


###  http://w3id.org/meta-share/meta-share/unix
ms:unix rdf:type owl:NamedIndividual ,
                 ms:OperatingSystem ;
        rdfs:label "UNIX"@en .


###  http://w3id.org/meta-share/meta-share/unknown
ms:unknown rdf:type owl:NamedIndividual ,
                    ms:Origin ;
           rdfs:label "unknown"@en .


###  http://w3id.org/meta-share/meta-share/unknown1
ms:unknown1 rdf:type owl:NamedIndividual ,
                     ms:Sex ,
                     ms:SexOfParticipants ;
            rdfs:label "unknown"@en .


###  http://w3id.org/meta-share/meta-share/unknownA
ms:unknownA rdf:type owl:NamedIndividual ,
                     ms:Anonymized ;
            rdfs:label "unknown"@en .


###  http://w3id.org/meta-share/meta-share/unknownP
ms:unknownP rdf:type owl:NamedIndividual ,
                     ms:PersonalDataIncluded ;
            rdfs:label "unknown"@en .


###  http://w3id.org/meta-share/meta-share/unknownS
ms:unknownS rdf:type owl:NamedIndividual ,
                     ms:SensitiveDataIncluded ;
            rdfs:label "unknown"@en .


###  http://w3id.org/meta-share/meta-share/unpublished
ms:unpublished rdf:type owl:NamedIndividual ,
                        ms:DocumentType ;
               rdfs:label "unpublished"@en .


###  http://w3id.org/meta-share/meta-share/unsignedInteger
ms:unsignedInteger rdf:type owl:NamedIndividual ,
                            ms:SignConvention ;
                   rdfs:label "unsigned integer"@en .


###  http://w3id.org/meta-share/meta-share/unspecified
ms:unspecified rdf:type owl:NamedIndividual ,
                        datacite:FunderIdentifierScheme ,
                        datacite:OrganizationIdentifierScheme ,
                        datacite:PersonalIdentifierScheme ,
                        ms:AnnotatedElement ,
                        ms:AudioGenre ,
                        ms:AudioGenreClassificationScheme ,
                        ms:AudioQualityMeasureIncluded ,
                        ms:BaseItem ,
                        ms:CapturingDeviceType ,
                        ms:CompatibleLexiconType ,
                        ms:CompressionName ,
                        ms:ConditionOfUse ,
                        ms:CorpusSubclass ,
                        ms:Currency ,
                        ms:DatasetDistributionForm ,
                        ms:DevelopmentFramework ,
                        ms:DivisionCategory ,
                        ms:DocumentIdentifierScheme ,
                        ms:DocumentType ,
                        ms:DocumentationType ,
                        ms:Domain ,
                        ms:DomainClassificationScheme ,
                        ms:EncodingLevel ,
                        ms:ExtratextualInformation ,
                        ms:ExtratextualInformationUnit ,
                        ms:Framework ,
                        ms:FundingType ,
                        ms:GrammaticalPhenomenaCoverage ,
                        ms:ImageGenreClassificationScheme ,
                        ms:Interactivity ,
                        ms:LCRSubclass ,
                        ms:LDTask ,
                        ms:LRIdentifierScheme ,
                        ms:LanguageVarietyType ,
                        ms:LicenceIdentifierScheme ,
                        ms:MembershipInstitution ,
                        ms:MetadataRecordIdentifierScheme ,
                        ms:Metric ,
                        ms:ModalityType ,
                        ms:ModelType ,
                        ms:MultilingualityType ,
                        ms:Naturality ,
                        ms:NonSpeechItem ,
                        ms:OperatingSystem ,
                        ms:OrganizationLegalStatus ,
                        ms:OrganizationRole ,
                        ms:ParameterType ,
                        ms:ProcessingResourceType ,
                        ms:ProjectIdentifierScheme ,
                        ms:RecordingDeviceType ,
                        ms:RecordingEnvironment ,
                        ms:RepositoryIdentifierScheme ,
                        ms:RequiredHardware ,
                        ms:RoleIdentifierScheme ,
                        ms:ScenarioType ,
                        ms:SceneIllumination ,
                        ms:SegmentationLevel ,
                        ms:SignalEncoding ,
                        ms:SizeUnit ,
                        ms:SocialMediaOccupationalAccountType ,
                        ms:SoftwareDistributionForm ,
                        ms:SourceChannel ,
                        ms:SourceChannelType ,
                        ms:SpeechGenre ,
                        ms:SpeechGenreClassificationScheme ,
                        ms:SpeechInfluence ,
                        ms:SpeechItem ,
                        ms:StandardBestPractice ,
                        ms:SubjectClassificationScheme ,
                        ms:SupportType ,
                        ms:TextGenre ,
                        ms:TextGenreClassificationScheme ,
                        ms:TextType ,
                        ms:TextTypeClassificationScheme ,
                        ms:VideoGenreClassificationScheme ,
                        ms:VocalTractCondition ,
                        ms:WebServiceType ;
               rdfs:comment "Value used for mandatory elements whose value is unknown or cannot be specified"@en ;
               rdfs:label "unspecified"@en .


###  http://w3id.org/meta-share/meta-share/updated
ms:updated rdf:type owl:NamedIndividual ,
                    ms:VersionType ;
           rdfs:comment "Value for 'Version type' used for versions that have been updated vis-a-vis the previous published version"@en ;
           rdfs:label "updated"@en .


###  http://w3id.org/meta-share/meta-share/url1
ms:url1 rdf:type owl:NamedIndividual ,
                 ms:ParameterType ;
        rdfs:label "url"@en .


###  http://w3id.org/meta-share/meta-share/usage
ms:usage rdf:type owl:NamedIndividual ,
                  ms:EvaluationLevel ;
         rdfs:label "usage"@en .


###  http://w3id.org/meta-share/meta-share/userIdentified
ms:userIdentified rdf:type owl:NamedIndividual ,
                           ms:ConditionOfUse ;
                  rdfs:comment "Value for 'ConditionOfUse' which states that the resource can only be accessed by identified/authenticated users"@en ;
                  rdfs:label "user identified"@en .


###  http://w3id.org/meta-share/meta-share/userInputText
ms:userInputText rdf:type owl:NamedIndividual ,
                          ms:ProcessingResourceType ;
                 rdfs:label "user input text"@en .


###  http://w3id.org/meta-share/meta-share/userManual
ms:userManual rdf:type owl:NamedIndividual ,
                       ms:DocumentationType ;
              rdfs:comment "Value for 'Documentation type' for documents that include instructions and examples on the usage of a tool/service (or resource in general)"@en ;
              rdfs:label "user manual"@en .


###  http://w3id.org/meta-share/meta-share/utterance
ms:utterance rdf:type owl:NamedIndividual ,
                      ms:SegmentationLevel ;
             rdfs:label "utterance"@en .


###  http://w3id.org/meta-share/meta-share/utterance1
ms:utterance1 rdf:type owl:NamedIndividual ,
                       ms:SizeUnit ;
              rdfs:label "utterance"@en .


###  http://w3id.org/meta-share/meta-share/variable
ms:variable rdf:type owl:NamedIndividual ,
                     ms:SceneIllumination ;
            rdfs:label "variable"@en .


###  http://w3id.org/meta-share/meta-share/variant1
ms:variant1 rdf:type owl:NamedIndividual ,
                     skos:Concept ;
            rdfs:label "variant"@en ;
            skos:broader ms:LemmaType ;
            skos:inScheme ms:ContentTypeScheme .


###  http://w3id.org/meta-share/meta-share/vcvSequence
ms:vcvSequence rdf:type owl:NamedIndividual ,
                        ms:SpeechItem ;
               rdfs:label "VCV sequence"@en .


###  http://w3id.org/meta-share/meta-share/vector
ms:vector rdf:type owl:NamedIndividual ,
                   ms:RasterOrVectorGraphics ;
          rdfs:label "vector"@en .


###  http://w3id.org/meta-share/meta-share/veryHigh
ms:veryHigh rdf:type owl:NamedIndividual ,
                     ms:RecordingQuality ;
            rdfs:label "very high"@en .


###  http://w3id.org/meta-share/meta-share/veryHigh1
ms:veryHigh1 rdf:type owl:NamedIndividual ,
                      ms:Quality ;
             rdfs:label "very high"@en .


###  http://w3id.org/meta-share/meta-share/veryLow
ms:veryLow rdf:type owl:NamedIndividual ,
                    ms:RecordingQuality ;
           rdfs:label "very low"@en .


###  http://w3id.org/meta-share/meta-share/veryLow1
ms:veryLow1 rdf:type owl:NamedIndividual ,
                     ms:Quality ;
            rdfs:label "very low"@en .


###  http://w3id.org/meta-share/meta-share/video
ms:video rdf:type owl:NamedIndividual ,
                  ms:MediaType ;
         rdfs:comment "Value for 'Media type' for the audiovisual form of a language resource (part)"@en ;
         rdfs:label "video"@en .


###  http://w3id.org/meta-share/meta-share/video1
ms:video1 rdf:type owl:NamedIndividual ,
                   ms:ExtratextualInformation ;
          rdfs:label "video"@en .


###  http://w3id.org/meta-share/meta-share/visualizationOutput
ms:visualizationOutput rdf:type owl:NamedIndividual ,
                                ms:ProcessingResourceType ;
                       rdfs:label "visualization output"@en .


###  http://w3id.org/meta-share/meta-share/voice
ms:voice rdf:type owl:NamedIndividual ,
                  ms:ModalityType ;
         rdfs:comment "Value for 'ModalityType' for voice"@en ;
         rdfs:label "voice"@en .


###  http://w3id.org/meta-share/meta-share/voice1
ms:voice1 rdf:type owl:NamedIndividual ,
                   skos:Concept ;
          rdfs:label "voice"@en ;
          skos:broader ms:MorphologicalType ;
          skos:inScheme ms:ContentTypeScheme .


###  http://w3id.org/meta-share/meta-share/webCam
ms:webCam rdf:type owl:NamedIndividual ,
                   ms:SourceChannel ;
          rdfs:label "webcam"@en .


###  http://w3id.org/meta-share/meta-share/webService
ms:webService rdf:type owl:NamedIndividual ,
                       ms:SoftwareDistributionForm ;
              rdfs:comment "Value for software distribution form, used for software objects that can be accessed through remote invocation typically using some REST-style APIs or SOAP protocols"@en ;
              rdfs:label "web service"@en .


###  http://w3id.org/meta-share/meta-share/webcam
ms:webcam rdf:type owl:NamedIndividual ,
                   ms:CapturingDeviceType ;
          rdfs:label "webcam"@en .


###  http://w3id.org/meta-share/meta-share/wholeBody
ms:wholeBody rdf:type owl:NamedIndividual ,
                      ms:BodyPart ;
             rdfs:label "whole body"@en .


###  http://w3id.org/meta-share/meta-share/windows
ms:windows rdf:type owl:NamedIndividual ,
                    ms:OperatingSystem ;
           rdfs:label "Windows"@en .


###  http://w3id.org/meta-share/meta-share/windows-1250
ms:windows-1250 rdf:type owl:NamedIndividual ,
                         ms:CharacterEncoding ;
                rdfs:label "windows-1250"@en .


###  http://w3id.org/meta-share/meta-share/windows-1251
ms:windows-1251 rdf:type owl:NamedIndividual ,
                         ms:CharacterEncoding ;
                rdfs:label "windows-1251"@en .


###  http://w3id.org/meta-share/meta-share/windows-1252
ms:windows-1252 rdf:type owl:NamedIndividual ,
                         ms:CharacterEncoding ;
                rdfs:label "windows-1252"@en .


###  http://w3id.org/meta-share/meta-share/windows-1253
ms:windows-1253 rdf:type owl:NamedIndividual ,
                         ms:CharacterEncoding ;
                rdfs:label "windows-1253"@en .


###  http://w3id.org/meta-share/meta-share/windows-1254
ms:windows-1254 rdf:type owl:NamedIndividual ,
                         ms:CharacterEncoding ;
                rdfs:label "windows-1254"@en .


###  http://w3id.org/meta-share/meta-share/windows-1255
ms:windows-1255 rdf:type owl:NamedIndividual ,
                         ms:CharacterEncoding ;
                rdfs:label "windows-1255"@en .


###  http://w3id.org/meta-share/meta-share/windows-1256
ms:windows-1256 rdf:type owl:NamedIndividual ,
                         ms:CharacterEncoding ;
                rdfs:label "windows-1256"@en .


###  http://w3id.org/meta-share/meta-share/windows-1257
ms:windows-1257 rdf:type owl:NamedIndividual ,
                         ms:CharacterEncoding ;
                rdfs:label "windows-1257"@en .


###  http://w3id.org/meta-share/meta-share/windows-1258
ms:windows-1258 rdf:type owl:NamedIndividual ,
                         ms:CharacterEncoding ;
                rdfs:label "windows-1258"@en .


###  http://w3id.org/meta-share/meta-share/windows-31j
ms:windows-31j rdf:type owl:NamedIndividual ,
                        ms:CharacterEncoding ;
               rdfs:label "windows-31j"@en .


###  http://w3id.org/meta-share/meta-share/wizardOfOz
ms:wizardOfOz rdf:type owl:NamedIndividual ,
                       ms:ScenarioType ;
              rdfs:label "wizard of Oz"@en .


###  http://w3id.org/meta-share/meta-share/word
ms:word rdf:type owl:NamedIndividual ,
                 ms:BaseItem ;
        rdfs:label "word"@en .


###  http://w3id.org/meta-share/meta-share/word1
ms:word1 rdf:type owl:NamedIndividual ,
                  ms:SegmentationLevel ;
         rdfs:label "word"@en .


###  http://w3id.org/meta-share/meta-share/word2
ms:word2 rdf:type owl:NamedIndividual ,
                  ms:ExtratextualInformationUnit ;
         rdfs:label "word"@en .


###  http://w3id.org/meta-share/meta-share/word3
ms:word3 rdf:type owl:NamedIndividual ,
                  ms:SizeUnit ;
         rdfs:label "word"@en .


###  http://w3id.org/meta-share/meta-share/wordGame
ms:wordGame rdf:type owl:NamedIndividual ,
                     ms:ScenarioType ;
            rdfs:label "word game"@en .


###  http://w3id.org/meta-share/meta-share/wordGroup
ms:wordGroup rdf:type owl:NamedIndividual ,
                      ms:SegmentationLevel ;
             rdfs:label "word group"@en .


###  http://w3id.org/meta-share/meta-share/wordNet
ms:wordNet rdf:type owl:NamedIndividual ,
                    ms:CompatibleLexiconType ,
                    ms:LCRSubclass ,
                    ms:StandardBestPractice ;
           rdfs:comment "A lexical database originally created for English and extended to other languages, which groups words into sets of synonyms called synsets, provides short definitions and usage examples, and records a number of relations among these synonym sets or their members"@en ;
           rdfs:label "WordNet"@en .


###  http://w3id.org/meta-share/meta-share/wordlist
ms:wordlist rdf:type owl:NamedIndividual ,
                     ms:CompatibleLexiconType ,
                     ms:LCRSubclass ;
            rdfs:comment "A written collection of all words derived from a particular source, or sharing some other characteristic [https://www.yourdictionary.com/wordlist]"@en ;
            rdfs:label "wordlist"@en .


###  http://w3id.org/meta-share/meta-share/workflowFile
ms:workflowFile rdf:type owl:NamedIndividual ,
                         ms:SoftwareDistributionForm ;
                rdfs:comment "Value for software distribution form, used for software workflows that are made available in the form of the workflow description file"@en ;
                rdfs:label "workflow file"@en .


###  http://w3id.org/meta-share/meta-share/writtenLanguage
ms:writtenLanguage rdf:type owl:NamedIndividual ,
                            ms:ModalityType ;
                   rdfs:comment "Value for 'ModalityType' for texts with written language"@en ;
                   rdfs:label "written language"@en .


###  http://w3id.org/meta-share/meta-share/x-EUC-CN
ms:x-EUC-CN rdf:type owl:NamedIndividual ,
                     ms:CharacterEncoding ;
            rdfs:label "x-EUC-CN"@en .


###  http://w3id.org/meta-share/meta-share/x-EUC-JP-LINUX
ms:x-EUC-JP-LINUX rdf:type owl:NamedIndividual ,
                           ms:CharacterEncoding ;
                  rdfs:label "x-EUC-JP-LINUX"@en .


###  http://w3id.org/meta-share/meta-share/x-EUC-TW
ms:x-EUC-TW rdf:type owl:NamedIndividual ,
                     ms:CharacterEncoding ;
            rdfs:label "x-EUC-TW"@en .


###  http://w3id.org/meta-share/meta-share/x-MS950-HKSCS
ms:x-MS950-HKSCS rdf:type owl:NamedIndividual ,
                          ms:CharacterEncoding ;
                 rdfs:label "x-MS950-HKSCS"@en .


###  http://w3id.org/meta-share/meta-share/x-mswin-936
ms:x-mswin-936 rdf:type owl:NamedIndividual ,
                        ms:CharacterEncoding ;
               rdfs:label "x-mswin-936"@en .


###  http://w3id.org/meta-share/meta-share/x-windows-949
ms:x-windows-949 rdf:type owl:NamedIndividual ,
                          ms:CharacterEncoding ;
                 rdfs:label "x-windows-949"@en .


###  http://w3id.org/meta-share/meta-share/x-windows-950
ms:x-windows-950 rdf:type owl:NamedIndividual ,
                          ms:CharacterEncoding ;
                 rdfs:label "x-windows-950"@en .


###  http://w3id.org/meta-share/meta-share/yes
ms:yes rdf:type owl:NamedIndividual ,
                ms:SpeakingImpairmentOfParticipants ;
       rdfs:label "yes"@en .


###  http://w3id.org/meta-share/meta-share/yesA
ms:yesA rdf:type owl:NamedIndividual ,
                 ms:Anonymized ;
        rdfs:label "yes"@en .


###  http://w3id.org/meta-share/meta-share/yesH
ms:yesH rdf:type owl:NamedIndividual ,
                 ms:HearingImpairmentOfParticipants ;
        rdfs:label "yes"@en .


###  http://w3id.org/meta-share/meta-share/yesNoQuestion
ms:yesNoQuestion rdf:type owl:NamedIndividual ,
                          ms:SpeechItem ;
                 rdfs:label "yes/no question"@en .


###  http://w3id.org/meta-share/meta-share/yesP
ms:yesP rdf:type owl:NamedIndividual ,
                 ms:PersonalDataIncluded ;
        rdfs:label "yes"@en .


###  http://w3id.org/meta-share/meta-share/yesS
ms:yesS rdf:type owl:NamedIndividual ,
                 ms:SensitiveDataIncluded ;
        rdfs:label "yes"@en .


###  http://w3id.org/meta-share/meta-share/youtube
ms:youtube rdf:type owl:NamedIndividual ,
                    ms:SocialMediaOccupationalAccountType ;
           rdfs:label "youtube" .


###  http://w3id.org/meta-share/omtd-share/AnnotationTypeScheme
omtd:AnnotationTypeScheme rdf:type owl:NamedIndividual ,
                                   skos:ConceptScheme .


###  http://w3id.org/meta-share/omtd-share/DataFormatScheme
omtd:DataFormatScheme rdf:type owl:NamedIndividual ,
                               skos:ConceptScheme .


###  http://w3id.org/meta-share/omtd-share/ModelFunctionScheme
omtd:ModelFunctionScheme rdf:type owl:NamedIndividual ,
                                  skos:ConceptScheme .


###  http://w3id.org/meta-share/omtd-share/OperationScheme
omtd:OperationScheme rdf:type owl:NamedIndividual ,
                              skos:ConceptScheme .


###  http://w3id.org/meta-share/omtd-share/OperationTypeScheme
omtd:OperationTypeScheme rdf:type owl:NamedIndividual .


###  http://w3id.org/meta-share/omtd-share/TdmMethodScheme
omtd:TdmMethodScheme rdf:type owl:NamedIndividual ,
                              skos:ConceptScheme .


[ odrl:action cc:CommericalUse ,
              cc:Distribution
] .

[ odrl:constraint [ odrl:operator odrl:eq
                   ]
 ] .

[ odrl:action cc:Reproduction
 ] .

[ odrl:action cc:CommercialUse
 ] .

#################################################################
#    Annotations
#################################################################

ms:CharacterEncodingSet dct:replaces msxml:characterEncoding .


ms:DomainClassification dct:replaces msxml:domainInfo .


ms:GeographicCoverageClassification dct:replaces msxml:geographicCoverageInfo .


ms:LicenseInfo rdfs:comment "Links a resource to the licence under which it is distributed; values are taken from a list of standard licences"@en .


ms:TimeCoverageClassification dct:replaces msxml:timeCoverageInfo .


ms:availableThroughOtherDistributor dct:replaces msxml:notAvailableThroughMetashare ;
                                    rdfs:label "Available Through Other Distributor"@en ;
                                    rdfs:comment "For resources that are documented in the catalogue but the contents of which can only be accessed through other distribution channels."@en .


ms:guidelines rdfs:comment "Links to the document used as guidelines for the creation or annotation of a corpus"@en ;
              rdfs:label "guidelines"@en .


ms:image3 rdfs:comment "Links to a URL with an image file (e.g., a photo, or cartoon image) that is used for identifying a person (e.g., on a home page)"@en ;
          rdfs:label "image"@en .


ms:licenseInfo rdfs:comment "Links a resource to the licence under which it is distributed; values are taken from a list of standard licences"@en .


ms:telephoneNumber skos:example "+123456789012"@en ;
                   rdfs:label "telephone number"@en ;
                   rdfs:comment "Introduces the telephone number of a person, group or organization; recommended format: +_international code_city code_number without spaces"@en .


<http://w3id.org/meta-share/meta-share/2.0.0/copyrightNotEvaluated> rdfs:label "Copyright Not Evaluated"@en .


<http://w3id.org/meta-share/meta-share/2.0.0/copyrightUndetermined> rdfs:label "Copyright Undetermined"@en .


<http://w3id.org/meta-share/meta-share/2.0.0/embargoedAccess> rdfs:label "embargoed access"@en ;
                                                              rdfs:comment "Embargoed access refers to a resource that is metadata only access until released for open access on a certain date. Embargoes can be required by publishers and funders policies, or set by the author (e.g such as in the case of theses and dissertations)."@en .


<http://w3id.org/meta-share/meta-share/2.0.0/inCopyright> rdfs:label "In Copyright"@en .


<http://w3id.org/meta-share/meta-share/2.0.0/inCopyrightEUOrphan> rdfs:label "In Copyright - EU Orphan Work"@en .


<http://w3id.org/meta-share/meta-share/2.0.0/inCopyrightEdu> rdfs:label "In Copyright - Educational Use Permitted"@en .


<http://w3id.org/meta-share/meta-share/2.0.0/inCopyrightNCPermitted> rdfs:label "In Copyright - Non-Commercial Use Permitted"@en .


<http://w3id.org/meta-share/meta-share/2.0.0/inCopyrightRightsHoldersUnlocatable> rdfs:label "In Copyright - Rights-holder(s) Unlocatable or Unidentifiable"@en .


<http://w3id.org/meta-share/meta-share/2.0.0/metadataOnlyAccess> rdfs:comment "Metadata only access refers to a resource in which access is limited to metadata only. The resource itself is described by the metadata, but neither is directly available through the system or platform nor can be referenced to an open access copy in an external journal or trustworthy archive."@en ;
                                                                 rdfs:label "metadata only access" .


<http://w3id.org/meta-share/meta-share/2.0.0/noCopyright> rdfs:label "No Copyright - Other Known Legal Restrictions"@en .


<http://w3id.org/meta-share/meta-share/2.0.0/noCopyrightContract> rdfs:label "No Copyright - Contractual Restrictions"@en .


<http://w3id.org/meta-share/meta-share/2.0.0/noCopyrightNC> rdfs:label "No Copyright - Non-Commercial Use Only"@en .


<http://w3id.org/meta-share/meta-share/2.0.0/noCopyrightUS> rdfs:label "No Copyright - United States"@en .


<http://w3id.org/meta-share/meta-share/2.0.0/noKnownCopyright> rdfs:label "No Known Copyright"@en .


<http://w3id.org/meta-share/meta-share/2.0.0/openAccess1> rdfs:comment "Open access refers to a resource that is immediately and permanently online, and free for all on the Web, without financial and technical barriers.The resource is either stored in the repository or referenced to an external journal or trustworthy archive."@en ;
                                                          rdfs:label "open access"@en .


<http://w3id.org/meta-share/meta-share/2.0.0/restrictedAccess1> rdfs:label "restricted access"@en ;
                                                                rdfs:comment "Restricted access refers to a resource that is available in a system but with some type of restriction for full open access. This type of access can occur in a number of different situations. Some examples are described below: The user must log-in to the system in order to access the resource The user must send an email to the author or system administrator to access the resource Access to the resource is restricted to a specific community (e.g., limited to a university community)"@en .


###  Generated by the OWL API (version 4.5.9.2019-02-01T07:24:44Z) https://github.com/owlcs/owlapi
